@prefix dcterms: <http://purl.org/dc/terms/> .
@prefix ns1: <https://w3id.org/emmo#> .
@prefix ns2: <http://www.lesfleursdunormal.fr/static/_downloads/owlready_ontology.owl#> .
@prefix owl: <http://www.w3.org/2002/07/owl#> .
@prefix rdf: <http://www.w3.org/1999/02/22-rdf-syntax-ns#> .
@prefix rdfs: <http://www.w3.org/2000/01/rdf-schema#> .
@prefix skos: <http://www.w3.org/2004/02/skos/core#> .
@prefix xsd: <http://www.w3.org/2001/XMLSchema#> .

ns1:AbsoluteHumidity a owl:Class ;
    rdfs:label "AbsoluteHumidity"@en ;
    rdfs:comment "Mass of the contained water vapour per volume."@en ;
    rdfs:subClassOf ns1:MassConcentration,
        ns1:ThermodynamicalQuantity ;
    skos:altLabel "MassConcentrationOfWaterVapour"@en ;
    skos:prefLabel "AbsoluteHumidity"@en ;
    ns1:IEVReference "https://www.electropedia.org/iev/iev.nsf/display?openform&ievref=113-04-60"^^xsd:string ;
    ns1:ISO80000Reference "5-28"^^xsd:string ;
    ns1:elucidation "Mass of the contained water vapour per volume."@en ;
    ns1:qudtReference "https://qudt.org/vocab/quantitykind/AbsoluteHumidity"^^xsd:string,
        "https://qudt.org/vocab/quantitykind/MassConcentrationOfWaterVapour"^^xsd:string ;
    ns1:wikidataReference "https://www.wikidata.org/wiki/Q76378808"^^xsd:string .

ns1:AbsorbedDose a owl:Class ;
    rdfs:label "AbsorbedDose"@en ;
    rdfs:comment "Energy imparted to matter by ionizing radiation in a suitable small element of volume divided by the mass of that element of volume."@en ;
    rdfs:subClassOf [ a owl:Restriction ;
            owl:onProperty ns1:hasMeasurementUnit ;
            owl:someValuesFrom ns1:AbsorbedDoseUnit ],
        ns1:AtomicAndNuclearPhysicsQuantity,
        ns1:ISQDerivedQuantity ;
    owl:disjointWith ns1:SpecificEnergyImparted ;
    skos:prefLabel "AbsorbedDose"@en ;
    ns1:ISO80000Reference "10-81.1"^^xsd:string ;
    ns1:elucidation "Energy imparted to matter by ionizing radiation in a suitable small element of volume divided by the mass of that element of volume."@en ;
    ns1:iupacReference "https://doi.org/10.1351/goldbook.A00031"^^xsd:string ;
    ns1:qudtReference "http://qudt.org/vocab/quantitykind/AbsorbedDose"^^xsd:string .

ns1:Acceleration a owl:Class ;
    rdfs:label "Acceleration"@en ;
    rdfs:comment "Derivative of velocity with respect to time."@en ;
    rdfs:subClassOf [ a owl:Restriction ;
            owl:onProperty ns1:hasMeasurementUnit ;
            owl:someValuesFrom ns1:AccelerationUnit ],
        ns1:ISQDerivedQuantity,
        ns1:SpaceAndTimeQuantity ;
    skos:prefLabel "Acceleration"@en ;
    ns1:ISO80000Reference "3-9.1"^^xsd:string ;
    ns1:elucidation "Derivative of velocity with respect to time."@en ;
    ns1:iupacReference "https://doi.org/10.1351/goldbook.A00051"^^xsd:string ;
    ns1:qudtReference "http://qudt.org/vocab/quantitykind/Acceleration"^^xsd:string .

ns1:AcceptorDensity a owl:Class ;
    rdfs:label "AcceptorDensity"@en ;
    rdfs:comment "quotient of number of acceptor levels and volume."@en ;
    rdfs:subClassOf [ a owl:Restriction ;
            owl:onProperty ns1:hasMeasurementUnit ;
            owl:someValuesFrom ns1:PerVolumeUnit ],
        ns1:CondensedMatterPhysicsQuantity,
        ns1:ISQDerivedQuantity ;
    skos:prefLabel "AcceptorDensity"@en ;
    ns1:ISO80000Reference "12-29.5"^^xsd:string ;
    ns1:elucidation "quotient of number of acceptor levels and volume."@en ;
    ns1:qudtReference "https://qudt.org/vocab/quantitykind/AcceptorDensity"^^xsd:string ;
    ns1:wikidataReference "https://www.wikidata.org/wiki/Q105979968"^^xsd:string .

ns1:AcousticQuantity a owl:Class ;
    rdfs:label "AcousticQuantity"@en ;
    rdfs:comment "Quantities categorised according to ISO 80000-8."@en ;
    rdfs:subClassOf ns1:ISO80000Categorised ;
    skos:prefLabel "AcousticQuantity"@en ;
    ns1:elucidation "Quantities categorised according to ISO 80000-8."@en .

ns1:Action a owl:Class ;
    rdfs:label "Action"@en ;
    rdfs:comment "Physical quantity of dimension energy × time."@en ;
    rdfs:subClassOf [ a owl:Restriction ;
            owl:onProperty ns1:hasMeasurementUnit ;
            owl:someValuesFrom ns1:AngularMomentumUnit ],
        ns1:ISQDerivedQuantity,
        ns1:MechanicalQuantity ;
    skos:prefLabel "Action"@en ;
    ns1:IEVReference "https://www.electropedia.org/iev/iev.nsf/display?openform&ievref=113-03-51"@en ;
    ns1:ISO80000Reference "4-32"^^xsd:string ;
    ns1:elucidation "Physical quantity of dimension energy × time."@en ;
    ns1:qudtReference "https://qudt.org/vocab/quantitykind/Action"@en ;
    ns1:wikidataReference "https://www.wikidata.org/wiki/Q846785"^^xsd:string .

ns1:ActiveEnergy a owl:Class ;
    rdfs:label "ActiveEnergy"@en ;
    rdfs:comment "The integral over a time interval of the instantaneous power."@en ;
    rdfs:subClassOf ns1:ElectromagneticQuantity,
        ns1:Energy ;
    skos:prefLabel "ActiveEnergy"@en ;
    ns1:IEVReference "https://www.electropedia.org/iev/iev.nsf/display?openform&ievref=601-01-19"^^xsd:string,
        "https://www.electropedia.org/iev/iev.nsf/display?openform&ievref=131-11-57"@en ;
    ns1:ISO80000Reference "6-62"^^xsd:string ;
    ns1:elucidation "The integral over a time interval of the instantaneous power."@en ;
    ns1:qudtReference "https://qudt.org/vocab/quantitykind/ActiveEnergy"^^xsd:string ;
    ns1:wikidataReference "https://www.wikidata.org/wiki/Q79813678"^^xsd:string .

ns1:ActivePower a owl:Class ;
    rdfs:label "ActivePower"@en ;
    rdfs:comment "Average power over a period."@en ;
    rdfs:subClassOf ns1:Power ;
    skos:prefLabel "ActivePower"@en ;
    ns1:IEVReference "https://www.electropedia.org/iev/iev.nsf/display?openform&ievref=131-11-42"^^xsd:string ;
    ns1:ISO80000Reference "6-56"^^xsd:string ;
    ns1:elucidation "Average power over a period."@en ;
    ns1:qudtReference "https://qudt.org/vocab/quantitykind/ActivePower"^^xsd:string ;
    ns1:wikidataReference "https://www.wikidata.org/wiki/Q20820042"^^xsd:string .

ns1:Activity a owl:Class ;
    rdfs:label "Activity"@en ;
    rdfs:comment "Number dN of spontaneous nuclear transitions or nuclear disintegrations for a radionuclide of amount N produced during a short time interval dt, divided by this time interval."@en ;
    rdfs:subClassOf ns1:AtomicAndNuclearPhysicsQuantity,
        ns1:Rate ;
    skos:prefLabel "Activity"@en ;
    ns1:IEVReference "https://www.electropedia.org/iev/iev.nsf/display?openform&ievref=395-01-05"^^xsd:string ;
    ns1:ISO80000Reference "10-27"^^xsd:string ;
    ns1:elucidation "Number dN of spontaneous nuclear transitions or nuclear disintegrations for a radionuclide of amount N produced during a short time interval dt, divided by this time interval."@en ;
    ns1:iupacReference "https://goldbook.iupac.org/terms/view/A00114"^^xsd:string ;
    ns1:qudtReference "https://qudt.org/vocab/quantitykind/Activity"^^xsd:string ;
    ns1:wikidataReference "https://www.wikidata.org/wiki/Q317949"^^xsd:string .

ns1:ActivityDensity a owl:Class ;
    rdfs:label "ActivityDensity"@en ;
    rdfs:comment "Activity per unit volume of the sample."@en ;
    rdfs:subClassOf [ a owl:Restriction ;
            owl:onProperty ns1:hasMeasurementUnit ;
            owl:someValuesFrom ns1:FrequencyPerVolumeUnit ],
        ns1:AtomicAndNuclearPhysicsQuantity,
        ns1:ISQDerivedQuantity ;
    skos:altLabel "ActivityConcentration"@en,
        "VolumetricActivity"@en,
        "VolumicActivity"@en ;
    skos:prefLabel "ActivityDensity"@en ;
    ns1:IEVReference "https://www.electropedia.org/iev/iev.nsf/display?openform&ievref=395-01-09"^^xsd:string ;
    ns1:ISO80000Reference "10-29"^^xsd:string ;
    ns1:elucidation "Activity per unit volume of the sample."@en ;
    ns1:qudtReference "https://qudt.org/vocab/quantitykind/ActivityConcentration"^^xsd:string ;
    ns1:wikidataReference "https://www.wikidata.org/wiki/Q423263"^^xsd:string .

ns1:ActivityFactor a owl:Class ;
    rdfs:label "ActivityFactor"@en ;
    rdfs:comment "For substance X in a liquid or a solid mixture; quotient of absolute activity of substance X and the product of absolute activity of the pure substance X at the same temperature and pressure and amount-of-substance fraction of substance X."@en ;
    rdfs:subClassOf ns1:ISQDimensionlessQuantity,
        ns1:PhysioChemicalQuantity ;
    owl:disjointWith ns1:ActivityCoefficient ;
    skos:prefLabel "ActivityFactor"@en ;
    ns1:ISO80000Reference "9-22"^^xsd:string ;
    ns1:elucidation "For substance X in a liquid or a solid mixture; quotient of absolute activity of substance X and the product of absolute activity of the pure substance X at the same temperature and pressure and amount-of-substance fraction of substance X."@en ;
    ns1:note "Activity factors can also be obtained applying Raoult's law or Henry's law."@en ;
    ns1:wikidataReference "https://www.wikidata.org/wiki/Q89335167"^^xsd:string .

ns1:ActivityOfSolvent a owl:Class ;
    rdfs:label "ActivityOfSolvent"@en ;
    rdfs:comment "For a solvent in a solution, quotient of the absolute activity and that of the pure substance at the same temperature and pressure."@en ;
    rdfs:subClassOf ns1:ISQDimensionlessQuantity,
        ns1:PhysioChemicalQuantity ;
    skos:prefLabel "ActivityOfSolvent"@en ;
    ns1:ISO80000Reference "9-27.1"^^xsd:string ;
    ns1:elucidation "For a solvent in a solution, quotient of the absolute activity and that of the pure substance at the same temperature and pressure."@en ;
    ns1:wikidataReference "https://www.wikidata.org/wiki/Q89486193"^^xsd:string .

ns1:Admittance a owl:Class ;
    rdfs:label "Admittance"@en ;
    rdfs:comment "Inverse of the impendance."@en ;
    rdfs:subClassOf ns1:ElectricConductance ;
    skos:altLabel "ComplexAdmittance"@en ;
    skos:prefLabel "Admittance"@en ;
    ns1:IEVReference "https://www.electropedia.org/iev/iev.nsf/display?openform&ievref=131-12-51"^^xsd:string ;
    ns1:ISO80000Reference "6-52.1"^^xsd:string ;
    ns1:dbpediaReference "https://dbpedia.org/page/Admittance"^^xsd:string ;
    ns1:elucidation "Inverse of the impendance."@en ;
    ns1:qudtReference "https://qudt.org/vocab/quantitykind/Admittance"^^xsd:string ;
    ns1:wikidataReference "https://www.wikidata.org/wiki/Q214518"^^xsd:string .

ns1:AffinityOfAChemicalReaction a owl:Class ;
    rdfs:label "AffinityOfAChemicalReaction"@en ;
    rdfs:comment "Describes elements' or compounds' readiness to form bonds."^^xsd:string ;
    rdfs:subClassOf [ a owl:Restriction ;
            owl:onProperty ns1:hasMeasurementUnit ;
            owl:someValuesFrom ns1:EnergyPerAmountUnit ],
        ns1:PhysioChemicalQuantity ;
    skos:altLabel "ChemicalAffinity"@en ;
    skos:prefLabel "AffinityOfAChemicalReaction"@en ;
    ns1:ISO80000Reference "9-30"^^xsd:string ;
    ns1:elucidation "Describes elements' or compounds' readiness to form bonds."^^xsd:string ;
    ns1:iupacReference "https://doi.org/10.1351/goldbook.A00178"^^xsd:string ;
    ns1:qudtReference "https://qudt.org/vocab/quantitykind/ChemicalAffinity"^^xsd:string ;
    ns1:wikidataReference "https://www.wikidata.org/wiki/Q382783"^^xsd:string .

ns1:AlphaDisintegrationEnergy a owl:Class ;
    rdfs:label "AlphaDisintegrationEnergy"@en ;
    rdfs:comment "Sum of the kinetic energy of the α-particle produced in the disintegration process and the recoil energy of the product atom in a reference frame in which the emitting nucleus is at rest before its disintegration."@en ;
    rdfs:subClassOf ns1:AtomicAndNuclearPhysicsQuantity,
        ns1:Energy ;
    skos:prefLabel "AlphaDisintegrationEnergy"@en ;
    ns1:ISO80000Reference "10-32"^^xsd:string ;
    ns1:elucidation "Sum of the kinetic energy of the α-particle produced in the disintegration process and the recoil energy of the product atom in a reference frame in which the emitting nucleus is at rest before its disintegration."@en ;
    ns1:qudtReference "http://qudt.org/vocab/quantitykind/AlphaDisintegrationEnergy"^^xsd:string ;
    ns1:wikidataReference "https://www.wikidata.org/wiki/Q98146025"^^xsd:string .

ns1:AmountFraction a owl:Class ;
    rdfs:label "AmountFraction"@en ;
    rdfs:comment "The amount of a constituent divided by the total amount of all constituents in a mixture."@en ;
    rdfs:subClassOf ns1:Intensive,
        ns1:RatioQuantity ;
    skos:altLabel "MoleFraction"@en ;
    skos:prefLabel "AmountFraction"@en ;
    ns1:elucidation "The amount of a constituent divided by the total amount of all constituents in a mixture."@en ;
    ns1:iupacReference "https://doi.org/10.1351/goldbook.A00296"^^xsd:string ;
    ns1:qudtReference "http://qudt.org/vocab/quantitykind/MoleFraction"^^xsd:string .

ns1:AmountPerAreaTimeUnit a owl:Class ;
    rdfs:label "AmountPerAreaTimeUnit"@en ;
    rdfs:comment "The class of units with dimensionality 'AmountPerAreaTime'."@en .

ns1:AmountPerAreaUnit a owl:Class ;
    rdfs:label "AmountPerAreaUnit"@en ;
    rdfs:comment "The class of units with dimensionality 'AmountPerArea'."@en .

ns1:AmountPerMassPressureUnit a owl:Class ;
    rdfs:label "AmountPerMassPressureUnit"@en ;
    rdfs:comment "The class of units with dimensionality 'AmountPerMassPressure'."@en .

ns1:AmountPerMassTimeUnit a owl:Class ;
    rdfs:label "AmountPerMassTimeUnit"@en ;
    rdfs:comment "The class of units with dimensionality 'AmountPerMassTime'."@en .

ns1:AmountPerVolumeTimeUnit a owl:Class ;
    rdfs:label "AmountPerVolumeTimeUnit"@en ;
    rdfs:comment "The class of units with dimensionality 'AmountPerVolumeTime'."@en .

ns1:AmountSquareTimePerMassVolumeUnit a owl:Class ;
    rdfs:label "AmountSquareTimePerMassVolumeUnit"@en ;
    rdfs:comment "The class of units with dimensionality 'AmountSquareTimePerMassVolume'."@en .

ns1:AmountTemperatureUnit a owl:Class ;
    rdfs:label "AmountTemperatureUnit"@en ;
    rdfs:comment "The class of units with dimensionality 'AmountTemperature'."@en .

ns1:AngularAcceleration a owl:Class ;
    rdfs:label "AngularAcceleration"@en ;
    rdfs:comment "Vector quantity giving the rate of change of angular velocity."@en ;
    rdfs:subClassOf [ a owl:Restriction ;
            owl:onProperty ns1:hasMeasurementUnit ;
            owl:someValuesFrom ns1:AngularFrequencyUnit ],
        ns1:ISQDerivedQuantity ;
    skos:prefLabel "AngularAcceleration"@en ;
    ns1:IEVReference "https://www.electropedia.org/iev/iev.nsf/display?openform&ievref=113-01-46"^^xsd:string ;
    ns1:ISO80000Reference "3-13"^^xsd:string ;
    ns1:dbpediaReference "https://dbpedia.org/page/Angular_acceleration"^^xsd:string ;
    ns1:elucidation "Vector quantity giving the rate of change of angular velocity."@en ;
    ns1:qudtReference "https://qudt.org/vocab/quantitykind/AngularAcceleration"^^xsd:string ;
    ns1:wikipediaReference "https://en.wikipedia.org/wiki/Angular_acceleration"^^xsd:string .

ns1:AngularMeasure a owl:Class ;
    rdfs:label "AngularMeasure"@en ;
    rdfs:comment "The abstract notion of angle."@en ;
    rdfs:subClassOf ns1:ISQDimensionlessQuantity,
        ns1:SpaceAndTimeQuantity ;
    owl:disjointWith ns1:Angle ;
    skos:prefLabel "AngularMeasure"@en ;
    ns1:IEVReference "https://www.electropedia.org/iev/iev.nsf/display?openform&ievref=102-04-14"^^xsd:string ;
    ns1:ISO80000Reference "3-5"^^xsd:string ;
    ns1:elucidation "The abstract notion of angle."@en ;
    ns1:iupacReference "https://doi.org/10.1351/goldbook.A00346"^^xsd:string ;
    ns1:qudtReference "https://qudt.org/vocab/quantitykind/Angle"^^xsd:string ;
    ns1:wikidataReference "https://www.wikidata.org/wiki/Q1357788"^^xsd:string .

ns1:AngularReciprocalLatticeVector a owl:Class ;
    rdfs:label "AngularReciprocalLatticeVector"@en ;
    rdfs:comment "Vector whose scalar products with all fundamental lattice vectors are integral multiples of 2pi."@en ;
    rdfs:subClassOf ns1:CondensedMatterPhysicsQuantity,
        ns1:ReciprocalLength ;
    skos:prefLabel "AngularReciprocalLatticeVector"@en ;
    ns1:ISO80000Reference "12-2.1"^^xsd:string ;
    ns1:elucidation "Vector whose scalar products with all fundamental lattice vectors are integral multiples of 2pi."@en ;
    ns1:qudtReference "https://qudt.org/vocab/quantitykind/AngularReciprocalLatticeVector"^^xsd:string ;
    ns1:wikidataReference "https://www.wikidata.org/wiki/Q105475278"^^xsd:string .

ns1:AngularVelocity a owl:Class ;
    rdfs:label "AngularVelocity"@en ;
    rdfs:comment "Axial vector quantity describing the rotation around an axis, with magnitude ω=|dφ/dt|, where dφ is the plane angle change during the infinitesimal time interval with duration dt, and with direction along the axis for which the rotation is clockwise."@en ;
    rdfs:subClassOf [ a owl:Restriction ;
            owl:onProperty ns1:hasMeasurementUnit ;
            owl:someValuesFrom ns1:FrequencyUnit ],
        ns1:ISQDerivedQuantity ;
    skos:prefLabel "AngularVelocity"@en ;
    ns1:IEVReference "https://www.electropedia.org/iev/iev.nsf/display?openform&ievref=113-01-41"^^xsd:string ;
    ns1:ISO80000Reference "3-12"^^xsd:string ;
    ns1:dbpediaReference "https://dbpedia.org/page/Angular_velocity"^^xsd:string ;
    ns1:elucidation "Axial vector quantity describing the rotation around an axis, with magnitude ω=|dφ/dt|, where dφ is the plane angle change during the infinitesimal time interval with duration dt, and with direction along the axis for which the rotation is clockwise."@en ;
    ns1:qudtReference "https://qudt.org/vocab/quantitykind/AngularVelocity"^^xsd:string ;
    ns1:wikipediaReference "https://en.wikipedia.org/wiki/Angular_velocity"^^xsd:string .

ns1:ApparentPower a owl:Class ;
    rdfs:label "ApparentPower"@en ;
    rdfs:comment "RMS value voltage multiplied by rms value of electric current."@en ;
    rdfs:subClassOf ns1:Power ;
    skos:prefLabel "ApparentPower"@en ;
    ns1:IEVReference "https://www.electropedia.org/iev/iev.nsf/display?openform&ievref=131-11-41"^^xsd:string ;
    ns1:ISO80000Reference "6-57"^^xsd:string ;
    ns1:elucidation "RMS value voltage multiplied by rms value of electric current."@en ;
    ns1:qudtReference "https://qudt.org/vocab/quantitykind/ApparentPower"^^xsd:string ;
    ns1:wikidataReference "https://www.wikidata.org/wiki/Q1930258"^^xsd:string .

ns1:AreaDensity a owl:Class ;
    rdfs:label "AreaDensity"@en ;
    rdfs:comment "Mass per unit area."@en ;
    rdfs:subClassOf [ a owl:Restriction ;
            owl:onProperty ns1:hasMeasurementUnit ;
            owl:someValuesFrom ns1:AreaDensityUnit ],
        ns1:ISQDerivedQuantity,
        ns1:Intensive ;
    skos:prefLabel "AreaDensity"@en ;
    ns1:elucidation "Mass per unit area."@en ;
    ns1:iupacReference "https://doi.org/10.1351/goldbook.S06167"^^xsd:string ;
    ns1:qudtReference "http://qudt.org/vocab/quantitykind/SurfaceDensity"^^xsd:string .

ns1:AreaPerQuarticTimeUnit a owl:Class ;
    rdfs:label "AreaPerQuarticTimeUnit"@en ;
    rdfs:comment "The class of units with dimensionality 'AreaPerQuarticTime'."@en .

ns1:AreaPerTemperatureUnit a owl:Class ;
    rdfs:label "AreaPerTemperatureUnit"@en ;
    rdfs:comment "The class of units with dimensionality 'AreaPerTemperature'."@en .

ns1:AreaSquareTimeUnit a owl:Class ;
    rdfs:label "AreaSquareTimeUnit"@en ;
    rdfs:comment "The class of units with dimensionality 'AreaSquareTime'."@en .

ns1:AreaTemperatureUnit a owl:Class ;
    rdfs:label "AreaTemperatureUnit"@en ;
    rdfs:comment "The class of units with dimensionality 'AreaTemperature'."@en .

ns1:AreaTimeUnit a owl:Class ;
    rdfs:label "AreaTimeUnit"@en ;
    rdfs:comment "The class of units with dimensionality 'AreaTime'."@en .

ns1:Array rdfs:label "Array"@en ;
    rdfs:comment "Arrays are ordered mathematical objects who's elementary spatial parts are numbers. Their dimensionality is constructed with spatial direct parthood, where 1-dimensional arrays have spatial direct parts Number and n-dimensional array have spatial direct parts (n-1)-dimensional arrays."@en .

ns1:AtomicAttenuationCoefficient a owl:Class ;
    rdfs:label "AtomicAttenuationCoefficient"@en ;
    rdfs:comment "Quotient of the linear attenuation coefficient µ and the number density, n, of atoms in the substance."@en ;
    rdfs:subClassOf [ a owl:Restriction ;
            owl:onProperty ns1:hasMeasurementUnit ;
            owl:someValuesFrom ns1:AreaUnit ],
        ns1:AtomicAndNuclearPhysicsQuantity,
        ns1:ISQDerivedQuantity ;
    skos:prefLabel "AtomicAttenuationCoefficient"@en ;
    ns1:ISO80000Reference "10-52"^^xsd:string ;
    ns1:elucidation "Quotient of the linear attenuation coefficient µ and the number density, n, of atoms in the substance."@en ;
    ns1:wikidataReference "https://www.wikidata.org/wiki/Q98592911"^^xsd:string .

ns1:AtomicMass a owl:Class ;
    rdfs:label "AtomicMass"@en ;
    rdfs:comment "Since the nucleus account for nearly all of the total mass of atoms  (with the electrons and nuclear binding energy making minor contributions), the atomic mass measured in Da has nearly the same value as the mass number."@en,
        "The atomic mass is often expressed as an average of the commonly found isotopes."@en,
        "The mass of an atom in the ground state."@en ;
    rdfs:subClassOf [ a owl:Restriction ;
            owl:allValuesFrom ns1:Atom ;
            owl:onProperty [ owl:inverseOf ns1:hasProperty ] ],
        ns1:Mass ;
    skos:prefLabel "AtomicMass"@en ;
    ns1:ISO80000Reference "10-4.1"^^xsd:string ;
    ns1:definition "The mass of an atom in the ground state."@en ;
    ns1:iupacReference "https://doi.org/10.1351/goldbook.A00496"^^xsd:string ;
    ns1:wikipediaReference "https://en.wikipedia.org/wiki/Atomic_mass"^^xsd:string .

ns1:AtomicNumber a owl:Class ;
    rdfs:label "AtomicNumber"@en ;
    rdfs:comment "Number of protons in an atomic nucleus."@en ;
    rdfs:subClassOf [ a owl:Restriction ;
            owl:allValuesFrom ns1:Atom ;
            owl:onProperty [ owl:inverseOf ns1:hasProperty ] ],
        ns1:IntegerData,
        ns1:PureNumberQuantity ;
    skos:prefLabel "AtomicNumber"@en ;
    ns1:ISO80000Reference "10-1.1"^^xsd:string ;
    ns1:elucidation "Number of protons in an atomic nucleus."@en ;
    ns1:iupacReference "https://doi.org/10.1351/goldbook.A00499"^^xsd:string ;
    ns1:qudtReference "http://qudt.org/vocab/quantitykind/AtomicNumber"^^xsd:string .

ns1:AtomicScatteringFactor a owl:Class ;
    rdfs:label "AtomicScatteringFactor"@en ;
    rdfs:comment "Quotient of radiation amplitude scattered by the atom and radiation amplitude scattered by a single electron."@en ;
    rdfs:subClassOf ns1:CondensedMatterPhysicsQuantity,
        ns1:RatioQuantity ;
    skos:prefLabel "AtomicScatteringFactor"@en ;
    ns1:ISO80000Reference "12-5.3"^^xsd:string ;
    ns1:elucidation "Quotient of radiation amplitude scattered by the atom and radiation amplitude scattered by a single electron."@en ;
    ns1:qudtReference "https://qudt.org/vocab/quantitykind/AtomScatteringFactor"^^xsd:string ;
    ns1:wikidataReference "https://www.wikidata.org/wiki/Q837866"^^xsd:string ;
    ns1:wikipediaReference "https://en.wikipedia.org/wiki/Atomic_form_factor"^^xsd:string .

ns1:Attenuation a owl:Class ;
    rdfs:label "Attenuation"@en ;
    rdfs:comment "Decrease in magnitude of any kind of flux through a medium."@en ;
    rdfs:subClassOf ns1:ReciprocalLength,
        ns1:SpaceAndTimeQuantity ;
    skos:altLabel "Extinction"@en ;
    skos:prefLabel "Attenuation"@en ;
    ns1:ISO80000Reference "3-26.1"^^xsd:string ;
    ns1:elucidation "Decrease in magnitude of any kind of flux through a medium."@en ;
    ns1:iupacReference "https://doi.org/10.1351/goldbook.A00515"^^xsd:string ;
    ns1:wikipediaReference "https://en.wikipedia.org/wiki/Attenuation"^^xsd:string .

ns1:AverageEnergyLossPerElementaryChargeProduced a owl:Class ;
    rdfs:label "AverageEnergyLossPerElementaryChargeProduced"@en ;
    rdfs:comment "Quotient of the initial kinetic energy Ek of an ionizing charged particle and the total ionization Ni produced by that particle."@en ;
    rdfs:subClassOf ns1:AtomicAndNuclearPhysicsQuantity,
        ns1:Energy ;
    skos:prefLabel "AverageEnergyLossPerElementaryChargeProduced"@en ;
    ns1:ISO80000Reference "10-60"^^xsd:string ;
    ns1:elucidation "Quotient of the initial kinetic energy Ek of an ionizing charged particle and the total ionization Ni produced by that particle."@en ;
    ns1:qudtReference "https://qudt.org/vocab/quantitykind/AverageEnergyLossPerElementaryChargeProduced"^^xsd:string ;
    ns1:wikidataReference "https://www.wikidata.org/wiki/Q98793042"^^xsd:string .

ns1:AverageLogarithmicEnergyDecrement a owl:Class ;
    rdfs:label "AverageLogarithmicEnergyDecrement"@en ;
    rdfs:comment "Average value of the increment of the lethargy per collision."@en ;
    rdfs:subClassOf ns1:AtomicAndNuclearPhysicsQuantity,
        ns1:ISQDimensionlessQuantity ;
    skos:prefLabel "AverageLogarithmicEnergyDecrement"@en ;
    ns1:IEVReference "https://www.electropedia.org/iev/iev.nsf/display?openform&ievref=395-07-02"^^xsd:string ;
    ns1:ISO80000Reference "10-70"^^xsd:string ;
    ns1:elucidation "Average value of the increment of the lethargy per collision."@en ;
    ns1:qudtReference "https://qudt.org/vocab/quantitykind/AverageLogarithmicEnergyDecrement.html"^^xsd:string ;
    ns1:wikidataReference "https://www.wikidata.org/wiki/Q1940739"^^xsd:string .

ns1:AvogadroConstant a owl:Class ;
    rdfs:label "AvogadroConstant"@en ;
    rdfs:comment "The DBpedia definition (http://dbpedia.org/page/Avogadro_constant) is outdated as May 20, 2019. It is now an exact quantity."@en,
        """The number of constituent particles, usually atoms or molecules, that are contained in the amount of substance given by one mole.

It defines the base unit mole in the SI system."""@en ;
    rdfs:subClassOf [ a owl:Restriction ;
            owl:onProperty ns1:hasMeasurementUnit ;
            owl:someValuesFrom ns1:PerAmountUnit ],
        ns1:SIExactConstant ;
    skos:prefLabel "AvogadroConstant"@en ;
    ns1:elucidation """The number of constituent particles, usually atoms or molecules, that are contained in the amount of substance given by one mole.

It defines the base unit mole in the SI system."""@en ;
    ns1:iupacReference "https://doi.org/10.1351/goldbook.A00543"^^xsd:string ;
    ns1:qudtReference "http://qudt.org/vocab/constant/AvogadroConstant"^^xsd:string .

ns1:BetaDisintegrationEnergy a owl:Class ;
    rdfs:label "BetaDisintegrationEnergy"@en ;
    rdfs:comment "Sum of the maximum beta-particle kinetic energy and the recoil energy of the atom produced in a reference frame in which the emitting nucleus is at rest before its disintegration."@en ;
    rdfs:subClassOf ns1:AtomicAndNuclearPhysicsQuantity,
        ns1:Energy ;
    skos:prefLabel "BetaDisintegrationEnergy"@en ;
    ns1:ISO80000Reference "10-34"^^xsd:string ;
    ns1:elucidation "Sum of the maximum beta-particle kinetic energy and the recoil energy of the atom produced in a reference frame in which the emitting nucleus is at rest before its disintegration."@en ;
    ns1:wikidataReference "https://www.wikidata.org/wiki/Q98148340"^^xsd:string .

ns1:BindingFraction a owl:Class ;
    rdfs:label "BindingFraction"@en ;
    rdfs:comment "The ratio of the binding energy of a nucleus to the atomic mass number."@en ;
    rdfs:subClassOf ns1:AtomicAndNuclearPhysicsQuantity,
        ns1:ISQDimensionlessQuantity ;
    skos:prefLabel "BindingFraction"@en ;
    ns1:ISO80000Reference "10-23.2"^^xsd:string ;
    ns1:elucidation "The ratio of the binding energy of a nucleus to the atomic mass number."@en ;
    ns1:qudtReference "https://qudt.org/vocab/quantitykind/BindingFraction"^^xsd:string ;
    ns1:wikidataReference "https://www.wikidata.org/wiki/Q98058362"^^xsd:string .

ns1:BohrMagneton a owl:Class ;
    rdfs:label "BohrMagneton"^^xsd:string ;
    rdfs:comment "Magnitude of the magnetic moment of an electron in a state with orbital angular momentum quantum number l=1 due to its orbital motion."@en ;
    rdfs:subClassOf [ a owl:Restriction ;
            owl:onProperty ns1:hasMeasurementUnit ;
            owl:someValuesFrom ns1:MagneticDipoleMomentUnit ],
        ns1:AtomicAndNuclearPhysicsQuantity,
        ns1:ISQDerivedQuantity ;
    skos:prefLabel "BohrMagneton"^^xsd:string ;
    ns1:ISO80000Reference "10-9.2"^^xsd:string ;
    ns1:elucidation "Magnitude of the magnetic moment of an electron in a state with orbital angular momentum quantum number l=1 due to its orbital motion."@en ;
    ns1:wikidataReference "https://www.wikidata.org/wiki/Q737120"^^xsd:string .

ns1:BohrRadius a owl:Class ;
    rdfs:label "BohrRadius"^^xsd:string ;
    rdfs:comment "Radius of the electron orbital in the hydrogen atom in its ground state in the Bohr model of the atom."@en ;
    rdfs:subClassOf ns1:AtomicAndNuclearPhysicsQuantity,
        ns1:Radius ;
    skos:prefLabel "BohrRadius"^^xsd:string ;
    ns1:ISO80000Reference "10-6"^^xsd:string ;
    ns1:elucidation "Radius of the electron orbital in the hydrogen atom in its ground state in the Bohr model of the atom."@en ;
    ns1:iupacReference "https://doi.org/10.1351/goldbook.B00693"^^xsd:string ;
    ns1:qudtReference "https://qudt.org/vocab/constant/BohrRadius"^^xsd:string ;
    ns1:wikidataReference "https://www.wikidata.org/wiki/Q652571"^^xsd:string .

ns1:BoltzmannConstant a owl:Class ;
    rdfs:label "BoltzmannConstant"@en ;
    rdfs:comment """A physical constant relating energy at the individual particle level with temperature. It is the gas constant R divided by the Avogadro constant.

It defines the Kelvin unit in the SI system."""@en,
        "The DBpedia definition (http://dbpedia.org/page/Boltzmann_constant) is outdated as May 20, 2019. It is now an exact quantity."@en ;
    rdfs:subClassOf ns1:Entropy,
        ns1:SIExactConstant ;
    skos:prefLabel "BoltzmannConstant"@en ;
    ns1:elucidation """A physical constant relating energy at the individual particle level with temperature. It is the gas constant R divided by the Avogadro constant.

It defines the Kelvin unit in the SI system."""@en ;
    ns1:iupacReference "https://doi.org/10.1351/goldbook.B00695"^^xsd:string ;
    ns1:qudtReference "http://qudt.org/vocab/constant/BoltzmannConstant"^^xsd:string .

ns1:BraggAngle a owl:Class ;
    rdfs:label "BraggAngle"@en ;
    rdfs:comment "Angle between the scattered ray and the lattice plane."@en ;
    rdfs:subClassOf ns1:Angle,
        ns1:CondensedMatterPhysicsQuantity ;
    skos:prefLabel "BraggAngle"@en ;
    ns1:ISO80000Reference "12-4"^^xsd:string ;
    ns1:elucidation "Angle between the scattered ray and the lattice plane."@en ;
    ns1:qudtReference "https://qudt.org/vocab/quantitykind/BraggAngle"^^xsd:string ;
    ns1:wikidataReference "https://www.wikidata.org/wiki/Q105488118"^^xsd:string .

ns1:BurgersVector a owl:Class ;
    rdfs:label "BurgersVector"@en ;
    rdfs:comment "Vector characterising a dislocation in a crystal lattice."@en ;
    rdfs:subClassOf [ a owl:Restriction ;
            owl:onProperty ns1:hasMeasurementUnit ;
            owl:someValuesFrom ns1:LengthUnit ],
        ns1:CondensedMatterPhysicsQuantity,
        ns1:Displacement ;
    skos:prefLabel "BurgersVector"@en ;
    ns1:ISO80000Reference "12-6"^^xsd:string ;
    ns1:elucidation "Vector characterising a dislocation in a crystal lattice."@en ;
    ns1:qudtReference "https://qudt.org/vocab/quantitykind/BurgersVector"^^xsd:string ;
    ns1:wikidataReference "https://www.wikidata.org/wiki/Q623093"^^xsd:string .

ns1:CanonicalPartitionFunction a owl:Class ;
    rdfs:label "CanonicalPartitionFunction"@en ;
    rdfs:comment "Sum over quantum states of energy in a system in equilibrium."@en ;
    rdfs:subClassOf ns1:ISQDimensionlessQuantity,
        ns1:PhysioChemicalQuantity ;
    skos:prefLabel "CanonicalPartitionFunction"@en ;
    ns1:ISO80000Reference "9-35.2"^^xsd:string ;
    ns1:elucidation "Sum over quantum states of energy in a system in equilibrium."@en ;
    ns1:note "In physics, a partition function describes the statistical properties of a system in thermodynamic equilibrium. Partition functions are functions of the thermodynamic state variables, such as the temperature and volume. Most of the aggregate thermodynamic variables of the system, such as the total energy, free energy, entropy, and pressure, can be expressed in terms of the partition function or its derivatives. The partition function is dimensionless."@en ;
    ns1:qudtReference "https://qudt.org/vocab/quantitykind/CanonicalPartitionFunction"^^xsd:string ;
    ns1:wikidataReference "https://www.wikidata.org/wiki/Q96142389"^^xsd:string .

ns1:Capacitance a owl:Class ;
    rdfs:label "Capacitance"@en ;
    rdfs:comment "The derivative of the electric charge of a system with respect to the electric potential."@en ;
    rdfs:subClassOf [ a owl:Restriction ;
            owl:onProperty ns1:hasMeasurementUnit ;
            owl:someValuesFrom ns1:CapacitanceUnit ],
        ns1:ElectromagneticQuantity,
        ns1:ISQDerivedQuantity ;
    skos:altLabel "ElectricCapacitance"@en ;
    skos:prefLabel "Capacitance"@en ;
    ns1:ISO80000Reference "6-13"^^xsd:string ;
    ns1:elucidation "The derivative of the electric charge of a system with respect to the electric potential."@en ;
    ns1:iupacReference "https://doi.org/10.1351/goldbook.C00791"^^xsd:string ;
    ns1:qudtReference "http://qudt.org/vocab/quantitykind/Capacitance"^^xsd:string .

ns1:CapacitancePerLengthUnit a owl:Class ;
    rdfs:label "CapacitancePerLengthUnit"@en ;
    rdfs:comment "The class of units with dimensionality 'CapacitancePerLength'."@en .

ns1:CarrierLifetime a owl:Class ;
    rdfs:label "CarrierLifetime"@en ;
    rdfs:comment "Time constant for recombination or trapping of minority charge carriers in semiconductors"@en ;
    rdfs:subClassOf ns1:CondensedMatterPhysicsQuantity,
        ns1:TimeConstant ;
    skos:prefLabel "CarrierLifetime"@en ;
    ns1:ISO80000Reference "12-32.2"^^xsd:string ;
    ns1:elucidation "Time constant for recombination or trapping of minority charge carriers in semiconductors"@en ;
    ns1:qudtReference "https://qudt.org/vocab/quantitykind/CarrierLifetime"^^xsd:string ;
    ns1:wikidataReference "https://www.wikidata.org/wiki/Q5046374"^^xsd:string .

ns1:CatalyticActivity a owl:Class ;
    rdfs:label "CatalyticActivity"@en ;
    rdfs:comment "Increase in the rate of reaction of a specified chemical reaction that an enzyme produces in a specific assay system."@en ;
    rdfs:subClassOf [ a owl:Restriction ;
            owl:onProperty ns1:hasMeasurementUnit ;
            owl:someValuesFrom ns1:CatalyticActivityUnit ],
        ns1:ISQDerivedQuantity,
        ns1:Intensive ;
    skos:prefLabel "CatalyticActivity"@en ;
    ns1:elucidation "Increase in the rate of reaction of a specified chemical reaction that an enzyme produces in a specific assay system."@en ;
    ns1:iupacReference "https://doi.org/10.1351/goldbook.C00881"^^xsd:string ;
    ns1:qudtReference "http://qudt.org/vocab/quantitykind/CatalyticActivity"^^xsd:string .

ns1:CelsiusTemperature a owl:Class ;
    rdfs:label "CelsiusTemperature"@en ;
    rdfs:comment """An objective comparative measure of hot or cold.

Temperature is a relative quantity that can be used to express temperature differences. Unlike ThermodynamicTemperature, it cannot express absolute temperatures."""@en ;
    rdfs:subClassOf [ a owl:Restriction ;
            owl:onProperty ns1:hasMeasurementUnit ;
            owl:someValuesFrom ns1:TemperatureUnit ],
        ns1:ISQDerivedQuantity,
        ns1:Intensive ;
    skos:prefLabel "CelsiusTemperature"@en ;
    ns1:ISO80000Reference "5-2"^^xsd:string ;
    ns1:elucidation """An objective comparative measure of hot or cold.

Temperature is a relative quantity that can be used to express temperature differences. Unlike ThermodynamicTemperature, it cannot express absolute temperatures."""@en ;
    ns1:iupacReference "https://doi.org/10.1351/goldbook.T06261"^^xsd:string ;
    ns1:qudtReference "http://qudt.org/vocab/quantitykind/CelciusTemperature"^^xsd:string .

ns1:CentreOfMass a owl:Class ;
    rdfs:label "CentreOfMass"@en ;
    rdfs:comment "In non-relativistic physics, the centre of mass doesn’t depend on the chosen reference frame."@en,
        "The unique point where the weighted relative position of the distributed mass of an Item sums to zero. Equivalently, it is the point where if a force is applied to the Item, causes the Item to move in direction of force without rotation."@en ;
    rdfs:subClassOf ns1:PositionVector ;
    skos:prefLabel "CentreOfMass"@en ;
    ns1:elucidation "The unique point where the weighted relative position of the distributed mass of an Item sums to zero. Equivalently, it is the point where if a force is applied to the Item, causes the Item to move in direction of force without rotation."@en ;
    ns1:wikipediaReference "https://en.wikipedia.org/wiki/Center_of_mass"^^xsd:string .

ns1:ChemicalCompositionQuantity rdfs:label "ChemicalCompositionQuantity"@en .

ns1:ChemicalPotential a owl:Class ;
    rdfs:label "ChemicalPotential"@en ;
    rdfs:comment "Energy per unit change in amount of substance."@en ;
    rdfs:subClassOf [ a owl:Restriction ;
            owl:onProperty ns1:hasMeasurementUnit ;
            owl:someValuesFrom ns1:EnergyPerAmountUnit ],
        ns1:ISQDerivedQuantity ;
    skos:prefLabel "ChemicalPotential"@en ;
    ns1:ISO80000Reference "9-17"^^xsd:string ;
    ns1:elucidation "Energy per unit change in amount of substance."@en ;
    ns1:iupacReference "https://doi.org/10.1351/goldbook.C01032"^^xsd:string ;
    ns1:qudtReference "http://qudt.org/vocab/quantitykind/ChemicalPotential"^^xsd:string .

ns1:Coercivity a owl:Class ;
    rdfs:label "Coercivity"@en ;
    rdfs:comment "Coercive field strength in a substance when either the magnetic flux density or the magnetic polarization and magnetization is brought from its value at magnetic saturation to zero by monotonic reduction of the applied magnetic field strength."@en ;
    rdfs:subClassOf [ a owl:Restriction ;
            owl:onProperty ns1:hasMeasurementUnit ;
            owl:someValuesFrom ns1:MagneticFieldStrengthUnit ],
        ns1:ElectromagneticQuantity,
        ns1:ISQDerivedQuantity ;
    skos:prefLabel "Coercivity"@en ;
    ns1:IEVReference "https://www.electropedia.org/iev/iev.nsf/display?openform&ievref=121-12-69"^^xsd:string ;
    ns1:ISO80000Reference "6-31"^^xsd:string ;
    ns1:elucidation "Coercive field strength in a substance when either the magnetic flux density or the magnetic polarization and magnetization is brought from its value at magnetic saturation to zero by monotonic reduction of the applied magnetic field strength."@en ;
    ns1:qudtReference "https://qudt.org/vocab/quantitykind/Coercivity"^^xsd:string ;
    ns1:wikidataReference "https://www.wikidata.org/wiki/Q432635"^^xsd:string .

ns1:CoherenceLength a owl:Class ;
    rdfs:label "CoherenceLength"@en ;
    rdfs:comment "Distance in a superconductor over which the effect of a perturbation is appreciable at zero thermodynamic temperature"@en ;
    rdfs:subClassOf ns1:CondensedMatterPhysicsQuantity,
        ns1:Length ;
    skos:prefLabel "CoherenceLength"@en ;
    ns1:ISO80000Reference "12-38.2"^^xsd:string ;
    ns1:elucidation "Distance in a superconductor over which the effect of a perturbation is appreciable at zero thermodynamic temperature"@en ;
    ns1:wikidataReference "https://www.wikidata.org/wiki/Q1778793"^^xsd:string .

ns1:ComplexPower a owl:Class ;
    rdfs:label "ComplexPower"@en ;
    rdfs:comment "Voltage phasor multiplied by complex conjugate of the current phasor."@en ;
    rdfs:subClassOf ns1:Power ;
    skos:altLabel "ComplexApparentPower"@en ;
    skos:prefLabel "ComplexPower"@en ;
    ns1:IEVReference "https://www.electropedia.org/iev/iev.nsf/display?openform&ievref=131-11-39"^^xsd:string ;
    ns1:ISO80000Reference "6-59"^^xsd:string ;
    ns1:elucidation "Voltage phasor multiplied by complex conjugate of the current phasor."@en ;
    ns1:qudtReference "https://qudt.org/vocab/quantitykind/ComplexPower"^^xsd:string ;
    ns1:wikidataReference "https://www.wikidata.org/wiki/Q65239736"^^xsd:string .

ns1:ComptonWavelength a owl:Class ;
    rdfs:label "ComptonWavelength"@en ;
    rdfs:comment "Quotient of the Planck constant and the product of the mass of the particle and the speed of light in vacuum."@en ;
    rdfs:subClassOf ns1:AtomicAndNuclearPhysicsQuantity,
        ns1:Wavelength ;
    skos:prefLabel "ComptonWavelength"@en ;
    ns1:ISO80000Reference "10-20"^^xsd:string ;
    ns1:elucidation "Quotient of the Planck constant and the product of the mass of the particle and the speed of light in vacuum."@en ;
    ns1:qudtReference "https://qudt.org/vocab/constant/ComptonWavelength"^^xsd:string ;
    ns1:wikidataReference "https://www.wikidata.org/wiki/Q1145377"^^xsd:string ;
    ns1:wikipediaReference "https://en.wikipedia.org/wiki/Compton_wavelength"^^xsd:string .

ns1:ConductanceForAlternatingCurrent a owl:Class ;
    rdfs:label "ConductanceForAlternatingCurrent"@en ;
    rdfs:comment "Real part of the admittance."@en ;
    rdfs:subClassOf ns1:ElectricConductance ;
    skos:prefLabel "ConductanceForAlternatingCurrent"@en ;
    ns1:IEVReference "https://www.electropedia.org/iev/iev.nsf/display?openform&ievref=131-12-53"^^xsd:string ;
    ns1:ISO80000Reference "6-52.2"^^xsd:string ;
    ns1:elucidation "Real part of the admittance."@en ;
    ns1:wikidataReference "https://www.wikidata.org/wiki/Q79464628"^^xsd:string .

ns1:CouplingFactor a owl:Class ;
    rdfs:label "CouplingFactor"@en ;
    rdfs:comment "Ratio of the absolute value of the mutual permeance related to two circuit elements  to the geometric average of their self-permeances."@en ;
    rdfs:subClassOf ns1:ElectromagneticQuantity,
        ns1:ISQDimensionlessQuantity ;
    skos:altLabel "InductiveCouplingFactor"@en ;
    skos:prefLabel "CouplingFactor"@en ;
    ns1:IEVReference "https://www.electropedia.org/iev/iev.nsf/display?openform&ievref=131-12-41"^^xsd:string ;
    ns1:ISO80000Reference "6-42.1"^^xsd:string ;
    ns1:elucidation "Ratio of the absolute value of the mutual permeance related to two circuit elements  to the geometric average of their self-permeances."@en ;
    ns1:wikidataReference "https://www.wikidata.org/wiki/Q78101715"^^xsd:string .

ns1:CubicElectricChargeLengthPerSquareEnergyUnit a owl:Class ;
    rdfs:label "CubicElectricChargeLengthPerSquareEnergyUnit"@en ;
    rdfs:comment "The class of units with dimensionality 'CubicElectricChargeLengthPerSquareEnergy'."@en .

ns1:CubicExpansionCoefficient a owl:Class ;
    rdfs:label "CubicExpansionCoefficient"@en ;
    rdfs:comment "Quantity characterizing the variation with thermodynamic temperature T of the volume V of a body, under given conditions."@en,
        "alpha_V = (1/V) * (dV/dT)"@en ;
    rdfs:subClassOf ns1:CoefficientOfThermalExpansion,
        ns1:ThermodynamicalQuantity ;
    owl:disjointWith ns1:LinearExpansionCoefficient ;
    skos:prefLabel "CubicExpansionCoefficient"@en ;
    ns1:IEVReference "https://www.electropedia.org/iev/iev.nsf/display?openform&ievref=113-04-28"@en ;
    ns1:ISO80000Reference "5-3.2"^^xsd:string ;
    ns1:elucidation "Quantity characterizing the variation with thermodynamic temperature T of the volume V of a body, under given conditions."@en ;
    ns1:qudtReference "https://qudt.org/vocab/quantitykind/CubicExpansionCoefficient"^^xsd:string ;
    ns1:wikidataReference "https://www.wikidata.org/wiki/Q74761076"^^xsd:string .

ns1:CurieTemperature a owl:Class ;
    rdfs:label "CurieTemperature"@en ;
    rdfs:comment "Critical thermodynamic temperature of a ferromagnet."@en ;
    rdfs:subClassOf ns1:CondensedMatterPhysicsQuantity,
        ns1:CriticalTemperature ;
    skos:prefLabel "CurieTemperature"@en ;
    ns1:IEVReference "https://www.electropedia.org/iev/iev.nsf/display?openform&ievref=121-12-51"^^xsd:string ;
    ns1:ISO80000Reference "12-35.1"^^xsd:string ;
    ns1:elucidation "Critical thermodynamic temperature of a ferromagnet."@en ;
    ns1:qudtReference "https://qudt.org/vocab/quantitykind/CurieTemperature"^^xsd:string ;
    ns1:wikidataReference "https://www.wikidata.org/wiki/Q191073"^^xsd:string .

ns1:CurrentLinkage a owl:Class ;
    rdfs:label "CurrentLinkage"@en ;
    rdfs:comment "For a closed path, scalar quantity equal to the electric current through any surface bounded by the path."@en ;
    rdfs:subClassOf ns1:ElectricCurrent ;
    skos:prefLabel "CurrentLinkage"@en ;
    ns1:IEVReference "https://www.electropedia.org/iev/iev.nsf/display?openform&ievref=121-11-46"^^xsd:string ;
    ns1:ISO80000Reference "6-37.4"^^xsd:string ;
    ns1:elucidation "For a closed path, scalar quantity equal to the electric current through any surface bounded by the path."@en ;
    ns1:qudtReference "https://qudt.org/vocab/quantitykind/CurrentLinkage"^^xsd:string ;
    ns1:wikidataReference "https://www.wikidata.org/wiki/Q77995703"^^xsd:string .

ns1:Curvature a owl:Class ;
    rdfs:label "Curvature"@en ;
    rdfs:comment "Inverse of the radius of curvature."@en ;
    rdfs:subClassOf ns1:ReciprocalLength,
        ns1:SpaceAndTimeQuantity ;
    skos:prefLabel "Curvature"@en ;
    ns1:IEVReference "https://www.electropedia.org/iev/iev.nsf/display?openform&ievref=113-01-31"^^xsd:string ;
    ns1:ISO80000Reference "3-2"^^xsd:string ;
    ns1:dbpediaReference "https://dbpedia.org/page/Curvature"^^xsd:string ;
    ns1:elucidation "Inverse of the radius of curvature."@en ;
    ns1:qudtReference "https://qudt.org/vocab/quantitykind/CurvatureFromRadius"^^xsd:string ;
    ns1:wikidataReference "https://www.wikidata.org/wiki/Q214881"^^xsd:string .

ns1:CyclotronAngularFrequency a owl:Class ;
    rdfs:label "CyclotronAngularFrequency"@en ;
    rdfs:comment "Quotient of the product of the electric charge of a particle and the magnitude of the magnetic flux density of the magnetic field, and the particle mass."@en ;
    rdfs:subClassOf ns1:AngularFrequency,
        ns1:AtomicAndNuclearPhysicsQuantity ;
    skos:prefLabel "CyclotronAngularFrequency"@en ;
    ns1:ISO80000Reference "10-16"^^xsd:string ;
    ns1:elucidation "Quotient of the product of the electric charge of a particle and the magnitude of the magnetic flux density of the magnetic field, and the particle mass."@en ;
    ns1:qudtReference "https://qudt.org/vocab/quantitykind/CyclotronAngularFrequency"^^xsd:string ;
    ns1:wikidataReference "https://www.wikidata.org/wiki/Q97708211"^^xsd:string .

ns1:DampingCoefficient a owl:Class ;
    rdfs:label "DampingCoefficient"@en ;
    rdfs:comment "Inverse of the time constant of an exponentially varying quantity."@en ;
    rdfs:subClassOf ns1:Rate ;
    skos:prefLabel "DampingCoefficient"@en ;
    ns1:IEVReference "https://www.electropedia.org/iev/iev.nsf/display?openform&ievref=103-05-24"^^xsd:string ;
    ns1:ISO80000Reference "3-24"^^xsd:string ;
    ns1:elucidation "Inverse of the time constant of an exponentially varying quantity."@en .

ns1:DebyeAngularFrequency a owl:Class ;
    rdfs:label "DebyeAngularFrequency"@en ;
    rdfs:comment "Cut-off angular frequency in the Debye model of the vibrational spectrum of a solid."@en ;
    rdfs:subClassOf ns1:AngularFrequency,
        ns1:CondensedMatterPhysicsQuantity ;
    skos:prefLabel "DebyeAngularFrequency"@en ;
    ns1:ISO80000Reference "12-10"^^xsd:string ;
    ns1:elucidation "Cut-off angular frequency in the Debye model of the vibrational spectrum of a solid."@en ;
    ns1:qudtReference "https://qudt.org/vocab/quantitykind/DebyeAngularFrequency"^^xsd:string ;
    ns1:wikidataReference "https://www.wikidata.org/wiki/Q105580986"^^xsd:string .

ns1:DebyeAngularWaveNumber a owl:Class ;
    rdfs:label "DebyeAngularWaveNumber"@en ;
    rdfs:comment "Cut-off angular wavenumber in the Debye model of the vibrational spectrum of a solid."@en ;
    rdfs:subClassOf ns1:AngularWaveNumber,
        ns1:CondensedMatterPhysicsQuantity ;
    skos:altLabel "DebyeAngluarRepetency"@en ;
    skos:prefLabel "DebyeAngularWaveNumber"@en ;
    ns1:ISO80000Reference "12-9.3"^^xsd:string ;
    ns1:elucidation "Cut-off angular wavenumber in the Debye model of the vibrational spectrum of a solid."@en ;
    ns1:qudtReference "https://qudt.org/vocab/quantitykind/DebyeAngularWavenumber"^^xsd:string ;
    ns1:wikidataReference "https://www.wikidata.org/wiki/Q105554370"^^xsd:string .

ns1:DebyeTemperature a owl:Class ;
    rdfs:label "DebyeTemperature"@en ;
    rdfs:subClassOf ns1:CondensedMatterPhysicsQuantity,
        ns1:ThermodynamicTemperature ;
    skos:prefLabel "DebyeTemperature"@en ;
    ns1:ISO80000Reference "12-11"^^xsd:string ;
    ns1:qudtReference "https://qudt.org/vocab/quantitykind/DebyeTemperature"^^xsd:string ;
    ns1:wikidataReference "https://www.wikidata.org/wiki/Q3517821"^^xsd:string .

ns1:DebyeWallerFactor a owl:Class ;
    rdfs:label "DebyeWallerFactor"@en ;
    rdfs:comment "Factor by which the intensity of a diffraction line is reduced because of the lattice vibrations."@en ;
    rdfs:subClassOf ns1:CondensedMatterPhysicsQuantity,
        ns1:ISQDimensionlessQuantity ;
    skos:prefLabel "DebyeWallerFactor"@en ;
    ns1:ISO80000Reference "12-8"^^xsd:string ;
    ns1:elucidation "Factor by which the intensity of a diffraction line is reduced because of the lattice vibrations."@en ;
    ns1:qudtReference "https://qudt.org/vocab/quantitykind/Debye-WallerFactor"^^xsd:string ;
    ns1:wikidataReference "https://www.wikidata.org/wiki/Q902587"^^xsd:string .

ns1:DecayConstant a owl:Class ;
    rdfs:label "DecayConstant"@en ;
    rdfs:comment "Disintegrations per unit time dN/dt for an atomic nucleus divided by the number of nuclei N existing at the same time t."@en ;
    rdfs:subClassOf [ a owl:Restriction ;
            owl:onProperty ns1:hasMeasurementUnit ;
            owl:someValuesFrom ns1:FrequencyUnit ],
        ns1:AtomicAndNuclearPhysicsQuantity,
        ns1:ISQDerivedQuantity ;
    skos:altLabel "DisintegrationConstant"@en ;
    skos:prefLabel "DecayConstant"@en ;
    ns1:IEVReference "https://www.electropedia.org/iev/iev.nsf/display?openform&ievref=395-01-11"^^xsd:string ;
    ns1:ISO80000Reference "10-24"^^xsd:string ;
    ns1:elucidation "Disintegrations per unit time dN/dt for an atomic nucleus divided by the number of nuclei N existing at the same time t."@en ;
    ns1:iupacReference "https://doi.org/10.1351/goldbook.D01538"^^xsd:string ;
    ns1:qudtReference "https://qudt.org/vocab/quantitykind/DecayConstant"^^xsd:string ;
    ns1:wikidataReference "https://www.wikidata.org/wiki/Q11477200"^^xsd:string .

ns1:Degenerency a owl:Class ;
    rdfs:label "Degenerency"@en ;
    rdfs:comment "For a quantum level, the statistical weight of that level."@en ;
    rdfs:subClassOf ns1:ISQDimensionlessQuantity,
        ns1:PhysioChemicalQuantity ;
    skos:altLabel "Multiplicity"@en ;
    skos:prefLabel "Degenerency"@en ;
    ns1:ISO80000Reference "9-36.2"^^xsd:string ;
    ns1:elucidation "For a quantum level, the statistical weight of that level."@en ;
    ns1:iupacReference "https://doi.org/10.1351/goldbook.D01556"^^xsd:string ;
    ns1:wikidataReference "https://www.wikidata.org/wiki/Q902301"^^xsd:string .

ns1:DegreeOfDissociation a owl:Class ;
    rdfs:label "DegreeOfDissociation"@en ;
    rdfs:comment "Dissociation may occur stepwise."@en,
        "Ratio of the number of dissociation events to the maximum number of theoretically possible dissociation events."@en ;
    rdfs:subClassOf ns1:ISQDimensionlessQuantity,
        ns1:PhysioChemicalQuantity ;
    skos:altLabel "DissociationFraction"@en ;
    skos:prefLabel "DegreeOfDissociation"@en ;
    ns1:IEVReference "https://www.electropedia.org/iev/iev.nsf/display?openform&ievref=114-01-09"@en ;
    ns1:ISO80000Reference "9-43"^^xsd:string ;
    ns1:elucidation "Ratio of the number of dissociation events to the maximum number of theoretically possible dissociation events."@en ;
    ns1:iupacReference "https://doi.org/10.1351/goldbook.D01566"^^xsd:string ;
    ns1:qudtReference "https://qudt.org/vocab/quantitykind/DegreeOfDissociation"^^xsd:string ;
    ns1:wikidataReference "https://www.wikidata.org/wiki/Q907334"^^xsd:string .

ns1:DewPointTemperature a owl:Class ;
    rdfs:label "DewPointTemperature"@en ;
    rdfs:comment "The corresponding Celsius temperature is denoted td and is also called dew point."@en,
        "Thermodynamic temperature at which vapour in air reaches saturation."@en ;
    rdfs:subClassOf ns1:ThermodynamicTemperature,
        ns1:ThermodynamicalQuantity ;
    skos:prefLabel "DewPointTemperature"@en ;
    ns1:IEVReference "https://www.electropedia.org/iev/iev.nsf/display?openform&ievref=113-04-67"^^xsd:string ;
    ns1:ISO80000Reference "5-36"^^xsd:string ;
    ns1:elucidation "Thermodynamic temperature at which vapour in air reaches saturation."@en ;
    ns1:iupacReference "https://doi.org/10.1351/goldbook.D01652"^^xsd:string ;
    ns1:wikidataReference "https://www.wikidata.org/wiki/Q178828"^^xsd:string .

ns1:Diameter a owl:Class ;
    rdfs:label "Diameter"@en ;
    rdfs:comment "The diameter of a circle or a sphere is twice its radius."^^xsd:string,
        "maximal distance of two points of an object, in a given direction or along a straight line passing through the centre."@en ;
    rdfs:subClassOf ns1:Length ;
    skos:prefLabel "Diameter"@en ;
    ns1:IEVReference "https://www.electropedia.org/iev/iev.nsf/display?openform&ievref=113-01-27"^^xsd:string ;
    ns1:ISO80000Reference "3-1.5"^^xsd:string ;
    ns1:dbpediaReference "https://dbpedia.org/page/Diameter"^^xsd:string ;
    ns1:elucidation "maximal distance of two points of an object, in a given direction or along a straight line passing through the centre."@en ;
    ns1:qudtReference "https://qudt.org/vocab/quantitykind/Diameter"^^xsd:string ;
    ns1:wikipediaReference "https://en.wikipedia.org/wiki/Diameter"^^xsd:string .

ns1:DiffusionArea a owl:Class ;
    rdfs:label "DiffusionArea"@en ;
    rdfs:comment "One-sixth of the mean square distance between the point where a neutron enters a specified class and the point where it leaves this class."@en ;
    rdfs:subClassOf [ a owl:Restriction ;
            owl:onProperty ns1:hasMeasurementUnit ;
            owl:someValuesFrom ns1:AreaUnit ],
        ns1:AtomicAndNuclearPhysicsQuantity,
        ns1:ISQDerivedQuantity ;
    skos:prefLabel "DiffusionArea"@en ;
    ns1:ISO80000Reference "10-72.2"^^xsd:string ;
    ns1:elucidation "One-sixth of the mean square distance between the point where a neutron enters a specified class and the point where it leaves this class."@en ;
    ns1:qudtReference "https://qudt.org/vocab/quantitykind/DiffusionArea"^^xsd:string ;
    ns1:wikidataReference "https://www.wikidata.org/wiki/Q98966292"^^xsd:string .

ns1:DiffusionCoefficientForFluenceRate a owl:Class ;
    rdfs:label "DiffusionCoefficientForFluenceRate"@en ;
    rdfs:comment "Proportionality constant between the particle current density J and the gradient of the particle fluence rate."@en ;
    rdfs:subClassOf ns1:AtomicAndNuclearPhysicsQuantity,
        ns1:Length ;
    skos:prefLabel "DiffusionCoefficientForFluenceRate"@en ;
    ns1:ISO80000Reference "10-65"^^xsd:string ;
    ns1:elucidation "Proportionality constant between the particle current density J and the gradient of the particle fluence rate."@en ;
    ns1:qudtReference "https://qudt.org/vocab/quantitykind/DiffusionCoefficientForFluenceRate"^^xsd:string ;
    ns1:wikidataReference "https://www.wikidata.org/wiki/Q98876254"^^xsd:string .

ns1:DiffusionCoefficientForParticleNumberDensity a owl:Class ;
    rdfs:label "DiffusionCoefficientForParticleNumberDensity"@en ;
    rdfs:comment "Proportionality constant between the particle current density J and the gradient of the particle number density n."@en ;
    rdfs:subClassOf ns1:AtomicAndNuclearPhysicsQuantity,
        ns1:DiffusionCoefficient ;
    skos:prefLabel "DiffusionCoefficientForParticleNumberDensity"@en ;
    ns1:ISO80000Reference "10-64"^^xsd:string ;
    ns1:elucidation "Proportionality constant between the particle current density J and the gradient of the particle number density n."@en ;
    ns1:wikidataReference "https://www.wikidata.org/wiki/Q98875545"^^xsd:string .

ns1:DiffusionLength a owl:Class ;
    rdfs:label "DiffusionLength"@en ;
    rdfs:comment "In condensed matter physics, the square root of the product of diffusion coefficient and lifetime."@en ;
    rdfs:subClassOf ns1:CondensedMatterPhysicsQuantity,
        ns1:Length ;
    skos:prefLabel "DiffusionLength"@en ;
    ns1:IEVReference "https://www.electropedia.org/iev/iev.nsf/display?openform&ievref=521-02-60"^^xsd:string ;
    ns1:ISO80000Reference "12-33"^^xsd:string ;
    ns1:elucidation "In condensed matter physics, the square root of the product of diffusion coefficient and lifetime."@en ;
    ns1:qudtReference "https://qudt.org/vocab/quantitykind/SolidStateDiffusionLength"^^xsd:string ;
    ns1:wikidataReference "https://www.wikidata.org/wiki/Q106097176"^^xsd:string .

ns1:DiffusivityUnit a owl:Class ;
    rdfs:label "DiffusivityUnit"@en ;
    rdfs:comment "The class of units with dimensionality 'Diffusivity'."@en .

ns1:DirectionAndEnergyDistributionOfCrossSection a owl:Class ;
    rdfs:label "DirectionAndEnergyDistributionOfCrossSection"@en ;
    rdfs:comment "Partial differential quotient of the cross section of a process with respect to the solid angle around a given direction and the energy of a particle scattered in that direction."@en ;
    rdfs:subClassOf [ a owl:Restriction ;
            owl:onProperty ns1:hasMeasurementUnit ;
            owl:someValuesFrom ns1:SquareTimePerMassUnit ],
        ns1:AtomicAndNuclearPhysicsQuantity,
        ns1:ISQDerivedQuantity ;
    skos:prefLabel "DirectionAndEnergyDistributionOfCrossSection"@en ;
    ns1:ISO80000Reference "10-41"^^xsd:string ;
    ns1:elucidation "Partial differential quotient of the cross section of a process with respect to the solid angle around a given direction and the energy of a particle scattered in that direction."@en ;
    ns1:qudtReference "https://qudt.org/vocab/quantitykind/SpectralAngularCrossSection"^^xsd:string ;
    ns1:wikidataReference "https://www.wikidata.org/wiki/Q98269571"^^xsd:string .

ns1:DirectionDistributionOfCrossSection a owl:Class ;
    rdfs:label "DirectionDistributionOfCrossSection"@en ;
    rdfs:comment "Differential quotient of the cross section for scattering a particle in a given direction and the solid angle around that direction."@en ;
    rdfs:subClassOf [ a owl:Restriction ;
            owl:onProperty ns1:hasMeasurementUnit ;
            owl:someValuesFrom ns1:AreaUnit ],
        ns1:AtomicAndNuclearPhysicsQuantity,
        ns1:ISQDerivedQuantity ;
    skos:prefLabel "DirectionDistributionOfCrossSection"@en ;
    ns1:ISO80000Reference "10-39"^^xsd:string ;
    ns1:elucidation "Differential quotient of the cross section for scattering a particle in a given direction and the solid angle around that direction."@en ;
    ns1:qudtReference "https://qudt.org/vocab/quantitykind/AngularCrossSection"^^xsd:string ;
    ns1:wikidataReference "https://www.wikidata.org/wiki/Q98266630"^^xsd:string .

ns1:DisplacementCurrent a owl:Class ;
    rdfs:label "DisplacementCurrent"@en ;
    rdfs:comment "Scalar quantity equal to the flux of the displacement current density JD through a given directed surface S."@en ;
    rdfs:subClassOf ns1:ElectricCurrent ;
    skos:prefLabel "DisplacementCurrent"@en ;
    ns1:IEVReference "https://www.electropedia.org/iev/iev.nsf/display?openform&ievref=121-11-43"^^xsd:string ;
    ns1:ISO80000Reference "6-19.1"^^xsd:string ;
    ns1:elucidation "Scalar quantity equal to the flux of the displacement current density JD through a given directed surface S."@en ;
    ns1:qudtReference "https://qudt.org/vocab/quantitykind/DisplacementCurrent"^^xsd:string ;
    ns1:wikidataReference "https://www.wikidata.org/wiki/Q853178"^^xsd:string .

ns1:DisplacementCurrentDensity a owl:Class ;
    rdfs:label "DisplacementCurrentDensity"@en ;
    rdfs:comment "Vector quantity equal to the time derivative of the electric flux density."@en ;
    rdfs:subClassOf ns1:ElectricCurrentDensity ;
    skos:prefLabel "DisplacementCurrentDensity"@en ;
    ns1:IEVReference "https://www.electropedia.org/iev/iev.nsf/display?openform&ievref=121-11-42"^^xsd:string ;
    ns1:ISO80000Reference "6-18"^^xsd:string ;
    ns1:elucidation "Vector quantity equal to the time derivative of the electric flux density."@en ;
    ns1:qudtReference "https://qudt.org/vocab/quantitykind/DisplacementCurrentDensity"^^xsd:string ;
    ns1:wikidataReference "https://www.wikidata.org/wiki/Q77614612"^^xsd:string .

ns1:DisplacementVector a owl:Class ;
    rdfs:label "DisplacementVector"@en ;
    rdfs:comment "In condensed matter physics, position vector of an atom or ion relative to its equilibrium position."@en ;
    rdfs:subClassOf ns1:CondensedMatterPhysicsQuantity,
        ns1:Displacement ;
    skos:prefLabel "DisplacementVector"@en ;
    ns1:ISO80000Reference "12-7.3"^^xsd:string ;
    ns1:elucidation "In condensed matter physics, position vector of an atom or ion relative to its equilibrium position."@en ;
    ns1:qudtReference "https://qudt.org/vocab/quantitykind/DisplacementVectorOfIon"^^xsd:string ;
    ns1:wikidataReference "https://www.wikidata.org/wiki/Q105533558"^^xsd:string .

ns1:DissociationConstant a owl:Class ;
    rdfs:label "DissociationConstant"@en ;
    rdfs:comment "Ratio of the number of dissociated molecules of a specified type to the total number of dissolved molecules of this type."@en ;
    rdfs:subClassOf [ a owl:Restriction ;
            owl:onProperty ns1:hasMeasurementUnit ;
            owl:someValuesFrom ns1:AmountConcentrationUnit ],
        ns1:EquilibriumConstant ;
    skos:prefLabel "DissociationConstant"@en ;
    ns1:IEVReference "https://www.electropedia.org/iev/iev.nsf/display?openform&ievref=114-01-10"@en ;
    ns1:elucidation "Ratio of the number of dissociated molecules of a specified type to the total number of dissolved molecules of this type."@en ;
    ns1:wikidataReference "https://www.wikidata.org/wiki/Q898254"^^xsd:string .

ns1:DonorDensity a owl:Class ;
    rdfs:label "DonorDensity"@en ;
    rdfs:comment "Number of donor levels per volume."@en ;
    rdfs:subClassOf ns1:CondensedMatterPhysicsQuantity,
        ns1:ReciprocalVolume ;
    skos:prefLabel "DonorDensity"@en ;
    ns1:ISO80000Reference "12-29.4"^^xsd:string ;
    ns1:elucidation "Number of donor levels per volume."@en ;
    ns1:qudtReference "https://qudt.org/vocab/quantitykind/DonorDensity"^^xsd:string ;
    ns1:wikidataReference "https://www.wikidata.org/wiki/Q105979886"^^xsd:string .

ns1:DoseEquivalent a owl:Class ;
    rdfs:label "DoseEquivalent"@en ;
    rdfs:comment "A dose quantity used in the International Commission on Radiological Protection (ICRP) system of radiological protection."@en ;
    rdfs:subClassOf [ a owl:Restriction ;
            owl:onProperty ns1:hasMeasurementUnit ;
            owl:someValuesFrom ns1:AbsorbedDoseUnit ],
        ns1:ISQDerivedQuantity,
        ns1:Intensive ;
    skos:prefLabel "DoseEquivalent"@en ;
    ns1:ISO80000Reference "10-83.1"^^xsd:string ;
    ns1:elucidation "A dose quantity used in the International Commission on Radiological Protection (ICRP) system of radiological protection."@en ;
    ns1:iupacReference "https://doi.org/10.1351/goldbook.E02101"^^xsd:string ;
    ns1:qudtReference "http://qudt.org/vocab/quantitykind/DoseEquivalent"^^xsd:string .

ns1:DoseEquivalentQualityFactor a owl:Class ;
    rdfs:label "DoseEquivalentQualityFactor"@en ;
    rdfs:comment "Factor taking into account health effects in the determination of the dose equivalent."@en ;
    rdfs:subClassOf ns1:AtomicAndNuclearPhysicsQuantity,
        ns1:ISQDimensionlessQuantity ;
    skos:prefLabel "DoseEquivalentQualityFactor"@en ;
    ns1:IEVReference "https://www.electropedia.org/iev/iev.nsf/display?openform&ievref=881-14-03"^^xsd:string ;
    ns1:ISO80000Reference "10-82"^^xsd:string ;
    ns1:elucidation "Factor taking into account health effects in the determination of the dose equivalent."@en ;
    ns1:qudtReference "https://qudt.org/vocab/quantitykind/DoseEquivalentQualityFactor"^^xsd:string ;
    ns1:wikidataReference "https://www.wikidata.org/wiki/Q2122099"^^xsd:string .

ns1:DoseEquivalentRate a owl:Class ;
    rdfs:label "DoseEquivalentRate"@en ;
    rdfs:comment "Time derivative of the dose equivalent."@en ;
    rdfs:subClassOf ns1:AbsorbedDoseRate ;
    skos:prefLabel "DoseEquivalentRate"@en ;
    ns1:IEVReference "https://www.electropedia.org/iev/iev.nsf/display?openform&ievref=881-14-02"^^xsd:string ;
    ns1:ISO80000Reference "10-83.2"^^xsd:string ;
    ns1:elucidation "Time derivative of the dose equivalent."@en ;
    ns1:wikidataReference "https://www.wikidata.org/wiki/Q99604810"^^xsd:string .

ns1:DragCoefficient a owl:Class ;
    rdfs:label "DragCoefficient"@en ;
    rdfs:comment "Dimensionless parameter to quantify fluid resistance."@en ;
    rdfs:subClassOf ns1:ISQDimensionlessQuantity,
        ns1:MechanicalQuantity ;
    skos:altLabel "DragFactor"@en ;
    skos:prefLabel "DragCoefficient"@en ;
    ns1:ISO80000Reference "4-23.4"^^xsd:string ;
    ns1:elucidation "Dimensionless parameter to quantify fluid resistance."@en ;
    ns1:qudtReference "https://qudt.org/vocab/quantitykind/DragCoefficient"^^xsd:string ;
    ns1:wikidataReference "https://www.wikidata.org/wiki/Q1778961"^^xsd:string .

ns1:DragForce a owl:Class ;
    rdfs:label "DragForce"@en ;
    rdfs:comment "Retarding force on a body moving in a fluid."@en ;
    rdfs:subClassOf ns1:Force,
        ns1:MechanicalQuantity ;
    skos:prefLabel "DragForce"@en ;
    ns1:ISO80000Reference "4-9.6"^^xsd:string ;
    ns1:elucidation "Retarding force on a body moving in a fluid."@en ;
    ns1:wikidataReference "https://www.wikidata.org/wiki/Q206621"^^xsd:string .

ns1:DynamicViscosity a owl:Class ;
    rdfs:label "DynamicViscosity"@en ;
    rdfs:comment "The measure of the resistance of a fluid to flow when an external force is applied."@en ;
    rdfs:subClassOf [ a owl:Restriction ;
            owl:onProperty ns1:hasMeasurementUnit ;
            owl:someValuesFrom ns1:MassPerLengthTimeUnit ],
        ns1:MechanicalQuantity ;
    skos:altLabel "Viscosity"@en ;
    skos:prefLabel "DynamicViscosity"@en ;
    ns1:IEVReference "https://www.electropedia.org/iev/iev.nsf/display?openform&ievref=113-03-34"@en ;
    ns1:ISO80000Reference "4-24"@en ;
    ns1:elucidation "The measure of the resistance of a fluid to flow when an external force is applied."@en ;
    ns1:iupacReference "https://doi.org/10.1351/goldbook.D01877"^^xsd:string ;
    ns1:qudtReference "https://qudt.org/vocab/quantitykind/DynamicViscosity"^^xsd:string ;
    ns1:wikidataReference "https://www.wikidata.org/wiki/Q15152757"^^xsd:string .

ns1:EffectiveDiffusionCoefficient a owl:Class ;
    rdfs:label "EffectiveDiffusionCoefficient"@en ;
    rdfs:comment "Diffusion coefficient through the pore space of a porous media."@en ;
    rdfs:subClassOf ns1:DiffusionCoefficient ;
    skos:prefLabel "EffectiveDiffusionCoefficient"@en ;
    ns1:elucidation "Diffusion coefficient through the pore space of a porous media."@en ;
    ns1:wikidataReference "https://www.wikidata.org/wiki/Q258852"^^xsd:string .

ns1:EffectiveMass a owl:Class ;
    rdfs:label "EffectiveMass"@en ;
    rdfs:comment "The mass that it seems to have when responding to forces, or the mass that it seems to have when interacting with other identical particles in a thermal distribution."@en ;
    rdfs:subClassOf ns1:CondensedMatterPhysicsQuantity,
        ns1:Mass ;
    skos:prefLabel "EffectiveMass"@en ;
    ns1:ISO80000Reference "12-30"^^xsd:string ;
    ns1:elucidation "The mass that it seems to have when responding to forces, or the mass that it seems to have when interacting with other identical particles in a thermal distribution."@en ;
    ns1:qudtReference "https://qudt.org/vocab/quantitykind/EffectiveMass"^^xsd:string ;
    ns1:wikidataReference "https://www.wikidata.org/wiki/Q1064434"^^xsd:string .

ns1:ElectricChargeAreaUnit a owl:Class ;
    rdfs:label "ElectricChargeAreaUnit"@en ;
    rdfs:comment "The class of units with dimensionality 'ElectricChargeArea'."@en .

ns1:ElectricChargeDensity a owl:Class ;
    rdfs:label "ElectricChargeDensity"@en ;
    rdfs:comment "Electric charge per volume."@en ;
    rdfs:subClassOf [ a owl:Restriction ;
            owl:onProperty ns1:hasMeasurementUnit ;
            owl:someValuesFrom ns1:ElectricChargeDensityUnit ],
        ns1:ElectromagneticQuantity,
        ns1:ISQDerivedQuantity ;
    skos:altLabel "VolumeElectricCharge"@en ;
    skos:prefLabel "ElectricChargeDensity"@en ;
    ns1:IEVReference "https://www.electropedia.org/iev/iev.nsf/display?openform&ievref=121-11-07"^^xsd:string ;
    ns1:ISO80000Reference "6-3"^^xsd:string ;
    ns1:elucidation "Electric charge per volume."@en ;
    ns1:iupacReference "https://doi.org/10.1351/goldbook.C00988"^^xsd:string ;
    ns1:qudtReference "https://qudt.org/vocab/quantitykind/ElectricChargeDensity"^^xsd:string ;
    ns1:wikidataReference "https://www.wikidata.org/wiki/Q69425629"^^xsd:string .

ns1:ElectricChargePerAmountUnit a owl:Class ;
    rdfs:label "ElectricChargePerAmountUnit"@en ;
    rdfs:comment "The class of units with dimensionality 'ElectricChargePerAmount'."@en .

ns1:ElectricChargePerTemperatureUnit a owl:Class ;
    rdfs:label "ElectricChargePerTemperatureUnit"@en ;
    rdfs:comment "The class of units with dimensionality 'ElectricChargePerTemperature'."@en .

ns1:ElectricConductivityPerAmountUnit a owl:Class ;
    rdfs:label "ElectricConductivityPerAmountUnit"@en ;
    rdfs:comment "The class of units with dimensionality 'ElectricConductivityPerAmount'."@en .

ns1:ElectricCurrentDensityPerTemperatureUnit a owl:Class ;
    rdfs:label "ElectricCurrentDensityPerTemperatureUnit"@en ;
    rdfs:comment "The class of units with dimensionality 'ElectricCurrentDensityPerTemperature'."@en .

ns1:ElectricCurrentPerAmountVolumeUnit a owl:Class ;
    rdfs:label "ElectricCurrentPerAmountVolumeUnit"@en ;
    rdfs:comment "The class of units with dimensionality 'ElectricCurrentPerAmountVolume'."@en .

ns1:ElectricCurrentPerTemperatureUnit a owl:Class ;
    rdfs:label "ElectricCurrentPerTemperatureUnit"@en ;
    rdfs:comment "The class of units with dimensionality 'ElectricCurrentPerTemperature'."@en .

ns1:ElectricCurrentPhasor a owl:Class ;
    rdfs:label "ElectricCurrentPhasor"@en ;
    rdfs:subClassOf ns1:ElectricCurrent ;
    skos:prefLabel "ElectricCurrentPhasor"@en ;
    ns1:ISO80000Reference "6-49"^^xsd:string ;
    ns1:qudtReference "https://qudt.org/vocab/quantitykind/ElectricCurrentPhasor"^^xsd:string ;
    ns1:wikidataReference "https://www.wikidata.org/wiki/Q78514596"^^xsd:string .

ns1:ElectricDipoleMoment a owl:Class ;
    rdfs:label "ElectricDipoleMoment"@en ;
    rdfs:comment "An electric dipole, vector quantity of magnitude equal to the product of the positive charge and the distance between the charges and directed from the negative charge to the positive charge."@en ;
    rdfs:subClassOf [ a owl:Restriction ;
            owl:onProperty ns1:hasMeasurementUnit ;
            owl:someValuesFrom ns1:ElectricDipoleMomentUnit ],
        ns1:ElectromagneticQuantity,
        ns1:ISQDerivedQuantity ;
    skos:prefLabel "ElectricDipoleMoment"@en ;
    ns1:IEVReference "https://www.electropedia.org/iev/iev.nsf/display?openform&ievref=121-11-35"^^xsd:string ;
    ns1:ISO80000Reference "6-6"^^xsd:string ;
    ns1:elucidation "An electric dipole, vector quantity of magnitude equal to the product of the positive charge and the distance between the charges and directed from the negative charge to the positive charge."@en ;
    ns1:iupacReference "https://doi.org/10.1351/goldbook.E01929"^^xsd:string ;
    ns1:qudtReference "http://qudt.org/vocab/quantitykind/ElectricDipoleMoment"^^xsd:string ;
    ns1:wikidataReference "https://www.wikidata.org/wiki/Q735135"^^xsd:string .

ns1:ElectricFieldStrength a owl:Class ;
    rdfs:label "ElectricFieldStrength"@en ;
    rdfs:comment "Vector field quantity E which exerts on any charged particle at rest a force F equal to the product of E and the electric charge Q of the particle."@en ;
    rdfs:subClassOf [ a owl:Restriction ;
            owl:onProperty ns1:hasMeasurementUnit ;
            owl:someValuesFrom ns1:ElectricFieldStrengthUnit ],
        ns1:ElectromagneticQuantity,
        ns1:ISQDerivedQuantity ;
    skos:prefLabel "ElectricFieldStrength"@en ;
    ns1:IEVReference "https://www.electropedia.org/iev/iev.nsf/display?openform&ievref=121-11-18"^^xsd:string ;
    ns1:ISO80000Reference "6-10"^^xsd:string ;
    ns1:elucidation "Vector field quantity E which exerts on any charged particle at rest a force F equal to the product of E and the electric charge Q of the particle."@en ;
    ns1:qudtReference "https://qudt.org/vocab/quantitykind/ElectricFieldStrength"^^xsd:string ;
    ns1:wikidataReference "https://www.wikidata.org/wiki/Q20989"^^xsd:string .

ns1:ElectricFlux a owl:Class ;
    rdfs:label "ElectricFlux"@en ;
    rdfs:comment "Scalar quantity equal to the flux of the electric flux density D through a given directed surface S."@en ;
    rdfs:subClassOf [ a owl:Restriction ;
            owl:onProperty ns1:hasMeasurementUnit ;
            owl:someValuesFrom ns1:ElectricChargeUnit ],
        ns1:ElectromagneticQuantity,
        ns1:ISQDerivedQuantity ;
    skos:prefLabel "ElectricFlux"@en ;
    ns1:IEVReference "https://www.electropedia.org/iev/iev.nsf/display?openform&ievref=121-11-41"^^xsd:string ;
    ns1:ISO80000Reference "6-17"^^xsd:string ;
    ns1:elucidation "Scalar quantity equal to the flux of the electric flux density D through a given directed surface S."@en ;
    ns1:qudtReference "https://qudt.org/vocab/quantitykind/ElectricFlux"^^xsd:string ;
    ns1:wikidataReference "https://www.wikidata.org/wiki/Q501267"^^xsd:string .

ns1:ElectricImpedance a owl:Class ;
    rdfs:label "ElectricImpedance"@en ;
    rdfs:comment "Measure of the opposition that a circuit presents to a current when a voltage is applied."@en ;
    rdfs:subClassOf ns1:ElectricResistance ;
    skos:altLabel "Impedance"^^xsd:string ;
    skos:prefLabel "ElectricImpedance"@en ;
    ns1:IEVReference "https://www.electropedia.org/iev/iev.nsf/display?openform&ievref=131-12-43"^^xsd:string ;
    ns1:ISO80000Reference "6-51.1"@en ;
    ns1:elucidation "Measure of the opposition that a circuit presents to a current when a voltage is applied."@en ;
    ns1:qudtReference "http://qudt.org/vocab/quantitykind/Impedance"^^xsd:string ;
    ns1:wikidataReference "https://www.wikidata.org/wiki/Q179043"^^xsd:string ;
    ns1:wikipediaReference "https://en.wikipedia.org/wiki/Electrical_impedance"^^xsd:string .

ns1:ElectricPolarization a owl:Class ;
    rdfs:label "ElectricPolarization"@en ;
    rdfs:comment "At a given point within a domain of quasi-infinitesimal volume V, vector quantity equal to the electric dipole moment p of the substance contained within the domain divided by the volume V."@en ;
    rdfs:subClassOf ns1:ElectricFluxDensity ;
    skos:prefLabel "ElectricPolarization"@en ;
    ns1:IEVReference "https://www.electropedia.org/iev/iev.nsf/display?openform&ievref=121-11-37"^^xsd:string ;
    ns1:ISO80000Reference "6-7"^^xsd:string ;
    ns1:elucidation "At a given point within a domain of quasi-infinitesimal volume V, vector quantity equal to the electric dipole moment p of the substance contained within the domain divided by the volume V."@en ;
    ns1:qudtReference "https://qudt.org/vocab/quantitykind/ElectricPolarization"^^xsd:string ;
    ns1:wikidataReference "https://www.wikidata.org/wiki/Q1050425"@en .

ns1:ElectricPotentialPerAreaUnit a owl:Class ;
    rdfs:label "ElectricPotentialPerAreaUnit"@en ;
    rdfs:comment "The class of units with dimensionality 'ElectricPotentialPerArea'."@en .

ns1:ElectricPotentialPerTimeUnit a owl:Class ;
    rdfs:label "ElectricPotentialPerTimeUnit"@en ;
    rdfs:comment "The class of units with dimensionality 'ElectricPotentialPerTime'."@en .

ns1:ElectricReactance a owl:Class ;
    rdfs:label "ElectricReactance"@en ;
    rdfs:comment "The opposition of a circuit element to a change in current or voltage, due to that element's inductance or capacitance."@en ;
    rdfs:subClassOf ns1:ElectricResistance ;
    skos:altLabel "Reactance"^^xsd:string ;
    skos:prefLabel "ElectricReactance"@en ;
    ns1:ISO80000Reference "6-51.3"@en ;
    ns1:elucidation "The opposition of a circuit element to a change in current or voltage, due to that element's inductance or capacitance."@en ;
    ns1:iupacReference "https://doi.org/10.1351/goldbook.R05162"^^xsd:string ;
    ns1:note "The imaginary part of the impedance."@en ;
    ns1:qudtReference "http://qudt.org/vocab/quantitykind/Reactance"^^xsd:string ;
    ns1:wikidataReference "https://www.wikidata.org/wiki/Q193972"^^xsd:string ;
    ns1:wikipediaReference "https://en.wikipedia.org/wiki/Electrical_reactance"^^xsd:string .

ns1:ElectricSusceptibility a owl:Class ;
    rdfs:label "ElectricSusceptibility"@en ;
    rdfs:comment "Electric polarization divided by electric constant and electric field strength."@en ;
    rdfs:subClassOf ns1:ElectromagneticQuantity,
        ns1:ISQDimensionlessQuantity ;
    skos:prefLabel "ElectricSusceptibility"@en ;
    ns1:IEVReference "https://www.electropedia.org/iev/iev.nsf/display?openform&ievref=121-12-19"^^xsd:string ;
    ns1:ISO80000Reference "6-16"^^xsd:string ;
    ns1:elucidation "Electric polarization divided by electric constant and electric field strength."@en ;
    ns1:qudtReference "https://qudt.org/vocab/quantitykind/ElectricSusceptibility"^^xsd:string ;
    ns1:wikidataReference "https://www.wikidata.org/wiki/Q598305"^^xsd:string ;
    ns1:wikipediaReference "https://en.wikipedia.org/wiki/Electric_susceptibility"^^xsd:string .

ns1:ElectrolyticConductivity a owl:Class ;
    rdfs:label "ElectrolyticConductivity"@en ;
    rdfs:comment "Electric conductivity of an electrolyte."@en ;
    rdfs:subClassOf ns1:ElectricConductivity,
        ns1:PhysioChemicalQuantity ;
    skos:prefLabel "ElectrolyticConductivity"@en ;
    ns1:IEVReference "https://www.electropedia.org/iev/iev.nsf/display?openform&ievref=114-01-03"^^xsd:string ;
    ns1:ISO80000Reference "9-44"@en ;
    ns1:elucidation "Electric conductivity of an electrolyte."@en ;
    ns1:qudtReference "https://qudt.org/vocab/quantitykind/ElectrolyticConductivity"^^xsd:string ;
    ns1:wikidataReference "https://www.wikidata.org/wiki/Q907564"^^xsd:string .

ns1:ElectromagneticEnergyDensity a owl:Class ;
    rdfs:label "ElectromagneticEnergyDensity"@en ;
    rdfs:comment "Arithmetic average of (electric field strength multiplied by electric flux density) and (magnetic field strength multiplied by magnetic flux density)."@en ;
    rdfs:subClassOf [ a owl:Restriction ;
            owl:onProperty ns1:hasMeasurementUnit ;
            owl:someValuesFrom ns1:PressureUnit ],
        ns1:ElectromagneticQuantity,
        ns1:ISQDerivedQuantity ;
    skos:altLabel "VolumicElectromagneticEnergy"@en ;
    skos:prefLabel "ElectromagneticEnergyDensity"@en ;
    ns1:IEVReference "https://www.electropedia.org/iev/iev.nsf/display?openform&ievref=121-11-65"^^xsd:string ;
    ns1:ISO80000Reference "6-33"^^xsd:string ;
    ns1:elucidation "Arithmetic average of (electric field strength multiplied by electric flux density) and (magnetic field strength multiplied by magnetic flux density)."@en ;
    ns1:qudtReference "https://qudt.org/vocab/quantitykind/ElectromagneticEnergyDensity"^^xsd:string ;
    ns1:wikidataReference "https://www.wikidata.org/wiki/Q77989624"^^xsd:string .

ns1:ElectronAffinity a owl:Class ;
    rdfs:label "ElectronAffinity"@en ;
    rdfs:comment "energy difference between an electron at rest at infinity and an electron at the lowest level of the conduction band in an insulator or semiconductor"@en ;
    rdfs:subClassOf ns1:CondensedMatterPhysicsQuantity,
        ns1:Energy ;
    skos:prefLabel "ElectronAffinity"@en ;
    ns1:IEVReference "https://www.electropedia.org/iev/iev.nsf/display?openform&ievref=113-06-22"^^xsd:string ;
    ns1:ISO80000Reference "12-25"^^xsd:string ;
    ns1:elucidation "energy difference between an electron at rest at infinity and an electron at the lowest level of the conduction band in an insulator or semiconductor"@en ;
    ns1:qudtReference "https://qudt.org/vocab/quantitykind/ElectronAffinity"^^xsd:string ;
    ns1:wikidataReference "https://www.wikidata.org/wiki/Q105846486"^^xsd:string .

ns1:ElectronCharge a owl:Class ;
    rdfs:label "ElectronCharge"@en ;
    rdfs:comment "The charge of an electron."@en,
        "The negative of ElementaryCharge."@en ;
    rdfs:subClassOf ns1:ElectricCharge,
        ns1:SIExactConstant ;
    skos:prefLabel "ElectronCharge"@en ;
    ns1:definition "The charge of an electron."@en ;
    ns1:elucidation "The negative of ElementaryCharge."@en ;
    ns1:iupacReference "https://doi.org/10.1351/goldbook.E01982"^^xsd:string .

ns1:ElectronDensity a owl:Class ;
    rdfs:label "ElectronDensity"@en ;
    rdfs:comment "Number of electrons in conduction band per volume."@en ;
    rdfs:subClassOf [ a owl:Restriction ;
            owl:onProperty ns1:hasMeasurementUnit ;
            owl:someValuesFrom ns1:PerVolumeUnit ],
        ns1:CondensedMatterPhysicsQuantity,
        ns1:ISQDerivedQuantity ;
    skos:prefLabel "ElectronDensity"@en ;
    ns1:IEVReference "https://www.electropedia.org/iev/iev.nsf/display?openform&ievref=705-06-05"^^xsd:string ;
    ns1:ISO80000Reference "12-29.1"^^xsd:string ;
    ns1:elucidation "Number of electrons in conduction band per volume."@en ;
    ns1:qudtReference "https://qudt.org/vocab/quantitykind/ElectronDensity"^^xsd:string .

ns1:ElectronMass a owl:Class ;
    rdfs:label "ElectronMass"@en ;
    rdfs:comment "The rest mass of an electron."@en ;
    rdfs:subClassOf ns1:Mass,
        ns1:MeasuredConstant ;
    skos:prefLabel "ElectronMass"@en ;
    ns1:iupacReference "https://doi.org/10.1351/goldbook.E02008"^^xsd:string ;
    ns1:qudtReference "http://qudt.org/vocab/constant/ElectronMass"^^xsd:string .

ns1:ElectronRadius a owl:Class ;
    rdfs:label "ElectronRadius"@en ;
    rdfs:comment "Radius of a sphere such that the relativistic electron energy is distributed uniformly."@en ;
    rdfs:subClassOf ns1:AtomicAndNuclearPhysicsQuantity,
        ns1:Radius ;
    skos:prefLabel "ElectronRadius"@en ;
    ns1:ISO80000Reference "10-19.2"^^xsd:string ;
    ns1:elucidation "Radius of a sphere such that the relativistic electron energy is distributed uniformly."@en ;
    ns1:wikidataReference "https://www.wikidata.org/wiki/Q2152581"^^xsd:string .

ns1:ElementaryCharge a owl:Class ;
    rdfs:label "ElementaryCharge"@en ;
    rdfs:comment "The DBpedia definition (http://dbpedia.org/page/Elementary_charge) is outdated as May 20, 2019. It is now an exact quantity."@en,
        "The magnitude of the electric charge carried by a single electron. It defines the base unit Ampere in the SI system."@en ;
    rdfs:subClassOf ns1:ElectricCharge,
        ns1:SIExactConstant ;
    skos:prefLabel "ElementaryCharge"@en ;
    ns1:ISO80000Reference "10-5.1"^^xsd:string ;
    ns1:elucidation "The magnitude of the electric charge carried by a single electron. It defines the base unit Ampere in the SI system."@en ;
    ns1:iupacReference "https://doi.org/10.1351/goldbook.E02032"^^xsd:string ;
    ns1:qudtReference "http://qudt.org/vocab/quantitykind/ElementaryCharge"^^xsd:string .

ns1:EnergyAreaUnit a owl:Class ;
    rdfs:label "EnergyAreaUnit"@en ;
    rdfs:comment "The class of units with dimensionality 'EnergyArea'."@en .

ns1:EnergyDensityOfStates a owl:Class ;
    rdfs:label "EnergyDensityOfStates"@en ;
    rdfs:comment "Quantity in condensed matter physics."@en ;
    rdfs:subClassOf [ a owl:Restriction ;
            owl:onProperty ns1:hasMeasurementUnit ;
            owl:someValuesFrom ns1:EnergyDensityOfStatesUnit ],
        ns1:CondensedMatterPhysicsQuantity,
        ns1:ISQDerivedQuantity ;
    owl:disjointWith ns1:DensityOfVibrationalStates ;
    skos:prefLabel "EnergyDensityOfStates"@en ;
    ns1:ISO80000Reference "12-16"^^xsd:string ;
    ns1:elucidation "Quantity in condensed matter physics."@en ;
    ns1:qudtReference "https://qudt.org/vocab/quantitykind/EnergyDensityOfStates"^^xsd:string ;
    ns1:wikidataReference "https://www.wikidata.org/wiki/Q105687031"^^xsd:string .

ns1:EnergyDistributionOfCrossSection a owl:Class ;
    rdfs:label "EnergyDistributionOfCrossSection"@en ;
    rdfs:comment "Differential quotient of the cross section for a process and the energy of the scattered particle."@en ;
    rdfs:subClassOf [ a owl:Restriction ;
            owl:onProperty ns1:hasMeasurementUnit ;
            owl:someValuesFrom ns1:ForcePerLengthUnit ],
        ns1:AtomicAndNuclearPhysicsQuantity,
        ns1:ISQDerivedQuantity ;
    skos:prefLabel "EnergyDistributionOfCrossSection"@en ;
    ns1:ISO80000Reference "10-40"^^xsd:string ;
    ns1:elucidation "Differential quotient of the cross section for a process and the energy of the scattered particle."@en ;
    ns1:qudtReference "https://qudt.org/vocab/quantitykind/SpectralCrossSection"^^xsd:string ;
    ns1:wikidataReference "https://www.wikidata.org/wiki/Q98267245"^^xsd:string .

ns1:EnergyFluence a owl:Class ;
    rdfs:label "EnergyFluence"@en ;
    rdfs:comment "In nuclear physics, incident radiant energy per cross-sectional area."@en ;
    rdfs:subClassOf [ a owl:Restriction ;
            owl:onProperty ns1:hasMeasurementUnit ;
            owl:someValuesFrom ns1:ForcePerLengthUnit ],
        ns1:AtomicAndNuclearPhysicsQuantity,
        ns1:ISQDerivedQuantity ;
    skos:prefLabel "EnergyFluence"@en ;
    ns1:IEVReference "https://www.electropedia.org/iev/iev.nsf/display?openform&ievref=395-01-17"^^xsd:string ;
    ns1:ISO80000Reference "10-46"^^xsd:string ;
    ns1:elucidation "In nuclear physics, incident radiant energy per cross-sectional area."@en ;
    ns1:qudtReference "https://qudt.org/vocab/quantitykind/EnergyFluence"^^xsd:string ;
    ns1:wikidataReference "https://www.wikidata.org/wiki/Q98538612"^^xsd:string .

ns1:EnergyFluenceRate a owl:Class ;
    rdfs:label "EnergyFluenceRate"@en ;
    rdfs:comment "In nuclear physics, time derivative of the energy fluence."@en ;
    rdfs:subClassOf [ a owl:Restriction ;
            owl:onProperty ns1:hasMeasurementUnit ;
            owl:someValuesFrom ns1:PowerDensityUnit ],
        ns1:AtomicAndNuclearPhysicsQuantity,
        ns1:ISQDerivedQuantity ;
    skos:prefLabel "EnergyFluenceRate"@en ;
    ns1:ISO80000Reference "10-47"^^xsd:string ;
    ns1:elucidation "In nuclear physics, time derivative of the energy fluence."@en ;
    ns1:qudtReference "https://qudt.org/vocab/quantitykind/EnergyFluenceRate"^^xsd:string ;
    ns1:wikidataReference "https://www.wikidata.org/wiki/Q98538655"^^xsd:string .

ns1:EnergyImparted a owl:Class ;
    rdfs:label "EnergyImparted"@en ;
    rdfs:comment "Sum of energies deposited by ionizing radiation in a given volume."@en ;
    rdfs:subClassOf ns1:AtomicAndNuclearPhysicsQuantity,
        ns1:Energy ;
    skos:prefLabel "EnergyImparted"@en ;
    ns1:IEVReference "https://www.electropedia.org/iev/iev.nsf/display?openform&ievref=395-01-34"^^xsd:string ;
    ns1:ISO80000Reference "10-80.1"^^xsd:string ;
    ns1:elucidation "Sum of energies deposited by ionizing radiation in a given volume."@en ;
    ns1:qudtReference "https://qudt.org/vocab/quantitykind/EnergyImparted"^^xsd:string ;
    ns1:wikidataReference "https://www.wikidata.org/wiki/Q99526944"^^xsd:string .

ns1:EnergyLengthPerAmountUnit a owl:Class ;
    rdfs:label "EnergyLengthPerAmountUnit"@en ;
    rdfs:comment "The class of units with dimensionality 'EnergyLengthPerAmount'."@en .

ns1:EnergyPerSquareMagneticFluxDensityUnit a owl:Class ;
    rdfs:label "EnergyPerSquareMagneticFluxDensityUnit"@en ;
    rdfs:comment "The class of units with dimensionality 'EnergyPerSquareMagneticFluxDensity'."@en .

ns1:EnergyTimePerAmountUnit a owl:Class ;
    rdfs:label "EnergyTimePerAmountUnit"@en ;
    rdfs:comment "The class of units with dimensionality 'EnergyTimePerAmount'."@en .

ns1:Enthalpy a owl:Class ;
    rdfs:label "Enthalpy"@en ;
    rdfs:comment "Measurement of energy in a thermodynamic system."@en ;
    rdfs:subClassOf ns1:Energy ;
    skos:prefLabel "Enthalpy"@en ;
    ns1:ISO80000Reference "5.20-3"^^xsd:string ;
    ns1:elucidation "Measurement of energy in a thermodynamic system."@en ;
    ns1:iupacReference "https://doi.org/10.1351/goldbook.E02141"^^xsd:string ;
    ns1:qudtReference "http://qudt.org/vocab/quantitykind/Enthalpy"^^xsd:string .

ns1:EquilibriumPositionVector a owl:Class ;
    rdfs:label "EquilibriumPositionVector"@en ;
    rdfs:comment "In condensed matter physics, position vector of an atom or ion in equilibrium."@en ;
    rdfs:subClassOf [ a owl:Restriction ;
            owl:onProperty ns1:hasMeasurementUnit ;
            owl:someValuesFrom ns1:LengthUnit ],
        ns1:CondensedMatterPhysicsQuantity,
        ns1:ISQDerivedQuantity ;
    skos:prefLabel "EquilibriumPositionVector"@en ;
    ns1:ISO80000Reference "12-7.2"^^xsd:string ;
    ns1:elucidation "In condensed matter physics, position vector of an atom or ion in equilibrium."@en ;
    ns1:qudtReference "https://qudt.org/vocab/quantitykind/EquilibriumPositionVectorOfIon"^^xsd:string ;
    ns1:wikidataReference "https://www.wikidata.org/wiki/Q105533477"^^xsd:string .

ns1:ExchangeIntegral a owl:Class ;
    rdfs:label "ExchangeIntegral"@en ;
    rdfs:comment "constituent of the interaction energy between the spins of adjacent electrons in matter arising from the overlap of electron state functions"@en ;
    rdfs:subClassOf ns1:CondensedMatterPhysicsQuantity,
        ns1:Energy ;
    skos:prefLabel "ExchangeIntegral"@en ;
    ns1:ISO80000Reference "12-34"^^xsd:string ;
    ns1:elucidation "constituent of the interaction energy between the spins of adjacent electrons in matter arising from the overlap of electron state functions"@en ;
    ns1:qudtReference "https://qudt.org/vocab/quantitykind/ExchangeIntegral"^^xsd:string ;
    ns1:wikidataReference "https://www.wikidata.org/wiki/Q10882959"^^xsd:string .

ns1:Exposure a owl:Class ;
    rdfs:label "Exposure"@en ;
    rdfs:comment "Absolute value of the electric charge of ions produced in dry air by X- or gamma radiation per mass of air."@en ;
    rdfs:subClassOf [ a owl:Restriction ;
            owl:onProperty ns1:hasMeasurementUnit ;
            owl:someValuesFrom ns1:ElectricChargePerMassUnit ],
        ns1:AtomicAndNuclearPhysicsQuantity,
        ns1:ISQDerivedQuantity ;
    skos:prefLabel "Exposure"@en ;
    ns1:IEVReference "https://www.electropedia.org/iev/iev.nsf/display?openform&ievref=395-01-32"^^xsd:string ;
    ns1:ISO80000Reference "10-88"^^xsd:string ;
    ns1:elucidation "Absolute value of the electric charge of ions produced in dry air by X- or gamma radiation per mass of air."@en ;
    ns1:qudtReference "https://qudt.org/vocab/quantitykind/Exposure"^^xsd:string ;
    ns1:wikidataReference "https://www.wikidata.org/wiki/Q336938"^^xsd:string .

ns1:ExposureRate a owl:Class ;
    rdfs:label "ExposureRate"@en ;
    rdfs:comment "Time derivative of exposure."@en ;
    rdfs:subClassOf [ a owl:Restriction ;
            owl:onProperty ns1:hasMeasurementUnit ;
            owl:someValuesFrom ns1:ElectricCurrentPerMassUnit ],
        ns1:AtomicAndNuclearPhysicsQuantity,
        ns1:ISQDerivedQuantity ;
    skos:prefLabel "ExposureRate"@en ;
    ns1:IEVReference "https://www.electropedia.org/iev/iev.nsf/display?openform&ievref=395-01-42"^^xsd:string ;
    ns1:ISO80000Reference "10-89"^^xsd:string ;
    ns1:elucidation "Time derivative of exposure."@en ;
    ns1:qudtReference "https://qudt.org/vocab/quantitykind/ExposureRate"^^xsd:string ;
    ns1:wikidataReference "https://www.wikidata.org/wiki/Q99720212"^^xsd:string .

ns1:ExtentOfReaction a owl:Class ;
    rdfs:label "ExtentOfReaction"@en ;
    rdfs:comment "Difference between equilibrium and initial amount of a substance, divided by its stoichiometric number."@en ;
    rdfs:subClassOf [ a owl:Restriction ;
            owl:onProperty ns1:hasMeasurementUnit ;
            owl:someValuesFrom ns1:AmountUnit ],
        ns1:ISQDerivedQuantity,
        ns1:PhysioChemicalQuantity ;
    skos:prefLabel "ExtentOfReaction"@en ;
    ns1:ISO80000Reference "9-31"^^xsd:string ;
    ns1:elucidation "Difference between equilibrium and initial amount of a substance, divided by its stoichiometric number."@en ;
    ns1:iupacReference "https://doi.org/10.1351/goldbook.E02283"^^xsd:string ;
    ns1:qudtReference "https://qudt.org/vocab/quantitykind/ExtentOfReaction"^^xsd:string ;
    ns1:wikidataReference "https://www.wikidata.org/wiki/Q899046"^^xsd:string .

ns1:FastFissionFactor a owl:Class ;
    rdfs:label "FastFissionFactor"@en ;
    rdfs:comment "In an infinite medium, the ratio of the mean number of neutrons produced by fission due to neutrons of all energies to the mean number of neutrons produced by fissions due to thermal neutrons only."@en ;
    rdfs:subClassOf ns1:AtomicAndNuclearPhysicsQuantity,
        ns1:RatioQuantity ;
    skos:prefLabel "FastFissionFactor"@en ;
    ns1:ISO80000Reference "10-75"^^xsd:string ;
    ns1:elucidation "In an infinite medium, the ratio of the mean number of neutrons produced by fission due to neutrons of all energies to the mean number of neutrons produced by fissions due to thermal neutrons only."@en ;
    ns1:qudtReference "https://qudt.org/vocab/quantitykind/FastFissionFactor"^^xsd:string ;
    ns1:wikidataReference "https://www.wikidata.org/wiki/Q99197493"^^xsd:string .

ns1:FermiAnglularWaveNumber a owl:Class ;
    rdfs:label "FermiAnglularWaveNumber"@en ;
    rdfs:comment "Angular wavenumber of electrons in states on the Fermi sphere."@en ;
    rdfs:subClassOf ns1:AngularWavenumber,
        ns1:CondensedMatterPhysicsQuantity ;
    skos:altLabel "FermiAnglularRepetency"@en ;
    skos:prefLabel "FermiAnglularWaveNumber"@en ;
    ns1:ISO80000Reference "12-9.2"^^xsd:string ;
    ns1:elucidation "Angular wavenumber of electrons in states on the Fermi sphere."@en ;
    ns1:qudtReference "https://qudt.org/vocab/quantitykind/FermiAngularWavenumber"^^xsd:string ;
    ns1:wikidataReference "https://www.wikidata.org/wiki/Q105554303"^^xsd:string .

ns1:FermiEnergy a owl:Class ;
    rdfs:label "FermiEnergy"@en ;
    rdfs:comment "In a metal, highest occupied energy level at zero thermodynamic temperature, where energy level means the energy of an electron in the interior of a substance."@en ;
    rdfs:subClassOf ns1:CondensedMatterPhysicsQuantity,
        ns1:Energy ;
    skos:prefLabel "FermiEnergy"@en ;
    ns1:IEVReference "https://www.electropedia.org/iev/iev.nsf/display?openform&ievref=113-06-18"^^xsd:string ;
    ns1:ISO80000Reference "12-27.1"^^xsd:string ;
    ns1:elucidation "In a metal, highest occupied energy level at zero thermodynamic temperature, where energy level means the energy of an electron in the interior of a substance."@en ;
    ns1:iupacReference "https://doi.org/10.1351/goldbook.F02340"^^xsd:string ;
    ns1:qudtReference "https://qudt.org/vocab/quantitykind/FermiEnergy"^^xsd:string ;
    ns1:wikidataReference "https://www.wikidata.org/wiki/Q431335"^^xsd:string .

ns1:FermiTemperature a owl:Class ;
    rdfs:label "FermiTemperature"@en ;
    rdfs:comment "in the free electron model, the Fermi energy divided by the Boltzmann constant"@en ;
    rdfs:subClassOf ns1:CondensedMatterPhysicsQuantity,
        ns1:ThermodynamicTemperature ;
    skos:prefLabel "FermiTemperature"@en ;
    ns1:ISO80000Reference "12-28"^^xsd:string ;
    ns1:elucidation "in the free electron model, the Fermi energy divided by the Boltzmann constant"@en ;
    ns1:qudtReference "https://qudt.org/vocab/quantitykind/FermiTemperature"^^xsd:string ;
    ns1:wikidataReference "https://www.wikidata.org/wiki/Q105942324"^^xsd:string .

ns1:FineStructureConstant a owl:Class ;
    rdfs:label "FineStructureConstant"@en ;
    rdfs:comment "A fundamental physical constant characterizing the strength of the electromagnetic interaction between elementary charged particles."@en ;
    rdfs:subClassOf [ a owl:Restriction ;
            owl:onProperty ns1:hasMeasurementUnit ;
            owl:someValuesFrom ns1:UnitOne ],
        ns1:MeasuredConstant ;
    skos:prefLabel "FineStructureConstant"@en ;
    ns1:iupacReference "https://doi.org/10.1351/goldbook.F02389"^^xsd:string ;
    ns1:qudtReference "http://qudt.org/vocab/constant/FineStructureConstant"^^xsd:string .

ns1:ForceAreaUnit a owl:Class ;
    rdfs:label "ForceAreaUnit"@en ;
    rdfs:comment "The class of units with dimensionality 'ForceArea'."@en .

ns1:FrequencyPerAreaTimeUnit a owl:Class ;
    rdfs:label "FrequencyPerAreaTimeUnit"@en ;
    rdfs:comment "The class of units with dimensionality 'FrequencyPerAreaTime'."@en .

ns1:Fugacity a owl:Class ;
    rdfs:label "Fugacity"@en ;
    rdfs:comment "Measure of the tendency of a substance to leave a phase."@en ;
    rdfs:subClassOf [ a owl:Restriction ;
            owl:onProperty ns1:hasMeasurementUnit ;
            owl:someValuesFrom ns1:PressureUnit ],
        ns1:ISQDerivedQuantity,
        ns1:PhysioChemicalQuantity ;
    skos:prefLabel "Fugacity"@en ;
    ns1:ISO80000Reference "9-20"^^xsd:string ;
    ns1:elucidation "Measure of the tendency of a substance to leave a phase."@en ;
    ns1:iupacReference "https://doi.org/10.1351/goldbook.F02543"^^xsd:string ;
    ns1:qudtReference "https://qudt.org/vocab/quantitykind/Fugacity"^^xsd:string ;
    ns1:wikidataReference "https://www.wikidata.org/wiki/Q898412"^^xsd:string .

ns1:FundamentalLatticeVector a owl:Class ;
    rdfs:label "FundamentalLatticeVector"@en ;
    rdfs:comment "Fundamental translation vector for the crystal lattice."@en ;
    rdfs:subClassOf [ a owl:Restriction ;
            owl:onProperty ns1:hasMeasurementUnit ;
            owl:someValuesFrom ns1:LengthUnit ],
        ns1:CondensedMatterPhysicsQuantity ;
    skos:prefLabel "FundamentalLatticeVector"@en ;
    ns1:ISO80000Reference "12-1.2"^^xsd:string ;
    ns1:elucidation "Fundamental translation vector for the crystal lattice."@en ;
    ns1:qudtReference "https://qudt.org/vocab/quantitykind/FundamentalLatticeVector"^^xsd:string ;
    ns1:wikidataReference "https://www.wikidata.org/wiki/Q105451063"^^xsd:string .

ns1:FundamentalReciprocalLatticeVector a owl:Class ;
    rdfs:label "FundamentalReciprocalLatticeVector"@en ;
    rdfs:comment "Fundamental translation vectors for the reciprocal lattice."@en ;
    rdfs:subClassOf [ a owl:Restriction ;
            owl:onProperty ns1:hasMeasurementUnit ;
            owl:someValuesFrom ns1:ReciprocalLengthUnit ],
        ns1:CondensedMatterPhysicsQuantity ;
    skos:prefLabel "FundamentalReciprocalLatticeVector"@en ;
    ns1:ISO80000Reference "12-2.2"^^xsd:string ;
    ns1:elucidation "Fundamental translation vectors for the reciprocal lattice."@en ;
    ns1:qudtReference "https://qudt.org/vocab/quantitykind/FundamentalReciprocalLatticeVector"^^xsd:string ;
    ns1:wikidataReference "https://www.wikidata.org/wiki/Q105475399"^^xsd:string .

ns1:GFactorOfNucleusOrNuclearParticle a owl:Class ;
    rdfs:label "GFactorOfNucleusOrNuclearParticle"@en ;
    rdfs:comment "Quotient of the magnetic dipole moment of an atom, and the product of the nuclear spin quantum number and the nuclear magneton."@en ;
    rdfs:subClassOf ns1:AtomicAndNuclearPhysicsQuantity,
        ns1:GFactor ;
    skos:altLabel "NuclearGFactor"@en ;
    skos:prefLabel "GFactorOfNucleusOrNuclearParticle"@en ;
    ns1:ISO80000Reference "10-14.2"^^xsd:string ;
    ns1:elucidation "Quotient of the magnetic dipole moment of an atom, and the product of the nuclear spin quantum number and the nuclear magneton."@en ;
    ns1:qudtReference "https://qudt.org/vocab/quantitykind/GFactorOfNucleus"^^xsd:string ;
    ns1:wikidataReference "https://www.wikidata.org/wiki/Q97591250"^^xsd:string .

ns1:GaugePressure a owl:Class ;
    rdfs:label "GaugePressure"@en ;
    rdfs:comment "The pressure measured relative to the ambient atmospheric pressure."@en ;
    rdfs:subClassOf [ a owl:Restriction ;
            owl:onProperty ns1:hasMeasurementUnit ;
            owl:someValuesFrom ns1:PressureUnit ],
        ns1:MechanicalQuantity,
        ns1:Pressure ;
    skos:prefLabel "GaugePressure"@en ;
    ns1:ISO80000Reference "4-14.2"^^xsd:string ;
    ns1:elucidation "The pressure measured relative to the ambient atmospheric pressure."@en ;
    ns1:note "Gauge pressure can be measured using a diaphragm sensor, where one side of the diaphragm is exposed to the pressure media that is to be measured, while the other side is exposed to the ambient atmospheric pressure."@en ;
    ns1:wikidataReference "https://www.wikidata.org/wiki/Q109594211"^^xsd:string .

ns1:GibbsEnergy a owl:Class ;
    rdfs:label "GibbsEnergy"@en ;
    rdfs:comment "Type of thermodynamic potential; useful for calculating reversible work in certain systems."@en ;
    rdfs:subClassOf ns1:Energy,
        ns1:ThermodynamicalQuantity ;
    skos:altLabel "GibbsFreeEnergy"@en ;
    skos:prefLabel "GibbsEnergy"@en ;
    ns1:IEVReference "https://www.electropedia.org/iev/iev.nsf/display?openform&ievref=113-04-23"^^xsd:string ;
    ns1:ISO80000Reference "5-20.5"^^xsd:string ;
    ns1:elucidation "Type of thermodynamic potential; useful for calculating reversible work in certain systems."@en ;
    ns1:iupacReference "https://doi.org/10.1351/goldbook.G02629"^^xsd:string ;
    ns1:wikidataReference "https://www.wikidata.org/wiki/Q334631"^^xsd:string .

ns1:GrandCanonicalPartionFunction a owl:Class ;
    rdfs:label "GrandCanonicalPartionFunction"@en ;
    rdfs:comment "Sum of canonical partition function Z (NA,NB,…) for the given number of particles A, B, ... multiplied by absolute activities of particles A, B, ..."@en ;
    rdfs:subClassOf ns1:ISQDimensionlessQuantity,
        ns1:PhysioChemicalQuantity ;
    skos:altLabel "GrandPartionFunction"@en ;
    skos:prefLabel "GrandCanonicalPartionFunction"@en ;
    ns1:ISO80000Reference "9-35.3"^^xsd:string ;
    ns1:elucidation "Sum of canonical partition function Z (NA,NB,…) for the given number of particles A, B, ... multiplied by absolute activities of particles A, B, ..."@en ;
    ns1:qudtReference "https://qudt.org/vocab/quantitykind/GrandCanonicalPartitionFunction"^^xsd:string ;
    ns1:wikidataReference "https://www.wikidata.org/wiki/Q96176022"^^xsd:string .

ns1:GroupVelocity a owl:Class ;
    rdfs:label "GroupVelocity"@en ;
    rdfs:comment "Speed with which the envelope of a wave propagates in space."@en ;
    rdfs:subClassOf ns1:Velocity ;
    skos:altLabel "GroupSpeed"@en ;
    skos:prefLabel "GroupVelocity"@en ;
    ns1:IEVReference "https://www.electropedia.org/iev/iev.nsf/display?openform&ievref=103-10-15"^^xsd:string ;
    ns1:ISO80000Reference "3-23.2"^^xsd:string ;
    ns1:dbpediaReference "https://dbpedia.org/page/Group_velocity"^^xsd:string ;
    ns1:elucidation "Speed with which the envelope of a wave propagates in space."@en ;
    ns1:wikidataReference "https://www.wikidata.org/wiki/Q217361"^^xsd:string ;
    ns1:wikipediaReference "https://en.wikipedia.org/wiki/Group_velocity"^^xsd:string .

ns1:GrueneisenParamter a owl:Class ;
    rdfs:label "GrueneisenParamter"@en ;
    rdfs:comment "Describes the effect that changing the volume of a crystal lattice has on its vibrational properties, and, as a consequence, the effect that changing temperature has on the size or dynamics of the lattice."@en ;
    rdfs:subClassOf ns1:CondensedMatterPhysicsQuantity,
        ns1:ISQDimensionlessQuantity ;
    skos:prefLabel "GrueneisenParamter"@en ;
    ns1:ISO80000Reference "12-14"^^xsd:string ;
    ns1:elucidation "Describes the effect that changing the volume of a crystal lattice has on its vibrational properties, and, as a consequence, the effect that changing temperature has on the size or dynamics of the lattice."@en ;
    ns1:wikidataReference "https://www.wikidata.org/wiki/Q444656"^^xsd:string .

ns1:GyromagneticRatioOfTheElectron a owl:Class ;
    rdfs:label "GyromagneticRatioOfTheElectron"^^xsd:string ;
    rdfs:comment "Proportionality constant between the magnetic dipole moment and the angular momentum of the electron."@en ;
    rdfs:subClassOf ns1:GyromagneticRatio ;
    skos:altLabel "GyromagneticCoefficientOfTheElectron"@en,
        "MagnetogyricRatioOfTheElectron"@en ;
    skos:prefLabel "GyromagneticRatioOfTheElectron"^^xsd:string ;
    ns1:ISO80000Reference "10-12.2"^^xsd:string ;
    ns1:elucidation "Proportionality constant between the magnetic dipole moment and the angular momentum of the electron."@en ;
    ns1:wikidataReference "https://www.wikidata.org/wiki/Q97543076"^^xsd:string .

ns1:Gyroradius a owl:Class ;
    rdfs:label "Gyroradius"@en ;
    rdfs:comment "Radius of the circular movement of an electrically charged particle in a magnetic field."@en ;
    rdfs:subClassOf ns1:AtomicAndNuclearPhysicsQuantity,
        ns1:Radius ;
    skos:altLabel "LarmorRadius"@en ;
    skos:prefLabel "Gyroradius"@en ;
    ns1:ISO80000Reference "10-17"^^xsd:string ;
    ns1:elucidation "Radius of the circular movement of an electrically charged particle in a magnetic field."@en ;
    ns1:wikidataReference "https://www.wikidata.org/wiki/Q1194458"^^xsd:string .

ns1:HalfLife a owl:Class ;
    rdfs:label "HalfLife"@en ;
    rdfs:comment "Mean duration required for the decay of one half of the atoms or nuclei."@en ;
    rdfs:subClassOf ns1:AtomicAndNuclearPhysicsQuantity,
        ns1:Duration ;
    skos:prefLabel "HalfLife"@en ;
    ns1:IEVReference "https://www.electropedia.org/iev/iev.nsf/display?openform&ievref=395-01-12"^^xsd:string ;
    ns1:ISO80000Reference "10-31"^^xsd:string ;
    ns1:elucidation "Mean duration required for the decay of one half of the atoms or nuclei."@en ;
    ns1:qudtReference "https://qudt.org/vocab/quantitykind/Half-Life"^^xsd:string ;
    ns1:wikidataReference "https://www.wikidata.org/wiki/Q98118544"^^xsd:string .

ns1:HalfValueThickness a owl:Class ;
    rdfs:label "HalfValueThickness"@en ;
    rdfs:comment "Thickness of the attenuating layer that reduces the quantity of interest of a unidirectional beam of infinitesimal width to half of its initial value."@en ;
    rdfs:subClassOf ns1:AtomicAndNuclearPhysicsQuantity,
        ns1:Thickness ;
    skos:prefLabel "HalfValueThickness"@en ;
    ns1:IEVReference "https://www.electropedia.org/iev/iev.nsf/display?openform&ievref=881-04-34"^^xsd:string ;
    ns1:ISO80000Reference "10-53"^^xsd:string ;
    ns1:elucidation "Thickness of the attenuating layer that reduces the quantity of interest of a unidirectional beam of infinitesimal width to half of its initial value."@en ;
    ns1:qudtReference "https://qudt.org/vocab/quantitykind/Half-ValueThickness"^^xsd:string ;
    ns1:wikidataReference "https://www.wikidata.org/wiki/Q127526"^^xsd:string .

ns1:HallCoefficient a owl:Class ;
    rdfs:label "HallCoefficient"@en ;
    rdfs:comment "The relation between electric field strength and current density in an isotropic conductor."@en ;
    rdfs:subClassOf [ a owl:Restriction ;
            owl:onProperty ns1:hasMeasurementUnit ;
            owl:someValuesFrom ns1:ReciprocalElectricChargeDensityUnit ],
        ns1:CondensedMatterPhysicsQuantity,
        ns1:ISQDerivedQuantity ;
    skos:prefLabel "HallCoefficient"@en ;
    ns1:IEVReference "https://www.electropedia.org/iev/iev.nsf/display?openform&ievref=521-09-02"^^xsd:string ;
    ns1:ISO80000Reference "12-19"^^xsd:string ;
    ns1:elucidation "The relation between electric field strength and current density in an isotropic conductor."@en ;
    ns1:qudtReference "https://qudt.org/vocab/quantitykind/HallCoefficient"^^xsd:string ;
    ns1:wikidataReference "https://www.wikidata.org/wiki/Q997439"^^xsd:string .

ns1:HartreeEnergy a owl:Class ;
    rdfs:label "HartreeEnergy"^^xsd:string ;
    rdfs:comment "Energy of the electron in a hydrogen atom in its ground state"@en ;
    rdfs:subClassOf ns1:AtomicAndNuclearPhysicsQuantity,
        ns1:Energy ;
    skos:prefLabel "HartreeEnergy"^^xsd:string ;
    ns1:ISO80000Reference "10-8"^^xsd:string ;
    ns1:dbpediaReference "https://dbpedia.org/page/Hartree"^^xsd:string ;
    ns1:elucidation "Energy of the electron in a hydrogen atom in its ground state"@en ;
    ns1:iupacReference "https://doi.org/10.1351/goldbook.H02748"^^xsd:string ;
    ns1:qudtReference "https://qudt.org/vocab/unit/E_h.html"^^xsd:string ;
    ns1:wikidataReference "https://www.wikidata.org/wiki/Q476572"^^xsd:string ;
    ns1:wikipediaReference "https://en.wikipedia.org/wiki/Hartree"^^xsd:string .

ns1:HeatFlowRate a owl:Class ;
    rdfs:label "HeatFlowRate"@en ;
    rdfs:comment "Amount of heat through a surface during a time interval divided by the duration of this interval."@en ;
    rdfs:subClassOf ns1:Power,
        ns1:ThermodynamicalQuantity ;
    owl:disjointWith ns1:DensityOfHeatFlowRate ;
    skos:prefLabel "HeatFlowRate"@en ;
    ns1:IEVReference "https://www.electropedia.org/iev/iev.nsf/display?openform&ievref=113-04-36"@en ;
    ns1:ISO80000Reference "5-7"@en ;
    ns1:elucidation "Amount of heat through a surface during a time interval divided by the duration of this interval."@en ;
    ns1:qudtReference "https://qudt.org/vocab/quantitykind/HeatFlowRate"^^xsd:string ;
    ns1:wikidataReference "https://www.wikidata.org/wiki/Q12160631"^^xsd:string .

ns1:Height a owl:Class ;
    rdfs:label "Height"@en ;
    rdfs:comment "Minimum length of a straight line segment between a point and a reference line or reference surface."@en ;
    rdfs:subClassOf ns1:Length ;
    skos:prefLabel "Height"@en ;
    ns1:IEVReference "https://www.electropedia.org/iev/iev.nsf/display?openform&ievref=113-01-21"^^xsd:string ;
    ns1:ISO80000Reference "3-1.3"^^xsd:string ;
    ns1:dbpediaReference "https://dbpedia.org/page/Height"^^xsd:string ;
    ns1:elucidation "Minimum length of a straight line segment between a point and a reference line or reference surface."@en ;
    ns1:qudtReference "https://qudt.org/vocab/quantitykind/Height"^^xsd:string ;
    ns1:wikidataReference "https://www.wikidata.org/wiki/Q208826"^^xsd:string ;
    ns1:wikipediaReference "https://en.wikipedia.org/wiki/Height"^^xsd:string .

ns1:HelmholtzEnergy a owl:Class ;
    rdfs:label "HelmholtzEnergy"@en ;
    rdfs:comment "Internal energy minus the product of thermodynamic temperature and entropy."@en ;
    rdfs:subClassOf ns1:Energy,
        ns1:ThermodynamicalQuantity ;
    skos:altLabel "HelmholtzFreeEnergy"@en ;
    skos:prefLabel "HelmholtzEnergy"@en ;
    ns1:IEVReference "https://www.electropedia.org/iev/iev.nsf/display?openform&ievref=113-04-24"^^xsd:string ;
    ns1:ISO80000Reference "5-20.4"^^xsd:string ;
    ns1:elucidation "Internal energy minus the product of thermodynamic temperature and entropy."@en ;
    ns1:iupacReference "https://doi.org/10.1351/goldbook.H02772"^^xsd:string ;
    ns1:wikidataReference "https://www.wikidata.org/wiki/Q865821"^^xsd:string .

ns1:HoleDensity a owl:Class ;
    rdfs:label "HoleDensity"@en ;
    rdfs:comment "Number of holes in valence band per volume."@en ;
    rdfs:subClassOf ns1:CondensedMatterPhysicsQuantity,
        ns1:VolumetricNumberDensity ;
    skos:prefLabel "HoleDensity"@en ;
    ns1:ISO80000Reference "12-29.2"^^xsd:string ;
    ns1:elucidation "Number of holes in valence band per volume."@en ;
    ns1:qudtReference "https://qudt.org/vocab/quantitykind/HoleDensity"^^xsd:string ;
    ns1:wikidataReference "https://www.wikidata.org/wiki/Q105971101"^^xsd:string .

ns1:HyperfineStructureQuantumNumber a owl:Class ;
    rdfs:label "HyperfineStructureQuantumNumber"^^xsd:string ;
    rdfs:comment "Quantum number of an atom describing the inclination of the nuclear spin with respect to a quantization axis given by the magnetic field produced by the orbital electrons."@en ;
    rdfs:subClassOf ns1:QuantumNumber ;
    skos:prefLabel "HyperfineStructureQuantumNumber"^^xsd:string ;
    ns1:ISO80000Reference "10-13.8"^^xsd:string ;
    ns1:elucidation "Quantum number of an atom describing the inclination of the nuclear spin with respect to a quantization axis given by the magnetic field produced by the orbital electrons."@en ;
    ns1:qudtReference "https://qudt.org/vocab/quantitykind/HyperfineStructureQuantumNumber"^^xsd:string ;
    ns1:wikidataReference "https://www.wikidata.org/wiki/Q97577449"^^xsd:string .

ns1:HyperfineTransitionFrequencyOfCs a owl:Class ;
    rdfs:label "HyperfineTransitionFrequencyOfCs"@en ;
    rdfs:comment """The frequency standard in the SI system in which the photon absorption by transitions between the two hyperfine ground states of caesium-133 atoms are used to control the output frequency.

It defines the base unit second in the SI system."""@en ;
    rdfs:subClassOf ns1:Frequency,
        ns1:SIExactConstant ;
    skos:prefLabel "HyperfineTransitionFrequencyOfCs"@en ;
    ns1:elucidation """The frequency standard in the SI system in which the photon absorption by transitions between the two hyperfine ground states of caesium-133 atoms are used to control the output frequency.

It defines the base unit second in the SI system."""@en .

ns1:IEVReference a owl:AnnotationProperty ;
    rdfs:label "IEVReference"@en ;
    ns2:python_name "IEVReference"@en ;
    rdfs:comment "URL for the entry in the International Electrotechnical Vocabulary (IEV)."@en ;
    rdfs:seeAlso "https://www.electropedia.org/"^^xsd:string ;
    rdfs:subPropertyOf rdfs:seeAlso ;
    skos:prefLabel "IEVReference"@en ;
    ns1:elucidation "URL for the entry in the International Electrotechnical Vocabulary (IEV)."@en .

ns1:ISO80000Reference a owl:AnnotationProperty ;
    rdfs:label "ISO80000Reference"@en ;
    ns2:python_name "ISO80000Reference"@en ;
    rdfs:comment "Corresponding item number in ISO 80 000."@en ;
    rdfs:seeAlso "https://www.iso.org/obp/ui/#iso:std:iso:80000:-1:ed-1:v1:en"@en ;
    rdfs:subPropertyOf rdfs:seeAlso ;
    skos:example "3-1.1  (ISO80000 reference to length)"@en ;
    skos:prefLabel "ISO80000Reference"@en ;
    ns1:elucidation "Corresponding item number in ISO 80 000."@en .

ns1:ISQBaseQuantity a owl:Class ;
    rdfs:label "ISQBaseQuantity"@en ;
    rdfs:comment "Base quantities defined in the International System of Quantities (ISQ)."@en ;
    rdfs:subClassOf ns1:BaseQuantity,
        ns1:InternationalSystemOfQuantity ;
    owl:disjointUnionOf ( ns1:LuminousIntensity ns1:AmountOfSubstance ns1:ThermodynamicTemperature ns1:ElectricCurrent ns1:Length ns1:Time ns1:Mass ) ;
    skos:prefLabel "ISQBaseQuantity"@en ;
    ns1:elucidation "Base quantities defined in the International System of Quantities (ISQ)."@en ;
    ns1:wikipediaReference "https://en.wikipedia.org/wiki/International_System_of_Quantities"^^xsd:string .

ns1:Illuminance a owl:Class ;
    rdfs:label "Illuminance"@en ;
    rdfs:comment "The total luminous flux incident on a surface, per unit area."@en ;
    rdfs:subClassOf [ a owl:Restriction ;
            owl:onProperty ns1:hasMeasurementUnit ;
            owl:someValuesFrom ns1:LuminanceUnit ],
        ns1:ISQDerivedQuantity ;
    skos:prefLabel "Illuminance"@en ;
    ns1:elucidation "The total luminous flux incident on a surface, per unit area."@en ;
    ns1:iupacReference "https://doi.org/10.1351/goldbook.I02941"^^xsd:string ;
    ns1:qudtReference "http://qudt.org/vocab/quantitykind/Illuminance"^^xsd:string .

ns1:IlluminanceTimeUnit a owl:Class ;
    rdfs:label "IlluminanceTimeUnit"@en ;
    rdfs:comment "The class of units with dimensionality 'IlluminanceTime'."@en .

ns1:InfiniteMultiplicationFactor a owl:Class ;
    rdfs:label "InfiniteMultiplicationFactor"@en ;
    rdfs:comment "In nuclear physics, the multiplication factor for an infinite medium."@en ;
    rdfs:subClassOf ns1:AtomicAndNuclearPhysicsQuantity,
        ns1:ISQDimensionlessQuantity ;
    skos:prefLabel "InfiniteMultiplicationFactor"@en ;
    ns1:ISO80000Reference "10-78.2"^^xsd:string ;
    ns1:elucidation "In nuclear physics, the multiplication factor for an infinite medium."@en ;
    ns1:qudtReference "https://qudt.org/vocab/quantitykind/InfiniteMultiplicationFactor"^^xsd:string ;
    ns1:wikidataReference "https://www.wikidata.org/wiki/Q99440487"^^xsd:string .

ns1:InternalConversionFactor a owl:Class ;
    rdfs:label "InternalConversionFactor"@en ;
    rdfs:comment "Quotient of the number of internal conversion electrons and the number of gamma quanta emitted by the radioactive atom in a given transition, where a conversion electron represents an orbital electron emitted through the radioactive decay."@en ;
    rdfs:subClassOf ns1:AtomicAndNuclearPhysicsQuantity,
        ns1:RatioQuantity ;
    skos:altLabel "InternalConversionCoefficient"@en ;
    skos:prefLabel "InternalConversionFactor"@en ;
    ns1:IEVReference "https://www.electropedia.org/iev/iev.nsf/display?openform&ievref=395-02-57"^^xsd:string ;
    ns1:ISO80000Reference "10-35"^^xsd:string ;
    ns1:elucidation "Quotient of the number of internal conversion electrons and the number of gamma quanta emitted by the radioactive atom in a given transition, where a conversion electron represents an orbital electron emitted through the radioactive decay."@en ;
    ns1:qudtReference "https://qudt.org/vocab/quantitykind/InternalConversionFactor"^^xsd:string ;
    ns1:wikidataReference "https://www.wikidata.org/wiki/Q6047819"^^xsd:string .

ns1:InternalEnergy a owl:Class ;
    rdfs:label "InternalEnergy"@en ;
    rdfs:comment "A state quantity equal to the difference between the total energy of a system and the sum of the macroscopic kinetic and potential energies of the system."@en ;
    rdfs:subClassOf ns1:Energy ;
    skos:altLabel "ThermodynamicEnergy"@en ;
    skos:prefLabel "InternalEnergy"@en ;
    ns1:ISO80000Reference "5.20-2"^^xsd:string ;
    ns1:elucidation "A state quantity equal to the difference between the total energy of a system and the sum of the macroscopic kinetic and potential energies of the system."@en ;
    ns1:iupacReference "https://doi.org/10.1351/goldbook.I03103"^^xsd:string ;
    ns1:qudtReference "http://qudt.org/vocab/quantitykind/InternalEnergy"^^xsd:string .

ns1:IntrinsicCarrierDensity a owl:Class ;
    rdfs:label "IntrinsicCarrierDensity"@en ;
    rdfs:comment "Square root of the product of electron and hole density in a semiconductor."@en ;
    rdfs:subClassOf ns1:CondensedMatterPhysicsQuantity,
        ns1:ReciprocalVolume ;
    skos:prefLabel "IntrinsicCarrierDensity"@en ;
    ns1:ISO80000Reference "12-29.3"^^xsd:string ;
    ns1:elucidation "Square root of the product of electron and hole density in a semiconductor."@en ;
    ns1:qudtReference "https://qudt.org/vocab/quantitykind/IntinsicCarrierDensity"@en ;
    ns1:wikidataReference "https://www.wikidata.org/wiki/Q1303188"^^xsd:string .

ns1:InversePermittivityUnit a owl:Class ;
    rdfs:label "InversePermittivityUnit"@en ;
    rdfs:comment "The class of units with dimensionality 'InversePermittivity'."@en .

ns1:IonNumberDensity a owl:Class ;
    rdfs:label "IonNumberDensity"@en ;
    rdfs:comment "Number of ions per volume."@en ;
    rdfs:subClassOf [ a owl:Restriction ;
            owl:onProperty ns1:hasMeasurementUnit ;
            owl:someValuesFrom ns1:PerVolumeUnit ],
        ns1:AtomicAndNuclearPhysicsQuantity,
        ns1:ISQDerivedQuantity ;
    skos:altLabel "IonDensity"@en ;
    skos:prefLabel "IonNumberDensity"@en ;
    ns1:ISO80000Reference "10-62.2"^^xsd:string ;
    ns1:elucidation "Number of ions per volume."@en ;
    ns1:wikidataReference "https://www.wikidata.org/wiki/Q98831218"^^xsd:string .

ns1:IonTransportNumber a owl:Class ;
    rdfs:label "IonTransportNumber"@en ;
    rdfs:comment "Faction of electrical current carried by given ionic species."@en ;
    rdfs:subClassOf ns1:PhysioChemicalQuantity,
        ns1:RatioQuantity ;
    skos:altLabel "CurrentFraction"@en,
        "TransferrenceNumber"@en ;
    skos:prefLabel "IonTransportNumber"@en ;
    ns1:ISO80000Reference "9-46"^^xsd:string ;
    ns1:elucidation "Faction of electrical current carried by given ionic species."@en ;
    ns1:iupacReference "https://doi.org/10.1351/goldbook.I03181"^^xsd:string,
        "https://doi.org/10.1351/goldbook.T06489"^^xsd:string ;
    ns1:qudtReference "https://qudt.org/vocab/quantitykind/IonTransportNumber"^^xsd:string ;
    ns1:wikidataReference "https://www.wikidata.org/wiki/Q331854"^^xsd:string .

ns1:IonicStrength a owl:Class ;
    rdfs:label "IonicStrength"@en ;
    rdfs:comment "Charge number is a quantity of dimension one defined in ChargeNumber."@en,
        "For all types of ions in a solution, half the sum of the products of their molality b_i and the square of their charge number z_i."@en ;
    rdfs:subClassOf [ a owl:Restriction ;
            owl:onProperty ns1:hasMeasurementUnit ;
            owl:someValuesFrom ns1:AmountPerMassUnit ],
        ns1:ISQDerivedQuantity,
        ns1:PhysioChemicalQuantity ;
    skos:prefLabel "IonicStrength"@en ;
    ns1:IEVReference "https://www.electropedia.org/iev/iev.nsf/display?openform&ievref=114-01-24"^^xsd:string ;
    ns1:ISO80000Reference "9-42"^^xsd:string ;
    ns1:elucidation "For all types of ions in a solution, half the sum of the products of their molality b_i and the square of their charge number z_i."@en ;
    ns1:iupacReference "https://doi.org/10.1351/goldbook.I03180"^^xsd:string ;
    ns1:qudtReference "https://qudt.org/vocab/quantitykind/IonicStrength"^^xsd:string ;
    ns1:wikidataReference "https://www.wikidata.org/wiki/Q898396"^^xsd:string .

ns1:IonizationEnergy a owl:Class ;
    rdfs:label "IonizationEnergy"@en ;
    rdfs:comment "Difference between energy of an electron at rest at infinity and a certain energy level which is the energy of an electron in the interior of a substance."@en ;
    rdfs:subClassOf ns1:CondensedMatterPhysicsQuantity,
        ns1:Energy ;
    skos:prefLabel "IonizationEnergy"@en ;
    ns1:IEVReference "https://www.electropedia.org/iev/iev.nsf/display?openform&ievref=113-06-39"^^xsd:string ;
    ns1:ISO80000Reference "12-24.2"^^xsd:string ;
    ns1:elucidation "Difference between energy of an electron at rest at infinity and a certain energy level which is the energy of an electron in the interior of a substance."@en ;
    ns1:iupacReference "https://doi.org/10.1351/goldbook.I03199"^^xsd:string ;
    ns1:qudtReference "https://qudt.org/vocab/quantitykind/IonizationEnergy"^^xsd:string ;
    ns1:wikidataReference "https://www.wikidata.org/wiki/Q483769"^^xsd:string .

ns1:IsentropicCompressibility a owl:Class ;
    rdfs:label "IsentropicCompressibility"@en ;
    rdfs:comment "Quantity characterizing the relative variation of volume V with pressure p at constant entropy."@en ;
    rdfs:subClassOf ns1:Compressibility,
        ns1:ThermodynamicalQuantity ;
    skos:prefLabel "IsentropicCompressibility"@en ;
    ns1:IEVReference "https://www.electropedia.org/iev/iev.nsf/display?openform&ievref=113-04-32"^^xsd:string ;
    ns1:ISO80000Reference "5-5.2"^^xsd:string ;
    ns1:elucidation "Quantity characterizing the relative variation of volume V with pressure p at constant entropy."@en ;
    ns1:note "The coherent SI unit of isentropic compressibility is pascal to the power minus one, 1/Pa."@en ;
    ns1:qudtReference "https://qudt.org/vocab/quantitykind/IsentropicCompressibility"^^xsd:string ;
    ns1:wikidataReference "https://www.wikidata.org/wiki/Q2990695"^^xsd:string .

ns1:IsentropicExponent a owl:Class ;
    rdfs:label "IsentropicExponent"@en ;
    rdfs:comment "For an ideal gas, isentropic exponent is equal to ratio of the specific heat capacities."@en ;
    rdfs:subClassOf ns1:ISQDimensionlessQuantity,
        ns1:ThermodynamicalQuantity ;
    skos:prefLabel "IsentropicExponent"@en ;
    ns1:IEVReference "https://www.electropedia.org/iev/iev.nsf/display?openform&ievref=113-04-52"^^xsd:string ;
    ns1:ISO80000Reference "5-17.2"^^xsd:string ;
    ns1:elucidation "For an ideal gas, isentropic exponent is equal to ratio of the specific heat capacities."@en ;
    ns1:qudtReference "https://qudt.org/vocab/quantitykind/IsentropicExponent"^^xsd:string ;
    ns1:wikidataReference "https://www.wikidata.org/wiki/Q75775739"^^xsd:string .

ns1:IsobaricHeatCapacity a owl:Class ;
    rdfs:label "IsobaricHeatCapacity"@en ;
    rdfs:comment "Heat capacity at constant pressure."@en ;
    rdfs:subClassOf ns1:HeatCapacity ;
    skos:altLabel "HeatCapacityAtConstantPressure"@en ;
    skos:prefLabel "IsobaricHeatCapacity"@en ;
    ns1:IEVReference "https://www.electropedia.org/iev/iev.nsf/display?openform&ievref=113-04-49"^^xsd:string ;
    ns1:ISO80000Reference "5-16.2"^^xsd:string ;
    ns1:elucidation "Heat capacity at constant pressure."@en ;
    ns1:wikidataReference "https://www.wikidata.org/wiki/Q112187490"^^xsd:string .

ns1:IsochoricHeatCapacity a owl:Class ;
    rdfs:label "IsochoricHeatCapacity"@en ;
    rdfs:comment "Heat capacity at constant volume."@en ;
    rdfs:subClassOf ns1:HeatCapacity ;
    skos:altLabel "HeatCapacityAtConstantVolume"@en ;
    skos:prefLabel "IsochoricHeatCapacity"@en ;
    ns1:IEVReference "https://www.electropedia.org/iev/iev.nsf/display?openform&ievref=113-04-50"^^xsd:string ;
    ns1:ISO80000Reference "5-16.3"^^xsd:string ;
    ns1:elucidation "Heat capacity at constant volume."@en ;
    ns1:wikidataReference "https://www.wikidata.org/wiki/Q112187521"^^xsd:string .

ns1:IsothermalCompressibility a owl:Class ;
    rdfs:label "IsothermalCompressibility"@en ;
    rdfs:subClassOf ns1:Compressibility,
        ns1:ThermodynamicalQuantity ;
    skos:prefLabel "IsothermalCompressibility"@en ;
    ns1:IEVReference "https://www.electropedia.org/iev/iev.nsf/display?openform&ievref=113-04-31"^^xsd:string ;
    ns1:ISO80000Reference "5-5.1"^^xsd:string ;
    ns1:note "Quantity characterising the relative variation of volume with pressure at constant thermodynamic temperature."@en ;
    ns1:qudtReference "https://qudt.org/vocab/quantitykind/IsothermalCompressibility"^^xsd:string ;
    ns1:wikidataReference "https://www.wikidata.org/wiki/Q2990696"^^xsd:string .

ns1:JosephsonConstant a owl:Class ;
    rdfs:label "JosephsonConstant"@en ;
    rdfs:comment "Inverse of the magnetic flux quantum."@en,
        "The DBpedia definition (http://dbpedia.org/page/Magnetic_flux_quantum) is outdated as May 20, 2019. It is now an exact quantity."@en ;
    rdfs:subClassOf [ a owl:Restriction ;
            owl:onProperty ns1:hasMeasurementUnit ;
            owl:someValuesFrom ns1:ElectricCurrentPerEnergyUnit ],
        ns1:SIExactConstant ;
    skos:prefLabel "JosephsonConstant"@en ;
    ns1:elucidation "Inverse of the magnetic flux quantum."@en ;
    ns1:qudtReference "http://qudt.org/vocab/constant/JosephsonConstant"^^xsd:string .

ns1:Kerma a owl:Class ;
    rdfs:label "Kerma"@en ;
    rdfs:comment "Kinetic energy released per mass."@en ;
    rdfs:subClassOf ns1:AtomicAndNuclearPhysicsQuantity,
        ns1:SpecificEnergy ;
    skos:prefLabel "Kerma"@en ;
    ns1:IEVReference "https://www.electropedia.org/iev/iev.nsf/display?openform&ievref=395-01-36"^^xsd:string ;
    ns1:ISO80000Reference "10-86.1"^^xsd:string ;
    ns1:elucidation "Kinetic energy released per mass."@en ;
    ns1:qudtReference "https://qudt.org/vocab/quantitykind/Kerma"^^xsd:string ;
    ns1:wikidataReference "https://www.wikidata.org/wiki/Q1739288"^^xsd:string .

ns1:KermaRate a owl:Class ;
    rdfs:label "KermaRate"@en ;
    rdfs:comment "Time derivative of kerma."@en ;
    rdfs:subClassOf [ a owl:Restriction ;
            owl:onProperty ns1:hasMeasurementUnit ;
            owl:someValuesFrom ns1:AbsorbedDoseRateUnit ],
        ns1:AtomicAndNuclearPhysicsQuantity,
        ns1:ISQDerivedQuantity ;
    skos:prefLabel "KermaRate"@en ;
    ns1:IEVReference "https://www.electropedia.org/iev/iev.nsf/display?openform&ievref=881-12-28"^^xsd:string ;
    ns1:ISO80000Reference "10-86.2"^^xsd:string ;
    ns1:elucidation "Time derivative of kerma."@en ;
    ns1:qudtReference "https://qudt.org/vocab/quantitykind/KermaRate"^^xsd:string ;
    ns1:wikidataReference "https://www.wikidata.org/wiki/Q99713105"^^xsd:string .

ns1:KinematicViscosity a owl:Class ;
    rdfs:label "KinematicViscosity"@en ;
    rdfs:comment "Quotient of dynamic viscosity and mass density of a fluid."@en ;
    rdfs:subClassOf [ a owl:Restriction ;
            owl:onProperty ns1:hasMeasurementUnit ;
            owl:someValuesFrom ns1:AreicSpeedUnit ],
        ns1:MechanicalQuantity ;
    skos:prefLabel "KinematicViscosity"@en ;
    ns1:IEVReference "https://www.electropedia.org/iev/iev.nsf/display?openform&ievref=113-03-35"^^xsd:string ;
    ns1:ISO80000Reference "4-25"^^xsd:string ;
    ns1:elucidation "Quotient of dynamic viscosity and mass density of a fluid."@en ;
    ns1:iupacReference "https://doi.org/10.1351/goldbook.K03395"^^xsd:string ;
    ns1:qudtReference "https://qudt.org/vocab/quantitykind/KinematicViscosity"^^xsd:string ;
    ns1:wikidataReference "https://www.wikidata.org/wiki/Q15106259"^^xsd:string .

ns1:KineticEnergy a owl:Class ;
    rdfs:label "KineticEnergy"@en ;
    rdfs:comment "The energy of an object due to its motion."@en ;
    rdfs:subClassOf ns1:Energy ;
    skos:prefLabel "KineticEnergy"@en ;
    ns1:ISO80000Reference "4-28.2"^^xsd:string ;
    ns1:elucidation "The energy of an object due to its motion."@en ;
    ns1:iupacReference "https://doi.org/10.1351/goldbook.K03402"^^xsd:string ;
    ns1:qudtReference "http://qudt.org/vocab/quantitykind/KineticEnergy"^^xsd:string .

ns1:KineticFrictionFactor a owl:Class ;
    rdfs:label "KineticFrictionFactor"@en ;
    rdfs:subClassOf ns1:CoefficientOfFriction,
        ns1:MechanicalQuantity ;
    skos:altLabel "DynamicFrictionFactor"@en ;
    skos:prefLabel "KineticFrictionFactor"@en ;
    ns1:IEVReference "https://www.electropedia.org/iev/iev.nsf/display?openform&ievref=113-03-32"^^xsd:string ;
    ns1:ISO80000Reference "4-23.2"^^xsd:string ;
    ns1:wikidataReference "https://www.wikidata.org/wiki/Q73695445"^^xsd:string .

ns1:KineticFrictionForce a owl:Class ;
    rdfs:label "KineticFrictionForce"@en ;
    rdfs:comment "Force opposing the motion of a body sliding on a surface."@en ;
    rdfs:subClassOf ns1:Force,
        ns1:MechanicalQuantity ;
    skos:altLabel "DynamicFrictionForce"@en ;
    skos:prefLabel "KineticFrictionForce"@en ;
    ns1:ISO80000Reference "4-9.4"^^xsd:string ;
    ns1:elucidation "Force opposing the motion of a body sliding on a surface."@en ;
    ns1:wikidataReference "https://www.wikidata.org/wiki/Q91005629"^^xsd:string .

ns1:LandeFactor a owl:Class ;
    rdfs:label "LandeFactor"^^xsd:string ;
    rdfs:comment "Quotient of the magnetic dipole moment of an atom, and the product of the total angular momentum quantum number and the Bohr magneton."@en ;
    rdfs:subClassOf ns1:AtomicAndNuclearPhysicsQuantity,
        ns1:GFactor ;
    skos:altLabel "GFactorOfAtom"@en ;
    skos:prefLabel "LandeFactor"^^xsd:string ;
    ns1:ISO80000Reference "10-14.1"^^xsd:string ;
    ns1:elucidation "Quotient of the magnetic dipole moment of an atom, and the product of the total angular momentum quantum number and the Bohr magneton."@en ;
    ns1:qudtReference "https://qudt.org/vocab/quantitykind/LandeGFactor"^^xsd:string ;
    ns1:wikidataReference "https://www.wikidata.org/wiki/Q1191684"^^xsd:string .

ns1:LarmonAngularFrequency a owl:Class ;
    rdfs:label "LarmonAngularFrequency"@en ;
    rdfs:comment "Angular frequency of the electron angular momentum vector precession about the axis of an external magnetic field."@en ;
    rdfs:subClassOf ns1:AngularFrequency,
        ns1:AtomicAndNuclearPhysicsQuantity ;
    skos:prefLabel "LarmonAngularFrequency"@en ;
    ns1:ISO80000Reference "10-15.1"^^xsd:string ;
    ns1:elucidation "Angular frequency of the electron angular momentum vector precession about the axis of an external magnetic field."@en .

ns1:LarmonFrequency a owl:Class ;
    rdfs:label "LarmonFrequency"@en ;
    rdfs:comment "Quotient of Larmor angular frequency and 2π."@en ;
    rdfs:subClassOf ns1:AtomicAndNuclearPhysicsQuantity,
        ns1:Frequency ;
    skos:prefLabel "LarmonFrequency"@en ;
    ns1:ISO80000Reference "10-15.2"^^xsd:string ;
    ns1:elucidation "Quotient of Larmor angular frequency and 2π."@en .

ns1:LatentHeatOfPhaseTransition a owl:Class ;
    rdfs:label "LatentHeatOfPhaseTransition"@en ;
    rdfs:comment "Energy to be added to or removed from a system under constant temperature and pressure to undergo a complete phase transition."@en ;
    rdfs:subClassOf ns1:LatentHeat,
        ns1:PhysioChemicalQuantity ;
    skos:prefLabel "LatentHeatOfPhaseTransition"@en ;
    ns1:ISO80000Reference "9-16"^^xsd:string ;
    ns1:elucidation "Energy to be added to or removed from a system under constant temperature and pressure to undergo a complete phase transition."@en ;
    ns1:wikidataReference "https://www.wikidata.org/wiki/Q106553458"^^xsd:string .

ns1:LatticePlaneSpacing a owl:Class ;
    rdfs:label "LatticePlaneSpacing"@en ;
    rdfs:comment "distance between successive lattice planes"@en ;
    rdfs:subClassOf ns1:CondensedMatterPhysicsQuantity,
        ns1:Distance ;
    skos:prefLabel "LatticePlaneSpacing"@en ;
    ns1:ISO80000Reference "12-3"^^xsd:string ;
    ns1:elucidation "distance between successive lattice planes"@en ;
    ns1:qudtReference "https://qudt.org/vocab/quantitykind/LatticePlaneSpacing"^^xsd:string ;
    ns1:wikidataReference "https://www.wikidata.org/wiki/Q105488046"^^xsd:string .

ns1:LatticeVector a owl:Class ;
    rdfs:label "LatticeVector"@en ;
    rdfs:comment "translation vector that maps the crystal lattice on itself"@en ;
    rdfs:subClassOf [ a owl:Restriction ;
            owl:onProperty ns1:hasMeasurementUnit ;
            owl:someValuesFrom ns1:LengthUnit ],
        ns1:CondensedMatterPhysicsQuantity,
        ns1:Displacement ;
    skos:prefLabel "LatticeVector"@en ;
    ns1:ISO80000Reference "12-1.1"^^xsd:string ;
    ns1:elucidation "translation vector that maps the crystal lattice on itself"@en ;
    ns1:qudtReference "https://qudt.org/vocab/quantitykind/LatticeVector"^^xsd:string ;
    ns1:wikidataReference "https://www.wikidata.org/wiki/Q105435234"^^xsd:string .

ns1:LeakageFactor a owl:Class ;
    rdfs:label "LeakageFactor"@en ;
    rdfs:comment "One minus the square of the coupling factor"@en ;
    rdfs:subClassOf ns1:ElectromagneticQuantity,
        ns1:ISQDimensionlessQuantity ;
    skos:prefLabel "LeakageFactor"@en ;
    ns1:IEVReference "https://www.electropedia.org/iev/iev.nsf/display?openform&ievref=131-12-42"^^xsd:string ;
    ns1:ISO80000Reference "6-42.2"^^xsd:string ;
    ns1:elucidation "One minus the square of the coupling factor"@en ;
    ns1:wikidataReference "https://www.wikidata.org/wiki/Q78102042"^^xsd:string .

ns1:LengthMassUnit a owl:Class ;
    rdfs:label "LengthMassUnit"@en ;
    rdfs:comment "The class of units with dimensionality 'LengthMass'."@en .

ns1:LengthPerAmountUnit a owl:Class ;
    rdfs:label "LengthPerAmountUnit"@en ;
    rdfs:comment "The class of units with dimensionality 'LengthPerAmount'."@en .

ns1:LengthPerTemperatureUnit a owl:Class ;
    rdfs:label "LengthPerTemperatureUnit"@en ;
    rdfs:comment "The class of units with dimensionality 'LengthPerTemperature'."@en .

ns1:LengthTemperatureUnit a owl:Class ;
    rdfs:label "LengthTemperatureUnit"@en ;
    rdfs:comment "The class of units with dimensionality 'LengthTemperature'."@en .

ns1:LengthTimePerMassUnit a owl:Class ;
    rdfs:label "LengthTimePerMassUnit"@en ;
    rdfs:comment "The class of units with dimensionality 'LengthTimePerMass'."@en .

ns1:LengthTimeTemperatureUnit a owl:Class ;
    rdfs:label "LengthTimeTemperatureUnit"@en ;
    rdfs:comment "The class of units with dimensionality 'LengthTimeTemperature'."@en .

ns1:Lethargy a owl:Class ;
    rdfs:label "Lethargy"@en ;
    rdfs:comment "Natural logarithm of the quotient of a reference energy and the kinetic energy of a neutron."@en ;
    rdfs:subClassOf ns1:AtomicAndNuclearPhysicsQuantity,
        ns1:ISQDimensionlessQuantity ;
    skos:prefLabel "Lethargy"@en ;
    ns1:IEVReference "https://www.electropedia.org/iev/iev.nsf/display?openform&ievref=395-07-01"^^xsd:string ;
    ns1:ISO80000Reference "10-69"^^xsd:string ;
    ns1:elucidation "Natural logarithm of the quotient of a reference energy and the kinetic energy of a neutron."@en ;
    ns1:qudtReference "https://qudt.org/vocab/quantitykind/Lethargy"^^xsd:string ;
    ns1:wikidataReference "https://www.wikidata.org/wiki/Q25508781"^^xsd:string .

ns1:LevelWidth a owl:Class ;
    rdfs:label "LevelWidth"@en ;
    rdfs:comment "In nuclear physics, quotient of the reduced Planck constant and the mean duration of life of an unstable particle or an excited state."@en ;
    rdfs:subClassOf ns1:AtomicAndNuclearPhysicsQuantity,
        ns1:Energy ;
    skos:prefLabel "LevelWidth"@en ;
    ns1:ISO80000Reference "10-26"^^xsd:string ;
    ns1:elucidation "In nuclear physics, quotient of the reduced Planck constant and the mean duration of life of an unstable particle or an excited state."@en ;
    ns1:iupacReference "https://doi.org/10.1351/goldbook.L03507"^^xsd:string ;
    ns1:qudtReference "https://qudt.org/vocab/quantitykind/LevelWidth"^^xsd:string ;
    ns1:wikidataReference "https://www.wikidata.org/wiki/Q98082340"^^xsd:string .

ns1:LinearAttenuationCoefficient a owl:Class ;
    rdfs:label "LinearAttenuationCoefficient"@en ;
    rdfs:comment "In nuclear physics, fraction of interacting particles per distance traversed in a given material."@en ;
    rdfs:subClassOf ns1:AtomicAndNuclearPhysicsQuantity,
        ns1:ReciprocalLength ;
    skos:prefLabel "LinearAttenuationCoefficient"@en ;
    ns1:IEVReference "https://www.electropedia.org/iev/iev.nsf/display?openform&ievref=881-04-31"^^xsd:string ;
    ns1:ISO80000Reference "10-49"^^xsd:string ;
    ns1:elucidation "In nuclear physics, fraction of interacting particles per distance traversed in a given material."@en ;
    ns1:wikidataReference "https://www.wikidata.org/wiki/Q98583077"^^xsd:string .

ns1:LinearDensityOfElectricCharge a owl:Class ;
    rdfs:label "LinearDensityOfElectricCharge"@en ;
    rdfs:comment "The derivative of the electric charge of a system with respect to the length."@en ;
    rdfs:subClassOf [ a owl:Restriction ;
            owl:onProperty ns1:hasMeasurementUnit ;
            owl:someValuesFrom ns1:ElectricChargePerLengthUnit ],
        ns1:ElectromagneticQuantity,
        ns1:ISQDerivedQuantity ;
    skos:prefLabel "LinearDensityOfElectricCharge"@en ;
    ns1:IEVReference "https://www.electropedia.org/iev/iev.nsf/display?openform&ievref=121-11-09"^^xsd:string ;
    ns1:ISO80000Reference "6-5"^^xsd:string ;
    ns1:elucidation "The derivative of the electric charge of a system with respect to the length."@en ;
    ns1:wikidataReference "https://www.wikidata.org/wiki/Q77267838"^^xsd:string .

ns1:LinearElectricCurrentDensity a owl:Class ;
    rdfs:label "LinearElectricCurrentDensity"@en ;
    rdfs:comment "Surface density of electric charge multiplied by velocity"@en ;
    rdfs:subClassOf [ a owl:Restriction ;
            owl:onProperty ns1:hasMeasurementUnit ;
            owl:someValuesFrom ns1:MagneticFieldStrengthUnit ],
        ns1:ElectromagneticQuantity,
        ns1:ISQDerivedQuantity ;
    skos:prefLabel "LinearElectricCurrentDensity"@en ;
    ns1:IEVReference "https://www.electropedia.org/iev/iev.nsf/display?openform&ievref=121-11-12"^^xsd:string ;
    ns1:ISO80000Reference "6-9"^^xsd:string ;
    ns1:elucidation "Surface density of electric charge multiplied by velocity"@en ;
    ns1:qudtReference "https://qudt.org/vocab/quantitykind/LinearElectricCurrentDensity"^^xsd:string ;
    ns1:wikidataReference "https://www.wikidata.org/wiki/Q2356741"^^xsd:string .

ns1:LinearEnergyTransfer a owl:Class ;
    rdfs:label "LinearEnergyTransfer"@en ;
    rdfs:comment "Measure for the energy lost by charged particles per traversed distance, including only interactions up to a given energy."@en ;
    rdfs:subClassOf [ a owl:Restriction ;
            owl:onProperty ns1:hasMeasurementUnit ;
            owl:someValuesFrom ns1:ForceUnit ],
        ns1:AtomicAndNuclearPhysicsQuantity,
        ns1:ISQDerivedQuantity ;
    skos:prefLabel "LinearEnergyTransfer"@en ;
    ns1:IEVReference "https://www.electropedia.org/iev/iev.nsf/display?openform&ievref=395-01-30"^^xsd:string ;
    ns1:ISO80000Reference "10-85"^^xsd:string ;
    ns1:elucidation "Measure for the energy lost by charged particles per traversed distance, including only interactions up to a given energy."@en ;
    ns1:iupacReference "https://doi.org/10.1351/goldbook.L03550"^^xsd:string ;
    ns1:qudtReference "https://qudt.org/vocab/quantitykind/LinearEnergyTransfer"^^xsd:string ;
    ns1:wikidataReference "https://www.wikidata.org/wiki/Q1699996"^^xsd:string .

ns1:LinearIonization a owl:Class ;
    rdfs:label "LinearIonization"@en ;
    rdfs:comment "Differential quotient of q with respect to l, where q is the average total charge of all positive ions produced by an ionizing charged particle over a path l, divided by the elementary charge."@en ;
    rdfs:subClassOf ns1:AtomicAndNuclearPhysicsQuantity,
        ns1:ReciprocalLength ;
    skos:prefLabel "LinearIonization"@en ;
    ns1:IEVReference "https://www.electropedia.org/iev/iev.nsf/display?openform&ievref=395-03-115"^^xsd:string ;
    ns1:ISO80000Reference "10-58"^^xsd:string ;
    ns1:elucidation "Differential quotient of q with respect to l, where q is the average total charge of all positive ions produced by an ionizing charged particle over a path l, divided by the elementary charge."@en ;
    ns1:qudtReference "https://qudt.org/vocab/quantitykind/LinearIonization"^^xsd:string ;
    ns1:wikidataReference "https://www.wikidata.org/wiki/Q98690755"^^xsd:string .

ns1:LinearMassDensity a owl:Class ;
    rdfs:label "LinearMassDensity"@en ;
    rdfs:comment "Mass per length."@en ;
    rdfs:subClassOf [ a owl:Restriction ;
            owl:onProperty ns1:hasMeasurementUnit ;
            owl:someValuesFrom ns1:MassPerLengthUnit ],
        ns1:ISQDerivedQuantity,
        ns1:MechanicalQuantity ;
    skos:altLabel "LinearDensity"@en,
        "LineicMass"@en ;
    skos:prefLabel "LinearMassDensity"@en ;
    ns1:IEVReference "https://www.electropedia.org/iev/iev.nsf/display?openform&ievref=113-03-11"^^xsd:string ;
    ns1:ISO80000Reference "4-6"^^xsd:string ;
    ns1:elucidation "Mass per length."@en ;
    ns1:qudtReference "https://qudt.org/vocab/quantitykind/LinearDensity"@en ;
    ns1:wikidataReference "https://www.wikidata.org/wiki/Q56298294"^^xsd:string .

ns1:LinkedFlux a owl:Class ;
    rdfs:label "LinkedFlux"@en ;
    rdfs:comment "Magnetic flux the integration area of which is such that magnetic field lines cross it in the same orientation more than once."@en ;
    rdfs:subClassOf ns1:MagneticFlux ;
    skos:prefLabel "LinkedFlux"@en ;
    ns1:IEVReference "https://www.electropedia.org/iev/iev.nsf/display?openform&ievref=121-11-77"^^xsd:string ;
    ns1:ISO80000Reference "6-22.2"^^xsd:string ;
    ns1:elucidation "Magnetic flux the integration area of which is such that magnetic field lines cross it in the same orientation more than once."@en ;
    ns1:qudtReference "https://qudt.org/vocab/quantitykind/MagneticFlux"^^xsd:string ;
    ns1:wikidataReference "https://www.wikidata.org/wiki/Q4374882"^^xsd:string .

ns1:LogarithmicDecrement a owl:Class ;
    rdfs:label "LogarithmicDecrement"@en ;
    rdfs:comment "Product of damping coefficient and period duration."@en ;
    rdfs:subClassOf ns1:ISQDimensionlessQuantity,
        ns1:SpaceAndTimeQuantity ;
    skos:prefLabel "LogarithmicDecrement"@en ;
    ns1:IEVReference "https://www.electropedia.org/iev/iev.nsf/display?openform&ievref=103-05-25"^^xsd:string ;
    ns1:ISO80000Reference "3-25"^^xsd:string ;
    ns1:elucidation "Product of damping coefficient and period duration."@en ;
    ns1:wikidataReference "https://www.wikidata.org/wiki/Q1399446"^^xsd:string .

ns1:LondonPenetrationDepth a owl:Class ;
    rdfs:label "LondonPenetrationDepth"@en ;
    rdfs:comment "Distance a magnetic field penetrates the plane surface of a semi-finite superconductor."@en ;
    rdfs:subClassOf ns1:CondensedMatterPhysicsQuantity,
        ns1:Length ;
    skos:prefLabel "LondonPenetrationDepth"@en ;
    ns1:IEVReference "https://www.electropedia.org/iev/iev.nsf/display?openform&ievref=815-10-33"^^xsd:string ;
    ns1:ISO80000Reference "12-38.1"^^xsd:string ;
    ns1:elucidation "Distance a magnetic field penetrates the plane surface of a semi-finite superconductor."@en ;
    ns1:qudtReference "https://qudt.org/vocab/quantitykind/LondonPenetrationDepth"^^xsd:string ;
    ns1:wikidataReference "https://www.wikidata.org/wiki/Q3277853"^^xsd:string .

ns1:LongRangeOrderParameter a owl:Class ;
    rdfs:label "LongRangeOrderParameter"@en ;
    rdfs:comment "Fraction of atoms in an Ising ferromagnet having magnetic moments in one direction, minus the fraction having magnetic moments in the opposite direction."@en ;
    rdfs:subClassOf ns1:CondensedMatterPhysicsQuantity,
        ns1:ISQDimensionlessQuantity ;
    skos:prefLabel "LongRangeOrderParameter"@en ;
    ns1:ISO80000Reference "12-5.2"^^xsd:string ;
    ns1:elucidation "Fraction of atoms in an Ising ferromagnet having magnetic moments in one direction, minus the fraction having magnetic moments in the opposite direction."@en ;
    ns1:qudtReference "https://qudt.org/vocab/quantitykind/Long-RangeOrderParameter"^^xsd:string ;
    ns1:wikidataReference "https://www.wikidata.org/wiki/Q105496124"^^xsd:string .

ns1:LorenzCoefficient a owl:Class ;
    rdfs:label "LorenzCoefficient"@en ;
    rdfs:comment "Quotient of thermal conductivity, and the product of electric conductivity and thermodynamic temperature."@en ;
    rdfs:subClassOf [ a owl:Restriction ;
            owl:onProperty ns1:hasMeasurementUnit ;
            owl:someValuesFrom ns1:LorenzNumberUnit ],
        ns1:CondensedMatterPhysicsQuantity,
        ns1:ISQDerivedQuantity ;
    skos:altLabel "LorenzNumber"@en ;
    skos:prefLabel "LorenzCoefficient"@en ;
    ns1:ISO80000Reference "12-18"^^xsd:string ;
    ns1:elucidation "Quotient of thermal conductivity, and the product of electric conductivity and thermodynamic temperature."@en ;
    ns1:qudtReference "https://qudt.org/vocab/quantitykind/LorenzCoefficient"^^xsd:string ;
    ns1:wikidataReference "https://www.wikidata.org/wiki/Q105728754"^^xsd:string .

ns1:LossAngle a owl:Class ;
    rdfs:label "LossAngle"@en ;
    rdfs:comment "Arctan of the loss factor"@en ;
    rdfs:subClassOf ns1:Angle,
        ns1:ElectromagneticQuantity ;
    skos:prefLabel "LossAngle"@en ;
    ns1:IEVReference "https://www.electropedia.org/iev/iev.nsf/display?openform&ievref=131-12-49"^^xsd:string ;
    ns1:ISO80000Reference "6-55"^^xsd:string ;
    ns1:elucidation "Arctan of the loss factor"@en ;
    ns1:qudtReference "https://www.qudt.org/vocab/quantitykind/LossAngle"^^xsd:string ;
    ns1:wikidataReference "https://www.wikidata.org/wiki/Q20820438"^^xsd:string .

ns1:LossFactor a owl:Class ;
    rdfs:label "LossFactor"@en ;
    rdfs:comment "Inverse of the quality factor."@en ;
    rdfs:subClassOf ns1:ElectromagneticQuantity,
        ns1:ISQDimensionlessQuantity ;
    skos:prefLabel "LossFactor"@en ;
    ns1:ISO80000Reference "6-54"^^xsd:string ;
    ns1:elucidation "Inverse of the quality factor."@en ;
    ns1:qudtReference "https://qudt.org/vocab/quantitykind/LossFactor"^^xsd:string ;
    ns1:wikidataReference "https://www.wikidata.org/wiki/Q79468728"^^xsd:string .

ns1:Luminance a owl:Class ;
    rdfs:label "Luminance"@en ;
    rdfs:comment "A photometric measure of the luminous intensity per unit area of light travelling in a given direction."@en,
        "Measured in cd/m². Not to confuse with Illuminance, which is measured in lux (cd sr/m²)."@en ;
    rdfs:subClassOf [ a owl:Restriction ;
            owl:onProperty ns1:hasMeasurementUnit ;
            owl:someValuesFrom ns1:LuminanceUnit ],
        ns1:ISQDerivedQuantity ;
    skos:prefLabel "Luminance"@en ;
    ns1:elucidation "A photometric measure of the luminous intensity per unit area of light travelling in a given direction."@en ;
    ns1:iupacReference "https://doi.org/10.1351/goldbook.L03640"^^xsd:string ;
    ns1:qudtReference "http://qudt.org/vocab/quantitykind/Luminance"^^xsd:string .

ns1:LuminousEfficacyOf540THzRadiation a owl:Class ;
    rdfs:label "LuminousEfficacyOf540THzRadiation"@en ;
    rdfs:comment "Defines the Candela base unit in the SI system."@en,
        "The luminous efficacy of monochromatic radiation of frequency 540 × 10 12 Hz, K cd , is a technical constant that gives an exact numerical relationship between the purely physical characteristics of the radiant power stimulating the human eye (W) and its photobiological response defined by the luminous flux due to the spectral responsivity of a standard observer (lm) at a frequency of 540 × 10 12 hertz."@en ;
    rdfs:subClassOf [ a owl:Restriction ;
            owl:onProperty ns1:hasMeasurementUnit ;
            owl:someValuesFrom ns1:LuminousEfficacyUnit ],
        ns1:SIExactConstant ;
    skos:prefLabel "LuminousEfficacyOf540THzRadiation"@en ;
    ns1:elucidation "The luminous efficacy of monochromatic radiation of frequency 540 × 10 12 Hz, K cd , is a technical constant that gives an exact numerical relationship between the purely physical characteristics of the radiant power stimulating the human eye (W) and its photobiological response defined by the luminous flux due to the spectral responsivity of a standard observer (lm) at a frequency of 540 × 10 12 hertz."@en .

ns1:LuminousFlux a owl:Class ;
    rdfs:label "LuminousFlux"@en ;
    rdfs:comment "Perceived power of light."@en ;
    rdfs:subClassOf [ a owl:Restriction ;
            owl:onProperty ns1:hasMeasurementUnit ;
            owl:someValuesFrom ns1:LuminousIntensityUnit ],
        ns1:ISQDerivedQuantity ;
    skos:prefLabel "LuminousFlux"@en ;
    ns1:ISO80000Reference "7-13"^^xsd:string ;
    ns1:elucidation "Perceived power of light."@en ;
    ns1:iupacReference "https://doi.org/10.1351/goldbook.L03646"^^xsd:string ;
    ns1:qudtReference "http://qudt.org/vocab/quantitykind/LuminousFlux"^^xsd:string .

ns1:MagneticDipoleMoment a owl:Class ;
    rdfs:label "MagneticDipoleMoment"@en ;
    rdfs:comment """For an atom or nucleus, this energy is quantized and can be written as:

    W = g μ M B

where g is the appropriate g factor, μ is mostly the Bohr magneton or nuclear magneton, M is magnetic quantum number, and B is magnitude of the magnetic flux density.

-- ISO 80000"""@en,
        """Vector quantity μ causing a change to its energy ΔW in an external magnetic field of field flux density B:

    ΔW = −μ · B"""@en ;
    rdfs:subClassOf [ a owl:Restriction ;
            owl:onProperty ns1:hasMeasurementUnit ;
            owl:someValuesFrom ns1:MagneticDipoleMomentUnit ],
        ns1:ElectromagneticQuantity,
        ns1:ISQDerivedQuantity ;
    skos:prefLabel "MagneticDipoleMoment"@en ;
    ns1:IEVReference "https://www.electropedia.org/iev/iev.nsf/display?openform&ievref=121-11-55"^^xsd:string ;
    ns1:ISO80000Reference "10-9.1"^^xsd:string,
        "6-30"^^xsd:string ;
    ns1:elucidation """Vector quantity μ causing a change to its energy ΔW in an external magnetic field of field flux density B:

    ΔW = −μ · B"""@en ;
    ns1:iupacReference "http://goldbook.iupac.org/terms/view/M03688"^^xsd:string ;
    ns1:qudtReference "http://qudt.org/vocab/quantitykind/MagneticDipoleMoment"^^xsd:string .

ns1:MagneticFieldStrength a owl:Class ;
    rdfs:label "MagneticFieldStrength"@en ;
    rdfs:comment "Strength of a magnetic field. Commonly denoted H."@en ;
    rdfs:subClassOf [ a owl:Restriction ;
            owl:onProperty ns1:hasMeasurementUnit ;
            owl:someValuesFrom ns1:MagneticFieldStrengthUnit ],
        ns1:ElectromagneticQuantity,
        ns1:ISQDerivedQuantity ;
    skos:altLabel "MagnetizingFieldStrength"@en ;
    skos:prefLabel "MagneticFieldStrength"@en ;
    ns1:IEVReference "https://www.electropedia.org/iev/iev.nsf/display?openform&ievref=121-11-56"^^xsd:string ;
    ns1:ISO80000Reference "6-25"^^xsd:string ;
    ns1:elucidation "Strength of a magnetic field. Commonly denoted H."@en ;
    ns1:iupacReference "https://doi.org/10.1351/goldbook.M03683"^^xsd:string ;
    ns1:qudtReference "http://qudt.org/vocab/quantitykind/MagneticFieldStrength"^^xsd:string ;
    ns1:wikidataReference "https://www.wikidata.org/wiki/Q28123"^^xsd:string .

ns1:MagneticMoment a owl:Class ;
    rdfs:label "MagneticMoment"@en ;
    rdfs:comment "A vector quantity equal to the product of the current, the loop area, and the unit vector normal to the loop plane, the direction of which corresponds to the loop orientation"@en ;
    rdfs:subClassOf [ a owl:Restriction ;
            owl:onProperty ns1:hasMeasurementUnit ;
            owl:someValuesFrom ns1:ElectricCurrentDensityUnit ],
        ns1:ElectromagneticQuantity ;
    skos:altLabel "MagneticAreaMoment"@en ;
    skos:prefLabel "MagneticMoment"@en ;
    ns1:IEVReference "https://www.electropedia.org/iev/iev.nsf/display?openform&ievref=121-11-49"^^xsd:string ;
    ns1:ISO80000Reference "6-23"^^xsd:string ;
    ns1:elucidation "A vector quantity equal to the product of the current, the loop area, and the unit vector normal to the loop plane, the direction of which corresponds to the loop orientation"@en ;
    ns1:iupacReference "https://doi.org/10.1351/goldbook.M03688"^^xsd:string ;
    ns1:qudtReference "https://qudt.org/vocab/quantitykind/MagneticMoment"^^xsd:string ;
    ns1:wikidataReference "https://www.wikidata.org/wiki/Q242657"^^xsd:string .

ns1:MagneticPolarisation a owl:Class ;
    rdfs:label "MagneticPolarisation"@en ;
    rdfs:comment "Vector quantity equal to the product of the magnetization M and the magnetic constant μ0."@en ;
    rdfs:subClassOf ns1:MagneticFluxDensity ;
    skos:prefLabel "MagneticPolarisation"@en ;
    ns1:IEVReference "https://www.electropedia.org/iev/iev.nsf/display?openform&ievref=121-11-54"^^xsd:string ;
    ns1:ISO80000Reference "6-29"^^xsd:string ;
    ns1:elucidation "Vector quantity equal to the product of the magnetization M and the magnetic constant μ0."@en ;
    ns1:qudtReference "https://qudt.org/vocab/quantitykind/MagneticPolarization"^^xsd:string ;
    ns1:wikidataReference "https://www.wikidata.org/wiki/Q856711"^^xsd:string .

ns1:MagneticQuantumNumber a owl:Class ;
    rdfs:label "MagneticQuantumNumber"^^xsd:string ;
    rdfs:comment "Atomic quantum number related to the z component lz, jz or sz, of the orbital, total, or spin angular momentum."@en ;
    rdfs:subClassOf ns1:QuantumNumber ;
    skos:prefLabel "MagneticQuantumNumber"^^xsd:string ;
    ns1:ISO80000Reference "10-13.4"^^xsd:string ;
    ns1:elucidation "Atomic quantum number related to the z component lz, jz or sz, of the orbital, total, or spin angular momentum."@en ;
    ns1:qudtReference "https://qudt.org/vocab/quantitykind/MagneticQuantumNumber"^^xsd:string ;
    ns1:wikidataReference "https://www.wikidata.org/wiki/Q2009727"^^xsd:string .

ns1:MagneticReluctance a owl:Class ;
    rdfs:label "MagneticReluctance"@en ;
    rdfs:comment "Magnetic tension divided by magnetic flux."@en ;
    rdfs:subClassOf [ a owl:Restriction ;
            owl:onProperty ns1:hasMeasurementUnit ;
            owl:someValuesFrom ns1:MagneticReluctanceUnit ],
        ns1:ElectromagneticQuantity,
        ns1:ISQDerivedQuantity ;
    skos:altLabel "Reluctance"@en ;
    skos:prefLabel "MagneticReluctance"@en ;
    ns1:IEVReference "https://www.electropedia.org/iev/iev.nsf/display?openform&ievref=131-12-28"^^xsd:string ;
    ns1:ISO80000Reference "6-39"^^xsd:string ;
    ns1:elucidation "Magnetic tension divided by magnetic flux."@en ;
    ns1:qudtReference "https://qudt.org/vocab/quantitykind/Reluctance"^^xsd:string ;
    ns1:wikidataReference "https://www.wikidata.org/wiki/Q863390"^^xsd:string .

ns1:MagneticReluctivityUnit a owl:Class ;
    rdfs:label "MagneticReluctivityUnit"@en ;
    rdfs:comment "The class of units with dimensionality 'MagneticReluctivity'."@en .

ns1:MagneticSusceptibility a owl:Class ;
    rdfs:label "MagneticSusceptibility"@en ;
    rdfs:comment "Scalar or tensor quantity the product of which by the magnetic constant μ0 and by the magnetic field strength H is equal to the magnetic polarization J."@en ;
    rdfs:subClassOf ns1:ElectromagneticQuantity,
        ns1:ISQDimensionlessQuantity ;
    skos:prefLabel "MagneticSusceptibility"@en ;
    ns1:IEVReference "https://www.electropedia.org/iev/iev.nsf/display?openform&ievref=121-12-37"^^xsd:string ;
    ns1:ISO80000Reference "6-28"^^xsd:string ;
    ns1:elucidation "Scalar or tensor quantity the product of which by the magnetic constant μ0 and by the magnetic field strength H is equal to the magnetic polarization J."@en ;
    ns1:qudtReference "https://qudt.org/vocab/unit/SUSCEPTIBILITY_MAG.html"^^xsd:string ;
    ns1:wikidataReference "https://www.wikidata.org/wiki/Q691463"^^xsd:string .

ns1:MagneticTension a owl:Class ;
    rdfs:label "MagneticTension"@en ;
    rdfs:comment "Scalar quantity equal to the line integral of the magnetic field strength H along a specified path linking two points a and b."@en ;
    rdfs:subClassOf [ a owl:Restriction ;
            owl:onProperty ns1:hasMeasurementUnit ;
            owl:someValuesFrom ns1:ElectricCurrentUnit ],
        ns1:ElectromagneticQuantity ;
    skos:prefLabel "MagneticTension"@en ;
    ns1:IEVReference "https://www.electropedia.org/iev/iev.nsf/display?openform&ievref=121-11-57"^^xsd:string ;
    ns1:ISO80000Reference "6-37.2"^^xsd:string ;
    ns1:elucidation "Scalar quantity equal to the line integral of the magnetic field strength H along a specified path linking two points a and b."@en ;
    ns1:qudtReference "https://qudt.org/vocab/quantitykind/MagneticTension"^^xsd:string ;
    ns1:wikidataReference "https://www.wikidata.org/wiki/Q77993836"^^xsd:string .

ns1:MagneticVectorPotential a owl:Class ;
    rdfs:label "MagneticVectorPotential"@en ;
    rdfs:comment "Vector potential of the magnetic flux density."@en ;
    rdfs:subClassOf [ a owl:Restriction ;
            owl:onProperty ns1:hasMeasurementUnit ;
            owl:someValuesFrom ns1:MagneticPotentialUnit ],
        ns1:ElectromagneticQuantity,
        ns1:ISQDerivedQuantity ;
    skos:prefLabel "MagneticVectorPotential"@en ;
    ns1:IEVReference "https://www.electropedia.org/iev/iev.nsf/display?openform&ievref=121-11-23"^^xsd:string ;
    ns1:ISO80000Reference "6-32"^^xsd:string ;
    ns1:elucidation "Vector potential of the magnetic flux density."@en ;
    ns1:qudtReference "https://qudt.org/vocab/quantitykind/MagneticVectorPotential"^^xsd:string ;
    ns1:wikidataReference "https://www.wikidata.org/wiki/Q2299100"^^xsd:string .

ns1:Magnetization a owl:Class ;
    rdfs:label "Magnetization"@en ;
    rdfs:comment "At a given point within a domain of quasi-infinitesimal volume V, vector quantity equal to the magnetic area moment m of the substance contained within the domain divided by the volume V."@en ;
    rdfs:subClassOf [ a owl:Restriction ;
            owl:onProperty ns1:hasMeasurementUnit ;
            owl:someValuesFrom ns1:MagneticFieldStrengthUnit ],
        ns1:ElectromagneticQuantity,
        ns1:ISQDerivedQuantity ;
    skos:prefLabel "Magnetization"@en ;
    ns1:IEVReference "https://www.electropedia.org/iev/iev.nsf/display?openform&ievref=121-11-52"^^xsd:string ;
    ns1:ISO80000Reference "6-24"^^xsd:string ;
    ns1:elucidation "At a given point within a domain of quasi-infinitesimal volume V, vector quantity equal to the magnetic area moment m of the substance contained within the domain divided by the volume V."@en ;
    ns1:qudtReference "https://qudt.org/vocab/quantitykind/Magnetization"^^xsd:string ;
    ns1:wikidataReference "https://www.wikidata.org/wiki/Q856711"^^xsd:string .

ns1:MagnetomotiveForce a owl:Class ;
    rdfs:label "MagnetomotiveForce"@en ;
    rdfs:comment "Scalar line integral of the magnetic field strength along a closed path."@en ;
    rdfs:subClassOf [ a owl:Restriction ;
            owl:onProperty ns1:hasMeasurementUnit ;
            owl:someValuesFrom ns1:ElectricCurrentUnit ],
        ns1:ElectromagneticQuantity,
        ns1:ISQDerivedQuantity ;
    skos:prefLabel "MagnetomotiveForce"@en ;
    ns1:IEVReference "https://www.electropedia.org/iev/iev.nsf/display?openform&ievref=121-11-60"^^xsd:string ;
    ns1:ISO80000Reference "6-37.3"^^xsd:string ;
    ns1:elucidation "Scalar line integral of the magnetic field strength along a closed path."@en ;
    ns1:qudtReference "https://qudt.org/vocab/quantitykind/MagnetomotiveForce"^^xsd:string ;
    ns1:wikidataReference "https://www.wikidata.org/wiki/Q1266982"^^xsd:string .

ns1:MassAttenuationCoefficient a owl:Class ;
    rdfs:label "MassAttenuationCoefficient"@en ;
    rdfs:comment "Quotient of the linear attenuation coefficient µ and the mass density ρ of the medium."@en ;
    rdfs:subClassOf [ a owl:Restriction ;
            owl:onProperty ns1:hasMeasurementUnit ;
            owl:someValuesFrom ns1:AreaPerMassUnit ],
        ns1:AtomicAndNuclearPhysicsQuantity,
        ns1:ISQDerivedQuantity ;
    skos:prefLabel "MassAttenuationCoefficient"@en ;
    ns1:IEVReference "https://www.electropedia.org/iev/iev.nsf/display?openform&ievref=881-04-27"^^xsd:string ;
    ns1:ISO80000Reference "10-50"^^xsd:string ;
    ns1:elucidation "Quotient of the linear attenuation coefficient µ and the mass density ρ of the medium."@en ;
    ns1:qudtReference "https://qudt.org/vocab/quantitykind/MassAttenuationCoefficient"^^xsd:string ;
    ns1:wikidataReference "https://www.wikidata.org/wiki/Q98591983"^^xsd:string .

ns1:MassChangeRate a owl:Class ;
    rdfs:label "MassChangeRate"@en ;
    rdfs:comment "Mass increment per time."@en ;
    rdfs:subClassOf [ a owl:Restriction ;
            owl:onProperty ns1:hasMeasurementUnit ;
            owl:someValuesFrom ns1:MassPerTimeUnit ],
        ns1:ISQDerivedQuantity,
        ns1:MechanicalQuantity ;
    skos:prefLabel "MassChangeRate"@en ;
    ns1:ISO80000Reference "4-30.3"^^xsd:string ;
    ns1:elucidation "Mass increment per time."@en ;
    ns1:wikidataReference "https://www.wikidata.org/wiki/Q92020547"^^xsd:string .

ns1:MassConcentrationOfWater a owl:Class ;
    rdfs:label "MassConcentrationOfWater"@en ;
    rdfs:comment "Quotient of the mass of water in a three-dimensional domain, irrespective of the form of aggregation, by the volume of the domain."@en,
        "The mass concentration of water at saturation is denoted wsat."@en ;
    rdfs:subClassOf ns1:MassConcentration,
        ns1:ThermodynamicalQuantity ;
    skos:prefLabel "MassConcentrationOfWater"@en ;
    ns1:IEVReference "https://www.electropedia.org/iev/iev.nsf/display?openform&ievref=113-04-59"^^xsd:string ;
    ns1:ISO80000Reference "5-27"^^xsd:string ;
    ns1:elucidation "Quotient of the mass of water in a three-dimensional domain, irrespective of the form of aggregation, by the volume of the domain."@en ;
    ns1:qudtReference "https://qudt.org/vocab/quantitykind/MassConcentrationOfWater"^^xsd:string ;
    ns1:wikidataReference "https://www.wikidata.org/wiki/Q76378758"^^xsd:string .

ns1:MassConcentrationOfWaterVapour a owl:Class ;
    rdfs:label "MassConcentrationOfWaterVapour"@en ;
    rdfs:comment "Quotient of the mass of water vapour in moist gas by the total gas volume."@en,
        "The mass concentration of water at saturation is denoted vsat."@en ;
    rdfs:subClassOf ns1:MassConcentration,
        ns1:ThermodynamicalQuantity ;
    skos:prefLabel "MassConcentrationOfWaterVapour"@en ;
    ns1:IEVReference "https://www.electropedia.org/iev/iev.nsf/display?openform&ievref=113-04-60"@en ;
    ns1:elucidation "Quotient of the mass of water vapour in moist gas by the total gas volume."@en ;
    ns1:qudtReference "https://qudt.org/vocab/quantitykind/MassConcentrationOfWaterVapour"^^xsd:string ;
    ns1:wikidataReference "https://www.wikidata.org/wiki/Q76378808"^^xsd:string .

ns1:MassDefect a owl:Class ;
    rdfs:label "MassDefect"@en ;
    rdfs:comment "Sum of the product of the proton number and the hydrogen atomic mass, and the neutron rest mass, minus the rest mass of the atom."@en ;
    rdfs:subClassOf ns1:AtomicAndNuclearPhysicsQuantity,
        ns1:Mass ;
    skos:prefLabel "MassDefect"@en ;
    ns1:ISO80000Reference "10-21.2"^^xsd:string ;
    ns1:elucidation "Sum of the product of the proton number and the hydrogen atomic mass, and the neutron rest mass, minus the rest mass of the atom."@en ;
    ns1:qudtReference "https://qudt.org/vocab/quantitykind/MassDefect"^^xsd:string ;
    ns1:wikidataReference "https://www.wikidata.org/wiki/Q26897126"^^xsd:string .

ns1:MassEnergyTransferCoefficient a owl:Class ;
    rdfs:label "MassEnergyTransferCoefficient"@en ;
    rdfs:comment "For ionizing uncharged particles of a given type and energy, the differential quotient of Rtr with respect to l. Where Rtr is the mean energy that is transferred to kinetic energy of charged particles by interactions of the uncharged particles of incident radiant energy R in traversing a distance  l in the material of density rho, divided by rho and R"@en ;
    rdfs:subClassOf [ a owl:Restriction ;
            owl:onProperty ns1:hasMeasurementUnit ;
            owl:someValuesFrom ns1:AreaPerMassUnit ],
        ns1:AtomicAndNuclearPhysicsQuantity,
        ns1:ISQDerivedQuantity ;
    skos:prefLabel "MassEnergyTransferCoefficient"@en ;
    ns1:IEVReference "https://www.electropedia.org/iev/iev.nsf/display?openform&ievref=881-04-32"^^xsd:string ;
    ns1:ISO80000Reference "10-87"^^xsd:string ;
    ns1:elucidation "For ionizing uncharged particles of a given type and energy, the differential quotient of Rtr with respect to l. Where Rtr is the mean energy that is transferred to kinetic energy of charged particles by interactions of the uncharged particles of incident radiant energy R in traversing a distance  l in the material of density rho, divided by rho and R"@en ;
    ns1:qudtReference "https://qudt.org/vocab/quantitykind/MassEnergyTransferCoefficient"^^xsd:string ;
    ns1:wikidataReference "https://www.wikidata.org/wiki/Q99714619"^^xsd:string .

ns1:MassExcess a owl:Class ;
    rdfs:label "MassExcess"@en ;
    rdfs:comment "Difference between the mass of an atom, and the product of its mass number and the unified mass constant."@en ;
    rdfs:subClassOf [ a owl:Restriction ;
            owl:onProperty ns1:hasMeasurementUnit ;
            owl:someValuesFrom ns1:MassUnit ],
        ns1:AtomicAndNuclearPhysicsQuantity,
        ns1:ISQDerivedQuantity ;
    skos:prefLabel "MassExcess"@en ;
    ns1:ISO80000Reference "10-21.1"^^xsd:string ;
    ns1:elucidation "Difference between the mass of an atom, and the product of its mass number and the unified mass constant."@en ;
    ns1:iupacReference "https://doi.org/10.1351/goldbook.M03719"^^xsd:string ;
    ns1:qudtReference "https://qudt.org/vocab/quantitykind/MassExcess"^^xsd:string ;
    ns1:wikidataReference "https://www.wikidata.org/wiki/Q1571163"^^xsd:string .

ns1:MassFlow a owl:Class ;
    rdfs:label "MassFlow"@en ;
    rdfs:comment "At a point in a fluid, the product of mass density and velocity."@en ;
    rdfs:subClassOf [ a owl:Restriction ;
            owl:onProperty ns1:hasMeasurementUnit ;
            owl:someValuesFrom ns1:MassFluxUnit ],
        ns1:ISQDerivedQuantity,
        ns1:MechanicalQuantity ;
    skos:prefLabel "MassFlow"@en ;
    ns1:ISO80000Reference "4-30.1"^^xsd:string ;
    ns1:elucidation "At a point in a fluid, the product of mass density and velocity."@en ;
    ns1:wikidataReference "https://www.wikidata.org/wiki/Q3265048"^^xsd:string .

ns1:MassFractionOfDryMatter a owl:Class ;
    rdfs:label "MassFractionOfDryMatter"@en ;
    rdfs:comment "Quantity wd = 1 − wH2O, where wH2O is mass fraction of water."@en ;
    rdfs:subClassOf ns1:MassFraction,
        ns1:ThermodynamicalQuantity ;
    skos:prefLabel "MassFractionOfDryMatter"@en ;
    ns1:IEVReference "https://www.electropedia.org/iev/iev.nsf/display?openform&ievref=113-04-64"^^xsd:string ;
    ns1:ISO80000Reference "5-32"^^xsd:string ;
    ns1:elucidation "Quantity wd = 1 − wH2O, where wH2O is mass fraction of water."@en ;
    ns1:qudtReference "https://qudt.org/vocab/quantitykind/MassFractionOfDryMatter"^^xsd:string ;
    ns1:wikidataReference "https://www.wikidata.org/wiki/Q76379189"^^xsd:string .

ns1:MassFractionOfWater a owl:Class ;
    rdfs:label "MassFractionOfWater"@en ;
    rdfs:comment "Quantity of dimension 1 equal to u/(1 + u), where u is mass ratio of water to dry matter."@en ;
    rdfs:subClassOf ns1:MassFraction,
        ns1:ThermodynamicalQuantity ;
    skos:prefLabel "MassFractionOfWater"@en ;
    ns1:IEVReference "https://www.electropedia.org/iev/iev.nsf/display?openform&ievref=113-04-63"^^xsd:string ;
    ns1:ISO80000Reference "5-31"^^xsd:string ;
    ns1:elucidation "Quantity of dimension 1 equal to u/(1 + u), where u is mass ratio of water to dry matter."@en ;
    ns1:qudtReference "https://qudt.org/vocab/quantitykind/MassFractionOfWater"^^xsd:string ;
    ns1:wikidataReference "https://www.wikidata.org/wiki/Q76379025"^^xsd:string .

ns1:MassLengthPerCubicTimeUnit a owl:Class ;
    rdfs:label "MassLengthPerCubicTimeUnit"@en ;
    rdfs:comment "The class of units with dimensionality 'MassLengthPerCubicTime'."@en .

ns1:MassNumber a owl:Class ;
    rdfs:label "MassNumber"@en ;
    rdfs:comment "Number of nucleons in an atomic nucleus."@en ;
    rdfs:subClassOf [ a owl:Restriction ;
            owl:allValuesFrom ns1:Atom ;
            owl:onProperty [ owl:inverseOf ns1:hasProperty ] ],
        ns1:PureNumberQuantity ;
    skos:altLabel "AtomicMassNumber"^^xsd:string,
        "NucleonNumber"^^xsd:string ;
    skos:prefLabel "MassNumber"@en ;
    ns1:elucidation "Number of nucleons in an atomic nucleus."@en ;
    ns1:qudtReference "http://qudt.org/vocab/quantitykind/MassNumber"^^xsd:string .

ns1:MassPerCubicTimeQuarticTemperatureUnit a owl:Class ;
    rdfs:label "MassPerCubicTimeQuarticTemperatureUnit"@en ;
    rdfs:comment "The class of units with dimensionality 'MassPerCubicTimeQuarticTemperature'."@en .

ns1:MassPerQuarticLengthTimeUnit a owl:Class ;
    rdfs:label "MassPerQuarticLengthTimeUnit"@en ;
    rdfs:comment "The class of units with dimensionality 'MassPerQuarticLengthTime'."@en .

ns1:MassPerQuarticTimeUnit a owl:Class ;
    rdfs:label "MassPerQuarticTimeUnit"@en ;
    rdfs:comment "The class of units with dimensionality 'MassPerQuarticTime'."@en .

ns1:MassPerSquareLengthSquareTimeUnit a owl:Class ;
    rdfs:label "MassPerSquareLengthSquareTimeUnit"@en ;
    rdfs:comment "The class of units with dimensionality 'MassPerSquareLengthSquareTime'."@en .

ns1:MassPerVolumeTimeUnit a owl:Class ;
    rdfs:label "MassPerVolumeTimeUnit"@en ;
    rdfs:comment "The class of units with dimensionality 'MassPerVolumeTime'."@en .

ns1:MassRatioOfWaterToDryMatter a owl:Class ;
    rdfs:label "MassRatioOfWaterToDryMatter"@en ;
    rdfs:comment "The mass concentration of water at saturation is denoted usat."^^xsd:string,
        "Ratio of the mass of water to the mass of dry matter in a given volume of matter."@en ;
    rdfs:subClassOf ns1:ISQDimensionlessQuantity,
        ns1:ThermodynamicalQuantity ;
    skos:prefLabel "MassRatioOfWaterToDryMatter"@en ;
    ns1:IEVReference "https://www.electropedia.org/iev/iev.nsf/display?openform&ievref=113-04-61"^^xsd:string ;
    ns1:ISO80000Reference "5-29"^^xsd:string ;
    ns1:elucidation "Ratio of the mass of water to the mass of dry matter in a given volume of matter."@en ;
    ns1:wikidataReference "https://www.wikidata.org/wiki/Q76378860"^^xsd:string .

ns1:MassSquareTimeUnit a owl:Class ;
    rdfs:label "MassSquareTimeUnit"@en ;
    rdfs:comment "The class of units with dimensionality 'MassSquareTime'."@en .

ns1:MassTemperatureUnit a owl:Class ;
    rdfs:label "MassTemperatureUnit"@en ;
    rdfs:comment "The class of units with dimensionality 'MassTemperature'."@en .

ns1:MassieuFunction a owl:Class ;
    rdfs:label "MassieuFunction"@en ;
    rdfs:comment "Negative quotient of Helmholtz energy and temperature."@en ;
    rdfs:subClassOf [ a owl:Restriction ;
            owl:onProperty ns1:hasMeasurementUnit ;
            owl:someValuesFrom ns1:EntropyUnit ],
        ns1:ISQDerivedQuantity,
        ns1:ThermodynamicalQuantity ;
    skos:prefLabel "MassieuFunction"@en ;
    ns1:IEVReference "https://www.electropedia.org/iev/iev.nsf/display?openform&ievref=113-04-26"^^xsd:string ;
    ns1:ISO80000Reference "5-22"^^xsd:string ;
    ns1:elucidation "Negative quotient of Helmholtz energy and temperature."@en ;
    ns1:qudtReference "https://qudt.org/vocab/quantitykind/MassieuFunction"^^xsd:string ;
    ns1:wikidataReference "https://www.wikidata.org/wiki/Q3077625"^^xsd:string .

ns1:MaximumBetaParticleEnergy a owl:Class ;
    rdfs:label "MaximumBetaParticleEnergy"@en ;
    rdfs:comment "Maximum kinetic energy of the emitted beta particle produced in the nuclear disintegration process."@en ;
    rdfs:subClassOf ns1:AtomicAndNuclearPhysicsQuantity,
        ns1:Energy ;
    skos:prefLabel "MaximumBetaParticleEnergy"@en ;
    ns1:ISO80000Reference "10-33"^^xsd:string ;
    ns1:elucidation "Maximum kinetic energy of the emitted beta particle produced in the nuclear disintegration process."@en ;
    ns1:qudtReference "https://qudt.org/vocab/quantitykind/MaximumBeta-ParticleEnergy"^^xsd:string ;
    ns1:wikidataReference "https://www.wikidata.org/wiki/Q98148038"^^xsd:string .

ns1:MaximumEfficiency a owl:Class ;
    rdfs:label "MaximumEfficiency"@en ;
    rdfs:comment "Efficiency of an ideal heat engine operating according to the Carnot process."@en ;
    rdfs:subClassOf ns1:ISQDimensionlessQuantity,
        ns1:ThermodynamicalQuantity ;
    skos:altLabel "CarnotEfficiency"@en ;
    skos:prefLabel "MaximumEfficiency"@en ;
    ns1:ISO80000Reference "5-25.2"^^xsd:string ;
    ns1:elucidation "Efficiency of an ideal heat engine operating according to the Carnot process."@en ;
    ns1:wikidataReference "https://www.wikidata.org/wiki/Q93949862"^^xsd:string .

ns1:MeanDurationOfLife a owl:Class ;
    rdfs:label "MeanDurationOfLife"@en ;
    rdfs:comment "Reciprocal of the decay constant λ."@en ;
    rdfs:subClassOf ns1:AtomicAndNuclearPhysicsQuantity,
        ns1:Duration ;
    skos:altLabel "MeanLifeTime"@en ;
    skos:prefLabel "MeanDurationOfLife"@en ;
    ns1:IEVReference "https://www.electropedia.org/iev/iev.nsf/display?openform&ievref=395-01-13"^^xsd:string,
        "https://www.electropedia.org/iev/iev.nsf/display?openform&ievref=881-04-47"^^xsd:string ;
    ns1:ISO80000Reference "10-25"^^xsd:string ;
    ns1:elucidation "Reciprocal of the decay constant λ."@en ;
    ns1:qudtReference "https://qudt.org/vocab/quantitykind/MeanLifetime"^^xsd:string,
        "https://www.wikidata.org/wiki/Q1758559"^^xsd:string .

ns1:MeanEnergyImparted a owl:Class ;
    rdfs:label "MeanEnergyImparted"@en ;
    rdfs:comment "Expectation value of the energy imparted."@en ;
    rdfs:subClassOf ns1:AtomicAndNuclearPhysicsQuantity,
        ns1:Energy ;
    skos:prefLabel "MeanEnergyImparted"@en ;
    ns1:IEVReference "https://www.electropedia.org/iev/iev.nsf/display?openform&ievref=881-12-44"^^xsd:string ;
    ns1:ISO80000Reference "10-80.2"^^xsd:string ;
    ns1:elucidation "Expectation value of the energy imparted."@en ;
    ns1:qudtReference "https://qudt.org/vocab/quantitykind/MeanEnergyImparted"^^xsd:string ;
    ns1:wikidataReference "https://www.wikidata.org/wiki/Q99526969"^^xsd:string .

ns1:MeanFreePathOfElectrons a owl:Class ;
    rdfs:label "MeanFreePathOfElectrons"@en ;
    rdfs:comment "Average distance that electrons travel between two successive interactions."@en ;
    rdfs:subClassOf ns1:CondensedMatterPhysicsQuantity,
        ns1:MeanFreePath ;
    skos:prefLabel "MeanFreePathOfElectrons"@en ;
    ns1:ISO80000Reference "12-15.2"^^xsd:string ;
    ns1:elucidation "Average distance that electrons travel between two successive interactions."@en ;
    ns1:qudtReference "https://qudt.org/vocab/quantitykind/ElectronMeanFreePath"^^xsd:string ;
    ns1:wikidataReference "https://www.wikidata.org/wiki/Q105672307"^^xsd:string .

ns1:MeanFreePathOfPhonons a owl:Class ;
    rdfs:label "MeanFreePathOfPhonons"@en ;
    rdfs:comment "average distance that phonons travel between two successive interactions"@en ;
    rdfs:subClassOf ns1:CondensedMatterPhysicsQuantity,
        ns1:MeanFreePath ;
    skos:prefLabel "MeanFreePathOfPhonons"@en ;
    ns1:ISO80000Reference "12-15.1"^^xsd:string ;
    ns1:elucidation "average distance that phonons travel between two successive interactions"@en ;
    ns1:qudtReference "https://qudt.org/vocab/quantitykind/PhononMeanFreePath"^^xsd:string ;
    ns1:wikidataReference "https://www.wikidata.org/wiki/Q105672255"^^xsd:string .

ns1:MeanLinearRange a owl:Class ;
    rdfs:label "MeanLinearRange"@en ;
    rdfs:comment "Mean total rectified path length travelled by a particle in the course of slowing down to rest in a given material averaged over a group of particles having the same initial energy."@en ;
    rdfs:subClassOf ns1:AtomicAndNuclearPhysicsQuantity,
        ns1:Length ;
    skos:prefLabel "MeanLinearRange"@en ;
    ns1:ISO80000Reference "10-56"^^xsd:string ;
    ns1:elucidation "Mean total rectified path length travelled by a particle in the course of slowing down to rest in a given material averaged over a group of particles having the same initial energy."@en ;
    ns1:iupacReference "https://doi.org/10.1351/goldbook.M03782"^^xsd:string ;
    ns1:qudtReference "https://qudt.org/vocab/quantitykind/MeanLinearRange"^^xsd:string ;
    ns1:wikidataReference "https://www.wikidata.org/wiki/Q98681589"^^xsd:string .

ns1:MeanMassRange a owl:Class ;
    rdfs:label "MeanMassRange"@en ;
    rdfs:comment "Product of the mean linear range R and the mass density ρ of the material."@en ;
    rdfs:subClassOf [ a owl:Restriction ;
            owl:onProperty ns1:hasMeasurementUnit ;
            owl:someValuesFrom ns1:AreaDensityUnit ],
        ns1:AtomicAndNuclearPhysicsQuantity,
        ns1:ISQDerivedQuantity ;
    skos:prefLabel "MeanMassRange"@en ;
    ns1:ISO80000Reference "10-57"^^xsd:string ;
    ns1:elucidation "Product of the mean linear range R and the mass density ρ of the material."@en ;
    ns1:iupacReference "https://doi.org/10.1351/goldbook.M03783"^^xsd:string ;
    ns1:qudtReference "https://qudt.org/vocab/quantitykind/MeanMassRange"^^xsd:string ;
    ns1:wikidataReference "https://www.wikidata.org/wiki/Q98681670"^^xsd:string .

ns1:MechanicalEfficiency a owl:Class ;
    rdfs:label "MechanicalEfficiency"@en ;
    rdfs:comment "Quotient of mechanical output and input power."@en ;
    rdfs:subClassOf ns1:MechanicalQuantity,
        ns1:RatioQuantity ;
    skos:prefLabel "MechanicalEfficiency"@en ;
    ns1:ISO80000Reference "4-29"^^xsd:string ;
    ns1:elucidation "Quotient of mechanical output and input power."@en ;
    ns1:wikidataReference "https://www.wikidata.org/wiki/Q2628085"^^xsd:string .

ns1:MicrocanonicalPartitionFunction a owl:Class ;
    rdfs:label "MicrocanonicalPartitionFunction"@en ;
    rdfs:comment "Number of all quantum states consistent with given energy, volume, and external fields."@en ;
    rdfs:subClassOf ns1:ISQDimensionlessQuantity,
        ns1:PhysioChemicalQuantity ;
    skos:prefLabel "MicrocanonicalPartitionFunction"@en ;
    ns1:ISO80000Reference "9-35.1"^^xsd:string ;
    ns1:elucidation "Number of all quantum states consistent with given energy, volume, and external fields."@en ;
    ns1:qudtReference "https://qudt.org/vocab/quantitykind/MicroCanonicalPartitionFunction"^^xsd:string ;
    ns1:wikidataReference "https://www.wikidata.org/wiki/Q96106546"^^xsd:string .

ns1:MigrationArea a owl:Class ;
    rdfs:label "MigrationArea"@en ;
    rdfs:comment "Sum of the slowing-down area from fission energy to thermal energy and the diffusion area for thermal neutrons."@en ;
    rdfs:subClassOf ns1:Area,
        ns1:AtomicAndNuclearPhysicsQuantity ;
    skos:prefLabel "MigrationArea"@en ;
    ns1:ISO80000Reference "10-72.3"^^xsd:string ;
    ns1:elucidation "Sum of the slowing-down area from fission energy to thermal energy and the diffusion area for thermal neutrons."@en ;
    ns1:qudtReference "https://qudt.org/vocab/quantitykind/MigrationArea"^^xsd:string ;
    ns1:wikidataReference "https://www.wikidata.org/wiki/Q98966325"^^xsd:string .

ns1:MigrationLength a owl:Class ;
    rdfs:label "MigrationLength"@en ;
    rdfs:comment "Square root of the migration area, M^2."@en ;
    rdfs:subClassOf ns1:AtomicAndNuclearPhysicsQuantity,
        ns1:Length ;
    skos:prefLabel "MigrationLength"@en ;
    ns1:ISO80000Reference "10-73.3"^^xsd:string ;
    ns1:elucidation "Square root of the migration area, M^2."@en ;
    ns1:qudtReference "https://qudt.org/vocab/quantitykind/MigrationLength"^^xsd:string ;
    ns1:wikidataReference "https://www.wikidata.org/wiki/Q98998318"^^xsd:string .

ns1:MixingRatio a owl:Class ;
    rdfs:label "MixingRatio"@en ;
    rdfs:comment "Ratio of the mass of water vapour to the mass of dry air in a given volume of air."@en,
        "The mixing ratio at saturation is denoted xsat."@en ;
    rdfs:subClassOf ns1:RatioQuantity,
        ns1:ThermodynamicalQuantity ;
    skos:altLabel "MassRatioOfWaterVapourToDryGas"@en ;
    skos:prefLabel "MixingRatio"@en ;
    ns1:IEVReference "https://www.electropedia.org/iev/iev.nsf/display?openform&ievref=113-04-62"@en ;
    ns1:ISO80000Reference "5-30"^^xsd:string ;
    ns1:elucidation "Ratio of the mass of water vapour to the mass of dry air in a given volume of air."@en ;
    ns1:wikidataReference "https://www.wikidata.org/wiki/Q76378940"^^xsd:string .

ns1:Mobility a owl:Class ;
    rdfs:label "Mobility"@en ;
    rdfs:comment "Quotient of average drift speed imparted to a charged particle in a medium by an electric field, and the electric field strength."@en ;
    rdfs:subClassOf [ a owl:Restriction ;
            owl:onProperty ns1:hasMeasurementUnit ;
            owl:someValuesFrom ns1:ElectricMobilityUnit ],
        ns1:AtomicAndNuclearPhysicsQuantity,
        ns1:ISQDerivedQuantity ;
    skos:prefLabel "Mobility"@en ;
    ns1:IEVReference "https://www.electropedia.org/iev/iev.nsf/display?openform&ievref=113-06-36"^^xsd:string,
        "https://www.electropedia.org/iev/iev.nsf/display?openform&ievref=881-02-77"^^xsd:string ;
    ns1:ISO80000Reference "10-61"^^xsd:string ;
    ns1:elucidation "Quotient of average drift speed imparted to a charged particle in a medium by an electric field, and the electric field strength."@en ;
    ns1:iupacReference "https://doi.org/10.1351/goldbook.M03955"^^xsd:string ;
    ns1:qudtReference "https://qudt.org/vocab/quantitykind/Mobility"^^xsd:string ;
    ns1:wikidataReference "https://www.wikidata.org/wiki/Q900648"^^xsd:string .

ns1:MobilityRatio a owl:Class ;
    rdfs:label "MobilityRatio"@en ;
    rdfs:comment "Quotient of electron and hole mobility."@en ;
    rdfs:subClassOf ns1:CondensedMatterPhysicsQuantity,
        ns1:RatioQuantity ;
    skos:prefLabel "MobilityRatio"@en ;
    ns1:ISO80000Reference "12-31"^^xsd:string ;
    ns1:elucidation "Quotient of electron and hole mobility."@en ;
    ns1:qudtReference "https://qudt.org/vocab/quantitykind/MobilityRatio"^^xsd:string ;
    ns1:wikidataReference "https://www.wikidata.org/wiki/Q106010255"^^xsd:string .

ns1:ModulusOfAdmittance a owl:Class ;
    rdfs:label "ModulusOfAdmittance"@en ;
    rdfs:comment "quotient of the rms value of the electric current in a two-terminal element or a two-terminal circuit by the rms value of the voltage between its terminals."@en ;
    rdfs:subClassOf ns1:ElectricConductance ;
    skos:prefLabel "ModulusOfAdmittance"@en ;
    ns1:IEVReference "https://www.electropedia.org/iev/iev.nsf/display?openform&ievref=131-12-52"^^xsd:string ;
    ns1:ISO80000Reference "6-52.4"^^xsd:string ;
    ns1:elucidation "quotient of the rms value of the electric current in a two-terminal element or a two-terminal circuit by the rms value of the voltage between its terminals."@en ;
    ns1:note "Apparent admittance is often denoted by Y ."@en ;
    ns1:qudtReference "https://qudt.org/vocab/quantitykind/ModulusOfAdmittance"^^xsd:string ;
    ns1:wikidataReference "https://www.wikidata.org/wiki/Q79466359"^^xsd:string .

ns1:ModulusOfCompression a owl:Class ;
    rdfs:label "ModulusOfCompression"@en ;
    rdfs:comment "Measure of how resistant to compressibility a substance is."@en ;
    rdfs:subClassOf [ a owl:Restriction ;
            owl:onProperty ns1:hasMeasurementUnit ;
            owl:someValuesFrom ns1:PressureUnit ],
        ns1:ISQDerivedQuantity,
        ns1:MechanicalQuantity ;
    skos:altLabel "BulkModulus"@en ;
    skos:prefLabel "ModulusOfCompression"@en ;
    ns1:IEVReference "https://www.electropedia.org/iev/iev.nsf/display?openform&ievref=113-03-69"^^xsd:string ;
    ns1:ISO80000Reference "4-19.3"^^xsd:string ;
    ns1:elucidation "Measure of how resistant to compressibility a substance is."@en ;
    ns1:qudtReference "https://qudt.org/vocab/quantitykind/BulkModulus"^^xsd:string ;
    ns1:wikidataReference "https://www.wikidata.org/wiki/Q900371"^^xsd:string .

ns1:ModulusOfElasticity a owl:Class ;
    rdfs:label "ModulusOfElasticity"@en ;
    rdfs:comment "Mechanical property of linear elastic solid materials."@en ;
    rdfs:subClassOf [ a owl:Restriction ;
            owl:onProperty ns1:hasMeasurementUnit ;
            owl:someValuesFrom ns1:PressureUnit ],
        ns1:ISQDerivedQuantity,
        ns1:MechanicalQuantity ;
    skos:altLabel "YoungsModulus"@en ;
    skos:prefLabel "ModulusOfElasticity"@en ;
    ns1:IEVReference "https://www.electropedia.org/iev/iev.nsf/display?openform&ievref=113-03-67"^^xsd:string ;
    ns1:ISO80000Reference "4-19.1"^^xsd:string ;
    ns1:elucidation "Mechanical property of linear elastic solid materials."@en ;
    ns1:iupacReference "https://doi.org/10.1351/goldbook.M03966"^^xsd:string ;
    ns1:wikidataReference "https://www.wikidata.org/wiki/Q2091584"^^xsd:string .

ns1:ModulusOfImpedance a owl:Class ;
    rdfs:label "ModulusOfImpedance"@en ;
    rdfs:comment "Quotient of the rms value of the voltage between the terminals of a two-terminal element or a two-terminal circuit by the rms value of the electric current in the element or circuit."@en ;
    rdfs:subClassOf ns1:ElectricResistance ;
    skos:prefLabel "ModulusOfImpedance"@en ;
    ns1:IEVReference "https://www.electropedia.org/iev/iev.nsf/display?openform&ievref=131-12-44"^^xsd:string ;
    ns1:ISO80000Reference "6-51.4"^^xsd:string ;
    ns1:elucidation "Quotient of the rms value of the voltage between the terminals of a two-terminal element or a two-terminal circuit by the rms value of the electric current in the element or circuit."@en ;
    ns1:qudtReference "https://qudt.org/vocab/quantitykind/ModulusOfImpedance"^^xsd:string ;
    ns1:wikidataReference "https://www.wikidata.org/wiki/Q25457909"^^xsd:string .

ns1:ModulusOfRigidity a owl:Class ;
    rdfs:label "ModulusOfRigidity"@en ;
    rdfs:comment "Ratio of shear stress to the shear strain."@en ;
    rdfs:subClassOf [ a owl:Restriction ;
            owl:onProperty ns1:hasMeasurementUnit ;
            owl:someValuesFrom ns1:PressureUnit ],
        ns1:ISQDerivedQuantity,
        ns1:MechanicalQuantity ;
    skos:altLabel "ShearModulus"@en ;
    skos:prefLabel "ModulusOfRigidity"@en ;
    ns1:IEVReference "https://www.electropedia.org/iev/iev.nsf/display?openform&ievref=113-03-68"^^xsd:string ;
    ns1:ISO80000Reference "4-19.2"^^xsd:string ;
    ns1:elucidation "Ratio of shear stress to the shear strain."@en ;
    ns1:iupacReference "https://doi.org/10.1351/goldbook.S05635"^^xsd:string ;
    ns1:qudtReference "https://qudt.org/vocab/quantitykind/ShearModulus"^^xsd:string ;
    ns1:wikidataReference "https://www.wikidata.org/wiki/Q461466"^^xsd:string .

ns1:Molality a owl:Class ;
    rdfs:label "Molality"@en ;
    rdfs:comment "quotient of the amount of substance nB of solute B by the mass m of the solvent: bB = nB / m."@en ;
    rdfs:subClassOf [ a owl:Restriction ;
            owl:onProperty ns1:hasMeasurementUnit ;
            owl:someValuesFrom ns1:AmountPerMassUnit ],
        ns1:ISQDerivedQuantity,
        ns1:PhysioChemicalQuantity ;
    skos:altLabel "AmountPerMass"@en ;
    skos:prefLabel "Molality"@en ;
    ns1:IEVReference "https://www.electropedia.org/iev/iev.nsf/display?openform&ievref=114-01-19"@en ;
    ns1:ISO80000Reference "9-15"^^xsd:string ;
    ns1:elucidation "quotient of the amount of substance nB of solute B by the mass m of the solvent: bB = nB / m."@en ;
    ns1:iupacReference "https://doi.org/10.1351/goldbook.M03970"^^xsd:string ;
    ns1:wikidataReference "https://www.wikidata.org/wiki/Q172623"^^xsd:string .

ns1:MolarAttenuationCoefficient a owl:Class ;
    rdfs:label "MolarAttenuationCoefficient"@en ;
    rdfs:comment "Quotient of linear attenuation coefficient µ and the amount c of the medium."@en ;
    rdfs:subClassOf [ a owl:Restriction ;
            owl:onProperty ns1:hasMeasurementUnit ;
            owl:someValuesFrom ns1:AreaPerAmountUnit ],
        ns1:AtomicAndNuclearPhysicsQuantity,
        ns1:ISQDerivedQuantity ;
    skos:prefLabel "MolarAttenuationCoefficient"@en ;
    ns1:ISO80000Reference "10-51"^^xsd:string ;
    ns1:elucidation "Quotient of linear attenuation coefficient µ and the amount c of the medium."@en ;
    ns1:wikidataReference "https://www.wikidata.org/wiki/Q98592828"^^xsd:string .

ns1:MolarConductivity a owl:Class ;
    rdfs:label "MolarConductivity"@en ;
    rdfs:comment "Conductivity per molar concentration of electrolyte."@en ;
    rdfs:subClassOf [ a owl:Restriction ;
            owl:onProperty ns1:hasMeasurementUnit ;
            owl:someValuesFrom ns1:AmountConductivityUnit ],
        ns1:ISQDerivedQuantity,
        ns1:PhysioChemicalQuantity ;
    skos:prefLabel "MolarConductivity"@en ;
    ns1:ISO80000Reference "9-45"^^xsd:string ;
    ns1:elucidation "Conductivity per molar concentration of electrolyte."@en ;
    ns1:iupacReference "https://doi.org/10.1351/goldbook.M03976"^^xsd:string ;
    ns1:qudtReference "https://qudt.org/vocab/quantitykind/MolarConductivity"^^xsd:string ;
    ns1:wikidataReference "https://www.wikidata.org/wiki/Q1943278"^^xsd:string .

ns1:MolarEnthalpy a owl:Class ;
    rdfs:label "MolarEnthalpy"@en ;
    rdfs:comment "Enthalpy per amount of substance."@en ;
    rdfs:subClassOf ns1:MolarEnergy,
        ns1:PhysioChemicalQuantity ;
    skos:prefLabel "MolarEnthalpy"@en ;
    ns1:ISO80000Reference "9-6.2"^^xsd:string ;
    ns1:elucidation "Enthalpy per amount of substance."@en ;
    ns1:wikidataReference "https://www.wikidata.org/wiki/Q88769977"^^xsd:string .

ns1:MolarEntropy a owl:Class ;
    rdfs:label "MolarEntropy"@en ;
    rdfs:comment "Entropy per amount of substance."@en ;
    rdfs:subClassOf [ a owl:Restriction ;
            owl:onProperty ns1:hasMeasurementUnit ;
            owl:someValuesFrom ns1:EntropyPerAmountUnit ],
        ns1:ISQDerivedQuantity,
        ns1:PhysioChemicalQuantity ;
    skos:prefLabel "MolarEntropy"@en ;
    ns1:ISO80000Reference "9-8"^^xsd:string ;
    ns1:elucidation "Entropy per amount of substance."@en ;
    ns1:qudtReference "https://qudt.org/vocab/quantitykind/MolarEntropy"^^xsd:string ;
    ns1:wikidataReference "https://www.wikidata.org/wiki/Q68972876"^^xsd:string .

ns1:MolarGasConstant a owl:Class ;
    rdfs:label "MolarGasConstant"@en ;
    rdfs:comment "Equivalent to the Boltzmann constant, but expressed in units of energy per temperature increment per mole (rather than energy per temperature increment per particle)."@en ;
    rdfs:subClassOf [ a owl:Restriction ;
            owl:onProperty ns1:hasMeasurementUnit ;
            owl:someValuesFrom ns1:EntropyPerAmountUnit ],
        ns1:SIExactConstant ;
    owl:disjointWith ns1:SpecificGasConstant ;
    skos:prefLabel "MolarGasConstant"@en ;
    ns1:ISO80000Reference "9-37.1"^^xsd:string ;
    ns1:elucidation "Equivalent to the Boltzmann constant, but expressed in units of energy per temperature increment per mole (rather than energy per temperature increment per particle)."@en ;
    ns1:iupacReference "https://doi.org/10.1351/goldbook.G02579"^^xsd:string ;
    ns1:qudtReference "http://qudt.org/vocab/constant/MolarGasConstant"^^xsd:string .

ns1:MolarGibbsEnergy a owl:Class ;
    rdfs:label "MolarGibbsEnergy"@en ;
    rdfs:comment "Gibbs energy per amount of substance."@en ;
    rdfs:subClassOf ns1:MolarEnergy,
        ns1:PhysioChemicalQuantity ;
    skos:prefLabel "MolarGibbsEnergy"@en ;
    ns1:ISO80000Reference "9-6.4"^^xsd:string ;
    ns1:elucidation "Gibbs energy per amount of substance."@en ;
    ns1:wikidataReference "https://www.wikidata.org/wiki/Q88863324"^^xsd:string .

ns1:MolarHelmholtzEnergy a owl:Class ;
    rdfs:label "MolarHelmholtzEnergy"@en ;
    rdfs:comment "Helmholtz energy per amount of substance."@en ;
    rdfs:subClassOf ns1:MolarEnergy,
        ns1:PhysioChemicalQuantity ;
    skos:prefLabel "MolarHelmholtzEnergy"@en ;
    ns1:ISO80000Reference "9-6.3"^^xsd:string ;
    ns1:elucidation "Helmholtz energy per amount of substance."@en ;
    ns1:wikidataReference "https://www.wikidata.org/wiki/Q88862986"^^xsd:string .

ns1:MolarInternalEnergy a owl:Class ;
    rdfs:label "MolarInternalEnergy"@en ;
    rdfs:comment "Internal energy per amount of substance."@en ;
    rdfs:subClassOf ns1:MolarEnergy,
        ns1:PhysioChemicalQuantity ;
    skos:prefLabel "MolarInternalEnergy"@en ;
    ns1:ISO80000Reference "9-6.1"^^xsd:string ;
    ns1:elucidation "Internal energy per amount of substance."@en ;
    ns1:wikidataReference "https://www.wikidata.org/wiki/Q88523106"^^xsd:string .

ns1:MolarMass a owl:Class ;
    rdfs:label "MolarMass"@en ;
    rdfs:comment "Mass per amount of substance."@en ;
    rdfs:subClassOf [ a owl:Restriction ;
            owl:onProperty ns1:hasMeasurementUnit ;
            owl:someValuesFrom ns1:MassPerAmountUnit ],
        ns1:ISQDerivedQuantity,
        ns1:PhysioChemicalQuantity ;
    skos:prefLabel "MolarMass"@en ;
    ns1:ISO80000Reference "9-4"^^xsd:string ;
    ns1:elucidation "Mass per amount of substance."@en ;
    ns1:qudtReference "https://qudt.org/vocab/quantitykind/MolarMass"^^xsd:string ;
    ns1:wikidataReference "https://www.wikidata.org/wiki/Q145623"^^xsd:string .

ns1:MolarVolume a owl:Class ;
    rdfs:label "MolarVolume"@en ;
    rdfs:comment "Volume per amount of substance."@en ;
    rdfs:subClassOf [ a owl:Restriction ;
            owl:onProperty ns1:hasMeasurementUnit ;
            owl:someValuesFrom ns1:VolumePerAmountUnit ],
        ns1:ISQDerivedQuantity,
        ns1:PhysioChemicalQuantity ;
    skos:prefLabel "MolarVolume"@en ;
    ns1:ISO80000Reference "9-5"^^xsd:string ;
    ns1:elucidation "Volume per amount of substance."@en ;
    ns1:qudtReference "https://qudt.org/vocab/quantitykind/MolarVolume"^^xsd:string ;
    ns1:wikidataReference "https://www.wikidata.org/wiki/Q487112"^^xsd:string .

ns1:MolecularPartitionFunction a owl:Class ;
    rdfs:label "MolecularPartitionFunction"@en ;
    rdfs:comment "Partition function of a molecule."@en ;
    rdfs:subClassOf ns1:ISQDimensionlessQuantity,
        ns1:PhysioChemicalQuantity ;
    skos:prefLabel "MolecularPartitionFunction"@en ;
    ns1:ISO80000Reference "9-35.4"^^xsd:string ;
    ns1:elucidation "Partition function of a molecule."@en ;
    ns1:wikidataReference "https://www.wikidata.org/wiki/Q96192064"^^xsd:string .

ns1:MomentOfIntertia a owl:Class ;
    rdfs:label "MomentOfIntertia"@en ;
    rdfs:comment "Scalar measure of the rotational inertia with respect to a fixed axis of rotation."@en ;
    rdfs:subClassOf [ a owl:Restriction ;
            owl:onProperty ns1:hasMeasurementUnit ;
            owl:someValuesFrom ns1:MassAreaUnit ],
        ns1:ISQDerivedQuantity,
        ns1:MechanicalQuantity ;
    skos:prefLabel "MomentOfIntertia"@en ;
    ns1:IEVReference "https://www.electropedia.org/iev/iev.nsf/display?openform&ievref=113-03-21"^^xsd:string ;
    ns1:ISO80000Reference "4-7"^^xsd:string ;
    ns1:elucidation "Scalar measure of the rotational inertia with respect to a fixed axis of rotation."@en ;
    ns1:iupacReference "https://doi.org/10.1351/goldbook.M04006"^^xsd:string ;
    ns1:qudtReference "https://qudt.org/vocab/quantitykind/MomentOfInertia"^^xsd:string ;
    ns1:wikidataReference "https://www.wikidata.org/wiki/Q165618"^^xsd:string .

ns1:Momentum a owl:Class ;
    rdfs:label "Momentum"@en ;
    rdfs:comment "Product of mass and velocity."@en ;
    rdfs:subClassOf [ a owl:Restriction ;
            owl:onProperty ns1:hasMeasurementUnit ;
            owl:someValuesFrom ns1:MomentumUnit ],
        ns1:Extensive,
        ns1:ISQDerivedQuantity ;
    skos:prefLabel "Momentum"@en ;
    ns1:ISO80000Reference "4-8"^^xsd:string ;
    ns1:elucidation "Product of mass and velocity."@en ;
    ns1:iupacReference "https://doi.org/10.1351/goldbook.M04007"^^xsd:string ;
    ns1:qudtReference "http://qudt.org/vocab/quantitykind/Momentum"^^xsd:string .

ns1:MultiplicationFactor a owl:Class ;
    rdfs:label "MultiplicationFactor"@en ;
    rdfs:comment "Quotient of the total number of fission or fission-dependent neutrons produced in the duration of a time interval and the total number of neutrons lost by absorption and leakage in that duration."@en ;
    rdfs:subClassOf ns1:AtomicAndNuclearPhysicsQuantity,
        ns1:RatioQuantity ;
    skos:prefLabel "MultiplicationFactor"@en ;
    ns1:ISO80000Reference "10-78.1"^^xsd:string ;
    ns1:elucidation "Quotient of the total number of fission or fission-dependent neutrons produced in the duration of a time interval and the total number of neutrons lost by absorption and leakage in that duration."@en ;
    ns1:qudtReference "https://qudt.org/vocab/quantitykind/MultiplicationFactor"^^xsd:string ;
    ns1:wikidataReference "https://www.wikidata.org/wiki/Q99440471"^^xsd:string .

ns1:MutualInductance a owl:Class ;
    rdfs:label "MutualInductance"@en ;
    rdfs:comment "Given an electric current in a thin conducting loop and the linked flux caused by that electric current in another loop, the mutual inductance of the two loops is the linked flux divided by the electric current."@en ;
    rdfs:subClassOf ns1:ElectricInductance ;
    skos:prefLabel "MutualInductance"@en ;
    ns1:IEVReference "https://www.electropedia.org/iev/iev.nsf/display?openform&ievref=131-12-36"^^xsd:string ;
    ns1:ISO80000Reference "6-41.2"^^xsd:string ;
    ns1:elucidation "Given an electric current in a thin conducting loop and the linked flux caused by that electric current in another loop, the mutual inductance of the two loops is the linked flux divided by the electric current."@en ;
    ns1:iupacReference "https://doi.org/10.1351/goldbook.M04076"^^xsd:string ;
    ns1:wikidataReference "https://www.wikidata.org/wiki/Q78101401"^^xsd:string .

ns1:NeelTemperature a owl:Class ;
    rdfs:label "NeelTemperature"@en ;
    rdfs:comment "Critical thermodynamic temperature of an antiferromagnet."@en ;
    rdfs:subClassOf ns1:CondensedMatterPhysicsQuantity,
        ns1:CriticalTemperature ;
    skos:prefLabel "NeelTemperature"@en ;
    ns1:IEVReference "https://www.electropedia.org/iev/iev.nsf/display?openform&ievref=121-12-52"^^xsd:string ;
    ns1:ISO80000Reference "12-35.2"^^xsd:string ;
    ns1:elucidation "Critical thermodynamic temperature of an antiferromagnet."@en ;
    ns1:wikidataReference "https://www.wikidata.org/wiki/Q830311"^^xsd:string .

ns1:NeutronNumber a owl:Class ;
    rdfs:label "NeutronNumber"@en ;
    rdfs:comment "Number of neutrons in an atomic nucleus."@en ;
    rdfs:subClassOf ns1:AtomicAndNuclearPhysicsQuantity,
        ns1:PureNumberQuantity ;
    skos:prefLabel "NeutronNumber"@en ;
    ns1:IEVReference "https://www.electropedia.org/iev/iev.nsf/display?openform&ievref=113-05-34"^^xsd:string ;
    ns1:ISO80000Reference "10-1.2"^^xsd:string ;
    ns1:elucidation "Number of neutrons in an atomic nucleus."@en ;
    ns1:iupacReference "https://doi.org/10.1351/goldbook.N04119"^^xsd:string ;
    ns1:note "Atomic number (proton number) plus neutron number equals mass number."@en ;
    ns1:wikidataReference "https://www.wikidata.org/wiki/Q970319"^^xsd:string ;
    ns1:wikipediaReference "https://en.wikipedia.org/wiki/Neutron_number"^^xsd:string .

ns1:NeutronYieldPerAbsorption a owl:Class ;
    rdfs:label "NeutronYieldPerAbsorption"@en ;
    rdfs:comment "Average number of fission neutrons, both prompt and delayed, emitted per neutron absorbed in a fissionable nuclide or in a nuclear fuel, as specified."@en ;
    rdfs:subClassOf ns1:AtomicAndNuclearPhysicsQuantity,
        ns1:PureNumberQuantity ;
    skos:prefLabel "NeutronYieldPerAbsorption"@en ;
    ns1:ISO80000Reference "10-74.2"^^xsd:string ;
    ns1:elucidation "Average number of fission neutrons, both prompt and delayed, emitted per neutron absorbed in a fissionable nuclide or in a nuclear fuel, as specified."@en ;
    ns1:qudtReference "https://qudt.org/vocab/quantitykind/NeutronYieldPerAbsorption"^^xsd:string ;
    ns1:wikidataReference "https://www.wikidata.org/wiki/Q99159075"^^xsd:string .

ns1:NeutronYieldPerFission a owl:Class ;
    rdfs:label "NeutronYieldPerFission"@en ;
    rdfs:comment "Average number of fission neutrons, both prompt and delayed, emitted per fission event."@en ;
    rdfs:subClassOf ns1:AtomicAndNuclearPhysicsQuantity,
        ns1:PureNumberQuantity ;
    skos:prefLabel "NeutronYieldPerFission"@en ;
    ns1:ISO80000Reference "10-74.1"^^xsd:string ;
    ns1:elucidation "Average number of fission neutrons, both prompt and delayed, emitted per fission event."@en ;
    ns1:qudtReference "https://qudt.org/vocab/quantitykind/NeutronYieldPerFission"^^xsd:string ;
    ns1:wikidataReference "https://www.wikidata.org/wiki/Q99157909"^^xsd:string .

ns1:NewtonianConstantOfGravity a owl:Class ;
    rdfs:label "NewtonianConstantOfGravity"@en ;
    rdfs:comment "Physical constant in Newton's law of gravitation and in Einstein's general theory of relativity."@en ;
    rdfs:subClassOf [ a owl:Restriction ;
            owl:onProperty ns1:hasMeasurementUnit ;
            owl:someValuesFrom ns1:NewtonianConstantOfGravityUnit ],
        ns1:MeasuredConstant ;
    skos:prefLabel "NewtonianConstantOfGravity"@en ;
    ns1:elucidation "Physical constant in Newton's law of gravitation and in Einstein's general theory of relativity."@en ;
    ns1:iupacReference "https://doi.org/10.1351/goldbook.G02695"^^xsd:string ;
    ns1:qudtReference "http://qudt.org/vocab/constant/NewtonianConstantOfGravitation"^^xsd:string .

ns1:NonActivePower a owl:Class ;
    rdfs:label "NonActivePower"@en ;
    rdfs:comment "For a two-terminal element or a two-terminal circuit under periodic conditions, quantity equal to the square root of the difference of the squares of the apparent power S and the active power P."@en ;
    rdfs:subClassOf ns1:Power ;
    skos:prefLabel "NonActivePower"@en ;
    ns1:IEVReference "https://www.electropedia.org/iev/iev.nsf/display?openform&ievref=131-11-43"^^xsd:string ;
    ns1:ISO80000Reference "6-61"^^xsd:string ;
    ns1:elucidation "For a two-terminal element or a two-terminal circuit under periodic conditions, quantity equal to the square root of the difference of the squares of the apparent power S and the active power P."@en ;
    ns1:qudtReference "https://qudt.org/vocab/quantitykind/NonActivePower"^^xsd:string ;
    ns1:wikidataReference "https://www.wikidata.org/wiki/Q79813060"^^xsd:string .

ns1:NonLeakageProbability a owl:Class ;
    rdfs:label "NonLeakageProbability"@en ;
    rdfs:comment "Probability that a neutron will not escape from the reactor during the slowing-down process or while it diffuses as a thermal neutron."@en ;
    rdfs:subClassOf ns1:AtomicAndNuclearPhysicsQuantity,
        ns1:Probability ;
    skos:prefLabel "NonLeakageProbability"@en ;
    ns1:ISO80000Reference "10-77"^^xsd:string ;
    ns1:elucidation "Probability that a neutron will not escape from the reactor during the slowing-down process or while it diffuses as a thermal neutron."@en ;
    ns1:qudtReference "https://qudt.org/vocab/quantitykind/Non-LeakageProbability"^^xsd:string ;
    ns1:wikidataReference "https://www.wikidata.org/wiki/Q99415566"^^xsd:string .

ns1:NuclearMagneton a owl:Class ;
    rdfs:label "NuclearMagneton"^^xsd:string ;
    rdfs:comment "Absolute value of the magnetic moment of a nucleus."@en ;
    rdfs:subClassOf [ a owl:Restriction ;
            owl:onProperty ns1:hasMeasurementUnit ;
            owl:someValuesFrom ns1:MagneticDipoleMomentUnit ],
        ns1:AtomicAndNuclearPhysicsQuantity,
        ns1:ISQDerivedQuantity ;
    skos:prefLabel "NuclearMagneton"^^xsd:string ;
    ns1:ISO80000Reference "10-9.3"^^xsd:string ;
    ns1:elucidation "Absolute value of the magnetic moment of a nucleus."@en ;
    ns1:iupacReference "https://doi.org/10.1351/goldbook.N04236"^^xsd:string ;
    ns1:wikidataReference "https://www.wikidata.org/wiki/Q1166093"^^xsd:string .

ns1:NuclearPrecessionAngularFrequency a owl:Class ;
    rdfs:label "NuclearPrecessionAngularFrequency"@en ;
    rdfs:comment "Frequency by which the nucleus angular momentum vector precesses about the axis of an external magnetic field."@en ;
    rdfs:subClassOf ns1:AngularFrequency,
        ns1:AtomicAndNuclearPhysicsQuantity ;
    skos:prefLabel "NuclearPrecessionAngularFrequency"@en ;
    ns1:ISO80000Reference "10-15.3"^^xsd:string ;
    ns1:elucidation "Frequency by which the nucleus angular momentum vector precesses about the axis of an external magnetic field."@en ;
    ns1:wikidataReference "https://www.wikidata.org/wiki/Q97641779"^^xsd:string .

ns1:NuclearQuadrupoleMoment a owl:Class ;
    rdfs:label "NuclearQuadrupoleMoment"@en ;
    rdfs:comment "z component of the diagonalized tensor of nuclear quadrupole moment, in the quantum state with the nuclear spin in the field direction (z)."@en ;
    rdfs:subClassOf [ a owl:Restriction ;
            owl:onProperty ns1:hasMeasurementUnit ;
            owl:someValuesFrom ns1:AreaUnit ],
        ns1:AtomicAndNuclearPhysicsQuantity,
        ns1:ISQDerivedQuantity ;
    skos:prefLabel "NuclearQuadrupoleMoment"@en ;
    ns1:ISO80000Reference "10-18"^^xsd:string ;
    ns1:elucidation "z component of the diagonalized tensor of nuclear quadrupole moment, in the quantum state with the nuclear spin in the field direction (z)."@en ;
    ns1:qudtReference "https://qudt.org/vocab/quantitykind/NuclearQuadrupoleMoment"^^xsd:string ;
    ns1:wikidataReference "https://www.wikidata.org/wiki/Q97921226"^^xsd:string .

ns1:NuclearRadius a owl:Class ;
    rdfs:label "NuclearRadius"@en ;
    rdfs:comment "Conventional radius of sphere in which the nuclear matter is included,"@en ;
    rdfs:subClassOf ns1:AtomicAndNuclearPhysicsQuantity,
        ns1:Radius ;
    skos:prefLabel "NuclearRadius"@en ;
    ns1:ISO80000Reference "10-19.1"^^xsd:string ;
    ns1:elucidation "Conventional radius of sphere in which the nuclear matter is included,"@en ;
    ns1:qudtReference "https://qudt.org/vocab/quantitykind/NuclearRadius"^^xsd:string ;
    ns1:wikidataReference "https://www.wikidata.org/wiki/Q3535676"^^xsd:string .

ns1:NuclearSpinQuantumNumber a owl:Class ;
    rdfs:label "NuclearSpinQuantumNumber"^^xsd:string ;
    rdfs:comment "Quantum number related to the total angular momentum, J, of a nucleus in any specified state, normally called nuclear spin."@en ;
    rdfs:subClassOf ns1:QuantumNumber ;
    skos:prefLabel "NuclearSpinQuantumNumber"^^xsd:string ;
    ns1:ISO80000Reference "10-13.7"^^xsd:string ;
    ns1:elucidation "Quantum number related to the total angular momentum, J, of a nucleus in any specified state, normally called nuclear spin."@en ;
    ns1:qudtReference "https://qudt.org/vocab/quantitykind/NuclearSpinQuantumNumber"^^xsd:string ;
    ns1:wikidataReference "https://www.wikidata.org/wiki/Q97577403"^^xsd:string .

ns1:NucleonNumber a owl:Class ;
    rdfs:label "NucleonNumber"@en ;
    rdfs:comment "number of nucleons in an atomic nucleus"@en ;
    rdfs:subClassOf ns1:AtomicAndNuclearPhysicsQuantity,
        ns1:PureNumberQuantity ;
    skos:altLabel "MassNumber"@en ;
    skos:prefLabel "NucleonNumber"@en ;
    ns1:IEVReference "https://www.electropedia.org/iev/iev.nsf/display?openform&ievref=113-05-32"^^xsd:string ;
    ns1:ISO80000Reference "10-1.3"^^xsd:string ;
    ns1:dbpediaReference "https://dbpedia.org/page/Mass_number"^^xsd:string ;
    ns1:elucidation "number of nucleons in an atomic nucleus"@en ;
    ns1:iupacReference "https://doi.org/10.1351/goldbook.M03726"^^xsd:string ;
    ns1:qudtReference "https://qudt.org/vocab/quantitykind/NucleonNumber"^^xsd:string ;
    ns1:wikidataReference "https://www.wikidata.org/wiki/Q101395"^^xsd:string ;
    ns1:wikipediaReference "https://en.wikipedia.org/wiki/Mass_number"^^xsd:string .

ns1:NuclidicMass a owl:Class ;
    rdfs:label "NuclidicMass"^^xsd:string ;
    rdfs:comment "Rest mass of a nuclide X in the ground state."@en ;
    rdfs:subClassOf ns1:AtomicAndNuclearPhysicsQuantity,
        ns1:RestMass ;
    skos:prefLabel "NuclidicMass"^^xsd:string ;
    ns1:ISO80000Reference "10-4.2"^^xsd:string ;
    ns1:elucidation "Rest mass of a nuclide X in the ground state."@en ;
    ns1:iupacReference "https://doi.org/10.1351/goldbook.N04258"^^xsd:string ;
    ns1:wikidataReference "https://www.wikidata.org/wiki/Q97010809"^^xsd:string .

ns1:NumberOfElements a owl:Class ;
    rdfs:label "NumberOfElements"@en ;
    rdfs:comment "Number of direct parts of a Reductionistic."@en,
        "Using direct parthood EMMO creates a well-defined broadcasting between granularity levels. This also make it possible to count the direct parts of each granularity level."@en ;
    rdfs:subClassOf [ a owl:Restriction ;
            owl:allValuesFrom ns1:Reductionistic ;
            owl:onProperty [ owl:inverseOf ns1:hasProperty ] ],
        ns1:PureNumberQuantity ;
    skos:prefLabel "NumberOfElements"@en ;
    ns1:elucidation "Number of direct parts of a Reductionistic."@en .

ns1:NumberOfEntities a owl:Class ;
    rdfs:label "NumberOfEntities"@en ;
    rdfs:comment "Discrete quantity; number of entities of a given kind in a system."@en ;
    rdfs:subClassOf ns1:PhysioChemicalQuantity,
        ns1:PureNumberQuantity ;
    skos:prefLabel "NumberOfEntities"@en ;
    ns1:IEVReference "https://www.electropedia.org/iev/iev.nsf/display?openform&ievref=112-01-09"^^xsd:string ;
    ns1:ISO80000Reference "9-1"^^xsd:string ;
    ns1:elucidation "Discrete quantity; number of entities of a given kind in a system."@en ;
    ns1:iupacReference "https://doi.org/10.1351/goldbook.N04266"^^xsd:string ;
    ns1:wikidataReference "https://www.wikidata.org/wiki/Q614112"^^xsd:string .

ns1:NumberOfTurnsInAWinding a owl:Class ;
    rdfs:label "NumberOfTurnsInAWinding"@en ;
    rdfs:comment "Number of turns in a winding."@en ;
    rdfs:subClassOf ns1:ElectromagneticQuantity,
        ns1:PureNumberQuantity ;
    skos:prefLabel "NumberOfTurnsInAWinding"@en ;
    ns1:ISO80000Reference "6-38"^^xsd:string ;
    ns1:elucidation "Number of turns in a winding."@en ;
    ns1:wikidataReference "https://www.wikidata.org/wiki/Q77995997"^^xsd:string .

ns1:OrbitalAngularMomentumQuantumNumber a owl:Class ;
    rdfs:label "OrbitalAngularMomentumQuantumNumber"^^xsd:string ;
    rdfs:comment "Atomic quantum number related to the orbital angular momentum l of a one-electron state."@en ;
    rdfs:subClassOf ns1:QuantumNumber ;
    skos:prefLabel "OrbitalAngularMomentumQuantumNumber"^^xsd:string ;
    ns1:ISO80000Reference "10-13.3"^^xsd:string ;
    ns1:elucidation "Atomic quantum number related to the orbital angular momentum l of a one-electron state."@en ;
    ns1:qudtReference "https://qudt.org/vocab/quantitykind/OrbitalAngularMomentumQuantumNumber"^^xsd:string ;
    ns1:wikidataReference "https://www.wikidata.org/wiki/Q1916324"^^xsd:string .

ns1:OsmoticCoefficientOfSolvent a owl:Class ;
    rdfs:label "OsmoticCoefficientOfSolvent"@en ;
    rdfs:comment "Quantity characterizing the deviation of a solvent from ideal behavior."@en ;
    rdfs:subClassOf ns1:ISQDimensionlessQuantity,
        ns1:PhysioChemicalQuantity ;
    skos:altLabel "OsmoticFactorOfSolvent"@en ;
    skos:prefLabel "OsmoticCoefficientOfSolvent"@en ;
    ns1:ISO80000Reference "9-27.2"^^xsd:string ;
    ns1:elucidation "Quantity characterizing the deviation of a solvent from ideal behavior."@en ;
    ns1:iupacReference "https://doi.org/10.1351/goldbook.O04342"^^xsd:string ;
    ns1:qudtReference "https://qudt.org/vocab/quantitykind/OsmoticCoefficient"^^xsd:string ;
    ns1:wikidataReference "https://www.wikidata.org/wiki/Q5776102"^^xsd:string .

ns1:OsmoticPressure a owl:Class ;
    rdfs:label "OsmoticPressure"@en ;
    rdfs:comment "Measure of the tendency of a solution to take in pure solvent by osmosis."@en ;
    rdfs:subClassOf ns1:PhysioChemicalQuantity,
        ns1:Pressure ;
    skos:prefLabel "OsmoticPressure"@en ;
    ns1:ISO80000Reference "9-28"^^xsd:string ;
    ns1:elucidation "Measure of the tendency of a solution to take in pure solvent by osmosis."@en ;
    ns1:iupacReference "https://doi.org/10.1351/goldbook.O04344"^^xsd:string ;
    ns1:qudtReference "https://qudt.org/vocab/quantitykind/OsmoticPressure"^^xsd:string ;
    ns1:wikidataReference "https://www.wikidata.org/wiki/Q193135"^^xsd:string .

ns1:OxidationNumber a owl:Class ;
    rdfs:label "OxidationNumber"@en ;
    rdfs:comment "Charge number that an atom within a molecule would have if all the ligands were removed along with the electron pairs that were shared."@en ;
    rdfs:subClassOf ns1:ChargeNumber ;
    skos:altLabel "OxidationState"@en ;
    skos:prefLabel "OxidationNumber"@en ;
    ns1:IEVReference "https://www.electropedia.org/iev/iev.nsf/display?openform&ievref=114-01-25"^^xsd:string ;
    ns1:dbpediaReference "https://dbpedia.org/page/Oxidation_state"^^xsd:string ;
    ns1:elucidation "Charge number that an atom within a molecule would have if all the ligands were removed along with the electron pairs that were shared."@en ;
    ns1:iupacReference "https://doi.org/10.1351/goldbook.O04363"^^xsd:string ;
    ns1:wikidataReference "https://www.wikidata.org/wiki/Q484152"^^xsd:string ;
    ns1:wikipediaReference "https://en.wikipedia.org/wiki/Oxidation_state"^^xsd:string .

ns1:POH a owl:Class ;
    rdfs:label "POH"@en ;
    rdfs:comment "Written as pOH"@en,
        """number quantifying the acidic or the alkaline character of a solution, equal to the negative of the decimal logarithm of ion activity aOH- of the hydroxide anion OH-
pH = −10 log(a_OH-)"""@en ;
    rdfs:subClassOf ns1:IonActivity ;
    owl:disjointWith ns1:PH ;
    skos:prefLabel "POH"@en ;
    ns1:elucidation """number quantifying the acidic or the alkaline character of a solution, equal to the negative of the decimal logarithm of ion activity aOH- of the hydroxide anion OH-
pH = −10 log(a_OH-)"""@en .

ns1:PackingFraction a owl:Class ;
    rdfs:label "PackingFraction"@en ;
    rdfs:comment "Quotient of relative mass excess and the nucleon number."@en ;
    rdfs:subClassOf ns1:AtomicAndNuclearPhysicsQuantity,
        ns1:ISQDimensionlessQuantity ;
    skos:prefLabel "PackingFraction"@en ;
    ns1:ISO80000Reference "10-23.1"^^xsd:string ;
    ns1:elucidation "Quotient of relative mass excess and the nucleon number."@en ;
    ns1:qudtReference "https://qudt.org/vocab/quantitykind/PackingFraction"^^xsd:string ;
    ns1:wikidataReference "https://www.wikidata.org/wiki/Q98058276"^^xsd:string .

ns1:PartialPressure a owl:Class ;
    rdfs:label "PartialPressure"@en ;
    rdfs:comment "Hypothetical pressure of gas if it alone occupied the volume of the mixture at the same temperature."@en ;
    rdfs:subClassOf ns1:PhysioChemicalQuantity,
        ns1:Pressure ;
    skos:prefLabel "PartialPressure"@en ;
    ns1:ISO80000Reference "9-19"^^xsd:string ;
    ns1:elucidation "Hypothetical pressure of gas if it alone occupied the volume of the mixture at the same temperature."@en ;
    ns1:iupacReference "https://doi.org/10.1351/goldbook.P04420"^^xsd:string ;
    ns1:qudtReference "https://qudt.org/vocab/quantitykind/PartialPressure"^^xsd:string ;
    ns1:wikidataReference "https://www.wikidata.org/wiki/Q27165"^^xsd:string .

ns1:ParticleConcentration a owl:Class ;
    rdfs:label "ParticleConcentration"@en ;
    rdfs:comment "Number of particles of a given species per volume."@en ;
    rdfs:subClassOf [ a owl:Restriction ;
            owl:onProperty ns1:hasMeasurementUnit ;
            owl:someValuesFrom ns1:PerVolumeUnit ],
        ns1:Concentration,
        ns1:ISQDerivedQuantity,
        ns1:PhysioChemicalQuantity ;
    owl:disjointWith ns1:MolecularConcentration,
        ns1:ParticleNumberDensity,
        ns1:VolumetricNumberDensity ;
    skos:prefLabel "ParticleConcentration"@en ;
    ns1:ISO80000Reference "9-9.1"^^xsd:string ;
    ns1:elucidation "Number of particles of a given species per volume."@en ;
    ns1:wikidataReference "https://www.wikidata.org/wiki/Q39078574"^^xsd:string .

ns1:ParticleCurrentDensity a owl:Class ;
    rdfs:label "ParticleCurrentDensity"@en ;
    rdfs:comment "Number of particles per time and area crossing a surface."@en ;
    rdfs:subClassOf [ a owl:Restriction ;
            owl:onProperty ns1:hasMeasurementUnit ;
            owl:someValuesFrom ns1:PerAreaTimeUnit ],
        ns1:AtomicAndNuclearPhysicsQuantity,
        ns1:ISQDerivedQuantity ;
    skos:prefLabel "ParticleCurrentDensity"@en ;
    ns1:ISO80000Reference "10-48"^^xsd:string ;
    ns1:elucidation "Number of particles per time and area crossing a surface."@en ;
    ns1:qudtReference "https://qudt.org/vocab/quantitykind/ParticleCurrent"^^xsd:string ;
    ns1:wikidataReference "https://www.wikidata.org/wiki/Q2400689"^^xsd:string .

ns1:ParticleEmissionRate a owl:Class ;
    rdfs:label "ParticleEmissionRate"@en ;
    rdfs:comment "Differential quotient of N with respect to time, where N is the number of particles being emitted from an infinitesimally small volume element in the time interval of duration dt, and dt."@en ;
    rdfs:subClassOf ns1:AtomicAndNuclearPhysicsQuantity,
        ns1:ReciprocalDuration ;
    skos:prefLabel "ParticleEmissionRate"@en ;
    ns1:ISO80000Reference "10-36"^^xsd:string ;
    ns1:elucidation "Differential quotient of N with respect to time, where N is the number of particles being emitted from an infinitesimally small volume element in the time interval of duration dt, and dt."@en ;
    ns1:wikidataReference "https://www.wikidata.org/wiki/Q98153151"^^xsd:string .

ns1:ParticleFluence a owl:Class ;
    rdfs:label "ParticleFluence"@en ;
    rdfs:comment "Differential quotient of N with respect to a, where N is the number of particles incident on a sphere of cross-sectional area a."@en ;
    rdfs:subClassOf [ a owl:Restriction ;
            owl:onProperty ns1:hasMeasurementUnit ;
            owl:someValuesFrom ns1:PerAreaUnit ],
        ns1:AtomicAndNuclearPhysicsQuantity,
        ns1:ISQDerivedQuantity ;
    skos:prefLabel "ParticleFluence"@en ;
    ns1:IEVReference "https://www.electropedia.org/iev/iev.nsf/display?openform&ievref=395-01-15"^^xsd:string,
        "https://www.electropedia.org/iev/iev.nsf/display?openform&ievref=881-04-18"^^xsd:string ;
    ns1:ISO80000Reference "10-43"^^xsd:string ;
    ns1:elucidation "Differential quotient of N with respect to a, where N is the number of particles incident on a sphere of cross-sectional area a."@en ;
    ns1:qudtReference "https://qudt.org/vocab/quantitykind/ParticleFluence"^^xsd:string ;
    ns1:wikidataReference "https://www.wikidata.org/wiki/Q82965908"^^xsd:string .

ns1:ParticleFluenceRate a owl:Class ;
    rdfs:label "ParticleFluenceRate"@en ;
    rdfs:comment "Differential quotient of fluence Φ with respect to time."@en ;
    rdfs:subClassOf [ a owl:Restriction ;
            owl:onProperty ns1:hasMeasurementUnit ;
            owl:someValuesFrom ns1:PerAreaTimeUnit ],
        ns1:AtomicAndNuclearPhysicsQuantity,
        ns1:ISQDerivedQuantity ;
    skos:prefLabel "ParticleFluenceRate"@en ;
    ns1:IEVReference "https://www.electropedia.org/iev/iev.nsf/display?openform&ievref=395-01-16"^^xsd:string,
        "https://www.electropedia.org/iev/iev.nsf/display?openform&ievref=881-04-19"^^xsd:string ;
    ns1:ISO80000Reference "10-44"^^xsd:string ;
    ns1:elucidation "Differential quotient of fluence Φ with respect to time."@en ;
    ns1:qudtReference "https://qudt.org/vocab/quantitykind/ParticleFluenceRate"^^xsd:string ;
    ns1:wikidataReference "https://www.wikidata.org/wiki/Q98497410"^^xsd:string .

ns1:ParticlePositionVector a owl:Class ;
    rdfs:label "ParticlePositionVector"@en ;
    rdfs:comment "Position vector of a particle."@en ;
    rdfs:subClassOf ns1:CondensedMatterPhysicsQuantity,
        ns1:PositionVector ;
    skos:prefLabel "ParticlePositionVector"@en ;
    ns1:ISO80000Reference "12-7.1"^^xsd:string ;
    ns1:elucidation "Position vector of a particle."@en ;
    ns1:qudtReference "https://qudt.org/vocab/quantitykind/ParticlePositionVector"^^xsd:string ;
    ns1:wikidataReference "https://www.wikidata.org/wiki/Q105533324"^^xsd:string .

ns1:ParticleSourceDensity a owl:Class ;
    rdfs:label "ParticleSourceDensity"@en ;
    rdfs:comment "Quotient of the mean rate of production of particles in a volume, and that volume."@en ;
    rdfs:subClassOf [ a owl:Restriction ;
            owl:onProperty ns1:hasMeasurementUnit ;
            owl:someValuesFrom ns1:FrequencyPerVolumeUnit ],
        ns1:AtomicAndNuclearPhysicsQuantity,
        ns1:ISQDerivedQuantity ;
    skos:prefLabel "ParticleSourceDensity"@en ;
    ns1:ISO80000Reference "10-66"^^xsd:string ;
    ns1:elucidation "Quotient of the mean rate of production of particles in a volume, and that volume."@en ;
    ns1:qudtReference "https://qudt.org/vocab/quantitykind/ParticleSourceDensity"^^xsd:string ;
    ns1:wikidataReference "https://www.wikidata.org/wiki/Q98915762"^^xsd:string .

ns1:PeltierCoefficient a owl:Class ;
    rdfs:label "PeltierCoefficient"@en ;
    rdfs:comment "Quotient of Peltier heat power developed at a junction, and the electric current flowing from substance a to substance b."@en ;
    rdfs:subClassOf [ a owl:Restriction ;
            owl:onProperty ns1:hasMeasurementUnit ;
            owl:someValuesFrom ns1:ElectricPotentialUnit ],
        ns1:CondensedMatterPhysicsQuantity,
        ns1:ISQDerivedQuantity ;
    skos:prefLabel "PeltierCoefficient"@en ;
    ns1:ISO80000Reference "12-22"^^xsd:string ;
    ns1:elucidation "Quotient of Peltier heat power developed at a junction, and the electric current flowing from substance a to substance b."@en ;
    ns1:qudtReference "https://qudt.org/vocab/quantitykind/PeltierCoefficient"^^xsd:string ;
    ns1:wikidataReference "https://www.wikidata.org/wiki/Q105801003"^^xsd:string .

ns1:PerEnergyUnit a owl:Class ;
    rdfs:label "PerEnergyUnit"@en ;
    rdfs:comment "The class of units with dimensionality 'PerEnergy'."@en .

ns1:PerLengthTemperatureUnit a owl:Class ;
    rdfs:label "PerLengthTemperatureUnit"@en ;
    rdfs:comment "The class of units with dimensionality 'PerLengthTemperature'."@en .

ns1:PerLengthTimeUnit a owl:Class ;
    rdfs:label "PerLengthTimeUnit"@en ;
    rdfs:comment "The class of units with dimensionality 'PerLengthTime'."@en .

ns1:PerTemperatureTimeUnit a owl:Class ;
    rdfs:label "PerTemperatureTimeUnit"@en ;
    rdfs:comment "The class of units with dimensionality 'PerTemperatureTime'."@en .

ns1:PeriodDuration a owl:Class ;
    rdfs:label "PeriodDuration"@en ;
    rdfs:comment "duration of one cycle of a periodic event"@en ;
    rdfs:subClassOf ns1:Duration ;
    skos:altLabel "Period"@en ;
    skos:prefLabel "PeriodDuration"@en ;
    ns1:IEVReference "https://www.electropedia.org/iev/iev.nsf/display?openform&ievref=103-06-01"^^xsd:string ;
    ns1:ISO80000Reference "3-14"^^xsd:string ;
    ns1:elucidation "duration of one cycle of a periodic event"@en ;
    ns1:iupacReference "https://doi.org/10.1351/goldbook.P04493"^^xsd:string ;
    ns1:qudtReference "https://qudt.org/vocab/quantitykind/Period"^^xsd:string ;
    ns1:wikidataReference "https://www.wikidata.org/wiki/Q2642727"^^xsd:string .

ns1:Permeance a owl:Class ;
    rdfs:label "Permeance"@en ;
    rdfs:comment "Inverse of the reluctance."@en ;
    rdfs:subClassOf [ a owl:Restriction ;
            owl:onProperty ns1:hasMeasurementUnit ;
            owl:someValuesFrom ns1:InductanceUnit ],
        ns1:ElectromagneticQuantity,
        ns1:ISQDerivedQuantity ;
    skos:prefLabel "Permeance"@en ;
    ns1:IEVReference "https://www.electropedia.org/iev/iev.nsf/display?openform&ievref=131-12-29"^^xsd:string ;
    ns1:ISO80000Reference "6-40"^^xsd:string ;
    ns1:elucidation "Inverse of the reluctance."@en ;
    ns1:qudtReference "https://qudt.org/vocab/quantitykind/Permeance"^^xsd:string ;
    ns1:wikidataReference "https://www.wikidata.org/wiki/Q77997985"^^xsd:string .

ns1:PhaseAngle a owl:Class ;
    rdfs:label "PhaseAngle"@en ;
    rdfs:comment "Angular measure between the positive real axis and the radius of the polar representation of the complex number in the complex plane."@en ;
    rdfs:subClassOf ns1:Angle,
        ns1:SpaceAndTimeQuantity ;
    skos:prefLabel "PhaseAngle"@en ;
    ns1:IEVReference "https://www.electropedia.org/iev/iev.nsf/display?openform&ievref=103-07-04"^^xsd:string,
        "https://www.electropedia.org/iev/iev.nsf/display?openform&ievref=141-01-01"^^xsd:string ;
    ns1:ISO80000Reference "3-7"^^xsd:string ;
    ns1:elucidation "Angular measure between the positive real axis and the radius of the polar representation of the complex number in the complex plane."@en ;
    ns1:wikidataReference "https://www.wikidata.org/wiki/Q415829"^^xsd:string .

ns1:PhaseCoefficient a owl:Class ;
    rdfs:label "PhaseCoefficient"@en ;
    rdfs:comment "Change of phase angle with the length along the path travelled by a plane wave."@en ;
    rdfs:subClassOf ns1:ReciprocalLength,
        ns1:SpaceAndTimeQuantity ;
    skos:altLabel "PhaseChangeCoefficient"@en ;
    skos:prefLabel "PhaseCoefficient"@en ;
    ns1:IEVReference "https://www.electropedia.org/iev/iev.nsf/display?openform&ievref=103-10-20"^^xsd:string ;
    ns1:ISO80000Reference "3-26.2"^^xsd:string ;
    ns1:elucidation "Change of phase angle with the length along the path travelled by a plane wave."@en ;
    ns1:note "The imaginary part of the propagation coefficient."@en ;
    ns1:qudtReference "https://qudt.org/vocab/quantitykind/PhaseCoefficient"^^xsd:string ;
    ns1:wikidataReference "https://www.wikidata.org/wiki/Q32745742"^^xsd:string ;
    ns1:wikipediaReference "https://en.wikipedia.org/wiki/Propagation_constant#Phase_constant"^^xsd:string .

ns1:PhaseDifference a owl:Class ;
    rdfs:label "PhaseDifference"@en ;
    rdfs:comment "Under sinusoidal conditions, phase difference between the voltage applied to a linear two-terminal element or two-terminal circuit and the electric current in the element or circuit."@en ;
    rdfs:subClassOf ns1:Angle,
        ns1:ElectromagneticQuantity ;
    skos:altLabel "DisplacementAngle"@en ;
    skos:prefLabel "PhaseDifference"@en ;
    ns1:IEVReference "https://www.electropedia.org/iev/iev.nsf/display?openform&ievref=131-11-48"^^xsd:string ;
    ns1:ISO80000Reference "6-48"^^xsd:string ;
    ns1:elucidation "Under sinusoidal conditions, phase difference between the voltage applied to a linear two-terminal element or two-terminal circuit and the electric current in the element or circuit."@en ;
    ns1:wikidataReference "https://www.wikidata.org/wiki/Q97222919"^^xsd:string .

ns1:PhaseSpeedOfElectromagneticWaves a owl:Class ;
    rdfs:label "PhaseSpeedOfElectromagneticWaves"@en ;
    rdfs:comment "Angular frequency divided by angular wavenumber."@en ;
    rdfs:subClassOf ns1:ElectromagneticQuantity,
        ns1:Speed ;
    skos:prefLabel "PhaseSpeedOfElectromagneticWaves"@en ;
    ns1:ISO80000Reference "6-35.1"^^xsd:string ;
    ns1:elucidation "Angular frequency divided by angular wavenumber."@en ;
    ns1:qudtReference "https://qudt.org/vocab/quantitykind/ElectromagneticWavePhaseSpeed"^^xsd:string ;
    ns1:wikidataReference "https://www.wikidata.org/wiki/Q77990619"^^xsd:string .

ns1:PhaseVelocity a owl:Class ;
    rdfs:label "PhaseVelocity"@en ;
    rdfs:comment "For a sinusoidal wave at a given point, velocity in the direction of propagation of the wavefront corresponding to a specified phase."@en ;
    rdfs:subClassOf ns1:Velocity ;
    skos:altLabel "PhaseSpeed"@en ;
    skos:prefLabel "PhaseVelocity"@en ;
    ns1:IEVReference "https://www.electropedia.org/iev/iev.nsf/display?openform&ievref=103-10-13"^^xsd:string ;
    ns1:ISO80000Reference "3-23.1"^^xsd:string ;
    ns1:dbpediaReference "https://dbpedia.org/page/Phase_velocity"^^xsd:string ;
    ns1:elucidation "For a sinusoidal wave at a given point, velocity in the direction of propagation of the wavefront corresponding to a specified phase."@en ;
    ns1:wikidataReference "https://www.wikidata.org/wiki/Q13824"^^xsd:string ;
    ns1:wikipediaReference "https://en.wikipedia.org/wiki/Phase_velocity"^^xsd:string .

ns1:PlanckConstant a owl:Class ;
    rdfs:label "PlanckConstant"@en ;
    rdfs:comment "The quantum of action. It defines the kg base unit in the SI system."@en ;
    rdfs:subClassOf ns1:AngularMomentum,
        ns1:SIExactConstant ;
    skos:prefLabel "PlanckConstant"@en ;
    ns1:elucidation "The quantum of action. It defines the kg base unit in the SI system."@en ;
    ns1:iupacReference "https://doi.org/10.1351/goldbook.P04685"^^xsd:string ;
    ns1:qudtReference "http://qudt.org/vocab/constant/PlanckConstant"^^xsd:string .

ns1:PlanckFunction a owl:Class ;
    rdfs:label "PlanckFunction"@en ;
    rdfs:comment "Ngative quotient of Gibbs energy and temperature."@en ;
    rdfs:subClassOf [ a owl:Restriction ;
            owl:onProperty ns1:hasMeasurementUnit ;
            owl:someValuesFrom ns1:EntropyUnit ],
        ns1:ISQDerivedQuantity,
        ns1:ThermodynamicalQuantity ;
    skos:prefLabel "PlanckFunction"@en ;
    ns1:IEVReference "https://www.electropedia.org/iev/iev.nsf/display?openform&ievref=113-04-25"^^xsd:string ;
    ns1:ISO80000Reference "5-23"^^xsd:string ;
    ns1:elucidation "Ngative quotient of Gibbs energy and temperature."@en ;
    ns1:qudtReference "https://qudt.org/vocab/quantitykind/PlanckFunction"^^xsd:string ;
    ns1:wikidataReference "https://www.wikidata.org/wiki/Q76364998"^^xsd:string .

ns1:PoissonNumber a owl:Class ;
    rdfs:label "PoissonNumber"@en ;
    rdfs:comment "Ratio of transverse strain to axial strain."@en ;
    rdfs:subClassOf ns1:MechanicalQuantity,
        ns1:RatioQuantity ;
    skos:altLabel "PoissonsRatio"@en ;
    skos:prefLabel "PoissonNumber"@en ;
    ns1:IEVReference "https://www.electropedia.org/iev/iev.nsf/display?openform&ievref=113-03-61"^^xsd:string ;
    ns1:ISO80000Reference "4-18"^^xsd:string ;
    ns1:elucidation "Ratio of transverse strain to axial strain."@en ;
    ns1:wikidataReference "https://www.wikidata.org/wiki/Q190453"^^xsd:string .

ns1:Porosity a owl:Class ;
    rdfs:label "Porosity"@en ;
    rdfs:comment "Ratio of void volume and total volume of a porous material."@en ;
    rdfs:subClassOf ns1:RatioQuantity ;
    skos:prefLabel "Porosity"@en ;
    ns1:IEVReference "https://www.electropedia.org/iev/iev.nsf/display?openform&ievref=801-31-32"^^xsd:string ;
    ns1:elucidation "Ratio of void volume and total volume of a porous material."@en ;
    ns1:iupacReference "https://doi.org/10.1351/goldbook.P04762"^^xsd:string ;
    ns1:wikidataReference "https://www.wikidata.org/wiki/Q622669"^^xsd:string .

ns1:PotentialEnergy a owl:Class ;
    rdfs:label "PotentialEnergy"@en ;
    rdfs:comment "The energy possessed by a body by virtue of its position or orientation in a potential field."@en ;
    rdfs:subClassOf ns1:Energy ;
    skos:prefLabel "PotentialEnergy"@en ;
    ns1:ISO80000Reference "4-28.1"^^xsd:string ;
    ns1:elucidation "The energy possessed by a body by virtue of its position or orientation in a potential field."@en ;
    ns1:iupacReference "https://doi.org/10.1351/goldbook.P04778"^^xsd:string ;
    ns1:qudtReference "http://qudt.org/vocab/quantitykind/PotentialEnergy"^^xsd:string .

ns1:PowerAreaUnit a owl:Class ;
    rdfs:label "PowerAreaUnit"@en ;
    rdfs:comment "The class of units with dimensionality 'PowerArea'."@en .

ns1:PowerFactor a owl:Class ;
    rdfs:label "PowerFactor"@en ;
    rdfs:comment "Under periodic conditions, ratio of the absolute value of the active power P to the apparent power S."@en ;
    rdfs:subClassOf ns1:ElectromagneticQuantity,
        ns1:RatioQuantity ;
    skos:prefLabel "PowerFactor"@en ;
    ns1:IEVReference "https://www.electropedia.org/iev/iev.nsf/display?openform&ievref=131-11-46"^^xsd:string ;
    ns1:ISO80000Reference "6-58"^^xsd:string ;
    ns1:elucidation "Under periodic conditions, ratio of the absolute value of the active power P to the apparent power S."@en ;
    ns1:qudtReference "https://qudt.org/vocab/quantitykind/PowerFactor"^^xsd:string ;
    ns1:wikidataReference "https://www.wikidata.org/wiki/Q750454"^^xsd:string .

ns1:PowerPerAreaVolumeUnit a owl:Class ;
    rdfs:label "PowerPerAreaVolumeUnit"@en ;
    rdfs:comment "The class of units with dimensionality 'PowerPerAreaVolume'."@en .

ns1:PoyntingVector a owl:Class ;
    rdfs:label "PoyntingVector"@en ;
    rdfs:comment "Electric field strength multiplied by magnetic field strength."@en ;
    rdfs:subClassOf [ a owl:Restriction ;
            owl:onProperty ns1:hasMeasurementUnit ;
            owl:someValuesFrom ns1:PowerDensityUnit ],
        ns1:ElectromagneticQuantity ;
    skos:prefLabel "PoyntingVector"@en ;
    ns1:IEVReference "https://www.electropedia.org/iev/iev.nsf/display?openform&ievref=121-11-66"^^xsd:string ;
    ns1:ISO80000Reference "6-34"^^xsd:string ;
    ns1:elucidation "Electric field strength multiplied by magnetic field strength."@en ;
    ns1:qudtReference "https://qudt.org/vocab/quantitykind/PoyntingVector"^^xsd:string ;
    ns1:wikidataReference "https://www.wikidata.org/wiki/Q504186"^^xsd:string .

ns1:PressurePerTimeUnit a owl:Class ;
    rdfs:label "PressurePerTimeUnit"@en ;
    rdfs:comment "The class of units with dimensionality 'PressurePerTime'."@en .

ns1:PrincipalQuantumNumber a owl:Class ;
    rdfs:label "PrincipalQuantumNumber"^^xsd:string ;
    rdfs:comment "Atomic quantum number related to the number n−1 of radial nodes of one-electron wave functions."@en ;
    rdfs:subClassOf ns1:QuantumNumber ;
    skos:prefLabel "PrincipalQuantumNumber"^^xsd:string ;
    ns1:ISO80000Reference "10-13.2"^^xsd:string ;
    ns1:elucidation "Atomic quantum number related to the number n−1 of radial nodes of one-electron wave functions."@en ;
    ns1:qudtReference "https://qudt.org/vocab/quantitykind/PrincipalQuantumNumber"^^xsd:string ;
    ns1:wikidataReference "https://www.wikidata.org/wiki/Q867448"^^xsd:string .

ns1:PropagationCoefficient a owl:Class ;
    rdfs:label "PropagationCoefficient"@en ;
    rdfs:comment "Measure of the change of amplitude and phase angle of a plane wave propagating in a given direction."@en ;
    rdfs:subClassOf ns1:ReciprocalLength,
        ns1:SpaceAndTimeQuantity ;
    skos:prefLabel "PropagationCoefficient"@en ;
    ns1:IEVReference "https://www.electropedia.org/iev/iev.nsf/display?openform&ievref=103-10-18"^^xsd:string ;
    ns1:ISO80000Reference "3-26.3"^^xsd:string ;
    ns1:elucidation "Measure of the change of amplitude and phase angle of a plane wave propagating in a given direction."@en ;
    ns1:qudtReference "https://qudt.org/vocab/quantitykind/PropagationCoefficient.html"^^xsd:string ;
    ns1:wikidataReference "https://www.wikidata.org/wiki/Q1434913"^^xsd:string .

ns1:ProtonMass a owl:Class ;
    rdfs:label "ProtonMass"@en ;
    rdfs:comment "The rest mass of a proton."@en ;
    rdfs:subClassOf ns1:Mass,
        ns1:MeasuredConstant ;
    skos:prefLabel "ProtonMass"@en ;
    ns1:iupacReference "https://doi.org/10.1351/goldbook.P04914"^^xsd:string ;
    ns1:qudtReference "http://qudt.org/vocab/constant/ProtonMass"^^xsd:string .

ns1:QualityFactor a owl:Class ;
    rdfs:label "QualityFactor"@en ;
    rdfs:comment "Dimensionless quantity in electromagnetism."@en ;
    rdfs:subClassOf ns1:ElectromagneticQuantity,
        ns1:RatioQuantity ;
    skos:prefLabel "QualityFactor"@en ;
    ns1:IEVReference "https://www.electropedia.org/iev/iev.nsf/display?openform&ievref=151-15-45"^^xsd:string ;
    ns1:ISO80000Reference "6-53"^^xsd:string ;
    ns1:elucidation "Dimensionless quantity in electromagnetism."@en ;
    ns1:qudtReference "https://qudt.org/vocab/quantitykind/QualityFactor"^^xsd:string ;
    ns1:wikidataReference "https://www.wikidata.org/wiki/Q79467569"^^xsd:string .

ns1:QuarticLengthPerTimeUnit a owl:Class ;
    rdfs:label "QuarticLengthPerTimeUnit"@en ;
    rdfs:comment "The class of units with dimensionality 'QuarticLengthPerTime'."@en .

ns1:RadiantEnergy a owl:Class ;
    rdfs:label "RadiantEnergy"@en ;
    rdfs:comment "Mean energy, excluding rest energy, of the particles that are emitted, transferred, or received."@en ;
    rdfs:subClassOf ns1:AtomicAndNuclearPhysicsQuantity,
        ns1:Energy ;
    skos:prefLabel "RadiantEnergy"@en ;
    ns1:ISO80000Reference "10-45"^^xsd:string ;
    ns1:elucidation "Mean energy, excluding rest energy, of the particles that are emitted, transferred, or received."@en ;
    ns1:wikidataReference "https://www.wikidata.org/wiki/Q1259526"^^xsd:string .

ns1:RadiantFlux a owl:Class ;
    rdfs:label "RadiantFlux"@en ;
    rdfs:comment "The radiant energy emitted, reflected, transmitted or received, per unit time."@en ;
    rdfs:subClassOf ns1:Power ;
    skos:prefLabel "RadiantFlux"@en ;
    ns1:elucidation "The radiant energy emitted, reflected, transmitted or received, per unit time."@en ;
    ns1:iupacReference "https://doi.org/10.1351/goldbook.R05046"^^xsd:string ;
    ns1:qudtReference "http://qudt.org/vocab/quantitykind/RadiantFlux"^^xsd:string .

ns1:Radioactivity a owl:Class ;
    rdfs:label "Radioactivity"@en ;
    rdfs:comment "Decays per unit time."@en ;
    rdfs:subClassOf [ a owl:Restriction ;
            owl:onProperty ns1:hasMeasurementUnit ;
            owl:someValuesFrom ns1:FrequencyUnit ],
        ns1:Extensive,
        ns1:ISQDerivedQuantity ;
    skos:altLabel "RadioactiveActivity"@en ;
    skos:prefLabel "Radioactivity"@en ;
    ns1:elucidation "Decays per unit time."@en ;
    ns1:iupacReference "https://doi.org/10.1351/goldbook.A00114"^^xsd:string ;
    ns1:qudtReference "http://qudt.org/vocab/quantitykind/SpecificActivity"^^xsd:string .

ns1:RadiusOfCurvature a owl:Class ;
    rdfs:label "RadiusOfCurvature"@en ;
    rdfs:comment "Radius of the osculating circle of a planar curve at a particular point of the curve."@en ;
    rdfs:subClassOf ns1:Radius ;
    skos:prefLabel "RadiusOfCurvature"@en ;
    ns1:IEVReference "https://www.electropedia.org/iev/iev.nsf/display?openform&ievref=113-01-30"^^xsd:string ;
    ns1:ISO80000Reference "3-1.12"^^xsd:string ;
    ns1:dbpediaReference "https://dbpedia.org/page/Radius_of_curvature"^^xsd:string ;
    ns1:elucidation "Radius of the osculating circle of a planar curve at a particular point of the curve."@en ;
    ns1:wikipediaReference "https://en.wikipedia.org/wiki/Radius_of_curvature"^^xsd:string .

ns1:RatioOfSpecificHeatCapacities a owl:Class ;
    rdfs:label "RatioOfSpecificHeatCapacities"@en ;
    rdfs:comment "Ratio of specific heat capacity at constant pressure cp to specific heat capacity at constant volume cV, thus γ = cp/cV."@en ;
    rdfs:subClassOf ns1:RatioQuantity,
        ns1:ThermodynamicalQuantity ;
    skos:prefLabel "RatioOfSpecificHeatCapacities"@en ;
    ns1:IEVReference "https://www.electropedia.org/iev/iev.nsf/display?openform&ievref=113-04-51"@en ;
    ns1:ISO80000Reference "5-17.1"^^xsd:string ;
    ns1:elucidation "Ratio of specific heat capacity at constant pressure cp to specific heat capacity at constant volume cV, thus γ = cp/cV."@en ;
    ns1:qudtReference "https://qudt.org/vocab/quantitykind/HeatCapacityRatio"^^xsd:string ;
    ns1:wikidataReference "https://www.wikidata.org/wiki/Q503869"^^xsd:string .

ns1:ReactionEnergy a owl:Class ;
    rdfs:label "ReactionEnergy"@en ;
    rdfs:comment "In a nuclear reaction, sum of the kinetic energies and photon energies of the reaction products minus the sum of the kinetic and photon energies of the reactants."@en ;
    rdfs:subClassOf ns1:AtomicAndNuclearPhysicsQuantity,
        ns1:Energy ;
    skos:prefLabel "ReactionEnergy"@en ;
    ns1:ISO80000Reference "10-37.1"^^xsd:string ;
    ns1:elucidation "In a nuclear reaction, sum of the kinetic energies and photon energies of the reaction products minus the sum of the kinetic and photon energies of the reactants."@en ;
    ns1:qudtReference "https://qudt.org/vocab/quantitykind/ReactionEnergy"^^xsd:string ;
    ns1:wikidataReference "https://www.wikidata.org/wiki/Q98164745"^^xsd:string .

ns1:ReactivePower a owl:Class ;
    rdfs:label "ReactivePower"@en ;
    rdfs:comment "Imaginary part of the complex power."@en ;
    rdfs:subClassOf ns1:Power ;
    skos:prefLabel "ReactivePower"@en ;
    ns1:IEVReference "https://www.electropedia.org/iev/iev.nsf/display?openform&ievref=131-11-44"^^xsd:string ;
    ns1:ISO80000Reference "6-60"^^xsd:string ;
    ns1:elucidation "Imaginary part of the complex power."@en ;
    ns1:qudtReference "https://qudt.org/vocab/quantitykind/ReactivePower"^^xsd:string ;
    ns1:wikidataReference "https://www.wikidata.org/wiki/Q2144613"^^xsd:string .

ns1:ReactorTimeConstant a owl:Class ;
    rdfs:label "ReactorTimeConstant"@en ;
    rdfs:comment "Duration required for the neutron fluence rate in a reactor to change by the factor e when the fluence rate is rising or falling exponentially."@en ;
    rdfs:subClassOf ns1:AtomicAndNuclearPhysicsQuantity,
        ns1:Duration ;
    skos:prefLabel "ReactorTimeConstant"@en ;
    ns1:IEVReference "https://www.electropedia.org/iev/iev.nsf/display?openform&ievref=395-07-04"^^xsd:string ;
    ns1:ISO80000Reference "10-79"^^xsd:string ;
    ns1:elucidation "Duration required for the neutron fluence rate in a reactor to change by the factor e when the fluence rate is rising or falling exponentially."@en ;
    ns1:qudtReference "https://qudt.org/vocab/quantitykind/ReactorTimeConstant"^^xsd:string ;
    ns1:wikidataReference "https://www.wikidata.org/wiki/Q99518950"^^xsd:string .

ns1:ReciprocalAmountPerVolumeUnit a owl:Class ;
    rdfs:label "ReciprocalAmountPerVolumeUnit"@en ;
    rdfs:comment "The class of units with dimensionality 'ReciprocalAmountPerVolume'."@en .

ns1:ReciprocalMassUnit a owl:Class ;
    rdfs:label "ReciprocalMassUnit"@en ;
    rdfs:comment "The class of units with dimensionality 'ReciprocalMass'."@en .

ns1:ReciprocalSquareEnergyUnit a owl:Class ;
    rdfs:label "ReciprocalSquareEnergyUnit"@en ;
    rdfs:comment "The class of units with dimensionality 'ReciprocalSquareEnergy'."@en .

ns1:RecombinationCoefficient a owl:Class ;
    rdfs:label "RecombinationCoefficient"@en ;
    rdfs:comment "Coefficient in the law of recombination,"@en ;
    rdfs:subClassOf [ a owl:Restriction ;
            owl:onProperty ns1:hasMeasurementUnit ;
            owl:someValuesFrom ns1:VolumePerTimeUnit ],
        ns1:AtomicAndNuclearPhysicsQuantity,
        ns1:ISQDerivedQuantity ;
    skos:prefLabel "RecombinationCoefficient"@en ;
    ns1:IEVReference "https://www.electropedia.org/iev/iev.nsf/display?openform&ievref=113-06-47"^^xsd:string ;
    ns1:ISO80000Reference "10-63"^^xsd:string ;
    ns1:elucidation "Coefficient in the law of recombination,"@en ;
    ns1:qudtReference "https://qudt.org/vocab/quantitykind/RecombinationCoefficient"^^xsd:string ;
    ns1:wikidataReference "https://www.wikidata.org/wiki/Q98842099"^^xsd:string .

ns1:RefractiveIndex a owl:Class ;
    rdfs:label "RefractiveIndex"@en ;
    rdfs:comment "Factor by which the phase velocity of light is reduced in a medium."@en ;
    rdfs:subClassOf ns1:RatioQuantity ;
    skos:prefLabel "RefractiveIndex"@en ;
    ns1:elucidation "Factor by which the phase velocity of light is reduced in a medium."@en ;
    ns1:iupacReference "https://doi.org/10.1351/goldbook.R05240"^^xsd:string ;
    ns1:qudtReference "http://qudt.org/vocab/quantitykind/RefractiveIndex"^^xsd:string .

ns1:RelativeHumidity a owl:Class ;
    rdfs:label "RelativeHumidity"@en ;
    rdfs:comment "Ratio of the partial pressure p of water vapour in moist air to its partial pressure psat at saturation, at the same temperature φ = p/psat."@en,
        "The relative humidity is often expressed in per cent."@en ;
    rdfs:subClassOf ns1:RatioQuantity,
        ns1:ThermodynamicalQuantity ;
    owl:disjointWith ns1:RelativeMassConcentrationOfWaterVapour ;
    skos:prefLabel "RelativeHumidity"@en ;
    ns1:IEVReference "https://www.electropedia.org/iev/iev.nsf/display?openform&ievref=113-04-65"@en ;
    ns1:ISO80000Reference "5-33"^^xsd:string ;
    ns1:elucidation "Ratio of the partial pressure p of water vapour in moist air to its partial pressure psat at saturation, at the same temperature φ = p/psat."@en ;
    ns1:qudtReference "https://qudt.org/vocab/quantitykind/RelativeHumidity"^^xsd:string ;
    ns1:wikidataReference "https://www.wikidata.org/wiki/Q2499617"^^xsd:string ;
    ns1:wikipediaReference "https://en.wikipedia.org/wiki/Humidity#Relative_humidity"^^xsd:string .

ns1:RelativeLinearStrain a owl:Class ;
    rdfs:label "RelativeLinearStrain"@en ;
    rdfs:comment "Relative change of length with respect the original length."@en ;
    rdfs:subClassOf ns1:ISQDimensionlessQuantity,
        ns1:MechanicalQuantity ;
    skos:prefLabel "RelativeLinearStrain"@en ;
    ns1:IEVReference "https://www.electropedia.org/iev/iev.nsf/display?openform&ievref=113-03-58"^^xsd:string ;
    ns1:ISO80000Reference "4-17.2"^^xsd:string ;
    ns1:elucidation "Relative change of length with respect the original length."@en ;
    ns1:iupacReference "https://doi.org/10.1351/goldbook.L03560"^^xsd:string ;
    ns1:qudtReference "https://qudt.org/vocab/quantitykind/LinearStrain"^^xsd:string ;
    ns1:wikidataReference "https://www.wikidata.org/wiki/Q1990546"^^xsd:string .

ns1:RelativeMassDefect a owl:Class ;
    rdfs:label "RelativeMassDefect"@en ;
    rdfs:comment "Quotient of mass defect and the unified atomic mass constant."@en ;
    rdfs:subClassOf ns1:AtomicAndNuclearPhysicsQuantity,
        ns1:ISQDimensionlessQuantity ;
    skos:prefLabel "RelativeMassDefect"@en ;
    ns1:ISO80000Reference "10-22.2"^^xsd:string ;
    ns1:elucidation "Quotient of mass defect and the unified atomic mass constant."@en ;
    ns1:qudtReference "https://qudt.org/vocab/quantitykind/RelativeMassDefect"^^xsd:string ;
    ns1:wikidataReference "https://www.wikidata.org/wiki/Q98038718"^^xsd:string .

ns1:RelativeMassDensity a owl:Class ;
    rdfs:label "RelativeMassDensity"@en ;
    rdfs:comment "Mass density ρ of a substance divided by the mass density ρ0 of a reference substance, under conditions that should be specified for both substances."@en ;
    rdfs:subClassOf ns1:MechanicalQuantity,
        ns1:RatioQuantity ;
    skos:altLabel "RelativeDensity"@en ;
    skos:prefLabel "RelativeMassDensity"@en ;
    ns1:IEVReference "https://www.electropedia.org/iev/iev.nsf/display?openform&ievref=113-03-08"^^xsd:string ;
    ns1:ISO80000Reference "4-4"@en ;
    ns1:elucidation "Mass density ρ of a substance divided by the mass density ρ0 of a reference substance, under conditions that should be specified for both substances."@en ;
    ns1:iupacReference "https://doi.org/10.1351/goldbook.R05262"^^xsd:string ;
    ns1:wikidataReference "https://www.wikidata.org/wiki/Q11027905"^^xsd:string .

ns1:RelativeMassExcess a owl:Class ;
    rdfs:label "RelativeMassExcess"@en ;
    rdfs:comment "Quotient of mass excess and the unified atomic mass constant."@en ;
    rdfs:subClassOf ns1:AtomicAndNuclearPhysicsQuantity,
        ns1:ISQDimensionlessQuantity ;
    skos:prefLabel "RelativeMassExcess"@en ;
    ns1:ISO80000Reference "10-22.1"^^xsd:string ;
    ns1:elucidation "Quotient of mass excess and the unified atomic mass constant."@en ;
    ns1:qudtReference "https://qudt.org/vocab/quantitykind/RelativeMassExcess"^^xsd:string ;
    ns1:wikidataReference "https://www.wikidata.org/wiki/Q98038610"^^xsd:string .

ns1:RelativeMassFractionOfVapour a owl:Class ;
    rdfs:label "RelativeMassFractionOfVapour"@en ;
    rdfs:comment """Quotient of mass concentration of water vapour and mass concentration at its saturation 

ψ = r/rsat

where r is mass ratio of water vapour to dry gas and rsat is the mass ratio of water vapour to dry gas at saturation of the same temperature."""@en ;
    rdfs:subClassOf ns1:RatioQuantity,
        ns1:ThermodynamicalQuantity ;
    skos:prefLabel "RelativeMassFractionOfVapour"@en ;
    ns1:ISO80000Reference "5-35"^^xsd:string ;
    ns1:elucidation """Quotient of mass concentration of water vapour and mass concentration at its saturation 

ψ = r/rsat

where r is mass ratio of water vapour to dry gas and rsat is the mass ratio of water vapour to dry gas at saturation of the same temperature."""@en .

ns1:RelativePermeability a owl:Class ;
    rdfs:label "RelativePermeability"@en ;
    rdfs:comment "Scalar quantity or tensor quantity equal to the absolute permeability divided by the magnetic constant."@en ;
    rdfs:subClassOf ns1:ElectromagneticQuantity,
        ns1:RatioQuantity ;
    skos:prefLabel "RelativePermeability"@en ;
    ns1:IEVReference "https://www.electropedia.org/iev/iev.nsf/display?openform&ievref=121-12-29"^^xsd:string ;
    ns1:ISO80000Reference "6-27"^^xsd:string ;
    ns1:elucidation "Scalar quantity or tensor quantity equal to the absolute permeability divided by the magnetic constant."@en ;
    ns1:iupacReference "https://doi.org/10.1351/goldbook.R05272"^^xsd:string ;
    ns1:qudtReference "https://qudt.org/vocab/quantitykind/ElectromagneticPermeabilityRatio"^^xsd:string ;
    ns1:wikidataReference "https://www.wikidata.org/wiki/Q77785645"^^xsd:string .

ns1:RelativePermittivity a owl:Class ;
    rdfs:label "RelativePermittivity"@en ;
    rdfs:comment "Permittivity divided by electric constant."@en ;
    rdfs:subClassOf ns1:ElectromagneticQuantity,
        ns1:RatioQuantity ;
    skos:prefLabel "RelativePermittivity"@en ;
    ns1:IEVReference "https://www.electropedia.org/iev/iev.nsf/display?openform&ievref=121-12-13"^^xsd:string ;
    ns1:ISO80000Reference "6-15"^^xsd:string ;
    ns1:elucidation "Permittivity divided by electric constant."@en ;
    ns1:qudtReference "https://qudt.org/vocab/unit/PERMITTIVITY_REL"^^xsd:string ;
    ns1:wikidataReference "https://www.wikidata.org/wiki/Q4027242"^^xsd:string .

ns1:RelativePressureCoefficient a owl:Class ;
    rdfs:label "RelativePressureCoefficient"@en ;
    rdfs:comment "Relative change of pressure with temperature at constant volume."@en ;
    rdfs:subClassOf [ a owl:Restriction ;
            owl:onProperty ns1:hasMeasurementUnit ;
            owl:someValuesFrom ns1:PerTemperatureUnit ],
        ns1:ISQDerivedQuantity,
        ns1:ThermodynamicalQuantity ;
    owl:disjointWith ns1:PressureCoefficient ;
    skos:prefLabel "RelativePressureCoefficient"@en ;
    ns1:IEVReference "https://www.electropedia.org/iev/iev.nsf/display?openform&ievref=113-04-30"^^xsd:string ;
    ns1:ISO80000Reference "5-3.3"^^xsd:string ;
    ns1:elucidation "Relative change of pressure with temperature at constant volume."@en ;
    ns1:qudtReference "https://qudt.org/vocab/quantitykind/RelativePressureCoefficient"^^xsd:string ;
    ns1:wikidataReference "https://www.wikidata.org/wiki/Q74761852"^^xsd:string .

ns1:RelativeVolumeStrain a owl:Class ;
    rdfs:label "RelativeVolumeStrain"@en ;
    rdfs:comment "Quotient of change of volume and original volume."@en ;
    rdfs:subClassOf ns1:MechanicalQuantity,
        ns1:RatioQuantity ;
    skos:altLabel "BulkStrain"@en,
        "VolumeStrain"@en ;
    skos:prefLabel "RelativeVolumeStrain"@en ;
    ns1:IEVReference "https://www.electropedia.org/iev/iev.nsf/display?openform&ievref=113-03-60"^^xsd:string ;
    ns1:ISO80000Reference "4-17.4"^^xsd:string ;
    ns1:elucidation "Quotient of change of volume and original volume."@en ;
    ns1:iupacReference "https://doi.org/10.1351/goldbook.V06648"^^xsd:string ;
    ns1:qudtReference "https://qudt.org/vocab/quantitykind/VolumeStrain"^^xsd:string ;
    ns1:wikidataReference "https://www.wikidata.org/wiki/Q73432507"^^xsd:string .

ns1:RelaxationTime a owl:Class ;
    rdfs:label "RelaxationTime"@en ;
    rdfs:comment "time constant for scattering, trapping or annihilation of charge carriers, phonons or other quasiparticles"@en ;
    rdfs:subClassOf ns1:CondensedMatterPhysicsQuantity,
        ns1:TimeConstant ;
    skos:prefLabel "RelaxationTime"@en ;
    ns1:ISO80000Reference "12-32.1"^^xsd:string ;
    ns1:elucidation "time constant for scattering, trapping or annihilation of charge carriers, phonons or other quasiparticles"@en ;
    ns1:wikidataReference "https://www.wikidata.org/wiki/Q106041085"^^xsd:string .

ns1:ResidualResistivity a owl:Class ;
    rdfs:label "ResidualResistivity"@en ;
    rdfs:comment "For metals, the resistivity extrapolated to zero thermodynamic temperature."@en ;
    rdfs:subClassOf ns1:CondensedMatterPhysicsQuantity,
        ns1:ElectricResistivity ;
    skos:prefLabel "ResidualResistivity"@en ;
    ns1:IEVReference "https://www.electropedia.org/iev/iev.nsf/display?openform&ievref=815-13-61"^^xsd:string ;
    ns1:ISO80000Reference "12-17"^^xsd:string ;
    ns1:elucidation "For metals, the resistivity extrapolated to zero thermodynamic temperature."@en ;
    ns1:qudtReference "https://qudt.org/vocab/quantitykind/ResidualResistivity"^^xsd:string ;
    ns1:wikidataReference "https://www.wikidata.org/wiki/Q25098876"^^xsd:string .

ns1:ResistanceToAlternativeCurrent a owl:Class ;
    rdfs:label "ResistanceToAlternativeCurrent"@en ;
    rdfs:comment "Real part of the impedance."@en ;
    rdfs:subClassOf ns1:ElectricResistance ;
    skos:prefLabel "ResistanceToAlternativeCurrent"@en ;
    ns1:IEVReference "https://www.electropedia.org/iev/iev.nsf/display?openform&ievref=131-12-45"^^xsd:string ;
    ns1:ISO80000Reference "6-51.2"^^xsd:string ;
    ns1:elucidation "Real part of the impedance."@en ;
    ns1:wikidataReference "https://www.wikidata.org/wiki/Q1048490"^^xsd:string .

ns1:ResonanceEnergy a owl:Class ;
    rdfs:label "ResonanceEnergy"@en ;
    rdfs:comment "Resonance in a nuclear reaction, determined by the kinetic energy of an incident particle in the reference frame of the target particle."@en ;
    rdfs:subClassOf ns1:AtomicAndNuclearPhysicsQuantity,
        ns1:Energy ;
    skos:prefLabel "ResonanceEnergy"@en ;
    ns1:ISO80000Reference "10-37.2"^^xsd:string ;
    ns1:elucidation "Resonance in a nuclear reaction, determined by the kinetic energy of an incident particle in the reference frame of the target particle."@en ;
    ns1:qudtReference "https://qudt.org/vocab/quantitykind/ResonanceEnergy"^^xsd:string ;
    ns1:wikidataReference "https://www.wikidata.org/wiki/Q98165187"^^xsd:string .

ns1:ResonanceEscapeProbability a owl:Class ;
    rdfs:label "ResonanceEscapeProbability"@en ;
    rdfs:comment "In an infinite medium, the probability that a neutron slowing down will traverse all or some specified portion of the range of resonance energies without being absorbed."@en ;
    rdfs:subClassOf ns1:AtomicAndNuclearPhysicsQuantity,
        ns1:Probability ;
    skos:prefLabel "ResonanceEscapeProbability"@en ;
    ns1:ISO80000Reference "10-68"^^xsd:string ;
    ns1:elucidation "In an infinite medium, the probability that a neutron slowing down will traverse all or some specified portion of the range of resonance energies without being absorbed."@en ;
    ns1:qudtReference "https://qudt.org/vocab/quantitykind/ResonanceEscapeProbability"^^xsd:string ;
    ns1:wikidataReference "https://www.wikidata.org/wiki/Q4108072"^^xsd:string .

ns1:RestEnergy a owl:Class ;
    rdfs:label "RestEnergy"^^xsd:string ;
    rdfs:comment "Product of the rest mass and the square of the speed of light in vacuum."@en ;
    rdfs:subClassOf ns1:AtomicAndNuclearPhysicsQuantity,
        ns1:Energy ;
    skos:prefLabel "RestEnergy"^^xsd:string ;
    ns1:IEVReference "https://www.electropedia.org/iev/iev.nsf/display?openform&ievref=113-03-05"^^xsd:string,
        "https://www.electropedia.org/iev/iev.nsf/display?openform&ievref=881-04-17"^^xsd:string ;
    ns1:ISO80000Reference "10-3"^^xsd:string ;
    ns1:elucidation "Product of the rest mass and the square of the speed of light in vacuum."@en ;
    ns1:note """E_0 = m_0 * c_0^2

where m_0 is the rest mass of that particle and c_0 is the speed of light in a vacuum."""@en ;
    ns1:wikidataReference "https://www.wikidata.org/wiki/Q11663629"^^xsd:string ;
    ns1:wikipediaReference "https://en.wikipedia.org/wiki/Invariant_mass#Rest_energy"^^xsd:string .

ns1:RichardsonConstant a owl:Class ;
    rdfs:label "RichardsonConstant"@en ;
    rdfs:comment "Parameter in the expression for the thermionic emission current density J for a metal in terms of the thermodynamic temperature T and work function."@en ;
    rdfs:subClassOf [ a owl:Restriction ;
            owl:onProperty ns1:hasMeasurementUnit ;
            owl:someValuesFrom ns1:RichardsonConstantUnit ],
        ns1:CondensedMatterPhysicsQuantity,
        ns1:ISQDerivedQuantity ;
    skos:prefLabel "RichardsonConstant"@en ;
    ns1:IEVReference "https://www.electropedia.org/iev/iev.nsf/display?openform&ievref=113-06-30"^^xsd:string ;
    ns1:ISO80000Reference "12-26"^^xsd:string ;
    ns1:elucidation "Parameter in the expression for the thermionic emission current density J for a metal in terms of the thermodynamic temperature T and work function."@en ;
    ns1:qudtReference "https://qudt.org/vocab/quantitykind/RichardsonConstant"^^xsd:string ;
    ns1:wikidataReference "https://www.wikidata.org/wiki/Q105883079"^^xsd:string .

ns1:RollingResistance a owl:Class ;
    rdfs:label "RollingResistance"@en ;
    rdfs:comment "Force resisting the motion when a body (such as a ball, tire, or wheel) rolls on a surface."@en ;
    rdfs:subClassOf ns1:Force,
        ns1:MechanicalQuantity ;
    owl:disjointWith ns1:RollingResistanceFactor ;
    skos:altLabel "RollingDrag"@en,
        "RollingFrictionForce"@en ;
    skos:prefLabel "RollingResistance"@en ;
    ns1:ISO80000Reference "4-9.5"@en ;
    ns1:elucidation "Force resisting the motion when a body (such as a ball, tire, or wheel) rolls on a surface."@en ;
    ns1:wikidataReference "https://www.wikidata.org/wiki/Q914921"^^xsd:string .

ns1:Rotation a owl:Class ;
    rdfs:label "Rotation"@en ;
    rdfs:comment "Number of turns."@en ;
    rdfs:subClassOf ns1:ISQDimensionlessQuantity,
        ns1:SpaceAndTimeQuantity ;
    skos:prefLabel "Rotation"@en ;
    ns1:IEVReference "https://www.electropedia.org/iev/iev.nsf/display?openform&ievref=102-05-22"^^xsd:string ;
    ns1:ISO80000Reference "3-14"^^xsd:string ;
    ns1:elucidation "Number of turns."@en,
        "Rotation is not necessarily integer."@en ;
    ns1:wikidataReference "https://www.wikidata.org/wiki/Q76435127"^^xsd:string .

ns1:RotationalDisplacement a owl:Class ;
    rdfs:label "RotationalDisplacement"@en ;
    rdfs:comment "Quotient of the traversed circular path length of a point in space during a rotation and its distance from the axis or centre of rotation."@en ;
    rdfs:subClassOf ns1:Angle,
        ns1:SpaceAndTimeQuantity ;
    skos:altLabel "AngularDisplacement"@en ;
    skos:prefLabel "RotationalDisplacement"@en ;
    ns1:ISO80000Reference "3-6"^^xsd:string ;
    ns1:elucidation "Quotient of the traversed circular path length of a point in space during a rotation and its distance from the axis or centre of rotation."@en ;
    ns1:wikidataReference "https://www.wikidata.org/wiki/Q3305038"^^xsd:string ;
    ns1:wikipediaReference "https://en.wikipedia.org/wiki/Angular_displacement"^^xsd:string .

ns1:RotationalFrequency a owl:Class ;
    rdfs:label "RotationalFrequency"@en ;
    rdfs:comment "Magnitude of the angular velocity ω divided by the angle 2π, thus n = |ω|/2π."@en ;
    rdfs:subClassOf ns1:Frequency ;
    skos:prefLabel "RotationalFrequency"@en ;
    ns1:IEVReference "https://www.electropedia.org/iev/iev.nsf/display?openform&ievref=113-01-42"^^xsd:string ;
    ns1:ISO80000Reference "3-17.2"^^xsd:string ;
    ns1:elucidation "Magnitude of the angular velocity ω divided by the angle 2π, thus n = |ω|/2π."@en .

ns1:RybergConstant a owl:Class ;
    rdfs:label "RybergConstant"@en ;
    rdfs:comment "The Rydberg constant represents the limiting value of the highest wavenumber (the inverse wavelength) of any photon that can be emitted from the hydrogen atom, or, alternatively, the wavenumber of the lowest-energy photon capable of ionizing the hydrogen atom from its ground state."@en ;
    rdfs:subClassOf ns1:MeasuredConstant,
        ns1:Wavenumber ;
    skos:prefLabel "RybergConstant"@en ;
    ns1:elucidation "The Rydberg constant represents the limiting value of the highest wavenumber (the inverse wavelength) of any photon that can be emitted from the hydrogen atom, or, alternatively, the wavenumber of the lowest-energy photon capable of ionizing the hydrogen atom from its ground state."@en ;
    ns1:iupacReference "https://doi.org/10.1351/goldbook.R05430"^^xsd:string ;
    ns1:qudtReference "http://qudt.org/vocab/constant/RydbergConstant"^^xsd:string .

ns1:ScalarMagneticPotential a owl:Class ;
    rdfs:label "ScalarMagneticPotential"@en ;
    rdfs:comment "Scalar potential of an irrotational magnetic field strength."@en ;
    rdfs:subClassOf [ a owl:Restriction ;
            owl:onProperty ns1:hasMeasurementUnit ;
            owl:someValuesFrom ns1:ElectricCurrentUnit ],
        ns1:ElectromagneticQuantity,
        ns1:ISQDerivedQuantity ;
    skos:prefLabel "ScalarMagneticPotential"@en ;
    ns1:IEVReference "https://www.electropedia.org/iev/iev.nsf/display?openform&ievref=121-11-58"^^xsd:string ;
    ns1:ISO80000Reference "6-37.1"^^xsd:string ;
    ns1:elucidation "Scalar potential of an irrotational magnetic field strength."@en ;
    ns1:wikidataReference "https://www.wikidata.org/wiki/Q17162107"^^xsd:string .

ns1:SecondPolarMomentOfArea a owl:Class ;
    rdfs:label "SecondPolarMomentOfArea"@en ;
    rdfs:comment "A geometrical property of an area which reflects how its points are distributed with regard to an arbitrary axis."@en ;
    rdfs:subClassOf [ a owl:Restriction ;
            owl:onProperty ns1:hasMeasurementUnit ;
            owl:someValuesFrom ns1:QuarticLengthUnit ],
        ns1:ISQDerivedQuantity,
        ns1:MechanicalQuantity ;
    owl:disjointWith ns1:SecondAxialMomentOfArea ;
    skos:prefLabel "SecondPolarMomentOfArea"@en ;
    ns1:IEVReference "https://www.electropedia.org/iev/iev.nsf/display?openform&ievref=113-03-30"^^xsd:string ;
    ns1:ISO80000Reference "4-21.2"^^xsd:string ;
    ns1:elucidation "A geometrical property of an area which reflects how its points are distributed with regard to an arbitrary axis."@en ;
    ns1:qudtReference "https://qudt.org/vocab/quantitykind/SecondPolarMomentOfArea"^^xsd:string ;
    ns1:wikidataReference "https://www.wikidata.org/wiki/Q1049636"^^xsd:string .

ns1:SectionModulus a owl:Class ;
    rdfs:label "SectionModulus"@en ;
    rdfs:comment "Geometrical characteristic of a shape of a body."@en ;
    rdfs:subClassOf [ a owl:Restriction ;
            owl:onProperty ns1:hasMeasurementUnit ;
            owl:someValuesFrom ns1:VolumeUnit ],
        ns1:ISQDerivedQuantity,
        ns1:MechanicalQuantity ;
    skos:prefLabel "SectionModulus"@en ;
    ns1:IEVReference "https://www.electropedia.org/iev/iev.nsf/display?openform&ievref=113-03-31"^^xsd:string ;
    ns1:ISO80000Reference "4-22"^^xsd:string ;
    ns1:elucidation "Geometrical characteristic of a shape of a body."@en ;
    ns1:qudtReference "https://qudt.org/vocab/quantitykind/SectionModulus"^^xsd:string ;
    ns1:wikidataReference "https://www.wikidata.org/wiki/Q1930808"^^xsd:string .

ns1:SeebeckCoefficient a owl:Class ;
    rdfs:label "SeebeckCoefficient"@en ;
    rdfs:comment "Measure of voltage induced by change of temperature."@en ;
    rdfs:subClassOf [ a owl:Restriction ;
            owl:onProperty ns1:hasMeasurementUnit ;
            owl:someValuesFrom ns1:ElectricPotentialPerTemperatureUnit ],
        ns1:CondensedMatterPhysicsQuantity,
        ns1:ISQDerivedQuantity ;
    skos:prefLabel "SeebeckCoefficient"@en ;
    ns1:ISO80000Reference "12-21"^^xsd:string ;
    ns1:elucidation "Measure of voltage induced by change of temperature."@en ;
    ns1:qudtReference "https://qudt.org/vocab/quantitykind/SeebeckCoefficient"^^xsd:string ;
    ns1:wikidataReference "https://www.wikidata.org/wiki/Q1091448"^^xsd:string .

ns1:SexticLengthUnit a owl:Class ;
    rdfs:label "SexticLengthUnit"@en ;
    rdfs:comment "The class of units with dimensionality 'SexticLength'."@en .

ns1:ShearStrain a owl:Class ;
    rdfs:label "ShearStrain"@en ;
    rdfs:comment "Displacement of one surface with respect to another divided by the distance between them."@en ;
    rdfs:subClassOf ns1:ISQDimensionlessQuantity,
        ns1:MechanicalQuantity ;
    skos:prefLabel "ShearStrain"@en ;
    ns1:IEVReference "https://www.electropedia.org/iev/iev.nsf/display?openform&ievref=113-03-59"^^xsd:string ;
    ns1:ISO80000Reference "4-17.3"^^xsd:string ;
    ns1:elucidation "Displacement of one surface with respect to another divided by the distance between them."@en ;
    ns1:iupacReference "https://doi.org/10.1351/goldbook.S05637"^^xsd:string ;
    ns1:qudtReference "https://qudt.org/vocab/quantitykind/ShearStrain"^^xsd:string ;
    ns1:wikidataReference "https://www.wikidata.org/wiki/Q7561704"^^xsd:string .

ns1:ShortRangeOrderParameter a owl:Class ;
    rdfs:label "ShortRangeOrderParameter"@en ;
    rdfs:comment "fraction of nearest-neighbour atom pairs in an Ising ferromagnet having magnetic moments in one direction, minus the fraction having magnetic moments in the opposite direction"@en ;
    rdfs:subClassOf ns1:CondensedMatterPhysicsQuantity,
        ns1:ISQDimensionlessQuantity ;
    skos:prefLabel "ShortRangeOrderParameter"@en ;
    ns1:ISO80000Reference "12-5.1"^^xsd:string ;
    ns1:elucidation "fraction of nearest-neighbour atom pairs in an Ising ferromagnet having magnetic moments in one direction, minus the fraction having magnetic moments in the opposite direction"@en ;
    ns1:qudtReference "https://qudt.org/vocab/quantitykind/Short-RangeOrderParameter"^^xsd:string ;
    ns1:wikidataReference "https://www.wikidata.org/wiki/Q105495979"^^xsd:string .

ns1:SlowingDownArea a owl:Class ;
    rdfs:label "SlowingDownArea"@en ;
    rdfs:comment "In an infinite homogenous medium, one-sixth of the mean square of the distance between the neutron source and the point where a neutron reaches a given energy."@en ;
    rdfs:subClassOf ns1:Area,
        ns1:AtomicAndNuclearPhysicsQuantity ;
    skos:prefLabel "SlowingDownArea"@en ;
    ns1:ISO80000Reference "10-72.1"^^xsd:string ;
    ns1:elucidation "In an infinite homogenous medium, one-sixth of the mean square of the distance between the neutron source and the point where a neutron reaches a given energy."@en ;
    ns1:qudtReference "https://qudt.org/vocab/quantitykind/Slowing-DownArea"^^xsd:string ;
    ns1:wikidataReference "https://www.wikidata.org/wiki/Q98950918"^^xsd:string .

ns1:SlowingDownDensity a owl:Class ;
    rdfs:label "SlowingDownDensity"@en ;
    rdfs:comment "Number of slowed-down particles per time and volume."@en ;
    rdfs:subClassOf [ a owl:Restriction ;
            owl:onProperty ns1:hasMeasurementUnit ;
            owl:someValuesFrom ns1:FrequencyPerVolumeUnit ],
        ns1:AtomicAndNuclearPhysicsQuantity,
        ns1:ISQDerivedQuantity ;
    skos:prefLabel "SlowingDownDensity"@en ;
    ns1:ISO80000Reference "10-67"^^xsd:string ;
    ns1:elucidation "Number of slowed-down particles per time and volume."@en ;
    ns1:qudtReference "https://qudt.org/vocab/quantitykind/Slowing-DownDensity"^^xsd:string ;
    ns1:wikidataReference "https://www.wikidata.org/wiki/Q98915830"^^xsd:string .

ns1:SlowingDownLength a owl:Class ;
    rdfs:label "SlowingDownLength"@en ;
    rdfs:comment "Square root of the slowing down area."@en ;
    rdfs:subClassOf ns1:AtomicAndNuclearPhysicsQuantity,
        ns1:Length ;
    skos:prefLabel "SlowingDownLength"@en ;
    ns1:ISO80000Reference "10-73.1"^^xsd:string ;
    ns1:elucidation "Square root of the slowing down area."@en ;
    ns1:qudtReference "https://qudt.org/vocab/quantitykind/Slowing-DownLength"^^xsd:string ;
    ns1:wikidataReference "https://www.wikidata.org/wiki/Q98996963"^^xsd:string .

ns1:SolidAngle a owl:Class ;
    rdfs:label "SolidAngle"@en ;
    rdfs:comment "Ratio of area on a sphere to its radius squared."@en ;
    rdfs:subClassOf ns1:RatioQuantity ;
    skos:prefLabel "SolidAngle"@en ;
    ns1:ISO80000Reference "3-6"^^xsd:string ;
    ns1:elucidation "Ratio of area on a sphere to its radius squared."@en ;
    ns1:iupacReference "https://doi.org/10.1351/goldbook.S05732"^^xsd:string ;
    ns1:qudtReference "http://qudt.org/vocab/quantitykind/SolidAngle"^^xsd:string .

ns1:SolidAngularMeasure a owl:Class ;
    rdfs:label "SolidAngularMeasure"@en ;
    rdfs:comment "Measure of a conical geometric figure, called solid angle, formed by all rays, originating from a common point, called the vertex of the solid angle, and passing through the points of a closed, non-self-intersecting curve in space considered as the border of a surface."@en ;
    rdfs:subClassOf ns1:Angle,
        ns1:SpaceAndTimeQuantity ;
    skos:altLabel "SolidAngle"@en ;
    skos:prefLabel "SolidAngularMeasure"@en ;
    ns1:IEVReference "https://www.electropedia.org/iev/iev.nsf/display?openform&ievref=102-04-46"^^xsd:string ;
    ns1:ISO80000Reference "3-8"^^xsd:string ;
    ns1:dbpediaReference "https://dbpedia.org/page/Solid_angle"^^xsd:string ;
    ns1:elucidation "Measure of a conical geometric figure, called solid angle, formed by all rays, originating from a common point, called the vertex of the solid angle, and passing through the points of a closed, non-self-intersecting curve in space considered as the border of a surface."@en ;
    ns1:qudtReference "https://qudt.org/vocab/quantitykind/SolidAngle"^^xsd:string ;
    ns1:wikidataReference "https://www.wikidata.org/wiki/Q208476"^^xsd:string ;
    ns1:wikipediaReference "https://en.wikipedia.org/wiki/Solid_angle"^^xsd:string .

ns1:Solubility a owl:Class ;
    rdfs:label "Solubility"@en ;
    rdfs:comment "The analytical composition of a saturated solution, expressed in terms of the proportion of a designated solute in a designated solvent, is the solubility of that solute."@en,
        "The solubility may be expressed as a concentration, molality, mole fraction, mole ratio, etc."@en ;
    rdfs:subClassOf ns1:ThermodynamicalQuantity ;
    skos:prefLabel "Solubility"@en ;
    ns1:IEVReference "https://www.electropedia.org/iev/iev.nsf/display?openform&ievref=114-01-15"^^xsd:string ;
    ns1:elucidation "The analytical composition of a saturated solution, expressed in terms of the proportion of a designated solute in a designated solvent, is the solubility of that solute."@en ;
    ns1:iupacReference "https://doi.org/10.1351/goldbook.S05740"^^xsd:string ;
    ns1:wikidataReference "https://www.wikidata.org/wiki/Q170731"^^xsd:string .

ns1:SolubilityProduct a owl:Class ;
    rdfs:label "SolubilityProduct"@en ;
    rdfs:comment "For the dissociation of a salt AmBn → mA + nB, the solubility product is KSP = am(A) ⋅ an(B), where a is ionic activity and m and n are the stoichiometric numbers."@en,
        "Product of the ion activities of the ions resulting from the dissociation of a solute in a saturated solution, raised to powers equal to their stoichiometric numbers."@en ;
    rdfs:subClassOf [ a owl:Restriction ;
            owl:onProperty ns1:hasMeasurementUnit ;
            owl:someValuesFrom ns1:DimensionlessUnit ],
        ns1:EquilibriumConstant ;
    skos:altLabel "SolubilityProductConstant"@en ;
    skos:prefLabel "SolubilityProduct"@en ;
    ns1:IEVReference "https://www.electropedia.org/iev/iev.nsf/display?openform&ievref=114-01-23"^^xsd:string ;
    ns1:elucidation "Product of the ion activities of the ions resulting from the dissociation of a solute in a saturated solution, raised to powers equal to their stoichiometric numbers."@en ;
    ns1:iupacReference "https://doi.org/10.1351/goldbook.S05742"^^xsd:string ;
    ns1:wikidataReference "https://www.wikidata.org/wiki/Q11229788"^^xsd:string .

ns1:SourceVoltage a owl:Class ;
    rdfs:label "SourceVoltage"@en ;
    rdfs:comment "Voltage between the two terminals of a voltage source when there is no electric current through the source."@en ;
    rdfs:subClassOf ns1:Voltage ;
    skos:altLabel "SourceTension"@en ;
    skos:prefLabel "SourceVoltage"@en ;
    ns1:ISO80000Reference "6-36"^^xsd:string ;
    ns1:elucidation "Voltage between the two terminals of a voltage source when there is no electric current through the source."@en ;
    ns1:qudtReference "https://qudt.org/vocab/quantitykind/SourceVoltage"^^xsd:string ;
    ns1:wikidataReference "https://www.wikidata.org/wiki/Q185329"^^xsd:string .

ns1:SpecificActivity a owl:Class ;
    rdfs:label "SpecificActivity"@en ;
    rdfs:comment "Quotient of the activity A of a sample and the mass m of that sample."@en ;
    rdfs:subClassOf [ a owl:Restriction ;
            owl:onProperty ns1:hasMeasurementUnit ;
            owl:someValuesFrom ns1:PerTimeMassUnit ],
        ns1:AtomicAndNuclearPhysicsQuantity,
        ns1:ISQDerivedQuantity ;
    skos:altLabel "MassicActivity"@en ;
    skos:prefLabel "SpecificActivity"@en ;
    ns1:IEVReference "https://www.electropedia.org/iev/iev.nsf/display?openform&ievref=395-01-08"^^xsd:string,
        "https://www.electropedia.org/iev/iev.nsf/display?openform&ievref=881-04-43"^^xsd:string ;
    ns1:ISO80000Reference "10-28"^^xsd:string ;
    ns1:elucidation "Quotient of the activity A of a sample and the mass m of that sample."@en ;
    ns1:iupacReference "https://doi.org/10.1351/goldbook.S05790"^^xsd:string ;
    ns1:qudtReference "https://qudt.org/vocab/quantitykind/SpecificActivity"^^xsd:string ;
    ns1:wikidataReference "https://www.wikidata.org/wiki/Q2823748"^^xsd:string .

ns1:SpecificEnthalpy a owl:Class ;
    rdfs:label "SpecificEnthalpy"@en ;
    rdfs:comment "Enthalpy per unit mass."@en ;
    rdfs:subClassOf ns1:SpecificEnergy ;
    skos:prefLabel "SpecificEnthalpy"@en ;
    ns1:ISO80000Reference "5-21.3"^^xsd:string ;
    ns1:elucidation "Enthalpy per unit mass."@en ;
    ns1:qudtReference "https://qudt.org/vocab/quantitykind/SpecificEnthalpy"^^xsd:string ;
    ns1:wikidataReference "https://www.wikidata.org/wiki/Q21572993"^^xsd:string ;
    ns1:wikipediaReference "https://en.wikipedia.org/wiki/Enthalpy#Specific_enthalpy"^^xsd:string .

ns1:SpecificEntropy a owl:Class ;
    rdfs:label "SpecificEntropy"@en ;
    rdfs:comment "Quotient of entropy and mass."@en ;
    rdfs:subClassOf [ a owl:Restriction ;
            owl:onProperty ns1:hasMeasurementUnit ;
            owl:someValuesFrom ns1:EntropyPerMassUnit ],
        ns1:ISQDerivedQuantity,
        ns1:ThermodynamicalQuantity ;
    skos:prefLabel "SpecificEntropy"@en ;
    ns1:ISO80000Reference "5-19"^^xsd:string ;
    ns1:elucidation "Quotient of entropy and mass."@en ;
    ns1:qudtReference "https://qudt.org/vocab/quantitykind/SpecificEntropy"^^xsd:string ;
    ns1:wikidataReference "https://www.wikidata.org/wiki/Q69423705"^^xsd:string .

ns1:SpecificGibbsEnergy a owl:Class ;
    rdfs:label "SpecificGibbsEnergy"@en ;
    rdfs:comment "Gibbs energy per unit mass."@en ;
    rdfs:subClassOf ns1:SpecificEnergy ;
    skos:prefLabel "SpecificGibbsEnergy"@en ;
    ns1:ISO80000Reference "5-21.5"^^xsd:string ;
    ns1:elucidation "Gibbs energy per unit mass."@en ;
    ns1:qudtReference "https://qudt.org/vocab/quantitykind/SpecificGibbsEnergy"^^xsd:string ;
    ns1:wikidataReference "https://www.wikidata.org/wiki/Q76360636"^^xsd:string .

ns1:SpecificHeatCapacityAtSaturatedVaporPressure a owl:Class ;
    rdfs:label "SpecificHeatCapacityAtSaturatedVaporPressure"@en ;
    rdfs:comment "Specific heat capacity at saturated vaport pressure."@en ;
    rdfs:subClassOf ns1:SpecificHeatCapacity ;
    skos:prefLabel "SpecificHeatCapacityAtSaturatedVaporPressure"@en ;
    ns1:ISO80000Reference "5-16.4"^^xsd:string ;
    ns1:elucidation "Specific heat capacity at saturated vaport pressure."@en ;
    ns1:qudtReference "https://qudt.org/vocab/quantitykind/SpecificHeatCapacityAtSaturation"^^xsd:string ;
    ns1:wikidataReference "https://www.wikidata.org/wiki/Q75775005"^^xsd:string .

ns1:SpecificHelmholtzEnergy a owl:Class ;
    rdfs:label "SpecificHelmholtzEnergy"@en ;
    rdfs:comment "Helmholtz energy per unit mass."@en ;
    rdfs:subClassOf ns1:SpecificEnergy ;
    skos:prefLabel "SpecificHelmholtzEnergy"@en ;
    ns1:ISO80000Reference "5-21.4"^^xsd:string ;
    ns1:elucidation "Helmholtz energy per unit mass."@en ;
    ns1:qudtReference "https://qudt.org/vocab/quantitykind/SpecificHelmholtzEnergy"^^xsd:string ;
    ns1:wikidataReference "https://www.wikidata.org/wiki/Q76359554"^^xsd:string .

ns1:SpecificInternalEnergy a owl:Class ;
    rdfs:label "SpecificInternalEnergy"@en ;
    rdfs:comment "Internal energy per unit mass."@en ;
    rdfs:subClassOf ns1:SpecificEnergy ;
    skos:prefLabel "SpecificInternalEnergy"@en ;
    ns1:ISO80000Reference "5-21.2"^^xsd:string ;
    ns1:elucidation "Internal energy per unit mass."@en ;
    ns1:qudtReference "https://qudt.org/vocab/quantitykind/SpecificInternalEnergy"^^xsd:string ;
    ns1:wikidataReference "https://www.wikidata.org/wiki/Q76357367"^^xsd:string .

ns1:SpecificVolume a owl:Class ;
    rdfs:label "SpecificVolume"@en ;
    rdfs:comment "inverse of the mass density ρ, thus v = 1/ρ."@en ;
    rdfs:subClassOf [ a owl:Restriction ;
            owl:onProperty ns1:hasMeasurementUnit ;
            owl:someValuesFrom ns1:VolumePerMassUnit ],
        ns1:ISQDerivedQuantity,
        ns1:MechanicalQuantity ;
    skos:altLabel "MassicVolume"@en ;
    skos:prefLabel "SpecificVolume"@en ;
    ns1:IEVReference "https://www.electropedia.org/iev/iev.nsf/display?openform&ievref=113-03-09"^^xsd:string ;
    ns1:ISO80000Reference "4-3"^^xsd:string ;
    ns1:elucidation "inverse of the mass density ρ, thus v = 1/ρ."@en ;
    ns1:iupacReference "https://doi.org/10.1351/goldbook.S05807"^^xsd:string ;
    ns1:qudtReference "https://qudt.org/vocab/quantitykind/SpecificVolume"^^xsd:string ;
    ns1:wikidataReference "https://www.wikidata.org/wiki/Q683556"^^xsd:string .

ns1:SpeedOfLightInVacuum a owl:Class ;
    rdfs:label "SpeedOfLightInVacuum"@en ;
    rdfs:comment "The speed of light in vacuum. Defines the base unit metre in the SI system."@en ;
    rdfs:subClassOf ns1:SIExactConstant,
        ns1:Speed ;
    skos:prefLabel "SpeedOfLightInVacuum"@en ;
    ns1:ISO80000Reference "6-35.2"^^xsd:string ;
    ns1:elucidation "The speed of light in vacuum. Defines the base unit metre in the SI system."@en ;
    ns1:iupacReference "https://doi.org/10.1351/goldbook.S05854"^^xsd:string ;
    ns1:qudtReference "http://qudt.org/vocab/constant/SpeedOfLight_Vacuum"^^xsd:string .

ns1:Spin a owl:Class ;
    rdfs:label "Spin"^^xsd:string ;
    rdfs:comment "Vector quantity expressing the internal angular momentum of a particle or a particle system."@en ;
    rdfs:subClassOf ns1:AngularMomentum,
        ns1:AtomicAndNuclearPhysicsQuantity ;
    skos:prefLabel "Spin"^^xsd:string ;
    ns1:IEVReference "https://www.electropedia.org/iev/iev.nsf/display?openform&ievref=113-05-09"^^xsd:string ;
    ns1:ISO80000Reference "10-10"^^xsd:string ;
    ns1:elucidation "Vector quantity expressing the internal angular momentum of a particle or a particle system."@en ;
    ns1:qudtReference "https://qudt.org/vocab/quantitykind/Spin"^^xsd:string ;
    ns1:wikidataReference "https://www.wikidata.org/wiki/Q133673"^^xsd:string .

ns1:SpinQuantumNumber a owl:Class ;
    rdfs:label "SpinQuantumNumber"^^xsd:string ;
    rdfs:comment "Characteristic quantum number s of a particle, related to its spin."@en ;
    rdfs:subClassOf ns1:QuantumNumber ;
    skos:prefLabel "SpinQuantumNumber"^^xsd:string ;
    ns1:ISO80000Reference "10-13.5"^^xsd:string ;
    ns1:elucidation "Characteristic quantum number s of a particle, related to its spin."@en ;
    ns1:qudtReference "https://qudt.org/vocab/quantitykind/SpinQuantumNumber"^^xsd:string ;
    ns1:wikidataReference "https://www.wikidata.org/wiki/Q3879445"^^xsd:string .

ns1:SquareCurrentQuarticTimePerMassUnit a owl:Class ;
    rdfs:label "SquareCurrentQuarticTimePerMassUnit"@en ;
    rdfs:comment "The class of units with dimensionality 'SquareCurrentQuarticTimePerMass'."@en .

ns1:SquareElectricPotentialPerSquareTemperatureUnit a owl:Class ;
    rdfs:label "SquareElectricPotentialPerSquareTemperatureUnit"@en ;
    rdfs:comment "The class of units with dimensionality 'SquareElectricPotentialPerSquareTemperature'."@en .

ns1:SquareMassPerSquareTimeUnit a owl:Class ;
    rdfs:label "SquareMassPerSquareTimeUnit"@en ;
    rdfs:comment "The class of units with dimensionality 'SquareMassPerSquareTime'."@en .

ns1:SquarePressurePerSquareTimeUnit a owl:Class ;
    rdfs:label "SquarePressurePerSquareTimeUnit"@en ;
    rdfs:comment "The class of units with dimensionality 'SquarePressurePerSquareTime'."@en .

ns1:SquarePressureTimeUnit a owl:Class ;
    rdfs:label "SquarePressureTimeUnit"@en ;
    rdfs:comment "The class of units with dimensionality 'SquarePressureTime'."@en .

ns1:SquareTemperaturePerTimeUnit a owl:Class ;
    rdfs:label "SquareTemperaturePerTimeUnit"@en ;
    rdfs:comment "The class of units with dimensionality 'SquareTemperaturePerTime'."@en .

ns1:SquareTemperatureUnit a owl:Class ;
    rdfs:label "SquareTemperatureUnit"@en ;
    rdfs:comment "The class of units with dimensionality 'SquareTemperature'."@en .

ns1:SquareTimeUnit a owl:Class ;
    rdfs:label "SquareTimeUnit"@en ;
    rdfs:comment "The class of units with dimensionality 'SquareTime'."@en .

ns1:StandardAbsoluteActivityOfMixture a owl:Class ;
    rdfs:label "StandardAbsoluteActivityOfMixture"@en ;
    rdfs:comment "For a substance in a mixture, the absolute activity of the pure substance at the same temperature but at standard pressure."@en ;
    rdfs:subClassOf ns1:AbsoluteActivity,
        ns1:PhysioChemicalQuantity ;
    skos:altLabel "StandardAbsoluteActivity"@en ;
    skos:prefLabel "StandardAbsoluteActivityOfMixture"@en ;
    ns1:ISO80000Reference "9-23"^^xsd:string ;
    ns1:elucidation "For a substance in a mixture, the absolute activity of the pure substance at the same temperature but at standard pressure."@en ;
    ns1:qudtReference "https://qudt.org/vocab/quantitykind/StandardAbsoluteActivity"^^xsd:string ;
    ns1:wikidataReference "https://www.wikidata.org/wiki/Q89406159"^^xsd:string .

ns1:StandardAbsoluteActivityOfSolution a owl:Class ;
    rdfs:label "StandardAbsoluteActivityOfSolution"@en ;
    rdfs:comment "Property of a solute in a solution."@en ;
    rdfs:subClassOf ns1:AbsoluteActivity,
        ns1:PhysioChemicalQuantity ;
    skos:altLabel "StandardAbsoluteActivity"@en ;
    skos:prefLabel "StandardAbsoluteActivityOfSolution"@en ;
    ns1:ISO80000Reference "9-26"^^xsd:string ;
    ns1:elucidation "Property of a solute in a solution."@en ;
    ns1:wikidataReference "https://www.wikidata.org/wiki/Q89485936"^^xsd:string .

ns1:StandardAbsoluteActivityOfSolvent a owl:Class ;
    rdfs:label "StandardAbsoluteActivityOfSolvent"@en ;
    rdfs:comment "For solvent A, standard absolute activity of the pure substance A at the same temperature and at a standard pressure."@en ;
    rdfs:subClassOf ns1:AbsoluteActivity,
        ns1:PhysioChemicalQuantity ;
    skos:prefLabel "StandardAbsoluteActivityOfSolvent"@en ;
    ns1:ISO80000Reference "9-27.3"^^xsd:string ;
    ns1:elucidation "For solvent A, standard absolute activity of the pure substance A at the same temperature and at a standard pressure."@en ;
    ns1:wikidataReference "https://www.wikidata.org/wiki/Q89556185"^^xsd:string .

ns1:StandardAmountConcentration a owl:Class ;
    rdfs:label "StandardAmountConcentration"@en ;
    rdfs:comment "Chosen value of amount concentration, usually equal to 1 mol dm−3."@en ;
    rdfs:subClassOf ns1:AmountConcentration,
        ns1:PhysioChemicalQuantity ;
    skos:altLabel "StandardConcentration"@en,
        "StandardMolarConcentration"@en ;
    skos:prefLabel "StandardAmountConcentration"@en ;
    ns1:ISO80000Reference "9-12.2"^^xsd:string ;
    ns1:elucidation "Chosen value of amount concentration, usually equal to 1 mol dm−3."@en ;
    ns1:iupacReference "https://doi.org/10.1351/goldbook.S05909"^^xsd:string ;
    ns1:wikidataReference "https://www.wikidata.org/wiki/Q88871689"^^xsd:string .

ns1:StandardChemicalPotential a owl:Class ;
    rdfs:label "StandardChemicalPotential"@en ;
    rdfs:comment "The value of the chemical potential under specified standard conditions (in the standard state)."@en ;
    rdfs:subClassOf ns1:MolarEnergy,
        ns1:PhysioChemicalQuantity ;
    skos:prefLabel "StandardChemicalPotential"@en ;
    ns1:ISO80000Reference "9-21"^^xsd:string ;
    ns1:elucidation "The value of the chemical potential under specified standard conditions (in the standard state)."@en ;
    ns1:iupacReference "https://doi.org/10.1351/goldbook.S05908"^^xsd:string ;
    ns1:qudtReference "https://qudt.org/vocab/quantitykind/StandardChemicalPotential"^^xsd:string ;
    ns1:wikidataReference "https://www.wikidata.org/wiki/Q89333468"^^xsd:string .

ns1:StandardEquilibriumConstant a owl:Class ;
    rdfs:label "StandardEquilibriumConstant"@en ;
    rdfs:comment "Constant of a chemical reaction. It is the value of its reaction quotient at chemical equilibrium, a state approached by a dynamic chemical system after sufficient time has elapsed at which its composition has no measurable tendency towards further change."@en ;
    rdfs:subClassOf ns1:EquilibriumConstant,
        ns1:PhysioChemicalQuantity ;
    skos:altLabel "ThermodynamicEquilibriumConstant"^^xsd:string ;
    skos:prefLabel "StandardEquilibriumConstant"@en ;
    ns1:ISO80000Reference "9-32"^^xsd:string ;
    ns1:elucidation "Constant of a chemical reaction. It is the value of its reaction quotient at chemical equilibrium, a state approached by a dynamic chemical system after sufficient time has elapsed at which its composition has no measurable tendency towards further change."@en ;
    ns1:iupacReference "https://doi.org/10.1351/goldbook.S05915"^^xsd:string ;
    ns1:wikidataReference "https://www.wikidata.org/wiki/Q95993378"^^xsd:string .

ns1:StaticFrictionCoefficient a owl:Class ;
    rdfs:label "StaticFrictionCoefficient"@en ;
    rdfs:subClassOf ns1:CoefficientOfFriction,
        ns1:MechanicalQuantity ;
    skos:altLabel "CoefficientOfStaticFriction"@en,
        "StaticFrictionFactor"@en ;
    skos:prefLabel "StaticFrictionCoefficient"@en ;
    ns1:IEVReference "https://www.electropedia.org/iev/iev.nsf/display?openform&ievref=113-03-33"^^xsd:string ;
    ns1:ISO80000Reference "4-23.1"^^xsd:string ;
    ns1:wikidataReference "https://www.wikidata.org/wiki/Q73695673"^^xsd:string .

ns1:StaticFrictionForce a owl:Class ;
    rdfs:label "StaticFrictionForce"@en ;
    rdfs:comment "Fhe force of friction on an object that is not moving."@en ;
    rdfs:subClassOf ns1:Force,
        ns1:MechanicalQuantity ;
    skos:altLabel "StaticFriction"@en ;
    skos:prefLabel "StaticFrictionForce"@en ;
    ns1:ISO80000Reference "4-9.3"^^xsd:string ;
    ns1:elucidation "Fhe force of friction on an object that is not moving."@en ;
    ns1:qudtReference "https://qudt.org/vocab/quantitykind/StaticFriction"^^xsd:string ;
    ns1:wikidataReference "https://www.wikidata.org/wiki/Q90862568"^^xsd:string .

ns1:StatisticalWeightOfSubsystem a owl:Class ;
    rdfs:label "StatisticalWeightOfSubsystem"@en ;
    rdfs:comment "Number of different microstates in a subsystem."@en ;
    rdfs:subClassOf ns1:ISQDimensionlessQuantity,
        ns1:PhysioChemicalQuantity ;
    skos:prefLabel "StatisticalWeightOfSubsystem"@en ;
    ns1:ISO80000Reference "9-36.1"^^xsd:string ;
    ns1:elucidation "Number of different microstates in a subsystem."@en ;
    ns1:wikidataReference "https://www.wikidata.org/wiki/Q96207431"^^xsd:string .

ns1:StoichiometricNumberOfSubstance a owl:Class ;
    rdfs:label "StoichiometricNumberOfSubstance"@en ;
    rdfs:comment "For substance B, an integer number or a simple fraction, being negative for a reactant and positive for a product, occurring in the expression for a chemical reaction."@en ;
    rdfs:subClassOf ns1:PhysioChemicalQuantity,
        ns1:PureNumberQuantity ;
    skos:example """The factors 1/2 and 3/2 in the chemical reaction formula below are stoicheiometric mumbers of substance.

    (1/2)N2 + (3/2)H2 = NH3"""@en ;
    skos:prefLabel "StoichiometricNumberOfSubstance"@en ;
    ns1:IEVReference "https://www.electropedia.org/iev/iev.nsf/display?openform&ievref=114-01-22"^^xsd:string ;
    ns1:ISO80000Reference "9-29"^^xsd:string ;
    ns1:elucidation "For substance B, an integer number or a simple fraction, being negative for a reactant and positive for a product, occurring in the expression for a chemical reaction."@en ;
    ns1:iupacReference "https://doi.org/10.1351/goldbook.S06025"^^xsd:string ;
    ns1:qudtReference "https://qudt.org/vocab/quantitykind/StoichiometricNumber"^^xsd:string ;
    ns1:wikidataReference "https://www.wikidata.org/wiki/Q95443720"^^xsd:string .

ns1:Strain a owl:Class ;
    rdfs:label "Strain"@en ;
    rdfs:comment "Change of the relative positions of parts of a body, excluding a displacement of the body as a whole."@en ;
    rdfs:subClassOf ns1:RatioQuantity ;
    skos:prefLabel "Strain"@en ;
    ns1:ISO80000Reference "4-17.1"^^xsd:string ;
    ns1:elucidation "Change of the relative positions of parts of a body, excluding a displacement of the body as a whole."@en ;
    ns1:qudtReference "http://qudt.org/vocab/quantitykind/Strain"^^xsd:string .

ns1:Stress a owl:Class ;
    rdfs:label "Stress"@en ;
    rdfs:comment "Force per unit oriented surface area ."@en,
        "Measure of the internal forces that neighboring particles of a continuous material exert on each other."@en ;
    rdfs:subClassOf [ a owl:Restriction ;
            owl:onProperty ns1:hasMeasurementUnit ;
            owl:someValuesFrom ns1:PressureUnit ],
        ns1:ISQDerivedQuantity ;
    skos:prefLabel "Stress"@en ;
    ns1:ISO80000Reference "4-15"^^xsd:string ;
    ns1:elucidation "Measure of the internal forces that neighboring particles of a continuous material exert on each other."@en ;
    ns1:qudtReference "http://qudt.org/vocab/quantitykind/Stress"^^xsd:string .

ns1:StructureFactor a owl:Class ;
    rdfs:label "StructureFactor"@en ;
    rdfs:comment "Mathematical description in crystallography."@en ;
    rdfs:subClassOf [ a owl:Restriction ;
            owl:onProperty ns1:hasMeasurementUnit ;
            owl:someValuesFrom ns1:DimensionlessUnit ],
        ns1:CondensedMatterPhysicsQuantity ;
    skos:prefLabel "StructureFactor"@en ;
    ns1:ISO80000Reference "12-5.4"^^xsd:string ;
    ns1:elucidation "Mathematical description in crystallography."@en ;
    ns1:qudtReference "https://qudt.org/vocab/quantitykind/StructureFactor"^^xsd:string ;
    ns1:wikidataReference "https://www.wikidata.org/wiki/Q900684"^^xsd:string .

ns1:SuperconductionTransitionTemperature a owl:Class ;
    rdfs:label "SuperconductionTransitionTemperature"@en ;
    rdfs:comment "Critical thermodynamic temperature of a superconductor."@en ;
    rdfs:subClassOf ns1:CondensedMatterPhysicsQuantity,
        ns1:CriticalTemperature ;
    skos:prefLabel "SuperconductionTransitionTemperature"@en ;
    ns1:IEVReference "https://www.electropedia.org/iev/iev.nsf/display?openform&ievref=815-10-09"^^xsd:string ;
    ns1:ISO80000Reference "12-35.3"^^xsd:string ;
    ns1:elucidation "Critical thermodynamic temperature of a superconductor."@en ;
    ns1:qudtReference "https://qudt.org/vocab/quantitykind/SuperconductionTransitionTemperature"^^xsd:string ;
    ns1:wikidataReference "https://www.wikidata.org/wiki/Q106103037"^^xsd:string .

ns1:SuperconductorEnergyGap a owl:Class ;
    rdfs:label "SuperconductorEnergyGap"@en ;
    rdfs:comment "Width of the forbidden energy band in a superconductor."@en ;
    rdfs:subClassOf ns1:CondensedMatterPhysicsQuantity,
        ns1:GapEnergy ;
    skos:prefLabel "SuperconductorEnergyGap"@en ;
    ns1:IEVReference "https://www.electropedia.org/iev/iev.nsf/display?openform&ievref=815-10-28"^^xsd:string ;
    ns1:ISO80000Reference "12-37"^^xsd:string ;
    ns1:elucidation "Width of the forbidden energy band in a superconductor."@en ;
    ns1:qudtReference "https://qudt.org/vocab/quantitykind/SuperconductorEnergyGap"^^xsd:string ;
    ns1:wikidataReference "https://www.wikidata.org/wiki/Q106127898"^^xsd:string .

ns1:SurfaceActivityDensity a owl:Class ;
    rdfs:label "SurfaceActivityDensity"@en ;
    rdfs:comment "Quotient of the activity A of a sample and the total area S of the surface of that sample."@en ;
    rdfs:subClassOf [ a owl:Restriction ;
            owl:onProperty ns1:hasMeasurementUnit ;
            owl:someValuesFrom ns1:PerAreaTimeUnit ],
        ns1:AtomicAndNuclearPhysicsQuantity,
        ns1:ISQDerivedQuantity ;
    skos:prefLabel "SurfaceActivityDensity"@en ;
    ns1:IEVReference "https://www.electropedia.org/iev/iev.nsf/display?openform&ievref=395-01-10"^^xsd:string ;
    ns1:ISO80000Reference "10-30"^^xsd:string ;
    ns1:elucidation "Quotient of the activity A of a sample and the total area S of the surface of that sample."@en ;
    ns1:qudtReference "https://qudt.org/vocab/quantitykind/SurfaceActivityDensity"^^xsd:string ;
    ns1:wikidataReference "https://www.wikidata.org/wiki/Q98103005"^^xsd:string .

ns1:SurfaceCoefficientOfHeatTransfer a owl:Class ;
    rdfs:label "SurfaceCoefficientOfHeatTransfer"@en ;
    rdfs:comment "Coefficient of heat transfer when heat exchange takes place between a body at thermodynamic temperature Ts and its surroundings that are at a reference temperature Tr."@en ;
    rdfs:subClassOf ns1:CoefficientOfHeatTransfer,
        ns1:ThermodynamicalQuantity ;
    skos:prefLabel "SurfaceCoefficientOfHeatTransfer"@en ;
    ns1:IEVReference "https://www.electropedia.org/iev/iev.nsf/display?openform&ievref=113-04-40"^^xsd:string ;
    ns1:ISO80000Reference "5-10.2"^^xsd:string ;
    ns1:elucidation "Coefficient of heat transfer when heat exchange takes place between a body at thermodynamic temperature Ts and its surroundings that are at a reference temperature Tr."@en ;
    ns1:qudtReference "https://qudt.org/vocab/quantitykind/SurfaceCoefficientOfHeatTransfer"^^xsd:string ;
    ns1:wikidataReference "https://www.wikidata.org/wiki/Q74770365"^^xsd:string .

ns1:SurfaceDensityOfElectricCharge a owl:Class ;
    rdfs:label "SurfaceDensityOfElectricCharge"@en ;
    rdfs:comment "The derivative of the electric charge of a system with respect to the area."@en ;
    rdfs:subClassOf ns1:ElectricFluxDensity ;
    skos:altLabel "AreicElectricCharge"@en,
        "SurfaceChargeDensity"@en ;
    skos:prefLabel "SurfaceDensityOfElectricCharge"@en ;
    ns1:IEVReference "https://www.electropedia.org/iev/iev.nsf/display?openform&ievref=121-11-08"^^xsd:string ;
    ns1:ISO80000Reference "6-4"^^xsd:string ;
    ns1:elucidation "The derivative of the electric charge of a system with respect to the area."@en ;
    ns1:iupacReference "https://doi.org/10.1351/goldbook.S06159"^^xsd:string ;
    ns1:wikidataReference "https://www.wikidata.org/wiki/Q12799324"^^xsd:string .

ns1:SurfaceMassDensity a owl:Class ;
    rdfs:label "SurfaceMassDensity"@en ;
    rdfs:comment "at a given point on a two-dimensional domain of quasi-infinitesimal area dA, scalar quantity equal to the mass dm within the domain divided by the area dA, thus ρA = dm/dA."@en ;
    rdfs:subClassOf [ a owl:Restriction ;
            owl:onProperty ns1:hasMeasurementUnit ;
            owl:someValuesFrom ns1:AreaDensityUnit ],
        ns1:ISQDerivedQuantity,
        ns1:MechanicalQuantity ;
    skos:altLabel "AreicMass"@en,
        "SurfaceDensity"@en ;
    skos:prefLabel "SurfaceMassDensity"@en ;
    ns1:IEVReference "https://www.electropedia.org/iev/iev.nsf/display?openform&ievref=113-03-10"^^xsd:string ;
    ns1:ISO80000Reference "4-5"^^xsd:string ;
    ns1:elucidation "at a given point on a two-dimensional domain of quasi-infinitesimal area dA, scalar quantity equal to the mass dm within the domain divided by the area dA, thus ρA = dm/dA."@en ;
    ns1:iupacReference "https://doi.org/10.1351/goldbook.S06167"^^xsd:string ;
    ns1:wikidataReference "https://www.wikidata.org/wiki/Q1907514"^^xsd:string .

ns1:SurfaceTension a owl:Class ;
    rdfs:label "SurfaceTension"@en ;
    rdfs:subClassOf [ a owl:Restriction ;
            owl:onProperty ns1:hasMeasurementUnit ;
            owl:someValuesFrom ns1:ForcePerLengthUnit ],
        ns1:MechanicalQuantity ;
    skos:altLabel "4-26"^^xsd:string ;
    skos:prefLabel "SurfaceTension"@en ;
    ns1:IEVReference "https://www.electropedia.org/iev/iev.nsf/display?openform&ievref=113-03-42"^^xsd:string ;
    ns1:iupacReference "https://doi.org/10.1351/goldbook.S06192"^^xsd:string ;
    ns1:qudtReference "https://qudt.org/vocab/quantitykind/SurfaceTension"^^xsd:string ;
    ns1:wikidataReference "https://www.wikidata.org/wiki/Q170749"^^xsd:string .

ns1:Susceptance a owl:Class ;
    rdfs:label "Susceptance"@en ;
    rdfs:comment "Imaginary part of the admittance."@en ;
    rdfs:subClassOf ns1:ElectricConductance ;
    skos:prefLabel "Susceptance"@en ;
    ns1:IEVReference "https://www.electropedia.org/iev/iev.nsf/display?openform&ievref=131-12-54"^^xsd:string ;
    ns1:ISO80000Reference "6-52.3"^^xsd:string ;
    ns1:elucidation "Imaginary part of the admittance."@en ;
    ns1:qudtReference "https://qudt.org/vocab/quantitykind/Susceptance"^^xsd:string ;
    ns1:wikidataReference "https://www.wikidata.org/wiki/Q509598"^^xsd:string .

ns1:TemperatureAreaPerMassTimeUnit a owl:Class ;
    rdfs:label "TemperatureAreaPerMassTimeUnit"@en ;
    rdfs:comment "The class of units with dimensionality 'TemperatureAreaPerMassTime'."@en .

ns1:TemperatureLengthPerTimeUnit a owl:Class ;
    rdfs:label "TemperatureLengthPerTimeUnit"@en ;
    rdfs:comment "The class of units with dimensionality 'TemperatureLengthPerTime'."@en .

ns1:TemperatureMassPerAreaUnit a owl:Class ;
    rdfs:label "TemperatureMassPerAreaUnit"@en ;
    rdfs:comment "The class of units with dimensionality 'TemperatureMassPerArea'."@en .

ns1:TemperaturePerLengthUnit a owl:Class ;
    rdfs:label "TemperaturePerLengthUnit"@en ;
    rdfs:comment "The class of units with dimensionality 'TemperaturePerLength'."@en .

ns1:TemperaturePerMagneticFluxDensityUnit a owl:Class ;
    rdfs:label "TemperaturePerMagneticFluxDensityUnit"@en ;
    rdfs:comment "The class of units with dimensionality 'TemperaturePerMagneticFluxDensity'."@en .

ns1:TemperaturePerTimeUnit a owl:Class ;
    rdfs:label "TemperaturePerTimeUnit"@en ;
    rdfs:comment "The class of units with dimensionality 'TemperaturePerTime'."@en .

ns1:TemperaturePressurePerTimeUnit a owl:Class ;
    rdfs:label "TemperaturePressurePerTimeUnit"@en ;
    rdfs:comment "The class of units with dimensionality 'TemperaturePressurePerTime'."@en .

ns1:TemperatureTimeUnit a owl:Class ;
    rdfs:label "TemperatureTimeUnit"@en ;
    rdfs:comment "The class of units with dimensionality 'TemperatureTime'."@en .

ns1:ThermalConductance a owl:Class ;
    rdfs:label "ThermalConductance"@en ;
    rdfs:comment "Reciprocal of the thermal resistance."@en ;
    rdfs:subClassOf [ a owl:Restriction ;
            owl:onProperty ns1:hasMeasurementUnit ;
            owl:someValuesFrom ns1:ThermalConductanceUnit ],
        ns1:ISQDerivedQuantity,
        ns1:ThermodynamicalQuantity ;
    skos:prefLabel "ThermalConductance"@en ;
    ns1:IEVReference "https://www.electropedia.org/iev/iev.nsf/display?openform&ievref=113-04-46"^^xsd:string ;
    ns1:ISO80000Reference "5-13"^^xsd:string ;
    ns1:elucidation "Reciprocal of the thermal resistance."@en ;
    ns1:iupacReference "https://doi.org/10.1351/goldbook.T06298"^^xsd:string ;
    ns1:qudtReference "https://qudt.org/vocab/quantitykind/ThermalConductance"^^xsd:string ;
    ns1:wikidataReference "https://www.wikidata.org/wiki/Q17176562"^^xsd:string .

ns1:ThermalConductivity a owl:Class ;
    rdfs:label "ThermalConductivity"@en ;
    rdfs:comment "At a point fixed in a medium with a temperature field, scalar quantity λ characterizing the ability of the medium to transmit heat through a surface element containing that point: φ = −λ grad T, where φ is the density of heat flow rate and T is thermodynamic temperature."@en,
        "In an anisotropic medium, thermal conductivity is a tensor quantity."@en ;
    rdfs:subClassOf [ a owl:Restriction ;
            owl:onProperty ns1:hasMeasurementUnit ;
            owl:someValuesFrom ns1:ThermalConductivityUnit ],
        ns1:ISQDerivedQuantity,
        ns1:Intensive,
        ns1:ThermodynamicalQuantity ;
    skos:prefLabel "ThermalConductivity"@en ;
    ns1:IEVReference "https://www.electropedia.org/iev/iev.nsf/display?openform&ievref=113-04-38"^^xsd:string ;
    ns1:ISO80000Reference "5-9"^^xsd:string ;
    ns1:dbpediaReference "https://dbpedia.org/page/Thermal_conductivity"^^xsd:string ;
    ns1:elucidation "At a point fixed in a medium with a temperature field, scalar quantity λ characterizing the ability of the medium to transmit heat through a surface element containing that point: φ = −λ grad T, where φ is the density of heat flow rate and T is thermodynamic temperature."@en ;
    ns1:qudtReference "https://qudt.org/vocab/quantitykind/ThermalConductivity"^^xsd:string ;
    ns1:wikidataReference "https://www.wikidata.org/wiki/Q487005"^^xsd:string .

ns1:ThermalDiffusionFactor a owl:Class ;
    rdfs:label "ThermalDiffusionFactor"@en ;
    rdfs:comment "Quotient of the thermal diffusion ratio and the product of the local amount-of-substance fractions."@en ;
    rdfs:subClassOf ns1:ISQDimensionlessQuantity,
        ns1:PhysioChemicalQuantity ;
    owl:disjointWith ns1:ThermalDiffusionRatio ;
    skos:prefLabel "ThermalDiffusionFactor"@en ;
    ns1:ISO80000Reference "9-40.2"^^xsd:string ;
    ns1:elucidation "Quotient of the thermal diffusion ratio and the product of the local amount-of-substance fractions."@en ;
    ns1:qudtReference "https://qudt.org/vocab/quantitykind/ThermalDiffusionFactor"^^xsd:string ;
    ns1:wikidataReference "https://www.wikidata.org/wiki/Q96249629"^^xsd:string .

ns1:ThermalDiffusivity a owl:Class ;
    rdfs:label "ThermalDiffusivity"@en ;
    rdfs:comment "Quotient of thermal conductivity and the product of mass density and specific heat capacity."@en ;
    rdfs:subClassOf [ a owl:Restriction ;
            owl:onProperty ns1:hasMeasurementUnit ;
            owl:someValuesFrom ns1:AreicSpeedUnit ],
        ns1:ISQDerivedQuantity,
        ns1:ThermodynamicalQuantity ;
    skos:altLabel "ThermalDiffusionCoefficient"^^xsd:string ;
    skos:prefLabel "ThermalDiffusivity"@en ;
    ns1:IEVReference "https://www.electropedia.org/iev/iev.nsf/display?openform&ievref=113-04-53"^^xsd:string ;
    ns1:ISO80000Reference "5-14"^^xsd:string ;
    ns1:elucidation "Quotient of thermal conductivity and the product of mass density and specific heat capacity."@en ;
    ns1:qudtReference "https://qudt.org/vocab/quantitykind/ThermalDiffusivity"^^xsd:string ;
    ns1:wikidataReference "https://www.wikidata.org/wiki/Q3381809"^^xsd:string .

ns1:ThermalInsulance a owl:Class ;
    rdfs:label "ThermalInsulance"@en ;
    rdfs:comment "Reciprocal of the coefficient of heat transfer."@en ;
    rdfs:subClassOf [ a owl:Restriction ;
            owl:onProperty ns1:hasMeasurementUnit ;
            owl:someValuesFrom ns1:PerThermalTransmittanceUnit ],
        ns1:ISQDerivedQuantity,
        ns1:ThermodynamicalQuantity ;
    skos:altLabel "CoefficientOfThermalInsulance"@en ;
    skos:prefLabel "ThermalInsulance"@en ;
    ns1:IEVReference "https://www.electropedia.org/iev/iev.nsf/display?openform&ievref=113-04-41"^^xsd:string ;
    ns1:ISO80000Reference "5-11"^^xsd:string ;
    ns1:elucidation "Reciprocal of the coefficient of heat transfer."@en ;
    ns1:qudtReference "https://qudt.org/vocab/quantitykind/ThermalInsulance"^^xsd:string ;
    ns1:wikidataReference "https://www.wikidata.org/wiki/Q2596212"^^xsd:string .

ns1:ThermalResistance a owl:Class ;
    rdfs:label "ThermalResistance"@en ;
    rdfs:comment "The name “thermal resistance” and the symbol R are used in building technology to designate thermal insulance."@en,
        "Thermodynamic temperature difference divided by heat flow rate."@en ;
    rdfs:subClassOf [ a owl:Restriction ;
            owl:onProperty ns1:hasMeasurementUnit ;
            owl:someValuesFrom ns1:ThermalResistanceUnit ],
        ns1:ISQDerivedQuantity,
        ns1:ThermodynamicalQuantity ;
    skos:prefLabel "ThermalResistance"@en ;
    ns1:IEVReference "https://www.electropedia.org/iev/iev.nsf/display?openform&ievref=113-04-45"^^xsd:string ;
    ns1:ISO80000Reference "5-12"^^xsd:string ;
    ns1:elucidation "Thermodynamic temperature difference divided by heat flow rate."@en ;
    ns1:qudtReference "https://qudt.org/vocab/quantitykind/ThermalResistance"^^xsd:string ;
    ns1:wikidataReference "https://www.wikidata.org/wiki/Q899628"^^xsd:string .

ns1:ThermalResistivityUnit a owl:Class ;
    rdfs:label "ThermalResistivityUnit"@en ;
    rdfs:comment "The class of units with dimensionality 'ThermalResistivity'."@en .

ns1:ThermalUtilizationFactor a owl:Class ;
    rdfs:label "ThermalUtilizationFactor"@en ;
    rdfs:comment "In an infinite medium, the quotient of the number of thermal neutrons absorbed in a fissionable nuclide or in a nuclear fuel, as specified, and the total number of thermal neutrons absorbed."@en ;
    rdfs:subClassOf ns1:AtomicAndNuclearPhysicsQuantity,
        ns1:ISQDimensionlessQuantity ;
    skos:prefLabel "ThermalUtilizationFactor"@en ;
    ns1:ISO80000Reference "10-76"^^xsd:string ;
    ns1:elucidation "In an infinite medium, the quotient of the number of thermal neutrons absorbed in a fissionable nuclide or in a nuclear fuel, as specified, and the total number of thermal neutrons absorbed."@en ;
    ns1:qudtReference "https://qudt.org/vocab/quantitykind/ThermalUtilizationFactor"^^xsd:string ;
    ns1:wikidataReference "https://www.wikidata.org/wiki/Q99197650"^^xsd:string .

ns1:ThermodynamicCriticalMagneticFluxDensity a owl:Class ;
    rdfs:label "ThermodynamicCriticalMagneticFluxDensity"@en ;
    rdfs:comment "The magnetic flux density for disappearance of superconductivity in a type I superconductor."@en ;
    rdfs:subClassOf ns1:CondensedMatterPhysicsQuantity,
        ns1:MagneticFluxDensity ;
    owl:disjointWith ns1:LowerCriticalMagneticFluxDensity,
        ns1:UpperCriticalMagneticFluxDensity ;
    skos:prefLabel "ThermodynamicCriticalMagneticFluxDensity"@en ;
    ns1:ISO80000Reference "12-36.1"^^xsd:string ;
    ns1:elucidation "The magnetic flux density for disappearance of superconductivity in a type I superconductor."@en ;
    ns1:qudtReference "https://qudt.org/vocab/quantitykind/ThermodynamicCriticalMagneticFluxDensity"^^xsd:string ;
    ns1:wikidataReference "https://www.wikidata.org/wiki/Q106103200"^^xsd:string .

ns1:ThermodynamicEfficiency a owl:Class ;
    rdfs:label "ThermodynamicEfficiency"@en ;
    rdfs:comment "Performance measure of a device that uses thermal energy, expressed as the ratio of work done over thermal energy used."@en ;
    rdfs:subClassOf ns1:RatioQuantity,
        ns1:ThermodynamicalQuantity ;
    skos:altLabel "ThermalEfficiency"@en ;
    skos:prefLabel "ThermodynamicEfficiency"@en ;
    ns1:ISO80000Reference "5-25.1"^^xsd:string ;
    ns1:elucidation "Performance measure of a device that uses thermal energy, expressed as the ratio of work done over thermal energy used."@en ;
    ns1:qudtReference "https://qudt.org/vocab/quantitykind/ThermalEfficiency"^^xsd:string ;
    ns1:wikidataReference "https://www.wikidata.org/wiki/Q1452104"^^xsd:string .

ns1:ThermodynamicGrueneisenParameter a owl:Class ;
    rdfs:label "ThermodynamicGrueneisenParameter"@en ;
    rdfs:comment "A dimensionless thermodynamic parameter named after German physicist Eduard Grüneisen."@en ;
    rdfs:subClassOf ns1:CondensedMatterPhysicsQuantity,
        ns1:ISQDimensionlessQuantity ;
    skos:prefLabel "ThermodynamicGrueneisenParameter"@en ;
    ns1:ISO80000Reference "12-13"^^xsd:string ;
    ns1:elucidation "A dimensionless thermodynamic parameter named after German physicist Eduard Grüneisen."@en ;
    ns1:wikidataReference "https://www.wikidata.org/wiki/Q105658620"^^xsd:string ;
    ns1:wikipediaReference "https://en.wikipedia.org/wiki/Gr%C3%BCneisen_parameter"^^xsd:anyURI .

ns1:ThermoelectricVoltage a owl:Class ;
    rdfs:label "ThermoelectricVoltage"@en ;
    rdfs:comment "Voltage between substances a and b caused by the thermoelectric effect."@en ;
    rdfs:subClassOf ns1:CondensedMatterPhysicsQuantity,
        ns1:Voltage ;
    skos:prefLabel "ThermoelectricVoltage"@en ;
    ns1:ISO80000Reference "12-20"^^xsd:string ;
    ns1:elucidation "Voltage between substances a and b caused by the thermoelectric effect."@en ;
    ns1:wikidataReference "https://www.wikidata.org/wiki/Q105761637"^^xsd:string .

ns1:ThomsonCoefficient a owl:Class ;
    rdfs:label "ThomsonCoefficient"@en ;
    rdfs:comment "Quotient of Thomson heat power developed, and the electric current and temperature difference."@en ;
    rdfs:subClassOf [ a owl:Restriction ;
            owl:onProperty ns1:hasMeasurementUnit ;
            owl:someValuesFrom ns1:ElectricPotentialPerTemperatureUnit ],
        ns1:CondensedMatterPhysicsQuantity,
        ns1:ISQDerivedQuantity ;
    owl:disjointWith ns1:JouleThomsonCoefficient ;
    skos:prefLabel "ThomsonCoefficient"@en ;
    ns1:ISO80000Reference "12-23"^^xsd:string ;
    ns1:elucidation "Quotient of Thomson heat power developed, and the electric current and temperature difference."@en ;
    ns1:qudtReference "https://qudt.org/vocab/quantitykind/ThomsonCoefficient"^^xsd:string ;
    ns1:wikidataReference "https://www.wikidata.org/wiki/Q105801233"^^xsd:string .

ns1:TimePerLengthUnit a owl:Class ;
    rdfs:label "TimePerLengthUnit"@en ;
    rdfs:comment "The class of units with dimensionality 'TimePerLength'."@en .

ns1:Torque a owl:Class ;
    rdfs:label "Torque"@en ;
    rdfs:comment "Even though torque has the same physical dimension as energy, it is not of the same kind and can not be measured with energy units like joule or electron volt."@en,
        "The effectiveness of a force to produce rotation about an axis, measured by the product of the force and the perpendicular distance from the line of action of the force to the axis."@en ;
    rdfs:subClassOf [ a owl:Restriction ;
            owl:onProperty ns1:hasMeasurementUnit ;
            owl:someValuesFrom ns1:EnergyUnit ],
        ns1:ISQDerivedQuantity ;
    skos:prefLabel "Torque"@en ;
    ns1:ISO80000Reference "4-12.2"^^xsd:string ;
    ns1:elucidation "The effectiveness of a force to produce rotation about an axis, measured by the product of the force and the perpendicular distance from the line of action of the force to the axis."@en ;
    ns1:iupacReference "https://doi.org/10.1351/goldbook.T06400"^^xsd:string ;
    ns1:qudtReference "http://qudt.org/vocab/quantitykind/Torque"^^xsd:string .

ns1:Tortuosity a owl:Class ;
    rdfs:label "Tortuosity"@en ;
    rdfs:comment "Parameter for diffusion and fluid flow in porous media."@en ;
    rdfs:subClassOf ns1:RatioQuantity ;
    skos:prefLabel "Tortuosity"@en ;
    ns1:elucidation "Parameter for diffusion and fluid flow in porous media."@en ;
    ns1:wikidataReference "https://www.wikidata.org/wiki/Q2301683"^^xsd:string .

ns1:TotalAngularMomentum a owl:Class ;
    rdfs:label "TotalAngularMomentum"^^xsd:string ;
    rdfs:comment "Vector quantity in a quantum system composed of the vectorial sum of angular momentum L and spin s."@en ;
    rdfs:subClassOf ns1:AngularMomentum,
        ns1:AtomicAndNuclearPhysicsQuantity ;
    skos:prefLabel "TotalAngularMomentum"^^xsd:string ;
    ns1:ISO80000Reference "10-11"^^xsd:string ;
    ns1:elucidation "Vector quantity in a quantum system composed of the vectorial sum of angular momentum L and spin s."@en ;
    ns1:qudtReference "https://qudt.org/vocab/quantitykind/TotalAngularMomentum"^^xsd:string ;
    ns1:wikidataReference "https://www.wikidata.org/wiki/Q97496506"^^xsd:string .

ns1:TotalAngularMomentumQuantumNumber a owl:Class ;
    rdfs:label "TotalAngularMomentumQuantumNumber"^^xsd:string ;
    rdfs:comment "Quantum number in an atom describing the magnitude of total angular momentum J."@en ;
    rdfs:subClassOf ns1:QuantumNumber ;
    skos:prefLabel "TotalAngularMomentumQuantumNumber"^^xsd:string ;
    ns1:ISO80000Reference "10-13.6"^^xsd:string ;
    ns1:elucidation "Quantum number in an atom describing the magnitude of total angular momentum J."@en ;
    ns1:qudtReference "https://qudt.org/vocab/quantitykind/TotalAngularMomentumQuantumNumber"^^xsd:string ;
    ns1:wikidataReference "https://www.wikidata.org/wiki/Q1141095"^^xsd:string .

ns1:TotalCrossSection a owl:Class ;
    rdfs:label "TotalCrossSection"@en ;
    rdfs:comment "Sum of all cross sections corresponding to the various reactions or processes between an incident particle of specified type and energy and a target entity."@en ;
    rdfs:subClassOf ns1:AtomicAndNuclearPhysicsQuantity,
        ns1:AtomicPhysicsCrossSection ;
    skos:prefLabel "TotalCrossSection"@en ;
    ns1:ISO80000Reference "10-38.2"^^xsd:string ;
    ns1:elucidation "Sum of all cross sections corresponding to the various reactions or processes between an incident particle of specified type and energy and a target entity."@en ;
    ns1:qudtReference "https://qudt.org/vocab/quantitykind/TotalCrossSection"^^xsd:string ;
    ns1:wikidataReference "https://www.wikidata.org/wiki/Q98206553"^^xsd:string .

ns1:TotalCurrent a owl:Class ;
    rdfs:label "TotalCurrent"@en ;
    rdfs:comment "Sum of electric current and displacement current"@en ;
    rdfs:subClassOf ns1:ElectricCurrent ;
    skos:prefLabel "TotalCurrent"@en ;
    ns1:IEVReference "https://www.electropedia.org/iev/iev.nsf/display?openform&ievref=121-11-45"^^xsd:string ;
    ns1:ISO80000Reference "6-19.2"^^xsd:string ;
    ns1:elucidation "Sum of electric current and displacement current"@en ;
    ns1:qudtReference "https://qudt.org/vocab/quantitykind/TotalCurrent"^^xsd:string ;
    ns1:wikidataReference "https://www.wikidata.org/wiki/Q77679732"^^xsd:string .

ns1:TotalCurrentDensity a owl:Class ;
    rdfs:label "TotalCurrentDensity"@en ;
    rdfs:comment "Sum of electric current density and displacement current density."@en ;
    rdfs:subClassOf ns1:ElectricCurrentDensity ;
    skos:prefLabel "TotalCurrentDensity"@en ;
    ns1:IEVReference "https://www.electropedia.org/iev/iev.nsf/display?openform&ievref=121-11-44"^^xsd:string ;
    ns1:ISO80000Reference "6-20"^^xsd:string ;
    ns1:elucidation "Sum of electric current density and displacement current density."@en ;
    ns1:qudtReference "https://qudt.org/vocab/quantitykind/TotalCurrentDensity"^^xsd:string ;
    ns1:wikidataReference "https://www.wikidata.org/wiki/Q77680811"^^xsd:string .

ns1:TotalIonization a owl:Class ;
    rdfs:label "TotalIonization"@en ;
    rdfs:comment "Quotient of the total mean charge of all positive ions produced by an ionizing charged particle along its entire path and along the paths of any secondary charged particles, and the elementary charge."@en ;
    rdfs:subClassOf ns1:AtomicAndNuclearPhysicsQuantity,
        ns1:ISQDimensionlessQuantity ;
    skos:prefLabel "TotalIonization"@en ;
    ns1:ISO80000Reference "10-59"^^xsd:string ;
    ns1:elucidation "Quotient of the total mean charge of all positive ions produced by an ionizing charged particle along its entire path and along the paths of any secondary charged particles, and the elementary charge."@en ;
    ns1:qudtReference "https://qudt.org/vocab/quantitykind/TotalIonization"^^xsd:string ;
    ns1:wikidataReference "https://www.wikidata.org/wiki/Q98690787"^^xsd:string .

ns1:TotalLinearStoppingPower a owl:Class ;
    rdfs:label "TotalLinearStoppingPower"@en ;
    rdfs:comment "For charged particles of a given type and energy E0 the differential quotient of E with respect to x, where E is the mean energy lost by the charged particles in traversing a distance x in the given material."@en ;
    rdfs:subClassOf [ a owl:Restriction ;
            owl:onProperty ns1:hasMeasurementUnit ;
            owl:someValuesFrom ns1:ForceUnit ],
        ns1:AtomicAndNuclearPhysicsQuantity,
        ns1:ISQDerivedQuantity ;
    skos:altLabel "LinearStoppingPower"@en ;
    skos:prefLabel "TotalLinearStoppingPower"@en ;
    ns1:IEVReference "https://www.electropedia.org/iev/iev.nsf/display?openform&ievref=395-01-27"^^xsd:string,
        "https://www.electropedia.org/iev/iev.nsf/display?openform&ievref=881-12-49"^^xsd:string ;
    ns1:ISO80000Reference "10-54"^^xsd:string ;
    ns1:elucidation "For charged particles of a given type and energy E0 the differential quotient of E with respect to x, where E is the mean energy lost by the charged particles in traversing a distance x in the given material."@en ;
    ns1:iupacReference "https://doi.org/10.1351/goldbook.S06035"^^xsd:string ;
    ns1:qudtReference "https://qudt.org/vocab/quantitykind/TotalLinearStoppingPower"^^xsd:string ;
    ns1:wikidataReference "https://www.wikidata.org/wiki/Q908474"^^xsd:string .

ns1:TotalMassStoppingPower a owl:Class ;
    rdfs:label "TotalMassStoppingPower"@en ;
    rdfs:comment "Quotient of the total linear stopping power S and the mass density ρ of the material."@en ;
    rdfs:subClassOf [ a owl:Restriction ;
            owl:onProperty ns1:hasMeasurementUnit ;
            owl:someValuesFrom ns1:MassStoppingPowerUnit ],
        ns1:AtomicAndNuclearPhysicsQuantity,
        ns1:ISQDerivedQuantity ;
    skos:altLabel "MassStoppingPower"@en ;
    skos:prefLabel "TotalMassStoppingPower"@en ;
    ns1:IEVReference "https://www.electropedia.org/iev/iev.nsf/display?openform&ievref=881-12-52"^^xsd:string ;
    ns1:ISO80000Reference "10-55"^^xsd:string ;
    ns1:elucidation "Quotient of the total linear stopping power S and the mass density ρ of the material."@en ;
    ns1:qudtReference "https://qudt.org/vocab/quantitykind/TotalMassStoppingPower"^^xsd:string ;
    ns1:wikidataReference "https://www.wikidata.org/wiki/Q98642795"^^xsd:string .

ns1:UnifiedAtomicMassConstant a owl:Class ;
    rdfs:label "UnifiedAtomicMassConstant"^^xsd:string ;
    rdfs:comment "1/12 of the mass of an atom of the nuclide 12C in the ground state at rest."@en ;
    rdfs:subClassOf [ a owl:Restriction ;
            owl:onProperty ns1:hasMeasurementUnit ;
            owl:someValuesFrom ns1:MassUnit ],
        ns1:AtomicAndNuclearPhysicsQuantity,
        ns1:PhysicalConstant ;
    skos:prefLabel "UnifiedAtomicMassConstant"^^xsd:string ;
    ns1:IEVReference "https://www.electropedia.org/iev/iev.nsf/display?openform&ievref=113-05-23"^^xsd:string ;
    ns1:ISO80000Reference "10-4.3"^^xsd:string ;
    ns1:elucidation "1/12 of the mass of an atom of the nuclide 12C in the ground state at rest."@en ;
    ns1:iupacReference "https://doi.org/10.1351/goldbook.A00497"^^xsd:string ;
    ns1:wikidataReference "https://www.wikidata.org/wiki/Q4817337"^^xsd:string .

ns1:VacuumElectricPermittivity a owl:Class ;
    rdfs:label "VacuumElectricPermittivity"@en ;
    rdfs:comment "The DBpedia definition (http://dbpedia.org/page/Vacuum_permittivity) is outdated since May 20, 2019. It is now a measured constant."@en,
        "The value of the absolute dielectric permittivity of classical vacuum."@en ;
    rdfs:subClassOf ns1:MeasuredConstant,
        ns1:Permittivity ;
    skos:altLabel "PermittivityOfVacuum"@en ;
    skos:prefLabel "VacuumElectricPermittivity"@en ;
    ns1:ISO80000Reference "6-14.1"^^xsd:string ;
    ns1:elucidation "The value of the absolute dielectric permittivity of classical vacuum."@en ;
    ns1:iupacReference "https://doi.org/10.1351/goldbook.P04508"^^xsd:string ;
    ns1:qudtReference "http://qudt.org/vocab/constant/PermittivityOfVacuum"^^xsd:string .

ns1:VacuumMagneticPermeability a owl:Class ;
    rdfs:label "VacuumMagneticPermeability"@en ;
    rdfs:comment "The DBpedia and UIPAC Gold Book definitions (http://dbpedia.org/page/Vacuum_permeability,  https://doi.org/10.1351/goldbook.P04504) are outdated since May 20, 2019. It is now a measured constant."@en,
        "The value of magnetic permeability in a classical vacuum."@en ;
    rdfs:subClassOf ns1:MeasuredConstant,
        ns1:Permeability ;
    skos:altLabel "PermeabilityOfVacuum"^^xsd:string ;
    skos:prefLabel "VacuumMagneticPermeability"@en ;
    ns1:ISO80000Reference "6-26.1"^^xsd:string ;
    ns1:elucidation "The value of magnetic permeability in a classical vacuum."@en ;
    ns1:qudtReference "http://qudt.org/vocab/constant/ElectromagneticPermeabilityOfVacuum"^^xsd:string .

ns1:Vergence a owl:Class ;
    rdfs:label "Vergence"@en ;
    rdfs:comment "In geometrical optics, vergence describes the curvature of optical wavefronts."@en ;
    rdfs:subClassOf [ a owl:Restriction ;
            owl:onProperty ns1:hasMeasurementUnit ;
            owl:someValuesFrom ns1:ReciprocalLengthUnit ],
        ns1:ISQDerivedQuantity ;
    skos:prefLabel "Vergence"@en ;
    ns1:elucidation "In geometrical optics, vergence describes the curvature of optical wavefronts."@en ;
    ns1:qudtReference "http://qudt.org/vocab/quantitykind/Curvature"^^xsd:string .

ns1:VoltagePhasor a owl:Class ;
    rdfs:label "VoltagePhasor"@en ;
    rdfs:comment "Complex representation of an oscillating voltage."@en ;
    rdfs:subClassOf ns1:ElectricPotential ;
    skos:prefLabel "VoltagePhasor"@en ;
    ns1:ISO80000Reference "6-50"^^xsd:string ;
    ns1:elucidation "Complex representation of an oscillating voltage."@en ;
    ns1:qudtReference "https://qudt.org/vocab/quantitykind/VoltagePhasor"^^xsd:string ;
    ns1:wikidataReference "https://www.wikidata.org/wiki/Q78514605"^^xsd:string .

ns1:Volume a owl:Class ;
    rdfs:label "Volume"@en ;
    rdfs:comment "Extent of an object in space."@en ;
    rdfs:subClassOf [ a owl:Restriction ;
            owl:onProperty ns1:hasMeasurementUnit ;
            owl:someValuesFrom ns1:VolumeUnit ],
        ns1:Extensive,
        ns1:ISQDerivedQuantity,
        ns1:SpaceAndTimeQuantity ;
    skos:prefLabel "Volume"@en ;
    ns1:IEVReference "https://www.electropedia.org/iev/iev.nsf/display?openform&ievref=102-04-40"^^xsd:string ;
    ns1:ISO80000Reference "3-4"^^xsd:string ;
    ns1:dbpediaReference "https://dbpedia.org/page/Volume"^^xsd:string ;
    ns1:elucidation "Extent of an object in space."@en ;
    ns1:qudtReference "http://qudt.org/vocab/quantitykind/Volume"^^xsd:string ;
    ns1:wikidataReference "https://www.wikidata.org/wiki/Q39297"^^xsd:string .

ns1:VolumeFlowRate a owl:Class ;
    rdfs:label "VolumeFlowRate"@en ;
    rdfs:comment "Quantity equal to the volume dV of substance crossing a given surface during a time interval with infinitesimal duration dt, divided by this duration, thus qV = dV / dt-"@en ;
    rdfs:subClassOf [ a owl:Restriction ;
            owl:onProperty ns1:hasMeasurementUnit ;
            owl:someValuesFrom ns1:VolumePerTimeUnit ],
        ns1:ISQDerivedQuantity,
        ns1:MechanicalQuantity ;
    skos:altLabel "VolumetricFlowRate"@en ;
    skos:prefLabel "VolumeFlowRate"@en ;
    ns1:IEVReference "https://www.electropedia.org/iev/iev.nsf/display?openform&ievref=113-03-72"^^xsd:string ;
    ns1:ISO80000Reference "4-31"^^xsd:string ;
    ns1:elucidation "Quantity equal to the volume dV of substance crossing a given surface during a time interval with infinitesimal duration dt, divided by this duration, thus qV = dV / dt-"@en ;
    ns1:qudtReference "https://qudt.org/vocab/quantitykind/VolumeFlowRate"^^xsd:string ;
    ns1:wikidataReference "https://www.wikidata.org/wiki/Q1134348"^^xsd:string ;
    ns1:wikipediaReference "https://en.wikipedia.org/wiki/Volumetric_flow_rate"^^xsd:string .

ns1:VolumeFraction a owl:Class ;
    rdfs:label "VolumeFraction"@en ;
    rdfs:comment "Volume of a constituent of a mixture divided by the sum of volumes of all constituents prior to mixing."@en ;
    rdfs:subClassOf ns1:Intensive,
        ns1:RatioQuantity ;
    skos:prefLabel "VolumeFraction"@en ;
    ns1:ISO80000Reference "9-14"^^xsd:string ;
    ns1:elucidation "Volume of a constituent of a mixture divided by the sum of volumes of all constituents prior to mixing."@en ;
    ns1:iupacReference "https://doi.org/10.1351/goldbook.V06643"@en ;
    ns1:qudtReference "http://qudt.org/vocab/quantitykind/VolumeFraction"^^xsd:string .

ns1:VolumePerAmountTimeUnit a owl:Class ;
    rdfs:label "VolumePerAmountTimeUnit"@en ;
    rdfs:comment "The class of units with dimensionality 'VolumePerAmountTime'."@en .

ns1:VolumePerSquareTimeUnit a owl:Class ;
    rdfs:label "VolumePerSquareTimeUnit"@en ;
    rdfs:comment "The class of units with dimensionality 'VolumePerSquareTime'."@en .

ns1:VolumePerTemperatureUnit a owl:Class ;
    rdfs:label "VolumePerTemperatureUnit"@en ;
    rdfs:comment "The class of units with dimensionality 'VolumePerTemperature'."@en .

ns1:VolumicCrossSection a owl:Class ;
    rdfs:label "VolumicCrossSection"@en ;
    rdfs:comment "In nuclear physics, product of the number density of atoms of a given type and the cross section."@en ;
    rdfs:subClassOf [ a owl:Restriction ;
            owl:onProperty ns1:hasMeasurementUnit ;
            owl:someValuesFrom ns1:ReciprocalLengthUnit ],
        ns1:AtomicAndNuclearPhysicsQuantity,
        ns1:ISQDerivedQuantity ;
    skos:altLabel "MacroscopicCrossSection"@en ;
    skos:prefLabel "VolumicCrossSection"@en ;
    ns1:ISO80000Reference "10-42.1"^^xsd:string ;
    ns1:elucidation "In nuclear physics, product of the number density of atoms of a given type and the cross section."@en ;
    ns1:iupacReference "https://doi.org/10.1351/goldbook.M03674"^^xsd:string ;
    ns1:qudtReference "https://qudt.org/vocab/quantitykind/MacroscopicCrossSection"^^xsd:string ;
    ns1:wikidataReference "https://www.wikidata.org/wiki/Q98280520"^^xsd:string .

ns1:VolumicTotalCrossSection a owl:Class ;
    rdfs:label "VolumicTotalCrossSection"@en ;
    rdfs:comment "Product of the number density na of the atoms and the cross section σ_tot for a given type of atoms."@en ;
    rdfs:subClassOf [ a owl:Restriction ;
            owl:onProperty ns1:hasMeasurementUnit ;
            owl:someValuesFrom ns1:ReciprocalLengthUnit ],
        ns1:AtomicAndNuclearPhysicsQuantity,
        ns1:ISQDerivedQuantity ;
    skos:altLabel "MacroscopicTotalCrossSection"@en ;
    skos:prefLabel "VolumicTotalCrossSection"@en ;
    ns1:ISO80000Reference "10-42.2"^^xsd:string ;
    ns1:elucidation "Product of the number density na of the atoms and the cross section σ_tot for a given type of atoms."@en ;
    ns1:qudtReference "https://qudt.org/vocab/quantitykind/MacroscopicTotalCrossSection"^^xsd:string ;
    ns1:wikidataReference "https://www.wikidata.org/wiki/Q98280548"^^xsd:string .

ns1:VonKlitzingConstant a owl:Class ;
    rdfs:label "VonKlitzingConstant"@en ;
    rdfs:comment "Resistance quantum."@en,
        "The von Klitzing constant is defined as Planck constant divided by the square of the elementary charge."@en ;
    rdfs:subClassOf ns1:ElectricResistance,
        ns1:SIExactConstant ;
    skos:prefLabel "VonKlitzingConstant"@en ;
    ns1:definition "The von Klitzing constant is defined as Planck constant divided by the square of the elementary charge."@en ;
    ns1:elucidation "Resistance quantum."@en ;
    ns1:qudtReference "http://qudt.org/vocab/constant/VonKlitzingConstant"^^xsd:string .

ns1:WaveVector a owl:Class ;
    rdfs:label "WaveVector"@en ;
    rdfs:comment "Vector k in the expression ω t−k⋅r+ϑ0 of the phase of a sinusoidal wave."@en ;
    rdfs:subClassOf ns1:ReciprocalLength,
        ns1:SpaceAndTimeQuantity ;
    skos:prefLabel "WaveVector"@en ;
    ns1:IEVReference "https://www.electropedia.org/iev/iev.nsf/display?openform&ievref=103-10-09"^^xsd:string ;
    ns1:ISO80000Reference "3-21"^^xsd:string ;
    ns1:elucidation "Vector k in the expression ω t−k⋅r+ϑ0 of the phase of a sinusoidal wave."@en ;
    ns1:wikidataReference "https://www.wikidata.org/wiki/Q657009"^^xsd:string ;
    ns1:wikipediaReference "https://en.wikipedia.org/wiki/Wave_vector"^^xsd:string .

ns1:Weight a owl:Class ;
    rdfs:label "Weight"@en ;
    rdfs:comment "Force of gravity acting on a body."@en ;
    rdfs:subClassOf ns1:Force ;
    skos:prefLabel "Weight"@en ;
    ns1:ISO80000Reference "4-9.2"^^xsd:string ;
    ns1:elucidation "Force of gravity acting on a body."@en ;
    ns1:iupacReference "https://doi.org/10.1351/goldbook.W06668"^^xsd:string ;
    ns1:qudtReference "http://qudt.org/vocab/quantitykind/Weight"^^xsd:string .

ns1:Width a owl:Class ;
    rdfs:label "Width"@en ;
    rdfs:comment "Length in a given direction regarded as horizontal."@en,
        "The terms breadth and width are often used by convention, as distinguished from length and from height or thickness."@en ;
    rdfs:subClassOf ns1:Length ;
    skos:altLabel "Breadth"@en ;
    skos:prefLabel "Width"@en ;
    ns1:IEVReference "https://www.electropedia.org/iev/iev.nsf/display?openform&ievref=113-01-20"^^xsd:string ;
    ns1:ISO80000Reference "3-1.2"^^xsd:string ;
    ns1:elucidation "Length in a given direction regarded as horizontal."@en ;
    ns1:qudtReference "https://qudt.org/vocab/quantitykind/Width"^^xsd:string ;
    ns1:wikidataReference "https://www.wikidata.org/wiki/Q35059"^^xsd:string .

ns1:Work a owl:Class ;
    rdfs:label "Work"@en ;
    rdfs:comment "Product of force and displacement."@en ;
    rdfs:subClassOf ns1:Energy ;
    skos:prefLabel "Work"@en ;
    ns1:ISO80000Reference "4-28.4"^^xsd:string ;
    ns1:elucidation "Product of force and displacement."@en ;
    ns1:iupacReference "https://doi.org/10.1351/goldbook.W06684"^^xsd:string ;
    ns1:qudtReference "http://qudt.org/vocab/quantitykind/Work"^^xsd:string .

ns1:WorkFunction a owl:Class ;
    rdfs:label "WorkFunction"@en ;
    rdfs:comment "Least energy required for the emission of a conduction electron."@en,
        "Work function is the energy difference between an electron at rest at infinity and an electron at the Fermi level in the interior of a substance."@en ;
    rdfs:subClassOf ns1:CondensedMatterPhysicsQuantity,
        ns1:Energy ;
    skos:altLabel "ElectronWorkFunction"@en ;
    skos:prefLabel "WorkFunction"@en ;
    ns1:IEVReference "https://www.electropedia.org/iev/iev.nsf/display?openform&ievref=113-06-35"^^xsd:string ;
    ns1:ISO80000Reference "12-24.1"^^xsd:string ;
    ns1:elucidation "Least energy required for the emission of a conduction electron."@en ;
    ns1:iupacReference "https://doi.org/10.1351/goldbook.E02015"^^xsd:string ;
    ns1:wikidataReference "https://www.wikidata.org/wiki/Q783800"^^xsd:string .

ns1:wikidataReference a owl:AnnotationProperty ;
    rdfs:label "wikidataReference"@en ;
    ns2:python_name "wikidataReference"@en ;
    rdfs:comment "URL corresponding to entry in Wikidata."@en ;
    rdfs:seeAlso "https://www.wikidata.org/"^^xsd:string ;
    rdfs:subPropertyOf rdfs:seeAlso ;
    skos:prefLabel "wikidataReference"@en ;
    ns1:elucidation "URL corresponding to entry in Wikidata."@en .

<https://w3id.org/emmo/disciplines/isq> a owl:Ontology ;
    dcterms:abstract """Defines physical quantities in the International System of Quantities (ISQ). ISQ was made an official ISO standard in 2009 and is defined in the ISO/IEC 80000 standard.

ISQ underlines the SI system and defines physical quanties that are measured with SI units.

ISQ has 7 base quantities and many derived quantities defined in terms of the 7 base quantities.

The number of derived quantities not closed and may increase based on the need by domain ontologies."""@en ;
    dcterms:contributor ns1:FrancescaBleken ;
    dcterms:creator ns1:EmanueleGhedini,
        ns1:GerhardGoldbeck,
        ns1:JesperFriis,
        ns1:SimonClark ;
    dcterms:license "https://creativecommons.org/licenses/by/4.0/legalcode"^^xsd:string ;
    dcterms:publisher <https://emmc.eu> ;
    dcterms:title "International System of Quantities (ISQ)"@en ;
    rdfs:comment "The EMMO requires HermiT reasoner plugin in order to visualize all inferences and class hierarchy (ctrl+R hotkey in Protege)."@en ;
    owl:imports <https://w3id.org/emmo/1.0.2/disciplines/materials>,
        <https://w3id.org/emmo/1.0.2/disciplines/units/sidimensionalunits>,
        <https://w3id.org/emmo/1.0.2/reference/symbolic> ;
    owl:versionIRI <https://w3id.org/emmo/1.0.2/disciplines/isq> ;
    owl:versionInfo "1.0.2"^^xsd:string ;
    ns1:contact "emmo@emmc.eu"^^xsd:string .

ns1:AbsorbedDoseRate a owl:Class ;
    rdfs:label "AbsorbedDoseRate"@en ;
    rdfs:comment "Differential quotient of the absorbed dose with respect to time."@en ;
    rdfs:subClassOf [ a owl:Restriction ;
            owl:onProperty ns1:hasMeasurementUnit ;
            owl:someValuesFrom ns1:AbsorbedDoseRateUnit ],
        ns1:AtomicAndNuclearPhysicsQuantity,
        ns1:ISQDerivedQuantity ;
    skos:prefLabel "AbsorbedDoseRate"@en ;
    ns1:IEVReference "https://www.electropedia.org/iev/iev.nsf/display?openform&ievref=881-12-07"^^xsd:string ;
    ns1:ISO80000Reference "10-84"^^xsd:string ;
    ns1:elucidation "Differential quotient of the absorbed dose with respect to time."@en ;
    ns1:qudtReference "https://qudt.org/vocab/quantitykind/AbsorbedDoseRate"^^xsd:string ;
    ns1:wikidataReference "https://www.wikidata.org/wiki/Q69428958"^^xsd:string .

ns1:ActivityCoefficient a owl:Class ;
    rdfs:label "ActivityCoefficient"@en ;
    rdfs:comment "A coefficient in thermodynamics used to account for deviation of a mixture of chemical substances from ideal behaviour."@en ;
    rdfs:subClassOf ns1:ISQDimensionlessQuantity,
        ns1:PhysioChemicalQuantity ;
    skos:prefLabel "ActivityCoefficient"@en ;
    ns1:ISO80000Reference "9-25"^^xsd:string ;
    ns1:elucidation "A coefficient in thermodynamics used to account for deviation of a mixture of chemical substances from ideal behaviour."@en ;
    ns1:iupacReference "https://doi.org/10.1351/goldbook.A00116"^^xsd:string ;
    ns1:qudtReference "https://qudt.org/vocab/quantitykind/ActivityCoefficient"^^xsd:string ;
    ns1:wikidataReference "https://www.wikidata.org/wiki/Q745224"^^xsd:string .

ns1:ActivityOfSolute a owl:Class ;
    rdfs:label "ActivityOfSolute"@en ;
    rdfs:comment "For a solute X in a solution; quantity proportional to the absolute activity."@en ;
    rdfs:subClassOf ns1:ISQDimensionlessQuantity,
        ns1:PhysioChemicalQuantity ;
    skos:altLabel "RelativeActivityOfSolute"@en ;
    skos:prefLabel "ActivityOfSolute"@en ;
    ns1:ISO80000Reference "9-24"^^xsd:string ;
    ns1:elucidation "For a solute X in a solution; quantity proportional to the absolute activity."@en ;
    ns1:wikidataReference "https://www.wikidata.org/wiki/Q89408862"^^xsd:string .

ns1:AmountConcentration a owl:Class ;
    rdfs:label "AmountConcentration"@en ;
    rdfs:comment "The amount of a constituent divided by the volume of the mixture."@en ;
    rdfs:subClassOf [ a owl:Restriction ;
            owl:onProperty ns1:hasMeasurementUnit ;
            owl:someValuesFrom ns1:AmountConcentrationUnit ],
        ns1:Concentration,
        ns1:ISQDerivedQuantity,
        ns1:Intensive ;
    skos:altLabel "Concentration"@en,
        "MolarConcentration"@en,
        "Molarity"@en ;
    skos:prefLabel "AmountConcentration"@en ;
    ns1:elucidation "The amount of a constituent divided by the volume of the mixture."@en ;
    ns1:iupacReference "https://doi.org/10.1351/goldbook.A00295"^^xsd:string ;
    ns1:qudtReference "http://qudt.org/vocab/quantitykind/AmountOfSubstanceConcentrationOfB"^^xsd:string .

ns1:AmountConductivityUnit a owl:Class ;
    rdfs:label "AmountConductivityUnit"@en ;
    rdfs:comment "The class of units with dimensionality 'AmountConductivity'."@en .

ns1:AmountOfSubstance a owl:Class ;
    rdfs:label "AmountOfSubstance"@en ;
    rdfs:comment """"In the name “amount of substance”, the word “substance” will typically be replaced by words to specify the substance concerned in any particular application, for example “amount of hydrogen chloride, HCl”, or “amount of benzene, C6H6 ”. It is important to give a precise definition of the entity involved (as emphasized in the definition of the mole); this should preferably be done by specifying the molecular chemical formula of the material involved. Although the word “amount” has a more general dictionary definition, the abbreviation of the full name “amount of substance” to “amount” may be used for brevity."

-- SI Brochure"""@en,
        "The number of elementary entities present."@en ;
    rdfs:subClassOf [ a owl:Restriction ;
            owl:onProperty ns1:hasMeasurementUnit ;
            owl:someValuesFrom ns1:AmountUnit ],
        ns1:Extensive,
        ns1:PhysioChemicalQuantity ;
    skos:prefLabel "AmountOfSubstance"@en ;
    ns1:ISO80000Reference "9-2"^^xsd:string ;
    ns1:elucidation "The number of elementary entities present."@en ;
    ns1:iupacReference "https://doi.org/10.1351/goldbook.A00297"^^xsd:string ;
    ns1:qudtReference "http://qudt.org/vocab/quantitykind/AmountOfSubstance"^^xsd:string .

ns1:AngularFrequencyUnit a owl:Class ;
    rdfs:label "AngularFrequencyUnit"@en ;
    rdfs:comment "The class of units with dimensionality 'AngularFrequency'."@en .

ns1:AngularWaveNumber a owl:Class ;
    rdfs:label "AngularWaveNumber"@en ;
    rdfs:comment "In condensed matter physics, quotient of momentum and the reduced Planck constant."@en ;
    rdfs:subClassOf ns1:CondensedMatterPhysicsQuantity,
        ns1:Wavenumber ;
    skos:altLabel "AngularRepetency"@en ;
    skos:prefLabel "AngularWaveNumber"@en ;
    ns1:ISO80000Reference "12-9.1"^^xsd:string ;
    ns1:elucidation "In condensed matter physics, quotient of momentum and the reduced Planck constant."@en ;
    ns1:qudtReference "https://qudt.org/vocab/quantitykind/AngularWavenumber"^^xsd:string ;
    ns1:wikidataReference "https://www.wikidata.org/wiki/Q105542089"^^xsd:string .

ns1:AngularWavenumber a owl:Class ;
    rdfs:label "AngularWavenumber"@en ;
    rdfs:comment "Magnitude of the wave vector."@en ;
    rdfs:subClassOf ns1:ReciprocalLength,
        ns1:SpaceAndTimeQuantity ;
    skos:altLabel "AngularRepetency"@en ;
    skos:prefLabel "AngularWavenumber"@en ;
    ns1:IEVReference "https://www.electropedia.org/iev/iev.nsf/display?openform&ievref=103-10-12"^^xsd:string ;
    ns1:ISO80000Reference "3-22"^^xsd:string ;
    ns1:elucidation "Magnitude of the wave vector."@en ;
    ns1:qudtReference "https://qudt.org/vocab/quantitykind/AngularWavenumber"^^xsd:string ;
    ns1:wikidataReference "https://www.wikidata.org/wiki/Q30338487"^^xsd:string .

ns1:AreaPerAmountUnit a owl:Class ;
    rdfs:label "AreaPerAmountUnit"@en ;
    rdfs:comment "The class of units with dimensionality 'AreaPerAmount'."@en .

ns1:AreaPerTimeUnit a owl:Class ;
    rdfs:label "AreaPerTimeUnit"@en ;
    rdfs:comment "The class of units with dimensionality 'AreaPerTime'."@en .

ns1:AtomicPhysicsCrossSection a owl:Class ;
    rdfs:label "AtomicPhysicsCrossSection"@en ;
    rdfs:comment "Measure of probability that a specific process will take place in a collision of two particles."@en ;
    rdfs:subClassOf [ a owl:Restriction ;
            owl:onProperty ns1:hasMeasurementUnit ;
            owl:someValuesFrom ns1:AreaUnit ],
        ns1:AtomicAndNuclearPhysicsQuantity ;
    skos:prefLabel "AtomicPhysicsCrossSection"@en ;
    ns1:ISO80000Reference "10-38.1"^^xsd:string ;
    ns1:elucidation "Measure of probability that a specific process will take place in a collision of two particles."@en ;
    ns1:qudtReference "https://qudt.org/vocab/quantitykind/Cross-Section.html"^^xsd:string ;
    ns1:wikidataReference "https://www.wikidata.org/wiki/Q17128025"^^xsd:string .

ns1:CapacitanceUnit a owl:Class .

ns1:CatalyticActivityUnit a owl:Class .

ns1:ChargeNumber a owl:Class ;
    rdfs:label "ChargeNumber"@en ;
    rdfs:comment "For a particle, electric charge q divided by elementary charge e."@en,
        "The charge number of a particle may be presented as a superscript to the symbol of that particle, e.g. H+, He++, Al3+, Cl−, S=, N3−."@en,
        "The charge number of an electrically charged particle can be positive or negative. The charge number of an electrically neutral particle is zero."@en ;
    rdfs:subClassOf ns1:PhysioChemicalQuantity,
        ns1:PureNumberQuantity ;
    skos:altLabel "IonizationNumber"@en ;
    skos:prefLabel "ChargeNumber"@en ;
    ns1:IEVReference "https://www.electropedia.org/iev/iev.nsf/display?openform&ievref=113-05-17"@en ;
    ns1:ISO80000Reference "10-5.2"@en ;
    ns1:dbpediaReference "https://dbpedia.org/page/Charge_number"^^xsd:string ;
    ns1:elucidation "For a particle, electric charge q divided by elementary charge e."@en ;
    ns1:iupacReference "https://doi.org/10.1351/goldbook.C00993"^^xsd:string ;
    ns1:qudtReference "https://qudt.org/vocab/quantitykind/ChargeNumber"^^xsd:string ;
    ns1:wikidataReference "https://www.wikidata.org/wiki/Q1800063"^^xsd:string ;
    ns1:wikipediaReference "https://en.wikipedia.org/wiki/Charge_number"^^xsd:string .

ns1:CoefficientOfHeatTransfer a owl:Class ;
    rdfs:label "CoefficientOfHeatTransfer"@en ;
    rdfs:comment "At a point on the surface separating two media with different thermodynamic temperatures, magnitude of the density of heat flow rate φ divided by the absolute value of temperature difference ΔT."@en ;
    rdfs:subClassOf [ a owl:Restriction ;
            owl:onProperty ns1:hasMeasurementUnit ;
            owl:someValuesFrom ns1:ThermalTransmittanceUnit ],
        ns1:ISQDerivedQuantity,
        ns1:ThermodynamicalQuantity ;
    skos:altLabel "ThermalTransmittance"@en ;
    skos:prefLabel "CoefficientOfHeatTransfer"@en ;
    ns1:IEVReference "https://www.electropedia.org/iev/iev.nsf/display?openform&ievref=113-04-39"^^xsd:string ;
    ns1:ISO80000Reference "5-10.1"^^xsd:string ;
    ns1:elucidation "At a point on the surface separating two media with different thermodynamic temperatures, magnitude of the density of heat flow rate φ divided by the absolute value of temperature difference ΔT."@en ;
    ns1:qudtReference "https://qudt.org/vocab/quantitykind/CoefficientOfHeatTransfer"^^xsd:string ;
    ns1:wikidataReference "https://www.wikidata.org/wiki/Q634340"^^xsd:string .

ns1:Density a owl:Class ;
    rdfs:label "Density"@en ;
    rdfs:comment "Quantity representing the spatial distribution of mass in a continuous material."@en ;
    rdfs:subClassOf [ a owl:Restriction ;
            owl:allValuesFrom ns1:Matter ;
            owl:onProperty [ owl:inverseOf ns1:hasProperty ] ],
        [ a owl:Restriction ;
            owl:onProperty ns1:hasMeasurementUnit ;
            owl:someValuesFrom ns1:DensityUnit ],
        ns1:ISQDerivedQuantity,
        ns1:Intensive ;
    skos:altLabel "MassConcentration"@en,
        "MassDensity"@en ;
    skos:prefLabel "Density"@en ;
    ns1:ISO80000Reference "4-2"^^xsd:string,
        "9-10"^^xsd:string,
        "Mass per volume."@en ;
    ns1:elucidation "Quantity representing the spatial distribution of mass in a continuous material."@en ;
    ns1:iupacReference "https://doi.org/10.1351/goldbook.D01590"^^xsd:string ;
    ns1:qudtReference "http://qudt.org/vocab/quantitykind/Density"^^xsd:string .

ns1:DensityOfHeatFlowRate a owl:Class ;
    rdfs:label "DensityOfHeatFlowRate"@en ;
    rdfs:comment "At a fixed point in a medium, the direction of propagation of heat is opposite to the temperature gradient. At a point on the surface separating two media with different temperatures, the direction of propagation of heat is normal to the surface, from higher to lower temperatures."@en,
        "Vector quantity with magnitude equal to the heat flow rate dΦ through a surface element divided by the area dA of the element, and direction eφ in the direction of propagation of heat."@en ;
    rdfs:subClassOf ns1:Intensity,
        ns1:ThermodynamicalQuantity ;
    skos:altLabel "AreicHeatFlowRate"@en ;
    skos:prefLabel "DensityOfHeatFlowRate"@en ;
    ns1:IEVReference "https://www.electropedia.org/iev/iev.nsf/display?openform&ievref=113-04-37"^^xsd:string ;
    ns1:ISO80000Reference "5-8"^^xsd:string ;
    ns1:elucidation "Vector quantity with magnitude equal to the heat flow rate dΦ through a surface element divided by the area dA of the element, and direction eφ in the direction of propagation of heat."@en ;
    ns1:iupacReference "https://doi.org/10.1351/goldbook.H02755"^^xsd:string ;
    ns1:wikidataReference "https://www.wikidata.org/wiki/Q1478382"^^xsd:string .

ns1:DensityOfVibrationalStates a owl:Class ;
    rdfs:label "DensityOfVibrationalStates"@en ;
    rdfs:comment "quotient of the number of vibrational modes in an infinitesimal interval of angular frequency, and the product of the width of that interval and volume"@en ;
    rdfs:subClassOf [ a owl:Restriction ;
            owl:onProperty ns1:hasMeasurementUnit ;
            owl:someValuesFrom ns1:TimePerVolumeUnit ],
        ns1:CondensedMatterPhysicsQuantity,
        ns1:ISQDerivedQuantity ;
    skos:prefLabel "DensityOfVibrationalStates"@en ;
    ns1:ISO80000Reference "12-12"^^xsd:string ;
    ns1:elucidation "quotient of the number of vibrational modes in an infinitesimal interval of angular frequency, and the product of the width of that interval and volume"@en ;
    ns1:qudtReference "https://qudt.org/vocab/quantitykind/DensityOfStates"^^xsd:string ;
    ns1:wikidataReference "https://www.wikidata.org/wiki/Q105637294"^^xsd:string .

ns1:DensityUnit a owl:Class ;
    rdfs:label "DensityUnit"@en ;
    rdfs:comment "The class of units with dimensionality 'Density'."@en .

ns1:ElectricChargeDensityUnit a owl:Class ;
    rdfs:label "ElectricChargeDensityUnit"@en ;
    rdfs:comment "The class of units with dimensionality 'ElectricChargeDensity'."@en .

ns1:ElectricChargePerLengthUnit a owl:Class ;
    rdfs:label "ElectricChargePerLengthUnit"@en ;
    rdfs:comment "The class of units with dimensionality 'ElectricChargePerLength'."@en .

ns1:ElectricConductivity a owl:Class ;
    rdfs:label "ElectricConductivity"@en ;
    rdfs:comment "Conductivity is equeal to the resiprocal of resistivity."@en,
        "Measure of a material's ability to conduct an electric current."@en ;
    rdfs:subClassOf [ a owl:Restriction ;
            owl:onProperty ns1:hasMeasurementUnit ;
            owl:someValuesFrom ns1:ElectricConductivityUnit ],
        ns1:ElectromagneticQuantity,
        ns1:ISQDerivedQuantity,
        ns1:Intensive ;
    skos:altLabel "Conductivity"^^xsd:string ;
    skos:prefLabel "ElectricConductivity"@en ;
    ns1:ISO80000Reference "6-43"^^xsd:string ;
    ns1:elucidation "Measure of a material's ability to conduct an electric current."@en ;
    ns1:iupacReference "https://doi.org/10.1351/goldbook.C01245"^^xsd:string ;
    ns1:qudtReference "http://qudt.org/vocab/quantitykind/ElectricConductivity"^^xsd:string ;
    ns1:wikidataReference "https://www.wikidata.org/wiki/Q4593291"^^xsd:string .

ns1:ElectricCurrentPerEnergyUnit a owl:Class ;
    rdfs:label "ElectricCurrentPerEnergyUnit"@en ;
    rdfs:comment "The class of units with dimensionality 'ElectricCurrentPerEnergy'."@en .

ns1:ElectricCurrentPerMassUnit a owl:Class ;
    rdfs:label "ElectricCurrentPerMassUnit"@en ;
    rdfs:comment "The class of units with dimensionality 'ElectricCurrentPerMass'."@en .

ns1:ElectricDisplacementFieldUnit a owl:Class ;
    rdfs:label "ElectricDisplacementFieldUnit"@en ;
    rdfs:comment "The class of units with dimensionality 'ElectricDisplacementField'."@en .

ns1:ElectricFieldStrengthUnit a owl:Class ;
    rdfs:label "ElectricFieldStrengthUnit"@en ;
    rdfs:comment "The class of units with dimensionality 'ElectricFieldStrength'."@en .

ns1:ElectricInductance a owl:Class ;
    rdfs:label "ElectricInductance"@en ;
    rdfs:comment "A property of an electrical conductor by which a change in current through it induces an electromotive force in both the conductor itself and in any nearby conductors by mutual inductance."@en ;
    rdfs:subClassOf [ a owl:Restriction ;
            owl:onProperty ns1:hasMeasurementUnit ;
            owl:someValuesFrom ns1:InductanceUnit ],
        ns1:ElectromagneticQuantity,
        ns1:ISQDerivedQuantity ;
    skos:altLabel "Inductance"@en ;
    skos:prefLabel "ElectricInductance"@en ;
    ns1:IEVReference "https://www.electropedia.org/iev/iev.nsf/display?openform&ievref=131-12-19"^^xsd:string ;
    ns1:ISO80000Reference "6-41.1"^^xsd:string ;
    ns1:elucidation "A property of an electrical conductor by which a change in current through it induces an electromotive force in both the conductor itself and in any nearby conductors by mutual inductance."@en ;
    ns1:iupacReference "https://doi.org/10.1351/goldbook.M04076"^^xsd:string ;
    ns1:qudtReference "http://qudt.org/vocab/quantitykind/Inductance"^^xsd:string ;
    ns1:wikidataReference "https://www.wikidata.org/wiki/Q177897"^^xsd:string .

ns1:ElectricMobilityUnit a owl:Class ;
    rdfs:label "ElectricMobilityUnit"@en ;
    rdfs:comment "The class of units with dimensionality 'ElectricMobility'."@en .

ns1:ElectricResistanceUnit a owl:Class .

ns1:ElectricResistivity a owl:Class ;
    rdfs:label "ElectricResistivity"@en ;
    rdfs:comment "Electric field strength divided by the current density."@en ;
    rdfs:subClassOf [ a owl:Restriction ;
            owl:onProperty ns1:hasMeasurementUnit ;
            owl:someValuesFrom ns1:ElectricResistivityUnit ],
        ns1:ElectromagneticQuantity,
        ns1:Extensive,
        ns1:ISQDerivedQuantity ;
    skos:altLabel "Resistivity"^^xsd:string ;
    skos:prefLabel "ElectricResistivity"@en ;
    ns1:IEVReference "https://www.electropedia.org/iev/iev.nsf/display?openform&ievref=121-12-04"^^xsd:string ;
    ns1:ISO80000Reference "6-44"^^xsd:string ;
    ns1:elucidation "Electric field strength divided by the current density."@en ;
    ns1:iupacReference "https://doi.org/10.1351/goldbook.R05316"^^xsd:string ;
    ns1:qudtReference "http://qudt.org/vocab/quantitykind/Resistivity"^^xsd:string ;
    ns1:wikidataReference "https://www.wikidata.org/wiki/Q108193"^^xsd:string .

ns1:ElectricResistivityUnit a owl:Class ;
    rdfs:label "ElectricResistivityUnit"@en ;
    rdfs:comment "The class of units with dimensionality 'ElectricResistivity'."@en .

ns1:EnergyDensityOfStatesUnit a owl:Class ;
    rdfs:label "EnergyDensityOfStatesUnit"@en ;
    rdfs:comment "The class of units with dimensionality 'EnergyDensityOfStates'."@en .

ns1:Entropy a owl:Class ;
    rdfs:label "Entropy"@en ;
    rdfs:comment "Logarithmic measure of the number of available states of a system."@en,
        "May also be referred to as a measure of order of  a system."@en ;
    rdfs:subClassOf [ a owl:Restriction ;
            owl:onProperty ns1:hasMeasurementUnit ;
            owl:someValuesFrom ns1:EntropyUnit ],
        ns1:Extensive,
        ns1:ISQDerivedQuantity ;
    skos:prefLabel "Entropy"@en ;
    ns1:ISO80000Reference "5-18"^^xsd:string ;
    ns1:elucidation "Logarithmic measure of the number of available states of a system."@en ;
    ns1:iupacReference "https://doi.org/10.1351/goldbook.E02149"^^xsd:string ;
    ns1:qudtReference "http://qudt.org/vocab/quantitykind/Entropy"^^xsd:string .

ns1:GapEnergy a owl:Class ;
    rdfs:label "GapEnergy"@en ;
    rdfs:comment "Smallest energy difference between the lowest level of conduction band and the highest level of valence band at zero thermodynamic temperature."@en ;
    rdfs:subClassOf ns1:CondensedMatterPhysicsQuantity,
        ns1:Energy ;
    skos:altLabel "BandgapEnergy"@en ;
    skos:prefLabel "GapEnergy"@en ;
    ns1:IEVReference "https://www.electropedia.org/iev/iev.nsf/display?openform&ievref=113-06-16"^^xsd:string ;
    ns1:ISO80000Reference "12-27.2"^^xsd:string ;
    ns1:elucidation "Smallest energy difference between the lowest level of conduction band and the highest level of valence band at zero thermodynamic temperature."@en ;
    ns1:iupacReference "https://doi.org/10.1351/goldbook.B00593"^^xsd:string ;
    ns1:wikidataReference "https://www.wikidata.org/wiki/Q103982939"^^xsd:string .

ns1:GyromagneticRatio a owl:Class ;
    rdfs:label "GyromagneticRatio"^^xsd:string ;
    rdfs:comment "Ratio of magnetic dipole moment to total angular momentum."@en ;
    rdfs:subClassOf [ a owl:Restriction ;
            owl:onProperty ns1:hasMeasurementUnit ;
            owl:someValuesFrom ns1:ElectricChargePerMassUnit ],
        ns1:AtomicAndNuclearPhysicsQuantity,
        ns1:ISQDerivedQuantity ;
    skos:altLabel "GyromagneticCoefficient"@en,
        "MagnetogyricRatio"@en ;
    skos:prefLabel "GyromagneticRatio"^^xsd:string ;
    ns1:ISO80000Reference "10-12.1"^^xsd:string ;
    ns1:elucidation "Ratio of magnetic dipole moment to total angular momentum."@en ;
    ns1:iupacReference "https://doi.org/10.1351/goldbook.M03693"^^xsd:string ;
    ns1:qudtReference "https://qudt.org/vocab/quantitykind/GyromagneticRatio"^^xsd:string ;
    ns1:wikidataReference "https://www.wikidata.org/wiki/Q634552"^^xsd:string .

ns1:Heat a owl:Class ;
    rdfs:label "Heat"@en ;
    rdfs:comment "Heat is energy in transfer to or from a thermodynamic system, by mechanisms other than thermodynamic work or transfer of matter."@en ;
    rdfs:subClassOf ns1:Energy ;
    skos:altLabel "AmountOfHeat"^^xsd:string ;
    skos:prefLabel "Heat"@en ;
    ns1:ISO80000Reference "5-6.1"^^xsd:string ;
    ns1:elucidation "Heat is energy in transfer to or from a thermodynamic system, by mechanisms other than thermodynamic work or transfer of matter."@en ;
    ns1:iupacReference "https://doi.org/10.1351/goldbook.H02752"^^xsd:string ;
    ns1:qudtReference "http://qudt.org/vocab/quantitykind/Heat"^^xsd:string .

ns1:Intensity a owl:Class ;
    rdfs:label "Intensity"@en ;
    rdfs:comment "Power transferred per unit area."@en ;
    rdfs:subClassOf [ a owl:Restriction ;
            owl:onProperty ns1:hasMeasurementUnit ;
            owl:someValuesFrom ns1:PowerDensityUnit ],
        ns1:ISQDerivedQuantity ;
    skos:prefLabel "Intensity"@en ;
    ns1:elucidation "Power transferred per unit area."@en ;
    ns1:wikipediaReference "https://en.wikipedia.org/wiki/Intensity_(physics)"@en .

ns1:JouleThomsonCoefficient a owl:Class ;
    rdfs:label "JouleThomsonCoefficient"@en ;
    rdfs:comment "Change of thermodynamic temperature with respect to pressure in a Joule-Thomson process at constant enthalpy."@en ;
    rdfs:subClassOf [ a owl:Restriction ;
            owl:onProperty ns1:hasMeasurementUnit ;
            owl:someValuesFrom ns1:TemperaturePerPressureUnit ],
        ns1:ISQDerivedQuantity,
        ns1:ThermodynamicalQuantity ;
    skos:prefLabel "JouleThomsonCoefficient"@en ;
    ns1:ISO80000Reference "5-24"^^xsd:string ;
    ns1:elucidation "Change of thermodynamic temperature with respect to pressure in a Joule-Thomson process at constant enthalpy."@en ;
    ns1:wikidataReference "https://www.wikidata.org/wiki/Q93946998"^^xsd:string .

ns1:LatentHeat a owl:Class ;
    rdfs:label "LatentHeat"@en ;
    rdfs:comment "Heat released or absorbed energy during a constant-temperature process."@en ;
    rdfs:subClassOf ns1:Heat,
        ns1:ThermodynamicalQuantity ;
    skos:prefLabel "LatentHeat"@en ;
    ns1:ISO80000Reference "5-6.2"@en ;
    ns1:elucidation "Heat released or absorbed energy during a constant-temperature process."@en ;
    ns1:wikidataReference "https://www.wikidata.org/wiki/Q207721"^^xsd:string .

ns1:LightAndRadiationQuantity a owl:Class ;
    rdfs:label "LightAndRadiationQuantity"@en ;
    rdfs:comment "Quantities categorised according to ISO 80000-7."@en ;
    rdfs:subClassOf ns1:ISO80000Categorised ;
    skos:prefLabel "LightAndRadiationQuantity"@en ;
    ns1:elucidation "Quantities categorised according to ISO 80000-7."@en .

ns1:LinearExpansionCoefficient a owl:Class ;
    rdfs:label "LinearExpansionCoefficient"@en ;
    rdfs:comment "Relative change of length per change of temperature."@en ;
    rdfs:subClassOf ns1:CoefficientOfThermalExpansion,
        ns1:ThermodynamicalQuantity ;
    skos:prefLabel "LinearExpansionCoefficient"@en ;
    ns1:IEVReference "https://www.electropedia.org/iev/iev.nsf/display?openform&ievref=113-04-27"^^xsd:string ;
    ns1:ISO80000Reference "5-3.1"^^xsd:string ;
    ns1:elucidation "Relative change of length per change of temperature."@en ;
    ns1:qudtReference "https://qudt.org/vocab/quantitykind/LinearExpansionCoefficient"^^xsd:string ;
    ns1:wikidataReference "https://www.wikidata.org/wiki/Q74760821"^^xsd:string .

ns1:LorenzNumberUnit a owl:Class ;
    rdfs:label "LorenzNumberUnit"@en ;
    rdfs:comment "The class of units with dimensionality 'LorenzNumber'."@en .

ns1:LowerCriticalMagneticFluxDensity a owl:Class ;
    rdfs:label "LowerCriticalMagneticFluxDensity"@en ;
    rdfs:comment "For type II superconductors, the threshold magnetic flux density for magnetic flux entering the superconductor."@en ;
    rdfs:subClassOf ns1:CondensedMatterPhysicsQuantity,
        ns1:MagneticFluxDensity ;
    skos:prefLabel "LowerCriticalMagneticFluxDensity"@en ;
    ns1:ISO80000Reference "12-36.2"^^xsd:string ;
    ns1:elucidation "For type II superconductors, the threshold magnetic flux density for magnetic flux entering the superconductor."@en ;
    ns1:qudtReference "https://qudt.org/vocab/quantitykind/LowerCriticalMagneticFluxDensity"^^xsd:string ;
    ns1:wikidataReference "https://www.wikidata.org/wiki/Q106127355"^^xsd:string .

ns1:LuminousIntensity a owl:Class ;
    rdfs:label "LuminousIntensity"@en ;
    rdfs:comment "A measure of the wavelength-weighted power emitted by a light source in a particular direction per unit solid angle. It is based on the luminosity function, which is a standardized model of the sensitivity of the human eye."@en ;
    rdfs:subClassOf [ a owl:Restriction ;
            owl:onProperty ns1:hasMeasurementUnit ;
            owl:someValuesFrom ns1:LuminousIntensityUnit ],
        ns1:LightAndRadiationQuantity ;
    skos:prefLabel "LuminousIntensity"@en ;
    ns1:ISO80000Reference "7-14"^^xsd:string ;
    ns1:elucidation "A measure of the wavelength-weighted power emitted by a light source in a particular direction per unit solid angle. It is based on the luminosity function, which is a standardized model of the sensitivity of the human eye."@en ;
    ns1:qudtReference "http://qudt.org/vocab/quantitykind/LuminousIntensity"^^xsd:string .

ns1:MagneticFlux a owl:Class ;
    rdfs:label "MagneticFlux"@en ;
    rdfs:comment "Measure of magnetism, taking account of the strength and the extent of a magnetic field."@en ;
    rdfs:subClassOf [ a owl:Restriction ;
            owl:onProperty ns1:hasMeasurementUnit ;
            owl:someValuesFrom ns1:MagneticFluxUnit ],
        ns1:ElectromagneticQuantity,
        ns1:ISQDerivedQuantity ;
    skos:prefLabel "MagneticFlux"@en ;
    ns1:IEVReference "https://www.electropedia.org/iev/iev.nsf/display?openform&ievref=121-11-21"^^xsd:string ;
    ns1:ISO80000Reference "6-22.1"^^xsd:string ;
    ns1:dbpediaReference "https://dbpedia.org/page/Magnetic_flux"^^xsd:string ;
    ns1:elucidation "Measure of magnetism, taking account of the strength and the extent of a magnetic field."@en ;
    ns1:iupacReference "https://doi.org/10.1351/goldbook.M03684"^^xsd:string ;
    ns1:qudtReference "http://qudt.org/vocab/quantitykind/MagneticFlux"^^xsd:string ;
    ns1:wikidataReference "https://www.wikidata.org/wiki/Q177831"^^xsd:string ;
    ns1:wikipediaReference "https://en.wikipedia.org/wiki/Magnetic_flux"^^xsd:string .

ns1:MagneticFluxDensityUnit a owl:Class .

ns1:MagneticFluxUnit a owl:Class .

ns1:MagneticPotentialUnit a owl:Class ;
    rdfs:label "MagneticPotentialUnit"@en ;
    rdfs:comment "The class of units with dimensionality 'MagneticPotential'."@en .

ns1:MagneticReluctanceUnit a owl:Class ;
    rdfs:label "MagneticReluctanceUnit"@en ;
    rdfs:comment "The class of units with dimensionality 'MagneticReluctance'."@en .

ns1:MassAreaUnit a owl:Class ;
    rdfs:label "MassAreaUnit"@en ;
    rdfs:comment "The class of units with dimensionality 'MassArea'."@en .

ns1:MassFluxUnit a owl:Class ;
    rdfs:label "MassFluxUnit"@en ;
    rdfs:comment "The class of units with dimensionality 'MassFlux'."@en .

ns1:MassPerAmountUnit a owl:Class ;
    rdfs:label "MassPerAmountUnit"@en ;
    rdfs:comment "The class of units with dimensionality 'MassPerAmount'."@en .

ns1:MassPerLengthTimeUnit a owl:Class ;
    rdfs:label "MassPerLengthTimeUnit"@en ;
    rdfs:comment "The class of units with dimensionality 'MassPerLengthTime'."@en .

ns1:MassPerLengthUnit a owl:Class ;
    rdfs:label "MassPerLengthUnit"@en ;
    rdfs:comment "The class of units with dimensionality 'MassPerLength'."@en .

ns1:MassPerTimeUnit a owl:Class ;
    rdfs:label "MassPerTimeUnit"@en ;
    rdfs:comment "The class of units with dimensionality 'MassPerTime'."@en .

ns1:MassStoppingPowerUnit a owl:Class ;
    rdfs:label "MassStoppingPowerUnit"@en ;
    rdfs:comment "The class of units with dimensionality 'MassStoppingPower'."@en .

ns1:MolecularConcentration a owl:Class ;
    rdfs:label "MolecularConcentration"@en ;
    rdfs:comment "Number of molecules of a substance in a mixture per volume."@en ;
    rdfs:subClassOf [ a owl:Restriction ;
            owl:onProperty ns1:hasMeasurementUnit ;
            owl:someValuesFrom ns1:PerVolumeUnit ],
        ns1:Concentration,
        ns1:ISQDerivedQuantity,
        ns1:PhysioChemicalQuantity ;
    skos:prefLabel "MolecularConcentration"@en ;
    ns1:ISO80000Reference "9-9.2"^^xsd:string ;
    ns1:elucidation "Number of molecules of a substance in a mixture per volume."@en ;
    ns1:qudtReference "https://qudt.org/vocab/quantitykind/MolecularConcentration"^^xsd:string ;
    ns1:wikidataReference "https://www.wikidata.org/wiki/Q88865973"^^xsd:string .

ns1:PH a owl:Class ;
    rdfs:label "PH"@en ;
    rdfs:comment """At about 25 °C aqueous solutions with:
pH < 7 are acidic;
pH = 7 are neutral;
pH > 7 are alkaline.
At temperatures far from 25 °C the pH of a neutral solution differs significantly from 7."""@en,
        """Number quantifying the acidic or the alkaline character of a solution, equal to the negative of the decimal logarithm of ion activity aH+ of the hydrogen cation H+
pH = −10 log(a_H+)."""@en,
        "Written as pH"@en ;
    rdfs:subClassOf ns1:IonActivity ;
    skos:prefLabel "PH"@en ;
    ns1:IEVReference "https://www.electropedia.org/iev/iev.nsf/display?openform&ievref=114-01-21"@en ;
    ns1:ISO80000Reference "For more details, see ISO 80000-9:2009, Annex C"@en ;
    ns1:elucidation """Number quantifying the acidic or the alkaline character of a solution, equal to the negative of the decimal logarithm of ion activity aH+ of the hydrogen cation H+
pH = −10 log(a_H+)."""@en ;
    ns1:iupacReference "https://doi.org/10.1351/goldbook.P04524"^^xsd:string .

ns1:ParticleNumberDensity a owl:Class ;
    rdfs:label "ParticleNumberDensity"@en ;
    rdfs:comment "Mean number of particles per volume."@en ;
    rdfs:subClassOf [ a owl:Restriction ;
            owl:onProperty ns1:hasMeasurementUnit ;
            owl:someValuesFrom ns1:PerVolumeUnit ],
        ns1:AtomicAndNuclearPhysicsQuantity,
        ns1:ISQDerivedQuantity ;
    skos:prefLabel "ParticleNumberDensity"@en ;
    ns1:ISO80000Reference "10-62.1"^^xsd:string ;
    ns1:elucidation "Mean number of particles per volume."@en ;
    ns1:iupacReference "https://doi.org/10.1351/goldbook.N04262"^^xsd:string ;
    ns1:qudtReference "https://qudt.org/vocab/quantitykind/ParticleNumberDensity"^^xsd:string ;
    ns1:wikidataReference "https://www.wikidata.org/wiki/Q98601569"^^xsd:string .

ns1:PathLength a owl:Class ;
    rdfs:label "PathLength"@en ;
    rdfs:comment "Length of a rectifiable curve between two of its points."@en ;
    rdfs:subClassOf ns1:Length ;
    skos:altLabel "ArcLength"@en ;
    skos:prefLabel "PathLength"@en ;
    ns1:ISO80000Reference "3-1.7"^^xsd:string ;
    ns1:dbpediaReference "https://dbpedia.org/page/Arc_length"^^xsd:string ;
    ns1:elucidation "Length of a rectifiable curve between two of its points."@en ;
    ns1:wikidataReference "https://www.wikidata.org/wiki/Q7144654"^^xsd:string ;
    ns1:wikipediaReference "https://en.wikipedia.org/wiki/Arc_length"^^xsd:string .

ns1:PerAreaUnit a owl:Class ;
    rdfs:label "PerAreaUnit"@en ;
    rdfs:comment "The class of units with dimensionality 'PerArea'."@en .

ns1:PerPressureUnit a owl:Class ;
    rdfs:label "PerPressureUnit"@en ;
    rdfs:comment "The class of units with dimensionality 'PerPressure'."@en .

ns1:PerThermalTransmittanceUnit a owl:Class ;
    rdfs:label "PerThermalTransmittanceUnit"@en ;
    rdfs:comment "The class of units with dimensionality 'PerThermalTransmittance'."@en .

ns1:PerTimeMassUnit a owl:Class ;
    rdfs:label "PerTimeMassUnit"@en ;
    rdfs:comment "The class of units with dimensionality 'PerTimeMass'."@en .

ns1:Permeability a owl:Class ;
    rdfs:label "Permeability"@en ;
    rdfs:comment "Measure for how the magnetization of material is affected by the application of an external magnetic field ."@en ;
    rdfs:subClassOf [ a owl:Restriction ;
            owl:onProperty ns1:hasMeasurementUnit ;
            owl:someValuesFrom ns1:PermeabilityUnit ],
        ns1:ElectromagneticQuantity,
        ns1:ISQDerivedQuantity,
        ns1:Intensive ;
    skos:altLabel "ElectromagneticPermeability"^^xsd:string ;
    skos:prefLabel "Permeability"@en ;
    ns1:ISO80000Reference "6-26.2"^^xsd:string ;
    ns1:elucidation "Measure for how the magnetization of material is affected by the application of an external magnetic field ."@en ;
    ns1:iupacReference "https://doi.org/10.1351/goldbook.P04503"^^xsd:string ;
    ns1:qudtReference "http://qudt.org/vocab/quantitykind/ElectromagneticPermeability"^^xsd:string .

ns1:Permittivity a owl:Class ;
    rdfs:label "Permittivity"@en ;
    rdfs:comment "Measure for how the polarization of a material is affected by the application of an external electric field."@en ;
    rdfs:subClassOf [ a owl:Restriction ;
            owl:onProperty ns1:hasMeasurementUnit ;
            owl:someValuesFrom ns1:PermittivityUnit ],
        ns1:ElectromagneticQuantity,
        ns1:ISQDerivedQuantity,
        ns1:Intensive ;
    skos:prefLabel "Permittivity"@en ;
    ns1:ISO80000Reference "6-14.1"^^xsd:string,
        "6-14.2"^^xsd:string ;
    ns1:elucidation "Measure for how the polarization of a material is affected by the application of an external electric field."@en ;
    ns1:iupacReference "https://doi.org/10.1351/goldbook.P04507"^^xsd:string ;
    ns1:qudtReference "http://qudt.org/vocab/quantitykind/Permittivity"^^xsd:string .

ns1:PowerUnit a owl:Class .

ns1:PressureCoefficient a owl:Class ;
    rdfs:label "PressureCoefficient"@en ;
    rdfs:comment "Change of pressure per change of temperature at constant volume."@en ;
    rdfs:subClassOf [ a owl:Restriction ;
            owl:onProperty ns1:hasMeasurementUnit ;
            owl:someValuesFrom ns1:PressurePerTemperatureUnit ],
        ns1:ISQDerivedQuantity,
        ns1:ThermodynamicalQuantity ;
    skos:prefLabel "PressureCoefficient"@en ;
    ns1:IEVReference "https://www.electropedia.org/iev/iev.nsf/display?openform&ievref=113-04-29"^^xsd:string ;
    ns1:ISO80000Reference "5-4"^^xsd:string ;
    ns1:elucidation "Change of pressure per change of temperature at constant volume."@en ;
    ns1:qudtReference "https://qudt.org/vocab/quantitykind/PressureCoefficient"^^xsd:string ;
    ns1:wikidataReference "https://www.wikidata.org/wiki/Q74762732"^^xsd:string .

ns1:PressurePerTemperatureUnit a owl:Class ;
    rdfs:label "PressurePerTemperatureUnit"@en ;
    rdfs:comment "The class of units with dimensionality 'PressurePerTemperature'."@en .

ns1:RadialDistance a owl:Class ;
    rdfs:label "RadialDistance"@en ;
    rdfs:comment "Distance, where one point is located on an axis or within a closed non self-intersecting curve or surface."@en ;
    rdfs:subClassOf ns1:Distance ;
    skos:prefLabel "RadialDistance"@en ;
    ns1:IEVReference "https://www.electropedia.org/iev/iev.nsf/display?openform&ievref=113-01-26"^^xsd:string ;
    ns1:ISO80000Reference "3-1.9"^^xsd:string ;
    ns1:elucidation "Distance, where one point is located on an axis or within a closed non self-intersecting curve or surface."@en ;
    ns1:qudtReference "https://qudt.org/vocab/quantitykind/RadialDistance"^^xsd:string ;
    ns1:wikidataReference "https://www.wikidata.org/wiki/Q1578234"^^xsd:string .

ns1:ReciprocalDuration a owl:Class ;
    rdfs:label "ReciprocalDuration"@en ;
    rdfs:comment "A quantity defined as the inverse of time."@en ;
    rdfs:subClassOf [ a owl:Restriction ;
            owl:onProperty ns1:hasMeasurementUnit ;
            owl:someValuesFrom ns1:FrequencyUnit ],
        ns1:ISQDerivedQuantity ;
    skos:altLabel "InverseDuration"@en,
        "InverseTime"@en,
        "ReciprocalTime"@en ;
    skos:example "Frequency or rate."@en ;
    skos:prefLabel "ReciprocalDuration"@en ;
    ns1:elucidation "A quantity defined as the inverse of time."@en ;
    ns1:qudtReference "https://qudt.org/vocab/quantitykind/InverseTime"@en ;
    ns1:wikidataReference "https://www.wikidata.org/wiki/Q98690850"@en .

ns1:ReciprocalElectricChargeDensityUnit a owl:Class ;
    rdfs:label "ReciprocalElectricChargeDensityUnit"@en ;
    rdfs:comment "The class of units with dimensionality 'ReciprocalElectricChargeDensity'."@en .

ns1:RelativeMassConcentrationOfWaterVapour a owl:Class ;
    rdfs:label "RelativeMassConcentrationOfWaterVapour"@en ;
    rdfs:comment "For normal cases, the relative humidity may be assumed to be equal to relative mass concentration of vapour."@en,
        "Ratio of the mass concentration of water vapour v to its mass concentration at saturation vsat, at the same temperature, thus ψ = v/vsat."@en ;
    rdfs:subClassOf ns1:RatioQuantity,
        ns1:ThermodynamicalQuantity ;
    skos:prefLabel "RelativeMassConcentrationOfWaterVapour"@en ;
    ns1:IEVReference "https://www.electropedia.org/iev/iev.nsf/display?openform&ievref=113-04-66"^^xsd:string ;
    ns1:elucidation "Ratio of the mass concentration of water vapour v to its mass concentration at saturation vsat, at the same temperature, thus ψ = v/vsat."@en ;
    ns1:qudtReference "https://qudt.org/vocab/quantitykind/RelativeMassConcentrationOfVapour"^^xsd:string ;
    ns1:wikidataReference "https://www.wikidata.org/wiki/Q76379357"^^xsd:string .

ns1:RestMass a owl:Class ;
    rdfs:label "RestMass"@en ;
    rdfs:comment "For particle X, mass of that particle at rest in an inertial frame."@en ;
    rdfs:subClassOf ns1:AtomicAndNuclearPhysicsQuantity,
        ns1:Mass ;
    skos:altLabel "InvariantMass"@en,
        "ProperMass"@en ;
    skos:prefLabel "RestMass"@en ;
    ns1:IEVReference "https://www.electropedia.org/iev/iev.nsf/display?openform&ievref=395-01-03"^^xsd:string,
        "https://www.electropedia.org/iev/iev.nsf/display?openform&ievref=881-04-16"^^xsd:string ;
    ns1:ISO80000Reference "10-2"^^xsd:string ;
    ns1:dbpediaReference "https://dbpedia.org/page/Mass_in_special_relativity"^^xsd:string ;
    ns1:elucidation "For particle X, mass of that particle at rest in an inertial frame."@en ;
    ns1:qudtReference "https://qudt.org/vocab/quantitykind/RestMass"^^xsd:string ;
    ns1:wikidataReference "https://www.wikidata.org/wiki/Q96941619"^^xsd:string ;
    ns1:wikipediaReference "https://en.wikipedia.org/wiki/Invariant_mass"^^xsd:string .

ns1:RichardsonConstantUnit a owl:Class ;
    rdfs:label "RichardsonConstantUnit"@en ;
    rdfs:comment "The class of units with dimensionality 'RichardsonConstant'."@en .

ns1:RollingResistanceFactor a owl:Class ;
    rdfs:label "RollingResistanceFactor"@en ;
    rdfs:comment "Quotient of tangential and normal component of the force applied to a body which is rolling at constant speed over a surface."@en ;
    rdfs:subClassOf ns1:MechanicalQuantity,
        ns1:RatioQuantity ;
    skos:prefLabel "RollingResistanceFactor"@en ;
    ns1:ISO80000Reference "4-23.3"^^xsd:string ;
    ns1:elucidation "Quotient of tangential and normal component of the force applied to a body which is rolling at constant speed over a surface."@en ;
    ns1:wikidataReference "https://www.wikidata.org/wiki/Q91738044"^^xsd:string .

ns1:SecondAxialMomentOfArea a owl:Class ;
    rdfs:label "SecondAxialMomentOfArea"@en ;
    rdfs:comment "A geometrical property of an area which reflects how its points are distributed with regard to an arbitrary axis."@en ;
    rdfs:subClassOf [ a owl:Restriction ;
            owl:onProperty ns1:hasMeasurementUnit ;
            owl:someValuesFrom ns1:QuarticLengthUnit ],
        ns1:ISQDerivedQuantity,
        ns1:MechanicalQuantity ;
    skos:prefLabel "SecondAxialMomentOfArea"@en ;
    ns1:IEVReference "https://www.electropedia.org/iev/iev.nsf/display?openform&ievref=113-03-29"^^xsd:string ;
    ns1:ISO80000Reference "4-21.1"^^xsd:string ;
    ns1:elucidation "A geometrical property of an area which reflects how its points are distributed with regard to an arbitrary axis."@en ;
    ns1:qudtReference "https://qudt.org/vocab/quantitykind/SecondAxialMomentOfArea"^^xsd:string ;
    ns1:wikidataReference "https://www.wikidata.org/wiki/Q91405496"^^xsd:string .

ns1:SpecificEnergyImparted a owl:Class ;
    rdfs:label "SpecificEnergyImparted"@en ;
    rdfs:comment "In nuclear physics, energy imparted per mass."@en ;
    rdfs:subClassOf ns1:AtomicAndNuclearPhysicsQuantity,
        ns1:SpecificEnergy ;
    skos:prefLabel "SpecificEnergyImparted"@en ;
    ns1:ISO80000Reference "10-81.2"^^xsd:string ;
    ns1:elucidation "In nuclear physics, energy imparted per mass."@en ;
    ns1:qudtReference "https://qudt.org/vocab/quantitykind/SpecificEnergyImparted"^^xsd:string ;
    ns1:wikidataReference "https://www.wikidata.org/wiki/Q99566195"^^xsd:string .

ns1:SpecificGasConstant a owl:Class ;
    rdfs:label "SpecificGasConstant"@en ;
    rdfs:comment "Quotient of the Boltzmann constant and the mass m."@en ;
    rdfs:subClassOf [ a owl:Restriction ;
            owl:onProperty ns1:hasMeasurementUnit ;
            owl:someValuesFrom ns1:EntropyPerMassUnit ],
        ns1:ISQDerivedQuantity,
        ns1:ThermodynamicalQuantity ;
    skos:prefLabel "SpecificGasConstant"@en ;
    ns1:ISO80000Reference "5-26"^^xsd:string ;
    ns1:elucidation "Quotient of the Boltzmann constant and the mass m."@en ;
    ns1:wikidataReference "https://www.wikidata.org/wiki/Q94372268"^^xsd:string .

ns1:SpecificHeatCapacity a owl:Class ;
    rdfs:label "SpecificHeatCapacity"@en ;
    rdfs:comment "Heat capacity divided by mass."@en ;
    rdfs:subClassOf [ a owl:Restriction ;
            owl:onProperty ns1:hasMeasurementUnit ;
            owl:someValuesFrom ns1:EntropyPerMassUnit ],
        ns1:ISQDerivedQuantity,
        ns1:Intensive,
        ns1:ThermodynamicalQuantity ;
    skos:prefLabel "SpecificHeatCapacity"@en ;
    ns1:IEVReference "https://www.electropedia.org/iev/iev.nsf/display?openform&ievref=113-04-48"^^xsd:string ;
    ns1:ISO80000Reference "5-16.1"^^xsd:string ;
    ns1:dbpediaReference "https://dbpedia.org/page/Specific_heat_capacity"^^xsd:string ;
    ns1:elucidation "Heat capacity divided by mass."@en ;
    ns1:iupacReference "https://doi.org/10.1351/goldbook.S05800"^^xsd:string ;
    ns1:qudtReference "https://qudt.org/vocab/quantitykind/SpecificHeatCapacity"^^xsd:string ;
    ns1:wikidataReference "https://www.wikidata.org/wiki/Q487756"^^xsd:string ;
    ns1:wikipediaReference "https://en.wikipedia.org/wiki/Specific_heat_capacity"^^xsd:string .

ns1:SquareTimePerMassUnit a owl:Class ;
    rdfs:label "SquareTimePerMassUnit"@en ;
    rdfs:comment "The class of units with dimensionality 'SquareTimePerMass'."@en .

ns1:TemperaturePerPressureUnit a owl:Class ;
    rdfs:label "TemperaturePerPressureUnit"@en ;
    rdfs:comment "The class of units with dimensionality 'TemperaturePerPressure'."@en .

ns1:ThermalConductanceUnit a owl:Class ;
    rdfs:label "ThermalConductanceUnit"@en ;
    rdfs:comment "The class of units with dimensionality 'ThermalConductance'."@en .

ns1:ThermalConductivityUnit a owl:Class ;
    rdfs:label "ThermalConductivityUnit"@en ;
    rdfs:comment "The class of units with dimensionality 'ThermalConductivity'."@en .

ns1:ThermalResistanceUnit a owl:Class ;
    rdfs:label "ThermalResistanceUnit"@en ;
    rdfs:comment "The class of units with dimensionality 'ThermalResistance'."@en .

ns1:ThermalTransmittanceUnit a owl:Class ;
    rdfs:label "ThermalTransmittanceUnit"@en ;
    rdfs:comment "The class of units with dimensionality 'ThermalTransmittance'."@en .

ns1:Thickness a owl:Class ;
    rdfs:label "Thickness"@en ;
    rdfs:comment "Shortest distance between two surfaces limiting a layer, when this distance can be considered to be constant over a region of a finite size."@en ;
    rdfs:subClassOf ns1:Length ;
    skos:prefLabel "Thickness"@en ;
    ns1:IEVReference "https://www.electropedia.org/iev/iev.nsf/display?openform&ievref=113-01-24"@en ;
    ns1:ISO80000Reference "3-1.4"^^xsd:string ;
    ns1:elucidation "Shortest distance between two surfaces limiting a layer, when this distance can be considered to be constant over a region of a finite size."@en ;
    ns1:wikidataReference "https://www.wikidata.org/wiki/Q3589038"^^xsd:string .

ns1:TimePerVolumeUnit a owl:Class ;
    rdfs:label "TimePerVolumeUnit"@en ;
    rdfs:comment "The class of units with dimensionality 'TimePerVolume'."@en .

ns1:TimeUnit a owl:Class .

ns1:UpperCriticalMagneticFluxDensity a owl:Class ;
    rdfs:label "UpperCriticalMagneticFluxDensity"@en ;
    rdfs:comment "For type II superconductors, the threshold magnetic flux density for disappearance of bulk superconductivity."@en ;
    rdfs:subClassOf ns1:CondensedMatterPhysicsQuantity,
        ns1:MagneticFluxDensity ;
    skos:prefLabel "UpperCriticalMagneticFluxDensity"@en ;
    ns1:ISO80000Reference "12-36.3"^^xsd:string ;
    ns1:elucidation "For type II superconductors, the threshold magnetic flux density for disappearance of bulk superconductivity."@en ;
    ns1:qudtReference "https://qudt.org/vocab/quantitykind/UpperCriticalMagneticFluxDensity"^^xsd:string ;
    ns1:wikidataReference "https://www.wikidata.org/wiki/Q106127634"^^xsd:string .

ns1:VolumePerAmountUnit a owl:Class ;
    rdfs:label "VolumePerAmountUnit"@en ;
    rdfs:comment "The class of units with dimensionality 'VolumePerAmount'."@en .

ns1:VolumePerMassUnit a owl:Class ;
    rdfs:label "VolumePerMassUnit"@en ;
    rdfs:comment "The class of units with dimensionality 'VolumePerMass'."@en .

ns1:Wavelength a owl:Class ;
    rdfs:label "Wavelength"@en ;
    rdfs:comment "Length of the repetition interval of a wave."@en ;
    rdfs:subClassOf ns1:Length ;
    skos:prefLabel "Wavelength"@en ;
    ns1:IEVReference "https://www.electropedia.org/iev/iev.nsf/display?openform&ievref=103-10-10"^^xsd:string ;
    ns1:ISO80000Reference "3-19"^^xsd:string ;
    ns1:dbpediaReference "https://dbpedia.org/page/Wavelength"^^xsd:string ;
    ns1:elucidation "Length of the repetition interval of a wave."@en ;
    ns1:iupacReference "https://doi.org/10.1351/goldbook.W06659"^^xsd:string ;
    ns1:qudtReference "https://qudt.org/vocab/quantitykind/Wavelength"^^xsd:string ;
    ns1:wikidataReference "https://www.wikidata.org/wiki/Q41364"^^xsd:string ;
    ns1:wikipediaReference "https://en.wikipedia.org/wiki/Wavelength"^^xsd:string .

ns1:AmountPerMassUnit a owl:Class ;
    rdfs:label "AmountPerMassUnit"@en ;
    rdfs:comment "The class of units with dimensionality 'AmountPerMass'."@en .

ns1:AmountUnit a owl:Class .

ns1:Area a owl:Class ;
    rdfs:label "Area"@en ;
    rdfs:comment "Extent of a surface."@en ;
    rdfs:subClassOf [ a owl:Restriction ;
            owl:onProperty ns1:hasMeasurementUnit ;
            owl:someValuesFrom ns1:AreaUnit ],
        ns1:Extensive,
        ns1:ISQDerivedQuantity,
        ns1:SpaceAndTimeQuantity ;
    skos:prefLabel "Area"@en ;
    ns1:ISO80000Reference "3-3"^^xsd:string ;
    ns1:elucidation "Extent of a surface."@en ;
    ns1:iupacReference "https://doi.org/10.1351/goldbook.A00429"^^xsd:string ;
    ns1:qudtReference "http://qudt.org/vocab/quantitykind/Area"^^xsd:string .

ns1:AreaPerMassUnit a owl:Class ;
    rdfs:label "AreaPerMassUnit"@en ;
    rdfs:comment "The class of units with dimensionality 'AreaPerMass'."@en .

ns1:AreicSpeedUnit a owl:Class ;
    rdfs:label "AreicSpeedUnit"@en ;
    rdfs:comment "The class of units with dimensionality 'AreicSpeed'."@en .

ns1:CoefficientOfFriction a owl:Class ;
    rdfs:label "CoefficientOfFriction"@en ;
    rdfs:comment "Dimensionless scalar value which describes the ratio of the force of friction between two bodies and the force pressing them together; depends on the materials used, ranges from near zero to greater than one."@en ;
    rdfs:subClassOf ns1:ISQDimensionlessQuantity,
        ns1:MechanicalQuantity ;
    skos:altLabel "FrictionCoefficient"@en,
        "FrictionFactor"@en ;
    skos:prefLabel "CoefficientOfFriction"@en ;
    ns1:elucidation "Dimensionless scalar value which describes the ratio of the force of friction between two bodies and the force pressing them together; depends on the materials used, ranges from near zero to greater than one."@en ;
    ns1:iupacReference "https://doi.org/10.1351/goldbook.F02530"^^xsd:string ;
    ns1:wikidataReference "https://www.wikidata.org/wiki/Q1932524"^^xsd:string .

ns1:CoefficientOfThermalExpansion a owl:Class ;
    rdfs:label "CoefficientOfThermalExpansion"@en ;
    rdfs:comment "Material property which describes how the size of an object changes with a change in temperature."@en ;
    rdfs:subClassOf [ a owl:Restriction ;
            owl:onProperty ns1:hasMeasurementUnit ;
            owl:someValuesFrom ns1:PerTemperatureUnit ],
        ns1:ThermodynamicalQuantity ;
    skos:altLabel "ThermalExpansionCoefficient"@en ;
    skos:prefLabel "CoefficientOfThermalExpansion"@en ;
    ns1:elucidation "Material property which describes how the size of an object changes with a change in temperature."@en ;
    ns1:wikidataReference "https://www.wikidata.org/wiki/Q45760"^^xsd:string .

ns1:Compressibility a owl:Class ;
    rdfs:label "Compressibility"@en ;
    rdfs:comment "Measure of the relative volume change of a fluid or solid as a response to a pressure change."@en ;
    rdfs:subClassOf [ a owl:Restriction ;
            owl:onProperty ns1:hasMeasurementUnit ;
            owl:someValuesFrom ns1:PerPressureUnit ],
        ns1:ISQDerivedQuantity,
        ns1:MechanicalQuantity ;
    skos:prefLabel "Compressibility"@en ;
    ns1:IEVReference "https://www.electropedia.org/iev/iev.nsf/display?openform&ievref=113-03-70"^^xsd:string ;
    ns1:ISO80000Reference "4-20"^^xsd:string ;
    ns1:elucidation "Measure of the relative volume change of a fluid or solid as a response to a pressure change."@en ;
    ns1:qudtReference "https://qudt.org/vocab/quantitykind/Compressibility"^^xsd:string ;
    ns1:wikidataReference "https://www.wikidata.org/wiki/Q8067817"^^xsd:string .

ns1:DiffusionCoefficient a owl:Class ;
    rdfs:label "DiffusionCoefficient"@en ;
    rdfs:comment "Proportionality constant in some physical laws."@en ;
    rdfs:subClassOf [ a owl:Restriction ;
            owl:onProperty ns1:hasMeasurementUnit ;
            owl:someValuesFrom ns1:AreaPerTimeUnit ],
        ns1:ISQDerivedQuantity ;
    owl:disjointWith ns1:ThermalDiffusionRatio ;
    skos:prefLabel "DiffusionCoefficient"@en ;
    ns1:elucidation "Proportionality constant in some physical laws."@en .

ns1:Distance a owl:Class ;
    rdfs:label "Distance"@en ;
    rdfs:comment "Distance is the norm of Displacement."@en,
        "Shortest path length between two points in a metric space."@en ;
    rdfs:subClassOf ns1:Length ;
    skos:prefLabel "Distance"@en ;
    ns1:IEVReference "https://www.electropedia.org/iev/iev.nsf/display?openform&ievref=102-03-24"^^xsd:string ;
    ns1:ISO80000Reference "3-1.8"^^xsd:string ;
    ns1:dbpediaReference "https://dbpedia.org/page/Distance"^^xsd:string ;
    ns1:elucidation "Shortest path length between two points in a metric space."@en ;
    ns1:qudtReference "https://qudt.org/vocab/quantitykind/Distance"^^xsd:string ;
    ns1:wikidataReference "https://www.wikidata.org/wiki/Q126017"^^xsd:string ;
    ns1:wikipediaReference "https://en.wikipedia.org/wiki/Distance"^^xsd:string .

ns1:ElectricCharge a owl:Class ;
    rdfs:label "ElectricCharge"@en ;
    rdfs:comment "The physical property of matter that causes it to experience a force when placed in an electromagnetic field."@en ;
    rdfs:subClassOf [ a owl:Restriction ;
            owl:onProperty ns1:hasMeasurementUnit ;
            owl:someValuesFrom ns1:ElectricChargeUnit ],
        ns1:ElectromagneticQuantity,
        ns1:Extensive,
        ns1:ISQDerivedQuantity ;
    skos:altLabel "Charge"@en ;
    skos:prefLabel "ElectricCharge"@en ;
    ns1:ISO80000Reference "6-2"^^xsd:string ;
    ns1:elucidation "The physical property of matter that causes it to experience a force when placed in an electromagnetic field."@en ;
    ns1:iupacReference "https://doi.org/10.1351/goldbook.E01923"^^xsd:string ;
    ns1:qudtReference "http://qudt.org/vocab/quantitykind/ElectricCharge"^^xsd:string ;
    ns1:wikidataReference "https://www.wikidata.org/wiki/Q1111"^^xsd:string .

ns1:ElectricChargePerMassUnit a owl:Class ;
    rdfs:label "ElectricChargePerMassUnit"@en ;
    rdfs:comment "The class of units with dimensionality 'ElectricChargePerMass'."@en .

ns1:ElectricChargeUnit a owl:Class .

ns1:ElectricCurrentDensity a owl:Class ;
    rdfs:label "ElectricCurrentDensity"@en ;
    rdfs:comment "Electric current divided by the cross-sectional area it is passing through."@en ;
    rdfs:subClassOf [ a owl:Restriction ;
            owl:onProperty ns1:hasMeasurementUnit ;
            owl:someValuesFrom ns1:ElectricCurrentDensityUnit ],
        ns1:ElectromagneticQuantity,
        ns1:ISQDerivedQuantity,
        ns1:Intensive ;
    skos:altLabel "AreicElectricCurrent"@en,
        "CurrentDensity"@en ;
    skos:prefLabel "ElectricCurrentDensity"@en ;
    ns1:IEVReference "https://www.electropedia.org/iev/iev.nsf/display?openform&ievref=121-11-11"^^xsd:string ;
    ns1:ISO80000Reference "6-8"^^xsd:string ;
    ns1:elucidation "Electric current divided by the cross-sectional area it is passing through."@en ;
    ns1:iupacReference "https://doi.org/10.1351/goldbook.E01928"^^xsd:string ;
    ns1:qudtReference "http://qudt.org/vocab/quantitykind/ElectricCurrentDensity"^^xsd:string ;
    ns1:wikidataReference "https://www.wikidata.org/wiki/Q234072"^^xsd:string ;
    ns1:wikipediaReference "https://en.wikipedia.org/wiki/Current_density"^^xsd:string .

ns1:ElectricFluxDensity a owl:Class ;
    rdfs:label "ElectricFluxDensity"@en ;
    rdfs:comment "Vector quantity obtained at a given point by adding the electric polarization P to the product of the electric field strength E and the electric constant ε0."@en ;
    rdfs:subClassOf [ a owl:Restriction ;
            owl:onProperty ns1:hasMeasurementUnit ;
            owl:someValuesFrom ns1:ElectricDisplacementFieldUnit ],
        ns1:ElectromagneticQuantity,
        ns1:ISQDerivedQuantity ;
    skos:altLabel "ElectricDisplacement"@en ;
    skos:prefLabel "ElectricFluxDensity"@en ;
    ns1:IEVReference "https://www.electropedia.org/iev/iev.nsf/display?openform&ievref=121-11-40"^^xsd:string ;
    ns1:ISO80000Reference "6-12"^^xsd:string ;
    ns1:elucidation "Vector quantity obtained at a given point by adding the electric polarization P to the product of the electric field strength E and the electric constant ε0."@en ;
    ns1:qudtReference "https://qudt.org/vocab/quantitykind/ElectricDisplacementField"@en ;
    ns1:wikidataReference "https://www.wikidata.org/wiki/Q371907"^^xsd:string .

ns1:ElectricPotential a owl:Class ;
    rdfs:label "ElectricPotential"@en ;
    rdfs:comment "Energy required to move a unit charge through an electric field from a reference point."@en,
        "The electric potential is not unique, since any constant scalar field quantity can be added to it without changing its gradient."@en ;
    rdfs:subClassOf [ a owl:Restriction ;
            owl:onProperty ns1:hasMeasurementUnit ;
            owl:someValuesFrom ns1:ElectricPotentialUnit ],
        ns1:ElectromagneticQuantity,
        ns1:Extensive,
        ns1:ISQDerivedQuantity ;
    skos:altLabel "ElectroStaticPotential"@en ;
    skos:prefLabel "ElectricPotential"@en ;
    ns1:IEVReference "https://www.electropedia.org/iev/iev.nsf/display?openform&ievref=121-11-25"^^xsd:string ;
    ns1:ISO80000Reference "6-11.1"^^xsd:string ;
    ns1:dbpediaReference "https://dbpedia.org/page/Electric_potential"^^xsd:string ;
    ns1:elucidation "Energy required to move a unit charge through an electric field from a reference point."@en ;
    ns1:iupacReference "https://doi.org/10.1351/goldbook.E01935"^^xsd:string ;
    ns1:qudtReference "http://qudt.org/vocab/quantitykind/ElectricPotential"^^xsd:string ;
    ns1:wikipediaReference "https://en.wikipedia.org/wiki/Electric_potential"^^xsd:string .

ns1:ElectricPotentialPerTemperatureUnit a owl:Class ;
    rdfs:label "ElectricPotentialPerTemperatureUnit"@en ;
    rdfs:comment "The class of units with dimensionality 'ElectricPotentialPerTemperature'."@en .

ns1:ElectricPotentialUnit a owl:Class .

ns1:EnergyUnit a owl:Class .

ns1:EntropyPerAmountUnit a owl:Class ;
    rdfs:label "EntropyPerAmountUnit"@en ;
    rdfs:comment "The class of units with dimensionality 'EntropyPerAmount'."@en .

ns1:GFactor a owl:Class ;
    rdfs:label "GFactor"@en ;
    rdfs:comment "Relation between observed magnetic moment of a particle and the related unit of magnetic moment."@en ;
    rdfs:subClassOf ns1:AtomicAndNuclearPhysicsQuantity,
        ns1:ISQDimensionlessQuantity ;
    skos:prefLabel "GFactor"@en ;
    ns1:elucidation "Relation between observed magnetic moment of a particle and the related unit of magnetic moment."@en ;
    ns1:wikidataReference "https://www.wikidata.org/wiki/Q1951266"^^xsd:string .

ns1:HeatCapacity a owl:Class ;
    rdfs:label "HeatCapacity"@en ;
    rdfs:comment "Examples of condition might be constant volume or constant pressure for a gas."@en,
        "Quantity C = dQ/dT, when the thermodynamic temperature of a system is increased by dT as a result of the addition of a amount of heat dQ, under given condition."@en ;
    rdfs:subClassOf [ a owl:Restriction ;
            owl:onProperty ns1:hasMeasurementUnit ;
            owl:someValuesFrom ns1:EntropyUnit ],
        ns1:ISQDerivedQuantity,
        ns1:ThermodynamicalQuantity ;
    skos:prefLabel "HeatCapacity"@en ;
    ns1:IEVReference "https://www.electropedia.org/iev/iev.nsf/display?openform&ievref=113-04-47"@en ;
    ns1:ISO80000Reference "5-15"^^xsd:string ;
    ns1:dbpediaReference "https://dbpedia.org/page/Heat_capacity"^^xsd:string ;
    ns1:elucidation "Quantity C = dQ/dT, when the thermodynamic temperature of a system is increased by dT as a result of the addition of a amount of heat dQ, under given condition."@en ;
    ns1:iupacReference "https://doi.org/10.1351/goldbook.H02753"^^xsd:string ;
    ns1:qudtReference "https://qudt.org/vocab/quantitykind/HeatCapacity"^^xsd:string ;
    ns1:wikidataReference "https://www.wikidata.org/wiki/Q179388"^^xsd:string ;
    ns1:wikipediaReference "https://en.wikipedia.org/wiki/Heat_capacity"^^xsd:string .

ns1:InductanceUnit a owl:Class .

ns1:InternationalSystemOfQuantity a owl:Class ;
    rdfs:label "InternationalSystemOfQuantity"@en ;
    rdfs:comment "Quantities declared under the ISO 80000."@en ;
    rdfs:seeAlso "https://www.iso.org/obp/ui/#iso:std:iso:80000:-1:ed-1:v1:en:sec:3.1"^^xsd:string ;
    rdfs:subClassOf ns1:StandardizedPhysicalQuantity ;
    skos:prefLabel "InternationalSystemOfQuantity"@en ;
    ns1:elucidation "Quantities declared under the ISO 80000."@en ;
    ns1:wikipediaReference "https://en.wikipedia.org/wiki/International_System_of_Quantities"^^xsd:string .

ns1:IonActivity a owl:Class ;
    rdfs:label "IonActivity"@en ;
    rdfs:comment "Normally a standard solution is a solution of the ion at a molality of 1 mol/kg (exactly). Standardized conditions are normally 1013,25 hPa and 25 °C."@en,
        "The correction factor is called activity coefficient and it is determined experimentally. See ActivityCoefficient"@en,
        "ratio of the product of ion molality b and a correction factor γ to the molality b° of the same ion in a standard solution under standardized conditions: a = bγ / b°."@en ;
    rdfs:subClassOf ns1:ActivityOfSolute ;
    skos:prefLabel "IonActivity"@en ;
    ns1:IEVReference "https://www.electropedia.org/iev/iev.nsf/display?openform&ievref=114-01-20"@en ;
    ns1:elucidation "ratio of the product of ion molality b and a correction factor γ to the molality b° of the same ion in a standard solution under standardized conditions: a = bγ / b°."@en .

ns1:LuminanceUnit a owl:Class .

ns1:LuminousIntensityUnit a owl:Class .

ns1:MassFraction a owl:Class ;
    rdfs:label "MassFraction"@en ;
    rdfs:comment "Mass of a constituent divided by the total mass of all constituents in the mixture."@en ;
    rdfs:subClassOf ns1:Intensive,
        ns1:RatioQuantity ;
    skos:prefLabel "MassFraction"@en ;
    ns1:ISO80000Reference "9-11"^^xsd:string ;
    ns1:elucidation "Mass of a constituent divided by the total mass of all constituents in the mixture."@en ;
    ns1:iupacReference "https://doi.org/10.1351/goldbook.M03722"^^xsd:string ;
    ns1:qudtReference "http://qudt.org/vocab/quantitykind/MassFraction"^^xsd:string .

ns1:MeanFreePath a owl:Class ;
    rdfs:label "MeanFreePath"@en ;
    rdfs:comment "The mean free path may thus be specified either for all interactions, i.e. total mean free path, or for particular types of interaction such as scattering, capture, or ionization."@en,
        "in a given medium, average distance that particles of a specified type travel between successive interactions of a specified type."@en ;
    rdfs:subClassOf ns1:PathLength,
        ns1:PhysioChemicalQuantity ;
    skos:prefLabel "MeanFreePath"@en ;
    ns1:IEVReference "https://www.electropedia.org/iev/iev.nsf/display?openform&ievref=113-06-37"^^xsd:string ;
    ns1:ISO80000Reference "9-38"^^xsd:string ;
    ns1:elucidation "in a given medium, average distance that particles of a specified type travel between successive interactions of a specified type."@en ;
    ns1:iupacReference "https://doi.org/10.1351/goldbook.M03778"^^xsd:string ;
    ns1:qudtReference "https://qudt.org/vocab/quantitykind/MeanFreePath"^^xsd:string ;
    ns1:wikidataReference "https://www.wikidata.org/wiki/Q756307"^^xsd:string .

ns1:PerTemperatureUnit a owl:Class ;
    rdfs:label "PerTemperatureUnit"@en ;
    rdfs:comment "The class of units with dimensionality 'PerTemperature'."@en .

ns1:PositionVector a owl:Class ;
    rdfs:label "PositionVector"@en ;
    rdfs:comment "Vector quantity from the origin of a coordinate system to a point in space."@en ;
    rdfs:subClassOf [ a owl:Restriction ;
            owl:onProperty ns1:hasMeasurementUnit ;
            owl:someValuesFrom ns1:LengthUnit ],
        ns1:ISQDerivedQuantity,
        ns1:SpaceAndTimeQuantity,
        ns1:Vector ;
    skos:altLabel "Position"@en ;
    skos:prefLabel "PositionVector"@en ;
    ns1:IEVReference "https://www.electropedia.org/iev/iev.nsf/display?openform&ievref=102-03-15"^^xsd:string ;
    ns1:ISO80000Reference "3-1.10"^^xsd:string ;
    ns1:dbpediaReference "https://dbpedia.org/page/Position_(geometry)"^^xsd:string ;
    ns1:elucidation "Vector quantity from the origin of a coordinate system to a point in space."@en ;
    ns1:note """In the usual geometrical three-dimensional space, position vectors are quantities of the dimension length.

-- IEC"""@en,
        """Position vectors are so-called bounded vectors, i.e. their magnitude and direction depend on the particular coordinate system used.

-- ISO 80000-3"""@en ;
    ns1:qudtReference "http://qudt.org/vocab/quantitykind/PositionVector"^^xsd:anyURI ;
    ns1:wikidataReference "https://www.wikidata.org/wiki/Q192388"^^xsd:string ;
    ns1:wikipediaReference "https://en.wikipedia.org/wiki/Position_(geometry)"^^xsd:string .

ns1:Probability a owl:Class ;
    rdfs:label "Probability"@en ;
    rdfs:comment "Probability is a dimensionless quantity that can attain values between 0 and 1; zero denotes the impossible event and 1 denotes a certain event."@en,
        "The propability for a certain outcome, is the ratio between the number of events leading to the given outcome and the total number of events."@en ;
    rdfs:subClassOf ns1:RatioQuantity ;
    skos:prefLabel "Probability"@en ;
    ns1:elucidation "Probability is a dimensionless quantity that can attain values between 0 and 1; zero denotes the impossible event and 1 denotes a certain event."@en ;
    ns1:iupacReference "https://doi.org/10.1351/goldbook.P04855"^^xsd:string .

ns1:QuarticLengthUnit a owl:Class ;
    rdfs:label "QuarticLengthUnit"@en ;
    rdfs:comment "The class of units with dimensionality 'QuarticLength'."@en .

ns1:Rate a owl:Class ;
    rdfs:label "Rate"@en ;
    rdfs:comment "Quotient of a quantity by a duration."@en ;
    rdfs:subClassOf [ a owl:Restriction ;
            owl:onProperty ns1:hasMeasurementUnit ;
            owl:someValuesFrom ns1:FrequencyUnit ],
        ns1:ISQDerivedQuantity,
        ns1:SpaceAndTimeQuantity ;
    skos:example """Activity
Specific absorption rate (SAR)
Rate of rise
Sampling rate
Modulation rate
Fading rate
Rain rate"""@en ;
    skos:prefLabel "Rate"@en ;
    ns1:IEVReference "112-03-18"^^xsd:string ;
    ns1:elucidation "Quotient of a quantity by a duration."@en .

ns1:TemperatureUnit a owl:Class .

ns1:ThermalDiffusionRatio a owl:Class ;
    rdfs:label "ThermalDiffusionRatio"@en ;
    rdfs:comment "In a steady-state of a binary mixture in which thermal diffusion occurs; proportionality factor between gradient of the amount-of-subsstance fraction of the heavier substance B, and negative gradient of the local thermodynamic temperature divided by that temperature."@en ;
    rdfs:subClassOf ns1:ISQDimensionlessQuantity,
        ns1:PhysioChemicalQuantity ;
    skos:prefLabel "ThermalDiffusionRatio"@en ;
    ns1:ISO80000Reference "9-40.1"^^xsd:string ;
    ns1:elucidation "In a steady-state of a binary mixture in which thermal diffusion occurs; proportionality factor between gradient of the amount-of-subsstance fraction of the heavier substance B, and negative gradient of the local thermodynamic temperature divided by that temperature."@en ;
    ns1:qudtReference "https://qudt.org/vocab/quantitykind/ThermalDiffusionRatio"^^xsd:string ;
    ns1:wikidataReference "https://www.wikidata.org/wiki/Q96249433"^^xsd:string .

ns1:Time a owl:Class ;
    rdfs:label "Time"@en ;
    rdfs:comment "One-dimensional subspace of space-time, which is locally orthogonal to space."@en,
        "The indefinite continued progress of existence and events that occur in apparently irreversible succession from the past through the present to the future."@en,
        "Time can be seen as the duration of an event or, more operationally, as \"what clocks read\"."@en ;
    rdfs:subClassOf [ a owl:Restriction ;
            owl:onProperty ns1:hasMeasurementUnit ;
            owl:someValuesFrom ns1:TimeUnit ],
        ns1:SpaceAndTimeQuantity ;
    skos:prefLabel "Time"@en ;
    ns1:ISO80000Reference "3-7"^^xsd:string ;
    ns1:definition "One-dimensional subspace of space-time, which is locally orthogonal to space."@en ;
    ns1:elucidation "The indefinite continued progress of existence and events that occur in apparently irreversible succession from the past through the present to the future."@en ;
    ns1:iupacReference "https://doi.org/10.1351/goldbook.T06375"^^xsd:string ;
    ns1:qudtReference "http://qudt.org/vocab/quantitykind/Time"^^xsd:string .

ns1:TimeConstant a owl:Class ;
    rdfs:label "TimeConstant"@en ;
    rdfs:comment "parameter characterizing the response to a step input of a first‑order, linear time‑invariant system"@en ;
    rdfs:subClassOf ns1:Duration ;
    skos:prefLabel "TimeConstant"@en ;
    ns1:IEVReference "https://www.electropedia.org/iev/iev.nsf/display?openform&ievref=103-05-26"^^xsd:string,
        "https://www.electropedia.org/iev/iev.nsf/display?openform&ievref=351-45-32"^^xsd:string ;
    ns1:ISO80000Reference "3-15"^^xsd:string ;
    ns1:elucidation "parameter characterizing the response to a step input of a first‑order, linear time‑invariant system"@en ;
    ns1:wikidataReference "https://www.wikidata.org/wiki/Q1335249"^^xsd:string .

ns1:Vector rdfs:label "Vector"@en ;
    rdfs:comment "1-dimensional array who's spatial direct parts are numbers."@en .

ns1:Velocity a owl:Class ;
    rdfs:label "Velocity"@en ;
    rdfs:comment """The velocity depends on the choice of the reference frame. Proper transformation between frames must be used: Galilean for non-relativistic description, Lorentzian for relativistic description.

-- IEC, note 2"""@en,
        """The velocity is related to a point described by its position vector. The point may localize a particle, or be attached to any other object such as a body or a wave.

-- IEC, note 1"""@en,
        """Vector quantity giving the rate of change of a position vector.

-- ISO 80000-3"""@en ;
    rdfs:subClassOf [ a owl:Restriction ;
            owl:onProperty ns1:hasMeasurementUnit ;
            owl:someValuesFrom ns1:SpeedUnit ],
        ns1:ISQDerivedQuantity,
        ns1:Intensive,
        ns1:SpaceAndTimeQuantity,
        ns1:Vector ;
    owl:disjointWith ns1:Speed ;
    skos:prefLabel "Velocity"@en ;
    ns1:ISO80000Reference "3-8.1"^^xsd:string,
        "3‑10.1"^^xsd:string ;
    ns1:elucidation """Vector quantity giving the rate of change of a position vector.

-- ISO 80000-3"""@en ;
    ns1:qudtReference "http://qudt.org/vocab/quantitykind/Velocity"^^xsd:string ;
    ns1:wikidataReference "https://www.wikidata.org/wiki/Q11465"^^xsd:string .

ns1:Voltage a owl:Class ;
    rdfs:label "Voltage"@en ;
    rdfs:comment "Correspond to the work needed per unit of charge to move a test charge between two points in a static electric field."@en,
        "The difference in electric potential between two points."@en ;
    rdfs:subClassOf ns1:ElectricPotential ;
    skos:altLabel "ElectricPotentialDifference"@en,
        "ElectricTension"@en ;
    skos:prefLabel "Voltage"@en ;
    ns1:ISO80000Reference "6-11.3"^^xsd:string ;
    ns1:elucidation "The difference in electric potential between two points."@en ;
    ns1:iupacReference "https://doi.org/10.1351/goldbook.A00424"^^xsd:string,
        "https://doi.org/10.1351/goldbook.V06635"@en ;
    ns1:qudtReference "http://qudt.org/vocab/quantitykind/Voltage"@en .

ns1:VolumePerTimeUnit a owl:Class ;
    rdfs:label "VolumePerTimeUnit"@en ;
    rdfs:comment "The class of units with dimensionality 'VolumePerTime'."@en .

ns1:VolumetricNumberDensity a owl:Class ;
    rdfs:label "VolumetricNumberDensity"@en ;
    rdfs:comment "Count per volume."@en ;
    rdfs:subClassOf ns1:ReciprocalVolume ;
    skos:prefLabel "VolumetricNumberDensity"@en ;
    ns1:elucidation "Count per volume."@en .

ns1:Wavenumber a owl:Class ;
    rdfs:label "Wavenumber"@en ;
    rdfs:comment "Reciprocal of the wavelength."@en ;
    rdfs:subClassOf ns1:ReciprocalLength,
        ns1:SpaceAndTimeQuantity ;
    skos:altLabel "Repetency"@en ;
    skos:prefLabel "Wavenumber"@en ;
    ns1:IEVReference "https://www.electropedia.org/iev/iev.nsf/display?openform&ievref=103-10-11"^^xsd:string ;
    ns1:ISO80000Reference "3-18"^^xsd:string ;
    ns1:dbpediaReference "https://dbpedia.org/page/Wavenumber"^^xsd:string ;
    ns1:elucidation "Reciprocal of the wavelength."@en ;
    ns1:iupacReference "https://doi.org/10.1351/goldbook.W06664"^^xsd:string ;
    ns1:note "The number of waves per unit length along the direction of propagation."@en ;
    ns1:qudtReference "https://qudt.org/vocab/quantitykind/Wavenumber"^^xsd:string ;
    ns1:wikidataReference "https://www.wikidata.org/wiki/Q192510"^^xsd:string ;
    ns1:wikipediaReference "https://en.wikipedia.org/wiki/Wavenumber"^^xsd:string .

ns1:AbsoluteActivity a owl:Class ;
    rdfs:label "AbsoluteActivity"@en ;
    rdfs:comment "The exponential of the ratio of the chemical potential to R*T where R is the gas constant and T the thermodynamic temperature."@en ;
    rdfs:subClassOf ns1:ISQDimensionlessQuantity,
        ns1:PhysioChemicalQuantity ;
    skos:prefLabel "AbsoluteActivity"@en ;
    ns1:ISO80000Reference "9-18"^^xsd:string ;
    ns1:elucidation "The exponential of the ratio of the chemical potential to R*T where R is the gas constant and T the thermodynamic temperature."@en ;
    ns1:iupacReference "https://goldbook.iupac.org/terms/view/A00019"^^xsd:string ;
    ns1:qudtReference "https://qudt.org/vocab/quantitykind/AbsoluteActivity"^^xsd:string ;
    ns1:wikidataReference "https://www.wikidata.org/wiki/Q56638155"^^xsd:string .

ns1:AbsorbedDoseUnit a owl:Class .

ns1:AngularMomentum a owl:Class ;
    rdfs:label "AngularMomentum"@en ;
    rdfs:comment "Measure of the extent and direction an object rotates about a reference point."@en ;
    rdfs:subClassOf [ a owl:Restriction ;
            owl:onProperty ns1:hasMeasurementUnit ;
            owl:someValuesFrom ns1:AngularMomentumUnit ],
        ns1:ISQDerivedQuantity,
        ns1:MechanicalQuantity ;
    skos:prefLabel "AngularMomentum"@en ;
    ns1:ISO80000Reference "4-11"^^xsd:string ;
    ns1:elucidation "Measure of the extent and direction an object rotates about a reference point."@en ;
    ns1:iupacReference "https://doi.org/10.1351/goldbook.A00353"^^xsd:string ;
    ns1:qudtReference "http://qudt.org/vocab/quantitykind/AngularMomentum"^^xsd:string .

ns1:CriticalTemperature a owl:Class ;
    rdfs:label "CriticalTemperature"@en ;
    rdfs:comment "Temperature below which quantum effects dominate."@en ;
    rdfs:subClassOf ns1:ThermodynamicTemperature ;
    skos:prefLabel "CriticalTemperature"@en ;
    ns1:elucidation "Temperature below which quantum effects dominate."@en ;
    ns1:wikidataReference "https://www.wikidata.org/wiki/Q1450516"^^xsd:string .

ns1:Displacement a owl:Class ;
    rdfs:label "Displacement"@en ;
    rdfs:comment "vector quantity between any two points in space"@en ;
    rdfs:subClassOf ns1:SpaceAndTimeQuantity ;
    skos:prefLabel "Displacement"@en ;
    ns1:IEVReference "https://www.electropedia.org/iev/iev.nsf/display?openform&ievref=113-01-29"^^xsd:string ;
    ns1:ISO80000Reference "3-1.11"^^xsd:string ;
    ns1:dbpediaReference "https://dbpedia.org/page/Displacement_(geometry)"^^xsd:string ;
    ns1:elucidation "vector quantity between any two points in space"@en ;
    ns1:qudtReference "https://qudt.org/vocab/quantitykind/Displacement"^^xsd:string ;
    ns1:wikidataReference "https://www.wikidata.org/wiki/Q190291"^^xsd:string ;
    ns1:wikipediaReference "https://en.wikipedia.org/wiki/Displacement_(geometry)"^^xsd:string .

ns1:EntropyPerMassUnit a owl:Class ;
    rdfs:label "EntropyPerMassUnit"@en ;
    rdfs:comment "The class of units with dimensionality 'EntropyPerMass'."@en .

ns1:EquilibriumConstant a owl:Class ;
    rdfs:label "EquilibriumConstant"@en ;
    rdfs:comment "The physical dimension can change based on the stoichiometric numbers of the substances involved."@en,
        "for solutions, product for all substances B of concentration c_B of substance B in power of its stoichiometric number v_B: K_p = \\sum_B{c_B^{v_B}}."@en ;
    rdfs:subClassOf ns1:ISQDerivedQuantity,
        ns1:PhysioChemicalQuantity ;
    skos:altLabel "EquilibriumConstantConcentrationBasis"@en ;
    skos:prefLabel "EquilibriumConstant"@en ;
    ns1:elucidation "for solutions, product for all substances B of concentration c_B of substance B in power of its stoichiometric number v_B: K_p = \\sum_B{c_B^{v_B}}."@en ;
    ns1:iupacReference "https://doi.org/10.1351/goldbook.E02177"^^xsd:string ;
    ns1:qudtReference "https://qudt.org/vocab/quantitykind/EquilibriumConstant"^^xsd:string ;
    ns1:wikidataReference "https://www.wikidata.org/wiki/Q857809"^^xsd:string ;
    ns1:wikipediaReference "https://en.wikipedia.org/wiki/Equilibrium_constant"@en .

ns1:ForcePerLengthUnit a owl:Class ;
    rdfs:label "ForcePerLengthUnit"@en ;
    rdfs:comment "The class of units with dimensionality 'ForcePerLength'."@en .

ns1:ForceUnit a owl:Class .

ns1:FrequencyPerVolumeUnit a owl:Class ;
    rdfs:label "FrequencyPerVolumeUnit"@en ;
    rdfs:comment "The class of units with dimensionality 'FrequencyPerVolume'."@en .

ns1:MassConcentration a owl:Class ;
    rdfs:label "MassConcentration"@en ;
    rdfs:comment "Mass of a constituent divided by the volume of the mixture."@en ;
    rdfs:subClassOf ns1:Concentration,
        ns1:Density ;
    skos:prefLabel "MassConcentration"@en ;
    ns1:elucidation "Mass of a constituent divided by the volume of the mixture."@en ;
    ns1:iupacReference "https://doi.org/10.1351/goldbook.M03713"^^xsd:string ;
    ns1:qudtReference "http://qudt.org/vocab/quantitykind/MassConcentration"^^xsd:string .

ns1:MassUnit a owl:Class .

ns1:PerAreaTimeUnit a owl:Class ;
    rdfs:label "PerAreaTimeUnit"@en ;
    rdfs:comment "The class of units with dimensionality 'PerAreaTime'."@en .

ns1:PowerDensityUnit a owl:Class ;
    rdfs:label "PowerDensityUnit"@en ;
    rdfs:comment "The class of units with dimensionality 'PowerDensity'."@en .

ns1:Pressure a owl:Class ;
    rdfs:label "Pressure"@en ;
    rdfs:comment "The force applied perpendicular to the surface of an object per unit area over which that force is distributed."@en ;
    rdfs:subClassOf [ a owl:Restriction ;
            owl:onProperty ns1:hasMeasurementUnit ;
            owl:someValuesFrom ns1:PressureUnit ],
        ns1:ISQDerivedQuantity,
        ns1:Intensive ;
    skos:prefLabel "Pressure"@en ;
    ns1:ISO80000Reference "4-14.1"^^xsd:string ;
    ns1:elucidation "The force applied perpendicular to the surface of an object per unit area over which that force is distributed."@en ;
    ns1:iupacReference "https://doi.org/10.1351/goldbook.P04819"^^xsd:string ;
    ns1:qudtReference "http://qudt.org/vocab/quantitykind/Pressure"^^xsd:string .

ns1:ReciprocalVolume a owl:Class ;
    rdfs:label "ReciprocalVolume"@en ;
    rdfs:comment "Physical quantity for measuring per volume."@en ;
    rdfs:subClassOf [ a owl:Restriction ;
            owl:onProperty ns1:hasMeasurementUnit ;
            owl:someValuesFrom ns1:PerVolumeUnit ],
        ns1:ISQDerivedQuantity ;
    skos:prefLabel "ReciprocalVolume"@en ;
    ns1:elucidation "Physical quantity for measuring per volume."@en .

ns1:Speed a owl:Class ;
    rdfs:label "Speed"@en ;
    rdfs:comment "Length per unit time."@en ;
    rdfs:subClassOf [ a owl:Restriction ;
            owl:onProperty ns1:hasMeasurementUnit ;
            owl:someValuesFrom ns1:SpeedUnit ],
        ns1:ISQDerivedQuantity ;
    skos:prefLabel "Speed"@en ;
    ns1:ISO80000Reference "3-8.2"^^xsd:string ;
    ns1:elucidation "Length per unit time."@en ;
    ns1:iupacReference "https://doi.org/10.1351/goldbook.S05852"^^xsd:string ;
    ns1:note "Speed in the absolute value of the velocity."@en ;
    ns1:qudtReference "http://qudt.org/vocab/quantitykind/Speed"^^xsd:string .

ns1:AngularFrequency a owl:Class ;
    rdfs:label "AngularFrequency"@en ;
    rdfs:comment "Rate of change of the phase angle."@en ;
    rdfs:subClassOf ns1:Frequency ;
    skos:prefLabel "AngularFrequency"@en ;
    ns1:IEVReference "https://www.electropedia.org/iev/iev.nsf/display?openform&ievref=103-07-03"^^xsd:string ;
    ns1:ISO80000Reference "3-18"^^xsd:string ;
    ns1:dbpediaReference "https://dbpedia.org/page/Angular_frequency"^^xsd:string ;
    ns1:elucidation "Rate of change of the phase angle."@en ;
    ns1:iupacReference "https://doi.org/10.1351/goldbook.A00352"^^xsd:string ;
    ns1:qudtReference "https://qudt.org/vocab/quantitykind/AngularFrequency"^^xsd:string ;
    ns1:wikipediaReference "https://en.wikipedia.org/wiki/Angular_frequency"^^xsd:string .

ns1:Concentration a owl:Class ;
    rdfs:label "Concentration"@en ;
    rdfs:comment "the abundance of a constituent divided by the total volume of a mixture."@en ;
    rdfs:subClassOf ns1:ISQDerivedQuantity ;
    skos:prefLabel "Concentration"@en ;
    ns1:dbpediaReference "https://dbpedia.org/page/Concentration"@en ;
    ns1:elucidation "the abundance of a constituent divided by the total volume of a mixture."@en ;
    ns1:iupacReference "https://goldbook.iupac.org/terms/view/C01222"@en ;
    ns1:qudtReference "https://qudt.org/vocab/quantitykind/Concentration"@en ;
    ns1:wikidataReference "https://www.wikidata.org/wiki/Q3686031"@en ;
    ns1:wikipediaReference "https://en.wikipedia.org/wiki/Concentration"@en .

ns1:ElectricConductance a owl:Class ;
    rdfs:label "ElectricConductance"@en ;
    rdfs:comment "Inverse of 'ElectricalResistance'."@en,
        "Measure of the ease for electric current to pass through a material."@en ;
    rdfs:subClassOf [ a owl:Restriction ;
            owl:onProperty ns1:hasMeasurementUnit ;
            owl:someValuesFrom ns1:ElectricConductanceUnit ],
        ns1:ElectromagneticQuantity,
        ns1:ISQDerivedQuantity,
        ns1:Intensive ;
    skos:altLabel "Conductance"@en ;
    skos:prefLabel "ElectricConductance"@en ;
    ns1:IEVReference "https://www.electropedia.org/iev/iev.nsf/display?openform&ievref=131-12-06"^^xsd:string ;
    ns1:ISO80000Reference "6-47"^^xsd:string ;
    ns1:elucidation "Measure of the ease for electric current to pass through a material."@en ;
    ns1:iupacReference "https://doi.org/10.1351/goldbook.E01925"^^xsd:string ;
    ns1:qudtReference "http://qudt.org/vocab/quantitykind/Conductance"^^xsd:string ;
    ns1:wikidataReference "https://www.wikidata.org/wiki/Q309017"^^xsd:string .

ns1:ElectricCurrentUnit a owl:Class .

ns1:Frequency a owl:Class ;
    rdfs:label "Frequency"@en ;
    rdfs:comment "Number of periods per time interval."@en ;
    rdfs:subClassOf [ a owl:Restriction ;
            owl:onProperty ns1:hasMeasurementUnit ;
            owl:someValuesFrom ns1:FrequencyUnit ],
        ns1:ISQDerivedQuantity,
        ns1:SpaceAndTimeQuantity ;
    skos:prefLabel "Frequency"@en ;
    ns1:IEVReference "https://www.electropedia.org/iev/iev.nsf/display?openform&ievref=103-06-02"^^xsd:string ;
    ns1:ISO80000Reference "3-15.1"^^xsd:string ;
    ns1:elucidation "Number of periods per time interval."@en ;
    ns1:iupacReference "https://doi.org/10.1351/goldbook.FT07383"^^xsd:string ;
    ns1:qudtReference "http://qudt.org/vocab/quantitykind/Frequency"^^xsd:string ;
    ns1:wikidataReference "https://www.wikidata.org/wiki/Q11652"^^xsd:string .

ns1:MagneticFluxDensity a owl:Class ;
    rdfs:label "MagneticFluxDensity"@en ;
    rdfs:comment "Often denoted B."@en,
        "Strength of the magnetic field."@en ;
    rdfs:subClassOf [ a owl:Restriction ;
            owl:onProperty ns1:hasMeasurementUnit ;
            owl:someValuesFrom ns1:MagneticFluxDensityUnit ],
        ns1:ElectromagneticQuantity,
        ns1:ISQDerivedQuantity ;
    skos:altLabel "MagneticInduction"@en ;
    skos:prefLabel "MagneticFluxDensity"@en ;
    ns1:IEVReference "https://www.electropedia.org/iev/iev.nsf/display?openform&ievref=121-11-19"^^xsd:string ;
    ns1:ISO80000Reference "6-21"^^xsd:string ;
    ns1:elucidation "Strength of the magnetic field."@en ;
    ns1:iupacReference "https://doi.org/10.1351/goldbook.M03686"^^xsd:string ;
    ns1:qudtReference "http://qudt.org/vocab/quantitykind/MagneticFluxDensity"^^xsd:string ;
    ns1:wikidataReference "https://www.wikidata.org/wiki/Q30204"^^xsd:string .

ns1:Duration a owl:Class ;
    rdfs:label "Duration"@en ;
    rdfs:comment "Physical quantity for describing the temporal distance between events."@en ;
    rdfs:subClassOf ns1:Time ;
    skos:prefLabel "Duration"@en ;
    ns1:IEVReference "https://www.electropedia.org/iev/iev.nsf/display?openform&ievref=113-01-13"^^xsd:string ;
    ns1:ISO80000Reference "3-9"^^xsd:string ;
    ns1:elucidation "Physical quantity for describing the temporal distance between events."@en ;
    ns1:wikidataReference "https://www.wikidata.org/wiki/Q2199864"^^xsd:string .

ns1:ElectricCurrent a owl:Class ;
    rdfs:label "ElectricCurrent"@en ;
    rdfs:comment "A flow of electric charge."@en ;
    rdfs:subClassOf [ a owl:Restriction ;
            owl:onProperty ns1:hasMeasurementUnit ;
            owl:someValuesFrom ns1:ElectricCurrentUnit ],
        ns1:ElectromagneticQuantity,
        ns1:Extensive ;
    skos:prefLabel "ElectricCurrent"@en ;
    ns1:ISO80000Reference "6-1"^^xsd:string ;
    ns1:elucidation "A flow of electric charge."@en ;
    ns1:iupacReference "https://doi.org/10.1351/goldbook.E01927"^^xsd:string ;
    ns1:qudtReference "http://qudt.org/vocab/quantitykind/ElectricCurrent"^^xsd:string .

ns1:ElectricResistance a owl:Class ;
    rdfs:label "ElectricResistance"@en ;
    rdfs:comment "Inverse of 'ElectricalConductance'."@en,
        "Measure of the difficulty to pass an electric current through a material."@en ;
    rdfs:subClassOf [ a owl:Restriction ;
            owl:onProperty ns1:hasMeasurementUnit ;
            owl:someValuesFrom ns1:ElectricResistanceUnit ],
        ns1:ElectromagneticQuantity,
        ns1:ISQDerivedQuantity ;
    skos:altLabel "Resistance"@en ;
    skos:prefLabel "ElectricResistance"@en ;
    ns1:ISO80000Reference "6-46"^^xsd:string ;
    ns1:elucidation "Measure of the difficulty to pass an electric current through a material."@en ;
    ns1:iupacReference "https://doi.org/10.1351/goldbook.E01936"^^xsd:string ;
    ns1:qudtReference "http://qudt.org/vocab/quantitykind/Resistance"^^xsd:string ;
    ns1:wikidataReference "https://www.wikidata.org/wiki/Q25358"^^xsd:string .

ns1:Force a owl:Class ;
    rdfs:label "Force"@en ;
    rdfs:comment "Any interaction that, when unopposed, will change the motion of an object"@en ;
    rdfs:subClassOf [ a owl:Restriction ;
            owl:onProperty ns1:hasMeasurementUnit ;
            owl:someValuesFrom ns1:ForceUnit ],
        ns1:Extensive,
        ns1:ISQDerivedQuantity ;
    skos:prefLabel "Force"@en ;
    ns1:ISO80000Reference "4-9.1"^^xsd:string ;
    ns1:elucidation "Any interaction that, when unopposed, will change the motion of an object"@en ;
    ns1:iupacReference "https://doi.org/10.1351/goldbook.F02480"^^xsd:string ;
    ns1:qudtReference "http://qudt.org/vocab/quantitykind/Force"^^xsd:string .

ns1:MolarEnergy a owl:Class ;
    rdfs:label "MolarEnergy"@en ;
    rdfs:comment "Energy per amount of substance."@en ;
    rdfs:subClassOf [ a owl:Restriction ;
            owl:onProperty ns1:hasMeasurementUnit ;
            owl:someValuesFrom ns1:EnergyPerAmountUnit ],
        ns1:ISQDerivedQuantity ;
    skos:prefLabel "MolarEnergy"@en ;
    ns1:elucidation "Energy per amount of substance."@en ;
    ns1:qudtReference "https://qudt.org/vocab/quantitykind/MolarEnergy"^^xsd:string ;
    ns1:wikidataReference "https://www.wikidata.org/wiki/Q69427512"^^xsd:string .

ns1:Radius a owl:Class ;
    rdfs:label "Radius"@en ;
    rdfs:comment "Distance from the centre of a circle to the circumference."@en ;
    rdfs:subClassOf ns1:RadialDistance ;
    skos:prefLabel "Radius"@en ;
    ns1:IEVReference "https://www.electropedia.org/iev/iev.nsf/display?openform&ievref=113-01-25"@en ;
    ns1:ISO80000Reference "3-1.6"^^xsd:string ;
    ns1:dbpediaReference "https://dbpedia.org/page/Radius"^^xsd:string ;
    ns1:elucidation "Distance from the centre of a circle to the circumference."@en ;
    ns1:qudtReference "https://qudt.org/vocab/quantitykind/Radius"^^xsd:string ;
    ns1:wikidataReference "https://www.wikidata.org/wiki/Q173817"^^xsd:string ;
    ns1:wikipediaReference "https://en.wikipedia.org/wiki/Radius"^^xsd:string .

ns1:ThermodynamicTemperature a owl:Class ;
    rdfs:label "ThermodynamicTemperature"@en ;
    rdfs:comment "Thermodynamic temperature is the absolute measure of temperature. It is defined by the third law of thermodynamics in which the theoretically lowest temperature is the null or zero point."@en ;
    rdfs:subClassOf [ a owl:Restriction ;
            owl:onProperty ns1:hasMeasurementUnit ;
            owl:someValuesFrom ns1:TemperatureUnit ],
        ns1:Intensive,
        ns1:ThermodynamicalQuantity ;
    skos:altLabel "Temperature"@en ;
    skos:prefLabel "ThermodynamicTemperature"@en ;
    ns1:ISO80000Reference "5-1"^^xsd:string ;
    ns1:elucidation "Thermodynamic temperature is the absolute measure of temperature. It is defined by the third law of thermodynamics in which the theoretically lowest temperature is the null or zero point."@en ;
    ns1:iupacReference "https://doi.org/10.1351/goldbook.T06321"^^xsd:string ;
    ns1:qudtReference "http://qudt.org/vocab/quantitykind/ThermodynamicTemperature"^^xsd:string .

ns1:FrequencyUnit a owl:Class .

ns1:LengthUnit a owl:Class .

ns1:SpecificEnergy a owl:Class ;
    rdfs:label "SpecificEnergy"@en ;
    rdfs:comment "Energy per unit mass"@en ;
    rdfs:subClassOf [ a owl:Restriction ;
            owl:onProperty ns1:hasMeasurementUnit ;
            owl:someValuesFrom ns1:AbsorbedDoseUnit ],
        ns1:ISQDerivedQuantity,
        ns1:Intensive,
        ns1:ThermodynamicalQuantity ;
    skos:prefLabel "SpecificEnergy"@en ;
    ns1:ISO80000Reference "5-21.1"^^xsd:string ;
    ns1:dbpediaReference "https://dbpedia.org/page/Specific_energy"^^xsd:string ;
    ns1:elucidation "Energy per unit mass"@en ;
    ns1:qudtReference "https://qudt.org/vocab/quantitykind/SpecificEnergy"^^xsd:string ;
    ns1:wikidataReference "https://www.wikidata.org/wiki/Q3023293"^^xsd:string ;
    ns1:wikipediaReference "https://en.wikipedia.org/wiki/Specific_energy"^^xsd:string .

ns1:Angle a owl:Class ;
    rdfs:label "Angle"@en ;
    rdfs:comment "Ratio of circular arc length to radius."@en ;
    rdfs:subClassOf ns1:RatioQuantity ;
    skos:altLabel "PlaneAngle"@en ;
    skos:prefLabel "Angle"@en ;
    ns1:ISO80000Reference "3-5"^^xsd:string ;
    ns1:elucidation "Ratio of circular arc length to radius."@en ;
    ns1:iupacReference "https://doi.org/10.1351/goldbook.A00346"^^xsd:string ;
    ns1:qudtReference "http://qudt.org/vocab/quantitykind/PlaneAngle"^^xsd:string .

ns1:Mass a owl:Class ;
    rdfs:label "Mass"@en ;
    rdfs:comment "Property of a physical body that express its resistance to acceleration (a change in its state of motion) when a force is applied."@en ;
    rdfs:subClassOf [ a owl:Restriction ;
            owl:allValuesFrom ns1:Matter ;
            owl:onProperty [ owl:inverseOf ns1:hasProperty ] ],
        [ a owl:Restriction ;
            owl:onProperty ns1:hasMeasurementUnit ;
            owl:someValuesFrom ns1:MassUnit ],
        ns1:Extensive,
        ns1:MechanicalQuantity ;
    skos:prefLabel "Mass"@en ;
    ns1:ISO80000Reference "4-1"^^xsd:string ;
    ns1:elucidation "Property of a physical body that express its resistance to acceleration (a change in its state of motion) when a force is applied."@en ;
    ns1:iupacReference "https://doi.org/10.1351/goldbook.M03709"^^xsd:string ;
    ns1:qudtReference "http://qudt.org/vocab/quantitykind/Mass"^^xsd:string .

ns1:PerVolumeUnit a owl:Class ;
    rdfs:label "PerVolumeUnit"@en ;
    rdfs:comment "The class of units with dimensionality 'PerVolume'."@en .

ns1:Power a owl:Class ;
    rdfs:label "Power"@en ;
    rdfs:comment "Rate of transfer of energy per unit time."@en ;
    rdfs:subClassOf [ a owl:Restriction ;
            owl:onProperty ns1:hasMeasurementUnit ;
            owl:someValuesFrom ns1:PowerUnit ],
        ns1:ElectromagneticQuantity,
        ns1:Extensive,
        ns1:ISQDerivedQuantity ;
    skos:prefLabel "Power"@en ;
    ns1:ISO80000Reference "4-27"^^xsd:string,
        "6-45"^^xsd:string ;
    ns1:elucidation "Rate of transfer of energy per unit time."@en ;
    ns1:iupacReference "https://doi.org/10.1351/goldbook.P04792"^^xsd:string ;
    ns1:qudtReference "http://qudt.org/vocab/quantitykind/Power"^^xsd:string .

ns1:QuantumNumber a owl:Class ;
    rdfs:label "QuantumNumber"^^xsd:string ;
    rdfs:comment "Number describing a particular state of a quantum system."@en ;
    rdfs:subClassOf ns1:AtomicAndNuclearPhysicsQuantity,
        ns1:PureNumberQuantity ;
    skos:prefLabel "QuantumNumber"^^xsd:string ;
    ns1:ISO80000Reference "10-13.1"^^xsd:string ;
    ns1:elucidation "Number describing a particular state of a quantum system."@en ;
    ns1:qudtReference "https://qudt.org/vocab/quantitykind/QuantumNumber"^^xsd:string ;
    ns1:wikidataReference "https://www.wikidata.org/wiki/Q232431"^^xsd:string .

ns1:PressureUnit a owl:Class .

ns1:ISO80000Categorised a owl:Class ;
    rdfs:label "ISO80000Categorised"@en ;
    rdfs:subClassOf ns1:CategorizedPhysicalQuantity ;
    skos:prefLabel "ISO80000Categorised"@en .

ns1:ReciprocalLength a owl:Class ;
    rdfs:label "ReciprocalLength"@en ;
    rdfs:comment "The inverse of length."@en ;
    rdfs:subClassOf [ a owl:Restriction ;
            owl:onProperty ns1:hasMeasurementUnit ;
            owl:someValuesFrom ns1:ReciprocalLengthUnit ],
        ns1:ISQDerivedQuantity ;
    skos:altLabel "InverseLength"^^xsd:string ;
    skos:prefLabel "ReciprocalLength"@en ;
    ns1:elucidation "The inverse of length."@en ;
    ns1:qudtReference "http://qudt.org/vocab/quantitykind/InverseLength"^^xsd:string ;
    ns1:wikipediaReference "https://en.wikipedia.org/wiki/Reciprocal_length"^^xsd:string .

ns1:SIExactConstant a owl:Class ;
    rdfs:label "SIExactConstant"@en ;
    rdfs:comment "Physical constant that by definition (after the latest revision of the SI system that was enforsed May 2019) has a known exact numerical value when expressed in SI units."@en ;
    rdfs:subClassOf ns1:ExactConstant ;
    skos:prefLabel "SIExactConstant"@en ;
    ns1:elucidation "Physical constant that by definition (after the latest revision of the SI system that was enforsed May 2019) has a known exact numerical value when expressed in SI units."@en .

ns1:PureNumberQuantity a owl:Class ;
    rdfs:label "PureNumberQuantity"@en ;
    rdfs:comment "A pure number, typically the number of something."@en,
        """According to the SI brochure counting does not automatically qualify a quantity as an amount of substance.

This quantity is used only to describe the outcome of a counting process, without regard of the type of entities.

There are also some quantities that cannot be described in terms of the seven base quantities of the SI, but have the nature of a count. Examples are a number of molecules, a number of cellular or biomolecular entities (for example copies of a particular nucleic acid sequence), or degeneracy in quantum mechanics. Counting quantities are also quantities with the associated unit one."""@en ;
    rdfs:subClassOf ns1:ISQDimensionlessQuantity ;
    skos:example """1,
i,
π,
the number of protons in the nucleus of an atom"""^^xsd:string ;
    skos:prefLabel "PureNumberQuantity"@en ;
    ns1:elucidation "A pure number, typically the number of something."@en .

ns1:Extensive a owl:Class ;
    rdfs:label "Extensive"@en ;
    rdfs:comment "A quantity whose magnitude is additive for subsystems."@en,
        "Note that not all physical quantities can be categorised as being either intensive or extensive. For example the square root of the mass."@en ;
    rdfs:subClassOf ns1:CategorizedPhysicalQuantity ;
    owl:disjointWith ns1:Intensive ;
    skos:example """Mass
Volume
Entropy"""@en ;
    skos:prefLabel "Extensive"@en ;
    ns1:elucidation "A quantity whose magnitude is additive for subsystems."@en .

ns1:Length a owl:Class ;
    rdfs:label "Length"@en ;
    rdfs:comment "Extend of a spatial dimension."@en,
        "Length is a non-negative additive quantity attributed to a one-dimensional object in space."@en ;
    rdfs:subClassOf [ a owl:Restriction ;
            owl:onProperty ns1:hasMeasurementUnit ;
            owl:someValuesFrom ns1:LengthUnit ],
        ns1:Extensive,
        ns1:SpaceAndTimeQuantity ;
    skos:prefLabel "Length"@en ;
    ns1:ISO80000Reference "3-1.1"^^xsd:string ;
    ns1:elucidation "Extend of a spatial dimension."@en ;
    ns1:iupacReference "https://doi.org/10.1351/goldbook.L03498"^^xsd:string ;
    ns1:qudtReference "http://qudt.org/vocab/quantitykind/Length"^^xsd:string .

ns1:Intensive a owl:Class ;
    rdfs:label "Intensive"@en ;
    rdfs:comment "A quantity whose magnitude is independent of the size of the system."@en,
        "Note that not all physical quantities can be categorised as being either intensive or extensive. For example the square root of the mass."@en ;
    rdfs:subClassOf ns1:CategorizedPhysicalQuantity ;
    skos:example """Temperature
Density
Pressure
ChemicalPotential"""@en ;
    skos:prefLabel "Intensive"@en ;
    ns1:elucidation "A quantity whose magnitude is independent of the size of the system."@en .

ns1:SpaceAndTimeQuantity a owl:Class ;
    rdfs:label "SpaceAndTimeQuantity"@en ;
    rdfs:comment "Quantities categorised according to ISO 80000-3."@en ;
    rdfs:subClassOf ns1:ISO80000Categorised ;
    skos:prefLabel "SpaceAndTimeQuantity"@en ;
    ns1:elucidation "Quantities categorised according to ISO 80000-3."@en .

ns1:Energy a owl:Class ;
    rdfs:label "Energy"@en ;
    rdfs:comment "A property of objects which can be transferred to other objects or converted into different forms."@en,
        "Energy is often defined as \"ability of a system to perform work\", but it might be misleading since is not necessarily available to do work."@en ;
    rdfs:subClassOf [ a owl:Restriction ;
            owl:onProperty ns1:hasMeasurementUnit ;
            owl:someValuesFrom ns1:EnergyUnit ],
        ns1:Extensive,
        ns1:ISQDerivedQuantity ;
    skos:prefLabel "Energy"@en ;
    ns1:ISO80000Reference "5-20-1"^^xsd:string ;
    ns1:elucidation "A property of objects which can be transferred to other objects or converted into different forms."@en ;
    ns1:iupacReference "https://doi.org/10.1351/goldbook.E02101"^^xsd:string ;
    ns1:qudtReference "http://qudt.org/vocab/quantitykind/Energy"^^xsd:string .

ns1:RatioQuantity a owl:Class ;
    rdfs:label "RatioQuantity"@en ;
    rdfs:comment """Quantities defined as ratios `Q=A/B` having equal dimensions in numerator and denominator are dimensionless quantities but still have a physical dimension defined as dim(A)/dim(B).

Johansson, Ingvar (2010). "Metrological thinking needs the notions of parametric quantities, units and dimensions". Metrologia. 47 (3): 219–230. doi:10.1088/0026-1394/47/3/012. ISSN 0026-1394."""@en,
        "The class of quantities that are the ratio of two quantities with the same physical dimensionality."@en ;
    rdfs:seeAlso "https://iopscience.iop.org/article/10.1088/0026-1394/47/3/012"^^xsd:string ;
    rdfs:subClassOf ns1:ISQDimensionlessQuantity ;
    skos:example """refractive index,
volume fraction,
fine structure constant"""^^xsd:string ;
    skos:prefLabel "RatioQuantity"@en ;
    ns1:elucidation "The class of quantities that are the ratio of two quantities with the same physical dimensionality."@en ;
    ns1:qudtReference "http://qudt.org/vocab/quantitykind/DimensionlessRatio"^^xsd:string .

ns1:MechanicalQuantity a owl:Class ;
    rdfs:label "MechanicalQuantity"@en ;
    rdfs:comment "Quantities categorised according to ISO 80000-4."@en ;
    rdfs:subClassOf ns1:ISO80000Categorised ;
    skos:prefLabel "MechanicalQuantity"@en ;
    ns1:elucidation "Quantities categorised according to ISO 80000-4."@en .

ns1:ThermodynamicalQuantity a owl:Class ;
    rdfs:label "ThermodynamicalQuantity"@en ;
    rdfs:comment "Quantities categorised according to ISO 80000-5."@en ;
    rdfs:subClassOf ns1:ISO80000Categorised ;
    skos:prefLabel "ThermodynamicalQuantity"@en ;
    ns1:elucidation "Quantities categorised according to ISO 80000-5."@en .

ns1:PhysioChemicalQuantity a owl:Class ;
    rdfs:label "PhysioChemicalQuantity"@en ;
    rdfs:comment "Quantities categorised according to ISO 80000-9."@en ;
    rdfs:subClassOf ns1:ISO80000Categorised ;
    skos:prefLabel "PhysioChemicalQuantity"@en ;
    ns1:elucidation "Quantities categorised according to ISO 80000-9."@en .

ns1:ISQDimensionlessQuantity a owl:Class ;
    rdfs:label "ISQDimensionlessQuantity"@en ;
    rdfs:comment "A quantity to which no physical dimension is assigned and with a corresponding unit of measurement in the SI of the unit one."@en ;
    rdfs:subClassOf [ a owl:Restriction ;
            owl:onProperty ns1:hasMetrologicalReference ;
            owl:someValuesFrom ns1:DimensionlessUnit ],
        ns1:ISQDerivedQuantity ;
    skos:prefLabel "ISQDimensionlessQuantity"@en ;
    ns1:elucidation "A quantity to which no physical dimension is assigned and with a corresponding unit of measurement in the SI of the unit one."@en ;
    ns1:iupacReference "https://doi.org/10.1351/goldbook.D01742"^^xsd:string ;
    ns1:qudtReference "http://qudt.org/vocab/quantitykind/Dimensionless"^^xsd:string ;
    ns1:wikipediaReference "https://en.wikipedia.org/wiki/Dimensionless_quantity"^^xsd:string .

ns1:ElectromagneticQuantity a owl:Class ;
    rdfs:label "ElectromagneticQuantity"@en ;
    rdfs:comment "Quantities categorised according to ISO 80000-6."@en ;
    rdfs:subClassOf ns1:ISO80000Categorised ;
    skos:prefLabel "ElectromagneticQuantity"@en ;
    ns1:elucidation "Quantities categorised according to ISO 80000-6."@en .

ns1:CondensedMatterPhysicsQuantity a owl:Class ;
    rdfs:label "CondensedMatterPhysicsQuantity"@en ;
    rdfs:comment "Quantities categorised according to ISO 80000-12."@en ;
    rdfs:subClassOf ns1:ISO80000Categorised ;
    skos:prefLabel "CondensedMatterPhysicsQuantity"@en ;
    ns1:elucidation "Quantities categorised according to ISO 80000-12."@en .

ns1:AtomicAndNuclearPhysicsQuantity a owl:Class ;
    rdfs:label "AtomicAndNuclearPhysicsQuantity"@en ;
    rdfs:comment "Quantities categorised according to ISO 80000-10."@en ;
    rdfs:subClassOf ns1:ISO80000Categorised ;
    skos:prefLabel "AtomicAndNuclearPhysicsQuantity"@en ;
    ns1:elucidation "Quantities categorised according to ISO 80000-10."@en .

ns1:ISQDerivedQuantity a owl:Class ;
    rdfs:label "ISQDerivedQuantity"@en ;
    rdfs:comment "Derived quantities defined in the International System of Quantities (ISQ)."@en ;
    rdfs:subClassOf ns1:DerivedQuantity,
        ns1:InternationalSystemOfQuantity ;
    skos:prefLabel "ISQDerivedQuantity"@en ;
    ns1:elucidation "Derived quantities defined in the International System of Quantities (ISQ)."@en .

