@prefix dcterms: <http://purl.org/dc/terms/> .
@prefix ns1: <https://w3id.org/emmo#> .
@prefix owl: <http://www.w3.org/2002/07/owl#> .
@prefix rdf: <http://www.w3.org/1999/02/22-rdf-syntax-ns#> .
@prefix rdfs: <http://www.w3.org/2000/01/rdf-schema#> .
@prefix skos: <http://www.w3.org/2004/02/skos/core#> .
@prefix xsd: <http://www.w3.org/2001/XMLSchema#> .

ns1:EMMO_084b4f77_6df7_4c6a_b705_2528aba5cdda a owl:Class ;
    rdfs:label "MaterialRelationComputation"@en ;
    rdfs:subClassOf ns1:EMMO_5dd63d84_57f5_4b79_b760_fe940c06680d ;
    skos:prefLabel "MaterialRelationComputation"@en .

ns1:EMMO_0cd58641_824c_4851_907f_f4c3be76630c skos:altLabel "Signal"@en .

ns1:EMMO_1c7f2dfe_0db4_4bf6_a0f6_853054a34ead a owl:Class ;
    rdfs:label "DataProcessing"@en ;
    rdfs:comment "A computation that provides a data output following the elaboration of some input data, using a data processing application."@en ;
    rdfs:subClassOf [ a owl:Restriction ;
            owl:onProperty ns1:EMMO_ae2d1a96_bfa1_409a_a7d2_03d69e8a125a ;
            owl:someValuesFrom ns1:EMMO_cbf42aa6_9e11_4be8_932a_ae3c792ab17d ],
        [ a owl:Restriction ;
            owl:onProperty ns1:EMMO_36e69413_8c59_4799_946c_10b05d266e22 ;
            owl:someValuesFrom ns1:EMMO_be8592a7_68d1_4a06_ad23_82f2b56ef926 ],
        [ a owl:Restriction ;
            owl:onProperty ns1:EMMO_c4bace1d_4db0_4cd3_87e9_18122bae2840 ;
            owl:someValuesFrom ns1:EMMO_be8592a7_68d1_4a06_ad23_82f2b56ef926 ],
        ns1:EMMO_eff42cb3_208e_4768_9a39_f8b6b3c3d7a2 ;
    skos:prefLabel "DataProcessing"@en ;
    ns1:EMMO_967080e5_2f42_4eb2_a3a9_c58143e835f9 "A computation that provides a data output following the elaboration of some input data, using a data processing application."@en .

ns1:EMMO_22522299_4091_4d1f_82a2_3890492df6db a owl:Class ;
    rdfs:label "Experiment"@en ;
    rdfs:comment "An experiment is a process that is intended to replicate a physical phenomenon in a controlled environment."@en ;
    rdfs:subClassOf ns1:EMMO_3b19eab4_79be_4b02_bdaf_ecf1f0067a68,
        ns1:EMMO_43e9a05d_98af_41b4_92f6_00f79a09bfce ;
    skos:prefLabel "Experiment"@en ;
    ns1:EMMO_967080e5_2f42_4eb2_a3a9_c58143e835f9 "An experiment is a process that is intended to replicate a physical phenomenon in a controlled environment."@en .

ns1:EMMO_24c71baf_6db6_48b9_86c8_8c70cf36db0c a owl:ObjectProperty ;
    rdfs:label "hasModel"@en ;
    rdfs:subPropertyOf ns1:EMMO_39c3815d_8cae_4c8f_b2ff_eeba24bec455 ;
    skos:prefLabel "hasModel"@en .

ns1:EMMO_57b9fd6c_84d6_43f2_8c4f_de6a1ab50aea a owl:Class ;
    rdfs:label "Guess"@en ;
    rdfs:comment "A guess is a theory, estimated and subjective, since its premises are subjective."@en ;
    rdfs:subClassOf ns1:EMMO_251cfb4f_5c75_4778_91ed_6c8395212fd8,
        ns1:EMMO_8d2d9374_ef3a_47e6_8595_6bc208e07519,
        ns1:EMMO_9b87d718_9dcc_4f7d_ad20_12c2aa4c76be ;
    skos:prefLabel "Guess"@en ;
    ns1:EMMO_967080e5_2f42_4eb2_a3a9_c58143e835f9 "A guess is a theory, estimated and subjective, since its premises are subjective."@en .

ns1:EMMO_67c70dcd_2adf_4e6c_b3f8_f33dd1512487 a owl:Class ;
    rdfs:label "EmpiricalSimulationSoftware"@en ;
    rdfs:comment "A computational application that uses an empiric equation to predict the behaviour of a system without relying on the knowledge of the actual physical phenomena occurring in the object."@en ;
    rdfs:subClassOf ns1:EMMO_8b66ada5_510c_44bd_a8d8_3c64d301a5e9 ;
    skos:prefLabel "EmpiricalSimulationSoftware"@en ;
    ns1:EMMO_967080e5_2f42_4eb2_a3a9_c58143e835f9 "A computational application that uses an empiric equation to predict the behaviour of a system without relying on the knowledge of the actual physical phenomena occurring in the object."@en .

ns1:EMMO_6c739b1a_a774_4416_bb31_1961486fa9ed a owl:Class ;
    rdfs:label "Theorisation"@en ;
    rdfs:comment "The 'semiosis' process of interpreting a 'physical' and provide a complec sign, 'theory' that stands for it and explain it to another interpreter."@en ;
    rdfs:subClassOf [ a owl:Restriction ;
            owl:onProperty ns1:EMMO_35c29eb6_f57e_48d8_85af_854f9e926e77 ;
            owl:someValuesFrom ns1:EMMO_8d2d9374_ef3a_47e6_8595_6bc208e07519 ],
        ns1:EMMO_10a5fd39_06aa_4648_9e70_f962a9cb2069 ;
    skos:altLabel "Theorization"@en ;
    skos:prefLabel "Theorisation"@en ;
    ns1:EMMO_967080e5_2f42_4eb2_a3a9_c58143e835f9 "The 'semiosis' process of interpreting a 'physical' and provide a complec sign, 'theory' that stands for it and explain it to another interpreter."@en .

ns1:EMMO_6e0664f2_4d4d_4407_bf60_e1b3c07198d7 a owl:Class ;
    rdfs:label "PhysicsEquationSolution"@en ;
    rdfs:comment "A function solution of a physics equation that provides a methods for the prediction of some quantitiative properties of an object."@en,
        """This must be a mathematical function v(t), x(t).
A dataset as solution is a conventional sign."""@en ;
    rdfs:subClassOf ns1:EMMO_54ee6b5e_5261_44a8_86eb_5717e7fdb9d0 ;
    skos:example "A parabolic function is a prediction of the trajectory of a falling object in a gravitational field. While it has predictive capabilities it lacks of an analogical character, since it does not show the law behind that trajectory."@en ;
    skos:prefLabel "PhysicsEquationSolution"@en ;
    ns1:EMMO_967080e5_2f42_4eb2_a3a9_c58143e835f9 "A function solution of a physics equation that provides a methods for the prediction of some quantitiative properties of an object."@en .

ns1:EMMO_8533871a_01e4_4935_8c7b_cedf8fcc3fa3 a owl:Class ;
    rdfs:label "Replica"@en ;
    rdfs:comment "An icon that not only resembles the object, but also can express some of the object's functions."@en ;
    rdfs:subClassOf ns1:EMMO_d7788d1a_020d_4c78_85a1_13563fcec168 ;
    owl:equivalentClass [ a owl:Class ;
            owl:intersectionOf ( ns1:EMMO_8c537c06_8e1d_4a3b_a251_1c89bb2c4790 ns1:EMMO_c7013b53_3071_410b_a5e4_a8d266dcdfb5 ) ] ;
    skos:example "A small scale replica of a plane tested in a wind gallery shares the same functionality in terms of aerodynamic behaviour of the bigger one."@en,
        "Pinocchio is a functional icon of a boy since it imitates the external behaviour without having the internal biological structure of a human being (it is made of magic wood...)."@en ;
    skos:prefLabel "Replica"@en ;
    ns1:EMMO_967080e5_2f42_4eb2_a3a9_c58143e835f9 "An icon that not only resembles the object, but also can express some of the object's functions."@en .

ns1:EMMO_8d4962d7_9608_44f7_a2f1_82a4bb173f4a a owl:Class ;
    rdfs:label "PhysicalBasedSimulationSoftware"@en ;
    rdfs:comment "A computational application that uses a physical model to predict the behaviour of a system, providing a identifiable analogy with the original object."@en ;
    rdfs:subClassOf ns1:EMMO_8b66ada5_510c_44bd_a8d8_3c64d301a5e9 ;
    skos:prefLabel "PhysicalBasedSimulationSoftware"@en ;
    ns1:EMMO_967080e5_2f42_4eb2_a3a9_c58143e835f9 "A computational application that uses a physical model to predict the behaviour of a system, providing a identifiable analogy with the original object."@en .

ns1:EMMO_90f18cf0_1225_4c64_b5f8_f65cd7f992c5 a owl:Class ;
    rdfs:label "MaterialsModel"@en ;
    rdfs:comment "A solvable set of one Physics Equation and one or more Materials Relations."@en ;
    rdfs:seeAlso "https://op.europa.eu/en/publication-detail/-/publication/ec1455c3-d7ca-11e6-ad7c-01aa75ed71a1"@en ;
    rdfs:subClassOf [ a owl:Restriction ;
            owl:onProperty ns1:EMMO_dc57d998_23db_4d8e_b2cd_f346b195b846 ;
            owl:someValuesFrom ns1:EMMO_e5438930_04e7_4d42_ade5_3700d4a52ab7 ],
        ns1:EMMO_b29fd350_39aa_4af7_9459_3faa0544cba6 ;
    owl:disjointUnionOf ( ns1:EMMO_4456a5d2_16a6_4ee1_9a8e_5c75956b28ea ns1:EMMO_53935db0_af45_4426_b9e9_244a0d77db00 ns1:EMMO_6eca09be_17e9_445e_abc9_000aa61b7a11 ns1:EMMO_84cadc45_6758_46f2_ba2a_5ead65c70213 ) ;
    skos:prefLabel "MaterialsModel"@en ;
    ns1:EMMO_967080e5_2f42_4eb2_a3a9_c58143e835f9 "A solvable set of one Physics Equation and one or more Materials Relations."@en .

ns1:EMMO_9c32fd69_f480_4130_83b3_fb25d9face14 a owl:Class ;
    rdfs:label "PhysicalLaw"@en ;
    rdfs:comment "A law that provides a connection between a property of the object and other properties, capturing a fundamental physical phenomena."@en ;
    rdfs:subClassOf ns1:EMMO_db9a009e_f097_43f5_9520_6cbc07e7610b ;
    skos:prefLabel "PhysicalLaw"@en ;
    ns1:EMMO_967080e5_2f42_4eb2_a3a9_c58143e835f9 "A law that provides a connection between a property of the object and other properties, capturing a fundamental physical phenomena."@en .

ns1:EMMO_a4b14b83_9392_4a5f_a2e8_b2b58793f59b a owl:Class ;
    rdfs:label "DataBasedSimulationSoftware"@en ;
    rdfs:comment "A computational application that uses existing data to predict the behaviour of a system without providing a identifiable analogy with the original object."@en ;
    rdfs:subClassOf ns1:EMMO_8b66ada5_510c_44bd_a8d8_3c64d301a5e9 ;
    skos:prefLabel "DataBasedSimulationSoftware"@en ;
    ns1:EMMO_967080e5_2f42_4eb2_a3a9_c58143e835f9 "A computational application that uses existing data to predict the behaviour of a system without providing a identifiable analogy with the original object."@en .

ns1:EMMO_d0bcf2ca_cd55_4f34_8fc2_2decc4c6087a a owl:Class ;
    rdfs:label "StandaloneModelSimulation"@en ;
    rdfs:comment "A standalone simulation, where a single physics equation is solved."@en ;
    rdfs:subClassOf ns1:EMMO_e97af6ec_4371_4bbc_8936_34b76e33302f ;
    skos:prefLabel "StandaloneModelSimulation"@en ;
    ns1:EMMO_967080e5_2f42_4eb2_a3a9_c58143e835f9 "A standalone simulation, where a single physics equation is solved."@en .

ns1:EMMO_e7cbc129_0d05_41a2_851a_10b198cd7ca2 a owl:Class ;
    rdfs:label "Hypothesis"@en ;
    rdfs:comment "A hypothesis is a theory, estimated and objective, since its estimated premises are objective."@en ;
    rdfs:subClassOf ns1:EMMO_2a888cdf_ec4a_4ec5_af1c_0343372fc978,
        ns1:EMMO_8d2d9374_ef3a_47e6_8595_6bc208e07519,
        ns1:EMMO_9b87d718_9dcc_4f7d_ad20_12c2aa4c76be ;
    skos:prefLabel "Hypothesis"@en ;
    ns1:EMMO_967080e5_2f42_4eb2_a3a9_c58143e835f9 "A hypothesis is a theory, estimated and objective, since its estimated premises are objective."@en .

ns1:EMMO_ec502e30_b9ec_4216_90c6_f67d2df75627 a owl:Class ;
    rdfs:label "LinkedModelsSimulation"@en ;
    rdfs:comment "A chain of linked physics based model simulations, where equations are solved sequentially."@en ;
    rdfs:subClassOf ns1:EMMO_7d56ec24_499d_487a_af7d_a91aaa787bfe ;
    skos:prefLabel "LinkedModelsSimulation"@en ;
    ns1:EMMO_967080e5_2f42_4eb2_a3a9_c58143e835f9 "A chain of linked physics based model simulations, where equations are solved sequentially."@en .

ns1:EMMO_f19ff3b4_6bfe_4c41_a2b2_9affd39c140b a owl:Class ;
    rdfs:label "MaterialLaw"@en ;
    rdfs:comment "A law that provides a connection between a material property and other properties of the object."@en ;
    rdfs:subClassOf ns1:EMMO_db9a009e_f097_43f5_9520_6cbc07e7610b ;
    skos:prefLabel "MaterialLaw"@en ;
    ns1:EMMO_967080e5_2f42_4eb2_a3a9_c58143e835f9 "A law that provides a connection between a material property and other properties of the object."@en .

<https://w3id.org/emmo/disciplines/models> a owl:Ontology ;
    dcterms:abstract "The models module defines models as semiotic signs that stands for an object by resembling or imitating it, in shape or by sharing a similar logical structure."@en ;
    dcterms:creator <https://orcid.org/0000-0003-4065-9742>,
        ns1:AdhamHashibon,
        ns1:EmanueleGhedini,
        ns1:GerhardGoldbeck,
        ns1:JesperFriis ;
    dcterms:license "https://creativecommons.org/licenses/by/4.0/legalcode"^^xsd:string ;
    dcterms:publisher <https://emmc.eu> ;
    dcterms:title "Models"@en ;
    rdfs:comment "The EMMO requires HermiT reasoner plugin in order to visualize all inferences and class hierarchy (ctrl+R hotkey in Protege)."@en ;
    owl:imports <https://w3id.org/emmo/1.0.2/disciplines/computerscience>,
        <https://w3id.org/emmo/1.0.2/disciplines/math>,
        <https://w3id.org/emmo/1.0.2/disciplines/metrology>,
        <https://w3id.org/emmo/1.0.2/perspectives/persistence>,
        <https://w3id.org/emmo/1.0.2/reference/data>,
        <https://w3id.org/emmo/1.0.2/reference/workflow> ;
    owl:versionIRI <https://w3id.org/emmo/1.0.2/disciplines/models> ;
    owl:versionInfo "1.0.2"^^xsd:string ;
    ns1:EMMO_1246b120_abbe_4840_b0f8_3e4348b24a17 "emmo@emmc.eu"^^xsd:string .

ns1:EMMO_01354ac2_cce1_4b7d_8b4a_7322d6cb10bc a owl:Class ;
    rdfs:label "IterativeCoupledModelsSimulation"@en ;
    rdfs:comment "A chain of linked physics based model simulations solved iteratively, where equations are segregated."@en ;
    rdfs:subClassOf ns1:EMMO_02c4890b_aef3_4173_9669_94d1f6baf611 ;
    skos:prefLabel "IterativeCoupledModelsSimulation"@en ;
    ns1:EMMO_967080e5_2f42_4eb2_a3a9_c58143e835f9 "A chain of linked physics based model simulations solved iteratively, where equations are segregated."@en .

ns1:EMMO_27c5d8c6_8af7_4d63_beb1_ec37cd8b3fa3 a owl:Class ;
    rdfs:label "PhysicsEquation"@en ;
    rdfs:comment "An 'equation' that stands for a 'physical_law' by mathematically defining the relations between physics_quantities."@en ;
    rdfs:subClassOf ns1:EMMO_b29fd350_39aa_4af7_9459_3faa0544cba6,
        ns1:EMMO_e56ee3eb_7609_4ae1_8bed_51974f0960a6 ;
    skos:example """The Newton's equation of motion.
The Schrödinger equation.
The Navier-Stokes equation."""@en ;
    skos:prefLabel "PhysicsEquation"@en ;
    ns1:EMMO_967080e5_2f42_4eb2_a3a9_c58143e835f9 "An 'equation' that stands for a 'physical_law' by mathematically defining the relations between physics_quantities."@en .

ns1:EMMO_4456a5d2_16a6_4ee1_9a8e_5c75956b28ea a owl:Class ;
    rdfs:label "ContinuumModel"@en ;
    rdfs:comment "A physics-based model based on a physics equation describing the behaviour of continuum volume."@en ;
    skos:prefLabel "ContinuumModel"@en ;
    ns1:EMMO_967080e5_2f42_4eb2_a3a9_c58143e835f9 "A physics-based model based on a physics equation describing the behaviour of continuum volume."@en .

ns1:EMMO_53935db0_af45_4426_b9e9_244a0d77db00 a owl:Class ;
    rdfs:label "MesoscopicModel"@en ;
    rdfs:comment "A physics-based model based on a physics equation describing the behaviour of mesoscopic entities, i.e. a set of bounded atoms like a molecule, bead or nanoparticle."@en ;
    skos:prefLabel "MesoscopicModel"@en ;
    ns1:EMMO_967080e5_2f42_4eb2_a3a9_c58143e835f9 "A physics-based model based on a physics equation describing the behaviour of mesoscopic entities, i.e. a set of bounded atoms like a molecule, bead or nanoparticle."@en .

ns1:EMMO_5dd63d84_57f5_4b79_b760_fe940c06680d a owl:Class ;
    rdfs:label "PhysicsMathematicalComputation"@en ;
    rdfs:comment "A functional icon that imitates the behaviour of the object through mathematical evaluations of some mathematical construct."@en ;
    rdfs:subClassOf ns1:EMMO_c7013b53_3071_410b_a5e4_a8d266dcdfb5,
        ns1:EMMO_eff42cb3_208e_4768_9a39_f8b6b3c3d7a2 ;
    skos:prefLabel "PhysicsMathematicalComputation"@en ;
    ns1:EMMO_967080e5_2f42_4eb2_a3a9_c58143e835f9 "A functional icon that imitates the behaviour of the object through mathematical evaluations of some mathematical construct."@en ;
    ns1:EMMO_c7b62dd7_063a_4c2a_8504_42f7264ba83f "The equation that describes the velocity of a uniform accelerated body v = v0 + a*t is a functional icon. In general every analitical solution of a mathematical model can be considered an icon. A functional icon expresses its similarity with the object when is part of a process the makes it imitate the behavior of the object. In the case of v = v0 + a*t, plotting the velocity over time or listing their values at certain instants is when the icon expresses it functionality."@en .

ns1:EMMO_6eca09be_17e9_445e_abc9_000aa61b7a11 a owl:Class ;
    rdfs:label "ElectronicModel"@en ;
    rdfs:comment "A physics-based model based on a physics equation describing the behaviour of electrons."@en ;
    skos:example """Density functional theory.
Hartree-Fock."""@en ;
    skos:prefLabel "ElectronicModel"@en ;
    ns1:EMMO_967080e5_2f42_4eb2_a3a9_c58143e835f9 "A physics-based model based on a physics equation describing the behaviour of electrons."@en .

ns1:EMMO_84cadc45_6758_46f2_ba2a_5ead65c70213 a owl:Class ;
    rdfs:label "AtomisticModel"@en ;
    rdfs:comment "A physics-based model based on a physics equation describing the behaviour of atoms."@en ;
    skos:prefLabel "AtomisticModel"@en ;
    ns1:EMMO_967080e5_2f42_4eb2_a3a9_c58143e835f9 "A physics-based model based on a physics equation describing the behaviour of atoms."@en .

ns1:EMMO_9335cf09_431f_4613_9dab_ce4ceaca965b a owl:Class ;
    rdfs:label "Simulation"@en ;
    rdfs:comment "A estimation of a property using a functional icon."@en ;
    rdfs:subClassOf ns1:EMMO_1c0b22a2_be82_4fa8_9e2b_a569a625d442,
        ns1:EMMO_eff42cb3_208e_4768_9a39_f8b6b3c3d7a2 ;
    skos:altLabel "Modelling"@en ;
    skos:example "I calculate the electrical conductivity of an Ar-He plasma with the Chapman-Enskog method and use the value as property for it."@en ;
    skos:prefLabel "Simulation"@en ;
    ns1:EMMO_967080e5_2f42_4eb2_a3a9_c58143e835f9 "A estimation of a property using a functional icon."@en .

ns1:EMMO_937757d3_ed79_4ae3_9513_3b135e58a6a1 a owl:Class ;
    rdfs:label "ScientificTheory"@en ;
    rdfs:comment "A scientific theory is a description, objective and observed, produced with scientific methodology."@en ;
    rdfs:subClassOf ns1:EMMO_1b6a95fb_3df7_44c9_ad3d_419c9c5fe7cb,
        ns1:EMMO_2a888cdf_ec4a_4ec5_af1c_0343372fc978,
        ns1:EMMO_8d2d9374_ef3a_47e6_8595_6bc208e07519 ;
    skos:prefLabel "ScientificTheory"@en ;
    ns1:EMMO_967080e5_2f42_4eb2_a3a9_c58143e835f9 "A scientific theory is a description, objective and observed, produced with scientific methodology."@en .

ns1:EMMO_cbf42aa6_9e11_4be8_932a_ae3c792ab17d a owl:Class ;
    rdfs:label "DataProcessingApplication"@en ;
    rdfs:subClassOf ns1:EMMO_3b031fa9_8623_4ea5_8b57_bcafb70c5c8b ;
    skos:prefLabel "DataProcessingApplication"@en .

ns1:EMMO_e5438930_04e7_4d42_ade5_3700d4a52ab7 a owl:Class ;
    rdfs:label "MaterialRelation"@en ;
    rdfs:comment "A material_relation can e.g. return a predefined number, return a database query, be an equation that depends on other physics_quantities."@en,
        "An 'equation' that stands for a physical assumption specific to a material, and provides an expression for a 'physics_quantity' (the dependent variable) as function of other variables, physics_quantity or data (independent variables)."@en ;
    rdfs:subClassOf ns1:EMMO_e56ee3eb_7609_4ae1_8bed_51974f0960a6 ;
    skos:example """The Lennard-Jones potential.
A force field.
An Hamiltonian."""@en ;
    skos:prefLabel "MaterialRelation"@en ;
    ns1:EMMO_967080e5_2f42_4eb2_a3a9_c58143e835f9 "An 'equation' that stands for a physical assumption specific to a material, and provides an expression for a 'physics_quantity' (the dependent variable) as function of other variables, physics_quantity or data (independent variables)."@en .

ns1:EMMO_f7ed665b_c2e1_42bc_889b_6b42ed3a36f0 a owl:Class ;
    rdfs:label "MathematicalModel"@en ;
    rdfs:comment """A mathematical model can be defined as a description of a system using mathematical concepts and language to facilitate proper explanation of a system or to study the effects of different components and to make predictions on patterns of behaviour.

Abramowitz and Stegun, 1968"""@en,
        "An analogical icon expressed in mathematical language."@en ;
    owl:equivalentClass [ a owl:Class ;
            owl:intersectionOf ( ns1:EMMO_4f2d1fcc_e20c_4479_9ad7_7a0480dd3e44 ns1:EMMO_54ee6b5e_5261_44a8_86eb_5717e7fdb9d0 ) ] ;
    skos:prefLabel "MathematicalModel"@en ;
    ns1:EMMO_967080e5_2f42_4eb2_a3a9_c58143e835f9 "An analogical icon expressed in mathematical language."@en .

ns1:EMMO_fbcc3aad_c58a_4185_bcc9_859db779b226 a owl:Class ;
    rdfs:label "TightlyCoupledModelsSimulation"@en ;
    rdfs:comment "A simulation in which more than one model are solved together with a coupled method."@en ;
    rdfs:subClassOf ns1:EMMO_02c4890b_aef3_4173_9669_94d1f6baf611 ;
    skos:example "Solving within the same linear system the discretised form of the pressure and momentum equation for a fluid, using the ideal gas law as material relation for connecting pressure to density."@en ;
    skos:prefLabel "TightlyCoupledModelsSimulation"@en ;
    ns1:EMMO_967080e5_2f42_4eb2_a3a9_c58143e835f9 "A simulation in which more than one model are solved together with a coupled method."@en .

ns1:EMMO_02c4890b_aef3_4173_9669_94d1f6baf611 a owl:Class ;
    rdfs:label "Coupled"@en ;
    rdfs:subClassOf ns1:EMMO_7d56ec24_499d_487a_af7d_a91aaa787bfe ;
    owl:equivalentClass [ a owl:Class ;
            owl:unionOf ( ns1:EMMO_01354ac2_cce1_4b7d_8b4a_7322d6cb10bc ns1:EMMO_fbcc3aad_c58a_4185_bcc9_859db779b226 ) ] ;
    skos:prefLabel "Coupled"@en .

ns1:EMMO_7d56ec24_499d_487a_af7d_a91aaa787bfe a owl:Class ;
    rdfs:label "MultiSimulation"@en ;
    rdfs:comment "A physics based simulation with multiple physics based models."@en ;
    rdfs:subClassOf ns1:EMMO_e97af6ec_4371_4bbc_8936_34b76e33302f ;
    skos:prefLabel "MultiSimulation"@en ;
    ns1:EMMO_967080e5_2f42_4eb2_a3a9_c58143e835f9 "A physics based simulation with multiple physics based models."@en .

ns1:EMMO_db9a009e_f097_43f5_9520_6cbc07e7610b a owl:Class ;
    rdfs:label "NaturalLaw"@en ;
    rdfs:comment "A scientific theory that focuses on a specific phenomena, for which a single statement (not necessariliy in mathematical form) can be expressed."@en ;
    rdfs:subClassOf ns1:EMMO_937757d3_ed79_4ae3_9513_3b135e58a6a1 ;
    skos:prefLabel "NaturalLaw"@en ;
    ns1:EMMO_967080e5_2f42_4eb2_a3a9_c58143e835f9 "A scientific theory that focuses on a specific phenomena, for which a single statement (not necessariliy in mathematical form) can be expressed."@en .

ns1:EMMO_8b66ada5_510c_44bd_a8d8_3c64d301a5e9 a owl:Class ;
    rdfs:label "SimulationApplication"@en ;
    rdfs:comment "An application aimed to functionally reproduce an object."@en ;
    rdfs:subClassOf ns1:EMMO_3b031fa9_8623_4ea5_8b57_bcafb70c5c8b,
        ns1:EMMO_c7013b53_3071_410b_a5e4_a8d266dcdfb5 ;
    skos:example "An application that predicts the pressure drop of a fluid in a pipe segment is aimed to functionally reproduce the outcome of a measurement of pressure before and after the segment."@en ;
    skos:prefLabel "SimulationApplication"@en ;
    ns1:EMMO_967080e5_2f42_4eb2_a3a9_c58143e835f9 "An application aimed to functionally reproduce an object."@en .

ns1:EMMO_b29fd350_39aa_4af7_9459_3faa0544cba6 a owl:Class ;
    rdfs:label "PhysicsBasedModel"@en ;
    rdfs:comment "A mathematical entity based on a fundamental physics theory which defines the relations between physics quantities of an entity."@en ;
    rdfs:isDefinedBy "CEN Workshop Agreement – CWA 17284 “Materials modelling – terminology, classification and metadata”"@en ;
    rdfs:subClassOf [ a owl:Restriction ;
            owl:onProperty ns1:EMMO_dc57d998_23db_4d8e_b2cd_f346b195b846 ;
            owl:someValuesFrom ns1:EMMO_27c5d8c6_8af7_4d63_beb1_ec37cd8b3fa3 ],
        ns1:EMMO_f7ed665b_c2e1_42bc_889b_6b42ed3a36f0 ;
    skos:prefLabel "PhysicsBasedModel"@en ;
    ns1:EMMO_967080e5_2f42_4eb2_a3a9_c58143e835f9 "A mathematical entity based on a fundamental physics theory which defines the relations between physics quantities of an entity."@en .

ns1:EMMO_c7013b53_3071_410b_a5e4_a8d266dcdfb5 skos:example "A guinea pig."@en .

ns1:EMMO_e97af6ec_4371_4bbc_8936_34b76e33302f a owl:Class ;
    rdfs:label "PhysicsBasedSimulation"@en ;
    rdfs:comment "A simulation that relies on physics based models, according to the Review of Materials Modelling and CWA 17284:2018."@en ;
    rdfs:isDefinedBy "CEN Workshop Agreement – CWA 17284 “Materials modelling – terminology, classification and metadata”"@en ;
    rdfs:subClassOf ns1:EMMO_9335cf09_431f_4613_9dab_ce4ceaca965b ;
    skos:prefLabel "PhysicsBasedSimulation"@en ;
    ns1:EMMO_967080e5_2f42_4eb2_a3a9_c58143e835f9 "A simulation that relies on physics based models, according to the Review of Materials Modelling and CWA 17284:2018."@en .

ns1:EMMO_8d2d9374_ef3a_47e6_8595_6bc208e07519 a owl:Class ;
    rdfs:label "Theory"@en ;
    rdfs:comment "A 'conventional' that stand for a 'physical'."@en,
        """The 'theory' is e.g. a proposition, a book or a paper whose sub-symbols suggest in the mind of the interpreter an interpretant structure that can represent a 'physical'.

It is not an 'icon' (like a math equation), because it has no common resemblance or logical structure with the 'physical'.

In Peirce semiotics: legisign-symbol-argument"""@en ;
    rdfs:subClassOf ns1:EMMO_35d4c439_fcb6_4399_a855_a89a207b41e9 ;
    skos:prefLabel "Theory"@en ;
    ns1:EMMO_967080e5_2f42_4eb2_a3a9_c58143e835f9 "A 'conventional' that stand for a 'physical'."@en .

ns1:EMMO_eff42cb3_208e_4768_9a39_f8b6b3c3d7a2 a owl:Class ;
    rdfs:label "Computation"@en ;
    rdfs:comment "A procedure that deals with quantitative symbols (i.e. symbols associated with a quantitative oriented language)."@en ;
    rdfs:subClassOf ns1:EMMO_472a0ca2_58bf_4618_b561_6fe68bd9fd49 ;
    skos:example """A mathematician that calculates 2+2.
A computation machine that calculate the average value of a dataset."""@en ;
    skos:prefLabel "Computation"@en ;
    ns1:EMMO_967080e5_2f42_4eb2_a3a9_c58143e835f9 "A procedure that deals with quantitative symbols (i.e. symbols associated with a quantitative oriented language)."@en .

[] a owl:Axiom ;
    owl:annotatedProperty skos:prefLabel ;
    owl:annotatedSource ns1:EMMO_eff42cb3_208e_4768_9a39_f8b6b3c3d7a2 ;
    owl:annotatedTarget "Computation"@en ;
    ns1:EMMO_705f27ae_954c_4f13_98aa_18473fc52b25 "From Latin con- +‎ putō (“I reckon”)."@en .

[] a owl:Axiom ;
    rdfs:seeAlso "https://www.cencenelec.eu/media/CEN-CENELEC/CWAs/RI/cwa17284_2018.pdf"^^xsd:anyURI ;
    owl:annotatedProperty rdfs:isDefinedBy ;
    owl:annotatedSource ns1:EMMO_e97af6ec_4371_4bbc_8936_34b76e33302f ;
    owl:annotatedTarget "CEN Workshop Agreement – CWA 17284 “Materials modelling – terminology, classification and metadata”"@en .

[] a owl:Axiom ;
    rdfs:seeAlso "https://www.cencenelec.eu/media/CEN-CENELEC/CWAs/RI/cwa17284_2018.pdf"^^xsd:anyURI ;
    owl:annotatedProperty rdfs:isDefinedBy ;
    owl:annotatedSource ns1:EMMO_b29fd350_39aa_4af7_9459_3faa0544cba6 ;
    owl:annotatedTarget "CEN Workshop Agreement – CWA 17284 “Materials modelling – terminology, classification and metadata”"@en .

