@prefix dcterms: <http://purl.org/dc/terms/> .
@prefix emmo: <https://w3id.org/emmo#> .
@prefix owl: <http://www.w3.org/2002/07/owl#> .
@prefix rdfs: <http://www.w3.org/2000/01/rdf-schema#> .
@prefix skos: <http://www.w3.org/2004/02/skos/core#> .
@prefix xsd: <http://www.w3.org/2001/XMLSchema#> .

emmo:EMMO_0277f24a_ea7f_4917_81b7_fb0406c8fc62 rdfs:label "Holistic"@en ;
    rdfs:comment """A perspective characterized by the belief that:
- a whole is more than merely the sum of its parts (wholism)
- the parts of a whole are interconnected in a way that can be explained only by reference to the whole (rolism)."""@en,
        """An holistic perspective considers each part of the whole as equally important, without the need to position the parts within a hierarchy (in time or space). The interest is on the whole, on its parts (how they contribute to the whole, i.e. their roles), and their types, without going further into specifying the spatial hierarchy or the temporal position of each part.
This class allows the picking of parts without necessarily going trough a rigid hierarchy of spatial compositions (e.g. body -> organ -> cell -> molecule) or temporal composition. This is inline with the transitive nature of parthood, as it is usually defined in literature."""@en,
        "The union of classes whole and part."@en .

emmo:EMMO_1823c7ec_e097_4cfb_ad1a_ddbe42cb904b a owl:Class ;
    rdfs:label "SharedAgency"@en ;
    rdfs:comment "Shared agency occurs when two or more individuals do something together."@en ;
    rdfs:isDefinedBy <https://plato.stanford.edu/entries/agency/#OthKinAgeMenShaColRelArt> ;
    rdfs:subClassOf [ a owl:Restriction ;
            owl:onProperty emmo:EMMO_cd24eb82_a11c_4a31_96ea_32f870c5580a ;
            owl:someValuesFrom emmo:EMMO_9b52133b_8f6c_47fb_93f1_419071db3f4b ],
        emmo:EMMO_8af3b008_0e32_4684_85ab_a52a8e7b6877 ;
    skos:prefLabel "SharedAgency"@en ;
    emmo:EMMO_967080e5_2f42_4eb2_a3a9_c58143e835f9 "Shared agency occurs when two or more individuals do something together."@en .

emmo:EMMO_7c2c9869_f6b4_4e5d_8195_4578b17add3e a owl:Class ;
    rdfs:label "SpontaneousProcess"@en ;
    rdfs:comment "A process that has no identifiable agent driving its occurence."@en ;
    rdfs:subClassOf emmo:EMMO_f53f45f2_c354_417c_a904_a2606ad584d7 ;
    skos:altLabel "NaturalProcess"@en ;
    skos:prefLabel "SpontaneousProcess"@en ;
    emmo:EMMO_967080e5_2f42_4eb2_a3a9_c58143e835f9 "A process that has no identifiable agent driving its occurence."@en .

emmo:EMMO_7e963f56_624a_4091_86ec_3b2c609e76bb a owl:Class ;
    rdfs:label "MentalAgency"@en ;
    rdfs:comment "An intentional agency caused by the agent’s mental states and events."@en ;
    rdfs:isDefinedBy <https://plato.stanford.edu/entries/agency/#OthKinAgeMenShaColRelArt> ;
    rdfs:subClassOf [ a owl:Restriction ;
            owl:onProperty emmo:EMMO_cd24eb82_a11c_4a31_96ea_32f870c5580a ;
            owl:someValuesFrom emmo:EMMO_3674bfb6_6636_4e9d_aae1_07023ad96d61 ],
        emmo:EMMO_8af3b008_0e32_4684_85ab_a52a8e7b6877 ;
    skos:prefLabel "MentalAgency"@en ;
    emmo:EMMO_967080e5_2f42_4eb2_a3a9_c58143e835f9 "An intentional agency caused by the agent’s mental states and events."@en ;
    emmo:EMMO_c7b62dd7_063a_4c2a_8504_42f7264ba83f "Mental states are strictly connected to the definition of mind, which is traditionally connected to high cognitive skills, such as the one provided by human beings brains."@en .

emmo:EMMO_8aba9715_d542_4a79_a778_6115d2b4febd a owl:Class ;
    rdfs:label "CollectiveAgency"@en ;
    rdfs:comment "Collective agency occurs when two or more individuals act as a group, in accordance with certain principles or procedures that constitute and organize the group."@en ;
    rdfs:isDefinedBy <https://plato.stanford.edu/entries/agency/#OthKinAgeMenShaColRelArt> ;
    rdfs:subClassOf [ a owl:Restriction ;
            owl:onProperty emmo:EMMO_cd24eb82_a11c_4a31_96ea_32f870c5580a ;
            owl:someValuesFrom emmo:EMMO_94c663c8_1d99_45aa_a172_93d19ea95856 ],
        emmo:EMMO_8af3b008_0e32_4684_85ab_a52a8e7b6877 ;
    skos:prefLabel "CollectiveAgency"@en ;
    emmo:EMMO_967080e5_2f42_4eb2_a3a9_c58143e835f9 "Collective agency occurs when two or more individuals act as a group, in accordance with certain principles or procedures that constitute and organize the group."@en ;
    emmo:EMMO_c7b62dd7_063a_4c2a_8504_42f7264ba83f "The group acting collectively is intended to be represented as an item, meaning that all members of the group should have had at least one causal interaction with another member. The collective action in fact is taken in accordance with certain principles or procedures that constitute and organize the group itself that requires implicitly a causal interaction between members."@en .

emmo:EMMO_90ae56e4_d197_49b6_be1a_0049e4756606 rdfs:label "Object"@en ;
    rdfs:comment "An item can be classified as an object according to a type ϕ (a ϕ-object) if it's a ϕ all its temporal item parts are also of type ϕ. This conceptualisation tries to catch the persistency of type in the temporal parts of an entity."@en,
        "The superclass for causal structure classes whose individuals have all temporal item parts of the same type of the whole."@en .

emmo:EMMO_946b5162_95b0_4801_81d4_efef43842a0d rdfs:label "QualifiedRole"@en ;
    rdfs:comment """The qualified role concept express the requirement for an entity of a type, say A, to be part of a larger entity of another type, say B, with A and B belonging to different taxonomical branches.
The concept of role is then defined as something that needs a wider and specific environment to exist.
For example, the car radio type requires all instances to be a part of a car, while the opposite (the car having a radio) is not mandatory for qualified roles.  The same applies for airplane winglets that are by definition an optional part of an airplane. Food preservatives are anothe optional part of foods."""@en,
        "The superclass for all classes of individuals that requires their individuals to be part of another specific class of entity of different type with a specific role with respect to it."@en .

emmo:EMMO_9d799b43_e188_4047_8167_121d96b31a26 rdfs:label "ObjectByContext"@en ;
    rdfs:comment "The superclass for all classes that categorise objects according to their mereological and persistence context"@en .

emmo:EMMO_b91749cd_0dec_43d1_8f77_e266c762bccd a owl:Class ;
    rdfs:label "UnintentionalAgency"@en ;
    rdfs:comment "A process that does not have an active participation of an intentional agent driving it."@en ;
    rdfs:subClassOf [ a owl:Restriction ;
            owl:onProperty emmo:EMMO_cd24eb82_a11c_4a31_96ea_32f870c5580a ;
            owl:someValuesFrom emmo:EMMO_fe1b173e_b3ce_403d_9d90_230a334eebf9 ],
        emmo:EMMO_a49c2441_1e54_43f0_a1cf_2f553a23ac34 ;
    skos:prefLabel "UnintentionalAgency"@en ;
    emmo:EMMO_967080e5_2f42_4eb2_a3a9_c58143e835f9 "A process that does not have an active participation of an intentional agent driving it."@en .

emmo:EMMO_e04884d9_eda6_487e_93d5_7722d7eda96b rdfs:label "Persistence"@en ;
    rdfs:comment "The union of the object or process classes."@en .

emmo:EMMO_eb50c9cb_9576_4a61_95ec_f81fb8218187 rdfs:label "QualifiedWhole"@en ;
    rdfs:comment """The qualified whole concept express the requirement for an entity of a type, say A, to have a part of another type, say B, with A and B belonging to different taxonomical branches.
The concept of whole is then defined as something that needs a part of a specific type to exist.
For example, an atom always requires a nucleus part to exist (but not viceversa)"""@en,
        "The superclass for all classes of individuals that requires to have a part of another specific class of entity of different type with a specific relation with it."@en .

emmo:EMMO_f1027c92_b145_48c7_aa42_3d831a6f2039 a owl:Class ;
    rdfs:label "NonAgent"@en ;
    rdfs:comment "A participant that does not have an active role in driving the process."@en ;
    rdfs:subClassOf emmo:EMMO_cede9297_c60d_4487_9207_62ac963202b5 ;
    skos:prefLabel "NonAgent"@en ;
    emmo:EMMO_967080e5_2f42_4eb2_a3a9_c58143e835f9 "A participant that does not have an active role in driving the process."@en .

emmo:EMMO_fe527062_5869_46af_a351_f81d0ca18fad a owl:Class ;
    rdfs:label "ArtificialAgency"@en ;
    rdfs:comment "An intentional agency exercised by artificial systems that have internal states that enables adaptive regulation of the agent’s coupling with the environment and metabolic self-maintenance."^^xsd:string ;
    rdfs:isDefinedBy <https://plato.stanford.edu/entries/agency/#OthKinAgeMenShaColRelArt> ;
    rdfs:subClassOf [ a owl:Restriction ;
            owl:onProperty emmo:EMMO_cd24eb82_a11c_4a31_96ea_32f870c5580a ;
            owl:someValuesFrom emmo:EMMO_7cb03f8e_6062_4106_9ffb_38cbe8eaa5f6 ],
        emmo:EMMO_8af3b008_0e32_4684_85ab_a52a8e7b6877 ;
    skos:prefLabel "ArtificialAgency"@en ;
    emmo:EMMO_967080e5_2f42_4eb2_a3a9_c58143e835f9 "An intentional agency exercised by artificial systems that have internal states that enables adaptive regulation of the agent’s coupling with the environment and metabolic self-maintenance."^^xsd:string .

<https://w3id.org/emmo/reference/agency> a owl:Ontology ;
    dcterms:abstract """This EMMO module deals with the representation of 'agency', meaning the manifestation of the capacity of an entity to act, the so called 'agent'. Moreover, based on philosophical motivations, the module provide a distinction between intentional and unintentional acts.
The represeantion is part of the EMMO framework and makes use of mereocausality to represent the agency act."""@en ;
    dcterms:contributor <https://orcid.org/0000-0002-1560-809X>,
        <https://orcid.org/0000-0002-4181-2852>,
        <https://orcid.org/0009-0008-8009-5009> ;
    dcterms:creator <https://orcid.org/0000-0003-3805-8761> ;
    dcterms:license "https://creativecommons.org/licenses/by/4.0/legalcode"^^xsd:string ;
    dcterms:publisher <https://emmc.eu> ;
    dcterms:title "Agency"@en ;
    rdfs:comment "The EMMO requires HermiT reasoner plugin in order to visualize all inferences and class hierarchy (ctrl+R hotkey in Protege)."@en ;
    owl:imports <https://w3id.org/emmo/1.0.3/perspectives/semiotics>,
        <https://w3id.org/emmo/1.0.3/reference/persholistic> ;
    owl:versionIRI <https://w3id.org/emmo/1.0.3/reference/agency> ;
    owl:versionInfo "1.0.3"^^xsd:string ;
    emmo:EMMO_1246b120_abbe_4840_b0f8_3e4348b24a17 "emmo@emmc.eu"^^xsd:string .

emmo:EMMO_13191289_6c2b_4741_93e1_82d53bd0e703 rdfs:label "Participant"@en ;
    rdfs:comment "An object which is a spatial part of a process."@en .

emmo:EMMO_1efe8b96_e006_4a33_bc9a_421406cbb9f0 rdfs:label "Whole"@en ;
    rdfs:comment "The superclass of entities which are defined by requiring the existence of some parts (at least one) of specifically given types, where the specified types are different with respect to the type of the whole."@en .

emmo:EMMO_3674bfb6_6636_4e9d_aae1_07023ad96d61 a owl:Class ;
    rdfs:label "MentalAgent"@en ;
    rdfs:comment "A biological agent possessing an intentional mental state."@en ;
    rdfs:isDefinedBy <https://plato.stanford.edu/entries/agency/#OthKinAgeMenShaColRelArt> ;
    rdfs:subClassOf emmo:EMMO_7a317af2_d2f7_4e8a_8fbd_aaebfb7d21cc ;
    skos:prefLabel "MentalAgent"@en ;
    emmo:EMMO_967080e5_2f42_4eb2_a3a9_c58143e835f9 "A biological agent possessing an intentional mental state."@en ;
    emmo:EMMO_c7b62dd7_063a_4c2a_8504_42f7264ba83f "A mental agent is typically attributed to a human but not nessesary."@en .

emmo:EMMO_4f226cf3_6d02_4d35_8566_a9e641bc6ff3 rdfs:label "Role"@en ;
    rdfs:comment """A role entity is categorized according to its relation with the whole, i.e. how it contribute to make a specific whole, and not as standalone entity.
This class is expected to host the definition of world objects as they appear in its relation with the surrounding whole (being a part implies being surrounded by something bigger to which it contributes).
For example. a human being is a stand alone type, but an instance of a human being can also be an instance of the type student (intended as a role) if it plays a part into a school environment (i.e., a student entity can exist only if it is part of a surrounding whole: the school).
The role type requires that also the whole type depends on the existence of parts of a specific type (e.g., there is no school without students)."""@en,
        "An entity that is categorized according to its relation with a whole through a parthood relation and that contributes to it according to an holistic criterion, where the type of the whole is not the type of the part."@en .

emmo:EMMO_7cb03f8e_6062_4106_9ffb_38cbe8eaa5f6 a owl:Class ;
    rdfs:label "ArtificialIntelligence"@en ;
    rdfs:comment "An agent that is a machine-learning or symbolic reasoning system (not biological-based)."@en ;
    rdfs:isDefinedBy <https://plato.stanford.edu/entries/agency/#OthKinAgeMenShaColRelArt> ;
    rdfs:subClassOf emmo:EMMO_7a317af2_d2f7_4e8a_8fbd_aaebfb7d21cc ;
    skos:altLabel "ArtificialAgent"@en ;
    skos:prefLabel "ArtificialIntelligence"@en ;
    emmo:EMMO_967080e5_2f42_4eb2_a3a9_c58143e835f9 "An agent that is a machine-learning or symbolic reasoning system (not biological-based)."@en .

emmo:EMMO_94c663c8_1d99_45aa_a172_93d19ea95856 a owl:Class ;
    rdfs:label "CollectiveAgent"@en ;
    rdfs:comment "An intentional agent that takes part in driving a process as part of a group."@en ;
    rdfs:isDefinedBy <https://plato.stanford.edu/entries/agency/#OthKinAgeMenShaColRelArt> ;
    rdfs:subClassOf emmo:EMMO_7a317af2_d2f7_4e8a_8fbd_aaebfb7d21cc ;
    skos:example "A catalyst that together with another catalyst drives a chemical process that needs both catalysts to occur."@en ;
    skos:prefLabel "CollectiveAgent"@en ;
    emmo:EMMO_967080e5_2f42_4eb2_a3a9_c58143e835f9 "An intentional agent that takes part in driving a process as part of a group."@en .

emmo:EMMO_9b52133b_8f6c_47fb_93f1_419071db3f4b a owl:Class ;
    rdfs:label "SharedAgent"@en ;
    rdfs:comment "An intentional agent that takes part in driving a process without being a group."@en ;
    rdfs:isDefinedBy <https://plato.stanford.edu/entries/agency/#OthKinAgeMenShaColRelArt> ;
    rdfs:subClassOf emmo:EMMO_7a317af2_d2f7_4e8a_8fbd_aaebfb7d21cc ;
    skos:example """Singing a song together with others.
Carrying a piece of furniture together with others."""@en ;
    skos:prefLabel "SharedAgent"@en ;
    emmo:EMMO_967080e5_2f42_4eb2_a3a9_c58143e835f9 "An intentional agent that takes part in driving a process without being a group."@en .

emmo:EMMO_fe1b173e_b3ce_403d_9d90_230a334eebf9 a owl:Class ;
    rdfs:label "UnintentionalAgent"@en ;
    rdfs:comment "An agent that is driven by the law of physics rather than the intention to reach a defined objective."@en ;
    rdfs:subClassOf emmo:EMMO_2480b72b_db8d_460f_9a5f_c2912f979046 ;
    skos:example "A catalyst."@en ;
    skos:prefLabel "UnintentionalAgent"@en ;
    emmo:EMMO_967080e5_2f42_4eb2_a3a9_c58143e835f9 "An agent that is driven by the law of physics rather than the intention to reach a defined objective."@en .

emmo:EMMO_43e9a05d_98af_41b4_92f6_00f79a09bfce rdfs:label "Process"@en ;
    rdfs:comment "The superclass for causal structure classes whose individuals have some temporal item parts that are not of the same type of the whole."@en .

emmo:EMMO_c130614a_2985_476d_a7ed_8a137847703c a owl:Class ;
    rdfs:label "IntentionalAgent"@en ;
    rdfs:comment "An agent that is driven by the intention to reach a defined objective in driving a process."@en ;
    rdfs:seeAlso <https://plato.stanford.edu/entries/agency> ;
    rdfs:subClassOf [ a owl:Restriction ;
            owl:onProperty [ owl:inverseOf emmo:EMMO_cd24eb82_a11c_4a31_96ea_32f870c5580a ] ;
            owl:someValuesFrom emmo:EMMO_bafc17b5_9be4_4823_8bbe_ab4e90b6738c ],
        emmo:EMMO_2480b72b_db8d_460f_9a5f_c2912f979046 ;
    skos:prefLabel "IntentionalAgent"@en ;
    emmo:EMMO_967080e5_2f42_4eb2_a3a9_c58143e835f9 "An agent that is driven by the intention to reach a defined objective in driving a process."@en ;
    emmo:EMMO_c7b62dd7_063a_4c2a_8504_42f7264ba83f "Intentionality is not limited to human agents, but in general to all agents that have the capacity to decide to act in driving a process according to a motivation."@en .

emmo:EMMO_cede9297_c60d_4487_9207_62ac963202b5 a owl:Class ;
    rdfs:label "ParticipantByAgency"@en ;
    rdfs:comment "Categorisation of participant in terms of being an agent or not an agent."@en ;
    rdfs:subClassOf emmo:EMMO_13191289_6c2b_4741_93e1_82d53bd0e703 ;
    skos:prefLabel "ParticipantByAgency"@en ;
    emmo:EMMO_8a137e9f_579c_4e28_baca_e8980eb0c3db "EquivalentTo: Agent or NonAgent"^^xsd:string ;
    emmo:EMMO_967080e5_2f42_4eb2_a3a9_c58143e835f9 "Categorisation of participant in terms of being an agent or not an agent."@en .

emmo:EMMO_f53f45f2_c354_417c_a904_a2606ad584d7 a owl:Class ;
    rdfs:label "ProcessByAgency"@en ;
    rdfs:comment "Categorisation of processes by whether they are driven by an agent or not."@en ;
    rdfs:subClassOf emmo:EMMO_43e9a05d_98af_41b4_92f6_00f79a09bfce ;
    skos:prefLabel "ProcessByAgency"@en ;
    emmo:EMMO_967080e5_2f42_4eb2_a3a9_c58143e835f9 "Categorisation of processes by whether they are driven by an agent or not."@en .

emmo:EMMO_a49c2441_1e54_43f0_a1cf_2f553a23ac34 a owl:Class ;
    rdfs:label "Agency"@en ;
    rdfs:comment "A process that occurs because of the exercise of the capacity to act of an agent."@en ;
    rdfs:subClassOf [ a owl:Restriction ;
            owl:onProperty emmo:EMMO_cd24eb82_a11c_4a31_96ea_32f870c5580a ;
            owl:someValuesFrom emmo:EMMO_2480b72b_db8d_460f_9a5f_c2912f979046 ],
        emmo:EMMO_1efe8b96_e006_4a33_bc9a_421406cbb9f0,
        emmo:EMMO_f53f45f2_c354_417c_a904_a2606ad584d7 ;
    skos:altLabel "AgentDrivenProcess"@en ;
    skos:prefLabel "Agency"@en ;
    emmo:EMMO_967080e5_2f42_4eb2_a3a9_c58143e835f9 "A process that occurs because of the exercise of the capacity to act of an agent."@en .

emmo:EMMO_7a317af2_d2f7_4e8a_8fbd_aaebfb7d21cc a owl:Class ;
    rdfs:label "IntentionalAgentByKind"@en ;
    rdfs:comment "Categorisation of intentional agents by their kind."@en ;
    rdfs:subClassOf emmo:EMMO_c130614a_2985_476d_a7ed_8a137847703c ;
    skos:prefLabel "IntentionalAgentByKind"@en ;
    emmo:EMMO_967080e5_2f42_4eb2_a3a9_c58143e835f9 "Categorisation of intentional agents by their kind."@en .

emmo:EMMO_8af3b008_0e32_4684_85ab_a52a8e7b6877 a owl:Class ;
    rdfs:label "IntentionalAgencyByKind"@en ;
    rdfs:comment "Categorisation of intentional agencies by their kind."@en ;
    rdfs:subClassOf emmo:EMMO_bafc17b5_9be4_4823_8bbe_ab4e90b6738c ;
    skos:prefLabel "IntentionalAgencyByKind"@en ;
    emmo:EMMO_967080e5_2f42_4eb2_a3a9_c58143e835f9 "Categorisation of intentional agencies by their kind."@en .

emmo:EMMO_bafc17b5_9be4_4823_8bbe_ab4e90b6738c a owl:Class ;
    rdfs:label "IntentionalAgency"@en ;
    rdfs:comment "A process occurring with the active participation of an intentional agent that drives the process according to a specific objective (intention)."@en ;
    rdfs:subClassOf [ a owl:Restriction ;
            owl:onProperty emmo:EMMO_cd24eb82_a11c_4a31_96ea_32f870c5580a ;
            owl:someValuesFrom emmo:EMMO_c130614a_2985_476d_a7ed_8a137847703c ],
        emmo:EMMO_a49c2441_1e54_43f0_a1cf_2f553a23ac34 ;
    skos:altLabel "IntentionalProcess"@en ;
    skos:prefLabel "IntentionalAgency"@en ;
    emmo:EMMO_8a137e9f_579c_4e28_baca_e8980eb0c3db "SubClassOf: hasAgent some IntentionalAgent"^^xsd:string ;
    emmo:EMMO_967080e5_2f42_4eb2_a3a9_c58143e835f9 "A process occurring with the active participation of an intentional agent that drives the process according to a specific objective (intention)."@en ;
    emmo:EMMO_c7b62dd7_063a_4c2a_8504_42f7264ba83f """The concept is not restricted to agencies where the agent accomplish its intention. For example, breaking a vase while reaching for a book is an intentional agency, because the action causing the vase to fall and break follows a volition (i.e., an act of willing).
Intentional agency may be further categorised acccording to the fact that the some of the resulting processes may or may not be coherent with the volition."""@en .

emmo:EMMO_2480b72b_db8d_460f_9a5f_c2912f979046 a owl:Class ;
    rdfs:label "Agent"@en ;
    rdfs:comment "A participant that is the driver of a process."@en ;
    rdfs:subClassOf [ a owl:Restriction ;
            owl:onProperty [ owl:inverseOf emmo:EMMO_cd24eb82_a11c_4a31_96ea_32f870c5580a ] ;
            owl:someValuesFrom emmo:EMMO_43e9a05d_98af_41b4_92f6_00f79a09bfce ],
        emmo:EMMO_4f226cf3_6d02_4d35_8566_a9e641bc6ff3,
        emmo:EMMO_cede9297_c60d_4487_9207_62ac963202b5 ;
    owl:priorVersion """The agent concept identifies the parts of a process that are also its drivers. An agent part has an active role with respect to any other generic part, meaning that is involved in the causal chain that characterize the process. An agent is a participant, meaning that is qualifiable as an object.
As for all holistic relations, there is a level of subjectivity in drawing whole-role relations, so that the identification of an agent within a process is not fully axiomatizable.
What is axiomatically expressible is that an agent requires to be part of a process (i.e., an agent exists only within a process) but a process may not require an agent to exist (qualified role). Agentless processes may have a distributed causality chain so that the agency is exerted collectively and there is no motivation to draw an holistic connection between the whole and some parts. For example, the breaking of a nail can be caused by an agent such as an hammer, or by the rusting process which is not a participant as required by the agent definition. 
This concept covers both intentional and non intentional agency."""@en ;
    skos:example "A catalyst. A bus driver. A substance that is initiating a reaction that would not occur without its presence."@en ;
    skos:prefLabel "Agent"@en ;
    emmo:EMMO_8a137e9f_579c_4e28_baca_e8980eb0c3db "EquivalentTo: IntentionalAgent or UnintentionalAgent"^^xsd:string ;
    emmo:EMMO_967080e5_2f42_4eb2_a3a9_c58143e835f9 "A participant that is the driver of a process."@en ;
    emmo:EMMO_c7b62dd7_063a_4c2a_8504_42f7264ba83f "An agent is not necessarily human. In fact, the concept of agent has been generalised to encompass both intentional and unintentional acts primarily to take into account usage of the term in chemistry (e.g., chemical agent that intiitate a reaction), inline also with the most recent development in the philosophical debate."@en .

emmo:EMMO_cd24eb82_a11c_4a31_96ea_32f870c5580a a owl:ObjectProperty ;
    rdfs:label "hasAgent"@en ;
    rdfs:comment "The relation within a process and an agengt participant."@en ;
    rdfs:domain emmo:EMMO_a49c2441_1e54_43f0_a1cf_2f553a23ac34 ;
    rdfs:range emmo:EMMO_2480b72b_db8d_460f_9a5f_c2912f979046 ;
    rdfs:subPropertyOf emmo:EMMO_8e52c42b_e879_4473_9fa1_4b23428b392b,
        emmo:EMMO_ae2d1a96_bfa1_409a_a7d2_03d69e8a125a ;
    skos:prefLabel "hasAgent"@en ;
    emmo:EMMO_967080e5_2f42_4eb2_a3a9_c58143e835f9 "The relation within a process and an agengt participant."@en .

[] a owl:Axiom ;
    rdfs:seeAlso <https://plato.stanford.edu/entries/agency> ;
    owl:annotatedProperty owl:priorVersion ;
    owl:annotatedSource emmo:EMMO_2480b72b_db8d_460f_9a5f_c2912f979046 ;
    owl:annotatedTarget """The agent concept identifies the parts of a process that are also its drivers. An agent part has an active role with respect to any other generic part, meaning that is involved in the causal chain that characterize the process. An agent is a participant, meaning that is qualifiable as an object.
As for all holistic relations, there is a level of subjectivity in drawing whole-role relations, so that the identification of an agent within a process is not fully axiomatizable.
What is axiomatically expressible is that an agent requires to be part of a process (i.e., an agent exists only within a process) but a process may not require an agent to exist (qualified role). Agentless processes may have a distributed causality chain so that the agency is exerted collectively and there is no motivation to draw an holistic connection between the whole and some parts. For example, the breaking of a nail can be caused by an agent such as an hammer, or by the rusting process which is not a participant as required by the agent definition. 
This concept covers both intentional and non intentional agency."""@en .

[] a owl:Axiom ;
    owl:annotatedProperty skos:altLabel ;
    owl:annotatedSource emmo:EMMO_bafc17b5_9be4_4823_8bbe_ab4e90b6738c ;
    owl:annotatedTarget "IntentionalProcess"@en ;
    emmo:EMMO_705f27ae_954c_4f13_98aa_18473fc52b25 "From Latin intentionem, derived from intendere (\"stretching out\")"@en .

[] a owl:Axiom ;
    owl:annotatedProperty skos:prefLabel ;
    owl:annotatedSource emmo:EMMO_bafc17b5_9be4_4823_8bbe_ab4e90b6738c ;
    owl:annotatedTarget "IntentionalAgency"@en ;
    emmo:EMMO_705f27ae_954c_4f13_98aa_18473fc52b25 "From Latin agēns (present participle of agere (“to act”))"@en .

