@prefix dcterms: <http://purl.org/dc/terms/> .
@prefix ns1: <https://w3id.org/emmo#> .
@prefix owl: <http://www.w3.org/2002/07/owl#> .
@prefix rdfs: <http://www.w3.org/2000/01/rdf-schema#> .
@prefix schema: <https://schema.org/> .
@prefix skos: <http://www.w3.org/2004/02/skos/core#> .
@prefix xsd: <http://www.w3.org/2001/XMLSchema#> .

ns1:AmperePerDegreeCelsius a owl:Class ;
    rdfs:label "AmperePerDegreeCelsius"@en ;
    rdfs:comment """A measure used to express how a current is subject to temperature. Originally used in Wien's Law to describe phenomena related to filaments. One use today is to express how a current generator derates with temperature.

-- QUDT"""@en ;
    rdfs:isDefinedBy "http://qudt.org/2.1/vocab/unit"^^xsd:string ;
    rdfs:seeAlso "http://web.mit.edu/course/21/21.guide/use-tab.htm"^^xsd:string ;
    rdfs:subClassOf [ a owl:Restriction ;
            owl:hasValue 0e+00 ;
            owl:onProperty ns1:hasSIConversionOffset ],
        [ a owl:Restriction ;
            owl:hasValue 5.729578e+01 ;
            owl:onProperty ns1:hasSIConversionMultiplier ],
        ns1:ElectricCurrentPerTemperatureUnit,
        ns1:SICoherentDerivedUnit ;
    skos:altLabel "Ampere per Degree Celsius"@en ;
    skos:prefLabel "AmperePerDegreeCelsius"@en ;
    ns1:elucidation """A measure used to express how a current is subject to temperature. Originally used in Wien's Law to describe phenomena related to filaments. One use today is to express how a current generator derates with temperature.

-- QUDT"""@en ;
    ns1:qudtReference "http://qudt.org/vocab/unit/A-PER-DEG_C"^^xsd:string ;
    ns1:ucumCode "A.Cel-1"^^xsd:string,
        "A/Cel"^^xsd:string ;
    ns1:unitSymbol "A/°C"^^xsd:string .

ns1:AmperePerJoule a owl:Class ;
    rdfs:label "AmperePerJoule"@en ;
    rdfs:comment """The inverse measure of joule-per-ampere or weber. The measure for the reciprical of magnetic flux.

-- QUDT"""@en ;
    rdfs:isDefinedBy "http://qudt.org/2.1/vocab/unit"^^xsd:string ;
    rdfs:subClassOf [ a owl:Restriction ;
            owl:hasValue 1e+00 ;
            owl:onProperty ns1:hasSIConversionMultiplier ],
        [ a owl:Restriction ;
            owl:hasValue 0e+00 ;
            owl:onProperty ns1:hasSIConversionOffset ],
        ns1:ElectricCurrentPerUnitEnergyUnit,
        ns1:SICoherentDerivedUnit ;
    skos:altLabel "Ampere per Joule"@en ;
    skos:prefLabel "AmperePerJoule"@en ;
    ns1:elucidation """The inverse measure of joule-per-ampere or weber. The measure for the reciprical of magnetic flux.

-- QUDT"""@en ;
    ns1:qudtReference "http://qudt.org/vocab/unit/A-PER-J"^^xsd:string ;
    ns1:ucumCode "A.J-1"^^xsd:string,
        "A/J"^^xsd:string ;
    ns1:unitSymbol "A/J"^^xsd:string .

ns1:AmperePerMetre a owl:Class ;
    rdfs:label "AmperePerMetre"@en ;
    rdfs:comment """ is the SI unit of magnetic field strength. One ampere per meter is equal to π/250 oersteds (12.566  371 millioersteds) in CGS units. The ampere per meter is also the SI unit of "magnetization" in the sense of magnetic dipole moment per unit volume; in this context 1 A/m = 0.001 emu per cubic centimeter.

-- QUDT"""@en ;
    rdfs:isDefinedBy "http://qudt.org/2.1/vocab/unit"^^xsd:string ;
    rdfs:subClassOf [ a owl:Restriction ;
            owl:hasValue 0e+00 ;
            owl:onProperty ns1:hasSIConversionOffset ],
        [ a owl:Restriction ;
            owl:hasValue 1e+00 ;
            owl:onProperty ns1:hasSIConversionMultiplier ],
        ns1:MagneticFieldStrengthUnit,
        ns1:SICoherentDerivedUnit ;
    skos:altLabel "Ampere per Metre"@en ;
    skos:prefLabel "AmperePerMetre"@en ;
    ns1:elucidation """ is the SI unit of magnetic field strength. One ampere per meter is equal to π/250 oersteds (12.566  371 millioersteds) in CGS units. The ampere per meter is also the SI unit of "magnetization" in the sense of magnetic dipole moment per unit volume; in this context 1 A/m = 0.001 emu per cubic centimeter.

-- QUDT"""@en ;
    ns1:qudtReference "http://qudt.org/vocab/unit/A-PER-M"^^xsd:string ;
    ns1:ucumCode "A.m-1"^^xsd:string,
        "A/m"^^xsd:string ;
    ns1:unitSymbol "A/m"^^xsd:string .

ns1:AmperePerRadian a owl:Class ;
    rdfs:label "AmperePerRadian"@en ;
    rdfs:comment """`Ampere per Radian` is a derived unit for measuring the amount of current per unit measure of angle, expressed in ampere per radian.

-- QUDT"""@en ;
    rdfs:isDefinedBy "http://qudt.org/2.1/vocab/unit"^^xsd:string ;
    rdfs:subClassOf [ a owl:Restriction ;
            owl:hasValue 1e+00 ;
            owl:onProperty ns1:hasSIConversionMultiplier ],
        [ a owl:Restriction ;
            owl:hasValue 0e+00 ;
            owl:onProperty ns1:hasSIConversionOffset ],
        ns1:ElectricCurrentUnit,
        ns1:SICoherentDerivedUnit ;
    skos:altLabel "Ampere per Radian"@en ;
    skos:prefLabel "AmperePerRadian"@en ;
    ns1:elucidation """`Ampere per Radian` is a derived unit for measuring the amount of current per unit measure of angle, expressed in ampere per radian.

-- QUDT"""@en ;
    ns1:qudtReference "http://qudt.org/vocab/unit/A-PER-RAD"^^xsd:string ;
    ns1:ucumCode "A.rad-1"^^xsd:string,
        "A/rad"^^xsd:string ;
    ns1:unitSymbol "A/rad"^^xsd:string .

ns1:AmperePerSquareMetre a owl:Class ;
    rdfs:label "AmperePerSquareMetre"@en ;
    rdfs:comment """`Ampere Per Square Meter` is a unit in the category of electric current density. This unit is commonly used in the SI unit system.

-- QUDT"""@en ;
    rdfs:isDefinedBy "http://qudt.org/2.1/vocab/unit"^^xsd:string ;
    rdfs:seeAlso "https://cdd.iec.ch/cdd/iec61360/iec61360.nsf/Units/0112-2---62720%23UAA105"^^xsd:string ;
    rdfs:subClassOf [ a owl:Restriction ;
            owl:hasValue 0e+00 ;
            owl:onProperty ns1:hasSIConversionOffset ],
        [ a owl:Restriction ;
            owl:hasValue 1e+00 ;
            owl:onProperty ns1:hasSIConversionMultiplier ],
        ns1:ElectricCurrentDensityUnit,
        ns1:SICoherentDerivedUnit ;
    skos:altLabel "Ampere per Square Metre"@en ;
    skos:prefLabel "AmperePerSquareMetre"@en ;
    ns1:elucidation """`Ampere Per Square Meter` is a unit in the category of electric current density. This unit is commonly used in the SI unit system.

-- QUDT"""@en ;
    ns1:qudtReference "http://qudt.org/vocab/unit/A-PER-M2"^^xsd:string ;
    ns1:ucumCode "A.m-2"^^xsd:string,
        "A/m2"^^xsd:string ;
    ns1:unitSymbol "A/m²"^^xsd:string .

ns1:AmperePerSquareMetreSquareKelvin a owl:Class ;
    rdfs:label "AmperePerSquareMetreSquareKelvin"@en ;
    rdfs:comment "Ampere per square metre and square Kelvin."@en ;
    rdfs:isDefinedBy "http://qudt.org/2.1/vocab/unit"^^xsd:string ;
    rdfs:seeAlso "http://www.iso.org/iso/catalogue_detail?csnumber=31897"^^xsd:string ;
    rdfs:subClassOf [ a owl:Restriction ;
            owl:hasValue 0e+00 ;
            owl:onProperty ns1:hasSIConversionOffset ],
        [ a owl:Restriction ;
            owl:hasValue 1e+00 ;
            owl:onProperty ns1:hasSIConversionMultiplier ],
        ns1:RichardsonConstantUnit,
        ns1:SICoherentDerivedUnit ;
    skos:prefLabel "AmperePerSquareMetreSquareKelvin"@en ;
    ns1:elucidation "Ampere per square metre and square Kelvin."@en ;
    ns1:qudtReference "http://qudt.org/vocab/unit/A-PER-M2-K2"^^xsd:string ;
    ns1:ucumCode "A.m-2.K-2"^^xsd:string,
        "A/(m2.K2)"^^xsd:string ;
    ns1:unitSymbol "A/m²⋅k²"^^xsd:string .

ns1:AmpereSecond a owl:Class ;
    rdfs:label "AmpereSecond"@en ;
    rdfs:comment """product out of the SI base unit ampere and the SI base unit second

-- QUDT"""@en ;
    rdfs:isDefinedBy "http://qudt.org/2.1/vocab/unit"^^xsd:string ;
    rdfs:subClassOf [ a owl:Restriction ;
            owl:hasValue 0e+00 ;
            owl:onProperty ns1:hasSIConversionOffset ],
        [ a owl:Restriction ;
            owl:hasValue 1e+00 ;
            owl:onProperty ns1:hasSIConversionMultiplier ],
        ns1:ElectricChargeUnit,
        ns1:SICoherentDerivedUnit ;
    skos:altLabel "Ampere Second"@en ;
    skos:prefLabel "AmpereSecond"@en ;
    ns1:elucidation """product out of the SI base unit ampere and the SI base unit second

-- QUDT"""@en ;
    ns1:qudtReference "http://qudt.org/vocab/unit/A-SEC"^^xsd:string ;
    ns1:ucumCode "A.s"^^xsd:string ;
    ns1:unitSymbol "A⋅s"^^xsd:string .

ns1:AmpereSquareMetre a owl:Class ;
    rdfs:label "AmpereSquareMetre"@en ;
    rdfs:comment """The SI unit of electromagnetic moment.

-- QUDT"""@en ;
    rdfs:isDefinedBy "http://qudt.org/2.1/vocab/unit"^^xsd:string ;
    rdfs:seeAlso "http://encyclopedia2.thefreedictionary.com/ampere+meter+squared"^^xsd:string ;
    rdfs:subClassOf [ a owl:Restriction ;
            owl:hasValue 1e+00 ;
            owl:onProperty ns1:hasSIConversionMultiplier ],
        [ a owl:Restriction ;
            owl:hasValue 0e+00 ;
            owl:onProperty ns1:hasSIConversionOffset ],
        ns1:MagneticDipoleMomentUnit,
        ns1:SICoherentDerivedUnit ;
    skos:altLabel "Ampere Square Metre"@en ;
    skos:prefLabel "AmpereSquareMetre"@en ;
    ns1:elucidation """The SI unit of electromagnetic moment.

-- QUDT"""@en ;
    ns1:qudtReference "http://qudt.org/vocab/unit/A-M2"^^xsd:string ;
    ns1:ucumCode "A.m2"^^xsd:string ;
    ns1:unitSymbol "A⋅m²"^^xsd:string .

ns1:AmpereSquareMetrePerJouleSecond a owl:Class ;
    rdfs:label "AmpereSquareMetrePerJouleSecond"@en ;
    rdfs:comment """The SI unit of gyromagnetic ratio.

-- QUDT"""@en ;
    rdfs:isDefinedBy "http://qudt.org/2.1/vocab/unit"^^xsd:string ;
    rdfs:seeAlso "http://encyclopedia2.thefreedictionary.com/ampere+square+meter+per+joule+second"^^xsd:string ;
    rdfs:subClassOf [ a owl:Restriction ;
            owl:hasValue 1e+00 ;
            owl:onProperty ns1:hasSIConversionMultiplier ],
        [ a owl:Restriction ;
            owl:hasValue 0e+00 ;
            owl:onProperty ns1:hasSIConversionOffset ],
        ns1:ElectricChargePerMassUnit,
        ns1:SICoherentDerivedUnit ;
    skos:altLabel "Ampere Square Metre Per Joule Second"@en ;
    skos:prefLabel "AmpereSquareMetrePerJouleSecond"@en ;
    ns1:elucidation """The SI unit of gyromagnetic ratio.

-- QUDT"""@en ;
    ns1:qudtReference "http://qudt.org/vocab/unit/A-M2-PER-J-SEC"^^xsd:string ;
    ns1:ucumCode "A.m2.J-1.s-1"^^xsd:string,
        "A.m2/(J.s)"^^xsd:string ;
    ns1:unitSymbol "A⋅m²/(J⋅s)"^^xsd:string .

ns1:BecquerelPerCubicMetre a owl:Class ;
    rdfs:label "BecquerelPerCubicMetre"@en ;
    rdfs:comment """The SI derived unit of unit in the category of Radioactivity concentration.

-- QUDT"""@en ;
    rdfs:isDefinedBy "http://qudt.org/2.1/vocab/unit"^^xsd:string ;
    rdfs:seeAlso "http://www.efunda.com/glossary/units/units--radioactivity_concentration--becquerel_per_cubic_meter.cfm"^^xsd:string ;
    rdfs:subClassOf [ a owl:Restriction ;
            owl:hasValue 0e+00 ;
            owl:onProperty ns1:hasSIConversionOffset ],
        [ a owl:Restriction ;
            owl:hasValue 1e+00 ;
            owl:onProperty ns1:hasSIConversionMultiplier ],
        ns1:FrequencyPerVolumeUnit,
        ns1:SICoherentDerivedUnit ;
    skos:altLabel "Becquerel per Cubic Metre"@en ;
    skos:prefLabel "BecquerelPerCubicMetre"@en ;
    ns1:elucidation """The SI derived unit of unit in the category of Radioactivity concentration.

-- QUDT"""@en ;
    ns1:qudtReference "http://qudt.org/vocab/unit/BQ-PER-M3"^^xsd:string ;
    ns1:ucumCode "Bq.m-3"^^xsd:string,
        "Bq/m3"^^xsd:string ;
    ns1:unitSymbol "Bq/m³"^^xsd:string .

ns1:BecquerelPerKilogram a owl:Class ;
    rdfs:label "BecquerelPerKilogram"^^xsd:string ;
    rdfs:comment """"Becquerel per Kilogram" is used to describe radioactivity, which is often expressed in becquerels per unit of volume or weight, to express how much radioactive material is contained in a sample.

-- QUDT"""@en ;
    rdfs:isDefinedBy "http://qudt.org/2.1/vocab/unit"^^xsd:string ;
    rdfs:seeAlso "http://www.efunda.com/glossary/units/units--specific_radioactivity--becquerel_per_kilogram.cfm"^^xsd:string ;
    rdfs:subClassOf [ a owl:Restriction ;
            owl:hasValue 1e+00 ;
            owl:onProperty ns1:hasSIConversionMultiplier ],
        [ a owl:Restriction ;
            owl:hasValue 0e+00 ;
            owl:onProperty ns1:hasSIConversionOffset ],
        ns1:PerTimeMassUnit,
        ns1:SICoherentDerivedUnit ;
    skos:altLabel "Becquerel per Kilogram"@en ;
    skos:prefLabel "BecquerelPerKilogram"^^xsd:string ;
    ns1:elucidation """"Becquerel per Kilogram" is used to describe radioactivity, which is often expressed in becquerels per unit of volume or weight, to express how much radioactive material is contained in a sample.

-- QUDT"""@en ;
    ns1:qudtReference "http://qudt.org/vocab/unit/BQ-PER-KiloGM"^^xsd:string ;
    ns1:ucumCode "Bq.kg-1"^^xsd:string,
        "Bq/kg"^^xsd:string ;
    ns1:unitSymbol "Bq/kg"^^xsd:string .

ns1:BecquerelPerSquareMetre a owl:Class ;
    rdfs:label "BecquerelPerSquareMetre"@en ;
    rdfs:comment "Becquerel per square metre."@en ;
    rdfs:isDefinedBy "http://qudt.org/2.1/vocab/unit"^^xsd:string ;
    rdfs:subClassOf [ a owl:Restriction ;
            owl:hasValue 0e+00 ;
            owl:onProperty ns1:hasSIConversionOffset ],
        [ a owl:Restriction ;
            owl:hasValue 1e+00 ;
            owl:onProperty ns1:hasSIConversionMultiplier ],
        ns1:PerAreaTimeUnit,
        ns1:SICoherentDerivedUnit ;
    skos:prefLabel "BecquerelPerSquareMetre"@en ;
    ns1:elucidation "Becquerel per square metre."@en ;
    ns1:qudtReference "http://qudt.org/vocab/unit/BQ-PER-M2"^^xsd:string ;
    ns1:ucumCode "Bq.m-2"^^xsd:string,
        "Bq/m2"^^xsd:string ;
    ns1:unitSymbol "Bq/m²"^^xsd:string .

ns1:BecquerelSecondPerCubicMetre a owl:Class ;
    rdfs:label "BecquerelSecondPerCubicMetre"^^xsd:string ;
    rdfs:comment "Becquerels second per cubic metre."@en ;
    rdfs:isDefinedBy "http://qudt.org/2.1/vocab/unit"^^xsd:string ;
    rdfs:subClassOf [ a owl:Restriction ;
            owl:hasValue 0e+00 ;
            owl:onProperty ns1:hasSIConversionOffset ],
        [ a owl:Restriction ;
            owl:hasValue 1e+00 ;
            owl:onProperty ns1:hasSIConversionMultiplier ],
        ns1:PerVolumeUnit,
        ns1:SICoherentDerivedUnit ;
    skos:prefLabel "BecquerelSecondPerCubicMetre"^^xsd:string ;
    ns1:elucidation "Becquerels second per cubic metre."@en ;
    ns1:qudtReference "http://qudt.org/vocab/unit/BQ-SEC-PER-M3"^^xsd:string ;
    ns1:ucumCode "Bq.s.m-3"^^xsd:string ;
    ns1:unitSymbol "Bq⋅s/m³"^^xsd:string .

ns1:CandelaPerLumen a owl:Class ;
    rdfs:label "CandelaPerLumen"@en ;
    rdfs:comment "Candela per Lumen."@en ;
    rdfs:isDefinedBy "http://qudt.org/2.1/vocab/unit"^^xsd:string ;
    rdfs:subClassOf [ a owl:Restriction ;
            owl:hasValue 0e+00 ;
            owl:onProperty ns1:hasSIConversionOffset ],
        [ a owl:Restriction ;
            owl:hasValue 1e+00 ;
            owl:onProperty ns1:hasSIConversionMultiplier ],
        ns1:FractionUnit,
        ns1:SICoherentDerivedUnit ;
    skos:prefLabel "CandelaPerLumen"@en ;
    ns1:elucidation "Candela per Lumen."@en ;
    ns1:qudtReference "http://qudt.org/vocab/unit/CD-PER-LM"^^xsd:string ;
    ns1:unitSymbol "cd/lm"^^xsd:string .

ns1:CandelaPerSquareMetre a owl:Class ;
    rdfs:label "CandelaPerSquareMetre"@en ;
    rdfs:comment """The candela per square metre (cd/m²) is the derived SI unit of luminance. The unit is based on the candela, the SI unit of luminous intensity, and the square metre, the SI unit of area. Nit (nt) is a deprecated non-SI name also used for this unit (1 nit = 1 cd/m²). As a measure of light emitted per unit area, this unit is frequently used to specify the brightness of a display device. Most consumer desktop liquid crystal displays have luminances of 200 to 300 cd/m²; the sRGB spec for monitors targets 80 cd/m2. HDTVs range from 450 to about 1000 cd/m2. Typically, calibrated monitors should have a brightness of 120 cd/m². Nit is believed to come from the Latin word nitere, to shine.

-- QUDT"""@en ;
    rdfs:isDefinedBy "http://qudt.org/2.1/vocab/unit"^^xsd:string ;
    rdfs:subClassOf [ a owl:Restriction ;
            owl:hasValue 0e+00 ;
            owl:onProperty ns1:hasSIConversionOffset ],
        [ a owl:Restriction ;
            owl:hasValue 1e+00 ;
            owl:onProperty ns1:hasSIConversionMultiplier ],
        ns1:LuminanceUnit,
        ns1:SICoherentDerivedUnit ;
    skos:altLabel "candela per square metre"@en ;
    skos:prefLabel "CandelaPerSquareMetre"@en ;
    ns1:elucidation """The candela per square metre (cd/m²) is the derived SI unit of luminance. The unit is based on the candela, the SI unit of luminous intensity, and the square metre, the SI unit of area. Nit (nt) is a deprecated non-SI name also used for this unit (1 nit = 1 cd/m²). As a measure of light emitted per unit area, this unit is frequently used to specify the brightness of a display device. Most consumer desktop liquid crystal displays have luminances of 200 to 300 cd/m²; the sRGB spec for monitors targets 80 cd/m2. HDTVs range from 450 to about 1000 cd/m2. Typically, calibrated monitors should have a brightness of 120 cd/m². Nit is believed to come from the Latin word nitere, to shine.

-- QUDT"""@en ;
    ns1:qudtReference "http://qudt.org/vocab/unit/CD-PER-M2"^^xsd:string ;
    ns1:ucumCode "cd.m-2"^^xsd:string,
        "cd/m2"^^xsd:string ;
    ns1:unitSymbol "cd/m²"^^xsd:string .

ns1:CoulombMetre a owl:Class ;
    rdfs:label "CoulombMetre"@en ;
    rdfs:comment """Coulomb Meter (C-m) is a unit in the category of Electric dipole moment. It is also known as atomic unit, u.a., au, ua. This unit is commonly used in the SI unit system. Coulomb Meter (C-m) has a dimension of LTI where L is length, T is time, and I is electric current. This unit is the standard SI unit in this category.

-- QUDT"""@en ;
    rdfs:subClassOf [ a owl:Restriction ;
            owl:hasValue 1e+00 ;
            owl:onProperty ns1:hasSIConversionMultiplier ],
        [ a owl:Restriction ;
            owl:hasValue 0e+00 ;
            owl:onProperty ns1:hasSIConversionOffset ],
        ns1:LengthTimeCurrentUnit,
        ns1:SICoherentDerivedUnit ;
    skos:prefLabel "CoulombMetre"@en ;
    schema:unitCode "A26"^^xsd:string ;
    ns1:elucidation """Coulomb Meter (C-m) is a unit in the category of Electric dipole moment. It is also known as atomic unit, u.a., au, ua. This unit is commonly used in the SI unit system. Coulomb Meter (C-m) has a dimension of LTI where L is length, T is time, and I is electric current. This unit is the standard SI unit in this category.

-- QUDT"""@en ;
    ns1:note "It is also known as atomic unit, u.a., au, ua. This unit is commonly used in the SI unit system. Coulomb Meter (C-m) has a dimension of LTI where L is length, T is time, and I is electric current. This unit is the standard SI unit in this category."^^xsd:string ;
    ns1:qudtReference "http://qudt.org/vocab/unit/C-M"^^xsd:anyURI ;
    ns1:ucumCode "C.m"^^xsd:string ;
    ns1:unitSymbol "C⋅m"^^xsd:string .

ns1:CoulombPerCubicMetre a owl:Class ;
    rdfs:label "CoulombPerCubicMetre"@en ;
    rdfs:comment """Coulomb Per Cubic Meter (C/m³) is a unit in the category of Electric charge density. It is also known as coulomb per cubic metre, coulombs per cubic meter, coulombs per cubic metre, coulomb/cubic meter, coulomb/cubic metre. This unit is commonly used in the SI unit system. Coulomb Per Cubic Meter has a dimension of L⁻³TI where L is length, T is time, and I is electric current. This unit is the standard SI unit in this category.

-- QUDT"""@en ;
    rdfs:isDefinedBy "http://qudt.org/2.1/vocab/unit"^^xsd:string ;
    rdfs:subClassOf [ a owl:Restriction ;
            owl:hasValue 0e+00 ;
            owl:onProperty ns1:hasSIConversionOffset ],
        [ a owl:Restriction ;
            owl:hasValue 1e+00 ;
            owl:onProperty ns1:hasSIConversionMultiplier ],
        ns1:ElectricChargeDensityUnit,
        ns1:SICoherentDerivedUnit ;
    skos:altLabel "Coulomb per Cubic Metre"@en ;
    skos:prefLabel "CoulombPerCubicMetre"@en ;
    ns1:elucidation """Coulomb Per Cubic Meter (C/m³) is a unit in the category of Electric charge density. It is also known as coulomb per cubic metre, coulombs per cubic meter, coulombs per cubic metre, coulomb/cubic meter, coulomb/cubic metre. This unit is commonly used in the SI unit system. Coulomb Per Cubic Meter has a dimension of L⁻³TI where L is length, T is time, and I is electric current. This unit is the standard SI unit in this category.

-- QUDT"""@en ;
    ns1:qudtReference "http://qudt.org/vocab/unit/C-PER-M3"^^xsd:string ;
    ns1:ucumCode "C.m-3"^^xsd:string,
        "C/m3"^^xsd:string ;
    ns1:unitSymbol "C/m³"^^xsd:string .

ns1:CoulombPerKilogram a owl:Class ;
    rdfs:label "CoulombPerKilogram"^^xsd:string ;
    rdfs:comment """`Coulomb Per Kilogram (C/kg)` is the unit in the category of Exposure. It is also known as coulombs per kilogram, coulomb/kilogram. This unit is commonly used in the SI unit system. Coulomb Per Kilogram (C/kg) has a dimension of M⁻¹TI where M is mass, T is time, and I is electric current. This unit is the standard SI unit in this category.

-- QUDT"""@en ;
    rdfs:isDefinedBy "http://qudt.org/2.1/vocab/unit"^^xsd:string ;
    rdfs:subClassOf [ a owl:Restriction ;
            owl:hasValue 0e+00 ;
            owl:onProperty ns1:hasSIConversionOffset ],
        [ a owl:Restriction ;
            owl:hasValue 1e+00 ;
            owl:onProperty ns1:hasSIConversionMultiplier ],
        ns1:ElectricChargePerMassUnit,
        ns1:SICoherentDerivedUnit ;
    skos:altLabel "Coulomb per Kilogram"@en ;
    skos:prefLabel "CoulombPerKilogram"^^xsd:string ;
    ns1:elucidation """`Coulomb Per Kilogram (C/kg)` is the unit in the category of Exposure. It is also known as coulombs per kilogram, coulomb/kilogram. This unit is commonly used in the SI unit system. Coulomb Per Kilogram (C/kg) has a dimension of M⁻¹TI where M is mass, T is time, and I is electric current. This unit is the standard SI unit in this category.

-- QUDT"""@en ;
    ns1:qudtReference "http://qudt.org/vocab/unit/C-PER-KiloGM"^^xsd:string ;
    ns1:ucumCode "C.kg-1"^^xsd:string,
        "C/kg"^^xsd:string ;
    ns1:unitSymbol "C/kg"^^xsd:string .

ns1:CoulombPerKilogramSecond a owl:Class ;
    rdfs:label "CoulombPerKilogramSecond"^^xsd:string ;
    rdfs:comment """The SI unit of exposure rate

-- QUDT"""@en ;
    rdfs:isDefinedBy "http://qudt.org/2.1/vocab/unit"^^xsd:string ;
    rdfs:seeAlso "http://en.wikibooks.org/wiki/Basic_Physics_of_Nuclear_Medicine/Units_of_Radiation_Measurement"^^xsd:string ;
    rdfs:subClassOf [ a owl:Restriction ;
            owl:hasValue 1e+00 ;
            owl:onProperty ns1:hasSIConversionMultiplier ],
        [ a owl:Restriction ;
            owl:hasValue 0e+00 ;
            owl:onProperty ns1:hasSIConversionOffset ],
        ns1:ElectricCurrentPerMassUnit,
        ns1:SICoherentDerivedUnit ;
    skos:altLabel "Coulomb Per Kilogram Second"@en ;
    skos:prefLabel "CoulombPerKilogramSecond"^^xsd:string ;
    ns1:elucidation """The SI unit of exposure rate

-- QUDT"""@en ;
    ns1:qudtReference "http://qudt.org/vocab/unit/C-PER-KiloGM-SEC"^^xsd:string ;
    ns1:ucumCode "C.kg-1.s-1"^^xsd:string,
        "C/(kg.s)"^^xsd:string ;
    ns1:unitSymbol "C/kg⋅s"^^xsd:string .

ns1:CoulombPerMetre a owl:Class ;
    rdfs:label "CoulombPerMetre"@en ;
    rdfs:comment """"Coulomb per Meter" is a unit for  'Electric Charge Line Density' expressed as C/m.

-- QUDT"""@en ;
    rdfs:isDefinedBy "http://qudt.org/2.1/vocab/unit"^^xsd:string ;
    rdfs:subClassOf [ a owl:Restriction ;
            owl:hasValue 1e+00 ;
            owl:onProperty ns1:hasSIConversionMultiplier ],
        [ a owl:Restriction ;
            owl:hasValue 0e+00 ;
            owl:onProperty ns1:hasSIConversionOffset ],
        ns1:ElectricChargePerLengthUnit,
        ns1:SICoherentDerivedUnit ;
    skos:altLabel "Coulomb per Metre"@en ;
    skos:prefLabel "CoulombPerMetre"@en ;
    ns1:elucidation """"Coulomb per Meter" is a unit for  'Electric Charge Line Density' expressed as C/m.

-- QUDT"""@en ;
    ns1:qudtReference "http://qudt.org/vocab/unit/C-PER-M"^^xsd:string ;
    ns1:ucumCode "C.m-1"^^xsd:string,
        "C/m"^^xsd:string ;
    ns1:unitSymbol "C/m"^^xsd:string .

ns1:CoulombPerMole a owl:Class ;
    rdfs:label "CoulombPerMole"@en ;
    rdfs:comment """ (C/mol) is a unit in the category of Molar electric charge. It is also known as coulombs/mol. Coulomb Per Mol has a dimension of TN{-1}I where T is time, N is amount of substance, and I is electric current. This unit is the standard SI unit in this category.

-- QUDT"""@en ;
    rdfs:isDefinedBy "http://qudt.org/2.1/vocab/unit"^^xsd:string ;
    rdfs:subClassOf [ a owl:Restriction ;
            owl:hasValue 0e+00 ;
            owl:onProperty ns1:hasSIConversionOffset ],
        [ a owl:Restriction ;
            owl:hasValue 1e+00 ;
            owl:onProperty ns1:hasSIConversionMultiplier ],
        ns1:ElectricChargePerAmountUnit,
        ns1:SICoherentDerivedUnit ;
    skos:altLabel "Coulomb per Mole"@en ;
    skos:prefLabel "CoulombPerMole"@en ;
    ns1:elucidation """ (C/mol) is a unit in the category of Molar electric charge. It is also known as coulombs/mol. Coulomb Per Mol has a dimension of TN{-1}I where T is time, N is amount of substance, and I is electric current. This unit is the standard SI unit in this category.

-- QUDT"""@en ;
    ns1:qudtReference "http://qudt.org/vocab/unit/C-PER-MOL"^^xsd:string ;
    ns1:ucumCode "C.mol-1"^^xsd:string,
        "C/mol"^^xsd:string ;
    ns1:unitSymbol "c/mol"^^xsd:string .

ns1:CoulombPerSquareMetre a owl:Class ;
    rdfs:label "CoulombPerSquareMetre"@en ;
    rdfs:comment """Coulomb Per Square Meter (C/m²) is a unit in the category of Electric charge surface density. It is also known as coulombs per square meter, coulomb per square metre, coulombs per square metre, coulomb/square meter, coulomb/square metre. This unit is commonly used in the SI unit system. Coulomb Per Square Meter (C/m2) has a dimension of L⁻²TI where L is length, T is time, and I is electric current. This unit is the standard SI unit in this category.

-- QUDT"""@en ;
    rdfs:isDefinedBy "http://qudt.org/2.1/vocab/unit"^^xsd:string ;
    rdfs:subClassOf [ a owl:Restriction ;
            owl:hasValue 0e+00 ;
            owl:onProperty ns1:hasSIConversionOffset ],
        [ a owl:Restriction ;
            owl:hasValue 1e+00 ;
            owl:onProperty ns1:hasSIConversionMultiplier ],
        ns1:ElectricDisplacementFieldUnit,
        ns1:SICoherentDerivedUnit ;
    skos:altLabel "Coulomb per Square Metre"@en ;
    skos:prefLabel "CoulombPerSquareMetre"@en ;
    ns1:elucidation """Coulomb Per Square Meter (C/m²) is a unit in the category of Electric charge surface density. It is also known as coulombs per square meter, coulomb per square metre, coulombs per square metre, coulomb/square meter, coulomb/square metre. This unit is commonly used in the SI unit system. Coulomb Per Square Meter (C/m2) has a dimension of L⁻²TI where L is length, T is time, and I is electric current. This unit is the standard SI unit in this category.

-- QUDT"""@en ;
    ns1:qudtReference "http://qudt.org/vocab/unit/C-PER-M2"^^xsd:string ;
    ns1:ucumCode "C.m-2"^^xsd:string,
        "C/m2"^^xsd:string ;
    ns1:unitSymbol "C/m²"^^xsd:string .

ns1:CoulombSquareMetre a owl:Class ;
    rdfs:label "CoulombSquareMetre"@en ;
    rdfs:comment """Coulomb Square Meter (C-m2) is a unit in the category of Electric quadrupole moment. This unit is commonly used in the SI unit system. Coulomb Square Meter (C-m2) has a dimension of L2TI where L is length, T is time, and I is electric current. This unit is the standard SI unit in this category.

-- QUDT"""@en ;
    rdfs:isDefinedBy "http://qudt.org/2.1/vocab/unit"^^xsd:string ;
    rdfs:subClassOf [ a owl:Restriction ;
            owl:hasValue 0e+00 ;
            owl:onProperty ns1:hasSIConversionOffset ],
        [ a owl:Restriction ;
            owl:hasValue 1e+00 ;
            owl:onProperty ns1:hasSIConversionMultiplier ],
        ns1:ElectricChargeAreaUnit,
        ns1:SICoherentDerivedUnit ;
    skos:altLabel "Coulomb Square Metre"@en ;
    skos:prefLabel "CoulombSquareMetre"@en ;
    ns1:elucidation """Coulomb Square Meter (C-m2) is a unit in the category of Electric quadrupole moment. This unit is commonly used in the SI unit system. Coulomb Square Meter (C-m2) has a dimension of L2TI where L is length, T is time, and I is electric current. This unit is the standard SI unit in this category.

-- QUDT"""@en ;
    ns1:qudtReference "http://qudt.org/vocab/unit/C-M2"^^xsd:string ;
    ns1:ucumCode "C.m2"^^xsd:string ;
    ns1:unitSymbol "C⋅m²"^^xsd:string .

ns1:CoulombSquareMetrePerVolt a owl:Class ;
    rdfs:label "CoulombSquareMetrePerVolt"@en ;
    rdfs:comment """Coulomb Square Meter (C-m2-per-volt) is a unit in the category of Electric polarizability.

-- QUDT"""@en ;
    rdfs:isDefinedBy "http://qudt.org/2.1/vocab/unit"^^xsd:string ;
    rdfs:subClassOf [ a owl:Restriction ;
            owl:hasValue 0e+00 ;
            owl:onProperty ns1:hasSIConversionOffset ],
        [ a owl:Restriction ;
            owl:hasValue 1e+00 ;
            owl:onProperty ns1:hasSIConversionMultiplier ],
        ns1:SICoherentDerivedUnit,
        ns1:SquareCurrentQuarticTimePerMassUnit ;
    skos:altLabel "Coulomb Square Metre Per Volt"@en ;
    skos:prefLabel "CoulombSquareMetrePerVolt"@en ;
    ns1:elucidation """Coulomb Square Meter (C-m2-per-volt) is a unit in the category of Electric polarizability.

-- QUDT"""@en ;
    ns1:qudtReference "http://qudt.org/vocab/unit/C-M2-PER-V"^^xsd:string ;
    ns1:ucumCode "C.m2.V-1"^^xsd:string,
        "C.m2/V"^^xsd:string ;
    ns1:unitSymbol "C⋅m²/V"^^xsd:string .

ns1:CubicCoulombMetrePerSquareJoule a owl:Class ;
    rdfs:label "CubicCoulombMetrePerSquareJoule"@en ;
    rdfs:comment """"Cubic Coulomb Meter per Square Joule" is a unit for  'Cubic Electric Dipole Moment Per Square Energy' expressed as C³ m³ J⁻².

-- QUDT"""@en ;
    rdfs:isDefinedBy "http://qudt.org/2.1/vocab/unit"^^xsd:string ;
    rdfs:subClassOf [ a owl:Restriction ;
            owl:hasValue 0e+00 ;
            owl:onProperty ns1:hasSIConversionOffset ],
        [ a owl:Restriction ;
            owl:hasValue 1e+00 ;
            owl:onProperty ns1:hasSIConversionMultiplier ],
        ns1:CubicElectricChargeLengthPerSquareEnergyUnit,
        ns1:SICoherentDerivedUnit ;
    skos:altLabel "Cubic Coulomb Metre per Square Joule"@en ;
    skos:prefLabel "CubicCoulombMetrePerSquareJoule"@en ;
    ns1:elucidation """"Cubic Coulomb Meter per Square Joule" is a unit for  'Cubic Electric Dipole Moment Per Square Energy' expressed as C³ m³ J⁻².

-- QUDT"""@en ;
    ns1:qudtReference "http://qudt.org/vocab/unit/C3-M-PER-J2"^^xsd:string ;
    ns1:ucumCode "C3.m.J-2"^^xsd:string,
        "C3.m/J2"^^xsd:string ;
    ns1:unitSymbol "C³⋅m/J²"^^xsd:string .

ns1:CubicMetre a owl:Class ;
    rdfs:label "CubicMetre"@en ;
    rdfs:comment """The SI unit of volume, equal to 1.0e6 cm3, 1000 liters, 35.3147 ft3, or 1.30795 yd3. A cubic meter holds about 264.17 U.S. liquid gallons or 219.99 British Imperial gallons.

-- QUDT"""@en ;
    rdfs:subClassOf [ a owl:Restriction ;
            owl:hasValue 1e+00 ;
            owl:onProperty ns1:hasSIConversionMultiplier ],
        [ a owl:Restriction ;
            owl:hasValue 0e+00 ;
            owl:onProperty ns1:hasSIConversionOffset ],
        ns1:SICoherentDerivedUnit,
        ns1:VolumeUnit ;
    skos:prefLabel "CubicMetre"@en ;
    schema:unitCode "MTQ"^^xsd:string ;
    ns1:dbpediaReference "http://dbpedia.org/resource/Cubic_metre"^^xsd:string ;
    ns1:elucidation """The SI unit of volume, equal to 1.0e6 cm3, 1000 liters, 35.3147 ft3, or 1.30795 yd3. A cubic meter holds about 264.17 U.S. liquid gallons or 219.99 British Imperial gallons.

-- QUDT"""@en ;
    ns1:omReference "http://www.ontology-of-units-of-measure.org/resource/om-2/cubicMetre"^^xsd:string ;
    ns1:qudtReference "http://qudt.org/vocab/unit/M3"^^xsd:string ;
    ns1:ucumCode "m3"^^xsd:string ;
    ns1:unitSymbol "m³"^^xsd:string ;
    ns1:wikipediaReference "http://en.wikipedia.org/wiki/Cubic_metre?oldid=490956678"^^xsd:anyURI .

ns1:CubicMetrePerCoulomb a owl:Class ;
    rdfs:label "CubicMetrePerCoulomb"@en ;
    rdfs:comment "Cubic metre per Coulomb."@en ;
    rdfs:isDefinedBy "http://qudt.org/2.1/vocab/unit"^^xsd:string ;
    rdfs:seeAlso "http://www.iso.org/iso/catalogue_detail?csnumber=31897"^^xsd:string ;
    rdfs:subClassOf [ a owl:Restriction ;
            owl:hasValue 1e+00 ;
            owl:onProperty ns1:hasSIConversionMultiplier ],
        [ a owl:Restriction ;
            owl:hasValue 0e+00 ;
            owl:onProperty ns1:hasSIConversionOffset ],
        ns1:ReciprocalElectricChargeDensityUnit,
        ns1:SICoherentDerivedUnit ;
    skos:prefLabel "CubicMetrePerCoulomb"@en ;
    ns1:elucidation "Cubic metre per Coulomb."@en ;
    ns1:qudtReference "http://qudt.org/vocab/unit/M3-PER-C"^^xsd:string ;
    ns1:ucumCode "m3.C-1"^^xsd:string ;
    ns1:unitSymbol "m³/C"^^xsd:string .

ns1:CubicMetrePerCubicMetre a owl:Class ;
    rdfs:label "CubicMetrePerCubicMetre"@en ;
    rdfs:comment """Power of the SI base unit metre with the exponent 3 divided by the power of the SI base unit metre with the exponent 3.

-- QUDT"""@en ;
    rdfs:isDefinedBy "http://qudt.org/2.1/vocab/unit"^^xsd:string ;
    rdfs:subClassOf [ a owl:Restriction ;
            owl:hasValue 1e+00 ;
            owl:onProperty ns1:hasSIConversionMultiplier ],
        [ a owl:Restriction ;
            owl:hasValue 0e+00 ;
            owl:onProperty ns1:hasSIConversionOffset ],
        ns1:SICoherentDerivedUnit,
        ns1:VolumeFractionUnit ;
    skos:altLabel "Cubic Metre Per Cubic Metre"@en ;
    skos:prefLabel "CubicMetrePerCubicMetre"@en ;
    ns1:elucidation """Power of the SI base unit metre with the exponent 3 divided by the power of the SI base unit metre with the exponent 3.

-- QUDT"""@en ;
    ns1:qudtReference "http://qudt.org/vocab/unit/M3-PER-M3"^^xsd:string ;
    ns1:ucumCode "m3.m-3"^^xsd:string ;
    ns1:unitSymbol "m³/m³"^^xsd:string .

ns1:CubicMetrePerKelvin a owl:Class ;
    rdfs:label "CubicMetrePerKelvin"@en ;
    rdfs:comment "Cubic metre per Kelvin."@en ;
    rdfs:isDefinedBy "http://qudt.org/2.1/vocab/unit"^^xsd:string ;
    rdfs:subClassOf [ a owl:Restriction ;
            owl:hasValue 0e+00 ;
            owl:onProperty ns1:hasSIConversionOffset ],
        [ a owl:Restriction ;
            owl:hasValue 1e+00 ;
            owl:onProperty ns1:hasSIConversionMultiplier ],
        ns1:SICoherentDerivedUnit,
        ns1:VolumePerTemperatureUnit ;
    skos:prefLabel "CubicMetrePerKelvin"@en ;
    ns1:elucidation "Cubic metre per Kelvin."@en ;
    ns1:qudtReference "http://qudt.org/vocab/unit/M3-PER-K"^^xsd:string ;
    ns1:ucumCode "m3.K-1"^^xsd:string ;
    ns1:unitSymbol "m³/K"^^xsd:string .

ns1:CubicMetrePerKilogram a owl:Class ;
    rdfs:label "CubicMetrePerKilogram"^^xsd:string ;
    rdfs:comment """Cubic Meter Per Kilogram (m3/kg) is a unit in the category of Specific volume. It is also known as cubic meters per kilogram, cubic metre per kilogram, cubic metres per kilogram, cubic meter/kilogram, cubic metre/kilogram. This unit is commonly used in the SI unit system. Cubic Meter Per Kilogram (m3/kg) has a dimension of M-1L3 where M is mass, and L is length. This unit is the standard SI unit in this category.

-- QUDT"""@en ;
    rdfs:isDefinedBy "http://qudt.org/2.1/vocab/unit"^^xsd:string ;
    rdfs:subClassOf [ a owl:Restriction ;
            owl:hasValue 0e+00 ;
            owl:onProperty ns1:hasSIConversionOffset ],
        [ a owl:Restriction ;
            owl:hasValue 1e+00 ;
            owl:onProperty ns1:hasSIConversionMultiplier ],
        ns1:SICoherentDerivedUnit,
        ns1:VolumePerMassUnit ;
    skos:altLabel "Cubic Metre per Kilogram"@en ;
    skos:prefLabel "CubicMetrePerKilogram"^^xsd:string ;
    ns1:elucidation """Cubic Meter Per Kilogram (m3/kg) is a unit in the category of Specific volume. It is also known as cubic meters per kilogram, cubic metre per kilogram, cubic metres per kilogram, cubic meter/kilogram, cubic metre/kilogram. This unit is commonly used in the SI unit system. Cubic Meter Per Kilogram (m3/kg) has a dimension of M-1L3 where M is mass, and L is length. This unit is the standard SI unit in this category.

-- QUDT"""@en ;
    ns1:qudtReference "http://qudt.org/vocab/unit/M3-PER-KiloGM"^^xsd:string ;
    ns1:ucumCode "m3.kg-1"^^xsd:string,
        "m3/kg"^^xsd:string ;
    ns1:unitSymbol "m³/kg"^^xsd:string .

ns1:CubicMetrePerKilogramSquareSecond a owl:Class ;
    rdfs:label "CubicMetrePerKilogramSquareSecond"^^xsd:string ;
    rdfs:comment "Cubic metre per kilogram and square second."@en ;
    rdfs:isDefinedBy "http://qudt.org/2.1/vocab/unit"^^xsd:string ;
    rdfs:subClassOf [ a owl:Restriction ;
            owl:hasValue 0e+00 ;
            owl:onProperty ns1:hasSIConversionOffset ],
        [ a owl:Restriction ;
            owl:hasValue 1e+00 ;
            owl:onProperty ns1:hasSIConversionMultiplier ],
        ns1:NewtonianConstantOfGravityUnit,
        ns1:SICoherentDerivedUnit ;
    skos:prefLabel "CubicMetrePerKilogramSquareSecond"^^xsd:string ;
    ns1:elucidation "Cubic metre per kilogram and square second."@en ;
    ns1:qudtReference "http://qudt.org/vocab/unit/M3-PER-KiloGM-SEC2"^^xsd:string ;
    ns1:ucumCode "m3.(kg.s2)-1"^^xsd:string,
        "m3.kg-1.s-2"^^xsd:string,
        "m3/(kg.s2)"^^xsd:string ;
    ns1:unitSymbol "m³/(kg⋅s²)"^^xsd:string .

ns1:CubicMetrePerMole a owl:Class ;
    rdfs:label "CubicMetrePerMole"@en ;
    rdfs:comment """The molar volume, symbol Vm, is the volume occupied by one mole of a substance (chemical element or chemical compound) at a given temperature and pressure. It is equal to the molar mass (M) divided by the mass density. It has the SI unit cubic metres per mole m3/mol, although it is more practical to use the units cubic decimetres per mole dm3/mol for gases and cubic centimetres per mole cm3/mol for liquids and solids.

-- QUDT"""@en ;
    rdfs:isDefinedBy "http://qudt.org/2.1/vocab/unit"^^xsd:string ;
    rdfs:subClassOf [ a owl:Restriction ;
            owl:hasValue 0e+00 ;
            owl:onProperty ns1:hasSIConversionOffset ],
        [ a owl:Restriction ;
            owl:hasValue 1e+00 ;
            owl:onProperty ns1:hasSIConversionMultiplier ],
        ns1:SICoherentDerivedUnit,
        ns1:VolumePerAmountUnit ;
    skos:altLabel "Cubic Metre per Mole"@en ;
    skos:prefLabel "CubicMetrePerMole"@en ;
    ns1:elucidation """The molar volume, symbol Vm, is the volume occupied by one mole of a substance (chemical element or chemical compound) at a given temperature and pressure. It is equal to the molar mass (M) divided by the mass density. It has the SI unit cubic metres per mole m3/mol, although it is more practical to use the units cubic decimetres per mole dm3/mol for gases and cubic centimetres per mole cm3/mol for liquids and solids.

-- QUDT"""@en ;
    ns1:qudtReference "http://qudt.org/vocab/unit/M3-PER-MOL"^^xsd:string ;
    ns1:ucumCode "m3.mol-1"^^xsd:string,
        "m3/mol"^^xsd:string ;
    ns1:unitSymbol "m³/mol"^^xsd:string .

ns1:CubicMetrePerSecond a owl:Class ;
    rdfs:label "CubicMetrePerSecond"@en ;
    rdfs:comment """A cubic metre per second (m³s⁻¹, m³/s), cumecs or cubic meter per second in American English) is a derived SI unit of flow rate equal to that of a stere or cube with sides of one metre ( u0303 39.37 in) in length exchanged or moving each second. It is popularly used for water flow, especially in rivers and streams, and fractions for HVAC values measuring air flow.

-- QUDT"""@en ;
    rdfs:isDefinedBy "http://qudt.org/2.1/vocab/unit"^^xsd:string ;
    rdfs:subClassOf [ a owl:Restriction ;
            owl:hasValue 1e+00 ;
            owl:onProperty ns1:hasSIConversionMultiplier ],
        [ a owl:Restriction ;
            owl:hasValue 0e+00 ;
            owl:onProperty ns1:hasSIConversionOffset ],
        ns1:SICoherentDerivedUnit,
        ns1:VolumePerTimeUnit ;
    skos:altLabel "Cubic Metre per Second"@en ;
    skos:prefLabel "CubicMetrePerSecond"@en ;
    ns1:elucidation """A cubic metre per second (m³s⁻¹, m³/s), cumecs or cubic meter per second in American English) is a derived SI unit of flow rate equal to that of a stere or cube with sides of one metre ( u0303 39.37 in) in length exchanged or moving each second. It is popularly used for water flow, especially in rivers and streams, and fractions for HVAC values measuring air flow.

-- QUDT"""@en ;
    ns1:qudtReference "http://qudt.org/vocab/unit/M3-PER-SEC"^^xsd:string ;
    ns1:ucumCode "m3.s-1"^^xsd:string,
        "m3/s"^^xsd:string ;
    ns1:unitSymbol "m³/s"^^xsd:string .

ns1:CubicMetrePerSquareMetre a owl:Class ;
    rdfs:label "CubicMetrePerSquareMetre"@en ;
    rdfs:comment """power of the SI base unit metre with the exponent 3 divided by the power of the SI base unit metre with the exponent 2

-- QUDT"""@en ;
    rdfs:isDefinedBy "http://qudt.org/2.1/vocab/unit"^^xsd:string ;
    rdfs:subClassOf [ a owl:Restriction ;
            owl:hasValue 1e+00 ;
            owl:onProperty ns1:hasSIConversionMultiplier ],
        [ a owl:Restriction ;
            owl:hasValue 0e+00 ;
            owl:onProperty ns1:hasSIConversionOffset ],
        ns1:LengthUnit,
        ns1:SICoherentDerivedUnit ;
    skos:altLabel "Cubic Metre Per Square Metre"@en ;
    skos:prefLabel "CubicMetrePerSquareMetre"@en ;
    ns1:elucidation """power of the SI base unit metre with the exponent 3 divided by the power of the SI base unit metre with the exponent 2

-- QUDT"""@en ;
    ns1:qudtReference "http://qudt.org/vocab/unit/M3-PER-M2"^^xsd:string ;
    ns1:ucumCode "m3.m-2"^^xsd:string ;
    ns1:unitSymbol "m³/m²"^^xsd:string .

ns1:CubicMetrePerSquareSecond a owl:Class ;
    rdfs:label "CubicMetrePerSquareSecond"@en ;
    rdfs:comment """`Cubic Meter per Square Second` is a C.G.S System unit for  `Standard Gravitational Parameter` expressed as m³/s²

-- QUDT"""@en ;
    rdfs:isDefinedBy "http://qudt.org/2.1/vocab/unit"^^xsd:string ;
    rdfs:subClassOf [ a owl:Restriction ;
            owl:hasValue 0e+00 ;
            owl:onProperty ns1:hasSIConversionOffset ],
        [ a owl:Restriction ;
            owl:hasValue 1e+00 ;
            owl:onProperty ns1:hasSIConversionMultiplier ],
        ns1:SICoherentDerivedUnit,
        ns1:VolumePerSquareTimeUnit ;
    skos:altLabel "Cubic Metre per Square Second"@en ;
    skos:prefLabel "CubicMetrePerSquareSecond"@en ;
    ns1:elucidation """`Cubic Meter per Square Second` is a C.G.S System unit for  `Standard Gravitational Parameter` expressed as m³/s²

-- QUDT"""@en ;
    ns1:qudtReference "http://qudt.org/vocab/unit/M3-PER-SEC2"^^xsd:string ;
    ns1:ucumCode "m3.s-2"^^xsd:string,
        "m3/s2"^^xsd:string ;
    ns1:unitSymbol "m³/s²"^^xsd:string .

ns1:DegreeCelsiusKilogramPerSquareMetre a owl:Class ;
    rdfs:label "DegreeCelsiusKilogramPerSquareMetre"^^xsd:string ;
    rdfs:comment """Derived unit for the product of the temperature in degrees Celsius and the mass density of a medium, integrated over vertical depth or height in metres.

-- QUDT"""@en ;
    rdfs:isDefinedBy "http://qudt.org/2.1/vocab/unit"^^xsd:string ;
    rdfs:subClassOf ns1:SICoherentUnit,
        ns1:TemperatureMassPerAreaUnit ;
    skos:altLabel "Degrees Celsius kilogram per square metre"@en ;
    skos:prefLabel "DegreeCelsiusKilogramPerSquareMetre"^^xsd:string ;
    ns1:elucidation """Derived unit for the product of the temperature in degrees Celsius and the mass density of a medium, integrated over vertical depth or height in metres.

-- QUDT"""@en ;
    ns1:qudtReference "http://qudt.org/vocab/unit/DEG_C-KiloGM-PER-M2"^^xsd:string ;
    ns1:ucumCode "Cel.kg.m-2"^^xsd:string ;
    ns1:unitSymbol "°C⋅kg/m²"^^xsd:string .

ns1:DegreeCelsiusPerKelvin a owl:Class ;
    rdfs:label "DegreeCelsiusPerKelvin"@en ;
    rdfs:comment """unit with the name Degree Celsius divided by the SI base unit kelvin

-- QUDT"""@en ;
    rdfs:isDefinedBy "http://qudt.org/2.1/vocab/unit"^^xsd:string ;
    rdfs:subClassOf ns1:DimensionlessUnit,
        ns1:SICoherentDerivedUnit ;
    skos:altLabel "Degree Celsius Per Kelvin"@en ;
    skos:prefLabel "DegreeCelsiusPerKelvin"@en ;
    ns1:elucidation """unit with the name Degree Celsius divided by the SI base unit kelvin

-- QUDT"""@en ;
    ns1:qudtReference "http://qudt.org/vocab/unit/DEG_C-PER-K"^^xsd:string ;
    ns1:ucumCode "Cel.K-1"^^xsd:string,
        "Cel/K"^^xsd:string ;
    ns1:unitSymbol "°C/K"^^xsd:string .

ns1:DegreeCelsiusPerMetre a owl:Class ;
    rdfs:label "DegreeCelsiusPerMetre"^^xsd:string ;
    rdfs:comment "Degree Celsius per metre unit."@en ;
    rdfs:isDefinedBy "http://qudt.org/2.1/vocab/unit"^^xsd:string ;
    rdfs:subClassOf ns1:SICoherentDerivedUnit,
        ns1:TemperaturePerLengthUnit ;
    skos:prefLabel "DegreeCelsiusPerMetre"^^xsd:string ;
    ns1:elucidation "Degree Celsius per metre unit."@en ;
    ns1:qudtReference "http://qudt.org/vocab/unit/DEG_C-PER-M"^^xsd:string ;
    ns1:ucumCode "Cel.m-1"^^xsd:string ;
    ns1:unitSymbol "°C/m"^^xsd:string .

ns1:DegreeCelsiusPerSecond a owl:Class ;
    rdfs:label "DegreeCelsiusPerSecond"@en ;
    rdfs:comment """`Degree Celsius per Second` is a unit for 'Temperature Per Time' expressed as degC / s.

-- QUDT"""@en ;
    rdfs:isDefinedBy "http://qudt.org/2.1/vocab/unit"^^xsd:string ;
    rdfs:subClassOf ns1:SICoherentDerivedUnit,
        ns1:TemperaturePerTimeUnit ;
    skos:altLabel "Degree Celsius per Second"@en ;
    skos:prefLabel "DegreeCelsiusPerSecond"@en ;
    ns1:elucidation """`Degree Celsius per Second` is a unit for 'Temperature Per Time' expressed as degC / s.

-- QUDT"""@en ;
    ns1:qudtReference "http://qudt.org/vocab/unit/DEG_C-PER-SEC"^^xsd:string ;
    ns1:ucumCode "Cel.s-1"^^xsd:string,
        "Cel/s"^^xsd:string ;
    ns1:unitSymbol "°C/s"^^xsd:string .

ns1:FaradPerMetre a owl:Class ;
    rdfs:label "FaradPerMetre"@en ;
    rdfs:comment """Farad Per Meter (F/m) is a unit in the category of Electric permittivity. It is also known as farad/meter. This unit is commonly used in the SI unit system. Farad Per Meter has a dimension of M-1L-3T4I2 where M is mass, L is length, T is time, and I is electric current. This unit is the standard SI unit in this category.

-- QUDT"""@en ;
    rdfs:isDefinedBy "http://qudt.org/2.1/vocab/unit"^^xsd:string ;
    rdfs:subClassOf [ a owl:Restriction ;
            owl:hasValue 1e+00 ;
            owl:onProperty ns1:hasSIConversionMultiplier ],
        [ a owl:Restriction ;
            owl:hasValue 0e+00 ;
            owl:onProperty ns1:hasSIConversionOffset ],
        ns1:PermittivityUnit,
        ns1:SICoherentDerivedUnit ;
    skos:altLabel "Farad per Metre"@en ;
    skos:prefLabel "FaradPerMetre"@en ;
    ns1:elucidation """Farad Per Meter (F/m) is a unit in the category of Electric permittivity. It is also known as farad/meter. This unit is commonly used in the SI unit system. Farad Per Meter has a dimension of M-1L-3T4I2 where M is mass, L is length, T is time, and I is electric current. This unit is the standard SI unit in this category.

-- QUDT"""@en ;
    ns1:qudtReference "http://qudt.org/vocab/unit/FARAD-PER-M"^^xsd:string ;
    ns1:ucumCode "F.m-1"^^xsd:string,
        "F/m"^^xsd:string ;
    ns1:unitSymbol "F/m"^^xsd:string .

ns1:Fraction a owl:Class ;
    rdfs:label "Fraction"@en ;
    rdfs:comment """Fraction is a unit for 'Dimensionless Ratio' expressed as the value of the ratio itself.

-- QUDT"""@en ;
    rdfs:isDefinedBy "http://qudt.org/2.1/vocab/unit"^^xsd:string ;
    rdfs:subClassOf [ a owl:Restriction ;
            owl:hasValue 1e+00 ;
            owl:onProperty ns1:hasSIConversionMultiplier ],
        [ a owl:Restriction ;
            owl:hasValue 0e+00 ;
            owl:onProperty ns1:hasSIConversionOffset ],
        ns1:FractionUnit,
        ns1:SICoherentDerivedUnit ;
    skos:prefLabel "Fraction"@en ;
    ns1:elucidation """Fraction is a unit for 'Dimensionless Ratio' expressed as the value of the ratio itself.

-- QUDT"""@en ;
    ns1:qudtReference "http://qudt.org/vocab/unit/FRACTION"^^xsd:string ;
    ns1:unitSymbol "÷"^^xsd:string .

ns1:GramPerGram a owl:Class ;
    rdfs:label "GramPerGram"@en ;
    rdfs:comment """mass ratio consisting of the 0.001-fold of the SI base unit kilogram divided by the 0.001-fold of the SI base unit kilogram.

-- QUDT"""@en ;
    rdfs:isDefinedBy "http://qudt.org/2.1/vocab/unit"^^xsd:string ;
    rdfs:subClassOf [ a owl:Restriction ;
            owl:hasValue 1e+00 ;
            owl:onProperty ns1:hasSIConversionMultiplier ],
        [ a owl:Restriction ;
            owl:hasValue 0e+00 ;
            owl:onProperty ns1:hasSIConversionOffset ],
        ns1:MassFractionUnit,
        ns1:MeasurementUnit,
        ns1:NonPrefixedUnit,
        ns1:SINonCoherentUnit ;
    skos:altLabel "Gram Per Gram"@en ;
    skos:prefLabel "GramPerGram"@en ;
    ns1:elucidation """mass ratio consisting of the 0.001-fold of the SI base unit kilogram divided by the 0.001-fold of the SI base unit kilogram.

-- QUDT"""@en ;
    ns1:qudtReference "http://qudt.org/vocab/unit/GM-PER-GM"^^xsd:string ;
    ns1:ucumCode "g.g-1"^^xsd:string,
        "g/g"^^xsd:string ;
    ns1:unitSymbol "g/g"^^xsd:string .

ns1:GrayPerSecond a owl:Class ;
    rdfs:label "GrayPerSecond"@en ;
    rdfs:comment """"Gray per Second" is a unit for  'Absorbed Dose Rate' expressed as Gy/s.

-- QUDT"""@en ;
    rdfs:isDefinedBy "http://qudt.org/2.1/vocab/unit"^^xsd:string ;
    rdfs:subClassOf [ a owl:Restriction ;
            owl:hasValue 1e+00 ;
            owl:onProperty ns1:hasSIConversionMultiplier ],
        [ a owl:Restriction ;
            owl:hasValue 0e+00 ;
            owl:onProperty ns1:hasSIConversionOffset ],
        ns1:AbsorbedDoseRateUnit,
        ns1:SICoherentDerivedUnit ;
    skos:altLabel "Gray per Second"@en ;
    skos:prefLabel "GrayPerSecond"@en ;
    ns1:elucidation """"Gray per Second" is a unit for  'Absorbed Dose Rate' expressed as Gy/s.

-- QUDT"""@en ;
    ns1:qudtReference "http://qudt.org/vocab/unit/GRAY-PER-SEC"^^xsd:string ;
    ns1:ucumCode "Gy.s-1"^^xsd:string ;
    ns1:unitSymbol "Gy/s"^^xsd:string .

ns1:HenryPerMetre a owl:Class ;
    rdfs:label "HenryPerMetre"@en ;
    rdfs:comment """The henry per meter (symbolized H/m) is the unit of magnetic permeability in the International System of Units ( SI ). Reduced to base units in SI, 1 H/m is the equivalent of one kilogram meter per square second per square ampere.

-- QUDT"""@en ;
    rdfs:isDefinedBy "http://qudt.org/2.1/vocab/unit"^^xsd:string ;
    rdfs:subClassOf [ a owl:Restriction ;
            owl:hasValue 0e+00 ;
            owl:onProperty ns1:hasSIConversionOffset ],
        [ a owl:Restriction ;
            owl:hasValue 1e+00 ;
            owl:onProperty ns1:hasSIConversionMultiplier ],
        ns1:PermeabilityUnit,
        ns1:SICoherentDerivedUnit ;
    skos:altLabel "Henry per Metre"@en ;
    skos:prefLabel "HenryPerMetre"@en ;
    ns1:elucidation """The henry per meter (symbolized H/m) is the unit of magnetic permeability in the International System of Units ( SI ). Reduced to base units in SI, 1 H/m is the equivalent of one kilogram meter per square second per square ampere.

-- QUDT"""@en ;
    ns1:qudtReference "http://qudt.org/vocab/unit/H-PER-M"^^xsd:string ;
    ns1:ucumCode "H.m-1"^^xsd:string ;
    ns1:unitSymbol "H/m"^^xsd:string ;
    ns1:wikipediaReference "http://en.wikipedia.org/wiki/Henry?oldid=491435978"^^xsd:string .

ns1:HenryPerOhm a owl:Class ;
    rdfs:label "HenryPerOhm"@en ;
    rdfs:comment """SI derived unit henry divided by the SI derived unit ohm

-- QUDT"""@en ;
    rdfs:isDefinedBy "http://qudt.org/2.1/vocab/unit"^^xsd:string ;
    rdfs:subClassOf [ a owl:Restriction ;
            owl:hasValue 0e+00 ;
            owl:onProperty ns1:hasSIConversionOffset ],
        [ a owl:Restriction ;
            owl:hasValue 1e+00 ;
            owl:onProperty ns1:hasSIConversionMultiplier ],
        ns1:SICoherentDerivedUnit,
        ns1:TimeUnit ;
    skos:altLabel "Henry Per Ohm"@en ;
    skos:prefLabel "HenryPerOhm"@en ;
    ns1:elucidation """SI derived unit henry divided by the SI derived unit ohm

-- QUDT"""@en ;
    ns1:qudtReference "http://qudt.org/vocab/unit/H-PER-OHM"^^xsd:string ;
    ns1:ucumCode "H.Ohm-1"^^xsd:string ;
    ns1:unitSymbol "H/Ω"^^xsd:string .

ns1:HertzMetre a owl:Class ;
    rdfs:label "HertzMetre"@en ;
    rdfs:comment """product of the SI derived unit hertz and the SI base unit metre

-- QUDT"""@en ;
    rdfs:isDefinedBy "http://qudt.org/2.1/vocab/unit"^^xsd:string ;
    rdfs:subClassOf [ a owl:Restriction ;
            owl:hasValue 1e+00 ;
            owl:onProperty ns1:hasSIConversionMultiplier ],
        [ a owl:Restriction ;
            owl:hasValue 0e+00 ;
            owl:onProperty ns1:hasSIConversionOffset ],
        ns1:SICoherentDerivedUnit,
        ns1:SpeedUnit ;
    skos:altLabel "Hertz Metre"@en ;
    skos:prefLabel "HertzMetre"@en ;
    ns1:elucidation """product of the SI derived unit hertz and the SI base unit metre

-- QUDT"""@en ;
    ns1:qudtReference "http://qudt.org/vocab/unit/HZ-M"^^xsd:string ;
    ns1:ucumCode "Hz.m"^^xsd:string ;
    ns1:unitSymbol "Hz⋅M"^^xsd:string .

ns1:HertzPerKelvin a owl:Class ;
    rdfs:label "HertzPerKelvin"@en ;
    rdfs:comment """`Hertz per Kelvin` is a unit for 'Inverse Time Temperature' expressed as Hz K⁻¹.

-- QUDT"""@en ;
    rdfs:isDefinedBy "http://qudt.org/2.1/vocab/unit"^^xsd:string ;
    rdfs:subClassOf [ a owl:Restriction ;
            owl:hasValue 1e+00 ;
            owl:onProperty ns1:hasSIConversionMultiplier ],
        [ a owl:Restriction ;
            owl:hasValue 0e+00 ;
            owl:onProperty ns1:hasSIConversionOffset ],
        ns1:PerTemperatureTimeUnit,
        ns1:SICoherentDerivedUnit ;
    skos:altLabel "Hertz per Kelvin"@en ;
    skos:prefLabel "HertzPerKelvin"@en ;
    ns1:elucidation """`Hertz per Kelvin` is a unit for 'Inverse Time Temperature' expressed as Hz K⁻¹.

-- QUDT"""@en ;
    ns1:qudtReference "http://qudt.org/vocab/unit/HZ-PER-K"^^xsd:string ;
    ns1:ucumCode "Hz.K-1"^^xsd:string ;
    ns1:unitSymbol "Hz/K"^^xsd:string .

ns1:HertzPerTesla a owl:Class ;
    rdfs:label "HertzPerTesla"@en ;
    rdfs:comment """"Hertz per Tesla" is a unit for  'Electric Charge Per Mass' expressed as Hz T⁻¹.

-- QUDT"""@en ;
    rdfs:isDefinedBy "http://qudt.org/2.1/vocab/unit"^^xsd:string ;
    rdfs:subClassOf [ a owl:Restriction ;
            owl:hasValue 0e+00 ;
            owl:onProperty ns1:hasSIConversionOffset ],
        [ a owl:Restriction ;
            owl:hasValue 1e+00 ;
            owl:onProperty ns1:hasSIConversionMultiplier ],
        ns1:ElectricChargePerMassUnit,
        ns1:SICoherentDerivedUnit ;
    skos:altLabel "Hertz per Tesla"@en ;
    skos:prefLabel "HertzPerTesla"@en ;
    ns1:elucidation """"Hertz per Tesla" is a unit for  'Electric Charge Per Mass' expressed as Hz T⁻¹.

-- QUDT"""@en ;
    ns1:qudtReference "http://qudt.org/vocab/unit/HZ-PER-T"^^xsd:string ;
    ns1:ucumCode "Hz.T-1"^^xsd:string ;
    ns1:unitSymbol "Hz/T"^^xsd:string .

ns1:HertzPerVolt a owl:Class ;
    rdfs:label "HertzPerVolt"@en ;
    rdfs:comment """In the Hertz per Volt standard the frequency of the note is directly related to the voltage. A pitch of a note goes up one octave when its frequency doubles, meaning that the voltage will have to double for every octave rise. Depending on the footage (octave) selected, nominally one volt gives 1000Hz, two volts 2000Hz and so on. In terms of notes, bottom C would be 0.25 volts, the next C up would be 0.5 volts, then 1V, 2V, 4V, 8V for the following octaves. This system was used mainly by Yamaha and Korg.

-- QUDT"""@en ;
    rdfs:isDefinedBy "http://qudt.org/2.1/vocab/unit"^^xsd:string ;
    rdfs:subClassOf [ a owl:Restriction ;
            owl:hasValue 0e+00 ;
            owl:onProperty ns1:hasSIConversionOffset ],
        [ a owl:Restriction ;
            owl:hasValue 1e+00 ;
            owl:onProperty ns1:hasSIConversionMultiplier ],
        ns1:ElectricCurrentPerEnergyUnit,
        ns1:SICoherentDerivedUnit ;
    skos:altLabel "Hertz per Volt"@en ;
    skos:prefLabel "HertzPerVolt"@en ;
    ns1:elucidation """In the Hertz per Volt standard the frequency of the note is directly related to the voltage. A pitch of a note goes up one octave when its frequency doubles, meaning that the voltage will have to double for every octave rise. Depending on the footage (octave) selected, nominally one volt gives 1000Hz, two volts 2000Hz and so on. In terms of notes, bottom C would be 0.25 volts, the next C up would be 0.5 volts, then 1V, 2V, 4V, 8V for the following octaves. This system was used mainly by Yamaha and Korg.

-- QUDT"""@en ;
    ns1:qudtReference "http://qudt.org/vocab/unit/HZ-PER-V"^^xsd:string ;
    ns1:ucumCode "Hz.V-1"^^xsd:string ;
    ns1:unitSymbol "Hz/V"^^xsd:string .

ns1:JouleMetrePerMole a owl:Class ;
    rdfs:label "JouleMetrePerMole"@en ;
    rdfs:comment """`Joule Meter per Mole` is a unit for 'Length Molar Energy' expressed as J · m · mol⁻¹.

-- QUDT"""@en ;
    rdfs:isDefinedBy "http://qudt.org/2.1/vocab/unit"^^xsd:string ;
    rdfs:subClassOf [ a owl:Restriction ;
            owl:hasValue 1e+00 ;
            owl:onProperty ns1:hasSIConversionMultiplier ],
        [ a owl:Restriction ;
            owl:hasValue 0e+00 ;
            owl:onProperty ns1:hasSIConversionOffset ],
        ns1:EnergyLengthPerAmountUnit,
        ns1:SICoherentDerivedUnit ;
    skos:altLabel "Joule Metre per Mole"@en ;
    skos:prefLabel "JouleMetrePerMole"@en ;
    ns1:elucidation """`Joule Meter per Mole` is a unit for 'Length Molar Energy' expressed as J · m · mol⁻¹.

-- QUDT"""@en ;
    ns1:qudtReference "http://qudt.org/vocab/unit/J-M-PER-MOL"^^xsd:string ;
    ns1:ucumCode "J.m.mol-1"^^xsd:string ;
    ns1:unitSymbol "J⋅m/mol"^^xsd:string .

ns1:JoulePerCubicMetre a owl:Class ;
    rdfs:label "JoulePerCubicMetre"@en ;
    rdfs:comment """`Joule Per Cubic Meter` (J/m³) is a unit in the category of Energy density. It is also known as joules per cubic meter, joule per cubic metre, joules per cubic metre, joule/cubic meter, joule/cubic metre. This unit is commonly used in the SI unit system.  It has a dimension of ML⁻¹T⁻² where M is mass, L is length, and T is time. This unit is the standard SI unit in this category.

-- QUDT"""@en ;
    rdfs:isDefinedBy "http://qudt.org/2.1/vocab/unit"^^xsd:string ;
    rdfs:subClassOf [ a owl:Restriction ;
            owl:hasValue 1e+00 ;
            owl:onProperty ns1:hasSIConversionMultiplier ],
        [ a owl:Restriction ;
            owl:hasValue 0e+00 ;
            owl:onProperty ns1:hasSIConversionOffset ],
        ns1:PressureUnit,
        ns1:SICoherentDerivedUnit ;
    skos:altLabel "Joule per Cubic Metre"@en ;
    skos:prefLabel "JoulePerCubicMetre"@en ;
    ns1:elucidation """`Joule Per Cubic Meter` (J/m³) is a unit in the category of Energy density. It is also known as joules per cubic meter, joule per cubic metre, joules per cubic metre, joule/cubic meter, joule/cubic metre. This unit is commonly used in the SI unit system.  It has a dimension of ML⁻¹T⁻² where M is mass, L is length, and T is time. This unit is the standard SI unit in this category.

-- QUDT"""@en ;
    ns1:qudtReference "http://qudt.org/vocab/unit/J-PER-M3"^^xsd:string ;
    ns1:ucumCode "J.m-3"^^xsd:string,
        "J/m3"^^xsd:string ;
    ns1:unitSymbol "J/m³"^^xsd:string .

ns1:JoulePerCubicMetreKelvin a owl:Class ;
    rdfs:label "JoulePerCubicMetreKelvin"@en ;
    rdfs:comment """`Joule per Cubic Meter Kelvin` is a unit for 'Volumetric Heat Capacity' expressed as J/(m³ K).

-- QUDT"""@en ;
    rdfs:isDefinedBy "http://qudt.org/2.1/vocab/unit"^^xsd:string ;
    rdfs:subClassOf [ a owl:Restriction ;
            owl:hasValue 1e+00 ;
            owl:onProperty ns1:hasSIConversionMultiplier ],
        [ a owl:Restriction ;
            owl:hasValue 0e+00 ;
            owl:onProperty ns1:hasSIConversionOffset ],
        ns1:PressurePerTemperatureUnit,
        ns1:SICoherentDerivedUnit ;
    skos:altLabel "Joule per Cubic Metre Kelvin"@en ;
    skos:prefLabel "JoulePerCubicMetreKelvin"@en ;
    ns1:elucidation """`Joule per Cubic Meter Kelvin` is a unit for 'Volumetric Heat Capacity' expressed as J/(m³ K).

-- QUDT"""@en ;
    ns1:qudtReference "http://qudt.org/vocab/unit/J-PER-M3-K"^^xsd:string ;
    ns1:ucumCode "J.m-3.K-1"^^xsd:string ;
    ns1:unitSymbol "J/(m³⋅K)"^^xsd:string .

ns1:JoulePerKelvin a owl:Class ;
    rdfs:label "JoulePerKelvin"@en ;
    rdfs:comment """Joule Per Kelvin (J/K) is a unit in the category of Entropy. It is also known as joules per kelvin, joule/kelvin. This unit is commonly used in the SI unit system. Joule Per Kelvin (J/K) has a dimension of ML²T⁻²Q⁻¹ where M is mass, L is length, T is time, and Q is temperature. This unit is the standard SI unit in this category.

-- QUDT"""@en ;
    rdfs:isDefinedBy "http://qudt.org/2.1/vocab/unit"^^xsd:string ;
    rdfs:subClassOf [ a owl:Restriction ;
            owl:hasValue 0e+00 ;
            owl:onProperty ns1:hasSIConversionOffset ],
        [ a owl:Restriction ;
            owl:hasValue 1e+00 ;
            owl:onProperty ns1:hasSIConversionMultiplier ],
        ns1:EntropyUnit,
        ns1:SICoherentDerivedUnit ;
    skos:altLabel "Joule per Kelvin"@en ;
    skos:prefLabel "JoulePerKelvin"@en ;
    ns1:elucidation """Joule Per Kelvin (J/K) is a unit in the category of Entropy. It is also known as joules per kelvin, joule/kelvin. This unit is commonly used in the SI unit system. Joule Per Kelvin (J/K) has a dimension of ML²T⁻²Q⁻¹ where M is mass, L is length, T is time, and Q is temperature. This unit is the standard SI unit in this category.

-- QUDT"""@en ;
    ns1:qudtReference "http://qudt.org/vocab/unit/J-PER-K"^^xsd:string ;
    ns1:ucumCode "J.K-1"^^xsd:string ;
    ns1:unitSymbol "J/K"^^xsd:string .

ns1:JoulePerKilogram a owl:Class ;
    rdfs:label "JoulePerKilogram"^^xsd:string ;
    rdfs:comment """Joule Per Kilogram} (J/kg) is a unit in the category of Thermal heat capacity. It is also known as `joule/kilogram`, `joules per kilogram`. This unit is commonly used in the SI unit system. The unit has a dimension of L2T⁻² where L is length, and T is time. This unit is the standard SI unit in this category.

-- QUDT"""@en ;
    rdfs:isDefinedBy "http://qudt.org/2.1/vocab/unit"^^xsd:string ;
    rdfs:subClassOf [ a owl:Restriction ;
            owl:hasValue 0e+00 ;
            owl:onProperty ns1:hasSIConversionOffset ],
        [ a owl:Restriction ;
            owl:hasValue 1e+00 ;
            owl:onProperty ns1:hasSIConversionMultiplier ],
        ns1:AbsorbedDoseUnit,
        ns1:SICoherentDerivedUnit ;
    skos:altLabel "Joule per Kilogram"@en ;
    skos:prefLabel "JoulePerKilogram"^^xsd:string ;
    ns1:elucidation """Joule Per Kilogram} (J/kg) is a unit in the category of Thermal heat capacity. It is also known as `joule/kilogram`, `joules per kilogram`. This unit is commonly used in the SI unit system. The unit has a dimension of L2T⁻² where L is length, and T is time. This unit is the standard SI unit in this category.

-- QUDT"""@en ;
    ns1:qudtReference "http://qudt.org/vocab/unit/J-PER-KiloGM"^^xsd:string ;
    ns1:ucumCode "J.kg-1"^^xsd:string,
        "J/kg"^^xsd:string ;
    ns1:unitSymbol "J/kg"^^xsd:string .

ns1:JoulePerKilogramKelvin a owl:Class ;
    rdfs:label "JoulePerKilogramKelvin"^^xsd:string ;
    rdfs:comment """Specific heat capacity - The heat required to raise unit mass of a substance by unit temperature interval under specified conditions, such as constant pressure: usually measured in joules per kelvin per kilogram. Symbol c_p (for constant pressure) Also called specific heat.

-- QUDT"""@en ;
    rdfs:isDefinedBy "http://qudt.org/2.1/vocab/unit"^^xsd:string ;
    rdfs:subClassOf [ a owl:Restriction ;
            owl:hasValue 0e+00 ;
            owl:onProperty ns1:hasSIConversionOffset ],
        [ a owl:Restriction ;
            owl:hasValue 1e+00 ;
            owl:onProperty ns1:hasSIConversionMultiplier ],
        ns1:EntropyPerMassUnit,
        ns1:SICoherentDerivedUnit ;
    skos:altLabel "Joule per Kilogram Kelvin"@en ;
    skos:prefLabel "JoulePerKilogramKelvin"^^xsd:string ;
    ns1:elucidation """Specific heat capacity - The heat required to raise unit mass of a substance by unit temperature interval under specified conditions, such as constant pressure: usually measured in joules per kelvin per kilogram. Symbol c_p (for constant pressure) Also called specific heat.

-- QUDT"""@en ;
    ns1:qudtReference "http://qudt.org/vocab/unit/J-PER-KiloGM-K"^^xsd:string ;
    ns1:ucumCode "J.kg-1.K-1"^^xsd:string ;
    ns1:unitSymbol "J/(kg⋅K)"^^xsd:string .

ns1:JoulePerKilogramKelvinCubicMetre a owl:Class ;
    rdfs:label "JoulePerKilogramKelvinCubicMetre"^^xsd:string ;
    rdfs:comment "Joule per kilogram and Kelvin and cubic metre."@en ;
    rdfs:isDefinedBy "http://qudt.org/2.1/vocab/unit"^^xsd:string ;
    rdfs:subClassOf [ a owl:Restriction ;
            owl:hasValue 1e+00 ;
            owl:onProperty ns1:hasSIConversionMultiplier ],
        [ a owl:Restriction ;
            owl:hasValue 0e+00 ;
            owl:onProperty ns1:hasSIConversionOffset ],
        ns1:EntropyPerMassUnit,
        ns1:SICoherentDerivedUnit ;
    skos:prefLabel "JoulePerKilogramKelvinCubicMetre"^^xsd:string ;
    ns1:elucidation "Joule per kilogram and Kelvin and cubic metre."@en ;
    ns1:qudtReference "http://qudt.org/vocab/unit/J-PER-KiloGM-K-M3"^^xsd:string ;
    ns1:ucumCode "J.kg-1.K.m-3"^^xsd:string ;
    ns1:unitSymbol "J/(kg⋅K⋅m³)"^^xsd:string .

ns1:JoulePerKilogramKelvinPerPascal a owl:Class ;
    rdfs:label "JoulePerKilogramKelvinPerPascal"^^xsd:string ;
    rdfs:comment "Joule per kilogram and Kelvin and Pascal."@en ;
    rdfs:isDefinedBy "http://qudt.org/2.1/vocab/unit"^^xsd:string ;
    rdfs:subClassOf [ a owl:Restriction ;
            owl:hasValue 0e+00 ;
            owl:onProperty ns1:hasSIConversionOffset ],
        [ a owl:Restriction ;
            owl:hasValue 1e+00 ;
            owl:onProperty ns1:hasSIConversionMultiplier ],
        ns1:EntropyPerMassUnit,
        ns1:SICoherentDerivedUnit ;
    skos:prefLabel "JoulePerKilogramKelvinPerPascal"^^xsd:string ;
    ns1:elucidation "Joule per kilogram and Kelvin and Pascal."@en ;
    ns1:qudtReference "http://qudt.org/vocab/unit/J-PER-KiloGM-K-PA"^^xsd:string ;
    ns1:ucumCode "J.kg-1.K-1.Pa-1"^^xsd:string ;
    ns1:unitSymbol "J/(kg⋅K⋅Pa)"^^xsd:string .

ns1:JoulePerMetre a owl:Class ;
    rdfs:label "JoulePerMetre"@en ;
    rdfs:comment "Joule per metre."@en ;
    rdfs:isDefinedBy "http://qudt.org/2.1/vocab/unit"^^xsd:string ;
    rdfs:subClassOf [ a owl:Restriction ;
            owl:hasValue 0e+00 ;
            owl:onProperty ns1:hasSIConversionOffset ],
        [ a owl:Restriction ;
            owl:hasValue 1e+00 ;
            owl:onProperty ns1:hasSIConversionMultiplier ],
        ns1:ForceUnit,
        ns1:SICoherentDerivedUnit ;
    skos:prefLabel "JoulePerMetre"@en ;
    ns1:elucidation "Joule per metre."@en ;
    ns1:qudtReference "http://qudt.org/vocab/unit/J-PER-M"^^xsd:string ;
    ns1:ucumCode "J.m-1"^^xsd:string,
        "J/m"^^xsd:string ;
    ns1:unitSymbol "J/m"^^xsd:string .

ns1:JoulePerMole a owl:Class ;
    rdfs:label "JoulePerMole"@en ;
    rdfs:comment """The joule per mole (symbol: J· mol⁻¹) is an SI derived unit of energy per amount of material. Energy is measured in joules, and the amount of material is measured in moles. Physical quantities measured in J· mol⁻¹) usually describe quantities of energy transferred during phase transformations or chemical reactions. Division by the number of moles facilitates comparison between processes involving different quantities of material and between similar processes involving different types of materials. The meaning of such a quantity is always context-dependent and, particularly for chemical reactions, is dependent on the (possibly arbitrary) definition of a 'mole' for a particular process.

-- QUDT"""@en ;
    rdfs:isDefinedBy "http://qudt.org/2.1/vocab/unit"^^xsd:string ;
    rdfs:subClassOf [ a owl:Restriction ;
            owl:hasValue 0e+00 ;
            owl:onProperty ns1:hasSIConversionOffset ],
        [ a owl:Restriction ;
            owl:hasValue 1e+00 ;
            owl:onProperty ns1:hasSIConversionMultiplier ],
        ns1:EnergyPerAmountUnit,
        ns1:SICoherentDerivedUnit ;
    skos:altLabel "Joule per Mole"@en ;
    skos:prefLabel "JoulePerMole"@en ;
    ns1:elucidation """The joule per mole (symbol: J· mol⁻¹) is an SI derived unit of energy per amount of material. Energy is measured in joules, and the amount of material is measured in moles. Physical quantities measured in J· mol⁻¹) usually describe quantities of energy transferred during phase transformations or chemical reactions. Division by the number of moles facilitates comparison between processes involving different quantities of material and between similar processes involving different types of materials. The meaning of such a quantity is always context-dependent and, particularly for chemical reactions, is dependent on the (possibly arbitrary) definition of a 'mole' for a particular process.

-- QUDT"""@en ;
    ns1:qudtReference "http://qudt.org/vocab/unit/J-PER-MOL"^^xsd:string ;
    ns1:ucumCode "J.mol-1"^^xsd:string ;
    ns1:unitSymbol "J/mol"^^xsd:string .

ns1:JoulePerMoleKelvin a owl:Class ;
    rdfs:label "JoulePerMoleKelvin"@en ;
    rdfs:comment """Energy needed to heat one mole of substance by 1 Kelvin, under standard conditions (not standard temperature and pressure STP). The standard molar entropy is usually given the symbol S, and has units of joules per mole kelvin (  J· mol⁻¹ K⁻¹). Unlike standard enthalpies of formation, the value of S is an absolute. That is, an element in its standard state has a nonzero value of S at room temperature.

-- QUDT"""@en ;
    rdfs:isDefinedBy "http://qudt.org/2.1/vocab/unit"^^xsd:string ;
    rdfs:subClassOf [ a owl:Restriction ;
            owl:hasValue 1e+00 ;
            owl:onProperty ns1:hasSIConversionMultiplier ],
        [ a owl:Restriction ;
            owl:hasValue 0e+00 ;
            owl:onProperty ns1:hasSIConversionOffset ],
        ns1:EntropyPerAmountUnit,
        ns1:SICoherentDerivedUnit ;
    skos:altLabel "Joule per Mole Kelvin"@en ;
    skos:prefLabel "JoulePerMoleKelvin"@en ;
    ns1:elucidation """Energy needed to heat one mole of substance by 1 Kelvin, under standard conditions (not standard temperature and pressure STP). The standard molar entropy is usually given the symbol S, and has units of joules per mole kelvin (  J· mol⁻¹ K⁻¹). Unlike standard enthalpies of formation, the value of S is an absolute. That is, an element in its standard state has a nonzero value of S at room temperature.

-- QUDT"""@en ;
    ns1:qudtReference "http://qudt.org/vocab/unit/J-PER-MOL-K"^^xsd:string ;
    ns1:ucumCode "J.mol-1.K-1"^^xsd:string ;
    ns1:unitSymbol "J/(mol⋅K)"^^xsd:string .

ns1:JoulePerQuarticMetre a owl:Class ;
    rdfs:label "JoulePerQuarticMetre"@en ;
    rdfs:comment """`Joule Per Quartic Meter` (J/m⁴) is a unit for the spectral concentration of radiant energy density (in terms of wavelength), or the spectral radiant energy density (in terms of wave length). This unit is commonly used in the SI unit system.

-- QUDT"""@en ;
    rdfs:isDefinedBy "http://qudt.org/2.1/vocab/unit"^^xsd:string ;
    rdfs:subClassOf ns1:MassPerSquareLengthSquareTimeUnit,
        ns1:SICoherentDerivedUnit ;
    skos:altLabel "Joule per Quartic Metre"@en ;
    skos:prefLabel "JoulePerQuarticMetre"@en ;
    ns1:elucidation """`Joule Per Quartic Meter` (J/m⁴) is a unit for the spectral concentration of radiant energy density (in terms of wavelength), or the spectral radiant energy density (in terms of wave length). This unit is commonly used in the SI unit system.

-- QUDT"""@en ;
    ns1:qudtReference "http://qudt.org/vocab/unit/J-PER-M4"^^xsd:string ;
    ns1:ucumCode "J.m-4"^^xsd:string ;
    ns1:unitSymbol "J/m⁴"^^xsd:string .

ns1:JoulePerSecond a owl:Class ;
    rdfs:label "JoulePerSecond"@en ;
    rdfs:comment """SI derived unit joule divided by the SI base unit second

-- QUDT"""@en ;
    rdfs:isDefinedBy "http://qudt.org/2.1/vocab/unit"^^xsd:string ;
    rdfs:subClassOf [ a owl:Restriction ;
            owl:hasValue 1e+00 ;
            owl:onProperty ns1:hasSIConversionMultiplier ],
        [ a owl:Restriction ;
            owl:hasValue 0e+00 ;
            owl:onProperty ns1:hasSIConversionOffset ],
        ns1:PowerUnit,
        ns1:SICoherentDerivedUnit ;
    skos:altLabel "Joule Per Second"@en ;
    skos:prefLabel "JoulePerSecond"@en ;
    ns1:elucidation """SI derived unit joule divided by the SI base unit second

-- QUDT"""@en ;
    ns1:qudtReference "http://qudt.org/vocab/unit/J-PER-SEC"^^xsd:string ;
    ns1:ucumCode "J.s-1"^^xsd:string ;
    ns1:unitSymbol "J/s"^^xsd:string .

ns1:JoulePerSquareMetre a owl:Class ;
    rdfs:label "JoulePerSquareMetre"@en ;
    rdfs:comment """Joule Per Square Meter (J/m²) is a unit in the category of Energy density. It is also known as joules per square meter, joule per square metre, joule/square meter, joule/square metre. This unit is commonly used in the SI unit system.

-- QUDT"""@en ;
    rdfs:isDefinedBy "http://qudt.org/2.1/vocab/unit"^^xsd:string ;
    rdfs:subClassOf [ a owl:Restriction ;
            owl:hasValue 1e+00 ;
            owl:onProperty ns1:hasSIConversionMultiplier ],
        [ a owl:Restriction ;
            owl:hasValue 0e+00 ;
            owl:onProperty ns1:hasSIConversionOffset ],
        ns1:ForcePerLengthUnit,
        ns1:SICoherentDerivedUnit ;
    skos:altLabel "Joule per Square Metre"@en ;
    skos:prefLabel "JoulePerSquareMetre"@en ;
    ns1:elucidation """Joule Per Square Meter (J/m²) is a unit in the category of Energy density. It is also known as joules per square meter, joule per square metre, joule/square meter, joule/square metre. This unit is commonly used in the SI unit system.

-- QUDT"""@en ;
    ns1:qudtReference "http://qudt.org/vocab/unit/J-PER-M2"^^xsd:string ;
    ns1:ucumCode "J.m-2"^^xsd:string,
        "J/m2"^^xsd:string ;
    ns1:unitSymbol "J/m²"^^xsd:string .

ns1:JoulePerSquareTesla a owl:Class ;
    rdfs:label "JoulePerSquareTesla"@en ;
    rdfs:comment """A measure of the diamagnetic energy, for a Bohr-radius spread around a magnetic axis, per square Tesla.

-- QUDT"""@en ;
    rdfs:isDefinedBy "http://qudt.org/2.1/vocab/unit"^^xsd:string ;
    rdfs:seeAlso "http://www.eng.fsu.edu/~dommelen/quantum/style_a/elecmagfld.html"^^xsd:string ;
    rdfs:subClassOf [ a owl:Restriction ;
            owl:hasValue 1e+00 ;
            owl:onProperty ns1:hasSIConversionMultiplier ],
        [ a owl:Restriction ;
            owl:hasValue 0e+00 ;
            owl:onProperty ns1:hasSIConversionOffset ],
        ns1:EnergyPerSquareMagneticFluxDensityUnit,
        ns1:SICoherentDerivedUnit ;
    skos:altLabel "Joule per Square Tesla"@en ;
    skos:prefLabel "JoulePerSquareTesla"@en ;
    ns1:elucidation """A measure of the diamagnetic energy, for a Bohr-radius spread around a magnetic axis, per square Tesla.

-- QUDT"""@en ;
    ns1:qudtReference "http://qudt.org/vocab/unit/J-PER-T2"^^xsd:string ;
    ns1:ucumCode "J.T-2"^^xsd:string ;
    ns1:unitSymbol "J/T²"^^xsd:string .

ns1:JoulePerTesla a owl:Class ;
    rdfs:label "JoulePerTesla"@en ;
    rdfs:comment """The magnetic moment of a magnet is a quantity that determines the force that the magnet can exert on electric currents and the torque that a magnetic field will exert on it. A loop of electric current, a bar magnet, an electron, a molecule, and a planet all have magnetic moments. The unit for magnetic moment is not a base unit in the International System of Units (SI) and it can be represented in more than one way. For example, in the current loop definition, the area is measured in square meters and I is measured in amperes, so the magnetic moment is measured in ampere-square meters (A m2). In the equation for torque on a moment, the torque is measured in joules and the magnetic field in tesla, so the moment is measured in Joules per Tesla (J u00b7T-1). These two representations are equivalent: 1 A u00b7m2 = 1 J u00b7T-1.

-- QUDT"""@en ;
    rdfs:isDefinedBy "http://qudt.org/2.1/vocab/unit"^^xsd:string ;
    rdfs:subClassOf [ a owl:Restriction ;
            owl:hasValue 1e+00 ;
            owl:onProperty ns1:hasSIConversionMultiplier ],
        [ a owl:Restriction ;
            owl:hasValue 0e+00 ;
            owl:onProperty ns1:hasSIConversionOffset ],
        ns1:MagneticDipoleMomentUnit,
        ns1:SICoherentDerivedUnit ;
    skos:altLabel "Joule per Tesla"@en ;
    skos:prefLabel "JoulePerTesla"@en ;
    ns1:elucidation """The magnetic moment of a magnet is a quantity that determines the force that the magnet can exert on electric currents and the torque that a magnetic field will exert on it. A loop of electric current, a bar magnet, an electron, a molecule, and a planet all have magnetic moments. The unit for magnetic moment is not a base unit in the International System of Units (SI) and it can be represented in more than one way. For example, in the current loop definition, the area is measured in square meters and I is measured in amperes, so the magnetic moment is measured in ampere-square meters (A m2). In the equation for torque on a moment, the torque is measured in joules and the magnetic field in tesla, so the moment is measured in Joules per Tesla (J u00b7T-1). These two representations are equivalent: 1 A u00b7m2 = 1 J u00b7T-1.

-- QUDT"""@en ;
    ns1:qudtReference "http://qudt.org/vocab/unit/J-PER-T"^^xsd:string ;
    ns1:ucumCode "J.T-1"^^xsd:string ;
    ns1:unitSymbol "J/T"^^xsd:string .

ns1:JouleSecond a owl:Class ;
    rdfs:label "JouleSecond"@en ;
    rdfs:comment """The joule-second is a unit equal to a joule multiplied by a second, used to measure action or angular momentum. The joule-second is the unit used for Planck's constant.

-- QUDT"""@en ;
    rdfs:isDefinedBy "http://qudt.org/2.1/vocab/unit"^^xsd:string ;
    rdfs:subClassOf [ a owl:Restriction ;
            owl:hasValue 0e+00 ;
            owl:onProperty ns1:hasSIConversionOffset ],
        [ a owl:Restriction ;
            owl:hasValue 1e+00 ;
            owl:onProperty ns1:hasSIConversionMultiplier ],
        ns1:AngularMomentumUnit,
        ns1:SICoherentDerivedUnit ;
    skos:altLabel "Joule Second"@en ;
    skos:prefLabel "JouleSecond"@en ;
    ns1:elucidation """The joule-second is a unit equal to a joule multiplied by a second, used to measure action or angular momentum. The joule-second is the unit used for Planck's constant.

-- QUDT"""@en ;
    ns1:qudtReference "http://qudt.org/vocab/unit/J-SEC"^^xsd:string ;
    ns1:ucumCode "J.s"^^xsd:string ;
    ns1:unitSymbol "J⋅s"^^xsd:string .

ns1:JouleSecondPerMole a owl:Class ;
    rdfs:label "JouleSecondPerMole"@en ;
    rdfs:comment """`Joule Second per Mole` is a unit for 'Molar Angular Momentum' expressed as J s mol⁻¹.

-- QUDT"""@en ;
    rdfs:isDefinedBy "http://qudt.org/2.1/vocab/unit"^^xsd:string ;
    rdfs:subClassOf [ a owl:Restriction ;
            owl:hasValue 1e+00 ;
            owl:onProperty ns1:hasSIConversionMultiplier ],
        [ a owl:Restriction ;
            owl:hasValue 0e+00 ;
            owl:onProperty ns1:hasSIConversionOffset ],
        ns1:EnergyTimePerAmountUnit,
        ns1:SICoherentDerivedUnit ;
    skos:altLabel "Joule Second per Mole"@en ;
    skos:prefLabel "JouleSecondPerMole"@en ;
    ns1:elucidation """`Joule Second per Mole` is a unit for 'Molar Angular Momentum' expressed as J s mol⁻¹.

-- QUDT"""@en ;
    ns1:qudtReference "http://qudt.org/vocab/unit/J-SEC-PER-MOL"^^xsd:string ;
    ns1:ucumCode "J.s.mol-1"^^xsd:string ;
    ns1:unitSymbol "J⋅s/mol"^^xsd:string .

ns1:JouleSquareMetre a owl:Class ;
    rdfs:label "JouleSquareMetre"@en ;
    rdfs:comment "Joule square metre."@en ;
    rdfs:isDefinedBy "http://qudt.org/2.1/vocab/unit"^^xsd:string ;
    rdfs:subClassOf [ a owl:Restriction ;
            owl:hasValue 0e+00 ;
            owl:onProperty ns1:hasSIConversionOffset ],
        [ a owl:Restriction ;
            owl:hasValue 1e+00 ;
            owl:onProperty ns1:hasSIConversionMultiplier ],
        ns1:EnergyAreaUnit,
        ns1:SICoherentDerivedUnit ;
    skos:prefLabel "JouleSquareMetre"@en ;
    ns1:elucidation "Joule square metre."@en ;
    ns1:qudtReference "http://qudt.org/vocab/unit/J-M2"^^xsd:string ;
    ns1:ucumCode "J.m2"^^xsd:string ;
    ns1:unitSymbol "J⋅m²"^^xsd:string .

ns1:JouleSquareMetrePerKilogram a owl:Class ;
    rdfs:label "JouleSquareMetrePerKilogram"^^xsd:string ;
    rdfs:comment "Joule square metre per kilogram."@en ;
    rdfs:isDefinedBy "http://qudt.org/2.1/vocab/unit"^^xsd:string ;
    rdfs:subClassOf [ a owl:Restriction ;
            owl:hasValue 0e+00 ;
            owl:onProperty ns1:hasSIConversionOffset ],
        [ a owl:Restriction ;
            owl:hasValue 1e+00 ;
            owl:onProperty ns1:hasSIConversionMultiplier ],
        ns1:MassStoppingPowerUnit,
        ns1:SICoherentDerivedUnit ;
    skos:prefLabel "JouleSquareMetrePerKilogram"^^xsd:string ;
    ns1:elucidation "Joule square metre per kilogram."@en ;
    ns1:qudtReference "http://qudt.org/vocab/unit/J-M2-PER-KiloGM"^^xsd:string ;
    ns1:ucumCode "J.m2.kg-1"^^xsd:string ;
    ns1:unitSymbol "j⋅m²/kg"^^xsd:string .

ns1:KelvinMetre a owl:Class ;
    rdfs:label "KelvinMetre"^^xsd:string ;
    rdfs:comment "Kelvin metre."@en ;
    rdfs:isDefinedBy "http://qudt.org/2.1/vocab/unit"^^xsd:string ;
    rdfs:subClassOf [ a owl:Restriction ;
            owl:hasValue 0e+00 ;
            owl:onProperty ns1:hasSIConversionOffset ],
        [ a owl:Restriction ;
            owl:hasValue 1e+00 ;
            owl:onProperty ns1:hasSIConversionMultiplier ],
        ns1:LengthTemperatureUnit,
        ns1:SICoherentDerivedUnit ;
    skos:prefLabel "KelvinMetre"^^xsd:string ;
    ns1:elucidation "Kelvin metre."@en ;
    ns1:qudtReference "http://qudt.org/vocab/unit/K-M"^^xsd:string ;
    ns1:ucumCode "K.m"^^xsd:string ;
    ns1:unitSymbol "K⋅m"^^xsd:string .

ns1:KelvinMetrePerSecond a owl:Class ;
    rdfs:label "KelvinMetrePerSecond"^^xsd:string ;
    rdfs:comment "Kelvin metre per second."@en ;
    rdfs:isDefinedBy "http://qudt.org/2.1/vocab/unit"^^xsd:string ;
    rdfs:subClassOf [ a owl:Restriction ;
            owl:hasValue 0e+00 ;
            owl:onProperty ns1:hasSIConversionOffset ],
        [ a owl:Restriction ;
            owl:hasValue 1e+00 ;
            owl:onProperty ns1:hasSIConversionMultiplier ],
        ns1:SICoherentDerivedUnit,
        ns1:TemperatureLengthPerTimeUnit ;
    skos:prefLabel "KelvinMetrePerSecond"^^xsd:string ;
    ns1:elucidation "Kelvin metre per second."@en ;
    ns1:qudtReference "http://qudt.org/vocab/unit/K-M-PER-SEC"^^xsd:string ;
    ns1:ucumCode "K.m.s-1"^^xsd:string ;
    ns1:unitSymbol "K⋅m/s"^^xsd:string .

ns1:KelvinMetrePerWatt a owl:Class ;
    rdfs:label "KelvinMetrePerWatt"@en ;
    rdfs:comment """product of the SI base unit kelvin and the SI base unit metre divided by the derived SI unit watt

-- QUDT"""@en ;
    rdfs:isDefinedBy "http://qudt.org/2.1/vocab/unit"^^xsd:string ;
    rdfs:subClassOf [ a owl:Restriction ;
            owl:hasValue 0e+00 ;
            owl:onProperty ns1:hasSIConversionOffset ],
        [ a owl:Restriction ;
            owl:hasValue 1e+00 ;
            owl:onProperty ns1:hasSIConversionMultiplier ],
        ns1:SICoherentDerivedUnit,
        ns1:ThermalResistivityUnit ;
    skos:altLabel "Kelvin Metre Per Watt"@en ;
    skos:prefLabel "KelvinMetrePerWatt"@en ;
    ns1:elucidation """product of the SI base unit kelvin and the SI base unit metre divided by the derived SI unit watt

-- QUDT"""@en ;
    ns1:qudtReference "http://qudt.org/vocab/unit/K-M-PER-W"^^xsd:anyURI ;
    ns1:ucumCode "K.m.W-1"^^xsd:string ;
    ns1:unitSymbol "K⋅m/W"^^xsd:string .

ns1:KelvinPascalPerSecond a owl:Class ;
    rdfs:label "KelvinPascalPerSecond"^^xsd:string ;
    rdfs:comment "Kelvin Pascal per second."@en ;
    rdfs:isDefinedBy "http://qudt.org/2.1/vocab/unit"^^xsd:string ;
    rdfs:subClassOf [ a owl:Restriction ;
            owl:hasValue 0e+00 ;
            owl:onProperty ns1:hasSIConversionOffset ],
        [ a owl:Restriction ;
            owl:hasValue 1e+00 ;
            owl:onProperty ns1:hasSIConversionMultiplier ],
        ns1:SICoherentDerivedUnit,
        ns1:TemperaturePressurePerTimeUnit ;
    skos:prefLabel "KelvinPascalPerSecond"^^xsd:string ;
    ns1:elucidation "Kelvin Pascal per second."@en ;
    ns1:qudtReference "http://qudt.org/vocab/unit/K-PA-PER-SEC"^^xsd:string ;
    ns1:ucumCode "K.Pa.s-1"^^xsd:string ;
    ns1:unitSymbol "K⋅Pa/s"^^xsd:string .

ns1:KelvinPerKelvin a owl:Class ;
    rdfs:label "KelvinPerKelvin"@en ;
    rdfs:comment """SI base unit kelvin divided by the SI base unit kelvin

-- QUDT"""@en ;
    rdfs:isDefinedBy "http://qudt.org/2.1/vocab/unit"^^xsd:string ;
    rdfs:subClassOf [ a owl:Restriction ;
            owl:hasValue 0e+00 ;
            owl:onProperty ns1:hasSIConversionOffset ],
        [ a owl:Restriction ;
            owl:hasValue 1e+00 ;
            owl:onProperty ns1:hasSIConversionMultiplier ],
        ns1:FractionUnit,
        ns1:SICoherentDerivedUnit ;
    skos:altLabel "Kelvin Per Kelvin"@en ;
    skos:prefLabel "KelvinPerKelvin"@en ;
    ns1:elucidation """SI base unit kelvin divided by the SI base unit kelvin

-- QUDT"""@en ;
    ns1:qudtReference "http://qudt.org/vocab/unit/K-PER-K"^^xsd:string ;
    ns1:ucumCode "K.K-1"^^xsd:string ;
    ns1:unitSymbol "K/K"^^xsd:string .

ns1:KelvinPerMetre a owl:Class ;
    rdfs:label "KelvinPerMetre"@en ;
    rdfs:comment """A change of temperature on the Kelvin temperature scale in one SI unit of length.

-- QUDT"""@en ;
    rdfs:isDefinedBy "http://qudt.org/2.1/vocab/unit"^^xsd:string ;
    rdfs:subClassOf [ a owl:Restriction ;
            owl:hasValue 0e+00 ;
            owl:onProperty ns1:hasSIConversionOffset ],
        [ a owl:Restriction ;
            owl:hasValue 1e+00 ;
            owl:onProperty ns1:hasSIConversionMultiplier ],
        ns1:SICoherentDerivedUnit,
        ns1:TemperaturePerLengthUnit ;
    skos:altLabel "KelvinPerMeter"@en ;
    skos:prefLabel "KelvinPerMetre"@en ;
    ns1:elucidation """A change of temperature on the Kelvin temperature scale in one SI unit of length.

-- QUDT"""@en ;
    ns1:qudtReference "http://qudt.org/vocab/unit/K-PER-M"^^xsd:string ;
    ns1:ucumCode "K.m-1"^^xsd:string ;
    ns1:unitSymbol "K/m"^^xsd:string .

ns1:KelvinPerSecond a owl:Class ;
    rdfs:label "KelvinPerSecond"@en ;
    rdfs:comment """`Kelvin per Second` is a unit for 'Temperature Per Time' expressed as K / s.

-- QUDT"""@en ;
    rdfs:isDefinedBy "http://qudt.org/2.1/vocab/unit"^^xsd:string ;
    rdfs:subClassOf [ a owl:Restriction ;
            owl:hasValue 0e+00 ;
            owl:onProperty ns1:hasSIConversionOffset ],
        [ a owl:Restriction ;
            owl:hasValue 1e+00 ;
            owl:onProperty ns1:hasSIConversionMultiplier ],
        ns1:SICoherentDerivedUnit,
        ns1:TemperaturePerTimeUnit ;
    skos:altLabel "Kelvin per Second"@en ;
    skos:prefLabel "KelvinPerSecond"@en ;
    ns1:elucidation """`Kelvin per Second` is a unit for 'Temperature Per Time' expressed as K / s.

-- QUDT"""@en ;
    ns1:qudtReference "http://qudt.org/vocab/unit/K-PER-SEC"^^xsd:string ;
    ns1:ucumCode "K.s-1"^^xsd:string,
        "K/s"^^xsd:string ;
    ns1:unitSymbol "K/s"^^xsd:string .

ns1:KelvinPerSquareSecond a owl:Class ;
    rdfs:label "KelvinPerSquareSecond"@en ;
    rdfs:comment """`Kelvin per Square Second` is a unit for 'Temperature Per Time Squared' expressed as K / s².

-- QUDT"""@en ;
    rdfs:isDefinedBy "http://qudt.org/2.1/vocab/unit"^^xsd:string ;
    rdfs:subClassOf [ a owl:Restriction ;
            owl:hasValue 1e+00 ;
            owl:onProperty ns1:hasSIConversionMultiplier ],
        [ a owl:Restriction ;
            owl:hasValue 0e+00 ;
            owl:onProperty ns1:hasSIConversionOffset ],
        ns1:SICoherentDerivedUnit,
        ns1:TemperaturePerSquareTimeUnit ;
    skos:altLabel "Kelvin per Square Second"@en ;
    skos:prefLabel "KelvinPerSquareSecond"@en ;
    ns1:elucidation """`Kelvin per Square Second` is a unit for 'Temperature Per Time Squared' expressed as K / s².

-- QUDT"""@en ;
    ns1:qudtReference "http://qudt.org/vocab/unit/K-PER-SEC2"^^xsd:string ;
    ns1:ucumCode "K.s-2"^^xsd:string,
        "K/s^2"^^xsd:string ;
    ns1:unitSymbol "K/s²"^^xsd:string .

ns1:KelvinPerTesla a owl:Class ;
    rdfs:label "KelvinPerTesla"@en ;
    rdfs:comment """`Kelvin per Tesla` is a unit for 'Temperature Per Magnetic Flux Density' expressed as K T⁻¹.

-- QUDT"""@en ;
    rdfs:isDefinedBy "http://qudt.org/2.1/vocab/unit"^^xsd:string ;
    rdfs:subClassOf [ a owl:Restriction ;
            owl:hasValue 1e+00 ;
            owl:onProperty ns1:hasSIConversionMultiplier ],
        [ a owl:Restriction ;
            owl:hasValue 0e+00 ;
            owl:onProperty ns1:hasSIConversionOffset ],
        ns1:SICoherentDerivedUnit,
        ns1:TemperaturePerMagneticFluxDensityUnit ;
    skos:altLabel "Kelvin per Tesla"@en ;
    skos:prefLabel "KelvinPerTesla"@en ;
    ns1:elucidation """`Kelvin per Tesla` is a unit for 'Temperature Per Magnetic Flux Density' expressed as K T⁻¹.

-- QUDT"""@en ;
    ns1:qudtReference "http://qudt.org/vocab/unit/K-PER-T"^^xsd:string ;
    ns1:ucumCode "K.T-1"^^xsd:string ;
    ns1:unitSymbol "K/T"^^xsd:string .

ns1:KelvinPerWatt a owl:Class ;
    rdfs:label "KelvinPerWatt"@en ;
    rdfs:comment """Thermal resistance is a heat property and a measure of a temperature difference by which an object or material resists a heat flow (heat per time unit or thermal resistance). Thermal resistance is the reciprocal thermal conductance. Absolute thermal resistance is the temperature difference across a structure when a unit of heat energy flows through it in unit time. It is the reciprocal of thermal conductance. The SI units of thermal resistance are kelvins per watt or the equivalent degrees Celsius per watt (the two are the same since as intervals).

-- QUDT"""@en ;
    rdfs:isDefinedBy "http://qudt.org/2.1/vocab/unit"^^xsd:string ;
    rdfs:subClassOf [ a owl:Restriction ;
            owl:hasValue 1e+00 ;
            owl:onProperty ns1:hasSIConversionMultiplier ],
        [ a owl:Restriction ;
            owl:hasValue 0e+00 ;
            owl:onProperty ns1:hasSIConversionOffset ],
        ns1:SICoherentDerivedUnit,
        ns1:ThermalResistanceUnit ;
    skos:altLabel "Kelvin per Watt"@en ;
    skos:prefLabel "KelvinPerWatt"@en ;
    ns1:elucidation """Thermal resistance is a heat property and a measure of a temperature difference by which an object or material resists a heat flow (heat per time unit or thermal resistance). Thermal resistance is the reciprocal thermal conductance. Absolute thermal resistance is the temperature difference across a structure when a unit of heat energy flows through it in unit time. It is the reciprocal of thermal conductance. The SI units of thermal resistance are kelvins per watt or the equivalent degrees Celsius per watt (the two are the same since as intervals).

-- QUDT"""@en ;
    ns1:qudtReference "http://qudt.org/vocab/unit/K-PER-W"^^xsd:string ;
    ns1:ucumCode "K.W-1"^^xsd:string,
        "K/W"^^xsd:string ;
    ns1:unitSymbol "K/W"^^xsd:string .

ns1:KelvinSecond a owl:Class ;
    rdfs:label "KelvinSecond"@en ;
    rdfs:comment "Kelvin second."@en ;
    rdfs:isDefinedBy "http://qudt.org/2.1/vocab/unit"^^xsd:string ;
    rdfs:subClassOf [ a owl:Restriction ;
            owl:hasValue 1e+00 ;
            owl:onProperty ns1:hasSIConversionMultiplier ],
        [ a owl:Restriction ;
            owl:hasValue 0e+00 ;
            owl:onProperty ns1:hasSIConversionOffset ],
        ns1:SICoherentDerivedUnit,
        ns1:TemperatureTimeUnit ;
    skos:prefLabel "KelvinSecond"@en ;
    ns1:elucidation "Kelvin second."@en ;
    ns1:qudtReference "http://qudt.org/vocab/unit/K-SEC"^^xsd:string ;
    ns1:ucumCode "K.s"^^xsd:string ;
    ns1:unitSymbol "K⋅s"^^xsd:string .

ns1:KelvinSquareMetrePerKilogramPerSecond a owl:Class ;
    rdfs:label "KelvinSquareMetrePerKilogramPerSecond"^^xsd:string ;
    rdfs:comment "Kelvin square metres per kilogram and second."@en ;
    rdfs:isDefinedBy "http://qudt.org/2.1/vocab/unit"^^xsd:string ;
    rdfs:subClassOf [ a owl:Restriction ;
            owl:hasValue 0e+00 ;
            owl:onProperty ns1:hasSIConversionOffset ],
        [ a owl:Restriction ;
            owl:hasValue 1e+00 ;
            owl:onProperty ns1:hasSIConversionMultiplier ],
        ns1:SICoherentDerivedUnit,
        ns1:TemperatureAreaPerMassTimeUnit ;
    skos:prefLabel "KelvinSquareMetrePerKilogramPerSecond"^^xsd:string ;
    ns1:elucidation "Kelvin square metres per kilogram and second."@en ;
    ns1:qudtReference "http://qudt.org/vocab/unit/K-M2-PER-KiloGM-SEC"^^xsd:string ;
    ns1:ucumCode "K.m2.kg-1.s-1"^^xsd:string ;
    ns1:unitSymbol "K⋅m²/(kg⋅s)"^^xsd:string .

ns1:KilogramKelvin a owl:Class ;
    rdfs:label "KilogramKelvin"^^xsd:string ;
    rdfs:comment """`Kilogram Kelvin` is a unit for 'Mass Temperature' expressed as kg-K.

-- QUDT"""@en ;
    rdfs:subClassOf [ a owl:Restriction ;
            owl:hasValue 0e+00 ;
            owl:onProperty ns1:hasSIConversionOffset ],
        [ a owl:Restriction ;
            owl:hasValue 1e+00 ;
            owl:onProperty ns1:hasSIConversionMultiplier ],
        ns1:MassTemperatureUnit,
        ns1:NonPrefixedUnit,
        ns1:SICoherentDerivedUnit ;
    skos:altLabel "Kilogram Kelvin"@en ;
    skos:prefLabel "KilogramKelvin"^^xsd:string ;
    ns1:elucidation """`Kilogram Kelvin` is a unit for 'Mass Temperature' expressed as kg-K.

-- QUDT"""@en ;
    ns1:qudtReference "http://qudt.org/vocab/unit/KiloGM-K"^^xsd:string ;
    ns1:ucumCode "kg.K"^^xsd:string ;
    ns1:unitSymbol "kg⋅K"^^xsd:string .

ns1:KilogramMetrePerSecond a owl:Class ;
    rdfs:label "KilogramMetrePerSecond"^^xsd:string ;
    rdfs:comment """"Kilogram Meter Per Second" is a unit for  'Linear Momentum' expressed as kg-m/s.

-- QUDT"""@en ;
    rdfs:subClassOf [ a owl:Restriction ;
            owl:hasValue 0e+00 ;
            owl:onProperty ns1:hasSIConversionOffset ],
        [ a owl:Restriction ;
            owl:hasValue 1e+00 ;
            owl:onProperty ns1:hasSIConversionMultiplier ],
        ns1:MomentumUnit,
        ns1:NonPrefixedUnit,
        ns1:SICoherentDerivedUnit ;
    skos:altLabel "Kilogram Metre Per Second"@en ;
    skos:prefLabel "KilogramMetrePerSecond"^^xsd:string ;
    ns1:elucidation """"Kilogram Meter Per Second" is a unit for  'Linear Momentum' expressed as kg-m/s.

-- QUDT"""@en ;
    ns1:qudtReference "http://qudt.org/vocab/unit/KiloGM-M-PER-SEC"^^xsd:string ;
    ns1:ucumCode "kg.m.s-1"^^xsd:string,
        "kg.m/s"^^xsd:string ;
    ns1:unitSymbol "kg⋅m/s"^^xsd:string .

ns1:KilogramPerCubicMetre a owl:Class ;
    rdfs:label "KilogramPerCubicMetre"^^xsd:string ;
    rdfs:comment """Kilogram per cubic metre is an SI derived unit of density, defined by mass in kilograms divided by volume in cubic metres. The official SI symbolic abbreviation is kg . m⁻³, or equivalently either kg/m³.

-- QUDT"""@en ;
    rdfs:subClassOf [ a owl:Restriction ;
            owl:hasValue 0e+00 ;
            owl:onProperty ns1:hasSIConversionOffset ],
        [ a owl:Restriction ;
            owl:hasValue 1e+00 ;
            owl:onProperty ns1:hasSIConversionMultiplier ],
        ns1:DensityUnit,
        ns1:NonPrefixedUnit,
        ns1:SICoherentDerivedUnit ;
    skos:altLabel "Kilogram per Cubic Metre"@en ;
    skos:prefLabel "KilogramPerCubicMetre"^^xsd:string ;
    ns1:elucidation """Kilogram per cubic metre is an SI derived unit of density, defined by mass in kilograms divided by volume in cubic metres. The official SI symbolic abbreviation is kg . m⁻³, or equivalently either kg/m³.

-- QUDT"""@en ;
    ns1:qudtReference "http://qudt.org/vocab/unit/KiloGM-PER-M3"^^xsd:string ;
    ns1:ucumCode "kg.m-3"^^xsd:string,
        "kg/m3"^^xsd:string ;
    ns1:unitSymbol "kg/m³"^^xsd:string .

ns1:KilogramPerCubicMetrePerSecond a owl:Class ;
    rdfs:label "KilogramPerCubicMetrePerSecond"^^xsd:string ;
    rdfs:subClassOf [ a owl:Restriction ;
            owl:hasValue 0e+00 ;
            owl:onProperty ns1:hasSIConversionOffset ],
        [ a owl:Restriction ;
            owl:hasValue 1e+00 ;
            owl:onProperty ns1:hasSIConversionMultiplier ],
        ns1:MassPerVolumeTimeUnit,
        ns1:NonPrefixedUnit,
        ns1:SICoherentDerivedUnit ;
    skos:altLabel "Kilograms per cubic metre per second"@en ;
    skos:prefLabel "KilogramPerCubicMetrePerSecond"^^xsd:string ;
    ns1:qudtReference "http://qudt.org/vocab/unit/KiloGM-PER-M3-SEC"^^xsd:string ;
    ns1:ucumCode "kg.m-3.s-1"^^xsd:string ;
    ns1:unitSymbol "kg/(m³⋅s)"^^xsd:string .

ns1:KilogramPerKilogram a owl:Class ;
    rdfs:label "KilogramPerKilogram"^^xsd:string ;
    rdfs:comment """SI base unit kilogram divided by the SI base unit kilogram

-- QUDT"""@en ;
    rdfs:subClassOf [ a owl:Restriction ;
            owl:hasValue 1e+00 ;
            owl:onProperty ns1:hasSIConversionMultiplier ],
        [ a owl:Restriction ;
            owl:hasValue 0e+00 ;
            owl:onProperty ns1:hasSIConversionOffset ],
        ns1:MassFractionUnit,
        ns1:NonPrefixedUnit,
        ns1:SICoherentDerivedUnit ;
    skos:altLabel "Kilogram Per Kilogram"@en ;
    skos:prefLabel "KilogramPerKilogram"^^xsd:string ;
    ns1:elucidation """SI base unit kilogram divided by the SI base unit kilogram

-- QUDT"""@en ;
    ns1:qudtReference "http://qudt.org/vocab/unit/KiloGM-PER-KiloGM"^^xsd:string ;
    ns1:ucumCode "kg.kg-1"^^xsd:string ;
    ns1:unitSymbol "kg/kg"^^xsd:string .

ns1:KilogramPerMetre a owl:Class ;
    rdfs:label "KilogramPerMetre"^^xsd:string ;
    rdfs:comment """Kilogram Per Meter (kg/m) is a unit in the category of Linear mass density. It is also known as kilogram/meter, kilogram/metre, kilograms per meter, kilogram per metre, kilograms per metre. This unit is commonly used in the SI unit system. Kilogram Per Meter (kg/m) has a dimension of ML-1 where M is mass, and L is length. This unit is the standard SI unit in this category.

-- QUDT"""@en ;
    rdfs:subClassOf [ a owl:Restriction ;
            owl:hasValue 1e+00 ;
            owl:onProperty ns1:hasSIConversionMultiplier ],
        [ a owl:Restriction ;
            owl:hasValue 0e+00 ;
            owl:onProperty ns1:hasSIConversionOffset ],
        ns1:MassPerLengthUnit,
        ns1:NonPrefixedUnit,
        ns1:SICoherentDerivedUnit ;
    skos:altLabel "Kilogram per Metre"@en ;
    skos:prefLabel "KilogramPerMetre"^^xsd:string ;
    ns1:elucidation """Kilogram Per Meter (kg/m) is a unit in the category of Linear mass density. It is also known as kilogram/meter, kilogram/metre, kilograms per meter, kilogram per metre, kilograms per metre. This unit is commonly used in the SI unit system. Kilogram Per Meter (kg/m) has a dimension of ML-1 where M is mass, and L is length. This unit is the standard SI unit in this category.

-- QUDT"""@en ;
    ns1:qudtReference "http://qudt.org/vocab/unit/KiloGM-PER-M"^^xsd:string ;
    ns1:ucumCode "kg.m-1"^^xsd:string,
        "kg/m"^^xsd:string ;
    ns1:unitSymbol "kg/m"^^xsd:string .

ns1:KilogramPerMetrePerSecond a owl:Class ;
    rdfs:label "KilogramPerMetrePerSecond"^^xsd:string ;
    rdfs:subClassOf [ a owl:Restriction ;
            owl:hasValue 0e+00 ;
            owl:onProperty ns1:hasSIConversionOffset ],
        [ a owl:Restriction ;
            owl:hasValue 1e+00 ;
            owl:onProperty ns1:hasSIConversionMultiplier ],
        ns1:MassPerLengthTimeUnit,
        ns1:NonPrefixedUnit,
        ns1:SICoherentDerivedUnit ;
    skos:altLabel "Kilograms per metre per second"@en ;
    skos:prefLabel "KilogramPerMetrePerSecond"^^xsd:string ;
    ns1:qudtReference "http://qudt.org/vocab/unit/KiloGM-PER-M-SEC"^^xsd:string ;
    ns1:ucumCode "kg.m-1.s-1"^^xsd:string ;
    ns1:unitSymbol "kg/(m⋅s)"^^xsd:string .

ns1:KilogramPerMetrePerSquareSecond a owl:Class ;
    rdfs:label "KilogramPerMetrePerSquareSecond"^^xsd:string ;
    rdfs:comment """The SI unit of pressure. The pascal is the standard pressure unit in the MKS metric system, equal to one newton per square meter or one "kilogram per meter per second per second." The unit is named for Blaise Pascal (1623-1662), French philosopher and mathematician, who was the first person to use a barometer to measure differences in altitude.

-- QUDT"""@en ;
    rdfs:subClassOf [ a owl:Restriction ;
            owl:hasValue 1e+00 ;
            owl:onProperty ns1:hasSIConversionMultiplier ],
        [ a owl:Restriction ;
            owl:hasValue 0e+00 ;
            owl:onProperty ns1:hasSIConversionOffset ],
        ns1:NonPrefixedUnit,
        ns1:PressureUnit,
        ns1:SICoherentDerivedUnit ;
    skos:altLabel "Kilograms per metre per square second"@en ;
    skos:prefLabel "KilogramPerMetrePerSquareSecond"^^xsd:string ;
    ns1:elucidation """The SI unit of pressure. The pascal is the standard pressure unit in the MKS metric system, equal to one newton per square meter or one "kilogram per meter per second per second." The unit is named for Blaise Pascal (1623-1662), French philosopher and mathematician, who was the first person to use a barometer to measure differences in altitude.

-- QUDT"""@en ;
    ns1:qudtReference "http://qudt.org/vocab/unit/KiloGM-PER-M-SEC2"^^xsd:string ;
    ns1:ucumCode "kg.m-1.s-2"^^xsd:string ;
    ns1:unitSymbol "kg/(m⋅s²)"^^xsd:string .

ns1:KilogramPerMole a owl:Class ;
    rdfs:label "KilogramPerMole"@en ;
    rdfs:comment """In chemistry, the molar mass M is defined as the mass of a given substance (chemical element or chemical compound) divided by its amount of substance. It is a physical property of a given substance. The base SI unit for molar mass is kg/mol. However, for historical reasons, molar masses are almost always expressed in g/mol. As an example, the molar mass of water is approximately: 18.01528(33) g/mol.

-- QUDT"""@en ;
    rdfs:subClassOf [ a owl:Restriction ;
            owl:hasValue 0e+00 ;
            owl:onProperty ns1:hasSIConversionOffset ],
        [ a owl:Restriction ;
            owl:hasValue 1e+00 ;
            owl:onProperty ns1:hasSIConversionMultiplier ],
        ns1:MassPerAmountUnit,
        ns1:NonPrefixedUnit,
        ns1:SICoherentDerivedUnit ;
    skos:altLabel "Kilogram per Mole"@en ;
    skos:prefLabel "KilogramPerMole"@en ;
    ns1:elucidation """In chemistry, the molar mass M is defined as the mass of a given substance (chemical element or chemical compound) divided by its amount of substance. It is a physical property of a given substance. The base SI unit for molar mass is kg/mol. However, for historical reasons, molar masses are almost always expressed in g/mol. As an example, the molar mass of water is approximately: 18.01528(33) g/mol.

-- QUDT"""@en ;
    ns1:qudtReference "http://qudt.org/vocab/unit/KiloGM-PER-MOL"^^xsd:string ;
    ns1:ucumCode "kg.mol-1"^^xsd:string,
        "kg/mol"^^xsd:string ;
    ns1:unitSymbol "kg/mol"^^xsd:string .

ns1:KilogramPerSecond a owl:Class ;
    rdfs:label "KilogramPerSecond"^^xsd:string ;
    rdfs:comment """Kilogram Per Second (kg/s) is a unit in the category of Mass flow rate. It is also known as kilogram/second, kilograms per second. This unit is commonly used in the SI unit system. Kilogram Per Second (kg/s) has a dimension of MT⁻¹ where M is mass, and T is time. This unit is the standard SI unit in this category.

-- QUDT"""@en ;
    rdfs:subClassOf [ a owl:Restriction ;
            owl:hasValue 0e+00 ;
            owl:onProperty ns1:hasSIConversionOffset ],
        [ a owl:Restriction ;
            owl:hasValue 1e+00 ;
            owl:onProperty ns1:hasSIConversionMultiplier ],
        ns1:MassPerTimeUnit,
        ns1:NonPrefixedUnit,
        ns1:SICoherentDerivedUnit ;
    skos:altLabel "Kilogram per Second"@en ;
    skos:prefLabel "KilogramPerSecond"^^xsd:string ;
    ns1:elucidation """Kilogram Per Second (kg/s) is a unit in the category of Mass flow rate. It is also known as kilogram/second, kilograms per second. This unit is commonly used in the SI unit system. Kilogram Per Second (kg/s) has a dimension of MT⁻¹ where M is mass, and T is time. This unit is the standard SI unit in this category.

-- QUDT"""@en ;
    ns1:qudtReference "http://qudt.org/vocab/unit/KiloGM-PER-SEC"^^xsd:string ;
    ns1:ucumCode "kg.s-1"^^xsd:string,
        "kg/s"^^xsd:string ;
    ns1:unitSymbol "kg/s"^^xsd:string .

ns1:KilogramPerSecondPerSquareMetre a owl:Class ;
    rdfs:label "KilogramPerSecondPerSquareMetre"^^xsd:string ;
    rdfs:comment """SI base unit kilogram divided by the product of the power of the SI base unit metre with the exponent 2 and the SI base unit second

-- QUDT"""@en ;
    rdfs:subClassOf [ a owl:Restriction ;
            owl:hasValue 0e+00 ;
            owl:onProperty ns1:hasSIConversionOffset ],
        [ a owl:Restriction ;
            owl:hasValue 1e+00 ;
            owl:onProperty ns1:hasSIConversionMultiplier ],
        ns1:MassFluxUnit,
        ns1:NonPrefixedUnit,
        ns1:SICoherentDerivedUnit ;
    skos:altLabel "Kilogram Per Second Per Square Metre"@en ;
    skos:prefLabel "KilogramPerSecondPerSquareMetre"^^xsd:string ;
    ns1:elucidation """SI base unit kilogram divided by the product of the power of the SI base unit metre with the exponent 2 and the SI base unit second

-- QUDT"""@en ;
    ns1:qudtReference "http://qudt.org/vocab/unit/KiloGM-PER-SEC-M2"^^xsd:string ;
    ns1:ucumCode "kg.(s.m2)-1"^^xsd:string,
        "kg.s-1.m-2"^^xsd:string,
        "kg/(s.m2)"^^xsd:string ;
    ns1:unitSymbol "kg/(s⋅m²)"^^xsd:string .

ns1:KilogramPerSquareMetre a owl:Class ;
    rdfs:label "KilogramPerSquareMetre"^^xsd:string ;
    rdfs:comment """Kilogram Per Square Meter (kg/m2) is a unit in the category of Surface density. It is also known as kilograms per square meter, kilogram per square metre, kilograms per square metre, kilogram/square meter, kilogram/square metre. This unit is commonly used in the SI unit system. Kilogram Per Square Meter (kg/m2) has a dimension of ML-2 where M is mass, and L is length. This unit is the standard SI unit in this category.

-- QUDT"""@en ;
    rdfs:subClassOf [ a owl:Restriction ;
            owl:hasValue 1e+00 ;
            owl:onProperty ns1:hasSIConversionMultiplier ],
        [ a owl:Restriction ;
            owl:hasValue 0e+00 ;
            owl:onProperty ns1:hasSIConversionOffset ],
        ns1:AreaDensityUnit,
        ns1:NonPrefixedUnit,
        ns1:SICoherentDerivedUnit ;
    skos:altLabel "Kilogram per Square Metre"@en ;
    skos:prefLabel "KilogramPerSquareMetre"^^xsd:string ;
    ns1:elucidation """Kilogram Per Square Meter (kg/m2) is a unit in the category of Surface density. It is also known as kilograms per square meter, kilogram per square metre, kilograms per square metre, kilogram/square meter, kilogram/square metre. This unit is commonly used in the SI unit system. Kilogram Per Square Meter (kg/m2) has a dimension of ML-2 where M is mass, and L is length. This unit is the standard SI unit in this category.

-- QUDT"""@en ;
    ns1:qudtReference "http://qudt.org/vocab/unit/KiloGM-PER-M2"^^xsd:string ;
    ns1:ucumCode "kg.m-2"^^xsd:string,
        "kg/m2"^^xsd:string ;
    ns1:unitSymbol "kg/m²"^^xsd:string .

ns1:KilogramPerSquareMetrePerPascalPerSecond a owl:Class ;
    rdfs:label "KilogramPerSquareMetrePerPascalPerSecond"^^xsd:string ;
    rdfs:subClassOf [ a owl:Restriction ;
            owl:hasValue 0e+00 ;
            owl:onProperty ns1:hasSIConversionOffset ],
        [ a owl:Restriction ;
            owl:hasValue 1e+00 ;
            owl:onProperty ns1:hasSIConversionMultiplier ],
        ns1:NonPrefixedUnit,
        ns1:SICoherentDerivedUnit,
        ns1:TimePerLengthUnit ;
    skos:altLabel "Kilograms per square metre per Pascal per second"@en ;
    skos:prefLabel "KilogramPerSquareMetrePerPascalPerSecond"^^xsd:string ;
    ns1:qudtReference "http://qudt.org/vocab/unit/KiloGM-PER-M2-PA-SEC"^^xsd:string ;
    ns1:unitSymbol "kg/(m²⋅s⋅Pa)"^^xsd:string ;
    ns1:wikipediaReference "https://en.wikipedia.org/wiki/Perm_(unit)"^^xsd:string .

ns1:KilogramPerSquareMetrePerSecond a owl:Class ;
    rdfs:label "KilogramPerSquareMetrePerSecond"^^xsd:string ;
    rdfs:subClassOf [ a owl:Restriction ;
            owl:hasValue 0e+00 ;
            owl:onProperty ns1:hasSIConversionOffset ],
        [ a owl:Restriction ;
            owl:hasValue 1e+00 ;
            owl:onProperty ns1:hasSIConversionMultiplier ],
        ns1:MassFluxUnit,
        ns1:NonPrefixedUnit,
        ns1:SICoherentDerivedUnit ;
    skos:altLabel "Kilograms per square metre per second"@en ;
    skos:prefLabel "KilogramPerSquareMetrePerSecond"^^xsd:string ;
    ns1:qudtReference "http://qudt.org/vocab/unit/KiloGM-PER-M2-SEC"^^xsd:string ;
    ns1:ucumCode "kg.m-2.s-1"^^xsd:string ;
    ns1:unitSymbol "kg/(m²⋅s)"^^xsd:string .

ns1:KilogramPerSquareMetreSquareSecond a owl:Class ;
    rdfs:label "KilogramPerSquareMetreSquareSecond"^^xsd:string ;
    rdfs:subClassOf [ a owl:Restriction ;
            owl:hasValue 0e+00 ;
            owl:onProperty ns1:hasSIConversionOffset ],
        [ a owl:Restriction ;
            owl:hasValue 1e+00 ;
            owl:onProperty ns1:hasSIConversionMultiplier ],
        ns1:MassPerSquareLengthSquareTimeUnit,
        ns1:NonPrefixedUnit,
        ns1:SICoherentDerivedUnit ;
    skos:altLabel "Kilogram per Square Metre Square Second"@en ;
    skos:prefLabel "KilogramPerSquareMetreSquareSecond"^^xsd:string ;
    ns1:qudtReference "http://qudt.org/vocab/unit/KiloGM-PER-M2-SEC2"^^xsd:string ;
    ns1:unitSymbol "kg/(m²⋅s²)"^^xsd:string .

ns1:KilogramPerSquareSecond a owl:Class ;
    rdfs:label "KilogramPerSquareSecond"^^xsd:string ;
    rdfs:subClassOf [ a owl:Restriction ;
            owl:hasValue 1e+00 ;
            owl:onProperty ns1:hasSIConversionMultiplier ],
        [ a owl:Restriction ;
            owl:hasValue 0e+00 ;
            owl:onProperty ns1:hasSIConversionOffset ],
        ns1:ForcePerLengthUnit,
        ns1:NonPrefixedUnit,
        ns1:SICoherentDerivedUnit ;
    skos:altLabel "Kilogram per Square Second"@en ;
    skos:prefLabel "KilogramPerSquareSecond"^^xsd:string ;
    ns1:qudtReference "http://qudt.org/vocab/unit/KiloGM-PER-SEC2"^^xsd:string ;
    ns1:ucumCode "kg.s-2"^^xsd:string,
        "kg/s2"^^xsd:string ;
    ns1:unitSymbol "kg/s²"^^xsd:string .

ns1:KilogramSquareMetre a owl:Class ;
    rdfs:label "KilogramSquareMetre"^^xsd:string ;
    rdfs:comment """"Kilogram Square Meter" is a unit for  'Moment Of Inertia' expressed as kg-m².

-- QUDT"""@en ;
    rdfs:subClassOf [ a owl:Restriction ;
            owl:hasValue 1e+00 ;
            owl:onProperty ns1:hasSIConversionMultiplier ],
        [ a owl:Restriction ;
            owl:hasValue 0e+00 ;
            owl:onProperty ns1:hasSIConversionOffset ],
        ns1:MassAreaUnit,
        ns1:NonPrefixedUnit,
        ns1:SICoherentDerivedUnit ;
    skos:altLabel "Kilogram Square Metre"@en ;
    skos:prefLabel "KilogramSquareMetre"^^xsd:string ;
    ns1:elucidation """"Kilogram Square Meter" is a unit for  'Moment Of Inertia' expressed as kg-m².

-- QUDT"""@en ;
    ns1:qudtReference "http://qudt.org/vocab/unit/KiloGM-M2"^^xsd:string ;
    ns1:ucumCode "kg.m2"^^xsd:string ;
    ns1:unitSymbol "kg⋅m²"^^xsd:string .

ns1:KilogramSquareMetrePerSecond a owl:Class ;
    rdfs:label "KilogramSquareMetrePerSecond"^^xsd:string ;
    rdfs:comment """"Kilogram Square Meter Per Second" is a unit for  'Angular Momentum' expressed as kg-m²-s⁻¹.

-- QUDT"""@en ;
    rdfs:subClassOf [ a owl:Restriction ;
            owl:hasValue 1e+00 ;
            owl:onProperty ns1:hasSIConversionMultiplier ],
        [ a owl:Restriction ;
            owl:hasValue 0e+00 ;
            owl:onProperty ns1:hasSIConversionOffset ],
        ns1:AngularMomentumUnit,
        ns1:NonPrefixedUnit,
        ns1:SICoherentDerivedUnit ;
    skos:altLabel "Kilogram Square Metre Per Second"@en ;
    skos:prefLabel "KilogramSquareMetrePerSecond"^^xsd:string ;
    ns1:elucidation """"Kilogram Square Meter Per Second" is a unit for  'Angular Momentum' expressed as kg-m²-s⁻¹.

-- QUDT"""@en ;
    ns1:qudtReference "http://qudt.org/vocab/unit/KiloGM-M2-PER-SEC"^^xsd:string ;
    ns1:ucumCode "kg.m2.s-1"^^xsd:string ;
    ns1:unitSymbol "kg⋅m²/s"^^xsd:string .

ns1:KilogramSquareSecond a owl:Class ;
    rdfs:label "KilogramSquareSecond"^^xsd:string ;
    rdfs:subClassOf [ a owl:Restriction ;
            owl:hasValue 1e+00 ;
            owl:onProperty ns1:hasSIConversionMultiplier ],
        [ a owl:Restriction ;
            owl:hasValue 0e+00 ;
            owl:onProperty ns1:hasSIConversionOffset ],
        ns1:MassSquareTimeUnit,
        ns1:NonPrefixedUnit,
        ns1:SICoherentDerivedUnit ;
    skos:altLabel "Kilogram Square Second"@en ;
    skos:prefLabel "KilogramSquareSecond"^^xsd:string ;
    ns1:qudtReference "http://qudt.org/vocab/unit/KiloGM-SEC2"^^xsd:string ;
    ns1:ucumCode "kg.s2"^^xsd:string ;
    ns1:unitSymbol "kg⋅s²"^^xsd:string .

ns1:LumenPerWatt a owl:Class ;
    rdfs:label "LumenPerWatt"@en ;
    rdfs:comment """A measurement of luminous efficacy, which is the light output in lumens using one watt of electricity.

-- QUDT"""@en ;
    rdfs:isDefinedBy "http://qudt.org/2.1/vocab/unit"^^xsd:string ;
    rdfs:subClassOf [ a owl:Restriction ;
            owl:hasValue 0e+00 ;
            owl:onProperty ns1:hasSIConversionOffset ],
        [ a owl:Restriction ;
            owl:hasValue 1e+00 ;
            owl:onProperty ns1:hasSIConversionMultiplier ],
        ns1:LuminousEfficacyUnit,
        ns1:SICoherentDerivedUnit ;
    skos:altLabel "Lumen per Watt"@en ;
    skos:prefLabel "LumenPerWatt"@en ;
    ns1:elucidation """A measurement of luminous efficacy, which is the light output in lumens using one watt of electricity.

-- QUDT"""@en ;
    ns1:qudtReference "http://qudt.org/vocab/unit/LM-PER-W"^^xsd:string ;
    ns1:ucumCode "lm.W-1"^^xsd:string ;
    ns1:unitSymbol "lm/W"^^xsd:string .

ns1:LumenSecond a owl:Class ;
    rdfs:label "LumenSecond"@en ;
    rdfs:comment """In photometry, the lumen second is the SI derived unit of luminous energy. It is based on the lumen, the SI unit of luminous flux, and the second, the SI base unit of time.  The lumen second is sometimes called the talbot (symbol T).  An older name for the lumen second was the lumberg.

-- QUDT"""@en ;
    rdfs:isDefinedBy "http://qudt.org/2.1/vocab/unit"^^xsd:string ;
    rdfs:subClassOf [ a owl:Restriction ;
            owl:hasValue 0e+00 ;
            owl:onProperty ns1:hasSIConversionOffset ],
        [ a owl:Restriction ;
            owl:hasValue 1e+00 ;
            owl:onProperty ns1:hasSIConversionMultiplier ],
        ns1:EnergyUnit,
        ns1:SICoherentDerivedUnit ;
    skos:altLabel "lumen second"@en ;
    skos:prefLabel "LumenSecond"@en ;
    ns1:elucidation """In photometry, the lumen second is the SI derived unit of luminous energy. It is based on the lumen, the SI unit of luminous flux, and the second, the SI base unit of time.  The lumen second is sometimes called the talbot (symbol T).  An older name for the lumen second was the lumberg.

-- QUDT"""@en ;
    ns1:qudtReference "http://qudt.org/vocab/unit/LM-SEC"^^xsd:string ;
    ns1:ucumCode "lm.s"^^xsd:string ;
    ns1:unitSymbol "lm⋅s"^^xsd:string .

ns1:MetreKelvin a owl:Class ;
    rdfs:label "MetreKelvin"@en ;
    rdfs:comment """`Meter Kelvin` is a unit for 'Length Temperature' expressed as m K.

-- QUDT"""@en ;
    rdfs:isDefinedBy "http://qudt.org/2.1/vocab/unit"^^xsd:string ;
    rdfs:subClassOf [ a owl:Restriction ;
            owl:hasValue 0e+00 ;
            owl:onProperty ns1:hasSIConversionOffset ],
        [ a owl:Restriction ;
            owl:hasValue 1e+00 ;
            owl:onProperty ns1:hasSIConversionMultiplier ],
        ns1:LengthTemperatureUnit,
        ns1:SICoherentDerivedUnit ;
    skos:altLabel "Metre Kelvin"@en ;
    skos:prefLabel "MetreKelvin"@en ;
    ns1:elucidation """`Meter Kelvin` is a unit for 'Length Temperature' expressed as m K.

-- QUDT"""@en ;
    ns1:qudtReference "http://qudt.org/vocab/unit/M-K"^^xsd:string ;
    ns1:ucumCode "m.K"^^xsd:string ;
    ns1:unitSymbol "m⋅K"^^xsd:string .

ns1:MetreKilogram a owl:Class ;
    rdfs:label "MetreKilogram"@en ;
    rdfs:comment "Kilogram metre."@en ;
    rdfs:isDefinedBy "http://qudt.org/2.1/vocab/unit"^^xsd:string ;
    rdfs:subClassOf [ a owl:Restriction ;
            owl:hasValue 0e+00 ;
            owl:onProperty ns1:hasSIConversionOffset ],
        [ a owl:Restriction ;
            owl:hasValue 1e+00 ;
            owl:onProperty ns1:hasSIConversionMultiplier ],
        ns1:LengthMassUnit,
        ns1:SICoherentDerivedUnit ;
    skos:prefLabel "MetreKilogram"@en ;
    ns1:elucidation "Kilogram metre."@en ;
    ns1:qudtReference "http://qudt.org/vocab/unit/M-KiloGM"^^xsd:string ;
    ns1:ucumCode "m.kg"^^xsd:string ;
    ns1:unitSymbol "m⋅kg"^^xsd:string .

ns1:MetrePerFarad a owl:Class ;
    rdfs:label "MetrePerFarad"@en ;
    rdfs:comment "Metre per Farad."@en ;
    rdfs:isDefinedBy "http://qudt.org/2.1/vocab/unit"^^xsd:string ;
    rdfs:subClassOf [ a owl:Restriction ;
            owl:hasValue 0e+00 ;
            owl:onProperty ns1:hasSIConversionOffset ],
        [ a owl:Restriction ;
            owl:hasValue 1e+00 ;
            owl:onProperty ns1:hasSIConversionMultiplier ],
        ns1:InversePermittivityUnit,
        ns1:SICoherentDerivedUnit ;
    skos:prefLabel "MetrePerFarad"@en ;
    ns1:elucidation "Metre per Farad."@en ;
    ns1:qudtReference "http://qudt.org/vocab/unit/M-PER-FARAD"^^xsd:string ;
    ns1:ucumCode "m.F-1"^^xsd:string ;
    ns1:unitSymbol "m/f"^^xsd:string .

ns1:MetrePerKelvin a owl:Class ;
    rdfs:label "MetrePerKelvin"@en ;
    rdfs:comment "Metre per Kelvin."@en ;
    rdfs:isDefinedBy "http://qudt.org/2.1/vocab/unit"^^xsd:string ;
    rdfs:subClassOf [ a owl:Restriction ;
            owl:hasValue 1e+00 ;
            owl:onProperty ns1:hasSIConversionMultiplier ],
        [ a owl:Restriction ;
            owl:hasValue 0e+00 ;
            owl:onProperty ns1:hasSIConversionOffset ],
        ns1:LengthPerTemperatureUnit,
        ns1:SICoherentDerivedUnit ;
    skos:prefLabel "MetrePerKelvin"@en ;
    ns1:elucidation "Metre per Kelvin."@en ;
    ns1:qudtReference "http://qudt.org/vocab/unit/M-PER-K"^^xsd:string ;
    ns1:ucumCode "m/K"^^xsd:string ;
    ns1:unitSymbol "m/k"^^xsd:string .

ns1:MetrePerSecond a owl:Class ;
    rdfs:label "MetrePerSecond"@en ;
    rdfs:comment """Metre per second is an SI derived unit of both speed (scalar) and velocity (vector quantity which specifies both magnitude and a specific direction), defined by distance in metres divided by time in seconds.
The official SI symbolic abbreviation is mu00b7s-1, or equivalently either m/s.

-- QUDT"""@en ;
    rdfs:subClassOf [ a owl:Restriction ;
            owl:hasValue 1e+00 ;
            owl:onProperty ns1:hasSIConversionMultiplier ],
        [ a owl:Restriction ;
            owl:hasValue 0e+00 ;
            owl:onProperty ns1:hasSIConversionOffset ],
        ns1:SICoherentDerivedUnit,
        ns1:SpeedUnit ;
    skos:prefLabel "MetrePerSecond"@en ;
    schema:unitCode "MTS"^^xsd:string ;
    ns1:elucidation """Metre per second is an SI derived unit of both speed (scalar) and velocity (vector quantity which specifies both magnitude and a specific direction), defined by distance in metres divided by time in seconds.
The official SI symbolic abbreviation is mu00b7s-1, or equivalently either m/s.

-- QUDT"""@en ;
    ns1:omReference "http://www.ontology-of-units-of-measure.org/resource/om-2/metrePerSecond-Time"^^xsd:string ;
    ns1:qudtReference "http://qudt.org/vocab/unit/M-PER-SEC"^^xsd:string ;
    ns1:ucumCode "m.s-1"^^xsd:string ;
    ns1:unitSymbol "m/s"^^xsd:string .

ns1:MetrePerSquareSecond a owl:Class ;
    rdfs:label "MetrePerSquareSecond"@en ;
    rdfs:comment """The `meter per Square second` is the unit of acceleration in the International System of Units (SI). As a derived unit it is composed from the SI base units of length, the metre, and the standard unit of time, the second. Its symbol is written in several forms as m/s², or m s⁻². As acceleration, the unit is interpreted physically as change in velocity or speed per time interval, that is, `metre per second per second`.

-- QUDT"""@en ;
    rdfs:isDefinedBy "http://qudt.org/2.1/vocab/unit"^^xsd:string ;
    rdfs:subClassOf [ a owl:Restriction ;
            owl:hasValue 0e+00 ;
            owl:onProperty ns1:hasSIConversionOffset ],
        [ a owl:Restriction ;
            owl:hasValue 1e+00 ;
            owl:onProperty ns1:hasSIConversionMultiplier ],
        ns1:AccelerationUnit,
        ns1:SICoherentDerivedUnit ;
    skos:altLabel "Metre per Square Second"@en ;
    skos:prefLabel "MetrePerSquareSecond"@en ;
    ns1:elucidation """The `meter per Square second` is the unit of acceleration in the International System of Units (SI). As a derived unit it is composed from the SI base units of length, the metre, and the standard unit of time, the second. Its symbol is written in several forms as m/s², or m s⁻². As acceleration, the unit is interpreted physically as change in velocity or speed per time interval, that is, `metre per second per second`.

-- QUDT"""@en ;
    ns1:qudtReference "http://qudt.org/vocab/unit/M-PER-SEC2"^^xsd:string ;
    ns1:ucumCode "m.s-2"^^xsd:string,
        "m/s2"^^xsd:string ;
    ns1:unitSymbol "m/s²"^^xsd:string .

ns1:MilliAmperePerGram a owl:Class ;
    rdfs:label "MilliAmperePerGram"@en ;
    rdfs:comment "a unit of electric current per mass"@en ;
    rdfs:subClassOf [ a owl:Restriction ;
            owl:hasValue 1e+00 ;
            owl:onProperty ns1:hasSIConversionMultiplier ],
        [ a owl:Restriction ;
            owl:hasValue 0e+00 ;
            owl:onProperty ns1:hasSIConversionOffset ],
        ns1:ElectricCurrentPerMassUnit,
        ns1:SICoherentDerivedUnit ;
    skos:prefLabel "MilliAmperePerGram"@en ;
    ns1:elucidation "a unit of electric current per mass"@en ;
    ns1:unitSymbol "mA/g"^^xsd:string .

ns1:MoleDegreeCelsius a owl:Class ;
    rdfs:label "MoleDegreeCelsius"@en ;
    rdfs:comment """`Mole Degree Celsius` is a C.G.S System unit for 'Temperature Amount Of Substance' expressed as mol-degC.

-- QUDT"""@en ;
    rdfs:isDefinedBy "http://qudt.org/2.1/vocab/unit"^^xsd:string ;
    rdfs:subClassOf ns1:AmountTemperatureUnit,
        ns1:NonPrefixedUnit,
        ns1:SICoherentDerivedUnit ;
    skos:altLabel "Mole Degree Celsius"@en ;
    skos:prefLabel "MoleDegreeCelsius"@en ;
    ns1:elucidation """`Mole Degree Celsius` is a C.G.S System unit for 'Temperature Amount Of Substance' expressed as mol-degC.

-- QUDT"""@en ;
    ns1:qudtReference "http://qudt.org/vocab/unit/MOL-DEG_C"^^xsd:string ;
    ns1:ucumCode "mol.Cel"^^xsd:string ;
    ns1:unitSymbol "mol⋅°C"^^xsd:string .

ns1:MoleFraction a owl:Class ;
    rdfs:label "MoleFraction"@en ;
    rdfs:comment "Number of one type of species divided by the number of all species."@en ;
    rdfs:isDefinedBy "http://qudt.org/2.1/vocab/unit"^^xsd:string ;
    rdfs:subClassOf [ a owl:Restriction ;
            owl:hasValue 1e+00 ;
            owl:onProperty ns1:hasSIConversionMultiplier ],
        [ a owl:Restriction ;
            owl:hasValue 0e+00 ;
            owl:onProperty ns1:hasSIConversionOffset ],
        ns1:AmountFractionUnit,
        ns1:SICoherentDerivedUnit ;
    skos:altLabel "AtomFraction"@en,
        "MolePerMole"@en,
        "Moles per mole"@en ;
    skos:prefLabel "MoleFraction"@en ;
    ns1:elucidation "Number of one type of species divided by the number of all species."@en ;
    ns1:qudtReference "http://qudt.org/vocab/unit/MOL-PER-MOL"^^xsd:string ;
    ns1:ucumCode "mol.mol-1"^^xsd:string ;
    ns1:unitSymbol "atom-fraction"^^xsd:string,
        "atom_fraction"^^xsd:string,
        "mol/mol"^^xsd:string,
        "mole-fraction"^^xsd:string,
        "mole_fraction"^^xsd:string .

ns1:MoleKelvin a owl:Class ;
    rdfs:label "MoleKelvin"@en ;
    rdfs:comment """Mole Kelvin is a unit for `Temperature Amount Of Substance` expressed as mol-K.

-- QUDT"""@en ;
    rdfs:isDefinedBy "http://qudt.org/2.1/vocab/unit"^^xsd:string ;
    rdfs:subClassOf [ a owl:Restriction ;
            owl:hasValue 0e+00 ;
            owl:onProperty ns1:hasSIConversionOffset ],
        [ a owl:Restriction ;
            owl:hasValue 1e+00 ;
            owl:onProperty ns1:hasSIConversionMultiplier ],
        ns1:AmountTemperatureUnit,
        ns1:SICoherentDerivedUnit ;
    skos:altLabel "Mole Kelvin"@en ;
    skos:prefLabel "MoleKelvin"@en ;
    ns1:elucidation """Mole Kelvin is a unit for `Temperature Amount Of Substance` expressed as mol-K.

-- QUDT"""@en ;
    ns1:qudtReference "http://qudt.org/vocab/unit/MOL-K"^^xsd:string ;
    ns1:ucumCode "mol.K"^^xsd:string ;
    ns1:unitSymbol "mol⋅K"^^xsd:string .

ns1:MolePerCubicMetre a owl:Class ;
    rdfs:label "MolePerCubicMetre"@en ;
    rdfs:comment """The SI derived unit for amount-of-substance concentration is the mole/cubic meter.

-- QUDT"""@en ;
    rdfs:isDefinedBy "http://qudt.org/2.1/vocab/unit"^^xsd:string ;
    rdfs:subClassOf [ a owl:Restriction ;
            owl:hasValue 1e+00 ;
            owl:onProperty ns1:hasSIConversionMultiplier ],
        [ a owl:Restriction ;
            owl:hasValue 0e+00 ;
            owl:onProperty ns1:hasSIConversionOffset ],
        ns1:AmountConcentrationUnit,
        ns1:SICoherentDerivedUnit ;
    skos:altLabel "Mole per Cubic Metre"@en ;
    skos:prefLabel "MolePerCubicMetre"@en ;
    ns1:elucidation """The SI derived unit for amount-of-substance concentration is the mole/cubic meter.

-- QUDT"""@en ;
    ns1:qudtReference "http://qudt.org/vocab/unit/MOL-PER-M3"^^xsd:string ;
    ns1:ucumCode "mol.m-3"^^xsd:string,
        "mol/m3"^^xsd:string ;
    ns1:unitSymbol "mol/m³"^^xsd:string .

ns1:MolePerCubicMetrePerSecond a owl:Class ;
    rdfs:label "MolePerCubicMetrePerSecond"^^xsd:string ;
    rdfs:comment """SI unit of quantity of matter per SI unit volume per SI unit of time.

-- QUDT"""@en ;
    rdfs:isDefinedBy "http://qudt.org/2.1/vocab/unit"^^xsd:string ;
    rdfs:subClassOf [ a owl:Restriction ;
            owl:hasValue 1e+00 ;
            owl:onProperty ns1:hasSIConversionMultiplier ],
        [ a owl:Restriction ;
            owl:hasValue 0e+00 ;
            owl:onProperty ns1:hasSIConversionOffset ],
        ns1:AmountPerVolumeTimeUnit,
        ns1:SICoherentDerivedUnit ;
    skos:altLabel "Moles per cubic metre per second"@en ;
    skos:prefLabel "MolePerCubicMetrePerSecond"^^xsd:string ;
    ns1:elucidation """SI unit of quantity of matter per SI unit volume per SI unit of time.

-- QUDT"""@en ;
    ns1:qudtReference "http://qudt.org/vocab/unit/MOL-PER-M3-SEC"^^xsd:string ;
    ns1:ucumCode "mol.m-3.s-1"^^xsd:string ;
    ns1:unitSymbol "mol/(m³⋅s)"^^xsd:string .

ns1:MolePerKilogram a owl:Class ;
    rdfs:label "MolePerKilogram"@en ;
    rdfs:comment """Mole Per Kilogram (mol/kg) is a unit of Molality

-- QUDT"""@en ;
    rdfs:isDefinedBy "http://qudt.org/2.1/vocab/unit"^^xsd:string ;
    rdfs:subClassOf [ a owl:Restriction ;
            owl:hasValue 1e+00 ;
            owl:onProperty ns1:hasSIConversionMultiplier ],
        [ a owl:Restriction ;
            owl:hasValue 0e+00 ;
            owl:onProperty ns1:hasSIConversionOffset ],
        ns1:AmountPerMassUnit,
        ns1:SICoherentDerivedUnit ;
    skos:altLabel "Mole per Kilogram"@en ;
    skos:prefLabel "MolePerKilogram"@en ;
    ns1:elucidation """Mole Per Kilogram (mol/kg) is a unit of Molality

-- QUDT"""@en ;
    ns1:qudtReference "http://qudt.org/vocab/unit/MOL-PER-KiloGM"^^xsd:string ;
    ns1:ucumCode "mol.kg-1"^^xsd:string,
        "mol/kg"^^xsd:string ;
    ns1:unitSymbol "mol/kg"^^xsd:string .

ns1:MolePerKilogramPascal a owl:Class ;
    rdfs:label "MolePerKilogramPascal"^^xsd:string ;
    rdfs:comment """Mole Per Kilogram Pascal (mol/kg-pa) is a unit of Molar Mass variation due to Pressure.

-- QUDT"""@en ;
    rdfs:isDefinedBy "http://qudt.org/2.1/vocab/unit"^^xsd:string ;
    rdfs:subClassOf [ a owl:Restriction ;
            owl:hasValue 0e+00 ;
            owl:onProperty ns1:hasSIConversionOffset ],
        [ a owl:Restriction ;
            owl:hasValue 1e+00 ;
            owl:onProperty ns1:hasSIConversionMultiplier ],
        ns1:AmountPerMassPressureUnit,
        ns1:SICoherentDerivedUnit ;
    skos:altLabel "Mole per Kilogram Pascal"@en ;
    skos:prefLabel "MolePerKilogramPascal"^^xsd:string ;
    ns1:elucidation """Mole Per Kilogram Pascal (mol/kg-pa) is a unit of Molar Mass variation due to Pressure.

-- QUDT"""@en ;
    ns1:qudtReference "http://qudt.org/vocab/unit/MOL-PER-KiloGM-PA"^^xsd:string ;
    ns1:ucumCode "mol.kg-1.Pa-1"^^xsd:string ;
    ns1:unitSymbol "mol/(kg⋅Pa)"^^xsd:string .

ns1:MolePerSecond a owl:Class ;
    rdfs:label "MolePerSecond"@en ;
    rdfs:comment """SI base unit mol divided by the SI base unit second

-- QUDT"""@en ;
    rdfs:isDefinedBy "http://qudt.org/2.1/vocab/unit"^^xsd:string ;
    rdfs:subClassOf [ a owl:Restriction ;
            owl:hasValue 1e+00 ;
            owl:onProperty ns1:hasSIConversionMultiplier ],
        [ a owl:Restriction ;
            owl:hasValue 0e+00 ;
            owl:onProperty ns1:hasSIConversionOffset ],
        ns1:CatalyticActivityUnit,
        ns1:SICoherentDerivedUnit ;
    skos:altLabel "Mole Per Second"@en ;
    skos:prefLabel "MolePerSecond"@en ;
    ns1:elucidation """SI base unit mol divided by the SI base unit second

-- QUDT"""@en ;
    ns1:qudtReference "http://qudt.org/vocab/unit/MOL-PER-SEC"^^xsd:string ;
    ns1:ucumCode "mol.s-1"^^xsd:string,
        "mol/s"^^xsd:string ;
    ns1:unitSymbol "mol/s"^^xsd:string .

ns1:MolePerSquareMetre a owl:Class ;
    rdfs:label "MolePerSquareMetre"^^xsd:string ;
    rdfs:comment """SI unit of quantity of matter per SI unit area.

-- QUDT"""@en ;
    rdfs:isDefinedBy "http://qudt.org/2.1/vocab/unit"^^xsd:string ;
    rdfs:subClassOf [ a owl:Restriction ;
            owl:hasValue 0e+00 ;
            owl:onProperty ns1:hasSIConversionOffset ],
        [ a owl:Restriction ;
            owl:hasValue 1e+00 ;
            owl:onProperty ns1:hasSIConversionMultiplier ],
        ns1:AmountPerAreaUnit,
        ns1:SICoherentDerivedUnit ;
    skos:altLabel "Moles per square metre"@en ;
    skos:prefLabel "MolePerSquareMetre"^^xsd:string ;
    ns1:elucidation """SI unit of quantity of matter per SI unit area.

-- QUDT"""@en ;
    ns1:qudtReference "http://qudt.org/vocab/unit/MOL-PER-M2"^^xsd:string ;
    ns1:ucumCode "mol.m-2"^^xsd:string ;
    ns1:unitSymbol "mol/m²"^^xsd:string .

ns1:MolePerSquareMetrePerSecond a owl:Class ;
    rdfs:label "MolePerSquareMetrePerSecond"^^xsd:string ;
    rdfs:comment """SI unit of quantity of matter per SI unit area per SI unit of time.

-- QUDT"""@en ;
    rdfs:isDefinedBy "http://qudt.org/2.1/vocab/unit"^^xsd:string ;
    rdfs:subClassOf [ a owl:Restriction ;
            owl:hasValue 1e+00 ;
            owl:onProperty ns1:hasSIConversionMultiplier ],
        [ a owl:Restriction ;
            owl:hasValue 0e+00 ;
            owl:onProperty ns1:hasSIConversionOffset ],
        ns1:AmountPerAreaTimeUnit,
        ns1:SICoherentDerivedUnit ;
    skos:altLabel "Moles per square metre per second"@en ;
    skos:prefLabel "MolePerSquareMetrePerSecond"^^xsd:string ;
    ns1:elucidation """SI unit of quantity of matter per SI unit area per SI unit of time.

-- QUDT"""@en ;
    ns1:qudtReference "http://qudt.org/vocab/unit/MOL-PER-M2-SEC"^^xsd:string ;
    ns1:ucumCode "mol.m-2.s-1"^^xsd:string ;
    ns1:unitSymbol "mol/(m²⋅s)"^^xsd:string .

ns1:MolePerSquareMetrePerSecondPerMetre a owl:Class ;
    rdfs:label "MolePerSquareMetrePerSecondPerMetre"^^xsd:string ;
    rdfs:comment "Moles per square metre and second and metre."@en ;
    rdfs:isDefinedBy "http://qudt.org/2.1/vocab/unit"^^xsd:string ;
    rdfs:subClassOf [ a owl:Restriction ;
            owl:hasValue 1e+00 ;
            owl:onProperty ns1:hasSIConversionMultiplier ],
        [ a owl:Restriction ;
            owl:hasValue 0e+00 ;
            owl:onProperty ns1:hasSIConversionOffset ],
        ns1:AmountPerVolumeTimeUnit,
        ns1:SICoherentDerivedUnit ;
    skos:prefLabel "MolePerSquareMetrePerSecondPerMetre"^^xsd:string ;
    ns1:elucidation "Moles per square metre and second and metre."@en ;
    ns1:qudtReference "http://qudt.org/vocab/unit/MOL-PER-M2-SEC-M"^^xsd:string ;
    ns1:ucumCode "mol.m-2.s-1.m-1"^^xsd:string ;
    ns1:unitSymbol "mol/(m²⋅s⋅m)"^^xsd:string .

ns1:MolePerSquareMetrePerSecondPerMetrePerSteradian a owl:Class ;
    rdfs:label "MolePerSquareMetrePerSecondPerMetrePerSteradian"^^xsd:string ;
    rdfs:comment "Moles per square metre per second per metre per steradian."@en ;
    rdfs:isDefinedBy "http://qudt.org/2.1/vocab/unit"^^xsd:string ;
    rdfs:subClassOf [ a owl:Restriction ;
            owl:hasValue 1e+00 ;
            owl:onProperty ns1:hasSIConversionMultiplier ],
        [ a owl:Restriction ;
            owl:hasValue 0e+00 ;
            owl:onProperty ns1:hasSIConversionOffset ],
        ns1:AmountPerVolumeTimeUnit,
        ns1:SICoherentDerivedUnit ;
    skos:prefLabel "MolePerSquareMetrePerSecondPerMetrePerSteradian"^^xsd:string ;
    ns1:elucidation "Moles per square metre per second per metre per steradian."@en ;
    ns1:qudtReference "http://qudt.org/vocab/unit/MOL-PER-M2-SEC-M-SR"^^xsd:string ;
    ns1:ucumCode "mol.m-2.s-1.m-1.sr-1"^^xsd:string ;
    ns1:unitSymbol "mol/(m²⋅s⋅m⋅sr)"^^xsd:string .

ns1:MolePerSquareMetrePerSecondPerSteradian a owl:Class ;
    rdfs:label "MolePerSquareMetrePerSecondPerSteradian"^^xsd:string ;
    rdfs:comment "Moles per square metre per second per steradian."@en ;
    rdfs:isDefinedBy "http://qudt.org/2.1/vocab/unit"^^xsd:string ;
    rdfs:subClassOf [ a owl:Restriction ;
            owl:hasValue 0e+00 ;
            owl:onProperty ns1:hasSIConversionOffset ],
        [ a owl:Restriction ;
            owl:hasValue 1e+00 ;
            owl:onProperty ns1:hasSIConversionMultiplier ],
        ns1:AmountPerAreaTimeUnit,
        ns1:SICoherentDerivedUnit ;
    skos:prefLabel "MolePerSquareMetrePerSecondPerSteradian"^^xsd:string ;
    ns1:elucidation "Moles per square metre per second per steradian."@en ;
    ns1:qudtReference "http://qudt.org/vocab/unit/MOL-PER-M2-SEC-SR"^^xsd:string ;
    ns1:ucumCode "mol.m-2.s-1.sr-1"^^xsd:string ;
    ns1:unitSymbol "mol/(m²⋅s⋅sr)"^^xsd:string .

ns1:NanoMeterPerMilliMeterMegaPascal a owl:Class ;
    rdfs:label "NanoMeterPerMilliMeterMegaPascal"^^xsd:string ;
    rdfs:subClassOf [ a owl:Restriction ;
            owl:hasValue 0e+00 ;
            owl:onProperty ns1:hasSIConversionOffset ],
        [ a owl:Restriction ;
            owl:hasValue 1e-12 ;
            owl:onProperty ns1:hasSIConversionMultiplier ],
        ns1:NanoPrefixedUnit,
        ns1:PerPressureUnit,
        ns1:PrefixedUnit,
        ns1:SINonCoherentUnit ;
    skos:altLabel "Nanometer Per Millimeter Megapascal"@en ;
    skos:prefLabel "NanoMeterPerMilliMeterMegaPascal"^^xsd:string ;
    ns1:qudtReference "http://qudt.org/vocab/unit/NanoM-PER-MilliM-MegaPA"^^xsd:string ;
    ns1:ucumCode "nm.mm-1.MPa-1"^^xsd:string ;
    ns1:unitSymbol "nm/(mm⋅MPa)"^^xsd:string .

ns1:NanoMolePerCubicCentiMetrePerHour a owl:Class ;
    rdfs:label "NanoMolePerCubicCentiMetrePerHour"^^xsd:string ;
    rdfs:subClassOf [ a owl:Restriction ;
            owl:hasValue 2.777778e-07 ;
            owl:onProperty ns1:hasSIConversionMultiplier ],
        [ a owl:Restriction ;
            owl:hasValue 0e+00 ;
            owl:onProperty ns1:hasSIConversionOffset ],
        ns1:AmountPerVolumeTimeUnit,
        ns1:NanoPrefixedUnit,
        ns1:PrefixedUnit,
        ns1:SINonCoherentUnit ;
    skos:altLabel "Nanomoles per cubic centimetre per hour"@en ;
    skos:prefLabel "NanoMolePerCubicCentiMetrePerHour"^^xsd:string ;
    ns1:qudtReference "http://qudt.org/vocab/unit/NanoMOL-PER-CentiM3-HR"^^xsd:string ;
    ns1:ucumCode "nmol.cm-3.h-1"^^xsd:string ;
    ns1:unitSymbol "nmol/(cm³⋅h)"^^xsd:string .

ns1:NanoMolePerGramPerSecond a owl:Class ;
    rdfs:label "NanoMolePerGramPerSecond"^^xsd:string ;
    rdfs:subClassOf [ a owl:Restriction ;
            owl:hasValue 0e+00 ;
            owl:onProperty ns1:hasSIConversionOffset ],
        [ a owl:Restriction ;
            owl:hasValue 1e-06 ;
            owl:onProperty ns1:hasSIConversionMultiplier ],
        ns1:AmountPerMassTimeUnit,
        ns1:NanoPrefixedUnit,
        ns1:PrefixedUnit,
        ns1:SINonCoherentUnit ;
    skos:altLabel "Nanomoles per gram per second"@en ;
    skos:prefLabel "NanoMolePerGramPerSecond"^^xsd:string ;
    ns1:qudtReference "http://qudt.org/vocab/unit/NanoMOL-PER-GM-SEC"^^xsd:string ;
    ns1:ucumCode "nmol.g-1.s-1"^^xsd:string ;
    ns1:unitSymbol "nmol/(g⋅s)"^^xsd:string .

ns1:NanoMolePerKilogram a owl:Class ;
    rdfs:label "NanoMolePerKilogram"^^xsd:string ;
    rdfs:subClassOf [ a owl:Restriction ;
            owl:hasValue 1e-09 ;
            owl:onProperty ns1:hasSIConversionMultiplier ],
        [ a owl:Restriction ;
            owl:hasValue 0e+00 ;
            owl:onProperty ns1:hasSIConversionOffset ],
        ns1:AmountPerMassUnit,
        ns1:NanoPrefixedUnit,
        ns1:PrefixedUnit,
        ns1:SINonCoherentUnit ;
    skos:altLabel "Nanomoles per kilogram"@en ;
    skos:prefLabel "NanoMolePerKilogram"^^xsd:string ;
    ns1:qudtReference "http://qudt.org/vocab/unit/NanoMOL-PER-KiloGM"^^xsd:string ;
    ns1:ucumCode "nmol.kg-1"^^xsd:string ;
    ns1:unitSymbol "nmol/kg"^^xsd:string .

ns1:NewtonMetre a owl:Class ;
    rdfs:label "NewtonMetre"@en ;
    rdfs:comment """"Torque" is the tendency of a force to cause a rotation, is the product of the force and the distance from the center of rotation to the point where the force is applied. Torque has the same units as work or energy, but it is a different physical concept. To stress the difference, scientists measure torque in newton meters rather than in joules, the SI unit of work. One newton meter is approximately 0.737562 pound foot.

-- QUDT"""@en,
        "Note that the physical dimension is the same as for Joule."@en ;
    rdfs:subClassOf [ a owl:Restriction ;
            owl:hasValue 1e+00 ;
            owl:onProperty ns1:hasSIConversionMultiplier ],
        [ a owl:Restriction ;
            owl:hasValue 0e+00 ;
            owl:onProperty ns1:hasSIConversionOffset ],
        ns1:EnergyUnit,
        ns1:SICoherentDerivedUnit ;
    skos:prefLabel "NewtonMetre"@en ;
    ns1:elucidation """"Torque" is the tendency of a force to cause a rotation, is the product of the force and the distance from the center of rotation to the point where the force is applied. Torque has the same units as work or energy, but it is a different physical concept. To stress the difference, scientists measure torque in newton meters rather than in joules, the SI unit of work. One newton meter is approximately 0.737562 pound foot.

-- QUDT"""@en ;
    ns1:omReference "http://www.ontology-of-units-of-measure.org/resource/om-2/newtonMetre"^^xsd:string ;
    ns1:qudtReference "http://qudt.org/vocab/unit/N-M"^^xsd:string ;
    ns1:unitSymbol "N⋅m"^^xsd:string .

ns1:NewtonMetrePerAmpere a owl:Class ;
    rdfs:label "NewtonMetrePerAmpere"@en ;
    rdfs:comment """product of the SI derived unit newton and the SI base unit metre divided by the SI base unit ampere

-- QUDT"""@en ;
    rdfs:isDefinedBy "http://qudt.org/2.1/vocab/unit"^^xsd:string ;
    rdfs:subClassOf [ a owl:Restriction ;
            owl:hasValue 0e+00 ;
            owl:onProperty ns1:hasSIConversionOffset ],
        [ a owl:Restriction ;
            owl:hasValue 1e+00 ;
            owl:onProperty ns1:hasSIConversionMultiplier ],
        ns1:MagneticFluxUnit,
        ns1:SICoherentDerivedUnit ;
    skos:altLabel "Newton Metre Per Ampere"@en ;
    skos:prefLabel "NewtonMetrePerAmpere"@en ;
    ns1:elucidation """product of the SI derived unit newton and the SI base unit metre divided by the SI base unit ampere

-- QUDT"""@en ;
    ns1:qudtReference "http://qudt.org/vocab/unit/N-M-PER-A"^^xsd:string ;
    ns1:ucumCode "N.m.A-1"^^xsd:string ;
    ns1:unitSymbol "N⋅m/A"^^xsd:string .

ns1:NewtonMetrePerKilogram a owl:Class ;
    rdfs:label "NewtonMetrePerKilogram"^^xsd:string ;
    rdfs:comment """product of the derived SI unit newton and the SI base unit metre divided by the SI base unit kilogram

-- QUDT"""@en ;
    rdfs:isDefinedBy "http://qudt.org/2.1/vocab/unit"^^xsd:string ;
    rdfs:subClassOf [ a owl:Restriction ;
            owl:hasValue 0e+00 ;
            owl:onProperty ns1:hasSIConversionOffset ],
        [ a owl:Restriction ;
            owl:hasValue 1e+00 ;
            owl:onProperty ns1:hasSIConversionMultiplier ],
        ns1:AbsorbedDoseUnit,
        ns1:SICoherentDerivedUnit ;
    skos:altLabel "Newton Metre Per Kilogram"@en ;
    skos:prefLabel "NewtonMetrePerKilogram"^^xsd:string ;
    ns1:elucidation """product of the derived SI unit newton and the SI base unit metre divided by the SI base unit kilogram

-- QUDT"""@en ;
    ns1:qudtReference "http://qudt.org/vocab/unit/N-M-PER-KiloGM"^^xsd:string ;
    ns1:ucumCode "N.m.kg-1"^^xsd:string ;
    ns1:unitSymbol "N⋅m/kg"^^xsd:string .

ns1:NewtonMetrePerMetre a owl:Class ;
    rdfs:label "NewtonMetrePerMetre"@en ;
    rdfs:comment """This is the SI unit for the rolling resistance, which is equivalent to drag force in newton

-- QUDT"""@en ;
    rdfs:isDefinedBy "http://qudt.org/2.1/vocab/unit"^^xsd:string ;
    rdfs:subClassOf [ a owl:Restriction ;
            owl:hasValue 1e+00 ;
            owl:onProperty ns1:hasSIConversionMultiplier ],
        [ a owl:Restriction ;
            owl:hasValue 0e+00 ;
            owl:onProperty ns1:hasSIConversionOffset ],
        ns1:ForceUnit,
        ns1:SICoherentDerivedUnit ;
    skos:altLabel "Newton metre per metre"@en ;
    skos:prefLabel "NewtonMetrePerMetre"@en ;
    ns1:elucidation """This is the SI unit for the rolling resistance, which is equivalent to drag force in newton

-- QUDT"""@en ;
    ns1:qudtReference "http://qudt.org/vocab/unit/N-M-PER-M"^^xsd:string ;
    ns1:unitSymbol "N⋅m/m"^^xsd:string .

ns1:NewtonMetrePerMetrePerRadian a owl:Class ;
    rdfs:label "NewtonMetrePerMetrePerRadian"^^xsd:string ;
    rdfs:comment "Newton metre per metre and radian."@en ;
    rdfs:isDefinedBy "http://qudt.org/2.1/vocab/unit"^^xsd:string ;
    rdfs:subClassOf [ a owl:Restriction ;
            owl:hasValue 1e+00 ;
            owl:onProperty ns1:hasSIConversionMultiplier ],
        [ a owl:Restriction ;
            owl:hasValue 0e+00 ;
            owl:onProperty ns1:hasSIConversionOffset ],
        ns1:ForceUnit,
        ns1:SICoherentDerivedUnit ;
    skos:prefLabel "NewtonMetrePerMetrePerRadian"^^xsd:string ;
    ns1:elucidation "Newton metre per metre and radian."@en ;
    ns1:qudtReference "http://qudt.org/vocab/unit/N-M-PER-M-RAD"^^xsd:string ;
    ns1:unitSymbol "N⋅m/(m⋅rad)"^^xsd:string .

ns1:NewtonMetrePerRadian a owl:Class ;
    rdfs:label "NewtonMetrePerRadian"@en ;
    rdfs:comment """Newton Meter per Radian is the SI unit for Torsion Constant

-- QUDT"""@en ;
    rdfs:isDefinedBy "http://qudt.org/2.1/vocab/unit"^^xsd:string ;
    rdfs:subClassOf [ a owl:Restriction ;
            owl:hasValue 0e+00 ;
            owl:onProperty ns1:hasSIConversionOffset ],
        [ a owl:Restriction ;
            owl:hasValue 1e+00 ;
            owl:onProperty ns1:hasSIConversionMultiplier ],
        ns1:EnergyUnit,
        ns1:SICoherentDerivedUnit ;
    skos:altLabel "Newton metre per radian"@en ;
    skos:prefLabel "NewtonMetrePerRadian"@en ;
    ns1:elucidation """Newton Meter per Radian is the SI unit for Torsion Constant

-- QUDT"""@en ;
    ns1:qudtReference "http://qudt.org/vocab/unit/N-M-PER-RAD"^^xsd:string ;
    ns1:unitSymbol "N⋅m/rad"^^xsd:string .

ns1:NewtonMetrePerSquareMetre a owl:Class ;
    rdfs:label "NewtonMetrePerSquareMetre"@en ;
    rdfs:comment """product of the SI derived unit newton and the SI base unit metre divided by the power of the SI base unit metre with the exponent 2

-- QUDT"""@en ;
    rdfs:isDefinedBy "http://qudt.org/2.1/vocab/unit"^^xsd:string ;
    rdfs:subClassOf [ a owl:Restriction ;
            owl:hasValue 1e+00 ;
            owl:onProperty ns1:hasSIConversionMultiplier ],
        [ a owl:Restriction ;
            owl:hasValue 0e+00 ;
            owl:onProperty ns1:hasSIConversionOffset ],
        ns1:ForcePerLengthUnit,
        ns1:SICoherentDerivedUnit ;
    skos:altLabel "Newton Metre Per Square Metre"@en ;
    skos:prefLabel "NewtonMetrePerSquareMetre"@en ;
    ns1:elucidation """product of the SI derived unit newton and the SI base unit metre divided by the power of the SI base unit metre with the exponent 2

-- QUDT"""@en ;
    ns1:qudtReference "http://qudt.org/vocab/unit/N-M-PER-M2"^^xsd:string ;
    ns1:ucumCode "N.m.m-2"^^xsd:string ;
    ns1:unitSymbol "N⋅m/m²"^^xsd:string .

ns1:NewtonMetreSecond a owl:Class ;
    rdfs:label "NewtonMetreSecond"@en ;
    rdfs:comment """The SI derived unit of angular momentum.

-- QUDT"""@en ;
    rdfs:isDefinedBy "http://qudt.org/2.1/vocab/unit"^^xsd:string ;
    rdfs:subClassOf [ a owl:Restriction ;
            owl:hasValue 0e+00 ;
            owl:onProperty ns1:hasSIConversionOffset ],
        [ a owl:Restriction ;
            owl:hasValue 1e+00 ;
            owl:onProperty ns1:hasSIConversionMultiplier ],
        ns1:AngularMomentumUnit,
        ns1:SICoherentDerivedUnit ;
    skos:altLabel "Newton Metre Second"@en ;
    skos:prefLabel "NewtonMetreSecond"@en ;
    ns1:elucidation """The SI derived unit of angular momentum.

-- QUDT"""@en ;
    ns1:qudtReference "http://qudt.org/vocab/unit/N-M-SEC"^^xsd:string ;
    ns1:ucumCode "N.m.s"^^xsd:string ;
    ns1:unitSymbol "N⋅m⋅s"^^xsd:string ;
    ns1:wikipediaReference "http://en.wikipedia.org/wiki/SI_derived_unit"^^xsd:string .

ns1:NewtonMetreSecondPerMetre a owl:Class ;
    rdfs:label "NewtonMetreSecondPerMetre"^^xsd:string ;
    rdfs:comment """Newton metre seconds measured per metre

-- QUDT"""@en ;
    rdfs:isDefinedBy "http://qudt.org/2.1/vocab/unit"^^xsd:string ;
    rdfs:subClassOf [ a owl:Restriction ;
            owl:hasValue 1e+00 ;
            owl:onProperty ns1:hasSIConversionMultiplier ],
        [ a owl:Restriction ;
            owl:hasValue 0e+00 ;
            owl:onProperty ns1:hasSIConversionOffset ],
        ns1:MomentumUnit,
        ns1:SICoherentDerivedUnit ;
    skos:altLabel "Newton metre seconds per metre"@en ;
    skos:prefLabel "NewtonMetreSecondPerMetre"^^xsd:string ;
    ns1:elucidation """Newton metre seconds measured per metre

-- QUDT"""@en ;
    ns1:qudtReference "http://qudt.org/vocab/unit/N-M-SEC-PER-M"^^xsd:string ;
    ns1:unitSymbol "N⋅m⋅s/m"^^xsd:string .

ns1:NewtonMetreSecondPerRadian a owl:Class ;
    rdfs:label "NewtonMetreSecondPerRadian"^^xsd:string ;
    rdfs:comment """Newton metre seconds measured per radian

-- QUDT"""@en ;
    rdfs:isDefinedBy "http://qudt.org/2.1/vocab/unit"^^xsd:string ;
    rdfs:subClassOf [ a owl:Restriction ;
            owl:hasValue 1e+00 ;
            owl:onProperty ns1:hasSIConversionMultiplier ],
        [ a owl:Restriction ;
            owl:hasValue 0e+00 ;
            owl:onProperty ns1:hasSIConversionOffset ],
        ns1:AngularMomentumUnit,
        ns1:SICoherentDerivedUnit ;
    skos:altLabel "Newton metre seconds per radian"@en ;
    skos:prefLabel "NewtonMetreSecondPerRadian"^^xsd:string ;
    ns1:elucidation """Newton metre seconds measured per radian

-- QUDT"""@en ;
    ns1:qudtReference "http://qudt.org/vocab/unit/N-M-SEC-PER-RAD"^^xsd:string ;
    ns1:unitSymbol "N⋅m⋅s/rad"^^xsd:string .

ns1:NewtonPerAmpere a owl:Class ;
    rdfs:label "NewtonPerAmpere"@en ;
    rdfs:comment """SI derived unit newton divided by the SI base unit ampere

-- QUDT"""@en ;
    rdfs:isDefinedBy "http://qudt.org/2.1/vocab/unit"^^xsd:string ;
    rdfs:subClassOf [ a owl:Restriction ;
            owl:hasValue 0e+00 ;
            owl:onProperty ns1:hasSIConversionOffset ],
        [ a owl:Restriction ;
            owl:hasValue 1e+00 ;
            owl:onProperty ns1:hasSIConversionMultiplier ],
        ns1:MagneticPotentialUnit,
        ns1:SICoherentDerivedUnit ;
    skos:altLabel "Newton Per Ampere"@en ;
    skos:prefLabel "NewtonPerAmpere"@en ;
    ns1:elucidation """SI derived unit newton divided by the SI base unit ampere

-- QUDT"""@en ;
    ns1:qudtReference "http://qudt.org/vocab/unit/N-PER-A"^^xsd:string ;
    ns1:ucumCode "N.A-1"^^xsd:string ;
    ns1:unitSymbol "N/A"^^xsd:string .

ns1:NewtonPerCoulomb a owl:Class ;
    rdfs:label "NewtonPerCoulomb"@en ;
    rdfs:comment """Newton Per Coulomb ( N/C) is a unit in the category of Electric field strength. It is also known as newtons/coulomb. Newton Per Coulomb ( N/C) has a dimension of MLT-3I-1 where M is mass, L is length, T is time, and I is electric current. It essentially the same as the corresponding standard SI unit V/m.

-- QUDT"""@en ;
    rdfs:isDefinedBy "http://qudt.org/2.1/vocab/unit"^^xsd:string ;
    rdfs:subClassOf [ a owl:Restriction ;
            owl:hasValue 1e+00 ;
            owl:onProperty ns1:hasSIConversionMultiplier ],
        [ a owl:Restriction ;
            owl:hasValue 0e+00 ;
            owl:onProperty ns1:hasSIConversionOffset ],
        ns1:ElectricFieldStrengthUnit,
        ns1:SICoherentDerivedUnit ;
    skos:altLabel "Newton per Coulomb"@en ;
    skos:prefLabel "NewtonPerCoulomb"@en ;
    ns1:elucidation """Newton Per Coulomb ( N/C) is a unit in the category of Electric field strength. It is also known as newtons/coulomb. Newton Per Coulomb ( N/C) has a dimension of MLT-3I-1 where M is mass, L is length, T is time, and I is electric current. It essentially the same as the corresponding standard SI unit V/m.

-- QUDT"""@en ;
    ns1:qudtReference "http://qudt.org/vocab/unit/N-PER-C"^^xsd:string ;
    ns1:ucumCode "N.C-1"^^xsd:string ;
    ns1:unitSymbol "N/C"^^xsd:string .

ns1:NewtonPerCubicMetre a owl:Class ;
    rdfs:label "NewtonPerCubicMetre"^^xsd:string ;
    rdfs:comment "Newton per cubic metre."@en ;
    rdfs:isDefinedBy "http://qudt.org/2.1/vocab/unit"^^xsd:string ;
    rdfs:subClassOf [ a owl:Restriction ;
            owl:hasValue 0e+00 ;
            owl:onProperty ns1:hasSIConversionOffset ],
        [ a owl:Restriction ;
            owl:hasValue 1e+00 ;
            owl:onProperty ns1:hasSIConversionMultiplier ],
        ns1:MassPerSquareLengthSquareTimeUnit,
        ns1:SICoherentDerivedUnit ;
    skos:prefLabel "NewtonPerCubicMetre"^^xsd:string ;
    ns1:elucidation "Newton per cubic metre."@en ;
    ns1:qudtReference "http://qudt.org/vocab/unit/N-PER-M3"^^xsd:string ;
    ns1:ucumCode "N.m-3"^^xsd:string ;
    ns1:unitSymbol "N/m³"^^xsd:string .

ns1:NewtonPerKilogram a owl:Class ;
    rdfs:label "NewtonPerKilogram"^^xsd:string ;
    rdfs:comment """Gravitational field strength at a point is the gravitational force per unit mass at that point. It is a vector and its S.I. unit is N kg-1.

-- QUDT"""@en ;
    rdfs:isDefinedBy "http://qudt.org/2.1/vocab/unit"^^xsd:string ;
    rdfs:subClassOf [ a owl:Restriction ;
            owl:hasValue 1e+00 ;
            owl:onProperty ns1:hasSIConversionMultiplier ],
        [ a owl:Restriction ;
            owl:hasValue 0e+00 ;
            owl:onProperty ns1:hasSIConversionOffset ],
        ns1:AccelerationUnit,
        ns1:SICoherentDerivedUnit ;
    skos:altLabel "Newton per Kilogram"@en ;
    skos:prefLabel "NewtonPerKilogram"^^xsd:string ;
    ns1:elucidation """Gravitational field strength at a point is the gravitational force per unit mass at that point. It is a vector and its S.I. unit is N kg-1.

-- QUDT"""@en ;
    ns1:qudtReference "http://qudt.org/vocab/unit/N-PER-KiloGM"^^xsd:string ;
    ns1:ucumCode "N.kg-1"^^xsd:string ;
    ns1:unitSymbol "N/kg"^^xsd:string .

ns1:NewtonPerMetre a owl:Class ;
    rdfs:label "NewtonPerMetre"@en ;
    rdfs:comment """Newton Per Meter (N/m) is a unit in the category of Surface tension. It is also known as newtons per meter, newton per metre, newtons per metre, newton/meter, newton/metre. This unit is commonly used in the SI unit system. Newton Per Meter (N/m) has a dimension of MT-2 where M is mass, and T is time. This unit is the standard SI unit in this category.

-- QUDT"""@en ;
    rdfs:isDefinedBy "http://qudt.org/2.1/vocab/unit"^^xsd:string ;
    rdfs:subClassOf [ a owl:Restriction ;
            owl:hasValue 1e+00 ;
            owl:onProperty ns1:hasSIConversionMultiplier ],
        [ a owl:Restriction ;
            owl:hasValue 0e+00 ;
            owl:onProperty ns1:hasSIConversionOffset ],
        ns1:ForcePerLengthUnit,
        ns1:SICoherentDerivedUnit ;
    skos:altLabel "Newton per Metre"@en ;
    skos:prefLabel "NewtonPerMetre"@en ;
    ns1:elucidation """Newton Per Meter (N/m) is a unit in the category of Surface tension. It is also known as newtons per meter, newton per metre, newtons per metre, newton/meter, newton/metre. This unit is commonly used in the SI unit system. Newton Per Meter (N/m) has a dimension of MT-2 where M is mass, and T is time. This unit is the standard SI unit in this category.

-- QUDT"""@en ;
    ns1:qudtReference "http://qudt.org/vocab/unit/N-PER-M"^^xsd:string ;
    ns1:ucumCode "N.m-1"^^xsd:string,
        "N/m"^^xsd:string ;
    ns1:unitSymbol "N/m"^^xsd:string .

ns1:NewtonPerRadian a owl:Class ;
    rdfs:label "NewtonPerRadian"@en ;
    rdfs:comment """A one-newton force applied for one angle/torsional torque

-- QUDT"""@en ;
    rdfs:isDefinedBy "http://qudt.org/2.1/vocab/unit"^^xsd:string ;
    rdfs:subClassOf [ a owl:Restriction ;
            owl:hasValue 0e+00 ;
            owl:onProperty ns1:hasSIConversionOffset ],
        [ a owl:Restriction ;
            owl:hasValue 1e+00 ;
            owl:onProperty ns1:hasSIConversionMultiplier ],
        ns1:ForceUnit,
        ns1:SICoherentDerivedUnit ;
    skos:altLabel "Newton per radian"@en ;
    skos:prefLabel "NewtonPerRadian"@en ;
    ns1:elucidation """A one-newton force applied for one angle/torsional torque

-- QUDT"""@en ;
    ns1:qudtReference "http://qudt.org/vocab/unit/N-PER-RAD"^^xsd:string ;
    ns1:unitSymbol "N/rad"^^xsd:string .

ns1:NewtonPerSquareMetre a owl:Class ;
    rdfs:label "NewtonPerSquareMetre"^^xsd:string ;
    rdfs:comment """The SI unit of pressure. The pascal is the standard pressure unit in the MKS metric system, equal to one newton per square meter or one "kilogram per meter per second per second." The unit is named for Blaise Pascal (1623-1662), French philosopher and mathematician, who was the first person to use a barometer to measure differences in altitude.

-- QUDT"""@en ;
    rdfs:isDefinedBy "http://qudt.org/2.1/vocab/unit"^^xsd:string ;
    rdfs:subClassOf [ a owl:Restriction ;
            owl:hasValue 0e+00 ;
            owl:onProperty ns1:hasSIConversionOffset ],
        [ a owl:Restriction ;
            owl:hasValue 1e+00 ;
            owl:onProperty ns1:hasSIConversionMultiplier ],
        ns1:PressureUnit,
        ns1:SICoherentDerivedUnit ;
    skos:altLabel "Newtons Per Square Metre"@en ;
    skos:prefLabel "NewtonPerSquareMetre"^^xsd:string ;
    ns1:elucidation """The SI unit of pressure. The pascal is the standard pressure unit in the MKS metric system, equal to one newton per square meter or one "kilogram per meter per second per second." The unit is named for Blaise Pascal (1623-1662), French philosopher and mathematician, who was the first person to use a barometer to measure differences in altitude.

-- QUDT"""@en ;
    ns1:qudtReference "http://qudt.org/vocab/unit/N-PER-M2"^^xsd:string ;
    ns1:ucumCode "N.m-2"^^xsd:string ;
    ns1:unitSymbol "N/m²"^^xsd:string ;
    ns1:wikipediaReference "http://en.wikipedia.org/wiki/Pascal?oldid=492989202"^^xsd:string .

ns1:NewtonSecond a owl:Class ;
    rdfs:label "NewtonSecond"@en ;
    rdfs:comment """product of the SI derived unit newton and the SI base unit second

-- QUDT"""@en ;
    rdfs:isDefinedBy "http://qudt.org/2.1/vocab/unit"^^xsd:string ;
    rdfs:subClassOf [ a owl:Restriction ;
            owl:hasValue 1e+00 ;
            owl:onProperty ns1:hasSIConversionMultiplier ],
        [ a owl:Restriction ;
            owl:hasValue 0e+00 ;
            owl:onProperty ns1:hasSIConversionOffset ],
        ns1:MomentumUnit,
        ns1:SICoherentDerivedUnit ;
    skos:altLabel "Newton Second"@en ;
    skos:prefLabel "NewtonSecond"@en ;
    ns1:elucidation """product of the SI derived unit newton and the SI base unit second

-- QUDT"""@en ;
    ns1:qudtReference "http://qudt.org/vocab/unit/N-SEC"^^xsd:string ;
    ns1:ucumCode "N.s"^^xsd:string ;
    ns1:unitSymbol "N⋅s"^^xsd:string .

ns1:NewtonSecondPerCubicMetre a owl:Class ;
    rdfs:label "NewtonSecondPerCubicMetre"@en ;
    rdfs:comment """The SI unit of specific acoustic impedance. When sound waves pass through any physical substance the pressure of the waves causes the particles of the substance to move. The sound specific impedance is the ratio between the sound pressure and the particle velocity it produces. The specific impedance is 1 N · s · m⁻³  if unit pressure produces unit velocity.

-- QUDT"""@en ;
    rdfs:isDefinedBy "http://qudt.org/2.1/vocab/unit"^^xsd:string ;
    rdfs:subClassOf [ a owl:Restriction ;
            owl:hasValue 1e+00 ;
            owl:onProperty ns1:hasSIConversionMultiplier ],
        [ a owl:Restriction ;
            owl:hasValue 0e+00 ;
            owl:onProperty ns1:hasSIConversionOffset ],
        ns1:MassFluxUnit,
        ns1:SICoherentDerivedUnit ;
    skos:altLabel "Newton second per Cubic Metre"@en ;
    skos:prefLabel "NewtonSecondPerCubicMetre"@en ;
    ns1:elucidation """The SI unit of specific acoustic impedance. When sound waves pass through any physical substance the pressure of the waves causes the particles of the substance to move. The sound specific impedance is the ratio between the sound pressure and the particle velocity it produces. The specific impedance is 1 N · s · m⁻³  if unit pressure produces unit velocity.

-- QUDT"""@en ;
    ns1:qudtReference "http://qudt.org/vocab/unit/N-SEC-PER-M3"^^xsd:string ;
    ns1:ucumCode "N.s.m-3"^^xsd:string ;
    ns1:unitSymbol "N⋅s/m³"^^xsd:string .

ns1:NewtonSecondPerMetre a owl:Class ;
    rdfs:label "NewtonSecondPerMetre"@en ;
    rdfs:comment """Newton second measured per metre

-- QUDT"""@en ;
    rdfs:isDefinedBy "http://qudt.org/2.1/vocab/unit"^^xsd:string ;
    rdfs:subClassOf [ a owl:Restriction ;
            owl:hasValue 1e+00 ;
            owl:onProperty ns1:hasSIConversionMultiplier ],
        [ a owl:Restriction ;
            owl:hasValue 0e+00 ;
            owl:onProperty ns1:hasSIConversionOffset ],
        ns1:MassPerTimeUnit,
        ns1:SICoherentDerivedUnit ;
    skos:altLabel "Newton Second per Metre"@en ;
    skos:prefLabel "NewtonSecondPerMetre"@en ;
    ns1:elucidation """Newton second measured per metre

-- QUDT"""@en ;
    ns1:qudtReference "http://qudt.org/vocab/unit/N-SEC-PER-M"^^xsd:string ;
    ns1:ucumCode "N.s.m-1"^^xsd:string ;
    ns1:unitSymbol "N⋅s/m"^^xsd:string .

ns1:NewtonSecondPerRadian a owl:Class ;
    rdfs:label "NewtonSecondPerRadian"^^xsd:string ;
    rdfs:comment """Newton seconds measured per radian

-- QUDT"""@en ;
    rdfs:isDefinedBy "http://qudt.org/2.1/vocab/unit"^^xsd:string ;
    rdfs:subClassOf [ a owl:Restriction ;
            owl:hasValue 0e+00 ;
            owl:onProperty ns1:hasSIConversionOffset ],
        [ a owl:Restriction ;
            owl:hasValue 1e+00 ;
            owl:onProperty ns1:hasSIConversionMultiplier ],
        ns1:MomentumUnit,
        ns1:SICoherentDerivedUnit ;
    skos:altLabel "Newton seconds per radian"@en ;
    skos:prefLabel "NewtonSecondPerRadian"^^xsd:string ;
    ns1:elucidation """Newton seconds measured per radian

-- QUDT"""@en ;
    ns1:qudtReference "http://qudt.org/vocab/unit/N-SEC-PER-RAD"^^xsd:string ;
    ns1:unitSymbol "N⋅s/rad"^^xsd:string .

ns1:NewtonSquareMetre a owl:Class ;
    rdfs:label "NewtonSquareMetre"@en ;
    rdfs:comment "Newton square metre."@en ;
    rdfs:isDefinedBy "http://qudt.org/2.1/vocab/unit"^^xsd:string ;
    rdfs:subClassOf [ a owl:Restriction ;
            owl:hasValue 1e+00 ;
            owl:onProperty ns1:hasSIConversionMultiplier ],
        [ a owl:Restriction ;
            owl:hasValue 0e+00 ;
            owl:onProperty ns1:hasSIConversionOffset ],
        ns1:ForceAreaUnit,
        ns1:SICoherentDerivedUnit ;
    skos:prefLabel "NewtonSquareMetre"@en ;
    ns1:elucidation "Newton square metre."@en ;
    ns1:qudtReference "http://qudt.org/vocab/unit/N-M2"^^xsd:string ;
    ns1:unitSymbol "N⋅m²"^^xsd:string .

ns1:NewtonSquareMetrePerAmpere a owl:Class ;
    rdfs:label "NewtonSquareMetrePerAmpere"@en ;
    rdfs:comment "Newton metre squared per Ampere."@en ;
    rdfs:isDefinedBy "http://qudt.org/2.1/vocab/unit"^^xsd:string ;
    rdfs:subClassOf [ a owl:Restriction ;
            owl:hasValue 0e+00 ;
            owl:onProperty ns1:hasSIConversionOffset ],
        [ a owl:Restriction ;
            owl:hasValue 1e+00 ;
            owl:onProperty ns1:hasSIConversionMultiplier ],
        ns1:NewtonSquareMetrePerAmpereUnit,
        ns1:SICoherentDerivedUnit ;
    skos:prefLabel "NewtonSquareMetrePerAmpere"@en ;
    ns1:elucidation "Newton metre squared per Ampere."@en ;
    ns1:qudtReference "http://qudt.org/vocab/unit/N-M2-PER-A"^^xsd:string ;
    ns1:ucumCode "N.m2.A-1"^^xsd:string,
        "N.m2/A"^^xsd:string ;
    ns1:unitSymbol "N⋅m²/A"^^xsd:string .

ns1:NewtonSquareMetrePerSquareKilogram a owl:Class ;
    rdfs:label "NewtonSquareMetrePerSquareKilogram"^^xsd:string ;
    rdfs:comment """unit of gravitational constant as product of the derived SI unit newton, the power of the SI base unit metre with the exponent 2 divided by the power of the SI base unit kilogram with the exponent 2

-- QUDT"""@en ;
    rdfs:isDefinedBy "http://qudt.org/2.1/vocab/unit"^^xsd:string ;
    rdfs:subClassOf [ a owl:Restriction ;
            owl:hasValue 1e+00 ;
            owl:onProperty ns1:hasSIConversionMultiplier ],
        [ a owl:Restriction ;
            owl:hasValue 0e+00 ;
            owl:onProperty ns1:hasSIConversionOffset ],
        ns1:NewtonianConstantOfGravityUnit,
        ns1:SICoherentDerivedUnit ;
    skos:altLabel "Newton Square Metre Per Square Kilogram"@en ;
    skos:prefLabel "NewtonSquareMetrePerSquareKilogram"^^xsd:string ;
    ns1:elucidation """unit of gravitational constant as product of the derived SI unit newton, the power of the SI base unit metre with the exponent 2 divided by the power of the SI base unit kilogram with the exponent 2

-- QUDT"""@en ;
    ns1:qudtReference "http://qudt.org/vocab/unit/N-M2-PER-KiloGM2"^^xsd:string ;
    ns1:ucumCode "N.m2.kg-2"^^xsd:string ;
    ns1:unitSymbol "N⋅m²/kg²"^^xsd:string .

ns1:OhmMetre a owl:Class ;
    rdfs:label "OhmMetre"@en ;
    rdfs:comment "Ohm metre."@en ;
    rdfs:isDefinedBy "http://qudt.org/2.1/vocab/unit"^^xsd:string ;
    rdfs:seeAlso "http://www.iso.org/iso/catalogue_detail?csnumber=31897"^^xsd:string ;
    rdfs:subClassOf [ a owl:Restriction ;
            owl:hasValue 1e+00 ;
            owl:onProperty ns1:hasSIConversionMultiplier ],
        [ a owl:Restriction ;
            owl:hasValue 0e+00 ;
            owl:onProperty ns1:hasSIConversionOffset ],
        ns1:ElectricResistivityUnit,
        ns1:SICoherentDerivedUnit ;
    skos:prefLabel "OhmMetre"@en ;
    ns1:elucidation "Ohm metre."@en ;
    ns1:qudtReference "http://qudt.org/vocab/unit/OHM-M"^^xsd:string ;
    ns1:ucumCode "Ohm.m"^^xsd:string ;
    ns1:unitSymbol "Ω⋅m"^^xsd:string .

ns1:OhmSquareMetrePerMetre a owl:Class ;
    rdfs:label "OhmSquareMetrePerMetre"@en ;
    rdfs:comment "Ohm square metre per metre."@en ;
    rdfs:isDefinedBy "http://qudt.org/2.1/vocab/unit"^^xsd:string ;
    rdfs:subClassOf [ a owl:Restriction ;
            owl:hasValue 1e+00 ;
            owl:onProperty ns1:hasSIConversionMultiplier ],
        [ a owl:Restriction ;
            owl:hasValue 0e+00 ;
            owl:onProperty ns1:hasSIConversionOffset ],
        ns1:ElectricResistivityUnit,
        ns1:SICoherentDerivedUnit ;
    skos:prefLabel "OhmSquareMetrePerMetre"@en ;
    ns1:elucidation "Ohm square metre per metre."@en ;
    ns1:qudtReference "http://qudt.org/vocab/unit/OHM-M2-PER-M"^^xsd:string ;
    ns1:ucumCode "Ohm2.m.m-1"^^xsd:string ;
    ns1:unitSymbol "Ω⋅m²/m"^^xsd:string .

ns1:PascalCubicMetrePerSecond a owl:Class ;
    rdfs:label "PascalCubicMetrePerSecond"@en ;
    rdfs:comment """product out of the SI derived unit pascal and the power of the SI base unit metre with the exponent 3 divided by the SI base unit second

-- QUDT"""@en ;
    rdfs:isDefinedBy "http://qudt.org/2.1/vocab/unit"^^xsd:string ;
    rdfs:subClassOf [ a owl:Restriction ;
            owl:hasValue 1e+00 ;
            owl:onProperty ns1:hasSIConversionMultiplier ],
        [ a owl:Restriction ;
            owl:hasValue 0e+00 ;
            owl:onProperty ns1:hasSIConversionOffset ],
        ns1:PowerUnit,
        ns1:SICoherentDerivedUnit ;
    skos:altLabel "Pascal Cubic Metre Per Second"@en ;
    skos:prefLabel "PascalCubicMetrePerSecond"@en ;
    ns1:elucidation """product out of the SI derived unit pascal and the power of the SI base unit metre with the exponent 3 divided by the SI base unit second

-- QUDT"""@en ;
    ns1:qudtReference "http://qudt.org/vocab/unit/PA-M3-PER-SEC"^^xsd:string ;
    ns1:ucumCode "Pa.m3.s-1"^^xsd:string ;
    ns1:unitSymbol "Pa⋅m³/s"^^xsd:string .

ns1:PascalMetre a owl:Class ;
    rdfs:label "PascalMetre"^^xsd:string ;
    rdfs:comment "Pascal metre."@en ;
    rdfs:isDefinedBy "http://qudt.org/2.1/vocab/unit"^^xsd:string ;
    rdfs:subClassOf [ a owl:Restriction ;
            owl:hasValue 1e+00 ;
            owl:onProperty ns1:hasSIConversionMultiplier ],
        [ a owl:Restriction ;
            owl:hasValue 0e+00 ;
            owl:onProperty ns1:hasSIConversionOffset ],
        ns1:ForcePerLengthUnit,
        ns1:SICoherentDerivedUnit ;
    skos:prefLabel "PascalMetre"^^xsd:string ;
    ns1:elucidation "Pascal metre."@en ;
    ns1:qudtReference "http://qudt.org/vocab/unit/PA-M"^^xsd:string ;
    ns1:ucumCode "Pa.m"^^xsd:string ;
    ns1:unitSymbol "Pa⋅m"^^xsd:string .

ns1:PascalMetrePerSecond a owl:Class ;
    rdfs:label "PascalMetrePerSecond"^^xsd:string ;
    rdfs:comment "Pascal metre per second."@en ;
    rdfs:isDefinedBy "http://qudt.org/2.1/vocab/unit"^^xsd:string ;
    rdfs:subClassOf [ a owl:Restriction ;
            owl:hasValue 1e+00 ;
            owl:onProperty ns1:hasSIConversionMultiplier ],
        [ a owl:Restriction ;
            owl:hasValue 0e+00 ;
            owl:onProperty ns1:hasSIConversionOffset ],
        ns1:PowerDensityUnit,
        ns1:SICoherentDerivedUnit ;
    skos:prefLabel "PascalMetrePerSecond"^^xsd:string ;
    ns1:elucidation "Pascal metre per second."@en ;
    ns1:qudtReference "http://qudt.org/vocab/unit/PA-M-PER-SEC"^^xsd:string ;
    ns1:ucumCode "Pa.m.s-1"^^xsd:string ;
    ns1:unitSymbol "Pa⋅m/s"^^xsd:string .

ns1:PascalMetrePerSquareSecond a owl:Class ;
    rdfs:label "PascalMetrePerSquareSecond"^^xsd:string ;
    rdfs:comment "Pascal metre per square second."@en ;
    rdfs:isDefinedBy "http://qudt.org/2.1/vocab/unit"^^xsd:string ;
    rdfs:subClassOf [ a owl:Restriction ;
            owl:hasValue 0e+00 ;
            owl:onProperty ns1:hasSIConversionOffset ],
        [ a owl:Restriction ;
            owl:hasValue 1e+00 ;
            owl:onProperty ns1:hasSIConversionMultiplier ],
        ns1:MassPerQuarticTimeUnit,
        ns1:SICoherentDerivedUnit ;
    skos:prefLabel "PascalMetrePerSquareSecond"^^xsd:string ;
    ns1:elucidation "Pascal metre per square second."@en ;
    ns1:qudtReference "http://qudt.org/vocab/unit/PA-M-PER-SEC2"^^xsd:string ;
    ns1:ucumCode "Pa.m.s-2"^^xsd:string ;
    ns1:unitSymbol "Pa⋅m/s²"^^xsd:string .

ns1:PascalPerKelvin a owl:Class ;
    rdfs:label "PascalPerKelvin"@en ;
    rdfs:comment "Pascal per Kelvin."@en ;
    rdfs:isDefinedBy "http://qudt.org/2.1/vocab/unit"^^xsd:string ;
    rdfs:subClassOf [ a owl:Restriction ;
            owl:hasValue 0e+00 ;
            owl:onProperty ns1:hasSIConversionOffset ],
        [ a owl:Restriction ;
            owl:hasValue 1e+00 ;
            owl:onProperty ns1:hasSIConversionMultiplier ],
        ns1:PressurePerTemperatureUnit,
        ns1:SICoherentDerivedUnit ;
    skos:prefLabel "PascalPerKelvin"@en ;
    ns1:elucidation "Pascal per Kelvin."@en ;
    ns1:qudtReference "http://qudt.org/vocab/unit/PA-PER-K"^^xsd:string ;
    ns1:ucumCode "Pa.K-1"^^xsd:string ;
    ns1:unitSymbol "P/K"^^xsd:string .

ns1:PascalPerMetre a owl:Class ;
    rdfs:label "PascalPerMetre"@en ;
    rdfs:comment """SI derived unit pascal divided by the SI base unit metre

-- QUDT"""@en ;
    rdfs:isDefinedBy "http://qudt.org/2.1/vocab/unit"^^xsd:string ;
    rdfs:subClassOf [ a owl:Restriction ;
            owl:hasValue 1e+00 ;
            owl:onProperty ns1:hasSIConversionMultiplier ],
        [ a owl:Restriction ;
            owl:hasValue 0e+00 ;
            owl:onProperty ns1:hasSIConversionOffset ],
        ns1:MassPerSquareLengthSquareTimeUnit,
        ns1:SICoherentDerivedUnit ;
    skos:altLabel "Pascal Per Metre"@en ;
    skos:prefLabel "PascalPerMetre"@en ;
    ns1:elucidation """SI derived unit pascal divided by the SI base unit metre

-- QUDT"""@en ;
    ns1:qudtReference "http://qudt.org/vocab/unit/PA-PER-M"^^xsd:string ;
    ns1:ucumCode "Pa.m-1"^^xsd:string,
        "Pa/m"^^xsd:string ;
    ns1:unitSymbol "Pa/m"^^xsd:string .

ns1:PascalPerSecond a owl:Class ;
    rdfs:label "PascalPerSecond"@en ;
    rdfs:comment """A rate of change of pressure measured as the number of Pascals in a period of one second.

-- QUDT"""@en ;
    rdfs:isDefinedBy "http://qudt.org/2.1/vocab/unit"^^xsd:string ;
    rdfs:subClassOf [ a owl:Restriction ;
            owl:hasValue 0e+00 ;
            owl:onProperty ns1:hasSIConversionOffset ],
        [ a owl:Restriction ;
            owl:hasValue 1e+00 ;
            owl:onProperty ns1:hasSIConversionMultiplier ],
        ns1:PressurePerTimeUnit,
        ns1:SICoherentDerivedUnit ;
    skos:altLabel "Pascal per Second"@en ;
    skos:prefLabel "PascalPerSecond"@en ;
    ns1:elucidation """A rate of change of pressure measured as the number of Pascals in a period of one second.

-- QUDT"""@en ;
    ns1:qudtReference "http://qudt.org/vocab/unit/PA-PER-SEC"^^xsd:string ;
    ns1:ucumCode "Pa.s-1"^^xsd:string,
        "Pa/s"^^xsd:string ;
    ns1:unitSymbol "P/s"^^xsd:string .

ns1:PascalSecond a owl:Class ;
    rdfs:label "PascalSecond"@en ;
    rdfs:comment """The SI unit of dynamic viscosity, equal to 10 poises or 1000 centipoises.

-- QUDT"""@en ;
    rdfs:isDefinedBy "http://qudt.org/2.1/vocab/unit"^^xsd:string ;
    rdfs:subClassOf [ a owl:Restriction ;
            owl:hasValue 1e+00 ;
            owl:onProperty ns1:hasSIConversionMultiplier ],
        [ a owl:Restriction ;
            owl:hasValue 0e+00 ;
            owl:onProperty ns1:hasSIConversionOffset ],
        ns1:MassPerLengthTimeUnit,
        ns1:SICoherentDerivedUnit ;
    skos:altLabel "Pascal Second"@en ;
    skos:prefLabel "PascalSecond"@en ;
    ns1:elucidation """The SI unit of dynamic viscosity, equal to 10 poises or 1000 centipoises.

-- QUDT"""@en ;
    ns1:qudtReference "http://qudt.org/vocab/unit/PA-SEC"^^xsd:string ;
    ns1:ucumCode "Pa.s"^^xsd:string ;
    ns1:unitSymbol "Pa⋅s"^^xsd:string .

ns1:PascalSecondPerCubicMetre a owl:Class ;
    rdfs:label "PascalSecondPerCubicMetre"@en ;
    rdfs:comment """`Pascal Second Per Cubic Meter` (Pa-s/m³) is a unit in the category of Acoustic impedance. It is also known as `pascal-second/cubic meter`. It has a dimension of ML⁻⁴T⁻¹ where M is mass, L is length, and T is time. This unit is the standard SI unit in this category.

-- QUDT"""@en ;
    rdfs:isDefinedBy "http://qudt.org/2.1/vocab/unit"^^xsd:string ;
    rdfs:seeAlso "http://www.efunda.com/glossary/units/units--acoustic_impedance--pascal_second_per_cubic_meter.cfm"^^xsd:string ;
    rdfs:subClassOf [ a owl:Restriction ;
            owl:hasValue 0e+00 ;
            owl:onProperty ns1:hasSIConversionOffset ],
        [ a owl:Restriction ;
            owl:hasValue 1e+00 ;
            owl:onProperty ns1:hasSIConversionMultiplier ],
        ns1:MassPerQuarticLengthTimeUnit,
        ns1:SICoherentDerivedUnit ;
    skos:altLabel "Pascal Second Per Cubic Metre"@en ;
    skos:prefLabel "PascalSecondPerCubicMetre"@en ;
    ns1:elucidation """`Pascal Second Per Cubic Meter` (Pa-s/m³) is a unit in the category of Acoustic impedance. It is also known as `pascal-second/cubic meter`. It has a dimension of ML⁻⁴T⁻¹ where M is mass, L is length, and T is time. This unit is the standard SI unit in this category.

-- QUDT"""@en ;
    ns1:qudtReference "http://qudt.org/vocab/unit/PA-SEC-PER-M3"^^xsd:string ;
    ns1:ucumCode "Pa.s.m-3"^^xsd:string ;
    ns1:unitSymbol "Pa⋅s/m³"^^xsd:string .

ns1:PascalSecondPerMetre a owl:Class ;
    rdfs:label "PascalSecondPerMetre"@en ;
    rdfs:comment """Pascal Second Per Meter (Pa-s/m) is a unit in the category of Specific acoustic impedance. It is also known as pascal-second/meter. Pascal Second Per Meter has a dimension of ML²T⁻¹ where M is mass, L is length, and T is time. It essentially the same as the corresponding standard SI unit kg/m2· s.

-- QUDT"""@en ;
    rdfs:isDefinedBy "http://qudt.org/2.1/vocab/unit"^^xsd:string ;
    rdfs:seeAlso "http://www.efunda.com/glossary/units/units--specific_acoustic_impedance--pascal_second_per_meter.cfm"^^xsd:string ;
    rdfs:subClassOf [ a owl:Restriction ;
            owl:hasValue 1e+00 ;
            owl:onProperty ns1:hasSIConversionMultiplier ],
        [ a owl:Restriction ;
            owl:hasValue 0e+00 ;
            owl:onProperty ns1:hasSIConversionOffset ],
        ns1:MassFluxUnit,
        ns1:SICoherentDerivedUnit ;
    skos:altLabel "Pascal Second Per Metre"@en ;
    skos:prefLabel "PascalSecondPerMetre"@en ;
    ns1:elucidation """Pascal Second Per Meter (Pa-s/m) is a unit in the category of Specific acoustic impedance. It is also known as pascal-second/meter. Pascal Second Per Meter has a dimension of ML²T⁻¹ where M is mass, L is length, and T is time. It essentially the same as the corresponding standard SI unit kg/m2· s.

-- QUDT"""@en ;
    ns1:qudtReference "http://qudt.org/vocab/unit/PA-SEC-PER-M"^^xsd:string ;
    ns1:ucumCode "Pa.s.m-1"^^xsd:string ;
    ns1:unitSymbol "Pa⋅s/m"^^xsd:string .

ns1:PerCubicMetre a owl:Class ;
    rdfs:label "PerCubicMetre"@en ;
    rdfs:comment """"Per Cubic Meter" is a denominator unit with dimensions /m³.

-- QUDT"""@en ;
    rdfs:isDefinedBy "http://qudt.org/2.1/vocab/unit"^^xsd:string ;
    rdfs:subClassOf [ a owl:Restriction ;
            owl:hasValue 0e+00 ;
            owl:onProperty ns1:hasSIConversionOffset ],
        [ a owl:Restriction ;
            owl:hasValue 1e+00 ;
            owl:onProperty ns1:hasSIConversionMultiplier ],
        ns1:PerVolumeUnit,
        ns1:SICoherentDerivedUnit ;
    skos:altLabel "Reciprocal Cubic Metre"@en ;
    skos:prefLabel "PerCubicMetre"@en ;
    ns1:elucidation """"Per Cubic Meter" is a denominator unit with dimensions /m³.

-- QUDT"""@en ;
    ns1:qudtReference "http://qudt.org/vocab/unit/PER-M3"^^xsd:string ;
    ns1:ucumCode "/m3"^^xsd:string,
        "m-3"^^xsd:string ;
    ns1:unitSymbol "/m³"^^xsd:string .

ns1:PerCubicMetreSecond a owl:Class ;
    rdfs:label "PerCubicMetreSecond"@en ;
    rdfs:comment "Per cubic metre and second."@en ;
    rdfs:isDefinedBy "http://qudt.org/2.1/vocab/unit"^^xsd:string ;
    rdfs:subClassOf [ a owl:Restriction ;
            owl:hasValue 1e+00 ;
            owl:onProperty ns1:hasSIConversionMultiplier ],
        [ a owl:Restriction ;
            owl:hasValue 0e+00 ;
            owl:onProperty ns1:hasSIConversionOffset ],
        ns1:FrequencyPerVolumeUnit,
        ns1:SICoherentDerivedUnit ;
    skos:prefLabel "PerCubicMetreSecond"@en ;
    ns1:elucidation "Per cubic metre and second."@en ;
    ns1:qudtReference "http://qudt.org/vocab/unit/PER-M3-SEC"^^xsd:string ;
    ns1:ucumCode "m-3.s-1"^^xsd:string ;
    ns1:unitSymbol "/(m³⋅s)"^^xsd:string .

ns1:PerHenry a owl:Class ;
    rdfs:label "PerHenry"@en ;
    rdfs:comment "Reciprocal Henry."@en ;
    rdfs:isDefinedBy "http://qudt.org/2.1/vocab/unit"^^xsd:string ;
    rdfs:subClassOf [ a owl:Restriction ;
            owl:hasValue 1e+00 ;
            owl:onProperty ns1:hasSIConversionMultiplier ],
        [ a owl:Restriction ;
            owl:hasValue 0e+00 ;
            owl:onProperty ns1:hasSIConversionOffset ],
        ns1:MagneticReluctanceUnit,
        ns1:SICoherentDerivedUnit ;
    skos:altLabel "ReciprocalHenry"@en ;
    skos:prefLabel "PerHenry"@en ;
    ns1:elucidation "Reciprocal Henry."@en ;
    ns1:qudtReference "http://qudt.org/vocab/unit/PER-H"^^xsd:string ;
    ns1:ucumCode "H-1"^^xsd:string ;
    ns1:unitSymbol "/H"^^xsd:string .

ns1:PerJouleCubicMetre a owl:Class ;
    rdfs:label "PerJouleCubicMetre"@en ;
    rdfs:comment "Per Joule cubic metre."@en ;
    rdfs:isDefinedBy "http://qudt.org/2.1/vocab/unit"^^xsd:string ;
    rdfs:seeAlso "http://www.iso.org/iso/catalogue_detail?csnumber=31897"^^xsd:string ;
    rdfs:subClassOf [ a owl:Restriction ;
            owl:hasValue 1e+00 ;
            owl:onProperty ns1:hasSIConversionMultiplier ],
        [ a owl:Restriction ;
            owl:hasValue 0e+00 ;
            owl:onProperty ns1:hasSIConversionOffset ],
        ns1:PerPressureUnit,
        ns1:SICoherentDerivedUnit ;
    skos:prefLabel "PerJouleCubicMetre"@en ;
    ns1:elucidation "Per Joule cubic metre."@en ;
    ns1:qudtReference "http://qudt.org/vocab/unit/PER-J-M3"^^xsd:string ;
    ns1:ucumCode "J-1.m-3"^^xsd:string ;
    ns1:unitSymbol "/(J⋅m³)"^^xsd:string .

ns1:PerKelvin a owl:Class ;
    rdfs:label "PerKelvin"@en ;
    rdfs:comment """Per Kelvin Unit is a denominator unit with dimensions /K.

-- QUDT"""@en ;
    rdfs:isDefinedBy "http://qudt.org/2.1/vocab/unit"^^xsd:string ;
    rdfs:subClassOf [ a owl:Restriction ;
            owl:hasValue 1e+00 ;
            owl:onProperty ns1:hasSIConversionMultiplier ],
        [ a owl:Restriction ;
            owl:hasValue 0e+00 ;
            owl:onProperty ns1:hasSIConversionOffset ],
        ns1:PerTemperatureUnit,
        ns1:SICoherentDerivedUnit ;
    skos:altLabel "Reciprocal Kelvin"@en ;
    skos:prefLabel "PerKelvin"@en ;
    ns1:elucidation """Per Kelvin Unit is a denominator unit with dimensions /K.

-- QUDT"""@en ;
    ns1:qudtReference "http://qudt.org/vocab/unit/PER-K"^^xsd:string ;
    ns1:ucumCode "K-1"^^xsd:string ;
    ns1:unitSymbol "/K"^^xsd:string .

ns1:PerMetre a owl:Class ;
    rdfs:label "PerMetre"@en ;
    rdfs:comment """Per Meter Unit is a denominator unit with dimensions /m.

-- QUDT"""@en ;
    rdfs:isDefinedBy "http://qudt.org/2.1/vocab/unit"^^xsd:string ;
    rdfs:subClassOf [ a owl:Restriction ;
            owl:hasValue 1e+00 ;
            owl:onProperty ns1:hasSIConversionMultiplier ],
        [ a owl:Restriction ;
            owl:hasValue 0e+00 ;
            owl:onProperty ns1:hasSIConversionOffset ],
        ns1:ReciprocalLengthUnit,
        ns1:SICoherentDerivedUnit ;
    skos:altLabel "Reciprocal metre"@en ;
    skos:prefLabel "PerMetre"@en ;
    ns1:elucidation """Per Meter Unit is a denominator unit with dimensions /m.

-- QUDT"""@en ;
    ns1:qudtReference "http://qudt.org/vocab/unit/PER-M"^^xsd:string ;
    ns1:ucumCode "/m"^^xsd:string,
        "m-1"^^xsd:string ;
    ns1:unitSymbol "/m"^^xsd:string .

ns1:PerMetreKelvin a owl:Class ;
    rdfs:label "PerMetreKelvin"@en ;
    rdfs:comment """Per Meter Kelvin Unit is a denominator unit with dimensions /m.k.

-- QUDT"""@en ;
    rdfs:isDefinedBy "http://qudt.org/2.1/vocab/unit"^^xsd:string ;
    rdfs:subClassOf [ a owl:Restriction ;
            owl:hasValue 0e+00 ;
            owl:onProperty ns1:hasSIConversionOffset ],
        [ a owl:Restriction ;
            owl:hasValue 1e+00 ;
            owl:onProperty ns1:hasSIConversionMultiplier ],
        ns1:PerLengthTemperatureUnit,
        ns1:SICoherentDerivedUnit ;
    skos:altLabel "ReciprocalMetreKelvin"@en ;
    skos:prefLabel "PerMetreKelvin"@en ;
    ns1:elucidation """Per Meter Kelvin Unit is a denominator unit with dimensions /m.k.

-- QUDT"""@en ;
    ns1:qudtReference "http://qudt.org/vocab/unit/PER-M-K"^^xsd:string ;
    ns1:ucumCode "m-1.K-1"^^xsd:string ;
    ns1:unitSymbol "/(m⋅K)"^^xsd:string .

ns1:PerMetreSecond a owl:Class ;
    rdfs:label "PerMetreSecond"@en ;
    rdfs:comment "Per metre and second."@en ;
    rdfs:isDefinedBy "http://qudt.org/2.1/vocab/unit"^^xsd:string ;
    rdfs:subClassOf [ a owl:Restriction ;
            owl:hasValue 0e+00 ;
            owl:onProperty ns1:hasSIConversionOffset ],
        [ a owl:Restriction ;
            owl:hasValue 1e+00 ;
            owl:onProperty ns1:hasSIConversionMultiplier ],
        ns1:PerLengthTimeUnit,
        ns1:SICoherentDerivedUnit ;
    skos:altLabel "ReciprocalMetreSecond"@en ;
    skos:prefLabel "PerMetreSecond"@en ;
    ns1:elucidation "Per metre and second."@en ;
    ns1:qudtReference "http://qudt.org/vocab/unit/PER-M-SEC"^^xsd:string ;
    ns1:ucumCode "m-1.s-1"^^xsd:string ;
    ns1:unitSymbol "/(m⋅s)"^^xsd:string .

ns1:PerMetreSteradian a owl:Class ;
    rdfs:label "PerMetreSteradian"@en ;
    rdfs:comment "Per metre and steradian."@en ;
    rdfs:isDefinedBy "http://qudt.org/2.1/vocab/unit"^^xsd:string ;
    rdfs:subClassOf [ a owl:Restriction ;
            owl:hasValue 0e+00 ;
            owl:onProperty ns1:hasSIConversionOffset ],
        [ a owl:Restriction ;
            owl:hasValue 1e+00 ;
            owl:onProperty ns1:hasSIConversionMultiplier ],
        ns1:ReciprocalLengthUnit,
        ns1:SICoherentDerivedUnit ;
    skos:altLabel "ReciprocalMetreSteradian"@en ;
    skos:prefLabel "PerMetreSteradian"@en ;
    ns1:elucidation "Per metre and steradian."@en ;
    ns1:qudtReference "http://qudt.org/vocab/unit/PER-M-SR"^^xsd:string ;
    ns1:ucumCode "m-1.sr-1"^^xsd:string ;
    ns1:unitSymbol "/(m⋅sr)"^^xsd:string .

ns1:PerMole a owl:Class ;
    rdfs:label "PerMole"@en ;
    rdfs:comment """Per Mole Unit is a denominator unit with dimensions mol⁻¹.

-- QUDT"""@en ;
    rdfs:isDefinedBy "http://qudt.org/2.1/vocab/unit"^^xsd:string ;
    rdfs:subClassOf [ a owl:Restriction ;
            owl:hasValue 0e+00 ;
            owl:onProperty ns1:hasSIConversionOffset ],
        [ a owl:Restriction ;
            owl:hasValue 1e+00 ;
            owl:onProperty ns1:hasSIConversionMultiplier ],
        ns1:PerAmountUnit,
        ns1:SICoherentDerivedUnit ;
    skos:altLabel "ReciprocalMole"@en ;
    skos:prefLabel "PerMole"@en ;
    ns1:elucidation """Per Mole Unit is a denominator unit with dimensions mol⁻¹.

-- QUDT"""@en ;
    ns1:qudtReference "http://qudt.org/vocab/unit/PER-MOL"^^xsd:string ;
    ns1:ucumCode "mol-1"^^xsd:string ;
    ns1:unitSymbol "/mol"^^xsd:string .

ns1:PerPascal a owl:Class ;
    rdfs:label "PerPascal"@en ;
    rdfs:comment "Per Pascal."@en ;
    rdfs:isDefinedBy "http://qudt.org/2.1/vocab/unit"^^xsd:string ;
    rdfs:subClassOf [ a owl:Restriction ;
            owl:hasValue 0e+00 ;
            owl:onProperty ns1:hasSIConversionOffset ],
        [ a owl:Restriction ;
            owl:hasValue 1e+00 ;
            owl:onProperty ns1:hasSIConversionMultiplier ],
        ns1:PerPressureUnit,
        ns1:SICoherentDerivedUnit ;
    skos:altLabel "ReciprocalPascal"@en ;
    skos:prefLabel "PerPascal"@en ;
    ns1:elucidation "Per Pascal."@en ;
    ns1:qudtReference "http://qudt.org/vocab/unit/PER-PA"^^xsd:string ;
    ns1:ucumCode "Pa-1"^^xsd:string ;
    ns1:unitSymbol "/Pa"^^xsd:string ;
    ns1:wikipediaReference "http://en.wikipedia.org/wiki/Pascal?oldid=492989202"^^xsd:string .

ns1:PerPascalSecond a owl:Class ;
    rdfs:label "PerPascalSecond"@en ;
    rdfs:comment "Per Pascal and Second."@en ;
    rdfs:isDefinedBy "http://qudt.org/2.1/vocab/unit"^^xsd:string ;
    rdfs:subClassOf [ a owl:Restriction ;
            owl:hasValue 0e+00 ;
            owl:onProperty ns1:hasSIConversionOffset ],
        [ a owl:Restriction ;
            owl:hasValue 1e+00 ;
            owl:onProperty ns1:hasSIConversionMultiplier ],
        ns1:LengthTimePerMassUnit,
        ns1:SICoherentDerivedUnit ;
    skos:altLabel "PerPascalSecond"@en ;
    skos:prefLabel "PerPascalSecond"@en ;
    ns1:elucidation "Per Pascal and Second."@en ;
    ns1:qudtReference "http://qudt.org/vocab/unit/PER-PA-SEC"^^xsd:string ;
    ns1:ucumCode "Pa-1.s-1"^^xsd:string ;
    ns1:unitSymbol "/(Pa⋅s)"^^xsd:string .

ns1:PerSecond a owl:Class ;
    rdfs:label "PerSecond"@en ;
    rdfs:comment """A reciprical unit of time for `reciprocal second` or `inverse second`. The `Per Second` is a unit of rate.

-- QUDT"""@en ;
    rdfs:isDefinedBy "http://qudt.org/2.1/vocab/unit"^^xsd:string ;
    rdfs:subClassOf [ a owl:Restriction ;
            owl:hasValue 1e+00 ;
            owl:onProperty ns1:hasSIConversionMultiplier ],
        [ a owl:Restriction ;
            owl:hasValue 0e+00 ;
            owl:onProperty ns1:hasSIConversionOffset ],
        ns1:FrequencyUnit,
        ns1:SICoherentDerivedUnit ;
    skos:altLabel "ReciprocalSecond"@en ;
    skos:prefLabel "PerSecond"@en ;
    ns1:elucidation """A reciprical unit of time for `reciprocal second` or `inverse second`. The `Per Second` is a unit of rate.

-- QUDT"""@en ;
    ns1:qudtReference "http://qudt.org/vocab/unit/PER-SEC"^^xsd:string ;
    ns1:ucumCode "/s"^^xsd:string,
        "s-1"^^xsd:string ;
    ns1:unitSymbol "/s"^^xsd:string .

ns1:PerSecondSquareMetre a owl:Class ;
    rdfs:label "PerSecondSquareMetre"@en ;
    rdfs:comment """`Per Second Square Meter` is a measure of flux with dimensions /sec-m².

-- QUDT"""@en ;
    rdfs:isDefinedBy "http://qudt.org/2.1/vocab/unit"^^xsd:string ;
    rdfs:subClassOf [ a owl:Restriction ;
            owl:hasValue 0e+00 ;
            owl:onProperty ns1:hasSIConversionOffset ],
        [ a owl:Restriction ;
            owl:hasValue 1e+00 ;
            owl:onProperty ns1:hasSIConversionMultiplier ],
        ns1:PerAreaTimeUnit,
        ns1:SICoherentDerivedUnit ;
    skos:altLabel "ReciprocalSecondSquareMetre"@en ;
    skos:prefLabel "PerSecondSquareMetre"@en ;
    ns1:elucidation """`Per Second Square Meter` is a measure of flux with dimensions /sec-m².

-- QUDT"""@en ;
    ns1:qudtReference "http://qudt.org/vocab/unit/PER-SEC-M2"^^xsd:string ;
    ns1:ucumCode "/(s1.m2)"^^xsd:string,
        "s-1.m-2"^^xsd:string ;
    ns1:unitSymbol "/s⋅m²"^^xsd:string .

ns1:PerSecondSquareMetreSteradian a owl:Class ;
    rdfs:label "PerSecondSquareMetreSteradian"@en ;
    rdfs:comment """Per Second Square Meter Steradian is a denominator unit with dimensions /sec-m²-sr.

-- QUDT"""@en ;
    rdfs:isDefinedBy "http://qudt.org/2.1/vocab/unit"^^xsd:string ;
    rdfs:subClassOf [ a owl:Restriction ;
            owl:hasValue 1e+00 ;
            owl:onProperty ns1:hasSIConversionMultiplier ],
        [ a owl:Restriction ;
            owl:hasValue 0e+00 ;
            owl:onProperty ns1:hasSIConversionOffset ],
        ns1:PerAreaTimeUnit,
        ns1:SICoherentDerivedUnit ;
    skos:altLabel "ReciprocalSecondSquareMetreSteradian"@en ;
    skos:prefLabel "PerSecondSquareMetreSteradian"@en ;
    ns1:elucidation """Per Second Square Meter Steradian is a denominator unit with dimensions /sec-m²-sr.

-- QUDT"""@en ;
    ns1:qudtReference "http://qudt.org/vocab/unit/PER-SEC-M2-SR"^^xsd:string ;
    ns1:ucumCode "/(s.m2.sr)"^^xsd:string,
        "s-1.m-2.sr-1"^^xsd:string ;
    ns1:unitSymbol "/s⋅m²⋅sr"^^xsd:string .

ns1:PerSecondSteradian a owl:Class ;
    rdfs:label "PerSecondSteradian"@en ;
    rdfs:comment """Per Second Steradian Unit is a denominator unit with dimensions /sec-sr.

-- QUDT"""@en ;
    rdfs:isDefinedBy "http://qudt.org/2.1/vocab/unit"^^xsd:string ;
    rdfs:subClassOf [ a owl:Restriction ;
            owl:hasValue 0e+00 ;
            owl:onProperty ns1:hasSIConversionOffset ],
        [ a owl:Restriction ;
            owl:hasValue 1e+00 ;
            owl:onProperty ns1:hasSIConversionMultiplier ],
        ns1:FrequencyUnit,
        ns1:SICoherentDerivedUnit ;
    skos:altLabel "ReciprocalSecondSteradian"@en ;
    skos:prefLabel "PerSecondSteradian"@en ;
    ns1:elucidation """Per Second Steradian Unit is a denominator unit with dimensions /sec-sr.

-- QUDT"""@en ;
    ns1:qudtReference "http://qudt.org/vocab/unit/PER-SEC-SR"^^xsd:string ;
    ns1:ucumCode "/(s.sr)"^^xsd:string,
        "s-1.sr-1"^^xsd:string ;
    ns1:unitSymbol "/s⋅sr"^^xsd:string .

ns1:PerSquareJoule a owl:Class ;
    rdfs:label "PerSquareJoule"@en ;
    rdfs:comment """Per Square Joule is a denominator unit with dimensions /eV².

-- QUDT"""@en ;
    rdfs:isDefinedBy "http://qudt.org/2.1/vocab/unit"^^xsd:string ;
    rdfs:subClassOf [ a owl:Restriction ;
            owl:hasValue 0e+00 ;
            owl:onProperty ns1:hasSIConversionOffset ],
        [ a owl:Restriction ;
            owl:hasValue 1e+00 ;
            owl:onProperty ns1:hasSIConversionMultiplier ],
        ns1:ReciprocalSquareEnergyUnit,
        ns1:SICoherentDerivedUnit ;
    skos:altLabel "ReciprocalSquareJoule"@en ;
    skos:prefLabel "PerSquareJoule"@en ;
    ns1:elucidation """Per Square Joule is a denominator unit with dimensions /eV².

-- QUDT"""@en ;
    ns1:qudtReference "http://qudt.org/vocab/unit/PER-J2"^^xsd:string ;
    ns1:ucumCode "J-2"^^xsd:string ;
    ns1:unitSymbol "/J²"^^xsd:string .

ns1:PerSquareKilogram a owl:Class ;
    rdfs:label "PerSquareKilogram"^^xsd:string ;
    rdfs:comment """Per Square Kilogram is a denominator unit with dimensions /kg².

-- QUDT"""@en ;
    rdfs:isDefinedBy "http://qudt.org/2.1/vocab/unit"^^xsd:string ;
    rdfs:subClassOf [ a owl:Restriction ;
            owl:hasValue 0e+00 ;
            owl:onProperty ns1:hasSIConversionOffset ],
        [ a owl:Restriction ;
            owl:hasValue 1e+00 ;
            owl:onProperty ns1:hasSIConversionMultiplier ],
        ns1:InverseSquareMassUnit,
        ns1:SICoherentDerivedUnit ;
    skos:altLabel "ReciprocalSquareKilogram"@en ;
    skos:prefLabel "PerSquareKilogram"^^xsd:string ;
    ns1:elucidation """Per Square Kilogram is a denominator unit with dimensions /kg².

-- QUDT"""@en ;
    ns1:qudtReference "http://qudt.org/vocab/unit/PER-KiloGM2"^^xsd:string ;
    ns1:ucumCode "kg-2"^^xsd:string ;
    ns1:unitSymbol "/kg²"^^xsd:string .

ns1:PerSquareMetre a owl:Class ;
    rdfs:label "PerSquareMetre"@en ;
    rdfs:comment """"Per Square Meter" is a denominator unit with dimensions /m².

-- QUDT"""@en ;
    rdfs:isDefinedBy "http://qudt.org/2.1/vocab/unit"^^xsd:string ;
    rdfs:subClassOf [ a owl:Restriction ;
            owl:hasValue 0e+00 ;
            owl:onProperty ns1:hasSIConversionOffset ],
        [ a owl:Restriction ;
            owl:hasValue 1e+00 ;
            owl:onProperty ns1:hasSIConversionMultiplier ],
        ns1:PerAreaUnit,
        ns1:SICoherentDerivedUnit ;
    skos:altLabel "ReciprocalSquareMetre"@en ;
    skos:prefLabel "PerSquareMetre"@en ;
    ns1:elucidation """"Per Square Meter" is a denominator unit with dimensions /m².

-- QUDT"""@en ;
    ns1:qudtReference "http://qudt.org/vocab/unit/PER-M2"^^xsd:string ;
    ns1:ucumCode "/m2"^^xsd:string,
        "m-2"^^xsd:string ;
    ns1:unitSymbol "/m²"^^xsd:string .

ns1:PerSquareMetreSecond a owl:Class ;
    rdfs:label "PerSquareMetreSecond"@en ;
    rdfs:comment "Per square metre and second."@en ;
    rdfs:isDefinedBy "http://qudt.org/2.1/vocab/unit"^^xsd:string ;
    rdfs:subClassOf [ a owl:Restriction ;
            owl:hasValue 1e+00 ;
            owl:onProperty ns1:hasSIConversionMultiplier ],
        [ a owl:Restriction ;
            owl:hasValue 0e+00 ;
            owl:onProperty ns1:hasSIConversionOffset ],
        ns1:PerAreaTimeUnit,
        ns1:SICoherentDerivedUnit ;
    skos:altLabel "ReciprocalSquareMetreSecond"@en ;
    skos:prefLabel "PerSquareMetreSecond"@en ;
    ns1:elucidation "Per square metre and second."@en ;
    ns1:qudtReference "http://qudt.org/vocab/unit/PER-M2-SEC"^^xsd:string ;
    ns1:ucumCode "m-2.s-1"^^xsd:string ;
    ns1:unitSymbol "/(m²⋅s)"^^xsd:string .

ns1:PerSquareSecond a owl:Class ;
    rdfs:label "PerSquareSecond"@en ;
    rdfs:comment "Per square second."@en ;
    rdfs:isDefinedBy "http://qudt.org/2.1/vocab/unit"^^xsd:string ;
    rdfs:subClassOf [ a owl:Restriction ;
            owl:hasValue 1e+00 ;
            owl:onProperty ns1:hasSIConversionMultiplier ],
        [ a owl:Restriction ;
            owl:hasValue 0e+00 ;
            owl:onProperty ns1:hasSIConversionOffset ],
        ns1:AngularFrequencyUnit,
        ns1:SICoherentDerivedUnit ;
    skos:altLabel "ReciprocalSquareSecond"@en ;
    skos:prefLabel "PerSquareSecond"@en ;
    ns1:elucidation "Per square second."@en ;
    ns1:qudtReference "http://qudt.org/vocab/unit/PER-SEC2"^^xsd:string ;
    ns1:ucumCode "s-2"^^xsd:string ;
    ns1:unitSymbol "/s²"^^xsd:string .

ns1:PerSteradian a owl:Class ;
    rdfs:label "PerSteradian"@en ;
    rdfs:comment "Per steradian."@en ;
    rdfs:isDefinedBy "http://qudt.org/2.1/vocab/unit"^^xsd:string ;
    rdfs:subClassOf [ a owl:Restriction ;
            owl:hasValue 1e+00 ;
            owl:onProperty ns1:hasSIConversionMultiplier ],
        [ a owl:Restriction ;
            owl:hasValue 0e+00 ;
            owl:onProperty ns1:hasSIConversionOffset ],
        ns1:FractionUnit,
        ns1:SICoherentDerivedUnit ;
    skos:altLabel "ReciprocalSteradian"@en ;
    skos:prefLabel "PerSteradian"@en ;
    ns1:elucidation "Per steradian."@en ;
    ns1:qudtReference "http://qudt.org/vocab/unit/PER-SR"^^xsd:string ;
    ns1:ucumCode "sr-1"^^xsd:string ;
    ns1:unitSymbol "/sr"^^xsd:string .

ns1:PerTeslaMetre a owl:Class ;
    rdfs:label "PerTeslaMetre"@en ;
    rdfs:comment """Per Tesla Meter Unit is a denominator unit with dimensions /m .· T.

-- QUDT"""@en ;
    rdfs:isDefinedBy "http://qudt.org/2.1/vocab/unit"^^xsd:string ;
    rdfs:subClassOf [ a owl:Restriction ;
            owl:hasValue 0e+00 ;
            owl:onProperty ns1:hasSIConversionOffset ],
        [ a owl:Restriction ;
            owl:hasValue 1e+00 ;
            owl:onProperty ns1:hasSIConversionMultiplier ],
        ns1:MagneticReluctivityUnit,
        ns1:SICoherentDerivedUnit ;
    skos:altLabel "ReciprocalTeslaMetre."@en ;
    skos:prefLabel "PerTeslaMetre"@en ;
    ns1:elucidation """Per Tesla Meter Unit is a denominator unit with dimensions /m .· T.

-- QUDT"""@en ;
    ns1:qudtReference "http://qudt.org/vocab/unit/PER-T-M"^^xsd:string ;
    ns1:ucumCode "T-1.m-1"^^xsd:string ;
    ns1:unitSymbol "/t⋅m"^^xsd:string .

ns1:PerTeslaSecond a owl:Class ;
    rdfs:label "PerTeslaSecond"@en ;
    rdfs:comment """Per Tesla Second Unit is a denominator unit with dimensions /s . T.

-- QUDT"""@en ;
    rdfs:isDefinedBy "http://qudt.org/2.1/vocab/unit"^^xsd:string ;
    rdfs:subClassOf ns1:ElectricChargePerMassUnit,
        ns1:SICoherentDerivedUnit ;
    skos:altLabel "Per Tesla and Second unit."@en ;
    skos:prefLabel "PerTeslaSecond"@en ;
    ns1:elucidation """Per Tesla Second Unit is a denominator unit with dimensions /s . T.

-- QUDT"""@en ;
    ns1:qudtReference "http://qudt.org/vocab/unit/PER-T-SEC"^^xsd:string ;
    ns1:ucumCode "T-1.s-1"^^xsd:string ;
    ns1:unitSymbol "/T⋅s"^^xsd:string .

ns1:PerWeber a owl:Class ;
    rdfs:label "PerWeber"@en ;
    rdfs:comment "Per Weber unit."@en ;
    rdfs:isDefinedBy "http://qudt.org/2.1/vocab/unit"^^xsd:string ;
    rdfs:seeAlso "http://www.iso.org/iso/catalogue_detail?csnumber=31897"^^xsd:string ;
    rdfs:subClassOf [ a owl:Restriction ;
            owl:hasValue 0e+00 ;
            owl:onProperty ns1:hasSIConversionOffset ],
        [ a owl:Restriction ;
            owl:hasValue 1e+00 ;
            owl:onProperty ns1:hasSIConversionMultiplier ],
        ns1:ElectricCurrentPerEnergyUnit,
        ns1:SICoherentDerivedUnit ;
    skos:altLabel "ReciprocalWeber"@en ;
    skos:prefLabel "PerWeber"@en ;
    ns1:elucidation "Per Weber unit."@en ;
    ns1:qudtReference "http://qudt.org/vocab/unit/PER-WB"^^xsd:string ;
    ns1:ucumCode "Wb-1"^^xsd:string ;
    ns1:unitSymbol "/Wb"^^xsd:string .

ns1:QuarticCoulombMetrePerCubicEnergy a owl:Class ;
    rdfs:label "QuarticCoulombMetrePerCubicEnergy"@en ;
    rdfs:comment """"Quartic Coulomb Meter per Cubic Energy" is a unit for  'Quartic Electric Dipole Moment Per Cubic Energy' expressed as C⁴ m⁴ J⁻³.

-- QUDT"""@en ;
    rdfs:isDefinedBy "http://qudt.org/2.1/vocab/unit"^^xsd:string ;
    rdfs:subClassOf ns1:QuarticElectricDipoleMomentPerCubicEnergyUnit,
        ns1:SICoherentDerivedUnit ;
    skos:altLabel "Quartic Coulomb Metre per Cubic Energy"@en ;
    skos:prefLabel "QuarticCoulombMetrePerCubicEnergy"@en ;
    ns1:elucidation """"Quartic Coulomb Meter per Cubic Energy" is a unit for  'Quartic Electric Dipole Moment Per Cubic Energy' expressed as C⁴ m⁴ J⁻³.

-- QUDT"""@en ;
    ns1:qudtReference "http://qudt.org/vocab/unit/C4-M4-PER-J3"^^xsd:string ;
    ns1:ucumCode "C4.m4.J-3"^^xsd:string,
        "C4.m4/J3"^^xsd:string ;
    ns1:unitSymbol "C⁴m⁴/J³"^^xsd:string .

ns1:QuarticMetre a owl:Class ;
    rdfs:label "QuarticMetre"@en ;
    rdfs:comment """A unit associated with area moments of inertia.

-- QUDT"""@en ;
    rdfs:isDefinedBy "http://qudt.org/2.1/vocab/unit"^^xsd:string ;
    rdfs:subClassOf ns1:QuarticLengthUnit,
        ns1:SICoherentDerivedUnit ;
    skos:altLabel "Quartic Metre"@en ;
    skos:prefLabel "QuarticMetre"@en ;
    ns1:elucidation """A unit associated with area moments of inertia.

-- QUDT"""@en ;
    ns1:qudtReference "http://qudt.org/vocab/unit/M4"^^xsd:string ;
    ns1:ucumCode "m4"^^xsd:string ;
    ns1:unitSymbol "m⁴"^^xsd:string .

ns1:QuarticMetrePerSecond a owl:Class ;
    rdfs:label "QuarticMetrePerSecond"^^xsd:string ;
    rdfs:comment "Metre to the power four per second."@en ;
    rdfs:isDefinedBy "http://qudt.org/2.1/vocab/unit"^^xsd:string ;
    rdfs:subClassOf ns1:QuarticLengthPerTimeUnit,
        ns1:SICoherentDerivedUnit ;
    skos:prefLabel "QuarticMetrePerSecond"^^xsd:string ;
    ns1:elucidation "Metre to the power four per second."@en ;
    ns1:qudtReference "http://qudt.org/vocab/unit/M4-PER-SEC"^^xsd:string ;
    ns1:ucumCode "m4.s-1"^^xsd:string ;
    ns1:unitSymbol "m⁴/s"^^xsd:string .

ns1:QuinticMetre a owl:Class ;
    rdfs:label "QuinticMetre"@en ;
    rdfs:comment "Metre to the power of five."@en ;
    rdfs:isDefinedBy "http://qudt.org/2.1/vocab/unit"^^xsd:string ;
    rdfs:subClassOf ns1:SICoherentDerivedUnit,
        ns1:SectionAreaIntegralUnit ;
    skos:prefLabel "QuinticMetre"@en ;
    ns1:elucidation "Metre to the power of five."@en ;
    ns1:qudtReference "http://qudt.org/vocab/unit/M5"^^xsd:string ;
    ns1:unitSymbol "m⁵"^^xsd:string .

ns1:RadianPerMetre a owl:Class ;
    rdfs:label "RadianPerMetre"@en ;
    rdfs:comment "Radian per metre."@en ;
    rdfs:isDefinedBy "http://qudt.org/2.1/vocab/unit"^^xsd:string ;
    rdfs:seeAlso "http://www.iso.org/iso/catalogue_detail?csnumber=31897"^^xsd:string ;
    rdfs:subClassOf [ a owl:Restriction ;
            owl:hasValue 1e+00 ;
            owl:onProperty ns1:hasSIConversionMultiplier ],
        [ a owl:Restriction ;
            owl:hasValue 0e+00 ;
            owl:onProperty ns1:hasSIConversionOffset ],
        ns1:ReciprocalLengthUnit,
        ns1:SICoherentDerivedUnit ;
    skos:prefLabel "RadianPerMetre"@en ;
    ns1:elucidation "Radian per metre."@en ;
    ns1:qudtReference "http://qudt.org/vocab/unit/RAD-PER-M"^^xsd:string ;
    ns1:ucumCode "rad.m-1"^^xsd:string ;
    ns1:unitSymbol "rad/m"^^xsd:string .

ns1:RadianPerSecond a owl:Class ;
    rdfs:label "RadianPerSecond"@en ;
    rdfs:comment """"Radian per Second" is the SI unit of rotational speed (angular velocity), and, also the unit of angular frequency. The radian per second is defined as the change in the orientation of an object, in radians, every second.

-- QUDT"""@en ;
    rdfs:isDefinedBy "http://qudt.org/2.1/vocab/unit"^^xsd:string ;
    rdfs:subClassOf [ a owl:Restriction ;
            owl:hasValue 0e+00 ;
            owl:onProperty ns1:hasSIConversionOffset ],
        [ a owl:Restriction ;
            owl:hasValue 1e+00 ;
            owl:onProperty ns1:hasSIConversionMultiplier ],
        ns1:FrequencyUnit,
        ns1:SICoherentDerivedUnit ;
    skos:altLabel "radian per second"@en ;
    skos:prefLabel "RadianPerSecond"@en ;
    ns1:elucidation """"Radian per Second" is the SI unit of rotational speed (angular velocity), and, also the unit of angular frequency. The radian per second is defined as the change in the orientation of an object, in radians, every second.

-- QUDT"""@en ;
    ns1:qudtReference "http://qudt.org/vocab/unit/RAD-PER-SEC"^^xsd:string ;
    ns1:ucumCode "rad.s-1"^^xsd:string,
        "rad/s"^^xsd:string ;
    ns1:unitSymbol "rad/s"^^xsd:string .

ns1:RadianPerSquareSecond a owl:Class ;
    rdfs:label "RadianPerSquareSecond"@en ;
    rdfs:comment """Angular acceleration is the rate of change of angular velocity. In SI units, it is measured in radians per Square second (rad/s²), and is usually denoted by the Greek letter α.

-- QUDT"""@en ;
    rdfs:isDefinedBy "http://qudt.org/2.1/vocab/unit"^^xsd:string ;
    rdfs:subClassOf [ a owl:Restriction ;
            owl:hasValue 0e+00 ;
            owl:onProperty ns1:hasSIConversionOffset ],
        [ a owl:Restriction ;
            owl:hasValue 1e+00 ;
            owl:onProperty ns1:hasSIConversionMultiplier ],
        ns1:AngularFrequencyUnit,
        ns1:SICoherentDerivedUnit ;
    skos:altLabel "Radian per Square Second"@en ;
    skos:prefLabel "RadianPerSquareSecond"@en ;
    ns1:elucidation """Angular acceleration is the rate of change of angular velocity. In SI units, it is measured in radians per Square second (rad/s²), and is usually denoted by the Greek letter α.

-- QUDT"""@en ;
    ns1:qudtReference "http://qudt.org/vocab/unit/RAD-PER-SEC2"^^xsd:string ;
    ns1:ucumCode "rad.s-2"^^xsd:string,
        "rad/s2"^^xsd:string ;
    ns1:unitSymbol "rad/s²"^^xsd:string .

ns1:RadianSquareMetrePerKilogram a owl:Class ;
    rdfs:label "RadianSquareMetrePerKilogram"^^xsd:string ;
    rdfs:comment "Radian square metre per kilogram."@en ;
    rdfs:isDefinedBy "http://qudt.org/2.1/vocab/unit"^^xsd:string ;
    rdfs:subClassOf [ a owl:Restriction ;
            owl:hasValue 0e+00 ;
            owl:onProperty ns1:hasSIConversionOffset ],
        [ a owl:Restriction ;
            owl:hasValue 1e+00 ;
            owl:onProperty ns1:hasSIConversionMultiplier ],
        ns1:AreaPerMassUnit,
        ns1:SICoherentDerivedUnit ;
    skos:prefLabel "RadianSquareMetrePerKilogram"^^xsd:string ;
    ns1:elucidation "Radian square metre per kilogram."@en ;
    ns1:qudtReference "http://qudt.org/vocab/unit/RAD-M2-PER-KiloGM"^^xsd:string ;
    ns1:ucumCode "rad.m2.kg-1"^^xsd:string ;
    ns1:unitSymbol "rad⋅m²/kg"^^xsd:string .

ns1:RadianSquareMetrePerMole a owl:Class ;
    rdfs:label "RadianSquareMetrePerMole"@en ;
    rdfs:comment "Radian square metre per mole."@en ;
    rdfs:isDefinedBy "http://qudt.org/2.1/vocab/unit"^^xsd:string ;
    rdfs:subClassOf [ a owl:Restriction ;
            owl:hasValue 1e+00 ;
            owl:onProperty ns1:hasSIConversionMultiplier ],
        [ a owl:Restriction ;
            owl:hasValue 0e+00 ;
            owl:onProperty ns1:hasSIConversionOffset ],
        ns1:AreaPerAmountUnit,
        ns1:SICoherentDerivedUnit ;
    skos:prefLabel "RadianSquareMetrePerMole"@en ;
    ns1:elucidation "Radian square metre per mole."@en ;
    ns1:qudtReference "http://qudt.org/vocab/unit/RAD-M2-PER-MOL"^^xsd:string ;
    ns1:ucumCode "rad.m2.mol-1"^^xsd:string ;
    ns1:unitSymbol "rad⋅m²/mol"^^xsd:string .

ns1:SecondPerMetre a owl:Class ;
    rdfs:label "SecondPerMetre"^^xsd:string ;
    rdfs:comment "Second per metre."@en ;
    rdfs:isDefinedBy "http://qudt.org/2.1/vocab/unit"^^xsd:string ;
    rdfs:subClassOf [ a owl:Restriction ;
            owl:hasValue 1e+00 ;
            owl:onProperty ns1:hasSIConversionMultiplier ],
        [ a owl:Restriction ;
            owl:hasValue 0e+00 ;
            owl:onProperty ns1:hasSIConversionOffset ],
        ns1:SICoherentDerivedUnit,
        ns1:TimePerLengthUnit ;
    skos:prefLabel "SecondPerMetre"^^xsd:string ;
    ns1:elucidation "Second per metre."@en ;
    ns1:qudtReference "http://qudt.org/vocab/unit/SEC-PER-M"^^xsd:string ;
    ns1:ucumCode "s.m-1"^^xsd:string ;
    ns1:unitSymbol "s/m"^^xsd:string .

ns1:SecondPerRadianCubicMetre a owl:Class ;
    rdfs:label "SecondPerRadianCubicMetre"@en ;
    rdfs:comment "Second per radian and cubic metre unit."@en ;
    rdfs:isDefinedBy "http://qudt.org/2.1/vocab/unit"^^xsd:string ;
    rdfs:seeAlso "http://www.iso.org/iso/catalogue_detail?csnumber=31897"^^xsd:string ;
    rdfs:subClassOf [ a owl:Restriction ;
            owl:hasValue 1e+00 ;
            owl:onProperty ns1:hasSIConversionMultiplier ],
        [ a owl:Restriction ;
            owl:hasValue 0e+00 ;
            owl:onProperty ns1:hasSIConversionOffset ],
        ns1:SICoherentDerivedUnit,
        ns1:TimePerVolumeUnit ;
    skos:prefLabel "SecondPerRadianCubicMetre"@en ;
    ns1:elucidation "Second per radian and cubic metre unit."@en ;
    ns1:qudtReference "http://qudt.org/vocab/unit/SEC-PER-RAD-M3"^^xsd:string ;
    ns1:ucumCode "s.rad-1.m-3"^^xsd:string ;
    ns1:unitSymbol "s/rad⋅m³"^^xsd:string .

ns1:SexticMetre a owl:Class ;
    rdfs:label "SexticMetre"@en ;
    rdfs:comment "Metre to the power of six."@en ;
    rdfs:isDefinedBy "http://qudt.org/2.1/vocab/unit"^^xsd:string ;
    rdfs:subClassOf ns1:SICoherentDerivedUnit,
        ns1:SexticLengthUnit ;
    skos:prefLabel "SexticMetre"@en ;
    ns1:elucidation "Metre to the power of six."@en ;
    ns1:qudtReference "http://qudt.org/vocab/unit/M6"^^xsd:string ;
    ns1:unitSymbol "m⁶"^^xsd:string .

ns1:SiemensPerMetre a owl:Class ;
    rdfs:label "SiemensPerMetre"@en ;
    rdfs:comment """SI derived unit siemens divided by the SI base unit metre.

-- QUDT"""@en ;
    rdfs:isDefinedBy "http://qudt.org/2.1/vocab/unit"^^xsd:string ;
    rdfs:subClassOf [ a owl:Restriction ;
            owl:hasValue 1e+00 ;
            owl:onProperty ns1:hasSIConversionMultiplier ],
        [ a owl:Restriction ;
            owl:hasValue 0e+00 ;
            owl:onProperty ns1:hasSIConversionOffset ],
        ns1:ElectricConductivityUnit,
        ns1:SICoherentDerivedUnit ;
    skos:altLabel "Siemens Per Metre"@en ;
    skos:prefLabel "SiemensPerMetre"@en ;
    ns1:elucidation """SI derived unit siemens divided by the SI base unit metre.

-- QUDT"""@en ;
    ns1:qudtReference "http://qudt.org/vocab/unit/S-PER-M"^^xsd:string ;
    ns1:ucumCode "S.m-1"^^xsd:string,
        "S/m"^^xsd:string ;
    ns1:unitSymbol "S/m"^^xsd:string .

ns1:SiemensSquareMetrePerMole a owl:Class ;
    rdfs:label "SiemensSquareMetrePerMole"@en ;
    rdfs:comment "Siemens square metre per mole."@en ;
    rdfs:isDefinedBy "http://qudt.org/2.1/vocab/unit"^^xsd:string ;
    rdfs:subClassOf [ a owl:Restriction ;
            owl:hasValue 0e+00 ;
            owl:onProperty ns1:hasSIConversionOffset ],
        [ a owl:Restriction ;
            owl:hasValue 1e+00 ;
            owl:onProperty ns1:hasSIConversionMultiplier ],
        ns1:AmountConductivityUnit,
        ns1:SICoherentDerivedUnit ;
    skos:prefLabel "SiemensSquareMetrePerMole"@en ;
    ns1:elucidation "Siemens square metre per mole."@en ;
    ns1:qudtReference "http://qudt.org/vocab/unit/S-M2-PER-MOL"^^xsd:string ;
    ns1:ucumCode "S.m2.mol-1"^^xsd:string ;
    ns1:unitSymbol "S⋅m²/mol"^^xsd:string .

ns1:SquareCoulombSquareMetrePerJoule a owl:Class ;
    rdfs:label "SquareCoulombSquareMetrePerJoule"@en ;
    rdfs:comment """"Square Coulomb Square Meter per Joule" is a unit for  'Polarizability' expressed as C² m² J⁻¹.

-- QUDT"""@en ;
    rdfs:isDefinedBy "http://qudt.org/2.1/vocab/unit"^^xsd:string ;
    rdfs:subClassOf [ a owl:Restriction ;
            owl:hasValue 1e+00 ;
            owl:onProperty ns1:hasSIConversionMultiplier ],
        [ a owl:Restriction ;
            owl:hasValue 0e+00 ;
            owl:onProperty ns1:hasSIConversionOffset ],
        ns1:SICoherentDerivedUnit,
        ns1:SquareCurrentQuarticTimePerMassUnit ;
    skos:altLabel "Square Coulomb Square Metre per Joule"@en ;
    skos:prefLabel "SquareCoulombSquareMetrePerJoule"@en ;
    ns1:elucidation """"Square Coulomb Square Meter per Joule" is a unit for  'Polarizability' expressed as C² m² J⁻¹.

-- QUDT"""@en ;
    ns1:qudtReference "http://qudt.org/vocab/unit/C2-M2-PER-J"^^xsd:string ;
    ns1:ucumCode "C2.m2.J-1"^^xsd:string,
        "C2.m2/J"^^xsd:string ;
    ns1:unitSymbol "C²⋅m²/J"^^xsd:string .

ns1:SquareDegreeCelsiusPerSecond a owl:Class ;
    rdfs:label "SquareDegreeCelsiusPerSecond"^^xsd:string ;
    rdfs:comment "Square degree Celsius per second."@en ;
    rdfs:isDefinedBy "http://qudt.org/2.1/vocab/unit"^^xsd:string ;
    rdfs:subClassOf ns1:SICoherentDerivedUnit,
        ns1:SquareTemperaturePerTimeUnit ;
    skos:prefLabel "SquareDegreeCelsiusPerSecond"^^xsd:string ;
    ns1:elucidation "Square degree Celsius per second."@en ;
    ns1:qudtReference "http://qudt.org/vocab/unit/DEG_C2-PER-SEC"^^xsd:string ;
    ns1:ucumCode "K2.s-1"^^xsd:string ;
    ns1:unitSymbol "°C²⋅s"^^xsd:string .

ns1:SquareKelvin a owl:Class ;
    rdfs:label "SquareKelvin"@en ;
    rdfs:comment "Square Kelvin."@en ;
    rdfs:isDefinedBy "http://qudt.org/2.1/vocab/unit"^^xsd:string ;
    rdfs:subClassOf [ a owl:Restriction ;
            owl:hasValue 1e+00 ;
            owl:onProperty ns1:hasSIConversionMultiplier ],
        [ a owl:Restriction ;
            owl:hasValue 0e+00 ;
            owl:onProperty ns1:hasSIConversionOffset ],
        ns1:SICoherentDerivedUnit,
        ns1:SquareTemperatureUnit ;
    skos:prefLabel "SquareKelvin"@en ;
    ns1:elucidation "Square Kelvin."@en ;
    ns1:qudtReference "http://qudt.org/vocab/unit/K2"^^xsd:string ;
    ns1:ucumCode "K2"^^xsd:string ;
    ns1:unitSymbol "K²"^^xsd:string .

ns1:SquareKilogramPerSquareSecond a owl:Class ;
    rdfs:label "SquareKilogramPerSquareSecond"^^xsd:string ;
    rdfs:comment "Square kilogram per square second."@en ;
    rdfs:isDefinedBy "http://qudt.org/2.1/vocab/unit"^^xsd:string ;
    rdfs:subClassOf [ a owl:Restriction ;
            owl:hasValue 1e+00 ;
            owl:onProperty ns1:hasSIConversionMultiplier ],
        [ a owl:Restriction ;
            owl:hasValue 0e+00 ;
            owl:onProperty ns1:hasSIConversionOffset ],
        ns1:SICoherentDerivedUnit,
        ns1:SquareMassPerSquareTimeUnit ;
    skos:prefLabel "SquareKilogramPerSquareSecond"^^xsd:string ;
    ns1:elucidation "Square kilogram per square second."@en ;
    ns1:qudtReference "http://qudt.org/vocab/unit/KiloGM2-PER-SEC2"^^xsd:string ;
    ns1:ucumCode "kg2.s-2"^^xsd:string ;
    ns1:unitSymbol "kg²/s²"^^xsd:string .

ns1:SquareMetre a owl:Class ;
    rdfs:label "SquareMetre"@en ;
    rdfs:comment """The S I unit of area is the square metre.

-- QUDT"""@en ;
    rdfs:subClassOf [ a owl:Restriction ;
            owl:hasValue 1e+00 ;
            owl:onProperty ns1:hasSIConversionMultiplier ],
        [ a owl:Restriction ;
            owl:hasValue 0e+00 ;
            owl:onProperty ns1:hasSIConversionOffset ],
        ns1:AreaUnit,
        ns1:SICoherentDerivedUnit ;
    skos:prefLabel "SquareMetre"@en ;
    schema:unitCode "MTK"^^xsd:string ;
    ns1:elucidation """The S I unit of area is the square metre.

-- QUDT"""@en ;
    ns1:omReference "http://www.ontology-of-units-of-measure.org/resource/om-2/squareMetre"^^xsd:string ;
    ns1:qudtReference "http://qudt.org/vocab/unit/M2"^^xsd:string ;
    ns1:ucumCode "m2"^^xsd:string ;
    ns1:unitSymbol "m²"^^xsd:string .

ns1:SquareMetreCubicHertz a owl:Class ;
    rdfs:label "SquareMetreCubicHertz"^^xsd:string ;
    rdfs:comment "Square metre and cubic Hertz."@en ;
    rdfs:isDefinedBy "http://qudt.org/2.1/vocab/unit"^^xsd:string ;
    rdfs:subClassOf [ a owl:Restriction ;
            owl:hasValue 1e+00 ;
            owl:onProperty ns1:hasSIConversionMultiplier ],
        [ a owl:Restriction ;
            owl:hasValue 0e+00 ;
            owl:onProperty ns1:hasSIConversionOffset ],
        ns1:AbsorbedDoseRateUnit,
        ns1:SICoherentDerivedUnit ;
    skos:prefLabel "SquareMetreCubicHertz"^^xsd:string ;
    ns1:elucidation "Square metre and cubic Hertz."@en ;
    ns1:qudtReference "http://qudt.org/vocab/unit/M2-HZ3"^^xsd:string ;
    ns1:ucumCode "m2.Hz3"^^xsd:string ;
    ns1:unitSymbol "m²⋅Hz³"^^xsd:string .

ns1:SquareMetreHertz a owl:Class ;
    rdfs:label "SquareMetreHertz"^^xsd:string ;
    rdfs:comment "Square metre Hertz."@en ;
    rdfs:isDefinedBy "http://qudt.org/2.1/vocab/unit"^^xsd:string ;
    rdfs:subClassOf [ a owl:Restriction ;
            owl:hasValue 0e+00 ;
            owl:onProperty ns1:hasSIConversionOffset ],
        [ a owl:Restriction ;
            owl:hasValue 1e+00 ;
            owl:onProperty ns1:hasSIConversionMultiplier ],
        ns1:AreicSpeedUnit,
        ns1:SICoherentDerivedUnit ;
    skos:prefLabel "SquareMetreHertz"^^xsd:string ;
    ns1:elucidation "Square metre Hertz."@en ;
    ns1:qudtReference "http://qudt.org/vocab/unit/M2-HZ"^^xsd:string ;
    ns1:ucumCode "m2.Hz"^^xsd:string ;
    ns1:unitSymbol "m²⋅Hz"^^xsd:string .

ns1:SquareMetreKelvin a owl:Class ;
    rdfs:label "SquareMetreKelvin"@en ;
    rdfs:comment """`Square Meter Kelvin` is a unit for 'Area Temperature' expressed as m²-K.

-- QUDT"""@en ;
    rdfs:isDefinedBy "http://qudt.org/2.1/vocab/unit"^^xsd:string ;
    rdfs:subClassOf [ a owl:Restriction ;
            owl:hasValue 1e+00 ;
            owl:onProperty ns1:hasSIConversionMultiplier ],
        [ a owl:Restriction ;
            owl:hasValue 0e+00 ;
            owl:onProperty ns1:hasSIConversionOffset ],
        ns1:AreaTemperatureUnit,
        ns1:SICoherentDerivedUnit ;
    skos:altLabel "Square Metre Kelvin"@en ;
    skos:prefLabel "SquareMetreKelvin"@en ;
    ns1:elucidation """`Square Meter Kelvin` is a unit for 'Area Temperature' expressed as m²-K.

-- QUDT"""@en ;
    ns1:qudtReference "http://qudt.org/vocab/unit/M2-K"^^xsd:string ;
    ns1:ucumCode "m2.K"^^xsd:string ;
    ns1:unitSymbol "m²⋅K"^^xsd:string .

ns1:SquareMetreKelvinPerWatt a owl:Class ;
    rdfs:label "SquareMetreKelvinPerWatt"@en ;
    rdfs:comment """`Square Meter Kelvin per Watt` is a unit for 'Thermal Insulance' expressed as (K²)m/W.

-- QUDT"""@en ;
    rdfs:isDefinedBy "http://qudt.org/2.1/vocab/unit"^^xsd:string ;
    rdfs:seeAlso "http://physics.nist.gov/Pubs/SP811/appenB9.html"^^xsd:string ;
    rdfs:subClassOf [ a owl:Restriction ;
            owl:hasValue 0e+00 ;
            owl:onProperty ns1:hasSIConversionOffset ],
        [ a owl:Restriction ;
            owl:hasValue 1e+00 ;
            owl:onProperty ns1:hasSIConversionMultiplier ],
        ns1:PerThermalTransmittanceUnit,
        ns1:SICoherentDerivedUnit ;
    skos:altLabel "Square Metre Kelvin per Watt"@en ;
    skos:prefLabel "SquareMetreKelvinPerWatt"@en ;
    ns1:elucidation """`Square Meter Kelvin per Watt` is a unit for 'Thermal Insulance' expressed as (K²)m/W.

-- QUDT"""@en ;
    ns1:qudtReference "http://qudt.org/vocab/unit/M2-K-PER-W"^^xsd:string ;
    ns1:ucumCode "m2.K.W-1"^^xsd:string ;
    ns1:unitSymbol "(K²)m/W"^^xsd:string .

ns1:SquareMetrePerGram a owl:Class ;
    rdfs:label "SquareMetrePerGram"^^xsd:string ;
    rdfs:comment "A unit in the category of specific area."@en ;
    rdfs:isDefinedBy "http://qudt.org/2.1/vocab/unit"^^xsd:string ;
    rdfs:subClassOf [ a owl:Restriction ;
            owl:hasValue 1e+03 ;
            owl:onProperty ns1:hasSIConversionMultiplier ],
        [ a owl:Restriction ;
            owl:hasValue 0e+00 ;
            owl:onProperty ns1:hasSIConversionOffset ],
        ns1:AreaPerMassUnit,
        ns1:MeasurementUnit,
        ns1:NonPrefixedUnit,
        ns1:SINonCoherentUnit ;
    skos:altLabel "Square metres per gram"@en ;
    skos:prefLabel "SquareMetrePerGram"^^xsd:string ;
    ns1:elucidation "A unit in the category of specific area."@en ;
    ns1:qudtReference "http://qudt.org/vocab/unit/M2-PER-GM"^^xsd:string ;
    ns1:ucumCode "m2.g-1"^^xsd:string ;
    ns1:unitSymbol "m²/g"^^xsd:string .

ns1:SquareMetrePerHertz a owl:Class ;
    rdfs:label "SquareMetrePerHertz"^^xsd:string ;
    rdfs:comment "Square metre per Hertz."@en ;
    rdfs:isDefinedBy "http://qudt.org/2.1/vocab/unit"^^xsd:string ;
    rdfs:subClassOf [ a owl:Restriction ;
            owl:hasValue 0e+00 ;
            owl:onProperty ns1:hasSIConversionOffset ],
        [ a owl:Restriction ;
            owl:hasValue 1e+00 ;
            owl:onProperty ns1:hasSIConversionMultiplier ],
        ns1:AreaTimeUnit,
        ns1:SICoherentDerivedUnit ;
    skos:prefLabel "SquareMetrePerHertz"^^xsd:string ;
    ns1:elucidation "Square metre per Hertz."@en ;
    ns1:qudtReference "http://qudt.org/vocab/unit/M2-PER-HZ"^^xsd:string ;
    ns1:ucumCode "m2.Hz-1"^^xsd:string ;
    ns1:unitSymbol "m²/Hz"^^xsd:string .

ns1:SquareMetrePerJoule a owl:Class ;
    rdfs:label "SquareMetrePerJoule"@en ;
    rdfs:comment "Square metre per Joule."@en ;
    rdfs:isDefinedBy "http://qudt.org/2.1/vocab/unit"^^xsd:string ;
    rdfs:subClassOf [ a owl:Restriction ;
            owl:hasValue 1e+00 ;
            owl:onProperty ns1:hasSIConversionMultiplier ],
        [ a owl:Restriction ;
            owl:hasValue 0e+00 ;
            owl:onProperty ns1:hasSIConversionOffset ],
        ns1:SICoherentDerivedUnit,
        ns1:SquareTimePerMassUnit ;
    skos:prefLabel "SquareMetrePerJoule"@en ;
    ns1:elucidation "Square metre per Joule."@en ;
    ns1:qudtReference "http://qudt.org/vocab/unit/M2-PER-J"^^xsd:string ;
    ns1:ucumCode "m2.J-1"^^xsd:string ;
    ns1:unitSymbol "m²/j"^^xsd:string .

ns1:SquareMetrePerKelvin a owl:Class ;
    rdfs:label "SquareMetrePerKelvin"@en ;
    rdfs:comment "Square metre per Kelvin."@en ;
    rdfs:isDefinedBy "http://qudt.org/2.1/vocab/unit"^^xsd:string ;
    rdfs:subClassOf [ a owl:Restriction ;
            owl:hasValue 0e+00 ;
            owl:onProperty ns1:hasSIConversionOffset ],
        [ a owl:Restriction ;
            owl:hasValue 1e+00 ;
            owl:onProperty ns1:hasSIConversionMultiplier ],
        ns1:AreaPerTemperatureUnit,
        ns1:SICoherentDerivedUnit ;
    skos:prefLabel "SquareMetrePerKelvin"@en ;
    ns1:elucidation "Square metre per Kelvin."@en ;
    ns1:qudtReference "http://qudt.org/vocab/unit/M2-PER-K"^^xsd:string ;
    ns1:ucumCode "m2.K-1"^^xsd:string ;
    ns1:unitSymbol "m²/k"^^xsd:string .

ns1:SquareMetrePerKilogram a owl:Class ;
    rdfs:label "SquareMetrePerKilogram"^^xsd:string ;
    rdfs:comment """Square Meter Per Kilogram (m2/kg) is a unit in the category of Specific Area. It is also known as square meters per kilogram, square metre per kilogram, square metres per kilogram, square meter/kilogram, square metre/kilogram. This unit is commonly used in the SI unit system. Square Meter Per Kilogram (m2/kg) has a dimension of M-1L2 where M is mass, and L is length. This unit is the standard SI unit in this category.

-- QUDT"""@en ;
    rdfs:isDefinedBy "http://qudt.org/2.1/vocab/unit"^^xsd:string ;
    rdfs:subClassOf [ a owl:Restriction ;
            owl:hasValue 1e+00 ;
            owl:onProperty ns1:hasSIConversionMultiplier ],
        [ a owl:Restriction ;
            owl:hasValue 0e+00 ;
            owl:onProperty ns1:hasSIConversionOffset ],
        ns1:AreaPerMassUnit,
        ns1:SICoherentDerivedUnit ;
    skos:altLabel "Square Metre per Kilogram"@en ;
    skos:prefLabel "SquareMetrePerKilogram"^^xsd:string ;
    ns1:elucidation """Square Meter Per Kilogram (m2/kg) is a unit in the category of Specific Area. It is also known as square meters per kilogram, square metre per kilogram, square metres per kilogram, square meter/kilogram, square metre/kilogram. This unit is commonly used in the SI unit system. Square Meter Per Kilogram (m2/kg) has a dimension of M-1L2 where M is mass, and L is length. This unit is the standard SI unit in this category.

-- QUDT"""@en ;
    ns1:qudtReference "http://qudt.org/vocab/unit/M2-PER-KiloGM"^^xsd:string ;
    ns1:ucumCode "m2.kg-1"^^xsd:string ;
    ns1:unitSymbol "m²/kg"^^xsd:string .

ns1:SquareMetrePerMole a owl:Class ;
    rdfs:label "SquareMetrePerMole"@en ;
    rdfs:comment """Square Meter Per Mole (m2/mol) is a unit in the category of Specific Area. It is also known as square meters per mole, square metre per per, square metres per per, square meter/per, square metre/per. This unit is commonly used in the SI unit system. Square Meter Per Mole (m2/mol) has a dimension of M-1L2 where M is mass, and L is length. This unit is the standard SI unit in this category.

-- QUDT"""@en ;
    rdfs:isDefinedBy "http://qudt.org/2.1/vocab/unit"^^xsd:string ;
    rdfs:subClassOf [ a owl:Restriction ;
            owl:hasValue 1e+00 ;
            owl:onProperty ns1:hasSIConversionMultiplier ],
        [ a owl:Restriction ;
            owl:hasValue 0e+00 ;
            owl:onProperty ns1:hasSIConversionOffset ],
        ns1:AreaPerAmountUnit,
        ns1:SICoherentDerivedUnit ;
    skos:altLabel "Square Metre per Mole"@en ;
    skos:prefLabel "SquareMetrePerMole"@en ;
    ns1:elucidation """Square Meter Per Mole (m2/mol) is a unit in the category of Specific Area. It is also known as square meters per mole, square metre per per, square metres per per, square meter/per, square metre/per. This unit is commonly used in the SI unit system. Square Meter Per Mole (m2/mol) has a dimension of M-1L2 where M is mass, and L is length. This unit is the standard SI unit in this category.

-- QUDT"""@en ;
    ns1:qudtReference "http://qudt.org/vocab/unit/M2-PER-MOL"^^xsd:string ;
    ns1:ucumCode "m2.mol-1"^^xsd:string ;
    ns1:unitSymbol "m²/mol"^^xsd:string .

ns1:SquareMetrePerNewton a owl:Class ;
    rdfs:label "SquareMetrePerNewton"@en ;
    rdfs:comment """power of the SI base unit metre with the exponent 2 divided by the derived SI unit newton

-- QUDT"""@en ;
    rdfs:isDefinedBy "http://qudt.org/2.1/vocab/unit"^^xsd:string ;
    rdfs:subClassOf [ a owl:Restriction ;
            owl:hasValue 0e+00 ;
            owl:onProperty ns1:hasSIConversionOffset ],
        [ a owl:Restriction ;
            owl:hasValue 1e+00 ;
            owl:onProperty ns1:hasSIConversionMultiplier ],
        ns1:PerPressureUnit,
        ns1:SICoherentDerivedUnit ;
    skos:altLabel "Square Metre Per Newton"@en ;
    skos:prefLabel "SquareMetrePerNewton"@en ;
    ns1:elucidation """power of the SI base unit metre with the exponent 2 divided by the derived SI unit newton

-- QUDT"""@en ;
    ns1:qudtReference "http://qudt.org/vocab/unit/M2-PER-N"^^xsd:string ;
    ns1:ucumCode "m2.N-1"^^xsd:string ;
    ns1:unitSymbol "m²/N"^^xsd:string .

ns1:SquareMetrePerSecond a owl:Class ;
    rdfs:label "SquareMetrePerSecond"@en ;
    rdfs:comment """Square Metres per second is the SI derived unit of angular momentum, defined by distance or displacement in metres multiplied by distance again in metres and divided by time in seconds. The unit is written in symbols as m2/s or m2u00b7s-1 or m2s-1. It may be better understood when phrased as "metres per second times metres", i.e. the momentum of an object with respect to a position.

-- QUDT"""@en ;
    rdfs:isDefinedBy "http://qudt.org/2.1/vocab/unit"^^xsd:string ;
    rdfs:subClassOf [ a owl:Restriction ;
            owl:hasValue 1e+00 ;
            owl:onProperty ns1:hasSIConversionMultiplier ],
        [ a owl:Restriction ;
            owl:hasValue 0e+00 ;
            owl:onProperty ns1:hasSIConversionOffset ],
        ns1:AreicSpeedUnit,
        ns1:SICoherentDerivedUnit ;
    skos:altLabel "Square Metre per Second"@en ;
    skos:prefLabel "SquareMetrePerSecond"@en ;
    ns1:elucidation """Square Metres per second is the SI derived unit of angular momentum, defined by distance or displacement in metres multiplied by distance again in metres and divided by time in seconds. The unit is written in symbols as m2/s or m2u00b7s-1 or m2s-1. It may be better understood when phrased as "metres per second times metres", i.e. the momentum of an object with respect to a position.

-- QUDT"""@en ;
    ns1:qudtReference "http://qudt.org/vocab/unit/M2-PER-SEC"^^xsd:string ;
    ns1:ucumCode "m2.s-1"^^xsd:string,
        "m2/s"^^xsd:string ;
    ns1:unitSymbol "m²/s"^^xsd:string .

ns1:SquareMetrePerSquareHertz a owl:Class ;
    rdfs:label "SquareMetrePerSquareHertz"^^xsd:string ;
    rdfs:comment "Square metres per square Hertz."@en ;
    rdfs:isDefinedBy "http://qudt.org/2.1/vocab/unit"^^xsd:string ;
    rdfs:subClassOf [ a owl:Restriction ;
            owl:hasValue 1e+00 ;
            owl:onProperty ns1:hasSIConversionMultiplier ],
        [ a owl:Restriction ;
            owl:hasValue 0e+00 ;
            owl:onProperty ns1:hasSIConversionOffset ],
        ns1:AreaSquareTimeUnit,
        ns1:SICoherentDerivedUnit ;
    skos:prefLabel "SquareMetrePerSquareHertz"^^xsd:string ;
    ns1:elucidation "Square metres per square Hertz."@en ;
    ns1:qudtReference "http://qudt.org/vocab/unit/M2-PER-HZ2"^^xsd:string ;
    ns1:ucumCode "m2.Hz-2"^^xsd:string ;
    ns1:unitSymbol "m²/Hz²"^^xsd:string .

ns1:SquareMetrePerSquareMetre a owl:Class ;
    rdfs:label "SquareMetrePerSquareMetre"@en ;
    rdfs:comment """A square metre unit of area per square metre

-- QUDT"""@en ;
    rdfs:isDefinedBy "http://qudt.org/2.1/vocab/unit"^^xsd:string ;
    rdfs:subClassOf [ a owl:Restriction ;
            owl:hasValue 1e+00 ;
            owl:onProperty ns1:hasSIConversionMultiplier ],
        [ a owl:Restriction ;
            owl:hasValue 0e+00 ;
            owl:onProperty ns1:hasSIConversionOffset ],
        ns1:AreaFractionUnit,
        ns1:SICoherentDerivedUnit ;
    skos:altLabel "square metre per square metre"@en ;
    skos:prefLabel "SquareMetrePerSquareMetre"@en ;
    ns1:elucidation """A square metre unit of area per square metre

-- QUDT"""@en ;
    ns1:qudtReference "http://qudt.org/vocab/unit/M2-PER-M2"^^xsd:string ;
    ns1:unitSymbol "m²/m²"^^xsd:string .

ns1:SquareMetrePerSquareSecond a owl:Class ;
    rdfs:label "SquareMetrePerSquareSecond"^^xsd:string ;
    rdfs:comment "Square metre per square second."@en ;
    rdfs:isDefinedBy "http://qudt.org/2.1/vocab/unit"^^xsd:string ;
    rdfs:subClassOf [ a owl:Restriction ;
            owl:hasValue 0e+00 ;
            owl:onProperty ns1:hasSIConversionOffset ],
        [ a owl:Restriction ;
            owl:hasValue 1e+00 ;
            owl:onProperty ns1:hasSIConversionMultiplier ],
        ns1:AbsorbedDoseUnit,
        ns1:SICoherentDerivedUnit ;
    skos:prefLabel "SquareMetrePerSquareSecond"^^xsd:string ;
    ns1:elucidation "Square metre per square second."@en ;
    ns1:qudtReference "http://qudt.org/vocab/unit/M2-PER-SEC2"^^xsd:string ;
    ns1:ucumCode "m2.s-2"^^xsd:string ;
    ns1:unitSymbol "m²/s²"^^xsd:string .

ns1:SquareMetrePerSteradian a owl:Class ;
    rdfs:label "SquareMetrePerSteradian"@en ;
    rdfs:comment "Square metre per steradian."@en ;
    rdfs:isDefinedBy "http://qudt.org/2.1/vocab/unit"^^xsd:string ;
    rdfs:subClassOf [ a owl:Restriction ;
            owl:hasValue 0e+00 ;
            owl:onProperty ns1:hasSIConversionOffset ],
        [ a owl:Restriction ;
            owl:hasValue 1e+00 ;
            owl:onProperty ns1:hasSIConversionMultiplier ],
        ns1:AreaUnit,
        ns1:SICoherentDerivedUnit ;
    skos:prefLabel "SquareMetrePerSteradian"@en ;
    ns1:elucidation "Square metre per steradian."@en ;
    ns1:qudtReference "http://qudt.org/vocab/unit/M2-PER-SR"^^xsd:string ;
    ns1:ucumCode "m2.sr-1"^^xsd:string ;
    ns1:unitSymbol "m²/sr"^^xsd:string ;
    ns1:wikipediaReference "http://en.wikipedia.org/wiki/Steradian?oldid=494317847"^^xsd:string .

ns1:SquareMetrePerSteradianJoule a owl:Class ;
    rdfs:label "SquareMetrePerSteradianJoule"@en ;
    rdfs:comment "Square metre per steradian and Joule."@en ;
    rdfs:isDefinedBy "http://qudt.org/2.1/vocab/unit"^^xsd:string ;
    rdfs:subClassOf [ a owl:Restriction ;
            owl:hasValue 1e+00 ;
            owl:onProperty ns1:hasSIConversionMultiplier ],
        [ a owl:Restriction ;
            owl:hasValue 0e+00 ;
            owl:onProperty ns1:hasSIConversionOffset ],
        ns1:SICoherentDerivedUnit,
        ns1:SquareTimePerMassUnit ;
    skos:prefLabel "SquareMetrePerSteradianJoule"@en ;
    ns1:elucidation "Square metre per steradian and Joule."@en ;
    ns1:qudtReference "http://qudt.org/vocab/unit/M2-PER-SR-J"^^xsd:string ;
    ns1:ucumCode "m2.sr-1.J-1"^^xsd:string ;
    ns1:unitSymbol "m²/(sr⋅J)"^^xsd:string .

ns1:SquareMetrePerVoltSecond a owl:Class ;
    rdfs:label "SquareMetrePerVoltSecond"@en ;
    rdfs:comment "Square metre per volt second."@en ;
    rdfs:isDefinedBy "http://qudt.org/2.1/vocab/unit"^^xsd:string ;
    rdfs:subClassOf [ a owl:Restriction ;
            owl:hasValue 0e+00 ;
            owl:onProperty ns1:hasSIConversionOffset ],
        [ a owl:Restriction ;
            owl:hasValue 1e+00 ;
            owl:onProperty ns1:hasSIConversionMultiplier ],
        ns1:SICoherentDerivedUnit,
        ns1:SquareLengthPerVoltageTimeUnit ;
    skos:prefLabel "SquareMetrePerVoltSecond"@en ;
    ns1:elucidation "Square metre per volt second."@en ;
    ns1:qudtReference "http://qudt.org/vocab/unit/M2-PER-V-SEC"^^xsd:string ;
    ns1:ucumCode "m2.V-1.s-1"^^xsd:string ;
    ns1:unitSymbol "m²/(V⋅s)"^^xsd:string .

ns1:SquareMetreQuarticHertz a owl:Class ;
    rdfs:label "SquareMetreQuarticHertz"^^xsd:string ;
    rdfs:comment "Square metre and quartic Hertz."@en ;
    rdfs:isDefinedBy "http://qudt.org/2.1/vocab/unit"^^xsd:string ;
    rdfs:subClassOf ns1:AreaPerQuarticTimeUnit,
        ns1:SICoherentDerivedUnit ;
    skos:prefLabel "SquareMetreQuarticHertz"^^xsd:string ;
    ns1:elucidation "Square metre and quartic Hertz."@en ;
    ns1:qudtReference "http://qudt.org/vocab/unit/M2-HZ4"^^xsd:string ;
    ns1:ucumCode "m2.Hz4"^^xsd:string ;
    ns1:unitSymbol "m²⋅Hz⁴"^^xsd:string .

ns1:SquareMetreSecondPerRadian a owl:Class ;
    rdfs:label "SquareMetreSecondPerRadian"^^xsd:string ;
    rdfs:comment "Square metre seconds per radian."@en ;
    rdfs:isDefinedBy "http://qudt.org/2.1/vocab/unit"^^xsd:string ;
    rdfs:subClassOf [ a owl:Restriction ;
            owl:hasValue 0e+00 ;
            owl:onProperty ns1:hasSIConversionOffset ],
        [ a owl:Restriction ;
            owl:hasValue 1e+00 ;
            owl:onProperty ns1:hasSIConversionMultiplier ],
        ns1:AreaTimeUnit,
        ns1:SICoherentDerivedUnit ;
    skos:prefLabel "SquareMetreSecondPerRadian"^^xsd:string ;
    ns1:elucidation "Square metre seconds per radian."@en ;
    ns1:qudtReference "http://qudt.org/vocab/unit/M2-SEC-PER-RAD"^^xsd:string ;
    ns1:ucumCode "m2.s.rad-1"^^xsd:string ;
    ns1:unitSymbol "m²⋅s/rad"^^xsd:string .

ns1:SquareMetreSquareHertz a owl:Class ;
    rdfs:label "SquareMetreSquareHertz"^^xsd:string ;
    rdfs:comment "Square metre and square Hertz."@en ;
    rdfs:isDefinedBy "http://qudt.org/2.1/vocab/unit"^^xsd:string ;
    rdfs:subClassOf [ a owl:Restriction ;
            owl:hasValue 1e+00 ;
            owl:onProperty ns1:hasSIConversionMultiplier ],
        [ a owl:Restriction ;
            owl:hasValue 0e+00 ;
            owl:onProperty ns1:hasSIConversionOffset ],
        ns1:AbsorbedDoseUnit,
        ns1:SICoherentDerivedUnit ;
    skos:prefLabel "SquareMetreSquareHertz"^^xsd:string ;
    ns1:elucidation "Square metre and square Hertz."@en ;
    ns1:qudtReference "http://qudt.org/vocab/unit/M2-HZ2"^^xsd:string ;
    ns1:ucumCode "m2.Hz2"^^xsd:string ;
    ns1:unitSymbol "m²⋅Hz²"^^xsd:string .

ns1:SquareMetreSteradian a owl:Class ;
    rdfs:label "SquareMetreSteradian"@en ;
    rdfs:comment """"Square Meter Steradian" is a unit for  'Area Angle' expressed as m²-sr.

-- QUDT"""@en ;
    rdfs:isDefinedBy "http://qudt.org/2.1/vocab/unit"^^xsd:string ;
    rdfs:subClassOf [ a owl:Restriction ;
            owl:hasValue 1e+00 ;
            owl:onProperty ns1:hasSIConversionMultiplier ],
        [ a owl:Restriction ;
            owl:hasValue 0e+00 ;
            owl:onProperty ns1:hasSIConversionOffset ],
        ns1:AreaUnit,
        ns1:SICoherentDerivedUnit ;
    skos:altLabel "Square Metre Steradian"@en ;
    skos:prefLabel "SquareMetreSteradian"@en ;
    ns1:elucidation """"Square Meter Steradian" is a unit for  'Area Angle' expressed as m²-sr.

-- QUDT"""@en ;
    ns1:qudtReference "http://qudt.org/vocab/unit/M2-SR"^^xsd:string ;
    ns1:ucumCode "m2.sr"^^xsd:string ;
    ns1:unitSymbol "m²⋅sr"^^xsd:string .

ns1:SquarePascalPerSquareSecond a owl:Class ;
    rdfs:label "SquarePascalPerSquareSecond"@en ;
    rdfs:comment "Square Pascal per square second."@en ;
    rdfs:isDefinedBy "http://qudt.org/2.1/vocab/unit"^^xsd:string ;
    rdfs:subClassOf [ a owl:Restriction ;
            owl:hasValue 0e+00 ;
            owl:onProperty ns1:hasSIConversionOffset ],
        [ a owl:Restriction ;
            owl:hasValue 1e+00 ;
            owl:onProperty ns1:hasSIConversionMultiplier ],
        ns1:SICoherentDerivedUnit,
        ns1:SquarePressurePerSquareTimeUnit ;
    skos:prefLabel "SquarePascalPerSquareSecond"@en ;
    ns1:elucidation "Square Pascal per square second."@en ;
    ns1:qudtReference "http://qudt.org/vocab/unit/PA2-PER-SEC2"^^xsd:string ;
    ns1:ucumCode "Pa2.s-2"^^xsd:string ;
    ns1:unitSymbol "Pa²/s²"^^xsd:string .

ns1:SquarePascalSecond a owl:Class ;
    rdfs:label "SquarePascalSecond"@en ;
    rdfs:comment """Square Pascal Second (Pa²· s) is a unit in the category of sound exposure.

-- QUDT"""@en ;
    rdfs:isDefinedBy "http://qudt.org/2.1/vocab/unit"^^xsd:string ;
    rdfs:seeAlso "http://www.efunda.com/glossary/units/units--specific_acoustic_impedance--pascal_second_per_meter.cfm"^^xsd:string ;
    rdfs:subClassOf [ a owl:Restriction ;
            owl:hasValue 1e+00 ;
            owl:onProperty ns1:hasSIConversionMultiplier ],
        [ a owl:Restriction ;
            owl:hasValue 0e+00 ;
            owl:onProperty ns1:hasSIConversionOffset ],
        ns1:SICoherentDerivedUnit,
        ns1:SquarePressureTimeUnit ;
    skos:altLabel "Square Pascal Second"@en ;
    skos:prefLabel "SquarePascalSecond"@en ;
    ns1:elucidation """Square Pascal Second (Pa²· s) is a unit in the category of sound exposure.

-- QUDT"""@en ;
    ns1:qudtReference "http://qudt.org/vocab/unit/PA2-SEC"^^xsd:string ;
    ns1:ucumCode "Pa2.s"^^xsd:string ;
    ns1:unitSymbol "Pa²⋅s"^^xsd:string .

ns1:SquareSecond a owl:Class ;
    rdfs:label "SquareSecond"@en ;
    rdfs:comment """"Square Second" is a unit for  'Square Time' expressed as s².

-- QUDT"""@en ;
    rdfs:isDefinedBy "http://qudt.org/2.1/vocab/unit"^^xsd:string ;
    rdfs:subClassOf [ a owl:Restriction ;
            owl:hasValue 1e+00 ;
            owl:onProperty ns1:hasSIConversionMultiplier ],
        [ a owl:Restriction ;
            owl:hasValue 0e+00 ;
            owl:onProperty ns1:hasSIConversionOffset ],
        ns1:SICoherentDerivedUnit,
        ns1:SquareTimeUnit ;
    skos:altLabel "Square Second"@en ;
    skos:prefLabel "SquareSecond"@en ;
    ns1:elucidation """"Square Second" is a unit for  'Square Time' expressed as s².

-- QUDT"""@en ;
    ns1:qudtReference "http://qudt.org/vocab/unit/SEC2"^^xsd:string ;
    ns1:ucumCode "s2"^^xsd:string ;
    ns1:unitSymbol "s²"^^xsd:string .

ns1:SquareVoltPerSquareKelvin a owl:Class ;
    rdfs:label "SquareVoltPerSquareKelvin"@en ;
    rdfs:comment "Square volt per square Kelvin."@en ;
    rdfs:isDefinedBy "http://qudt.org/2.1/vocab/unit"^^xsd:string ;
    rdfs:seeAlso "http://www.iso.org/iso/catalogue_detail?csnumber=31897"^^xsd:string ;
    rdfs:subClassOf [ a owl:Restriction ;
            owl:hasValue 1e+00 ;
            owl:onProperty ns1:hasSIConversionMultiplier ],
        [ a owl:Restriction ;
            owl:hasValue 0e+00 ;
            owl:onProperty ns1:hasSIConversionOffset ],
        ns1:SICoherentDerivedUnit,
        ns1:SquareElectricPotentialPerSquareTemperatureUnit ;
    skos:prefLabel "SquareVoltPerSquareKelvin"@en ;
    ns1:elucidation "Square volt per square Kelvin."@en ;
    ns1:qudtReference "http://qudt.org/vocab/unit/V2-PER-K2"^^xsd:string ;
    ns1:ucumCode "V2.K-2"^^xsd:string ;
    ns1:unitSymbol "V²/K²"^^xsd:string .

ns1:VoltAmpere a owl:Class ;
    rdfs:label "VoltAmpere"@en ;
    rdfs:comment """product of the SI derived unit volt and the SI base unit ampere

-- QUDT"""@en ;
    rdfs:isDefinedBy "http://qudt.org/2.1/vocab/unit"^^xsd:string ;
    rdfs:subClassOf [ a owl:Restriction ;
            owl:hasValue 0e+00 ;
            owl:onProperty ns1:hasSIConversionOffset ],
        [ a owl:Restriction ;
            owl:hasValue 1e+00 ;
            owl:onProperty ns1:hasSIConversionMultiplier ],
        ns1:PowerUnit,
        ns1:SICoherentDerivedUnit ;
    skos:altLabel "Volt Ampere"@en ;
    skos:prefLabel "VoltAmpere"@en ;
    ns1:elucidation """product of the SI derived unit volt and the SI base unit ampere

-- QUDT"""@en ;
    ns1:qudtReference "http://qudt.org/vocab/unit/V-A"^^xsd:string ;
    ns1:ucumCode "V.A"^^xsd:string ;
    ns1:unitSymbol "V⋅A"^^xsd:string .

ns1:VoltPerKelvin a owl:Class ;
    rdfs:label "VoltPerKelvin"@en ;
    rdfs:comment "Volt per Kelvin."@en ;
    rdfs:isDefinedBy "http://qudt.org/2.1/vocab/unit"^^xsd:string ;
    rdfs:seeAlso "http://www.iso.org/iso/catalogue_detail?csnumber=31897"^^xsd:string ;
    rdfs:subClassOf [ a owl:Restriction ;
            owl:hasValue 0e+00 ;
            owl:onProperty ns1:hasSIConversionOffset ],
        [ a owl:Restriction ;
            owl:hasValue 1e+00 ;
            owl:onProperty ns1:hasSIConversionMultiplier ],
        ns1:ElectricPotentialPerTemperatureUnit,
        ns1:SICoherentDerivedUnit ;
    skos:prefLabel "VoltPerKelvin"@en ;
    ns1:elucidation "Volt per Kelvin."@en ;
    ns1:qudtReference "http://qudt.org/vocab/unit/V-PER-K"^^xsd:string ;
    ns1:ucumCode "V.K-1"^^xsd:string ;
    ns1:unitSymbol "V/K"^^xsd:string .

ns1:VoltPerMetre a owl:Class ;
    rdfs:label "VoltPerMetre"@en ;
    rdfs:comment """Volt Per Meter (V/m) is a unit in the category of Electric field strength. It is also known as volts per meter, volt/meter, volt/metre, volt per metre, volts per metre. This unit is commonly used in the SI unit system. Volt Per Meter (V/m) has a dimension of MLT⁻³I⁻¹ where M is mass, L is length, T is time, and I is electric current. This unit is the standard SI unit in this category.

-- QUDT"""@en ;
    rdfs:isDefinedBy "http://qudt.org/2.1/vocab/unit"^^xsd:string ;
    rdfs:seeAlso "http://www.efunda.com/glossary/units/units--electric_field_strength--volt_per_meter.cfm"^^xsd:string ;
    rdfs:subClassOf [ a owl:Restriction ;
            owl:hasValue 1e+00 ;
            owl:onProperty ns1:hasSIConversionMultiplier ],
        [ a owl:Restriction ;
            owl:hasValue 0e+00 ;
            owl:onProperty ns1:hasSIConversionOffset ],
        ns1:ElectricFieldStrengthUnit,
        ns1:SICoherentDerivedUnit ;
    skos:altLabel "Volt per Metre"@en ;
    skos:prefLabel "VoltPerMetre"@en ;
    ns1:elucidation """Volt Per Meter (V/m) is a unit in the category of Electric field strength. It is also known as volts per meter, volt/meter, volt/metre, volt per metre, volts per metre. This unit is commonly used in the SI unit system. Volt Per Meter (V/m) has a dimension of MLT⁻³I⁻¹ where M is mass, L is length, T is time, and I is electric current. This unit is the standard SI unit in this category.

-- QUDT"""@en ;
    ns1:qudtReference "http://qudt.org/vocab/unit/V-PER-M"^^xsd:string ;
    ns1:ucumCode "V.m-1"^^xsd:string ;
    ns1:unitSymbol "V/m"^^xsd:string .

ns1:VoltPerSecond a owl:Class ;
    rdfs:label "VoltPerSecond"@en ;
    rdfs:comment """'Volt per Second' is a unit of magnetic flux equaling one weber. This is the flux passing through a conducting loop and reduced to zero at a uniform rate in one second inducing an electric potential of one volt in the loop.

-- QUDT"""@en ;
    rdfs:isDefinedBy "http://qudt.org/2.1/vocab/unit"^^xsd:string ;
    rdfs:seeAlso "http://www.thefreedictionary.com/Webers"^^xsd:string ;
    rdfs:subClassOf [ a owl:Restriction ;
            owl:hasValue 1e+00 ;
            owl:onProperty ns1:hasSIConversionMultiplier ],
        [ a owl:Restriction ;
            owl:hasValue 0e+00 ;
            owl:onProperty ns1:hasSIConversionOffset ],
        ns1:ElectricPotentialPerTimeUnit,
        ns1:SICoherentDerivedUnit ;
    skos:altLabel "Volt per second"@en ;
    skos:prefLabel "VoltPerSecond"@en ;
    ns1:elucidation """'Volt per Second' is a unit of magnetic flux equaling one weber. This is the flux passing through a conducting loop and reduced to zero at a uniform rate in one second inducing an electric potential of one volt in the loop.

-- QUDT"""@en ;
    ns1:qudtReference "http://qudt.org/vocab/unit/V-PER-SEC"^^xsd:string ;
    ns1:ucumCode "V.s-1"^^xsd:string ;
    ns1:unitSymbol "V/s"^^xsd:string .

ns1:VoltPerSquareMetre a owl:Class ;
    rdfs:label "VoltPerSquareMetre"@en ;
    rdfs:comment """The divergence at a particular point in a vector field is (roughly) how much the vector field 'spreads out' from that point. Operationally, we take the partial derivative of each of the field with respect to each of its space variables and add all the derivatives together to get the divergence. Electric field (V/m) differentiated with respect to distance (m) yields V/(m²).

-- QUDT"""@en ;
    rdfs:isDefinedBy "http://qudt.org/2.1/vocab/unit"^^xsd:string ;
    rdfs:seeAlso "http://www.funtrivia.com/en/subtopics/Physical-Quantities-310909.html"^^xsd:string ;
    rdfs:subClassOf [ a owl:Restriction ;
            owl:hasValue 0e+00 ;
            owl:onProperty ns1:hasSIConversionOffset ],
        [ a owl:Restriction ;
            owl:hasValue 1e+00 ;
            owl:onProperty ns1:hasSIConversionMultiplier ],
        ns1:ElectricPotentialPerAreaUnit,
        ns1:SICoherentDerivedUnit ;
    skos:altLabel "Volt per Square Metre"@en ;
    skos:prefLabel "VoltPerSquareMetre"@en ;
    ns1:elucidation """The divergence at a particular point in a vector field is (roughly) how much the vector field 'spreads out' from that point. Operationally, we take the partial derivative of each of the field with respect to each of its space variables and add all the derivatives together to get the divergence. Electric field (V/m) differentiated with respect to distance (m) yields V/(m²).

-- QUDT"""@en ;
    ns1:qudtReference "http://qudt.org/vocab/unit/V-PER-M2"^^xsd:string ;
    ns1:ucumCode "V.m-2"^^xsd:string ;
    ns1:unitSymbol "V/m²"^^xsd:string .

ns1:VoltSecondPerMetre a owl:Class ;
    rdfs:label "VoltSecondPerMetre"@en ;
    rdfs:comment """product of the SI derived unit volt and the SI base unit second divided by the SI base unit metre

-- QUDT"""@en ;
    rdfs:isDefinedBy "http://qudt.org/2.1/vocab/unit"^^xsd:string ;
    rdfs:subClassOf [ a owl:Restriction ;
            owl:hasValue 0e+00 ;
            owl:onProperty ns1:hasSIConversionOffset ],
        [ a owl:Restriction ;
            owl:hasValue 1e+00 ;
            owl:onProperty ns1:hasSIConversionMultiplier ],
        ns1:MagneticPotentialUnit,
        ns1:SICoherentDerivedUnit ;
    skos:altLabel "Volt Second Per Metre"@en ;
    skos:prefLabel "VoltSecondPerMetre"@en ;
    ns1:elucidation """product of the SI derived unit volt and the SI base unit second divided by the SI base unit metre

-- QUDT"""@en ;
    ns1:qudtReference "http://qudt.org/vocab/unit/V-SEC-PER-M"^^xsd:string ;
    ns1:ucumCode "V.s.m-1"^^xsd:string ;
    ns1:unitSymbol "V⋅s/m"^^xsd:string .

ns1:WattMetrePerSquareMetreSteradian a owl:Class ;
    rdfs:label "WattMetrePerSquareMetreSteradian"^^xsd:string ;
    rdfs:comment """The power per unit area of radiation of a given wavenumber illuminating a target at a given incident angle.

-- QUDT"""@en ;
    rdfs:isDefinedBy "http://qudt.org/2.1/vocab/unit"^^xsd:string ;
    rdfs:subClassOf [ a owl:Restriction ;
            owl:hasValue 0e+00 ;
            owl:onProperty ns1:hasSIConversionOffset ],
        [ a owl:Restriction ;
            owl:hasValue 1e+00 ;
            owl:onProperty ns1:hasSIConversionMultiplier ],
        ns1:MassLengthPerCubicTimeUnit,
        ns1:SICoherentDerivedUnit ;
    skos:altLabel "Watts metre per square metre steradian"@en ;
    skos:prefLabel "WattMetrePerSquareMetreSteradian"^^xsd:string ;
    ns1:elucidation """The power per unit area of radiation of a given wavenumber illuminating a target at a given incident angle.

-- QUDT"""@en ;
    ns1:qudtReference "http://qudt.org/vocab/unit/W-M-PER-M2-SR"^^xsd:string ;
    ns1:ucumCode "W.m-2.m.sr-1"^^xsd:string ;
    ns1:unitSymbol "W⋅m/m²⋅sr"^^xsd:string .

ns1:WattPerCubicMetre a owl:Class ;
    rdfs:label "WattPerCubicMetre"@en ;
    rdfs:comment """SI derived unit watt divided by the power of the SI base unit metre with the exponent 3

-- QUDT"""@en ;
    rdfs:isDefinedBy "http://qudt.org/2.1/vocab/unit"^^xsd:string ;
    rdfs:subClassOf [ a owl:Restriction ;
            owl:hasValue 1e+00 ;
            owl:onProperty ns1:hasSIConversionMultiplier ],
        [ a owl:Restriction ;
            owl:hasValue 0e+00 ;
            owl:onProperty ns1:hasSIConversionOffset ],
        ns1:PressurePerTimeUnit,
        ns1:SICoherentDerivedUnit ;
    skos:altLabel "Watt Per Cubic Metre"@en ;
    skos:prefLabel "WattPerCubicMetre"@en ;
    ns1:elucidation """SI derived unit watt divided by the power of the SI base unit metre with the exponent 3

-- QUDT"""@en ;
    ns1:qudtReference "http://qudt.org/vocab/unit/W-PER-M3"^^xsd:string ;
    ns1:ucumCode "W.m-3"^^xsd:string ;
    ns1:unitSymbol "W/m³"^^xsd:string .

ns1:WattPerKelvin a owl:Class ;
    rdfs:label "WattPerKelvin"@en ;
    rdfs:comment """Watt Per Kelvin (W/K) is a unit in the category of Thermal conductivity.

-- QUDT"""@en ;
    rdfs:isDefinedBy "http://qudt.org/2.1/vocab/unit"^^xsd:string ;
    rdfs:subClassOf [ a owl:Restriction ;
            owl:hasValue 0e+00 ;
            owl:onProperty ns1:hasSIConversionOffset ],
        [ a owl:Restriction ;
            owl:hasValue 1e+00 ;
            owl:onProperty ns1:hasSIConversionMultiplier ],
        ns1:SICoherentDerivedUnit,
        ns1:ThermalConductanceUnit ;
    skos:altLabel "Watt per Kelvin"@en ;
    skos:prefLabel "WattPerKelvin"@en ;
    ns1:elucidation """Watt Per Kelvin (W/K) is a unit in the category of Thermal conductivity.

-- QUDT"""@en ;
    ns1:qudtReference "http://qudt.org/vocab/unit/W-PER-K"^^xsd:string ;
    ns1:ucumCode "W.K-1"^^xsd:string ;
    ns1:unitSymbol "w/K"^^xsd:string .

ns1:WattPerKilogram a owl:Class ;
    rdfs:label "WattPerKilogram"^^xsd:string ;
    rdfs:comment """SI derived unit watt divided by the SI base unit kilogram

-- QUDT"""@en ;
    rdfs:isDefinedBy "http://qudt.org/2.1/vocab/unit"^^xsd:string ;
    rdfs:subClassOf [ a owl:Restriction ;
            owl:hasValue 0e+00 ;
            owl:onProperty ns1:hasSIConversionOffset ],
        [ a owl:Restriction ;
            owl:hasValue 1e+00 ;
            owl:onProperty ns1:hasSIConversionMultiplier ],
        ns1:AbsorbedDoseRateUnit,
        ns1:SICoherentDerivedUnit ;
    skos:altLabel "Watt Per Kilogram"@en ;
    skos:prefLabel "WattPerKilogram"^^xsd:string ;
    ns1:elucidation """SI derived unit watt divided by the SI base unit kilogram

-- QUDT"""@en ;
    ns1:qudtReference "http://qudt.org/vocab/unit/W-PER-KiloGM"^^xsd:string ;
    ns1:ucumCode "W.kg-1"^^xsd:string,
        "W/kg"^^xsd:string ;
    ns1:unitSymbol "W/kg"^^xsd:string .

ns1:WattPerMetre a owl:Class ;
    rdfs:label "WattPerMetre"^^xsd:string ;
    rdfs:comment "Watts per metre."@en ;
    rdfs:isDefinedBy "http://qudt.org/2.1/vocab/unit"^^xsd:string ;
    rdfs:subClassOf [ a owl:Restriction ;
            owl:hasValue 1e+00 ;
            owl:onProperty ns1:hasSIConversionMultiplier ],
        [ a owl:Restriction ;
            owl:hasValue 0e+00 ;
            owl:onProperty ns1:hasSIConversionOffset ],
        ns1:MassLengthPerCubicTimeUnit,
        ns1:SICoherentDerivedUnit ;
    skos:prefLabel "WattPerMetre"^^xsd:string ;
    ns1:elucidation "Watts per metre."@en ;
    ns1:qudtReference "http://qudt.org/vocab/unit/W-PER-M"^^xsd:string ;
    ns1:ucumCode "W.m-1"^^xsd:string ;
    ns1:unitSymbol "W/m"^^xsd:string .

ns1:WattPerMetreKelvin a owl:Class ;
    rdfs:label "WattPerMetreKelvin"@en ;
    rdfs:comment "Watt per metre and Kelvin unit."@en ;
    rdfs:isDefinedBy "http://qudt.org/2.1/vocab/unit"^^xsd:string ;
    rdfs:subClassOf [ a owl:Restriction ;
            owl:hasValue 1e+00 ;
            owl:onProperty ns1:hasSIConversionMultiplier ],
        [ a owl:Restriction ;
            owl:hasValue 0e+00 ;
            owl:onProperty ns1:hasSIConversionOffset ],
        ns1:SICoherentDerivedUnit,
        ns1:ThermalConductivityUnit ;
    skos:prefLabel "WattPerMetreKelvin"@en ;
    ns1:elucidation "Watt per metre and Kelvin unit."@en ;
    ns1:qudtReference "http://qudt.org/vocab/unit/W-PER-M-K"^^xsd:string ;
    ns1:ucumCode "W.m-1.K-1"^^xsd:string ;
    ns1:unitSymbol "W/(m⋅K)"^^xsd:string ;
    ns1:wikipediaReference "http://en.wikipedia.org/wiki/Thermal_conductivity"^^xsd:string .

ns1:WattPerSquareMetre a owl:Class ;
    rdfs:label "WattPerSquareMetre"@en ;
    rdfs:comment """"Watt per Square Meter} is a unit of irradiance defined as the power received per area. This is a unit in the category of Energy flux. It is also known as watts per square meter, watt per square metre, watts per square metre, watt/square meter, watt/square metre. This unit is commonly used in the SI unit system. Watt Per Square Meter (W/m²) has a dimension of MT^{-3" where M is mass, and T is time. This unit is the standard SI unit in this category.

-- QUDT"""@en ;
    rdfs:isDefinedBy "http://qudt.org/2.1/vocab/unit"^^xsd:string ;
    rdfs:seeAlso "http://www.efunda.com/glossary/units/units--energy_flux--watt_per_square_meter.cfm"^^xsd:string ;
    rdfs:subClassOf [ a owl:Restriction ;
            owl:hasValue 0e+00 ;
            owl:onProperty ns1:hasSIConversionOffset ],
        [ a owl:Restriction ;
            owl:hasValue 1e+00 ;
            owl:onProperty ns1:hasSIConversionMultiplier ],
        ns1:PowerDensityUnit,
        ns1:SICoherentDerivedUnit ;
    skos:altLabel "Watt per Square Metre"@en ;
    skos:prefLabel "WattPerSquareMetre"@en ;
    ns1:elucidation """"Watt per Square Meter} is a unit of irradiance defined as the power received per area. This is a unit in the category of Energy flux. It is also known as watts per square meter, watt per square metre, watts per square metre, watt/square meter, watt/square metre. This unit is commonly used in the SI unit system. Watt Per Square Meter (W/m²) has a dimension of MT^{-3" where M is mass, and T is time. This unit is the standard SI unit in this category.

-- QUDT"""@en ;
    ns1:qudtReference "http://qudt.org/vocab/unit/W-PER-M2"^^xsd:string ;
    ns1:ucumCode "W.m-2"^^xsd:string,
        "W/m2"^^xsd:string ;
    ns1:unitSymbol "W/m²"^^xsd:string .

ns1:WattPerSquareMetreKelvin a owl:Class ;
    rdfs:label "WattPerSquareMetreKelvin"@en ;
    rdfs:comment """`Watt Per Square Meter Per Kelvin `(W m⁻² K⁻¹) is a unit in the category of Thermal heat transfer coefficient. It is also known as watt/square meter-kelvin. This unit is commonly used in the SI unit system. Watt Per Square Meter Per Kelvin (W m⁻² K⁻¹) has a dimension of MT⁻¹Q⁻¹ where M is mass, T is time, and Q is temperature. This unit is the standard SI unit in this category.

-- QUDT"""@en ;
    rdfs:isDefinedBy "http://qudt.org/2.1/vocab/unit"^^xsd:string ;
    rdfs:subClassOf [ a owl:Restriction ;
            owl:hasValue 0e+00 ;
            owl:onProperty ns1:hasSIConversionOffset ],
        [ a owl:Restriction ;
            owl:hasValue 1e+00 ;
            owl:onProperty ns1:hasSIConversionMultiplier ],
        ns1:SICoherentDerivedUnit,
        ns1:ThermalTransmittanceUnit ;
    skos:altLabel "Watt per Square Metre Kelvin"@en ;
    skos:prefLabel "WattPerSquareMetreKelvin"@en ;
    ns1:elucidation """`Watt Per Square Meter Per Kelvin `(W m⁻² K⁻¹) is a unit in the category of Thermal heat transfer coefficient. It is also known as watt/square meter-kelvin. This unit is commonly used in the SI unit system. Watt Per Square Meter Per Kelvin (W m⁻² K⁻¹) has a dimension of MT⁻¹Q⁻¹ where M is mass, T is time, and Q is temperature. This unit is the standard SI unit in this category.

-- QUDT"""@en ;
    ns1:qudtReference "http://qudt.org/vocab/unit/W-PER-M2-K"^^xsd:string ;
    ns1:ucumCode "W.m-2.K-1"^^xsd:string ;
    ns1:unitSymbol "W/(m²⋅K)"^^xsd:string .

ns1:WattPerSquareMetrePascal a owl:Class ;
    rdfs:label "WattPerSquareMetrePascal"@en ;
    rdfs:comment """Watt Per Square Meter Per Pascal (W/m²-pa) is a unit of Evaporative Heat Transfer.

-- QUDT"""@en ;
    rdfs:isDefinedBy "http://qudt.org/2.1/vocab/unit"^^xsd:string ;
    rdfs:subClassOf [ a owl:Restriction ;
            owl:hasValue 1e+00 ;
            owl:onProperty ns1:hasSIConversionMultiplier ],
        [ a owl:Restriction ;
            owl:hasValue 0e+00 ;
            owl:onProperty ns1:hasSIConversionOffset ],
        ns1:SICoherentDerivedUnit,
        ns1:SpeedUnit ;
    skos:altLabel "Watt per Square Metre Pascal"@en ;
    skos:prefLabel "WattPerSquareMetrePascal"@en ;
    ns1:elucidation """Watt Per Square Meter Per Pascal (W/m²-pa) is a unit of Evaporative Heat Transfer.

-- QUDT"""@en ;
    ns1:qudtReference "http://qudt.org/vocab/unit/W-PER-M2-PA"^^xsd:string ;
    ns1:ucumCode "W.m-2.Pa-1"^^xsd:string ;
    ns1:unitSymbol "W/(m²⋅pa)"^^xsd:string .

ns1:WattPerSquareMetrePerMetre a owl:Class ;
    rdfs:label "WattPerSquareMetrePerMetre"^^xsd:string ;
    rdfs:comment "Watts per square metre per metre."@en ;
    rdfs:isDefinedBy "http://qudt.org/2.1/vocab/unit"^^xsd:string ;
    rdfs:subClassOf [ a owl:Restriction ;
            owl:hasValue 0e+00 ;
            owl:onProperty ns1:hasSIConversionOffset ],
        [ a owl:Restriction ;
            owl:hasValue 1e+00 ;
            owl:onProperty ns1:hasSIConversionMultiplier ],
        ns1:PressurePerTimeUnit,
        ns1:SICoherentDerivedUnit ;
    skos:prefLabel "WattPerSquareMetrePerMetre"^^xsd:string ;
    ns1:elucidation "Watts per square metre per metre."@en ;
    ns1:qudtReference "http://qudt.org/vocab/unit/W-PER-M2-M"^^xsd:string ;
    ns1:ucumCode "W.m-2.m-1"^^xsd:string ;
    ns1:unitSymbol "W/m²⋅m"^^xsd:string .

ns1:WattPerSquareMetrePerMetrePerSteradian a owl:Class ;
    rdfs:label "WattPerSquareMetrePerMetrePerSteradian"^^xsd:string ;
    rdfs:comment "Watts per square metre and metre and steradian."@en ;
    rdfs:isDefinedBy "http://qudt.org/2.1/vocab/unit"^^xsd:string ;
    rdfs:subClassOf [ a owl:Restriction ;
            owl:hasValue 0e+00 ;
            owl:onProperty ns1:hasSIConversionOffset ],
        [ a owl:Restriction ;
            owl:hasValue 1e+00 ;
            owl:onProperty ns1:hasSIConversionMultiplier ],
        ns1:PressurePerTimeUnit,
        ns1:SICoherentDerivedUnit ;
    skos:prefLabel "WattPerSquareMetrePerMetrePerSteradian"^^xsd:string ;
    ns1:elucidation "Watts per square metre and metre and steradian."@en ;
    ns1:qudtReference "http://qudt.org/vocab/unit/W-PER-M2-M-SR"^^xsd:string ;
    ns1:ucumCode "W.m-2.m-1.sr-1"^^xsd:string ;
    ns1:unitSymbol "W/m²⋅m⋅sr"^^xsd:string .

ns1:WattPerSquareMetreQuarticKelvin a owl:Class ;
    rdfs:label "WattPerSquareMetreQuarticKelvin"@en ;
    rdfs:comment """Watt Per Square Meter Per Quartic Kelvin (W/m2·K4) is a unit in the category of light.

-- QUDT"""@en ;
    rdfs:isDefinedBy "http://qudt.org/2.1/vocab/unit"^^xsd:string ;
    rdfs:subClassOf ns1:MassPerCubicTimeQuarticTemperatureUnit,
        ns1:SICoherentDerivedUnit ;
    skos:altLabel "Watt per Square Metre Quartic Kelvin"@en ;
    skos:prefLabel "WattPerSquareMetreQuarticKelvin"@en ;
    ns1:elucidation """Watt Per Square Meter Per Quartic Kelvin (W/m2·K4) is a unit in the category of light.

-- QUDT"""@en ;
    ns1:qudtReference "http://qudt.org/vocab/unit/W-PER-M2-K4"^^xsd:string ;
    ns1:ucumCode "W.m-2.K-4"^^xsd:string ;
    ns1:unitSymbol "W/(m²⋅K⁴)"^^xsd:string .

ns1:WattPerSquareMetreSteradian a owl:Class ;
    rdfs:label "WattPerSquareMetreSteradian"@en ;
    rdfs:comment """`Watt per steradian per square metre` is the SI unit of radiance (W·sr⁻¹·m⁻²), while that of spectral radiance in frequency is the watt per steradian per square metre per hertz (W·sr⁻¹·m⁻²·Hz⁻¹) and that of spectral radiance in wavelength is the watt per steradian per square metre, per metre (W·sr⁻¹·m⁻³), commonly the watt per steradian per square metre per nanometre (W·sr⁻¹·m⁻²·nm⁻¹). It has a dimension of ML⁻⁴T⁻³ where M is mass, L is length, and T is time. This unit is the standard SI unit in this category.

-- QUDT"""@en ;
    rdfs:isDefinedBy "http://qudt.org/2.1/vocab/unit"^^xsd:string ;
    rdfs:seeAlso "http://www.efunda.com/glossary/units/units--radiance--watt_per_square_meter_per_steradian.cfm"^^xsd:string ;
    rdfs:subClassOf [ a owl:Restriction ;
            owl:hasValue 0e+00 ;
            owl:onProperty ns1:hasSIConversionOffset ],
        [ a owl:Restriction ;
            owl:hasValue 1e+00 ;
            owl:onProperty ns1:hasSIConversionMultiplier ],
        ns1:PowerDensityUnit,
        ns1:SICoherentDerivedUnit ;
    skos:altLabel "Watt per Square Metre Steradian"@en ;
    skos:prefLabel "WattPerSquareMetreSteradian"@en ;
    ns1:elucidation """`Watt per steradian per square metre` is the SI unit of radiance (W·sr⁻¹·m⁻²), while that of spectral radiance in frequency is the watt per steradian per square metre per hertz (W·sr⁻¹·m⁻²·Hz⁻¹) and that of spectral radiance in wavelength is the watt per steradian per square metre, per metre (W·sr⁻¹·m⁻³), commonly the watt per steradian per square metre per nanometre (W·sr⁻¹·m⁻²·nm⁻¹). It has a dimension of ML⁻⁴T⁻³ where M is mass, L is length, and T is time. This unit is the standard SI unit in this category.

-- QUDT"""@en ;
    ns1:qudtReference "http://qudt.org/vocab/unit/W-PER-M2-SR"^^xsd:string ;
    ns1:ucumCode "W.m-2.sr-1"^^xsd:string ;
    ns1:unitSymbol "W/(m²⋅sr)"^^xsd:string ;
    ns1:wikipediaReference "https://en.wikipedia.org/wiki/Radiance"^^xsd:string .

ns1:WattPerSteradian a owl:Class ;
    rdfs:label "WattPerSteradian"@en ;
    rdfs:comment """`Watt Per Steradian (W/sr)` is the unit in the category of Radiant intensity. It is also known as watts per steradian. This unit is commonly used in the SI unit system. Watt Per Steradian (W/sr) has a dimension of M· L⁻²· T⁻³ where M is mass, L is length, and T is time. This unit is the standard SI unit in this category.

-- QUDT"""@en ;
    rdfs:isDefinedBy "http://qudt.org/2.1/vocab/unit"^^xsd:string ;
    rdfs:subClassOf [ a owl:Restriction ;
            owl:hasValue 0e+00 ;
            owl:onProperty ns1:hasSIConversionOffset ],
        [ a owl:Restriction ;
            owl:hasValue 1e+00 ;
            owl:onProperty ns1:hasSIConversionMultiplier ],
        ns1:PowerUnit,
        ns1:SICoherentDerivedUnit ;
    skos:altLabel "Watt per Steradian"@en ;
    skos:prefLabel "WattPerSteradian"@en ;
    ns1:elucidation """`Watt Per Steradian (W/sr)` is the unit in the category of Radiant intensity. It is also known as watts per steradian. This unit is commonly used in the SI unit system. Watt Per Steradian (W/sr) has a dimension of M· L⁻²· T⁻³ where M is mass, L is length, and T is time. This unit is the standard SI unit in this category.

-- QUDT"""@en ;
    ns1:qudtReference "http://qudt.org/vocab/unit/W-PER-SR"^^xsd:string ;
    ns1:ucumCode "W.sr-1"^^xsd:string ;
    ns1:unitSymbol "W/sr"^^xsd:string .

ns1:WattSecond a owl:Class ;
    rdfs:label "WattSecond"@en ;
    rdfs:comment """product of the SI derived unit watt and SI base unit second

-- QUDT"""@en ;
    rdfs:isDefinedBy "http://qudt.org/2.1/vocab/unit"^^xsd:string ;
    rdfs:subClassOf [ a owl:Restriction ;
            owl:hasValue 1e+00 ;
            owl:onProperty ns1:hasSIConversionMultiplier ],
        [ a owl:Restriction ;
            owl:hasValue 0e+00 ;
            owl:onProperty ns1:hasSIConversionOffset ],
        ns1:EnergyUnit,
        ns1:SICoherentDerivedUnit ;
    skos:altLabel "Watt Second"@en ;
    skos:prefLabel "WattSecond"@en ;
    ns1:elucidation """product of the SI derived unit watt and SI base unit second

-- QUDT"""@en ;
    ns1:qudtReference "http://qudt.org/vocab/unit/W-SEC"^^xsd:string ;
    ns1:ucumCode "W.s"^^xsd:string ;
    ns1:unitSymbol "W⋅s"^^xsd:string .

ns1:WattSecondPerSquareMetre a owl:Class ;
    rdfs:label "WattSecondPerSquareMetre"^^xsd:string ;
    rdfs:comment "Watt second per square metre."@en ;
    rdfs:isDefinedBy "http://qudt.org/2.1/vocab/unit"^^xsd:string ;
    rdfs:subClassOf [ a owl:Restriction ;
            owl:hasValue 1e+00 ;
            owl:onProperty ns1:hasSIConversionMultiplier ],
        [ a owl:Restriction ;
            owl:hasValue 0e+00 ;
            owl:onProperty ns1:hasSIConversionOffset ],
        ns1:ForcePerLengthUnit,
        ns1:SICoherentDerivedUnit ;
    skos:prefLabel "WattSecondPerSquareMetre"^^xsd:string ;
    ns1:elucidation "Watt second per square metre."@en ;
    ns1:qudtReference "http://qudt.org/vocab/unit/W-SEC-PER-M2"^^xsd:string ;
    ns1:ucumCode "W.s.m-2"^^xsd:string ;
    ns1:unitSymbol "W⋅s/m²"^^xsd:string .

ns1:WeberMetre a owl:Class ;
    rdfs:label "WeberMetre"@en ;
    rdfs:comment "Weber metre."@en ;
    rdfs:isDefinedBy "http://qudt.org/2.1/vocab/unit"^^xsd:string ;
    rdfs:seeAlso "http://www.simetric.co.uk/siderived.htm"^^xsd:string ;
    rdfs:subClassOf [ a owl:Restriction ;
            owl:hasValue 0e+00 ;
            owl:onProperty ns1:hasSIConversionOffset ],
        [ a owl:Restriction ;
            owl:hasValue 1e+00 ;
            owl:onProperty ns1:hasSIConversionMultiplier ],
        ns1:NewtonSquareMetrePerAmpereUnit,
        ns1:SICoherentDerivedUnit ;
    skos:prefLabel "WeberMetre"@en ;
    ns1:elucidation "Weber metre."@en ;
    ns1:qudtReference "http://qudt.org/vocab/unit/WB-M"^^xsd:string ;
    ns1:ucumCode "Wb.m"^^xsd:string ;
    ns1:unitSymbol "Wb⋅m"^^xsd:string .

ns1:WeberPerMetre a owl:Class ;
    rdfs:label "WeberPerMetre"@en ;
    rdfs:comment """SI derived unit weber divided by the SI base unit metre

-- QUDT"""@en ;
    rdfs:isDefinedBy "http://qudt.org/2.1/vocab/unit"^^xsd:string ;
    rdfs:subClassOf [ a owl:Restriction ;
            owl:hasValue 0e+00 ;
            owl:onProperty ns1:hasSIConversionOffset ],
        [ a owl:Restriction ;
            owl:hasValue 1e+00 ;
            owl:onProperty ns1:hasSIConversionMultiplier ],
        ns1:MagneticPotentialUnit,
        ns1:SICoherentDerivedUnit ;
    skos:altLabel "Weber Per Metre"@en ;
    skos:prefLabel "WeberPerMetre"@en ;
    ns1:elucidation """SI derived unit weber divided by the SI base unit metre

-- QUDT"""@en ;
    ns1:qudtReference "http://qudt.org/vocab/unit/WB-PER-M"^^xsd:string ;
    ns1:ucumCode "Wb.m-1"^^xsd:string ;
    ns1:unitSymbol "Wb/m"^^xsd:string .

<https://w3id.org/emmo/disciplines/units/coherentsiunits> a owl:Ontology ;
    dcterms:abstract """The module 'coherentsiunits' contain coherent derived SI units.

A coherent SI unit is the product of powers of the 7 base and 22 derived SI units.  It can always be written as a product of powers of the 7 base SI units with a numerical factor in front of the product that is equal to one.  Examples: m/s, Pa·m, etc...

Note that this module is not complete and may be extended with more coherent SI units over time."""@en ;
    dcterms:contributor ns1:FrancescaBleken,
        ns1:GerhardGoldbeck,
        ns1:SimonClark ;
    dcterms:creator ns1:EmanueleGhedini,
        ns1:JesperFriis ;
    dcterms:license "https://creativecommons.org/licenses/by/4.0/legalcode"^^xsd:string ;
    dcterms:publisher <https://emmc.eu> ;
    dcterms:title "Coherent SI units"@en ;
    rdfs:comment """Note: this file has automatically been populated with units from QUDT.

We kindly acknowledge NIST for reusing their content, including the selection of units, their elucidations and conversion multiplier."""@en,
        "The EMMO should be reasoned with HermiT to visualize all inferences and class hierarchy (ctrl+R hotkey in Protege)."@en ;
    owl:imports <https://w3id.org/emmo/1.0.2/disciplines/units/siunits> ;
    owl:versionIRI <https://w3id.org/emmo/1.0.2/disciplines/units/coherentsiunits> ;
    owl:versionInfo "1.0.2"^^xsd:string ;
    ns1:contact "emmo@emmc.eu"^^xsd:string .

ns1:AmountConcentrationUnit rdfs:label "AmountConcentrationUnit"@en ;
    rdfs:comment "The class of units with dimensionality 'AmountConcentration'."@en .

ns1:AmountConductivityUnit rdfs:label "AmountConductivityUnit"@en ;
    rdfs:comment "The class of units with dimensionality 'AmountConductivity'."@en .

ns1:AmountFractionUnit rdfs:label "AmountFractionUnit"@en ;
    rdfs:comment "Unit for quantities of dimension one that are the fraction of two amount of substance."@en .

ns1:AmountPerAreaUnit rdfs:label "AmountPerAreaUnit"@en ;
    rdfs:comment "The class of units with dimensionality 'AmountPerArea'."@en .

ns1:AmountPerMassPressureUnit rdfs:label "AmountPerMassPressureUnit"@en ;
    rdfs:comment "The class of units with dimensionality 'AmountPerMassPressure'."@en .

ns1:AmountPerMassTimeUnit rdfs:label "AmountPerMassTimeUnit"@en ;
    rdfs:comment "The class of units with dimensionality 'AmountPerMassTime'."@en .

ns1:AreaDensityUnit rdfs:label "AreaDensityUnit"@en ;
    rdfs:comment "The class of units with dimensionality 'AreaDensity'."@en .

ns1:AreaPerQuarticTimeUnit rdfs:label "AreaPerQuarticTimeUnit"@en ;
    rdfs:comment "The class of units with dimensionality 'AreaPerQuarticTime'."@en .

ns1:AreaPerTemperatureUnit rdfs:label "AreaPerTemperatureUnit"@en ;
    rdfs:comment "The class of units with dimensionality 'AreaPerTemperature'."@en .

ns1:AreaSquareTimeUnit rdfs:label "AreaSquareTimeUnit"@en ;
    rdfs:comment "The class of units with dimensionality 'AreaSquareTime'."@en .

ns1:AreaTemperatureUnit rdfs:label "AreaTemperatureUnit"@en ;
    rdfs:comment "The class of units with dimensionality 'AreaTemperature'."@en .

ns1:CubicElectricChargeLengthPerSquareEnergyUnit rdfs:label "CubicElectricChargeLengthPerSquareEnergyUnit"@en ;
    rdfs:comment "The class of units with dimensionality 'CubicElectricChargeLengthPerSquareEnergy'."@en .

ns1:DensityUnit rdfs:label "DensityUnit"@en ;
    rdfs:comment "The class of units with dimensionality 'Density'."@en .

ns1:ElectricChargeAreaUnit rdfs:label "ElectricChargeAreaUnit"@en ;
    rdfs:comment "The class of units with dimensionality 'ElectricChargeArea'."@en .

ns1:ElectricChargeDensityUnit rdfs:label "ElectricChargeDensityUnit"@en ;
    rdfs:comment "The class of units with dimensionality 'ElectricChargeDensity'."@en .

ns1:ElectricChargePerAmountUnit rdfs:label "ElectricChargePerAmountUnit"@en ;
    rdfs:comment "The class of units with dimensionality 'ElectricChargePerAmount'."@en .

ns1:ElectricChargePerLengthUnit rdfs:label "ElectricChargePerLengthUnit"@en ;
    rdfs:comment "The class of units with dimensionality 'ElectricChargePerLength'."@en .

ns1:ElectricConductivityUnit rdfs:label "ElectricConductivityUnit"@en ;
    rdfs:comment "The class of units with dimensionality 'ElectricConductivity'."@en .

ns1:ElectricCurrentDensityUnit rdfs:label "ElectricCurrentDensityUnit"@en ;
    rdfs:comment "The class of units with dimensionality 'ElectricCurrentDensity'."@en .

ns1:ElectricCurrentPerTemperatureUnit rdfs:label "ElectricCurrentPerTemperatureUnit"@en ;
    rdfs:comment "The class of units with dimensionality 'ElectricCurrentPerTemperature'."@en .

ns1:ElectricCurrentPerUnitEnergyUnit rdfs:label "ElectricCurrentPerUnitEnergyUnit"@en ;
    rdfs:comment "The class of units with dimensionality 'ElectricCurrentPerUnitEnergy'."@en .

ns1:ElectricDisplacementFieldUnit rdfs:label "ElectricDisplacementFieldUnit"@en ;
    rdfs:comment "The class of units with dimensionality 'ElectricDisplacementField'."@en .

ns1:ElectricPotentialPerAreaUnit rdfs:label "ElectricPotentialPerAreaUnit"@en ;
    rdfs:comment "The class of units with dimensionality 'ElectricPotentialPerArea'."@en .

ns1:ElectricPotentialPerTemperatureUnit rdfs:label "ElectricPotentialPerTemperatureUnit"@en ;
    rdfs:comment "The class of units with dimensionality 'ElectricPotentialPerTemperature'."@en .

ns1:ElectricPotentialPerTimeUnit rdfs:label "ElectricPotentialPerTimeUnit"@en ;
    rdfs:comment "The class of units with dimensionality 'ElectricPotentialPerTime'."@en .

ns1:EnergyAreaUnit rdfs:label "EnergyAreaUnit"@en ;
    rdfs:comment "The class of units with dimensionality 'EnergyArea'."@en .

ns1:EnergyLengthPerAmountUnit rdfs:label "EnergyLengthPerAmountUnit"@en ;
    rdfs:comment "The class of units with dimensionality 'EnergyLengthPerAmount'."@en .

ns1:EnergyPerAmountUnit rdfs:label "EnergyPerAmountUnit"@en ;
    rdfs:comment "The class of units with dimensionality 'EnergyPerAmount'."@en .

ns1:EnergyPerSquareMagneticFluxDensityUnit rdfs:label "EnergyPerSquareMagneticFluxDensityUnit"@en ;
    rdfs:comment "The class of units with dimensionality 'EnergyPerSquareMagneticFluxDensity'."@en .

ns1:EnergyTimePerAmountUnit rdfs:label "EnergyTimePerAmountUnit"@en ;
    rdfs:comment "The class of units with dimensionality 'EnergyTimePerAmount'."@en .

ns1:EntropyPerAmountUnit rdfs:label "EntropyPerAmountUnit"@en ;
    rdfs:comment "The class of units with dimensionality 'EntropyPerAmount'."@en .

ns1:EntropyUnit rdfs:label "EntropyUnit"@en ;
    rdfs:comment "The class of units with dimensionality 'Entropy'."@en .

ns1:ForceAreaUnit rdfs:label "ForceAreaUnit"@en ;
    rdfs:comment "The class of units with dimensionality 'ForceArea'."@en .

ns1:InversePermittivityUnit rdfs:label "InversePermittivityUnit"@en ;
    rdfs:comment "The class of units with dimensionality 'InversePermittivity'."@en .

ns1:InverseSquareMassUnit rdfs:label "InverseSquareMassUnit"@en ;
    rdfs:comment "The class of units with dimensionality 'InverseSquareMass'."@en .

ns1:LengthMassUnit rdfs:label "LengthMassUnit"@en ;
    rdfs:comment "The class of units with dimensionality 'LengthMass'."@en .

ns1:LengthPerTemperatureUnit rdfs:label "LengthPerTemperatureUnit"@en ;
    rdfs:comment "The class of units with dimensionality 'LengthPerTemperature'."@en .

ns1:LengthTimeCurrentUnit rdfs:label "LengthTimeCurrentUnit"@en ;
    rdfs:comment "The class of units with dimensionality 'LengthTimeCurrent'."@en .

ns1:LengthTimePerMassUnit rdfs:label "LengthTimePerMassUnit"@en ;
    rdfs:comment "The class of units with dimensionality 'LengthTimePerMass'."@en .

ns1:LuminousEfficacyUnit rdfs:label "LuminousEfficacyUnit"@en ;
    rdfs:comment "The class of units with dimensionality 'LuminousEfficacy'."@en .

ns1:MagneticFieldStrengthUnit rdfs:label "MagneticFieldStrengthUnit"@en ;
    rdfs:comment "The class of units with dimensionality 'MagneticFieldStrength'."@en .

ns1:MagneticReluctanceUnit rdfs:label "MagneticReluctanceUnit"@en ;
    rdfs:comment "The class of units with dimensionality 'MagneticReluctance'."@en .

ns1:MagneticReluctivityUnit rdfs:label "MagneticReluctivityUnit"@en ;
    rdfs:comment "The class of units with dimensionality 'MagneticReluctivity'."@en .

ns1:MassAreaUnit rdfs:label "MassAreaUnit"@en ;
    rdfs:comment "The class of units with dimensionality 'MassArea'."@en .

ns1:MassPerAmountUnit rdfs:label "MassPerAmountUnit"@en ;
    rdfs:comment "The class of units with dimensionality 'MassPerAmount'."@en .

ns1:MassPerCubicTimeQuarticTemperatureUnit rdfs:label "MassPerCubicTimeQuarticTemperatureUnit"@en ;
    rdfs:comment "The class of units with dimensionality 'MassPerCubicTimeQuarticTemperature'."@en .

ns1:MassPerLengthUnit rdfs:label "MassPerLengthUnit"@en ;
    rdfs:comment "The class of units with dimensionality 'MassPerLength'."@en .

ns1:MassPerQuarticLengthTimeUnit rdfs:label "MassPerQuarticLengthTimeUnit"@en ;
    rdfs:comment "The class of units with dimensionality 'MassPerQuarticLengthTime'."@en .

ns1:MassPerQuarticTimeUnit rdfs:label "MassPerQuarticTimeUnit"@en ;
    rdfs:comment "The class of units with dimensionality 'MassPerQuarticTime'."@en .

ns1:MassPerVolumeTimeUnit rdfs:label "MassPerVolumeTimeUnit"@en ;
    rdfs:comment "The class of units with dimensionality 'MassPerVolumeTime'."@en .

ns1:MassSquareTimeUnit rdfs:label "MassSquareTimeUnit"@en ;
    rdfs:comment "The class of units with dimensionality 'MassSquareTime'."@en .

ns1:MassStoppingPowerUnit rdfs:label "MassStoppingPowerUnit"@en ;
    rdfs:comment "The class of units with dimensionality 'MassStoppingPower'."@en .

ns1:MassTemperatureUnit rdfs:label "MassTemperatureUnit"@en ;
    rdfs:comment "The class of units with dimensionality 'MassTemperature'."@en .

ns1:PerAmountUnit rdfs:label "PerAmountUnit"@en ;
    rdfs:comment "The class of units with dimensionality 'PerAmount'."@en .

ns1:PerAreaUnit rdfs:label "PerAreaUnit"@en ;
    rdfs:comment "The class of units with dimensionality 'PerArea'."@en .

ns1:PerLengthTemperatureUnit rdfs:label "PerLengthTemperatureUnit"@en ;
    rdfs:comment "The class of units with dimensionality 'PerLengthTemperature'."@en .

ns1:PerLengthTimeUnit rdfs:label "PerLengthTimeUnit"@en ;
    rdfs:comment "The class of units with dimensionality 'PerLengthTime'."@en .

ns1:PerTemperatureTimeUnit rdfs:label "PerTemperatureTimeUnit"@en ;
    rdfs:comment "The class of units with dimensionality 'PerTemperatureTime'."@en .

ns1:PerTemperatureUnit rdfs:label "PerTemperatureUnit"@en ;
    rdfs:comment "The class of units with dimensionality 'PerTemperature'."@en .

ns1:PerThermalTransmittanceUnit rdfs:label "PerThermalTransmittanceUnit"@en ;
    rdfs:comment "The class of units with dimensionality 'PerThermalTransmittance'."@en .

ns1:PerTimeMassUnit rdfs:label "PerTimeMassUnit"@en ;
    rdfs:comment "The class of units with dimensionality 'PerTimeMass'."@en .

ns1:PermeabilityUnit rdfs:label "PermeabilityUnit"@en ;
    rdfs:comment "The class of units with dimensionality 'Permeability'."@en .

ns1:PermittivityUnit rdfs:label "PermittivityUnit"@en ;
    rdfs:comment "The class of units with dimensionality 'Permittivity'."@en .

ns1:QuarticElectricDipoleMomentPerCubicEnergyUnit rdfs:label "QuarticElectricDipoleMomentPerCubicEnergyUnit"@en ;
    rdfs:comment "The class of units with dimensionality 'QuarticElectricDipoleMomentPerCubicEnergy'."@en .

ns1:QuarticLengthPerTimeUnit rdfs:label "QuarticLengthPerTimeUnit"@en ;
    rdfs:comment "The class of units with dimensionality 'QuarticLengthPerTime'."@en .

ns1:QuarticLengthUnit rdfs:label "QuarticLengthUnit"@en ;
    rdfs:comment "The class of units with dimensionality 'QuarticLength'."@en .

ns1:ReciprocalElectricChargeDensityUnit rdfs:label "ReciprocalElectricChargeDensityUnit"@en ;
    rdfs:comment "The class of units with dimensionality 'ReciprocalElectricChargeDensity'."@en .

ns1:ReciprocalSquareEnergyUnit rdfs:label "ReciprocalSquareEnergyUnit"@en ;
    rdfs:comment "The class of units with dimensionality 'ReciprocalSquareEnergy'."@en .

ns1:RichardsonConstantUnit rdfs:label "RichardsonConstantUnit"@en ;
    rdfs:comment "The class of units with dimensionality 'RichardsonConstant'."@en .

ns1:SectionAreaIntegralUnit rdfs:label "SectionAreaIntegralUnit"@en ;
    rdfs:comment "The class of units with dimensionality 'SectionAreaIntegral'."@en .

ns1:SexticLengthUnit rdfs:label "SexticLengthUnit"@en ;
    rdfs:comment "The class of units with dimensionality 'SexticLength'."@en .

ns1:SquareElectricPotentialPerSquareTemperatureUnit rdfs:label "SquareElectricPotentialPerSquareTemperatureUnit"@en ;
    rdfs:comment "The class of units with dimensionality 'SquareElectricPotentialPerSquareTemperature'."@en .

ns1:SquareLengthPerVoltageTimeUnit rdfs:label "SquareLengthPerVoltageTimeUnit"@en ;
    rdfs:comment "The class of units with dimensionality 'SquareLengthPerVoltageTime'."@en .

ns1:SquareMassPerSquareTimeUnit rdfs:label "SquareMassPerSquareTimeUnit"@en ;
    rdfs:comment "The class of units with dimensionality 'SquareMassPerSquareTime'."@en .

ns1:SquarePressurePerSquareTimeUnit rdfs:label "SquarePressurePerSquareTimeUnit"@en ;
    rdfs:comment "The class of units with dimensionality 'SquarePressurePerSquareTime'."@en .

ns1:SquarePressureTimeUnit rdfs:label "SquarePressureTimeUnit"@en ;
    rdfs:comment "The class of units with dimensionality 'SquarePressureTime'."@en .

ns1:SquareTemperaturePerTimeUnit rdfs:label "SquareTemperaturePerTimeUnit"@en ;
    rdfs:comment "The class of units with dimensionality 'SquareTemperaturePerTime'."@en .

ns1:SquareTemperatureUnit rdfs:label "SquareTemperatureUnit"@en ;
    rdfs:comment "The class of units with dimensionality 'SquareTemperature'."@en .

ns1:SquareTimeUnit rdfs:label "SquareTimeUnit"@en ;
    rdfs:comment "The class of units with dimensionality 'SquareTime'."@en .

ns1:TemperatureAreaPerMassTimeUnit rdfs:label "TemperatureAreaPerMassTimeUnit"@en ;
    rdfs:comment "The class of units with dimensionality 'TemperatureAreaPerMassTime'."@en .

ns1:TemperatureLengthPerTimeUnit rdfs:label "TemperatureLengthPerTimeUnit"@en ;
    rdfs:comment "The class of units with dimensionality 'TemperatureLengthPerTime'."@en .

ns1:TemperatureMassPerAreaUnit rdfs:label "TemperatureMassPerAreaUnit"@en ;
    rdfs:comment "The class of units with dimensionality 'TemperatureMassPerArea'."@en .

ns1:TemperaturePerMagneticFluxDensityUnit rdfs:label "TemperaturePerMagneticFluxDensityUnit"@en ;
    rdfs:comment "The class of units with dimensionality 'TemperaturePerMagneticFluxDensity'."@en .

ns1:TemperaturePerSquareTimeUnit rdfs:label "TemperaturePerSquareTimeUnit"@en ;
    rdfs:comment "The class of units with dimensionality 'TemperaturePerSquareTime'."@en .

ns1:TemperaturePressurePerTimeUnit rdfs:label "TemperaturePressurePerTimeUnit"@en ;
    rdfs:comment "The class of units with dimensionality 'TemperaturePressurePerTime'."@en .

ns1:TemperatureTimeUnit rdfs:label "TemperatureTimeUnit"@en ;
    rdfs:comment "The class of units with dimensionality 'TemperatureTime'."@en .

ns1:ThermalConductanceUnit rdfs:label "ThermalConductanceUnit"@en ;
    rdfs:comment "The class of units with dimensionality 'ThermalConductance'."@en .

ns1:ThermalConductivityUnit rdfs:label "ThermalConductivityUnit"@en ;
    rdfs:comment "The class of units with dimensionality 'ThermalConductivity'."@en .

ns1:ThermalResistanceUnit rdfs:label "ThermalResistanceUnit"@en ;
    rdfs:comment "The class of units with dimensionality 'ThermalResistance'."@en .

ns1:ThermalResistivityUnit rdfs:label "ThermalResistivityUnit"@en ;
    rdfs:comment "The class of units with dimensionality 'ThermalResistivity'."@en .

ns1:ThermalTransmittanceUnit rdfs:label "ThermalTransmittanceUnit"@en ;
    rdfs:comment "The class of units with dimensionality 'ThermalTransmittance'."@en .

ns1:TimePerVolumeUnit rdfs:label "TimePerVolumeUnit"@en ;
    rdfs:comment "The class of units with dimensionality 'TimePerVolume'."@en .

ns1:VolumeFractionUnit rdfs:label "VolumeFractionUnit"@en ;
    rdfs:comment "Unit for quantities of dimension one that are the fraction of two volumes."@en .

ns1:VolumePerAmountUnit rdfs:label "VolumePerAmountUnit"@en ;
    rdfs:comment "The class of units with dimensionality 'VolumePerAmount'."@en .

ns1:VolumePerMassUnit rdfs:label "VolumePerMassUnit"@en ;
    rdfs:comment "The class of units with dimensionality 'VolumePerMass'."@en .

ns1:VolumePerSquareTimeUnit rdfs:label "VolumePerSquareTimeUnit"@en ;
    rdfs:comment "The class of units with dimensionality 'VolumePerSquareTime'."@en .

ns1:VolumePerTemperatureUnit rdfs:label "VolumePerTemperatureUnit"@en ;
    rdfs:comment "The class of units with dimensionality 'VolumePerTemperature'."@en .

ns1:VolumePerTimeUnit rdfs:label "VolumePerTimeUnit"@en ;
    rdfs:comment "The class of units with dimensionality 'VolumePerTime'."@en .

ns1:VolumeUnit rdfs:label "VolumeUnit"@en ;
    rdfs:comment "The class of units with dimensionality 'Volume'."@en .

ns1:AccelerationUnit rdfs:label "AccelerationUnit"@en ;
    rdfs:comment "The class of units with dimensionality 'Acceleration'."@en .

ns1:AmountPerAreaTimeUnit rdfs:label "AmountPerAreaTimeUnit"@en ;
    rdfs:comment "The class of units with dimensionality 'AmountPerAreaTime'."@en .

ns1:AmountPerMassUnit rdfs:label "AmountPerMassUnit"@en ;
    rdfs:comment "The class of units with dimensionality 'AmountPerMass'."@en .

ns1:AmountTemperatureUnit rdfs:label "AmountTemperatureUnit"@en ;
    rdfs:comment "The class of units with dimensionality 'AmountTemperature'."@en .

ns1:AngularFrequencyUnit rdfs:label "AngularFrequencyUnit"@en ;
    rdfs:comment "The class of units with dimensionality 'AngularFrequency'."@en .

ns1:AreaPerAmountUnit rdfs:label "AreaPerAmountUnit"@en ;
    rdfs:comment "The class of units with dimensionality 'AreaPerAmount'."@en .

ns1:AreaTimeUnit rdfs:label "AreaTimeUnit"@en ;
    rdfs:comment "The class of units with dimensionality 'AreaTime'."@en .

ns1:AreicSpeedUnit rdfs:label "AreicSpeedUnit"@en ;
    rdfs:comment "The class of units with dimensionality 'AreicSpeed'."@en .

ns1:ElectricCurrentPerEnergyUnit rdfs:label "ElectricCurrentPerEnergyUnit"@en ;
    rdfs:comment "The class of units with dimensionality 'ElectricCurrentPerEnergy'."@en .

ns1:ElectricCurrentPerMassUnit rdfs:label "ElectricCurrentPerMassUnit"@en ;
    rdfs:comment "The class of units with dimensionality 'ElectricCurrentPerMass'."@en .

ns1:ElectricFieldStrengthUnit rdfs:label "ElectricFieldStrengthUnit"@en ;
    rdfs:comment "The class of units with dimensionality 'ElectricFieldStrength'."@en .

ns1:ElectricResistivityUnit rdfs:label "ElectricResistivityUnit"@en ;
    rdfs:comment "The class of units with dimensionality 'ElectricResistivity'."@en .

ns1:FrequencyPerVolumeUnit rdfs:label "FrequencyPerVolumeUnit"@en ;
    rdfs:comment "The class of units with dimensionality 'FrequencyPerVolume'."@en .

ns1:LengthTemperatureUnit rdfs:label "LengthTemperatureUnit"@en ;
    rdfs:comment "The class of units with dimensionality 'LengthTemperature'."@en .

ns1:MagneticDipoleMomentUnit rdfs:label "MagneticDipoleMomentUnit"@en ;
    rdfs:comment "The class of units with dimensionality 'MagneticDipoleMoment'."@en .

ns1:MassFractionUnit rdfs:label "MassFractionUnit"@en ;
    rdfs:comment "Unit for quantities of dimension one that are the fraction of two masses."@en .

ns1:MassLengthPerCubicTimeUnit rdfs:label "MassLengthPerCubicTimeUnit"@en ;
    rdfs:comment "The class of units with dimensionality 'MassLengthPerCubicTime'."@en .

ns1:MassPerLengthTimeUnit rdfs:label "MassPerLengthTimeUnit"@en ;
    rdfs:comment "The class of units with dimensionality 'MassPerLengthTime'."@en .

ns1:MassPerTimeUnit rdfs:label "MassPerTimeUnit"@en ;
    rdfs:comment "The class of units with dimensionality 'MassPerTime'."@en .

ns1:NewtonSquareMetrePerAmpereUnit rdfs:label "NewtonSquareMetrePerAmpereUnit"@en ;
    rdfs:comment "The class of units with dimensionality 'NewtonSquareMetrePerAmpere'."@en .

ns1:NewtonianConstantOfGravityUnit rdfs:label "NewtonianConstantOfGravityUnit"@en ;
    rdfs:comment "The class of units with dimensionality 'NewtonianConstantOfGravity'."@en .

ns1:PerVolumeUnit rdfs:label "PerVolumeUnit"@en ;
    rdfs:comment "The class of units with dimensionality 'PerVolume'."@en .

ns1:PressurePerTemperatureUnit rdfs:label "PressurePerTemperatureUnit"@en ;
    rdfs:comment "The class of units with dimensionality 'PressurePerTemperature'."@en .

ns1:SquareCurrentQuarticTimePerMassUnit rdfs:label "SquareCurrentQuarticTimePerMassUnit"@en ;
    rdfs:comment "The class of units with dimensionality 'SquareCurrentQuarticTimePerMass'."@en .

ns1:SquareTimePerMassUnit rdfs:label "SquareTimePerMassUnit"@en ;
    rdfs:comment "The class of units with dimensionality 'SquareTimePerMass'."@en .

ns1:TemperaturePerLengthUnit rdfs:label "TemperaturePerLengthUnit"@en ;
    rdfs:comment "The class of units with dimensionality 'TemperaturePerLength'."@en .

ns1:TemperaturePerTimeUnit rdfs:label "TemperaturePerTimeUnit"@en ;
    rdfs:comment "The class of units with dimensionality 'TemperaturePerTime'."@en .

ns1:TimePerLengthUnit rdfs:label "TimePerLengthUnit"@en ;
    rdfs:comment "The class of units with dimensionality 'TimePerLength'."@en .

ns1:AbsorbedDoseRateUnit rdfs:label "AbsorbedDoseRateUnit"@en ;
    rdfs:comment "The class of units with dimensionality 'AbsorbedDoseRate'."@en .

ns1:AreaPerMassUnit rdfs:label "AreaPerMassUnit"@en ;
    rdfs:comment "The class of units with dimensionality 'AreaPerMass'."@en .

ns1:AreaUnit rdfs:label "AreaUnit"@en ;
    rdfs:comment "The class of units with dimensionality 'Area'."@en .

ns1:EntropyPerMassUnit rdfs:label "EntropyPerMassUnit"@en ;
    rdfs:comment "The class of units with dimensionality 'EntropyPerMass'."@en .

ns1:MagneticPotentialUnit rdfs:label "MagneticPotentialUnit"@en ;
    rdfs:comment "The class of units with dimensionality 'MagneticPotential'."@en .

ns1:PowerDensityUnit rdfs:label "PowerDensityUnit"@en ;
    rdfs:comment "The class of units with dimensionality 'PowerDensity'."@en .

ns1:ReciprocalLengthUnit rdfs:label "ReciprocalLengthUnit"@en ;
    rdfs:comment "The class of units with dimensionality 'ReciprocalLength'."@en .

ns1:SpeedUnit rdfs:label "SpeedUnit"@en ;
    rdfs:comment "The class of units with dimensionality 'Speed'."@en .

ns1:AmountPerVolumeTimeUnit rdfs:label "AmountPerVolumeTimeUnit"@en ;
    rdfs:comment "The class of units with dimensionality 'AmountPerVolumeTime'."@en .

ns1:AngularMomentumUnit rdfs:label "AngularMomentumUnit"@en ;
    rdfs:comment "The class of units with dimensionality 'AngularMomentum'."@en .

ns1:ElectricChargePerMassUnit rdfs:label "ElectricChargePerMassUnit"@en ;
    rdfs:comment "The class of units with dimensionality 'ElectricChargePerMass'."@en .

ns1:MassFluxUnit rdfs:label "MassFluxUnit"@en ;
    rdfs:comment "The class of units with dimensionality 'MassFlux'."@en .

ns1:MassPerSquareLengthSquareTimeUnit rdfs:label "MassPerSquareLengthSquareTimeUnit"@en ;
    rdfs:comment "The class of units with dimensionality 'MassPerSquareLengthSquareTime'."@en .

ns1:MomentumUnit rdfs:label "MomentumUnit"@en ;
    rdfs:comment "The class of units with dimensionality 'Momentum'."@en .

ns1:PerAreaTimeUnit rdfs:label "PerAreaTimeUnit"@en ;
    rdfs:comment "The class of units with dimensionality 'PerAreaTime'."@en .

ns1:PerPressureUnit rdfs:label "PerPressureUnit"@en ;
    rdfs:comment "The class of units with dimensionality 'PerPressure'."@en .

ns1:PressurePerTimeUnit rdfs:label "PressurePerTimeUnit"@en ;
    rdfs:comment "The class of units with dimensionality 'PressurePerTime'."@en .

ns1:ForcePerLengthUnit rdfs:label "ForcePerLengthUnit"@en ;
    rdfs:comment "The class of units with dimensionality 'ForcePerLength'."@en .

