@prefix dcterms: <http://purl.org/dc/terms/> .
@prefix ns1: <https://w3id.org/emmo#> .
@prefix owl: <http://www.w3.org/2002/07/owl#> .
@prefix rdfs: <http://www.w3.org/2000/01/rdf-schema#> .
@prefix schema: <https://schema.org/> .
@prefix skos: <http://www.w3.org/2004/02/skos/core#> .
@prefix xsd: <http://www.w3.org/2001/XMLSchema#> .

ns1:AmperePerCentiMetre a owl:Class ;
    rdfs:label "AmperePerCentiMetre"@en ;
    rdfs:comment """SI base unit ampere divided by the 0.01-fold of the SI base unit metre

-- QUDT"""@en ;
    rdfs:isDefinedBy "http://qudt.org/2.1/vocab/unit"^^xsd:string ;
    rdfs:subClassOf [ a owl:Restriction ;
            owl:hasValue 0e+00 ;
            owl:onProperty ns1:hasSIConversionOffset ],
        [ a owl:Restriction ;
            owl:hasValue 1e+02 ;
            owl:onProperty ns1:hasSIConversionMultiplier ],
        ns1:MagneticFieldStrengthUnit,
        ns1:SINonCoherentDerivedUnit ;
    skos:altLabel "Ampere Per Centimetre"@en ;
    skos:prefLabel "AmperePerCentiMetre"@en ;
    ns1:elucidation """SI base unit ampere divided by the 0.01-fold of the SI base unit metre

-- QUDT"""@en ;
    ns1:qudtReference "http://qudt.org/vocab/unit/A-PER-CentiM"^^xsd:string ;
    ns1:ucumCode "A.cm-1"^^xsd:string ;
    ns1:unitSymbol "A/cm"^^xsd:string .

ns1:AmperePerGram a owl:Class ;
    rdfs:label "AmperePerGram"@en ;
    rdfs:comment """`Ampere per gram` is a practical unit to describe an (applied) current relative to the involved amount of material. This unit is often found in electrochemistry to standardize test conditions and compare various scales of investigated materials.

-- QUDT"""@en ;
    rdfs:isDefinedBy "http://qudt.org/2.1/vocab/unit"^^xsd:string ;
    rdfs:subClassOf [ a owl:Restriction ;
            owl:hasValue 0e+00 ;
            owl:onProperty ns1:hasSIConversionOffset ],
        [ a owl:Restriction ;
            owl:hasValue 1e+03 ;
            owl:onProperty ns1:hasSIConversionMultiplier ],
        ns1:ElectricCurrentPerMassUnit,
        ns1:NonPrefixedUnit,
        ns1:SINonCoherentUnit ;
    skos:altLabel "Ampere per Gram"@en ;
    skos:prefLabel "AmperePerGram"@en ;
    ns1:elucidation """`Ampere per gram` is a practical unit to describe an (applied) current relative to the involved amount of material. This unit is often found in electrochemistry to standardize test conditions and compare various scales of investigated materials.

-- QUDT"""@en ;
    ns1:qudtReference "http://qudt.org/vocab/unit/A-PER-GM"^^xsd:string ;
    ns1:unitSymbol "A⋅/g"^^xsd:string .

ns1:AmperePerSquareCentiMetre a owl:Class ;
    rdfs:label "AmperePerSquareCentiMetre"@en ;
    rdfs:comment """SI base unit ampere divided by the 0.0001-fold  of the power of the SI base unit metre by exponent 2

-- QUDT"""@en ;
    rdfs:isDefinedBy "http://qudt.org/2.1/vocab/unit"^^xsd:string ;
    rdfs:subClassOf [ a owl:Restriction ;
            owl:hasValue 0e+00 ;
            owl:onProperty ns1:hasSIConversionOffset ],
        [ a owl:Restriction ;
            owl:hasValue 1e+04 ;
            owl:onProperty ns1:hasSIConversionMultiplier ],
        ns1:ElectricCurrentDensityUnit,
        ns1:SINonCoherentDerivedUnit ;
    skos:altLabel "Ampere Per Square Centimetre"@en ;
    skos:prefLabel "AmperePerSquareCentiMetre"@en ;
    ns1:elucidation """SI base unit ampere divided by the 0.0001-fold  of the power of the SI base unit metre by exponent 2

-- QUDT"""@en ;
    ns1:qudtReference "http://qudt.org/vocab/unit/A-PER-CentiM2"^^xsd:string ;
    ns1:ucumCode "A.cm-2"^^xsd:string,
        "A/cm2"^^xsd:string ;
    ns1:unitSymbol "A/cm²"^^xsd:string .

ns1:AmperePerSquareMilliMetre a owl:Class ;
    rdfs:label "AmperePerSquareMilliMetre"@en ;
    rdfs:comment """SI base unit ampere divided by the 0.000 001-fold of the power of the SI base unit metre by exponent 2

-- QUDT"""@en ;
    rdfs:isDefinedBy "http://qudt.org/2.1/vocab/unit"^^xsd:string ;
    rdfs:subClassOf [ a owl:Restriction ;
            owl:hasValue 0e+00 ;
            owl:onProperty ns1:hasSIConversionOffset ],
        [ a owl:Restriction ;
            owl:hasValue 1e+06 ;
            owl:onProperty ns1:hasSIConversionMultiplier ],
        ns1:ElectricCurrentDensityUnit,
        ns1:SINonCoherentDerivedUnit ;
    skos:altLabel "Ampere Per Square Millimetre"@en ;
    skos:prefLabel "AmperePerSquareMilliMetre"@en ;
    ns1:elucidation """SI base unit ampere divided by the 0.000 001-fold of the power of the SI base unit metre by exponent 2

-- QUDT"""@en ;
    ns1:qudtReference "http://qudt.org/vocab/unit/A-PER-MilliM2"^^xsd:string ;
    ns1:ucumCode "A.mm-2"^^xsd:string,
        "A/mm2"^^xsd:string ;
    ns1:unitSymbol "A/mm²"^^xsd:string .

ns1:AttoJouleSecond a owl:Class ;
    rdfs:label "AttoJouleSecond"^^xsd:string ;
    rdfs:comment """unit of the Planck's constant as product of the SI derived unit joule and the SI base unit second

-- QUDT"""@en ;
    rdfs:subClassOf [ a owl:Restriction ;
            owl:hasValue 0e+00 ;
            owl:onProperty ns1:hasSIConversionOffset ],
        [ a owl:Restriction ;
            owl:hasValue 1e-18 ;
            owl:onProperty ns1:hasSIConversionMultiplier ],
        [ a owl:Restriction ;
            owl:onProperty ns1:hasUnitSymbol ;
            owl:someValuesFrom ns1:JouleSecond ],
        ns1:AngularMomentumUnit,
        ns1:AttoPrefixedUnit,
        ns1:PrefixedUnit,
        ns1:SINonCoherentUnit ;
    skos:altLabel "Attojoule Second"@en ;
    skos:prefLabel "AttoJouleSecond"^^xsd:string ;
    ns1:elucidation """unit of the Planck's constant as product of the SI derived unit joule and the SI base unit second

-- QUDT"""@en ;
    ns1:qudtReference "http://qudt.org/vocab/unit/AttoJ-SEC"^^xsd:string ;
    ns1:ucumCode "aJ.s"^^xsd:string ;
    ns1:unitSymbol "aJ⋅s"^^xsd:string .

ns1:CentiMetrePerKelvin a owl:Class ;
    rdfs:label "CentiMetrePerKelvin"^^xsd:string ;
    rdfs:comment """0,01-fold of the SI base unit metre divided by the SI base unit kelvin

-- QUDT"""@en ;
    rdfs:subClassOf [ a owl:Restriction ;
            owl:onProperty ns1:hasUnitSymbol ;
            owl:someValuesFrom ns1:MetrePerKelvin ],
        [ a owl:Restriction ;
            owl:hasValue 0e+00 ;
            owl:onProperty ns1:hasSIConversionOffset ],
        [ a owl:Restriction ;
            owl:hasValue 1e-02 ;
            owl:onProperty ns1:hasSIConversionMultiplier ],
        ns1:CentiPrefixedUnit,
        ns1:LengthPerTemperatureUnit,
        ns1:PrefixedUnit,
        ns1:SINonCoherentUnit ;
    skos:altLabel "Centimetre Per Kelvin"@en ;
    skos:prefLabel "CentiMetrePerKelvin"^^xsd:string ;
    ns1:elucidation """0,01-fold of the SI base unit metre divided by the SI base unit kelvin

-- QUDT"""@en ;
    ns1:qudtReference "http://qudt.org/vocab/unit/CentiM-PER-K"^^xsd:string ;
    ns1:ucumCode "cm.K-1"^^xsd:string,
        "cm/K"^^xsd:string ;
    ns1:unitSymbol "cm/K"^^xsd:string .

ns1:CentiMetrePerSecond a owl:Class ;
    rdfs:label "CentiMetrePerSecond"^^xsd:string ;
    rdfs:comment """"Centimeter per Second" is a C.G.S System unit for  'Linear Velocity' expressed as cm/s.

-- QUDT"""@en ;
    rdfs:subClassOf [ a owl:Restriction ;
            owl:hasValue 1e-02 ;
            owl:onProperty ns1:hasSIConversionMultiplier ],
        [ a owl:Restriction ;
            owl:hasValue 0e+00 ;
            owl:onProperty ns1:hasSIConversionOffset ],
        [ a owl:Restriction ;
            owl:onProperty ns1:hasUnitNonPrefixPart ;
            owl:someValuesFrom ns1:MetrePerSecond ],
        ns1:CentiPrefixedUnit,
        ns1:PrefixedUnit,
        ns1:SINonCoherentUnit,
        ns1:SpeedUnit ;
    skos:altLabel "centimetre per second"@en ;
    skos:prefLabel "CentiMetrePerSecond"^^xsd:string ;
    ns1:elucidation """"Centimeter per Second" is a C.G.S System unit for  'Linear Velocity' expressed as cm/s.

-- QUDT"""@en ;
    ns1:qudtReference "http://qudt.org/vocab/unit/CentiM-PER-SEC"^^xsd:string ;
    ns1:ucumCode "cm.s-1"^^xsd:string,
        "cm/s"^^xsd:string ;
    ns1:unitSymbol "cm/s"^^xsd:string .

ns1:CentiMetrePerSquareSecond a owl:Class ;
    rdfs:label "CentiMetrePerSquareSecond"^^xsd:string ;
    rdfs:comment """`Centimeter per Square Second` is a C.G.S System unit for  `Linear Acceleration` expressed as cm/s².

-- QUDT"""@en ;
    rdfs:subClassOf [ a owl:Restriction ;
            owl:hasValue 1e-02 ;
            owl:onProperty ns1:hasSIConversionMultiplier ],
        [ a owl:Restriction ;
            owl:hasValue 0e+00 ;
            owl:onProperty ns1:hasSIConversionOffset ],
        [ a owl:Restriction ;
            owl:onProperty ns1:hasUnitSymbol ;
            owl:someValuesFrom ns1:MetrePerSquareSecond ],
        ns1:AccelerationUnit,
        ns1:CentiPrefixedUnit,
        ns1:PrefixedUnit,
        ns1:SINonCoherentUnit ;
    skos:altLabel "Centimetre per Square Second"@en ;
    skos:prefLabel "CentiMetrePerSquareSecond"^^xsd:string ;
    ns1:elucidation """`Centimeter per Square Second` is a C.G.S System unit for  `Linear Acceleration` expressed as cm/s².

-- QUDT"""@en ;
    ns1:qudtReference "http://qudt.org/vocab/unit/CentiM-PER-SEC2"^^xsd:string ;
    ns1:ucumCode "cm.s-2"^^xsd:string,
        "cm/s2"^^xsd:string ;
    ns1:unitSymbol "cm/s²"^^xsd:string .

ns1:CentiMetreSecondDegreeCelsius a owl:Class ;
    rdfs:label "CentiMetreSecondDegreeCelsius"^^xsd:string ;
    rdfs:comment """`Centimeter Second Degree Celsius` is a C.G.S System unit for 'Length Temperature Time' expressed as cm-s-degC.

-- QUDT"""@en ;
    rdfs:subClassOf ns1:CentiPrefixedUnit,
        ns1:LengthTimeTemperatureUnit,
        ns1:NonSIUnit,
        ns1:PrefixedUnit ;
    skos:altLabel "Centimetre Second Degree Celsius"@en ;
    skos:prefLabel "CentiMetreSecondDegreeCelsius"^^xsd:string ;
    ns1:elucidation """`Centimeter Second Degree Celsius` is a C.G.S System unit for 'Length Temperature Time' expressed as cm-s-degC.

-- QUDT"""@en ;
    ns1:qudtReference "http://qudt.org/vocab/unit/CentiM-SEC-DEG_C"^^xsd:string ;
    ns1:ucumCode "cm.s.Cel-1"^^xsd:string,
        "cm.s/Cel"^^xsd:string ;
    ns1:unitSymbol "cm⋅s⋅°C"^^xsd:string .

ns1:CentiMolePerKilogram a owl:Class ;
    rdfs:label "CentiMolePerKilogram"^^xsd:string ;
    rdfs:comment """1/100 of SI unit of amount of substance per kilogram

-- QUDT"""@en ;
    rdfs:subClassOf [ a owl:Restriction ;
            owl:hasValue 1e-02 ;
            owl:onProperty ns1:hasSIConversionMultiplier ],
        [ a owl:Restriction ;
            owl:hasValue 0e+00 ;
            owl:onProperty ns1:hasSIConversionOffset ],
        ns1:AmountPerMassUnit,
        ns1:CentiPrefixedUnit,
        ns1:PrefixedUnit,
        ns1:SINonCoherentUnit ;
    skos:altLabel "Centimole per kilogram"@en ;
    skos:prefLabel "CentiMolePerKilogram"^^xsd:string ;
    ns1:elucidation """1/100 of SI unit of amount of substance per kilogram

-- QUDT"""@en ;
    ns1:qudtReference "http://qudt.org/vocab/unit/CentiMOL-PER-KiloGM"^^xsd:string ;
    ns1:ucumCode "cmol.kg-1"^^xsd:string,
        "cmol/kg"^^xsd:string ;
    ns1:unitSymbol "cmol/kg"^^xsd:string .

ns1:CentiNewtonMetre a owl:Class ;
    rdfs:label "CentiNewtonMetre"^^xsd:string ;
    rdfs:comment """0,01-fold of the product of the SI derived unit newton and SI base unit metre

-- QUDT"""@en ;
    rdfs:subClassOf [ a owl:Restriction ;
            owl:hasValue 1e-02 ;
            owl:onProperty ns1:hasSIConversionMultiplier ],
        [ a owl:Restriction ;
            owl:onProperty ns1:hasUnitNonPrefixPart ;
            owl:someValuesFrom ns1:NewtonMetre ],
        [ a owl:Restriction ;
            owl:hasValue 0e+00 ;
            owl:onProperty ns1:hasSIConversionOffset ],
        ns1:CentiPrefixedUnit,
        ns1:EnergyUnit,
        ns1:PrefixedUnit,
        ns1:SINonCoherentUnit ;
    skos:altLabel "Centinewton Metre"@en ;
    skos:prefLabel "CentiNewtonMetre"^^xsd:string ;
    ns1:elucidation """0,01-fold of the product of the SI derived unit newton and SI base unit metre

-- QUDT"""@en ;
    ns1:qudtReference "http://qudt.org/vocab/unit/CentiN-M"^^xsd:string ;
    ns1:ucumCode "cN.m"^^xsd:string ;
    ns1:unitSymbol "cN⋅m"^^xsd:string .

ns1:CoulombPerCubicCentiMetre a owl:Class ;
    rdfs:label "CoulombPerCubicCentiMetre"@en ;
    rdfs:comment """derived SI unit coulomb divided by the 0.000 001-fold of the power of the SI base unit metre by exponent 3

-- QUDT"""@en ;
    rdfs:isDefinedBy "http://qudt.org/2.1/vocab/unit"^^xsd:string ;
    rdfs:subClassOf [ a owl:Restriction ;
            owl:hasValue 0e+00 ;
            owl:onProperty ns1:hasSIConversionOffset ],
        [ a owl:Restriction ;
            owl:hasValue 1e+06 ;
            owl:onProperty ns1:hasSIConversionMultiplier ],
        ns1:ElectricChargeDensityUnit,
        ns1:SINonCoherentDerivedUnit ;
    skos:altLabel "Coulomb Per Cubic Centimetre"@en ;
    skos:prefLabel "CoulombPerCubicCentiMetre"@en ;
    ns1:elucidation """derived SI unit coulomb divided by the 0.000 001-fold of the power of the SI base unit metre by exponent 3

-- QUDT"""@en ;
    ns1:qudtReference "http://qudt.org/vocab/unit/C-PER-CentiM3"^^xsd:string ;
    ns1:ucumCode "C.cm-3"^^xsd:string,
        "C/cm3"^^xsd:string ;
    ns1:unitSymbol "C/cm³"^^xsd:string .

ns1:CoulombPerCubicMilliMetre a owl:Class ;
    rdfs:label "CoulombPerCubicMilliMetre"@en ;
    rdfs:comment """derived SI unit coulomb divided by the 0.000 000 001-fold of the power of the SI base unit metre by exponent 3

-- QUDT"""@en ;
    rdfs:isDefinedBy "http://qudt.org/2.1/vocab/unit"^^xsd:string ;
    rdfs:subClassOf [ a owl:Restriction ;
            owl:hasValue 1e+09 ;
            owl:onProperty ns1:hasSIConversionMultiplier ],
        [ a owl:Restriction ;
            owl:hasValue 0e+00 ;
            owl:onProperty ns1:hasSIConversionOffset ],
        ns1:ElectricChargeDensityUnit,
        ns1:SINonCoherentDerivedUnit ;
    skos:altLabel "Coulomb Per Cubic Millimetre"@en ;
    skos:prefLabel "CoulombPerCubicMilliMetre"@en ;
    ns1:elucidation """derived SI unit coulomb divided by the 0.000 000 001-fold of the power of the SI base unit metre by exponent 3

-- QUDT"""@en ;
    ns1:qudtReference "http://qudt.org/vocab/unit/C-PER-MilliM3"^^xsd:string ;
    ns1:ucumCode "C.mm-3"^^xsd:string,
        "C/mm3"^^xsd:string ;
    ns1:unitSymbol "C/mm³"^^xsd:string .

ns1:CoulombPerSquareCentiMetre a owl:Class ;
    rdfs:label "CoulombPerSquareCentiMetre"@en ;
    rdfs:comment """derived SI unit coulomb divided by the 0.0001-fold of the power of the SI base unit metre by exponent 2

-- QUDT"""@en ;
    rdfs:isDefinedBy "http://qudt.org/2.1/vocab/unit"^^xsd:string ;
    rdfs:subClassOf [ a owl:Restriction ;
            owl:hasValue 0e+00 ;
            owl:onProperty ns1:hasSIConversionOffset ],
        [ a owl:Restriction ;
            owl:hasValue 1e+04 ;
            owl:onProperty ns1:hasSIConversionMultiplier ],
        ns1:ElectricDisplacementFieldUnit,
        ns1:SINonCoherentDerivedUnit ;
    skos:altLabel "Coulomb Per Square Centimetre"@en ;
    skos:prefLabel "CoulombPerSquareCentiMetre"@en ;
    ns1:elucidation """derived SI unit coulomb divided by the 0.0001-fold of the power of the SI base unit metre by exponent 2

-- QUDT"""@en ;
    ns1:qudtReference "http://qudt.org/vocab/unit/C-PER-CentiM2"^^xsd:string ;
    ns1:ucumCode "C.cm-2"^^xsd:string,
        "C/cm2"^^xsd:string ;
    ns1:unitSymbol "C/cm²"^^xsd:string .

ns1:CoulombPerSquareMilliMetre a owl:Class ;
    rdfs:label "CoulombPerSquareMilliMetre"@en ;
    rdfs:comment """derived SI unit coulomb divided by the 0.000 001-fold of the power of the SI base unit metre by exponent 2

-- QUDT"""@en ;
    rdfs:isDefinedBy "http://qudt.org/2.1/vocab/unit"^^xsd:string ;
    rdfs:subClassOf [ a owl:Restriction ;
            owl:hasValue 1e+06 ;
            owl:onProperty ns1:hasSIConversionMultiplier ],
        [ a owl:Restriction ;
            owl:hasValue 0e+00 ;
            owl:onProperty ns1:hasSIConversionOffset ],
        ns1:ElectricDisplacementFieldUnit,
        ns1:SINonCoherentDerivedUnit ;
    skos:altLabel "Coulomb Per Square Millimetre"@en ;
    skos:prefLabel "CoulombPerSquareMilliMetre"@en ;
    ns1:elucidation """derived SI unit coulomb divided by the 0.000 001-fold of the power of the SI base unit metre by exponent 2

-- QUDT"""@en ;
    ns1:qudtReference "http://qudt.org/vocab/unit/C-PER-MilliM2"^^xsd:string ;
    ns1:ucumCode "C.mm-2"^^xsd:string,
        "C/mm2"^^xsd:string ;
    ns1:unitSymbol "C/mm²"^^xsd:string .

ns1:CubicCentiMetre a owl:Class ;
    rdfs:label "CubicCentiMetre"@en ;
    rdfs:comment """The CGS unit of volume, equal to 10-6 cubic meter, 1 milliliter, or about 0.061 023 7 cubic inch

-- QUDT"""@en ;
    rdfs:isDefinedBy "http://qudt.org/2.1/vocab/unit"^^xsd:string ;
    rdfs:subClassOf [ a owl:Restriction ;
            owl:hasValue 0e+00 ;
            owl:onProperty ns1:hasSIConversionOffset ],
        [ a owl:Restriction ;
            owl:hasValue 1e-06 ;
            owl:onProperty ns1:hasSIConversionMultiplier ],
        ns1:SINonCoherentDerivedUnit,
        ns1:VolumeUnit ;
    skos:altLabel "cubic centimetre"@en ;
    skos:prefLabel "CubicCentiMetre"@en ;
    ns1:elucidation """The CGS unit of volume, equal to 10-6 cubic meter, 1 milliliter, or about 0.061 023 7 cubic inch

-- QUDT"""@en ;
    ns1:qudtReference "http://qudt.org/vocab/unit/CentiM3"^^xsd:string ;
    ns1:ucumCode "cm3"^^xsd:string ;
    ns1:unitSymbol "cm³"^^xsd:string .

ns1:CubicCentiMetrePerCubicCentiMetre a owl:Class ;
    rdfs:label "CubicCentiMetrePerCubicCentiMetre"@en ;
    rdfs:comment """volume ratio consisting of the 0.000 001-fold of the power of the SI base unit metre with the exponent 3 divided by the power of the SI base unit metre with the exponent 3

-- QUDT"""@en ;
    rdfs:isDefinedBy "http://qudt.org/2.1/vocab/unit"^^xsd:string ;
    rdfs:subClassOf [ a owl:Restriction ;
            owl:hasValue 0e+00 ;
            owl:onProperty ns1:hasSIConversionOffset ],
        [ a owl:Restriction ;
            owl:hasValue 1e+00 ;
            owl:onProperty ns1:hasSIConversionMultiplier ],
        ns1:SINonCoherentDerivedUnit,
        ns1:VolumeFractionUnit ;
    skos:altLabel "Cubic Centimetre Per Cubic Centimetre"@en ;
    skos:prefLabel "CubicCentiMetrePerCubicCentiMetre"@en ;
    ns1:elucidation """volume ratio consisting of the 0.000 001-fold of the power of the SI base unit metre with the exponent 3 divided by the power of the SI base unit metre with the exponent 3

-- QUDT"""@en ;
    ns1:qudtReference "http://qudt.org/vocab/unit/CentiM3-PER-CentiM3"^^xsd:string ;
    ns1:ucumCode "cm3.cm-3"^^xsd:string,
        "cm3/cm3"^^xsd:string ;
    ns1:unitSymbol "cm³/cm³"^^xsd:string .

ns1:CubicCentiMetrePerCubicMetre a owl:Class ;
    rdfs:label "CubicCentiMetrePerCubicMetre"@en ;
    rdfs:comment """volume ratio consisting of the 0.000 001-fold of the power of the SI base unit metre with the exponent 3 divided by the power of the SI base unit metre with the exponent 3

-- QUDT"""@en ;
    rdfs:isDefinedBy "http://qudt.org/2.1/vocab/unit"^^xsd:string ;
    rdfs:subClassOf [ a owl:Restriction ;
            owl:hasValue 0e+00 ;
            owl:onProperty ns1:hasSIConversionOffset ],
        [ a owl:Restriction ;
            owl:hasValue 1e-06 ;
            owl:onProperty ns1:hasSIConversionMultiplier ],
        ns1:SINonCoherentDerivedUnit,
        ns1:VolumeFractionUnit ;
    skos:altLabel "Cubic Centimetre Per Cubic Metre"@en ;
    skos:prefLabel "CubicCentiMetrePerCubicMetre"@en ;
    ns1:elucidation """volume ratio consisting of the 0.000 001-fold of the power of the SI base unit metre with the exponent 3 divided by the power of the SI base unit metre with the exponent 3

-- QUDT"""@en ;
    ns1:qudtReference "http://qudt.org/vocab/unit/CentiM3-PER-M3"^^xsd:string ;
    ns1:ucumCode "cm3.m-3"^^xsd:string,
        "cm3/m3"^^xsd:string ;
    ns1:unitSymbol "cm³/m³"^^xsd:string .

ns1:CubicCentiMetrePerKelvin a owl:Class ;
    rdfs:label "CubicCentiMetrePerKelvin"@en ;
    rdfs:comment """0,000 001-fold of the power of the SI base unit metre with the exponent 3 divided by the SI base unit kelvin

-- QUDT"""@en ;
    rdfs:isDefinedBy "http://qudt.org/2.1/vocab/unit"^^xsd:string ;
    rdfs:subClassOf [ a owl:Restriction ;
            owl:hasValue 0e+00 ;
            owl:onProperty ns1:hasSIConversionOffset ],
        [ a owl:Restriction ;
            owl:hasValue 1e-06 ;
            owl:onProperty ns1:hasSIConversionMultiplier ],
        ns1:SINonCoherentDerivedUnit,
        ns1:VolumePerTemperatureUnit ;
    skos:altLabel "Cubic Centimetre Per Kelvin"@en ;
    skos:prefLabel "CubicCentiMetrePerKelvin"@en ;
    ns1:elucidation """0,000 001-fold of the power of the SI base unit metre with the exponent 3 divided by the SI base unit kelvin

-- QUDT"""@en ;
    ns1:qudtReference "http://qudt.org/vocab/unit/CentiM3-PER-K"^^xsd:string ;
    ns1:ucumCode "cm3.K-1"^^xsd:string,
        "cm3/K"^^xsd:string ;
    ns1:unitSymbol "cm³/K"^^xsd:string .

ns1:CubicCentiMetrePerMole a owl:Class ;
    rdfs:label "CubicCentiMetrePerMole"@en ;
    rdfs:comment """0.000 001-fold of the power of the SI base unit metre with the exponent 3 divided by the SI base unit mol

-- QUDT"""@en ;
    rdfs:isDefinedBy "http://qudt.org/2.1/vocab/unit"^^xsd:string ;
    rdfs:subClassOf [ a owl:Restriction ;
            owl:hasValue 0e+00 ;
            owl:onProperty ns1:hasSIConversionOffset ],
        [ a owl:Restriction ;
            owl:hasValue 1e-06 ;
            owl:onProperty ns1:hasSIConversionMultiplier ],
        ns1:SINonCoherentDerivedUnit,
        ns1:VolumePerAmountUnit ;
    skos:altLabel "Cubic Centimetre Per Mole"@en ;
    skos:prefLabel "CubicCentiMetrePerMole"@en ;
    ns1:elucidation """0.000 001-fold of the power of the SI base unit metre with the exponent 3 divided by the SI base unit mol

-- QUDT"""@en ;
    ns1:qudtReference "http://qudt.org/vocab/unit/CentiM3-PER-MOL"^^xsd:string ;
    ns1:ucumCode "cm3.mol-1"^^xsd:string,
        "cm3/mol"^^xsd:string ;
    ns1:unitSymbol "cm³/mol"^^xsd:string .

ns1:CubicCentiMetrePerMoleSecond a owl:Class ;
    rdfs:label "CubicCentiMetrePerMoleSecond"@en ;
    rdfs:comment """A unit that is the 0.000001-fold of the power of the SI base unit metre with the exponent 3 divided by the SI base unit mol multiplied by the SI base unit second.

-- QUDT"""@en ;
    rdfs:isDefinedBy "http://qudt.org/2.1/vocab/unit"^^xsd:string ;
    rdfs:subClassOf [ a owl:Restriction ;
            owl:hasValue 1e-06 ;
            owl:onProperty ns1:hasSIConversionMultiplier ],
        [ a owl:Restriction ;
            owl:hasValue 0e+00 ;
            owl:onProperty ns1:hasSIConversionOffset ],
        ns1:SINonCoherentDerivedUnit,
        ns1:VolumePerAmountTimeUnit ;
    skos:altLabel "Cubic centimeter per mole second"@en ;
    skos:prefLabel "CubicCentiMetrePerMoleSecond"@en ;
    ns1:elucidation """A unit that is the 0.000001-fold of the power of the SI base unit metre with the exponent 3 divided by the SI base unit mol multiplied by the SI base unit second.

-- QUDT"""@en ;
    ns1:qudtReference "http://qudt.org/vocab/unit/CentiM3-PER-MOL-SEC"^^xsd:string ;
    ns1:unitSymbol "cm³/(mol⋅s)"^^xsd:string .

ns1:CubicCentiMetrePerSecond a owl:Class ;
    rdfs:label "CubicCentiMetrePerSecond"@en ;
    rdfs:comment """0,000 001-fold of the power of the SI base unit metre with the exponent 3 divided by the SI base unit second

-- QUDT"""@en ;
    rdfs:isDefinedBy "http://qudt.org/2.1/vocab/unit"^^xsd:string ;
    rdfs:subClassOf [ a owl:Restriction ;
            owl:hasValue 0e+00 ;
            owl:onProperty ns1:hasSIConversionOffset ],
        [ a owl:Restriction ;
            owl:hasValue 1e-06 ;
            owl:onProperty ns1:hasSIConversionMultiplier ],
        ns1:SINonCoherentDerivedUnit,
        ns1:VolumePerTimeUnit ;
    skos:altLabel "Cubic Centimetre Per Second"@en ;
    skos:prefLabel "CubicCentiMetrePerSecond"@en ;
    ns1:elucidation """0,000 001-fold of the power of the SI base unit metre with the exponent 3 divided by the SI base unit second

-- QUDT"""@en ;
    ns1:qudtReference "http://qudt.org/vocab/unit/CentiM3-PER-SEC"^^xsd:string ;
    ns1:ucumCode "cm3.s-1"^^xsd:string,
        "cm3/s"^^xsd:string ;
    ns1:unitSymbol "cm³/s"^^xsd:string .

ns1:CubicDecaMetre a owl:Class ;
    rdfs:label "CubicDecaMetre"@en ;
    rdfs:comment """1 000-fold of the power of the SI base unit metre by exponent 3

-- QUDT"""@en ;
    rdfs:isDefinedBy "http://qudt.org/2.1/vocab/unit"^^xsd:string ;
    rdfs:subClassOf [ a owl:Restriction ;
            owl:hasValue 0e+00 ;
            owl:onProperty ns1:hasSIConversionOffset ],
        [ a owl:Restriction ;
            owl:hasValue 1e+03 ;
            owl:onProperty ns1:hasSIConversionMultiplier ],
        ns1:SINonCoherentDerivedUnit,
        ns1:VolumeUnit ;
    skos:altLabel "Cubic Decametre"@en ;
    skos:prefLabel "CubicDecaMetre"@en ;
    ns1:elucidation """1 000-fold of the power of the SI base unit metre by exponent 3

-- QUDT"""@en ;
    ns1:qudtReference "http://qudt.org/vocab/unit/DecaM3"^^xsd:string ;
    ns1:ucumCode "dam3"^^xsd:string ;
    ns1:unitSymbol "dam³"^^xsd:string .

ns1:CubicDeciMetre a owl:Class ;
    rdfs:label "CubicDeciMetre"@en ;
    rdfs:comment """0.1-fold of the power of the SI base unit metre with the exponent 3

-- QUDT"""@en ;
    rdfs:isDefinedBy "http://qudt.org/2.1/vocab/unit"^^xsd:string ;
    rdfs:subClassOf [ a owl:Restriction ;
            owl:hasValue 0e+00 ;
            owl:onProperty ns1:hasSIConversionOffset ],
        [ a owl:Restriction ;
            owl:hasValue 1e-03 ;
            owl:onProperty ns1:hasSIConversionMultiplier ],
        ns1:SINonCoherentDerivedUnit,
        ns1:VolumeUnit ;
    skos:altLabel "Cubic Decimetre"@en ;
    skos:prefLabel "CubicDeciMetre"@en ;
    ns1:elucidation """0.1-fold of the power of the SI base unit metre with the exponent 3

-- QUDT"""@en ;
    ns1:qudtReference "http://qudt.org/vocab/unit/DeciM3"^^xsd:string ;
    ns1:ucumCode "dm3"^^xsd:string ;
    ns1:unitSymbol "dm³"^^xsd:string .

ns1:CubicDeciMetrePerCubicMetre a owl:Class ;
    rdfs:label "CubicDeciMetrePerCubicMetre"@en ;
    rdfs:comment """volume ratio consisting of the 0.001-fold of the power of the SI base unit metre with the exponent 3 divided by the power of the SI base unit metre with the exponent 3

-- QUDT"""@en ;
    rdfs:isDefinedBy "http://qudt.org/2.1/vocab/unit"^^xsd:string ;
    rdfs:subClassOf [ a owl:Restriction ;
            owl:hasValue 1e-03 ;
            owl:onProperty ns1:hasSIConversionMultiplier ],
        [ a owl:Restriction ;
            owl:hasValue 0e+00 ;
            owl:onProperty ns1:hasSIConversionOffset ],
        ns1:SINonCoherentDerivedUnit,
        ns1:VolumeFractionUnit ;
    skos:altLabel "Cubic Decimetre Per Cubic Metre"@en ;
    skos:prefLabel "CubicDeciMetrePerCubicMetre"@en ;
    ns1:elucidation """volume ratio consisting of the 0.001-fold of the power of the SI base unit metre with the exponent 3 divided by the power of the SI base unit metre with the exponent 3

-- QUDT"""@en ;
    ns1:qudtReference "http://qudt.org/vocab/unit/DeciM3-PER-M3"^^xsd:string ;
    ns1:ucumCode "dm3.m-3"^^xsd:string,
        "dm3/m3"^^xsd:string ;
    ns1:unitSymbol "dm³/m³"^^xsd:string .

ns1:CubicDeciMetrePerMole a owl:Class ;
    rdfs:label "CubicDeciMetrePerMole"@en ;
    rdfs:comment """0,001-fold of the power of the SI base unit metre with the exponent 3 divided by the SI base unit mol

-- QUDT"""@en ;
    rdfs:isDefinedBy "http://qudt.org/2.1/vocab/unit"^^xsd:string ;
    rdfs:subClassOf [ a owl:Restriction ;
            owl:hasValue 0e+00 ;
            owl:onProperty ns1:hasSIConversionOffset ],
        [ a owl:Restriction ;
            owl:hasValue 1e-03 ;
            owl:onProperty ns1:hasSIConversionMultiplier ],
        ns1:SINonCoherentDerivedUnit,
        ns1:VolumePerAmountUnit ;
    skos:altLabel "Cubic Decimetre Per Mole"@en ;
    skos:prefLabel "CubicDeciMetrePerMole"@en ;
    ns1:elucidation """0,001-fold of the power of the SI base unit metre with the exponent 3 divided by the SI base unit mol

-- QUDT"""@en ;
    ns1:qudtReference "http://qudt.org/vocab/unit/DeciM3-PER-MOL"^^xsd:string ;
    ns1:ucumCode "dm3.mol-1"^^xsd:string,
        "dm3/mol"^^xsd:string ;
    ns1:unitSymbol "dm³/mol"^^xsd:string .

ns1:CubicDeciMetrePerSecond a owl:Class ;
    rdfs:label "CubicDeciMetrePerSecond"@en ;
    rdfs:comment """0,001-fold of the power of the SI base unit metre with the exponent 3 divided by the unit for time second

-- QUDT"""@en ;
    rdfs:isDefinedBy "http://qudt.org/2.1/vocab/unit"^^xsd:string ;
    rdfs:subClassOf [ a owl:Restriction ;
            owl:hasValue 1e-03 ;
            owl:onProperty ns1:hasSIConversionMultiplier ],
        [ a owl:Restriction ;
            owl:hasValue 0e+00 ;
            owl:onProperty ns1:hasSIConversionOffset ],
        ns1:SINonCoherentDerivedUnit,
        ns1:VolumePerTimeUnit ;
    skos:altLabel "Cubic Decimetre Per Second"@en ;
    skos:prefLabel "CubicDeciMetrePerSecond"@en ;
    ns1:elucidation """0,001-fold of the power of the SI base unit metre with the exponent 3 divided by the unit for time second

-- QUDT"""@en ;
    ns1:qudtReference "http://qudt.org/vocab/unit/DeciM3-PER-SEC"^^xsd:string ;
    ns1:ucumCode "dm3.s-1"^^xsd:string,
        "dm3/s"^^xsd:string ;
    ns1:unitSymbol "dm³/s"^^xsd:string .

ns1:CubicKiloMetrePerSquareSecond a owl:Class ;
    rdfs:label "CubicKiloMetrePerSquareSecond"@en ;
    rdfs:comment """`Cubic Kilometer per Square Second` is a unit for `Standard Gravitational Parameter` expressed as km³/s².

-- QUDT"""@en ;
    rdfs:isDefinedBy "http://qudt.org/2.1/vocab/unit"^^xsd:string ;
    rdfs:subClassOf [ a owl:Restriction ;
            owl:hasValue 0e+00 ;
            owl:onProperty ns1:hasSIConversionOffset ],
        [ a owl:Restriction ;
            owl:hasValue 1e+09 ;
            owl:onProperty ns1:hasSIConversionMultiplier ],
        ns1:SINonCoherentDerivedUnit,
        ns1:VolumePerSquareTimeUnit ;
    skos:altLabel "Cubic Kilometre per Square Second"@en ;
    skos:prefLabel "CubicKiloMetrePerSquareSecond"@en ;
    ns1:elucidation """`Cubic Kilometer per Square Second` is a unit for `Standard Gravitational Parameter` expressed as km³/s².

-- QUDT"""@en ;
    ns1:qudtReference "http://qudt.org/vocab/unit/KiloM3-PER-SEC2"^^xsd:string ;
    ns1:ucumCode "km3.s-2"^^xsd:string,
        "km3/s2"^^xsd:string ;
    ns1:unitSymbol "km³/s²"^^xsd:string .

ns1:CubicMicroMetrePerCubicMetre a owl:Class ;
    rdfs:label "CubicMicroMetrePerCubicMetre"@en ;
    rdfs:comment "Cubic micrometre per cubic metre unit."@en ;
    rdfs:isDefinedBy "http://qudt.org/2.1/vocab/unit"^^xsd:string ;
    rdfs:subClassOf [ a owl:Restriction ;
            owl:hasValue 1e-18 ;
            owl:onProperty ns1:hasSIConversionMultiplier ],
        [ a owl:Restriction ;
            owl:hasValue 0e+00 ;
            owl:onProperty ns1:hasSIConversionOffset ],
        ns1:SINonCoherentDerivedUnit,
        ns1:VolumeFractionUnit ;
    skos:prefLabel "CubicMicroMetrePerCubicMetre"@en ;
    ns1:elucidation "Cubic micrometre per cubic metre unit."@en ;
    ns1:qudtReference "http://qudt.org/vocab/unit/MicroM3-PER-M3"^^xsd:string ;
    ns1:ucumCode "um3.m-3"^^xsd:string ;
    ns1:unitSymbol "µm³/m³"^^xsd:string .

ns1:CubicMilliMetre a owl:Class ;
    rdfs:label "CubicMilliMetre"@en ;
    rdfs:comment """A metric measure of volume or capacity equal to a cube 1 millimeter on each edge

-- QUDT"""@en ;
    rdfs:isDefinedBy "http://qudt.org/2.1/vocab/unit"^^xsd:string ;
    rdfs:subClassOf [ a owl:Restriction ;
            owl:hasValue 1e-09 ;
            owl:onProperty ns1:hasSIConversionMultiplier ],
        [ a owl:Restriction ;
            owl:hasValue 0e+00 ;
            owl:onProperty ns1:hasSIConversionOffset ],
        ns1:SINonCoherentDerivedUnit,
        ns1:VolumeUnit ;
    skos:altLabel "Cubic Millimetre"@en ;
    skos:prefLabel "CubicMilliMetre"@en ;
    ns1:elucidation """A metric measure of volume or capacity equal to a cube 1 millimeter on each edge

-- QUDT"""@en ;
    ns1:qudtReference "http://qudt.org/vocab/unit/MilliM3"^^xsd:string ;
    ns1:ucumCode "mm3"^^xsd:string ;
    ns1:unitSymbol "mm³"^^xsd:string .

ns1:CubicMilliMetrePerCubicMetre a owl:Class ;
    rdfs:label "CubicMilliMetrePerCubicMetre"@en ;
    rdfs:comment """volume ratio consisting of the 0.000000001-fold of the power of the SI base unit metre with the exponent 3 divided by the power of the SI base unit metre with the exponent 3

-- QUDT"""@en ;
    rdfs:isDefinedBy "http://qudt.org/2.1/vocab/unit"^^xsd:string ;
    rdfs:subClassOf [ a owl:Restriction ;
            owl:hasValue 0e+00 ;
            owl:onProperty ns1:hasSIConversionOffset ],
        [ a owl:Restriction ;
            owl:hasValue 1e-09 ;
            owl:onProperty ns1:hasSIConversionMultiplier ],
        ns1:SINonCoherentDerivedUnit,
        ns1:VolumeFractionUnit ;
    skos:altLabel "Cubic Millimetre Per Cubic Metre"@en ;
    skos:prefLabel "CubicMilliMetrePerCubicMetre"@en ;
    ns1:elucidation """volume ratio consisting of the 0.000000001-fold of the power of the SI base unit metre with the exponent 3 divided by the power of the SI base unit metre with the exponent 3

-- QUDT"""@en ;
    ns1:qudtReference "http://qudt.org/vocab/unit/MilliM3-PER-M3"^^xsd:string ;
    ns1:ucumCode "mm3.m-3"^^xsd:string ;
    ns1:unitSymbol "mm³/m³"^^xsd:string .

ns1:DeciNewtonMetre a owl:Class ;
    rdfs:label "DeciNewtonMetre"^^xsd:string ;
    rdfs:comment """0.1-fold of the product of the derived SI unit joule and the SI base unit metre

-- QUDT"""@en ;
    rdfs:subClassOf [ a owl:Restriction ;
            owl:onProperty ns1:hasUnitNonPrefixPart ;
            owl:someValuesFrom ns1:NewtonMetre ],
        [ a owl:Restriction ;
            owl:hasValue 0e+00 ;
            owl:onProperty ns1:hasSIConversionOffset ],
        [ a owl:Restriction ;
            owl:hasValue 1e-01 ;
            owl:onProperty ns1:hasSIConversionMultiplier ],
        ns1:DeciPrefixedUnit,
        ns1:EnergyUnit,
        ns1:PrefixedUnit,
        ns1:SINonCoherentUnit ;
    skos:altLabel "Decinewton Metre"@en ;
    skos:prefLabel "DeciNewtonMetre"^^xsd:string ;
    ns1:elucidation """0.1-fold of the product of the derived SI unit joule and the SI base unit metre

-- QUDT"""@en ;
    ns1:qudtReference "http://qudt.org/vocab/unit/DeciN-M"^^xsd:string ;
    ns1:ucumCode "dN.m"^^xsd:string ;
    ns1:unitSymbol "dN⋅m"^^xsd:string .

ns1:DeciSiemensPerMetre a owl:Class ;
    rdfs:label "DeciSiemensPerMetre"^^xsd:string ;
    rdfs:comment """Decisiemens per metre.

-- QUDT"""@en ;
    rdfs:subClassOf [ a owl:Restriction ;
            owl:hasValue 1e-01 ;
            owl:onProperty ns1:hasSIConversionMultiplier ],
        [ a owl:Restriction ;
            owl:onProperty ns1:hasUnitSymbol ;
            owl:someValuesFrom ns1:SiemensPerMetre ],
        [ a owl:Restriction ;
            owl:hasValue 0e+00 ;
            owl:onProperty ns1:hasSIConversionOffset ],
        ns1:DeciPrefixedUnit,
        ns1:ElectricConductivityUnit,
        ns1:PrefixedUnit,
        ns1:SINonCoherentUnit ;
    skos:altLabel "decisiemens per metre"@en ;
    skos:prefLabel "DeciSiemensPerMetre"^^xsd:string ;
    ns1:elucidation """Decisiemens per metre.

-- QUDT"""@en ;
    ns1:qudtReference "http://qudt.org/vocab/unit/DeciS-PER-M"^^xsd:string ;
    ns1:ucumCode "dS.m-1"^^xsd:string,
        "dS/m"^^xsd:string ;
    ns1:unitSymbol "dS/m"^^xsd:string .

ns1:DegreeCelsiusCentiMetre a owl:Class ;
    rdfs:label "DegreeCelsiusCentiMetre"^^xsd:string ;
    rdfs:comment """`Degree Celsius Centimeter` is a C.G.S System unit for 'Length Temperature' expressed as cm-degC.

-- QUDT"""@en ;
    rdfs:isDefinedBy "http://qudt.org/2.1/vocab/unit"^^xsd:string ;
    rdfs:subClassOf ns1:LengthTemperatureUnit,
        ns1:SINonCoherentDerivedUnit ;
    skos:altLabel "Degree Celsius Centimetre"@en ;
    skos:prefLabel "DegreeCelsiusCentiMetre"^^xsd:string ;
    ns1:elucidation """`Degree Celsius Centimeter` is a C.G.S System unit for 'Length Temperature' expressed as cm-degC.

-- QUDT"""@en ;
    ns1:qudtReference "http://qudt.org/vocab/unit/DEG_C-CentiM"^^xsd:string ;
    ns1:ucumCode "Cel.cm"^^xsd:string ;
    ns1:unitSymbol "°C⋅cm"^^xsd:string .

ns1:FaradPerKiloMetre a owl:Class ;
    rdfs:label "FaradPerKiloMetre"@en ;
    rdfs:comment """SI derived unit farad divided by the 1 000-fold of the SI base unit metre

-- QUDT"""@en ;
    rdfs:isDefinedBy "http://qudt.org/2.1/vocab/unit"^^xsd:string ;
    rdfs:subClassOf [ a owl:Restriction ;
            owl:hasValue 1e-03 ;
            owl:onProperty ns1:hasSIConversionMultiplier ],
        [ a owl:Restriction ;
            owl:hasValue 0e+00 ;
            owl:onProperty ns1:hasSIConversionOffset ],
        ns1:PermittivityUnit,
        ns1:SINonCoherentDerivedUnit ;
    skos:altLabel "Farad Per Kilometre"@en ;
    skos:prefLabel "FaradPerKiloMetre"@en ;
    ns1:elucidation """SI derived unit farad divided by the 1 000-fold of the SI base unit metre

-- QUDT"""@en ;
    ns1:qudtReference "http://qudt.org/vocab/unit/FARAD-PER-KiloM"^^xsd:string ;
    ns1:ucumCode "F.km-1"^^xsd:string,
        "F/km"^^xsd:string ;
    ns1:unitSymbol "F/km"^^xsd:string .

ns1:FemtoGramPerKilogram a owl:Class ;
    rdfs:label "FemtoGramPerKilogram"^^xsd:string ;
    rdfs:comment """One part per 10**18 by mass of the measurand in the matrix.

-- QUDT"""@en ;
    rdfs:subClassOf [ a owl:Restriction ;
            owl:hasValue 1e-18 ;
            owl:onProperty ns1:hasSIConversionMultiplier ],
        [ a owl:Restriction ;
            owl:hasValue 0e+00 ;
            owl:onProperty ns1:hasSIConversionOffset ],
        [ a owl:Restriction ;
            owl:onProperty ns1:hasUnitSymbol ;
            owl:someValuesFrom ns1:GramPerKilogram ],
        ns1:FemtoPrefixedUnit,
        ns1:MassFractionUnit,
        ns1:PrefixedUnit,
        ns1:SINonCoherentUnit ;
    skos:altLabel "Femtograms per kilogram"@en ;
    skos:prefLabel "FemtoGramPerKilogram"^^xsd:string ;
    ns1:elucidation """One part per 10**18 by mass of the measurand in the matrix.

-- QUDT"""@en ;
    ns1:qudtReference "http://qudt.org/vocab/unit/FemtoGM-PER-KiloGM"^^xsd:string ;
    ns1:ucumCode "fg.kg-1"^^xsd:string ;
    ns1:unitSymbol "fg/kg"^^xsd:string .

ns1:FemtoMolePerKilogram a owl:Class ;
    rdfs:label "FemtoMolePerKilogram"^^xsd:string ;
    rdfs:comment """A 10**15 part quantity of substance of the measurand per kilogram mass of matrix.

-- QUDT"""@en ;
    rdfs:subClassOf [ a owl:Restriction ;
            owl:hasValue 1e-15 ;
            owl:onProperty ns1:hasSIConversionMultiplier ],
        [ a owl:Restriction ;
            owl:hasValue 0e+00 ;
            owl:onProperty ns1:hasSIConversionOffset ],
        ns1:AmountPerMassUnit,
        ns1:FemtoPrefixedUnit,
        ns1:PrefixedUnit,
        ns1:SINonCoherentUnit ;
    skos:altLabel "Femtomoles per kilogram"@en ;
    skos:prefLabel "FemtoMolePerKilogram"^^xsd:string ;
    ns1:elucidation """A 10**15 part quantity of substance of the measurand per kilogram mass of matrix.

-- QUDT"""@en ;
    ns1:qudtReference "http://qudt.org/vocab/unit/FemtoMOL-PER-KiloGM"^^xsd:string ;
    ns1:ucumCode "fmol.kg-1"^^xsd:string ;
    ns1:unitSymbol "fmol/kg"^^xsd:string .

ns1:GigaCoulombPerCubicMetre a owl:Class ;
    rdfs:label "GigaCoulombPerCubicMetre"^^xsd:string ;
    rdfs:comment """1 000 000 000-fold of the SI derived unit coulomb divided by the power of the SI base unit metre with the exponent 3

-- QUDT"""@en ;
    rdfs:subClassOf [ a owl:Restriction ;
            owl:hasValue 0e+00 ;
            owl:onProperty ns1:hasSIConversionOffset ],
        [ a owl:Restriction ;
            owl:onProperty ns1:hasUnitSymbol ;
            owl:someValuesFrom ns1:CoulombPerCubicMetre ],
        [ a owl:Restriction ;
            owl:hasValue 1e+09 ;
            owl:onProperty ns1:hasSIConversionMultiplier ],
        ns1:GigaPrefixedUnit,
        ns1:PrefixedUnit,
        ns1:SINonCoherentUnit,
        ns1:SpeedUnit ;
    skos:altLabel "Gigacoulomb Per Cubic Metre"@en ;
    skos:prefLabel "GigaCoulombPerCubicMetre"^^xsd:string ;
    ns1:elucidation """1 000 000 000-fold of the SI derived unit coulomb divided by the power of the SI base unit metre with the exponent 3

-- QUDT"""@en ;
    ns1:qudtReference "http://qudt.org/vocab/unit/GigaC-PER-M3"^^xsd:string ;
    ns1:ucumCode "GC.m-3"^^xsd:string ;
    ns1:unitSymbol "GC/m³"^^xsd:string .

ns1:GigaHertzMetre a owl:Class ;
    rdfs:label "GigaHertzMetre"^^xsd:string ;
    rdfs:comment """product of the 1 000 000 000-fold of the SI derived unit hertz and the SI base unit metre

-- QUDT"""@en ;
    rdfs:subClassOf [ a owl:Restriction ;
            owl:onProperty ns1:hasUnitSymbol ;
            owl:someValuesFrom ns1:HertzMetre ],
        [ a owl:Restriction ;
            owl:hasValue 0e+00 ;
            owl:onProperty ns1:hasSIConversionOffset ],
        [ a owl:Restriction ;
            owl:hasValue 1e+09 ;
            owl:onProperty ns1:hasSIConversionMultiplier ],
        ns1:GigaPrefixedUnit,
        ns1:PrefixedUnit,
        ns1:SINonCoherentUnit,
        ns1:SpeedUnit ;
    skos:altLabel "Gigahertz Metre"@en ;
    skos:prefLabel "GigaHertzMetre"^^xsd:string ;
    ns1:elucidation """product of the 1 000 000 000-fold of the SI derived unit hertz and the SI base unit metre

-- QUDT"""@en ;
    ns1:qudtReference "http://qudt.org/vocab/unit/GigaHZ-M"^^xsd:string ;
    ns1:ucumCode "GHz.m"^^xsd:string ;
    ns1:unitSymbol "GHz⋅M"^^xsd:string .

ns1:Gram a owl:Class ;
    rdfs:label "Gram"@en ;
    rdfs:comment """A unit of mass in the metric system. The name comes from the Greek gramma, a small weight identified in later Roman and Byzantine times with the Latin scripulum or scruple (the English scruple is equal to about 1.3 grams). The gram was originally defined to be the mass of one cubic centimeter of pure water, but to provide precise standards it was necessary to construct physical objects of specified mass. One gram is now defined to be 1/1000 of the mass of the standard kilogram, a platinum-iridium bar carefully guarded by the International Bureau of Weights and Measures in Paris for more than a century. (The kilogram, rather than the gram, is considered the base unit of mass in the SI.) The gram is a small mass, equal to about 15.432 grains or 0.035 273 966 ounce.

-- QUDT"""@en,
        "Gram is defined as one thousandth of the SI unit kilogram."@en ;
    rdfs:subClassOf [ a owl:Restriction ;
            owl:hasValue "g"^^xsd:string ;
            owl:onProperty ns1:unitSymbolValue ],
        [ a owl:Restriction ;
            owl:hasValue 0e+00 ;
            owl:onProperty ns1:hasSIConversionOffset ],
        [ a owl:Restriction ;
            owl:hasValue 1e-03 ;
            owl:onProperty ns1:hasSIConversionMultiplier ],
        ns1:MassUnit,
        ns1:NonPrefixedUnit,
        ns1:SINonCoherentUnit ;
    skos:prefLabel "Gram"@en ;
    schema:unitCode "GRM"^^xsd:string ;
    ns1:definition "Gram is defined as one thousandth of the SI unit kilogram."@en ;
    ns1:elucidation """A unit of mass in the metric system. The name comes from the Greek gramma, a small weight identified in later Roman and Byzantine times with the Latin scripulum or scruple (the English scruple is equal to about 1.3 grams). The gram was originally defined to be the mass of one cubic centimeter of pure water, but to provide precise standards it was necessary to construct physical objects of specified mass. One gram is now defined to be 1/1000 of the mass of the standard kilogram, a platinum-iridium bar carefully guarded by the International Bureau of Weights and Measures in Paris for more than a century. (The kilogram, rather than the gram, is considered the base unit of mass in the SI.) The gram is a small mass, equal to about 15.432 grains or 0.035 273 966 ounce.

-- QUDT"""@en ;
    ns1:iupacReference "https://doi.org/10.1351/goldbook.G02680"^^xsd:string ;
    ns1:qudtReference "http://qudt.org/vocab/unit/GM"^^xsd:string ;
    ns1:ucumCode "g"^^xsd:string ;
    ns1:wikipediaReference "https://en.wikipedia.org/wiki/Gram"^^xsd:string .

ns1:GramDegreeCelsius a owl:Class ;
    rdfs:label "GramDegreeCelsius"@en ;
    rdfs:comment """`Gram Degree Celsius` is a C.G.S System unit for 'Mass Temperature' expressed as g · degC.

-- QUDT"""@en ;
    rdfs:isDefinedBy "http://qudt.org/2.1/vocab/unit"^^xsd:string ;
    rdfs:subClassOf ns1:MassTemperatureUnit,
        ns1:SINonCoherentDerivedUnit ;
    skos:altLabel "Gram Degree Celsius"@en ;
    skos:prefLabel "GramDegreeCelsius"@en ;
    ns1:elucidation """`Gram Degree Celsius` is a C.G.S System unit for 'Mass Temperature' expressed as g · degC.

-- QUDT"""@en ;
    ns1:qudtReference "http://qudt.org/vocab/unit/GM-PER-DEG_C"^^xsd:string ;
    ns1:ucumCode "d.Cel-1"^^xsd:string ;
    ns1:unitSymbol "g/°C"^^xsd:string .

ns1:GramMilliMetre a owl:Class ;
    rdfs:label "GramMilliMetre"^^xsd:string ;
    rdfs:comment """unit of the imbalance as product of the 0.001-fold of the SI base unit kilogram and the 0.001-fold of the SI base unit metre

-- QUDT"""@en ;
    rdfs:isDefinedBy "http://qudt.org/2.1/vocab/unit"^^xsd:string ;
    rdfs:subClassOf [ a owl:Restriction ;
            owl:hasValue 1e-06 ;
            owl:onProperty ns1:hasSIConversionMultiplier ],
        [ a owl:Restriction ;
            owl:hasValue 0e+00 ;
            owl:onProperty ns1:hasSIConversionOffset ],
        ns1:LengthMassUnit,
        ns1:MeasurementUnit,
        ns1:PrefixedUnit,
        ns1:SINonCoherentUnit ;
    skos:altLabel "Gram Millimetre"@en ;
    skos:prefLabel "GramMilliMetre"^^xsd:string ;
    ns1:elucidation """unit of the imbalance as product of the 0.001-fold of the SI base unit kilogram and the 0.001-fold of the SI base unit metre

-- QUDT"""@en ;
    ns1:qudtReference "http://qudt.org/vocab/unit/GM-MilliM"^^xsd:string ;
    ns1:ucumCode "g.mm"^^xsd:string ;
    ns1:unitSymbol "g·mm"^^xsd:string .

ns1:GramPerCubicCentiMetre a owl:Class ;
    rdfs:label "GramPerCubicCentiMetre"^^xsd:string ;
    rdfs:comment """0,001-fold of the SI base unit kilogram divided by the 0.000 001-fold of the power of the SI base unit metre with the exponent 3

-- QUDT"""@en ;
    rdfs:isDefinedBy "http://qudt.org/2.1/vocab/unit"^^xsd:string ;
    rdfs:subClassOf [ a owl:Restriction ;
            owl:hasValue 1e+03 ;
            owl:onProperty ns1:hasSIConversionMultiplier ],
        [ a owl:Restriction ;
            owl:hasValue 0e+00 ;
            owl:onProperty ns1:hasSIConversionOffset ],
        ns1:DensityUnit,
        ns1:MeasurementUnit,
        ns1:PrefixedUnit,
        ns1:SINonCoherentUnit ;
    skos:altLabel "Gram Per Cubic Centimetre"@en ;
    skos:prefLabel "GramPerCubicCentiMetre"^^xsd:string ;
    ns1:elucidation """0,001-fold of the SI base unit kilogram divided by the 0.000 001-fold of the power of the SI base unit metre with the exponent 3

-- QUDT"""@en ;
    ns1:qudtReference "http://qudt.org/vocab/unit/GM-PER-CentiM3"^^xsd:string ;
    ns1:ucumCode "g.cm-3"^^xsd:string,
        "g/cm3"^^xsd:string ;
    ns1:unitSymbol "g/cm³"^^xsd:string .

ns1:GramPerCubicDeciMetre a owl:Class ;
    rdfs:label "GramPerCubicDeciMetre"^^xsd:string ;
    rdfs:comment """0,001-fold of the SI base unit kilogram divided by the 0.001-fold of the power of the SI base unit metre with the exponent 3

-- QUDT"""@en ;
    rdfs:isDefinedBy "http://qudt.org/2.1/vocab/unit"^^xsd:string ;
    rdfs:subClassOf [ a owl:Restriction ;
            owl:hasValue 0e+00 ;
            owl:onProperty ns1:hasSIConversionOffset ],
        [ a owl:Restriction ;
            owl:hasValue 1e+00 ;
            owl:onProperty ns1:hasSIConversionMultiplier ],
        ns1:DensityUnit,
        ns1:MeasurementUnit,
        ns1:PrefixedUnit,
        ns1:SINonCoherentUnit ;
    skos:altLabel "Gram Per Cubic Decimetre"@en ;
    skos:prefLabel "GramPerCubicDeciMetre"^^xsd:string ;
    ns1:elucidation """0,001-fold of the SI base unit kilogram divided by the 0.001-fold of the power of the SI base unit metre with the exponent 3

-- QUDT"""@en ;
    ns1:qudtReference "http://qudt.org/vocab/unit/GM-PER-DeciM3"^^xsd:string ;
    ns1:ucumCode "g.dm-3"^^xsd:string ;
    ns1:unitSymbol "g/dm³"^^xsd:string .

ns1:GramPerKiloMetre a owl:Class ;
    rdfs:label "GramPerKiloMetre"^^xsd:string ;
    rdfs:comment """0,001-fold of the SI base unit kilogram divided by the 1000-fold of the SI base unit metre

-- QUDT"""@en ;
    rdfs:isDefinedBy "http://qudt.org/2.1/vocab/unit"^^xsd:string ;
    rdfs:subClassOf [ a owl:Restriction ;
            owl:hasValue 0e+00 ;
            owl:onProperty ns1:hasSIConversionOffset ],
        [ a owl:Restriction ;
            owl:hasValue 1e-06 ;
            owl:onProperty ns1:hasSIConversionMultiplier ],
        ns1:MassPerLengthUnit,
        ns1:MeasurementUnit,
        ns1:PrefixedUnit,
        ns1:SINonCoherentUnit ;
    skos:altLabel "Gram Per Kilometre"@en ;
    skos:prefLabel "GramPerKiloMetre"^^xsd:string ;
    ns1:elucidation """0,001-fold of the SI base unit kilogram divided by the 1000-fold of the SI base unit metre

-- QUDT"""@en ;
    ns1:qudtReference "http://qudt.org/vocab/unit/GM-PER-KiloM"^^xsd:string ;
    ns1:ucumCode "g.km-1"^^xsd:string ;
    ns1:unitSymbol "g/km"^^xsd:string .

ns1:GramPerMilliMetre a owl:Class ;
    rdfs:label "GramPerMilliMetre"^^xsd:string ;
    rdfs:comment """0,001-fold of the SI base unit kilogram divided by the 0.001-fold the SI base unit meter

-- QUDT"""@en ;
    rdfs:isDefinedBy "http://qudt.org/2.1/vocab/unit"^^xsd:string ;
    rdfs:subClassOf [ a owl:Restriction ;
            owl:hasValue 1e+00 ;
            owl:onProperty ns1:hasSIConversionMultiplier ],
        [ a owl:Restriction ;
            owl:hasValue 0e+00 ;
            owl:onProperty ns1:hasSIConversionOffset ],
        ns1:MassPerLengthUnit,
        ns1:MeasurementUnit,
        ns1:PrefixedUnit,
        ns1:SINonCoherentUnit ;
    skos:altLabel "Gram Per Millimetre"@en ;
    skos:prefLabel "GramPerMilliMetre"^^xsd:string ;
    ns1:elucidation """0,001-fold of the SI base unit kilogram divided by the 0.001-fold the SI base unit meter

-- QUDT"""@en ;
    ns1:qudtReference "http://qudt.org/vocab/unit/GM-PER-MilliM"^^xsd:string ;
    ns1:ucumCode "g.mm-1"^^xsd:string ;
    ns1:unitSymbol "g/mm"^^xsd:string .

ns1:GramPerMole a owl:Class ;
    rdfs:label "GramPerMole"@en ;
    rdfs:comment """0,01-fold of the SI base unit kilogram divided by the SI base unit mol

-- QUDT"""@en ;
    rdfs:isDefinedBy "http://qudt.org/2.1/vocab/unit"^^xsd:string ;
    rdfs:subClassOf [ a owl:Restriction ;
            owl:hasValue 0e+00 ;
            owl:onProperty ns1:hasSIConversionOffset ],
        [ a owl:Restriction ;
            owl:hasValue 1e-03 ;
            owl:onProperty ns1:hasSIConversionMultiplier ],
        ns1:MassPerAmountUnit,
        ns1:MeasurementUnit,
        ns1:NonPrefixedUnit,
        ns1:SINonCoherentUnit ;
    skos:altLabel "Gram Per Mole"@en ;
    skos:prefLabel "GramPerMole"@en ;
    ns1:elucidation """0,01-fold of the SI base unit kilogram divided by the SI base unit mol

-- QUDT"""@en ;
    ns1:qudtReference "http://qudt.org/vocab/unit/GM-PER-MOL"^^xsd:string ;
    ns1:ucumCode "g.mol-1"^^xsd:string ;
    ns1:unitSymbol "g/mol"^^xsd:string .

ns1:HectoPascalCubicMetrePerSecond a owl:Class ;
    rdfs:label "HectoPascalCubicMetrePerSecond"^^xsd:string ;
    rdfs:comment """product out of the 100-fold of the SI unit pascal and the power of the SI base unit metre with the exponent 3 divided by the SI base unit second

-- QUDT"""@en ;
    rdfs:subClassOf [ a owl:Restriction ;
            owl:hasValue 1e+02 ;
            owl:onProperty ns1:hasSIConversionMultiplier ],
        [ a owl:Restriction ;
            owl:hasValue 0e+00 ;
            owl:onProperty ns1:hasSIConversionOffset ],
        [ a owl:Restriction ;
            owl:onProperty ns1:hasUnitSymbol ;
            owl:someValuesFrom ns1:PascalCubicMetrePerSecond ],
        ns1:HectoPrefixedUnit,
        ns1:PowerAreaUnit,
        ns1:PrefixedUnit,
        ns1:SINonCoherentUnit ;
    skos:altLabel "Hectopascal Cubic Metre Per Second"@en ;
    skos:prefLabel "HectoPascalCubicMetrePerSecond"^^xsd:string ;
    ns1:elucidation """product out of the 100-fold of the SI unit pascal and the power of the SI base unit metre with the exponent 3 divided by the SI base unit second

-- QUDT"""@en ;
    ns1:qudtReference "http://qudt.org/vocab/unit/HectoPA-M3-PER-SEC"^^xsd:string ;
    ns1:ucumCode "hPa.m3.s-1"^^xsd:string ;
    ns1:unitSymbol "hPa⋅m³/s"^^xsd:string .

ns1:HectoPascalPerKelvin a owl:Class ;
    rdfs:label "HectoPascalPerKelvin"^^xsd:string ;
    rdfs:comment """100-fold of the SI derived unit pascal divided by the SI base unit kelvin

-- QUDT"""@en ;
    rdfs:subClassOf [ a owl:Restriction ;
            owl:hasValue 1e+02 ;
            owl:onProperty ns1:hasSIConversionMultiplier ],
        [ a owl:Restriction ;
            owl:hasValue 0e+00 ;
            owl:onProperty ns1:hasSIConversionOffset ],
        [ a owl:Restriction ;
            owl:onProperty ns1:hasUnitSymbol ;
            owl:someValuesFrom ns1:PascalPerKelvin ],
        ns1:HectoPrefixedUnit,
        ns1:PrefixedUnit,
        ns1:PressurePerTemperatureUnit,
        ns1:SINonCoherentUnit ;
    skos:altLabel "Hectopascal Per Kelvin"@en ;
    skos:prefLabel "HectoPascalPerKelvin"^^xsd:string ;
    ns1:elucidation """100-fold of the SI derived unit pascal divided by the SI base unit kelvin

-- QUDT"""@en ;
    ns1:qudtReference "http://qudt.org/vocab/unit/HectoPA-PER-K"^^xsd:string ;
    ns1:ucumCode "hPa.K-1"^^xsd:string ;
    ns1:unitSymbol "hPa/K"^^xsd:string .

ns1:JoulePerGram a owl:Class ;
    rdfs:label "JoulePerGram"@en ;
    rdfs:comment """SI derived unit joule divided by the 0.001-fold of the SI base unit kilogram

-- QUDT"""@en ;
    rdfs:isDefinedBy "http://qudt.org/2.1/vocab/unit"^^xsd:string ;
    rdfs:subClassOf [ a owl:Restriction ;
            owl:hasValue 1e+03 ;
            owl:onProperty ns1:hasSIConversionMultiplier ],
        [ a owl:Restriction ;
            owl:hasValue 0e+00 ;
            owl:onProperty ns1:hasSIConversionOffset ],
        ns1:AbsorbedDoseUnit,
        ns1:MeasurementUnit,
        ns1:NonPrefixedUnit,
        ns1:SINonCoherentUnit ;
    skos:altLabel "Joule Per Gram"@en ;
    skos:prefLabel "JoulePerGram"@en ;
    ns1:elucidation """SI derived unit joule divided by the 0.001-fold of the SI base unit kilogram

-- QUDT"""@en ;
    ns1:qudtReference "http://qudt.org/vocab/unit/J-PER-GM"^^xsd:string ;
    ns1:ucumCode "J.g-1"^^xsd:string ;
    ns1:unitSymbol "J/g"^^xsd:string .

ns1:JoulePerSquareCentiMetre a owl:Class ;
    rdfs:label "JoulePerSquareCentiMetre"@en ;
    rdfs:comment """derived SI unit joule divided by the 0.0001-fold of the power of the SI base unit metre by exponent 2

-- QUDT"""@en ;
    rdfs:isDefinedBy "http://qudt.org/2.1/vocab/unit"^^xsd:string ;
    rdfs:subClassOf [ a owl:Restriction ;
            owl:hasValue 1e+04 ;
            owl:onProperty ns1:hasSIConversionMultiplier ],
        [ a owl:Restriction ;
            owl:hasValue 0e+00 ;
            owl:onProperty ns1:hasSIConversionOffset ],
        ns1:ForcePerLengthUnit,
        ns1:SINonCoherentDerivedUnit ;
    skos:altLabel "Joule Per Square Centimetre"@en ;
    skos:prefLabel "JoulePerSquareCentiMetre"@en ;
    ns1:elucidation """derived SI unit joule divided by the 0.0001-fold of the power of the SI base unit metre by exponent 2

-- QUDT"""@en ;
    ns1:qudtReference "http://qudt.org/vocab/unit/J-PER-CentiM2"^^xsd:string ;
    ns1:ucumCode "J.cm-2"^^xsd:string ;
    ns1:unitSymbol "J/cm²"^^xsd:string .

ns1:KiloAmperePerMetre a owl:Class ;
    rdfs:label "KiloAmperePerMetre"^^xsd:string ;
    rdfs:comment """1 000-fold of the SI base unit ampere divided by the SI base unit metre

-- QUDT"""@en ;
    rdfs:subClassOf [ a owl:Restriction ;
            owl:onProperty ns1:hasUnitSymbol ;
            owl:someValuesFrom ns1:AmperePerMetre ],
        [ a owl:Restriction ;
            owl:hasValue 0e+00 ;
            owl:onProperty ns1:hasSIConversionOffset ],
        [ a owl:Restriction ;
            owl:hasValue 1e+03 ;
            owl:onProperty ns1:hasSIConversionMultiplier ],
        ns1:KiloPrefixedUnit,
        ns1:MagneticFieldStrengthUnit,
        ns1:PrefixedUnit,
        ns1:SINonCoherentUnit ;
    skos:altLabel "Kiloampere Per Metre"@en ;
    skos:prefLabel "KiloAmperePerMetre"^^xsd:string ;
    ns1:elucidation """1 000-fold of the SI base unit ampere divided by the SI base unit metre

-- QUDT"""@en ;
    ns1:qudtReference "http://qudt.org/vocab/unit/KiloA-PER-M"^^xsd:string ;
    ns1:ucumCode "kA.m-1"^^xsd:string ;
    ns1:unitSymbol "kA/m"^^xsd:string .

ns1:KiloAmperePerSquareMetre a owl:Class ;
    rdfs:label "KiloAmperePerSquareMetre"^^xsd:string ;
    rdfs:comment """1 000-fold of the SI base unit ampere divided by the power of the SI base unit metre with the exponent 2

-- QUDT"""@en ;
    rdfs:subClassOf [ a owl:Restriction ;
            owl:hasValue 0e+00 ;
            owl:onProperty ns1:hasSIConversionOffset ],
        [ a owl:Restriction ;
            owl:onProperty ns1:hasUnitSymbol ;
            owl:someValuesFrom ns1:AmperePerSquareMetre ],
        [ a owl:Restriction ;
            owl:hasValue 1e+03 ;
            owl:onProperty ns1:hasSIConversionMultiplier ],
        ns1:ElectricCurrentDensityUnit,
        ns1:KiloPrefixedUnit,
        ns1:PrefixedUnit,
        ns1:SINonCoherentUnit ;
    skos:altLabel "Kiloampere Per Square Metre"@en ;
    skos:prefLabel "KiloAmperePerSquareMetre"^^xsd:string ;
    ns1:elucidation """1 000-fold of the SI base unit ampere divided by the power of the SI base unit metre with the exponent 2

-- QUDT"""@en ;
    ns1:qudtReference "http://qudt.org/vocab/unit/KiloA-PER-M2"^^xsd:string ;
    ns1:ucumCode "kA.m-2"^^xsd:string ;
    ns1:unitSymbol "kA/m²"^^xsd:string .

ns1:KiloCoulombPerCubicMetre a owl:Class ;
    rdfs:label "KiloCoulombPerCubicMetre"^^xsd:string ;
    rdfs:comment """1 000-fold of the SI derived unit coulomb divided by the power of the SI base unit metre with the exponent 3

-- QUDT"""@en ;
    rdfs:subClassOf [ a owl:Restriction ;
            owl:hasValue 0e+00 ;
            owl:onProperty ns1:hasSIConversionOffset ],
        [ a owl:Restriction ;
            owl:hasValue 1e+03 ;
            owl:onProperty ns1:hasSIConversionMultiplier ],
        [ a owl:Restriction ;
            owl:onProperty ns1:hasUnitSymbol ;
            owl:someValuesFrom ns1:CoulombPerCubicMetre ],
        ns1:ElectricChargeDensityUnit,
        ns1:KiloPrefixedUnit,
        ns1:PrefixedUnit,
        ns1:SINonCoherentUnit ;
    skos:altLabel "Kilocoulomb Per Cubic Metre"@en ;
    skos:prefLabel "KiloCoulombPerCubicMetre"^^xsd:string ;
    ns1:elucidation """1 000-fold of the SI derived unit coulomb divided by the power of the SI base unit metre with the exponent 3

-- QUDT"""@en ;
    ns1:qudtReference "http://qudt.org/vocab/unit/KiloC-PER-M3"^^xsd:string ;
    ns1:ucumCode "kC.m-3"^^xsd:string ;
    ns1:unitSymbol "kC/m³"^^xsd:string .

ns1:KiloCoulombPerSquareMetre a owl:Class ;
    rdfs:label "KiloCoulombPerSquareMetre"^^xsd:string ;
    rdfs:comment """1 000-fold of the SI derived unit coulomb divided by the power of the SI base unit metre with the exponent 2

-- QUDT"""@en ;
    rdfs:subClassOf [ a owl:Restriction ;
            owl:onProperty ns1:hasUnitSymbol ;
            owl:someValuesFrom ns1:CoulombPerSquareMetre ],
        [ a owl:Restriction ;
            owl:hasValue 0e+00 ;
            owl:onProperty ns1:hasSIConversionOffset ],
        [ a owl:Restriction ;
            owl:hasValue 1e+03 ;
            owl:onProperty ns1:hasSIConversionMultiplier ],
        ns1:ElectricDisplacementFieldUnit,
        ns1:KiloPrefixedUnit,
        ns1:PrefixedUnit,
        ns1:SINonCoherentUnit ;
    skos:altLabel "Kilocoulomb Per Square Metre"@en ;
    skos:prefLabel "KiloCoulombPerSquareMetre"^^xsd:string ;
    ns1:elucidation """1 000-fold of the SI derived unit coulomb divided by the power of the SI base unit metre with the exponent 2

-- QUDT"""@en ;
    ns1:qudtReference "http://qudt.org/vocab/unit/KiloC-PER-M2"^^xsd:string ;
    ns1:ucumCode "kC.m-2"^^xsd:string ;
    ns1:unitSymbol "kC/m²"^^xsd:string .

ns1:KiloHertzMetre a owl:Class ;
    rdfs:label "KiloHertzMetre"^^xsd:string ;
    rdfs:comment """product of the 1 000-fold of the SI derived unit hertz and the SI base unit metre

-- QUDT"""@en ;
    rdfs:subClassOf [ a owl:Restriction ;
            owl:onProperty ns1:hasUnitSymbol ;
            owl:someValuesFrom ns1:HertzMetre ],
        [ a owl:Restriction ;
            owl:hasValue 1e+03 ;
            owl:onProperty ns1:hasSIConversionMultiplier ],
        [ a owl:Restriction ;
            owl:hasValue 0e+00 ;
            owl:onProperty ns1:hasSIConversionOffset ],
        ns1:KiloPrefixedUnit,
        ns1:PrefixedUnit,
        ns1:SINonCoherentUnit,
        ns1:SpeedUnit ;
    skos:altLabel "Kilohertz Metre"@en ;
    skos:prefLabel "KiloHertzMetre"^^xsd:string ;
    ns1:elucidation """product of the 1 000-fold of the SI derived unit hertz and the SI base unit metre

-- QUDT"""@en ;
    ns1:qudtReference "http://qudt.org/vocab/unit/KiloHZ-M"^^xsd:string ;
    ns1:ucumCode "kHz.m"^^xsd:string ;
    ns1:unitSymbol "kHz⋅m"^^xsd:string .

ns1:KiloJoulePerKelvin a owl:Class ;
    rdfs:label "KiloJoulePerKelvin"^^xsd:string ;
    rdfs:comment """1 000-fold of the SI derived unit joule divided by the SI base unit kelvin

-- QUDT"""@en ;
    rdfs:subClassOf [ a owl:Restriction ;
            owl:onProperty ns1:hasUnitSymbol ;
            owl:someValuesFrom ns1:JoulePerKelvin ],
        [ a owl:Restriction ;
            owl:hasValue 1e+03 ;
            owl:onProperty ns1:hasSIConversionMultiplier ],
        [ a owl:Restriction ;
            owl:hasValue 0e+00 ;
            owl:onProperty ns1:hasSIConversionOffset ],
        ns1:EntropyUnit,
        ns1:KiloPrefixedUnit,
        ns1:PrefixedUnit,
        ns1:SINonCoherentUnit ;
    skos:altLabel "Kilojoule Per Kelvin"@en ;
    skos:prefLabel "KiloJoulePerKelvin"^^xsd:string ;
    ns1:elucidation """1 000-fold of the SI derived unit joule divided by the SI base unit kelvin

-- QUDT"""@en ;
    ns1:qudtReference "http://qudt.org/vocab/unit/KiloJ-PER-K"^^xsd:string ;
    ns1:ucumCode "kJ.K-1"^^xsd:string,
        "kJ/K"^^xsd:string ;
    ns1:unitSymbol "kJ/K"^^xsd:string .

ns1:KiloJoulePerKilogram a owl:Class ;
    rdfs:label "KiloJoulePerKilogram"^^xsd:string ;
    rdfs:comment """1 000-fold of the SI derived unit joule divided by the SI base unit kilogram

-- QUDT"""@en ;
    rdfs:subClassOf [ a owl:Restriction ;
            owl:onProperty ns1:hasUnitSymbol ;
            owl:someValuesFrom ns1:JoulePerKilogram ],
        [ a owl:Restriction ;
            owl:hasValue 1e+03 ;
            owl:onProperty ns1:hasSIConversionMultiplier ],
        [ a owl:Restriction ;
            owl:hasValue 0e+00 ;
            owl:onProperty ns1:hasSIConversionOffset ],
        ns1:AbsorbedDoseUnit,
        ns1:KiloPrefixedUnit,
        ns1:PrefixedUnit,
        ns1:SINonCoherentUnit ;
    skos:altLabel "Kilojoule Per Kilogram"@en ;
    skos:prefLabel "KiloJoulePerKilogram"^^xsd:string ;
    ns1:elucidation """1 000-fold of the SI derived unit joule divided by the SI base unit kilogram

-- QUDT"""@en ;
    ns1:qudtReference "http://qudt.org/vocab/unit/KiloJ-PER-KiloGM"^^xsd:string ;
    ns1:ucumCode "kJ.kg-1"^^xsd:string,
        "kJ/kg"^^xsd:string ;
    ns1:unitSymbol "kJ/kg"^^xsd:string .

ns1:KiloJoulePerKilogramKelvin a owl:Class ;
    rdfs:label "KiloJoulePerKilogramKelvin"^^xsd:string ;
    rdfs:comment """1 000-fold of the SI derived unit joule divided by the product of the SI base unit kilogram and the SI base unit kelvin

-- QUDT"""@en ;
    rdfs:subClassOf [ a owl:Restriction ;
            owl:hasValue 0e+00 ;
            owl:onProperty ns1:hasSIConversionOffset ],
        [ a owl:Restriction ;
            owl:onProperty ns1:hasUnitSymbol ;
            owl:someValuesFrom ns1:JoulePerKilogramKelvin ],
        [ a owl:Restriction ;
            owl:hasValue 1e+03 ;
            owl:onProperty ns1:hasSIConversionMultiplier ],
        ns1:EntropyPerMassUnit,
        ns1:KiloPrefixedUnit,
        ns1:PrefixedUnit,
        ns1:SINonCoherentUnit ;
    skos:altLabel "Kilojoule Per Kilogram Kelvin"@en ;
    skos:prefLabel "KiloJoulePerKilogramKelvin"^^xsd:string ;
    ns1:elucidation """1 000-fold of the SI derived unit joule divided by the product of the SI base unit kilogram and the SI base unit kelvin

-- QUDT"""@en ;
    ns1:qudtReference "http://qudt.org/vocab/unit/KiloJ-PER-KiloGM-K"^^xsd:string ;
    ns1:ucumCode "kJ.(kg.K)-1"^^xsd:string,
        "kJ.kg-1.K-1"^^xsd:string,
        "kJ/(kg.K)"^^xsd:string ;
    ns1:unitSymbol "kJ/(kg⋅K)"^^xsd:string .

ns1:KiloJoulePerMole a owl:Class ;
    rdfs:label "KiloJoulePerMole"^^xsd:string ;
    rdfs:comment """1 000-fold of the SI derived unit joule divided by the SI base unit mol

-- QUDT"""@en ;
    rdfs:subClassOf [ a owl:Restriction ;
            owl:onProperty ns1:hasUnitSymbol ;
            owl:someValuesFrom ns1:JoulePerMole ],
        [ a owl:Restriction ;
            owl:hasValue 0e+00 ;
            owl:onProperty ns1:hasSIConversionOffset ],
        [ a owl:Restriction ;
            owl:hasValue 1e+03 ;
            owl:onProperty ns1:hasSIConversionMultiplier ],
        ns1:EnergyPerAmountUnit,
        ns1:KiloPrefixedUnit,
        ns1:PrefixedUnit,
        ns1:SINonCoherentUnit ;
    skos:altLabel "Kilojoule Per Mole"@en ;
    skos:prefLabel "KiloJoulePerMole"^^xsd:string ;
    ns1:elucidation """1 000-fold of the SI derived unit joule divided by the SI base unit mol

-- QUDT"""@en ;
    ns1:qudtReference "http://qudt.org/vocab/unit/KiloJ-PER-MOL"^^xsd:string ;
    ns1:ucumCode "kJ.mol-1"^^xsd:string ;
    ns1:unitSymbol "kJ/mol"^^xsd:string .

ns1:KiloMetrePerSecond a owl:Class ;
    rdfs:label "KiloMetrePerSecond"^^xsd:string ;
    rdfs:comment """"Kilometer per Second" is a C.G.S System unit for  'Linear Velocity' expressed as km/s.

-- QUDT"""@en ;
    rdfs:subClassOf [ a owl:Restriction ;
            owl:onProperty ns1:hasUnitNonPrefixPart ;
            owl:someValuesFrom ns1:MetrePerSecond ],
        [ a owl:Restriction ;
            owl:hasValue 0e+00 ;
            owl:onProperty ns1:hasSIConversionOffset ],
        [ a owl:Restriction ;
            owl:hasValue 1e+03 ;
            owl:onProperty ns1:hasSIConversionMultiplier ],
        ns1:KiloPrefixedUnit,
        ns1:PrefixedUnit,
        ns1:SINonCoherentUnit,
        ns1:SpeedUnit ;
    skos:altLabel "Kilometre per Second"@en ;
    skos:prefLabel "KiloMetrePerSecond"^^xsd:string ;
    ns1:elucidation """"Kilometer per Second" is a C.G.S System unit for  'Linear Velocity' expressed as km/s.

-- QUDT"""@en ;
    ns1:qudtReference "http://qudt.org/vocab/unit/KiloM-PER-SEC"^^xsd:string ;
    ns1:ucumCode "km.s-1"^^xsd:string,
        "km/s"^^xsd:string ;
    ns1:unitSymbol "km/s"^^xsd:string .

ns1:KiloMolePerCubicMetre a owl:Class ;
    rdfs:label "KiloMolePerCubicMetre"^^xsd:string ;
    rdfs:comment """1 000-fold of the SI base unit mol divided by the power of the SI base unit metre with the exponent 3

-- QUDT"""@en ;
    rdfs:subClassOf [ a owl:Restriction ;
            owl:onProperty ns1:hasUnitSymbol ;
            owl:someValuesFrom ns1:MolePerCubicMetre ],
        [ a owl:Restriction ;
            owl:hasValue 1e+03 ;
            owl:onProperty ns1:hasSIConversionMultiplier ],
        [ a owl:Restriction ;
            owl:hasValue 0e+00 ;
            owl:onProperty ns1:hasSIConversionOffset ],
        ns1:AmountConcentrationUnit,
        ns1:KiloPrefixedUnit,
        ns1:PrefixedUnit,
        ns1:SINonCoherentUnit ;
    skos:altLabel "Kilomole Per Cubic Metre"@en ;
    skos:prefLabel "KiloMolePerCubicMetre"^^xsd:string ;
    ns1:elucidation """1 000-fold of the SI base unit mol divided by the power of the SI base unit metre with the exponent 3

-- QUDT"""@en ;
    ns1:qudtReference "http://qudt.org/vocab/unit/KiloMOL-PER-M3"^^xsd:string ;
    ns1:ucumCode "kmol.m-3"^^xsd:string ;
    ns1:unitSymbol "kmol/m³"^^xsd:string .

ns1:KiloMolePerKilogram a owl:Class ;
    rdfs:label "KiloMolePerKilogram"@en ;
    rdfs:comment """Kilomole Per Kilogram (kmol/kg) is a unit of Molality

-- QUDT"""@en ;
    rdfs:subClassOf [ a owl:Restriction ;
            owl:hasValue 0e+00 ;
            owl:onProperty ns1:hasSIConversionOffset ],
        [ a owl:Restriction ;
            owl:onProperty ns1:hasUnitSymbol ;
            owl:someValuesFrom ns1:MolePerKilogram ],
        [ a owl:Restriction ;
            owl:hasValue 1e+03 ;
            owl:onProperty ns1:hasSIConversionMultiplier ],
        ns1:AmountPerMassUnit,
        ns1:KiloPrefixedUnit,
        ns1:PrefixedUnit,
        ns1:SINonCoherentUnit ;
    skos:altLabel "Kilomole per Kilogram"@en ;
    skos:prefLabel "KiloMolePerKilogram"@en ;
    ns1:elucidation """Kilomole Per Kilogram (kmol/kg) is a unit of Molality

-- QUDT"""@en ;
    ns1:qudtReference "http://qudt.org/vocab/unit/KiloMOL-PER-KiloGM"^^xsd:string ;
    ns1:ucumCode "kmol.kg-1"^^xsd:string,
        "kmol/kg"^^xsd:string ;
    ns1:unitSymbol "kmol/kg"^^xsd:string .

ns1:KiloMolePerSecond a owl:Class ;
    rdfs:label "KiloMolePerSecond"^^xsd:string ;
    rdfs:comment """1 000-fold of the SI base unit mol divided by the SI base unit second

-- QUDT"""@en ;
    rdfs:subClassOf [ a owl:Restriction ;
            owl:hasValue 0e+00 ;
            owl:onProperty ns1:hasSIConversionOffset ],
        [ a owl:Restriction ;
            owl:onProperty ns1:hasUnitSymbol ;
            owl:someValuesFrom ns1:MolePerSecond ],
        [ a owl:Restriction ;
            owl:hasValue 1e+03 ;
            owl:onProperty ns1:hasSIConversionMultiplier ],
        ns1:CatalyticActivityUnit,
        ns1:KiloPrefixedUnit,
        ns1:PrefixedUnit,
        ns1:SINonCoherentUnit ;
    skos:altLabel "Kilomole Per Second"@en ;
    skos:prefLabel "KiloMolePerSecond"^^xsd:string ;
    ns1:elucidation """1 000-fold of the SI base unit mol divided by the SI base unit second

-- QUDT"""@en ;
    ns1:qudtReference "http://qudt.org/vocab/unit/KiloMOL-PER-SEC"^^xsd:string ;
    ns1:ucumCode "kmol.s-1"^^xsd:string ;
    ns1:unitSymbol "kmol/s"^^xsd:string .

ns1:KiloNewtonMetre a owl:Class ;
    rdfs:label "KiloNewtonMetre"^^xsd:string ;
    rdfs:comment """1 000-fold of the product of the SI derived unit newton and the SI base unit metre

-- QUDT"""@en ;
    rdfs:subClassOf [ a owl:Restriction ;
            owl:hasValue 0e+00 ;
            owl:onProperty ns1:hasSIConversionOffset ],
        [ a owl:Restriction ;
            owl:hasValue 1e+03 ;
            owl:onProperty ns1:hasSIConversionMultiplier ],
        [ a owl:Restriction ;
            owl:onProperty ns1:hasUnitNonPrefixPart ;
            owl:someValuesFrom ns1:NewtonMetre ],
        ns1:EnergyUnit,
        ns1:KiloPrefixedUnit,
        ns1:PrefixedUnit,
        ns1:SINonCoherentUnit ;
    skos:altLabel "Kilonewton Metre"@en ;
    skos:prefLabel "KiloNewtonMetre"^^xsd:string ;
    ns1:elucidation """1 000-fold of the product of the SI derived unit newton and the SI base unit metre

-- QUDT"""@en ;
    ns1:qudtReference "http://qudt.org/vocab/unit/KiloN-M"^^xsd:string ;
    ns1:ucumCode "kN.m"^^xsd:string ;
    ns1:unitSymbol "kN⋅m"^^xsd:string .

ns1:KiloNewtonSquareMetre a owl:Class ;
    rdfs:label "KiloNewtonSquareMetre"@en ;
    rdfs:subClassOf [ a owl:Restriction ;
            owl:onProperty ns1:hasUnitSymbol ;
            owl:someValuesFrom ns1:NewtonSquareMetre ],
        [ a owl:Restriction ;
            owl:hasValue 1e+03 ;
            owl:onProperty ns1:hasSIConversionMultiplier ],
        [ a owl:Restriction ;
            owl:hasValue 0e+00 ;
            owl:onProperty ns1:hasSIConversionOffset ],
        ns1:ForceAreaUnit,
        ns1:KiloPrefixedUnit,
        ns1:PrefixedUnit,
        ns1:SINonCoherentUnit ;
    skos:altLabel "Kilo Newton Square Metre"@en ;
    skos:prefLabel "KiloNewtonSquareMetre"@en ;
    ns1:qudtReference "http://qudt.org/vocab/unit/KiloN-M2"^^xsd:string ;
    ns1:unitSymbol "kN⋅m²"^^xsd:string .

ns1:KiloPascalPerKelvin a owl:Class ;
    rdfs:label "KiloPascalPerKelvin"^^xsd:string ;
    rdfs:comment """1 000-fold of the SI derived unit pascal divided by the SI base unit kelvin

-- QUDT"""@en ;
    rdfs:subClassOf [ a owl:Restriction ;
            owl:hasValue 0e+00 ;
            owl:onProperty ns1:hasSIConversionOffset ],
        [ a owl:Restriction ;
            owl:onProperty ns1:hasUnitSymbol ;
            owl:someValuesFrom ns1:PascalPerKelvin ],
        [ a owl:Restriction ;
            owl:hasValue 1e+03 ;
            owl:onProperty ns1:hasSIConversionMultiplier ],
        ns1:KiloPrefixedUnit,
        ns1:PrefixedUnit,
        ns1:PressurePerTemperatureUnit,
        ns1:SINonCoherentUnit ;
    skos:altLabel "Kilopascal Per Kelvin"@en ;
    skos:prefLabel "KiloPascalPerKelvin"^^xsd:string ;
    ns1:elucidation """1 000-fold of the SI derived unit pascal divided by the SI base unit kelvin

-- QUDT"""@en ;
    ns1:qudtReference "http://qudt.org/vocab/unit/KiloPA-PER-K"^^xsd:string ;
    ns1:ucumCode "kPa.K-1"^^xsd:string ;
    ns1:unitSymbol "kPa/K"^^xsd:string .

ns1:KiloPascalPerMilliMetre a owl:Class ;
    rdfs:label "KiloPascalPerMilliMetre"^^xsd:string ;
    rdfs:comment """1 000-fold of the derived SI unit pascal divided by the 0.001-fold of the SI base unit metre

-- QUDT"""@en ;
    rdfs:subClassOf [ a owl:Restriction ;
            owl:hasValue 0e+00 ;
            owl:onProperty ns1:hasSIConversionOffset ],
        [ a owl:Restriction ;
            owl:hasValue 1e+05 ;
            owl:onProperty ns1:hasSIConversionMultiplier ],
        ns1:KiloPrefixedUnit,
        ns1:MassPerSquareLengthSquareTimeUnit,
        ns1:PrefixedUnit,
        ns1:SINonCoherentUnit ;
    skos:altLabel "Kilopascal Per Millimetre"@en ;
    skos:prefLabel "KiloPascalPerMilliMetre"^^xsd:string ;
    ns1:elucidation """1 000-fold of the derived SI unit pascal divided by the 0.001-fold of the SI base unit metre

-- QUDT"""@en ;
    ns1:qudtReference "http://qudt.org/vocab/unit/KiloPA-PER-MilliM"^^xsd:string ;
    ns1:ucumCode "kPa.mm-1"^^xsd:string ;
    ns1:unitSymbol "kPa/mm"^^xsd:string .

ns1:KiloPascalSquareMetrePerGram a owl:Class ;
    rdfs:label "KiloPascalSquareMetrePerGram"^^xsd:string ;
    rdfs:comment """sector-specific unit of the burst index as 1 000-fold of the derived unit for pressure pascal related to the substance, represented as a quotient from the 0.001-fold of the SI base unit kilogram divided by the power of the SI base unit metre by exponent 2

-- QUDT"""@en ;
    rdfs:subClassOf [ a owl:Restriction ;
            owl:hasValue 0e+00 ;
            owl:onProperty ns1:hasSIConversionOffset ],
        [ a owl:Restriction ;
            owl:hasValue 1e+06 ;
            owl:onProperty ns1:hasSIConversionMultiplier ],
        ns1:AccelerationUnit,
        ns1:KiloPrefixedUnit,
        ns1:PrefixedUnit,
        ns1:SINonCoherentUnit ;
    skos:altLabel "Kilopascal Square Metre per Gram"@en ;
    skos:prefLabel "KiloPascalSquareMetrePerGram"^^xsd:string ;
    ns1:elucidation """sector-specific unit of the burst index as 1 000-fold of the derived unit for pressure pascal related to the substance, represented as a quotient from the 0.001-fold of the SI base unit kilogram divided by the power of the SI base unit metre by exponent 2

-- QUDT"""@en ;
    ns1:qudtReference "http://qudt.org/vocab/unit/KiloPA-M2-PER-GM"^^xsd:string ;
    ns1:ucumCode "kPa.m2.g-1"^^xsd:string ;
    ns1:unitSymbol "kPa⋅m²/g"^^xsd:string .

ns1:KiloSiemensPerMetre a owl:Class ;
    rdfs:label "KiloSiemensPerMetre"^^xsd:string ;
    rdfs:comment """1 000-fold of the SI derived unit siemens divided by the SI base unit metre

-- QUDT"""@en ;
    rdfs:subClassOf [ a owl:Restriction ;
            owl:hasValue 0e+00 ;
            owl:onProperty ns1:hasSIConversionOffset ],
        [ a owl:Restriction ;
            owl:onProperty ns1:hasUnitSymbol ;
            owl:someValuesFrom ns1:SiemensPerMetre ],
        [ a owl:Restriction ;
            owl:hasValue 1e+03 ;
            owl:onProperty ns1:hasSIConversionMultiplier ],
        ns1:ElectricConductivityUnit,
        ns1:KiloPrefixedUnit,
        ns1:PrefixedUnit,
        ns1:SINonCoherentUnit ;
    skos:altLabel "Kilosiemens Per Metre"@en ;
    skos:prefLabel "KiloSiemensPerMetre"^^xsd:string ;
    ns1:elucidation """1 000-fold of the SI derived unit siemens divided by the SI base unit metre

-- QUDT"""@en ;
    ns1:qudtReference "http://qudt.org/vocab/unit/KiloS-PER-M"^^xsd:string ;
    ns1:ucumCode "kS.m-1"^^xsd:string ;
    ns1:unitSymbol "kS/m"^^xsd:string .

ns1:KiloVoltAmpere a owl:Class ;
    rdfs:label "KiloVoltAmpere"^^xsd:string ;
    rdfs:comment """1 000-fold of the product of the SI derived unit volt and the SI base unit ampere

-- QUDT"""@en ;
    rdfs:subClassOf [ a owl:Restriction ;
            owl:hasValue 1e+03 ;
            owl:onProperty ns1:hasSIConversionMultiplier ],
        [ a owl:Restriction ;
            owl:onProperty ns1:hasUnitSymbol ;
            owl:someValuesFrom ns1:VoltAmpere ],
        [ a owl:Restriction ;
            owl:hasValue 0e+00 ;
            owl:onProperty ns1:hasSIConversionOffset ],
        ns1:KiloPrefixedUnit,
        ns1:PowerUnit,
        ns1:PrefixedUnit,
        ns1:SINonCoherentUnit ;
    skos:altLabel "Kilovolt Ampere"@en ;
    skos:prefLabel "KiloVoltAmpere"^^xsd:string ;
    ns1:elucidation """1 000-fold of the product of the SI derived unit volt and the SI base unit ampere

-- QUDT"""@en ;
    ns1:qudtReference "http://qudt.org/vocab/unit/KiloV-A"^^xsd:string ;
    ns1:ucumCode "kV.A"^^xsd:string ;
    ns1:unitSymbol "kV⋅A"^^xsd:string .

ns1:KiloVoltPerMetre a owl:Class ;
    rdfs:label "KiloVoltPerMetre"^^xsd:string ;
    rdfs:comment """1 000-fold of the SI derived unit volt divided by the SI base unit metre

-- QUDT"""@en ;
    rdfs:subClassOf [ a owl:Restriction ;
            owl:hasValue 1e+03 ;
            owl:onProperty ns1:hasSIConversionMultiplier ],
        [ a owl:Restriction ;
            owl:hasValue 0e+00 ;
            owl:onProperty ns1:hasSIConversionOffset ],
        [ a owl:Restriction ;
            owl:onProperty ns1:hasUnitSymbol ;
            owl:someValuesFrom ns1:VoltPerMetre ],
        ns1:ElectricFieldStrengthUnit,
        ns1:KiloPrefixedUnit,
        ns1:PrefixedUnit,
        ns1:SINonCoherentUnit ;
    skos:altLabel "Kilovolt Per Metre"@en ;
    skos:prefLabel "KiloVoltPerMetre"^^xsd:string ;
    ns1:elucidation """1 000-fold of the SI derived unit volt divided by the SI base unit metre

-- QUDT"""@en ;
    ns1:qudtReference "http://qudt.org/vocab/unit/KiloV-PER-M"^^xsd:string ;
    ns1:ucumCode "kV.m-1"^^xsd:string ;
    ns1:unitSymbol "kV/m"^^xsd:string .

ns1:KiloWeberPerMetre a owl:Class ;
    rdfs:label "KiloWeberPerMetre"^^xsd:string ;
    rdfs:comment """1 000-fold of the SI derived unit weber divided by the SI base unit metre

-- QUDT"""@en ;
    rdfs:subClassOf [ a owl:Restriction ;
            owl:hasValue 1e+03 ;
            owl:onProperty ns1:hasSIConversionMultiplier ],
        [ a owl:Restriction ;
            owl:onProperty ns1:hasUnitSymbol ;
            owl:someValuesFrom ns1:WeberPerMetre ],
        [ a owl:Restriction ;
            owl:hasValue 0e+00 ;
            owl:onProperty ns1:hasSIConversionOffset ],
        ns1:KiloPrefixedUnit,
        ns1:MagneticPotentialUnit,
        ns1:PrefixedUnit,
        ns1:SINonCoherentUnit ;
    skos:altLabel "Kiloweber Per Metre"@en ;
    skos:prefLabel "KiloWeberPerMetre"^^xsd:string ;
    ns1:elucidation """1 000-fold of the SI derived unit weber divided by the SI base unit metre

-- QUDT"""@en ;
    ns1:qudtReference "http://qudt.org/vocab/unit/KiloWB-PER-M"^^xsd:string ;
    ns1:ucumCode "kWb.m-1"^^xsd:string ;
    ns1:unitSymbol "kWb/m"^^xsd:string .

ns1:KilogramPerCubicCentiMetre a owl:Class ;
    rdfs:label "KilogramPerCubicCentiMetre"^^xsd:string ;
    rdfs:comment """SI base unit kilogram divided by the 0.000 001-fold of the power of the SI base unit metre with the exponent 3

-- QUDT"""@en ;
    rdfs:subClassOf [ a owl:Restriction ;
            owl:hasValue 0e+00 ;
            owl:onProperty ns1:hasSIConversionOffset ],
        [ a owl:Restriction ;
            owl:hasValue 1e+06 ;
            owl:onProperty ns1:hasSIConversionMultiplier ],
        ns1:DensityUnit,
        ns1:PrefixedUnit,
        ns1:SINonCoherentUnit ;
    skos:altLabel "Kilogram Per Cubic Centimetre"@en ;
    skos:prefLabel "KilogramPerCubicCentiMetre"^^xsd:string ;
    ns1:elucidation """SI base unit kilogram divided by the 0.000 001-fold of the power of the SI base unit metre with the exponent 3

-- QUDT"""@en ;
    ns1:qudtReference "http://qudt.org/vocab/unit/KiloGM-PER-CentiM3"^^xsd:string ;
    ns1:ucumCode "kg.cm-3"^^xsd:string ;
    ns1:unitSymbol "kg/cm³"^^xsd:string .

ns1:KilogramPerCubicDeciMetre a owl:Class ;
    rdfs:label "KilogramPerCubicDeciMetre"^^xsd:string ;
    rdfs:comment """SI base unit kilogram divided by the 0.001-fold of the power of the SI base unit metre with the exponent 3

-- QUDT"""@en ;
    rdfs:subClassOf [ a owl:Restriction ;
            owl:hasValue 0e+00 ;
            owl:onProperty ns1:hasSIConversionOffset ],
        [ a owl:Restriction ;
            owl:hasValue 1e+03 ;
            owl:onProperty ns1:hasSIConversionMultiplier ],
        ns1:DensityUnit,
        ns1:PrefixedUnit,
        ns1:SINonCoherentUnit ;
    skos:altLabel "Kilogram Per Cubic Decimetre"@en ;
    skos:prefLabel "KilogramPerCubicDeciMetre"^^xsd:string ;
    ns1:elucidation """SI base unit kilogram divided by the 0.001-fold of the power of the SI base unit metre with the exponent 3

-- QUDT"""@en ;
    ns1:qudtReference "http://qudt.org/vocab/unit/KiloGM-PER-DeciM3"^^xsd:string ;
    ns1:ucumCode "kg.dm-3"^^xsd:string ;
    ns1:unitSymbol "kg/dm³"^^xsd:string .

ns1:KilogramPerKiloMole a owl:Class ;
    rdfs:label "KilogramPerKiloMole"@en ;
    rdfs:comment """SI base unit kilogram divided by the 1 000-fold of the SI base unit mol

-- QUDT"""@en ;
    rdfs:subClassOf [ a owl:Restriction ;
            owl:hasValue 1e-03 ;
            owl:onProperty ns1:hasSIConversionMultiplier ],
        [ a owl:Restriction ;
            owl:hasValue 0e+00 ;
            owl:onProperty ns1:hasSIConversionOffset ],
        ns1:KiloPrefixedUnit,
        ns1:MassPerAmountUnit,
        ns1:PrefixedUnit,
        ns1:SINonCoherentUnit ;
    skos:altLabel "Kilogram Per Kilomole"@en ;
    skos:prefLabel "KilogramPerKiloMole"@en ;
    ns1:elucidation """SI base unit kilogram divided by the 1 000-fold of the SI base unit mol

-- QUDT"""@en ;
    ns1:qudtReference "http://qudt.org/vocab/unit/KiloGM-PER-KiloMOL"^^xsd:string ;
    ns1:ucumCode "kg.kmol-1"^^xsd:string ;
    ns1:unitSymbol "kg/kmol"^^xsd:string .

ns1:KilogramPerMilliMetre a owl:Class ;
    rdfs:label "KilogramPerMilliMetre"^^xsd:string ;
    rdfs:comment """SI base unit kilogram divided by the 0.001-fold of the SI base unit metre

-- QUDT"""@en ;
    rdfs:subClassOf [ a owl:Restriction ;
            owl:hasValue 0e+00 ;
            owl:onProperty ns1:hasSIConversionOffset ],
        [ a owl:Restriction ;
            owl:hasValue 1e+03 ;
            owl:onProperty ns1:hasSIConversionMultiplier ],
        ns1:MassPerLengthUnit,
        ns1:PrefixedUnit,
        ns1:SINonCoherentUnit ;
    skos:altLabel "Kilogram Per Millimetre"@en ;
    skos:prefLabel "KilogramPerMilliMetre"^^xsd:string ;
    ns1:elucidation """SI base unit kilogram divided by the 0.001-fold of the SI base unit metre

-- QUDT"""@en ;
    ns1:qudtReference "http://qudt.org/vocab/unit/KiloGM-PER-MilliM"^^xsd:string ;
    ns1:ucumCode "kg.mm-1"^^xsd:string ;
    ns1:unitSymbol "kg/mm"^^xsd:string .

ns1:KilogramPerSquareCentiMetre a owl:Class ;
    rdfs:label "KilogramPerSquareCentiMetre"^^xsd:string ;
    rdfs:comment """SI base unit kilogram divided by the 0.0001-fold of the power of the SI base unit metre by exponent 2

-- QUDT"""@en ;
    rdfs:subClassOf [ a owl:Restriction ;
            owl:hasValue 1e+04 ;
            owl:onProperty ns1:hasSIConversionMultiplier ],
        [ a owl:Restriction ;
            owl:hasValue 0e+00 ;
            owl:onProperty ns1:hasSIConversionOffset ],
        ns1:AreaDensityUnit,
        ns1:PrefixedUnit,
        ns1:SINonCoherentUnit ;
    skos:altLabel "Kilogram Per Square Centimetre"@en ;
    skos:prefLabel "KilogramPerSquareCentiMetre"^^xsd:string ;
    ns1:elucidation """SI base unit kilogram divided by the 0.0001-fold of the power of the SI base unit metre by exponent 2

-- QUDT"""@en ;
    ns1:qudtReference "http://qudt.org/vocab/unit/KiloGM-PER-CentiM2"^^xsd:string ;
    ns1:ucumCode "kg.cm-2"^^xsd:string ;
    ns1:unitSymbol "kg/cm²"^^xsd:string .

ns1:KilogramPerSquareKiloMetre a owl:Class ;
    rdfs:label "KilogramPerSquareKiloMetre"^^xsd:string ;
    rdfs:comment """One SI standard unit of mass over the square of one thousand standard unit of length.

-- QUDT"""@en ;
    rdfs:subClassOf [ a owl:Restriction ;
            owl:hasValue 0e+00 ;
            owl:onProperty ns1:hasSIConversionOffset ],
        [ a owl:Restriction ;
            owl:hasValue 1e-06 ;
            owl:onProperty ns1:hasSIConversionMultiplier ],
        ns1:AreaDensityUnit,
        ns1:KiloPrefixedUnit,
        ns1:PrefixedUnit,
        ns1:SINonCoherentUnit ;
    skos:altLabel "Kilograms per square kilometre"@en ;
    skos:prefLabel "KilogramPerSquareKiloMetre"^^xsd:string ;
    ns1:elucidation """One SI standard unit of mass over the square of one thousand standard unit of length.

-- QUDT"""@en ;
    ns1:qudtReference "http://qudt.org/vocab/unit/KiloGM-PER-KiloM2"^^xsd:string ;
    ns1:ucumCode "kg.km-2"^^xsd:string ;
    ns1:unitSymbol "kg/km²"^^xsd:string .

ns1:KilogramSquareCentiMetre a owl:Class ;
    rdfs:label "KilogramSquareCentiMetre"^^xsd:string ;
    rdfs:comment """product of the SI base unit kilogram and the 0 0001fold of the power of the SI base unit metre with the exponent 2

-- QUDT"""@en ;
    rdfs:subClassOf [ a owl:Restriction ;
            owl:hasValue 0e+00 ;
            owl:onProperty ns1:hasSIConversionOffset ],
        [ a owl:Restriction ;
            owl:hasValue 1e-04 ;
            owl:onProperty ns1:hasSIConversionMultiplier ],
        ns1:KiloPrefixedUnit,
        ns1:MassAreaUnit,
        ns1:PrefixedUnit,
        ns1:SINonCoherentUnit ;
    skos:altLabel "Kilogram Square Centimetre"@en ;
    skos:prefLabel "KilogramSquareCentiMetre"^^xsd:string ;
    ns1:elucidation """product of the SI base unit kilogram and the 0 0001fold of the power of the SI base unit metre with the exponent 2

-- QUDT"""@en ;
    ns1:qudtReference "http://qudt.org/vocab/unit/KiloGM-CentiM2"^^xsd:string ;
    ns1:ucumCode "kg.cm2"^^xsd:string ;
    ns1:unitSymbol "kg⋅cm²"^^xsd:string .

ns1:KilogramSquareMilliMetre a owl:Class ;
    rdfs:label "KilogramSquareMilliMetre"^^xsd:string ;
    rdfs:comment """product of the SI base kilogram and the  0.001-fold of the power of the SI base metre with the exponent 2

-- QUDT"""@en ;
    rdfs:subClassOf [ a owl:Restriction ;
            owl:hasValue 1e-06 ;
            owl:onProperty ns1:hasSIConversionMultiplier ],
        [ a owl:Restriction ;
            owl:hasValue 0e+00 ;
            owl:onProperty ns1:hasSIConversionOffset ],
        ns1:KiloPrefixedUnit,
        ns1:MassAreaUnit,
        ns1:PrefixedUnit,
        ns1:SINonCoherentUnit ;
    skos:altLabel "Kilogram Square Millimetre"@en ;
    skos:prefLabel "KilogramSquareMilliMetre"^^xsd:string ;
    ns1:elucidation """product of the SI base kilogram and the  0.001-fold of the power of the SI base metre with the exponent 2

-- QUDT"""@en ;
    ns1:qudtReference "http://qudt.org/vocab/unit/KiloGM-MilliM2"^^xsd:string ;
    ns1:ucumCode "kg.mm2"^^xsd:string ;
    ns1:unitSymbol "kg⋅mm²"^^xsd:string .

ns1:MegaAmperePerSquareMetre a owl:Class ;
    rdfs:label "MegaAmperePerSquareMetre"@en ;
    rdfs:comment """1 000 000-fold of the SI base unit ampere divided by the power of the SI base unit metre with the exponent 2

-- QUDT"""@en ;
    rdfs:isDefinedBy "http://qudt.org/2.1/vocab/unit"^^xsd:string ;
    rdfs:subClassOf [ a owl:Restriction ;
            owl:hasValue 0e+00 ;
            owl:onProperty ns1:hasSIConversionOffset ],
        [ a owl:Restriction ;
            owl:hasValue 1e+06 ;
            owl:onProperty ns1:hasSIConversionMultiplier ],
        ns1:ElectricCurrentDensityUnit,
        ns1:SINonCoherentDerivedUnit ;
    skos:altLabel "Megaampere Per Square Metre"@en ;
    skos:prefLabel "MegaAmperePerSquareMetre"@en ;
    ns1:elucidation """1 000 000-fold of the SI base unit ampere divided by the power of the SI base unit metre with the exponent 2

-- QUDT"""@en ;
    ns1:qudtReference "http://qudt.org/vocab/unit/MegaA-PER-M2"^^xsd:string ;
    ns1:ucumCode "MA.m-2"^^xsd:string ;
    ns1:unitSymbol "MA/m²"^^xsd:string .

ns1:MegaCoulombPerCubicMetre a owl:Class ;
    rdfs:label "MegaCoulombPerCubicMetre"^^xsd:string ;
    rdfs:comment """1 000 000-fold of the SI derived unit coulomb divided by the power of the SI base unit metre with the exponent 3

-- QUDT"""@en ;
    rdfs:subClassOf [ a owl:Restriction ;
            owl:onProperty ns1:hasUnitSymbol ;
            owl:someValuesFrom ns1:CoulombPerCubicMetre ],
        [ a owl:Restriction ;
            owl:hasValue 0e+00 ;
            owl:onProperty ns1:hasSIConversionOffset ],
        [ a owl:Restriction ;
            owl:hasValue 1e+06 ;
            owl:onProperty ns1:hasSIConversionMultiplier ],
        ns1:ElectricChargeDensityUnit,
        ns1:MegaPrefixedUnit,
        ns1:PrefixedUnit,
        ns1:SINonCoherentUnit ;
    skos:altLabel "Megacoulomb Per Cubic Metre"@en ;
    skos:prefLabel "MegaCoulombPerCubicMetre"^^xsd:string ;
    ns1:elucidation """1 000 000-fold of the SI derived unit coulomb divided by the power of the SI base unit metre with the exponent 3

-- QUDT"""@en ;
    ns1:qudtReference "http://qudt.org/vocab/unit/MegaC-PER-M3"^^xsd:string ;
    ns1:ucumCode "MC.m-3"^^xsd:string ;
    ns1:unitSymbol "MC/m³"^^xsd:string .

ns1:MegaCoulombPerSquareMetre a owl:Class ;
    rdfs:label "MegaCoulombPerSquareMetre"^^xsd:string ;
    rdfs:comment """1 000 000-fold of the SI derived unit coulomb divided by the power of the SI base unit metre with the exponent 2

-- QUDT"""@en ;
    rdfs:subClassOf [ a owl:Restriction ;
            owl:hasValue 1e+06 ;
            owl:onProperty ns1:hasSIConversionMultiplier ],
        [ a owl:Restriction ;
            owl:onProperty ns1:hasUnitSymbol ;
            owl:someValuesFrom ns1:CoulombPerSquareMetre ],
        [ a owl:Restriction ;
            owl:hasValue 0e+00 ;
            owl:onProperty ns1:hasSIConversionOffset ],
        ns1:ElectricDisplacementFieldUnit,
        ns1:MegaPrefixedUnit,
        ns1:PrefixedUnit,
        ns1:SINonCoherentUnit ;
    skos:altLabel "Megacoulomb Per Square Metre"@en ;
    skos:prefLabel "MegaCoulombPerSquareMetre"^^xsd:string ;
    ns1:elucidation """1 000 000-fold of the SI derived unit coulomb divided by the power of the SI base unit metre with the exponent 2

-- QUDT"""@en ;
    ns1:qudtReference "http://qudt.org/vocab/unit/MegaC-PER-M2"^^xsd:string ;
    ns1:ucumCode "MC.m-2"^^xsd:string ;
    ns1:unitSymbol "MC/m²"^^xsd:string .

ns1:MegaGramPerCubicMetre a owl:Class ;
    rdfs:label "MegaGramPerCubicMetre"^^xsd:string ;
    rdfs:comment """1 000-fold of the SI base unit kilogram divided by the power of the SI base unit metre with the exponent 3

-- QUDT"""@en ;
    rdfs:subClassOf [ a owl:Restriction ;
            owl:hasValue 0e+00 ;
            owl:onProperty ns1:hasSIConversionOffset ],
        [ a owl:Restriction ;
            owl:hasValue 1e+03 ;
            owl:onProperty ns1:hasSIConversionMultiplier ],
        [ a owl:Restriction ;
            owl:onProperty ns1:hasUnitSymbol ;
            owl:someValuesFrom ns1:GramPerCubicMetre ],
        ns1:DensityUnit,
        ns1:MegaPrefixedUnit,
        ns1:PrefixedUnit,
        ns1:SINonCoherentUnit ;
    skos:altLabel "Megagram Per Cubic Metre"@en ;
    skos:prefLabel "MegaGramPerCubicMetre"^^xsd:string ;
    ns1:elucidation """1 000-fold of the SI base unit kilogram divided by the power of the SI base unit metre with the exponent 3

-- QUDT"""@en ;
    ns1:qudtReference "http://qudt.org/vocab/unit/MegaGM-PER-M3"^^xsd:string ;
    ns1:ucumCode "Mg.m-3"^^xsd:string ;
    ns1:unitSymbol "Mg/m³"^^xsd:string .

ns1:MegaHertzMetre a owl:Class ;
    rdfs:label "MegaHertzMetre"^^xsd:string ;
    rdfs:comment """product of the 1 000 000-fold of the SI derived unit hertz and the 1 000-fold of the SI base unit metre

-- QUDT"""@en ;
    rdfs:subClassOf [ a owl:Restriction ;
            owl:hasValue 1e+06 ;
            owl:onProperty ns1:hasSIConversionMultiplier ],
        [ a owl:Restriction ;
            owl:hasValue 0e+00 ;
            owl:onProperty ns1:hasSIConversionOffset ],
        [ a owl:Restriction ;
            owl:onProperty ns1:hasUnitSymbol ;
            owl:someValuesFrom ns1:HertzMetre ],
        ns1:MegaPrefixedUnit,
        ns1:PrefixedUnit,
        ns1:SINonCoherentUnit,
        ns1:SpeedUnit ;
    skos:altLabel "Megahertz Metre"@en ;
    skos:prefLabel "MegaHertzMetre"^^xsd:string ;
    ns1:elucidation """product of the 1 000 000-fold of the SI derived unit hertz and the 1 000-fold of the SI base unit metre

-- QUDT"""@en ;
    ns1:qudtReference "http://qudt.org/vocab/unit/MegaHZ-M"^^xsd:string ;
    ns1:ucumCode "MHz.m"^^xsd:string ;
    ns1:unitSymbol "MHz⋅m"^^xsd:string .

ns1:MegaHertzPerKelvin a owl:Class ;
    rdfs:label "MegaHertzPerKelvin"@en ;
    rdfs:comment """`Mega Hertz per Kelvin` is a unit for 'Inverse Time Temperature' expressed as MHz K⁻¹.

-- QUDT"""@en ;
    rdfs:subClassOf [ a owl:Restriction ;
            owl:hasValue 0e+00 ;
            owl:onProperty ns1:hasSIConversionOffset ],
        [ a owl:Restriction ;
            owl:hasValue 1e+06 ;
            owl:onProperty ns1:hasSIConversionMultiplier ],
        [ a owl:Restriction ;
            owl:onProperty ns1:hasUnitSymbol ;
            owl:someValuesFrom ns1:HertzPerKelvin ],
        ns1:MegaPrefixedUnit,
        ns1:PerTemperatureTimeUnit,
        ns1:PrefixedUnit,
        ns1:SINonCoherentUnit ;
    skos:altLabel "Mega Hertz per Kelvin"@en ;
    skos:prefLabel "MegaHertzPerKelvin"@en ;
    ns1:elucidation """`Mega Hertz per Kelvin` is a unit for 'Inverse Time Temperature' expressed as MHz K⁻¹.

-- QUDT"""@en ;
    ns1:qudtReference "http://qudt.org/vocab/unit/MegaHZ-PER-K"^^xsd:string ;
    ns1:ucumCode "MHz.K-1"^^xsd:string ;
    ns1:unitSymbol "MHz/K"^^xsd:string .

ns1:MegaHertzPerTesla a owl:Class ;
    rdfs:label "MegaHertzPerTesla"@en ;
    rdfs:comment """"Mega Hertz per Tesla" is a unit for  'Electric Charge Per Mass' expressed as MHz T⁻¹.

-- QUDT"""@en ;
    rdfs:subClassOf [ a owl:Restriction ;
            owl:onProperty ns1:hasUnitSymbol ;
            owl:someValuesFrom ns1:HertzPerTesla ],
        [ a owl:Restriction ;
            owl:hasValue 1e+06 ;
            owl:onProperty ns1:hasSIConversionMultiplier ],
        [ a owl:Restriction ;
            owl:hasValue 0e+00 ;
            owl:onProperty ns1:hasSIConversionOffset ],
        ns1:ElectricChargePerMassUnit,
        ns1:MegaPrefixedUnit,
        ns1:PrefixedUnit,
        ns1:SINonCoherentUnit ;
    skos:altLabel "Mega Hertz per Tesla"@en ;
    skos:prefLabel "MegaHertzPerTesla"@en ;
    ns1:elucidation """"Mega Hertz per Tesla" is a unit for  'Electric Charge Per Mass' expressed as MHz T⁻¹.

-- QUDT"""@en ;
    ns1:qudtReference "http://qudt.org/vocab/unit/MegaHZ-PER-T"^^xsd:string ;
    ns1:ucumCode "MHz.T-1"^^xsd:string ;
    ns1:unitSymbol "MHz/T"^^xsd:string .

ns1:MegaJoulePerCubicMetre a owl:Class ;
    rdfs:label "MegaJoulePerCubicMetre"^^xsd:string ;
    rdfs:comment """1,000,000-fold of the SI derived unit joule divided by the power of the SI base unit metre with the exponent 3

-- QUDT"""@en ;
    rdfs:subClassOf [ a owl:Restriction ;
            owl:hasValue 0e+00 ;
            owl:onProperty ns1:hasSIConversionOffset ],
        [ a owl:Restriction ;
            owl:hasValue 1e+06 ;
            owl:onProperty ns1:hasSIConversionMultiplier ],
        [ a owl:Restriction ;
            owl:onProperty ns1:hasUnitSymbol ;
            owl:someValuesFrom ns1:JoulePerCubicMetre ],
        ns1:MegaPrefixedUnit,
        ns1:PrefixedUnit,
        ns1:PressureUnit,
        ns1:SINonCoherentUnit ;
    skos:altLabel "Megajoule Per Cubic Metre"@en ;
    skos:prefLabel "MegaJoulePerCubicMetre"^^xsd:string ;
    ns1:elucidation """1,000,000-fold of the SI derived unit joule divided by the power of the SI base unit metre with the exponent 3

-- QUDT"""@en ;
    ns1:qudtReference "http://qudt.org/vocab/unit/MegaJ-PER-M3"^^xsd:string ;
    ns1:ucumCode "MJ.m-3"^^xsd:string ;
    ns1:unitSymbol "MJ/m³"^^xsd:string .

ns1:MegaJoulePerKelvin a owl:Class ;
    rdfs:label "MegaJoulePerKelvin"^^xsd:string ;
    rdfs:comment """MegaJoule Per Kelvin (MegaJ/K) is a unit in the category of Entropy.

-- QUDT"""@en ;
    rdfs:subClassOf [ a owl:Restriction ;
            owl:onProperty ns1:hasUnitSymbol ;
            owl:someValuesFrom ns1:JoulePerKelvin ],
        [ a owl:Restriction ;
            owl:hasValue 0e+00 ;
            owl:onProperty ns1:hasSIConversionOffset ],
        [ a owl:Restriction ;
            owl:hasValue 1e+06 ;
            owl:onProperty ns1:hasSIConversionMultiplier ],
        ns1:EntropyUnit,
        ns1:MegaPrefixedUnit,
        ns1:PrefixedUnit,
        ns1:SINonCoherentUnit ;
    skos:altLabel "MegaJoule per Kelvin"@en ;
    skos:prefLabel "MegaJoulePerKelvin"^^xsd:string ;
    ns1:elucidation """MegaJoule Per Kelvin (MegaJ/K) is a unit in the category of Entropy.

-- QUDT"""@en ;
    ns1:qudtReference "http://qudt.org/vocab/unit/MegaJ-PER-K"^^xsd:string ;
    ns1:ucumCode "MJ.K-1"^^xsd:string ;
    ns1:unitSymbol "MJ/K"^^xsd:string .

ns1:MegaJoulePerKilogram a owl:Class ;
    rdfs:label "MegaJoulePerKilogram"^^xsd:string ;
    rdfs:comment """1,000,000-fold of the derived SI unit joule divided by the SI base unit kilogram

-- QUDT"""@en ;
    rdfs:subClassOf [ a owl:Restriction ;
            owl:onProperty ns1:hasUnitSymbol ;
            owl:someValuesFrom ns1:JoulePerKilogram ],
        [ a owl:Restriction ;
            owl:hasValue 1e+06 ;
            owl:onProperty ns1:hasSIConversionMultiplier ],
        [ a owl:Restriction ;
            owl:hasValue 0e+00 ;
            owl:onProperty ns1:hasSIConversionOffset ],
        ns1:AbsorbedDoseUnit,
        ns1:MegaPrefixedUnit,
        ns1:PrefixedUnit,
        ns1:SINonCoherentUnit ;
    skos:altLabel "Megajoule Per Kilogram"@en ;
    skos:prefLabel "MegaJoulePerKilogram"^^xsd:string ;
    ns1:elucidation """1,000,000-fold of the derived SI unit joule divided by the SI base unit kilogram

-- QUDT"""@en ;
    ns1:qudtReference "http://qudt.org/vocab/unit/MegaJ-PER-KiloGM"^^xsd:string ;
    ns1:ucumCode "MJ.kg-1"^^xsd:string ;
    ns1:unitSymbol "MJ/kg"^^xsd:string .

ns1:MegaJoulePerSecond a owl:Class ;
    rdfs:label "MegaJoulePerSecond"^^xsd:string ;
    rdfs:comment """quotient of the 1,000,000-fold of the derived SI unit joule divided by the SI base unit second

-- QUDT"""@en ;
    rdfs:subClassOf [ a owl:Restriction ;
            owl:hasValue 1e+06 ;
            owl:onProperty ns1:hasSIConversionMultiplier ],
        [ a owl:Restriction ;
            owl:onProperty ns1:hasUnitSymbol ;
            owl:someValuesFrom ns1:JoulePerSecond ],
        [ a owl:Restriction ;
            owl:hasValue 0e+00 ;
            owl:onProperty ns1:hasSIConversionOffset ],
        ns1:MegaPrefixedUnit,
        ns1:PowerUnit,
        ns1:PrefixedUnit,
        ns1:SINonCoherentUnit ;
    skos:altLabel "Megajoule Per Second"@en ;
    skos:prefLabel "MegaJoulePerSecond"^^xsd:string ;
    ns1:elucidation """quotient of the 1,000,000-fold of the derived SI unit joule divided by the SI base unit second

-- QUDT"""@en ;
    ns1:qudtReference "http://qudt.org/vocab/unit/MegaJ-PER-SEC"^^xsd:string ;
    ns1:ucumCode "MJ.s-1"^^xsd:string ;
    ns1:unitSymbol "MJ/s"^^xsd:string .

ns1:MegaJoulePerSquareMetre a owl:Class ;
    rdfs:label "MegaJoulePerSquareMetre"^^xsd:string ;
    rdfs:comment """1,000,000-fold of the SI derived unit joule divided by the power of the SI base unit metre with the exponent 2

-- QUDT"""@en ;
    rdfs:subClassOf [ a owl:Restriction ;
            owl:hasValue 1e+06 ;
            owl:onProperty ns1:hasSIConversionMultiplier ],
        [ a owl:Restriction ;
            owl:onProperty ns1:hasUnitSymbol ;
            owl:someValuesFrom ns1:JoulePerSquareMetre ],
        [ a owl:Restriction ;
            owl:hasValue 0e+00 ;
            owl:onProperty ns1:hasSIConversionOffset ],
        ns1:ForcePerLengthUnit,
        ns1:MegaPrefixedUnit,
        ns1:PrefixedUnit,
        ns1:SINonCoherentUnit ;
    skos:altLabel "Megajoule Per Square Metre"@en ;
    skos:prefLabel "MegaJoulePerSquareMetre"^^xsd:string ;
    ns1:elucidation """1,000,000-fold of the SI derived unit joule divided by the power of the SI base unit metre with the exponent 2

-- QUDT"""@en ;
    ns1:qudtReference "http://qudt.org/vocab/unit/MegaJ-PER-M2"^^xsd:string ;
    ns1:ucumCode "MJ.m-2"^^xsd:string ;
    ns1:unitSymbol "MJ/m²"^^xsd:string .

ns1:MegaNewtonMetre a owl:Class ;
    rdfs:label "MegaNewtonMetre"^^xsd:string ;
    rdfs:comment """1,000,000-fold of the product of the SI derived unit newton and the SI base unit metre

-- QUDT"""@en ;
    rdfs:subClassOf [ a owl:Restriction ;
            owl:onProperty ns1:hasUnitNonPrefixPart ;
            owl:someValuesFrom ns1:NewtonMetre ],
        [ a owl:Restriction ;
            owl:hasValue 0e+00 ;
            owl:onProperty ns1:hasSIConversionOffset ],
        [ a owl:Restriction ;
            owl:hasValue 1e+06 ;
            owl:onProperty ns1:hasSIConversionMultiplier ],
        ns1:EnergyUnit,
        ns1:MegaPrefixedUnit,
        ns1:PrefixedUnit,
        ns1:SINonCoherentUnit ;
    skos:altLabel "Meganewton Metre"@en ;
    skos:prefLabel "MegaNewtonMetre"^^xsd:string ;
    ns1:elucidation """1,000,000-fold of the product of the SI derived unit newton and the SI base unit metre

-- QUDT"""@en ;
    ns1:qudtReference "http://qudt.org/vocab/unit/MegaN-M"^^xsd:string ;
    ns1:ucumCode "MN.m"^^xsd:string ;
    ns1:unitSymbol "MN⋅m"^^xsd:string .

ns1:MegaPascalCubicMetrePerSecond a owl:Class ;
    rdfs:label "MegaPascalCubicMetrePerSecond"^^xsd:string ;
    rdfs:comment """product out of the 1,000,000-fold of the SI derived unit pascal and the power of the SI base unit metre with the exponent 3 divided by the SI base unit second

-- QUDT"""@en ;
    rdfs:subClassOf [ a owl:Restriction ;
            owl:hasValue 1e+06 ;
            owl:onProperty ns1:hasSIConversionMultiplier ],
        [ a owl:Restriction ;
            owl:hasValue 0e+00 ;
            owl:onProperty ns1:hasSIConversionOffset ],
        [ a owl:Restriction ;
            owl:onProperty ns1:hasUnitSymbol ;
            owl:someValuesFrom ns1:PascalCubicMetrePerSecond ],
        ns1:MegaPrefixedUnit,
        ns1:PowerUnit,
        ns1:PrefixedUnit,
        ns1:SINonCoherentUnit ;
    skos:altLabel "Megapascal Cubic Metre Per Second"@en ;
    skos:prefLabel "MegaPascalCubicMetrePerSecond"^^xsd:string ;
    ns1:elucidation """product out of the 1,000,000-fold of the SI derived unit pascal and the power of the SI base unit metre with the exponent 3 divided by the SI base unit second

-- QUDT"""@en ;
    ns1:qudtReference "http://qudt.org/vocab/unit/MegaPA-M3-PER-SEC"^^xsd:string ;
    ns1:ucumCode "MPa.m3.s-1"^^xsd:string ;
    ns1:unitSymbol "MPa⋅m³/s"^^xsd:string .

ns1:MegaPascalPerKelvin a owl:Class ;
    rdfs:label "MegaPascalPerKelvin"^^xsd:string ;
    rdfs:comment """1,000,000-fold of the SI derived unit pascal divided by the SI base unit kelvin

-- QUDT"""@en ;
    rdfs:subClassOf [ a owl:Restriction ;
            owl:onProperty ns1:hasUnitSymbol ;
            owl:someValuesFrom ns1:PascalPerKelvin ],
        [ a owl:Restriction ;
            owl:hasValue 0e+00 ;
            owl:onProperty ns1:hasSIConversionOffset ],
        [ a owl:Restriction ;
            owl:hasValue 1e+06 ;
            owl:onProperty ns1:hasSIConversionMultiplier ],
        ns1:MegaPrefixedUnit,
        ns1:PrefixedUnit,
        ns1:PressurePerTemperatureUnit,
        ns1:SINonCoherentUnit ;
    skos:altLabel "Megapascal Per Kelvin"@en ;
    skos:prefLabel "MegaPascalPerKelvin"^^xsd:string ;
    ns1:elucidation """1,000,000-fold of the SI derived unit pascal divided by the SI base unit kelvin

-- QUDT"""@en ;
    ns1:qudtReference "http://qudt.org/vocab/unit/MegaPA-PER-K"^^xsd:string ;
    ns1:ucumCode "MPa.K-1"^^xsd:string ;
    ns1:unitSymbol "MPa/K"^^xsd:string .

ns1:MegaSiemensPerMetre a owl:Class ;
    rdfs:label "MegaSiemensPerMetre"^^xsd:string ;
    rdfs:comment """1,000,000-fold of the SI derived unit siemens divided by the SI base unit metre

-- QUDT"""@en ;
    rdfs:subClassOf [ a owl:Restriction ;
            owl:hasValue 1e+06 ;
            owl:onProperty ns1:hasSIConversionMultiplier ],
        [ a owl:Restriction ;
            owl:hasValue 0e+00 ;
            owl:onProperty ns1:hasSIConversionOffset ],
        [ a owl:Restriction ;
            owl:onProperty ns1:hasUnitSymbol ;
            owl:someValuesFrom ns1:SiemensPerMetre ],
        ns1:ElectricConductivityUnit,
        ns1:MegaPrefixedUnit,
        ns1:PrefixedUnit,
        ns1:SINonCoherentUnit ;
    skos:altLabel "Megasiemens Per Metre"@en ;
    skos:prefLabel "MegaSiemensPerMetre"^^xsd:string ;
    ns1:elucidation """1,000,000-fold of the SI derived unit siemens divided by the SI base unit metre

-- QUDT"""@en ;
    ns1:qudtReference "http://qudt.org/vocab/unit/MegaS-PER-M"^^xsd:string ;
    ns1:ucumCode "MS.m-1"^^xsd:string ;
    ns1:unitSymbol "MS/m"^^xsd:string .

ns1:MegaVoltAmpere a owl:Class ;
    rdfs:label "MegaVoltAmpere"^^xsd:string ;
    rdfs:comment """1,000,000-fold of the product of the SI derived unit volt and the SI base unit ampere

-- QUDT"""@en ;
    rdfs:subClassOf [ a owl:Restriction ;
            owl:hasValue 0e+00 ;
            owl:onProperty ns1:hasSIConversionOffset ],
        [ a owl:Restriction ;
            owl:hasValue 1e+06 ;
            owl:onProperty ns1:hasSIConversionMultiplier ],
        [ a owl:Restriction ;
            owl:onProperty ns1:hasUnitSymbol ;
            owl:someValuesFrom ns1:VoltAmpere ],
        ns1:MegaPrefixedUnit,
        ns1:PowerUnit,
        ns1:PrefixedUnit,
        ns1:SINonCoherentUnit ;
    skos:altLabel "Megavolt Ampere"@en ;
    skos:prefLabel "MegaVoltAmpere"^^xsd:string ;
    ns1:elucidation """1,000,000-fold of the product of the SI derived unit volt and the SI base unit ampere

-- QUDT"""@en ;
    ns1:qudtReference "http://qudt.org/vocab/unit/MegaV-A"^^xsd:string ;
    ns1:ucumCode "MV.A"^^xsd:string ;
    ns1:unitSymbol "MV⋅A"^^xsd:string .

ns1:MegaVoltPerMetre a owl:Class ;
    rdfs:label "MegaVoltPerMetre"^^xsd:string ;
    rdfs:comment """1,000,000-fold of the SI derived unit volt divided by the SI base unit metre

-- QUDT"""@en ;
    rdfs:subClassOf [ a owl:Restriction ;
            owl:hasValue 1e+06 ;
            owl:onProperty ns1:hasSIConversionMultiplier ],
        [ a owl:Restriction ;
            owl:hasValue 0e+00 ;
            owl:onProperty ns1:hasSIConversionOffset ],
        [ a owl:Restriction ;
            owl:onProperty ns1:hasUnitSymbol ;
            owl:someValuesFrom ns1:VoltPerMetre ],
        ns1:ElectricFieldStrengthUnit,
        ns1:MegaPrefixedUnit,
        ns1:PrefixedUnit,
        ns1:SINonCoherentUnit ;
    skos:altLabel "Megavolt Per Metre"@en ;
    skos:prefLabel "MegaVoltPerMetre"^^xsd:string ;
    ns1:elucidation """1,000,000-fold of the SI derived unit volt divided by the SI base unit metre

-- QUDT"""@en ;
    ns1:qudtReference "http://qudt.org/vocab/unit/MegaV-PER-M"^^xsd:string ;
    ns1:ucumCode "MV.m-1"^^xsd:string ;
    ns1:unitSymbol "MV/m"^^xsd:string .

ns1:MicroBecquerelPerKilogram a owl:Class ;
    rdfs:label "MicroBecquerelPerKilogram"^^xsd:string ;
    rdfs:comment """One radioactive disintegration per hundred thousand seconds from an SI standard unit of mass of sample.

-- QUDT"""@en ;
    rdfs:subClassOf [ a owl:Restriction ;
            owl:hasValue 0e+00 ;
            owl:onProperty ns1:hasSIConversionOffset ],
        [ a owl:Restriction ;
            owl:onProperty ns1:hasUnitSymbol ;
            owl:someValuesFrom ns1:BecquerelPerKilogram ],
        [ a owl:Restriction ;
            owl:hasValue 1e-06 ;
            owl:onProperty ns1:hasSIConversionMultiplier ],
        ns1:MicroPrefixedUnit,
        ns1:PerTimeMassUnit,
        ns1:PrefixedUnit,
        ns1:SINonCoherentUnit ;
    skos:altLabel "Microbecquerels per kilogram"@en ;
    skos:prefLabel "MicroBecquerelPerKilogram"^^xsd:string ;
    ns1:elucidation """One radioactive disintegration per hundred thousand seconds from an SI standard unit of mass of sample.

-- QUDT"""@en ;
    ns1:qudtReference "http://qudt.org/vocab/unit/MicroBQ-PER-KiloGM"^^xsd:string ;
    ns1:ucumCode "uBq.kg-1"^^xsd:string ;
    ns1:unitSymbol "µBq/kg"^^xsd:string .

ns1:MicroCoulombPerCubicMetre a owl:Class ;
    rdfs:label "MicroCoulombPerCubicMetre"@en ;
    rdfs:comment """0.000001-fold of the SI derived unit coulomb divided by the power of the SI base unit metre with the exponent 3

-- QUDT"""@en ;
    rdfs:isDefinedBy "http://qudt.org/2.1/vocab/unit"^^xsd:string ;
    rdfs:subClassOf [ a owl:Restriction ;
            owl:hasValue 1e-06 ;
            owl:onProperty ns1:hasSIConversionMultiplier ],
        [ a owl:Restriction ;
            owl:hasValue 0e+00 ;
            owl:onProperty ns1:hasSIConversionOffset ],
        ns1:ElectricChargeDensityUnit,
        ns1:SINonCoherentDerivedUnit ;
    skos:altLabel "Microcoulomb Per Cubic Metre"@en ;
    skos:prefLabel "MicroCoulombPerCubicMetre"@en ;
    ns1:elucidation """0.000001-fold of the SI derived unit coulomb divided by the power of the SI base unit metre with the exponent 3

-- QUDT"""@en ;
    ns1:qudtReference "http://qudt.org/vocab/unit/MicroC-PER-M3"^^xsd:string ;
    ns1:ucumCode "uC.m-3"^^xsd:string ;
    ns1:unitSymbol "μC/m³"^^xsd:string .

ns1:MicroCoulombPerSquareMetre a owl:Class ;
    rdfs:label "MicroCoulombPerSquareMetre"@en ;
    rdfs:comment """0.000001-fold of the SI derived unit coulomb divided by the power of the SI base unit metre with the exponent 2

-- QUDT"""@en ;
    rdfs:isDefinedBy "http://qudt.org/2.1/vocab/unit"^^xsd:string ;
    rdfs:subClassOf [ a owl:Restriction ;
            owl:hasValue 0e+00 ;
            owl:onProperty ns1:hasSIConversionOffset ],
        [ a owl:Restriction ;
            owl:hasValue 1e-06 ;
            owl:onProperty ns1:hasSIConversionMultiplier ],
        ns1:ElectricDisplacementFieldUnit,
        ns1:SINonCoherentDerivedUnit ;
    skos:altLabel "Microcoulomb Per Square Metre"@en ;
    skos:prefLabel "MicroCoulombPerSquareMetre"@en ;
    ns1:elucidation """0.000001-fold of the SI derived unit coulomb divided by the power of the SI base unit metre with the exponent 2

-- QUDT"""@en ;
    ns1:qudtReference "http://qudt.org/vocab/unit/MicroC-PER-M2"^^xsd:string ;
    ns1:ucumCode "uC.m-2"^^xsd:string ;
    ns1:unitSymbol "μC/m²"^^xsd:string .

ns1:MicroFaradPerKiloMetre a owl:Class ;
    rdfs:label "MicroFaradPerKiloMetre"@en ;
    rdfs:comment """0.000001-fold of the SI derived unit farad divided by the 1,000-fold of the SI base unit metre

-- QUDT"""@en ;
    rdfs:isDefinedBy "http://qudt.org/2.1/vocab/unit"^^xsd:string ;
    rdfs:subClassOf [ a owl:Restriction ;
            owl:hasValue 0e+00 ;
            owl:onProperty ns1:hasSIConversionOffset ],
        [ a owl:Restriction ;
            owl:hasValue 1e-09 ;
            owl:onProperty ns1:hasSIConversionMultiplier ],
        ns1:PermittivityUnit,
        ns1:SINonCoherentDerivedUnit ;
    skos:altLabel "Microfarad Per Kilometre"@en ;
    skos:prefLabel "MicroFaradPerKiloMetre"@en ;
    ns1:elucidation """0.000001-fold of the SI derived unit farad divided by the 1,000-fold of the SI base unit metre

-- QUDT"""@en ;
    ns1:qudtReference "http://qudt.org/vocab/unit/MicroFARAD-PER-KiloM"^^xsd:string ;
    ns1:ucumCode "uF.km-1"^^xsd:string ;
    ns1:unitSymbol "μF/km"^^xsd:string .

ns1:MicroFaradPerMetre a owl:Class ;
    rdfs:label "MicroFaradPerMetre"@en ;
    rdfs:comment """0.000001-fold of the SI derived unit farad divided by the SI base unit metre.

-- QUDT"""@en ;
    rdfs:isDefinedBy "http://qudt.org/2.1/vocab/unit"^^xsd:string ;
    rdfs:subClassOf [ a owl:Restriction ;
            owl:hasValue 0e+00 ;
            owl:onProperty ns1:hasSIConversionOffset ],
        [ a owl:Restriction ;
            owl:hasValue 1e-06 ;
            owl:onProperty ns1:hasSIConversionMultiplier ],
        ns1:PermittivityUnit,
        ns1:SINonCoherentDerivedUnit ;
    skos:altLabel "Microfarad Per Metre"@en ;
    skos:prefLabel "MicroFaradPerMetre"@en ;
    ns1:elucidation """0.000001-fold of the SI derived unit farad divided by the SI base unit metre.

-- QUDT"""@en ;
    ns1:qudtReference "http://qudt.org/vocab/unit/MicroFARAD-PER-M"^^xsd:string ;
    ns1:ucumCode "uF.m-1"^^xsd:string ;
    ns1:unitSymbol "μF/m"^^xsd:string .

ns1:MicroGramPerCubicMetre a owl:Class ;
    rdfs:label "MicroGramPerCubicMetre"^^xsd:string ;
    rdfs:comment """0.000000001-fold of the SI base unit kilogram divided by the power of the SI base unit metre with the exponent 3

-- QUDT"""@en ;
    rdfs:isDefinedBy "http://qudt.org/2.1/vocab/unit"^^xsd:string ;
    rdfs:subClassOf [ a owl:Restriction ;
            owl:hasValue 1e-09 ;
            owl:onProperty ns1:hasSIConversionMultiplier ],
        [ a owl:Restriction ;
            owl:hasValue 0e+00 ;
            owl:onProperty ns1:hasSIConversionOffset ],
        ns1:DensityUnit,
        ns1:MeasurementUnit,
        ns1:PrefixedUnit,
        ns1:SINonCoherentUnit ;
    skos:altLabel "Microgram Per Cubic Metre"@en ;
    skos:prefLabel "MicroGramPerCubicMetre"^^xsd:string ;
    ns1:elucidation """0.000000001-fold of the SI base unit kilogram divided by the power of the SI base unit metre with the exponent 3

-- QUDT"""@en ;
    ns1:qudtReference "http://qudt.org/vocab/unit/MicroGM-PER-M3"^^xsd:string ;
    ns1:ucumCode "ug.m-3"^^xsd:string,
        "ug/m3"^^xsd:string ;
    ns1:unitSymbol "μg/m³"^^xsd:string .

ns1:MicroGramPerGram a owl:Class ;
    rdfs:label "MicroGramPerGram"^^xsd:string ;
    rdfs:comment """One part per 10**6 (million) by mass of the measurand in the matrix.

-- QUDT"""@en ;
    rdfs:subClassOf [ a owl:Restriction ;
            owl:hasValue 0e+00 ;
            owl:onProperty ns1:hasSIConversionOffset ],
        [ a owl:Restriction ;
            owl:hasValue 1e-06 ;
            owl:onProperty ns1:hasSIConversionMultiplier ],
        [ a owl:Restriction ;
            owl:onProperty ns1:hasUnitSymbol ;
            owl:someValuesFrom ns1:GramPerGram ],
        ns1:MassFractionUnit,
        ns1:MicroPrefixedUnit,
        ns1:PrefixedUnit,
        ns1:SINonCoherentUnit ;
    skos:altLabel "Micrograms per gram"@en ;
    skos:prefLabel "MicroGramPerGram"^^xsd:string ;
    ns1:elucidation """One part per 10**6 (million) by mass of the measurand in the matrix.

-- QUDT"""@en ;
    ns1:qudtReference "http://qudt.org/vocab/unit/MicroGM-PER-GM"^^xsd:string ;
    ns1:ucumCode "ug.g-1"^^xsd:string ;
    ns1:unitSymbol "µg/g"^^xsd:string .

ns1:MicroGramPerKilogram a owl:Class ;
    rdfs:label "MicroGramPerKilogram"^^xsd:string ;
    rdfs:comment """mass ratio as 0.000000001-fold of the SI base unit kilogram divided by the SI base unit kilogram

-- QUDT"""@en ;
    rdfs:isDefinedBy "http://qudt.org/2.1/vocab/unit"^^xsd:string ;
    rdfs:subClassOf [ a owl:Restriction ;
            owl:hasValue 1e-09 ;
            owl:onProperty ns1:hasSIConversionMultiplier ],
        [ a owl:Restriction ;
            owl:hasValue 0e+00 ;
            owl:onProperty ns1:hasSIConversionOffset ],
        ns1:MassFractionUnit,
        ns1:MeasurementUnit,
        ns1:PrefixedUnit,
        ns1:SINonCoherentUnit ;
    skos:altLabel "Microgram Per Kilogram"@en ;
    skos:prefLabel "MicroGramPerKilogram"^^xsd:string ;
    ns1:elucidation """mass ratio as 0.000000001-fold of the SI base unit kilogram divided by the SI base unit kilogram

-- QUDT"""@en ;
    ns1:qudtReference "http://qudt.org/vocab/unit/MicroGM-PER-KiloGM"^^xsd:string ;
    ns1:ucumCode "ug.kg-1"^^xsd:string,
        "ug/kg"^^xsd:string ;
    ns1:unitSymbol "μg/kg"^^xsd:string .

ns1:MicroGramPerSquareCentiMetre a owl:Class ;
    rdfs:label "MicroGramPerSquareCentiMetre"^^xsd:string ;
    rdfs:comment """A unit of mass per area, equivalent to 0.01 grammes per square metre

-- QUDT"""@en ;
    rdfs:subClassOf [ a owl:Restriction ;
            owl:hasValue 1e-02 ;
            owl:onProperty ns1:hasSIConversionMultiplier ],
        [ a owl:Restriction ;
            owl:hasValue 0e+00 ;
            owl:onProperty ns1:hasSIConversionOffset ],
        [ a owl:Restriction ;
            owl:onProperty ns1:hasUnitNonPrefixPart ;
            owl:someValuesFrom ns1:GramPerSquareCentiMetre ],
        ns1:AreaDensityUnit,
        ns1:MicroPrefixedUnit,
        ns1:PrefixedUnit,
        ns1:SINonCoherentUnit ;
    skos:altLabel "Microgram per square centimetre"@en ;
    skos:prefLabel "MicroGramPerSquareCentiMetre"^^xsd:string ;
    ns1:elucidation """A unit of mass per area, equivalent to 0.01 grammes per square metre

-- QUDT"""@en ;
    ns1:qudtReference "http://qudt.org/vocab/unit/MicroG-PER-CentiM2"^^xsd:string ;
    ns1:unitSymbol "µg/cm²"^^xsd:string .

ns1:MicroHenryPerKiloOhm a owl:Class ;
    rdfs:label "MicroHenryPerKiloOhm"^^xsd:string ;
    rdfs:comment """0.000001-fold of the SI derived unit henry divided by the 1,000-fold of the SI derived unit ohm

-- QUDT"""@en ;
    rdfs:subClassOf [ a owl:Restriction ;
            owl:hasValue 1e-09 ;
            owl:onProperty ns1:hasSIConversionMultiplier ],
        [ a owl:Restriction ;
            owl:onProperty ns1:hasUnitNonPrefixPart ;
            owl:someValuesFrom ns1:HenryPerKiloOhm ],
        [ a owl:Restriction ;
            owl:hasValue 0e+00 ;
            owl:onProperty ns1:hasSIConversionOffset ],
        ns1:MicroPrefixedUnit,
        ns1:PrefixedUnit,
        ns1:SINonCoherentUnit,
        ns1:TimeUnit ;
    skos:altLabel "Microhenry Per Kiloohm"@en ;
    skos:prefLabel "MicroHenryPerKiloOhm"^^xsd:string ;
    ns1:elucidation """0.000001-fold of the SI derived unit henry divided by the 1,000-fold of the SI derived unit ohm

-- QUDT"""@en ;
    ns1:qudtReference "http://qudt.org/vocab/unit/MicroH-PER-KiloOHM"^^xsd:string ;
    ns1:ucumCode "uH.kOhm-1"^^xsd:string ;
    ns1:unitSymbol "µH/kΩ"^^xsd:string .

ns1:MicroHenryPerMetre a owl:Class ;
    rdfs:label "MicroHenryPerMetre"^^xsd:string ;
    rdfs:comment """0.000001-fold of the SI derived unit henry divided by the SI base unit metre

-- QUDT"""@en ;
    rdfs:subClassOf [ a owl:Restriction ;
            owl:hasValue 1e-06 ;
            owl:onProperty ns1:hasSIConversionMultiplier ],
        [ a owl:Restriction ;
            owl:hasValue 0e+00 ;
            owl:onProperty ns1:hasSIConversionOffset ],
        ns1:PermeabilityUnit,
        ns1:SINonCoherentDerivedUnit ;
    skos:altLabel "Microhenry Per Metre"@en ;
    skos:prefLabel "MicroHenryPerMetre"^^xsd:string ;
    ns1:elucidation """0.000001-fold of the SI derived unit henry divided by the SI base unit metre

-- QUDT"""@en ;
    ns1:qudtReference "http://qudt.org/vocab/unit/MicroH-PER-M"^^xsd:string ;
    ns1:ucumCode "uH.m-1"^^xsd:string ;
    ns1:unitSymbol "μH/m"^^xsd:string .

ns1:MicroHenryPerOhm a owl:Class ;
    rdfs:label "MicroHenryPerOhm"^^xsd:string ;
    rdfs:comment """0.000001-fold of the SI derived unit henry divided by the SI derived unit ohm

-- QUDT"""@en ;
    rdfs:subClassOf [ a owl:Restriction ;
            owl:hasValue 1e-06 ;
            owl:onProperty ns1:hasSIConversionMultiplier ],
        [ a owl:Restriction ;
            owl:onProperty ns1:hasUnitSymbol ;
            owl:someValuesFrom ns1:HenryPerOhm ],
        [ a owl:Restriction ;
            owl:hasValue 0e+00 ;
            owl:onProperty ns1:hasSIConversionOffset ],
        ns1:MicroPrefixedUnit,
        ns1:PrefixedUnit,
        ns1:SINonCoherentUnit,
        ns1:TimeUnit ;
    skos:altLabel "Microhenry Per Ohm"@en ;
    skos:prefLabel "MicroHenryPerOhm"^^xsd:string ;
    ns1:elucidation """0.000001-fold of the SI derived unit henry divided by the SI derived unit ohm

-- QUDT"""@en ;
    ns1:qudtReference "http://qudt.org/vocab/unit/MicroH-PER-OHM"^^xsd:string ;
    ns1:ucumCode "uH.Ohm-1"^^xsd:string ;
    ns1:unitSymbol "µH/Ω"^^xsd:string .

ns1:MicroMetrePerKelvin a owl:Class ;
    rdfs:label "MicroMetrePerKelvin"@en ;
    rdfs:comment """0.000001-fold of the SI base unit metre divided by the SI base unit kelvin

-- QUDT"""@en ;
    rdfs:isDefinedBy "http://qudt.org/2.1/vocab/unit"^^xsd:string ;
    rdfs:subClassOf [ a owl:Restriction ;
            owl:hasValue 1e-06 ;
            owl:onProperty ns1:hasSIConversionMultiplier ],
        [ a owl:Restriction ;
            owl:hasValue 0e+00 ;
            owl:onProperty ns1:hasSIConversionOffset ],
        ns1:LengthPerTemperatureUnit,
        ns1:SINonCoherentDerivedUnit ;
    skos:altLabel "Micrometre Per Kelvin"@en ;
    skos:prefLabel "MicroMetrePerKelvin"@en ;
    ns1:elucidation """0.000001-fold of the SI base unit metre divided by the SI base unit kelvin

-- QUDT"""@en ;
    ns1:qudtReference "http://qudt.org/vocab/unit/MicroM-PER-K"^^xsd:string ;
    ns1:ucumCode "um.K-1"^^xsd:string ;
    ns1:unitSymbol "μm/K"^^xsd:string .

ns1:MicroMetrePerNewton a owl:Class ;
    rdfs:label "MicroMetrePerNewton"@en ;
    rdfs:comment """Micro metres measured per Newton

-- QUDT"""@en ;
    rdfs:subClassOf [ a owl:Restriction ;
            owl:hasValue 0e+00 ;
            owl:onProperty ns1:hasSIConversionOffset ],
        [ a owl:Restriction ;
            owl:hasValue 1e-06 ;
            owl:onProperty ns1:hasSIConversionMultiplier ],
        ns1:MicroPrefixedUnit,
        ns1:PrefixedUnit,
        ns1:SINonCoherentUnit,
        ns1:SquareTimePerMassUnit ;
    skos:altLabel "Micro metre per Newton"@en ;
    skos:prefLabel "MicroMetrePerNewton"@en ;
    ns1:elucidation """Micro metres measured per Newton

-- QUDT"""@en ;
    ns1:qudtReference "http://qudt.org/vocab/unit/MicroM-PER-N"^^xsd:string ;
    ns1:unitSymbol "µJ/N"^^xsd:string .

ns1:MicroMolePerGram a owl:Class ;
    rdfs:label "MicroMolePerGram"^^xsd:string ;
    rdfs:comment """0.000001-fold of the SI base unit mol divided by the 0.001-fold of the SI base unit kilogram

-- QUDT"""@en ;
    rdfs:subClassOf [ a owl:Restriction ;
            owl:hasValue 0e+00 ;
            owl:onProperty ns1:hasSIConversionOffset ],
        [ a owl:Restriction ;
            owl:hasValue 1e-03 ;
            owl:onProperty ns1:hasSIConversionMultiplier ],
        ns1:AmountPerMassUnit,
        ns1:MicroPrefixedUnit,
        ns1:PrefixedUnit,
        ns1:SINonCoherentUnit ;
    skos:altLabel "Micromoles per gram"@en ;
    skos:prefLabel "MicroMolePerGram"^^xsd:string ;
    ns1:elucidation """0.000001-fold of the SI base unit mol divided by the 0.001-fold of the SI base unit kilogram

-- QUDT"""@en ;
    ns1:qudtReference "http://qudt.org/vocab/unit/MicroMOL-PER-GM"^^xsd:string ;
    ns1:ucumCode "umol.g-1"^^xsd:string,
        "umol/g"^^xsd:string ;
    ns1:unitSymbol "µmol/g"^^xsd:string .

ns1:MicroMolePerGramPerSecond a owl:Class ;
    rdfs:label "MicroMolePerGramPerSecond"^^xsd:string ;
    rdfs:subClassOf [ a owl:Restriction ;
            owl:hasValue 1e-04 ;
            owl:onProperty ns1:hasSIConversionMultiplier ],
        [ a owl:Restriction ;
            owl:hasValue 0e+00 ;
            owl:onProperty ns1:hasSIConversionOffset ],
        ns1:AmountPerMassTimeUnit,
        ns1:SINonCoherentDerivedUnit ;
    skos:altLabel "Micromoles per gram per second"@en ;
    skos:prefLabel "MicroMolePerGramPerSecond"^^xsd:string ;
    ns1:qudtReference "http://qudt.org/vocab/unit/MicroMOL-PER-GM-SEC"^^xsd:string ;
    ns1:ucumCode "umol.g-1.s-1"^^xsd:string,
        "umol/g/s"^^xsd:string ;
    ns1:unitSymbol "μmol/(g⋅s)"^^xsd:string .

ns1:MicroMolePerKilogram a owl:Class ;
    rdfs:label "MicroMolePerKilogram"^^xsd:string ;
    rdfs:subClassOf [ a owl:Restriction ;
            owl:hasValue 1e-06 ;
            owl:onProperty ns1:hasSIConversionMultiplier ],
        [ a owl:Restriction ;
            owl:hasValue 0e+00 ;
            owl:onProperty ns1:hasSIConversionOffset ],
        ns1:AmountPerMassUnit,
        ns1:MicroPrefixedUnit,
        ns1:PrefixedUnit,
        ns1:SINonCoherentUnit ;
    skos:altLabel "Micromoles per kilogram"@en ;
    skos:prefLabel "MicroMolePerKilogram"^^xsd:string ;
    ns1:qudtReference "http://qudt.org/vocab/unit/MicroMOL-PER-KiloGM"^^xsd:string ;
    ns1:ucumCode "umol.kg-1"^^xsd:string,
        "umol/kg"^^xsd:string ;
    ns1:unitSymbol "µmol/kg"^^xsd:string .

ns1:MicroMolePerMole a owl:Class ;
    rdfs:label "MicroMolePerMole"@en ;
    rdfs:subClassOf [ a owl:Restriction ;
            owl:hasValue 0e+00 ;
            owl:onProperty ns1:hasSIConversionOffset ],
        [ a owl:Restriction ;
            owl:hasValue 1e-06 ;
            owl:onProperty ns1:hasSIConversionMultiplier ],
        ns1:AmountFractionUnit,
        ns1:MicroPrefixedUnit,
        ns1:PrefixedUnit,
        ns1:SINonCoherentUnit ;
    skos:altLabel "Micromoles per mole"@en ;
    skos:prefLabel "MicroMolePerMole"@en ;
    ns1:qudtReference "http://qudt.org/vocab/unit/MicroMOL-PER-MOL"^^xsd:string ;
    ns1:ucumCode "umol.mol-1"^^xsd:string,
        "umol/mol"^^xsd:string ;
    ns1:unitSymbol "µmol/mol"^^xsd:string .

ns1:MicroMolePerSecond a owl:Class ;
    rdfs:label "MicroMolePerSecond"^^xsd:string ;
    rdfs:comment """ This unit is used commonly to describe Photosynthetic Photon Flux (PPF) - the total number of photons emitted by a light source each second within the PAR wavelength range.

-- QUDT"""@en ;
    rdfs:subClassOf [ a owl:Restriction ;
            owl:hasValue 1e-06 ;
            owl:onProperty ns1:hasSIConversionMultiplier ],
        [ a owl:Restriction ;
            owl:onProperty ns1:hasUnitSymbol ;
            owl:someValuesFrom ns1:MolePerSecond ],
        [ a owl:Restriction ;
            owl:hasValue 0e+00 ;
            owl:onProperty ns1:hasSIConversionOffset ],
        ns1:CatalyticActivityUnit,
        ns1:MicroPrefixedUnit,
        ns1:PrefixedUnit,
        ns1:SINonCoherentUnit ;
    skos:altLabel "Micromoles per second"@en ;
    skos:prefLabel "MicroMolePerSecond"^^xsd:string ;
    ns1:elucidation """ This unit is used commonly to describe Photosynthetic Photon Flux (PPF) - the total number of photons emitted by a light source each second within the PAR wavelength range.

-- QUDT"""@en ;
    ns1:qudtReference "http://qudt.org/vocab/unit/MicroMOL-PER-SEC"^^xsd:string ;
    ns1:ucumCode "umol.s-1"^^xsd:string,
        "umol/s"^^xsd:string ;
    ns1:unitSymbol "µmol/s"^^xsd:string .

ns1:MicroMolePerSquareMetre a owl:Class ;
    rdfs:label "MicroMolePerSquareMetre"^^xsd:string ;
    rdfs:comment """One part per 10**6 (million) of the SI unit of quantity of matter (the mole) per SI unit area.

-- QUDT"""@en ;
    rdfs:subClassOf [ a owl:Restriction ;
            owl:onProperty ns1:hasUnitSymbol ;
            owl:someValuesFrom ns1:MolePerSquareMetre ],
        [ a owl:Restriction ;
            owl:hasValue 1e-06 ;
            owl:onProperty ns1:hasSIConversionMultiplier ],
        [ a owl:Restriction ;
            owl:hasValue 0e+00 ;
            owl:onProperty ns1:hasSIConversionOffset ],
        ns1:AmountPerAreaUnit,
        ns1:MicroPrefixedUnit,
        ns1:PrefixedUnit,
        ns1:SINonCoherentUnit ;
    skos:altLabel "Micromoles per square metre"@en ;
    skos:prefLabel "MicroMolePerSquareMetre"^^xsd:string ;
    ns1:elucidation """One part per 10**6 (million) of the SI unit of quantity of matter (the mole) per SI unit area.

-- QUDT"""@en ;
    ns1:qudtReference "http://qudt.org/vocab/unit/MicroMOL-PER-M2"^^xsd:string ;
    ns1:ucumCode "umol.m-2"^^xsd:string,
        "umol/m2"^^xsd:string ;
    ns1:unitSymbol "µmol/m²"^^xsd:string .

ns1:MicroMolePerSquareMetrePerSecond a owl:Class ;
    rdfs:label "MicroMolePerSquareMetrePerSecond"^^xsd:string ;
    rdfs:comment """One part per 10**6 (million) of the SI unit of quantity of matter (the mole) per SI unit area per SI unit of time.  This term is based on the number of photons in a certain waveband incident per unit time (s) on a unit area (m2) divided by the Avogadro constant (6.022 x 1023 mol-1). It is used commonly to describe PAR in the 400-700 nm waveband. Definition Source: Thimijan, Richard W., and Royal D. Heins. 1982. Photometric, Radiometric, and Quantum Light Units of Measure: A Review of Procedures for Interconversion. HortScience 18:818-822.

-- QUDT"""@en ;
    rdfs:subClassOf [ a owl:Restriction ;
            owl:onProperty ns1:hasUnitSymbol ;
            owl:someValuesFrom ns1:MolePerSquareMetrePerSecond ],
        [ a owl:Restriction ;
            owl:hasValue 1e-06 ;
            owl:onProperty ns1:hasSIConversionMultiplier ],
        [ a owl:Restriction ;
            owl:hasValue 0e+00 ;
            owl:onProperty ns1:hasSIConversionOffset ],
        ns1:AmountPerAreaTimeUnit,
        ns1:MicroPrefixedUnit,
        ns1:PrefixedUnit,
        ns1:SINonCoherentUnit ;
    skos:altLabel "Micromoles per square metre per second"@en ;
    skos:prefLabel "MicroMolePerSquareMetrePerSecond"^^xsd:string ;
    ns1:elucidation """One part per 10**6 (million) of the SI unit of quantity of matter (the mole) per SI unit area per SI unit of time.  This term is based on the number of photons in a certain waveband incident per unit time (s) on a unit area (m2) divided by the Avogadro constant (6.022 x 1023 mol-1). It is used commonly to describe PAR in the 400-700 nm waveband. Definition Source: Thimijan, Richard W., and Royal D. Heins. 1982. Photometric, Radiometric, and Quantum Light Units of Measure: A Review of Procedures for Interconversion. HortScience 18:818-822.

-- QUDT"""@en ;
    ns1:qudtReference "http://qudt.org/vocab/unit/MicroMOL-PER-M2-SEC"^^xsd:string ;
    ns1:ucumCode "umol.m-2.s-1"^^xsd:string,
        "umol/m2/s"^^xsd:string ;
    ns1:unitSymbol "µmol/(m²⋅s)"^^xsd:string .

ns1:MicroNewtonMetre a owl:Class ;
    rdfs:label "MicroNewtonMetre"@en ;
    rdfs:comment """0.000001-fold of the product out of the derived SI newton and the SI base unit metre

-- QUDT"""@en ;
    rdfs:isDefinedBy "http://qudt.org/2.1/vocab/unit"^^xsd:string ;
    rdfs:subClassOf [ a owl:Restriction ;
            owl:hasValue 1e-06 ;
            owl:onProperty ns1:hasSIConversionMultiplier ],
        [ a owl:Restriction ;
            owl:hasValue 0e+00 ;
            owl:onProperty ns1:hasSIConversionOffset ],
        ns1:EnergyUnit,
        ns1:SINonCoherentDerivedUnit ;
    skos:altLabel "Micronewton Metre"@en ;
    skos:prefLabel "MicroNewtonMetre"@en ;
    ns1:elucidation """0.000001-fold of the product out of the derived SI newton and the SI base unit metre

-- QUDT"""@en ;
    ns1:qudtReference "http://qudt.org/vocab/unit/MicroN-M"^^xsd:string ;
    ns1:ucumCode "uN.m"^^xsd:string ;
    ns1:unitSymbol "μN⋅m"^^xsd:string .

ns1:MicroSiemensPerCentiMetre a owl:Class ;
    rdfs:label "MicroSiemensPerCentiMetre"@en ;
    rdfs:comment """0.000001-fold of the SI derived unit Siemens divided by the 0.01-fold of the SI base unit metre

-- QUDT"""@en ;
    rdfs:isDefinedBy "http://qudt.org/2.1/vocab/unit"^^xsd:string ;
    rdfs:subClassOf [ a owl:Restriction ;
            owl:hasValue 1e-04 ;
            owl:onProperty ns1:hasSIConversionMultiplier ],
        [ a owl:Restriction ;
            owl:hasValue 0e+00 ;
            owl:onProperty ns1:hasSIConversionOffset ],
        ns1:ElectricConductivityUnit,
        ns1:SINonCoherentDerivedUnit ;
    skos:altLabel "Microsiemens Per Centimetre"@en ;
    skos:prefLabel "MicroSiemensPerCentiMetre"@en ;
    ns1:elucidation """0.000001-fold of the SI derived unit Siemens divided by the 0.01-fold of the SI base unit metre

-- QUDT"""@en ;
    ns1:qudtReference "http://qudt.org/vocab/unit/MicroS-PER-CentiM"^^xsd:string ;
    ns1:ucumCode "uS.cm-1"^^xsd:string ;
    ns1:unitSymbol "μS/cm"^^xsd:string .

ns1:MicroSiemensPerMetre a owl:Class ;
    rdfs:label "MicroSiemensPerMetre"@en ;
    rdfs:comment """0.000001-fold of the SI derived unit Siemens divided by the SI base unit metre

-- QUDT"""@en ;
    rdfs:isDefinedBy "http://qudt.org/2.1/vocab/unit"^^xsd:string ;
    rdfs:subClassOf [ a owl:Restriction ;
            owl:hasValue 1e-06 ;
            owl:onProperty ns1:hasSIConversionMultiplier ],
        [ a owl:Restriction ;
            owl:hasValue 0e+00 ;
            owl:onProperty ns1:hasSIConversionOffset ],
        ns1:ElectricConductivityUnit,
        ns1:SINonCoherentDerivedUnit ;
    skos:altLabel "Microsiemens Per Metre"@en ;
    skos:prefLabel "MicroSiemensPerMetre"@en ;
    ns1:elucidation """0.000001-fold of the SI derived unit Siemens divided by the SI base unit metre

-- QUDT"""@en ;
    ns1:qudtReference "http://qudt.org/vocab/unit/MicroS-PER-M"^^xsd:string ;
    ns1:ucumCode "uS.m-1"^^xsd:string ;
    ns1:unitSymbol "μS/m"^^xsd:string .

ns1:MicroVoltPerMetre a owl:Class ;
    rdfs:label "MicroVoltPerMetre"^^xsd:string ;
    rdfs:comment """0.000001-fold of the SI derived unit volt divided by the SI base unit metre

-- QUDT"""@en ;
    rdfs:subClassOf [ a owl:Restriction ;
            owl:hasValue 1e-06 ;
            owl:onProperty ns1:hasSIConversionMultiplier ],
        [ a owl:Restriction ;
            owl:hasValue 0e+00 ;
            owl:onProperty ns1:hasSIConversionOffset ],
        [ a owl:Restriction ;
            owl:onProperty ns1:hasUnitSymbol ;
            owl:someValuesFrom ns1:VoltPerMetre ],
        ns1:ElectricFieldStrengthUnit,
        ns1:MicroPrefixedUnit,
        ns1:PrefixedUnit,
        ns1:SINonCoherentUnit ;
    skos:altLabel "Microvolt Per Metre"@en ;
    skos:prefLabel "MicroVoltPerMetre"^^xsd:string ;
    ns1:elucidation """0.000001-fold of the SI derived unit volt divided by the SI base unit metre

-- QUDT"""@en ;
    ns1:qudtReference "http://qudt.org/vocab/unit/MicroV-PER-M"^^xsd:string ;
    ns1:ucumCode "uV.m-1"^^xsd:string ;
    ns1:unitSymbol "µV/m"^^xsd:string .

ns1:MicroWattPerSquareMetre a owl:Class ;
    rdfs:label "MicroWattPerSquareMetre"^^xsd:string ;
    rdfs:comment """0.000001-fold of the SI derived unit watt divided by the power of the SI base unit metre with the exponent 2

-- QUDT"""@en ;
    rdfs:subClassOf [ a owl:Restriction ;
            owl:onProperty ns1:hasUnitSymbol ;
            owl:someValuesFrom ns1:WattPerSquareMetre ],
        [ a owl:Restriction ;
            owl:hasValue 1e-06 ;
            owl:onProperty ns1:hasSIConversionMultiplier ],
        [ a owl:Restriction ;
            owl:hasValue 0e+00 ;
            owl:onProperty ns1:hasSIConversionOffset ],
        ns1:MicroPrefixedUnit,
        ns1:PowerDensityUnit,
        ns1:PrefixedUnit,
        ns1:SINonCoherentUnit ;
    skos:altLabel "Microwatt Per Square Metre"@en ;
    skos:prefLabel "MicroWattPerSquareMetre"^^xsd:string ;
    ns1:elucidation """0.000001-fold of the SI derived unit watt divided by the power of the SI base unit metre with the exponent 2

-- QUDT"""@en ;
    ns1:qudtReference "http://qudt.org/vocab/unit/MicroW-PER-M2"^^xsd:string ;
    ns1:ucumCode "uW.m-2"^^xsd:string ;
    ns1:unitSymbol "µW/m²"^^xsd:string .

ns1:MilliAmperePerMilliMetre a owl:Class ;
    rdfs:label "MilliAmperePerMilliMetre"^^xsd:string ;
    rdfs:comment """0.001-fold of the SI base unit ampere  divided by the 0.001-fold of the SI base unit metre

-- QUDT"""@en ;
    rdfs:subClassOf [ a owl:Restriction ;
            owl:hasValue 0e+00 ;
            owl:onProperty ns1:hasSIConversionOffset ],
        [ a owl:Restriction ;
            owl:hasValue 1e+00 ;
            owl:onProperty ns1:hasSIConversionMultiplier ],
        [ a owl:Restriction ;
            owl:onProperty ns1:hasUnitNonPrefixPart ;
            owl:someValuesFrom ns1:AmperePerMilliMetre ],
        ns1:MagneticFieldStrengthUnit,
        ns1:MilliPrefixedUnit,
        ns1:PrefixedUnit,
        ns1:SINonCoherentUnit ;
    skos:altLabel "Milliampere Per Millimetre"@en ;
    skos:prefLabel "MilliAmperePerMilliMetre"^^xsd:string ;
    ns1:elucidation """0.001-fold of the SI base unit ampere  divided by the 0.001-fold of the SI base unit metre

-- QUDT"""@en ;
    ns1:qudtReference "http://qudt.org/vocab/unit/MilliA-PER-MilliM"^^xsd:string ;
    ns1:ucumCode "mA.mm-1"^^xsd:string ;
    ns1:unitSymbol "mA/mm"^^xsd:string .

ns1:MilliAmperePerSquareCentiMetre a owl:Class ;
    rdfs:label "MilliAmperePerSquareCentiMetre"@en ;
    rdfs:comment "0.001-fold of the SI base unit ampere divided by the 0.0001-fold  of the power of the SI base unit metre by exponent 2"@en ;
    rdfs:subClassOf [ a owl:Restriction ;
            owl:hasValue 0e+00 ;
            owl:onProperty ns1:hasSIConversionOffset ],
        [ a owl:Restriction ;
            owl:hasValue 1e+01 ;
            owl:onProperty ns1:hasSIConversionMultiplier ],
        ns1:ElectricCurrentDensityUnit,
        ns1:MilliPrefixedUnit,
        ns1:SINonCoherentUnit ;
    skos:prefLabel "MilliAmperePerSquareCentiMetre"@en ;
    ns1:elucidation "0.001-fold of the SI base unit ampere divided by the 0.0001-fold  of the power of the SI base unit metre by exponent 2"@en ;
    ns1:unitSymbol "mA/cm²"^^xsd:string .

ns1:MilliBecquerelPerGram a owl:Class ;
    rdfs:label "MilliBecquerelPerGram"^^xsd:string ;
    rdfs:comment """One radioactive disintegration per thousand seconds per 1000th SI unit of sample mass.

-- QUDT"""@en ;
    rdfs:subClassOf [ a owl:Restriction ;
            owl:hasValue 0e+00 ;
            owl:onProperty ns1:hasSIConversionOffset ],
        [ a owl:Restriction ;
            owl:hasValue 1e+00 ;
            owl:onProperty ns1:hasSIConversionMultiplier ],
        ns1:MilliPrefixedUnit,
        ns1:PerTimeMassUnit,
        ns1:PrefixedUnit,
        ns1:SINonCoherentUnit ;
    skos:altLabel "Millibecquerels per gram"@en ;
    skos:prefLabel "MilliBecquerelPerGram"^^xsd:string ;
    ns1:elucidation """One radioactive disintegration per thousand seconds per 1000th SI unit of sample mass.

-- QUDT"""@en ;
    ns1:qudtReference "http://qudt.org/vocab/unit/MilliBQ-PER-GM"^^xsd:string ;
    ns1:ucumCode "mBq.g-1"^^xsd:string ;
    ns1:unitSymbol "mBq/g"^^xsd:string .

ns1:MilliBecquerelPerKilogram a owl:Class ;
    rdfs:label "MilliBecquerelPerKilogram"^^xsd:string ;
    rdfs:comment """One radioactive disintegration per thousand seconds from an SI standard unit of mass of sample.

-- QUDT"""@en ;
    rdfs:subClassOf [ a owl:Restriction ;
            owl:hasValue 0e+00 ;
            owl:onProperty ns1:hasSIConversionOffset ],
        [ a owl:Restriction ;
            owl:onProperty ns1:hasUnitSymbol ;
            owl:someValuesFrom ns1:BecquerelPerKilogram ],
        [ a owl:Restriction ;
            owl:hasValue 1e-03 ;
            owl:onProperty ns1:hasSIConversionMultiplier ],
        ns1:MilliPrefixedUnit,
        ns1:PerTimeMassUnit,
        ns1:PrefixedUnit,
        ns1:SINonCoherentUnit ;
    skos:altLabel "Millibecquerels per kilogram"@en ;
    skos:prefLabel "MilliBecquerelPerKilogram"^^xsd:string ;
    ns1:elucidation """One radioactive disintegration per thousand seconds from an SI standard unit of mass of sample.

-- QUDT"""@en ;
    ns1:qudtReference "http://qudt.org/vocab/unit/MilliBQ-PER-KiloGM"^^xsd:string ;
    ns1:ucumCode "mBq.kg-1"^^xsd:string ;
    ns1:unitSymbol "mBq/kg"^^xsd:string .

ns1:MilliCoulombPerCubicMetre a owl:Class ;
    rdfs:label "MilliCoulombPerCubicMetre"^^xsd:string ;
    rdfs:comment """0.001-fold of the SI derived unit coulomb divided by the power of the SI base unit metre with the exponent 3

-- QUDT"""@en ;
    rdfs:subClassOf [ a owl:Restriction ;
            owl:hasValue 0e+00 ;
            owl:onProperty ns1:hasSIConversionOffset ],
        [ a owl:Restriction ;
            owl:hasValue 1e-03 ;
            owl:onProperty ns1:hasSIConversionMultiplier ],
        [ a owl:Restriction ;
            owl:onProperty ns1:hasUnitSymbol ;
            owl:someValuesFrom ns1:CoulombPerCubicMetre ],
        ns1:ElectricChargeDensityUnit,
        ns1:MilliPrefixedUnit,
        ns1:PrefixedUnit,
        ns1:SINonCoherentUnit ;
    skos:altLabel "Millicoulomb Per Cubic Metre"@en ;
    skos:prefLabel "MilliCoulombPerCubicMetre"^^xsd:string ;
    ns1:elucidation """0.001-fold of the SI derived unit coulomb divided by the power of the SI base unit metre with the exponent 3

-- QUDT"""@en ;
    ns1:qudtReference "http://qudt.org/vocab/unit/MilliC-PER-M3"^^xsd:string ;
    ns1:ucumCode "mC.m-3"^^xsd:string ;
    ns1:unitSymbol "mC/m³"^^xsd:string .

ns1:MilliCoulombPerKilogram a owl:Class ;
    rdfs:label "MilliCoulombPerKilogram"^^xsd:string ;
    rdfs:comment """0.001-fold of the SI derived unit coulomb divided by the SI base unit kilogram

-- QUDT"""@en ;
    rdfs:subClassOf [ a owl:Restriction ;
            owl:onProperty ns1:hasUnitSymbol ;
            owl:someValuesFrom ns1:CoulombPerKilogram ],
        [ a owl:Restriction ;
            owl:hasValue 1e-03 ;
            owl:onProperty ns1:hasSIConversionMultiplier ],
        [ a owl:Restriction ;
            owl:hasValue 0e+00 ;
            owl:onProperty ns1:hasSIConversionOffset ],
        ns1:ElectricChargePerMassUnit,
        ns1:MilliPrefixedUnit,
        ns1:PrefixedUnit,
        ns1:SINonCoherentUnit ;
    skos:altLabel "Millicoulomb Per Kilogram"@en ;
    skos:prefLabel "MilliCoulombPerKilogram"^^xsd:string ;
    ns1:elucidation """0.001-fold of the SI derived unit coulomb divided by the SI base unit kilogram

-- QUDT"""@en ;
    ns1:qudtReference "http://qudt.org/vocab/unit/MilliC-PER-KiloGM"^^xsd:string ;
    ns1:ucumCode "mC.kg-1"^^xsd:string ;
    ns1:unitSymbol "mC/kg"^^xsd:string .

ns1:MilliCoulombPerSquareMetre a owl:Class ;
    rdfs:label "MilliCoulombPerSquareMetre"^^xsd:string ;
    rdfs:comment """0.001-fold of the SI derived unit coulomb divided by the power of the SI base unit metre with the exponent 2

-- QUDT"""@en ;
    rdfs:subClassOf [ a owl:Restriction ;
            owl:hasValue 1e-03 ;
            owl:onProperty ns1:hasSIConversionMultiplier ],
        [ a owl:Restriction ;
            owl:onProperty ns1:hasUnitSymbol ;
            owl:someValuesFrom ns1:CoulombPerSquareMetre ],
        [ a owl:Restriction ;
            owl:hasValue 0e+00 ;
            owl:onProperty ns1:hasSIConversionOffset ],
        ns1:ElectricDisplacementFieldUnit,
        ns1:MilliPrefixedUnit,
        ns1:PrefixedUnit,
        ns1:SINonCoherentUnit ;
    skos:altLabel "Millicoulomb Per Square Metre"@en ;
    skos:prefLabel "MilliCoulombPerSquareMetre"^^xsd:string ;
    ns1:elucidation """0.001-fold of the SI derived unit coulomb divided by the power of the SI base unit metre with the exponent 2

-- QUDT"""@en ;
    ns1:qudtReference "http://qudt.org/vocab/unit/MilliC-PER-M2"^^xsd:string ;
    ns1:ucumCode "mC.m-2"^^xsd:string ;
    ns1:unitSymbol "mC/m²"^^xsd:string .

ns1:MilliGramPerCubicMetre a owl:Class ;
    rdfs:label "MilliGramPerCubicMetre"^^xsd:string ;
    rdfs:comment """0.000001-fold of the SI base unit kilogram divided by the power of the SI base unit metre with the exponent 3

-- QUDT"""@en ;
    rdfs:subClassOf [ a owl:Restriction ;
            owl:hasValue 0e+00 ;
            owl:onProperty ns1:hasSIConversionOffset ],
        [ a owl:Restriction ;
            owl:onProperty ns1:hasUnitSymbol ;
            owl:someValuesFrom ns1:GramPerCubicMetre ],
        [ a owl:Restriction ;
            owl:hasValue 1e-06 ;
            owl:onProperty ns1:hasSIConversionMultiplier ],
        ns1:DensityUnit,
        ns1:MilliPrefixedUnit,
        ns1:PrefixedUnit,
        ns1:SINonCoherentUnit ;
    skos:altLabel "Milligram Per Cubic Metre"@en ;
    skos:prefLabel "MilliGramPerCubicMetre"^^xsd:string ;
    ns1:elucidation """0.000001-fold of the SI base unit kilogram divided by the power of the SI base unit metre with the exponent 3

-- QUDT"""@en ;
    ns1:qudtReference "http://qudt.org/vocab/unit/MilliGM-PER-M3"^^xsd:string ;
    ns1:ucumCode "mg.m-3"^^xsd:string,
        "mg/m3"^^xsd:string ;
    ns1:unitSymbol "mg/m³"^^xsd:string .

ns1:MilliGramPerCubicMetrePerSecond a owl:Class ;
    rdfs:label "MilliGramPerCubicMetrePerSecond"^^xsd:string ;
    rdfs:subClassOf [ a owl:Restriction ;
            owl:hasValue 0e+00 ;
            owl:onProperty ns1:hasSIConversionOffset ],
        [ a owl:Restriction ;
            owl:hasValue 1e-06 ;
            owl:onProperty ns1:hasSIConversionMultiplier ],
        ns1:MassPerVolumeTimeUnit,
        ns1:MilliPrefixedUnit,
        ns1:PrefixedUnit,
        ns1:SINonCoherentUnit ;
    skos:altLabel "Milligrams per cubic metre per second"@en ;
    skos:prefLabel "MilliGramPerCubicMetrePerSecond"^^xsd:string ;
    ns1:qudtReference "http://qudt.org/vocab/unit/MilliGM-PER-M3-SEC"^^xsd:string ;
    ns1:ucumCode "mg.m-3.s-1"^^xsd:string ;
    ns1:unitSymbol "mg/(m³⋅s)"^^xsd:string .

ns1:MilliGramPerGram a owl:Class ;
    rdfs:label "MilliGramPerGram"^^xsd:string ;
    rdfs:comment """0.000001-fold of the SI base unit kilogram divided by the 0.001-fold of the SI base unit kilogram

-- QUDT"""@en ;
    rdfs:subClassOf [ a owl:Restriction ;
            owl:onProperty ns1:hasUnitSymbol ;
            owl:someValuesFrom ns1:GramPerGram ],
        [ a owl:Restriction ;
            owl:hasValue 1e-03 ;
            owl:onProperty ns1:hasSIConversionMultiplier ],
        [ a owl:Restriction ;
            owl:hasValue 0e+00 ;
            owl:onProperty ns1:hasSIConversionOffset ],
        ns1:MassFractionUnit,
        ns1:MilliPrefixedUnit,
        ns1:PrefixedUnit,
        ns1:SINonCoherentUnit ;
    skos:altLabel "Milligram Per Gram"@en ;
    skos:prefLabel "MilliGramPerGram"^^xsd:string ;
    ns1:elucidation """0.000001-fold of the SI base unit kilogram divided by the 0.001-fold of the SI base unit kilogram

-- QUDT"""@en ;
    ns1:qudtReference "http://qudt.org/vocab/unit/MilliGM-PER-GM"^^xsd:string ;
    ns1:ucumCode "mg.g-1"^^xsd:string,
        "mg/g"^^xsd:string ;
    ns1:unitSymbol "mg/gm"^^xsd:string .

ns1:MilliGramPerKilogram a owl:Class ;
    rdfs:label "MilliGramPerKilogram"^^xsd:string ;
    rdfs:comment """0.000001-fold of the SI base unit kilogram divided by the SI base unit kilogram

-- QUDT"""@en ;
    rdfs:subClassOf [ a owl:Restriction ;
            owl:onProperty ns1:hasUnitSymbol ;
            owl:someValuesFrom ns1:GramPerKilogram ],
        [ a owl:Restriction ;
            owl:hasValue 0e+00 ;
            owl:onProperty ns1:hasSIConversionOffset ],
        [ a owl:Restriction ;
            owl:hasValue 1e-06 ;
            owl:onProperty ns1:hasSIConversionMultiplier ],
        ns1:MassFractionUnit,
        ns1:MilliPrefixedUnit,
        ns1:PrefixedUnit,
        ns1:SINonCoherentUnit ;
    skos:altLabel "Milligram Per Kilogram"@en ;
    skos:prefLabel "MilliGramPerKilogram"^^xsd:string ;
    ns1:elucidation """0.000001-fold of the SI base unit kilogram divided by the SI base unit kilogram

-- QUDT"""@en ;
    ns1:qudtReference "http://qudt.org/vocab/unit/MilliGM-PER-KiloGM"^^xsd:string ;
    ns1:ucumCode "mg.kg-1"^^xsd:string,
        "mg/kg"^^xsd:string ;
    ns1:unitSymbol "mg/kg"^^xsd:string .

ns1:MilliGramPerMetre a owl:Class ;
    rdfs:label "MilliGramPerMetre"^^xsd:string ;
    rdfs:comment """0.000001-fold of the SI base unit kilogram divided by the SI base unit metre

-- QUDT"""@en ;
    rdfs:subClassOf [ a owl:Restriction ;
            owl:onProperty ns1:hasUnitSymbol ;
            owl:someValuesFrom ns1:GramPerMetre ],
        [ a owl:Restriction ;
            owl:hasValue 0e+00 ;
            owl:onProperty ns1:hasSIConversionOffset ],
        [ a owl:Restriction ;
            owl:hasValue 1e-06 ;
            owl:onProperty ns1:hasSIConversionMultiplier ],
        ns1:MassPerLengthUnit,
        ns1:MilliPrefixedUnit,
        ns1:PrefixedUnit,
        ns1:SINonCoherentUnit ;
    skos:altLabel "Milligram Per Metre"@en ;
    skos:prefLabel "MilliGramPerMetre"^^xsd:string ;
    ns1:elucidation """0.000001-fold of the SI base unit kilogram divided by the SI base unit metre

-- QUDT"""@en ;
    ns1:qudtReference "http://qudt.org/vocab/unit/MilliGM-PER-M"^^xsd:string ;
    ns1:ucumCode "mg.m-1"^^xsd:string ;
    ns1:unitSymbol "mg/m"^^xsd:string .

ns1:MilliGramPerSecond a owl:Class ;
    rdfs:label "MilliGramPerSecond"^^xsd:string ;
    rdfs:comment """0.000001-fold of the SI base unit kilogram divided by the SI base unit second

-- QUDT"""@en ;
    rdfs:subClassOf [ a owl:Restriction ;
            owl:hasValue 0e+00 ;
            owl:onProperty ns1:hasSIConversionOffset ],
        [ a owl:Restriction ;
            owl:hasValue 1e-06 ;
            owl:onProperty ns1:hasSIConversionMultiplier ],
        [ a owl:Restriction ;
            owl:onProperty ns1:hasUnitSymbol ;
            owl:someValuesFrom ns1:GramPerSecond ],
        ns1:MassPerTimeUnit,
        ns1:MilliPrefixedUnit,
        ns1:PrefixedUnit,
        ns1:SINonCoherentUnit ;
    skos:altLabel "Milligram Per Second"@en ;
    skos:prefLabel "MilliGramPerSecond"^^xsd:string ;
    ns1:elucidation """0.000001-fold of the SI base unit kilogram divided by the SI base unit second

-- QUDT"""@en ;
    ns1:qudtReference "http://qudt.org/vocab/unit/MilliGM-PER-SEC"^^xsd:string ;
    ns1:ucumCode "mg/s"^^xsd:string ;
    ns1:unitSymbol "mg/s"^^xsd:string .

ns1:MilliGramPerSquareCentiMetre a owl:Class ;
    rdfs:label "MilliGramPerSquareCentiMetre"^^xsd:string ;
    rdfs:comment """0.000001-fold of the SI base unit kilogram divided by the 0.0001-fold of the power of the SI base unit metre with the exponent 2

-- QUDT"""@en ;
    rdfs:subClassOf [ a owl:Restriction ;
            owl:hasValue 0e+00 ;
            owl:onProperty ns1:hasSIConversionOffset ],
        [ a owl:Restriction ;
            owl:hasValue 1e-02 ;
            owl:onProperty ns1:hasSIConversionMultiplier ],
        [ a owl:Restriction ;
            owl:onProperty ns1:hasUnitNonPrefixPart ;
            owl:someValuesFrom ns1:GramPerSquareCentiMetre ],
        ns1:AreaDensityUnit,
        ns1:MilliPrefixedUnit,
        ns1:PrefixedUnit,
        ns1:SINonCoherentUnit ;
    skos:altLabel "Milligram Per Square Centimetre"@en ;
    skos:prefLabel "MilliGramPerSquareCentiMetre"^^xsd:string ;
    ns1:elucidation """0.000001-fold of the SI base unit kilogram divided by the 0.0001-fold of the power of the SI base unit metre with the exponent 2

-- QUDT"""@en ;
    ns1:qudtReference "http://qudt.org/vocab/unit/MilliGM-PER-CentiM2"^^xsd:string ;
    ns1:ucumCode "mg.cm-2"^^xsd:string ;
    ns1:unitSymbol "mg/cm²"^^xsd:string .

ns1:MilliGramPerSquareMetre a owl:Class ;
    rdfs:label "MilliGramPerSquareMetre"^^xsd:string ;
    rdfs:comment """0.000001-fold of the SI base unit kilogram divided by the power of the SI base unit metre with the exponent 2

-- QUDT"""@en ;
    rdfs:subClassOf [ a owl:Restriction ;
            owl:onProperty ns1:hasUnitSymbol ;
            owl:someValuesFrom ns1:GramPerSquareMetre ],
        [ a owl:Restriction ;
            owl:hasValue 1e-06 ;
            owl:onProperty ns1:hasSIConversionMultiplier ],
        [ a owl:Restriction ;
            owl:hasValue 0e+00 ;
            owl:onProperty ns1:hasSIConversionOffset ],
        ns1:AreaDensityUnit,
        ns1:MilliPrefixedUnit,
        ns1:PrefixedUnit,
        ns1:SINonCoherentUnit ;
    skos:altLabel "Milligram Per Square Metre"@en ;
    skos:prefLabel "MilliGramPerSquareMetre"^^xsd:string ;
    ns1:elucidation """0.000001-fold of the SI base unit kilogram divided by the power of the SI base unit metre with the exponent 2

-- QUDT"""@en ;
    ns1:qudtReference "http://qudt.org/vocab/unit/MilliGM-PER-M2"^^xsd:string ;
    ns1:ucumCode "mg.m-2"^^xsd:string,
        "mg/m2"^^xsd:string ;
    ns1:unitSymbol "mg/m²"^^xsd:string .

ns1:MilliGramPerSquareMetrePerSecond a owl:Class ;
    rdfs:label "MilliGramPerSquareMetrePerSecond"^^xsd:string ;
    rdfs:subClassOf [ a owl:Restriction ;
            owl:hasValue 1e-06 ;
            owl:onProperty ns1:hasSIConversionMultiplier ],
        [ a owl:Restriction ;
            owl:hasValue 0e+00 ;
            owl:onProperty ns1:hasSIConversionOffset ],
        ns1:MassFluxUnit,
        ns1:MilliPrefixedUnit,
        ns1:PrefixedUnit,
        ns1:SINonCoherentUnit ;
    skos:altLabel "Milligrams per square metre per second"@en ;
    skos:prefLabel "MilliGramPerSquareMetrePerSecond"^^xsd:string ;
    ns1:qudtReference "http://qudt.org/vocab/unit/MilliGM-PER-M2-SEC"^^xsd:string ;
    ns1:ucumCode "mg.m-2.s-1"^^xsd:string ;
    ns1:unitSymbol "mg/(m²⋅s)"^^xsd:string .

ns1:MilliHenryPerKiloOhm a owl:Class ;
    rdfs:label "MilliHenryPerKiloOhm"^^xsd:string ;
    rdfs:comment """0.001-fold of the SI derived unit henry divided by the 1 000-fold of the SI derived unit ohm

-- QUDT"""@en ;
    rdfs:subClassOf [ a owl:Restriction ;
            owl:hasValue 1e-06 ;
            owl:onProperty ns1:hasSIConversionMultiplier ],
        [ a owl:Restriction ;
            owl:hasValue 0e+00 ;
            owl:onProperty ns1:hasSIConversionOffset ],
        [ a owl:Restriction ;
            owl:onProperty ns1:hasUnitNonPrefixPart ;
            owl:someValuesFrom ns1:HenryPerKiloOhm ],
        ns1:MilliPrefixedUnit,
        ns1:PrefixedUnit,
        ns1:SINonCoherentUnit,
        ns1:TimeUnit ;
    skos:altLabel "Millihenry Per Kiloohm"@en ;
    skos:prefLabel "MilliHenryPerKiloOhm"^^xsd:string ;
    ns1:elucidation """0.001-fold of the SI derived unit henry divided by the 1 000-fold of the SI derived unit ohm

-- QUDT"""@en ;
    ns1:qudtReference "http://qudt.org/vocab/unit/MilliH-PER-KiloOHM"^^xsd:string ;
    ns1:ucumCode "mH.kOhm-1"^^xsd:string ;
    ns1:unitSymbol "mH/kΩ"^^xsd:string .

ns1:MilliHenryPerOhm a owl:Class ;
    rdfs:label "MilliHenryPerOhm"^^xsd:string ;
    rdfs:comment """0.001-fold of the SI derived unit henry divided by the SI derived unit ohm

-- QUDT"""@en ;
    rdfs:subClassOf [ a owl:Restriction ;
            owl:hasValue 0e+00 ;
            owl:onProperty ns1:hasSIConversionOffset ],
        [ a owl:Restriction ;
            owl:onProperty ns1:hasUnitSymbol ;
            owl:someValuesFrom ns1:HenryPerOhm ],
        [ a owl:Restriction ;
            owl:hasValue 1e-03 ;
            owl:onProperty ns1:hasSIConversionMultiplier ],
        ns1:MilliPrefixedUnit,
        ns1:PrefixedUnit,
        ns1:SINonCoherentUnit,
        ns1:TimeUnit ;
    skos:altLabel "Millihenry Per Ohm"@en ;
    skos:prefLabel "MilliHenryPerOhm"^^xsd:string ;
    ns1:elucidation """0.001-fold of the SI derived unit henry divided by the SI derived unit ohm

-- QUDT"""@en ;
    ns1:qudtReference "http://qudt.org/vocab/unit/MilliH-PER-OHM"^^xsd:string ;
    ns1:ucumCode "mH.Ohm-1"^^xsd:string ;
    ns1:unitSymbol "mH/Ω"^^xsd:string .

ns1:MilliMetrePerKelvin a owl:Class ;
    rdfs:label "MilliMetrePerKelvin"^^xsd:string ;
    rdfs:comment """0.001-fold of the SI base unit metre divided by the SI base unit kelvin

-- QUDT"""@en ;
    rdfs:subClassOf [ a owl:Restriction ;
            owl:hasValue 0e+00 ;
            owl:onProperty ns1:hasSIConversionOffset ],
        [ a owl:Restriction ;
            owl:hasValue 1e-03 ;
            owl:onProperty ns1:hasSIConversionMultiplier ],
        [ a owl:Restriction ;
            owl:onProperty ns1:hasUnitSymbol ;
            owl:someValuesFrom ns1:MetrePerKelvin ],
        ns1:LengthPerTemperatureUnit,
        ns1:MilliPrefixedUnit,
        ns1:PrefixedUnit,
        ns1:SINonCoherentUnit ;
    skos:altLabel "Millimetre Per Kelvin"@en ;
    skos:prefLabel "MilliMetrePerKelvin"^^xsd:string ;
    ns1:elucidation """0.001-fold of the SI base unit metre divided by the SI base unit kelvin

-- QUDT"""@en ;
    ns1:qudtReference "http://qudt.org/vocab/unit/MilliM-PER-K"^^xsd:string ;
    ns1:ucumCode "mm.K-1"^^xsd:string ;
    ns1:unitSymbol "mm/K"^^xsd:string .

ns1:MilliMetrePerSecond a owl:Class ;
    rdfs:label "MilliMetrePerSecond"^^xsd:string ;
    rdfs:comment """0.001-fold of the SI base unit metre divided by the SI base unit second

-- QUDT"""@en ;
    rdfs:subClassOf [ a owl:Restriction ;
            owl:onProperty ns1:hasUnitNonPrefixPart ;
            owl:someValuesFrom ns1:MetrePerSecond ],
        [ a owl:Restriction ;
            owl:hasValue 1e-03 ;
            owl:onProperty ns1:hasSIConversionMultiplier ],
        [ a owl:Restriction ;
            owl:hasValue 0e+00 ;
            owl:onProperty ns1:hasSIConversionOffset ],
        ns1:MilliPrefixedUnit,
        ns1:PrefixedUnit,
        ns1:SINonCoherentUnit,
        ns1:SpeedUnit ;
    skos:altLabel "Millimetre Per Second"@en ;
    skos:prefLabel "MilliMetrePerSecond"^^xsd:string ;
    ns1:elucidation """0.001-fold of the SI base unit metre divided by the SI base unit second

-- QUDT"""@en ;
    ns1:qudtReference "http://qudt.org/vocab/unit/MilliM-PER-SEC"^^xsd:string ;
    ns1:ucumCode "mm.s-1"^^xsd:string ;
    ns1:unitSymbol "mm/s"^^xsd:string .

ns1:MilliMolePerCubicMetre a owl:Class ;
    rdfs:label "MilliMolePerCubicMetre"^^xsd:string ;
    rdfs:comment """Unavailable.

-- QUDT"""@en ;
    rdfs:subClassOf [ a owl:Restriction ;
            owl:hasValue 1e-03 ;
            owl:onProperty ns1:hasSIConversionMultiplier ],
        [ a owl:Restriction ;
            owl:onProperty ns1:hasUnitSymbol ;
            owl:someValuesFrom ns1:MolePerCubicMetre ],
        [ a owl:Restriction ;
            owl:hasValue 0e+00 ;
            owl:onProperty ns1:hasSIConversionOffset ],
        ns1:AmountConcentrationUnit,
        ns1:MilliPrefixedUnit,
        ns1:PrefixedUnit,
        ns1:SINonCoherentUnit ;
    skos:altLabel "Millimoles per cubic metre"@en ;
    skos:prefLabel "MilliMolePerCubicMetre"^^xsd:string ;
    ns1:elucidation """Unavailable.

-- QUDT"""@en ;
    ns1:qudtReference "http://qudt.org/vocab/unit/MilliMOL-PER-M3"^^xsd:string ;
    ns1:ucumCode "mmol.m-3"^^xsd:string ;
    ns1:unitSymbol "mmol/m³"^^xsd:string .

ns1:MilliMolePerGram a owl:Class ;
    rdfs:label "MilliMolePerGram"^^xsd:string ;
    rdfs:comment """0.001-fold of the SI base unit mol divided by the 0.001-fold of the SI base unit kilogram

-- QUDT"""@en ;
    rdfs:subClassOf [ a owl:Restriction ;
            owl:hasValue 1e+00 ;
            owl:onProperty ns1:hasSIConversionMultiplier ],
        [ a owl:Restriction ;
            owl:hasValue 0e+00 ;
            owl:onProperty ns1:hasSIConversionOffset ],
        ns1:AmountPerMassUnit,
        ns1:MilliPrefixedUnit,
        ns1:PrefixedUnit,
        ns1:SINonCoherentUnit ;
    skos:altLabel "Millimole Per Gram"@en ;
    skos:prefLabel "MilliMolePerGram"^^xsd:string ;
    ns1:elucidation """0.001-fold of the SI base unit mol divided by the 0.001-fold of the SI base unit kilogram

-- QUDT"""@en ;
    ns1:qudtReference "http://qudt.org/vocab/unit/MilliMOL-PER-GM"^^xsd:string ;
    ns1:ucumCode "mmol.g-1"^^xsd:string ;
    ns1:unitSymbol "mmol/g"^^xsd:string .

ns1:MilliMolePerKilogram a owl:Class ;
    rdfs:label "MilliMolePerKilogram"^^xsd:string ;
    rdfs:comment """0.001-fold of the SI base unit mol divided by the SI base unit kilogram

-- QUDT"""@en ;
    rdfs:subClassOf [ a owl:Restriction ;
            owl:hasValue 0e+00 ;
            owl:onProperty ns1:hasSIConversionOffset ],
        [ a owl:Restriction ;
            owl:hasValue 1e-03 ;
            owl:onProperty ns1:hasSIConversionMultiplier ],
        ns1:AmountPerMassUnit,
        ns1:MilliPrefixedUnit,
        ns1:PrefixedUnit,
        ns1:SINonCoherentUnit ;
    skos:altLabel "Millimole Per Kilogram"@en ;
    skos:prefLabel "MilliMolePerKilogram"^^xsd:string ;
    ns1:elucidation """0.001-fold of the SI base unit mol divided by the SI base unit kilogram

-- QUDT"""@en ;
    ns1:qudtReference "http://qudt.org/vocab/unit/MilliMOL-PER-KiloGM"^^xsd:string ;
    ns1:ucumCode "mmol.kg-1"^^xsd:string,
        "mmol/kg"^^xsd:string ;
    ns1:unitSymbol "mmol/kg"^^xsd:string .

ns1:MilliMolePerMole a owl:Class ;
    rdfs:label "MilliMolePerMole"^^xsd:string ;
    rdfs:subClassOf [ a owl:Restriction ;
            owl:hasValue 0e+00 ;
            owl:onProperty ns1:hasSIConversionOffset ],
        [ a owl:Restriction ;
            owl:hasValue 1e-03 ;
            owl:onProperty ns1:hasSIConversionMultiplier ],
        ns1:AmountFractionUnit,
        ns1:MilliPrefixedUnit,
        ns1:PrefixedUnit,
        ns1:SINonCoherentUnit ;
    skos:altLabel "Millimoles per mole"@en ;
    skos:prefLabel "MilliMolePerMole"^^xsd:string ;
    ns1:qudtReference "http://qudt.org/vocab/unit/MilliMOL-PER-MOL"^^xsd:string ;
    ns1:ucumCode "mmol.mol-1"^^xsd:string ;
    ns1:unitSymbol "mmol/mol"^^xsd:string .

ns1:MilliMolePerSquareMetre a owl:Class ;
    rdfs:label "MilliMolePerSquareMetre"^^xsd:string ;
    rdfs:comment """Unavailable.

-- QUDT"""@en ;
    rdfs:subClassOf [ a owl:Restriction ;
            owl:onProperty ns1:hasUnitSymbol ;
            owl:someValuesFrom ns1:MolePerSquareMetre ],
        [ a owl:Restriction ;
            owl:hasValue 1e-03 ;
            owl:onProperty ns1:hasSIConversionMultiplier ],
        [ a owl:Restriction ;
            owl:hasValue 0e+00 ;
            owl:onProperty ns1:hasSIConversionOffset ],
        ns1:AmountPerAreaUnit,
        ns1:MilliPrefixedUnit,
        ns1:PrefixedUnit,
        ns1:SINonCoherentUnit ;
    skos:altLabel "Millimoles per square metre"@en ;
    skos:prefLabel "MilliMolePerSquareMetre"^^xsd:string ;
    ns1:elucidation """Unavailable.

-- QUDT"""@en ;
    ns1:qudtReference "http://qudt.org/vocab/unit/MilliMOL-PER-M2"^^xsd:string ;
    ns1:ucumCode "mmol.m-2"^^xsd:string ;
    ns1:unitSymbol "mmol/m²"^^xsd:string .

ns1:MilliMolePerSquareMetrePerSecond a owl:Class ;
    rdfs:label "MilliMolePerSquareMetrePerSecond"^^xsd:string ;
    rdfs:isDefinedBy "http://qudt.org/2.1/vocab/unit"^^xsd:string ;
    rdfs:subClassOf [ a owl:Restriction ;
            owl:hasValue 0e+00 ;
            owl:onProperty ns1:hasSIConversionOffset ],
        [ a owl:Restriction ;
            owl:hasValue 1e-03 ;
            owl:onProperty ns1:hasSIConversionMultiplier ],
        ns1:AmountPerAreaTimeUnit,
        ns1:MeasurementUnit,
        ns1:PrefixedUnit,
        ns1:SINonCoherentUnit ;
    skos:altLabel "Millimoles per square metre per second"@en ;
    skos:prefLabel "MilliMolePerSquareMetrePerSecond"^^xsd:string ;
    ns1:qudtReference "http://qudt.org/vocab/unit/MilliMOL-PER-M2-SEC"^^xsd:string ;
    ns1:ucumCode "mmol.m-2.s-1"^^xsd:string,
        "mmol/m2/s1"^^xsd:string ;
    ns1:unitSymbol "µg/(m²⋅s)"^^xsd:string .

ns1:MilliNewtonMetre a owl:Class ;
    rdfs:label "MilliNewtonMetre"^^xsd:string ;
    rdfs:comment """0.001-fold of the product of the SI derived unit newton and the SI base unit metre

-- QUDT"""@en ;
    rdfs:subClassOf [ a owl:Restriction ;
            owl:onProperty ns1:hasUnitNonPrefixPart ;
            owl:someValuesFrom ns1:NewtonMetre ],
        [ a owl:Restriction ;
            owl:hasValue 1e-03 ;
            owl:onProperty ns1:hasSIConversionMultiplier ],
        [ a owl:Restriction ;
            owl:hasValue 0e+00 ;
            owl:onProperty ns1:hasSIConversionOffset ],
        ns1:EnergyUnit,
        ns1:MilliPrefixedUnit,
        ns1:PrefixedUnit,
        ns1:SINonCoherentUnit ;
    skos:altLabel "Millinewton Metre"@en ;
    skos:prefLabel "MilliNewtonMetre"^^xsd:string ;
    ns1:elucidation """0.001-fold of the product of the SI derived unit newton and the SI base unit metre

-- QUDT"""@en ;
    ns1:qudtReference "http://qudt.org/vocab/unit/MilliN-M"^^xsd:string ;
    ns1:ucumCode "mN.m"^^xsd:string ;
    ns1:unitSymbol "mN⋅m"^^xsd:string .

ns1:MilliNewtonPerMetre a owl:Class ;
    rdfs:label "MilliNewtonPerMetre"^^xsd:string ;
    rdfs:comment """0.001-fold of the SI derived unit newton divided by the SI base unit metre

-- QUDT"""@en ;
    rdfs:subClassOf [ a owl:Restriction ;
            owl:hasValue 1e-03 ;
            owl:onProperty ns1:hasSIConversionMultiplier ],
        [ a owl:Restriction ;
            owl:hasValue 0e+00 ;
            owl:onProperty ns1:hasSIConversionOffset ],
        [ a owl:Restriction ;
            owl:onProperty ns1:hasUnitSymbol ;
            owl:someValuesFrom ns1:NewtonPerMetre ],
        ns1:ForcePerLengthUnit,
        ns1:MilliPrefixedUnit,
        ns1:PrefixedUnit,
        ns1:SINonCoherentUnit ;
    skos:altLabel "Millinewton Per Metre"@en ;
    skos:prefLabel "MilliNewtonPerMetre"^^xsd:string ;
    ns1:elucidation """0.001-fold of the SI derived unit newton divided by the SI base unit metre

-- QUDT"""@en ;
    ns1:qudtReference "http://qudt.org/vocab/unit/MilliN-PER-M"^^xsd:string ;
    ns1:ucumCode "mN.m-1"^^xsd:string ;
    ns1:unitSymbol "mN/m"^^xsd:string .

ns1:MilliPascalSecond a owl:Class ;
    rdfs:label "MilliPascalSecond"^^xsd:string ;
    rdfs:comment """0.001-fold of the product of the SI derived unit pascal and the SI base unit second

-- QUDT"""@en ;
    rdfs:subClassOf [ a owl:Restriction ;
            owl:hasValue 0e+00 ;
            owl:onProperty ns1:hasSIConversionOffset ],
        [ a owl:Restriction ;
            owl:hasValue 1e-03 ;
            owl:onProperty ns1:hasSIConversionMultiplier ],
        [ a owl:Restriction ;
            owl:onProperty ns1:hasUnitSymbol ;
            owl:someValuesFrom ns1:PascalSecond ],
        ns1:MassPerLengthTimeUnit,
        ns1:MilliPrefixedUnit,
        ns1:PrefixedUnit,
        ns1:SINonCoherentUnit ;
    skos:altLabel "Millipascal Second"@en ;
    skos:prefLabel "MilliPascalSecond"^^xsd:string ;
    ns1:elucidation """0.001-fold of the product of the SI derived unit pascal and the SI base unit second

-- QUDT"""@en ;
    ns1:qudtReference "http://qudt.org/vocab/unit/MilliPA-SEC"^^xsd:string ;
    ns1:ucumCode "mPa.s"^^xsd:string ;
    ns1:unitSymbol "mPa⋅s"^^xsd:string .

ns1:MilliSiemensPerCentiMetre a owl:Class ;
    rdfs:label "MilliSiemensPerCentiMetre"^^xsd:string ;
    rdfs:comment """0.001-fold of the SI derived unit Siemens divided by the 0.01-fold of the SI base unit metre

-- QUDT"""@en ;
    rdfs:subClassOf [ a owl:Restriction ;
            owl:hasValue 0e+00 ;
            owl:onProperty ns1:hasSIConversionOffset ],
        [ a owl:Restriction ;
            owl:hasValue 1e-01 ;
            owl:onProperty ns1:hasSIConversionMultiplier ],
        [ a owl:Restriction ;
            owl:onProperty ns1:hasUnitNonPrefixPart ;
            owl:someValuesFrom ns1:SiemensPerCentiMetre ],
        ns1:ElectricConductivityUnit,
        ns1:MilliPrefixedUnit,
        ns1:PrefixedUnit,
        ns1:SINonCoherentUnit ;
    skos:altLabel "Millisiemens Per Centimetre"@en ;
    skos:prefLabel "MilliSiemensPerCentiMetre"^^xsd:string ;
    ns1:elucidation """0.001-fold of the SI derived unit Siemens divided by the 0.01-fold of the SI base unit metre

-- QUDT"""@en ;
    ns1:qudtReference "http://qudt.org/vocab/unit/MilliS-PER-CentiM"^^xsd:string ;
    ns1:ucumCode "mS.cm-1"^^xsd:string,
        "mS/cm"^^xsd:string ;
    ns1:unitSymbol "mS/cm"^^xsd:string .

ns1:MilliSiemensPerMetre a owl:Class ;
    rdfs:label "MilliSiemensPerMetre"^^xsd:string ;
    rdfs:subClassOf [ a owl:Restriction ;
            owl:onProperty ns1:hasUnitSymbol ;
            owl:someValuesFrom ns1:SiemensPerMetre ],
        [ a owl:Restriction ;
            owl:hasValue 1e-03 ;
            owl:onProperty ns1:hasSIConversionMultiplier ],
        [ a owl:Restriction ;
            owl:hasValue 0e+00 ;
            owl:onProperty ns1:hasSIConversionOffset ],
        ns1:ElectricConductivityUnit,
        ns1:MilliPrefixedUnit,
        ns1:PrefixedUnit,
        ns1:SINonCoherentUnit ;
    skos:altLabel "MilliSiemens per metre"@en ;
    skos:prefLabel "MilliSiemensPerMetre"^^xsd:string ;
    ns1:qudtReference "http://qudt.org/vocab/unit/MilliS-PER-M"^^xsd:string ;
    ns1:ucumCode "mS.m-1"^^xsd:string ;
    ns1:unitSymbol "mS/m"^^xsd:string .

ns1:MilliVoltPerMetre a owl:Class ;
    rdfs:label "MilliVoltPerMetre"^^xsd:string ;
    rdfs:comment """0.000001-fold of the SI derived unit volt divided by the SI base unit metre

-- QUDT"""@en ;
    rdfs:subClassOf [ a owl:Restriction ;
            owl:onProperty ns1:hasUnitSymbol ;
            owl:someValuesFrom ns1:VoltPerMetre ],
        [ a owl:Restriction ;
            owl:hasValue 1e-03 ;
            owl:onProperty ns1:hasSIConversionMultiplier ],
        [ a owl:Restriction ;
            owl:hasValue 0e+00 ;
            owl:onProperty ns1:hasSIConversionOffset ],
        ns1:ElectricFieldStrengthUnit,
        ns1:MilliPrefixedUnit,
        ns1:PrefixedUnit,
        ns1:SINonCoherentUnit ;
    skos:altLabel "Millivolt Per Metre"@en ;
    skos:prefLabel "MilliVoltPerMetre"^^xsd:string ;
    ns1:elucidation """0.000001-fold of the SI derived unit volt divided by the SI base unit metre

-- QUDT"""@en ;
    ns1:qudtReference "http://qudt.org/vocab/unit/MilliV-PER-M"^^xsd:string ;
    ns1:ucumCode "mV.m-1"^^xsd:string ;
    ns1:unitSymbol "mV/m"^^xsd:string .

ns1:MilliWattPerSquareCentiMetrePerMicroMetrePerSteradian a owl:Class ;
    rdfs:label "MilliWattPerSquareCentiMetrePerMicroMetrePerSteradian"^^xsd:string ;
    rdfs:subClassOf [ a owl:Restriction ;
            owl:hasValue 0e+00 ;
            owl:onProperty ns1:hasSIConversionOffset ],
        [ a owl:Restriction ;
            owl:hasValue 1e+07 ;
            owl:onProperty ns1:hasSIConversionMultiplier ],
        ns1:MilliPrefixedUnit,
        ns1:PrefixedUnit,
        ns1:PressurePerTimeUnit,
        ns1:SINonCoherentUnit ;
    skos:altLabel "Milliwatts per square centimetre per micrometre per steradian"@en ;
    skos:prefLabel "MilliWattPerSquareCentiMetrePerMicroMetrePerSteradian"^^xsd:string ;
    ns1:qudtReference "http://qudt.org/vocab/unit/MilliW-PER-CentiM2-MicroM-SR"^^xsd:string ;
    ns1:ucumCode "mW.cm-2.um-1.sr-1"^^xsd:string ;
    ns1:unitSymbol "mW/(cm⋅µm⋅sr)"^^xsd:string .

ns1:MilliWattPerSquareMetre a owl:Class ;
    rdfs:label "MilliWattPerSquareMetre"^^xsd:string ;
    rdfs:comment """0.001-fold of the SI derived unit weber divided by the power of the SI base unit metre with the exponent 2

-- QUDT"""@en ;
    rdfs:subClassOf [ a owl:Restriction ;
            owl:hasValue 1e-03 ;
            owl:onProperty ns1:hasSIConversionMultiplier ],
        [ a owl:Restriction ;
            owl:hasValue 0e+00 ;
            owl:onProperty ns1:hasSIConversionOffset ],
        [ a owl:Restriction ;
            owl:onProperty ns1:hasUnitSymbol ;
            owl:someValuesFrom ns1:WattPerSquareMetre ],
        ns1:MilliPrefixedUnit,
        ns1:PowerDensityUnit,
        ns1:PrefixedUnit,
        ns1:SINonCoherentUnit ;
    skos:altLabel "Milliwatt Per Square Metre"@en ;
    skos:prefLabel "MilliWattPerSquareMetre"^^xsd:string ;
    ns1:elucidation """0.001-fold of the SI derived unit weber divided by the power of the SI base unit metre with the exponent 2

-- QUDT"""@en ;
    ns1:qudtReference "http://qudt.org/vocab/unit/MilliW-PER-M2"^^xsd:string ;
    ns1:ucumCode "mW.m-2"^^xsd:string ;
    ns1:unitSymbol "mW/m²"^^xsd:string .

ns1:MilliWattPerSquareMetrePerNanoMetre a owl:Class ;
    rdfs:label "MilliWattPerSquareMetrePerNanoMetre"^^xsd:string ;
    rdfs:subClassOf [ a owl:Restriction ;
            owl:hasValue 1e+06 ;
            owl:onProperty ns1:hasSIConversionMultiplier ],
        [ a owl:Restriction ;
            owl:hasValue 0e+00 ;
            owl:onProperty ns1:hasSIConversionOffset ],
        [ a owl:Restriction ;
            owl:onProperty ns1:hasUnitNonPrefixPart ;
            owl:someValuesFrom ns1:WattPerSquareMetrePerNanoMetre ],
        ns1:MilliPrefixedUnit,
        ns1:PrefixedUnit,
        ns1:PressurePerTimeUnit,
        ns1:SINonCoherentUnit ;
    skos:altLabel "Milliwatts per square metre per nanometre"@en ;
    skos:prefLabel "MilliWattPerSquareMetrePerNanoMetre"^^xsd:string ;
    ns1:qudtReference "http://qudt.org/vocab/unit/MilliW-PER-M2-NanoM"^^xsd:string ;
    ns1:ucumCode "mW.m-2.nm-1"^^xsd:string ;
    ns1:unitSymbol "mW/(cm⋅nm)"^^xsd:string .

ns1:MilliWattPerSquareMetrePerNanoMetrePerSteradian a owl:Class ;
    rdfs:label "MilliWattPerSquareMetrePerNanoMetrePerSteradian"^^xsd:string ;
    rdfs:subClassOf [ a owl:Restriction ;
            owl:hasValue 0e+00 ;
            owl:onProperty ns1:hasSIConversionOffset ],
        [ a owl:Restriction ;
            owl:hasValue 1e+06 ;
            owl:onProperty ns1:hasSIConversionMultiplier ],
        [ a owl:Restriction ;
            owl:onProperty ns1:hasUnitNonPrefixPart ;
            owl:someValuesFrom ns1:WattPerSquareMetrePerNanoMetrePerSteradian ],
        ns1:MilliPrefixedUnit,
        ns1:PrefixedUnit,
        ns1:PressurePerTimeUnit,
        ns1:SINonCoherentUnit ;
    skos:altLabel "Milliwatts per square metre per nanometre per steradian"@en ;
    skos:prefLabel "MilliWattPerSquareMetrePerNanoMetrePerSteradian"^^xsd:string ;
    ns1:qudtReference "http://qudt.org/vocab/unit/MilliW-PER-M2-NanoM-SR"^^xsd:string ;
    ns1:ucumCode "mW.m-2.nm-1.sr-1"^^xsd:string ;
    ns1:unitSymbol "mW/(cm⋅nm⋅sr)"^^xsd:string .

ns1:MolePerCubicDeciMetre a owl:Class ;
    rdfs:label "MolePerCubicDeciMetre"@en ;
    rdfs:comment """SI base unit mol divided by the 0.001-fold of the power of the SI base unit metre with the exponent 3

-- QUDT"""@en ;
    rdfs:isDefinedBy "http://qudt.org/2.1/vocab/unit"^^xsd:string ;
    rdfs:subClassOf [ a owl:Restriction ;
            owl:hasValue 0e+00 ;
            owl:onProperty ns1:hasSIConversionOffset ],
        [ a owl:Restriction ;
            owl:hasValue 1e+03 ;
            owl:onProperty ns1:hasSIConversionMultiplier ],
        ns1:AmountConcentrationUnit,
        ns1:SINonCoherentDerivedUnit ;
    skos:altLabel "Mole Per Cubic Decimetre"@en ;
    skos:prefLabel "MolePerCubicDeciMetre"@en ;
    ns1:elucidation """SI base unit mol divided by the 0.001-fold of the power of the SI base unit metre with the exponent 3

-- QUDT"""@en ;
    ns1:qudtReference "http://qudt.org/vocab/unit/MOL-PER-DeciM3"^^xsd:string ;
    ns1:ucumCode "mol.dm-3"^^xsd:string ;
    ns1:unitSymbol "mol/dm³"^^xsd:string .

ns1:NanoFaradPerMetre a owl:Class ;
    rdfs:label "NanoFaradPerMetre"^^xsd:string ;
    rdfs:comment """0.000000001-fold of the SI derived unit farad divided by the SI base unit metre

-- QUDT"""@en ;
    rdfs:subClassOf [ a owl:Restriction ;
            owl:hasValue 1e-09 ;
            owl:onProperty ns1:hasSIConversionMultiplier ],
        [ a owl:Restriction ;
            owl:onProperty ns1:hasUnitSymbol ;
            owl:someValuesFrom ns1:FaradPerMetre ],
        [ a owl:Restriction ;
            owl:hasValue 0e+00 ;
            owl:onProperty ns1:hasSIConversionOffset ],
        ns1:NanoPrefixedUnit,
        ns1:PermittivityUnit,
        ns1:PrefixedUnit,
        ns1:SINonCoherentUnit ;
    skos:altLabel "Nanofarad Per Metre"@en ;
    skos:prefLabel "NanoFaradPerMetre"^^xsd:string ;
    ns1:elucidation """0.000000001-fold of the SI derived unit farad divided by the SI base unit metre

-- QUDT"""@en ;
    ns1:qudtReference "http://qudt.org/vocab/unit/NanoFARAD-PER-M"^^xsd:string ;
    ns1:ucumCode "nF.m-1"^^xsd:string ;
    ns1:unitSymbol "nF/m"^^xsd:string .

ns1:NanoGramPerCubicMetre a owl:Class ;
    rdfs:label "NanoGramPerCubicMetre"^^xsd:string ;
    rdfs:comment """0.000000000001-fold of the SI base unit kilogram divided by the power of the SI base unit metre with the exponent 3

-- QUDT"""@en ;
    rdfs:subClassOf [ a owl:Restriction ;
            owl:hasValue 1e-12 ;
            owl:onProperty ns1:hasSIConversionMultiplier ],
        [ a owl:Restriction ;
            owl:onProperty ns1:hasUnitSymbol ;
            owl:someValuesFrom ns1:GramPerCubicMetre ],
        [ a owl:Restriction ;
            owl:hasValue 0e+00 ;
            owl:onProperty ns1:hasSIConversionOffset ],
        ns1:DensityUnit,
        ns1:NanoPrefixedUnit,
        ns1:PrefixedUnit,
        ns1:SINonCoherentUnit ;
    skos:altLabel "Nanogram Per Cubic Metre"@en ;
    skos:prefLabel "NanoGramPerCubicMetre"^^xsd:string ;
    ns1:elucidation """0.000000000001-fold of the SI base unit kilogram divided by the power of the SI base unit metre with the exponent 3

-- QUDT"""@en ;
    ns1:qudtReference "http://qudt.org/vocab/unit/NanoGM-PER-M3"^^xsd:string ;
    ns1:ucumCode "ng.m-3"^^xsd:string ;
    ns1:unitSymbol "ng/m³"^^xsd:string .

ns1:NanoGramPerKilogram a owl:Class ;
    rdfs:label "NanoGramPerKilogram"^^xsd:string ;
    rdfs:comment """mass ratio consisting of the 0.000000000001-fold of the SI base unit kilogram divided by the SI base unit kilogram

-- QUDT"""@en ;
    rdfs:subClassOf [ a owl:Restriction ;
            owl:hasValue 0e+00 ;
            owl:onProperty ns1:hasSIConversionOffset ],
        [ a owl:Restriction ;
            owl:onProperty ns1:hasUnitSymbol ;
            owl:someValuesFrom ns1:GramPerKilogram ],
        [ a owl:Restriction ;
            owl:hasValue 1e-12 ;
            owl:onProperty ns1:hasSIConversionMultiplier ],
        ns1:MassFractionUnit,
        ns1:NanoPrefixedUnit,
        ns1:PrefixedUnit,
        ns1:SINonCoherentUnit ;
    skos:altLabel "Nanogram Per Kilogram"@en ;
    skos:prefLabel "NanoGramPerKilogram"^^xsd:string ;
    ns1:elucidation """mass ratio consisting of the 0.000000000001-fold of the SI base unit kilogram divided by the SI base unit kilogram

-- QUDT"""@en ;
    ns1:qudtReference "http://qudt.org/vocab/unit/NanoGM-PER-KiloGM"^^xsd:string ;
    ns1:ucumCode "ng.kg-1"^^xsd:string,
        "ng/kg"^^xsd:string ;
    ns1:unitSymbol "ng/Kg"^^xsd:string .

ns1:NanoGramPerSquareMetrePerPascalPerSecond a owl:Class ;
    rdfs:label "NanoGramPerSquareMetrePerPascalPerSecond"^^xsd:string ;
    rdfs:subClassOf [ a owl:Restriction ;
            owl:hasValue 1e-12 ;
            owl:onProperty ns1:hasSIConversionMultiplier ],
        [ a owl:Restriction ;
            owl:hasValue 0e+00 ;
            owl:onProperty ns1:hasSIConversionOffset ],
        ns1:PerLengthTimeUnit,
        ns1:SINonCoherentDerivedUnit ;
    skos:altLabel "Nanograms per square metre per Pascal per second"@en ;
    skos:prefLabel "NanoGramPerSquareMetrePerPascalPerSecond"^^xsd:string ;
    ns1:qudtReference "http://qudt.org/vocab/unit/NanoGM-PER-M2-PA-SEC"^^xsd:string ;
    ns1:unitSymbol "ng/(m²⋅s⋅Pa)"^^xsd:string ;
    ns1:wikipediaReference "https://en.wikipedia.org/wiki/Perm_(unit)"^^xsd:string .

ns1:NanoHenryPerMetre a owl:Class ;
    rdfs:label "NanoHenryPerMetre"^^xsd:string ;
    rdfs:comment """0.000000001-fold of the SI derived unit henry divided by the SI base unit metre

-- QUDT"""@en ;
    rdfs:subClassOf [ a owl:Restriction ;
            owl:hasValue 0e+00 ;
            owl:onProperty ns1:hasSIConversionOffset ],
        [ a owl:Restriction ;
            owl:hasValue 1e-09 ;
            owl:onProperty ns1:hasSIConversionMultiplier ],
        [ a owl:Restriction ;
            owl:onProperty ns1:hasUnitSymbol ;
            owl:someValuesFrom ns1:HenryPerMetre ],
        ns1:NanoPrefixedUnit,
        ns1:PermeabilityUnit,
        ns1:PrefixedUnit,
        ns1:SINonCoherentUnit ;
    skos:altLabel "Nanohenry Per Metre"@en ;
    skos:prefLabel "NanoHenryPerMetre"^^xsd:string ;
    ns1:elucidation """0.000000001-fold of the SI derived unit henry divided by the SI base unit metre

-- QUDT"""@en ;
    ns1:qudtReference "http://qudt.org/vocab/unit/NanoH-PER-M"^^xsd:string ;
    ns1:ucumCode "nH.m-1"^^xsd:string ;
    ns1:unitSymbol "nH/m"^^xsd:string .

ns1:NanoMolePerMicroMole a owl:Class ;
    rdfs:label "NanoMolePerMicroMole"^^xsd:string ;
    rdfs:comment """Unavailable.

-- QUDT"""@en ;
    rdfs:subClassOf [ a owl:Restriction ;
            owl:hasValue 0e+00 ;
            owl:onProperty ns1:hasSIConversionOffset ],
        [ a owl:Restriction ;
            owl:hasValue 1e-03 ;
            owl:onProperty ns1:hasSIConversionMultiplier ],
        ns1:AmountFractionUnit,
        ns1:NanoPrefixedUnit,
        ns1:PrefixedUnit,
        ns1:SINonCoherentUnit ;
    skos:altLabel "Nanomoles per micromole"@en ;
    skos:prefLabel "NanoMolePerMicroMole"^^xsd:string ;
    ns1:elucidation """Unavailable.

-- QUDT"""@en ;
    ns1:qudtReference "http://qudt.org/vocab/unit/NanoMOL-PER-MicroMOL"^^xsd:string ;
    ns1:ucumCode "nmol.umol-1"^^xsd:string ;
    ns1:unitSymbol "nmol/µmol"^^xsd:string .

ns1:NanoSiemensPerCentiMetre a owl:Class ;
    rdfs:label "NanoSiemensPerCentiMetre"^^xsd:string ;
    rdfs:comment """0.000000001-fold of the SI derived unit Siemens by the 0.01 fol of the SI base unit metre

-- QUDT"""@en ;
    rdfs:subClassOf [ a owl:Restriction ;
            owl:hasValue 0e+00 ;
            owl:onProperty ns1:hasSIConversionOffset ],
        [ a owl:Restriction ;
            owl:hasValue 1e-07 ;
            owl:onProperty ns1:hasSIConversionMultiplier ],
        [ a owl:Restriction ;
            owl:onProperty ns1:hasUnitNonPrefixPart ;
            owl:someValuesFrom ns1:SiemensPerCentiMetre ],
        ns1:ElectricConductivityUnit,
        ns1:NanoPrefixedUnit,
        ns1:PrefixedUnit,
        ns1:SINonCoherentUnit ;
    skos:altLabel "Nanosiemens Per Centimetre"@en ;
    skos:prefLabel "NanoSiemensPerCentiMetre"^^xsd:string ;
    ns1:elucidation """0.000000001-fold of the SI derived unit Siemens by the 0.01 fol of the SI base unit metre

-- QUDT"""@en ;
    ns1:qudtReference "http://qudt.org/vocab/unit/NanoS-PER-CentiM"^^xsd:string ;
    ns1:ucumCode "nS.cm-1"^^xsd:string ;
    ns1:unitSymbol "nS/cm"^^xsd:string .

ns1:NanoSiemensPerMetre a owl:Class ;
    rdfs:label "NanoSiemensPerMetre"^^xsd:string ;
    rdfs:comment """0.000000001-fold of the SI derived unit Siemens divided by the SI base unit metre

-- QUDT"""@en ;
    rdfs:subClassOf [ a owl:Restriction ;
            owl:onProperty ns1:hasUnitSymbol ;
            owl:someValuesFrom ns1:SiemensPerMetre ],
        [ a owl:Restriction ;
            owl:hasValue 0e+00 ;
            owl:onProperty ns1:hasSIConversionOffset ],
        [ a owl:Restriction ;
            owl:hasValue 1e-09 ;
            owl:onProperty ns1:hasSIConversionMultiplier ],
        ns1:ElectricConductivityUnit,
        ns1:NanoPrefixedUnit,
        ns1:PrefixedUnit,
        ns1:SINonCoherentUnit ;
    skos:altLabel "Nanosiemens Per Metre"@en ;
    skos:prefLabel "NanoSiemensPerMetre"^^xsd:string ;
    ns1:elucidation """0.000000001-fold of the SI derived unit Siemens divided by the SI base unit metre

-- QUDT"""@en ;
    ns1:qudtReference "http://qudt.org/vocab/unit/NanoS-PER-M"^^xsd:string ;
    ns1:ucumCode "nS.m-1"^^xsd:string ;
    ns1:unitSymbol "nS/m"^^xsd:string .

ns1:NewtonCentiMetre a owl:Class ;
    rdfs:label "NewtonCentiMetre"@en ;
    rdfs:comment """product of the SI derived unit newton and the 0.01-fold of the SI base unit metre

-- QUDT"""@en ;
    rdfs:isDefinedBy "http://qudt.org/2.1/vocab/unit"^^xsd:string ;
    rdfs:subClassOf [ a owl:Restriction ;
            owl:hasValue 1e-02 ;
            owl:onProperty ns1:hasSIConversionMultiplier ],
        [ a owl:Restriction ;
            owl:hasValue 0e+00 ;
            owl:onProperty ns1:hasSIConversionOffset ],
        ns1:EnergyUnit,
        ns1:SINonCoherentDerivedUnit ;
    skos:altLabel "Newton Centimetre"@en ;
    skos:prefLabel "NewtonCentiMetre"@en ;
    ns1:elucidation """product of the SI derived unit newton and the 0.01-fold of the SI base unit metre

-- QUDT"""@en ;
    ns1:qudtReference "http://qudt.org/vocab/unit/N-CentiM"^^xsd:string ;
    ns1:ucumCode "N.cm"^^xsd:string ;
    ns1:unitSymbol "N⋅cm"^^xsd:string .

ns1:NewtonPerCentiMetre a owl:Class ;
    rdfs:label "NewtonPerCentiMetre"@en ;
    rdfs:comment """SI derived unit newton divided by the 0.01-fold of the SI base unit metre

-- QUDT"""@en ;
    rdfs:isDefinedBy "http://qudt.org/2.1/vocab/unit"^^xsd:string ;
    rdfs:subClassOf [ a owl:Restriction ;
            owl:hasValue 0e+00 ;
            owl:onProperty ns1:hasSIConversionOffset ],
        [ a owl:Restriction ;
            owl:hasValue 1e+02 ;
            owl:onProperty ns1:hasSIConversionMultiplier ],
        ns1:ForcePerLengthUnit,
        ns1:SINonCoherentDerivedUnit ;
    skos:altLabel "Newton Per Centimetre"@en ;
    skos:prefLabel "NewtonPerCentiMetre"@en ;
    ns1:elucidation """SI derived unit newton divided by the 0.01-fold of the SI base unit metre

-- QUDT"""@en ;
    ns1:qudtReference "http://qudt.org/vocab/unit/N-PER-CentiM"^^xsd:string ;
    ns1:ucumCode "N.cm-1"^^xsd:string ;
    ns1:unitSymbol "N/cm"^^xsd:string .

ns1:NewtonPerMilliMetre a owl:Class ;
    rdfs:label "NewtonPerMilliMetre"@en ;
    rdfs:comment """SI derived unit newton divided by the 0.001-fold of the SI base unit metre

-- QUDT"""@en ;
    rdfs:isDefinedBy "http://qudt.org/2.1/vocab/unit"^^xsd:string ;
    rdfs:subClassOf [ a owl:Restriction ;
            owl:hasValue 1e+03 ;
            owl:onProperty ns1:hasSIConversionMultiplier ],
        [ a owl:Restriction ;
            owl:hasValue 0e+00 ;
            owl:onProperty ns1:hasSIConversionOffset ],
        ns1:ForcePerLengthUnit,
        ns1:SINonCoherentDerivedUnit ;
    skos:altLabel "Newton Per Millimetre"@en ;
    skos:prefLabel "NewtonPerMilliMetre"@en ;
    ns1:elucidation """SI derived unit newton divided by the 0.001-fold of the SI base unit metre

-- QUDT"""@en ;
    ns1:qudtReference "http://qudt.org/vocab/unit/N-PER-MilliM"^^xsd:string ;
    ns1:ucumCode "N.mm-1"^^xsd:string ;
    ns1:unitSymbol "N/mm"^^xsd:string .

ns1:NewtonPerSquareCentiMetre a owl:Class ;
    rdfs:label "NewtonPerSquareCentiMetre"@en ;
    rdfs:comment """derived SI unit newton divided by the 0.0001-fold of the power of the SI base unit metre by exponent 2

-- QUDT"""@en ;
    rdfs:isDefinedBy "http://qudt.org/2.1/vocab/unit"^^xsd:string ;
    rdfs:subClassOf [ a owl:Restriction ;
            owl:hasValue 1e+04 ;
            owl:onProperty ns1:hasSIConversionMultiplier ],
        [ a owl:Restriction ;
            owl:hasValue 0e+00 ;
            owl:onProperty ns1:hasSIConversionOffset ],
        ns1:PressureUnit,
        ns1:SINonCoherentDerivedUnit ;
    skos:altLabel "Newton Per Square Centimetre"@en ;
    skos:prefLabel "NewtonPerSquareCentiMetre"@en ;
    ns1:elucidation """derived SI unit newton divided by the 0.0001-fold of the power of the SI base unit metre by exponent 2

-- QUDT"""@en ;
    ns1:qudtReference "http://qudt.org/vocab/unit/N-PER-CentiM2"^^xsd:string ;
    ns1:ucumCode "N.cm-2"^^xsd:string ;
    ns1:unitSymbol "N/cm²"^^xsd:string .

ns1:NewtonPerSquareMilliMetre a owl:Class ;
    rdfs:label "NewtonPerSquareMilliMetre"@en ;
    rdfs:comment """SI derived unit newton divided by the 0.000001-fold of the power of the SI base unit metre with the exponent 2

-- QUDT"""@en ;
    rdfs:isDefinedBy "http://qudt.org/2.1/vocab/unit"^^xsd:string ;
    rdfs:subClassOf [ a owl:Restriction ;
            owl:hasValue 1e+06 ;
            owl:onProperty ns1:hasSIConversionMultiplier ],
        [ a owl:Restriction ;
            owl:hasValue 0e+00 ;
            owl:onProperty ns1:hasSIConversionOffset ],
        ns1:PressureUnit,
        ns1:SINonCoherentDerivedUnit ;
    skos:altLabel "Newton Per Square Millimetre"@en ;
    skos:prefLabel "NewtonPerSquareMilliMetre"@en ;
    ns1:elucidation """SI derived unit newton divided by the 0.000001-fold of the power of the SI base unit metre with the exponent 2

-- QUDT"""@en ;
    ns1:qudtReference "http://qudt.org/vocab/unit/N-PER-MilliM2"^^xsd:string ;
    ns1:ucumCode "N.mm-2"^^xsd:string ;
    ns1:unitSymbol "N/mm²"^^xsd:string .

ns1:PerCentiMetre a owl:Class ;
    rdfs:label "PerCentiMetre"@en ;
    rdfs:comment """reciprocal of the 0.01-fold of the SI base unit metre

-- QUDT"""@en ;
    rdfs:isDefinedBy "http://qudt.org/2.1/vocab/unit"^^xsd:string ;
    rdfs:subClassOf [ a owl:Restriction ;
            owl:hasValue 1e+02 ;
            owl:onProperty ns1:hasSIConversionMultiplier ],
        [ a owl:Restriction ;
            owl:hasValue 0e+00 ;
            owl:onProperty ns1:hasSIConversionOffset ],
        ns1:ReciprocalLengthUnit,
        ns1:SINonCoherentDerivedUnit ;
    skos:altLabel "ReciprocalCentimetre"@en ;
    skos:prefLabel "PerCentiMetre"@en ;
    ns1:elucidation """reciprocal of the 0.01-fold of the SI base unit metre

-- QUDT"""@en ;
    ns1:qudtReference "http://qudt.org/vocab/unit/PER-CentiM"^^xsd:string ;
    ns1:ucumCode "/cm"^^xsd:string,
        "cm-1"^^xsd:string ;
    ns1:unitSymbol "/cm"^^xsd:string .

ns1:PerCubicCentiMetre a owl:Class ;
    rdfs:label "PerCubicCentiMetre"@en ;
    rdfs:comment """reciprocal of the 0.000001-fold of the power of the SI base unit metre with the exponent 3

-- QUDT"""@en ;
    rdfs:isDefinedBy "http://qudt.org/2.1/vocab/unit"^^xsd:string ;
    rdfs:subClassOf [ a owl:Restriction ;
            owl:hasValue 0e+00 ;
            owl:onProperty ns1:hasSIConversionOffset ],
        [ a owl:Restriction ;
            owl:hasValue 1e+06 ;
            owl:onProperty ns1:hasSIConversionMultiplier ],
        ns1:PerVolumeUnit,
        ns1:SINonCoherentDerivedUnit ;
    skos:altLabel "ReciprocalCubicCentiMetre"@en ;
    skos:prefLabel "PerCubicCentiMetre"@en ;
    ns1:elucidation """reciprocal of the 0.000001-fold of the power of the SI base unit metre with the exponent 3

-- QUDT"""@en ;
    ns1:qudtReference "http://qudt.org/vocab/unit/PER-CentiM3"^^xsd:string ;
    ns1:ucumCode "cm-3"^^xsd:string ;
    ns1:unitSymbol "/cm³"^^xsd:string .

ns1:PerCubicMilliMetre a owl:Class ;
    rdfs:label "PerCubicMilliMetre"@en ;
    rdfs:comment """reciprocal value of the 0.000000001-fold of the power of the SI base unit metre with the exponent 3

-- QUDT"""@en ;
    rdfs:isDefinedBy "http://qudt.org/2.1/vocab/unit"^^xsd:string ;
    rdfs:subClassOf [ a owl:Restriction ;
            owl:hasValue 1e+09 ;
            owl:onProperty ns1:hasSIConversionMultiplier ],
        [ a owl:Restriction ;
            owl:hasValue 0e+00 ;
            owl:onProperty ns1:hasSIConversionOffset ],
        ns1:PerVolumeUnit,
        ns1:SINonCoherentDerivedUnit ;
    skos:altLabel "ReciprocalCubicMilliMetre"@en ;
    skos:prefLabel "PerCubicMilliMetre"@en ;
    ns1:elucidation """reciprocal value of the 0.000000001-fold of the power of the SI base unit metre with the exponent 3

-- QUDT"""@en ;
    ns1:qudtReference "http://qudt.org/vocab/unit/PER-MilliM3"^^xsd:string ;
    ns1:ucumCode "mm-3"^^xsd:string ;
    ns1:unitSymbol "/mm³"^^xsd:string .

ns1:PerKiloMetre a owl:Class ;
    rdfs:label "PerKiloMetre"@en ;
    rdfs:comment """Per Kilometer Unit is a denominator unit with dimensions /km.

-- QUDT"""@en ;
    rdfs:isDefinedBy "http://qudt.org/2.1/vocab/unit"^^xsd:string ;
    rdfs:subClassOf [ a owl:Restriction ;
            owl:hasValue 0e+00 ;
            owl:onProperty ns1:hasSIConversionOffset ],
        [ a owl:Restriction ;
            owl:hasValue 1e-03 ;
            owl:onProperty ns1:hasSIConversionMultiplier ],
        ns1:ReciprocalLengthUnit,
        ns1:SINonCoherentDerivedUnit ;
    skos:altLabel "ReciprocalKiloMetre"@en ;
    skos:prefLabel "PerKiloMetre"@en ;
    ns1:elucidation """Per Kilometer Unit is a denominator unit with dimensions /km.

-- QUDT"""@en ;
    ns1:qudtReference "http://qudt.org/vocab/unit/PER-KiloM"^^xsd:string ;
    ns1:ucumCode "/km"^^xsd:string,
        "km-1"^^xsd:string ;
    ns1:unitSymbol "/km"^^xsd:string .

ns1:PerMetreNanoMetre a owl:Class ;
    rdfs:label "PerMetreNanoMetre"@en ;
    rdfs:comment "Per metre and nanometre."@en ;
    rdfs:isDefinedBy "http://qudt.org/2.1/vocab/unit"^^xsd:string ;
    rdfs:subClassOf [ a owl:Restriction ;
            owl:hasValue 1e+09 ;
            owl:onProperty ns1:hasSIConversionMultiplier ],
        [ a owl:Restriction ;
            owl:hasValue 0e+00 ;
            owl:onProperty ns1:hasSIConversionOffset ],
        ns1:PerAreaUnit,
        ns1:SINonCoherentDerivedUnit ;
    skos:altLabel "ReciprocalMetreNanoMetre"@en ;
    skos:prefLabel "PerMetreNanoMetre"@en ;
    ns1:elucidation "Per metre and nanometre."@en ;
    ns1:qudtReference "http://qudt.org/vocab/unit/PER-M-NanoM"^^xsd:string ;
    ns1:ucumCode "m-1.nm-1"^^xsd:string ;
    ns1:unitSymbol "/(m⋅nm)"^^xsd:string .

ns1:PerMetreNanoMetreSteradian a owl:Class ;
    rdfs:label "PerMetreNanoMetreSteradian"@en ;
    rdfs:comment "Per metre and nanometre and steradian."@en ;
    rdfs:isDefinedBy "http://qudt.org/2.1/vocab/unit"^^xsd:string ;
    rdfs:subClassOf [ a owl:Restriction ;
            owl:hasValue 1e+09 ;
            owl:onProperty ns1:hasSIConversionMultiplier ],
        [ a owl:Restriction ;
            owl:hasValue 0e+00 ;
            owl:onProperty ns1:hasSIConversionOffset ],
        ns1:PerAreaUnit,
        ns1:SINonCoherentDerivedUnit ;
    skos:altLabel "ReciprocalMetreNanoMetreSteradian"@en ;
    skos:prefLabel "PerMetreNanoMetreSteradian"@en ;
    ns1:elucidation "Per metre and nanometre and steradian."@en ;
    ns1:qudtReference "http://qudt.org/vocab/unit/PER-M-NanoM-SR"^^xsd:string ;
    ns1:ucumCode "m-1.nm-1.sr-1"^^xsd:string ;
    ns1:unitSymbol "/(m⋅nm⋅sr)"^^xsd:string .

ns1:PerMicroMetre a owl:Class ;
    rdfs:label "PerMicroMetre"@en ;
    rdfs:comment """Per Micrometer Unit is a denominator unit with dimensions /microm.

-- QUDT"""@en ;
    rdfs:isDefinedBy "http://qudt.org/2.1/vocab/unit"^^xsd:string ;
    rdfs:subClassOf [ a owl:Restriction ;
            owl:hasValue 0e+00 ;
            owl:onProperty ns1:hasSIConversionOffset ],
        [ a owl:Restriction ;
            owl:hasValue 1e+06 ;
            owl:onProperty ns1:hasSIConversionMultiplier ],
        ns1:ReciprocalLengthUnit,
        ns1:SINonCoherentDerivedUnit ;
    skos:altLabel "ReciprocalMicroMetre"@en ;
    skos:prefLabel "PerMicroMetre"@en ;
    ns1:elucidation """Per Micrometer Unit is a denominator unit with dimensions /microm.

-- QUDT"""@en ;
    ns1:qudtReference "http://qudt.org/vocab/unit/PER-MicroM"^^xsd:string ;
    ns1:ucumCode "/um"^^xsd:string,
        "um-1"^^xsd:string ;
    ns1:unitSymbol "/µm"^^xsd:string .

ns1:PerMilliMetre a owl:Class ;
    rdfs:label "PerMilliMetre"@en ;
    rdfs:comment """Per Millimeter Unit is a denominator unit with dimensions /mm.

-- QUDT"""@en ;
    rdfs:isDefinedBy "http://qudt.org/2.1/vocab/unit"^^xsd:string ;
    rdfs:subClassOf [ a owl:Restriction ;
            owl:hasValue 0e+00 ;
            owl:onProperty ns1:hasSIConversionOffset ],
        [ a owl:Restriction ;
            owl:hasValue 1e+03 ;
            owl:onProperty ns1:hasSIConversionMultiplier ],
        ns1:ReciprocalLengthUnit,
        ns1:SINonCoherentDerivedUnit ;
    skos:altLabel "ReciprocalMilliMetre"@en ;
    skos:prefLabel "PerMilliMetre"@en ;
    ns1:elucidation """Per Millimeter Unit is a denominator unit with dimensions /mm.

-- QUDT"""@en ;
    ns1:qudtReference "http://qudt.org/vocab/unit/PER-MilliM"^^xsd:string ;
    ns1:ucumCode "/mm"^^xsd:string,
        "mm-1"^^xsd:string ;
    ns1:unitSymbol "/mm"^^xsd:string .

ns1:PerMilliSecond a owl:Class ;
    rdfs:label "PerMilliSecond"@en ;
    rdfs:comment "Per millisecond."@en ;
    rdfs:isDefinedBy "http://qudt.org/2.1/vocab/unit"^^xsd:string ;
    rdfs:subClassOf [ a owl:Restriction ;
            owl:hasValue 1e+03 ;
            owl:onProperty ns1:hasSIConversionMultiplier ],
        [ a owl:Restriction ;
            owl:hasValue 0e+00 ;
            owl:onProperty ns1:hasSIConversionOffset ],
        ns1:FrequencyUnit,
        ns1:SINonCoherentDerivedUnit ;
    skos:altLabel "ReciprocalMilliSecond"@en ;
    skos:prefLabel "PerMilliSecond"@en ;
    ns1:elucidation "Per millisecond."@en ;
    ns1:qudtReference "http://qudt.org/vocab/unit/PER-MilliSEC"^^xsd:string ;
    ns1:ucumCode "ms-1"^^xsd:string ;
    ns1:unitSymbol "/ms"^^xsd:string .

ns1:PerNanoMetre a owl:Class ;
    rdfs:label "PerNanoMetre"@en ;
    rdfs:comment """Per Nanometer Unit is a denominator unit with dimensions /nm.

-- QUDT"""@en ;
    rdfs:isDefinedBy "http://qudt.org/2.1/vocab/unit"^^xsd:string ;
    rdfs:subClassOf [ a owl:Restriction ;
            owl:hasValue 1e+09 ;
            owl:onProperty ns1:hasSIConversionMultiplier ],
        [ a owl:Restriction ;
            owl:hasValue 0e+00 ;
            owl:onProperty ns1:hasSIConversionOffset ],
        ns1:ReciprocalLengthUnit,
        ns1:SINonCoherentDerivedUnit ;
    skos:altLabel "ReciprocalNanoMetre"@en ;
    skos:prefLabel "PerNanoMetre"@en ;
    ns1:elucidation """Per Nanometer Unit is a denominator unit with dimensions /nm.

-- QUDT"""@en ;
    ns1:qudtReference "http://qudt.org/vocab/unit/PER-NanoM"^^xsd:string ;
    ns1:ucumCode "/nm"^^xsd:string,
        "nm-1"^^xsd:string ;
    ns1:unitSymbol "/nm"^^xsd:string .

ns1:PerPicoMetre a owl:Class ;
    rdfs:label "PerPicoMetre"@en ;
    rdfs:comment """Per Picoometer Unit is a denominator unit with dimensions /pm.

-- QUDT"""@en ;
    rdfs:isDefinedBy "http://qudt.org/2.1/vocab/unit"^^xsd:string ;
    rdfs:subClassOf [ a owl:Restriction ;
            owl:hasValue 0e+00 ;
            owl:onProperty ns1:hasSIConversionOffset ],
        [ a owl:Restriction ;
            owl:hasValue 1e+12 ;
            owl:onProperty ns1:hasSIConversionMultiplier ],
        ns1:ReciprocalLengthUnit,
        ns1:SINonCoherentDerivedUnit ;
    skos:altLabel "ReciprocalPicoMetre"@en ;
    skos:prefLabel "PerPicoMetre"@en ;
    ns1:elucidation """Per Picoometer Unit is a denominator unit with dimensions /pm.

-- QUDT"""@en ;
    ns1:qudtReference "http://qudt.org/vocab/unit/PER-PicoM"^^xsd:string ;
    ns1:ucumCode "/pm"^^xsd:string,
        "pm-1"^^xsd:string ;
    ns1:unitSymbol "/pm"^^xsd:string .

ns1:PicoFaradPerMetre a owl:Class ;
    rdfs:label "PicoFaradPerMetre"^^xsd:string ;
    rdfs:comment """1e-12 fold of the SI derived unit farad divided by the SI base unit metre.

-- QUDT"""@en ;
    rdfs:subClassOf [ a owl:Restriction ;
            owl:onProperty ns1:hasUnitSymbol ;
            owl:someValuesFrom ns1:FaradPerMetre ],
        [ a owl:Restriction ;
            owl:hasValue 1e-12 ;
            owl:onProperty ns1:hasSIConversionMultiplier ],
        [ a owl:Restriction ;
            owl:hasValue 0e+00 ;
            owl:onProperty ns1:hasSIConversionOffset ],
        ns1:PermittivityUnit,
        ns1:PicoPrefixedUnit,
        ns1:PrefixedUnit,
        ns1:SINonCoherentUnit ;
    skos:altLabel "Picofarad Per Metre"@en ;
    skos:prefLabel "PicoFaradPerMetre"^^xsd:string ;
    ns1:elucidation """1e-12 fold of the SI derived unit farad divided by the SI base unit metre.

-- QUDT"""@en ;
    ns1:qudtReference "http://qudt.org/vocab/unit/PicoFARAD-PER-M"^^xsd:string ;
    ns1:ucumCode "pF.m-1"^^xsd:string ;
    ns1:unitSymbol "pF/m"^^xsd:string .

ns1:PicoGramPerGram a owl:Class ;
    rdfs:label "PicoGramPerGram"^^xsd:string ;
    rdfs:comment """One part per 10**12 (trillion) by mass of the measurand in the matrix.

-- QUDT"""@en ;
    rdfs:subClassOf [ a owl:Restriction ;
            owl:hasValue 0e+00 ;
            owl:onProperty ns1:hasSIConversionOffset ],
        [ a owl:Restriction ;
            owl:onProperty ns1:hasUnitSymbol ;
            owl:someValuesFrom ns1:GramPerGram ],
        [ a owl:Restriction ;
            owl:hasValue 1e-12 ;
            owl:onProperty ns1:hasSIConversionMultiplier ],
        ns1:MassFractionUnit,
        ns1:PicoPrefixedUnit,
        ns1:PrefixedUnit,
        ns1:SINonCoherentUnit ;
    skos:altLabel "Picograms per gram"@en ;
    skos:prefLabel "PicoGramPerGram"^^xsd:string ;
    ns1:elucidation """One part per 10**12 (trillion) by mass of the measurand in the matrix.

-- QUDT"""@en ;
    ns1:qudtReference "http://qudt.org/vocab/unit/PicoGM-PER-GM"^^xsd:string ;
    ns1:ucumCode "pg.g-1"^^xsd:string ;
    ns1:unitSymbol "pg/g"^^xsd:string .

ns1:PicoGramPerKilogram a owl:Class ;
    rdfs:label "PicoGramPerKilogram"^^xsd:string ;
    rdfs:comment """One part per 10**15 by mass of the measurand in the matrix.

-- QUDT"""@en ;
    rdfs:subClassOf [ a owl:Restriction ;
            owl:onProperty ns1:hasUnitSymbol ;
            owl:someValuesFrom ns1:GramPerKilogram ],
        [ a owl:Restriction ;
            owl:hasValue 0e+00 ;
            owl:onProperty ns1:hasSIConversionOffset ],
        [ a owl:Restriction ;
            owl:hasValue 1e-15 ;
            owl:onProperty ns1:hasSIConversionMultiplier ],
        ns1:MassFractionUnit,
        ns1:PicoPrefixedUnit,
        ns1:PrefixedUnit,
        ns1:SINonCoherentUnit ;
    skos:altLabel "Picograms per kilogram"@en ;
    skos:prefLabel "PicoGramPerKilogram"^^xsd:string ;
    ns1:elucidation """One part per 10**15 by mass of the measurand in the matrix.

-- QUDT"""@en ;
    ns1:qudtReference "http://qudt.org/vocab/unit/PicoGM-PER-KiloGM"^^xsd:string ;
    ns1:ucumCode "pg.kg-1"^^xsd:string ;
    ns1:unitSymbol "pg/kg"^^xsd:string .

ns1:PicoMolePerCubicMetre a owl:Class ;
    rdfs:label "PicoMolePerCubicMetre"^^xsd:string ;
    rdfs:subClassOf [ a owl:Restriction ;
            owl:hasValue 1e-12 ;
            owl:onProperty ns1:hasSIConversionMultiplier ],
        [ a owl:Restriction ;
            owl:onProperty ns1:hasUnitSymbol ;
            owl:someValuesFrom ns1:MolePerCubicMetre ],
        [ a owl:Restriction ;
            owl:hasValue 0e+00 ;
            owl:onProperty ns1:hasSIConversionOffset ],
        ns1:AmountConcentrationUnit,
        ns1:PicoPrefixedUnit,
        ns1:PrefixedUnit,
        ns1:SINonCoherentUnit ;
    skos:altLabel "Picomoles per cubic metre"@en ;
    skos:prefLabel "PicoMolePerCubicMetre"^^xsd:string ;
    ns1:qudtReference "http://qudt.org/vocab/unit/PicoMOL-PER-M3"^^xsd:string ;
    ns1:ucumCode "pmol.m-3"^^xsd:string ;
    ns1:unitSymbol "pmol/m³"^^xsd:string .

ns1:PicoMolePerCubicMetrePerSecond a owl:Class ;
    rdfs:label "PicoMolePerCubicMetrePerSecond"^^xsd:string ;
    rdfs:subClassOf [ a owl:Restriction ;
            owl:hasValue 0e+00 ;
            owl:onProperty ns1:hasSIConversionOffset ],
        [ a owl:Restriction ;
            owl:onProperty ns1:hasUnitSymbol ;
            owl:someValuesFrom ns1:MolePerCubicMetrePerSecond ],
        [ a owl:Restriction ;
            owl:hasValue 1e-12 ;
            owl:onProperty ns1:hasSIConversionMultiplier ],
        ns1:AmountPerVolumeTimeUnit,
        ns1:PicoPrefixedUnit,
        ns1:PrefixedUnit,
        ns1:SINonCoherentUnit ;
    skos:altLabel "Picomoles per cubic metre per second"@en ;
    skos:prefLabel "PicoMolePerCubicMetrePerSecond"^^xsd:string ;
    ns1:qudtReference "http://qudt.org/vocab/unit/PicoMOL-PER-M3-SEC"^^xsd:string ;
    ns1:ucumCode "pmol.m-3.s-1"^^xsd:string ;
    ns1:unitSymbol "pmol/(m³⋅s)"^^xsd:string .

ns1:PicoMolePerKilogram a owl:Class ;
    rdfs:label "PicoMolePerKilogram"^^xsd:string ;
    rdfs:subClassOf [ a owl:Restriction ;
            owl:hasValue 0e+00 ;
            owl:onProperty ns1:hasSIConversionOffset ],
        [ a owl:Restriction ;
            owl:hasValue 1e-12 ;
            owl:onProperty ns1:hasSIConversionMultiplier ],
        ns1:AmountPerMassUnit,
        ns1:PicoPrefixedUnit,
        ns1:PrefixedUnit,
        ns1:SINonCoherentUnit ;
    skos:altLabel "Picomoles per kilogram"@en ;
    skos:prefLabel "PicoMolePerKilogram"^^xsd:string ;
    ns1:qudtReference "http://qudt.org/vocab/unit/PicoMOL-PER-KiloGM"^^xsd:string ;
    ns1:ucumCode "pmol.kg-1"^^xsd:string ;
    ns1:unitSymbol "pmol/kg"^^xsd:string .

ns1:PicoMolePerMetrePerWattPerSecond a owl:Class ;
    rdfs:label "PicoMolePerMetrePerWattPerSecond"^^xsd:string ;
    rdfs:subClassOf [ a owl:Restriction ;
            owl:hasValue 1e-12 ;
            owl:onProperty ns1:hasSIConversionMultiplier ],
        [ a owl:Restriction ;
            owl:hasValue 0e+00 ;
            owl:onProperty ns1:hasSIConversionOffset ],
        ns1:AmountSquareTimePerMassVolumeUnit,
        ns1:PicoPrefixedUnit,
        ns1:PrefixedUnit,
        ns1:SINonCoherentUnit ;
    skos:altLabel "Picomoles per metre per watt per second"@en ;
    skos:prefLabel "PicoMolePerMetrePerWattPerSecond"^^xsd:string ;
    ns1:qudtReference "http://qudt.org/vocab/unit/PicoMOL-PER-M-W-SEC"^^xsd:string ;
    ns1:ucumCode "pmol.m-1.W-1.s-1"^^xsd:string ;
    ns1:unitSymbol "pmol/(m⋅W⋅s)"^^xsd:string .

ns1:PicoPascalPerKiloMetre a owl:Class ;
    rdfs:label "PicoPascalPerKiloMetre"^^xsd:string ;
    rdfs:comment """0.000000000001-fold of the SI derived unit pascal divided by the 1 000-fold of the SI base unit metre

-- QUDT"""@en ;
    rdfs:subClassOf [ a owl:Restriction ;
            owl:hasValue 1e-15 ;
            owl:onProperty ns1:hasSIConversionMultiplier ],
        [ a owl:Restriction ;
            owl:hasValue 0e+00 ;
            owl:onProperty ns1:hasSIConversionOffset ],
        ns1:ForcePerLengthUnit,
        ns1:PicoPrefixedUnit,
        ns1:PrefixedUnit,
        ns1:SINonCoherentUnit ;
    skos:altLabel "Picopascal Per Kilometre"@en ;
    skos:prefLabel "PicoPascalPerKiloMetre"^^xsd:string ;
    ns1:elucidation """0.000000000001-fold of the SI derived unit pascal divided by the 1 000-fold of the SI base unit metre

-- QUDT"""@en ;
    ns1:qudtReference "http://qudt.org/vocab/unit/PicoPA-PER-KiloM"^^xsd:string ;
    ns1:ucumCode "pPa.km-1"^^xsd:string ;
    ns1:unitSymbol "pPa/km"^^xsd:string .

ns1:PicoSiemensPerMetre a owl:Class ;
    rdfs:label "PicoSiemensPerMetre"^^xsd:string ;
    rdfs:comment """0.000000000001-fold of the SI derived unit Siemens divided by the SI base unit metre

-- QUDT"""@en ;
    rdfs:subClassOf [ a owl:Restriction ;
            owl:onProperty ns1:hasUnitSymbol ;
            owl:someValuesFrom ns1:SiemensPerMetre ],
        [ a owl:Restriction ;
            owl:hasValue 0e+00 ;
            owl:onProperty ns1:hasSIConversionOffset ],
        [ a owl:Restriction ;
            owl:hasValue 1e-12 ;
            owl:onProperty ns1:hasSIConversionMultiplier ],
        ns1:ElectricConductivityUnit,
        ns1:PicoPrefixedUnit,
        ns1:PrefixedUnit,
        ns1:SINonCoherentUnit ;
    skos:altLabel "Picosiemens Per Metre"@en ;
    skos:prefLabel "PicoSiemensPerMetre"^^xsd:string ;
    ns1:elucidation """0.000000000001-fold of the SI derived unit Siemens divided by the SI base unit metre

-- QUDT"""@en ;
    ns1:qudtReference "http://qudt.org/vocab/unit/PicoS-PER-M"^^xsd:string ;
    ns1:ucumCode "pS.m-1"^^xsd:string ;
    ns1:unitSymbol "pS/m"^^xsd:string .

ns1:PicoWattPerSquareMetre a owl:Class ;
    rdfs:label "PicoWattPerSquareMetre"^^xsd:string ;
    rdfs:comment """0.000000000001-fold of the SI derived unit watt divided by the power of the SI base unit metre with the exponent 2

-- QUDT"""@en ;
    rdfs:subClassOf [ a owl:Restriction ;
            owl:hasValue 1e-12 ;
            owl:onProperty ns1:hasSIConversionMultiplier ],
        [ a owl:Restriction ;
            owl:onProperty ns1:hasUnitSymbol ;
            owl:someValuesFrom ns1:WattPerSquareMetre ],
        [ a owl:Restriction ;
            owl:hasValue 0e+00 ;
            owl:onProperty ns1:hasSIConversionOffset ],
        ns1:PicoPrefixedUnit,
        ns1:PowerDensityUnit,
        ns1:PrefixedUnit,
        ns1:SINonCoherentUnit ;
    skos:altLabel "Picowatt Per Square Metre"@en ;
    skos:prefLabel "PicoWattPerSquareMetre"^^xsd:string ;
    ns1:elucidation """0.000000000001-fold of the SI derived unit watt divided by the power of the SI base unit metre with the exponent 2

-- QUDT"""@en ;
    ns1:qudtReference "http://qudt.org/vocab/unit/PicoW-PER-M2"^^xsd:string ;
    ns1:ucumCode "pW.m-2"^^xsd:string ;
    ns1:unitSymbol "pW/m²"^^xsd:string .

ns1:QuarticMilliMetre a owl:Class ;
    rdfs:label "QuarticMilliMetre"@en ;
    rdfs:comment """0.001-fold of the power of the SI base unit metre with the exponent 4

-- QUDT"""@en ;
    rdfs:isDefinedBy "http://qudt.org/2.1/vocab/unit"^^xsd:string ;
    rdfs:subClassOf [ a owl:Restriction ;
            owl:hasValue 0e+00 ;
            owl:onProperty ns1:hasSIConversionOffset ],
        [ a owl:Restriction ;
            owl:hasValue 1e-12 ;
            owl:onProperty ns1:hasSIConversionMultiplier ],
        ns1:QuarticLengthUnit,
        ns1:SINonCoherentDerivedUnit ;
    skos:altLabel "Quartic Millimetre"@en ;
    skos:prefLabel "QuarticMilliMetre"@en ;
    ns1:elucidation """0.001-fold of the power of the SI base unit metre with the exponent 4

-- QUDT"""@en ;
    ns1:qudtReference "http://qudt.org/vocab/unit/MilliM4"^^xsd:string ;
    ns1:ucumCode "mm4"^^xsd:string ;
    ns1:unitSymbol "mm⁴"^^xsd:string .

ns1:SquareCentiMetre a owl:Class ;
    rdfs:label "SquareCentiMetre"^^xsd:string ;
    rdfs:comment """A unit of area equal to that of a square, of sides 1cm

-- QUDT"""@en ;
    rdfs:isDefinedBy "http://qudt.org/2.1/vocab/unit"^^xsd:string ;
    rdfs:subClassOf [ a owl:Restriction ;
            owl:hasValue 0e+00 ;
            owl:onProperty ns1:hasSIConversionOffset ],
        [ a owl:Restriction ;
            owl:hasValue 1e-04 ;
            owl:onProperty ns1:hasSIConversionMultiplier ],
        ns1:AreaUnit,
        ns1:SINonCoherentDerivedUnit ;
    skos:altLabel "Square Centimetre"@en ;
    skos:prefLabel "SquareCentiMetre"^^xsd:string ;
    ns1:elucidation """A unit of area equal to that of a square, of sides 1cm

-- QUDT"""@en ;
    ns1:qudtReference "http://qudt.org/vocab/unit/CentiM2"^^xsd:string ;
    ns1:ucumCode "cm2"^^xsd:string ;
    ns1:unitSymbol "cm²"^^xsd:string .

ns1:SquareCentiMetrePerCubicCentiMetre a owl:Class ;
    rdfs:label "SquareCentiMetrePerCubicCentiMetre"^^xsd:string ;
    rdfs:comment "Square centimetre per cubic centimetre."@en ;
    rdfs:isDefinedBy "http://qudt.org/2.1/vocab/unit"^^xsd:string ;
    rdfs:subClassOf [ a owl:Restriction ;
            owl:hasValue 1e+02 ;
            owl:onProperty ns1:hasSIConversionMultiplier ],
        [ a owl:Restriction ;
            owl:hasValue 0e+00 ;
            owl:onProperty ns1:hasSIConversionOffset ],
        ns1:ReciprocalLengthUnit,
        ns1:SINonCoherentDerivedUnit ;
    skos:prefLabel "SquareCentiMetrePerCubicCentiMetre"^^xsd:string ;
    ns1:elucidation "Square centimetre per cubic centimetre."@en ;
    ns1:qudtReference "http://qudt.org/vocab/unit/CentiM2-PER-CentiM3"^^xsd:string ;
    ns1:ucumCode "cm2.cm-3"^^xsd:string ;
    ns1:unitSymbol "cm²/cm³"^^xsd:string .

ns1:SquareCentiMetrePerGram a owl:Class ;
    rdfs:label "SquareCentiMetrePerGram"@en ;
    rdfs:subClassOf [ a owl:Restriction ;
            owl:hasValue 0e+00 ;
            owl:onProperty ns1:hasSIConversionOffset ],
        [ a owl:Restriction ;
            owl:hasValue 1e-01 ;
            owl:onProperty ns1:hasSIConversionMultiplier ],
        ns1:AreaPerMassUnit,
        ns1:SINonCoherentDerivedUnit ;
    skos:prefLabel "SquareCentiMetrePerGram"@en ;
    ns1:unitSymbol "cm²/g"^^xsd:string .

ns1:SquareCentiMetrePerSecond a owl:Class ;
    rdfs:label "SquareCentiMetrePerSecond"^^xsd:string ;
    rdfs:comment "Square centimetre per second."@en ;
    rdfs:isDefinedBy "http://qudt.org/2.1/vocab/unit"^^xsd:string ;
    rdfs:subClassOf [ a owl:Restriction ;
            owl:hasValue 0e+00 ;
            owl:onProperty ns1:hasSIConversionOffset ],
        [ a owl:Restriction ;
            owl:hasValue 1e-04 ;
            owl:onProperty ns1:hasSIConversionMultiplier ],
        ns1:AreicSpeedUnit,
        ns1:SINonCoherentDerivedUnit ;
    skos:prefLabel "SquareCentiMetrePerSecond"^^xsd:string ;
    ns1:elucidation "Square centimetre per second."@en ;
    ns1:qudtReference "http://qudt.org/vocab/unit/CentiM2-PER-SEC"^^xsd:string ;
    ns1:ucumCode "cm2.s-1"^^xsd:string ;
    ns1:unitSymbol "cm²/s"^^xsd:string .

ns1:SquareCentiMetreSecond a owl:Class ;
    rdfs:label "SquareCentiMetreSecond"^^xsd:string ;
    rdfs:comment """"Square Centimeter Second" is a C.G.S System unit for  'Area Time' expressed as cm² . s.

-- QUDT"""@en ;
    rdfs:isDefinedBy "http://qudt.org/2.1/vocab/unit"^^xsd:string ;
    rdfs:subClassOf [ a owl:Restriction ;
            owl:hasValue 1e-04 ;
            owl:onProperty ns1:hasSIConversionMultiplier ],
        [ a owl:Restriction ;
            owl:hasValue 0e+00 ;
            owl:onProperty ns1:hasSIConversionOffset ],
        ns1:AreaTimeUnit,
        ns1:SINonCoherentDerivedUnit ;
    skos:altLabel "Square Centimetre Second"@en ;
    skos:prefLabel "SquareCentiMetreSecond"^^xsd:string ;
    ns1:elucidation """"Square Centimeter Second" is a C.G.S System unit for  'Area Time' expressed as cm² . s.

-- QUDT"""@en ;
    ns1:qudtReference "http://qudt.org/vocab/unit/CentiM2-SEC"^^xsd:string ;
    ns1:ucumCode "cm2.s"^^xsd:string ;
    ns1:unitSymbol "cm²⋅s"^^xsd:string .

ns1:SquareDeciMetre a owl:Class ;
    rdfs:label "SquareDeciMetre"^^xsd:string ;
    rdfs:comment """0.1-fold of the power of the SI base unit metre with the exponent 2

-- QUDT"""@en ;
    rdfs:isDefinedBy "http://qudt.org/2.1/vocab/unit"^^xsd:string ;
    rdfs:subClassOf [ a owl:Restriction ;
            owl:hasValue 1e-02 ;
            owl:onProperty ns1:hasSIConversionMultiplier ],
        [ a owl:Restriction ;
            owl:hasValue 0e+00 ;
            owl:onProperty ns1:hasSIConversionOffset ],
        ns1:AreaUnit,
        ns1:SINonCoherentDerivedUnit ;
    skos:altLabel "Square Decimetre"@en ;
    skos:prefLabel "SquareDeciMetre"^^xsd:string ;
    ns1:elucidation """0.1-fold of the power of the SI base unit metre with the exponent 2

-- QUDT"""@en ;
    ns1:qudtReference "http://qudt.org/vocab/unit/DeciM2"^^xsd:string ;
    ns1:ucumCode "dm2"^^xsd:string ;
    ns1:unitSymbol "dm²"^^xsd:string .

ns1:SquareMicroMetre a owl:Class ;
    rdfs:label "SquareMicroMetre"^^xsd:string ;
    rdfs:comment """0.000000000001-fold of the power of the SI base unit metre with the exponent 2

-- QUDT"""@en ;
    rdfs:isDefinedBy "http://qudt.org/2.1/vocab/unit"^^xsd:string ;
    rdfs:subClassOf [ a owl:Restriction ;
            owl:hasValue 1e-12 ;
            owl:onProperty ns1:hasSIConversionMultiplier ],
        [ a owl:Restriction ;
            owl:hasValue 0e+00 ;
            owl:onProperty ns1:hasSIConversionOffset ],
        ns1:AreaUnit,
        ns1:SINonCoherentDerivedUnit ;
    skos:altLabel "Square Micrometre"@en ;
    skos:prefLabel "SquareMicroMetre"^^xsd:string ;
    ns1:elucidation """0.000000000001-fold of the power of the SI base unit metre with the exponent 2

-- QUDT"""@en ;
    ns1:qudtReference "http://qudt.org/vocab/unit/MicroM2"^^xsd:string ;
    ns1:ucumCode "um2"^^xsd:string ;
    ns1:unitSymbol "μm²"^^xsd:string .

ns1:SquareMilliMetre a owl:Class ;
    rdfs:label "SquareMilliMetre"^^xsd:string ;
    rdfs:comment """0.000001-fold of the power of the SI base unit metre with the exponent 2

-- QUDT"""@en ;
    rdfs:isDefinedBy "http://qudt.org/2.1/vocab/unit"^^xsd:string ;
    rdfs:subClassOf [ a owl:Restriction ;
            owl:hasValue 1e-06 ;
            owl:onProperty ns1:hasSIConversionMultiplier ],
        [ a owl:Restriction ;
            owl:hasValue 0e+00 ;
            owl:onProperty ns1:hasSIConversionOffset ],
        ns1:AreaUnit,
        ns1:SINonCoherentDerivedUnit ;
    skos:altLabel "Square Millimetre"@en ;
    skos:prefLabel "SquareMilliMetre"^^xsd:string ;
    ns1:elucidation """0.000001-fold of the power of the SI base unit metre with the exponent 2

-- QUDT"""@en ;
    ns1:qudtReference "http://qudt.org/vocab/unit/MilliM2"^^xsd:string ;
    ns1:ucumCode "mm2"^^xsd:string ;
    ns1:unitSymbol "mm²"^^xsd:string .

ns1:SquareMilliMetrePerSecond a owl:Class ;
    rdfs:label "SquareMilliMetrePerSecond"^^xsd:string ;
    rdfs:comment """0.000001-fold of the power of the SI base unit metre with the exponent 2 divided by the SI base unit second

-- QUDT"""@en ;
    rdfs:isDefinedBy "http://qudt.org/2.1/vocab/unit"^^xsd:string ;
    rdfs:subClassOf [ a owl:Restriction ;
            owl:hasValue 1e-06 ;
            owl:onProperty ns1:hasSIConversionMultiplier ],
        [ a owl:Restriction ;
            owl:hasValue 0e+00 ;
            owl:onProperty ns1:hasSIConversionOffset ],
        ns1:AreicSpeedUnit,
        ns1:SINonCoherentDerivedUnit ;
    skos:altLabel "Square Millimetre Per Second"@en ;
    skos:prefLabel "SquareMilliMetrePerSecond"^^xsd:string ;
    ns1:elucidation """0.000001-fold of the power of the SI base unit metre with the exponent 2 divided by the SI base unit second

-- QUDT"""@en ;
    ns1:qudtReference "http://qudt.org/vocab/unit/MilliM2-PER-SEC"^^xsd:string ;
    ns1:ucumCode "mm2.s-1"^^xsd:string ;
    ns1:unitSymbol "mm²/s"^^xsd:string .

ns1:SquareNanoMetre a owl:Class ;
    rdfs:label "SquareNanoMetre"^^xsd:string ;
    rdfs:comment """A unit of area equal to that of a square, of sides 1nm

-- QUDT"""@en ;
    rdfs:isDefinedBy "http://qudt.org/2.1/vocab/unit"^^xsd:string ;
    rdfs:subClassOf [ a owl:Restriction ;
            owl:hasValue 0e+00 ;
            owl:onProperty ns1:hasSIConversionOffset ],
        [ a owl:Restriction ;
            owl:hasValue 1e-18 ;
            owl:onProperty ns1:hasSIConversionMultiplier ],
        ns1:AreaUnit,
        ns1:SINonCoherentDerivedUnit ;
    skos:altLabel "Square Nanometre"@en ;
    skos:prefLabel "SquareNanoMetre"^^xsd:string ;
    ns1:elucidation """A unit of area equal to that of a square, of sides 1nm

-- QUDT"""@en ;
    ns1:qudtReference "http://qudt.org/vocab/unit/NanoM2"^^xsd:string ;
    ns1:ucumCode "nm2"^^xsd:string ;
    ns1:unitSymbol "nm²"^^xsd:string .

ns1:VoltPerCentiMetre a owl:Class ;
    rdfs:label "VoltPerCentiMetre"^^xsd:string ;
    rdfs:comment """derived SI unit volt divided by the 0.01-fold of the SI base unit metre

-- QUDT"""@en ;
    rdfs:isDefinedBy "http://qudt.org/2.1/vocab/unit"^^xsd:string ;
    rdfs:subClassOf [ a owl:Restriction ;
            owl:hasValue 0e+00 ;
            owl:onProperty ns1:hasSIConversionOffset ],
        [ a owl:Restriction ;
            owl:hasValue 1e+02 ;
            owl:onProperty ns1:hasSIConversionMultiplier ],
        ns1:ElectricFieldStrengthUnit,
        ns1:SINonCoherentDerivedUnit ;
    skos:altLabel "Volt Per Centimetre"@en ;
    skos:prefLabel "VoltPerCentiMetre"^^xsd:string ;
    ns1:elucidation """derived SI unit volt divided by the 0.01-fold of the SI base unit metre

-- QUDT"""@en ;
    ns1:qudtReference "http://qudt.org/vocab/unit/V-PER-CentiM"^^xsd:string ;
    ns1:ucumCode "V.cm-1"^^xsd:string ;
    ns1:unitSymbol "V/cm"^^xsd:string .

ns1:VoltPerMicroSecond a owl:Class ;
    rdfs:label "VoltPerMicroSecond"^^xsd:string ;
    rdfs:comment """SI derived unit volt divided by the 0.000001-fold of the SI base unit second

-- QUDT"""@en ;
    rdfs:isDefinedBy "http://qudt.org/2.1/vocab/unit"^^xsd:string ;
    rdfs:subClassOf [ a owl:Restriction ;
            owl:hasValue 1e+06 ;
            owl:onProperty ns1:hasSIConversionMultiplier ],
        [ a owl:Restriction ;
            owl:hasValue 0e+00 ;
            owl:onProperty ns1:hasSIConversionOffset ],
        ns1:ElectricPotentialPerTimeUnit,
        ns1:SINonCoherentDerivedUnit ;
    skos:altLabel "Volt Per Microsecond"@en ;
    skos:prefLabel "VoltPerMicroSecond"^^xsd:string ;
    ns1:elucidation """SI derived unit volt divided by the 0.000001-fold of the SI base unit second

-- QUDT"""@en ;
    ns1:qudtReference "http://qudt.org/vocab/unit/V-PER-MicroSEC"^^xsd:string ;
    ns1:ucumCode "V.us-1"^^xsd:string ;
    ns1:unitSymbol "V/µs"^^xsd:string .

ns1:VoltPerMilliMetre a owl:Class ;
    rdfs:label "VoltPerMilliMetre"^^xsd:string ;
    rdfs:comment """SI derived unit volt divided by the 0.001-fold of the SI base unit metre

-- QUDT"""@en ;
    rdfs:isDefinedBy "http://qudt.org/2.1/vocab/unit"^^xsd:string ;
    rdfs:subClassOf [ a owl:Restriction ;
            owl:hasValue 0e+00 ;
            owl:onProperty ns1:hasSIConversionOffset ],
        [ a owl:Restriction ;
            owl:hasValue 1e+03 ;
            owl:onProperty ns1:hasSIConversionMultiplier ],
        ns1:ElectricFieldStrengthUnit,
        ns1:SINonCoherentDerivedUnit ;
    skos:altLabel "Volt Per Millimetre"@en ;
    skos:prefLabel "VoltPerMilliMetre"^^xsd:string ;
    ns1:elucidation """SI derived unit volt divided by the 0.001-fold of the SI base unit metre

-- QUDT"""@en ;
    ns1:qudtReference "http://qudt.org/vocab/unit/V-PER-MilliM"^^xsd:string ;
    ns1:ucumCode "V.mm-1"^^xsd:string ;
    ns1:unitSymbol "V/mm"^^xsd:string .

ns1:WattPerSquareCentiMetre a owl:Class ;
    rdfs:label "WattPerSquareCentiMetre"^^xsd:string ;
    rdfs:comment """Watt Per Square Centimeter is a unit of heat flux or thermal flux, the rate of heat energy transfer through a given surface.

-- QUDT"""@en ;
    rdfs:isDefinedBy "http://qudt.org/2.1/vocab/unit"^^xsd:string ;
    rdfs:subClassOf [ a owl:Restriction ;
            owl:hasValue 1e+04 ;
            owl:onProperty ns1:hasSIConversionMultiplier ],
        [ a owl:Restriction ;
            owl:hasValue 0e+00 ;
            owl:onProperty ns1:hasSIConversionOffset ],
        ns1:PowerDensityUnit,
        ns1:SINonCoherentDerivedUnit ;
    skos:altLabel "Watt per Square Centimetre"@en ;
    skos:prefLabel "WattPerSquareCentiMetre"^^xsd:string ;
    ns1:elucidation """Watt Per Square Centimeter is a unit of heat flux or thermal flux, the rate of heat energy transfer through a given surface.

-- QUDT"""@en ;
    ns1:qudtReference "http://qudt.org/vocab/unit/W-PER-CentiM2"^^xsd:string ;
    ns1:ucumCode "W.cm-2"^^xsd:string ;
    ns1:unitSymbol "W/cm²"^^xsd:string .

ns1:WeberPerMilliMetre a owl:Class ;
    rdfs:label "WeberPerMilliMetre"^^xsd:string ;
    rdfs:comment """derived SI unit weber divided by the 0.001-fold of the SI base unit metre

-- QUDT"""@en ;
    rdfs:isDefinedBy "http://qudt.org/2.1/vocab/unit"^^xsd:string ;
    rdfs:subClassOf [ a owl:Restriction ;
            owl:hasValue 0e+00 ;
            owl:onProperty ns1:hasSIConversionOffset ],
        [ a owl:Restriction ;
            owl:hasValue 1e+03 ;
            owl:onProperty ns1:hasSIConversionMultiplier ],
        ns1:MagneticPotentialUnit,
        ns1:SINonCoherentDerivedUnit ;
    skos:altLabel "Weber Per Millimetre"@en ;
    skos:prefLabel "WeberPerMilliMetre"^^xsd:string ;
    ns1:elucidation """derived SI unit weber divided by the 0.001-fold of the SI base unit metre

-- QUDT"""@en ;
    ns1:qudtReference "http://qudt.org/vocab/unit/WB-PER-MilliM"^^xsd:string ;
    ns1:ucumCode "Wb.mm-1"^^xsd:string ;
    ns1:unitSymbol "Wb/mm"^^xsd:string .

<https://w3id.org/emmo/disciplines/units/noncoherentsiunits> a owl:Ontology ;
    dcterms:abstract "The 'noncoherentsiunits' module contains non-coherent derived SI units (and SI-accepted units) that are not prefixed units (units made of a metric prefix followed by a unit symbol).  Examples: km/h, A/g."@en ;
    dcterms:contributor ns1:FrancescaBleken,
        ns1:GerhardGoldbeck,
        ns1:SimonClark ;
    dcterms:creator ns1:EmanueleGhedini,
        ns1:JesperFriis ;
    dcterms:license "https://creativecommons.org/licenses/by/4.0/legalcode"^^xsd:string ;
    dcterms:publisher <https://emmc.eu> ;
    dcterms:title "Non-coherent SI units"@en ;
    rdfs:comment """Note: this file has automatically been populated with units from QUDT.

We kindly acknowledge NIST for reusing their content, including the selection of units, their elucidations and conversion multiplier."""@en,
        "The EMMO should be reasoned with HermiT to visualize all inferences and class hierarchy (ctrl+R hotkey in Protege)."@en ;
    owl:imports <https://w3id.org/emmo/1.0.2/disciplines/units/coherentsiunits> ;
    owl:versionIRI <https://w3id.org/emmo/1.0.2/disciplines/units/noncoherentsiunits> ;
    owl:versionInfo "1.0.2"^^xsd:string ;
    ns1:contact "emmo@emmc.eu"^^xsd:string .

ns1:AmperePerMilliMetre a owl:Class ;
    rdfs:label "AmperePerMilliMetre"@en ;
    rdfs:comment """SI base unit ampere divided by the 0.001-fold of the SI base unit metre

-- QUDT"""@en ;
    rdfs:isDefinedBy "http://qudt.org/2.1/vocab/unit"^^xsd:string ;
    rdfs:subClassOf [ a owl:Restriction ;
            owl:hasValue 0e+00 ;
            owl:onProperty ns1:hasSIConversionOffset ],
        [ a owl:Restriction ;
            owl:hasValue 1e+03 ;
            owl:onProperty ns1:hasSIConversionMultiplier ],
        ns1:MagneticFieldStrengthUnit,
        ns1:SINonCoherentDerivedUnit ;
    skos:altLabel "Ampere Per Millimetre"@en ;
    skos:prefLabel "AmperePerMilliMetre"@en ;
    ns1:elucidation """SI base unit ampere divided by the 0.001-fold of the SI base unit metre

-- QUDT"""@en ;
    ns1:qudtReference "http://qudt.org/vocab/unit/A-PER-MilliM"^^xsd:string ;
    ns1:ucumCode "A.mm-1"^^xsd:string,
        "A/mm"^^xsd:string ;
    ns1:unitSymbol "A/mm"^^xsd:string .

ns1:GramPerMetre a owl:Class ;
    rdfs:label "GramPerMetre"@en ;
    rdfs:comment """0,001-fold of the SI base unit kilogram divided by the SI base unit metre

-- QUDT"""@en ;
    rdfs:isDefinedBy "http://qudt.org/2.1/vocab/unit"^^xsd:string ;
    rdfs:subClassOf [ a owl:Restriction ;
            owl:hasValue 1e-03 ;
            owl:onProperty ns1:hasSIConversionMultiplier ],
        [ a owl:Restriction ;
            owl:hasValue 0e+00 ;
            owl:onProperty ns1:hasSIConversionOffset ],
        ns1:MassPerLengthUnit,
        ns1:MeasurementUnit,
        ns1:NonPrefixedUnit,
        ns1:SINonCoherentUnit ;
    skos:altLabel "Gram Per Metre"@en ;
    skos:prefLabel "GramPerMetre"@en ;
    ns1:elucidation """0,001-fold of the SI base unit kilogram divided by the SI base unit metre

-- QUDT"""@en ;
    ns1:qudtReference "http://qudt.org/vocab/unit/GM-PER-M"^^xsd:string ;
    ns1:ucumCode "g.m-1"^^xsd:string ;
    ns1:unitSymbol "g/m"^^xsd:string .

ns1:GramPerSecond a owl:Class ;
    rdfs:label "GramPerSecond"@en ;
    rdfs:comment """0,001fold of the SI base unit kilogram divided by the SI base unit second

-- QUDT"""@en ;
    rdfs:isDefinedBy "http://qudt.org/2.1/vocab/unit"^^xsd:string ;
    rdfs:subClassOf [ a owl:Restriction ;
            owl:hasValue 0e+00 ;
            owl:onProperty ns1:hasSIConversionOffset ],
        [ a owl:Restriction ;
            owl:hasValue 1e-03 ;
            owl:onProperty ns1:hasSIConversionMultiplier ],
        ns1:MassPerTimeUnit,
        ns1:MeasurementUnit,
        ns1:NonPrefixedUnit,
        ns1:SINonCoherentUnit ;
    skos:altLabel "Gram Per Second"@en ;
    skos:prefLabel "GramPerSecond"@en ;
    ns1:elucidation """0,001fold of the SI base unit kilogram divided by the SI base unit second

-- QUDT"""@en ;
    ns1:qudtReference "http://qudt.org/vocab/unit/GM-PER-SEC"^^xsd:string ;
    ns1:ucumCode "g.s-1"^^xsd:string ;
    ns1:unitSymbol "g/s"^^xsd:string .

ns1:GramPerSquareMetre a owl:Class ;
    rdfs:label "GramPerSquareMetre"@en ;
    rdfs:comment """0,001-fold of the SI base unit kilogram divided by the power of the SI base unit metre with the exponent 2

-- QUDT"""@en ;
    rdfs:isDefinedBy "http://qudt.org/2.1/vocab/unit"^^xsd:string ;
    rdfs:subClassOf [ a owl:Restriction ;
            owl:hasValue 0e+00 ;
            owl:onProperty ns1:hasSIConversionOffset ],
        [ a owl:Restriction ;
            owl:hasValue 1e-03 ;
            owl:onProperty ns1:hasSIConversionMultiplier ],
        ns1:AreaDensityUnit,
        ns1:MeasurementUnit,
        ns1:NonPrefixedUnit,
        ns1:SINonCoherentUnit ;
    skos:altLabel "Gram Per Square Metre"@en ;
    skos:prefLabel "GramPerSquareMetre"@en ;
    ns1:elucidation """0,001-fold of the SI base unit kilogram divided by the power of the SI base unit metre with the exponent 2

-- QUDT"""@en ;
    ns1:qudtReference "http://qudt.org/vocab/unit/GM-PER-M2"^^xsd:string ;
    ns1:ucumCode "g.m-2"^^xsd:string,
        "g/m2"^^xsd:string ;
    ns1:unitSymbol "g/m²"^^xsd:string .

ns1:WattPerSquareMetrePerNanoMetre a owl:Class ;
    rdfs:label "WattPerSquareMetrePerNanoMetre"^^xsd:string ;
    rdfs:comment "Watt per square metre and nanometre."@en ;
    rdfs:isDefinedBy "http://qudt.org/2.1/vocab/unit"^^xsd:string ;
    rdfs:subClassOf [ a owl:Restriction ;
            owl:hasValue 1e+09 ;
            owl:onProperty ns1:hasSIConversionMultiplier ],
        [ a owl:Restriction ;
            owl:hasValue 0e+00 ;
            owl:onProperty ns1:hasSIConversionOffset ],
        ns1:PressurePerTimeUnit,
        ns1:SINonCoherentDerivedUnit ;
    skos:prefLabel "WattPerSquareMetrePerNanoMetre"^^xsd:string ;
    ns1:elucidation "Watt per square metre and nanometre."@en ;
    ns1:qudtReference "http://qudt.org/vocab/unit/W-PER-M2-NanoM"^^xsd:string ;
    ns1:ucumCode "W.m-2.nm-1"^^xsd:string ;
    ns1:unitSymbol "W/m²⋅nm"^^xsd:string .

ns1:WattPerSquareMetrePerNanoMetrePerSteradian a owl:Class ;
    rdfs:label "WattPerSquareMetrePerNanoMetrePerSteradian"^^xsd:string ;
    rdfs:comment "Watt per square metre and nanometre and steradian unit."@en ;
    rdfs:isDefinedBy "http://qudt.org/2.1/vocab/unit"^^xsd:string ;
    rdfs:subClassOf [ a owl:Restriction ;
            owl:hasValue 1e+09 ;
            owl:onProperty ns1:hasSIConversionMultiplier ],
        [ a owl:Restriction ;
            owl:hasValue 0e+00 ;
            owl:onProperty ns1:hasSIConversionOffset ],
        ns1:PressurePerTimeUnit,
        ns1:SINonCoherentDerivedUnit ;
    skos:prefLabel "WattPerSquareMetrePerNanoMetrePerSteradian"^^xsd:string ;
    ns1:elucidation "Watt per square metre and nanometre and steradian unit."@en ;
    ns1:qudtReference "http://qudt.org/vocab/unit/W-PER-M2-NanoM-SR"^^xsd:string ;
    ns1:ucumCode "W.m-2.nm-1.sr-1"^^xsd:string ;
    ns1:unitSymbol "W/m²⋅nm⋅sr"^^xsd:string .

ns1:GramPerSquareCentiMetre a owl:Class ;
    rdfs:label "GramPerSquareCentiMetre"^^xsd:string ;
    rdfs:comment """0,001-fold of the SI base unit kilogram divided by the 0.0001-fold of the power of the SI base unit metre and exponent 2

-- QUDT"""@en ;
    rdfs:isDefinedBy "http://qudt.org/2.1/vocab/unit"^^xsd:string ;
    rdfs:subClassOf [ a owl:Restriction ;
            owl:hasValue 1e+01 ;
            owl:onProperty ns1:hasSIConversionMultiplier ],
        [ a owl:Restriction ;
            owl:hasValue 0e+00 ;
            owl:onProperty ns1:hasSIConversionOffset ],
        ns1:AreaDensityUnit,
        ns1:MeasurementUnit,
        ns1:PrefixedUnit,
        ns1:SINonCoherentUnit ;
    skos:altLabel "Gram Per Square Centimetre"@en ;
    skos:prefLabel "GramPerSquareCentiMetre"^^xsd:string ;
    ns1:elucidation """0,001-fold of the SI base unit kilogram divided by the 0.0001-fold of the power of the SI base unit metre and exponent 2

-- QUDT"""@en ;
    ns1:qudtReference "http://qudt.org/vocab/unit/GM-PER-CentiM2"^^xsd:string ;
    ns1:ucumCode "g.cm-2"^^xsd:string,
        "g/cm2"^^xsd:string ;
    ns1:unitSymbol "g/cm²"^^xsd:string .

ns1:HenryPerKiloOhm a owl:Class ;
    rdfs:label "HenryPerKiloOhm"@en ;
    rdfs:comment """SI derived unit henry divided by the 1 000-fold of the SI derived unit ohm

-- QUDT"""@en ;
    rdfs:isDefinedBy "http://qudt.org/2.1/vocab/unit"^^xsd:string ;
    rdfs:subClassOf [ a owl:Restriction ;
            owl:hasValue 0e+00 ;
            owl:onProperty ns1:hasSIConversionOffset ],
        [ a owl:Restriction ;
            owl:hasValue 1e-03 ;
            owl:onProperty ns1:hasSIConversionMultiplier ],
        ns1:SINonCoherentDerivedUnit,
        ns1:TimeUnit ;
    skos:altLabel "Henry Per Kiloohm"@en ;
    skos:prefLabel "HenryPerKiloOhm"@en ;
    ns1:elucidation """SI derived unit henry divided by the 1 000-fold of the SI derived unit ohm

-- QUDT"""@en ;
    ns1:qudtReference "http://qudt.org/vocab/unit/H-PER-KiloOHM"^^xsd:string ;
    ns1:ucumCode "H.kOhm-1"^^xsd:string ;
    ns1:unitSymbol "H/kΩ"^^xsd:string .

ns1:SiemensPerCentiMetre a owl:Class ;
    rdfs:label "SiemensPerCentiMetre"^^xsd:string ;
    rdfs:comment """SI derived unit Siemens divided by the 0.01-fold of the SI base unit metre

-- QUDT"""@en ;
    rdfs:isDefinedBy "http://qudt.org/2.1/vocab/unit"^^xsd:string ;
    rdfs:subClassOf [ a owl:Restriction ;
            owl:hasValue 0e+00 ;
            owl:onProperty ns1:hasSIConversionOffset ],
        [ a owl:Restriction ;
            owl:hasValue 1e+02 ;
            owl:onProperty ns1:hasSIConversionMultiplier ],
        ns1:ElectricConductivityUnit,
        ns1:SINonCoherentDerivedUnit ;
    skos:altLabel "Siemens Per Centimetre"@en ;
    skos:prefLabel "SiemensPerCentiMetre"^^xsd:string ;
    ns1:elucidation """SI derived unit Siemens divided by the 0.01-fold of the SI base unit metre

-- QUDT"""@en ;
    ns1:qudtReference "http://qudt.org/vocab/unit/S-PER-CentiM"^^xsd:string ;
    ns1:ucumCode "S.cm-1"^^xsd:string ;
    ns1:unitSymbol "S/cm"^^xsd:string .

ns1:GramPerCubicMetre a owl:Class ;
    rdfs:label "GramPerCubicMetre"@en ;
    rdfs:comment """0,001-fold of the SI base unit kilogram divided by the power of the SI base unit metre with the exponent 3

-- QUDT"""@en ;
    rdfs:isDefinedBy "http://qudt.org/2.1/vocab/unit"^^xsd:string ;
    rdfs:subClassOf [ a owl:Restriction ;
            owl:hasValue 0e+00 ;
            owl:onProperty ns1:hasSIConversionOffset ],
        [ a owl:Restriction ;
            owl:hasValue 1e-03 ;
            owl:onProperty ns1:hasSIConversionMultiplier ],
        ns1:DensityUnit,
        ns1:MeasurementUnit,
        ns1:NonPrefixedUnit,
        ns1:SINonCoherentUnit ;
    skos:altLabel "Gram Per Cubic Metre"@en ;
    skos:prefLabel "GramPerCubicMetre"@en ;
    ns1:elucidation """0,001-fold of the SI base unit kilogram divided by the power of the SI base unit metre with the exponent 3

-- QUDT"""@en ;
    ns1:qudtReference "http://qudt.org/vocab/unit/GM-PER-M3"^^xsd:string ;
    ns1:ucumCode "g.m-3"^^xsd:string,
        "g/m3"^^xsd:string ;
    ns1:unitSymbol "g/m³"^^xsd:string .

ns1:GramPerKilogram a owl:Class ;
    rdfs:label "GramPerKilogram"^^xsd:string ;
    rdfs:comment """0,001 fold of the SI base unit kilogram divided by the SI base unit kilogram

-- QUDT"""@en ;
    rdfs:isDefinedBy "http://qudt.org/2.1/vocab/unit"^^xsd:string ;
    rdfs:subClassOf [ a owl:Restriction ;
            owl:hasValue 0e+00 ;
            owl:onProperty ns1:hasSIConversionOffset ],
        [ a owl:Restriction ;
            owl:hasValue 1e-03 ;
            owl:onProperty ns1:hasSIConversionMultiplier ],
        ns1:MassFractionUnit,
        ns1:NonPrefixedUnit,
        ns1:SINonCoherentUnit ;
    skos:altLabel "Gram Per Kilogram"@en ;
    skos:prefLabel "GramPerKilogram"^^xsd:string ;
    ns1:elucidation """0,001 fold of the SI base unit kilogram divided by the SI base unit kilogram

-- QUDT"""@en ;
    ns1:qudtReference "http://qudt.org/vocab/unit/GM-PER-KiloGM"^^xsd:string ;
    ns1:ucumCode "g.kg-1"^^xsd:string,
        "g/kg"^^xsd:string ;
    ns1:unitSymbol "g/kg"^^xsd:string .

