<?xml version="1.0" encoding="UTF-8"?>
<rdf:RDF
   xmlns="http://emmo.info/emmo#"
   xmlns:dcterms="http://purl.org/dc/terms/"
   xmlns:owl="http://www.w3.org/2002/07/owl#"
   xmlns:rdf="http://www.w3.org/1999/02/22-rdf-syntax-ns#"
   xmlns:rdfs="http://www.w3.org/2000/01/rdf-schema#"
   xmlns:skos="http://www.w3.org/2004/02/skos/core#"
>
  <rdf:Description rdf:about="http://emmo.info/emmo/middle/perspective">
    <dcterms:contributor>Access, DE</dcterms:contributor>
    <owl:versionInfo>1.0.0-beta</owl:versionInfo>
    <dcterms:creator>Georg Schmitz</dcterms:creator>
    <dcterms:creator>Jesper Friis</dcterms:creator>
    <rdf:type rdf:resource="http://www.w3.org/2002/07/owl#Ontology"/>
    <dcterms:contributor>Fraunhofer IWM, DE</dcterms:contributor>
    <dcterms:publisher>EMMC ASBL</dcterms:publisher>
    <dcterms:creator>Emanuele Ghedini</dcterms:creator>
    <dcterms:contributor>University of Bologna, IT</dcterms:contributor>
    <dcterms:contributor>Goldbeck Consulting Ltd (UK)</dcterms:contributor>
    <dcterms:contributor>SINTEF, NO</dcterms:contributor>
    <dcterms:creator>Gerhard Goldbeck</dcterms:creator>
    <rdfs:comment xml:lang="en">Contacts:
Gerhard Goldbeck
Goldbeck Consulting Ltd (UK)
email: gerhard@goldbeck-consulting.com

Emanuele Ghedini
University of Bologna (IT)
email: emanuele.ghedini@unibo.it</rdfs:comment>
    <dcterms:title xml:lang="en">European Materials &amp; Modelling Ontology</dcterms:title>
    <dcterms:creator>Adham Hashibon</dcterms:creator>
    <rdfs:comment xml:lang="en">The EMMO requires FacT++ reasoner plugin in order to visualize all inferences and class hierarchy (ctrl+R hotkey in Protege).</rdfs:comment>
    <dcterms:license>https://creativecommons.org/licenses/by/4.0/legalcode</dcterms:license>
    <dcterms:abstract xml:lang="en">European Materials &amp; Modelling Ontology (EMMO)

EMMO is a multidisciplinary effort to develop a standard representational framework (the ontology) based on current materials modelling knowledge, including physical sciences, analytical philosophy and information and communication technologies.

It provides the connection between the physical world, materials characterisation world and materials modelling world.

EMMO is released under a Creative Commons license Attribution 4.0 International (CC BY 4.0).</dcterms:abstract>
    <owl:versionIRI rdf:resource="http://emmo.info/emmo/1.0.0-beta/middle/perspective"/>
  </rdf:Description>
  <rdf:Description rdf:about="http://emmo.info/emmo/middle">
    <dcterms:license>https://creativecommons.org/licenses/by/4.0/legalcode</dcterms:license>
    <dcterms:contributor>Goldbeck Consulting Ltd (UK)</dcterms:contributor>
    <dcterms:contributor>SINTEF, NO</dcterms:contributor>
    <dcterms:abstract xml:lang="en">European Materials &amp; Modelling Ontology (EMMO)

EMMO is a multidisciplinary effort to develop a standard representational framework (the ontology) based on current materials modelling knowledge, including physical sciences, analytical philosophy and information and communication technologies.

It provides the connection between the physical world, materials characterisation world and materials modelling world.

EMMO is released under a Creative Commons license Attribution 4.0 International (CC BY 4.0).</dcterms:abstract>
    <dcterms:contributor>University of Bologna, IT</dcterms:contributor>
    <dcterms:creator>Jesper Friis</dcterms:creator>
    <owl:versionInfo>1.0.0-beta</owl:versionInfo>
    <dcterms:creator>Emanuele Ghedini</dcterms:creator>
    <dcterms:creator>Georg Schmitz</dcterms:creator>
    <dcterms:publisher>EMMC ASBL</dcterms:publisher>
    <dcterms:contributor>Fraunhofer IWM, DE</dcterms:contributor>
    <dcterms:contributor>Access, DE</dcterms:contributor>
    <dcterms:title xml:lang="en">European Materials &amp; Modelling Ontology</dcterms:title>
    <owl:versionIRI rdf:resource="http://emmo.info/emmo/1.0.0-beta/middle"/>
    <rdfs:comment xml:lang="en">The EMMO requires FacT++ reasoner plugin in order to visualize all inferences and class hierarchy (ctrl+R hotkey in Protege).</rdfs:comment>
    <dcterms:creator>Adham Hashibon</dcterms:creator>
    <rdf:type rdf:resource="http://www.w3.org/2002/07/owl#Ontology"/>
    <rdfs:comment xml:lang="en">Contacts:
Gerhard Goldbeck
Goldbeck Consulting Ltd (UK)
email: gerhard@goldbeck-consulting.com

Emanuele Ghedini
University of Bologna (IT)
email: emanuele.ghedini@unibo.it</rdfs:comment>
    <dcterms:creator>Gerhard Goldbeck</dcterms:creator>
  </rdf:Description>
  <rdf:Description rdf:nodeID="f05bdaa1e617a4bccafc519daf7bf4785b122">
    <rdf:type rdf:resource="http://www.w3.org/2002/07/owl#Restriction"/>
    <owl:onProperty rdf:resource="http://emmo.info/emmo#EMMO_23b579e1_8088_45b5_9975_064014026c42"/>
    <owl:hasValue>F</owl:hasValue>
  </rdf:Description>
  <rdf:Description rdf:about="http://emmo.info/emmo#EMMO_b20be325_8bfd_4237_bee7_201ab0fd9c75">
    <EMMO_1f1b164d_ec6a_4faa_8d5e_88bda62316cc>http://qudt.org/vocab/unit/DEG_C</EMMO_1f1b164d_ec6a_4faa_8d5e_88bda62316cc>
    <skos:prefLabel xml:lang="en">DegreeCelsius</skos:prefLabel>
    <EMMO_fe015383_afb3_44a6_ae86_043628697aa2>https://doi.org/10.1351/goldbook.D01561</EMMO_fe015383_afb3_44a6_ae86_043628697aa2>
    <rdfs:comment xml:lang="en">Measurement unit for Celsius temperature. This unit can only be used for expressing temperature differences.</rdfs:comment>
    <rdfs:subClassOf rdf:nodeID="f05bdaa1e617a4bccafc519daf7bf4785b128"/>
    <rdfs:subClassOf rdf:nodeID="f05bdaa1e617a4bccafc519daf7bf4785b127"/>
    <rdf:type rdf:resource="http://www.w3.org/2002/07/owl#Class"/>
  </rdf:Description>
  <rdf:Description rdf:nodeID="f0b819106611c4b798f33b16c65f4398db3">
    <rdf:type rdf:resource="http://www.w3.org/1999/02/22-rdf-syntax-ns#List"/>
    <rdf:first rdf:resource="http://emmo.info/emmo#EMMO_49804605_c0fe_4538_abda_f70ba1dc8a5d"/>
    <rdf:rest rdf:resource="http://www.w3.org/1999/02/22-rdf-syntax-ns#nil"/>
  </rdf:Description>
  <rdf:Description rdf:nodeID="f05bdaa1e617a4bccafc519daf7bf4785b125">
    <owl:onProperty rdf:resource="http://emmo.info/emmo#EMMO_bed1d005_b04e_4a90_94cf_02bc678a8569"/>
    <owl:someValuesFrom rdf:resource="http://emmo.info/emmo#EMMO_ec903946_ddc9_464a_903c_7373e0d1eeb5"/>
    <rdf:type rdf:resource="http://www.w3.org/2002/07/owl#Restriction"/>
  </rdf:Description>
  <rdf:Description rdf:about="http://emmo.info/emmo#EMMO_89a0c87c_0804_4013_937a_6fe234d9499c">
    <rdfs:subClassOf rdf:nodeID="f38ecd0eaa78747b4ad569754ea441153b3"/>
    <rdfs:subClassOf rdf:resource="http://emmo.info/emmo#EMMO_057e7d57_aff0_49de_911a_8861d85cef40"/>
    <rdf:type rdf:resource="http://www.w3.org/2002/07/owl#Class"/>
    <skos:prefLabel xml:lang="en">SymbolicComposition</skos:prefLabel>
    <EMMO_967080e5_2f42_4eb2_a3a9_c58143e835f9 xml:lang="en">A symbolic entity made of other symbolic entities according to a specific spatial configuration.</EMMO_967080e5_2f42_4eb2_a3a9_c58143e835f9>
    <rdfs:comment xml:lang="en">This class collects individuals that represents arrangements of strings, or other symbolic compositions, without any particular predifined arrangement schema.</rdfs:comment>
  </rdf:Description>
  <rdf:Description rdf:nodeID="f05bdaa1e617a4bccafc519daf7bf4785b161">
    <owl:allValuesFrom rdf:nodeID="f05bdaa1e617a4bccafc519daf7bf4785b163"/>
    <rdf:type rdf:resource="http://www.w3.org/2002/07/owl#Restriction"/>
    <owl:onProperty rdf:nodeID="f05bdaa1e617a4bccafc519daf7bf4785b162"/>
  </rdf:Description>
  <rdf:Description rdf:nodeID="ffcb99037244f48d590430c228d02afdbb33">
    <rdf:type rdf:resource="http://www.w3.org/2002/07/owl#Restriction"/>
    <owl:onProperty rdf:resource="http://emmo.info/emmo#EMMO_bed1d005_b04e_4a90_94cf_02bc678a8569"/>
    <owl:someValuesFrom rdf:resource="http://emmo.info/emmo#EMMO_3227b821_26a5_4c7c_9c01_5c24483e0bd0"/>
  </rdf:Description>
  <rdf:Description rdf:about="http://emmo.info/emmo#EMMO_de021e4f_918f_47ef_a67b_11120f56b9d7">
    <EMMO_de178b12_5d35_4bca_8efa_a4193162571d>T-2 L+1 M+1 I-2 Θ0 N0 J0</EMMO_de178b12_5d35_4bca_8efa_a4193162571d>
    <rdf:type rdf:resource="http://www.w3.org/2002/07/owl#Class"/>
    <rdfs:comment xml:lang="en">The DBpedia and UIPAC Gold Book definitions (http://dbpedia.org/page/Vacuum_permeability,  https://doi.org/10.1351/goldbook.P04504) are outdated since May 20, 2019. It is now a measured constant.</rdfs:comment>
    <skos:prefLabel xml:lang="en">VacuumMagneticPermeability</skos:prefLabel>
    <EMMO_1f1b164d_ec6a_4faa_8d5e_88bda62316cc>http://qudt.org/vocab/constant/ElectromagneticPermeabilityOfVacuum</EMMO_1f1b164d_ec6a_4faa_8d5e_88bda62316cc>
    <rdfs:subClassOf rdf:resource="http://emmo.info/emmo#EMMO_09663630_1b84_4202_91e6_e641104f579e"/>
    <rdfs:subClassOf rdf:resource="http://emmo.info/emmo#EMMO_3f15d200_c97b_42c8_8ac0_d81d150361e2"/>
    <rdfs:comment xml:lang="en">The value of magnetic permeability in a classical vacuum.</rdfs:comment>
    <EMMO_a9b3d04c_7ceb_40a2_b8d3_28d514a770a8>https://physics.nist.gov/cgi-bin/cuu/Value?mu0</EMMO_a9b3d04c_7ceb_40a2_b8d3_28d514a770a8>
  </rdf:Description>
  <rdf:Description rdf:about="http://emmo.info/emmo#EMMO_21f56795_ee72_4858_b571_11cfaa59c1a8">
    <skos:prefLabel xml:lang="en">Number</skos:prefLabel>
    <rdf:type rdf:resource="http://www.w3.org/2002/07/owl#Class"/>
    <rdfs:subClassOf rdf:resource="http://emmo.info/emmo#EMMO_4ce76d7f_03f8_45b6_9003_90052a79bfaa"/>
    <rdfs:comment xml:lang="en">In math usually number and numeral are distinct concepts, the numeral being the symbol or a composition of symbols (e.g. 3.14, 010010, three) and the number is the idea behind it.

More than one numeral stand for the same number.

In the EMMO abstract entities does not exists, and numbers are simply defined by other numerals, so that a number is the class of all the numerals that are equivalent (e.g. 3 and 0011 are numerals that stands for the same number).

Or alternatively, an integer numeral may also stands for a set of a specific cardinality (e.g. 3 stands for a set of three apples). Rational and real numbers are simply a syntactic arrangment of integers (digits, in decimal system).

The fact that you can't give a name to a number without using a numeral or, in case of positive integers, without referring to a real world objects set with specific cardinality, suggests that the abstract concept of number is not a concept that can be practically used.

For these reasons, the EMMO will consider numerals and numbers as the same concept.</rdfs:comment>
    <rdfs:comment xml:lang="en">A number is actually a string (e.g. 1.4, 1e-8) of numerical digits and other symbols. However, in order not to increase complexity of the taxonomy and relations, here we take a number as an "atomic" object (i.e. we do not include digits in the EMMO as alphabet for numbers).

A 'Number' individual provide the link between the ontology and the actual data, through the data property hasNumericalValue.</rdfs:comment>
    <rdfs:subClassOf rdf:resource="http://emmo.info/emmo#EMMO_a1083d0a_c1fb_471f_8e20_a98f881ad527"/>
    <EMMO_967080e5_2f42_4eb2_a3a9_c58143e835f9 xml:lang="en">A numerical data value.</EMMO_967080e5_2f42_4eb2_a3a9_c58143e835f9>
  </rdf:Description>
  <rdf:Description rdf:about="http://emmo.info/emmo#EMMO_dd4a7f3e_ef56_466c_ac1a_d2716b5f87ec">
    <EMMO_967080e5_2f42_4eb2_a3a9_c58143e835f9 xml:lang="en">A 'Quantity' that can be quantified with respect to a standardized reference physical instance (e.g. the prototype meter bar, the kg prototype) or method (e.g. resilience) through a measurement process.</EMMO_967080e5_2f42_4eb2_a3a9_c58143e835f9>
    <rdfs:comment xml:lang="en">Subclasses of 'QuantitativeProperty' classify objects according to the type semiosis that is used to connect the property to the object (e.g. by measurement, by convention, by modelling).</rdfs:comment>
    <rdfs:subClassOf rdf:resource="http://emmo.info/emmo#EMMO_2a888cdf_ec4a_4ec5_af1c_0343372fc978"/>
    <rdf:type rdf:resource="http://www.w3.org/2002/07/owl#Class"/>
    <rdfs:subClassOf rdf:resource="http://emmo.info/emmo#EMMO_f658c301_ce93_46cf_9639_4eace2c5d1d5"/>
    <EMMO_70fe84ff_99b6_4206_a9fc_9a8931836d84 xml:lang="en">"A property of a phenomenon, body, or substance, where the property has a magnitude that can be expressed by means of a number and a reference"
ISO 80000-1

"A reference can be a measurement unit, a measurement procedure, a reference material, or a combination of such."
International vocabulary of metrology (VIM)</EMMO_70fe84ff_99b6_4206_a9fc_9a8931836d84>
    <rdfs:comment xml:lang="en">A quantitative property is always expresssed as a quantity (i.e. a number and a reference unit). For the EMMO, a nominalistic ontology, there is no property as abstract object.

A property is a sign that stands for an object according to a specific code shared by some observers.

For quantititative properties, one possible code that is shared between the scientific community (the observers) is the SI system of units.</rdfs:comment>
    <owl:equivalentClass rdf:nodeID="fdb1489b80bcc4ee28afe0be8feb9b935b13"/>
    <skos:prefLabel xml:lang="en">QuantitativeProperty</skos:prefLabel>
  </rdf:Description>
  <rdf:Description rdf:about="http://emmo.info/emmo#EMMO_506f7823_52bc_40cb_be07_b3b1e10cce13">
    <EMMO_a9b3d04c_7ceb_40a2_b8d3_28d514a770a8>https://physics.nist.gov/cgi-bin/cuu/Value?kcd</EMMO_a9b3d04c_7ceb_40a2_b8d3_28d514a770a8>
    <skos:prefLabel xml:lang="en">LuminousEfficacyOf540THzRadiation</skos:prefLabel>
    <rdf:type rdf:resource="http://www.w3.org/2002/07/owl#Class"/>
    <rdfs:comment xml:lang="en">Defines the Candela base unit in the SI system.</rdfs:comment>
    <rdfs:subClassOf rdf:resource="http://emmo.info/emmo#EMMO_f2ca6dd0_0e5f_4392_a92d_cafdae6cfc95"/>
    <EMMO_967080e5_2f42_4eb2_a3a9_c58143e835f9 xml:lang="en">The luminous efficacy of monochromatic radiation of frequency 540 × 10 12 Hz, K cd , is a technical constant that gives an exact numerical relationship between the purely physical characteristics of the radiant power stimulating the human eye (W) and its photobiological response defined by the luminous flux due to the spectral responsivity of a standard observer (lm) at a frequency of 540 × 10 12 hertz.</EMMO_967080e5_2f42_4eb2_a3a9_c58143e835f9>
    <EMMO_de178b12_5d35_4bca_8efa_a4193162571d>T+3 L-1 M-1 I0 Θ0 N0 J+1</EMMO_de178b12_5d35_4bca_8efa_a4193162571d>
  </rdf:Description>
  <rdf:Description rdf:about="http://emmo.info/emmo#EMMO_a3c78d6f_ae49_47c8_a634_9b6d86b79382">
    <EMMO_1f1b164d_ec6a_4faa_8d5e_88bda62316cc>http://qudt.org/vocab/constant/RydbergConstant</EMMO_1f1b164d_ec6a_4faa_8d5e_88bda62316cc>
    <EMMO_fe015383_afb3_44a6_ae86_043628697aa2>https://doi.org/10.1351/goldbook.R05430</EMMO_fe015383_afb3_44a6_ae86_043628697aa2>
    <EMMO_a9b3d04c_7ceb_40a2_b8d3_28d514a770a8>https://physics.nist.gov/cgi-bin/cuu/Value?ryd</EMMO_a9b3d04c_7ceb_40a2_b8d3_28d514a770a8>
    <EMMO_6dd685dd_1895_46e4_b227_be9f7d643c25>http://dbpedia.org/page/Rydberg_constant</EMMO_6dd685dd_1895_46e4_b227_be9f7d643c25>
    <EMMO_de178b12_5d35_4bca_8efa_a4193162571d>T0 L-1 M0 I0 Θ0 N0 J0</EMMO_de178b12_5d35_4bca_8efa_a4193162571d>
    <skos:prefLabel xml:lang="en">RybergConstant</skos:prefLabel>
    <rdfs:comment xml:lang="en">The Rydberg constant represents the limiting value of the highest wavenumber (the inverse wavelength) of any photon that can be emitted from the hydrogen atom, or, alternatively, the wavenumber of the lowest-energy photon capable of ionizing the hydrogen atom from its ground state.</rdfs:comment>
    <rdfs:subClassOf rdf:resource="http://emmo.info/emmo#EMMO_d859588d_44dc_4614_bc75_5fcd0058acc8"/>
    <rdf:type rdf:resource="http://www.w3.org/2002/07/owl#Class"/>
    <rdfs:subClassOf rdf:resource="http://emmo.info/emmo#EMMO_3f15d200_c97b_42c8_8ac0_d81d150361e2"/>
  </rdf:Description>
  <rdf:Description rdf:nodeID="f627ff42579444148ae27fcacfb5f8528b4">
    <owl:inverseOf rdf:resource="http://emmo.info/emmo#EMMO_24c71baf_6db6_48b9_86c8_8c70cf36db0c"/>
  </rdf:Description>
  <rdf:Description rdf:about="http://emmo.info/emmo/middle/metrology">
    <dcterms:license>https://creativecommons.org/licenses/by/4.0/legalcode</dcterms:license>
    <dcterms:contributor>Fraunhofer IWM, DE</dcterms:contributor>
    <dcterms:creator>Adham Hashibon</dcterms:creator>
    <rdfs:comment xml:lang="en">The EMMO requires FacT++ reasoner plugin in order to visualize all inferences and class hierarchy (ctrl+R hotkey in Protege).</rdfs:comment>
    <dcterms:creator>Jesper Friis</dcterms:creator>
    <dcterms:creator>Emanuele Ghedini</dcterms:creator>
    <owl:versionInfo>1.0.0-beta</owl:versionInfo>
    <dcterms:contributor>University of Bologna, IT</dcterms:contributor>
    <dcterms:creator>Gerhard Goldbeck</dcterms:creator>
    <dcterms:contributor>Access, DE</dcterms:contributor>
    <rdf:type rdf:resource="http://www.w3.org/2002/07/owl#Ontology"/>
    <dcterms:title xml:lang="en">European Materials &amp; Modelling Ontology</dcterms:title>
    <dcterms:publisher>EMMC ASBL</dcterms:publisher>
    <dcterms:abstract xml:lang="en">European Materials &amp; Modelling Ontology (EMMO)

EMMO is a multidisciplinary effort to develop a standard representational framework (the ontology) based on current materials modelling knowledge, including physical sciences, analytical philosophy and information and communication technologies.

It provides the connection between the physical world, materials characterisation world and materials modelling world.

EMMO is released under a Creative Commons license Attribution 4.0 International (CC BY 4.0).</dcterms:abstract>
    <owl:versionIRI rdf:resource="http://emmo.info/emmo/1.0.0-beta/middle/metrology"/>
    <dcterms:contributor>Goldbeck Consulting Ltd (UK)</dcterms:contributor>
    <dcterms:creator>Georg Schmitz</dcterms:creator>
    <rdfs:comment xml:lang="en">Contacts:
Gerhard Goldbeck
Goldbeck Consulting Ltd (UK)
email: gerhard@goldbeck-consulting.com

Emanuele Ghedini
University of Bologna (IT)
email: emanuele.ghedini@unibo.it</rdfs:comment>
    <dcterms:contributor>SINTEF, NO</dcterms:contributor>
  </rdf:Description>
  <rdf:Description rdf:nodeID="fe24a777e3fd743f986ce83488d2cf30bb5">
    <owl:someValuesFrom rdf:resource="http://emmo.info/emmo#EMMO_54ee6b5e_5261_44a8_86eb_5717e7fdb9d0"/>
    <owl:onProperty rdf:nodeID="fe24a777e3fd743f986ce83488d2cf30bb6"/>
    <rdf:type rdf:resource="http://www.w3.org/2002/07/owl#Restriction"/>
  </rdf:Description>
  <rdf:Description rdf:about="http://emmo.info/emmo#EMMO_ba882f34_0d71_4e4f_9d92_0c076c633a2c">
    <rdfs:comment xml:lang="en">According to the SI brochure counting does not automatically qualify a quantity as an amount of substance.

This quantity is used only to describe the outcome of a counting process, without regard of the type of entities.

"There are also some quantities that cannot be described in terms of the seven base quantities of the SI, but have the nature of a count. Examples are a number of molecules, a number of cellular or biomolecular entities (for example copies of a particular nucleic acid sequence), or degeneracy in quantum mechanics. Counting quantities are also quantities with the associated unit one."</rdfs:comment>
    <EMMO_b432d2d5_25f4_4165_99c5_5935a7763c1a>1, 
i, 
π,
the number of protons in the nucleus of an atom</EMMO_b432d2d5_25f4_4165_99c5_5935a7763c1a>
    <rdf:type rdf:resource="http://www.w3.org/2002/07/owl#Class"/>
    <skos:prefLabel xml:lang="en">PureNumberQuantity</skos:prefLabel>
    <rdfs:subClassOf rdf:resource="http://emmo.info/emmo#EMMO_a66427d1_9932_4363_9ec5_7d91f2bfda1e"/>
    <EMMO_967080e5_2f42_4eb2_a3a9_c58143e835f9 xml:lang="en">A pure number, typically the number of something.</EMMO_967080e5_2f42_4eb2_a3a9_c58143e835f9>
    <EMMO_de178b12_5d35_4bca_8efa_a4193162571d>T0 L0 M0 I0 Θ0 N0 J0</EMMO_de178b12_5d35_4bca_8efa_a4193162571d>
  </rdf:Description>
  <rdf:Description rdf:about="http://emmo.info/emmo#EMMO_28fbea28_2204_4613_87ff_6d877b855fcd">
    <skos:prefLabel xml:lang="en">Array</skos:prefLabel>
    <rdf:type rdf:resource="http://www.w3.org/2002/07/owl#Class"/>
    <rdfs:subClassOf rdf:resource="http://emmo.info/emmo#EMMO_54ee6b5e_5261_44a8_86eb_5717e7fdb9d0"/>
  </rdf:Description>
  <rdf:Description rdf:about="http://emmo.info/emmo#EMMO_c84c6752_6d64_48cc_9500_e54a3c34898d">
    <rdf:type rdf:resource="http://www.w3.org/2002/07/owl#AnnotationProperty"/>
    <rdfs:comment xml:lang="en">URL to corresponding Wikipedia entry.</rdfs:comment>
    <skos:prefLabel xml:lang="en">wikipediaEntry</skos:prefLabel>
    <rdfs:range rdf:resource="http://www.w3.org/2001/XMLSchema#anyURI"/>
    <rdfs:subPropertyOf rdf:resource="http://www.w3.org/2000/01/rdf-schema#seeAlso"/>
    <rdfs:seeAlso>https://www.wikipedia.org/</rdfs:seeAlso>
  </rdf:Description>
  <rdf:Description rdf:about="http://purl.org/dc/terms/contributor">
    <rdf:type rdf:resource="http://www.w3.org/2002/07/owl#AnnotationProperty"/>
  </rdf:Description>
  <rdf:Description rdf:about="http://emmo.info/emmo#EMMO_3e309118_e8b7_4021_80f4_642d2df65d94">
    <rdfs:subClassOf rdf:resource="http://emmo.info/emmo#EMMO_0c576e13_4ee7_4f3d_bfe9_1614243df018"/>
    <skos:prefLabel xml:lang="en">Line</skos:prefLabel>
    <rdf:type rdf:resource="http://www.w3.org/2002/07/owl#Class"/>
  </rdf:Description>
  <rdf:Description rdf:about="http://emmo.info/emmo#EMMO_649bf97b_4397_4005_90d9_219755d92e34">
    <rdfs:subClassOf rdf:resource="http://emmo.info/emmo#EMMO_49267eba_5548_4163_8f36_518d65b583f9"/>
    <rdf:type rdf:resource="http://www.w3.org/2002/07/owl#Class"/>
    <rdfs:comment xml:lang="en">A 'Perceptual' is a meta-object, meaning that is addressed by the ontologist (the meta-interpreter) in a meta-semiotic process occurring outside the EMMO.

A 'Perceptual' becomes an 'Object', when it is part of a 'Semiotic' process described by the ontologist through the EMMO.</rdfs:comment>
    <rdfs:comment xml:lang="en">'Perceptual' includes real world objects that:
- are part of a communication system (e.g. words, speech, alphabets)
- are not part of a communication system, but can be identified and referred by an interpreter</rdfs:comment>
    <rdfs:comment xml:lang="en">This class is the most general superclass for the categorization of real world objects that are recognizable by an interpreter (agent).

A 'Perceptual' can stand for something else in a semiotic process (acting as sign or as object). 

However, a perceptual is not necessarily a 'Sign' (e.g. a line sketched on a blackboard is a recognizable 'Perceptual' but it may stand for nothing).</rdfs:comment>
    <skos:prefLabel xml:lang="en">Perceptual</skos:prefLabel>
    <rdfs:comment xml:lang="en">From Latin perceptiō (“a receiving or collecting, perception, comprehension”), from perceptus (“perceived, observed”).</rdfs:comment>
    <EMMO_b432d2d5_25f4_4165_99c5_5935a7763c1a xml:lang="en">A line scratched on a surface.
A sound.
A smell.
The word 'cat' and the sound of the word 'cat' (the first one is graphical and the second acoustical).</EMMO_b432d2d5_25f4_4165_99c5_5935a7763c1a>
    <EMMO_b432d2d5_25f4_4165_99c5_5935a7763c1a xml:lang="en">The meta-semiotic process:
I see a cloud in the sky. Since I'm an EMMO ontologist, I create an individual named Cloud under the 'Impression' class.  This semiotic process occurs at meta-level: it's how I use the EMMO as tool for a direct representation of the world.

The semiotic process within EMMO:
My friend looks at the same cloud and says: "It is an elephant".
I use the EMMO to record this experience by declaring:
    - my friend as MyFriend individual, belonging to 'Interpreter' classes
    - the sound of the word "elephant" as an acoustical impression individual named ElephantWord, belonging to 'Impression'
    - a relation hasSign between Cloud and ElephantWord, that makes ElephantWord also belonging to 'Sign' class and Cloud belonging also to 'Object' class
    - a 'Semiosis' individual called MyFriendElephantCloud that hasParticipant: Cloud, ElephantWord and MyFriend, respectively as object, sign and interpreter.</EMMO_b432d2d5_25f4_4165_99c5_5935a7763c1a>
    <EMMO_967080e5_2f42_4eb2_a3a9_c58143e835f9 xml:lang="en">A 'Physical' which stands for a real world object that can stimulate a perception (e.g. a mental impression, the excitation of a sensor) to an interpreter (human or non-human).</EMMO_967080e5_2f42_4eb2_a3a9_c58143e835f9>
  </rdf:Description>
  <rdf:Description rdf:about="http://emmo.info/emmo#EMMO_d7f11b34_a121_4519_87c0_aa754f1c4737">
    <EMMO_1f1b164d_ec6a_4faa_8d5e_88bda62316cc>http://qudt.org/vocab/unit/WB</EMMO_1f1b164d_ec6a_4faa_8d5e_88bda62316cc>
    <rdfs:comment xml:lang="en">Measurement unit for magnetic flux.</rdfs:comment>
    <rdfs:subClassOf rdf:nodeID="f05bdaa1e617a4bccafc519daf7bf4785b140"/>
    <rdfs:subClassOf rdf:nodeID="f05bdaa1e617a4bccafc519daf7bf4785b139"/>
    <skos:prefLabel xml:lang="en">Weber</skos:prefLabel>
    <EMMO_fe015383_afb3_44a6_ae86_043628697aa2>https://doi.org/10.1351/goldbook.W06666</EMMO_fe015383_afb3_44a6_ae86_043628697aa2>
    <rdf:type rdf:resource="http://www.w3.org/2002/07/owl#Class"/>
  </rdf:Description>
  <rdf:Description rdf:about="http://emmo.info/emmo#EMMO_ba380bc6_2bfd_4f11_94c7_b3cbaafd1631">
    <rdf:type rdf:resource="http://www.w3.org/2002/07/owl#Class"/>
    <EMMO_967080e5_2f42_4eb2_a3a9_c58143e835f9 xml:lang="en">Inverse of the magnetic flux quantum.</EMMO_967080e5_2f42_4eb2_a3a9_c58143e835f9>
    <skos:prefLabel xml:lang="en">JosephsonConstant</skos:prefLabel>
    <rdfs:comment xml:lang="en">The DBpedia definition (http://dbpedia.org/page/Magnetic_flux_quantum) is outdated as May 20, 2019. It is now an exact quantity.</rdfs:comment>
    <EMMO_de178b12_5d35_4bca_8efa_a4193162571d>T+2 L-1 M-1 I+1 Θ0 N0 J0</EMMO_de178b12_5d35_4bca_8efa_a4193162571d>
    <EMMO_1f1b164d_ec6a_4faa_8d5e_88bda62316cc>http://qudt.org/vocab/constant/JosephsonConstant</EMMO_1f1b164d_ec6a_4faa_8d5e_88bda62316cc>
    <EMMO_a9b3d04c_7ceb_40a2_b8d3_28d514a770a8>https://physics.nist.gov/cgi-bin/cuu/Value?kjos</EMMO_a9b3d04c_7ceb_40a2_b8d3_28d514a770a8>
    <rdfs:subClassOf rdf:resource="http://emmo.info/emmo#EMMO_f2ca6dd0_0e5f_4392_a92d_cafdae6cfc95"/>
  </rdf:Description>
  <rdf:Description rdf:nodeID="fa691b5894b3543efa24f9838ff46c3eab7">
    <rdf:rest rdf:nodeID="fa691b5894b3543efa24f9838ff46c3eab8"/>
    <rdf:type rdf:resource="http://www.w3.org/1999/02/22-rdf-syntax-ns#List"/>
    <rdf:first rdf:resource="http://emmo.info/emmo#EMMO_35d2e130_6e01_41ed_94f7_00b333d46cf9"/>
  </rdf:Description>
  <rdf:Description rdf:about="http://emmo.info/emmo#EMMO_12d4ba9b_2f89_4ea3_b206_cd376f96c875">
    <skos:prefLabel xml:lang="en">Heat</skos:prefLabel>
    <rdfs:comment xml:lang="en">Heat is energy in transfer to or from a thermodynamic system, by mechanisms other than thermodynamic work or transfer of matter.</rdfs:comment>
    <rdfs:subClassOf rdf:resource="http://emmo.info/emmo#EMMO_31ec09ba_1713_42cb_83c7_b38bf6f9ced2"/>
    <EMMO_fe015383_afb3_44a6_ae86_043628697aa2>https://doi.org/10.1351/goldbook.H02752</EMMO_fe015383_afb3_44a6_ae86_043628697aa2>
    <EMMO_de178b12_5d35_4bca_8efa_a4193162571d>T-2 L+2 M+1 I0 Θ0 N0 J0</EMMO_de178b12_5d35_4bca_8efa_a4193162571d>
    <rdf:type rdf:resource="http://www.w3.org/2002/07/owl#Class"/>
    <EMMO_1f1b164d_ec6a_4faa_8d5e_88bda62316cc>http://qudt.org/vocab/quantitykind/Heat</EMMO_1f1b164d_ec6a_4faa_8d5e_88bda62316cc>
  </rdf:Description>
  <rdf:Description rdf:nodeID="f05bdaa1e617a4bccafc519daf7bf4785b73">
    <rdf:first rdf:resource="http://emmo.info/emmo#EMMO_e1981c25_7c55_4020_aa7a_d2e14ced86d4"/>
    <rdf:type rdf:resource="http://www.w3.org/1999/02/22-rdf-syntax-ns#List"/>
    <rdf:rest rdf:nodeID="f05bdaa1e617a4bccafc519daf7bf4785b74"/>
  </rdf:Description>
  <rdf:Description rdf:about="http://emmo.info/emmo/middle/semiotics">
    <dcterms:publisher>EMMC ASBL</dcterms:publisher>
    <rdfs:comment xml:lang="en">The EMMO requires FacT++ reasoner plugin in order to visualize all inferences and class hierarchy (ctrl+R hotkey in Protege).</rdfs:comment>
    <dcterms:title xml:lang="en">European Materials &amp; Modelling Ontology</dcterms:title>
    <dcterms:creator>Gerhard Goldbeck</dcterms:creator>
    <dcterms:creator>Georg Schmitz</dcterms:creator>
    <owl:versionInfo>1.0.0-beta</owl:versionInfo>
    <dcterms:contributor>Fraunhofer IWM, DE</dcterms:contributor>
    <rdfs:comment xml:lang="en">Contacts:
Gerhard Goldbeck
Goldbeck Consulting Ltd (UK)
email: gerhard@goldbeck-consulting.com

Emanuele Ghedini
University of Bologna (IT)
email: emanuele.ghedini@unibo.it</rdfs:comment>
    <dcterms:abstract xml:lang="en">European Materials &amp; Modelling Ontology (EMMO)

EMMO is a multidisciplinary effort to develop a standard representational framework (the ontology) based on current materials modelling knowledge, including physical sciences, analytical philosophy and information and communication technologies.

It provides the connection between the physical world, materials characterisation world and materials modelling world.

EMMO is released under a Creative Commons license Attribution 4.0 International (CC BY 4.0).</dcterms:abstract>
    <dcterms:contributor>University of Bologna, IT</dcterms:contributor>
    <dcterms:creator>Adham Hashibon</dcterms:creator>
    <rdf:type rdf:resource="http://www.w3.org/2002/07/owl#Ontology"/>
    <dcterms:creator>Emanuele Ghedini</dcterms:creator>
    <owl:versionIRI rdf:resource="http://emmo.info/emmo/1.0.0-beta/middle/semiotics"/>
    <dcterms:contributor>Access, DE</dcterms:contributor>
    <dcterms:contributor>SINTEF, NO</dcterms:contributor>
    <dcterms:creator>Jesper Friis</dcterms:creator>
    <dcterms:contributor>Goldbeck Consulting Ltd (UK)</dcterms:contributor>
    <dcterms:license>https://creativecommons.org/licenses/by/4.0/legalcode</dcterms:license>
  </rdf:Description>
  <rdf:Description rdf:about="http://emmo.info/emmo#EMMO_2337e25c_3c60_43fc_a8f9_b11a3f974291">
    <EMMO_967080e5_2f42_4eb2_a3a9_c58143e835f9 xml:lang="en">The generic EMMO semiotical relation.</EMMO_967080e5_2f42_4eb2_a3a9_c58143e835f9>
    <skos:prefLabel xml:lang="en">semiotical</skos:prefLabel>
    <rdf:type rdf:resource="http://www.w3.org/2002/07/owl#ObjectProperty"/>
    <rdfs:subPropertyOf rdf:resource="http://emmo.info/emmo#EMMO_ec2472ae_cf4a_46a5_8555_1556f5a6c3c5"/>
  </rdf:Description>
  <rdf:Description rdf:about="http://emmo.info/emmo#EMMO_04b3300c_98bd_42dc_a3b5_e6c29d69f1ac">
    <EMMO_de178b12_5d35_4bca_8efa_a4193162571d>T0 L0 M0 I0 Θ0 N0 J0</EMMO_de178b12_5d35_4bca_8efa_a4193162571d>
    <skos:altLabel xml:lang="en">MoleFraction</skos:altLabel>
    <rdf:type rdf:resource="http://www.w3.org/2002/07/owl#Class"/>
    <rdfs:subClassOf rdf:resource="http://emmo.info/emmo#EMMO_faab3f84_e475_4a46_af9c_7d249f0b9aef"/>
    <EMMO_1f1b164d_ec6a_4faa_8d5e_88bda62316cc>http://qudt.org/vocab/quantitykind/MoleFraction</EMMO_1f1b164d_ec6a_4faa_8d5e_88bda62316cc>
    <EMMO_70fe84ff_99b6_4206_a9fc_9a8931836d84 xml:lang="en">The amount of a constituent divided by the total amount of all constituents in a mixture.</EMMO_70fe84ff_99b6_4206_a9fc_9a8931836d84>
    <EMMO_fe015383_afb3_44a6_ae86_043628697aa2>https://doi.org/10.1351/goldbook.A00296</EMMO_fe015383_afb3_44a6_ae86_043628697aa2>
    <EMMO_e55f2d7c_9893_48cd_b4a4_fdf38253bd20>http://www.ontology-of-units-of-measure.org/resource/om-2/AmountOfSubstanceFraction</EMMO_e55f2d7c_9893_48cd_b4a4_fdf38253bd20>
    <skos:prefLabel xml:lang="en">AmountFraction</skos:prefLabel>
    <rdfs:subClassOf rdf:nodeID="ffcb99037244f48d590430c228d02afdbb3"/>
    <EMMO_6dd685dd_1895_46e4_b227_be9f7d643c25>http://dbpedia.org/page/Mole_fraction</EMMO_6dd685dd_1895_46e4_b227_be9f7d643c25>
  </rdf:Description>
  <rdf:Description rdf:about="http://emmo.info/emmo#EMMO_314ba716_2d3d_4462_9a4f_d3419ae1df43">
    <rdfs:subClassOf rdf:nodeID="f05bdaa1e617a4bccafc519daf7bf4785b31"/>
    <rdfs:subClassOf rdf:nodeID="f05bdaa1e617a4bccafc519daf7bf4785b32"/>
    <EMMO_70fe84ff_99b6_4206_a9fc_9a8931836d84 xml:lang="en">The second, symbol s, is the SI unit of time. It is defined by taking the fixed numerical value of the caesium frequency ∆νCs, the unperturbed ground-state hyperfine transition frequency of the caesium 133 atom, to be 9192631770 when expressed in the unit Hz, which is equal to s−1.</EMMO_70fe84ff_99b6_4206_a9fc_9a8931836d84>
    <EMMO_1f1b164d_ec6a_4faa_8d5e_88bda62316cc>http://qudt.org/vocab/unit/SEC</EMMO_1f1b164d_ec6a_4faa_8d5e_88bda62316cc>
    <rdf:type rdf:resource="http://www.w3.org/2002/07/owl#Class"/>
    <skos:prefLabel xml:lang="en">Second</skos:prefLabel>
    <EMMO_fe015383_afb3_44a6_ae86_043628697aa2>https://doi.org/10.1351/goldbook.S05513</EMMO_fe015383_afb3_44a6_ae86_043628697aa2>
  </rdf:Description>
  <rdf:Description rdf:nodeID="f05bdaa1e617a4bccafc519daf7bf4785b100">
    <rdf:type rdf:resource="http://www.w3.org/2002/07/owl#Restriction"/>
    <owl:hasValue>J</owl:hasValue>
    <owl:onProperty rdf:resource="http://emmo.info/emmo#EMMO_23b579e1_8088_45b5_9975_064014026c42"/>
  </rdf:Description>
  <rdf:Description rdf:about="http://emmo.info/emmo#EMMO_44fc8c60_7a9c_49af_a046_e1878c88862c">
    <rdfs:subClassOf rdf:resource="http://emmo.info/emmo#EMMO_ed4af7ae_63a2_497e_bb88_2309619ea405"/>
    <EMMO_6dd685dd_1895_46e4_b227_be9f7d643c25>http://dbpedia.org/page/Electron_rest_mass</EMMO_6dd685dd_1895_46e4_b227_be9f7d643c25>
    <skos:prefLabel xml:lang="en">ElectronMass</skos:prefLabel>
    <EMMO_de178b12_5d35_4bca_8efa_a4193162571d>T0 L0 M+1 I0 Θ0 N0 J0</EMMO_de178b12_5d35_4bca_8efa_a4193162571d>
    <EMMO_1f1b164d_ec6a_4faa_8d5e_88bda62316cc>http://qudt.org/vocab/constant/ElectronMass</EMMO_1f1b164d_ec6a_4faa_8d5e_88bda62316cc>
    <EMMO_fe015383_afb3_44a6_ae86_043628697aa2>https://doi.org/10.1351/goldbook.E02008</EMMO_fe015383_afb3_44a6_ae86_043628697aa2>
    <rdfs:subClassOf rdf:resource="http://emmo.info/emmo#EMMO_3f15d200_c97b_42c8_8ac0_d81d150361e2"/>
    <EMMO_a9b3d04c_7ceb_40a2_b8d3_28d514a770a8>https://physics.nist.gov/cgi-bin/cuu/Value?me</EMMO_a9b3d04c_7ceb_40a2_b8d3_28d514a770a8>
    <rdfs:comment xml:lang="en">The rest mass of an electron.</rdfs:comment>
    <rdf:type rdf:resource="http://www.w3.org/2002/07/owl#Class"/>
  </rdf:Description>
  <rdf:Description rdf:nodeID="f05bdaa1e617a4bccafc519daf7bf4785b61">
    <rdf:first rdf:resource="http://emmo.info/emmo#EMMO_254472c6_3dbd_4f02_bc43_571389cd281f"/>
    <rdf:rest rdf:nodeID="f05bdaa1e617a4bccafc519daf7bf4785b62"/>
    <rdf:type rdf:resource="http://www.w3.org/1999/02/22-rdf-syntax-ns#List"/>
  </rdf:Description>
  <rdf:Description rdf:about="http://emmo.info/emmo#EMMO_5c003f53_20a2_4bd7_8445_58187e582578">
    <skos:prefLabel xml:lang="en">LuminousEfficacyDimension</skos:prefLabel>
    <owl:equivalentClass rdf:nodeID="fe0b20157736f4a31909181349b2e6219b22"/>
    <rdf:type rdf:resource="http://www.w3.org/2002/07/owl#Class"/>
    <rdfs:subClassOf rdf:resource="http://emmo.info/emmo#EMMO_9895a1b4_f0a5_4167_ac5e_97db40b8bfcc"/>
  </rdf:Description>
  <rdf:Description rdf:about="http://emmo.info/emmo#EMMO_27c530c4_dfcd_486e_b324_54ad4448cd26">
    <EMMO_fe015383_afb3_44a6_ae86_043628697aa2>https://doi.org/10.1351/goldbook.N00350</EMMO_fe015383_afb3_44a6_ae86_043628697aa2>
    <rdfs:comment xml:lang="en">Ångström is not mentioned in the SI system and deprecated by the International Bureau of Weights and Measures (BIPM).

Dispite of that, it is often used in the natural sciences and technology.</rdfs:comment>
    <rdfs:subClassOf rdf:nodeID="ffcb99037244f48d590430c228d02afdbb11"/>
    <EMMO_70fe84ff_99b6_4206_a9fc_9a8931836d84 xml:lang="en">Measure of length defined as 1e-10 metres.</EMMO_70fe84ff_99b6_4206_a9fc_9a8931836d84>
    <rdfs:subClassOf rdf:nodeID="ffcb99037244f48d590430c228d02afdbb12"/>
    <rdf:type rdf:resource="http://www.w3.org/2002/07/owl#Class"/>
    <skos:prefLabel xml:lang="en">Ångström</skos:prefLabel>
    <skos:altLabel xml:lang="en">Angstrom</skos:altLabel>
    <EMMO_6dd685dd_1895_46e4_b227_be9f7d643c25>http://dbpedia.org/page/%C3%85ngstr%C3%B6m</EMMO_6dd685dd_1895_46e4_b227_be9f7d643c25>
    <EMMO_c84c6752_6d64_48cc_9500_e54a3c34898d>https://en.wikipedia.org/wiki/Angstrom</EMMO_c84c6752_6d64_48cc_9500_e54a3c34898d>
    <rdfs:subClassOf rdf:resource="http://emmo.info/emmo#EMMO_591e02fd_8d37_45a6_9d11_bb21cef391a0"/>
    <EMMO_1f1b164d_ec6a_4faa_8d5e_88bda62316cc>http://qudt.org/vocab/unit/ANGSTROM</EMMO_1f1b164d_ec6a_4faa_8d5e_88bda62316cc>
  </rdf:Description>
  <rdf:Description rdf:about="http://emmo.info/emmo#EMMO_43776fc9_d712_4571_85f0_72183678039a">
    <EMMO_6dd685dd_1895_46e4_b227_be9f7d643c25>http://dbpedia.org/page/Momentum</EMMO_6dd685dd_1895_46e4_b227_be9f7d643c25>
    <EMMO_de178b12_5d35_4bca_8efa_a4193162571d>T-1 L+1 M+1 I0 Θ0 N0 J0</EMMO_de178b12_5d35_4bca_8efa_a4193162571d>
    <EMMO_fe015383_afb3_44a6_ae86_043628697aa2>https://doi.org/10.1351/goldbook.M04007</EMMO_fe015383_afb3_44a6_ae86_043628697aa2>
    <rdfs:subClassOf rdf:resource="http://emmo.info/emmo#EMMO_2946d40b_24a1_47fa_8176_e3f79bb45064"/>
    <rdf:type rdf:resource="http://www.w3.org/2002/07/owl#Class"/>
    <skos:prefLabel xml:lang="en">Momentum</skos:prefLabel>
    <rdfs:comment xml:lang="en">Product of mass and velocity.</rdfs:comment>
    <EMMO_1f1b164d_ec6a_4faa_8d5e_88bda62316cc>http://qudt.org/vocab/quantitykind/Momentum</EMMO_1f1b164d_ec6a_4faa_8d5e_88bda62316cc>
  </rdf:Description>
  <rdf:Description rdf:about="http://emmo.info/emmo#EMMO_6f4d704a_a7c6_4c07_b8a7_ea0bab04128f">
    <EMMO_b432d2d5_25f4_4165_99c5_5935a7763c1a xml:lang="en">Unit for solid angle.</EMMO_b432d2d5_25f4_4165_99c5_5935a7763c1a>
    <rdf:type rdf:resource="http://www.w3.org/2002/07/owl#Class"/>
    <skos:prefLabel xml:lang="en">AreaFractionUnit</skos:prefLabel>
    <EMMO_967080e5_2f42_4eb2_a3a9_c58143e835f9 xml:lang="en">Unit for quantities of dimension one that are the fraction of two areas.</EMMO_967080e5_2f42_4eb2_a3a9_c58143e835f9>
    <rdfs:subClassOf rdf:resource="http://emmo.info/emmo#EMMO_c2f5ee66_579c_44c6_a2e9_fa2eaa9fa4da"/>
  </rdf:Description>
  <rdf:Description rdf:nodeID="f8fb83657cd5f496db3c2b94baf326f26b34">
    <rdf:type rdf:resource="http://www.w3.org/1999/02/22-rdf-syntax-ns#List"/>
    <rdf:rest rdf:nodeID="f8fb83657cd5f496db3c2b94baf326f26b35"/>
    <rdf:first rdf:resource="http://emmo.info/emmo#EMMO_216f448e_cdbc_4aeb_a529_7a5fe7fc38bb"/>
  </rdf:Description>
  <rdf:Description rdf:about="http://emmo.info/emmo#EMMO_8159c26a_494b_4fa0_9959_10888f152298">
    <EMMO_fe015383_afb3_44a6_ae86_043628697aa2>https://doi.org/10.1351/goldbook.A00297</EMMO_fe015383_afb3_44a6_ae86_043628697aa2>
    <skos:prefLabel xml:lang="en">AmountOfSubstance</skos:prefLabel>
    <EMMO_1f1b164d_ec6a_4faa_8d5e_88bda62316cc>http://qudt.org/vocab/quantitykind/AmountOfSubstance</EMMO_1f1b164d_ec6a_4faa_8d5e_88bda62316cc>
    <EMMO_967080e5_2f42_4eb2_a3a9_c58143e835f9 xml:lang="en">The number of elementary entities present.</EMMO_967080e5_2f42_4eb2_a3a9_c58143e835f9>
    <rdf:type rdf:resource="http://www.w3.org/2002/07/owl#Class"/>
    <rdfs:comment xml:lang="en">"In the name “amount of substance”, the word “substance” will typically be replaced by words to specify the substance concerned in any particular application, for example “amount of hydrogen chloride, HCl”, or “amount of benzene, C6H6 ”. It is important to give a precise definition of the entity involved (as emphasized in the definition of the mole); this should preferably be done by specifying the molecular chemical formula of the material involved. Although the word “amount” has a more general dictionary definition, the abbreviation of the full name “amount of substance” to “amount” may be used for brevity."

-- SI Brochure</rdfs:comment>
    <EMMO_6dd685dd_1895_46e4_b227_be9f7d643c25>http://dbpedia.org/page/Amount_of_substance</EMMO_6dd685dd_1895_46e4_b227_be9f7d643c25>
    <EMMO_de178b12_5d35_4bca_8efa_a4193162571d>T0 L0 M0 I0 Θ0 N+1 J0</EMMO_de178b12_5d35_4bca_8efa_a4193162571d>
  </rdf:Description>
  <rdf:Description rdf:about="http://emmo.info/emmo#EMMO_6795a4b8_ffd0_4588_a581_a9413fe49cac">
    <rdfs:subClassOf rdf:resource="http://emmo.info/emmo#EMMO_3ee80521_3c23_4dd1_935d_9d522614a3e2"/>
    <EMMO_c84c6752_6d64_48cc_9500_e54a3c34898d>https://en.wikipedia.org/wiki/Non-SI_units_mentioned_in_the_SI</EMMO_c84c6752_6d64_48cc_9500_e54a3c34898d>
    <EMMO_967080e5_2f42_4eb2_a3a9_c58143e835f9 xml:lang="en">Non-SI units mentioned in the SI.</EMMO_967080e5_2f42_4eb2_a3a9_c58143e835f9>
    <owl:disjointUnionOf rdf:nodeID="ffcb99037244f48d590430c228d02afdbb17"/>
    <rdf:type rdf:resource="http://www.w3.org/2002/07/owl#Class"/>
    <skos:prefLabel xml:lang="en">SIAcceptedSpecialUnit</skos:prefLabel>
    <rdfs:comment xml:lang="en">This is a list of units that are not defined as part of the International System of Units (SI), but are otherwise mentioned in the SI brouchure, because either the General Conference on Weights and Measures (CGPM) accepts their use as being multiples or submultiples of SI-units, they have important contemporary application worldwide, or are otherwise commonly encountered worldwide.</rdfs:comment>
  </rdf:Description>
  <rdf:Description rdf:about="http://emmo.info/emmo#EMMO_e37ac288_aa60_415a_8cb7_c375724ac8e1">
    <skos:prefLabel xml:lang="en">Acceleration</skos:prefLabel>
    <rdfs:comment xml:lang="en">Derivative of velocity with respect to time.</rdfs:comment>
    <EMMO_1f1b164d_ec6a_4faa_8d5e_88bda62316cc>http://qudt.org/vocab/quantitykind/Acceleration</EMMO_1f1b164d_ec6a_4faa_8d5e_88bda62316cc>
    <EMMO_fe015383_afb3_44a6_ae86_043628697aa2>https://doi.org/10.1351/goldbook.A00051</EMMO_fe015383_afb3_44a6_ae86_043628697aa2>
    <rdf:type rdf:resource="http://www.w3.org/2002/07/owl#Class"/>
    <EMMO_6dd685dd_1895_46e4_b227_be9f7d643c25>http://dbpedia.org/page/Acceleration</EMMO_6dd685dd_1895_46e4_b227_be9f7d643c25>
    <EMMO_de178b12_5d35_4bca_8efa_a4193162571d>T-2 L+1 M0 I0 Θ0 N0 J0</EMMO_de178b12_5d35_4bca_8efa_a4193162571d>
    <rdfs:subClassOf rdf:resource="http://emmo.info/emmo#EMMO_2946d40b_24a1_47fa_8176_e3f79bb45064"/>
  </rdf:Description>
  <rdf:Description rdf:nodeID="f05bdaa1e617a4bccafc519daf7bf4785b39">
    <rdf:type rdf:resource="http://www.w3.org/1999/02/22-rdf-syntax-ns#List"/>
    <rdf:rest rdf:nodeID="f05bdaa1e617a4bccafc519daf7bf4785b40"/>
    <rdf:first rdf:resource="http://emmo.info/emmo#EMMO_7db11dbf_a643_464a_9b56_07eabcc3e9c5"/>
  </rdf:Description>
  <rdf:Description rdf:about="http://emmo.info/emmo#EMMO_d1917609_db5e_4b8a_9b76_ef1d6f860a81">
    <skos:prefLabel xml:lang="en">Stress</skos:prefLabel>
    <rdfs:comment xml:lang="en">Measure of the internal forces that neighboring particles of a continuous material exert on each other.</rdfs:comment>
    <EMMO_1f1b164d_ec6a_4faa_8d5e_88bda62316cc>http://qudt.org/vocab/quantitykind/Stress</EMMO_1f1b164d_ec6a_4faa_8d5e_88bda62316cc>
    <rdf:type rdf:resource="http://www.w3.org/2002/07/owl#Class"/>
    <rdfs:subClassOf rdf:resource="http://emmo.info/emmo#EMMO_2946d40b_24a1_47fa_8176_e3f79bb45064"/>
    <EMMO_de178b12_5d35_4bca_8efa_a4193162571d>T-2 L-1 M+1 I0 Θ0 N0 J0</EMMO_de178b12_5d35_4bca_8efa_a4193162571d>
    <EMMO_6dd685dd_1895_46e4_b227_be9f7d643c25>http://dbpedia.org/page/Stress_(mechanics)</EMMO_6dd685dd_1895_46e4_b227_be9f7d643c25>
    <rdfs:comment xml:lang="en">Force per unit oriented surface area .</rdfs:comment>
  </rdf:Description>
  <rdf:Description rdf:about="http://emmo.info/emmo#EMMO_c8d084ad_f88e_4596_8e4d_982c6655ce6f">
    <rdf:type rdf:resource="http://www.w3.org/2002/07/owl#Class"/>
    <skos:prefLabel xml:lang="en">PowerDimension</skos:prefLabel>
    <owl:equivalentClass rdf:nodeID="fe0b20157736f4a31909181349b2e6219b33"/>
    <rdfs:subClassOf rdf:resource="http://emmo.info/emmo#EMMO_9895a1b4_f0a5_4167_ac5e_97db40b8bfcc"/>
  </rdf:Description>
  <rdf:Description rdf:about="http://emmo.info/emmo/middle/perceptual">
    <dcterms:contributor>Access, DE</dcterms:contributor>
    <rdf:type rdf:resource="http://www.w3.org/2002/07/owl#Ontology"/>
    <owl:versionIRI rdf:resource="http://emmo.info/emmo/1.0.0-beta/middle/perceptual"/>
    <dcterms:license>https://creativecommons.org/licenses/by/4.0/legalcode</dcterms:license>
    <dcterms:contributor>SINTEF, NO</dcterms:contributor>
    <dcterms:creator>Jesper Friis</dcterms:creator>
    <dcterms:contributor>Goldbeck Consulting Ltd (UK)</dcterms:contributor>
    <dcterms:publisher>EMMC ASBL</dcterms:publisher>
    <rdfs:comment xml:lang="en">The EMMO requires FacT++ reasoner plugin in order to visualize all inferences and class hierarchy (ctrl+R hotkey in Protege).</rdfs:comment>
    <dcterms:title xml:lang="en">European Materials &amp; Modelling Ontology</dcterms:title>
    <dcterms:creator>Gerhard Goldbeck</dcterms:creator>
    <dcterms:contributor>Fraunhofer IWM, DE</dcterms:contributor>
    <rdfs:comment xml:lang="en">Contacts:
Gerhard Goldbeck
Goldbeck Consulting Ltd (UK)
email: gerhard@goldbeck-consulting.com

Emanuele Ghedini
University of Bologna (IT)
email: emanuele.ghedini@unibo.it</rdfs:comment>
    <owl:versionInfo>1.0.0-beta</owl:versionInfo>
    <dcterms:creator>Georg Schmitz</dcterms:creator>
    <dcterms:creator>Adham Hashibon</dcterms:creator>
    <dcterms:abstract xml:lang="en">European Materials &amp; Modelling Ontology (EMMO)

EMMO is a multidisciplinary effort to develop a standard representational framework (the ontology) based on current materials modelling knowledge, including physical sciences, analytical philosophy and information and communication technologies.

It provides the connection between the physical world, materials characterisation world and materials modelling world.

EMMO is released under a Creative Commons license Attribution 4.0 International (CC BY 4.0).</dcterms:abstract>
    <dcterms:contributor>University of Bologna, IT</dcterms:contributor>
    <dcterms:creator>Emanuele Ghedini</dcterms:creator>
  </rdf:Description>
  <rdf:Description rdf:about="http://emmo.info/emmo#EMMO_d893d373_b579_4867_841e_1c2b31a8d2c6">
    <rdfs:subPropertyOf rdf:resource="http://emmo.info/emmo#EMMO_6703954e_34c4_4a15_a9e7_f313760ae1a8"/>
    <rdf:type rdf:resource="http://www.w3.org/2002/07/owl#ObjectProperty"/>
    <rdf:type rdf:resource="http://www.w3.org/2002/07/owl#SymmetricProperty"/>
    <skos:prefLabel xml:lang="en">hasOverlapWith</skos:prefLabel>
  </rdf:Description>
  <rdf:Description rdf:about="http://emmo.info/emmo#EMMO_09b9021b_f97b_43eb_b83d_0a764b472bc2">
    <rdf:type rdf:resource="http://www.w3.org/2002/07/owl#Class"/>
    <rdfs:subClassOf rdf:resource="http://emmo.info/emmo#EMMO_2946d40b_24a1_47fa_8176_e3f79bb45064"/>
    <EMMO_de178b12_5d35_4bca_8efa_a4193162571d>T-3 L+2 M+1 I0 Θ0 N0 J0</EMMO_de178b12_5d35_4bca_8efa_a4193162571d>
    <EMMO_967080e5_2f42_4eb2_a3a9_c58143e835f9 xml:lang="en">Rate of transfer of energy per unit time.</EMMO_967080e5_2f42_4eb2_a3a9_c58143e835f9>
    <skos:prefLabel xml:lang="en">Power</skos:prefLabel>
    <EMMO_fe015383_afb3_44a6_ae86_043628697aa2>https://doi.org/10.1351/goldbook.P04792</EMMO_fe015383_afb3_44a6_ae86_043628697aa2>
    <EMMO_6dd685dd_1895_46e4_b227_be9f7d643c25>http://dbpedia.org/page/Power_(physics)</EMMO_6dd685dd_1895_46e4_b227_be9f7d643c25>
    <EMMO_1f1b164d_ec6a_4faa_8d5e_88bda62316cc>http://qudt.org/vocab/quantitykind/Power</EMMO_1f1b164d_ec6a_4faa_8d5e_88bda62316cc>
  </rdf:Description>
  <rdf:Description rdf:about="http://emmo.info/emmo#EMMO_4bc29b0f_8fcc_4026_a291_f9774a66d9b8">
    <EMMO_b432d2d5_25f4_4165_99c5_5935a7763c1a xml:lang="en">y = f(x)</EMMO_b432d2d5_25f4_4165_99c5_5935a7763c1a>
    <EMMO_967080e5_2f42_4eb2_a3a9_c58143e835f9 xml:lang="en">A function defined using functional notation.</EMMO_967080e5_2f42_4eb2_a3a9_c58143e835f9>
    <rdfs:subClassOf rdf:resource="http://emmo.info/emmo#EMMO_29afdf54_90ae_4c98_8845_fa9ea3f143a8"/>
    <skos:prefLabel xml:lang="en">FunctionDefinition</skos:prefLabel>
    <rdf:type rdf:resource="http://www.w3.org/2002/07/owl#Class"/>
  </rdf:Description>
  <rdf:Description rdf:about="http://emmo.info/emmo#EMMO_5525a055_dda5_4556_8b91_f0d22fa676cc">
    <skos:prefLabel xml:lang="en">license</skos:prefLabel>
    <rdfs:subPropertyOf rdf:resource="http://www.w3.org/2000/01/rdf-schema#comment"/>
    <rdf:type rdf:resource="http://www.w3.org/2002/07/owl#AnnotationProperty"/>
    <owl:deprecated>Replaced by dcterms:license</owl:deprecated>
  </rdf:Description>
  <rdf:Description rdf:about="http://emmo.info/emmo#EMMO_faf79f53_749d_40b2_807c_d34244c192f4">
    <skos:prefLabel xml:lang="en">hasNumericalData</skos:prefLabel>
    <rdfs:subPropertyOf rdf:resource="http://www.w3.org/2002/07/owl#topDataProperty"/>
    <rdfs:domain rdf:resource="http://emmo.info/emmo#EMMO_4ce76d7f_03f8_45b6_9003_90052a79bfaa"/>
    <rdf:type rdf:resource="http://www.w3.org/2002/07/owl#DatatypeProperty"/>
  </rdf:Description>
  <rdf:Description rdf:about="http://emmo.info/emmo#EMMO_50a44256_9dc5_434b_bad4_74a4d9a29989">
    <rdfs:subClassOf rdf:resource="http://emmo.info/emmo#EMMO_2946d40b_24a1_47fa_8176_e3f79bb45064"/>
    <EMMO_fe015383_afb3_44a6_ae86_043628697aa2>https://doi.org/10.1351/goldbook.P04819</EMMO_fe015383_afb3_44a6_ae86_043628697aa2>
    <rdf:type rdf:resource="http://www.w3.org/2002/07/owl#Class"/>
    <EMMO_6dd685dd_1895_46e4_b227_be9f7d643c25>http://dbpedia.org/page/Pressure</EMMO_6dd685dd_1895_46e4_b227_be9f7d643c25>
    <skos:prefLabel xml:lang="en">Pressure</skos:prefLabel>
    <EMMO_1f1b164d_ec6a_4faa_8d5e_88bda62316cc>http://qudt.org/vocab/quantitykind/Pressure</EMMO_1f1b164d_ec6a_4faa_8d5e_88bda62316cc>
    <EMMO_967080e5_2f42_4eb2_a3a9_c58143e835f9 xml:lang="en">The force applied perpendicular to the surface of an object per unit area over which that force is distributed.</EMMO_967080e5_2f42_4eb2_a3a9_c58143e835f9>
    <EMMO_de178b12_5d35_4bca_8efa_a4193162571d>T-2 L-1 M+1 I0 Θ0 N0 J0</EMMO_de178b12_5d35_4bca_8efa_a4193162571d>
  </rdf:Description>
  <rdf:Description rdf:nodeID="ffcb99037244f48d590430c228d02afdbb5">
    <owl:onProperty rdf:resource="http://emmo.info/emmo#EMMO_23b579e1_8088_45b5_9975_064014026c42"/>
    <rdf:type rdf:resource="http://www.w3.org/2002/07/owl#Restriction"/>
    <owl:hasValue>au</owl:hasValue>
  </rdf:Description>
  <rdf:Description rdf:nodeID="f8fb83657cd5f496db3c2b94baf326f26b27">
    <owl:qualifiedCardinality rdf:datatype="http://www.w3.org/2001/XMLSchema#nonNegativeInteger">1</owl:qualifiedCardinality>
    <rdf:type rdf:resource="http://www.w3.org/2002/07/owl#Restriction"/>
    <owl:onProperty rdf:resource="http://emmo.info/emmo#EMMO_bed1d005_b04e_4a90_94cf_02bc678a8569"/>
    <owl:onClass rdf:resource="http://emmo.info/emmo#EMMO_9895a1b4_f0a5_4167_ac5e_97db40b8bfcc"/>
  </rdf:Description>
  <rdf:Description rdf:about="http://emmo.info/emmo#EMMO_7c8007b0_58a7_4486_bf1c_4772852caca0">
    <rdfs:comment xml:lang="en">Electric current divided by the cross-sectional area it is passing through.</rdfs:comment>
    <skos:prefLabel xml:lang="en">CurrentDensity</skos:prefLabel>
    <EMMO_1f1b164d_ec6a_4faa_8d5e_88bda62316cc>http://qudt.org/vocab/quantitykind/ElectricCurrentDensity</EMMO_1f1b164d_ec6a_4faa_8d5e_88bda62316cc>
    <EMMO_fe015383_afb3_44a6_ae86_043628697aa2>https://doi.org/10.1351/goldbook.E01928</EMMO_fe015383_afb3_44a6_ae86_043628697aa2>
    <rdf:type rdf:resource="http://www.w3.org/2002/07/owl#Class"/>
    <EMMO_de178b12_5d35_4bca_8efa_a4193162571d>T0 L-2 M0 I+1 Θ0 N0 J0</EMMO_de178b12_5d35_4bca_8efa_a4193162571d>
    <rdfs:subClassOf rdf:resource="http://emmo.info/emmo#EMMO_2946d40b_24a1_47fa_8176_e3f79bb45064"/>
    <EMMO_6dd685dd_1895_46e4_b227_be9f7d643c25>http://dbpedia.org/page/Current_density</EMMO_6dd685dd_1895_46e4_b227_be9f7d643c25>
  </rdf:Description>
  <rdf:Description rdf:about="http://emmo.info/emmo#EMMO_f2d5d3ad_2e00_417f_8849_686f3988d929">
    <skos:prefLabel xml:lang="en">MeasurementInstrument</skos:prefLabel>
    <rdfs:subClassOf rdf:resource="http://emmo.info/emmo#EMMO_1b52ee70_121e_4d8d_8419_3f97cd0bd89c"/>
    <rdf:type rdf:resource="http://www.w3.org/2002/07/owl#Class"/>
  </rdf:Description>
  <rdf:Description rdf:about="http://emmo.info/emmo#EMMO_4f5c7c54_1c63_4d17_b12b_ea0792c2b187">
    <owl:equivalentClass rdf:nodeID="fe0b20157736f4a31909181349b2e6219b16"/>
    <skos:prefLabel xml:lang="en">SpeedDimension</skos:prefLabel>
    <rdf:type rdf:resource="http://www.w3.org/2002/07/owl#Class"/>
    <rdfs:subClassOf rdf:resource="http://emmo.info/emmo#EMMO_9895a1b4_f0a5_4167_ac5e_97db40b8bfcc"/>
  </rdf:Description>
  <rdf:Description rdf:nodeID="f05bdaa1e617a4bccafc519daf7bf4785b9">
    <owl:onProperty rdf:nodeID="f05bdaa1e617a4bccafc519daf7bf4785b10"/>
    <rdf:type rdf:resource="http://www.w3.org/2002/07/owl#Restriction"/>
    <owl:allValuesFrom rdf:nodeID="f05bdaa1e617a4bccafc519daf7bf4785b11"/>
  </rdf:Description>
  <rdf:Description rdf:about="http://emmo.info/emmo#EMMO_29072ec4_ffcb_42fb_bdc7_26f05a2e9873">
    <EMMO_705f27ae_954c_4f13_98aa_18473fc52b25 xml:lang="en">From Latin vacuus, “empty”.</EMMO_705f27ae_954c_4f13_98aa_18473fc52b25>
    <EMMO_967080e5_2f42_4eb2_a3a9_c58143e835f9 xml:lang="en">A 'Item' that has no 'Physical' parts.</EMMO_967080e5_2f42_4eb2_a3a9_c58143e835f9>
    <rdf:type rdf:resource="http://www.w3.org/2002/07/owl#Class"/>
    <rdfs:subClassOf rdf:nodeID="fc2fcd8f8eb3649bcbbaff76ba54058acb3"/>
    <skos:prefLabel xml:lang="en">Void</skos:prefLabel>
    <rdfs:comment xml:lang="en">The void concept is paramount for the representation of physical systems according to quantum theory.</rdfs:comment>
  </rdf:Description>
  <rdf:Description rdf:about="http://emmo.info/emmo#EMMO_624d72ee_e676_4470_9434_c22b4190d3d5">
    <EMMO_70fe84ff_99b6_4206_a9fc_9a8931836d84 xml:lang="en">Product of force and displacement.</EMMO_70fe84ff_99b6_4206_a9fc_9a8931836d84>
    <EMMO_6dd685dd_1895_46e4_b227_be9f7d643c25>http://dbpedia.org/page/Work_(physics)</EMMO_6dd685dd_1895_46e4_b227_be9f7d643c25>
    <rdfs:subClassOf rdf:resource="http://emmo.info/emmo#EMMO_31ec09ba_1713_42cb_83c7_b38bf6f9ced2"/>
    <EMMO_6dd685dd_1895_46e4_b227_be9f7d643c25>http://dbpedia.org/page/Heat</EMMO_6dd685dd_1895_46e4_b227_be9f7d643c25>
    <EMMO_de178b12_5d35_4bca_8efa_a4193162571d>T-2 L+2 M+1 I0 Θ0 N0 J0</EMMO_de178b12_5d35_4bca_8efa_a4193162571d>
    <EMMO_fe015383_afb3_44a6_ae86_043628697aa2>https://doi.org/10.1351/goldbook.W06684</EMMO_fe015383_afb3_44a6_ae86_043628697aa2>
    <skos:prefLabel xml:lang="en">Work</skos:prefLabel>
    <EMMO_1f1b164d_ec6a_4faa_8d5e_88bda62316cc>http://qudt.org/vocab/quantitykind/Work</EMMO_1f1b164d_ec6a_4faa_8d5e_88bda62316cc>
    <rdf:type rdf:resource="http://www.w3.org/2002/07/owl#Class"/>
  </rdf:Description>
  <rdf:Description rdf:about="http://emmo.info/emmo/top/annotations">
    <dcterms:license>https://creativecommons.org/licenses/by/4.0/legalcode</dcterms:license>
    <dcterms:contributor>Fraunhofer IWM, DE</dcterms:contributor>
    <owl:versionIRI rdf:resource="http://emmo.info/emmo/1.0.0-beta/top/annotations"/>
    <rdfs:comment xml:lang="en">The EMMO requires FacT++ reasoner plugin in order to visualize all inferences and class hierarchy (ctrl+R hotkey in Protege).</rdfs:comment>
    <dcterms:creator>Emanuele Ghedini</dcterms:creator>
    <rdfs:comment xml:lang="en">Contacts:
Gerhard Goldbeck
Goldbeck Consulting Ltd (UK)
email: gerhard@goldbeck-consulting.com

Emanuele Ghedini
University of Bologna (IT)
email: emanuele.ghedini@unibo.it</rdfs:comment>
    <dcterms:contributor>SINTEF, NO</dcterms:contributor>
    <owl:versionInfo>1.0.0-beta</owl:versionInfo>
    <dcterms:contributor>University of Bologna, IT</dcterms:contributor>
    <dcterms:contributor>Goldbeck Consulting Ltd (UK)</dcterms:contributor>
    <dcterms:creator>Gerhard Goldbeck</dcterms:creator>
    <dcterms:contributor>Access, DE</dcterms:contributor>
    <rdf:type rdf:resource="http://www.w3.org/2002/07/owl#Ontology"/>
    <dcterms:title xml:lang="en">European Materials &amp; Modelling Ontology</dcterms:title>
    <dcterms:publisher>EMMC ASBL</dcterms:publisher>
    <dcterms:abstract xml:lang="en">European Materials &amp; Modelling Ontology (EMMO)

EMMO is a multidisciplinary effort to develop a standard representational framework (the ontology) based on current materials modelling knowledge, including physical sciences, analytical philosophy and information and communication technologies.

It provides the connection between the physical world, materials characterisation world and materials modelling world.

EMMO is released under a Creative Commons license Attribution 4.0 International (CC BY 4.0).</dcterms:abstract>
    <dcterms:creator>Adham Hashibon</dcterms:creator>
    <dcterms:creator>Georg Schmitz</dcterms:creator>
    <dcterms:creator>Jesper Friis</dcterms:creator>
  </rdf:Description>
  <rdf:Description rdf:about="http://emmo.info/emmo#EMMO_e0edfb9e_9a96_4fae_b942_831ffe27b84a">
    <EMMO_b432d2d5_25f4_4165_99c5_5935a7763c1a xml:lang="en">Rain, spray.</EMMO_b432d2d5_25f4_4165_99c5_5935a7763c1a>
    <EMMO_967080e5_2f42_4eb2_a3a9_c58143e835f9 xml:lang="en">A coarse dispersion of liquid in a gas continuum phase.</EMMO_967080e5_2f42_4eb2_a3a9_c58143e835f9>
    <rdf:type rdf:resource="http://www.w3.org/2002/07/owl#Class"/>
    <skos:prefLabel xml:lang="en">GasLiquidSuspension</skos:prefLabel>
    <rdfs:subClassOf rdf:resource="http://emmo.info/emmo#EMMO_04f2a2d5_e799_4692_a654_420e76f5acc1"/>
  </rdf:Description>
  <rdf:Description rdf:nodeID="f627ff42579444148ae27fcacfb5f8528b12">
    <rdf:first rdf:resource="http://emmo.info/emmo#EMMO_939483b1_0148_43d1_8b35_851d2cd5d939"/>
    <rdf:type rdf:resource="http://www.w3.org/1999/02/22-rdf-syntax-ns#List"/>
    <rdf:rest rdf:resource="http://www.w3.org/1999/02/22-rdf-syntax-ns#nil"/>
  </rdf:Description>
  <rdf:Description rdf:nodeID="ffcb99037244f48d590430c228d02afdbb25">
    <rdf:type rdf:resource="http://www.w3.org/1999/02/22-rdf-syntax-ns#List"/>
    <rdf:first rdf:resource="http://emmo.info/emmo#EMMO_b41515a9_28d8_4d78_8165_74b2fc72f89e"/>
    <rdf:rest rdf:nodeID="ffcb99037244f48d590430c228d02afdbb26"/>
  </rdf:Description>
  <rdf:Description rdf:about="http://emmo.info/emmo#EMMO_a9201b2f_e6de_442a_b3a6_d292a5820bc5">
    <EMMO_1f1b164d_ec6a_4faa_8d5e_88bda62316cc>http://qudt.org/vocab/unit/FARAD</EMMO_1f1b164d_ec6a_4faa_8d5e_88bda62316cc>
    <rdf:type rdf:resource="http://www.w3.org/2002/07/owl#Class"/>
    <rdfs:comment xml:lang="en">Measurement unit for electric capacitance.</rdfs:comment>
    <skos:prefLabel xml:lang="en">Farad</skos:prefLabel>
    <EMMO_fe015383_afb3_44a6_ae86_043628697aa2>https://doi.org/10.1351/goldbook.F02320</EMMO_fe015383_afb3_44a6_ae86_043628697aa2>
    <rdfs:subClassOf rdf:nodeID="f05bdaa1e617a4bccafc519daf7bf4785b122"/>
    <rdfs:subClassOf rdf:nodeID="f05bdaa1e617a4bccafc519daf7bf4785b121"/>
  </rdf:Description>
  <rdf:Description rdf:about="http://emmo.info/emmo#EMMO_1eed0732_e3f1_4b2c_a9c4_b4e75eeb5895">
    <skos:prefLabel xml:lang="en">Variable</skos:prefLabel>
    <rdfs:subClassOf rdf:nodeID="fe24a777e3fd743f986ce83488d2cf30bb5"/>
    <EMMO_b432d2d5_25f4_4165_99c5_5935a7763c1a xml:lang="en">x
k</EMMO_b432d2d5_25f4_4165_99c5_5935a7763c1a>
    <rdf:type rdf:resource="http://www.w3.org/2002/07/owl#Class"/>
    <EMMO_967080e5_2f42_4eb2_a3a9_c58143e835f9 xml:lang="en">A 'Variable' is a symbolic object that stands for a numerical defined 'Mathematical' object like e.g. a number, a vector, a matrix.</EMMO_967080e5_2f42_4eb2_a3a9_c58143e835f9>
    <rdfs:subClassOf rdf:resource="http://emmo.info/emmo#EMMO_54ee6b5e_5261_44a8_86eb_5717e7fdb9d0"/>
  </rdf:Description>
  <rdf:Description rdf:about="http://emmo.info/emmo/middle/reductionistic">
    <dcterms:abstract xml:lang="en">European Materials &amp; Modelling Ontology (EMMO)

EMMO is a multidisciplinary effort to develop a standard representational framework (the ontology) based on current materials modelling knowledge, including physical sciences, analytical philosophy and information and communication technologies.

It provides the connection between the physical world, materials characterisation world and materials modelling world.

EMMO is released under a Creative Commons license Attribution 4.0 International (CC BY 4.0).</dcterms:abstract>
    <rdfs:comment xml:lang="en">Contacts:
Gerhard Goldbeck
Goldbeck Consulting Ltd (UK)
email: gerhard@goldbeck-consulting.com

Emanuele Ghedini
University of Bologna (IT)
email: emanuele.ghedini@unibo.it</rdfs:comment>
    <dcterms:contributor>Goldbeck Consulting Ltd (UK)</dcterms:contributor>
    <dcterms:contributor>SINTEF, NO</dcterms:contributor>
    <dcterms:license>https://creativecommons.org/licenses/by/4.0/legalcode</dcterms:license>
    <owl:versionIRI rdf:resource="http://emmo.info/emmo/1.0.0-beta/middle/reductionistic"/>
    <owl:versionInfo>1.0.0-beta</owl:versionInfo>
    <rdfs:comment xml:lang="en">The EMMO requires FacT++ reasoner plugin in order to visualize all inferences and class hierarchy (ctrl+R hotkey in Protege).</rdfs:comment>
    <dcterms:creator>Emanuele Ghedini</dcterms:creator>
    <dcterms:contributor>Fraunhofer IWM, DE</dcterms:contributor>
    <dcterms:creator>Gerhard Goldbeck</dcterms:creator>
    <dcterms:contributor>Access, DE</dcterms:contributor>
    <dcterms:title xml:lang="en">European Materials &amp; Modelling Ontology</dcterms:title>
    <dcterms:creator>Adham Hashibon</dcterms:creator>
    <dcterms:contributor>University of Bologna, IT</dcterms:contributor>
    <rdf:type rdf:resource="http://www.w3.org/2002/07/owl#Ontology"/>
    <dcterms:publisher>EMMC ASBL</dcterms:publisher>
    <dcterms:creator>Georg Schmitz</dcterms:creator>
    <dcterms:creator>Jesper Friis</dcterms:creator>
  </rdf:Description>
  <rdf:Description rdf:about="http://emmo.info/emmo#EMMO_df6eeb01_1b41_4bd8_9257_a04fbd7cf000">
    <skos:prefLabel xml:lang="en">Mole</skos:prefLabel>
    <EMMO_1f1b164d_ec6a_4faa_8d5e_88bda62316cc>http://qudt.org/vocab/unit/MOL</EMMO_1f1b164d_ec6a_4faa_8d5e_88bda62316cc>
    <rdfs:subClassOf rdf:nodeID="f05bdaa1e617a4bccafc519daf7bf4785b151"/>
    <EMMO_fe015383_afb3_44a6_ae86_043628697aa2>https://doi.org/10.1351/goldbook.M03980</EMMO_fe015383_afb3_44a6_ae86_043628697aa2>
    <rdf:type rdf:resource="http://www.w3.org/2002/07/owl#Class"/>
    <EMMO_70fe84ff_99b6_4206_a9fc_9a8931836d84 xml:lang="en">The mole, symbol mol, is the SI unit of amount of substance. One mole contains exactly 6.022 140 76 × 1023 elementary entities. This number is the fixed numerical value of the Avogadro constant, NA, when expressed in the unit mol−1 and is called the Avogadro number. The amount of substance, symbol n, of a system is a measure of the number of specified elementary entities. An elementary entity may be an atom, a molecule, an ion, an electron, any other particle or specified group of particles.</EMMO_70fe84ff_99b6_4206_a9fc_9a8931836d84>
    <rdfs:subClassOf rdf:nodeID="f05bdaa1e617a4bccafc519daf7bf4785b152"/>
  </rdf:Description>
  <rdf:Description rdf:about="http://emmo.info/emmo#EMMO_98ada9d8_f1c8_4f13_99b5_d890f5354152">
    <skos:prefLabel xml:lang="en">Physicalistic</skos:prefLabel>
    <owl:equivalentClass rdf:nodeID="fea11ca01461e402d8f697c19c5d8de88b12"/>
    <rdf:type rdf:resource="http://www.w3.org/2002/07/owl#Class"/>
    <rdfs:subClassOf rdf:resource="http://emmo.info/emmo#EMMO_49267eba_5548_4163_8f36_518d65b583f9"/>
    <EMMO_967080e5_2f42_4eb2_a3a9_c58143e835f9 xml:lang="en">The perspective for which physical objects are categorized only by concepts coming from applied physical sciences.</EMMO_967080e5_2f42_4eb2_a3a9_c58143e835f9>
  </rdf:Description>
  <rdf:Description rdf:nodeID="ffcb99037244f48d590430c228d02afdbb42">
    <owl:someValuesFrom rdf:resource="http://emmo.info/emmo#EMMO_3227b821_26a5_4c7c_9c01_5c24483e0bd0"/>
    <rdf:type rdf:resource="http://www.w3.org/2002/07/owl#Restriction"/>
    <owl:onProperty rdf:resource="http://emmo.info/emmo#EMMO_bed1d005_b04e_4a90_94cf_02bc678a8569"/>
  </rdf:Description>
  <rdf:Description rdf:nodeID="fe24a777e3fd743f986ce83488d2cf30bb12">
    <owl:onDataRange rdf:resource="http://www.w3.org/2001/XMLSchema#boolean"/>
    <owl:onProperty rdf:resource="http://emmo.info/emmo#EMMO_faf79f53_749d_40b2_807c_d34244c192f4"/>
    <rdf:type rdf:resource="http://www.w3.org/2002/07/owl#Restriction"/>
    <owl:qualifiedCardinality rdf:datatype="http://www.w3.org/2001/XMLSchema#nonNegativeInteger">1</owl:qualifiedCardinality>
  </rdf:Description>
  <rdf:Description rdf:nodeID="f05bdaa1e617a4bccafc519daf7bf4785b188">
    <owl:hasValue>S</owl:hasValue>
    <owl:onProperty rdf:resource="http://emmo.info/emmo#EMMO_23b579e1_8088_45b5_9975_064014026c42"/>
    <rdf:type rdf:resource="http://www.w3.org/2002/07/owl#Restriction"/>
  </rdf:Description>
  <rdf:Description rdf:about="http://emmo.info/emmo#EMMO_5eedba4d_105b_44d8_b1bc_e33606276ea2">
    <rdfs:comment xml:lang="en">Factor by which the phase velocity of light is reduced in a medium.</rdfs:comment>
    <EMMO_de178b12_5d35_4bca_8efa_a4193162571d>T0 L0 M0 I0 Θ0 N0 J0</EMMO_de178b12_5d35_4bca_8efa_a4193162571d>
    <rdf:type rdf:resource="http://www.w3.org/2002/07/owl#Class"/>
    <rdfs:subClassOf rdf:resource="http://emmo.info/emmo#EMMO_faab3f84_e475_4a46_af9c_7d249f0b9aef"/>
    <EMMO_1f1b164d_ec6a_4faa_8d5e_88bda62316cc>http://qudt.org/vocab/quantitykind/RefractiveIndex</EMMO_1f1b164d_ec6a_4faa_8d5e_88bda62316cc>
    <EMMO_fe015383_afb3_44a6_ae86_043628697aa2>https://doi.org/10.1351/goldbook.R05240</EMMO_fe015383_afb3_44a6_ae86_043628697aa2>
    <rdfs:subClassOf rdf:nodeID="ffcb99037244f48d590430c228d02afdbb16"/>
    <EMMO_6dd685dd_1895_46e4_b227_be9f7d643c25>http://dbpedia.org/page/Refractive_index</EMMO_6dd685dd_1895_46e4_b227_be9f7d643c25>
    <skos:prefLabel xml:lang="en">RefractiveIndex</skos:prefLabel>
  </rdf:Description>
  <rdf:Description rdf:about="http://emmo.info/emmo#EMMO_3df10765_f6ff_4c9e_be3d_10b1809d78bd">
    <EMMO_de178b12_5d35_4bca_8efa_a4193162571d>T-2 L+2 M0 I0 Θ0 N0 J0</EMMO_de178b12_5d35_4bca_8efa_a4193162571d>
    <skos:prefLabel xml:lang="en">DoseEquivalent</skos:prefLabel>
    <rdfs:subClassOf rdf:resource="http://emmo.info/emmo#EMMO_2946d40b_24a1_47fa_8176_e3f79bb45064"/>
    <rdf:type rdf:resource="http://www.w3.org/2002/07/owl#Class"/>
    <EMMO_1f1b164d_ec6a_4faa_8d5e_88bda62316cc>http://qudt.org/vocab/quantitykind/DoseEquivalent</EMMO_1f1b164d_ec6a_4faa_8d5e_88bda62316cc>
    <EMMO_6dd685dd_1895_46e4_b227_be9f7d643c25>http://dbpedia.org/page/Energy</EMMO_6dd685dd_1895_46e4_b227_be9f7d643c25>
    <EMMO_fe015383_afb3_44a6_ae86_043628697aa2>https://doi.org/10.1351/goldbook.E02101</EMMO_fe015383_afb3_44a6_ae86_043628697aa2>
    <EMMO_967080e5_2f42_4eb2_a3a9_c58143e835f9 xml:lang="en">A dose quantity used in the International Commission on Radiological Protection (ICRP) system of radiological protection.</EMMO_967080e5_2f42_4eb2_a3a9_c58143e835f9>
  </rdf:Description>
  <rdf:Description rdf:about="http://emmo.info/emmo#EMMO_b803f122_4acb_4064_9d71_c1e5fd091fc9">
    <owl:equivalentClass rdf:nodeID="fa691b5894b3543efa24f9838ff46c3eab9"/>
    <rdfs:comment xml:lang="en">Semiotic subclasse are defined using Peirce's semiotic theory.

"Namely, a sign is something, A, which brings something, B, its interpretant sign determined or created by it, into the same sort of correspondence with something, C, its object, as that in which itself stands to C." (Peirce 1902, NEM 4, 20–21).

The triadic elements:
- 'sign': the sign A (e.g. a name)
- 'interpretant': the sign B as the effects of the sign A on the interpreter (e.g. the mental concept of what a name means)
- 'object': the object C (e.g. the entity to which the sign A and B refer to)

This class includes also the 'interpeter' i.e. the entity that connects the 'sign' to the 'object'</rdfs:comment>
    <rdf:type rdf:resource="http://www.w3.org/2002/07/owl#Class"/>
    <skos:prefLabel xml:lang="en">Semiotic</skos:prefLabel>
    <rdfs:subClassOf rdf:nodeID="fa691b5894b3543efa24f9838ff46c3eab13"/>
    <EMMO_967080e5_2f42_4eb2_a3a9_c58143e835f9 xml:lang="en">The class of individuals that stands for semiotic objects, i.e. objects that take part on a semiotic process.</EMMO_967080e5_2f42_4eb2_a3a9_c58143e835f9>
    <rdfs:subClassOf rdf:resource="http://emmo.info/emmo#EMMO_49804605_c0fe_4538_abda_f70ba1dc8a5d"/>
  </rdf:Description>
  <rdf:Description rdf:about="http://emmo.info/emmo#EMMO_acd1a504_ca32_4f30_86ad_0b62cea5bc02">
    <EMMO_b432d2d5_25f4_4165_99c5_5935a7763c1a xml:lang="en">Arbitrary amount-of-substance concentration of lutropin in a given sample of plasma (WHO international standard 80/552): 5.0 International Unit/l</EMMO_b432d2d5_25f4_4165_99c5_5935a7763c1a>
    <skos:prefLabel xml:lang="en">StandardUnit</skos:prefLabel>
    <EMMO_967080e5_2f42_4eb2_a3a9_c58143e835f9 xml:lang="en">A reference unit provided by a reference material.
International vocabulary of metrology (VIM)</EMMO_967080e5_2f42_4eb2_a3a9_c58143e835f9>
    <rdfs:subClassOf rdf:resource="http://emmo.info/emmo#EMMO_18ce5200_00f5_45bb_8c6f_6fb128cd41ae"/>
    <rdf:type rdf:resource="http://www.w3.org/2002/07/owl#Class"/>
  </rdf:Description>
  <rdf:Description rdf:about="http://emmo.info/emmo#EMMO_02e894c3_b793_4197_b120_3442e08f58d1">
    <rdfs:subClassOf rdf:resource="http://emmo.info/emmo#EMMO_9895a1b4_f0a5_4167_ac5e_97db40b8bfcc"/>
    <owl:equivalentClass rdf:nodeID="fe0b20157736f4a31909181349b2e6219b1"/>
    <rdf:type rdf:resource="http://www.w3.org/2002/07/owl#Class"/>
    <skos:prefLabel xml:lang="en">TimeDimension</skos:prefLabel>
  </rdf:Description>
  <rdf:Description rdf:about="http://emmo.info/emmo#EMMO_00dd79e0_31a6_427e_9b9c_90f3097e4a96">
    <EMMO_fe015383_afb3_44a6_ae86_043628697aa2>https://doi.org/10.1351/goldbook.D01514</EMMO_fe015383_afb3_44a6_ae86_043628697aa2>
    <EMMO_1f1b164d_ec6a_4faa_8d5e_88bda62316cc>http://qudt.org/vocab/unit/Dalton</EMMO_1f1b164d_ec6a_4faa_8d5e_88bda62316cc>
    <EMMO_6dd685dd_1895_46e4_b227_be9f7d643c25>http://dbpedia.org/page/Unified_atomic_mass_unit</EMMO_6dd685dd_1895_46e4_b227_be9f7d643c25>
    <rdfs:subClassOf rdf:nodeID="ffcb99037244f48d590430c228d02afdbb1"/>
    <skos:prefLabel xml:lang="en">Dalton</skos:prefLabel>
    <EMMO_70fe84ff_99b6_4206_a9fc_9a8931836d84 xml:lang="en">One dalton is defined as one twelfth of the mass of an unbound neutral atom of carbon-12 in its nuclear and electronic ground state.</EMMO_70fe84ff_99b6_4206_a9fc_9a8931836d84>
    <rdf:type rdf:resource="http://www.w3.org/2002/07/owl#Class"/>
    <rdfs:subClassOf rdf:resource="http://emmo.info/emmo#EMMO_591e02fd_8d37_45a6_9d11_bb21cef391a0"/>
    <rdfs:subClassOf rdf:nodeID="ffcb99037244f48d590430c228d02afdbb2"/>
  </rdf:Description>
  <rdf:Description rdf:nodeID="fea11ca01461e402d8f697c19c5d8de88b22">
    <rdf:rest rdf:nodeID="fea11ca01461e402d8f697c19c5d8de88b23"/>
    <rdf:first rdf:resource="http://emmo.info/emmo#EMMO_7db59e56_f68b_48b7_ae99_891c35ae5c3b"/>
    <rdf:type rdf:resource="http://www.w3.org/1999/02/22-rdf-syntax-ns#List"/>
  </rdf:Description>
  <rdf:Description rdf:about="http://emmo.info/emmo#EMMO_a8eb87b5_4d10_4137_a75c_e04ee59ca095">
    <EMMO_967080e5_2f42_4eb2_a3a9_c58143e835f9 xml:lang="en">Volume of a constituent of a mixture divided by the sum of volumes of all constituents prior to mixing.</EMMO_967080e5_2f42_4eb2_a3a9_c58143e835f9>
    <EMMO_6dd685dd_1895_46e4_b227_be9f7d643c25 xml:lang="en">http://dbpedia.org/page/Volume_fraction</EMMO_6dd685dd_1895_46e4_b227_be9f7d643c25>
    <EMMO_fe015383_afb3_44a6_ae86_043628697aa2 xml:lang="en">https://doi.org/10.1351/goldbook.V06643</EMMO_fe015383_afb3_44a6_ae86_043628697aa2>
    <skos:prefLabel xml:lang="en">VolumeFraction</skos:prefLabel>
    <EMMO_e55f2d7c_9893_48cd_b4a4_fdf38253bd20 xml:lang="en">http://www.ontology-of-units-of-measure.org/resource/om-2/VolumeFraction</EMMO_e55f2d7c_9893_48cd_b4a4_fdf38253bd20>
    <EMMO_1f1b164d_ec6a_4faa_8d5e_88bda62316cc>http://qudt.org/vocab/quantitykind/VolumeFraction</EMMO_1f1b164d_ec6a_4faa_8d5e_88bda62316cc>
    <rdfs:subClassOf rdf:nodeID="ffcb99037244f48d590430c228d02afdbb39"/>
    <rdfs:subClassOf rdf:resource="http://emmo.info/emmo#EMMO_faab3f84_e475_4a46_af9c_7d249f0b9aef"/>
    <EMMO_de178b12_5d35_4bca_8efa_a4193162571d>T0 L0 M0 I0 Θ0 N0 J0</EMMO_de178b12_5d35_4bca_8efa_a4193162571d>
    <rdf:type rdf:resource="http://www.w3.org/2002/07/owl#Class"/>
  </rdf:Description>
  <rdf:Description rdf:about="http://emmo.info/emmo#EMMO_1d8b370b_c672_4d0c_964e_eaafcbf2f51f">
    <rdfs:subClassOf rdf:nodeID="f05bdaa1e617a4bccafc519daf7bf4785b16"/>
    <rdfs:subClassOf rdf:nodeID="f05bdaa1e617a4bccafc519daf7bf4785b13"/>
    <skos:prefLabel xml:lang="en">Deka</skos:prefLabel>
    <rdf:type rdf:resource="http://www.w3.org/2002/07/owl#Class"/>
  </rdf:Description>
  <rdf:Description rdf:nodeID="f05bdaa1e617a4bccafc519daf7bf4785b76">
    <rdf:type rdf:resource="http://www.w3.org/2002/07/owl#Restriction"/>
    <owl:onProperty rdf:resource="http://emmo.info/emmo#EMMO_bed1d005_b04e_4a90_94cf_02bc678a8569"/>
    <owl:someValuesFrom rdf:resource="http://emmo.info/emmo#EMMO_7610efb8_c7c6_4684_abc1_774783c62472"/>
  </rdf:Description>
  <rdf:Description rdf:about="http://emmo.info/emmo#EMMO_aaf9dd7f_0474_40d0_9606_02def8515249">
    <EMMO_967080e5_2f42_4eb2_a3a9_c58143e835f9 xml:lang="en">The effectiveness of a force to produce rotation about an axis, measured by the product of the force and the perpendicular distance from the line of action of the force to the axis.</EMMO_967080e5_2f42_4eb2_a3a9_c58143e835f9>
    <EMMO_fe015383_afb3_44a6_ae86_043628697aa2>https://doi.org/10.1351/goldbook.T06400</EMMO_fe015383_afb3_44a6_ae86_043628697aa2>
    <rdfs:subClassOf rdf:resource="http://emmo.info/emmo#EMMO_2946d40b_24a1_47fa_8176_e3f79bb45064"/>
    <rdf:type rdf:resource="http://www.w3.org/2002/07/owl#Class"/>
    <rdfs:comment xml:lang="en">Even though torque has the same physical dimension as energy, it is not of the same kind and can not be measured with energy units like joule or electron volt.</rdfs:comment>
    <EMMO_1f1b164d_ec6a_4faa_8d5e_88bda62316cc>http://qudt.org/vocab/quantitykind/Torque</EMMO_1f1b164d_ec6a_4faa_8d5e_88bda62316cc>
    <EMMO_6dd685dd_1895_46e4_b227_be9f7d643c25>http://dbpedia.org/page/Torque</EMMO_6dd685dd_1895_46e4_b227_be9f7d643c25>
    <EMMO_e55f2d7c_9893_48cd_b4a4_fdf38253bd20>http://www.ontology-of-units-of-measure.org/resource/om-2/Torque</EMMO_e55f2d7c_9893_48cd_b4a4_fdf38253bd20>
    <EMMO_50c298c2_55a2_4068_b3ac_4e948c33181f>http://www.electropedia.org/iev/iev.nsf/display?openform&amp;ievref=113-03-26</EMMO_50c298c2_55a2_4068_b3ac_4e948c33181f>
    <EMMO_de178b12_5d35_4bca_8efa_a4193162571d>T-2 L+2 M+1 I0 Θ0 N0 J0</EMMO_de178b12_5d35_4bca_8efa_a4193162571d>
    <skos:prefLabel xml:lang="en">Torque</skos:prefLabel>
  </rdf:Description>
  <rdf:Description rdf:about="http://emmo.info/emmo#EMMO_04f2a2d5_e799_4692_a654_420e76f5acc1">
    <skos:prefLabel xml:lang="en">Gas</skos:prefLabel>
    <rdfs:subClassOf rdf:resource="http://emmo.info/emmo#EMMO_87ac88ff_8379_4f5a_8c7b_424a8fff1ee8"/>
    <rdf:type rdf:resource="http://www.w3.org/2002/07/owl#Class"/>
    <EMMO_967080e5_2f42_4eb2_a3a9_c58143e835f9 xml:lang="en">Gas is a compressible fluid, a state of matter that has no fixed shape and no fixed volume.</EMMO_967080e5_2f42_4eb2_a3a9_c58143e835f9>
  </rdf:Description>
  <rdf:Description rdf:about="http://emmo.info/emmo#EMMO_ae15fb4f_8e4d_41de_a0f9_3997f89ba6a2">
    <EMMO_b432d2d5_25f4_4165_99c5_5935a7763c1a xml:lang="en">π refers to the constant number ~3.14</EMMO_b432d2d5_25f4_4165_99c5_5935a7763c1a>
    <rdfs:subClassOf rdf:resource="http://emmo.info/emmo#EMMO_1eed0732_e3f1_4b2c_a9c4_b4e75eeb5895"/>
    <EMMO_967080e5_2f42_4eb2_a3a9_c58143e835f9 xml:lang="en">A 'varaible' that stand for a well known constant.</EMMO_967080e5_2f42_4eb2_a3a9_c58143e835f9>
    <rdfs:subClassOf rdf:nodeID="fe24a777e3fd743f986ce83488d2cf30bb23"/>
    <rdf:type rdf:resource="http://www.w3.org/2002/07/owl#Class"/>
    <skos:prefLabel xml:lang="en">Constant</skos:prefLabel>
  </rdf:Description>
  <rdf:Description rdf:nodeID="fe0b20157736f4a31909181349b2e6219b37">
    <owl:hasValue>T-2 L0 M+1 I-1 Θ0 N0 J0</owl:hasValue>
    <owl:onProperty rdf:resource="http://emmo.info/emmo#EMMO_23b579e1_8088_45b5_9975_064014026c42"/>
    <rdf:type rdf:resource="http://www.w3.org/2002/07/owl#Restriction"/>
  </rdf:Description>
  <rdf:Description rdf:about="http://emmo.info/emmo#EMMO_53935db0_af45_4426_b9e9_244a0d77db00">
    <skos:prefLabel xml:lang="en">MesoscopicModel</skos:prefLabel>
    <EMMO_967080e5_2f42_4eb2_a3a9_c58143e835f9 xml:lang="en">A physics-based model based on a physics equation describing the behaviour of mesoscopic entities, i.e. a set of bounded atoms like a molecule, bead or nanoparticle.</EMMO_967080e5_2f42_4eb2_a3a9_c58143e835f9>
    <rdfs:subClassOf rdf:resource="http://emmo.info/emmo#EMMO_b29fd350_39aa_4af7_9459_3faa0544cba6"/>
    <rdf:type rdf:resource="http://www.w3.org/2002/07/owl#Class"/>
  </rdf:Description>
  <rdf:Description rdf:about="http://emmo.info/emmo#EMMO_92b2fb85_2143_4bc7_bbca_df3e6944bfc1">
    <EMMO_de178b12_5d35_4bca_8efa_a4193162571d>T-3 L+2 M+1 I-2 Θ0 N0 J0</EMMO_de178b12_5d35_4bca_8efa_a4193162571d>
    <skos:prefLabel xml:lang="en">ElectricReactance</skos:prefLabel>
    <rdf:type rdf:resource="http://www.w3.org/2002/07/owl#Class"/>
    <skos:altLabel>Reactance</skos:altLabel>
    <rdfs:comment xml:lang="en">The opposition of a circuit element to a change in current or voltage, due to that element's inductance or capacitance.</rdfs:comment>
    <EMMO_1f1b164d_ec6a_4faa_8d5e_88bda62316cc>http://qudt.org/vocab/quantitykind/Reactance</EMMO_1f1b164d_ec6a_4faa_8d5e_88bda62316cc>
    <EMMO_6dd685dd_1895_46e4_b227_be9f7d643c25>http://dbpedia.org/page/Electrical_reactance</EMMO_6dd685dd_1895_46e4_b227_be9f7d643c25>
    <rdfs:subClassOf rdf:resource="http://emmo.info/emmo#EMMO_e88f75d6_9a17_4cfc_bdf7_43d7cea5a9a1"/>
  </rdf:Description>
  <rdf:Description rdf:about="http://emmo.info/emmo#EMMO_f835f4d4_c665_403d_ab25_dca5cc74be52">
    <rdf:type rdf:resource="http://www.w3.org/2002/07/owl#Class"/>
    <skos:prefLabel xml:lang="en">Nucleus</skos:prefLabel>
    <rdfs:subClassOf rdf:resource="http://emmo.info/emmo#EMMO_7d66bde4_b68d_41cc_b5fc_6fd98c5e2ff0"/>
    <rdfs:subClassOf rdf:nodeID="ff14b31ebf90e4bc5ba2839064d29e543b25"/>
  </rdf:Description>
  <rdf:Description rdf:about="http://emmo.info/emmo#EMMO_c74da218_9147_4f03_92d1_8894abca55f3">
    <EMMO_967080e5_2f42_4eb2_a3a9_c58143e835f9 xml:lang="en">A 'Perceptual' which stands for a real world object whose spatial configuration shows a pattern identifiable by an observer.</EMMO_967080e5_2f42_4eb2_a3a9_c58143e835f9>
    <rdf:type rdf:resource="http://www.w3.org/2002/07/owl#Class"/>
    <rdfs:comment xml:lang="en">From the Ancient Greek γραφή (graphḗ) which means drawing, painting, writing, a writing, description, and from γράφω (gráphō) which means scratch, carve.</rdfs:comment>
    <skos:prefLabel xml:lang="en">Graphical</skos:prefLabel>
    <EMMO_b432d2d5_25f4_4165_99c5_5935a7763c1a xml:lang="en">'Graphical' objects include writings, pictures, sketches ...</EMMO_b432d2d5_25f4_4165_99c5_5935a7763c1a>
    <rdfs:subClassOf rdf:resource="http://emmo.info/emmo#EMMO_649bf97b_4397_4005_90d9_219755d92e34"/>
  </rdf:Description>
  <rdf:Description rdf:nodeID="fe24a777e3fd743f986ce83488d2cf30bb11">
    <rdf:type rdf:resource="http://www.w3.org/2002/07/owl#Restriction"/>
    <owl:onProperty rdf:resource="http://emmo.info/emmo#EMMO_faf79f53_749d_40b2_807c_d34244c192f4"/>
    <owl:allValuesFrom rdf:resource="http://www.w3.org/2001/XMLSchema#boolean"/>
  </rdf:Description>
  <rdf:Description rdf:about="http://emmo.info/emmo#EMMO_25f8b804_9a0b_4387_a3e7_b35bce5365ee">
    <rdfs:subClassOf rdf:resource="http://emmo.info/emmo#EMMO_0f795e3e_c602_4577_9a43_d5a231aa1360"/>
    <rdf:type rdf:resource="http://www.w3.org/2002/07/owl#Class"/>
    <skos:prefLabel xml:lang="en">Photon</skos:prefLabel>
    <EMMO_967080e5_2f42_4eb2_a3a9_c58143e835f9 xml:lang="en">The class of individuals that stand for photons elementary particles.</EMMO_967080e5_2f42_4eb2_a3a9_c58143e835f9>
  </rdf:Description>
  <rdf:Description rdf:nodeID="f05bdaa1e617a4bccafc519daf7bf4785b19">
    <owl:onProperty rdf:resource="http://emmo.info/emmo#EMMO_faf79f53_749d_40b2_807c_d34244c192f4"/>
    <owl:hasValue rdf:datatype="http://www.w3.org/2001/XMLSchema#double">100.0</owl:hasValue>
    <rdf:type rdf:resource="http://www.w3.org/2002/07/owl#Restriction"/>
  </rdf:Description>
  <rdf:Description rdf:about="http://emmo.info/emmo#EMMO_5ebd5e01_0ed3_49a2_a30d_cd05cbe72978">
    <rdfs:subClassOf rdf:resource="http://emmo.info/emmo#EMMO_08b308d4_31cd_4779_a784_aa92fc730f39"/>
    <skos:prefLabel xml:lang="en">UnitOne</skos:prefLabel>
    <EMMO_b432d2d5_25f4_4165_99c5_5935a7763c1a xml:lang="en">Refractive index or volume fraction.</EMMO_b432d2d5_25f4_4165_99c5_5935a7763c1a>
    <EMMO_967080e5_2f42_4eb2_a3a9_c58143e835f9 xml:lang="en">Represents the number 1, used as an explicit unit to say something has no units.</EMMO_967080e5_2f42_4eb2_a3a9_c58143e835f9>
    <rdfs:subClassOf rdf:nodeID="f8fb83657cd5f496db3c2b94baf326f26b20"/>
    <EMMO_b432d2d5_25f4_4165_99c5_5935a7763c1a xml:lang="en">Typically used for ratios of two units whos dimensions cancels out.</EMMO_b432d2d5_25f4_4165_99c5_5935a7763c1a>
    <EMMO_1f1b164d_ec6a_4faa_8d5e_88bda62316cc>http://qudt.org/vocab/unit/UNITLESS</EMMO_1f1b164d_ec6a_4faa_8d5e_88bda62316cc>
    <rdf:type rdf:resource="http://www.w3.org/2002/07/owl#Class"/>
  </rdf:Description>
  <rdf:Description rdf:about="http://emmo.info/emmo#EMMO_a121bb1d_5225_4c78_809b_0268c3012208">
    <rdfs:subClassOf rdf:resource="http://emmo.info/emmo#EMMO_cdc962d8_f3ea_4764_a57a_c7caa4859179"/>
    <rdfs:subClassOf rdf:nodeID="f05bdaa1e617a4bccafc519daf7bf4785b109"/>
    <EMMO_fe015383_afb3_44a6_ae86_043628697aa2>https://doi.org/10.1351/goldbook.R05036</EMMO_fe015383_afb3_44a6_ae86_043628697aa2>
    <skos:prefLabel xml:lang="en">Radian</skos:prefLabel>
    <EMMO_1f1b164d_ec6a_4faa_8d5e_88bda62316cc>http://qudt.org/vocab/unit/RAD</EMMO_1f1b164d_ec6a_4faa_8d5e_88bda62316cc>
    <rdfs:comment xml:lang="en">Dimensionless measurement unit for plane angle.</rdfs:comment>
    <rdf:type rdf:resource="http://www.w3.org/2002/07/owl#Class"/>
    <EMMO_967080e5_2f42_4eb2_a3a9_c58143e835f9 xml:lang="en">Measure of plane angle.</EMMO_967080e5_2f42_4eb2_a3a9_c58143e835f9>
    <rdfs:subClassOf rdf:nodeID="f05bdaa1e617a4bccafc519daf7bf4785b110"/>
  </rdf:Description>
  <rdf:Description rdf:nodeID="f627ff42579444148ae27fcacfb5f8528b2">
    <owl:someValuesFrom rdf:resource="http://emmo.info/emmo#EMMO_02c0621e_a527_4790_8a0f_2bb51973c819"/>
    <owl:onProperty rdf:resource="http://emmo.info/emmo#EMMO_b2282816_b7a3_44c6_b2cb_3feff1ceb7fe"/>
    <rdf:type rdf:resource="http://www.w3.org/2002/07/owl#Restriction"/>
  </rdf:Description>
  <rdf:Description rdf:about="http://emmo.info/emmo#EMMO_e29f84db_4c1c_46ae_aa38_c4d47536b972">
    <rdfs:subClassOf rdf:nodeID="ffcb99037244f48d590430c228d02afdbb51"/>
    <skos:prefLabel xml:lang="en">ElectronVolt</skos:prefLabel>
    <EMMO_6dd685dd_1895_46e4_b227_be9f7d643c25>http://dbpedia.org/page/Electronvolt</EMMO_6dd685dd_1895_46e4_b227_be9f7d643c25>
    <EMMO_70fe84ff_99b6_4206_a9fc_9a8931836d84 xml:lang="en">The amount of energy gained (or lost) by the charge of a single electron moving across an electric potential difference of one volt.</EMMO_70fe84ff_99b6_4206_a9fc_9a8931836d84>
    <rdf:type rdf:resource="http://www.w3.org/2002/07/owl#Class"/>
    <EMMO_1f1b164d_ec6a_4faa_8d5e_88bda62316cc>http://qudt.org/vocab/unit/EV</EMMO_1f1b164d_ec6a_4faa_8d5e_88bda62316cc>
    <rdfs:subClassOf rdf:resource="http://emmo.info/emmo#EMMO_591e02fd_8d37_45a6_9d11_bb21cef391a0"/>
    <EMMO_fe015383_afb3_44a6_ae86_043628697aa2>https://doi.org/10.1351/goldbook.E02014</EMMO_fe015383_afb3_44a6_ae86_043628697aa2>
    <rdfs:subClassOf rdf:nodeID="ffcb99037244f48d590430c228d02afdbb52"/>
  </rdf:Description>
  <rdf:Description rdf:about="http://emmo.info/emmo#EMMO_07de47e0_6bb6_45b9_b55a_4f238efbb105">
    <EMMO_fe015383_afb3_44a6_ae86_043628697aa2>https://doi.org/10.1351/goldbook.A00499</EMMO_fe015383_afb3_44a6_ae86_043628697aa2>
    <rdfs:subClassOf rdf:resource="http://emmo.info/emmo#EMMO_ba882f34_0d71_4e4f_9d92_0c076c633a2c"/>
    <EMMO_de178b12_5d35_4bca_8efa_a4193162571d>T0 L0 M0 I0 Θ0 N0 J0</EMMO_de178b12_5d35_4bca_8efa_a4193162571d>
    <EMMO_1f1b164d_ec6a_4faa_8d5e_88bda62316cc>http://qudt.org/vocab/quantitykind/AtomicNumber</EMMO_1f1b164d_ec6a_4faa_8d5e_88bda62316cc>
    <skos:prefLabel xml:lang="en">AtomicNumber</skos:prefLabel>
    <EMMO_70fe84ff_99b6_4206_a9fc_9a8931836d84 xml:lang="en">Number of protons in an atomic nucleus.</EMMO_70fe84ff_99b6_4206_a9fc_9a8931836d84>
    <rdf:type rdf:resource="http://www.w3.org/2002/07/owl#Class"/>
    <EMMO_6dd685dd_1895_46e4_b227_be9f7d643c25>http://dbpedia.org/page/Atomic_number</EMMO_6dd685dd_1895_46e4_b227_be9f7d643c25>
  </rdf:Description>
  <rdf:Description rdf:nodeID="ff14b31ebf90e4bc5ba2839064d29e543b24">
    <rdf:type rdf:resource="http://www.w3.org/2002/07/owl#Restriction"/>
    <owl:onProperty rdf:resource="http://emmo.info/emmo#EMMO_b2282816_b7a3_44c6_b2cb_3feff1ceb7fe"/>
    <owl:someValuesFrom rdf:resource="http://emmo.info/emmo#EMMO_f835f4d4_c665_403d_ab25_dca5cc74be52"/>
  </rdf:Description>
  <rdf:Description rdf:about="http://emmo.info/emmo#EMMO_29afdf54_90ae_4c98_8845_fa9ea3f143a8">
    <rdfs:subClassOf rdf:resource="http://emmo.info/emmo#EMMO_e56ee3eb_7609_4ae1_8bed_51974f0960a6"/>
    <skos:prefLabel xml:lang="en">DefiningEquation</skos:prefLabel>
    <EMMO_967080e5_2f42_4eb2_a3a9_c58143e835f9 xml:lang="en">An equation that define a new variable in terms of other mathematical entities.</EMMO_967080e5_2f42_4eb2_a3a9_c58143e835f9>
    <rdf:type rdf:resource="http://www.w3.org/2002/07/owl#Class"/>
    <EMMO_b432d2d5_25f4_4165_99c5_5935a7763c1a xml:lang="en">The definition of velocity as v = dx/dt.

The definition of density as mass/volume.

y = f(x)</EMMO_b432d2d5_25f4_4165_99c5_5935a7763c1a>
  </rdf:Description>
  <rdf:Description rdf:about="http://emmo.info/emmo#EMMO_b306ae38_938e_48fe_83e9_6141e08b596f">
    <rdfs:comment xml:lang="en">URL to corresponding concept in the Basic Datatype Ontology (DBO)</rdfs:comment>
    <rdf:type rdf:resource="http://www.w3.org/2002/07/owl#AnnotationProperty"/>
    <rdfs:subPropertyOf rdf:resource="http://www.w3.org/2000/01/rdf-schema#seeAlso"/>
    <rdfs:seeAlso rdf:datatype="http://www.w3.org/2001/XMLSchema#anyURI">https://github.com/TechnicalBuildingSystems/Ontologies/blob/master/BasicDataTypeOntology/ontology.ttl</rdfs:seeAlso>
    <rdfs:range rdf:resource="http://www.w3.org/2001/XMLSchema#anyURI"/>
    <skos:prefLabel xml:lang="en">bdoMatch</skos:prefLabel>
  </rdf:Description>
  <rdf:Description rdf:nodeID="ffcb99037244f48d590430c228d02afdbb13">
    <owl:someValuesFrom rdf:resource="http://emmo.info/emmo#EMMO_02e894c3_b793_4197_b120_3442e08f58d1"/>
    <owl:onProperty rdf:resource="http://emmo.info/emmo#EMMO_bed1d005_b04e_4a90_94cf_02bc678a8569"/>
    <rdf:type rdf:resource="http://www.w3.org/2002/07/owl#Restriction"/>
  </rdf:Description>
  <rdf:Description rdf:nodeID="ffcb99037244f48d590430c228d02afdbb12">
    <owl:hasValue>Å</owl:hasValue>
    <owl:onProperty rdf:resource="http://emmo.info/emmo#EMMO_23b579e1_8088_45b5_9975_064014026c42"/>
    <rdf:type rdf:resource="http://www.w3.org/2002/07/owl#Restriction"/>
  </rdf:Description>
  <rdf:Description rdf:about="http://emmo.info/emmo#EMMO_70dac51e_bddd_48c2_8a98_7d8395e91fc2">
    <rdfs:subClassOf rdf:nodeID="fea11ca01461e402d8f697c19c5d8de88b10"/>
    <rdfs:comment xml:lang="en">The concepts of matter and field for classical physics, upon which we can categorize physical entities, are replaced in quantum physics by the more general concepts of quantum field.

Here the class 'Field' refers to the quantum field of massless bosonic particles (i.e. photons, gluons), while the class 'Matter' refers to the quantum field of massive fermionic or bosonic particles (e.g. quarks, electrons).</rdfs:comment>
    <rdf:type rdf:resource="http://www.w3.org/2002/07/owl#Class"/>
    <rdfs:subClassOf rdf:resource="http://emmo.info/emmo#EMMO_c5ddfdba_c074_4aa4_ad6b_1ac4942d300d"/>
    <EMMO_967080e5_2f42_4eb2_a3a9_c58143e835f9 xml:lang="en">A 'Physical' with 'Massless' parts that are mediators of interactions.</EMMO_967080e5_2f42_4eb2_a3a9_c58143e835f9>
    <skos:prefLabel xml:lang="en">Field</skos:prefLabel>
    <rdfs:subClassOf rdf:nodeID="fea11ca01461e402d8f697c19c5d8de88b11"/>
  </rdf:Description>
  <rdf:Description rdf:about="http://emmo.info/emmo#EMMO_d69d2e95_b22f_499a_a552_17fde0d778fc">
    <rdfs:subClassOf rdf:resource="http://emmo.info/emmo#EMMO_7509da43_56b1_4d7f_887a_65d1663df4ba"/>
    <rdf:type rdf:resource="http://www.w3.org/2002/07/owl#Class"/>
    <skos:prefLabel xml:lang="en">LiquidFoam</skos:prefLabel>
    <EMMO_967080e5_2f42_4eb2_a3a9_c58143e835f9 xml:lang="en">A foam of trapped gas in a liquid.</EMMO_967080e5_2f42_4eb2_a3a9_c58143e835f9>
    <rdfs:subClassOf rdf:resource="http://emmo.info/emmo#EMMO_1f5e3e7e_72c9_40d4_91dd_ae432d7b7018"/>
  </rdf:Description>
  <rdf:Description rdf:about="http://emmo.info/emmo#EMMO_517dfaf9_4970_41ac_81ee_d031627d2c7c">
    <skos:prefLabel xml:lang="en">disconnected</skos:prefLabel>
    <rdf:type rdf:resource="http://www.w3.org/2002/07/owl#ObjectProperty"/>
    <rdf:type rdf:resource="http://www.w3.org/2002/07/owl#SymmetricProperty"/>
    <rdfs:subPropertyOf rdf:resource="http://emmo.info/emmo#EMMO_03212fd7_abfd_4828_9c8e_62c293052d4b"/>
  </rdf:Description>
  <rdf:Description rdf:nodeID="fa691b5894b3543efa24f9838ff46c3eab9">
    <owl:unionOf rdf:nodeID="fa691b5894b3543efa24f9838ff46c3eab10"/>
    <rdf:type rdf:resource="http://www.w3.org/2002/07/owl#Class"/>
  </rdf:Description>
  <rdf:Description rdf:nodeID="f05bdaa1e617a4bccafc519daf7bf4785b139">
    <rdf:type rdf:resource="http://www.w3.org/2002/07/owl#Restriction"/>
    <owl:onProperty rdf:resource="http://emmo.info/emmo#EMMO_bed1d005_b04e_4a90_94cf_02bc678a8569"/>
    <owl:someValuesFrom rdf:resource="http://emmo.info/emmo#EMMO_4c49ab58_a6f6_409e_b849_f873ae1dcbee"/>
  </rdf:Description>
  <rdf:Description rdf:about="http://emmo.info/emmo#EMMO_8a70dea4_d6ab_4260_b931_a3e990982416">
    <rdf:type rdf:resource="http://www.w3.org/2002/07/owl#Class"/>
    <rdfs:comment xml:lang="en">Measurement unit for energy.</rdfs:comment>
    <EMMO_1f1b164d_ec6a_4faa_8d5e_88bda62316cc>http://qudt.org/vocab/unit/J</EMMO_1f1b164d_ec6a_4faa_8d5e_88bda62316cc>
    <EMMO_fe015383_afb3_44a6_ae86_043628697aa2>https://doi.org/10.1351/goldbook.J03363</EMMO_fe015383_afb3_44a6_ae86_043628697aa2>
    <rdfs:subClassOf rdf:nodeID="f05bdaa1e617a4bccafc519daf7bf4785b100"/>
    <rdfs:subClassOf rdf:nodeID="f05bdaa1e617a4bccafc519daf7bf4785b99"/>
    <skos:prefLabel xml:lang="en">Joule</skos:prefLabel>
  </rdf:Description>
  <rdf:Description rdf:about="http://emmo.info/emmo#EMMO_b3600e73_3e05_479d_9714_c041c3acf5cc">
    <rdfs:subClassOf rdf:resource="http://emmo.info/emmo#EMMO_9895a1b4_f0a5_4167_ac5e_97db40b8bfcc"/>
    <owl:equivalentClass rdf:nodeID="fe0b20157736f4a31909181349b2e6219b32"/>
    <skos:prefLabel xml:lang="en">LengthDimension</skos:prefLabel>
    <rdf:type rdf:resource="http://www.w3.org/2002/07/owl#Class"/>
  </rdf:Description>
  <rdf:Description rdf:nodeID="f8fb83657cd5f496db3c2b94baf326f26b43">
    <rdf:rest rdf:resource="http://www.w3.org/1999/02/22-rdf-syntax-ns#nil"/>
    <rdf:first rdf:resource="http://emmo.info/emmo#EMMO_c46f091c_0420_4c1a_af30_0a2c8ebcf7d7"/>
    <rdf:type rdf:resource="http://www.w3.org/1999/02/22-rdf-syntax-ns#List"/>
  </rdf:Description>
  <rdf:Description rdf:about="http://emmo.info/emmo#EMMO_7d2afa66_ae9e_4095_a9bf_421d0be401b6">
    <rdfs:seeAlso>https://en.wikipedia.org/wiki/Metric_prefix</rdfs:seeAlso>
    <rdf:type rdf:resource="http://www.w3.org/2002/07/owl#Class"/>
    <skos:prefLabel xml:lang="en">MetricPrefix</skos:prefLabel>
    <rdfs:subClassOf rdf:resource="http://emmo.info/emmo#EMMO_ae15fb4f_8e4d_41de_a0f9_3997f89ba6a2"/>
    <rdfs:subClassOf rdf:resource="http://emmo.info/emmo#EMMO_985bec21_989f_4b9e_a4b3_735d88099c3c"/>
    <rdfs:subClassOf rdf:resource="http://emmo.info/emmo#EMMO_a1083d0a_c1fb_471f_8e20_a98f881ad527"/>
    <EMMO_967080e5_2f42_4eb2_a3a9_c58143e835f9 xml:lang="en">Dimensionless multiplicative unit prefix.</EMMO_967080e5_2f42_4eb2_a3a9_c58143e835f9>
  </rdf:Description>
  <rdf:Description rdf:nodeID="f05bdaa1e617a4bccafc519daf7bf4785b64">
    <rdf:rest rdf:nodeID="f05bdaa1e617a4bccafc519daf7bf4785b65"/>
    <rdf:type rdf:resource="http://www.w3.org/1999/02/22-rdf-syntax-ns#List"/>
    <rdf:first rdf:resource="http://emmo.info/emmo#EMMO_43a6b269_da31_4bb6_a537_c97df4fff32a"/>
  </rdf:Description>
  <rdf:Description rdf:nodeID="fdb1489b80bcc4ee28afe0be8feb9b935b14">
    <rdf:rest rdf:nodeID="fdb1489b80bcc4ee28afe0be8feb9b935b15"/>
    <rdf:type rdf:resource="http://www.w3.org/1999/02/22-rdf-syntax-ns#List"/>
    <rdf:first rdf:resource="http://emmo.info/emmo#EMMO_873b0ab3_88e6_4054_b901_5531e01f14a4"/>
  </rdf:Description>
  <rdf:Description rdf:about="http://emmo.info/emmo#EMMO_a77a0a4b_6bd2_42b2_be27_4b63cebbb59e">
    <skos:prefLabel xml:lang="en">TemperatureDimension</skos:prefLabel>
    <rdf:type rdf:resource="http://www.w3.org/2002/07/owl#Class"/>
    <owl:equivalentClass rdf:nodeID="fe0b20157736f4a31909181349b2e6219b28"/>
    <rdfs:subClassOf rdf:resource="http://emmo.info/emmo#EMMO_9895a1b4_f0a5_4167_ac5e_97db40b8bfcc"/>
  </rdf:Description>
  <rdf:Description rdf:about="http://emmo.info/emmo#EMMO_ffc7735f_c177_46a4_98e9_a54440d29209">
    <EMMO_1f1b164d_ec6a_4faa_8d5e_88bda62316cc>http://qudt.org/vocab/constant/BoltzmannConstant</EMMO_1f1b164d_ec6a_4faa_8d5e_88bda62316cc>
    <EMMO_fe015383_afb3_44a6_ae86_043628697aa2>https://doi.org/10.1351/goldbook.B00695</EMMO_fe015383_afb3_44a6_ae86_043628697aa2>
    <rdfs:subClassOf rdf:resource="http://emmo.info/emmo#EMMO_9bbab0be_f9cc_4f46_9f46_0fd271911b79"/>
    <rdfs:subClassOf rdf:resource="http://emmo.info/emmo#EMMO_f2ca6dd0_0e5f_4392_a92d_cafdae6cfc95"/>
    <EMMO_de178b12_5d35_4bca_8efa_a4193162571d>T-2 L+2 M+1 I0 Θ-1 N0 J0</EMMO_de178b12_5d35_4bca_8efa_a4193162571d>
    <rdf:type rdf:resource="http://www.w3.org/2002/07/owl#Class"/>
    <rdfs:comment xml:lang="en">The DBpedia definition (http://dbpedia.org/page/Boltzmann_constant) is outdated as May 20, 2019. It is now an exact quantity.</rdfs:comment>
    <EMMO_6dd685dd_1895_46e4_b227_be9f7d643c25>http://dbpedia.org/page/Boltzmann_constant</EMMO_6dd685dd_1895_46e4_b227_be9f7d643c25>
    <EMMO_a9b3d04c_7ceb_40a2_b8d3_28d514a770a8>https://physics.nist.gov/cgi-bin/cuu/Value?k</EMMO_a9b3d04c_7ceb_40a2_b8d3_28d514a770a8>
    <EMMO_967080e5_2f42_4eb2_a3a9_c58143e835f9 xml:lang="en">A physical constant relating energy at the individual particle level with temperature. It is the gas constant R divided by the Avogadro constant.

It defines the Kelvin unit in the SI system.</EMMO_967080e5_2f42_4eb2_a3a9_c58143e835f9>
    <skos:prefLabel xml:lang="en">BoltzmannConstant</skos:prefLabel>
  </rdf:Description>
  <rdf:Description rdf:about="http://emmo.info/emmo#EMMO_8786cb47_8e1f_4968_9b15_f6d41fc51252">
    <EMMO_967080e5_2f42_4eb2_a3a9_c58143e835f9 xml:lang="en">A manufacturing process aimed to the production of a device made of specific components.</EMMO_967080e5_2f42_4eb2_a3a9_c58143e835f9>
    <EMMO_b432d2d5_25f4_4165_99c5_5935a7763c1a xml:lang="en">Assemblying a bicycle, building a car.</EMMO_b432d2d5_25f4_4165_99c5_5935a7763c1a>
    <rdfs:subClassOf rdf:resource="http://emmo.info/emmo#EMMO_a4d66059_5dd3_4b90_b4cb_10960559441b"/>
    <rdf:type rdf:resource="http://www.w3.org/2002/07/owl#Class"/>
    <skos:prefLabel xml:lang="en">DiscreteManufacturing</skos:prefLabel>
  </rdf:Description>
  <rdf:Description rdf:nodeID="fe0b20157736f4a31909181349b2e6219b38">
    <owl:onProperty rdf:nodeID="fe0b20157736f4a31909181349b2e6219b39"/>
    <owl:allValuesFrom rdf:resource="http://emmo.info/emmo#EMMO_5b2222df_4da6_442f_8244_96e9e45887d1"/>
    <rdf:type rdf:resource="http://www.w3.org/2002/07/owl#Restriction"/>
  </rdf:Description>
  <rdf:Description rdf:about="http://emmo.info/emmo#EMMO_16f2fe60_2db7_43ca_8fee_5b3e416bfe87">
    <EMMO_de178b12_5d35_4bca_8efa_a4193162571d>T0 L-3 M+1 I0 Θ0 N0 J0</EMMO_de178b12_5d35_4bca_8efa_a4193162571d>
    <rdf:type rdf:resource="http://www.w3.org/2002/07/owl#Class"/>
    <EMMO_1f1b164d_ec6a_4faa_8d5e_88bda62316cc>http://qudt.org/vocab/quantitykind/MassConcentration</EMMO_1f1b164d_ec6a_4faa_8d5e_88bda62316cc>
    <rdfs:subClassOf rdf:resource="http://emmo.info/emmo#EMMO_06448f64_8db6_4304_8b2c_e785dba82044"/>
    <EMMO_fe015383_afb3_44a6_ae86_043628697aa2>https://doi.org/10.1351/goldbook.M03713</EMMO_fe015383_afb3_44a6_ae86_043628697aa2>
    <skos:prefLabel xml:lang="en">MassConcentration</skos:prefLabel>
    <rdfs:comment xml:lang="en">Mass of a constituent divided by the volume of the mixture.</rdfs:comment>
    <EMMO_6dd685dd_1895_46e4_b227_be9f7d643c25>http://dbpedia.org/page/Mass_concentration_(chemistry)</EMMO_6dd685dd_1895_46e4_b227_be9f7d643c25>
  </rdf:Description>
  <rdf:Description rdf:about="http://emmo.info/emmo#EMMO_9bbab0be_f9cc_4f46_9f46_0fd271911b79">
    <EMMO_6dd685dd_1895_46e4_b227_be9f7d643c25>http://dbpedia.org/page/Entropy</EMMO_6dd685dd_1895_46e4_b227_be9f7d643c25>
    <skos:prefLabel xml:lang="en">Entropy</skos:prefLabel>
    <EMMO_1f1b164d_ec6a_4faa_8d5e_88bda62316cc>http://qudt.org/vocab/quantitykind/Entropy</EMMO_1f1b164d_ec6a_4faa_8d5e_88bda62316cc>
    <EMMO_fe015383_afb3_44a6_ae86_043628697aa2>https://doi.org/10.1351/goldbook.E02149</EMMO_fe015383_afb3_44a6_ae86_043628697aa2>
    <rdfs:subClassOf rdf:resource="http://emmo.info/emmo#EMMO_2946d40b_24a1_47fa_8176_e3f79bb45064"/>
    <EMMO_de178b12_5d35_4bca_8efa_a4193162571d>T-2 L+2 M+1 I0 Θ-1 N0 J0</EMMO_de178b12_5d35_4bca_8efa_a4193162571d>
    <rdfs:comment xml:lang="en">Logarithmic measure of the number of available states of a system.</rdfs:comment>
    <rdfs:comment xml:lang="en">May also be referred to as a measure of order of  a system.</rdfs:comment>
    <rdf:type rdf:resource="http://www.w3.org/2002/07/owl#Class"/>
  </rdf:Description>
  <rdf:Description rdf:about="http://emmo.info/emmo#EMMO_e9e02156_651f_41c8_9efb_d5da0d4ce5e2">
    <rdf:type rdf:resource="http://www.w3.org/2002/07/owl#Class"/>
    <EMMO_967080e5_2f42_4eb2_a3a9_c58143e835f9 xml:lang="en">A coarse dispersion of solids in a liquid continuum phase.</EMMO_967080e5_2f42_4eb2_a3a9_c58143e835f9>
    <rdfs:subClassOf rdf:resource="http://emmo.info/emmo#EMMO_7509da43_56b1_4d7f_887a_65d1663df4ba"/>
    <EMMO_b432d2d5_25f4_4165_99c5_5935a7763c1a xml:lang="en">Mud</EMMO_b432d2d5_25f4_4165_99c5_5935a7763c1a>
    <skos:prefLabel xml:lang="en">LiquidSolidSuspension</skos:prefLabel>
  </rdf:Description>
  <rdf:Description rdf:about="http://emmo.info/emmo#EMMO_db03061b_db31_4132_a47a_6a634846578b">
    <skos:prefLabel xml:lang="en">IonAtom</skos:prefLabel>
    <rdfs:comment xml:lang="en">The ion_atom is the basic part of a pure ionic bonded compound i.e. without eclectron sharing,</rdfs:comment>
    <EMMO_967080e5_2f42_4eb2_a3a9_c58143e835f9 xml:lang="en">A standalone atom with an unbalanced number of electrons with respect to its atomic number.</EMMO_967080e5_2f42_4eb2_a3a9_c58143e835f9>
    <rdf:type rdf:resource="http://www.w3.org/2002/07/owl#Class"/>
  </rdf:Description>
  <rdf:Description rdf:about="http://emmo.info/emmo#EMMO_ecec2983_7c26_4f8d_a981_51ca29668baf">
    <rdf:type rdf:resource="http://www.w3.org/2002/07/owl#Class"/>
    <skos:prefLabel xml:lang="en">ReciprocalLength</skos:prefLabel>
    <EMMO_1f1b164d_ec6a_4faa_8d5e_88bda62316cc>http://qudt.org/vocab/quantitykind/InverseLength</EMMO_1f1b164d_ec6a_4faa_8d5e_88bda62316cc>
    <EMMO_6dd685dd_1895_46e4_b227_be9f7d643c25>http://dbpedia.org/page/Reciprocal_length</EMMO_6dd685dd_1895_46e4_b227_be9f7d643c25>
    <EMMO_c84c6752_6d64_48cc_9500_e54a3c34898d>https://en.wikipedia.org/wiki/Reciprocal_length</EMMO_c84c6752_6d64_48cc_9500_e54a3c34898d>
    <EMMO_967080e5_2f42_4eb2_a3a9_c58143e835f9 xml:lang="en">The inverse of length.</EMMO_967080e5_2f42_4eb2_a3a9_c58143e835f9>
    <skos:altLabel>InverseLength</skos:altLabel>
    <rdfs:subClassOf rdf:resource="http://emmo.info/emmo#EMMO_2946d40b_24a1_47fa_8176_e3f79bb45064"/>
    <EMMO_de178b12_5d35_4bca_8efa_a4193162571d>T0 L-1 M0 I0 Θ0 N0 J0</EMMO_de178b12_5d35_4bca_8efa_a4193162571d>
  </rdf:Description>
  <rdf:Description rdf:about="http://emmo.info/emmo#EMMO_f1a51559_aa3d_43a0_9327_918039f0dfed">
    <skos:prefLabel xml:lang="en">Volume</skos:prefLabel>
    <rdf:type rdf:resource="http://www.w3.org/2002/07/owl#Class"/>
    <EMMO_1f1b164d_ec6a_4faa_8d5e_88bda62316cc>http://qudt.org/vocab/quantitykind/Volume</EMMO_1f1b164d_ec6a_4faa_8d5e_88bda62316cc>
    <EMMO_de178b12_5d35_4bca_8efa_a4193162571d>T0 L-3 M0 I0 Θ0 N0 J0</EMMO_de178b12_5d35_4bca_8efa_a4193162571d>
    <rdfs:subClassOf rdf:resource="http://emmo.info/emmo#EMMO_2946d40b_24a1_47fa_8176_e3f79bb45064"/>
    <rdfs:comment xml:lang="en">Extent of an object in space.</rdfs:comment>
    <EMMO_6dd685dd_1895_46e4_b227_be9f7d643c25>http://dbpedia.org/page/Volume</EMMO_6dd685dd_1895_46e4_b227_be9f7d643c25>
  </rdf:Description>
  <rdf:Description rdf:about="http://emmo.info/emmo#EMMO_8d3da9ac_2265_4382_bee5_db72046722f8">
    <skos:prefLabel xml:lang="en">Radioactivity</skos:prefLabel>
    <EMMO_fe015383_afb3_44a6_ae86_043628697aa2>https://doi.org/10.1351/goldbook.A00114</EMMO_fe015383_afb3_44a6_ae86_043628697aa2>
    <EMMO_de178b12_5d35_4bca_8efa_a4193162571d>T-1 L0 M0 I0 Θ0 N0 J0</EMMO_de178b12_5d35_4bca_8efa_a4193162571d>
    <EMMO_967080e5_2f42_4eb2_a3a9_c58143e835f9 xml:lang="en">Decays per unit time.</EMMO_967080e5_2f42_4eb2_a3a9_c58143e835f9>
    <rdf:type rdf:resource="http://www.w3.org/2002/07/owl#Class"/>
    <EMMO_1f1b164d_ec6a_4faa_8d5e_88bda62316cc>http://qudt.org/vocab/quantitykind/SpecificActivity</EMMO_1f1b164d_ec6a_4faa_8d5e_88bda62316cc>
    <rdfs:subClassOf rdf:resource="http://emmo.info/emmo#EMMO_2946d40b_24a1_47fa_8176_e3f79bb45064"/>
  </rdf:Description>
  <rdf:Description rdf:about="http://emmo.info/emmo#EMMO_db5dd38d_ac79_4af6_8782_fee7e7150ae8">
    <rdfs:subClassOf rdf:nodeID="f05bdaa1e617a4bccafc519daf7bf4785b147"/>
    <EMMO_1f1b164d_ec6a_4faa_8d5e_88bda62316cc>http://qudt.org/vocab/unit/A</EMMO_1f1b164d_ec6a_4faa_8d5e_88bda62316cc>
    <rdfs:subClassOf rdf:nodeID="f05bdaa1e617a4bccafc519daf7bf4785b148"/>
    <EMMO_70fe84ff_99b6_4206_a9fc_9a8931836d84 xml:lang="en">The ampere, symbol A, is the SI unit of electric current. It is defined by taking the fixed numerical value of the elementary charge e to be 1.602176634×10−19 when expressed in the unit C, which is equal to A s, where the second is defined in terms of ∆νCs.</EMMO_70fe84ff_99b6_4206_a9fc_9a8931836d84>
    <EMMO_fe015383_afb3_44a6_ae86_043628697aa2>https://doi.org/10.1351/goldbook.A00300</EMMO_fe015383_afb3_44a6_ae86_043628697aa2>
    <rdf:type rdf:resource="http://www.w3.org/2002/07/owl#Class"/>
    <skos:prefLabel xml:lang="en">Ampere</skos:prefLabel>
  </rdf:Description>
  <rdf:Description rdf:nodeID="f8fb83657cd5f496db3c2b94baf326f26b41">
    <rdf:type rdf:resource="http://www.w3.org/2002/07/owl#Restriction"/>
    <owl:onProperty rdf:resource="http://emmo.info/emmo#EMMO_8ef3cd6d_ae58_4a8d_9fc0_ad8f49015cd0"/>
    <owl:qualifiedCardinality rdf:datatype="http://www.w3.org/2001/XMLSchema#nonNegativeInteger">1</owl:qualifiedCardinality>
    <owl:onClass rdf:resource="http://emmo.info/emmo#EMMO_4ce76d7f_03f8_45b6_9003_90052a79bfaa"/>
  </rdf:Description>
  <rdf:Description rdf:about="http://emmo.info/emmo#EMMO_8e5dd473_808b_4a8a_b7cd_63068c12ff57">
    <EMMO_de178b12_5d35_4bca_8efa_a4193162571d>T-2 L+2 M0 I0 Θ0 N0 J0</EMMO_de178b12_5d35_4bca_8efa_a4193162571d>
    <rdf:type rdf:resource="http://www.w3.org/2002/07/owl#Class"/>
    <EMMO_6dd685dd_1895_46e4_b227_be9f7d643c25>http://dbpedia.org/page/Absorbed_dose</EMMO_6dd685dd_1895_46e4_b227_be9f7d643c25>
    <skos:prefLabel xml:lang="en">AbsorbedDose</skos:prefLabel>
    <EMMO_fe015383_afb3_44a6_ae86_043628697aa2>https://doi.org/10.1351/goldbook.A00031</EMMO_fe015383_afb3_44a6_ae86_043628697aa2>
    <rdfs:subClassOf rdf:resource="http://emmo.info/emmo#EMMO_2946d40b_24a1_47fa_8176_e3f79bb45064"/>
    <EMMO_1f1b164d_ec6a_4faa_8d5e_88bda62316cc>http://qudt.org/vocab/quantitykind/AbsorbedDose</EMMO_1f1b164d_ec6a_4faa_8d5e_88bda62316cc>
    <EMMO_70fe84ff_99b6_4206_a9fc_9a8931836d84 xml:lang="en">Energy imparted to matter by ionizing radiation in a suitable small element of volume divided by the mass of that element of volume.</EMMO_70fe84ff_99b6_4206_a9fc_9a8931836d84>
  </rdf:Description>
  <rdf:Description rdf:about="http://emmo.info/emmo#EMMO_97589322_710c_4af4_9431_1e5027f2be42">
    <rdf:type rdf:resource="http://www.w3.org/2002/07/owl#Class"/>
    <skos:prefLabel xml:lang="en">Luminance</skos:prefLabel>
    <rdfs:subClassOf rdf:resource="http://emmo.info/emmo#EMMO_2946d40b_24a1_47fa_8176_e3f79bb45064"/>
    <EMMO_fe015383_afb3_44a6_ae86_043628697aa2>https://doi.org/10.1351/goldbook.L03640</EMMO_fe015383_afb3_44a6_ae86_043628697aa2>
    <rdfs:comment xml:lang="en">a photometric measure of the luminous intensity per unit area of light travelling in a given direction.</rdfs:comment>
    <EMMO_6dd685dd_1895_46e4_b227_be9f7d643c25>http://dbpedia.org/page/Luminance</EMMO_6dd685dd_1895_46e4_b227_be9f7d643c25>
    <EMMO_de178b12_5d35_4bca_8efa_a4193162571d>T0 L-2 M0 I0 Θ0 N0 J+1</EMMO_de178b12_5d35_4bca_8efa_a4193162571d>
    <EMMO_1f1b164d_ec6a_4faa_8d5e_88bda62316cc>http://qudt.org/vocab/quantitykind/Luminance</EMMO_1f1b164d_ec6a_4faa_8d5e_88bda62316cc>
    <rdfs:comment xml:lang="en">Measured in cd/m². Not to confuse with Illuminance, which is measured in lux (cd sr/m²).</rdfs:comment>
  </rdf:Description>
  <rdf:Description rdf:about="http://emmo.info/emmo#EMMO_3ee80521_3c23_4dd1_935d_9d522614a3e2">
    <rdfs:comment xml:lang="en">Special units are semiotic shortcuts to more complex composed symbolic objects.</rdfs:comment>
    <skos:prefLabel xml:lang="en">SpecialUnit</skos:prefLabel>
    <rdf:type rdf:resource="http://www.w3.org/2002/07/owl#Class"/>
    <rdfs:subClassOf rdf:nodeID="f8fb83657cd5f496db3c2b94baf326f26b13"/>
    <EMMO_b432d2d5_25f4_4165_99c5_5935a7763c1a xml:lang="en">Pa stands for N/m2
J stands for N m</EMMO_b432d2d5_25f4_4165_99c5_5935a7763c1a>
    <EMMO_967080e5_2f42_4eb2_a3a9_c58143e835f9 xml:lang="en">A unit symbol that stands for a derived unit.</EMMO_967080e5_2f42_4eb2_a3a9_c58143e835f9>
    <rdfs:subClassOf rdf:resource="http://emmo.info/emmo#EMMO_08b308d4_31cd_4779_a784_aa92fc730f39"/>
  </rdf:Description>
  <rdf:Description rdf:nodeID="f05bdaa1e617a4bccafc519daf7bf4785b110">
    <rdf:type rdf:resource="http://www.w3.org/2002/07/owl#Restriction"/>
    <owl:onProperty rdf:resource="http://emmo.info/emmo#EMMO_23b579e1_8088_45b5_9975_064014026c42"/>
    <owl:hasValue>rad</owl:hasValue>
  </rdf:Description>
  <rdf:Description rdf:nodeID="ff14b31ebf90e4bc5ba2839064d29e543b14">
    <rdf:first rdf:resource="http://emmo.info/emmo#EMMO_e0edfb9e_9a96_4fae_b942_831ffe27b84a"/>
    <rdf:type rdf:resource="http://www.w3.org/1999/02/22-rdf-syntax-ns#List"/>
    <rdf:rest rdf:nodeID="ff14b31ebf90e4bc5ba2839064d29e543b15"/>
  </rdf:Description>
  <rdf:Description rdf:nodeID="f15a17d1fb53e4dd795c7db922ceff6acb2">
    <owl:onProperty rdf:resource="http://emmo.info/emmo#EMMO_9380ab64_0363_4804_b13f_3a8a94119a76"/>
    <owl:allValuesFrom rdf:resource="http://www.w3.org/2002/07/owl#Nothing"/>
    <rdf:type rdf:resource="http://www.w3.org/2002/07/owl#Restriction"/>
  </rdf:Description>
  <rdf:Description rdf:about="http://emmo.info/emmo#EMMO_2031516a_2be7_48e8_9af7_7e1270e308fe">
    <rdfs:subClassOf rdf:resource="http://emmo.info/emmo#EMMO_0e6378df_1ce8_4321_b00c_ee9beea60a67"/>
    <rdfs:comment xml:lang="en">Solutions are characterized by the occurrence of Rayleigh scattering on light,</rdfs:comment>
    <rdf:type rdf:resource="http://www.w3.org/2002/07/owl#Class"/>
    <EMMO_967080e5_2f42_4eb2_a3a9_c58143e835f9 xml:lang="en">A solution is a homogeneous mixture composed of two or more substances.</EMMO_967080e5_2f42_4eb2_a3a9_c58143e835f9>
    <skos:prefLabel xml:lang="en">Solution</skos:prefLabel>
  </rdf:Description>
  <rdf:Description rdf:nodeID="ffcb99037244f48d590430c228d02afdbb10">
    <owl:onProperty rdf:resource="http://emmo.info/emmo#EMMO_23b579e1_8088_45b5_9975_064014026c42"/>
    <owl:hasValue>h</owl:hasValue>
    <rdf:type rdf:resource="http://www.w3.org/2002/07/owl#Restriction"/>
  </rdf:Description>
  <rdf:Description rdf:about="http://emmo.info/emmo#EMMO_e2207e91_02b0_4a8a_b13e_61d2a2a839f1">
    <rdfs:subClassOf rdf:nodeID="f05bdaa1e617a4bccafc519daf7bf4785b157"/>
    <EMMO_1f1b164d_ec6a_4faa_8d5e_88bda62316cc>http://qudt.org/vocab/unit/V</EMMO_1f1b164d_ec6a_4faa_8d5e_88bda62316cc>
    <EMMO_fe015383_afb3_44a6_ae86_043628697aa2>https://doi.org/10.1351/goldbook.V06634</EMMO_fe015383_afb3_44a6_ae86_043628697aa2>
    <rdf:type rdf:resource="http://www.w3.org/2002/07/owl#Class"/>
    <skos:prefLabel xml:lang="en">Volt</skos:prefLabel>
    <rdfs:comment xml:lang="en">Measurement unit for voltage.</rdfs:comment>
    <rdfs:subClassOf rdf:nodeID="f05bdaa1e617a4bccafc519daf7bf4785b158"/>
  </rdf:Description>
  <rdf:Description rdf:about="http://emmo.info/emmo#EMMO_c2f5ee66_579c_44c6_a2e9_fa2eaa9fa4da">
    <rdf:type rdf:resource="http://www.w3.org/2002/07/owl#Class"/>
    <EMMO_967080e5_2f42_4eb2_a3a9_c58143e835f9 xml:lang="en">Unit for fractions of quantities of the same kind, to aid the understanding of the quantity being expressed.</EMMO_967080e5_2f42_4eb2_a3a9_c58143e835f9>
    <rdfs:comment xml:lang="en">Quantities that are ratios of quantities of the same kind (for example length ratios and amount fractions) have the option of being expressed with units (m/m, mol/mol to aid the understanding of the quantity being expressed and also allow the use of SI prefixes, if this
is desirable (μm/m, nmol/mol).
-- SI Brochure</rdfs:comment>
    <skos:prefLabel xml:lang="en">FractionUnit</skos:prefLabel>
    <rdfs:subClassOf rdf:resource="http://emmo.info/emmo#EMMO_5ebd5e01_0ed3_49a2_a30d_cd05cbe72978"/>
  </rdf:Description>
  <rdf:Description rdf:nodeID="f8fb83657cd5f496db3c2b94baf326f26b42">
    <rdf:rest rdf:nodeID="f8fb83657cd5f496db3c2b94baf326f26b43"/>
    <rdf:type rdf:resource="http://www.w3.org/1999/02/22-rdf-syntax-ns#List"/>
    <rdf:first rdf:resource="http://emmo.info/emmo#EMMO_02c0621e_a527_4790_8a0f_2bb51973c819"/>
  </rdf:Description>
  <rdf:Description rdf:nodeID="f05bdaa1e617a4bccafc519daf7bf4785b153">
    <rdf:type rdf:resource="http://www.w3.org/2002/07/owl#Restriction"/>
    <owl:onProperty rdf:nodeID="f05bdaa1e617a4bccafc519daf7bf4785b154"/>
    <owl:allValuesFrom rdf:nodeID="f05bdaa1e617a4bccafc519daf7bf4785b155"/>
  </rdf:Description>
  <rdf:Description rdf:about="http://emmo.info/emmo#EMMO_fe7e56ce_118b_4243_9aad_20eb9f4f31f6">
    <EMMO_b432d2d5_25f4_4165_99c5_5935a7763c1a xml:lang="en">Velocity, for the Navier-Stokes equation.</EMMO_b432d2d5_25f4_4165_99c5_5935a7763c1a>
    <rdfs:subClassOf rdf:resource="http://emmo.info/emmo#EMMO_1eed0732_e3f1_4b2c_a9c4_b4e75eeb5895"/>
    <skos:prefLabel xml:lang="en">Unknown</skos:prefLabel>
    <EMMO_967080e5_2f42_4eb2_a3a9_c58143e835f9 xml:lang="en">The dependent variable for which an equation has been written.</EMMO_967080e5_2f42_4eb2_a3a9_c58143e835f9>
    <rdf:type rdf:resource="http://www.w3.org/2002/07/owl#Class"/>
  </rdf:Description>
  <rdf:Description rdf:about="http://emmo.info/emmo#EMMO_86ca9b93_1183_4b65_81b8_c0fcd3bba5ad">
    <rdf:type rdf:resource="http://www.w3.org/2002/07/owl#Class"/>
    <EMMO_967080e5_2f42_4eb2_a3a9_c58143e835f9 xml:lang="en">A 'physical' that stands for a real world object that has been designed and manufactured for a particular purpose.</EMMO_967080e5_2f42_4eb2_a3a9_c58143e835f9>
    <skos:prefLabel xml:lang="en">Engineered</skos:prefLabel>
    <rdfs:subClassOf rdf:nodeID="ffbe75b10062f400ea693809785c50a44b3"/>
    <rdfs:comment xml:lang="en">The 'Engineered' branch represents real world objects that show some level of complexity/heterogeneity in their composition, and are made for a specific use.</rdfs:comment>
    <EMMO_b432d2d5_25f4_4165_99c5_5935a7763c1a xml:lang="en">Car, tire, composite material.</EMMO_b432d2d5_25f4_4165_99c5_5935a7763c1a>
  </rdf:Description>
  <rdf:Description rdf:nodeID="fea11ca01461e402d8f697c19c5d8de88b14">
    <rdf:rest rdf:resource="http://www.w3.org/1999/02/22-rdf-syntax-ns#nil"/>
    <rdf:first rdf:resource="http://emmo.info/emmo#EMMO_70dac51e_bddd_48c2_8a98_7d8395e91fc2"/>
    <rdf:type rdf:resource="http://www.w3.org/1999/02/22-rdf-syntax-ns#List"/>
  </rdf:Description>
  <rdf:Description rdf:nodeID="f05bdaa1e617a4bccafc519daf7bf4785b107">
    <rdf:type rdf:resource="http://www.w3.org/2002/07/owl#Restriction"/>
    <owl:onProperty rdf:resource="http://emmo.info/emmo#EMMO_faf79f53_749d_40b2_807c_d34244c192f4"/>
    <owl:hasValue rdf:datatype="http://www.w3.org/2001/XMLSchema#double">1e-06</owl:hasValue>
  </rdf:Description>
  <rdf:Description rdf:nodeID="ffcb99037244f48d590430c228d02afdbb38">
    <owl:onProperty rdf:resource="http://emmo.info/emmo#EMMO_23b579e1_8088_45b5_9975_064014026c42"/>
    <rdf:type rdf:resource="http://www.w3.org/2002/07/owl#Restriction"/>
    <owl:hasValue>l</owl:hasValue>
  </rdf:Description>
  <rdf:Description rdf:about="http://emmo.info/emmo#EMMO_d5be1faf_0c56_4f5a_9b78_581e6dee949f">
    <skos:altLabel xml:lang="en">MolarConcentration</skos:altLabel>
    <rdfs:comment xml:lang="en">The amount of a constituent divided by the volume of the mixture.</rdfs:comment>
    <skos:altLabel xml:lang="en">Concentration</skos:altLabel>
    <EMMO_de178b12_5d35_4bca_8efa_a4193162571d>T0 L-3 M0 I0 Θ0 N+1 J0</EMMO_de178b12_5d35_4bca_8efa_a4193162571d>
    <EMMO_1f1b164d_ec6a_4faa_8d5e_88bda62316cc>http://qudt.org/vocab/quantitykind/AmountOfSubstanceConcentrationOfB</EMMO_1f1b164d_ec6a_4faa_8d5e_88bda62316cc>
    <skos:altLabel xml:lang="en">Molarity</skos:altLabel>
    <rdf:type rdf:resource="http://www.w3.org/2002/07/owl#Class"/>
    <EMMO_6dd685dd_1895_46e4_b227_be9f7d643c25>http://dbpedia.org/page/Molar_concentration</EMMO_6dd685dd_1895_46e4_b227_be9f7d643c25>
    <skos:prefLabel xml:lang="en">AmountConcentration</skos:prefLabel>
    <EMMO_fe015383_afb3_44a6_ae86_043628697aa2>https://doi.org/10.1351/goldbook.A00295</EMMO_fe015383_afb3_44a6_ae86_043628697aa2>
    <rdfs:subClassOf rdf:resource="http://emmo.info/emmo#EMMO_2946d40b_24a1_47fa_8176_e3f79bb45064"/>
  </rdf:Description>
  <rdf:Description rdf:about="http://emmo.info/emmo#EMMO_27367073_ed8a_481a_9b07_f836dfe31f7f">
    <rdfs:subClassOf rdf:resource="http://emmo.info/emmo#EMMO_ed4af7ae_63a2_497e_bb88_2309619ea405"/>
    <skos:prefLabel xml:lang="en">AtomicMass</skos:prefLabel>
    <EMMO_fe015383_afb3_44a6_ae86_043628697aa2>https://doi.org/10.1351/goldbook.A00496</EMMO_fe015383_afb3_44a6_ae86_043628697aa2>
    <EMMO_c84c6752_6d64_48cc_9500_e54a3c34898d>https://en.wikipedia.org/wiki/Atomic_mass</EMMO_c84c6752_6d64_48cc_9500_e54a3c34898d>
    <rdfs:comment xml:lang="en">The atomic mass is often expressed as an average of the commonly found isotopes.</rdfs:comment>
    <rdfs:comment xml:lang="en">Since the nucleus account for nearly all of the total mass of atoms  (with the electrons and nuclear binding energy making minor contributions), the atomic mass measured in Da has nearly the same value as the mass number.</rdfs:comment>
    <EMMO_de178b12_5d35_4bca_8efa_a4193162571d>T0 L0 M+1 I0 Θ0 N0 J0</EMMO_de178b12_5d35_4bca_8efa_a4193162571d>
    <rdf:type rdf:resource="http://www.w3.org/2002/07/owl#Class"/>
    <EMMO_70fe84ff_99b6_4206_a9fc_9a8931836d84 xml:lang="en">The mass of an atom in the ground state.</EMMO_70fe84ff_99b6_4206_a9fc_9a8931836d84>
  </rdf:Description>
  <rdf:Description rdf:nodeID="ffcb99037244f48d590430c228d02afdbb27">
    <rdf:rest rdf:nodeID="ffcb99037244f48d590430c228d02afdbb28"/>
    <rdf:first rdf:resource="http://emmo.info/emmo#EMMO_cabb20f0_05c7_448f_9485_e129725f15a4"/>
    <rdf:type rdf:resource="http://www.w3.org/1999/02/22-rdf-syntax-ns#List"/>
  </rdf:Description>
  <rdf:Description rdf:about="http://emmo.info/emmo#EMMO_9bfd6f1e_b0ce_459c_beb7_8f1f41708bba">
    <rdfs:subClassOf rdf:nodeID="f05bdaa1e617a4bccafc519daf7bf4785b104"/>
    <EMMO_1f1b164d_ec6a_4faa_8d5e_88bda62316cc>http://qudt.org/vocab/unit/KiloGM</EMMO_1f1b164d_ec6a_4faa_8d5e_88bda62316cc>
    <skos:prefLabel xml:lang="en">Kilogram</skos:prefLabel>
    <EMMO_70fe84ff_99b6_4206_a9fc_9a8931836d84 xml:lang="en">The kilogram, symbol kg, is the SI unit of mass. It is defined by taking the fixed numerical value of the Planck constant h to be 6.62607015×10−34 when expressed in the unit J s, which is equal to kg m2 s−1, where the metre and the second are defined in terms of c and ∆νCs.</EMMO_70fe84ff_99b6_4206_a9fc_9a8931836d84>
    <EMMO_fe015383_afb3_44a6_ae86_043628697aa2>https://doi.org/10.1351/goldbook.K03391</EMMO_fe015383_afb3_44a6_ae86_043628697aa2>
    <rdf:type rdf:resource="http://www.w3.org/2002/07/owl#Class"/>
    <rdfs:subClassOf rdf:nodeID="f05bdaa1e617a4bccafc519daf7bf4785b103"/>
  </rdf:Description>
  <rdf:Description rdf:about="http://emmo.info/emmo#EMMO_8de5d5bf_db1c_40ac_b698_095ba3b18578">
    <rdfs:comment xml:lang="en">Corresponding item number in ISO 80 000.</rdfs:comment>
    <rdfs:range rdf:resource="http://www.w3.org/1999/02/22-rdf-syntax-ns#PlainLiteral"/>
    <rdfs:seeAlso rdf:datatype="http://www.w3.org/2001/XMLSchema#anyURI">https://www.iso.org/obp/ui/#iso:std:iso:80000:-1:ed-1:v1:en</rdfs:seeAlso>
    <skos:prefLabel xml:lang="en">ISO80000Ref</skos:prefLabel>
    <EMMO_b432d2d5_25f4_4165_99c5_5935a7763c1a xml:lang="en">3‑1.1  (refers to length)</EMMO_b432d2d5_25f4_4165_99c5_5935a7763c1a>
    <rdfs:subPropertyOf rdf:resource="http://www.w3.org/2000/01/rdf-schema#isDefinedBy"/>
    <rdf:type rdf:resource="http://www.w3.org/2002/07/owl#AnnotationProperty"/>
  </rdf:Description>
  <rdf:Description rdf:about="http://emmo.info/emmo#EMMO_65a2c5b8_e4d8_4a51_b2f8_e55effc0547d">
    <rdf:type rdf:resource="http://www.w3.org/2002/07/owl#IrreflexiveProperty"/>
    <rdf:type rdf:resource="http://www.w3.org/2002/07/owl#AsymmetricProperty"/>
    <rdf:type rdf:resource="http://www.w3.org/2002/07/owl#InverseFunctionalProperty"/>
    <skos:prefLabel xml:lang="en">hasTemporalDirectPart</skos:prefLabel>
    <rdf:type rdf:resource="http://www.w3.org/2002/07/owl#ObjectProperty"/>
    <rdfs:range rdf:resource="http://emmo.info/emmo#EMMO_36c79456_e29c_400d_8bd3_0eedddb82652"/>
    <rdfs:domain rdf:resource="http://emmo.info/emmo#EMMO_52211e5e_d767_4812_845e_eb6b402c476a"/>
    <rdfs:subPropertyOf rdf:resource="http://emmo.info/emmo#EMMO_7afbed84_7593_4a23_bd88_9d9c6b04e8f6"/>
  </rdf:Description>
  <rdf:Description rdf:about="http://emmo.info/emmo#EMMO_4ce76d7f_03f8_45b6_9003_90052a79bfaa">
    <skos:prefLabel xml:lang="en">Numerical</skos:prefLabel>
    <EMMO_967080e5_2f42_4eb2_a3a9_c58143e835f9 xml:lang="en">A 'Mathematical' that has no unknown value, i.e. all its 'Variable"-s parts refers to a 'Number' (for scalars that have a built-in datatype) or to another 'Numerical' (for complex numerical data structures that should rely on external implementations).</EMMO_967080e5_2f42_4eb2_a3a9_c58143e835f9>
    <rdf:type rdf:resource="http://www.w3.org/2002/07/owl#Class"/>
    <rdfs:subClassOf rdf:resource="http://emmo.info/emmo#EMMO_54ee6b5e_5261_44a8_86eb_5717e7fdb9d0"/>
  </rdf:Description>
  <rdf:Description rdf:about="http://emmo.info/emmo#EMMO_66d01570_36dd_42fd_844d_29b81b029cd5">
    <EMMO_6dd685dd_1895_46e4_b227_be9f7d643c25>http://dbpedia.org/page/Angular_momentum</EMMO_6dd685dd_1895_46e4_b227_be9f7d643c25>
    <EMMO_1f1b164d_ec6a_4faa_8d5e_88bda62316cc>http://qudt.org/vocab/quantitykind/AngularMomentum</EMMO_1f1b164d_ec6a_4faa_8d5e_88bda62316cc>
    <rdf:type rdf:resource="http://www.w3.org/2002/07/owl#Class"/>
    <EMMO_de178b12_5d35_4bca_8efa_a4193162571d>T-1 L+2 M+1 I0 Θ0 N0 J0</EMMO_de178b12_5d35_4bca_8efa_a4193162571d>
    <skos:prefLabel xml:lang="en">AngularMomentum</skos:prefLabel>
    <rdfs:subClassOf rdf:resource="http://emmo.info/emmo#EMMO_2946d40b_24a1_47fa_8176_e3f79bb45064"/>
    <EMMO_fe015383_afb3_44a6_ae86_043628697aa2>https://doi.org/10.1351/goldbook.A00353</EMMO_fe015383_afb3_44a6_ae86_043628697aa2>
    <rdfs:comment xml:lang="en">Measure of the extent and direction an object rotates about a reference point.</rdfs:comment>
  </rdf:Description>
  <rdf:Description rdf:about="http://emmo.info/emmo#EMMO_a055d311_9990_40a5_b2f2_288412f5d6a5">
    <EMMO_1f1b164d_ec6a_4faa_8d5e_88bda62316cc>http://qudt.org/vocab/unit/M3</EMMO_1f1b164d_ec6a_4faa_8d5e_88bda62316cc>
    <rdf:type rdf:resource="http://www.w3.org/2002/07/owl#Class"/>
    <EMMO_967080e5_2f42_4eb2_a3a9_c58143e835f9 xml:lang="en">SI coherent measurement unit for volume.</EMMO_967080e5_2f42_4eb2_a3a9_c58143e835f9>
    <rdfs:subClassOf rdf:resource="http://emmo.info/emmo#EMMO_1273eb34_de48_43a9_925f_104110469dd2"/>
    <rdfs:subClassOf rdf:nodeID="ffcb99037244f48d590430c228d02afdbb36"/>
    <skos:prefLabel xml:lang="en">CubicMetre</skos:prefLabel>
    <EMMO_e55f2d7c_9893_48cd_b4a4_fdf38253bd20>http://www.ontology-of-units-of-measure.org/resource/om-2/cubicMetre</EMMO_e55f2d7c_9893_48cd_b4a4_fdf38253bd20>
  </rdf:Description>
  <rdf:Description rdf:nodeID="f05bdaa1e617a4bccafc519daf7bf4785b113">
    <owl:onProperty rdf:resource="http://emmo.info/emmo#EMMO_faf79f53_749d_40b2_807c_d34244c192f4"/>
    <owl:hasValue rdf:datatype="http://www.w3.org/2001/XMLSchema#double">0.001</owl:hasValue>
    <rdf:type rdf:resource="http://www.w3.org/2002/07/owl#Restriction"/>
  </rdf:Description>
  <rdf:Description rdf:nodeID="f8fb83657cd5f496db3c2b94baf326f26b7">
    <owl:intersectionOf rdf:nodeID="f8fb83657cd5f496db3c2b94baf326f26b8"/>
    <rdf:type rdf:resource="http://www.w3.org/2002/07/owl#Class"/>
  </rdf:Description>
  <rdf:Description rdf:about="http://emmo.info/emmo#EMMO_67fc0a36_8dcb_4ffa_9a43_31074efa3296">
    <rdfs:domain rdf:resource="http://emmo.info/emmo#EMMO_f658c301_ce93_46cf_9639_4eace2c5d1d5"/>
    <rdf:type rdf:resource="http://www.w3.org/2002/07/owl#IrreflexiveProperty"/>
    <rdf:type rdf:resource="http://www.w3.org/2002/07/owl#AsymmetricProperty"/>
    <owl:versionInfo>In EMMO version 1.0.0-beta, physical quantities used the hasReferenceUnit object property to relate them to their units via physical dimensionality. This was simplified in 1.0.0-alpha3 in order to make reasoning faster.

The restriction (e.g. for the physical quantity Length)

    Length hasReferenceUnit only (hasPhysicsDimension only LengthDimension)

was in 1.0.0-alpha3 changed to

    Length hasPhysicsDimension some LengthDimension

Likewise were the universal restrictions on the corresponding unit changed to excistential. E.g.

    Metre hasPhysicsDimension only LengthDimension

was changed to

    Metre hasPhysicsDimension some LengthDimension

The label of this class was also changed from PhysicsDimension to PhysicalDimension.</owl:versionInfo>
    <rdf:type rdf:resource="http://www.w3.org/2002/07/owl#InverseFunctionalProperty"/>
    <rdf:type rdf:resource="http://www.w3.org/2002/07/owl#ObjectProperty"/>
    <skos:prefLabel xml:lang="en">hasReferenceUnit</skos:prefLabel>
    <rdfs:comment xml:lang="en">Relates the physical quantity to its unit through spatial direct parthood.</rdfs:comment>
    <rdfs:range rdf:resource="http://emmo.info/emmo#EMMO_18ce5200_00f5_45bb_8c6f_6fb128cd41ae"/>
    <rdfs:subPropertyOf rdf:resource="http://emmo.info/emmo#EMMO_b2282816_b7a3_44c6_b2cb_3feff1ceb7fe"/>
  </rdf:Description>
  <rdf:Description rdf:nodeID="ffcb99037244f48d590430c228d02afdbb6">
    <owl:onProperty rdf:resource="http://emmo.info/emmo#EMMO_67fc0a36_8dcb_4ffa_9a43_31074efa3296"/>
    <rdf:type rdf:resource="http://www.w3.org/2002/07/owl#Restriction"/>
    <owl:allValuesFrom rdf:resource="http://emmo.info/emmo#EMMO_5ebd5e01_0ed3_49a2_a30d_cd05cbe72978"/>
  </rdf:Description>
  <rdf:Description rdf:about="http://emmo.info/emmo#EMMO_6c487fb3_03d1_4e56_91ed_c2e16dcbef60">
    <EMMO_967080e5_2f42_4eb2_a3a9_c58143e835f9 xml:lang="en">A mixture in which one substance of microscopically dispersed insoluble or soluble particles (from 1 nm to 1 μm) is suspended throughout another substance and that does not settle, or would take a very long time to settle appreciably.</EMMO_967080e5_2f42_4eb2_a3a9_c58143e835f9>
    <rdf:type rdf:resource="http://www.w3.org/2002/07/owl#Class"/>
    <rdfs:comment xml:lang="en">Colloids are characterized by the occurring of the Tyndall effect on light.</rdfs:comment>
    <skos:prefLabel xml:lang="en">Colloid</skos:prefLabel>
    <rdfs:subClassOf rdf:resource="http://emmo.info/emmo#EMMO_0e030040_98a7_49b2_a871_dced1f3a6131"/>
  </rdf:Description>
  <rdf:Description rdf:about="http://emmo.info/emmo#EMMO_471cb92b_edca_4cf9_bce8_a75084d876b8">
    <owl:disjointUnionOf rdf:nodeID="f05bdaa1e617a4bccafc519daf7bf4785b56"/>
    <rdfs:subClassOf rdf:resource="http://emmo.info/emmo#EMMO_7d2afa66_ae9e_4095_a9bf_421d0be401b6"/>
    <rdf:type rdf:resource="http://www.w3.org/2002/07/owl#Class"/>
    <skos:prefLabel xml:lang="en">SIMetricPrefix</skos:prefLabel>
  </rdf:Description>
  <rdf:Description rdf:nodeID="ffcb99037244f48d590430c228d02afdbb22">
    <rdf:first rdf:resource="http://emmo.info/emmo#EMMO_6a4547ab_3abb_430d_b81b_ce32d47729f5"/>
    <rdf:rest rdf:nodeID="ffcb99037244f48d590430c228d02afdbb23"/>
    <rdf:type rdf:resource="http://www.w3.org/1999/02/22-rdf-syntax-ns#List"/>
  </rdf:Description>
  <rdf:Description rdf:about="http://emmo.info/emmo#EMMO_2dd512a1_5187_47cc_b0b8_141214e22b59">
    <skos:prefLabel xml:lang="en">SolidSolidSuspension</skos:prefLabel>
    <EMMO_967080e5_2f42_4eb2_a3a9_c58143e835f9 xml:lang="en">A coarse dispersion of solid in a solid continuum phase.</EMMO_967080e5_2f42_4eb2_a3a9_c58143e835f9>
    <rdfs:subClassOf rdf:resource="http://emmo.info/emmo#EMMO_a2b006f2_bbfd_4dba_bcaa_3fca20cd6be1"/>
    <EMMO_b432d2d5_25f4_4165_99c5_5935a7763c1a xml:lang="en">Granite, sand, dried concrete.</EMMO_b432d2d5_25f4_4165_99c5_5935a7763c1a>
    <rdf:type rdf:resource="http://www.w3.org/2002/07/owl#Class"/>
  </rdf:Description>
  <rdf:Description rdf:about="http://emmo.info/emmo/middle/materials">
    <dcterms:creator>Jesper Friis</dcterms:creator>
    <dcterms:abstract xml:lang="en">European Materials &amp; Modelling Ontology (EMMO)

EMMO is a multidisciplinary effort to develop a standard representational framework (the ontology) based on current materials modelling knowledge, including physical sciences, analytical philosophy and information and communication technologies.

It provides the connection between the physical world, materials characterisation world and materials modelling world.

EMMO is released under a Creative Commons license Attribution 4.0 International (CC BY 4.0).</dcterms:abstract>
    <dcterms:contributor>University of Bologna, IT</dcterms:contributor>
    <dcterms:publisher>EMMC ASBL</dcterms:publisher>
    <dcterms:creator>Emanuele Ghedini</dcterms:creator>
    <dcterms:creator>Gerhard Goldbeck</dcterms:creator>
    <rdf:type rdf:resource="http://www.w3.org/2002/07/owl#Ontology"/>
    <rdfs:comment xml:lang="en">Contacts:
Gerhard Goldbeck
Goldbeck Consulting Ltd (UK)
email: gerhard@goldbeck-consulting.com

Emanuele Ghedini
University of Bologna (IT)
email: emanuele.ghedini@unibo.it</rdfs:comment>
    <dcterms:contributor>Goldbeck Consulting Ltd (UK)</dcterms:contributor>
    <dcterms:contributor>SINTEF, NO</dcterms:contributor>
    <dcterms:creator>Adham Hashibon</dcterms:creator>
    <rdfs:comment xml:lang="en">The EMMO requires FacT++ reasoner plugin in order to visualize all inferences and class hierarchy (ctrl+R hotkey in Protege).</rdfs:comment>
    <dcterms:title xml:lang="en">European Materials &amp; Modelling Ontology</dcterms:title>
    <dcterms:creator>Georg Schmitz</dcterms:creator>
    <dcterms:contributor>Access, DE</dcterms:contributor>
    <owl:versionIRI rdf:resource="http://emmo.info/emmo/1.0.0-beta/middle/materials"/>
    <dcterms:contributor>Fraunhofer IWM, DE</dcterms:contributor>
    <dcterms:license>https://creativecommons.org/licenses/by/4.0/legalcode</dcterms:license>
    <owl:versionInfo>1.0.0-beta</owl:versionInfo>
  </rdf:Description>
  <rdf:Description rdf:about="http://emmo.info/emmo#EMMO_03212fd7_abfd_4828_9c8e_62c293052d4b">
    <rdf:type rdf:resource="http://www.w3.org/2002/07/owl#SymmetricProperty"/>
    <EMMO_967080e5_2f42_4eb2_a3a9_c58143e835f9 xml:lang="en">The superclass for all EMMO mereotopological relations.</EMMO_967080e5_2f42_4eb2_a3a9_c58143e835f9>
    <rdfs:subPropertyOf rdf:resource="http://emmo.info/emmo#EMMO_ec2472ae_cf4a_46a5_8555_1556f5a6c3c5"/>
    <rdf:type rdf:resource="http://www.w3.org/2002/07/owl#ObjectProperty"/>
    <skos:prefLabel xml:lang="en">mereotopological</skos:prefLabel>
    <rdf:type rdf:resource="http://www.w3.org/2002/07/owl#TransitiveProperty"/>
    <rdfs:comment xml:lang="en">Mereotopology merges mereological and topological concepts and provides relations between wholes, parts, boundaries, etc.</rdfs:comment>
  </rdf:Description>
  <rdf:Description rdf:nodeID="f05bdaa1e617a4bccafc519daf7bf4785b44">
    <owl:allValuesFrom rdf:nodeID="f05bdaa1e617a4bccafc519daf7bf4785b46"/>
    <owl:onProperty rdf:nodeID="f05bdaa1e617a4bccafc519daf7bf4785b45"/>
    <rdf:type rdf:resource="http://www.w3.org/2002/07/owl#Restriction"/>
  </rdf:Description>
  <rdf:Description rdf:nodeID="fe24a777e3fd743f986ce83488d2cf30bb9">
    <owl:onProperty rdf:resource="http://emmo.info/emmo#EMMO_23b579e1_8088_45b5_9975_064014026c42"/>
    <rdf:type rdf:resource="http://www.w3.org/2002/07/owl#Restriction"/>
    <owl:hasValue>=</owl:hasValue>
  </rdf:Description>
  <rdf:Description rdf:nodeID="f05bdaa1e617a4bccafc519daf7bf4785b75">
    <rdf:type rdf:resource="http://www.w3.org/1999/02/22-rdf-syntax-ns#List"/>
    <rdf:first rdf:resource="http://emmo.info/emmo#EMMO_f5769206_9257_4b08_bf7b_dad7868c6afc"/>
    <rdf:rest rdf:resource="http://www.w3.org/1999/02/22-rdf-syntax-ns#nil"/>
  </rdf:Description>
  <rdf:Description rdf:about="http://emmo.info/emmo/middle/properties">
    <rdfs:comment xml:lang="en">The EMMO requires FacT++ reasoner plugin in order to visualize all inferences and class hierarchy (ctrl+R hotkey in Protege).</rdfs:comment>
    <dcterms:license>https://creativecommons.org/licenses/by/4.0/legalcode</dcterms:license>
    <owl:versionInfo>1.0.0-beta</owl:versionInfo>
    <dcterms:creator>Emanuele Ghedini</dcterms:creator>
    <dcterms:publisher>EMMC ASBL</dcterms:publisher>
    <dcterms:contributor>Fraunhofer IWM, DE</dcterms:contributor>
    <dcterms:contributor>Goldbeck Consulting Ltd (UK)</dcterms:contributor>
    <dcterms:creator>Gerhard Goldbeck</dcterms:creator>
    <dcterms:contributor>Access, DE</dcterms:contributor>
    <owl:versionIRI rdf:resource="http://emmo.info/emmo/1.0.0-beta/middle/properties"/>
    <dcterms:title xml:lang="en">European Materials &amp; Modelling Ontology</dcterms:title>
    <dcterms:contributor>University of Bologna, IT</dcterms:contributor>
    <dcterms:creator>Adham Hashibon</dcterms:creator>
    <dcterms:creator>Georg Schmitz</dcterms:creator>
    <rdfs:comment xml:lang="en">Contacts:
Gerhard Goldbeck
Goldbeck Consulting Ltd (UK)
email: gerhard@goldbeck-consulting.com

Emanuele Ghedini
University of Bologna (IT)
email: emanuele.ghedini@unibo.it</rdfs:comment>
    <dcterms:creator>Jesper Friis</dcterms:creator>
    <rdf:type rdf:resource="http://www.w3.org/2002/07/owl#Ontology"/>
    <dcterms:abstract xml:lang="en">European Materials &amp; Modelling Ontology (EMMO)

EMMO is a multidisciplinary effort to develop a standard representational framework (the ontology) based on current materials modelling knowledge, including physical sciences, analytical philosophy and information and communication technologies.

It provides the connection between the physical world, materials characterisation world and materials modelling world.

EMMO is released under a Creative Commons license Attribution 4.0 International (CC BY 4.0).</dcterms:abstract>
    <dcterms:contributor>SINTEF, NO</dcterms:contributor>
  </rdf:Description>
  <rdf:Description rdf:about="http://emmo.info/emmo#EMMO_b5957cef_a287_442d_a3ce_fd39f20ba1cd">
    <EMMO_967080e5_2f42_4eb2_a3a9_c58143e835f9 xml:lang="en">A 'graphical' aimed to represent a geometrical concept.</EMMO_967080e5_2f42_4eb2_a3a9_c58143e835f9>
    <rdfs:subClassOf rdf:resource="http://emmo.info/emmo#EMMO_c74da218_9147_4f03_92d1_8894abca55f3"/>
    <skos:prefLabel xml:lang="en">Geometrical</skos:prefLabel>
    <rdfs:comment xml:lang="en">A 'geometrical' stands for real world objects that express a geometrical concept.

This can be achieved in many different ways. For example, a line can be expressed by:
a) an equation like y=mx+q, which is both an 'equation' and a 'geometrical'
b) a line drawn with a pencil on a paper, which is simply a 'graphical' object
c) a set of axioms, when the properties of a line are inferred by the interpreter reading them, that are both 'graphical' and also 'formula'

The case a) is a geometrical and mathematical, b) is geometrical and pictorial, while c) is geometrical and a composition of idiomatic strings.</rdfs:comment>
    <rdf:type rdf:resource="http://www.w3.org/2002/07/owl#Class"/>
  </rdf:Description>
  <rdf:Description rdf:about="http://emmo.info/emmo#EMMO_31557fae_b039_491c_bcbb_0ccb8711d5a6">
    <rdfs:subClassOf rdf:resource="http://emmo.info/emmo#EMMO_6c487fb3_03d1_4e56_91ed_c2e16dcbef60"/>
    <EMMO_967080e5_2f42_4eb2_a3a9_c58143e835f9 xml:lang="en">A colloid in which small particles (1 nm to 100 nm) are suspended in a continuum phase.</EMMO_967080e5_2f42_4eb2_a3a9_c58143e835f9>
    <rdf:type rdf:resource="http://www.w3.org/2002/07/owl#Class"/>
    <skos:prefLabel xml:lang="en">Sol</skos:prefLabel>
  </rdf:Description>
  <rdf:Description rdf:about="http://emmo.info/emmo#EMMO_1181c938_c8f0_4ad6_bc7a_2bfdc0903d29">
    <skos:prefLabel xml:lang="en">Deci</skos:prefLabel>
    <rdfs:subClassOf rdf:nodeID="f05bdaa1e617a4bccafc519daf7bf4785b9"/>
    <rdf:type rdf:resource="http://www.w3.org/2002/07/owl#Class"/>
    <rdfs:subClassOf rdf:nodeID="f05bdaa1e617a4bccafc519daf7bf4785b12"/>
  </rdf:Description>
  <rdf:Description rdf:nodeID="ffcb99037244f48d590430c228d02afdbb41">
    <rdf:type rdf:resource="http://www.w3.org/2002/07/owl#Restriction"/>
    <owl:onProperty rdf:resource="http://emmo.info/emmo#EMMO_bed1d005_b04e_4a90_94cf_02bc678a8569"/>
    <owl:someValuesFrom rdf:resource="http://emmo.info/emmo#EMMO_33433bb1_c68f_45ee_a466_f01e2c57b214"/>
  </rdf:Description>
  <rdf:Description rdf:nodeID="f05bdaa1e617a4bccafc519daf7bf4785b182">
    <rdf:first rdf:resource="http://emmo.info/emmo#EMMO_dc232f53_8ed8_4ddd_9f41_cc057985eadb"/>
    <rdf:rest rdf:nodeID="f05bdaa1e617a4bccafc519daf7bf4785b183"/>
    <rdf:type rdf:resource="http://www.w3.org/1999/02/22-rdf-syntax-ns#List"/>
  </rdf:Description>
  <rdf:Description rdf:about="http://emmo.info/emmo#EMMO_50bf79a6_a48b_424d_9d2c_813bd631231a">
    <EMMO_1f1b164d_ec6a_4faa_8d5e_88bda62316cc>http://qudt.org/vocab/quantitykind/Length</EMMO_1f1b164d_ec6a_4faa_8d5e_88bda62316cc>
    <skos:prefLabel xml:lang="en">LuminousIntensity</skos:prefLabel>
    <EMMO_967080e5_2f42_4eb2_a3a9_c58143e835f9 xml:lang="en">A measure of the wavelength-weighted power emitted by a light source in a particular direction per unit solid angle. It is based on the luminosity function, which is a standardized model of the sensitivity of the human eye.</EMMO_967080e5_2f42_4eb2_a3a9_c58143e835f9>
    <rdf:type rdf:resource="http://www.w3.org/2002/07/owl#Class"/>
    <EMMO_de178b12_5d35_4bca_8efa_a4193162571d>T0 L0 M0 I0 Θ0 N0 J+1</EMMO_de178b12_5d35_4bca_8efa_a4193162571d>
    <EMMO_6dd685dd_1895_46e4_b227_be9f7d643c25>http://dbpedia.org/page/Luminous_intensity</EMMO_6dd685dd_1895_46e4_b227_be9f7d643c25>
  </rdf:Description>
  <rdf:Description rdf:about="http://emmo.info/emmo#EMMO_cde4368c_1d4d_4c94_8548_604749523c6d">
    <EMMO_fe015383_afb3_44a6_ae86_043628697aa2>https://doi.org/10.1351/goldbook.C01245</EMMO_fe015383_afb3_44a6_ae86_043628697aa2>
    <EMMO_1f1b164d_ec6a_4faa_8d5e_88bda62316cc>http://qudt.org/vocab/quantitykind/ElectricConductivity</EMMO_1f1b164d_ec6a_4faa_8d5e_88bda62316cc>
    <rdfs:comment xml:lang="en">Measure of a material's ability to conduct an electric current. 

Conductivity is equeal to the resiprocal of resistivity.</rdfs:comment>
    <skos:prefLabel xml:lang="en">ElectricConductivity</skos:prefLabel>
    <EMMO_de178b12_5d35_4bca_8efa_a4193162571d>T+3 L-3 M-1 I+2 Θ0 N0 J0</EMMO_de178b12_5d35_4bca_8efa_a4193162571d>
    <rdfs:subClassOf rdf:resource="http://emmo.info/emmo#EMMO_2946d40b_24a1_47fa_8176_e3f79bb45064"/>
    <skos:altLabel>Conductivity</skos:altLabel>
    <rdf:type rdf:resource="http://www.w3.org/2002/07/owl#Class"/>
    <EMMO_6dd685dd_1895_46e4_b227_be9f7d643c25>http://dbpedia.org/page/Electrical_resistivity_and_conductivity</EMMO_6dd685dd_1895_46e4_b227_be9f7d643c25>
  </rdf:Description>
  <rdf:Description rdf:about="http://emmo.info/emmo#EMMO_ffb73b1e_5786_43e4_a964_cb32ac7affb7">
    <rdfs:subClassOf rdf:resource="http://emmo.info/emmo#EMMO_2946d40b_24a1_47fa_8176_e3f79bb45064"/>
    <rdfs:comment xml:lang="en">Inverse of 'ElectricalResistance'.</rdfs:comment>
    <EMMO_6dd685dd_1895_46e4_b227_be9f7d643c25>http://dbpedia.org/page/Electrical_resistance_and_conductance</EMMO_6dd685dd_1895_46e4_b227_be9f7d643c25>
    <skos:altLabel xml:lang="en">Conductance</skos:altLabel>
    <skos:prefLabel xml:lang="en">ElectricConductance</skos:prefLabel>
    <EMMO_de178b12_5d35_4bca_8efa_a4193162571d>T+3 L-2 M-1 I+2 Θ0 N0 J0</EMMO_de178b12_5d35_4bca_8efa_a4193162571d>
    <EMMO_967080e5_2f42_4eb2_a3a9_c58143e835f9 xml:lang="en">Measure of the ease for electric current to pass through a material.</EMMO_967080e5_2f42_4eb2_a3a9_c58143e835f9>
    <EMMO_fe015383_afb3_44a6_ae86_043628697aa2>https://doi.org/10.1351/goldbook.E01925</EMMO_fe015383_afb3_44a6_ae86_043628697aa2>
    <EMMO_1f1b164d_ec6a_4faa_8d5e_88bda62316cc>http://qudt.org/vocab/quantitykind/Conductance</EMMO_1f1b164d_ec6a_4faa_8d5e_88bda62316cc>
    <rdf:type rdf:resource="http://www.w3.org/2002/07/owl#Class"/>
  </rdf:Description>
  <rdf:Description rdf:about="http://emmo.info/emmo#EMMO_99296e55_53f7_4333_9e06_760ad175a1b9">
    <EMMO_de178b12_5d35_4bca_8efa_a4193162571d>T-1 L+1 M0 I0 Θ0 N0 J0</EMMO_de178b12_5d35_4bca_8efa_a4193162571d>
    <EMMO_1f1b164d_ec6a_4faa_8d5e_88bda62316cc>http://qudt.org/vocab/constant/SpeedOfLight_Vacuum</EMMO_1f1b164d_ec6a_4faa_8d5e_88bda62316cc>
    <EMMO_6dd685dd_1895_46e4_b227_be9f7d643c25>http://dbpedia.org/page/Speed_of_light</EMMO_6dd685dd_1895_46e4_b227_be9f7d643c25>
    <skos:prefLabel xml:lang="en">SpeedOfLightInVacuum</skos:prefLabel>
    <rdf:type rdf:resource="http://www.w3.org/2002/07/owl#Class"/>
    <EMMO_fe015383_afb3_44a6_ae86_043628697aa2>https://doi.org/10.1351/goldbook.S05854</EMMO_fe015383_afb3_44a6_ae86_043628697aa2>
    <EMMO_a9b3d04c_7ceb_40a2_b8d3_28d514a770a8>https://physics.nist.gov/cgi-bin/cuu/Value?c</EMMO_a9b3d04c_7ceb_40a2_b8d3_28d514a770a8>
    <EMMO_967080e5_2f42_4eb2_a3a9_c58143e835f9 xml:lang="en">The speed of light in vacuum. Defines the base unit metre in the SI system.</EMMO_967080e5_2f42_4eb2_a3a9_c58143e835f9>
    <rdfs:subClassOf rdf:resource="http://emmo.info/emmo#EMMO_81369540_1b0e_471b_9bae_6801af22800e"/>
    <rdfs:subClassOf rdf:resource="http://emmo.info/emmo#EMMO_f2ca6dd0_0e5f_4392_a92d_cafdae6cfc95"/>
  </rdf:Description>
  <rdf:Description rdf:about="http://emmo.info/emmo#EMMO_6703954e_34c4_4a15_a9e7_f313760ae1a8">
    <skos:prefLabel xml:lang="en">connected</skos:prefLabel>
    <rdfs:comment xml:lang="en">Items being connected means that there is a topological contact or "interaction" between them.</rdfs:comment>
    <rdf:type rdf:resource="http://www.w3.org/2002/07/owl#SymmetricProperty"/>
    <rdfs:subPropertyOf rdf:resource="http://emmo.info/emmo#EMMO_03212fd7_abfd_4828_9c8e_62c293052d4b"/>
    <rdfs:comment xml:lang="en">Causality is a topological property between connected items.</rdfs:comment>
    <rdf:type rdf:resource="http://www.w3.org/2002/07/owl#ObjectProperty"/>
  </rdf:Description>
  <rdf:Description rdf:nodeID="f05bdaa1e617a4bccafc519daf7bf4785b198">
    <rdf:type rdf:resource="http://www.w3.org/1999/02/22-rdf-syntax-ns#List"/>
    <rdf:rest rdf:nodeID="f05bdaa1e617a4bccafc519daf7bf4785b199"/>
    <rdf:first rdf:resource="http://emmo.info/emmo#EMMO_d41ce84b_4317_41fb_a5d1_6cd281fca106"/>
  </rdf:Description>
  <rdf:Description rdf:nodeID="fe24a777e3fd743f986ce83488d2cf30bb3">
    <owl:onProperty rdf:resource="http://emmo.info/emmo#EMMO_faf79f53_749d_40b2_807c_d34244c192f4"/>
    <owl:allValuesFrom rdf:resource="http://www.w3.org/2001/XMLSchema#double"/>
    <rdf:type rdf:resource="http://www.w3.org/2002/07/owl#Restriction"/>
  </rdf:Description>
  <rdf:Description rdf:about="http://www.w3.org/2000/01/rdf-schema#label">
    <rdfs:range rdf:resource="http://www.w3.org/2000/01/rdf-schema#Literal"/>
  </rdf:Description>
  <rdf:Description rdf:nodeID="ff14b31ebf90e4bc5ba2839064d29e543b10">
    <rdf:type rdf:resource="http://www.w3.org/1999/02/22-rdf-syntax-ns#List"/>
    <rdf:rest rdf:nodeID="ff14b31ebf90e4bc5ba2839064d29e543b11"/>
    <rdf:first rdf:resource="http://emmo.info/emmo#EMMO_42185fe7_122c_4e0c_a3cd_659d3e21c389"/>
  </rdf:Description>
  <rdf:Description rdf:nodeID="f05bdaa1e617a4bccafc519daf7bf4785b116">
    <owl:hasValue>Pa</owl:hasValue>
    <rdf:type rdf:resource="http://www.w3.org/2002/07/owl#Restriction"/>
    <owl:onProperty rdf:resource="http://emmo.info/emmo#EMMO_23b579e1_8088_45b5_9975_064014026c42"/>
  </rdf:Description>
  <rdf:Description rdf:about="http://emmo.info/emmo#EMMO_09007bc0_b5f2_4fb9_af01_caf948cf2044">
    <rdf:type rdf:resource="http://www.w3.org/2002/07/owl#Class"/>
    <skos:prefLabel xml:lang="en">Java</skos:prefLabel>
    <rdfs:subClassOf rdf:resource="http://emmo.info/emmo#EMMO_8681074a_e225_4e38_b586_e85b0f43ce38"/>
  </rdf:Description>
  <rdf:Description rdf:about="http://emmo.info/emmo#EMMO_7afbed84_7593_4a23_bd88_9d9c6b04e8f6">
    <rdf:type rdf:resource="http://www.w3.org/2002/07/owl#TransitiveProperty"/>
    <skos:prefLabel xml:lang="en">hasTemporalPart</skos:prefLabel>
    <rdfs:range rdf:resource="http://emmo.info/emmo#EMMO_eb3a768e_d53e_4be9_a23b_0714833c36de"/>
    <rdf:type rdf:resource="http://www.w3.org/2002/07/owl#ObjectProperty"/>
    <rdfs:subPropertyOf rdf:resource="http://emmo.info/emmo#EMMO_9380ab64_0363_4804_b13f_3a8a94119a76"/>
    <rdfs:domain rdf:resource="http://emmo.info/emmo#EMMO_eb3a768e_d53e_4be9_a23b_0714833c36de"/>
    <EMMO_967080e5_2f42_4eb2_a3a9_c58143e835f9>A relation that isolate a proper part that covers the total spatial extension of a whole within a time interval.</EMMO_967080e5_2f42_4eb2_a3a9_c58143e835f9>
  </rdf:Description>
  <rdf:Description rdf:about="http://emmo.info/emmo#EMMO_affe07e4_e9bc_4852_86c6_69e26182a17f">
    <skos:prefLabel xml:lang="en">ThermodynamicTemperature</skos:prefLabel>
    <rdf:type rdf:resource="http://www.w3.org/2002/07/owl#Class"/>
    <EMMO_6dd685dd_1895_46e4_b227_be9f7d643c25>http://dbpedia.org/page/Thermodynamic_temperature</EMMO_6dd685dd_1895_46e4_b227_be9f7d643c25>
    <EMMO_967080e5_2f42_4eb2_a3a9_c58143e835f9 xml:lang="en">Thermodynamic temperature is the absolute measure of temperature. It is defined by the third law of thermodynamics in which the theoretically lowest temperature is the null or zero point.</EMMO_967080e5_2f42_4eb2_a3a9_c58143e835f9>
    <EMMO_de178b12_5d35_4bca_8efa_a4193162571d>T0 L0 M0 I0 Θ+1 N0 J0</EMMO_de178b12_5d35_4bca_8efa_a4193162571d>
    <EMMO_fe015383_afb3_44a6_ae86_043628697aa2>https://doi.org/10.1351/goldbook.T06321</EMMO_fe015383_afb3_44a6_ae86_043628697aa2>
    <EMMO_1f1b164d_ec6a_4faa_8d5e_88bda62316cc>qudt.org/vocab/quantitykind/ThermodynamicTemperature</EMMO_1f1b164d_ec6a_4faa_8d5e_88bda62316cc>
  </rdf:Description>
  <rdf:Description rdf:about="http://emmo.info/emmo#EMMO_9cb984ca_48ad_4864_b09e_50d3fff19420">
    <rdf:type rdf:resource="http://www.w3.org/2002/07/owl#SymmetricProperty"/>
    <skos:prefLabel xml:lang="en">overcrosses</skos:prefLabel>
    <rdf:type rdf:resource="http://www.w3.org/2002/07/owl#ObjectProperty"/>
    <rdfs:subPropertyOf rdf:resource="http://emmo.info/emmo#EMMO_d893d373_b579_4867_841e_1c2b31a8d2c6"/>
  </rdf:Description>
  <rdf:Description rdf:nodeID="fc2fcd8f8eb3649bcbbaff76ba54058acb1">
    <owl:allValuesFrom rdf:resource="http://emmo.info/emmo#EMMO_0f795e3e_c602_4577_9a43_d5a231aa1360"/>
    <rdf:type rdf:resource="http://www.w3.org/2002/07/owl#Restriction"/>
    <owl:onProperty rdf:resource="http://emmo.info/emmo#EMMO_7afbed84_7593_4a23_bd88_9d9c6b04e8f6"/>
  </rdf:Description>
  <rdf:Description rdf:about="http://emmo.info/emmo#EMMO_2fd3f574_5e93_47fe_afca_ed80b0a21ab4">
    <rdfs:subClassOf rdf:resource="http://emmo.info/emmo#EMMO_eb77076b_a104_42ac_a065_798b2d2809ad"/>
    <skos:prefLabel xml:lang="en">StandaloneAtom</skos:prefLabel>
    <EMMO_967080e5_2f42_4eb2_a3a9_c58143e835f9 xml:lang="en">An atom that does not share electrons with other atoms.</EMMO_967080e5_2f42_4eb2_a3a9_c58143e835f9>
    <rdfs:comment xml:lang="en">A standalone atom can be bonded with other atoms by intermolecular forces (i.e. dipole–dipole, London dispersion force, hydrogen bonding), since this bonds does not involve electron sharing.</rdfs:comment>
    <owl:disjointUnionOf rdf:nodeID="ff14b31ebf90e4bc5ba2839064d29e543b6"/>
    <rdf:type rdf:resource="http://www.w3.org/2002/07/owl#Class"/>
  </rdf:Description>
  <rdf:Description rdf:about="http://emmo.info/emmo#EMMO_f19ff3b4_6bfe_4c41_a2b2_9affd39c140b">
    <rdfs:subClassOf rdf:resource="http://emmo.info/emmo#EMMO_db9a009e_f097_43f5_9520_6cbc07e7610b"/>
    <rdf:type rdf:resource="http://www.w3.org/2002/07/owl#Class"/>
    <skos:prefLabel xml:lang="en">MaterialLaw</skos:prefLabel>
  </rdf:Description>
  <rdf:Description rdf:nodeID="f05bdaa1e617a4bccafc519daf7bf4785b178">
    <rdf:rest rdf:nodeID="f05bdaa1e617a4bccafc519daf7bf4785b179"/>
    <rdf:type rdf:resource="http://www.w3.org/1999/02/22-rdf-syntax-ns#List"/>
    <rdf:first rdf:resource="http://emmo.info/emmo#EMMO_cf3dd6cc_c5d6_4b3d_aef4_82f3b7a361af"/>
  </rdf:Description>
  <rdf:Description rdf:about="http://emmo.info/emmo#EMMO_8ef3cd6d_ae58_4a8d_9fc0_ad8f49015cd0">
    <rdfs:subPropertyOf rdf:resource="http://emmo.info/emmo#EMMO_b2282816_b7a3_44c6_b2cb_3feff1ceb7fe"/>
    <rdf:type rdf:resource="http://www.w3.org/2002/07/owl#IrreflexiveProperty"/>
    <rdf:type rdf:resource="http://www.w3.org/2002/07/owl#AsymmetricProperty"/>
    <rdfs:range rdf:resource="http://emmo.info/emmo#EMMO_4ce76d7f_03f8_45b6_9003_90052a79bfaa"/>
    <skos:prefLabel xml:lang="en">hasQuantityValue</skos:prefLabel>
    <rdf:type rdf:resource="http://www.w3.org/2002/07/owl#InverseFunctionalProperty"/>
    <rdfs:comment xml:lang="en">Relates a quantity to its reference unit through spatial direct parthood.</rdfs:comment>
    <rdf:type rdf:resource="http://www.w3.org/2002/07/owl#ObjectProperty"/>
    <rdfs:domain rdf:resource="http://emmo.info/emmo#EMMO_f658c301_ce93_46cf_9639_4eace2c5d1d5"/>
  </rdf:Description>
  <rdf:Description rdf:nodeID="fe0b20157736f4a31909181349b2e6219b29">
    <owl:onProperty rdf:resource="http://emmo.info/emmo#EMMO_23b579e1_8088_45b5_9975_064014026c42"/>
    <owl:hasValue>T+1 L0 M0 I+1 Θ0 N0 J0</owl:hasValue>
    <rdf:type rdf:resource="http://www.w3.org/2002/07/owl#Restriction"/>
  </rdf:Description>
  <rdf:Description rdf:about="http://emmo.info/emmo#EMMO_1a179ce4_3724_47f8_bee5_6292e3ac9942">
    <EMMO_e55f2d7c_9893_48cd_b4a4_fdf38253bd20>http://www.ontology-of-units-of-measure.org/resource/om-2/ElectricDipoleMoment</EMMO_e55f2d7c_9893_48cd_b4a4_fdf38253bd20>
    <EMMO_6dd685dd_1895_46e4_b227_be9f7d643c25>http://dbpedia.org/page/Electric_dipole_moment</EMMO_6dd685dd_1895_46e4_b227_be9f7d643c25>
    <EMMO_50c298c2_55a2_4068_b3ac_4e948c33181f>http://www.electropedia.org/iev/iev.nsf/display?openform&amp;ievref=121-11-36</EMMO_50c298c2_55a2_4068_b3ac_4e948c33181f>
    <EMMO_1f1b164d_ec6a_4faa_8d5e_88bda62316cc>http://qudt.org/vocab/quantitykind/ElectricDipoleMoment</EMMO_1f1b164d_ec6a_4faa_8d5e_88bda62316cc>
    <rdfs:subClassOf rdf:resource="http://emmo.info/emmo#EMMO_2946d40b_24a1_47fa_8176_e3f79bb45064"/>
    <EMMO_967080e5_2f42_4eb2_a3a9_c58143e835f9 xml:lang="en">An electric dipole, vector quantity of magnitude equal to the product of the positive charge and the distance between the charges and directed from the negative charge to the positive charge.</EMMO_967080e5_2f42_4eb2_a3a9_c58143e835f9>
    <EMMO_50c298c2_55a2_4068_b3ac_4e948c33181f>http://www.electropedia.org/iev/iev.nsf/display?openform&amp;ievref=121-11-35</EMMO_50c298c2_55a2_4068_b3ac_4e948c33181f>
    <rdf:type rdf:resource="http://www.w3.org/2002/07/owl#Class"/>
    <EMMO_fe015383_afb3_44a6_ae86_043628697aa2>https://doi.org/10.1351/goldbook.E01929</EMMO_fe015383_afb3_44a6_ae86_043628697aa2>
    <skos:prefLabel xml:lang="en">ElectricDipoleMoment</skos:prefLabel>
    <EMMO_de178b12_5d35_4bca_8efa_a4193162571d>T+1 L+1 M0 I+1 Θ0 N0 J0</EMMO_de178b12_5d35_4bca_8efa_a4193162571d>
  </rdf:Description>
  <rdf:Description rdf:about="http://emmo.info/emmo/middle/math">
    <rdfs:comment xml:lang="en">Contacts:
Gerhard Goldbeck
Goldbeck Consulting Ltd (UK)
email: gerhard@goldbeck-consulting.com

Emanuele Ghedini
University of Bologna (IT)
email: emanuele.ghedini@unibo.it</rdfs:comment>
    <dcterms:creator>Adham Hashibon</dcterms:creator>
    <owl:versionIRI rdf:resource="http://emmo.info/emmo/1.0.0-beta/middle/math"/>
    <dcterms:title xml:lang="en">European Materials &amp; Modelling Ontology</dcterms:title>
    <rdfs:comment xml:lang="en">The EMMO requires FacT++ reasoner plugin in order to visualize all inferences and class hierarchy (ctrl+R hotkey in Protege).</rdfs:comment>
    <dcterms:contributor>Access, DE</dcterms:contributor>
    <dcterms:creator>Georg Schmitz</dcterms:creator>
    <owl:versionInfo>1.0.0-beta</owl:versionInfo>
    <dcterms:creator>Jesper Friis</dcterms:creator>
    <dcterms:contributor>Fraunhofer IWM, DE</dcterms:contributor>
    <dcterms:license>https://creativecommons.org/licenses/by/4.0/legalcode</dcterms:license>
    <dcterms:abstract xml:lang="en">European Materials &amp; Modelling Ontology (EMMO)

EMMO is a multidisciplinary effort to develop a standard representational framework (the ontology) based on current materials modelling knowledge, including physical sciences, analytical philosophy and information and communication technologies.

It provides the connection between the physical world, materials characterisation world and materials modelling world.

EMMO is released under a Creative Commons license Attribution 4.0 International (CC BY 4.0).</dcterms:abstract>
    <dcterms:contributor>Goldbeck Consulting Ltd (UK)</dcterms:contributor>
    <dcterms:contributor>University of Bologna, IT</dcterms:contributor>
    <rdf:type rdf:resource="http://www.w3.org/2002/07/owl#Ontology"/>
    <dcterms:publisher>EMMC ASBL</dcterms:publisher>
    <dcterms:creator>Emanuele Ghedini</dcterms:creator>
    <dcterms:creator>Gerhard Goldbeck</dcterms:creator>
    <dcterms:contributor>SINTEF, NO</dcterms:contributor>
  </rdf:Description>
  <rdf:Description rdf:nodeID="f627ff42579444148ae27fcacfb5f8528b10">
    <owl:intersectionOf rdf:nodeID="f627ff42579444148ae27fcacfb5f8528b11"/>
    <rdf:type rdf:resource="http://www.w3.org/2002/07/owl#Class"/>
  </rdf:Description>
  <rdf:Description rdf:nodeID="f8fb83657cd5f496db3c2b94baf326f26b3">
    <rdf:rest rdf:resource="http://www.w3.org/1999/02/22-rdf-syntax-ns#nil"/>
    <rdf:first rdf:resource="http://emmo.info/emmo#EMMO_acaaa124_3dde_48b6_86e6_6ec6f364f408"/>
    <rdf:type rdf:resource="http://www.w3.org/1999/02/22-rdf-syntax-ns#List"/>
  </rdf:Description>
  <rdf:Description rdf:about="http://emmo.info/emmo/middle/models">
    <dcterms:title xml:lang="en">European Materials &amp; Modelling Ontology</dcterms:title>
    <dcterms:abstract xml:lang="en">European Materials &amp; Modelling Ontology (EMMO)

EMMO is a multidisciplinary effort to develop a standard representational framework (the ontology) based on current materials modelling knowledge, including physical sciences, analytical philosophy and information and communication technologies.

It provides the connection between the physical world, materials characterisation world and materials modelling world.

EMMO is released under a Creative Commons license Attribution 4.0 International (CC BY 4.0).</dcterms:abstract>
    <dcterms:creator>Emanuele Ghedini</dcterms:creator>
    <owl:versionInfo>1.0.0-beta</owl:versionInfo>
    <dcterms:creator>Jesper Friis</dcterms:creator>
    <rdfs:comment xml:lang="en">Contacts:
Gerhard Goldbeck
Goldbeck Consulting Ltd (UK)
email: gerhard@goldbeck-consulting.com

Emanuele Ghedini
University of Bologna (IT)
email: emanuele.ghedini@unibo.it</rdfs:comment>
    <dcterms:contributor>Fraunhofer IWM, DE</dcterms:contributor>
    <rdf:type rdf:resource="http://www.w3.org/2002/07/owl#Ontology"/>
    <dcterms:publisher>EMMC ASBL</dcterms:publisher>
    <dcterms:creator>Adham Hashibon</dcterms:creator>
    <dcterms:contributor>Goldbeck Consulting Ltd (UK)</dcterms:contributor>
    <dcterms:contributor>SINTEF, NO</dcterms:contributor>
    <dcterms:license>https://creativecommons.org/licenses/by/4.0/legalcode</dcterms:license>
    <rdfs:comment xml:lang="en">The EMMO requires FacT++ reasoner plugin in order to visualize all inferences and class hierarchy (ctrl+R hotkey in Protege).</rdfs:comment>
    <dcterms:creator>Gerhard Goldbeck</dcterms:creator>
    <dcterms:contributor>Access, DE</dcterms:contributor>
    <owl:versionIRI rdf:resource="http://emmo.info/emmo/1.0.0-beta/middle/models"/>
    <dcterms:creator>Georg Schmitz</dcterms:creator>
    <dcterms:contributor>University of Bologna, IT</dcterms:contributor>
  </rdf:Description>
  <rdf:Description rdf:about="http://emmo.info/emmo#EMMO_1e7603a7_1365_49b8_b5e5_3711c8e6b904">
    <rdf:type rdf:resource="http://www.w3.org/2002/07/owl#Class"/>
    <EMMO_6dd685dd_1895_46e4_b227_be9f7d643c25>http://dbpedia.org/page/Vergence</EMMO_6dd685dd_1895_46e4_b227_be9f7d643c25>
    <rdfs:subClassOf rdf:resource="http://emmo.info/emmo#EMMO_2946d40b_24a1_47fa_8176_e3f79bb45064"/>
    <skos:prefLabel xml:lang="en">Vergence</skos:prefLabel>
    <EMMO_de178b12_5d35_4bca_8efa_a4193162571d>T0 L-1 M0 I0 Θ0 N0 J0</EMMO_de178b12_5d35_4bca_8efa_a4193162571d>
    <rdfs:comment xml:lang="en">In geometrical optics, vergence describes the curvature of optical wavefronts.</rdfs:comment>
  </rdf:Description>
  <rdf:Description rdf:nodeID="fea11ca01461e402d8f697c19c5d8de88b6">
    <rdf:rest rdf:resource="http://www.w3.org/1999/02/22-rdf-syntax-ns#nil"/>
    <rdf:type rdf:resource="http://www.w3.org/1999/02/22-rdf-syntax-ns#List"/>
    <rdf:first rdf:nodeID="fea11ca01461e402d8f697c19c5d8de88b7"/>
  </rdf:Description>
  <rdf:Description rdf:nodeID="fdb1489b80bcc4ee28afe0be8feb9b935b1">
    <owl:someValuesFrom rdf:resource="http://emmo.info/emmo#EMMO_1b52ee70_121e_4d8d_8419_3f97cd0bd89c"/>
    <owl:onProperty rdf:resource="http://emmo.info/emmo#EMMO_ae2d1a96_bfa1_409a_a7d2_03d69e8a125a"/>
    <rdf:type rdf:resource="http://www.w3.org/2002/07/owl#Restriction"/>
  </rdf:Description>
  <rdf:Description rdf:about="http://emmo.info/emmo#EMMO_6b7276a4_4b9d_440a_b577_0277539c0fc4">
    <rdfs:subPropertyOf rdf:resource="http://emmo.info/emmo#EMMO_9380ab64_0363_4804_b13f_3a8a94119a76"/>
    <rdfs:domain rdf:resource="http://emmo.info/emmo#EMMO_2d2ecd97_067f_4d0e_950c_d746b7700a31"/>
    <rdf:type rdf:resource="http://www.w3.org/2002/07/owl#IrreflexiveProperty"/>
    <rdf:type rdf:resource="http://www.w3.org/2002/07/owl#AsymmetricProperty"/>
    <skos:prefLabel xml:lang="en">hasMember</skos:prefLabel>
    <rdfs:range rdf:resource="http://emmo.info/emmo#EMMO_eb3a768e_d53e_4be9_a23b_0714833c36de"/>
    <rdf:type rdf:resource="http://www.w3.org/2002/07/owl#ObjectProperty"/>
  </rdf:Description>
  <rdf:Description rdf:about="http://emmo.info/emmo#EMMO_daa9ee97_4c5f_42e5_918c_44d7523e8958">
    <rdfs:subClassOf rdf:nodeID="f05bdaa1e617a4bccafc519daf7bf4785b146"/>
    <skos:prefLabel xml:lang="en">Zetta</skos:prefLabel>
    <rdfs:subClassOf rdf:nodeID="f05bdaa1e617a4bccafc519daf7bf4785b143"/>
    <rdf:type rdf:resource="http://www.w3.org/2002/07/owl#Class"/>
  </rdf:Description>
  <rdf:Description rdf:about="http://emmo.info/emmo/middle/units-extension">
    <owl:versionInfo>1.0.0-beta</owl:versionInfo>
    <rdfs:comment xml:lang="en">Contacts:
Gerhard Goldbeck
Goldbeck Consulting Ltd (UK)
email: gerhard@goldbeck-consulting.com

Emanuele Ghedini
University of Bologna (IT)
email: emanuele.ghedini@unibo.it</rdfs:comment>
    <dcterms:creator>Jesper Friis</dcterms:creator>
    <dcterms:contributor>Fraunhofer IWM, DE</dcterms:contributor>
    <dcterms:abstract xml:lang="en">European Materials &amp; Modelling Ontology (EMMO)

EMMO is a multidisciplinary effort to develop a standard representational framework (the ontology) based on current materials modelling knowledge, including physical sciences, analytical philosophy and information and communication technologies.

It provides the connection between the physical world, materials characterisation world and materials modelling world.

EMMO is released under a Creative Commons license Attribution 4.0 International (CC BY 4.0).</dcterms:abstract>
    <dcterms:creator>Adham Hashibon</dcterms:creator>
    <dcterms:creator>Emanuele Ghedini</dcterms:creator>
    <rdfs:comment xml:lang="en">The EMMO requires FacT++ reasoner plugin in order to visualize all inferences and class hierarchy (ctrl+R hotkey in Protege).</rdfs:comment>
    <rdf:type rdf:resource="http://www.w3.org/2002/07/owl#Ontology"/>
    <dcterms:publisher>EMMC ASBL</dcterms:publisher>
    <dcterms:creator>Gerhard Goldbeck</dcterms:creator>
    <dcterms:contributor>Access, DE</dcterms:contributor>
    <dcterms:contributor>SINTEF, NO</dcterms:contributor>
    <dcterms:contributor>Goldbeck Consulting Ltd (UK)</dcterms:contributor>
    <dcterms:license>https://creativecommons.org/licenses/by/4.0/legalcode</dcterms:license>
    <dcterms:creator>Georg Schmitz</dcterms:creator>
    <dcterms:contributor>University of Bologna, IT</dcterms:contributor>
    <owl:versionIRI rdf:resource="http://emmo.info/emmo/1.0.0-beta/middle/units-extension"/>
    <dcterms:title xml:lang="en">European Materials &amp; Modelling Ontology</dcterms:title>
  </rdf:Description>
  <rdf:Description rdf:about="http://emmo.info/emmo#EMMO_52e4cb25_da39_45e2_a6db_063ec5730499">
    <EMMO_c84c6752_6d64_48cc_9500_e54a3c34898d>https://en.wikipedia.org/wiki/Centimetre%E2%80%93gram%E2%80%93second_system_of_units</EMMO_c84c6752_6d64_48cc_9500_e54a3c34898d>
    <rdfs:subClassOf rdf:resource="http://emmo.info/emmo#EMMO_b081b346_7279_46ef_9a3d_2c088fcd79f4"/>
    <EMMO_967080e5_2f42_4eb2_a3a9_c58143e835f9 xml:lang="en">The centimetre–gram–second (CGS) system of units.</EMMO_967080e5_2f42_4eb2_a3a9_c58143e835f9>
    <rdf:type rdf:resource="http://www.w3.org/2002/07/owl#Class"/>
    <skos:prefLabel xml:lang="en">CGSUnit</skos:prefLabel>
    <rdfs:comment xml:lang="en">CGS is a variant of the metric system.</rdfs:comment>
  </rdf:Description>
  <rdf:Description rdf:about="http://emmo.info/emmo#EMMO_3c424d37_cf62_41b1_ac9d_a316f8d113d6">
    <rdf:type rdf:resource="http://www.w3.org/2002/07/owl#Class"/>
    <skos:prefLabel xml:lang="en">AlgebricOperator</skos:prefLabel>
    <rdfs:subClassOf rdf:resource="http://emmo.info/emmo#EMMO_f6d0c26a_98b6_4cf8_8632_aa259131faaa"/>
  </rdf:Description>
  <rdf:Description rdf:about="http://emmo.info/emmo#EMMO_59c10c5c_47bd_4348_ba39_38836607dfa1">
    <rdfs:subClassOf rdf:nodeID="f05bdaa1e617a4bccafc519daf7bf4785b77"/>
    <EMMO_1f1b164d_ec6a_4faa_8d5e_88bda62316cc>http://qudt.org/vocab/unit/OHM</EMMO_1f1b164d_ec6a_4faa_8d5e_88bda62316cc>
    <skos:prefLabel xml:lang="en">Ohm</skos:prefLabel>
    <rdfs:comment xml:lang="en">Measurement unit for resistance.</rdfs:comment>
    <rdfs:subClassOf rdf:nodeID="f05bdaa1e617a4bccafc519daf7bf4785b76"/>
    <EMMO_fe015383_afb3_44a6_ae86_043628697aa2>https://doi.org/10.1351/goldbook.O04280</EMMO_fe015383_afb3_44a6_ae86_043628697aa2>
    <rdf:type rdf:resource="http://www.w3.org/2002/07/owl#Class"/>
  </rdf:Description>
  <rdf:Description rdf:nodeID="f05bdaa1e617a4bccafc519daf7bf4785b101">
    <owl:someValuesFrom rdf:resource="http://emmo.info/emmo#EMMO_14ff4393_0f28_4fb4_abc7_c2cc00bc761d"/>
    <owl:onProperty rdf:resource="http://emmo.info/emmo#EMMO_bed1d005_b04e_4a90_94cf_02bc678a8569"/>
    <rdf:type rdf:resource="http://www.w3.org/2002/07/owl#Restriction"/>
  </rdf:Description>
  <rdf:Description rdf:about="http://emmo.info/emmo#EMMO_f76f5a24_d703_4e8c_b368_f9a7777cb73a">
    <skos:prefLabel xml:lang="en">AmountFractionUnit</skos:prefLabel>
    <rdfs:subClassOf rdf:resource="http://emmo.info/emmo#EMMO_c2f5ee66_579c_44c6_a2e9_fa2eaa9fa4da"/>
    <rdf:type rdf:resource="http://www.w3.org/2002/07/owl#Class"/>
    <EMMO_b432d2d5_25f4_4165_99c5_5935a7763c1a xml:lang="en">Unit for amount fraction.</EMMO_b432d2d5_25f4_4165_99c5_5935a7763c1a>
    <EMMO_967080e5_2f42_4eb2_a3a9_c58143e835f9 xml:lang="en">Unit for quantities of dimension one that are the fraction of two amount of substance.</EMMO_967080e5_2f42_4eb2_a3a9_c58143e835f9>
  </rdf:Description>
  <rdf:Description rdf:about="http://emmo.info/emmo#EMMO_a155dc93_d266_487e_b5e7_2a2c72d5ebf9">
    <rdfs:subClassOf rdf:nodeID="ffcb99037244f48d590430c228d02afdbb37"/>
    <EMMO_70fe84ff_99b6_4206_a9fc_9a8931836d84 xml:lang="en">A non-SI unit of volume defined as 1 cubic decimetre (dm3),</EMMO_70fe84ff_99b6_4206_a9fc_9a8931836d84>
    <EMMO_fe015383_afb3_44a6_ae86_043628697aa2>https://doi.org/10.1351/goldbook.L03594</EMMO_fe015383_afb3_44a6_ae86_043628697aa2>
    <rdfs:subClassOf rdf:nodeID="ffcb99037244f48d590430c228d02afdbb38"/>
    <rdf:type rdf:resource="http://www.w3.org/2002/07/owl#Class"/>
    <rdfs:subClassOf rdf:resource="http://emmo.info/emmo#EMMO_591e02fd_8d37_45a6_9d11_bb21cef391a0"/>
    <EMMO_1f1b164d_ec6a_4faa_8d5e_88bda62316cc>http://qudt.org/vocab/unit/L</EMMO_1f1b164d_ec6a_4faa_8d5e_88bda62316cc>
    <skos:prefLabel xml:lang="en">Litre</skos:prefLabel>
  </rdf:Description>
  <rdf:Description rdf:nodeID="ffcb99037244f48d590430c228d02afdbb31">
    <owl:onProperty rdf:resource="http://emmo.info/emmo#EMMO_bed1d005_b04e_4a90_94cf_02bc678a8569"/>
    <rdf:type rdf:resource="http://www.w3.org/2002/07/owl#Restriction"/>
    <owl:someValuesFrom rdf:resource="http://emmo.info/emmo#EMMO_3227b821_26a5_4c7c_9c01_5c24483e0bd0"/>
  </rdf:Description>
  <rdf:Description rdf:about="http://emmo.info/emmo#EMMO_f6d0c26a_98b6_4cf8_8632_aa259131faaa">
    <rdf:type rdf:resource="http://www.w3.org/2002/07/owl#Class"/>
    <skos:prefLabel xml:lang="en">MathematicalOperator</skos:prefLabel>
    <rdfs:subClassOf rdf:resource="http://emmo.info/emmo#EMMO_54ee6b5e_5261_44a8_86eb_5717e7fdb9d0"/>
    <rdfs:subClassOf rdf:resource="http://emmo.info/emmo#EMMO_a1083d0a_c1fb_471f_8e20_a98f881ad527"/>
  </rdf:Description>
  <rdf:Description rdf:about="http://emmo.info/emmo#EMMO_49267eba_5548_4163_8f36_518d65b583f9">
    <EMMO_967080e5_2f42_4eb2_a3a9_c58143e835f9 xml:lang="en">The class of individuals that stand for real world objects according to a specific representational perspective.</EMMO_967080e5_2f42_4eb2_a3a9_c58143e835f9>
    <rdf:type rdf:resource="http://www.w3.org/2002/07/owl#Class"/>
    <rdfs:subClassOf rdf:resource="http://emmo.info/emmo#EMMO_c5ddfdba_c074_4aa4_ad6b_1ac4942d300d"/>
    <rdfs:comment xml:lang="en">This class is the practical implementation of the EMMO pluralistic approach for which the only objective categorization is provided by the Universe individual and all the Quantum individuals.

Between these two extremes, there are several subjective ways to categorize real world objects, each one provide under a 'Perspective' subclass.</rdfs:comment>
    <skos:prefLabel xml:lang="en">Perspective</skos:prefLabel>
  </rdf:Description>
  <rdf:Description rdf:about="http://emmo.info/emmo#EMMO_3f15d200_c97b_42c8_8ac0_d81d150361e2">
    <rdf:type rdf:resource="http://www.w3.org/2002/07/owl#Class"/>
    <skos:prefLabel xml:lang="en">MeasuredConstant</skos:prefLabel>
    <EMMO_967080e5_2f42_4eb2_a3a9_c58143e835f9 xml:lang="en">For a given unit system, measured constants are physical constants that are not used to define the unit system. Hence, these constants have to be measured and will therefore be associated with an uncertainty.</EMMO_967080e5_2f42_4eb2_a3a9_c58143e835f9>
  </rdf:Description>
  <rdf:Description rdf:nodeID="ffcb99037244f48d590430c228d02afdbb8">
    <owl:onProperty rdf:resource="http://emmo.info/emmo#EMMO_23b579e1_8088_45b5_9975_064014026c42"/>
    <rdf:type rdf:resource="http://www.w3.org/2002/07/owl#Restriction"/>
    <owl:hasValue>′</owl:hasValue>
  </rdf:Description>
  <rdf:Description rdf:about="http://emmo.info/emmo#EMMO_b7bcff25_ffc3_474e_9ab5_01b1664bd4ba">
    <skos:prefLabel xml:lang="en">Property</skos:prefLabel>
    <rdfs:comment xml:lang="en">We know real world entities through observation/perception.

A non-perceivable real world entity does not exist (or it exists on a plane of existance that has no intersection with us and we can say nothing about it).

Perception/observation of a real wolrd entity occurs when the entity stimulate an observer in a peculiar way through a well defined perception channel.

For this reason each property is related to a specific observation process which involves a specific observer with its own perception mechanisms.

The observation process (e.g. a look, a photo shot, a measurement) is performed  by an observer (e.g. you, a camera, an instrument) through a specific perception mechanism (e.g. retina impression, CMOS excitation, piezoelectric sensor activation) and involves an observed entity.

An observation is a semiotic process, since it stimulate an interpretant within the interpreter who can communicate the perception result to other interpreters through a sign which is the property. 

Property subclasses are specializations that depend on the type of observation processes.

e.g. the property 'colour' is related to a process that involves emission or interaction of photon and an observer who can perceive electromagnetic radiation in the visible frequency range. 

Properties usually relies on symbolic systems (e.g. for colour it can be palette or RGB).</rdfs:comment>
    <rdfs:comment xml:lang="en">A 'Property' is a sort of name or label that we put upon objects that interact with an observer in the same specific way.

e.g. "hot" objects are objects that interact with an observer through a perception mechanism aimed to perceive an heat source.</rdfs:comment>
    <EMMO_b432d2d5_25f4_4165_99c5_5935a7763c1a xml:lang="en">Hardness is a subclass of properties.

Vickers hardness is a subclass of hardness that involves the procedures and instruments defined by the standard hardness test.</EMMO_b432d2d5_25f4_4165_99c5_5935a7763c1a>
    <EMMO_b432d2d5_25f4_4165_99c5_5935a7763c1a xml:lang="en">Let's define the class 'colour' as the subclass of the properties that involve photon emission and an electromagnetic radiation sensible observer.

An individual C of this class 'colour' can be defined be declaring the process individual (e.g. daylight illumination) and the observer (e.g. my eyes)

Stating that an entity E hasProperty C, we mean that it can be observed by such setup of process + observer (i.e. observed by my eyes under daylight).

This definition can be generalized by using a generic human eye, so that the observer can be a generic human.

This can be used in material characterization, to define exactly the type of measurement done, including the instrument type.</EMMO_b432d2d5_25f4_4165_99c5_5935a7763c1a>
    <rdf:type rdf:resource="http://www.w3.org/2002/07/owl#Class"/>
    <rdfs:subClassOf rdf:nodeID="fdb1489b80bcc4ee28afe0be8feb9b935b9"/>
    <owl:disjointUnionOf rdf:nodeID="fdb1489b80bcc4ee28afe0be8feb9b935b11"/>
    <rdfs:subClassOf rdf:nodeID="fdb1489b80bcc4ee28afe0be8feb9b935b7"/>
    <EMMO_967080e5_2f42_4eb2_a3a9_c58143e835f9 xml:lang="en">A 'Perceptual' referring to a specific code that is used as 'Conventional' sign to represent an 'Object' according to a specific interaction mechanism by an 'Observer'.

(A property is always a partial representation of an 'Object' since it reflects the 'Object' capability to be part of a specific 'Observation' process)</EMMO_967080e5_2f42_4eb2_a3a9_c58143e835f9>
    <rdfs:subClassOf rdf:resource="http://emmo.info/emmo#EMMO_35d2e130_6e01_41ed_94f7_00b333d46cf9"/>
  </rdf:Description>
  <rdf:Description rdf:about="http://emmo.info/emmo#EMMO_f3dd74c0_f480_49e8_9764_33b78638c235">
    <skos:prefLabel xml:lang="en">Angle</skos:prefLabel>
    <EMMO_70fe84ff_99b6_4206_a9fc_9a8931836d84 xml:lang="en">Ratio of circular arc length to radius.</EMMO_70fe84ff_99b6_4206_a9fc_9a8931836d84>
    <rdfs:subClassOf rdf:nodeID="ffcb99037244f48d590430c228d02afdbb55"/>
    <skos:altLabel xml:lang="en">PlaneAngle</skos:altLabel>
    <EMMO_1f1b164d_ec6a_4faa_8d5e_88bda62316cc>http://qudt.org/vocab/quantitykind/PlaneAngle</EMMO_1f1b164d_ec6a_4faa_8d5e_88bda62316cc>
    <EMMO_6dd685dd_1895_46e4_b227_be9f7d643c25>http://dbpedia.org/page/Angle</EMMO_6dd685dd_1895_46e4_b227_be9f7d643c25>
    <rdfs:subClassOf rdf:resource="http://emmo.info/emmo#EMMO_faab3f84_e475_4a46_af9c_7d249f0b9aef"/>
    <rdf:type rdf:resource="http://www.w3.org/2002/07/owl#Class"/>
    <EMMO_fe015383_afb3_44a6_ae86_043628697aa2>https://doi.org/10.1351/goldbook.A00346</EMMO_fe015383_afb3_44a6_ae86_043628697aa2>
    <EMMO_de178b12_5d35_4bca_8efa_a4193162571d>T0 L0 M0 I0 Θ0 N0 J0</EMMO_de178b12_5d35_4bca_8efa_a4193162571d>
  </rdf:Description>
  <rdf:Description rdf:about="http://emmo.info/emmo#EMMO_a979c531_f9fa_4a6e_93c1_a2960241ca64">
    <EMMO_1f1b164d_ec6a_4faa_8d5e_88bda62316cc>http://qudt.org/vocab/unit/N</EMMO_1f1b164d_ec6a_4faa_8d5e_88bda62316cc>
    <rdfs:subClassOf rdf:nodeID="f05bdaa1e617a4bccafc519daf7bf4785b124"/>
    <rdfs:comment xml:lang="en">Measurement unit for force.</rdfs:comment>
    <skos:prefLabel xml:lang="en">Newton</skos:prefLabel>
    <rdf:type rdf:resource="http://www.w3.org/2002/07/owl#Class"/>
    <rdfs:subClassOf rdf:nodeID="f05bdaa1e617a4bccafc519daf7bf4785b123"/>
    <EMMO_fe015383_afb3_44a6_ae86_043628697aa2>https://doi.org/10.1351/goldbook.N04135</EMMO_fe015383_afb3_44a6_ae86_043628697aa2>
  </rdf:Description>
  <rdf:Description rdf:about="http://emmo.info/emmo#EMMO_ac540a9d_0131_43f6_a33b_17e5cfc432ed">
    <EMMO_50c298c2_55a2_4068_b3ac_4e948c33181f>http://www.electropedia.org/iev/iev.nsf/display?openform&amp;ievref=113-03-49</EMMO_50c298c2_55a2_4068_b3ac_4e948c33181f>
    <EMMO_967080e5_2f42_4eb2_a3a9_c58143e835f9 xml:lang="en">The energy of an object due to its motion.</EMMO_967080e5_2f42_4eb2_a3a9_c58143e835f9>
    <skos:prefLabel xml:lang="en">KineticEnergy</skos:prefLabel>
    <EMMO_e55f2d7c_9893_48cd_b4a4_fdf38253bd20>http://www.ontology-of-units-of-measure.org/resource/om-2/KineticEnergy</EMMO_e55f2d7c_9893_48cd_b4a4_fdf38253bd20>
    <rdfs:subClassOf rdf:resource="http://emmo.info/emmo#EMMO_31ec09ba_1713_42cb_83c7_b38bf6f9ced2"/>
    <EMMO_1f1b164d_ec6a_4faa_8d5e_88bda62316cc>http://qudt.org/vocab/quantitykind/KineticEnergy</EMMO_1f1b164d_ec6a_4faa_8d5e_88bda62316cc>
    <EMMO_fe015383_afb3_44a6_ae86_043628697aa2>https://doi.org/10.1351/goldbook.K03402</EMMO_fe015383_afb3_44a6_ae86_043628697aa2>
    <rdf:type rdf:resource="http://www.w3.org/2002/07/owl#Class"/>
    <EMMO_6dd685dd_1895_46e4_b227_be9f7d643c25>http://dbpedia.org/page/Kinetic_energy</EMMO_6dd685dd_1895_46e4_b227_be9f7d643c25>
    <EMMO_de178b12_5d35_4bca_8efa_a4193162571d>T-2 L+2 M+1 I0 Θ0 N0 J0</EMMO_de178b12_5d35_4bca_8efa_a4193162571d>
  </rdf:Description>
  <rdf:Description rdf:nodeID="f05bdaa1e617a4bccafc519daf7bf4785b166">
    <rdf:rest rdf:nodeID="f05bdaa1e617a4bccafc519daf7bf4785b167"/>
    <rdf:first rdf:resource="http://emmo.info/emmo#EMMO_080052a1_f295_44be_a60f_1326ce13f1ba"/>
    <rdf:type rdf:resource="http://www.w3.org/1999/02/22-rdf-syntax-ns#List"/>
  </rdf:Description>
  <rdf:Description rdf:about="http://www.w3.org/2004/02/skos/core#altLabel">
    <rdf:type rdf:resource="http://www.w3.org/2002/07/owl#AnnotationProperty"/>
    <rdfs:subPropertyOf rdf:resource="http://www.w3.org/2000/01/rdf-schema#label"/>
    <rdfs:range rdf:resource="http://www.w3.org/1999/02/22-rdf-syntax-ns#PlainLiteral"/>
  </rdf:Description>
  <rdf:Description rdf:nodeID="fe0b20157736f4a31909181349b2e6219b13">
    <rdf:type rdf:resource="http://www.w3.org/2002/07/owl#Restriction"/>
    <owl:onProperty rdf:resource="http://emmo.info/emmo#EMMO_23b579e1_8088_45b5_9975_064014026c42"/>
    <owl:hasValue>T0 L2 M0 I0 Θ0 N0 J0</owl:hasValue>
  </rdf:Description>
  <rdf:Description rdf:about="http://emmo.info/emmo#EMMO_048a14e3_65fb_457d_8695_948965c89492">
    <owl:equivalentClass rdf:nodeID="fe24a777e3fd743f986ce83488d2cf30bb1"/>
    <rdfs:subClassOf rdf:resource="http://emmo.info/emmo#EMMO_f8a2fe9f_458b_4771_9aba_a50e76afc52d"/>
    <rdf:type rdf:resource="http://www.w3.org/2002/07/owl#Class"/>
    <skos:prefLabel xml:lang="en">Laplacian</skos:prefLabel>
  </rdf:Description>
  <rdf:Description rdf:nodeID="fe0b20157736f4a31909181349b2e6219b33">
    <owl:onProperty rdf:resource="http://emmo.info/emmo#EMMO_23b579e1_8088_45b5_9975_064014026c42"/>
    <owl:hasValue>T-3 L+2 M+1 I0 Θ0 N0 J0</owl:hasValue>
    <rdf:type rdf:resource="http://www.w3.org/2002/07/owl#Restriction"/>
  </rdf:Description>
  <rdf:Description rdf:about="http://emmo.info/emmo#EMMO_7610efb8_c7c6_4684_abc1_774783c62472">
    <skos:prefLabel xml:lang="en">ElectricResistanceDimension</skos:prefLabel>
    <owl:equivalentClass rdf:nodeID="fe0b20157736f4a31909181349b2e6219b24"/>
    <rdf:type rdf:resource="http://www.w3.org/2002/07/owl#Class"/>
    <rdfs:subClassOf rdf:resource="http://emmo.info/emmo#EMMO_9895a1b4_f0a5_4167_ac5e_97db40b8bfcc"/>
  </rdf:Description>
  <rdf:Description rdf:about="http://emmo.info/emmo#EMMO_2e5e45fc_f52c_4294_bdc2_5ed7a06dfce7">
    <skos:prefLabel xml:lang="en">Kelvin</skos:prefLabel>
    <EMMO_1f1b164d_ec6a_4faa_8d5e_88bda62316cc>http://qudt.org/vocab/unit/K</EMMO_1f1b164d_ec6a_4faa_8d5e_88bda62316cc>
    <rdfs:subClassOf rdf:nodeID="f05bdaa1e617a4bccafc519daf7bf4785b29"/>
    <EMMO_fe015383_afb3_44a6_ae86_043628697aa2>https://doi.org/10.1351/goldbook.K03374</EMMO_fe015383_afb3_44a6_ae86_043628697aa2>
    <rdf:type rdf:resource="http://www.w3.org/2002/07/owl#Class"/>
    <EMMO_70fe84ff_99b6_4206_a9fc_9a8931836d84 xml:lang="en">The kelvin, symbol K, is the SI unit of thermodynamic temperature. It is defined by taking the fixed numerical value of the Boltzmann constant k to be 1.380649×10−23 when expressed in the unit J K−1, which is equal to kg m2 s−2 K−1, where the kilogram, metre and second are defined in terms of h, c and ∆νCs.</EMMO_70fe84ff_99b6_4206_a9fc_9a8931836d84>
    <rdfs:subClassOf rdf:nodeID="f05bdaa1e617a4bccafc519daf7bf4785b30"/>
  </rdf:Description>
  <rdf:Description rdf:about="http://emmo.info/emmo#EMMO_cc01751d_dd05_429b_9d0c_1b7a74d1f277">
    <rdfs:subClassOf rdf:resource="http://emmo.info/emmo#EMMO_f2ca6dd0_0e5f_4392_a92d_cafdae6cfc95"/>
    <EMMO_de178b12_5d35_4bca_8efa_a4193162571d>T+1 L0 M0 I+1 Θ0 N0 J0</EMMO_de178b12_5d35_4bca_8efa_a4193162571d>
    <EMMO_fe015383_afb3_44a6_ae86_043628697aa2>https://doi.org/10.1351/goldbook.E01982</EMMO_fe015383_afb3_44a6_ae86_043628697aa2>
    <rdf:type rdf:resource="http://www.w3.org/2002/07/owl#Class"/>
    <EMMO_70fe84ff_99b6_4206_a9fc_9a8931836d84 xml:lang="en">The charge of an electron.</EMMO_70fe84ff_99b6_4206_a9fc_9a8931836d84>
    <skos:prefLabel xml:lang="en">ElectronCharge</skos:prefLabel>
    <rdfs:subClassOf rdf:resource="http://emmo.info/emmo#EMMO_1604f495_328a_4f28_9962_f4cc210739dd"/>
    <rdfs:comment xml:lang="en">The negative of ElementaryCharge.</rdfs:comment>
  </rdf:Description>
  <rdf:Description rdf:nodeID="f05bdaa1e617a4bccafc519daf7bf4785b11">
    <owl:onProperty rdf:resource="http://emmo.info/emmo#EMMO_faf79f53_749d_40b2_807c_d34244c192f4"/>
    <rdf:type rdf:resource="http://www.w3.org/2002/07/owl#Restriction"/>
    <owl:hasValue rdf:datatype="http://www.w3.org/2001/XMLSchema#double">0.1</owl:hasValue>
  </rdf:Description>
  <rdf:Description rdf:about="http://emmo.info/emmo#EMMO_50c298c2_55a2_4068_b3ac_4e948c33181f">
    <rdfs:range rdf:resource="http://www.w3.org/2001/XMLSchema#anyURI"/>
    <rdfs:seeAlso rdf:datatype="http://www.w3.org/2001/XMLSchema#anyURI">http://www.electropedia.org/</rdfs:seeAlso>
    <skos:prefLabel xml:lang="en">IECEntry</skos:prefLabel>
    <rdfs:comment xml:lang="en">URL to corresponding entry in the IEC Electropedia online database of ISO 80000 terms and definitions of quantities and units available at http://www.electropedia.org/.</rdfs:comment>
    <rdfs:subPropertyOf rdf:resource="http://www.w3.org/2000/01/rdf-schema#isDefinedBy"/>
    <rdf:type rdf:resource="http://www.w3.org/2002/07/owl#AnnotationProperty"/>
  </rdf:Description>
  <rdf:Description rdf:about="http://emmo.info/emmo#EMMO_9d8f708a_f291_4d72_80ec_362c6e6bbca6">
    <EMMO_50c298c2_55a2_4068_b3ac_4e948c33181f>http://www.electropedia.org/iev/iev.nsf/display?openform&amp;ievref=113-03-12</EMMO_50c298c2_55a2_4068_b3ac_4e948c33181f>
    <EMMO_6dd685dd_1895_46e4_b227_be9f7d643c25>http://dbpedia.org/page/Center_of_mass</EMMO_6dd685dd_1895_46e4_b227_be9f7d643c25>
    <EMMO_de178b12_5d35_4bca_8efa_a4193162571d>T0 L+1 M0 I0 Θ0 N0 J0</EMMO_de178b12_5d35_4bca_8efa_a4193162571d>
    <skos:prefLabel xml:lang="en">CentreOfMass</skos:prefLabel>
    <rdfs:subClassOf rdf:resource="http://emmo.info/emmo#EMMO_44da6d75_54a4_4aa8_bd3a_156f6e9abb8e"/>
    <EMMO_c84c6752_6d64_48cc_9500_e54a3c34898d>https://en.wikipedia.org/wiki/Center_of_mass</EMMO_c84c6752_6d64_48cc_9500_e54a3c34898d>
    <rdfs:comment xml:lang="en">In non-relativistic physics, the centre of mass doesn’t depend on the chosen reference frame.</rdfs:comment>
    <rdf:type rdf:resource="http://www.w3.org/2002/07/owl#Class"/>
    <EMMO_967080e5_2f42_4eb2_a3a9_c58143e835f9 xml:lang="en">The unique point where the weighted relative position of the distributed mass of an Item sums to zero. Equivalently, it is the point where if a force is applied to the Item, causes the Item to move in direction of force without rotation.</EMMO_967080e5_2f42_4eb2_a3a9_c58143e835f9>
  </rdf:Description>
  <rdf:Description rdf:about="http://emmo.info/emmo#EMMO_868ae137_4d25_493e_b270_21ea3d94849e">
    <rdfs:subClassOf rdf:nodeID="f8fb83657cd5f496db3c2b94baf326f26b24"/>
    <owl:equivalentClass rdf:nodeID="f8fb83657cd5f496db3c2b94baf326f26b21"/>
    <skos:prefLabel xml:lang="en">NonPrefixedUnit</skos:prefLabel>
    <rdf:type rdf:resource="http://www.w3.org/2002/07/owl#Class"/>
    <EMMO_967080e5_2f42_4eb2_a3a9_c58143e835f9 xml:lang="en">A measurement unit symbol that do not have a metric prefix as a direct spatial part.</EMMO_967080e5_2f42_4eb2_a3a9_c58143e835f9>
  </rdf:Description>
  <rdf:Description rdf:about="http://emmo.info/emmo#EMMO_e75f580e_52bf_4dd5_af70_df409cec08fd">
    <rdfs:comment xml:lang="en">Measurement unit for frequence.</rdfs:comment>
    <skos:prefLabel xml:lang="en">Hertz</skos:prefLabel>
    <EMMO_fe015383_afb3_44a6_ae86_043628697aa2>https://doi.org/10.1351/goldbook.H02785</EMMO_fe015383_afb3_44a6_ae86_043628697aa2>
    <rdf:type rdf:resource="http://www.w3.org/2002/07/owl#Class"/>
    <rdfs:subClassOf rdf:nodeID="f05bdaa1e617a4bccafc519daf7bf4785b160"/>
    <EMMO_1f1b164d_ec6a_4faa_8d5e_88bda62316cc>http://qudt.org/vocab/unit/HZ</EMMO_1f1b164d_ec6a_4faa_8d5e_88bda62316cc>
    <rdfs:subClassOf rdf:nodeID="f05bdaa1e617a4bccafc519daf7bf4785b159"/>
  </rdf:Description>
  <rdf:Description rdf:about="http://emmo.info/emmo#EMMO_75fe4fd1_0f7e_429b_b91d_59d248561bae">
    <EMMO_967080e5_2f42_4eb2_a3a9_c58143e835f9 xml:lang="en">A Material occurring in nature, without the need of human intervention.</EMMO_967080e5_2f42_4eb2_a3a9_c58143e835f9>
    <skos:prefLabel xml:lang="en">NaturalMaterial</skos:prefLabel>
    <rdf:type rdf:resource="http://www.w3.org/2002/07/owl#Class"/>
    <rdfs:subClassOf rdf:resource="http://emmo.info/emmo#EMMO_4207e895_8b83_4318_996a_72cfb32acd94"/>
  </rdf:Description>
  <rdf:Description rdf:about="http://emmo.info/emmo#EMMO_9895a1b4_f0a5_4167_ac5e_97db40b8bfcc">
    <skos:prefLabel xml:lang="en">PhysicalDimension</skos:prefLabel>
    <rdfs:subClassOf rdf:resource="http://emmo.info/emmo#EMMO_985bec21_989f_4b9e_a4b3_735d88099c3c"/>
    <rdf:type rdf:resource="http://www.w3.org/2002/07/owl#Class"/>
    <rdfs:subClassOf rdf:resource="http://emmo.info/emmo#EMMO_a1083d0a_c1fb_471f_8e20_a98f881ad527"/>
    <rdfs:comment xml:lang="en">All physical quantities, with the exception of counts, are derived quantities, which may be written in terms of base quantities according to the equations of physics. The dimensions of the derived quantities are written as products of powers of the dimensions of the base quantities using the equations that relate the derived quantities to the base quantities.
In general the dimension of any quantity Q is written in the form of a dimensional product,

dim Q = T^α L^β M^γ I^δ Θ^ε N^ζ J^η

where the exponents α, β, γ, δ, ε, ζ and η, which are generally small integers, which can be positive, negative, or zero, are called the dimensional exponents.
(SI brochure)</rdfs:comment>
    <rdfs:comment xml:lang="en">The conventional symbolic representation of the dimension of a base quantity is a single upper case letter in roman (upright) type. The conventional symbolic representation of the dimension of a derived quantity is the product of powers of the dimensions of the base quantities according to the definition of the derived quantity. The dimension of a quantity Q is denoted by dim Q.
ISO 80000-1</rdfs:comment>
    <rdfs:comment xml:lang="en">The expression used by the EMMO for physical dimensions is a metrological symbol (but a string at meta level, i.e. the ontologist level) like this:
 
Ta Lb Mc Id Θe Nf Jg

where a, b, c, d, e, f and g are 0 or signed integers.

Regex for the physical dimension symbol for the EMMO is:
^T([+-][1-9]|0) L([+-][1-9]|0) M([+-][1-9]|0) I([+-][1-9]|0) Θ([+-][1-9]|0) N([+-][1-9]|0) J([+-][1-9]|0)$

Examples of correspondance between base units and physical dimensions are:
mol -&gt; T0 L0 M0 I0 Θ0 N+1 J0
s -&gt; T+1 L0 M0 I0 Θ0 N0 J0
A/m2 -&gt; T0 L0 M-2 I+1 Θ0 N0 J0</rdfs:comment>
    <EMMO_967080e5_2f42_4eb2_a3a9_c58143e835f9 xml:lang="en">A symbol that, following SI specifications, describe the physical dimensionality of a physical quantity and the exponents of the base units in a measurement unit.</EMMO_967080e5_2f42_4eb2_a3a9_c58143e835f9>
  </rdf:Description>
  <rdf:Description rdf:about="http://emmo.info/emmo#EMMO_cd2cd0de_e0cc_4ef1_b27e_2e88db027bac">
    <rdfs:comment xml:lang="en">Length is a non-negative additive quantity attributed to a one-dimensional object in space.</rdfs:comment>
    <rdf:type rdf:resource="http://www.w3.org/2002/07/owl#Class"/>
    <skos:prefLabel xml:lang="en">Length</skos:prefLabel>
    <EMMO_967080e5_2f42_4eb2_a3a9_c58143e835f9 xml:lang="en">Extend of a spatial dimension.</EMMO_967080e5_2f42_4eb2_a3a9_c58143e835f9>
    <EMMO_50c298c2_55a2_4068_b3ac_4e948c33181f>http://www.electropedia.org/iev/iev.nsf/display?openform&amp;ievref=113-01-19</EMMO_50c298c2_55a2_4068_b3ac_4e948c33181f>
    <EMMO_fe015383_afb3_44a6_ae86_043628697aa2>https://doi.org/10.1351/goldbook.L03498</EMMO_fe015383_afb3_44a6_ae86_043628697aa2>
    <EMMO_6dd685dd_1895_46e4_b227_be9f7d643c25>http://dbpedia.org/page/Length</EMMO_6dd685dd_1895_46e4_b227_be9f7d643c25>
    <EMMO_de178b12_5d35_4bca_8efa_a4193162571d>T0 L+1 M0 I0 Θ0 N0 J0</EMMO_de178b12_5d35_4bca_8efa_a4193162571d>
  </rdf:Description>
  <rdf:Description rdf:nodeID="ffcb99037244f48d590430c228d02afdbb40">
    <rdf:type rdf:resource="http://www.w3.org/2002/07/owl#Restriction"/>
    <owl:allValuesFrom rdf:resource="http://emmo.info/emmo#EMMO_cdc962d8_f3ea_4764_a57a_c7caa4859179"/>
    <owl:onProperty rdf:resource="http://emmo.info/emmo#EMMO_67fc0a36_8dcb_4ffa_9a43_31074efa3296"/>
  </rdf:Description>
  <rdf:Description rdf:about="http://emmo.info/emmo#EMMO_eb3a768e_d53e_4be9_a23b_0714833c36de">
    <rdfs:comment xml:lang="en">An 'Item' individual stands for a real world self-connected object which can be represented as a whole made of connected parts (e.g. a car made of components).

In the EMMO, connectivity is the topological foundation of causality.

All physical systems, i.e. systems whose behaviour is explained by physics laws, are represented only by 'Item'-s.

Members of a 'Collection' lack of causality connection, i.e. they do not constitute a physical system as a whole.</rdfs:comment>
    <rdf:type rdf:resource="http://www.w3.org/2002/07/owl#Class"/>
    <EMMO_705f27ae_954c_4f13_98aa_18473fc52b25 xml:lang="en">From Latin item, "likewise, just so, moreover".</EMMO_705f27ae_954c_4f13_98aa_18473fc52b25>
    <skos:prefLabel xml:lang="en">Item</skos:prefLabel>
    <owl:disjointUnionOf rdf:nodeID="fc2fcd8f8eb3649bcbbaff76ba54058acb6"/>
    <rdfs:comment xml:lang="en">A real world object is self-connected if any two parts that make up the whole are connected to each other (here the concept of connection is primitive). 

Alternatively, using the primitive path-connectivity concept we can define a self-connected real world object as an object for which each couple of points is path-connected.</rdfs:comment>
  </rdf:Description>
  <rdf:Description rdf:about="http://emmo.info/emmo#EMMO_7fb7fe7e_bdf9_4eeb_adad_e384dd5285c6">
    <skos:prefLabel xml:lang="en">hasInterpretant</skos:prefLabel>
    <rdfs:range rdf:resource="http://emmo.info/emmo#EMMO_054af807_85cd_4a13_8eba_119dfdaaf38b"/>
    <rdf:type rdf:resource="http://www.w3.org/2002/07/owl#ObjectProperty"/>
    <rdfs:subPropertyOf rdf:resource="http://emmo.info/emmo#EMMO_60577dea_9019_4537_ac41_80b0fb563d41"/>
  </rdf:Description>
  <rdf:Description rdf:about="http://emmo.info/emmo#EMMO_bed1d005_b04e_4a90_94cf_02bc678a8569">
    <skos:prefLabel xml:lang="en">hasPhysicalDimension</skos:prefLabel>
    <rdfs:subPropertyOf rdf:resource="http://emmo.info/emmo#EMMO_e1097637_70d2_4895_973f_2396f04fa204"/>
    <rdfs:range rdf:resource="http://emmo.info/emmo#EMMO_9895a1b4_f0a5_4167_ac5e_97db40b8bfcc"/>
    <rdf:type rdf:resource="http://www.w3.org/2002/07/owl#ObjectProperty"/>
  </rdf:Description>
  <rdf:Description rdf:about="http://emmo.info/emmo#EMMO_176cae33_b83e_4cd2_a6bc_281f42f0ccc8">
    <rdfs:comment xml:lang="en">The DBpedia definition (http://dbpedia.org/page/Avogadro_constant) is outdated as May 20, 2019. It is now an exact quantity.</rdfs:comment>
    <EMMO_1f1b164d_ec6a_4faa_8d5e_88bda62316cc>http://qudt.org/vocab/constant/AvogadroConstant</EMMO_1f1b164d_ec6a_4faa_8d5e_88bda62316cc>
    <EMMO_de178b12_5d35_4bca_8efa_a4193162571d>T0 L0 M0 I0 Θ0 N-1 J0</EMMO_de178b12_5d35_4bca_8efa_a4193162571d>
    <rdf:type rdf:resource="http://www.w3.org/2002/07/owl#Class"/>
    <rdfs:subClassOf rdf:resource="http://emmo.info/emmo#EMMO_f2ca6dd0_0e5f_4392_a92d_cafdae6cfc95"/>
    <skos:prefLabel xml:lang="en">AvogadroConstant</skos:prefLabel>
    <EMMO_a9b3d04c_7ceb_40a2_b8d3_28d514a770a8>https://physics.nist.gov/cgi-bin/cuu/Value?na</EMMO_a9b3d04c_7ceb_40a2_b8d3_28d514a770a8>
    <EMMO_fe015383_afb3_44a6_ae86_043628697aa2>https://doi.org/10.1351/goldbook.A00543</EMMO_fe015383_afb3_44a6_ae86_043628697aa2>
    <EMMO_967080e5_2f42_4eb2_a3a9_c58143e835f9 xml:lang="en">The number of constituent particles, usually atoms or molecules, that are contained in the amount of substance given by one mole.

It defines the base unit mole in the SI system.</EMMO_967080e5_2f42_4eb2_a3a9_c58143e835f9>
  </rdf:Description>
  <rdf:Description rdf:nodeID="f05bdaa1e617a4bccafc519daf7bf4785b172">
    <rdf:type rdf:resource="http://www.w3.org/1999/02/22-rdf-syntax-ns#List"/>
    <rdf:rest rdf:nodeID="f05bdaa1e617a4bccafc519daf7bf4785b173"/>
    <rdf:first rdf:resource="http://emmo.info/emmo#EMMO_a80dc6f5_b1aa_41a7_a3a8_cd5040da2162"/>
  </rdf:Description>
  <rdf:Description rdf:about="http://emmo.info/emmo#EMMO_4c151909_6f26_4ef9_b43d_7c9e9514883a">
    <EMMO_1f1b164d_ec6a_4faa_8d5e_88bda62316cc>http://qudt.org/vocab/quantitykind/PotentialEnergy</EMMO_1f1b164d_ec6a_4faa_8d5e_88bda62316cc>
    <EMMO_50c298c2_55a2_4068_b3ac_4e948c33181f>http://www.electropedia.org/iev/iev.nsf/display?openform&amp;ievref=113-03-48</EMMO_50c298c2_55a2_4068_b3ac_4e948c33181f>
    <EMMO_de178b12_5d35_4bca_8efa_a4193162571d>T-2 L+2 M+1 I0 Θ0 N0 J0</EMMO_de178b12_5d35_4bca_8efa_a4193162571d>
    <EMMO_fe015383_afb3_44a6_ae86_043628697aa2>https://doi.org/10.1351/goldbook.P04778</EMMO_fe015383_afb3_44a6_ae86_043628697aa2>
    <rdf:type rdf:resource="http://www.w3.org/2002/07/owl#Class"/>
    <rdfs:subClassOf rdf:resource="http://emmo.info/emmo#EMMO_31ec09ba_1713_42cb_83c7_b38bf6f9ced2"/>
    <EMMO_6dd685dd_1895_46e4_b227_be9f7d643c25>http://dbpedia.org/page/Potential_energy</EMMO_6dd685dd_1895_46e4_b227_be9f7d643c25>
    <EMMO_e55f2d7c_9893_48cd_b4a4_fdf38253bd20>http://www.ontology-of-units-of-measure.org/resource/om-2/PotentialEnergy</EMMO_e55f2d7c_9893_48cd_b4a4_fdf38253bd20>
    <EMMO_967080e5_2f42_4eb2_a3a9_c58143e835f9 xml:lang="en">The energy possessed by a body by virtue of its position or orientation in a potential field.</EMMO_967080e5_2f42_4eb2_a3a9_c58143e835f9>
    <skos:prefLabel xml:lang="en">PotentialEnergy</skos:prefLabel>
  </rdf:Description>
  <rdf:Description rdf:nodeID="f627ff42579444148ae27fcacfb5f8528b7">
    <owl:someValuesFrom rdf:resource="http://emmo.info/emmo#EMMO_27c5d8c6_8af7_4d63_beb1_ec37cd8b3fa3"/>
    <owl:onProperty rdf:resource="http://emmo.info/emmo#EMMO_f68030be_94b8_4c61_a161_886468558054"/>
    <rdf:type rdf:resource="http://www.w3.org/2002/07/owl#Restriction"/>
  </rdf:Description>
  <rdf:Description rdf:about="http://emmo.info/emmo#EMMO_ad6c76cf_b400_423e_820f_cf0c4e77f455">
    <EMMO_1f1b164d_ec6a_4faa_8d5e_88bda62316cc>http://qudt.org/vocab/constant/MolarGasConstant</EMMO_1f1b164d_ec6a_4faa_8d5e_88bda62316cc>
    <EMMO_a9b3d04c_7ceb_40a2_b8d3_28d514a770a8>https://physics.nist.gov/cgi-bin/cuu/Value?r</EMMO_a9b3d04c_7ceb_40a2_b8d3_28d514a770a8>
    <EMMO_fe015383_afb3_44a6_ae86_043628697aa2>https://doi.org/10.1351/goldbook.G02579</EMMO_fe015383_afb3_44a6_ae86_043628697aa2>
    <rdfs:subClassOf rdf:resource="http://emmo.info/emmo#EMMO_f2ca6dd0_0e5f_4392_a92d_cafdae6cfc95"/>
    <EMMO_de178b12_5d35_4bca_8efa_a4193162571d>T-2 L+2 M+1 I0 Θ-1 N-1 J0</EMMO_de178b12_5d35_4bca_8efa_a4193162571d>
    <EMMO_967080e5_2f42_4eb2_a3a9_c58143e835f9 xml:lang="en">Equivalent to the Boltzmann constant, but expressed in units of energy per temperature increment per mole (rather than energy per temperature increment per particle).</EMMO_967080e5_2f42_4eb2_a3a9_c58143e835f9>
    <EMMO_6dd685dd_1895_46e4_b227_be9f7d643c25>http://dbpedia.org/page/Gas_constant</EMMO_6dd685dd_1895_46e4_b227_be9f7d643c25>
    <skos:prefLabel xml:lang="en">MolarGasConstant</skos:prefLabel>
    <rdf:type rdf:resource="http://www.w3.org/2002/07/owl#Class"/>
  </rdf:Description>
  <rdf:Description rdf:about="http://emmo.info/emmo#EMMO_32129fb5_df25_48fd_a29c_18a2f22a2dd5">
    <owl:disjointUnionOf rdf:nodeID="f05bdaa1e617a4bccafc519daf7bf4785b33"/>
    <rdf:type rdf:resource="http://www.w3.org/2002/07/owl#Class"/>
    <skos:prefLabel xml:lang="en">SIUnitSymbol</skos:prefLabel>
  </rdf:Description>
  <rdf:Description rdf:about="http://emmo.info/emmo#EMMO_e55f2d7c_9893_48cd_b4a4_fdf38253bd20">
    <rdfs:range rdf:resource="http://www.w3.org/2001/XMLSchema#anyURI"/>
    <rdfs:subPropertyOf rdf:resource="http://www.w3.org/2000/01/rdf-schema#seeAlso"/>
    <rdfs:seeAlso rdf:datatype="http://www.w3.org/2001/XMLSchema#anyURI">https://enterpriseintegrationlab.github.io/icity/OM/doc/index-en.html</rdfs:seeAlso>
    <skos:prefLabel xml:lang="en">omMatch</skos:prefLabel>
    <rdfs:comment xml:lang="en">IRI to corresponding concept in the Ontology of units of Measure</rdfs:comment>
    <rdf:type rdf:resource="http://www.w3.org/2002/07/owl#AnnotationProperty"/>
    <rdfs:seeAlso rdf:datatype="http://www.w3.org/2001/XMLSchema#anyURI">https://github.com/HajoRijgersberg/OM</rdfs:seeAlso>
  </rdf:Description>
  <rdf:Description rdf:about="http://emmo.info/emmo#EMMO_74931b1b_c133_4e59_9a75_1bf0e1626201">
    <rdfs:subClassOf rdf:nodeID="f05bdaa1e617a4bccafc519daf7bf4785b94"/>
    <rdf:type rdf:resource="http://www.w3.org/2002/07/owl#Class"/>
    <skos:prefLabel xml:lang="en">Kilo</skos:prefLabel>
    <rdfs:subClassOf rdf:nodeID="f05bdaa1e617a4bccafc519daf7bf4785b91"/>
  </rdf:Description>
  <rdf:Description rdf:about="http://emmo.info/emmo#EMMO_36c79456_e29c_400d_8bd3_0eedddb82652">
    <rdfs:comment xml:lang="en">The definition of 'State' implies that its spatial direct parts (i.e. 'physicals') are not gained or lost during its temporal extension (they exist from the left to the right side of the time interval), so that the cardinality of spatial direct parts in a 'State' is constant.

This does not mean that there cannot be a change in the internal structure of the 'State' direct parts. It means only that this change must not affect the existence of the direct part itself.

There is no change in granularity or cardinality of direct parts of a 'State'.

The use of spatial direct parthood in 'State' definition means that a 'State' cannot overlap in space another 'State'.</rdfs:comment>
    <rdfs:comment xml:lang="en">There is no change in granularity or cardinality of parts within a state.

The use of spatial direct parthood in state definition means that a state cannot overlap in space another state that is direct part of the same whole.</rdfs:comment>
    <rdf:type rdf:resource="http://www.w3.org/2002/07/owl#Class"/>
    <EMMO_967080e5_2f42_4eb2_a3a9_c58143e835f9 xml:lang="en">A 'Physical' which is a tessellation of spatial direct parts.</EMMO_967080e5_2f42_4eb2_a3a9_c58143e835f9>
    <rdfs:comment xml:lang="en">Direct partitions declaration is a choice of the ontologist that choses the classes to be used as direct parts, according to its own world view.

A 'State' can always be direct partitioned in 'Elementary'-s and 'Void' or 'Physical'.

e.g. the water in my glass can be seen as a single object without declaring direct parts, or as made of H2O molecules direct parts.</rdfs:comment>
    <rdfs:subClassOf rdf:nodeID="f3b8e3e5cecf14b688acdf306cd5f62cbb4"/>
    <EMMO_b432d2d5_25f4_4165_99c5_5935a7763c1a xml:lang="en">e.g. the existent in my glass is declared at t = t_start as made of two direct parts: the ice and the water. It will continue to exists as state as long as the ice is completely melt at t = t_end. The new state will be completely made of water. Between t_start and t_end there is an exchange of molecules between the ice and the water, but this does not affect the existence of the two states.

If we partition the existent in my glass as ice surrounded by several molecules (we do not use the object water as direct part) then the appearance of a molecule coming from the ice will cause a state to end and another state to begin.</EMMO_b432d2d5_25f4_4165_99c5_5935a7763c1a>
    <skos:prefLabel xml:lang="en">State</skos:prefLabel>
    <rdfs:comment xml:lang="en">The usefulness of 'State' is that it makes it possible to describe the evolution in time of an 'Existent' in terms of series of 'State'-s that can take into account the disappearance or appearance of parts within a 'Physical'. 

A 'State' is a recognizable granularity level of matter, in the sense that its direct parts do not appear or disappear within its lifetime as it can be for a generic 'Existent'.</rdfs:comment>
  </rdf:Description>
  <rdf:Description rdf:about="http://emmo.info/emmo#EMMO_bd67d149_24c2_4bc9_833a_c2bc26f98fd3">
    <EMMO_1f1b164d_ec6a_4faa_8d5e_88bda62316cc>http://qudt.org/vocab/quantitykind/CatalyticActivity</EMMO_1f1b164d_ec6a_4faa_8d5e_88bda62316cc>
    <EMMO_967080e5_2f42_4eb2_a3a9_c58143e835f9 xml:lang="en">Increase in the rate of reaction of a specified chemical reaction that an enzyme produces in a specific assay system.</EMMO_967080e5_2f42_4eb2_a3a9_c58143e835f9>
    <skos:prefLabel xml:lang="en">CatalyticActivity</skos:prefLabel>
    <rdf:type rdf:resource="http://www.w3.org/2002/07/owl#Class"/>
    <EMMO_de178b12_5d35_4bca_8efa_a4193162571d>T-1 L0 M0 I0 Θ0 N+1 J0</EMMO_de178b12_5d35_4bca_8efa_a4193162571d>
    <rdfs:subClassOf rdf:resource="http://emmo.info/emmo#EMMO_2946d40b_24a1_47fa_8176_e3f79bb45064"/>
    <EMMO_fe015383_afb3_44a6_ae86_043628697aa2>https://doi.org/10.1351/goldbook.C00881</EMMO_fe015383_afb3_44a6_ae86_043628697aa2>
  </rdf:Description>
  <rdf:Description rdf:nodeID="f05bdaa1e617a4bccafc519daf7bf4785b158">
    <owl:onProperty rdf:resource="http://emmo.info/emmo#EMMO_23b579e1_8088_45b5_9975_064014026c42"/>
    <rdf:type rdf:resource="http://www.w3.org/2002/07/owl#Restriction"/>
    <owl:hasValue>V</owl:hasValue>
  </rdf:Description>
  <rdf:Description rdf:nodeID="fe0b20157736f4a31909181349b2e6219b28">
    <owl:hasValue>T0 L0 M0 I0 Θ+1 N0 J0</owl:hasValue>
    <rdf:type rdf:resource="http://www.w3.org/2002/07/owl#Restriction"/>
    <owl:onProperty rdf:resource="http://emmo.info/emmo#EMMO_23b579e1_8088_45b5_9975_064014026c42"/>
  </rdf:Description>
  <rdf:Description rdf:about="http://emmo.info/emmo#EMMO_3f9ae00e_810c_4518_aec2_7200e424cf68">
    <rdfs:comment xml:lang="en">A 'Quantum' is the most fundamental subclass of 'Item', since its individuals stand for the smallest possible self-connected 4D real world objects.

The quantum concept recalls the fact that there is lower epistemological limit to our knowledge of the universe, related to the uncertainity principle.</rdfs:comment>
    <rdfs:subClassOf rdf:nodeID="f15a17d1fb53e4dd795c7db922ceff6acb2"/>
    <EMMO_705f27ae_954c_4f13_98aa_18473fc52b25 xml:lang="en">From Latin quantum (plural quanta) "as much as, so much as;", introduced in physics directly from Latin by Max Planck, 1900.</EMMO_705f27ae_954c_4f13_98aa_18473fc52b25>
    <rdfs:comment xml:lang="en">A quantum is the EMMO mereological 4D a-tomic entity. 

To avoid confusion with the concept of atom coming from physics, we will use the expression quantum mereology, instead of a-tomistic mereology.</rdfs:comment>
    <EMMO_b432d2d5_25f4_4165_99c5_5935a7763c1a xml:lang="en">For a physics based ontology the 'Quantum' can stand for the smallest identifiable portion of spacetime defined by the Planck limit in length (1.616e-35 m) and time (5.39e-44 s).

However, the quantum mereotopology approach is not restricted only to physics. For example, in a manpower management ontology, a 'Quantum' can stand for an hour (time) of a worker (space) activity.</EMMO_b432d2d5_25f4_4165_99c5_5935a7763c1a>
    <rdfs:comment xml:lang="en">A 'Quantum' stands for a 4D real world object.</rdfs:comment>
    <EMMO_967080e5_2f42_4eb2_a3a9_c58143e835f9 xml:lang="en">The class of 'EMMO' individuals that stand for real world objects that can't be further divided in time nor in space.</EMMO_967080e5_2f42_4eb2_a3a9_c58143e835f9>
    <skos:prefLabel xml:lang="en">Quantum</skos:prefLabel>
    <rdf:type rdf:resource="http://www.w3.org/2002/07/owl#Class"/>
    <rdfs:subClassOf rdf:resource="http://emmo.info/emmo#EMMO_802d3e92_8770_4f98_a289_ccaaab7fdddf"/>
  </rdf:Description>
  <rdf:Description rdf:about="http://emmo.info/emmo#EMMO_e501069c_34d3_4dc7_ac87_c90c7342192b">
    <rdfs:subClassOf rdf:resource="http://emmo.info/emmo#EMMO_9895a1b4_f0a5_4167_ac5e_97db40b8bfcc"/>
    <skos:prefLabel xml:lang="en">AmountDimension</skos:prefLabel>
    <rdf:type rdf:resource="http://www.w3.org/2002/07/owl#Class"/>
    <owl:equivalentClass rdf:nodeID="fe0b20157736f4a31909181349b2e6219b36"/>
  </rdf:Description>
  <rdf:Description rdf:about="http://emmo.info/emmo#EMMO_4b3e2374_52a1_4420_8e3f_3ae6b9bf7dff">
    <skos:prefLabel xml:lang="en">LiquidSolution</skos:prefLabel>
    <EMMO_967080e5_2f42_4eb2_a3a9_c58143e835f9 xml:lang="en">A liquid solution made of two or more component substances.</EMMO_967080e5_2f42_4eb2_a3a9_c58143e835f9>
    <rdf:type rdf:resource="http://www.w3.org/2002/07/owl#Class"/>
    <rdfs:subClassOf rdf:resource="http://emmo.info/emmo#EMMO_2031516a_2be7_48e8_9af7_7e1270e308fe"/>
    <rdfs:subClassOf rdf:resource="http://emmo.info/emmo#EMMO_7509da43_56b1_4d7f_887a_65d1663df4ba"/>
  </rdf:Description>
  <rdf:Description rdf:nodeID="fe0b20157736f4a31909181349b2e6219b34">
    <owl:hasValue>T-1 L0 M0 I0 Θ0 N+1 J0</owl:hasValue>
    <owl:onProperty rdf:resource="http://emmo.info/emmo#EMMO_23b579e1_8088_45b5_9975_064014026c42"/>
    <rdf:type rdf:resource="http://www.w3.org/2002/07/owl#Restriction"/>
  </rdf:Description>
  <rdf:Description rdf:about="http://emmo.info/emmo#EMMO_21ef2ed6_c086_4d24_8a75_980d2bcc9282">
    <rdfs:subClassOf rdf:resource="http://emmo.info/emmo#EMMO_591e02fd_8d37_45a6_9d11_bb21cef391a0"/>
    <EMMO_1f1b164d_ec6a_4faa_8d5e_88bda62316cc>http://qudt.org/vocab/unit/HR</EMMO_1f1b164d_ec6a_4faa_8d5e_88bda62316cc>
    <rdf:type rdf:resource="http://www.w3.org/2002/07/owl#Class"/>
    <rdfs:subClassOf rdf:nodeID="ffcb99037244f48d590430c228d02afdbb10"/>
    <EMMO_70fe84ff_99b6_4206_a9fc_9a8931836d84 xml:lang="en">Measure of time defined as 3600 seconds.</EMMO_70fe84ff_99b6_4206_a9fc_9a8931836d84>
    <skos:prefLabel xml:lang="en">Hour</skos:prefLabel>
    <EMMO_fe015383_afb3_44a6_ae86_043628697aa2>https://doi.org/10.1351/goldbook.H02866</EMMO_fe015383_afb3_44a6_ae86_043628697aa2>
    <rdfs:subClassOf rdf:nodeID="ffcb99037244f48d590430c228d02afdbb9"/>
  </rdf:Description>
  <rdf:Description rdf:nodeID="ffcb99037244f48d590430c228d02afdbb26">
    <rdf:first rdf:resource="http://emmo.info/emmo#EMMO_b8830065_3809_41b7_be3c_e33795567fd9"/>
    <rdf:rest rdf:nodeID="ffcb99037244f48d590430c228d02afdbb27"/>
    <rdf:type rdf:resource="http://www.w3.org/1999/02/22-rdf-syntax-ns#List"/>
  </rdf:Description>
  <rdf:Description rdf:about="http://emmo.info/emmo/middle/physicalistic">
    <dcterms:abstract xml:lang="en">European Materials &amp; Modelling Ontology (EMMO)

EMMO is a multidisciplinary effort to develop a standard representational framework (the ontology) based on current materials modelling knowledge, including physical sciences, analytical philosophy and information and communication technologies.

It provides the connection between the physical world, materials characterisation world and materials modelling world.

EMMO is released under a Creative Commons license Attribution 4.0 International (CC BY 4.0).</dcterms:abstract>
    <rdf:type rdf:resource="http://www.w3.org/2002/07/owl#Ontology"/>
    <dcterms:contributor>Fraunhofer IWM, DE</dcterms:contributor>
    <owl:versionInfo>1.0.0-beta</owl:versionInfo>
    <dcterms:creator>Emanuele Ghedini</dcterms:creator>
    <rdfs:comment xml:lang="en">The EMMO requires FacT++ reasoner plugin in order to visualize all inferences and class hierarchy (ctrl+R hotkey in Protege).</rdfs:comment>
    <dcterms:contributor>SINTEF, NO</dcterms:contributor>
    <dcterms:creator>Jesper Friis</dcterms:creator>
    <dcterms:contributor>Goldbeck Consulting Ltd (UK)</dcterms:contributor>
    <dcterms:creator>Georg Schmitz</dcterms:creator>
    <rdfs:comment xml:lang="en">Contacts:
Gerhard Goldbeck
Goldbeck Consulting Ltd (UK)
email: gerhard@goldbeck-consulting.com

Emanuele Ghedini
University of Bologna (IT)
email: emanuele.ghedini@unibo.it</rdfs:comment>
    <dcterms:publisher>EMMC ASBL</dcterms:publisher>
    <dcterms:creator>Adham Hashibon</dcterms:creator>
    <dcterms:contributor>University of Bologna, IT</dcterms:contributor>
    <owl:versionIRI rdf:resource="http://emmo.info/emmo/1.0.0-beta/middle/physicalistic"/>
    <dcterms:license>https://creativecommons.org/licenses/by/4.0/legalcode</dcterms:license>
    <dcterms:creator>Gerhard Goldbeck</dcterms:creator>
    <dcterms:contributor>Access, DE</dcterms:contributor>
    <dcterms:title xml:lang="en">European Materials &amp; Modelling Ontology</dcterms:title>
  </rdf:Description>
  <rdf:Description rdf:about="http://emmo.info/emmo#EMMO_60577dea_9019_4537_ac41_80b0fb563d41">
    <rdfs:domain rdf:resource="http://emmo.info/emmo#EMMO_6f5af708_f825_4feb_a0d1_a8d813d3022b"/>
    <rdfs:subPropertyOf rdf:resource="http://emmo.info/emmo#EMMO_2337e25c_3c60_43fc_a8f9_b11a3f974291"/>
    <rdfs:range rdf:resource="http://emmo.info/emmo#EMMO_b21a56ed_f969_4612_a6ec_cb7766f7f31d"/>
    <skos:prefLabel xml:lang="en">hasSign</skos:prefLabel>
    <rdf:type rdf:resource="http://www.w3.org/2002/07/owl#ObjectProperty"/>
  </rdf:Description>
  <rdf:Description rdf:about="http://emmo.info/emmo#EMMO_ab79e92b_5377_454d_be06_d61b50db295a">
    <rdf:type rdf:resource="http://www.w3.org/2002/07/owl#Class"/>
    <skos:prefLabel xml:lang="en">ElectricChargeDimension</skos:prefLabel>
    <rdfs:subClassOf rdf:resource="http://emmo.info/emmo#EMMO_9895a1b4_f0a5_4167_ac5e_97db40b8bfcc"/>
    <owl:equivalentClass rdf:nodeID="fe0b20157736f4a31909181349b2e6219b29"/>
  </rdf:Description>
  <rdf:Description rdf:about="http://emmo.info/emmo/middle/siunits">
    <dcterms:contributor>University of Bologna, IT</dcterms:contributor>
    <dcterms:creator>Jesper Friis</dcterms:creator>
    <dcterms:title xml:lang="en">European Materials &amp; Modelling Ontology</dcterms:title>
    <dcterms:abstract xml:lang="en">European Materials &amp; Modelling Ontology (EMMO)

EMMO is a multidisciplinary effort to develop a standard representational framework (the ontology) based on current materials modelling knowledge, including physical sciences, analytical philosophy and information and communication technologies.

It provides the connection between the physical world, materials characterisation world and materials modelling world.

EMMO is released under a Creative Commons license Attribution 4.0 International (CC BY 4.0).</dcterms:abstract>
    <rdfs:comment xml:lang="en">Contacts:
Gerhard Goldbeck
Goldbeck Consulting Ltd (UK)
email: gerhard@goldbeck-consulting.com

Emanuele Ghedini
University of Bologna (IT)
email: emanuele.ghedini@unibo.it</rdfs:comment>
    <rdf:type rdf:resource="http://www.w3.org/2002/07/owl#Ontology"/>
    <dcterms:contributor>Fraunhofer IWM, DE</dcterms:contributor>
    <dcterms:publisher>EMMC ASBL</dcterms:publisher>
    <owl:versionInfo>1.0.0-beta</owl:versionInfo>
    <dcterms:creator>Adham Hashibon</dcterms:creator>
    <dcterms:creator>Emanuele Ghedini</dcterms:creator>
    <owl:versionIRI rdf:resource="http://emmo.info/emmo/1.0.0-beta/middle/siunits"/>
    <dcterms:license>https://creativecommons.org/licenses/by/4.0/legalcode</dcterms:license>
    <rdfs:comment xml:lang="en">The EMMO requires FacT++ reasoner plugin in order to visualize all inferences and class hierarchy (ctrl+R hotkey in Protege).</rdfs:comment>
    <dcterms:creator>Gerhard Goldbeck</dcterms:creator>
    <dcterms:contributor>SINTEF, NO</dcterms:contributor>
    <dcterms:contributor>Goldbeck Consulting Ltd (UK)</dcterms:contributor>
    <dcterms:contributor>Access, DE</dcterms:contributor>
    <dcterms:creator>Georg Schmitz</dcterms:creator>
  </rdf:Description>
  <rdf:Description rdf:about="http://emmo.info/emmo#EMMO_54dc83cb_06e1_4739_9e45_bc09cead7f48">
    <owl:equivalentClass rdf:nodeID="fe24a777e3fd743f986ce83488d2cf30bb10"/>
    <rdf:type rdf:resource="http://www.w3.org/2002/07/owl#Class"/>
    <skos:prefLabel xml:lang="en">Boolean</skos:prefLabel>
    <rdfs:subClassOf rdf:resource="http://emmo.info/emmo#EMMO_21f56795_ee72_4858_b571_11cfaa59c1a8"/>
    <rdfs:subClassOf rdf:nodeID="fe24a777e3fd743f986ce83488d2cf30bb12"/>
    <rdfs:subClassOf rdf:nodeID="fe24a777e3fd743f986ce83488d2cf30bb11"/>
  </rdf:Description>
  <rdf:Description rdf:about="http://emmo.info/emmo#EMMO_a4b14b83_9392_4a5f_a2e8_b2b58793f59b">
    <EMMO_967080e5_2f42_4eb2_a3a9_c58143e835f9 xml:lang="en">A computational model that uses existing data to create new insight into the behaviour of a system.</EMMO_967080e5_2f42_4eb2_a3a9_c58143e835f9>
    <rdf:type rdf:resource="http://www.w3.org/2002/07/owl#Class"/>
    <rdfs:subClassOf rdf:resource="http://emmo.info/emmo#EMMO_f7ed665b_c2e1_42bc_889b_6b42ed3a36f0"/>
    <skos:prefLabel xml:lang="en">DataBasedModel</skos:prefLabel>
  </rdf:Description>
  <rdf:Description rdf:about="http://emmo.info/emmo#EMMO_6a4547ab_3abb_430d_b81b_ce32d47729f5">
    <rdfs:subClassOf rdf:nodeID="ffcb99037244f48d590430c228d02afdbb31"/>
    <rdf:type rdf:resource="http://www.w3.org/2002/07/owl#Class"/>
    <rdfs:subClassOf rdf:resource="http://emmo.info/emmo#EMMO_591e02fd_8d37_45a6_9d11_bb21cef391a0"/>
    <rdfs:subClassOf rdf:nodeID="ffcb99037244f48d590430c228d02afdbb32"/>
    <skos:prefLabel xml:lang="en">ArcSecond</skos:prefLabel>
    <EMMO_1f1b164d_ec6a_4faa_8d5e_88bda62316cc>http://qudt.org/vocab/unit/ARCSEC</EMMO_1f1b164d_ec6a_4faa_8d5e_88bda62316cc>
    <skos:altLabel xml:lang="en">SecondOfArc</skos:altLabel>
    <EMMO_70fe84ff_99b6_4206_a9fc_9a8931836d84 xml:lang="en">Measure of plane angle defined as 1/3600 or a degree.</EMMO_70fe84ff_99b6_4206_a9fc_9a8931836d84>
  </rdf:Description>
  <rdf:Description rdf:about="http://emmo.info/emmo#EMMO_e5438930_04e7_4d42_ade5_3700d4a52ab7">
    <EMMO_967080e5_2f42_4eb2_a3a9_c58143e835f9 xml:lang="en">An 'equation' that stands for a physical assumption specific to a material, and provides an expression for a 'physics_quantity' (the dependent variable) as function of other variables, physics_quantity or data (independent variables).</EMMO_967080e5_2f42_4eb2_a3a9_c58143e835f9>
    <rdfs:comment xml:lang="en">A material_relation can e.g. return a predefined number, return a database query, be an equation that depends on other physics_quantities.</rdfs:comment>
    <rdfs:subClassOf rdf:resource="http://emmo.info/emmo#EMMO_e56ee3eb_7609_4ae1_8bed_51974f0960a6"/>
    <rdfs:subClassOf rdf:nodeID="f627ff42579444148ae27fcacfb5f8528b9"/>
    <rdf:type rdf:resource="http://www.w3.org/2002/07/owl#Class"/>
    <EMMO_b432d2d5_25f4_4165_99c5_5935a7763c1a xml:lang="en">The Lennard-Jones potential.

A force field.

An Hamiltonian.</EMMO_b432d2d5_25f4_4165_99c5_5935a7763c1a>
    <skos:prefLabel xml:lang="en">MaterialRelation</skos:prefLabel>
  </rdf:Description>
  <rdf:Description rdf:about="http://emmo.info/emmo#EMMO_c10b7090_7284_4719_8e15_c743b13ca6ad">
    <EMMO_967080e5_2f42_4eb2_a3a9_c58143e835f9 xml:lang="en">SI coherent measurement unit for torque.</EMMO_967080e5_2f42_4eb2_a3a9_c58143e835f9>
    <rdf:type rdf:resource="http://www.w3.org/2002/07/owl#Class"/>
    <rdfs:subClassOf rdf:nodeID="ffcb99037244f48d590430c228d02afdbb46"/>
    <rdfs:comment xml:lang="en">Note that the physical dimension is the same as for Joule.</rdfs:comment>
    <rdfs:subClassOf rdf:resource="http://emmo.info/emmo#EMMO_1273eb34_de48_43a9_925f_104110469dd2"/>
    <EMMO_1f1b164d_ec6a_4faa_8d5e_88bda62316cc>http://qudt.org/vocab/unit/N-M</EMMO_1f1b164d_ec6a_4faa_8d5e_88bda62316cc>
    <skos:prefLabel xml:lang="en">NewtonMetre</skos:prefLabel>
    <EMMO_e55f2d7c_9893_48cd_b4a4_fdf38253bd20>http://www.ontology-of-units-of-measure.org/resource/om-2/newtonMetre</EMMO_e55f2d7c_9893_48cd_b4a4_fdf38253bd20>
  </rdf:Description>
  <rdf:Description rdf:nodeID="f05bdaa1e617a4bccafc519daf7bf4785b117">
    <owl:allValuesFrom rdf:nodeID="f05bdaa1e617a4bccafc519daf7bf4785b119"/>
    <owl:onProperty rdf:nodeID="f05bdaa1e617a4bccafc519daf7bf4785b118"/>
    <rdf:type rdf:resource="http://www.w3.org/2002/07/owl#Restriction"/>
  </rdf:Description>
  <rdf:Description rdf:nodeID="fe0b20157736f4a31909181349b2e6219b2">
    <rdf:type rdf:resource="http://www.w3.org/2002/07/owl#Restriction"/>
    <owl:onProperty rdf:resource="http://emmo.info/emmo#EMMO_23b579e1_8088_45b5_9975_064014026c42"/>
    <owl:hasValue>T0 L0 M0 I0 Θ0 N0 J+1</owl:hasValue>
  </rdf:Description>
  <rdf:Description rdf:about="http://emmo.info/emmo#EMMO_7c055d65_2929_40e1_af4f_4bf10995ad50">
    <EMMO_e55f2d7c_9893_48cd_b4a4_fdf38253bd20>http://www.ontology-of-units-of-measure.org/resource/om-2/MassFraction</EMMO_e55f2d7c_9893_48cd_b4a4_fdf38253bd20>
    <rdf:type rdf:resource="http://www.w3.org/2002/07/owl#Class"/>
    <rdfs:subClassOf rdf:resource="http://emmo.info/emmo#EMMO_faab3f84_e475_4a46_af9c_7d249f0b9aef"/>
    <skos:prefLabel xml:lang="en">MassFraction</skos:prefLabel>
    <EMMO_de178b12_5d35_4bca_8efa_a4193162571d>T0 L0 M0 I0 Θ0 N0 J0</EMMO_de178b12_5d35_4bca_8efa_a4193162571d>
    <rdfs:subClassOf rdf:nodeID="ffcb99037244f48d590430c228d02afdbb35"/>
    <rdfs:comment xml:lang="en">Mass of a constituent divided by the total mass of all constituents in the mixture.</rdfs:comment>
    <EMMO_6dd685dd_1895_46e4_b227_be9f7d643c25>http://dbpedia.org/page/Mass_fraction_(chemistry)</EMMO_6dd685dd_1895_46e4_b227_be9f7d643c25>
    <EMMO_1f1b164d_ec6a_4faa_8d5e_88bda62316cc>http://qudt.org/vocab/quantitykind/MassFraction</EMMO_1f1b164d_ec6a_4faa_8d5e_88bda62316cc>
    <EMMO_fe015383_afb3_44a6_ae86_043628697aa2>https://doi.org/10.1351/goldbook.M03722</EMMO_fe015383_afb3_44a6_ae86_043628697aa2>
  </rdf:Description>
  <rdf:Description rdf:about="http://emmo.info/emmo#EMMO_1a4c1a97_88a7_4d8e_b2f9_2ca58e92dde4">
    <rdfs:subClassOf rdf:resource="http://emmo.info/emmo#EMMO_acaaa124_3dde_48b6_86e6_6ec6f364f408"/>
    <EMMO_c84c6752_6d64_48cc_9500_e54a3c34898d>https://en.wikipedia.org/wiki/International_System_of_Quantities</EMMO_c84c6752_6d64_48cc_9500_e54a3c34898d>
    <rdfs:subClassOf rdf:resource="http://emmo.info/emmo#EMMO_f35cff4d_dc09_44cf_a729_22fb79e3bfb2"/>
    <skos:prefLabel xml:lang="en">ISQBaseQuantity</skos:prefLabel>
    <owl:disjointUnionOf rdf:nodeID="fe0b20157736f4a31909181349b2e6219b3"/>
    <rdf:type rdf:resource="http://www.w3.org/2002/07/owl#Class"/>
    <EMMO_967080e5_2f42_4eb2_a3a9_c58143e835f9 xml:lang="en">Base quantities defined in the International System of Quantities (ISQ).</EMMO_967080e5_2f42_4eb2_a3a9_c58143e835f9>
  </rdf:Description>
  <rdf:Description rdf:about="http://emmo.info/emmo#EMMO_faab3f84_e475_4a46_af9c_7d249f0b9aef">
    <EMMO_b432d2d5_25f4_4165_99c5_5935a7763c1a>refractive index,
volume fraction,
fine structure constant</EMMO_b432d2d5_25f4_4165_99c5_5935a7763c1a>
    <rdfs:subClassOf rdf:resource="http://emmo.info/emmo#EMMO_a66427d1_9932_4363_9ec5_7d91f2bfda1e"/>
    <rdf:type rdf:resource="http://www.w3.org/2002/07/owl#Class"/>
    <rdfs:comment xml:lang="en">Quantities defined as ratios `Q=A/B` having equal dimensions in numerator and denominator are dimensionless quantities but still have a physical dimension defined as dim(A)/dim(B).

Johansson, Ingvar (2010). "Metrological thinking needs the notions of parametric quantities, units and dimensions". Metrologia. 47 (3): 219–230. doi:10.1088/0026-1394/47/3/012. ISSN 0026-1394.</rdfs:comment>
    <rdfs:seeAlso>https://iopscience.iop.org/article/10.1088/0026-1394/47/3/012</rdfs:seeAlso>
    <skos:prefLabel xml:lang="en">RatioQuantity</skos:prefLabel>
    <EMMO_967080e5_2f42_4eb2_a3a9_c58143e835f9 xml:lang="en">The class of quantities that are the ratio of two quantities with the same physical dimensionality.</EMMO_967080e5_2f42_4eb2_a3a9_c58143e835f9>
    <EMMO_de178b12_5d35_4bca_8efa_a4193162571d>T0 L0 M0 I0 Θ0 N0 J0</EMMO_de178b12_5d35_4bca_8efa_a4193162571d>
  </rdf:Description>
  <rdf:Description rdf:nodeID="fe24a777e3fd743f986ce83488d2cf30bb14">
    <rdf:first rdf:resource="http://emmo.info/emmo#EMMO_54ee6b5e_5261_44a8_86eb_5717e7fdb9d0"/>
    <rdf:type rdf:resource="http://www.w3.org/1999/02/22-rdf-syntax-ns#List"/>
    <rdf:rest rdf:nodeID="fe24a777e3fd743f986ce83488d2cf30bb15"/>
  </rdf:Description>
  <rdf:Description rdf:nodeID="f05bdaa1e617a4bccafc519daf7bf4785b52">
    <owl:allValuesFrom rdf:nodeID="f05bdaa1e617a4bccafc519daf7bf4785b54"/>
    <rdf:type rdf:resource="http://www.w3.org/2002/07/owl#Restriction"/>
    <owl:onProperty rdf:nodeID="f05bdaa1e617a4bccafc519daf7bf4785b53"/>
  </rdf:Description>
  <rdf:Description rdf:about="http://emmo.info/emmo#EMMO_802d3e92_8770_4f98_a289_ccaaab7fdddf">
    <skos:prefLabel xml:lang="en">EMMO</skos:prefLabel>
    <EMMO_967080e5_2f42_4eb2_a3a9_c58143e835f9 xml:lang="en">The class representing the collection of all the individuals declared in this ontology standing for real world objects.</EMMO_967080e5_2f42_4eb2_a3a9_c58143e835f9>
    <owl:equivalentClass rdf:nodeID="f15a17d1fb53e4dd795c7db922ceff6acb3"/>
    <rdfs:comment xml:lang="en">In the EMMO we will refer to the universe as a Minkowski space, restricting the ontology to special relativity only. However, exension to general relativity, will adding more complexity, should not change the overall approach.</rdfs:comment>
    <rdfs:comment xml:lang="en">For the EMMO ontologist the whole universe is represented as a 4D path-connected topological manifold (i.e. the spacetime).

A real world object is then a 4D topological sub-region of the universe. 

A universe sub-region is isolated and defined as a real world object by the ontologist. Then, through a semiotic process that occurs at meta-ontological level (i.e. outside the ontology). an EMMO ontology entity (e.g. an OWL individual) is assigned to represent that real world object.

The fundamental distinction between real world objects, upon which the EMMO is based, is self-connectedness: a real world object can be self-connected xor not self-connected.</rdfs:comment>
    <rdfs:comment xml:lang="en">'EMMO' is the disjoint union of 'Item' and 'Collection' (covering axiom).

The union implies that 'EMMO' individuals can only be 'Item' individuals (standing for self-connected real world objects) or 'Collection' individuals (standing for a collection of disconnected items).

Disjointness means that a 'Collection' individual cannot be an 'Item' individual and viceversa, representing the fact that a real world object cannot be self-connected and non-self connected at the same time.</rdfs:comment>
    <owl:equivalentClass rdf:nodeID="f15a17d1fb53e4dd795c7db922ceff6acb4"/>
    <rdf:type rdf:resource="http://www.w3.org/2002/07/owl#Class"/>
    <rdfs:comment xml:lang="en">Mereotopology is the fundamental logical representation used by the EMMO ontologist to characterize the universe and to provide the definitions to connect real world objects to the EMMO concepts.

Parthood relations do not change dimensionality of the real world object referred by an 'EMMO' individual, i.e. every part of a real world object always retains its 4D dimensionality. 

The smallest part of a real world object (i.e. a part that has no proper parts) is referred in the EMMO by a 'Quantum' individual.

It follows that, for the EMMO, real world objects of dimensionality lower than 4D (e.g. surfaces, lines) do not exist.</rdfs:comment>
    <owl:disjointUnionOf rdf:nodeID="f15a17d1fb53e4dd795c7db922ceff6acb6"/>
  </rdf:Description>
  <rdf:Description rdf:about="http://emmo.info/emmo#EMMO_8043d3c6_a4c1_4089_ba34_9744e28e5b3d">
    <EMMO_967080e5_2f42_4eb2_a3a9_c58143e835f9 xml:lang="en">The class of individuals that stand for electrons elemntary particles.</EMMO_967080e5_2f42_4eb2_a3a9_c58143e835f9>
    <skos:prefLabel xml:lang="en">Electron</skos:prefLabel>
    <rdf:type rdf:resource="http://www.w3.org/2002/07/owl#Class"/>
    <rdfs:subClassOf rdf:resource="http://emmo.info/emmo#EMMO_0f795e3e_c602_4577_9a43_d5a231aa1360"/>
  </rdf:Description>
  <rdf:Description rdf:about="http://emmo.info/emmo#EMMO_15d62b55_38ea_4aec_b7c4_25db1a2e5a01">
    <EMMO_967080e5_2f42_4eb2_a3a9_c58143e835f9 xml:lang="en">Unit for dimensionless units that cannot be expressed as a 'FractionUnit'.</EMMO_967080e5_2f42_4eb2_a3a9_c58143e835f9>
    <skos:prefLabel xml:lang="en">PureNumberUnit</skos:prefLabel>
    <rdf:type rdf:resource="http://www.w3.org/2002/07/owl#Class"/>
    <rdfs:subClassOf rdf:resource="http://emmo.info/emmo#EMMO_5ebd5e01_0ed3_49a2_a30d_cd05cbe72978"/>
    <owl:disjointWith rdf:resource="http://emmo.info/emmo#EMMO_c2f5ee66_579c_44c6_a2e9_fa2eaa9fa4da"/>
    <EMMO_b432d2d5_25f4_4165_99c5_5935a7763c1a xml:lang="en">Unit of AtomicNumber</EMMO_b432d2d5_25f4_4165_99c5_5935a7763c1a>
  </rdf:Description>
  <rdf:Description rdf:nodeID="f8fb83657cd5f496db3c2b94baf326f26b37">
    <owl:onProperty rdf:resource="http://emmo.info/emmo#EMMO_b2282816_b7a3_44c6_b2cb_3feff1ceb7fe"/>
    <owl:onClass rdf:resource="http://emmo.info/emmo#EMMO_7d2afa66_ae9e_4095_a9bf_421d0be401b6"/>
    <rdf:type rdf:resource="http://www.w3.org/2002/07/owl#Restriction"/>
    <owl:qualifiedCardinality rdf:datatype="http://www.w3.org/2001/XMLSchema#nonNegativeInteger">1</owl:qualifiedCardinality>
  </rdf:Description>
  <rdf:Description rdf:about="http://emmo.info/emmo#EMMO_6f5af708_f825_4feb_a0d1_a8d813d3022b">
    <rdf:type rdf:resource="http://www.w3.org/2002/07/owl#Class"/>
    <rdfs:subClassOf rdf:resource="http://emmo.info/emmo#EMMO_b803f122_4acb_4064_9d71_c1e5fd091fc9"/>
    <skos:prefLabel xml:lang="en">Object</skos:prefLabel>
    <EMMO_967080e5_2f42_4eb2_a3a9_c58143e835f9 xml:lang="en">The object, in Peirce semiotics.</EMMO_967080e5_2f42_4eb2_a3a9_c58143e835f9>
    <rdfs:comment xml:lang="en">Here is assumed that the concept of 'object' is always relative to a 'semiotic' process. An 'object' does not exists per se, but it's always part of an interpretation.

The EMMO relies on strong reductionism, i.e. everything real is a formless collection of elementary particles: we give a meaning to real world entities only by giving them boundaries and defining them using 'sign'-s. 

In this way the 'sign'-ed entity become and 'object', and the 'object' is the basic entity needed in order to apply a logical formalism to the real world entities (i.e. we can speak of it through its sign, and use logics on it through its sign).</rdfs:comment>
  </rdf:Description>
  <rdf:Description rdf:nodeID="ffcb99037244f48d590430c228d02afdbb30">
    <rdf:first rdf:resource="http://emmo.info/emmo#EMMO_f8b92999_3cde_46e3_99d5_664da3090a02"/>
    <rdf:rest rdf:resource="http://www.w3.org/1999/02/22-rdf-syntax-ns#nil"/>
    <rdf:type rdf:resource="http://www.w3.org/1999/02/22-rdf-syntax-ns#List"/>
  </rdf:Description>
  <rdf:Description rdf:about="http://emmo.info/emmo#EMMO_a1083d0a_c1fb_471f_8e20_a98f881ad527">
    <rdfs:comment xml:lang="en">Subclasses of 'Symbol' are alphabets, in formal languages terminology.

A 'Symbol' is atomic for that alphabet, i.e. it has no parts that are symbols for the same alphabet.
e.g. a math symbol is not made of other math symbols

A Symbol may be a String in another language.
e.g. "Bq" is the symbol for Becquerel units when dealing with metrology, or a string of "B" and "q" symbols when dealing with characters.</rdfs:comment>
    <rdfs:comment xml:lang="en">Symbols of a formal language need not be symbols of anything. For instance there are logical constants which do not refer to any idea, but rather serve as a form of punctuation in the language (e.g. parentheses). 

Symbols of a formal language must be capable of being specified without any reference to any interpretation of them. 
(Wikipedia)</rdfs:comment>
    <rdfs:subClassOf rdf:resource="http://emmo.info/emmo#EMMO_057e7d57_aff0_49de_911a_8861d85cef40"/>
    <EMMO_b432d2d5_25f4_4165_99c5_5935a7763c1a xml:lang="en">The class of letter "A" is the symbol as idea and the letter A that you see on the screen is the mark.</EMMO_b432d2d5_25f4_4165_99c5_5935a7763c1a>
    <rdf:type rdf:resource="http://www.w3.org/2002/07/owl#Class"/>
    <skos:prefLabel xml:lang="en">Symbol</skos:prefLabel>
    <rdfs:comment xml:lang="en">The class is the idea of the symbol, while the individual of that class stands for a specific mark (or token) of that idea.</rdfs:comment>
    <EMMO_967080e5_2f42_4eb2_a3a9_c58143e835f9 xml:lang="en">The class of individuals that stand for an elementary mark of a specific symbolic code (alphabet).</EMMO_967080e5_2f42_4eb2_a3a9_c58143e835f9>
  </rdf:Description>
  <rdf:Description rdf:nodeID="f05bdaa1e617a4bccafc519daf7bf4785b167">
    <rdf:first rdf:resource="http://emmo.info/emmo#EMMO_33b67e69_3645_4c73_b100_5ea6759221b4"/>
    <rdf:rest rdf:nodeID="f05bdaa1e617a4bccafc519daf7bf4785b168"/>
    <rdf:type rdf:resource="http://www.w3.org/1999/02/22-rdf-syntax-ns#List"/>
  </rdf:Description>
  <rdf:Description rdf:nodeID="fea11ca01461e402d8f697c19c5d8de88b16">
    <rdf:rest rdf:nodeID="fea11ca01461e402d8f697c19c5d8de88b17"/>
    <rdf:type rdf:resource="http://www.w3.org/1999/02/22-rdf-syntax-ns#List"/>
    <rdf:first rdf:resource="http://emmo.info/emmo#EMMO_72d53756_7fb1_46ed_980f_83f47efbe105"/>
  </rdf:Description>
  <rdf:Description rdf:nodeID="f8fb83657cd5f496db3c2b94baf326f26b20">
    <rdf:type rdf:resource="http://www.w3.org/2002/07/owl#Restriction"/>
    <owl:onProperty rdf:resource="http://emmo.info/emmo#EMMO_bed1d005_b04e_4a90_94cf_02bc678a8569"/>
    <owl:someValuesFrom rdf:resource="http://emmo.info/emmo#EMMO_3227b821_26a5_4c7c_9c01_5c24483e0bd0"/>
  </rdf:Description>
  <rdf:Description rdf:nodeID="f05bdaa1e617a4bccafc519daf7bf4785b36">
    <rdf:type rdf:resource="http://www.w3.org/2002/07/owl#Restriction"/>
    <owl:hasValue>kat</owl:hasValue>
    <owl:onProperty rdf:resource="http://emmo.info/emmo#EMMO_23b579e1_8088_45b5_9975_064014026c42"/>
  </rdf:Description>
  <rdf:Description rdf:nodeID="fa691b5894b3543efa24f9838ff46c3eab3">
    <rdf:type rdf:resource="http://www.w3.org/2002/07/owl#Restriction"/>
    <owl:onProperty rdf:resource="http://emmo.info/emmo#EMMO_c5aae418_1622_4d02_93c5_21159e28e6c1"/>
    <owl:someValuesFrom rdf:resource="http://emmo.info/emmo#EMMO_b21a56ed_f969_4612_a6ec_cb7766f7f31d"/>
  </rdf:Description>
  <rdf:Description rdf:about="http://emmo.info/emmo#EMMO_1273eb34_de48_43a9_925f_104110469dd2">
    <rdf:type rdf:resource="http://www.w3.org/2002/07/owl#Class"/>
    <EMMO_b432d2d5_25f4_4165_99c5_5935a7763c1a>m/s
kg/m^3</EMMO_b432d2d5_25f4_4165_99c5_5935a7763c1a>
    <EMMO_967080e5_2f42_4eb2_a3a9_c58143e835f9 xml:lang="en">A SI derived unit whos numerical factor in front of the product of SI base units is one.</EMMO_967080e5_2f42_4eb2_a3a9_c58143e835f9>
    <rdfs:subClassOf rdf:resource="http://emmo.info/emmo#EMMO_08b308d4_31cd_4779_a784_aa92fc730f39"/>
    <skos:prefLabel xml:lang="en">SICoherentDerivedUnit</skos:prefLabel>
    <rdfs:comment xml:lang="en">This class collects all units that are products or powers of SI base or SI special units only.</rdfs:comment>
  </rdf:Description>
  <rdf:Description rdf:about="http://emmo.info/emmo#EMMO_223d9523_4169_4ecd_b8af_acad1215e1ff">
    <rdf:type rdf:resource="http://www.w3.org/2002/07/owl#Class"/>
    <rdfs:subClassOf rdf:resource="http://emmo.info/emmo#EMMO_3c424d37_cf62_41b1_ac9d_a316f8d113d6"/>
    <skos:prefLabel xml:lang="en">Exponent</skos:prefLabel>
  </rdf:Description>
  <rdf:Description rdf:about="http://emmo.info/emmo#EMMO_4456a5d2_16a6_4ee1_9a8e_5c75956b28ea">
    <EMMO_967080e5_2f42_4eb2_a3a9_c58143e835f9 xml:lang="en">A physics-based model based on a physics equation describing the behaviour of continuum volume.</EMMO_967080e5_2f42_4eb2_a3a9_c58143e835f9>
    <rdfs:subClassOf rdf:resource="http://emmo.info/emmo#EMMO_b29fd350_39aa_4af7_9459_3faa0544cba6"/>
    <rdf:type rdf:resource="http://www.w3.org/2002/07/owl#Class"/>
    <skos:prefLabel xml:lang="en">ContinuumModel</skos:prefLabel>
  </rdf:Description>
  <rdf:Description rdf:about="http://emmo.info/emmo#EMMO_9fd1e79d_41d1_44f8_8142_66dbdf0fc7ad">
    <rdf:type rdf:resource="http://www.w3.org/2002/07/owl#Class"/>
    <skos:prefLabel xml:lang="en">VolumeFractionUnit</skos:prefLabel>
    <EMMO_b432d2d5_25f4_4165_99c5_5935a7763c1a xml:lang="en">Unit for volume fraction.</EMMO_b432d2d5_25f4_4165_99c5_5935a7763c1a>
    <rdfs:subClassOf rdf:resource="http://emmo.info/emmo#EMMO_c2f5ee66_579c_44c6_a2e9_fa2eaa9fa4da"/>
    <EMMO_967080e5_2f42_4eb2_a3a9_c58143e835f9 xml:lang="en">Unit for quantities of dimension one that are the fraction of two volumes.</EMMO_967080e5_2f42_4eb2_a3a9_c58143e835f9>
  </rdf:Description>
  <rdf:Description rdf:about="http://emmo.info/emmo#EMMO_b21a56ed_f969_4612_a6ec_cb7766f7f31d">
    <rdf:type rdf:resource="http://www.w3.org/2002/07/owl#Class"/>
    <owl:equivalentClass rdf:nodeID="fa691b5894b3543efa24f9838ff46c3eab5"/>
    <skos:prefLabel xml:lang="en">Sign</skos:prefLabel>
    <EMMO_b432d2d5_25f4_4165_99c5_5935a7763c1a xml:lang="en">A novel is made of chapters, paragraphs, sentences, words and characters (in a direct parthood mereological hierarchy). 

Each of them are 'sign'-s. 

A character can be the a-tomistic 'sign' for the class of texts.

The horizontal segment in the character "A" is direct part of "A" but it is not a 'sign' itself.

For plain text we can propose the ASCII symbols, for math the fundamental math symbols.</EMMO_b432d2d5_25f4_4165_99c5_5935a7763c1a>
    <rdfs:subClassOf rdf:resource="http://emmo.info/emmo#EMMO_b803f122_4acb_4064_9d71_c1e5fd091fc9"/>
    <EMMO_967080e5_2f42_4eb2_a3a9_c58143e835f9 xml:lang="en">An 'Physical' that is used as sign ("semeion" in greek) that stands for another 'Physical' through an semiotic process.</EMMO_967080e5_2f42_4eb2_a3a9_c58143e835f9>
    <rdfs:comment xml:lang="en">A 'Sign' can have temporal-direct-parts which are 'Sign' themselves.

A 'Sign' usually have 'sign' spatial direct parts only up to a certain elementary semiotic level, in which the part is only a 'Physical' and no more a 'Sign' (i.e. it stands for nothing). This elementary semiotic level is peculiar to each particular system of signs (e.g. text, painting).

Just like an 'Elementary' in the 'Physical' branch, each 'Sign' branch should have an a-tomistic mereological part.</rdfs:comment>
    <rdfs:comment xml:lang="en">According to Peirce, 'Sign' includes three subcategories:
- symbols: that stand for an object through convention
- indeces: that stand for an object due to causal continguity
- icon: that stand for an object due to similitudes e.g. in shape or composition</rdfs:comment>
  </rdf:Description>
  <rdf:Description rdf:about="http://emmo.info/emmo#EMMO_00199e76_69dc_45b6_a9c6_98cc90cdc0f5">
    <skos:prefLabel xml:lang="en">Gray</skos:prefLabel>
    <EMMO_1f1b164d_ec6a_4faa_8d5e_88bda62316cc>http://qudt.org/vocab/unit/GRAY</EMMO_1f1b164d_ec6a_4faa_8d5e_88bda62316cc>
    <EMMO_fe015383_afb3_44a6_ae86_043628697aa2>https://doi.org/10.1351/goldbook.G02696</EMMO_fe015383_afb3_44a6_ae86_043628697aa2>
    <rdfs:subClassOf rdf:nodeID="f05bdaa1e617a4bccafc519daf7bf4785b2"/>
    <rdf:type rdf:resource="http://www.w3.org/2002/07/owl#Class"/>
    <rdfs:subClassOf rdf:nodeID="f05bdaa1e617a4bccafc519daf7bf4785b1"/>
    <rdfs:comment xml:lang="en">Measurement unit for absorbed dose.</rdfs:comment>
  </rdf:Description>
  <rdf:Description rdf:nodeID="f05bdaa1e617a4bccafc519daf7bf4785b175">
    <rdf:rest rdf:nodeID="f05bdaa1e617a4bccafc519daf7bf4785b176"/>
    <rdf:first rdf:resource="http://emmo.info/emmo#EMMO_acb50123_87a2_4753_b36c_f87114ad4de2"/>
    <rdf:type rdf:resource="http://www.w3.org/1999/02/22-rdf-syntax-ns#List"/>
  </rdf:Description>
  <rdf:Description rdf:about="http://emmo.info/emmo#EMMO_fab003c8_f7a6_4346_9988_7161325ed7a3">
    <skos:prefLabel xml:lang="en">Henry</skos:prefLabel>
    <rdfs:comment xml:lang="en">Measurement unit for electrical inductance.</rdfs:comment>
    <rdfs:subClassOf rdf:nodeID="f05bdaa1e617a4bccafc519daf7bf4785b193"/>
    <EMMO_fe015383_afb3_44a6_ae86_043628697aa2>https://doi.org/10.1351/goldbook.H02782</EMMO_fe015383_afb3_44a6_ae86_043628697aa2>
    <EMMO_1f1b164d_ec6a_4faa_8d5e_88bda62316cc>http://qudt.org/vocab/unit/H</EMMO_1f1b164d_ec6a_4faa_8d5e_88bda62316cc>
    <rdf:type rdf:resource="http://www.w3.org/2002/07/owl#Class"/>
    <rdfs:subClassOf rdf:nodeID="f05bdaa1e617a4bccafc519daf7bf4785b194"/>
  </rdf:Description>
  <rdf:Description rdf:about="http://emmo.info/emmo#EMMO_5d659e25_a508_43ed_903c_3707c7c7cd4b">
    <EMMO_967080e5_2f42_4eb2_a3a9_c58143e835f9 xml:lang="en">Nanomaterials are Materials possessing, at minimum, one external dimension measuring 1-100nm</EMMO_967080e5_2f42_4eb2_a3a9_c58143e835f9>
    <skos:prefLabel xml:lang="en">NanoMaterial</skos:prefLabel>
    <rdfs:subClassOf rdf:resource="http://emmo.info/emmo#EMMO_4207e895_8b83_4318_996a_72cfb32acd94"/>
    <rdf:type rdf:resource="http://www.w3.org/2002/07/owl#Class"/>
  </rdf:Description>
  <rdf:Description rdf:about="http://purl.org/dc/terms/license">
    <rdf:type rdf:resource="http://www.w3.org/2002/07/owl#AnnotationProperty"/>
  </rdf:Description>
  <rdf:Description rdf:about="http://emmo.info/emmo#EMMO_b2282816_b7a3_44c6_b2cb_3feff1ceb7fe">
    <rdf:type rdf:resource="http://www.w3.org/2002/07/owl#AsymmetricProperty"/>
    <rdfs:subPropertyOf rdf:resource="http://emmo.info/emmo#EMMO_f68030be_94b8_4c61_a161_886468558054"/>
    <rdf:type rdf:resource="http://www.w3.org/2002/07/owl#ObjectProperty"/>
    <rdfs:domain rdf:resource="http://emmo.info/emmo#EMMO_36c79456_e29c_400d_8bd3_0eedddb82652"/>
    <rdf:type rdf:resource="http://www.w3.org/2002/07/owl#InverseFunctionalProperty"/>
    <skos:prefLabel xml:lang="en">hasSpatialDirectPart</skos:prefLabel>
    <rdf:type rdf:resource="http://www.w3.org/2002/07/owl#IrreflexiveProperty"/>
  </rdf:Description>
  <rdf:Description rdf:nodeID="f8fb83657cd5f496db3c2b94baf326f26b5">
    <rdf:rest rdf:nodeID="f8fb83657cd5f496db3c2b94baf326f26b6"/>
    <rdf:type rdf:resource="http://www.w3.org/1999/02/22-rdf-syntax-ns#List"/>
    <rdf:first rdf:resource="http://emmo.info/emmo#EMMO_48716718_225f_4c88_89e2_d819d30c90a2"/>
  </rdf:Description>
  <rdf:Description rdf:nodeID="ffcb99037244f48d590430c228d02afdbb47">
    <rdf:type rdf:resource="http://www.w3.org/2002/07/owl#Restriction"/>
    <owl:someValuesFrom rdf:resource="http://emmo.info/emmo#EMMO_02e894c3_b793_4197_b120_3442e08f58d1"/>
    <owl:onProperty rdf:resource="http://emmo.info/emmo#EMMO_bed1d005_b04e_4a90_94cf_02bc678a8569"/>
  </rdf:Description>
  <rdf:Description rdf:nodeID="f3b8e3e5cecf14b688acdf306cd5f62cbb2">
    <rdf:type rdf:resource="http://www.w3.org/1999/02/22-rdf-syntax-ns#List"/>
    <rdf:first rdf:resource="http://emmo.info/emmo#EMMO_36c79456_e29c_400d_8bd3_0eedddb82652"/>
    <rdf:rest rdf:nodeID="f3b8e3e5cecf14b688acdf306cd5f62cbb3"/>
  </rdf:Description>
  <rdf:Description rdf:nodeID="ff14b31ebf90e4bc5ba2839064d29e543b5">
    <owl:onProperty rdf:resource="http://emmo.info/emmo#EMMO_b2282816_b7a3_44c6_b2cb_3feff1ceb7fe"/>
    <rdf:type rdf:resource="http://www.w3.org/2002/07/owl#Restriction"/>
    <owl:someValuesFrom rdf:resource="http://emmo.info/emmo#EMMO_8043d3c6_a4c1_4089_ba34_9744e28e5b3d"/>
  </rdf:Description>
  <rdf:Description rdf:about="http://emmo.info/emmo#EMMO_81369540_1b0e_471b_9bae_6801af22800e">
    <EMMO_1f1b164d_ec6a_4faa_8d5e_88bda62316cc>http://qudt.org/vocab/quantitykind/Speed</EMMO_1f1b164d_ec6a_4faa_8d5e_88bda62316cc>
    <rdfs:comment xml:lang="en">Length per unit time. 

Speed in the absolute value of the velocity.</rdfs:comment>
    <EMMO_6dd685dd_1895_46e4_b227_be9f7d643c25>http://dbpedia.org/page/Speed</EMMO_6dd685dd_1895_46e4_b227_be9f7d643c25>
    <EMMO_e55f2d7c_9893_48cd_b4a4_fdf38253bd20>http://www.ontology-of-units-of-measure.org/resource/om-2/Speed</EMMO_e55f2d7c_9893_48cd_b4a4_fdf38253bd20>
    <skos:prefLabel xml:lang="en">Speed</skos:prefLabel>
    <EMMO_de178b12_5d35_4bca_8efa_a4193162571d>T-1 L+1 M0 I0 Θ0 N0 J0</EMMO_de178b12_5d35_4bca_8efa_a4193162571d>
    <EMMO_fe015383_afb3_44a6_ae86_043628697aa2>https://doi.org/10.1351/goldbook.S05852</EMMO_fe015383_afb3_44a6_ae86_043628697aa2>
    <rdfs:subClassOf rdf:resource="http://emmo.info/emmo#EMMO_2946d40b_24a1_47fa_8176_e3f79bb45064"/>
    <rdf:type rdf:resource="http://www.w3.org/2002/07/owl#Class"/>
  </rdf:Description>
  <rdf:Description rdf:about="http://emmo.info/emmo#EMMO_f9bc8b52_85e9_4b53_b969_dd7724d5b8e4">
    <skos:prefLabel xml:lang="en">Expression</skos:prefLabel>
    <rdf:type rdf:resource="http://www.w3.org/2002/07/owl#Class"/>
    <rdfs:subClassOf rdf:resource="http://emmo.info/emmo#EMMO_89a0c87c_0804_4013_937a_6fe234d9499c"/>
    <rdfs:subClassOf rdf:resource="http://emmo.info/emmo#EMMO_54ee6b5e_5261_44a8_86eb_5717e7fdb9d0"/>
    <EMMO_967080e5_2f42_4eb2_a3a9_c58143e835f9 xml:lang="en">A well-formed finite combination of mathematical symbols according to some specific rules.</EMMO_967080e5_2f42_4eb2_a3a9_c58143e835f9>
  </rdf:Description>
  <rdf:Description rdf:nodeID="f05bdaa1e617a4bccafc519daf7bf4785b71">
    <rdf:rest rdf:nodeID="f05bdaa1e617a4bccafc519daf7bf4785b72"/>
    <rdf:type rdf:resource="http://www.w3.org/1999/02/22-rdf-syntax-ns#List"/>
    <rdf:first rdf:resource="http://emmo.info/emmo#EMMO_b55cd09a_e54d_4eb1_81dd_03c29d1b878e"/>
  </rdf:Description>
  <rdf:Description rdf:nodeID="f05bdaa1e617a4bccafc519daf7bf4785b3">
    <owl:onProperty rdf:nodeID="f05bdaa1e617a4bccafc519daf7bf4785b4"/>
    <owl:allValuesFrom rdf:nodeID="f05bdaa1e617a4bccafc519daf7bf4785b5"/>
    <rdf:type rdf:resource="http://www.w3.org/2002/07/owl#Restriction"/>
  </rdf:Description>
  <rdf:Description rdf:nodeID="f05bdaa1e617a4bccafc519daf7bf4785b55">
    <owl:onProperty rdf:resource="http://emmo.info/emmo#EMMO_23b579e1_8088_45b5_9975_064014026c42"/>
    <rdf:type rdf:resource="http://www.w3.org/2002/07/owl#Restriction"/>
    <owl:hasValue>P</owl:hasValue>
  </rdf:Description>
  <rdf:Description rdf:about="http://emmo.info/emmo#EMMO_22522299_4091_4d1f_82a2_3890492df6db">
    <EMMO_967080e5_2f42_4eb2_a3a9_c58143e835f9 xml:lang="en">An experiment is a process that is intended to replicate a physical phenomenon in a controlled environment.</EMMO_967080e5_2f42_4eb2_a3a9_c58143e835f9>
    <rdfs:subClassOf rdf:nodeID="f627ff42579444148ae27fcacfb5f8528b1"/>
    <skos:prefLabel xml:lang="en">Experiment</skos:prefLabel>
    <rdfs:subClassOf rdf:resource="http://emmo.info/emmo#EMMO_10a5fd39_06aa_4648_9e70_f962a9cb2069"/>
    <rdf:type rdf:resource="http://www.w3.org/2002/07/owl#Class"/>
  </rdf:Description>
  <rdf:Description rdf:about="http://emmo.info/emmo#EMMO_74b05aed_66bf_43c8_aa2c_752a9ca8be03">
    <rdf:type rdf:resource="http://www.w3.org/2002/07/owl#Class"/>
    <skos:prefLabel xml:lang="en">Numeral</skos:prefLabel>
    <rdfs:subClassOf rdf:resource="http://emmo.info/emmo#EMMO_a1083d0a_c1fb_471f_8e20_a98f881ad527"/>
  </rdf:Description>
  <rdf:Description rdf:about="http://emmo.info/emmo#EMMO_e88f75d6_9a17_4cfc_bdf7_43d7cea5a9a1">
    <EMMO_967080e5_2f42_4eb2_a3a9_c58143e835f9 xml:lang="en">Measure of the difficulty to pass an electric current through a material.</EMMO_967080e5_2f42_4eb2_a3a9_c58143e835f9>
    <rdfs:subClassOf rdf:resource="http://emmo.info/emmo#EMMO_2946d40b_24a1_47fa_8176_e3f79bb45064"/>
    <skos:altLabel xml:lang="en">Resistance</skos:altLabel>
    <EMMO_1f1b164d_ec6a_4faa_8d5e_88bda62316cc>http://qudt.org/vocab/quantitykind/Resistance</EMMO_1f1b164d_ec6a_4faa_8d5e_88bda62316cc>
    <skos:prefLabel xml:lang="en">ElectricResistance</skos:prefLabel>
    <rdfs:comment xml:lang="en">Inverse of 'ElectricalConductance'.</rdfs:comment>
    <EMMO_de178b12_5d35_4bca_8efa_a4193162571d>T-3 L+2 M+1 I-2 Θ0 N0 J0</EMMO_de178b12_5d35_4bca_8efa_a4193162571d>
    <rdf:type rdf:resource="http://www.w3.org/2002/07/owl#Class"/>
    <EMMO_fe015383_afb3_44a6_ae86_043628697aa2>https://doi.org/10.1351/goldbook.E01936</EMMO_fe015383_afb3_44a6_ae86_043628697aa2>
    <EMMO_6dd685dd_1895_46e4_b227_be9f7d643c25>http://dbpedia.org/page/Electrical_resistance_and_conductance</EMMO_6dd685dd_1895_46e4_b227_be9f7d643c25>
  </rdf:Description>
  <rdf:Description rdf:about="http://emmo.info/emmo#EMMO_f96feb3f_4438_4e43_aa44_7458c4d87fc2">
    <EMMO_a9b3d04c_7ceb_40a2_b8d3_28d514a770a8>https://physics.nist.gov/cgi-bin/cuu/Value?nucs</EMMO_a9b3d04c_7ceb_40a2_b8d3_28d514a770a8>
    <rdfs:subClassOf rdf:resource="http://emmo.info/emmo#EMMO_852b4ab8_fc29_4749_a8c7_b92d4fca7d5a"/>
    <skos:prefLabel xml:lang="en">HyperfineTransitionFrequencyOfCs</skos:prefLabel>
    <rdfs:subClassOf rdf:resource="http://emmo.info/emmo#EMMO_f2ca6dd0_0e5f_4392_a92d_cafdae6cfc95"/>
    <rdf:type rdf:resource="http://www.w3.org/2002/07/owl#Class"/>
    <EMMO_de178b12_5d35_4bca_8efa_a4193162571d>T-1 L0 M0 I0 Θ0 N0 J0</EMMO_de178b12_5d35_4bca_8efa_a4193162571d>
    <EMMO_967080e5_2f42_4eb2_a3a9_c58143e835f9 xml:lang="en">The frequency standard in the SI system in which the photon absorption by transitions between the two hyperfine ground states of caesium-133 atoms are used to control the output frequency.

It defines the base unit second in the SI system.</EMMO_967080e5_2f42_4eb2_a3a9_c58143e835f9>
  </rdf:Description>
  <rdf:Description rdf:about="http://emmo.info/emmo#EMMO_76cc4efc_231e_42b4_be83_2547681caed6">
    <EMMO_967080e5_2f42_4eb2_a3a9_c58143e835f9 xml:lang="en">The quantum of action. It defines the kg base unit in the SI system.</EMMO_967080e5_2f42_4eb2_a3a9_c58143e835f9>
    <EMMO_6dd685dd_1895_46e4_b227_be9f7d643c25>http://dbpedia.org/page/Planck_constant</EMMO_6dd685dd_1895_46e4_b227_be9f7d643c25>
    <rdf:type rdf:resource="http://www.w3.org/2002/07/owl#Class"/>
    <rdfs:subClassOf rdf:resource="http://emmo.info/emmo#EMMO_f2ca6dd0_0e5f_4392_a92d_cafdae6cfc95"/>
    <EMMO_a9b3d04c_7ceb_40a2_b8d3_28d514a770a8>https://physics.nist.gov/cgi-bin/cuu/Value?h</EMMO_a9b3d04c_7ceb_40a2_b8d3_28d514a770a8>
    <EMMO_de178b12_5d35_4bca_8efa_a4193162571d>T-1 L+2 M+1 I0 Θ0 N0 J0</EMMO_de178b12_5d35_4bca_8efa_a4193162571d>
    <rdfs:subClassOf rdf:resource="http://emmo.info/emmo#EMMO_66d01570_36dd_42fd_844d_29b81b029cd5"/>
    <EMMO_1f1b164d_ec6a_4faa_8d5e_88bda62316cc>http://qudt.org/vocab/constant/PlanckConstant</EMMO_1f1b164d_ec6a_4faa_8d5e_88bda62316cc>
    <skos:prefLabel xml:lang="en">PlanckConstant</skos:prefLabel>
    <EMMO_fe015383_afb3_44a6_ae86_043628697aa2>https://doi.org/10.1351/goldbook.P04685</EMMO_fe015383_afb3_44a6_ae86_043628697aa2>
  </rdf:Description>
  <rdf:Description rdf:about="http://emmo.info/emmo#EMMO_98d65021_4574_4890_b2fb_46430841077f">
    <rdfs:subClassOf rdf:nodeID="fe24a777e3fd743f986ce83488d2cf30bb21"/>
    <skos:prefLabel xml:lang="en">AlgebricEquation</skos:prefLabel>
    <rdfs:subClassOf rdf:resource="http://emmo.info/emmo#EMMO_e56ee3eb_7609_4ae1_8bed_51974f0960a6"/>
    <rdf:type rdf:resource="http://www.w3.org/2002/07/owl#Class"/>
    <EMMO_b432d2d5_25f4_4165_99c5_5935a7763c1a xml:lang="en">2 * a - b = c</EMMO_b432d2d5_25f4_4165_99c5_5935a7763c1a>
    <rdfs:comment xml:lang="en">An 'equation' that has parts two 'polynomial'-s</rdfs:comment>
  </rdf:Description>
  <rdf:Description rdf:about="http://emmo.info/emmo#EMMO_eb3518bf_f799_4f9e_8c3e_ce59af11453b">
    <rdf:type rdf:resource="http://www.w3.org/2002/07/owl#ObjectProperty"/>
    <skos:prefLabel xml:lang="en">hasConvention</skos:prefLabel>
    <rdfs:subPropertyOf rdf:resource="http://emmo.info/emmo#EMMO_60577dea_9019_4537_ac41_80b0fb563d41"/>
    <rdfs:range rdf:resource="http://emmo.info/emmo#EMMO_35d2e130_6e01_41ed_94f7_00b333d46cf9"/>
  </rdf:Description>
  <rdf:Description rdf:about="http://emmo.info/emmo#EMMO_535d75a4_1972_40bc_88c6_ca566386934f">
    <EMMO_967080e5_2f42_4eb2_a3a9_c58143e835f9 xml:lang="en">The equals symbol.</EMMO_967080e5_2f42_4eb2_a3a9_c58143e835f9>
    <rdfs:subClassOf rdf:resource="http://emmo.info/emmo#EMMO_54ee6b5e_5261_44a8_86eb_5717e7fdb9d0"/>
    <skos:prefLabel xml:lang="en">Equals</skos:prefLabel>
    <owl:equivalentClass rdf:nodeID="fe24a777e3fd743f986ce83488d2cf30bb9"/>
    <rdfs:subClassOf rdf:resource="http://emmo.info/emmo#EMMO_a1083d0a_c1fb_471f_8e20_a98f881ad527"/>
    <rdf:type rdf:resource="http://www.w3.org/2002/07/owl#Class"/>
  </rdf:Description>
  <rdf:Description rdf:about="http://emmo.info/emmo#EMMO_71f6ab56_342c_484b_bbe0_de86b7367cb3">
    <skos:prefLabel xml:lang="en">DerivedQuantity</skos:prefLabel>
    <rdf:type rdf:resource="http://www.w3.org/2002/07/owl#Class"/>
    <EMMO_967080e5_2f42_4eb2_a3a9_c58143e835f9 xml:lang="en">"Quantity, in a system of quantities, defined in terms of the base quantities of that system".</EMMO_967080e5_2f42_4eb2_a3a9_c58143e835f9>
  </rdf:Description>
  <rdf:Description rdf:nodeID="f05bdaa1e617a4bccafc519daf7bf4785b32">
    <rdf:type rdf:resource="http://www.w3.org/2002/07/owl#Restriction"/>
    <owl:onProperty rdf:resource="http://emmo.info/emmo#EMMO_23b579e1_8088_45b5_9975_064014026c42"/>
    <owl:hasValue>s</owl:hasValue>
  </rdf:Description>
  <rdf:Description rdf:nodeID="f15a17d1fb53e4dd795c7db922ceff6acb1">
    <owl:someValuesFrom rdf:resource="http://emmo.info/emmo#EMMO_eb3a768e_d53e_4be9_a23b_0714833c36de"/>
    <owl:onProperty rdf:resource="http://emmo.info/emmo#EMMO_6b7276a4_4b9d_440a_b577_0277539c0fc4"/>
    <rdf:type rdf:resource="http://www.w3.org/2002/07/owl#Restriction"/>
  </rdf:Description>
  <rdf:Description rdf:about="http://emmo.info/emmo#EMMO_6c739b1a_a774_4416_bb31_1961486fa9ed">
    <EMMO_967080e5_2f42_4eb2_a3a9_c58143e835f9 xml:lang="en">The 'semiosis' process of interpreting a 'physical' and provide a complec sign, 'theory' that stands for it and explain it to another interpreter.</EMMO_967080e5_2f42_4eb2_a3a9_c58143e835f9>
    <skos:prefLabel xml:lang="en">Theorization</skos:prefLabel>
    <rdfs:subClassOf rdf:resource="http://emmo.info/emmo#EMMO_10a5fd39_06aa_4648_9e70_f962a9cb2069"/>
    <rdf:type rdf:resource="http://www.w3.org/2002/07/owl#Class"/>
  </rdf:Description>
  <rdf:Description rdf:nodeID="ffcb99037244f48d590430c228d02afdbb39">
    <owl:allValuesFrom rdf:resource="http://emmo.info/emmo#EMMO_9fd1e79d_41d1_44f8_8142_66dbdf0fc7ad"/>
    <rdf:type rdf:resource="http://www.w3.org/2002/07/owl#Restriction"/>
    <owl:onProperty rdf:resource="http://emmo.info/emmo#EMMO_67fc0a36_8dcb_4ffa_9a43_31074efa3296"/>
  </rdf:Description>
  <rdf:Description rdf:nodeID="ff14b31ebf90e4bc5ba2839064d29e543b19">
    <rdf:type rdf:resource="http://www.w3.org/1999/02/22-rdf-syntax-ns#List"/>
    <rdf:first rdf:resource="http://emmo.info/emmo#EMMO_04f2a2d5_e799_4692_a654_420e76f5acc1"/>
    <rdf:rest rdf:nodeID="ff14b31ebf90e4bc5ba2839064d29e543b20"/>
  </rdf:Description>
  <rdf:Description rdf:nodeID="f05bdaa1e617a4bccafc519daf7bf4785b89">
    <rdf:type rdf:resource="http://www.w3.org/1999/02/22-rdf-syntax-ns#List"/>
    <rdf:rest rdf:nodeID="f05bdaa1e617a4bccafc519daf7bf4785b90"/>
    <rdf:first rdf:resource="http://emmo.info/emmo#EMMO_3a185e6c_9e19_4776_b583_19c978156aa0"/>
  </rdf:Description>
  <rdf:Description rdf:about="http://emmo.info/emmo#EMMO_09663630_1b84_4202_91e6_e641104f579e">
    <rdfs:comment xml:lang="en">Measure for how the magnetization of material is affected by the application of an external magnetic field .</rdfs:comment>
    <EMMO_6dd685dd_1895_46e4_b227_be9f7d643c25>http://dbpedia.org/page/Permeability_(electromagnetism)</EMMO_6dd685dd_1895_46e4_b227_be9f7d643c25>
    <EMMO_1f1b164d_ec6a_4faa_8d5e_88bda62316cc>http://qudt.org/vocab/quantitykind/ElectromagneticPermeability</EMMO_1f1b164d_ec6a_4faa_8d5e_88bda62316cc>
    <EMMO_fe015383_afb3_44a6_ae86_043628697aa2>https://doi.org/10.1351/goldbook.P04503</EMMO_fe015383_afb3_44a6_ae86_043628697aa2>
    <skos:prefLabel xml:lang="en">Permeability</skos:prefLabel>
    <rdf:type rdf:resource="http://www.w3.org/2002/07/owl#Class"/>
    <rdfs:subClassOf rdf:resource="http://emmo.info/emmo#EMMO_2946d40b_24a1_47fa_8176_e3f79bb45064"/>
    <skos:altLabel>ElectromagneticPermeability</skos:altLabel>
    <EMMO_de178b12_5d35_4bca_8efa_a4193162571d>T-2 L+1 M+1 I-2 Θ0 N0 J0</EMMO_de178b12_5d35_4bca_8efa_a4193162571d>
  </rdf:Description>
  <rdf:Description rdf:about="http://emmo.info/emmo#EMMO_43e9a05d_98af_41b4_92f6_00f79a09bfce">
    <rdf:type rdf:resource="http://www.w3.org/2002/07/owl#Class"/>
    <rdfs:comment xml:lang="en">A 'Process' is always a 'Physical', since a 'Void' does not have elements that evolves in time.</rdfs:comment>
    <skos:prefLabel xml:lang="en">Process</skos:prefLabel>
    <rdfs:comment xml:lang="en">Following the common definition of process, the reader may think that every 'Physical' should be a process, since every 4D object always has a time dimension. 

However, in the EMMO we restrict the meaning of the word process to 'Physical'-s whose evolution in time have a particular meaning for the ontologist (i.e. every 4D object unfolds in time, but not every 4D object may be of interest for the ontologist). 

A 'Process' is not only something that unfolds in time (which is automatically represented in a 4D ontology), but something that has a meaning for the ontologist (i.e. that the ontologist can separate from the rest of the 4D physical for any reason).</rdfs:comment>
    <rdfs:subClassOf rdf:nodeID="f0b819106611c4b798f33b16c65f4398db4"/>
    <EMMO_967080e5_2f42_4eb2_a3a9_c58143e835f9 xml:lang="en">A temporal part of a physical that identifies a particular type of evolution in time.</EMMO_967080e5_2f42_4eb2_a3a9_c58143e835f9>
    <rdfs:subClassOf rdf:resource="http://emmo.info/emmo#EMMO_c5ddfdba_c074_4aa4_ad6b_1ac4942d300d"/>
  </rdf:Description>
  <rdf:Description rdf:about="http://emmo.info/emmo#EMMO_ce7d4720_aa20_4a8c_93e8_df41a35b6723">
    <rdfs:subClassOf rdf:resource="http://emmo.info/emmo#EMMO_9895a1b4_f0a5_4167_ac5e_97db40b8bfcc"/>
    <skos:prefLabel xml:lang="en">CatalyticActivityDimension</skos:prefLabel>
    <owl:equivalentClass rdf:nodeID="fe0b20157736f4a31909181349b2e6219b34"/>
    <rdf:type rdf:resource="http://www.w3.org/2002/07/owl#Class"/>
  </rdf:Description>
  <rdf:Description rdf:about="http://emmo.info/emmo#EMMO_7d66bde4_b68d_41cc_b5fc_6fd98c5e2ff0">
    <skos:prefLabel xml:lang="en">Subatomic</skos:prefLabel>
    <rdfs:subClassOf rdf:resource="http://emmo.info/emmo#EMMO_5b2222df_4da6_442f_8244_96e9e45887d1"/>
    <rdf:type rdf:resource="http://www.w3.org/2002/07/owl#Class"/>
  </rdf:Description>
  <rdf:Description rdf:about="http://emmo.info/emmo#EMMO_89083bab_f69c_4d06_bf6d_62973b56cdc7">
    <rdfs:subClassOf rdf:nodeID="fe24a777e3fd743f986ce83488d2cf30bb18"/>
    <EMMO_b432d2d5_25f4_4165_99c5_5935a7763c1a xml:lang="en">2+2</EMMO_b432d2d5_25f4_4165_99c5_5935a7763c1a>
    <skos:prefLabel xml:lang="en">ArithmeticExpression</skos:prefLabel>
    <rdfs:subClassOf rdf:resource="http://emmo.info/emmo#EMMO_1aed91a3_d00c_48af_8f43_a0c958b2512a"/>
    <rdf:type rdf:resource="http://www.w3.org/2002/07/owl#Class"/>
  </rdf:Description>
  <rdf:Description rdf:nodeID="f05bdaa1e617a4bccafc519daf7bf4785b56">
    <rdf:type rdf:resource="http://www.w3.org/1999/02/22-rdf-syntax-ns#List"/>
    <rdf:first rdf:resource="http://emmo.info/emmo#EMMO_068c4e58_2470_4b1c_8454_010dd4906100"/>
    <rdf:rest rdf:nodeID="f05bdaa1e617a4bccafc519daf7bf4785b57"/>
  </rdf:Description>
  <rdf:Description rdf:nodeID="f8fb83657cd5f496db3c2b94baf326f26b36">
    <rdf:type rdf:resource="http://www.w3.org/2002/07/owl#Restriction"/>
    <owl:onProperty rdf:resource="http://emmo.info/emmo#EMMO_b2282816_b7a3_44c6_b2cb_3feff1ceb7fe"/>
    <owl:onClass rdf:resource="http://emmo.info/emmo#EMMO_216f448e_cdbc_4aeb_a529_7a5fe7fc38bb"/>
    <owl:qualifiedCardinality rdf:datatype="http://www.w3.org/2001/XMLSchema#nonNegativeInteger">1</owl:qualifiedCardinality>
  </rdf:Description>
  <rdf:Description rdf:nodeID="f3b8e3e5cecf14b688acdf306cd5f62cbb4">
    <rdf:type rdf:resource="http://www.w3.org/2002/07/owl#Restriction"/>
    <owl:onProperty rdf:resource="http://emmo.info/emmo#EMMO_b2282816_b7a3_44c6_b2cb_3feff1ceb7fe"/>
    <owl:someValuesFrom rdf:resource="http://emmo.info/emmo#EMMO_c5ddfdba_c074_4aa4_ad6b_1ac4942d300d"/>
  </rdf:Description>
  <rdf:Description rdf:nodeID="f05bdaa1e617a4bccafc519daf7bf4785b88">
    <rdf:first rdf:resource="http://emmo.info/emmo#EMMO_1273eb34_de48_43a9_925f_104110469dd2"/>
    <rdf:rest rdf:nodeID="f05bdaa1e617a4bccafc519daf7bf4785b89"/>
    <rdf:type rdf:resource="http://www.w3.org/1999/02/22-rdf-syntax-ns#List"/>
  </rdf:Description>
  <rdf:Description rdf:about="http://emmo.info/emmo#EMMO_2d2ecd97_067f_4d0e_950c_d746b7700a31">
    <rdfs:comment xml:lang="en">Formally, 'Collection' is axiomatized as the class of individuals that hasMember some 'Item'.

A 'Collection' cannot have as member another 'Collection'.</rdfs:comment>
    <rdfs:comment xml:lang="en">e.g. the collection of users of a particular software, the collection of atoms that have been part of that just dissociated molecule, or even the collection of atoms that are part of a molecule considered as single individual non-connected objects and not as a mereotopological self-connected fusion.</rdfs:comment>
    <EMMO_705f27ae_954c_4f13_98aa_18473fc52b25 xml:lang="en">From Latin collectio, from colligere ‘gather together’.</EMMO_705f27ae_954c_4f13_98aa_18473fc52b25>
    <rdfs:subClassOf rdf:nodeID="f15a17d1fb53e4dd795c7db922ceff6acb1"/>
    <rdfs:comment xml:lang="en">A 'Collection' individual stands for a non-self-connected real world object.

A 'Collection' individual is related to each 'Item' individuals of the collection (i.e. the members) through the membership relation.

An 'Item' individual stands for a real world self-connected object which can be represented as a whole made of connected parts (e.g. a car made of components).</rdfs:comment>
    <skos:prefLabel xml:lang="en">Collection</skos:prefLabel>
    <EMMO_967080e5_2f42_4eb2_a3a9_c58143e835f9 xml:lang="en">The class of all individuals that stand for a real world not self-connected object.</EMMO_967080e5_2f42_4eb2_a3a9_c58143e835f9>
    <rdf:type rdf:resource="http://www.w3.org/2002/07/owl#Class"/>
  </rdf:Description>
  <rdf:Description rdf:nodeID="fe0b20157736f4a31909181349b2e6219b21">
    <owl:onProperty rdf:resource="http://emmo.info/emmo#EMMO_23b579e1_8088_45b5_9975_064014026c42"/>
    <rdf:type rdf:resource="http://www.w3.org/2002/07/owl#Restriction"/>
    <owl:hasValue>T-2 L+2 M+1 I-2 Θ0 N0 J0</owl:hasValue>
  </rdf:Description>
  <rdf:Description rdf:nodeID="f05bdaa1e617a4bccafc519daf7bf4785b30">
    <owl:hasValue>K</owl:hasValue>
    <rdf:type rdf:resource="http://www.w3.org/2002/07/owl#Restriction"/>
    <owl:onProperty rdf:resource="http://emmo.info/emmo#EMMO_23b579e1_8088_45b5_9975_064014026c42"/>
  </rdf:Description>
  <rdf:Description rdf:about="http://emmo.info/emmo#EMMO_77e9dc31_5b19_463e_b000_44c6e79f98aa">
    <owl:equivalentClass rdf:nodeID="fe0b20157736f4a31909181349b2e6219b25"/>
    <skos:prefLabel xml:lang="en">MassDimension</skos:prefLabel>
    <rdfs:subClassOf rdf:resource="http://emmo.info/emmo#EMMO_9895a1b4_f0a5_4167_ac5e_97db40b8bfcc"/>
    <rdf:type rdf:resource="http://www.w3.org/2002/07/owl#Class"/>
  </rdf:Description>
  <rdf:Description rdf:about="http://emmo.info/emmo#EMMO_6dd685dd_1895_46e4_b227_be9f7d643c25">
    <skos:prefLabel xml:lang="en">dbpediaEntry</skos:prefLabel>
    <rdfs:subPropertyOf rdf:resource="http://www.w3.org/2000/01/rdf-schema#seeAlso"/>
    <rdf:type rdf:resource="http://www.w3.org/2002/07/owl#AnnotationProperty"/>
    <rdfs:comment xml:lang="en">URL to corresponding concept in DBpedia.</rdfs:comment>
    <rdfs:seeAlso rdf:datatype="http://www.w3.org/2001/XMLSchema#anyURI">https://wiki.dbpedia.org/</rdfs:seeAlso>
    <rdfs:range rdf:resource="http://www.w3.org/2001/XMLSchema#anyURI"/>
  </rdf:Description>
  <rdf:Description rdf:about="http://emmo.info/emmo#EMMO_e5488299_8dab_4ebb_900a_26d2abed8396">
    <skos:prefLabel xml:lang="en">Massless</skos:prefLabel>
    <EMMO_967080e5_2f42_4eb2_a3a9_c58143e835f9 xml:lang="en">The union of classes of elementary particles that do not possess mass.</EMMO_967080e5_2f42_4eb2_a3a9_c58143e835f9>
    <owl:equivalentClass rdf:nodeID="fea11ca01461e402d8f697c19c5d8de88b20"/>
    <rdf:type rdf:resource="http://www.w3.org/2002/07/owl#Class"/>
  </rdf:Description>
  <rdf:Description rdf:nodeID="fe0b20157736f4a31909181349b2e6219b11">
    <rdf:type rdf:resource="http://www.w3.org/2002/07/owl#Restriction"/>
    <owl:onProperty rdf:resource="http://emmo.info/emmo#EMMO_23b579e1_8088_45b5_9975_064014026c42"/>
    <owl:hasValue>T-3 L+2 M+1 I-1 Θ0 N0 J0</owl:hasValue>
  </rdf:Description>
  <rdf:Description rdf:about="http://emmo.info/emmo#EMMO_6c7160fc_cc64_46f0_b43b_aba65e9952e3">
    <rdfs:comment xml:lang="en">bel is used to express the ratio of one value of a power or field quantity to another, on a logarithmic scale, the logarithmic quantity being called the power level or field level, respectively.</rdfs:comment>
    <EMMO_1f1b164d_ec6a_4faa_8d5e_88bda62316cc>http://qudt.org/vocab/unit/B</EMMO_1f1b164d_ec6a_4faa_8d5e_88bda62316cc>
    <rdfs:comment xml:lang="en">Today decibel (one tenth of a bel) is commonly used instead of bel.</rdfs:comment>
    <rdfs:subClassOf rdf:nodeID="ffcb99037244f48d590430c228d02afdbb33"/>
    <skos:prefLabel xml:lang="en">Bel</skos:prefLabel>
    <rdfs:subClassOf rdf:resource="http://emmo.info/emmo#EMMO_591e02fd_8d37_45a6_9d11_bb21cef391a0"/>
    <rdf:type rdf:resource="http://www.w3.org/2002/07/owl#Class"/>
    <EMMO_967080e5_2f42_4eb2_a3a9_c58143e835f9 xml:lang="en">Unit of measurement for quantities of type level or level difference.</EMMO_967080e5_2f42_4eb2_a3a9_c58143e835f9>
    <rdfs:subClassOf rdf:nodeID="ffcb99037244f48d590430c228d02afdbb34"/>
    <EMMO_70fe84ff_99b6_4206_a9fc_9a8931836d84 xml:lang="en">One bel is defined as `1⁄2 ln(10) neper`.</EMMO_70fe84ff_99b6_4206_a9fc_9a8931836d84>
    <EMMO_c84c6752_6d64_48cc_9500_e54a3c34898d>https://en.wikipedia.org/wiki/Decibel</EMMO_c84c6752_6d64_48cc_9500_e54a3c34898d>
  </rdf:Description>
  <rdf:Description rdf:about="http://emmo.info/emmo#EMMO_8303a247_f9d9_4616_bdcd_f5cbd7b298e3">
    <EMMO_967080e5_2f42_4eb2_a3a9_c58143e835f9 xml:lang="en">An bonded atom that shares at least one electron to the atom-based entity of which is part of.</EMMO_967080e5_2f42_4eb2_a3a9_c58143e835f9>
    <rdfs:subClassOf rdf:resource="http://emmo.info/emmo#EMMO_eb77076b_a104_42ac_a065_798b2d2809ad"/>
    <rdf:type rdf:resource="http://www.w3.org/2002/07/owl#Class"/>
    <skos:prefLabel xml:lang="en">BondedAtom</skos:prefLabel>
    <rdfs:comment xml:lang="en">The bond types that are covered by this definition are the strong electonic bonds: covalent, metallic and ionic.</rdfs:comment>
    <rdfs:comment xml:lang="en">This class can be used to represent molecules as simplified quantum systems, in which outer molecule shared electrons are un-entangled with the inner shells of the atoms composing the molecule.</rdfs:comment>
    <rdfs:comment xml:lang="en">A real bond between atoms is always something hybrid between covalent, metallic and ionic.

In general, metallic and ionic bonds have atoms sharing electrons.</rdfs:comment>
  </rdf:Description>
  <rdf:Description rdf:about="http://emmo.info/emmo#EMMO_18448443_dcf1_49b8_a321_cf46e2c393e1">
    <EMMO_967080e5_2f42_4eb2_a3a9_c58143e835f9 xml:lang="en">Unit for quantities of dimension one that are the fraction of two masses.</EMMO_967080e5_2f42_4eb2_a3a9_c58143e835f9>
    <skos:prefLabel xml:lang="en">MassFractionUnit</skos:prefLabel>
    <rdfs:subClassOf rdf:resource="http://emmo.info/emmo#EMMO_c2f5ee66_579c_44c6_a2e9_fa2eaa9fa4da"/>
    <EMMO_b432d2d5_25f4_4165_99c5_5935a7763c1a xml:lang="en">Unit for mass fraction.</EMMO_b432d2d5_25f4_4165_99c5_5935a7763c1a>
    <rdf:type rdf:resource="http://www.w3.org/2002/07/owl#Class"/>
  </rdf:Description>
  <rdf:Description rdf:about="http://emmo.info/emmo#EMMO_c457b6b9_5e73_4853_ae08_d776c12b8058">
    <EMMO_967080e5_2f42_4eb2_a3a9_c58143e835f9 xml:lang="en">A coarse dispersion of gas in a solid continuum phase.</EMMO_967080e5_2f42_4eb2_a3a9_c58143e835f9>
    <rdfs:subClassOf rdf:resource="http://emmo.info/emmo#EMMO_a2b006f2_bbfd_4dba_bcaa_3fca20cd6be1"/>
    <rdf:type rdf:resource="http://www.w3.org/2002/07/owl#Class"/>
    <skos:prefLabel xml:lang="en">SolidGasSuspension</skos:prefLabel>
  </rdf:Description>
  <rdf:Description rdf:nodeID="f8fb83657cd5f496db3c2b94baf326f26b12">
    <owl:onProperty rdf:resource="http://emmo.info/emmo#EMMO_23b579e1_8088_45b5_9975_064014026c42"/>
    <rdf:type rdf:resource="http://www.w3.org/2002/07/owl#Restriction"/>
    <owl:hasValue>T0 L0 M0 I0 Θ0 N0 J0</owl:hasValue>
  </rdf:Description>
  <rdf:Description rdf:nodeID="f05bdaa1e617a4bccafc519daf7bf4785b77">
    <owl:onProperty rdf:resource="http://emmo.info/emmo#EMMO_23b579e1_8088_45b5_9975_064014026c42"/>
    <rdf:type rdf:resource="http://www.w3.org/2002/07/owl#Restriction"/>
    <owl:hasValue>Ω</owl:hasValue>
  </rdf:Description>
  <rdf:Description rdf:about="http://emmo.info/emmo#EMMO_6e046dd0_9634_4013_b2b1_9cc468087c83">
    <rdfs:subPropertyOf rdf:resource="http://emmo.info/emmo#EMMO_9380ab64_0363_4804_b13f_3a8a94119a76"/>
    <rdf:type rdf:resource="http://www.w3.org/2002/07/owl#TransitiveProperty"/>
    <rdfs:domain rdf:resource="http://emmo.info/emmo#EMMO_eb3a768e_d53e_4be9_a23b_0714833c36de"/>
    <skos:prefLabel xml:lang="en">hasSpatioTemporalPart</skos:prefLabel>
    <EMMO_967080e5_2f42_4eb2_a3a9_c58143e835f9>A relation that isolates a proper part that extends itself in time through a portion of the lifetime whole.</EMMO_967080e5_2f42_4eb2_a3a9_c58143e835f9>
    <rdfs:range rdf:resource="http://emmo.info/emmo#EMMO_eb3a768e_d53e_4be9_a23b_0714833c36de"/>
    <rdf:type rdf:resource="http://www.w3.org/2002/07/owl#ObjectProperty"/>
  </rdf:Description>
  <rdf:Description rdf:nodeID="f8fb83657cd5f496db3c2b94baf326f26b24">
    <owl:allValuesFrom rdf:nodeID="f8fb83657cd5f496db3c2b94baf326f26b25"/>
    <owl:onProperty rdf:resource="http://emmo.info/emmo#EMMO_b2282816_b7a3_44c6_b2cb_3feff1ceb7fe"/>
    <rdf:type rdf:resource="http://www.w3.org/2002/07/owl#Restriction"/>
  </rdf:Description>
  <rdf:Description rdf:about="http://emmo.info/emmo#EMMO_1e0b665d_db6c_4752_a6d4_262d3a8dbb46">
    <EMMO_70fe84ff_99b6_4206_a9fc_9a8931836d84 xml:lang="en">Measure of plane angle defined as 1/60 or a degree.</EMMO_70fe84ff_99b6_4206_a9fc_9a8931836d84>
    <rdfs:subClassOf rdf:resource="http://emmo.info/emmo#EMMO_591e02fd_8d37_45a6_9d11_bb21cef391a0"/>
    <rdfs:subClassOf rdf:nodeID="ffcb99037244f48d590430c228d02afdbb7"/>
    <rdf:type rdf:resource="http://www.w3.org/2002/07/owl#Class"/>
    <skos:prefLabel xml:lang="en">ArcMinute</skos:prefLabel>
    <skos:altLabel xml:lang="en">MinuteOfArc</skos:altLabel>
    <rdfs:subClassOf rdf:nodeID="ffcb99037244f48d590430c228d02afdbb8"/>
    <EMMO_1f1b164d_ec6a_4faa_8d5e_88bda62316cc>http://qudt.org/vocab/unit/ARCMIN</EMMO_1f1b164d_ec6a_4faa_8d5e_88bda62316cc>
  </rdf:Description>
  <rdf:Description rdf:about="http://emmo.info/emmo#EMMO_44da6d75_54a4_4aa8_bd3a_156f6e9abb8e">
    <EMMO_70fe84ff_99b6_4206_a9fc_9a8931836d84 xml:lang="en">Vector r characterizing a point P in a point space with a given origin point O.</EMMO_70fe84ff_99b6_4206_a9fc_9a8931836d84>
    <rdfs:comment xml:lang="en">In the usual geometrical three-dimensional space, position vectors are quantities of the dimension length. 

-- IEC</rdfs:comment>
    <EMMO_de178b12_5d35_4bca_8efa_a4193162571d>T0 L+1 M0 I0 Θ0 N0 J0</EMMO_de178b12_5d35_4bca_8efa_a4193162571d>
    <skos:prefLabel xml:lang="en">PositionVector</skos:prefLabel>
    <skos:altLabel xml:lang="en">Position</skos:altLabel>
    <rdfs:subClassOf rdf:resource="http://emmo.info/emmo#EMMO_cd2cd0de_e0cc_4ef1_b27e_2e88db027bac"/>
    <rdf:type rdf:resource="http://www.w3.org/2002/07/owl#Class"/>
    <EMMO_50c298c2_55a2_4068_b3ac_4e948c33181f>http://www.electropedia.org/iev/iev.nsf/display?openform&amp;ievref=113-03-12</EMMO_50c298c2_55a2_4068_b3ac_4e948c33181f>
    <rdfs:comment xml:lang="en">Position vectors are so-called bounded vectors, i.e. their magnitude and direction depend on the particular coordinate system used.

-- ISO 80000-3</rdfs:comment>
  </rdf:Description>
  <rdf:Description rdf:nodeID="f05bdaa1e617a4bccafc519daf7bf4785b82">
    <owl:onProperty rdf:nodeID="f05bdaa1e617a4bccafc519daf7bf4785b83"/>
    <owl:allValuesFrom rdf:nodeID="f05bdaa1e617a4bccafc519daf7bf4785b84"/>
    <rdf:type rdf:resource="http://www.w3.org/2002/07/owl#Restriction"/>
  </rdf:Description>
  <rdf:Description rdf:about="http://emmo.info/emmo#EMMO_080052a1_f295_44be_a60f_1326ce13f1ba">
    <skos:prefLabel xml:lang="en">Watt</skos:prefLabel>
    <EMMO_fe015383_afb3_44a6_ae86_043628697aa2>https://doi.org/10.1351/goldbook.W06656</EMMO_fe015383_afb3_44a6_ae86_043628697aa2>
    <EMMO_1f1b164d_ec6a_4faa_8d5e_88bda62316cc>http://qudt.org/vocab/unit/W</EMMO_1f1b164d_ec6a_4faa_8d5e_88bda62316cc>
    <rdfs:subClassOf rdf:nodeID="f05bdaa1e617a4bccafc519daf7bf4785b8"/>
    <rdf:type rdf:resource="http://www.w3.org/2002/07/owl#Class"/>
    <rdfs:comment xml:lang="en">Measurement unit for power.</rdfs:comment>
    <rdfs:subClassOf rdf:nodeID="f05bdaa1e617a4bccafc519daf7bf4785b7"/>
  </rdf:Description>
  <rdf:Description rdf:nodeID="fe0b20157736f4a31909181349b2e6219b7">
    <rdf:type rdf:resource="http://www.w3.org/1999/02/22-rdf-syntax-ns#List"/>
    <rdf:rest rdf:nodeID="fe0b20157736f4a31909181349b2e6219b8"/>
    <rdf:first rdf:resource="http://emmo.info/emmo#EMMO_cd2cd0de_e0cc_4ef1_b27e_2e88db027bac"/>
  </rdf:Description>
  <rdf:Description rdf:nodeID="f8fb83657cd5f496db3c2b94baf326f26b17">
    <rdf:rest rdf:resource="http://www.w3.org/1999/02/22-rdf-syntax-ns#nil"/>
    <rdf:first rdf:resource="http://emmo.info/emmo#EMMO_a1083d0a_c1fb_471f_8e20_a98f881ad527"/>
    <rdf:type rdf:resource="http://www.w3.org/1999/02/22-rdf-syntax-ns#List"/>
  </rdf:Description>
  <rdf:Description rdf:about="http://emmo.info/emmo#EMMO_385b8f6e_43ac_4596_ad76_ac322c68b7ca">
    <rdf:type rdf:resource="http://www.w3.org/2002/07/owl#Class"/>
    <skos:prefLabel xml:lang="en">Massive</skos:prefLabel>
    <EMMO_967080e5_2f42_4eb2_a3a9_c58143e835f9 xml:lang="en">The union of classes of elementary particles that possess mass.</EMMO_967080e5_2f42_4eb2_a3a9_c58143e835f9>
    <owl:equivalentClass rdf:nodeID="fea11ca01461e402d8f697c19c5d8de88b1"/>
  </rdf:Description>
  <rdf:Description rdf:about="http://emmo.info/emmo#EMMO_25f5ca8e_8f7f_44d8_a392_bd3fe8894458">
    <rdf:type rdf:resource="http://www.w3.org/2002/07/owl#Class"/>
    <skos:prefLabel xml:lang="en">Plane</skos:prefLabel>
    <rdfs:subClassOf rdf:resource="http://emmo.info/emmo#EMMO_9268958f_7f54_48ab_a693_febe2645892b"/>
  </rdf:Description>
  <rdf:Description rdf:about="http://emmo.info/emmo#EMMO_b14d9be5_f81e_469b_abca_379c2e83feab">
    <rdfs:subClassOf rdf:resource="http://emmo.info/emmo#EMMO_9895a1b4_f0a5_4167_ac5e_97db40b8bfcc"/>
    <owl:equivalentClass rdf:nodeID="fe0b20157736f4a31909181349b2e6219b31"/>
    <skos:prefLabel xml:lang="en">CapacitanceDimension</skos:prefLabel>
    <rdf:type rdf:resource="http://www.w3.org/2002/07/owl#Class"/>
  </rdf:Description>
  <rdf:Description rdf:nodeID="f05bdaa1e617a4bccafc519daf7bf4785b78">
    <owl:allValuesFrom rdf:nodeID="f05bdaa1e617a4bccafc519daf7bf4785b80"/>
    <rdf:type rdf:resource="http://www.w3.org/2002/07/owl#Restriction"/>
    <owl:onProperty rdf:nodeID="f05bdaa1e617a4bccafc519daf7bf4785b79"/>
  </rdf:Description>
  <rdf:Description rdf:about="http://emmo.info/emmo#EMMO_df808271_df91_4f27_ba59_fa423c51896c">
    <rdf:type rdf:resource="http://www.w3.org/2002/07/owl#Class"/>
    <skos:prefLabel xml:lang="en">Neutron</skos:prefLabel>
  </rdf:Description>
  <rdf:Description rdf:about="http://emmo.info/emmo#EMMO_0e030040_98a7_49b2_a871_dced1f3a6131">
    <rdfs:subClassOf rdf:resource="http://emmo.info/emmo#EMMO_ec2c8ac8_98c5_4c74_b85b_ff8e8ca6655c"/>
    <EMMO_967080e5_2f42_4eb2_a3a9_c58143e835f9 xml:lang="en">A mixture in which more than one phases of matter cohexists.</EMMO_967080e5_2f42_4eb2_a3a9_c58143e835f9>
    <rdf:type rdf:resource="http://www.w3.org/2002/07/owl#Class"/>
    <skos:prefLabel xml:lang="en">PhaseHeterogeneousMixture</skos:prefLabel>
    <rdfs:subClassOf rdf:nodeID="ff14b31ebf90e4bc5ba2839064d29e543b4"/>
    <rdfs:comment xml:lang="en">Phase heterogenous mixture may share the same state of matter.

For example, immiscibile liquid phases (e.g. oil and water) constitute a mixture whose phases are clearly separated but share the same state of matter.</rdfs:comment>
  </rdf:Description>
  <rdf:Description rdf:nodeID="f05bdaa1e617a4bccafc519daf7bf4785b2">
    <rdf:type rdf:resource="http://www.w3.org/2002/07/owl#Restriction"/>
    <owl:onProperty rdf:resource="http://emmo.info/emmo#EMMO_23b579e1_8088_45b5_9975_064014026c42"/>
    <owl:hasValue>Gy</owl:hasValue>
  </rdf:Description>
  <rdf:Description rdf:nodeID="fe24a777e3fd743f986ce83488d2cf30bb30">
    <owl:qualifiedCardinality rdf:datatype="http://www.w3.org/2001/XMLSchema#nonNegativeInteger">1</owl:qualifiedCardinality>
  </rdf:Description>
  <rdf:Description rdf:about="http://emmo.info/emmo#EMMO_8d689295_7d84_421b_bc01_d5cceb2c2086">
    <EMMO_1f1b164d_ec6a_4faa_8d5e_88bda62316cc>http://qudt.org/vocab/constant/ProtonMass</EMMO_1f1b164d_ec6a_4faa_8d5e_88bda62316cc>
    <EMMO_fe015383_afb3_44a6_ae86_043628697aa2>https://doi.org/10.1351/goldbook.P04914</EMMO_fe015383_afb3_44a6_ae86_043628697aa2>
    <rdfs:comment xml:lang="en">The rest mass of a proton.</rdfs:comment>
    <rdf:type rdf:resource="http://www.w3.org/2002/07/owl#Class"/>
    <EMMO_a9b3d04c_7ceb_40a2_b8d3_28d514a770a8>https://physics.nist.gov/cgi-bin/cuu/Value?mp</EMMO_a9b3d04c_7ceb_40a2_b8d3_28d514a770a8>
    <rdfs:subClassOf rdf:resource="http://emmo.info/emmo#EMMO_3f15d200_c97b_42c8_8ac0_d81d150361e2"/>
    <EMMO_de178b12_5d35_4bca_8efa_a4193162571d>T0 L0 M+1 I0 Θ0 N0 J0</EMMO_de178b12_5d35_4bca_8efa_a4193162571d>
    <skos:prefLabel xml:lang="en">ProtonMass</skos:prefLabel>
    <rdfs:subClassOf rdf:resource="http://emmo.info/emmo#EMMO_ed4af7ae_63a2_497e_bb88_2309619ea405"/>
  </rdf:Description>
  <rdf:Description rdf:about="http://emmo.info/emmo#EMMO_1aed91a3_d00c_48af_8f43_a0c958b2512a">
    <rdfs:subClassOf rdf:resource="http://emmo.info/emmo#EMMO_f9bc8b52_85e9_4b53_b969_dd7724d5b8e4"/>
    <rdfs:comment xml:lang="en">An expression that has parts only integer constants, variables, and the algebraic operations (addition, subtraction, multiplication, division and exponentiation by an exponent that is a rational number)</rdfs:comment>
    <skos:prefLabel xml:lang="en">AlgebricExpression</skos:prefLabel>
    <rdf:type rdf:resource="http://www.w3.org/2002/07/owl#Class"/>
    <EMMO_b432d2d5_25f4_4165_99c5_5935a7763c1a xml:lang="en">2x+3</EMMO_b432d2d5_25f4_4165_99c5_5935a7763c1a>
  </rdf:Description>
  <rdf:Description rdf:about="http://emmo.info/emmo#EMMO_53e825d9_1a09_483c_baa7_37501ebfbe1c">
    <rdfs:subClassOf rdf:resource="http://emmo.info/emmo#EMMO_9895a1b4_f0a5_4167_ac5e_97db40b8bfcc"/>
    <owl:equivalentClass rdf:nodeID="fe0b20157736f4a31909181349b2e6219b20"/>
    <skos:prefLabel xml:lang="en">ForceDimension</skos:prefLabel>
    <rdf:type rdf:resource="http://www.w3.org/2002/07/owl#Class"/>
  </rdf:Description>
  <rdf:Description rdf:about="http://emmo.info/emmo#EMMO_d4f7d378_5e3b_468a_baa1_a7e98358cda7">
    <rdfs:comment xml:lang="en">Time can be seen as the duration of an event or, more operationally, as "what clocks read".</rdfs:comment>
    <EMMO_1f1b164d_ec6a_4faa_8d5e_88bda62316cc>qudt.org/vocab/quantitykind/Time</EMMO_1f1b164d_ec6a_4faa_8d5e_88bda62316cc>
    <EMMO_6dd685dd_1895_46e4_b227_be9f7d643c25>http://dbpedia.org/page/Time</EMMO_6dd685dd_1895_46e4_b227_be9f7d643c25>
    <EMMO_fe015383_afb3_44a6_ae86_043628697aa2>https://doi.org/10.1351/goldbook.T06375</EMMO_fe015383_afb3_44a6_ae86_043628697aa2>
    <EMMO_70fe84ff_99b6_4206_a9fc_9a8931836d84 xml:lang="en">One-dimensional subspace of space-time, which is locally orthogonal to space.</EMMO_70fe84ff_99b6_4206_a9fc_9a8931836d84>
    <EMMO_967080e5_2f42_4eb2_a3a9_c58143e835f9 xml:lang="en">The indefinite continued progress of existence and events that occur in apparently irreversible succession from the past through the present to the future.</EMMO_967080e5_2f42_4eb2_a3a9_c58143e835f9>
    <EMMO_50c298c2_55a2_4068_b3ac_4e948c33181f>http://www.electropedia.org/iev/iev.nsf/display?openform&amp;ievref=113-01-03</EMMO_50c298c2_55a2_4068_b3ac_4e948c33181f>
    <rdf:type rdf:resource="http://www.w3.org/2002/07/owl#Class"/>
    <skos:prefLabel xml:lang="en">Time</skos:prefLabel>
    <EMMO_de178b12_5d35_4bca_8efa_a4193162571d>T+1 L0 M0 I0 Θ0 N0 J0</EMMO_de178b12_5d35_4bca_8efa_a4193162571d>
  </rdf:Description>
  <rdf:Description rdf:about="http://emmo.info/emmo#EMMO_d8aa8e1f_b650_416d_88a0_5118de945456">
    <EMMO_b432d2d5_25f4_4165_99c5_5935a7763c1a xml:lang="en">The thermal conductivity of a copper sample in my laboratory can be assumed to be the conductivity that appears in the vendor specification. This value has been obtained by measurement of a sample which is not the one I have in my laboratory. This conductivity value is then a conventional quantitiative property assigned to my sample through a semiotic process in which no actual measurement is done by my laboratory.

If I don't believe the vendor, then I can measure the actual thermal conductivity. I then perform a measurement process that semiotically assign another value for the conductivity, which is a measured property, since is part of a measurement process.

Then I have two different physical quantities that are properties thanks to two different semiotic processes.</EMMO_b432d2d5_25f4_4165_99c5_5935a7763c1a>
    <rdf:type rdf:resource="http://www.w3.org/2002/07/owl#Class"/>
    <skos:prefLabel xml:lang="en">ConventionalQuantitativeProperty</skos:prefLabel>
    <rdfs:comment xml:lang="en">A property that is associated to an object by convention, or assumption.</rdfs:comment>
    <EMMO_967080e5_2f42_4eb2_a3a9_c58143e835f9 xml:lang="en">A quantitative property attributed by agreement to a quantity for a given purpose.</EMMO_967080e5_2f42_4eb2_a3a9_c58143e835f9>
  </rdf:Description>
  <rdf:Description rdf:nodeID="f05bdaa1e617a4bccafc519daf7bf4785b114">
    <owl:onProperty rdf:resource="http://emmo.info/emmo#EMMO_23b579e1_8088_45b5_9975_064014026c42"/>
    <rdf:type rdf:resource="http://www.w3.org/2002/07/owl#Restriction"/>
    <owl:hasValue>m</owl:hasValue>
  </rdf:Description>
  <rdf:Description rdf:about="http://emmo.info/emmo#EMMO_f8a2fe9f_458b_4771_9aba_a50e76afc52d">
    <rdf:type rdf:resource="http://www.w3.org/2002/07/owl#Class"/>
    <rdfs:subClassOf rdf:resource="http://emmo.info/emmo#EMMO_f6d0c26a_98b6_4cf8_8632_aa259131faaa"/>
    <skos:prefLabel xml:lang="en">DifferentialOperator</skos:prefLabel>
  </rdf:Description>
  <rdf:Description rdf:nodeID="f8fb83657cd5f496db3c2b94baf326f26b23">
    <rdf:rest rdf:resource="http://www.w3.org/1999/02/22-rdf-syntax-ns#nil"/>
    <rdf:type rdf:resource="http://www.w3.org/1999/02/22-rdf-syntax-ns#List"/>
    <rdf:first rdf:resource="http://emmo.info/emmo#EMMO_216f448e_cdbc_4aeb_a529_7a5fe7fc38bb"/>
  </rdf:Description>
  <rdf:Description rdf:about="http://emmo.info/emmo#EMMO_4a464c8d_8895_44a8_a628_aed13509f1bd">
    <rdf:type rdf:resource="http://www.w3.org/2002/07/owl#Class"/>
    <rdfs:comment xml:lang="en">Suspensions show no significant effect on light.</rdfs:comment>
    <rdfs:subClassOf rdf:resource="http://emmo.info/emmo#EMMO_0e030040_98a7_49b2_a871_dced1f3a6131"/>
    <skos:prefLabel xml:lang="en">Suspension</skos:prefLabel>
    <EMMO_967080e5_2f42_4eb2_a3a9_c58143e835f9 xml:lang="en">An heterogeneous mixture that contains coarsly dispersed particles (no Tyndall effect), that generally tend to separate in time to the dispersion medium phase.</EMMO_967080e5_2f42_4eb2_a3a9_c58143e835f9>
    <owl:disjointUnionOf rdf:nodeID="ff14b31ebf90e4bc5ba2839064d29e543b8"/>
  </rdf:Description>
  <rdf:Description rdf:about="http://emmo.info/emmo#EMMO_c6d4a5e0_7e95_44df_a6db_84ee0a8bbc8e">
    <rdfs:subClassOf rdf:nodeID="f8fb83657cd5f496db3c2b94baf326f26b36"/>
    <EMMO_967080e5_2f42_4eb2_a3a9_c58143e835f9 xml:lang="en">A measurement unit that is made of a metric prefix and a unit symbol.</EMMO_967080e5_2f42_4eb2_a3a9_c58143e835f9>
    <skos:prefLabel xml:lang="en">PrefixedUnit</skos:prefLabel>
    <owl:disjointUnionOf rdf:nodeID="f8fb83657cd5f496db3c2b94baf326f26b38"/>
    <rdfs:subClassOf rdf:nodeID="f8fb83657cd5f496db3c2b94baf326f26b37"/>
    <rdfs:subClassOf rdf:nodeID="f8fb83657cd5f496db3c2b94baf326f26b32"/>
    <rdf:type rdf:resource="http://www.w3.org/2002/07/owl#Class"/>
  </rdf:Description>
  <rdf:Description rdf:about="http://emmo.info/emmo#EMMO_a6138ba7_e365_4f2d_b6b4_fe5a5918d403">
    <rdfs:subClassOf rdf:resource="http://emmo.info/emmo#EMMO_e56ee3eb_7609_4ae1_8bed_51974f0960a6"/>
    <rdf:type rdf:resource="http://www.w3.org/2002/07/owl#Class"/>
    <skos:prefLabel xml:lang="en">ArithmeticEquation</skos:prefLabel>
    <EMMO_b432d2d5_25f4_4165_99c5_5935a7763c1a xml:lang="en">1 + 1 = 2</EMMO_b432d2d5_25f4_4165_99c5_5935a7763c1a>
  </rdf:Description>
  <rdf:Description rdf:about="http://emmo.info/emmo#EMMO_da831168_975a_41f8_baae_279c298569da">
    <rdf:type rdf:resource="http://www.w3.org/2002/07/owl#Class"/>
    <rdfs:subClassOf rdf:resource="http://emmo.info/emmo#EMMO_3f15d200_c97b_42c8_8ac0_d81d150361e2"/>
    <EMMO_a9b3d04c_7ceb_40a2_b8d3_28d514a770a8>https://physics.nist.gov/cgi-bin/cuu/Value?bg</EMMO_a9b3d04c_7ceb_40a2_b8d3_28d514a770a8>
    <EMMO_1f1b164d_ec6a_4faa_8d5e_88bda62316cc>http://qudt.org/vocab/constant/NewtonianConstantOfGravitation</EMMO_1f1b164d_ec6a_4faa_8d5e_88bda62316cc>
    <EMMO_de178b12_5d35_4bca_8efa_a4193162571d>T-2 L+3 M-1 I0 Θ0 N0 J0</EMMO_de178b12_5d35_4bca_8efa_a4193162571d>
    <EMMO_6dd685dd_1895_46e4_b227_be9f7d643c25>http://dbpedia.org/page/Gravitational_constant</EMMO_6dd685dd_1895_46e4_b227_be9f7d643c25>
    <skos:prefLabel xml:lang="en">NewtonianConstantOfGravity</skos:prefLabel>
    <EMMO_fe015383_afb3_44a6_ae86_043628697aa2>https://doi.org/10.1351/goldbook.G02695</EMMO_fe015383_afb3_44a6_ae86_043628697aa2>
    <rdfs:comment xml:lang="en">Physical constant in Newton's law of gravitation and in Einstein's general theory of relativity.</rdfs:comment>
  </rdf:Description>
  <rdf:Description rdf:nodeID="f05bdaa1e617a4bccafc519daf7bf4785b27">
    <owl:onProperty rdf:resource="http://emmo.info/emmo#EMMO_faf79f53_749d_40b2_807c_d34244c192f4"/>
    <owl:hasValue rdf:datatype="http://www.w3.org/2001/XMLSchema#double">1e-21</owl:hasValue>
    <rdf:type rdf:resource="http://www.w3.org/2002/07/owl#Restriction"/>
  </rdf:Description>
  <rdf:Description rdf:nodeID="fe0b20157736f4a31909181349b2e6219b12">
    <owl:hasValue>T+3 L-2 M-1 I+2 Θ0 N0 J0</owl:hasValue>
    <owl:onProperty rdf:resource="http://emmo.info/emmo#EMMO_23b579e1_8088_45b5_9975_064014026c42"/>
    <rdf:type rdf:resource="http://www.w3.org/2002/07/owl#Restriction"/>
  </rdf:Description>
  <rdf:Description rdf:about="http://emmo.info/emmo#EMMO_707c6032_e272_4a20_98b5_d35c4f67be68">
    <rdf:type rdf:resource="http://www.w3.org/2002/07/owl#Class"/>
    <rdfs:comment xml:lang="en">Derived units are defined as products of powers of the base units. When the numerical factor of this product is one, the derived units are called coherent derived units. The base and coherent derived units of the SI form a coherent set, designated the set of coherent SI units.</rdfs:comment>
    <owl:disjointUnionOf rdf:nodeID="f05bdaa1e617a4bccafc519daf7bf4785b88"/>
    <skos:prefLabel xml:lang="en">SICoherentUnit</skos:prefLabel>
  </rdf:Description>
  <rdf:Description rdf:about="http://emmo.info/emmo#EMMO_3397f270_dfc1_4500_8f6f_4d0d85ac5f71">
    <rdfs:subClassOf rdf:resource="http://emmo.info/emmo#EMMO_5b2222df_4da6_442f_8244_96e9e45887d1"/>
    <rdf:type rdf:resource="http://www.w3.org/2002/07/owl#Class"/>
    <rdfs:comment xml:lang="en">This definition states that this object is a non-periodic set of atoms or a set with a finite periodicity.

Removing an atom from the state will result in another type of atom_based state.

e.g. you cannot remove H from H20 without changing the molecule type (essential). However, you can remove a C from a nanotube (redundant). C60 fullerene is a molecule, since it has a finite periodicity and is made of a well defined number of atoms (essential). A C nanotube is not a molecule, since it has an infinite periodicity (redundant).</rdfs:comment>
    <rdfs:comment xml:lang="en">An entity is called essential if removing one direct part will lead to a change in entity class.

An entity is called redundand if removing one direct part will not lead to a change in entity class.</rdfs:comment>
    <EMMO_b432d2d5_25f4_4165_99c5_5935a7763c1a xml:lang="en">H20, C6H12O6, CH4</EMMO_b432d2d5_25f4_4165_99c5_5935a7763c1a>
    <EMMO_967080e5_2f42_4eb2_a3a9_c58143e835f9 xml:lang="en">An atom_based state defined by an exact number of e-bonded atomic species and an electron cloud made of the shared electrons.</EMMO_967080e5_2f42_4eb2_a3a9_c58143e835f9>
    <skos:prefLabel xml:lang="en">Molecule</skos:prefLabel>
  </rdf:Description>
  <rdf:Description rdf:nodeID="f05bdaa1e617a4bccafc519daf7bf4785b162">
    <owl:inverseOf rdf:resource="http://emmo.info/emmo#EMMO_3446e167_c576_49d6_846c_215bb8878a55"/>
  </rdf:Description>
  <rdf:Description rdf:nodeID="fe0b20157736f4a31909181349b2e6219b40">
    <rdf:type rdf:resource="http://www.w3.org/2002/07/owl#Restriction"/>
    <owl:onProperty rdf:resource="http://emmo.info/emmo#EMMO_23b579e1_8088_45b5_9975_064014026c42"/>
    <owl:hasValue>T-2 L+2 M+1 I0 Θ0 N0 J0</owl:hasValue>
  </rdf:Description>
  <rdf:Description rdf:nodeID="f05bdaa1e617a4bccafc519daf7bf4785b181">
    <rdf:rest rdf:nodeID="f05bdaa1e617a4bccafc519daf7bf4785b182"/>
    <rdf:first rdf:resource="http://emmo.info/emmo#EMMO_da1dd4a7_c611_4ad4_bef6_7646f28aa598"/>
    <rdf:type rdf:resource="http://www.w3.org/1999/02/22-rdf-syntax-ns#List"/>
  </rdf:Description>
  <rdf:Description rdf:about="http://emmo.info/emmo#EMMO_3ecff38b_b3cf_4a78_b49f_8580abf8715b">
    <rdf:type rdf:resource="http://www.w3.org/2002/07/owl#Class"/>
    <skos:prefLabel xml:lang="en">EntropyDimension</skos:prefLabel>
    <owl:equivalentClass rdf:nodeID="fe0b20157736f4a31909181349b2e6219b14"/>
    <rdfs:subClassOf rdf:resource="http://emmo.info/emmo#EMMO_9895a1b4_f0a5_4167_ac5e_97db40b8bfcc"/>
  </rdf:Description>
  <rdf:Description rdf:about="http://emmo.info/emmo/middle/manufacturing">
    <rdfs:comment xml:lang="en">Contacts:
Gerhard Goldbeck
Goldbeck Consulting Ltd (UK)
email: gerhard@goldbeck-consulting.com

Emanuele Ghedini
University of Bologna (IT)
email: emanuele.ghedini@unibo.it</rdfs:comment>
    <dcterms:contributor>Goldbeck Consulting Ltd (UK)</dcterms:contributor>
    <dcterms:abstract xml:lang="en">European Materials &amp; Modelling Ontology (EMMO)

EMMO is a multidisciplinary effort to develop a standard representational framework (the ontology) based on current materials modelling knowledge, including physical sciences, analytical philosophy and information and communication technologies.

It provides the connection between the physical world, materials characterisation world and materials modelling world.

EMMO is released under a Creative Commons license Attribution 4.0 International (CC BY 4.0).</dcterms:abstract>
    <owl:versionIRI rdf:resource="http://emmo.info/emmo/1.0.0-beta/middle/manufacturing"/>
    <dcterms:creator>Gerhard Goldbeck</dcterms:creator>
    <dcterms:creator>Emanuele Ghedini</dcterms:creator>
    <dcterms:publisher>EMMC ASBL</dcterms:publisher>
    <dcterms:contributor>University of Bologna, IT</dcterms:contributor>
    <dcterms:creator>Jesper Friis</dcterms:creator>
    <dcterms:creator>Georg Schmitz</dcterms:creator>
    <owl:versionInfo>1.0.0-beta</owl:versionInfo>
    <dcterms:contributor>Fraunhofer IWM, DE</dcterms:contributor>
    <dcterms:contributor>Access, DE</dcterms:contributor>
    <rdf:type rdf:resource="http://www.w3.org/2002/07/owl#Ontology"/>
    <dcterms:title xml:lang="en">European Materials &amp; Modelling Ontology</dcterms:title>
    <rdfs:comment xml:lang="en">The EMMO requires FacT++ reasoner plugin in order to visualize all inferences and class hierarchy (ctrl+R hotkey in Protege).</rdfs:comment>
    <dcterms:creator>Adham Hashibon</dcterms:creator>
    <dcterms:license>https://creativecommons.org/licenses/by/4.0/legalcode</dcterms:license>
    <dcterms:contributor>SINTEF, NO</dcterms:contributor>
  </rdf:Description>
  <rdf:Description rdf:about="http://emmo.info/emmo#EMMO_4a27950a_0d31_4175_bd4e_14995aa94702">
    <rdf:type rdf:resource="http://www.w3.org/2002/07/owl#Class"/>
    <EMMO_e55f2d7c_9893_48cd_b4a4_fdf38253bd20>http://www.ontology-of-units-of-measure.org/resource/om-2/metrePerSecond-Time</EMMO_e55f2d7c_9893_48cd_b4a4_fdf38253bd20>
    <rdfs:subClassOf rdf:resource="http://emmo.info/emmo#EMMO_1273eb34_de48_43a9_925f_104110469dd2"/>
    <skos:prefLabel xml:lang="en">MetrePerSecond</skos:prefLabel>
    <rdfs:subClassOf rdf:nodeID="ffcb99037244f48d590430c228d02afdbb15"/>
    <EMMO_1f1b164d_ec6a_4faa_8d5e_88bda62316cc>http://qudt.org/vocab/unit/M-PER-SEC</EMMO_1f1b164d_ec6a_4faa_8d5e_88bda62316cc>
    <EMMO_967080e5_2f42_4eb2_a3a9_c58143e835f9 xml:lang="en">SI coherent measurement unit for speed.</EMMO_967080e5_2f42_4eb2_a3a9_c58143e835f9>
  </rdf:Description>
  <rdf:Description rdf:about="http://emmo.info/emmo#EMMO_4f2d3939_91b1_4001_b8ab_7d19074bf845">
    <EMMO_6dd685dd_1895_46e4_b227_be9f7d643c25>http://dbpedia.org/page/Voltage</EMMO_6dd685dd_1895_46e4_b227_be9f7d643c25>
    <EMMO_967080e5_2f42_4eb2_a3a9_c58143e835f9 xml:lang="en">Energy required to move a unit charge through an electric field from a reference point.</EMMO_967080e5_2f42_4eb2_a3a9_c58143e835f9>
    <rdf:type rdf:resource="http://www.w3.org/2002/07/owl#Class"/>
    <skos:prefLabel xml:lang="en">ElectricPotential</skos:prefLabel>
    <rdfs:subClassOf rdf:resource="http://emmo.info/emmo#EMMO_2946d40b_24a1_47fa_8176_e3f79bb45064"/>
    <skos:altLabel xml:lang="en">Voltage</skos:altLabel>
    <EMMO_fe015383_afb3_44a6_ae86_043628697aa2>https://doi.org/10.1351/goldbook.A00424</EMMO_fe015383_afb3_44a6_ae86_043628697aa2>
    <EMMO_1f1b164d_ec6a_4faa_8d5e_88bda62316cc>http://qudt.org/vocab/quantitykind/Voltage</EMMO_1f1b164d_ec6a_4faa_8d5e_88bda62316cc>
    <EMMO_de178b12_5d35_4bca_8efa_a4193162571d>T-3 L+2 M+1 I-1 Θ0 N0 J0</EMMO_de178b12_5d35_4bca_8efa_a4193162571d>
  </rdf:Description>
  <rdf:Description rdf:about="http://emmo.info/emmo#EMMO_6eca09be_17e9_445e_abc9_000aa61b7a11">
    <EMMO_b432d2d5_25f4_4165_99c5_5935a7763c1a xml:lang="en">Density functional theory.
Hartree-Fock.</EMMO_b432d2d5_25f4_4165_99c5_5935a7763c1a>
    <rdf:type rdf:resource="http://www.w3.org/2002/07/owl#Class"/>
    <EMMO_967080e5_2f42_4eb2_a3a9_c58143e835f9 xml:lang="en">A physics-based model based on a physics equation describing the behaviour of electrons.</EMMO_967080e5_2f42_4eb2_a3a9_c58143e835f9>
    <rdfs:subClassOf rdf:resource="http://emmo.info/emmo#EMMO_b29fd350_39aa_4af7_9459_3faa0544cba6"/>
    <skos:prefLabel xml:lang="en">ElectronicModel</skos:prefLabel>
  </rdf:Description>
  <rdf:Description rdf:about="http://emmo.info/emmo/top/mereotopology">
    <dcterms:creator>Adham Hashibon</dcterms:creator>
    <owl:versionInfo>1.0.0-beta</owl:versionInfo>
    <dcterms:license>https://creativecommons.org/licenses/by/4.0/legalcode</dcterms:license>
    <dcterms:contributor>Fraunhofer IWM, DE</dcterms:contributor>
    <dcterms:creator>Jesper Friis</dcterms:creator>
    <rdfs:comment xml:lang="en">Contacts:
Gerhard Goldbeck
Goldbeck Consulting Ltd (UK)
email: gerhard@goldbeck-consulting.com

Emanuele Ghedini
University of Bologna (IT)
email: emanuele.ghedini@unibo.it</rdfs:comment>
    <rdf:type rdf:resource="http://www.w3.org/2002/07/owl#Ontology"/>
    <dcterms:title xml:lang="en">European Materials &amp; Modelling Ontology</dcterms:title>
    <owl:versionIRI rdf:resource="http://emmo.info/emmo/1.0.0-beta/top/mereotopology"/>
    <dcterms:contributor>University of Bologna, IT</dcterms:contributor>
    <dcterms:abstract xml:lang="en">European Materials &amp; Modelling Ontology (EMMO)

EMMO is a multidisciplinary effort to develop a standard representational framework (the ontology) based on current materials modelling knowledge, including physical sciences, analytical philosophy and information and communication technologies.

It provides the connection between the physical world, materials characterisation world and materials modelling world.

EMMO is released under a Creative Commons license Attribution 4.0 International (CC BY 4.0).</dcterms:abstract>
    <rdfs:comment xml:lang="en">The EMMO requires FacT++ reasoner plugin in order to visualize all inferences and class hierarchy (ctrl+R hotkey in Protege).</rdfs:comment>
    <dcterms:contributor>Goldbeck Consulting Ltd (UK)</dcterms:contributor>
    <dcterms:contributor>SINTEF, NO</dcterms:contributor>
    <dcterms:creator>Georg Schmitz</dcterms:creator>
    <dcterms:creator>Gerhard Goldbeck</dcterms:creator>
    <dcterms:contributor>Access, DE</dcterms:contributor>
    <dcterms:creator>Emanuele Ghedini</dcterms:creator>
    <dcterms:publisher>EMMC ASBL</dcterms:publisher>
  </rdf:Description>
  <rdf:Description rdf:about="http://emmo.info/emmo#EMMO_4354ac74_7425_43ab_92e4_6dc19d1afee9">
    <EMMO_967080e5_2f42_4eb2_a3a9_c58143e835f9 xml:lang="en">A type of sol in the form of one solid dispersed in liquid.</EMMO_967080e5_2f42_4eb2_a3a9_c58143e835f9>
    <rdfs:subClassOf rdf:resource="http://emmo.info/emmo#EMMO_7509da43_56b1_4d7f_887a_65d1663df4ba"/>
    <rdfs:subClassOf rdf:resource="http://emmo.info/emmo#EMMO_31557fae_b039_491c_bcbb_0ccb8711d5a6"/>
    <rdf:type rdf:resource="http://www.w3.org/2002/07/owl#Class"/>
    <skos:prefLabel xml:lang="en">LiquidSol</skos:prefLabel>
  </rdf:Description>
  <rdf:Description rdf:about="http://emmo.info/emmo#EMMO_c995ae70_3b84_4ebb_bcfc_69e6a281bb88">
    <EMMO_1f1b164d_ec6a_4faa_8d5e_88bda62316cc>http://qudt.org/vocab/quantitykind/ElectricCurrent</EMMO_1f1b164d_ec6a_4faa_8d5e_88bda62316cc>
    <EMMO_fe015383_afb3_44a6_ae86_043628697aa2>https://doi.org/10.1351/goldbook.E01927</EMMO_fe015383_afb3_44a6_ae86_043628697aa2>
    <EMMO_de178b12_5d35_4bca_8efa_a4193162571d>T0 L0 M0 I+1 Θ0 N0 J0</EMMO_de178b12_5d35_4bca_8efa_a4193162571d>
    <EMMO_967080e5_2f42_4eb2_a3a9_c58143e835f9 xml:lang="en">A flow of electric charge.</EMMO_967080e5_2f42_4eb2_a3a9_c58143e835f9>
    <skos:prefLabel xml:lang="en">ElectricCurrent</skos:prefLabel>
    <EMMO_6dd685dd_1895_46e4_b227_be9f7d643c25>http://dbpedia.org/page/Electric_current</EMMO_6dd685dd_1895_46e4_b227_be9f7d643c25>
    <rdf:type rdf:resource="http://www.w3.org/2002/07/owl#Class"/>
  </rdf:Description>
  <rdf:Description rdf:about="http://emmo.info/emmo#EMMO_08b308d4_31cd_4779_a784_aa92fc730f39">
    <skos:prefLabel xml:lang="en">DerivedUnit</skos:prefLabel>
    <rdf:type rdf:resource="http://www.w3.org/2002/07/owl#Class"/>
    <EMMO_967080e5_2f42_4eb2_a3a9_c58143e835f9 xml:lang="en">Derived units are defined as products of powers of the base units corresponding to the relations defining the derived quantities in terms of the base quantities.</EMMO_967080e5_2f42_4eb2_a3a9_c58143e835f9>
  </rdf:Description>
  <rdf:Description rdf:nodeID="ffbe75b10062f400ea693809785c50a44b2">
    <owl:inverseOf rdf:resource="http://emmo.info/emmo#EMMO_c5aae418_1622_4d02_93c5_21159e28e6c1"/>
  </rdf:Description>
  <rdf:Description rdf:nodeID="fdb1489b80bcc4ee28afe0be8feb9b935b6">
    <owl:someValuesFrom rdf:resource="http://emmo.info/emmo#EMMO_f2d5d3ad_2e00_417f_8849_686f3988d929"/>
    <rdf:type rdf:resource="http://www.w3.org/2002/07/owl#Restriction"/>
    <owl:onProperty rdf:resource="http://emmo.info/emmo#EMMO_ae2d1a96_bfa1_409a_a7d2_03d69e8a125a"/>
  </rdf:Description>
  <rdf:Description rdf:nodeID="ffcb99037244f48d590430c228d02afdbb19">
    <rdf:type rdf:resource="http://www.w3.org/1999/02/22-rdf-syntax-ns#List"/>
    <rdf:first rdf:resource="http://emmo.info/emmo#EMMO_1e0b665d_db6c_4752_a6d4_262d3a8dbb46"/>
    <rdf:rest rdf:nodeID="ffcb99037244f48d590430c228d02afdbb20"/>
  </rdf:Description>
  <rdf:Description rdf:nodeID="ff14b31ebf90e4bc5ba2839064d29e543b21">
    <rdf:first rdf:resource="http://emmo.info/emmo#EMMO_7509da43_56b1_4d7f_887a_65d1663df4ba"/>
    <rdf:rest rdf:nodeID="ff14b31ebf90e4bc5ba2839064d29e543b22"/>
    <rdf:type rdf:resource="http://www.w3.org/1999/02/22-rdf-syntax-ns#List"/>
  </rdf:Description>
  <rdf:Description rdf:nodeID="ffcb99037244f48d590430c228d02afdbb3">
    <rdf:type rdf:resource="http://www.w3.org/2002/07/owl#Restriction"/>
    <owl:allValuesFrom rdf:resource="http://emmo.info/emmo#EMMO_f76f5a24_d703_4e8c_b368_f9a7777cb73a"/>
    <owl:onProperty rdf:resource="http://emmo.info/emmo#EMMO_67fc0a36_8dcb_4ffa_9a43_31074efa3296"/>
  </rdf:Description>
  <rdf:Description rdf:about="http://emmo.info/emmo#EMMO_9380ab64_0363_4804_b13f_3a8a94119a76">
    <rdfs:subPropertyOf rdf:resource="http://emmo.info/emmo#EMMO_17e27c22_37e1_468c_9dd7_95e137f73e7f"/>
    <rdf:type rdf:resource="http://www.w3.org/2002/07/owl#ObjectProperty"/>
    <rdf:type rdf:resource="http://www.w3.org/2002/07/owl#TransitiveProperty"/>
    <skos:prefLabel xml:lang="en">hasProperPart</skos:prefLabel>
  </rdf:Description>
  <rdf:Description rdf:nodeID="f05bdaa1e617a4bccafc519daf7bf4785b115">
    <owl:someValuesFrom rdf:resource="http://emmo.info/emmo#EMMO_53bd0c90_41c3_46e2_8779_cd2a80f7e18b"/>
    <owl:onProperty rdf:resource="http://emmo.info/emmo#EMMO_bed1d005_b04e_4a90_94cf_02bc678a8569"/>
    <rdf:type rdf:resource="http://www.w3.org/2002/07/owl#Restriction"/>
  </rdf:Description>
  <rdf:Description rdf:nodeID="f05bdaa1e617a4bccafc519daf7bf4785b131">
    <rdf:type rdf:resource="http://www.w3.org/2002/07/owl#Restriction"/>
    <owl:onProperty rdf:resource="http://emmo.info/emmo#EMMO_faf79f53_749d_40b2_807c_d34244c192f4"/>
    <owl:hasValue rdf:datatype="http://www.w3.org/2001/XMLSchema#double">0.01</owl:hasValue>
  </rdf:Description>
  <rdf:Description rdf:about="http://emmo.info/emmo/top/physical">
    <owl:versionIRI rdf:resource="http://emmo.info/emmo/1.0.0-beta/top/physical"/>
    <dcterms:abstract xml:lang="en">European Materials &amp; Modelling Ontology (EMMO)

EMMO is a multidisciplinary effort to develop a standard representational framework (the ontology) based on current materials modelling knowledge, including physical sciences, analytical philosophy and information and communication technologies.

It provides the connection between the physical world, materials characterisation world and materials modelling world.

EMMO is released under a Creative Commons license Attribution 4.0 International (CC BY 4.0).</dcterms:abstract>
    <dcterms:license>https://creativecommons.org/licenses/by/4.0/legalcode</dcterms:license>
    <dcterms:creator>Jesper Friis</dcterms:creator>
    <dcterms:contributor>SINTEF, NO</dcterms:contributor>
    <dcterms:contributor>Goldbeck Consulting Ltd (UK)</dcterms:contributor>
    <dcterms:contributor>Access, DE</dcterms:contributor>
    <dcterms:creator>Emanuele Ghedini</dcterms:creator>
    <dcterms:creator>Adham Hashibon</dcterms:creator>
    <dcterms:contributor>University of Bologna, IT</dcterms:contributor>
    <rdfs:comment xml:lang="en">Contacts:
Gerhard Goldbeck
Goldbeck Consulting Ltd (UK)
email: gerhard@goldbeck-consulting.com

Emanuele Ghedini
University of Bologna (IT)
email: emanuele.ghedini@unibo.it</rdfs:comment>
    <dcterms:contributor>Fraunhofer IWM, DE</dcterms:contributor>
    <owl:versionInfo>1.0.0-beta</owl:versionInfo>
    <dcterms:creator>Georg Schmitz</dcterms:creator>
    <dcterms:creator>Gerhard Goldbeck</dcterms:creator>
    <rdfs:comment xml:lang="en">The EMMO requires FacT++ reasoner plugin in order to visualize all inferences and class hierarchy (ctrl+R hotkey in Protege).</rdfs:comment>
    <rdf:type rdf:resource="http://www.w3.org/2002/07/owl#Ontology"/>
    <dcterms:title xml:lang="en">European Materials &amp; Modelling Ontology</dcterms:title>
    <dcterms:publisher>EMMC ASBL</dcterms:publisher>
  </rdf:Description>
  <rdf:Description rdf:about="http://emmo.info/emmo#EMMO_81e767f1_59b1_4d7a_bf69_17f322241831">
    <EMMO_967080e5_2f42_4eb2_a3a9_c58143e835f9 xml:lang="en">Vector quantity μ causing a change to its energy ΔW in an external magnetic field of field flux density B:

    ΔW = −μ · B</EMMO_967080e5_2f42_4eb2_a3a9_c58143e835f9>
    <EMMO_de178b12_5d35_4bca_8efa_a4193162571d>T0 L+2 M0 I+1 Θ0 N0 J0</EMMO_de178b12_5d35_4bca_8efa_a4193162571d>
    <EMMO_50c298c2_55a2_4068_b3ac_4e948c33181f>http://www.electropedia.org/iev/iev.nsf/display?openform&amp;ievref=121-11-55</EMMO_50c298c2_55a2_4068_b3ac_4e948c33181f>
    <EMMO_6dd685dd_1895_46e4_b227_be9f7d643c25>http://dbpedia.org/page/Magnetic_moment</EMMO_6dd685dd_1895_46e4_b227_be9f7d643c25>
    <EMMO_1f1b164d_ec6a_4faa_8d5e_88bda62316cc>http://qudt.org/vocab/quantitykind/MagneticDipoleMoment</EMMO_1f1b164d_ec6a_4faa_8d5e_88bda62316cc>
    <skos:prefLabel xml:lang="en">MagneticDipoleMoment</skos:prefLabel>
    <rdfs:comment xml:lang="en">For an atom or nucleus, this energy is quantized and can be written as:

    W = g μ M B

where g is the appropriate g factor, μ is mostly the Bohr magneton or nuclear magneton, M is magnetic quantum number, and B is magnitude of the magnetic flux density.

-- ISO 80000</rdfs:comment>
    <rdfs:subClassOf rdf:resource="http://emmo.info/emmo#EMMO_2946d40b_24a1_47fa_8176_e3f79bb45064"/>
    <EMMO_fe015383_afb3_44a6_ae86_043628697aa2>http://goldbook.iupac.org/terms/view/M03688</EMMO_fe015383_afb3_44a6_ae86_043628697aa2>
    <rdf:type rdf:resource="http://www.w3.org/2002/07/owl#Class"/>
    <EMMO_8de5d5bf_db1c_40ac_b698_095ba3b18578>10-9.1</EMMO_8de5d5bf_db1c_40ac_b698_095ba3b18578>
  </rdf:Description>
  <rdf:Description rdf:about="http://emmo.info/emmo#EMMO_04cc9451_5306_45d0_8554_22cee4d6e785">
    <EMMO_de178b12_5d35_4bca_8efa_a4193162571d>T-2 L+2 M+1 I-2 Θ0 N0 J0</EMMO_de178b12_5d35_4bca_8efa_a4193162571d>
    <rdf:type rdf:resource="http://www.w3.org/2002/07/owl#Class"/>
    <EMMO_fe015383_afb3_44a6_ae86_043628697aa2>https://doi.org/10.1351/goldbook.M04076</EMMO_fe015383_afb3_44a6_ae86_043628697aa2>
    <EMMO_6dd685dd_1895_46e4_b227_be9f7d643c25>http://dbpedia.org/page/Inductance</EMMO_6dd685dd_1895_46e4_b227_be9f7d643c25>
    <EMMO_967080e5_2f42_4eb2_a3a9_c58143e835f9 xml:lang="en">A property of an electrical conductor by which a change in current through it induces an electromotive force in both the conductor itself and in any nearby conductors by mutual inductance.</EMMO_967080e5_2f42_4eb2_a3a9_c58143e835f9>
    <EMMO_1f1b164d_ec6a_4faa_8d5e_88bda62316cc>http://qudt.org/vocab/quantitykind/Inductance</EMMO_1f1b164d_ec6a_4faa_8d5e_88bda62316cc>
    <rdfs:subClassOf rdf:resource="http://emmo.info/emmo#EMMO_2946d40b_24a1_47fa_8176_e3f79bb45064"/>
    <skos:altLabel xml:lang="en">Inductance</skos:altLabel>
    <skos:prefLabel xml:lang="en">ElectricInductance</skos:prefLabel>
  </rdf:Description>
  <rdf:Description rdf:about="http://emmo.info/emmo#EMMO_668fbd5b_6f1b_405c_9c6b_d6067bd0595a">
    <EMMO_967080e5_2f42_4eb2_a3a9_c58143e835f9 xml:lang="en">A matter object throughout which all physical properties of a material are essentially uniform.</EMMO_967080e5_2f42_4eb2_a3a9_c58143e835f9>
    <skos:prefLabel xml:lang="en">PhaseOfMatter</skos:prefLabel>
    <rdfs:subClassOf rdf:resource="http://emmo.info/emmo#EMMO_5b2222df_4da6_442f_8244_96e9e45887d1"/>
    <rdf:type rdf:resource="http://www.w3.org/2002/07/owl#Class"/>
    <rdfs:comment xml:lang="en">In the physical sciences, a phase is a region of space (a thermodynamic system), throughout which all physical properties of a material are essentially uniform. Examples of physical properties include density, index of refraction, magnetization and chemical composition. A simple description is that a phase is a region of material that is chemically uniform, physically distinct, and (often) mechanically separable. In a system consisting of ice and water in a glass jar, the ice cubes are one phase, the water is a second phase, and the humid air is a third phase over the ice and water. The glass of the jar is another separate phase.

The term phase is sometimes used as a synonym for state of matter, but there can be several immiscible phases of the same state of matter. Also, the term phase is sometimes used to refer to a set of equilibrium states demarcated in terms of state variables such as pressure and temperature by a phase boundary on a phase diagram. Because phase boundaries relate to changes in the organization of matter, such as a change from liquid to solid or a more subtle change from one crystal structure to another, this latter usage is similar to the use of "phase" as a synonym for state of matter. However, the state of matter and phase diagram usages are not commensurate with the formal definition given above and the intended meaning must be determined in part from the context in which the term is used.

[https://en.wikipedia.org/wiki/Phase_(matter)]</rdfs:comment>
    <rdfs:subClassOf rdf:resource="http://emmo.info/emmo#EMMO_8b0923ab_b500_477b_9ce9_8b3a3e4dc4f2"/>
  </rdf:Description>
  <rdf:Description rdf:about="http://emmo.info/emmo#EMMO_d7d2ca25_03e1_4099_9220_c1a58df13ad0">
    <rdf:type rdf:resource="http://www.w3.org/2002/07/owl#Class"/>
    <EMMO_a9b3d04c_7ceb_40a2_b8d3_28d514a770a8>https://physics.nist.gov/cgi-bin/cuu/Value?alph</EMMO_a9b3d04c_7ceb_40a2_b8d3_28d514a770a8>
    <EMMO_de178b12_5d35_4bca_8efa_a4193162571d>T0 L0 M0 I0 Θ0 N0 J0</EMMO_de178b12_5d35_4bca_8efa_a4193162571d>
    <rdfs:comment xml:lang="en">A fundamental physical constant characterizing the strength of the electromagnetic interaction between elementary charged particles.</rdfs:comment>
    <EMMO_fe015383_afb3_44a6_ae86_043628697aa2>https://doi.org/10.1351/goldbook.F02389</EMMO_fe015383_afb3_44a6_ae86_043628697aa2>
    <rdfs:subClassOf rdf:resource="http://emmo.info/emmo#EMMO_3f15d200_c97b_42c8_8ac0_d81d150361e2"/>
    <EMMO_6dd685dd_1895_46e4_b227_be9f7d643c25>http://dbpedia.org/page/Fine-structure_constant</EMMO_6dd685dd_1895_46e4_b227_be9f7d643c25>
    <EMMO_1f1b164d_ec6a_4faa_8d5e_88bda62316cc>http://qudt.org/vocab/constant/FineStructureConstant</EMMO_1f1b164d_ec6a_4faa_8d5e_88bda62316cc>
    <skos:prefLabel xml:lang="en">FineStructureConstant</skos:prefLabel>
  </rdf:Description>
  <rdf:Description rdf:about="http://emmo.info/emmo">
    <owl:versionIRI rdf:resource="http://emmo.info/emmo/1.0.0-beta"/>
    <dcterms:title xml:lang="en">European Materials &amp; Modelling Ontology</dcterms:title>
    <rdfs:comment xml:lang="en">The EMMO requires FacT++ reasoner plugin in order to visualize all inferences and class hierarchy (ctrl+R hotkey in Protege).</rdfs:comment>
    <dcterms:creator>Gerhard Goldbeck</dcterms:creator>
    <dcterms:abstract xml:lang="en">European Materials &amp; Modelling Ontology (EMMO)

EMMO is a multidisciplinary effort to develop a standard representational framework (the ontology) based on current materials modelling knowledge, including physical sciences, analytical philosophy and information and communication technologies.

It provides the connection between the physical world, materials characterisation world and materials modelling world.

EMMO is released under a Creative Commons license Attribution 4.0 International (CC BY 4.0).</dcterms:abstract>
    <dcterms:contributor>Fraunhofer IWM, DE</dcterms:contributor>
    <rdfs:comment xml:lang="en">Contacts:
Gerhard Goldbeck
Goldbeck Consulting Ltd (UK)
email: gerhard@goldbeck-consulting.com

Emanuele Ghedini
University of Bologna (IT)
email: emanuele.ghedini@unibo.it</rdfs:comment>
    <dcterms:creator>Emanuele Ghedini</dcterms:creator>
    <dcterms:creator>Georg Schmitz</dcterms:creator>
    <owl:versionInfo>1.0.0-beta</owl:versionInfo>
    <dcterms:creator>Adham Hashibon</dcterms:creator>
    <rdf:type rdf:resource="http://www.w3.org/2002/07/owl#Ontology"/>
    <dcterms:contributor>University of Bologna, IT</dcterms:contributor>
    <dcterms:license>https://creativecommons.org/licenses/by/4.0/legalcode</dcterms:license>
    <dcterms:contributor>Goldbeck Consulting Ltd (UK)</dcterms:contributor>
    <dcterms:contributor>SINTEF, NO</dcterms:contributor>
    <dcterms:contributor>Access, DE</dcterms:contributor>
    <dcterms:publisher>EMMC ASBL</dcterms:publisher>
    <dcterms:creator>Jesper Friis</dcterms:creator>
  </rdf:Description>
  <rdf:Description rdf:nodeID="f8fb83657cd5f496db3c2b94baf326f26b32">
    <rdf:type rdf:resource="http://www.w3.org/2002/07/owl#Restriction"/>
    <owl:onProperty rdf:resource="http://emmo.info/emmo#EMMO_b2282816_b7a3_44c6_b2cb_3feff1ceb7fe"/>
    <owl:allValuesFrom rdf:nodeID="f8fb83657cd5f496db3c2b94baf326f26b33"/>
  </rdf:Description>
  <rdf:Description rdf:about="http://emmo.info/emmo/middle/holistic">
    <dcterms:contributor>University of Bologna, IT</dcterms:contributor>
    <dcterms:abstract xml:lang="en">European Materials &amp; Modelling Ontology (EMMO)

EMMO is a multidisciplinary effort to develop a standard representational framework (the ontology) based on current materials modelling knowledge, including physical sciences, analytical philosophy and information and communication technologies.

It provides the connection between the physical world, materials characterisation world and materials modelling world.

EMMO is released under a Creative Commons license Attribution 4.0 International (CC BY 4.0).</dcterms:abstract>
    <rdfs:comment xml:lang="en">The EMMO requires FacT++ reasoner plugin in order to visualize all inferences and class hierarchy (ctrl+R hotkey in Protege).</rdfs:comment>
    <dcterms:contributor>Goldbeck Consulting Ltd (UK)</dcterms:contributor>
    <dcterms:contributor>SINTEF, NO</dcterms:contributor>
    <dcterms:creator>Georg Schmitz</dcterms:creator>
    <dcterms:creator>Gerhard Goldbeck</dcterms:creator>
    <owl:versionIRI rdf:resource="http://emmo.info/emmo/1.0.0-beta/middle/holistic"/>
    <dcterms:contributor>Access, DE</dcterms:contributor>
    <dcterms:creator>Emanuele Ghedini</dcterms:creator>
    <dcterms:publisher>EMMC ASBL</dcterms:publisher>
    <dcterms:creator>Adham Hashibon</dcterms:creator>
    <owl:versionInfo>1.0.0-beta</owl:versionInfo>
    <dcterms:license>https://creativecommons.org/licenses/by/4.0/legalcode</dcterms:license>
    <dcterms:contributor>Fraunhofer IWM, DE</dcterms:contributor>
    <dcterms:creator>Jesper Friis</dcterms:creator>
    <rdfs:comment xml:lang="en">Contacts:
Gerhard Goldbeck
Goldbeck Consulting Ltd (UK)
email: gerhard@goldbeck-consulting.com

Emanuele Ghedini
University of Bologna (IT)
email: emanuele.ghedini@unibo.it</rdfs:comment>
    <rdf:type rdf:resource="http://www.w3.org/2002/07/owl#Ontology"/>
    <dcterms:title xml:lang="en">European Materials &amp; Modelling Ontology</dcterms:title>
  </rdf:Description>
  <rdf:Description rdf:about="http://emmo.info/emmo#EMMO_4207e895_8b83_4318_996a_72cfb32acd94">
    <skos:prefLabel xml:lang="en">Material</skos:prefLabel>
    <EMMO_967080e5_2f42_4eb2_a3a9_c58143e835f9 xml:lang="en">A matter individual that stands for a real world object representing an amount of a physical substance (or mixture of substances) in different states of matter or phases.</EMMO_967080e5_2f42_4eb2_a3a9_c58143e835f9>
    <rdf:type rdf:resource="http://www.w3.org/2002/07/owl#Class"/>
    <rdfs:comment xml:lang="en">Material usually means some definite kind, quality, or quantity of matter, especially as intended for use.</rdfs:comment>
    <rdfs:subClassOf rdf:resource="http://emmo.info/emmo#EMMO_5b2222df_4da6_442f_8244_96e9e45887d1"/>
    <rdfs:comment xml:lang="en">A instance of a material (e.g. nitrogen) can represent different states of matter. The fact that the individual also belongs to other classes (e.g. Gas) would reveal the actual form in which the material is found.</rdfs:comment>
  </rdf:Description>
  <rdf:Description rdf:about="http://emmo.info/emmo#EMMO_4d6504f1_c470_4ce9_b941_bbbebc9ab05d">
    <skos:prefLabel xml:lang="en">hasContactWith</skos:prefLabel>
    <rdf:type rdf:resource="http://www.w3.org/2002/07/owl#SymmetricProperty"/>
    <rdf:type rdf:resource="http://www.w3.org/2002/07/owl#ObjectProperty"/>
    <rdfs:subPropertyOf rdf:resource="http://emmo.info/emmo#EMMO_6703954e_34c4_4a15_a9e7_f313760ae1a8"/>
  </rdf:Description>
  <rdf:Description rdf:nodeID="ff14b31ebf90e4bc5ba2839064d29e543b6">
    <rdf:type rdf:resource="http://www.w3.org/1999/02/22-rdf-syntax-ns#List"/>
    <rdf:first rdf:resource="http://emmo.info/emmo#EMMO_4588526f_8553_4f4d_aa73_a483e88d599b"/>
    <rdf:rest rdf:nodeID="ff14b31ebf90e4bc5ba2839064d29e543b7"/>
  </rdf:Description>
  <rdf:Description rdf:about="http://emmo.info/emmo#EMMO_79a02de5_b884_4eab_bc18_f67997d597a2">
    <rdfs:comment xml:lang="en">Measure of the opposition that a circuit presents to a current when a voltage is applied.</rdfs:comment>
    <EMMO_1f1b164d_ec6a_4faa_8d5e_88bda62316cc>http://qudt.org/vocab/quantitykind/Impedance</EMMO_1f1b164d_ec6a_4faa_8d5e_88bda62316cc>
    <rdf:type rdf:resource="http://www.w3.org/2002/07/owl#Class"/>
    <skos:prefLabel xml:lang="en">ElectricImpedance</skos:prefLabel>
    <EMMO_de178b12_5d35_4bca_8efa_a4193162571d>T-3 L+2 M+1 I-2 Θ0 N0 J0</EMMO_de178b12_5d35_4bca_8efa_a4193162571d>
    <EMMO_6dd685dd_1895_46e4_b227_be9f7d643c25>http://dbpedia.org/page/Electrical_impedance</EMMO_6dd685dd_1895_46e4_b227_be9f7d643c25>
    <rdfs:subClassOf rdf:resource="http://emmo.info/emmo#EMMO_e88f75d6_9a17_4cfc_bdf7_43d7cea5a9a1"/>
    <skos:altLabel>Impedance</skos:altLabel>
  </rdf:Description>
  <rdf:Description rdf:about="http://emmo.info/emmo#EMMO_c26a0340_d619_4928_b1a1_1a04e88bb89d">
    <owl:disjointUnionOf rdf:nodeID="fea11ca01461e402d8f697c19c5d8de88b15"/>
    <EMMO_967080e5_2f42_4eb2_a3a9_c58143e835f9 xml:lang="en">The union of all classes categorizing elementary particles according to the Standard Model.</EMMO_967080e5_2f42_4eb2_a3a9_c58143e835f9>
    <rdfs:subClassOf rdf:resource="http://emmo.info/emmo#EMMO_0f795e3e_c602_4577_9a43_d5a231aa1360"/>
    <rdfs:comment xml:lang="en">Only a subset of elementary particles from the Standard Model are here included for the sake of simplicity.</rdfs:comment>
    <rdf:type rdf:resource="http://www.w3.org/2002/07/owl#Class"/>
    <skos:prefLabel xml:lang="en">ElementaryParticle</skos:prefLabel>
    <rdfs:subClassOf rdf:resource="http://emmo.info/emmo#EMMO_98ada9d8_f1c8_4f13_99b5_d890f5354152"/>
  </rdf:Description>
  <rdf:Description rdf:nodeID="fe24a777e3fd743f986ce83488d2cf30bb1">
    <owl:hasValue>Δ</owl:hasValue>
    <owl:onProperty rdf:resource="http://emmo.info/emmo#EMMO_23b579e1_8088_45b5_9975_064014026c42"/>
    <rdf:type rdf:resource="http://www.w3.org/2002/07/owl#Restriction"/>
  </rdf:Description>
  <rdf:Description rdf:nodeID="ffcb99037244f48d590430c228d02afdbb55">
    <owl:onProperty rdf:resource="http://emmo.info/emmo#EMMO_67fc0a36_8dcb_4ffa_9a43_31074efa3296"/>
    <rdf:type rdf:resource="http://www.w3.org/2002/07/owl#Restriction"/>
    <owl:allValuesFrom rdf:resource="http://emmo.info/emmo#EMMO_cdc962d8_f3ea_4764_a57a_c7caa4859179"/>
  </rdf:Description>
  <rdf:Description rdf:about="http://purl.org/dc/terms/publisher">
    <rdf:type rdf:resource="http://www.w3.org/2002/07/owl#AnnotationProperty"/>
  </rdf:Description>
  <rdf:Description rdf:about="http://emmo.info/emmo#EMMO_ec2472ae_cf4a_46a5_8555_1556f5a6c3c5">
    <rdf:type rdf:resource="http://www.w3.org/2002/07/owl#SymmetricProperty"/>
    <rdfs:domain rdf:resource="http://emmo.info/emmo#EMMO_802d3e92_8770_4f98_a289_ccaaab7fdddf"/>
    <rdfs:subPropertyOf rdf:resource="http://www.w3.org/2002/07/owl#topObjectProperty"/>
    <rdf:type rdf:resource="http://www.w3.org/2002/07/owl#TransitiveProperty"/>
    <EMMO_967080e5_2f42_4eb2_a3a9_c58143e835f9 xml:lang="en">The superclass for all relations used by the EMMO.</EMMO_967080e5_2f42_4eb2_a3a9_c58143e835f9>
    <rdf:type rdf:resource="http://www.w3.org/2002/07/owl#ObjectProperty"/>
    <skos:prefLabel xml:lang="en">EMMORelation</skos:prefLabel>
    <rdfs:range rdf:resource="http://emmo.info/emmo#EMMO_802d3e92_8770_4f98_a289_ccaaab7fdddf"/>
  </rdf:Description>
  <rdf:Description rdf:about="http://emmo.info/emmo#EMMO_f658c301_ce93_46cf_9639_4eace2c5d1d5">
    <rdfs:subClassOf rdf:nodeID="f8fb83657cd5f496db3c2b94baf326f26b41"/>
    <EMMO_967080e5_2f42_4eb2_a3a9_c58143e835f9 xml:lang="en">A symbolic that has parts a reference unit and a numerical object separated by a space expressing the value of a quantitative property (expressed as the product of the numerical and the unit).</EMMO_967080e5_2f42_4eb2_a3a9_c58143e835f9>
    <rdfs:comment xml:lang="en">A quantity is not necessarily a property, since it is possible to write "10 kg", without assigning this quantity to a specific object.

However, a quantitative property is always a quantity.</rdfs:comment>
    <rdfs:subClassOf rdf:nodeID="f8fb83657cd5f496db3c2b94baf326f26b40"/>
    <rdfs:comment xml:lang="en">Referred as Quantity Value in International vocabulary of metrology (VIM)</rdfs:comment>
    <rdfs:subClassOf rdf:resource="http://emmo.info/emmo#EMMO_985bec21_989f_4b9e_a4b3_735d88099c3c"/>
    <rdf:type rdf:resource="http://www.w3.org/2002/07/owl#Class"/>
    <EMMO_b432d2d5_25f4_4165_99c5_5935a7763c1a xml:lang="en">6.8 m
0.9 km
8 K
6 MeV
43.5 HRC(150 kg)</EMMO_b432d2d5_25f4_4165_99c5_5935a7763c1a>
    <owl:disjointUnionOf rdf:nodeID="f8fb83657cd5f496db3c2b94baf326f26b42"/>
    <rdfs:comment xml:lang="en">SI distinguishes between a quantity (an abstract concept) and the quantity value (a number and a reference). 

The EMMO, following strict nominalism, denies the existence of abstract objects and then collapses the two concepts of SI quantity and SI quantity value into a single one: the 'Quantity'.

So, for the EMMO the symbol "kg" is not a physical quantity but simply a 'Symbolic' object categorized as a 'MeasurementUnit'.

While the string "1 kg" is a 'Physical Quantity'.</rdfs:comment>
    <skos:prefLabel xml:lang="en">Quantity</skos:prefLabel>
  </rdf:Description>
  <rdf:Description rdf:about="http://emmo.info/emmo#EMMO_c5ddfdba_c074_4aa4_ad6b_1ac4942d300d">
    <rdfs:comment xml:lang="en">In the EMMO there are no relations such as occupiesSpace, since 'Physical'-s are themselves the 4D regions.</rdfs:comment>
    <rdfs:comment xml:lang="en">The EMMO can be used to represent real world entities as 'Physical'-s that are easy to connect to classical or quantum mechanical based models.

Classical mechanics poses no representational issues, for the EMMO: the 4D representation of 'Physical'-s is consistent with classical physics systems.

However, the representation of 'Physical'-s that are typically analized through quantum mechanics (e.g. molecules, atoms, clusters), is not straightforward.

1) De Broglie - Bohm interpretation
The most simple approach is to rely on Bohmian mechanics, in which each particle is supposed to exists in a specific position between measurements (hidden variables approach), while its trajectory is calculated using a Guiding Equation based on a quantum field calculated with the Schroedinger Equation.

While this approach is really easy to implement in an ontology, since each entity has its own well defined 4D region, its mathematical representation failed to receive large consensus due to the difficulties to include relativistic effects, to be extended to subnuclear scale and the strong non-locality assumtpion of the quantum field.

Nevertheless, the Bohmian mechanics is a numerical approach that is used in electronic models to reduce the computational effort of the solution of Schroedinger Equation.

In practice, an EMMO user can declare a 'physical' individual that stand for the whole quantum system to be described, and at the same time all sub-parts individuals can be declared, having them a well defined position in time, according to De Broglie - Bohm interpretation. The Hamiltonian can be calculated by considering the sub-part individuals.

'physical'-s are then made of 'physical' parts and 'void' parts that stand for the space between 'physical'-s (e.g. the void between electrons and nucleus in an atom).

2) Copenhagen interpretation
In this interpretation the properties (e.g. energy level, position, spin) of a particle are not defined in the interval between two measurements and the quantum system is entangled (i.e. properties of particles in the sysyem are correlated) and described by a global wavefunction obtained solving the Schroedinger Equation. 

Upon measurement, the wavefunction collapses to a combination of close eigenstates that provide information about bservables of the system components (e.g. position, energy).

The EMMO can be used to represent 'physical'-s that can be related to Copenhagen based models. In practice, the user should follow these steps:

a) define the quantum system as a 'physical' individual (e.g. an H2 molecule) under a specific class (e.g. 'h2_molecule'). This individual is the whole.

b) define the axioms of the  class that describe how many sub-parts are expected for the whole and their class types (e.g. 'h2_molecule' has axioms 'has_proper_part exactly 2 electron' and 'has_proper_part exactly 2 nucleus)

c) the user can now connect the whole to a Schroedinger equation based model whose Hamiltonian is calculated trough the information coming only from the axioms. No individuals are declared for the subparts!

d) a measurement done on the quantum system that provides information on the sub-part observables is interpreted as wavefunction collapse and leads to the end of the whole and the declaration of the sub-parts individuals which can be themselves other quantum systems 

e.g. if the outer electron of the H2 molecule interacts with another entity defining its state, then the whole that stands for the entangled H2 molecule becomes a 'physical' made of an electron individual, a quantum system made of one electron and two nuclei and the void between them.

e.g. in the Born-Oppenheimer approximation the user represent the atom by un-entangling nucleus and electronic cloud. The un-entanglement comes in the form of declaration of individual as parts.

e.g. the double slit experiment can be represent in the EMMO as:
a) before the slit: a 'physical' that extend in space and has parts 'electron' and 'void', called 'single_electron_wave_function'. 'electron' and 'void' are only in the axioms and not decalred individuals.
b) during slit passage: a 'physical' made of one declared individual, the 'electron'.
c) after the slit: again 'single_electron_wave_function'
d) upon collision with the detector:  'physical' made of one declared individual, the 'electron'.</rdfs:comment>
    <rdfs:comment xml:lang="en">A 'Physical' is the class that contains all the individuals that stand for real world objects that interact physically with the ontologist, i.e. physical objects.

A physical object must be perceived through physical interaction by the ontologist. Then the ontologist can declare an individual standing for the physical object just perceived.

Perception is a subcategory of physical interactions. It is an interaction that stimulate a representation of the physical object within the ontologist (the agent).</rdfs:comment>
    <rdfs:comment xml:lang="en">A 'Physical' must include at least an 'Elementary' part, and can include 'Void' parts.

A 'Physical' may include as part also the 'Void' surrounding or enclosed by its 'Physical' sub parts.

There are no particular criteria for 'Physical'-s structure, except that is made of some 'Elementary'-s as proper parts and not only 'Void'.

This is done in order to take into account the quantum nature of physical systems, in which the actual position of sub-components (e.g. electrons in an atom) is not known except for its probability distribution function (according to the Copenhagen interpretation.)

e.g. a real world object that has spatial parts an atom and a cubic light year of void, extending for some time, can be a physical object.</rdfs:comment>
    <rdfs:comment xml:lang="en">A 'Physical' with dimensions other than 4D cannot exist, following the restriction of the parent 'EMMO' class.

It follows from the fact that perception is always unfolding in time.

e.g. you always have an aperture time when you take a picture or measure a property. Instantaneous perceptions are idealizations (abstractions) or a very small time measurement.</rdfs:comment>
    <rdfs:subClassOf rdf:nodeID="fc2fcd8f8eb3649bcbbaff76ba54058acb5"/>
    <rdf:type rdf:resource="http://www.w3.org/2002/07/owl#Class"/>
    <EMMO_967080e5_2f42_4eb2_a3a9_c58143e835f9 xml:lang="en">A 'Item' that has part some 'Elementary' and whose temporal proper parts are only 'Physical'-s (i.e. it can be perceived without interruptions in time).</EMMO_967080e5_2f42_4eb2_a3a9_c58143e835f9>
    <EMMO_705f27ae_954c_4f13_98aa_18473fc52b25 xml:lang="en">From Latin physica "study of nature" (and Ancient Greek φυσικός, “natural”). 

Here the word relates to things perceived through the senses as opposed to the mind; tangible or concrete.</EMMO_705f27ae_954c_4f13_98aa_18473fc52b25>
    <rdfs:subClassOf rdf:nodeID="fc2fcd8f8eb3649bcbbaff76ba54058acb4"/>
    <skos:prefLabel xml:lang="en">Physical</skos:prefLabel>
    <rdfs:comment xml:lang="en">The purpose of the 'Physical' branch is to provide a representation of the real world objects, while the models used to name, explain or predict the behaviour of the real world objects lay under the 'Semiotic' branch.

More than one semiotic representation can be connected to the same 'Physical'.

e.g. Navier-Stokes or Euler equation applied to the same fluid are an example of mathematical model used to represent a physical object for some specific interpreter.</rdfs:comment>
  </rdf:Description>
  <rdf:Description rdf:nodeID="ff14b31ebf90e4bc5ba2839064d29e543b2">
    <rdf:rest rdf:nodeID="ff14b31ebf90e4bc5ba2839064d29e543b3"/>
    <rdf:first rdf:resource="http://emmo.info/emmo#EMMO_4a464c8d_8895_44a8_a628_aed13509f1bd"/>
    <rdf:type rdf:resource="http://www.w3.org/1999/02/22-rdf-syntax-ns#List"/>
  </rdf:Description>
  <rdf:Description rdf:nodeID="f05bdaa1e617a4bccafc519daf7bf4785b151">
    <rdf:type rdf:resource="http://www.w3.org/2002/07/owl#Restriction"/>
    <owl:someValuesFrom rdf:resource="http://emmo.info/emmo#EMMO_e501069c_34d3_4dc7_ac87_c90c7342192b"/>
    <owl:onProperty rdf:resource="http://emmo.info/emmo#EMMO_bed1d005_b04e_4a90_94cf_02bc678a8569"/>
  </rdf:Description>
  <rdf:Description rdf:about="http://emmo.info/emmo#EMMO_939483b1_0148_43d1_8b35_851d2cd5d939">
    <rdfs:comment xml:lang="en">A 'model' prediction is always a prediction of the properties of an entity, since an entity is known by an interpreter only through perception.</rdfs:comment>
    <skos:prefLabel xml:lang="en">Model</skos:prefLabel>
    <rdf:type rdf:resource="http://www.w3.org/2002/07/owl#Class"/>
    <owl:equivalentClass rdf:nodeID="f627ff42579444148ae27fcacfb5f8528b5"/>
    <EMMO_967080e5_2f42_4eb2_a3a9_c58143e835f9 xml:lang="en">A 'sign' that not only stands for a 'physical' or a 'process', but it is also a simplified representation, aimed to assist calculations for its description or for predictions of its behaviour.

A 'model' represents a 'physical' or a 'process' by direct similitude (e.g. small scale replica) or by capturing in a logical framework the relations between its properties (e.g. mathematical model).</EMMO_967080e5_2f42_4eb2_a3a9_c58143e835f9>
  </rdf:Description>
  <rdf:Description rdf:nodeID="ffcb99037244f48d590430c228d02afdbb2">
    <owl:hasValue>Da</owl:hasValue>
    <owl:onProperty rdf:resource="http://emmo.info/emmo#EMMO_23b579e1_8088_45b5_9975_064014026c42"/>
    <rdf:type rdf:resource="http://www.w3.org/2002/07/owl#Restriction"/>
  </rdf:Description>
  <rdf:Description rdf:about="http://emmo.info/emmo#EMMO_254472c6_3dbd_4f02_bc43_571389cd281f">
    <rdfs:subClassOf rdf:nodeID="f05bdaa1e617a4bccafc519daf7bf4785b25"/>
    <rdfs:subClassOf rdf:nodeID="f05bdaa1e617a4bccafc519daf7bf4785b28"/>
    <skos:prefLabel xml:lang="en">Zepto</skos:prefLabel>
    <rdf:type rdf:resource="http://www.w3.org/2002/07/owl#Class"/>
  </rdf:Description>
  <rdf:Description rdf:nodeID="f05bdaa1e617a4bccafc519daf7bf4785b84">
    <owl:hasValue rdf:datatype="http://www.w3.org/2001/XMLSchema#double">1000000.0</owl:hasValue>
    <owl:onProperty rdf:resource="http://emmo.info/emmo#EMMO_faf79f53_749d_40b2_807c_d34244c192f4"/>
    <rdf:type rdf:resource="http://www.w3.org/2002/07/owl#Restriction"/>
  </rdf:Description>
  <rdf:Description rdf:nodeID="f05bdaa1e617a4bccafc519daf7bf4785b185">
    <rdf:first rdf:resource="http://emmo.info/emmo#EMMO_f2523820_04a6_44ab_bb67_8237dda2b0c2"/>
    <rdf:rest rdf:nodeID="f05bdaa1e617a4bccafc519daf7bf4785b186"/>
    <rdf:type rdf:resource="http://www.w3.org/1999/02/22-rdf-syntax-ns#List"/>
  </rdf:Description>
  <rdf:Description rdf:nodeID="f05bdaa1e617a4bccafc519daf7bf4785b10">
    <owl:inverseOf rdf:resource="http://emmo.info/emmo#EMMO_3446e167_c576_49d6_846c_215bb8878a55"/>
  </rdf:Description>
  <rdf:Description rdf:about="http://emmo.info/emmo#EMMO_dc6c8de0_cfc4_4c66_a7dc_8f720e732d54">
    <rdf:type rdf:resource="http://www.w3.org/2002/07/owl#Class"/>
    <skos:altLabel>NucleonNumber</skos:altLabel>
    <EMMO_70fe84ff_99b6_4206_a9fc_9a8931836d84 xml:lang="en">Number of nucleons in an atomic nucleus.</EMMO_70fe84ff_99b6_4206_a9fc_9a8931836d84>
    <skos:altLabel>AtomicMassNumber</skos:altLabel>
    <rdfs:subClassOf rdf:resource="http://emmo.info/emmo#EMMO_ba882f34_0d71_4e4f_9d92_0c076c633a2c"/>
    <skos:prefLabel xml:lang="en">MassNumber</skos:prefLabel>
    <EMMO_1f1b164d_ec6a_4faa_8d5e_88bda62316cc>http://qudt.org/vocab/quantitykind/MassNumber</EMMO_1f1b164d_ec6a_4faa_8d5e_88bda62316cc>
    <EMMO_de178b12_5d35_4bca_8efa_a4193162571d>T0 L0 M0 I0 Θ0 N0 J0</EMMO_de178b12_5d35_4bca_8efa_a4193162571d>
  </rdf:Description>
  <rdf:Description rdf:nodeID="ffcb99037244f48d590430c228d02afdbb49">
    <rdf:type rdf:resource="http://www.w3.org/2002/07/owl#Restriction"/>
    <owl:onProperty rdf:resource="http://emmo.info/emmo#EMMO_bed1d005_b04e_4a90_94cf_02bc678a8569"/>
    <owl:someValuesFrom rdf:resource="http://emmo.info/emmo#EMMO_33433bb1_c68f_45ee_a466_f01e2c57b214"/>
  </rdf:Description>
  <rdf:Description rdf:about="http://emmo.info/emmo#EMMO_e7bc8939_7ff8_4917_beb5_c42730b390f3">
    <skos:prefLabel xml:lang="en">SpeedFractionUnit</skos:prefLabel>
    <EMMO_967080e5_2f42_4eb2_a3a9_c58143e835f9 xml:lang="en">Unit for quantities of dimension one that are the fraction of two speeds.</EMMO_967080e5_2f42_4eb2_a3a9_c58143e835f9>
    <rdfs:subClassOf rdf:resource="http://emmo.info/emmo#EMMO_c2f5ee66_579c_44c6_a2e9_fa2eaa9fa4da"/>
    <EMMO_b432d2d5_25f4_4165_99c5_5935a7763c1a xml:lang="en">Unit for refractive index.</EMMO_b432d2d5_25f4_4165_99c5_5935a7763c1a>
    <rdf:type rdf:resource="http://www.w3.org/2002/07/owl#Class"/>
  </rdf:Description>
  <rdf:Description rdf:nodeID="f0b819106611c4b798f33b16c65f4398db4">
    <owl:onProperty rdf:resource="http://emmo.info/emmo#EMMO_ae2d1a96_bfa1_409a_a7d2_03d69e8a125a"/>
    <owl:someValuesFrom rdf:resource="http://emmo.info/emmo#EMMO_49804605_c0fe_4538_abda_f70ba1dc8a5d"/>
    <rdf:type rdf:resource="http://www.w3.org/2002/07/owl#Restriction"/>
  </rdf:Description>
  <rdf:Description rdf:about="http://www.w3.org/2002/07/owl#qualifiedCardinality">
    <rdf:type rdf:resource="http://www.w3.org/2002/07/owl#AnnotationProperty"/>
  </rdf:Description>
  <rdf:Description rdf:nodeID="ffbe75b10062f400ea693809785c50a44b1">
    <owl:onProperty rdf:nodeID="ffbe75b10062f400ea693809785c50a44b2"/>
    <owl:someValuesFrom rdf:resource="http://emmo.info/emmo#EMMO_8786cb47_8e1f_4968_9b15_f6d41fc51252"/>
    <rdf:type rdf:resource="http://www.w3.org/2002/07/owl#Restriction"/>
  </rdf:Description>
  <rdf:Description rdf:nodeID="ffcb99037244f48d590430c228d02afdbb44">
    <owl:someValuesFrom rdf:resource="http://emmo.info/emmo#EMMO_3227b821_26a5_4c7c_9c01_5c24483e0bd0"/>
    <rdf:type rdf:resource="http://www.w3.org/2002/07/owl#Restriction"/>
    <owl:onProperty rdf:resource="http://emmo.info/emmo#EMMO_bed1d005_b04e_4a90_94cf_02bc678a8569"/>
  </rdf:Description>
  <rdf:Description rdf:about="http://emmo.info/emmo#EMMO_7db11dbf_a643_464a_9b56_07eabcc3e9c5">
    <rdfs:subClassOf rdf:nodeID="f05bdaa1e617a4bccafc519daf7bf4785b96"/>
    <EMMO_fe015383_afb3_44a6_ae86_043628697aa2>https://doi.org/10.1351/goldbook.M03884</EMMO_fe015383_afb3_44a6_ae86_043628697aa2>
    <EMMO_1f1b164d_ec6a_4faa_8d5e_88bda62316cc>http://qudt.org/vocab/unit/M</EMMO_1f1b164d_ec6a_4faa_8d5e_88bda62316cc>
    <skos:prefLabel xml:lang="en">Metre</skos:prefLabel>
    <rdfs:subClassOf rdf:nodeID="f05bdaa1e617a4bccafc519daf7bf4785b95"/>
    <EMMO_70fe84ff_99b6_4206_a9fc_9a8931836d84 xml:lang="en">The metre, symbol m, is the SI unit of length. It is defined by taking the fixed numerical value of the speed of light in vacuum c to be 299792458 when expressed in the unit m s−1, where the second is defined in terms of ∆νCs.</EMMO_70fe84ff_99b6_4206_a9fc_9a8931836d84>
    <rdf:type rdf:resource="http://www.w3.org/2002/07/owl#Class"/>
  </rdf:Description>
  <rdf:Description rdf:nodeID="fc2fcd8f8eb3649bcbbaff76ba54058acb2">
    <rdf:type rdf:resource="http://www.w3.org/2002/07/owl#Restriction"/>
    <owl:allValuesFrom rdf:resource="http://www.w3.org/2002/07/owl#Nothing"/>
    <owl:onProperty rdf:resource="http://emmo.info/emmo#EMMO_f68030be_94b8_4c61_a161_886468558054"/>
  </rdf:Description>
  <rdf:Description rdf:nodeID="fe24a777e3fd743f986ce83488d2cf30bb18">
    <owl:complementOf rdf:nodeID="fe24a777e3fd743f986ce83488d2cf30bb19"/>
    <rdf:type rdf:resource="http://www.w3.org/2002/07/owl#Class"/>
  </rdf:Description>
  <rdf:Description rdf:about="http://emmo.info/emmo#EMMO_e46f3f24_c2ec_4552_8dd4_cfc5c0a89c09">
    <rdf:type rdf:resource="http://www.w3.org/2002/07/owl#Class"/>
    <EMMO_1f1b164d_ec6a_4faa_8d5e_88bda62316cc>http://qudt.org/vocab/quantitykind/RadiantFlux</EMMO_1f1b164d_ec6a_4faa_8d5e_88bda62316cc>
    <rdfs:comment xml:lang="en">The radiant energy emitted, reflected, transmitted or received, per unit time.</rdfs:comment>
    <rdfs:subClassOf rdf:resource="http://emmo.info/emmo#EMMO_09b9021b_f97b_43eb_b83d_0a764b472bc2"/>
    <EMMO_de178b12_5d35_4bca_8efa_a4193162571d>T-3 L+2 M+1 I0 Θ0 N0 J0</EMMO_de178b12_5d35_4bca_8efa_a4193162571d>
    <EMMO_6dd685dd_1895_46e4_b227_be9f7d643c25>http://dbpedia.org/page/Radiant_flux</EMMO_6dd685dd_1895_46e4_b227_be9f7d643c25>
    <skos:prefLabel xml:lang="en">RadiantFlux</skos:prefLabel>
    <EMMO_fe015383_afb3_44a6_ae86_043628697aa2>https://doi.org/10.1351/goldbook.R05046</EMMO_fe015383_afb3_44a6_ae86_043628697aa2>
  </rdf:Description>
  <rdf:Description rdf:about="http://emmo.info/emmo#EMMO_696ed548_9477_45ea_993c_6a8f5271914a">
    <rdfs:subClassOf rdf:nodeID="f05bdaa1e617a4bccafc519daf7bf4785b86"/>
    <rdfs:subClassOf rdf:nodeID="f05bdaa1e617a4bccafc519daf7bf4785b87"/>
    <EMMO_1f1b164d_ec6a_4faa_8d5e_88bda62316cc>http://qudt.org/vocab/unit/C</EMMO_1f1b164d_ec6a_4faa_8d5e_88bda62316cc>
    <rdf:type rdf:resource="http://www.w3.org/2002/07/owl#Class"/>
    <skos:prefLabel xml:lang="en">Coulomb</skos:prefLabel>
    <EMMO_fe015383_afb3_44a6_ae86_043628697aa2>https://doi.org/10.1351/goldbook.C01365</EMMO_fe015383_afb3_44a6_ae86_043628697aa2>
    <rdfs:comment xml:lang="en">Measurement unit for electric charge.</rdfs:comment>
  </rdf:Description>
  <rdf:Description rdf:nodeID="fa691b5894b3543efa24f9838ff46c3eab12">
    <rdf:type rdf:resource="http://www.w3.org/1999/02/22-rdf-syntax-ns#List"/>
    <rdf:first rdf:resource="http://emmo.info/emmo#EMMO_b21a56ed_f969_4612_a6ec_cb7766f7f31d"/>
    <rdf:rest rdf:resource="http://www.w3.org/1999/02/22-rdf-syntax-ns#nil"/>
  </rdf:Description>
  <rdf:Description rdf:about="http://emmo.info/emmo#EMMO_02c0621e_a527_4790_8a0f_2bb51973c819">
    <EMMO_967080e5_2f42_4eb2_a3a9_c58143e835f9 xml:lang="en">A 'Mathematical' entity that is made of a 'Numeral' and a 'MeasurementUnit' defined by a physical law, connected to a physical entity through a model perspective. Measurement is done according to the same model.</EMMO_967080e5_2f42_4eb2_a3a9_c58143e835f9>
    <rdfs:subClassOf rdf:nodeID="f8fb83657cd5f496db3c2b94baf326f26b1"/>
    <rdfs:comment xml:lang="en">— quantities of the same kind have the same quantity dimension,
— quantities of different quantity dimensions are always of different kinds, and
— quantities having the same quantity dimension are not necessarily of the same kind.
ISO 80000-1</rdfs:comment>
    <rdfs:comment xml:lang="en">Measured or simulated 'physical propertiy'-s are always defined by a physical law, connected to a physical entity through a model perspective and measurement is done according to the same model.

Systems of units suggests that this is the correct approach, since except for the fundamental units (length, time, charge) every other unit is derived by mathematical relations between these fundamental units, implying a physical laws or definitions.</rdfs:comment>
    <skos:prefLabel xml:lang="en">PhysicalQuantity</skos:prefLabel>
    <rdfs:comment xml:lang="en">Measurement units of quantities of the same quantity dimension may be designated by the same name and symbol even when the quantities are not of the same kind. 

For example, joule per kelvin and J/K are respectively the name and symbol of both a measurement unit of heat capacity and a measurement unit of entropy, which are generally not considered to be quantities of the same kind. 

However, in some cases special measurement unit names are restricted to be used with quantities of specific kind only. 

For example, the measurement unit ‘second to the power minus one’ (1/s) is called hertz (Hz) when used for frequencies and becquerel (Bq) when used for activities of radionuclides. 

As another example, the joule (J) is used as a unit of energy, but never as a unit of moment of force, i.e. the newton metre (N · m).</rdfs:comment>
    <rdfs:comment xml:lang="en">In the same system of quantities, dim ρB = ML−3 is the quantity dimension of mass concentration of component B, and ML−3 is also the quantity dimension of mass density, ρ.
ISO 80000-1</rdfs:comment>
    <rdfs:subClassOf rdf:resource="http://emmo.info/emmo#EMMO_54ee6b5e_5261_44a8_86eb_5717e7fdb9d0"/>
    <owl:disjointUnionOf rdf:nodeID="f8fb83657cd5f496db3c2b94baf326f26b2"/>
    <rdf:type rdf:resource="http://www.w3.org/2002/07/owl#Class"/>
  </rdf:Description>
  <rdf:Description rdf:nodeID="ffcb99037244f48d590430c228d02afdbb14">
    <rdf:type rdf:resource="http://www.w3.org/2002/07/owl#Restriction"/>
    <owl:onProperty rdf:resource="http://emmo.info/emmo#EMMO_23b579e1_8088_45b5_9975_064014026c42"/>
    <owl:hasValue>d</owl:hasValue>
  </rdf:Description>
  <rdf:Description rdf:about="http://emmo.info/emmo#EMMO_216f448e_cdbc_4aeb_a529_7a5fe7fc38bb">
    <owl:disjointUnionOf rdf:nodeID="f8fb83657cd5f496db3c2b94baf326f26b10"/>
    <EMMO_b432d2d5_25f4_4165_99c5_5935a7763c1a xml:lang="en">Some examples are "Pa", "m" and "J".</EMMO_b432d2d5_25f4_4165_99c5_5935a7763c1a>
    <skos:prefLabel xml:lang="en">UnitSymbol</skos:prefLabel>
    <owl:equivalentClass rdf:nodeID="f8fb83657cd5f496db3c2b94baf326f26b7"/>
    <EMMO_967080e5_2f42_4eb2_a3a9_c58143e835f9 xml:lang="en">A symbol that stands for a single unit.</EMMO_967080e5_2f42_4eb2_a3a9_c58143e835f9>
    <rdf:type rdf:resource="http://www.w3.org/2002/07/owl#Class"/>
  </rdf:Description>
  <rdf:Description rdf:about="http://emmo.info/emmo#EMMO_58a650f0_a638_4743_8439_535a325e5c4c">
    <EMMO_1f1b164d_ec6a_4faa_8d5e_88bda62316cc>http://qudt.org/vocab/quantitykind/ElementaryCharge</EMMO_1f1b164d_ec6a_4faa_8d5e_88bda62316cc>
    <EMMO_6dd685dd_1895_46e4_b227_be9f7d643c25>http://dbpedia.org/page/Elementary_charge</EMMO_6dd685dd_1895_46e4_b227_be9f7d643c25>
    <EMMO_fe015383_afb3_44a6_ae86_043628697aa2>https://doi.org/10.1351/goldbook.E02032</EMMO_fe015383_afb3_44a6_ae86_043628697aa2>
    <EMMO_a9b3d04c_7ceb_40a2_b8d3_28d514a770a8>https://physics.nist.gov/cgi-bin/cuu/Value?e</EMMO_a9b3d04c_7ceb_40a2_b8d3_28d514a770a8>
    <rdf:type rdf:resource="http://www.w3.org/2002/07/owl#Class"/>
    <rdfs:subClassOf rdf:resource="http://emmo.info/emmo#EMMO_1604f495_328a_4f28_9962_f4cc210739dd"/>
    <EMMO_967080e5_2f42_4eb2_a3a9_c58143e835f9 xml:lang="en">The magnitude of the electric charge carried by a single electron. It defines the base unit Ampere in the SI system.</EMMO_967080e5_2f42_4eb2_a3a9_c58143e835f9>
    <skos:prefLabel xml:lang="en">ElementaryCharge</skos:prefLabel>
    <rdfs:subClassOf rdf:resource="http://emmo.info/emmo#EMMO_f2ca6dd0_0e5f_4392_a92d_cafdae6cfc95"/>
    <EMMO_de178b12_5d35_4bca_8efa_a4193162571d>T+1 L0 M0 I+1 Θ0 N0 J0</EMMO_de178b12_5d35_4bca_8efa_a4193162571d>
    <rdfs:comment xml:lang="en">The DBpedia definition (http://dbpedia.org/page/Elementary_charge) is outdated as May 20, 2019. It is now an exact quantity.</rdfs:comment>
  </rdf:Description>
  <rdf:Description rdf:nodeID="f05bdaa1e617a4bccafc519daf7bf4785b127">
    <rdf:type rdf:resource="http://www.w3.org/2002/07/owl#Restriction"/>
    <owl:onProperty rdf:resource="http://emmo.info/emmo#EMMO_bed1d005_b04e_4a90_94cf_02bc678a8569"/>
    <owl:someValuesFrom rdf:resource="http://emmo.info/emmo#EMMO_a77a0a4b_6bd2_42b2_be27_4b63cebbb59e"/>
  </rdf:Description>
  <rdf:Description rdf:nodeID="f0b819106611c4b798f33b16c65f4398db2">
    <rdf:type rdf:resource="http://www.w3.org/1999/02/22-rdf-syntax-ns#List"/>
    <rdf:rest rdf:nodeID="f0b819106611c4b798f33b16c65f4398db3"/>
    <rdf:first rdf:resource="http://emmo.info/emmo#EMMO_43e9a05d_98af_41b4_92f6_00f79a09bfce"/>
  </rdf:Description>
  <rdf:Description rdf:about="http://emmo.info/emmo#EMMO_0c576e13_4ee7_4f3d_bfe9_1614243df018">
    <rdf:type rdf:resource="http://www.w3.org/2002/07/owl#Class"/>
    <rdfs:subClassOf rdf:resource="http://emmo.info/emmo#EMMO_b5957cef_a287_442d_a3ce_fd39f20ba1cd"/>
    <skos:prefLabel xml:lang="en">1-manifold</skos:prefLabel>
  </rdf:Description>
  <rdf:Description rdf:nodeID="fdb1489b80bcc4ee28afe0be8feb9b935b9">
    <rdf:type rdf:resource="http://www.w3.org/2002/07/owl#Restriction"/>
    <owl:onProperty rdf:nodeID="fdb1489b80bcc4ee28afe0be8feb9b935b10"/>
    <owl:someValuesFrom rdf:resource="http://emmo.info/emmo#EMMO_6f5af708_f825_4feb_a0d1_a8d813d3022b"/>
  </rdf:Description>
  <rdf:Description rdf:about="http://emmo.info/emmo#EMMO_27c5d8c6_8af7_4d63_beb1_ec37cd8b3fa3">
    <EMMO_b432d2d5_25f4_4165_99c5_5935a7763c1a xml:lang="en">The Newton's equation of motion.

The Schrödinger equation.

The Navier-Stokes equation.</EMMO_b432d2d5_25f4_4165_99c5_5935a7763c1a>
    <EMMO_967080e5_2f42_4eb2_a3a9_c58143e835f9 xml:lang="en">An 'equation' that stands for a 'physical_law' by mathematically defining the relations between physics_quantities.</EMMO_967080e5_2f42_4eb2_a3a9_c58143e835f9>
    <rdfs:subClassOf rdf:nodeID="f627ff42579444148ae27fcacfb5f8528b2"/>
    <rdfs:subClassOf rdf:resource="http://emmo.info/emmo#EMMO_e56ee3eb_7609_4ae1_8bed_51974f0960a6"/>
    <rdfs:subClassOf rdf:nodeID="f627ff42579444148ae27fcacfb5f8528b3"/>
    <rdf:type rdf:resource="http://www.w3.org/2002/07/owl#Class"/>
    <skos:prefLabel xml:lang="en">PhysicsEquation</skos:prefLabel>
  </rdf:Description>
  <rdf:Description rdf:about="http://emmo.info/emmo#EMMO_f68030be_94b8_4c61_a161_886468558054">
    <rdf:type rdf:resource="http://www.w3.org/2002/07/owl#TransitiveProperty"/>
    <rdfs:range rdf:resource="http://emmo.info/emmo#EMMO_eb3a768e_d53e_4be9_a23b_0714833c36de"/>
    <rdf:type rdf:resource="http://www.w3.org/2002/07/owl#ObjectProperty"/>
    <rdfs:subPropertyOf rdf:resource="http://emmo.info/emmo#EMMO_9380ab64_0363_4804_b13f_3a8a94119a76"/>
    <rdfs:domain rdf:resource="http://emmo.info/emmo#EMMO_eb3a768e_d53e_4be9_a23b_0714833c36de"/>
    <skos:prefLabel xml:lang="en">hasSpatialPart</skos:prefLabel>
    <EMMO_967080e5_2f42_4eb2_a3a9_c58143e835f9>A relation that isolates a proper part that extends itself in time within the overall lifetime of the whole, without covering the full spatial extension of the 4D whole (i.e. is not a temporal part).</EMMO_967080e5_2f42_4eb2_a3a9_c58143e835f9>
  </rdf:Description>
  <rdf:Description rdf:nodeID="fe24a777e3fd743f986ce83488d2cf30bb29">
    <owl:onProperty rdf:resource="http://emmo.info/emmo#EMMO_faf79f53_749d_40b2_807c_d34244c192f4"/>
    <owl:onDataRange rdf:resource="http://www.w3.org/2001/XMLSchema#integer"/>
    <owl:qualifiedCardinality rdf:datatype="http://www.w3.org/2001/XMLSchema#nonNegativeInteger">1</owl:qualifiedCardinality>
    <rdf:type rdf:resource="http://www.w3.org/2002/07/owl#Restriction"/>
  </rdf:Description>
  <rdf:Description rdf:about="http://emmo.info/emmo#EMMO_66bc9029_f473_45ff_bab9_c3509ff37a22">
    <EMMO_967080e5_2f42_4eb2_a3a9_c58143e835f9 xml:lang="en">An objective comparative measure of hot or cold. 

Temperature is a relative quantity that can be used to express temperature differences. Unlike ThermodynamicTemperature, it cannot express absolute temperatures.</EMMO_967080e5_2f42_4eb2_a3a9_c58143e835f9>
    <skos:prefLabel xml:lang="en">CelsiusTemperature</skos:prefLabel>
    <EMMO_6dd685dd_1895_46e4_b227_be9f7d643c25>http://dbpedia.org/page/Temperature</EMMO_6dd685dd_1895_46e4_b227_be9f7d643c25>
    <rdfs:subClassOf rdf:resource="http://emmo.info/emmo#EMMO_2946d40b_24a1_47fa_8176_e3f79bb45064"/>
    <EMMO_de178b12_5d35_4bca_8efa_a4193162571d>T-1 L0 M0 I0 Θ0 N+1 J0</EMMO_de178b12_5d35_4bca_8efa_a4193162571d>
    <rdf:type rdf:resource="http://www.w3.org/2002/07/owl#Class"/>
    <EMMO_fe015383_afb3_44a6_ae86_043628697aa2>https://doi.org/10.1351/goldbook.T06261</EMMO_fe015383_afb3_44a6_ae86_043628697aa2>
  </rdf:Description>
  <rdf:Description rdf:nodeID="fe0b20157736f4a31909181349b2e6219b23">
    <owl:onProperty rdf:resource="http://emmo.info/emmo#EMMO_23b579e1_8088_45b5_9975_064014026c42"/>
    <rdf:type rdf:resource="http://www.w3.org/2002/07/owl#Restriction"/>
    <owl:hasValue>T0 L-2 M0 I0 Θ0 N0 J+1</owl:hasValue>
  </rdf:Description>
  <rdf:Description rdf:about="http://emmo.info/emmo#EMMO_d859588d_44dc_4614_bc75_5fcd0058acc8">
    <skos:prefLabel xml:lang="en">Wavenumber</skos:prefLabel>
    <EMMO_6dd685dd_1895_46e4_b227_be9f7d643c25>http://dbpedia.org/page/Wavenumber</EMMO_6dd685dd_1895_46e4_b227_be9f7d643c25>
    <rdfs:subClassOf rdf:resource="http://emmo.info/emmo#EMMO_ecec2983_7c26_4f8d_a981_51ca29668baf"/>
    <rdfs:comment xml:lang="en">The number of waves per unit length along the direction of propagation.</rdfs:comment>
    <rdf:type rdf:resource="http://www.w3.org/2002/07/owl#Class"/>
    <EMMO_fe015383_afb3_44a6_ae86_043628697aa2>https://doi.org/10.1351/goldbook.W06664</EMMO_fe015383_afb3_44a6_ae86_043628697aa2>
    <EMMO_1f1b164d_ec6a_4faa_8d5e_88bda62316cc>http://qudt.org/vocab/quantitykind/Wavenumber</EMMO_1f1b164d_ec6a_4faa_8d5e_88bda62316cc>
    <EMMO_e55f2d7c_9893_48cd_b4a4_fdf38253bd20>http://www.ontology-of-units-of-measure.org/resource/om-2/Wavenumber</EMMO_e55f2d7c_9893_48cd_b4a4_fdf38253bd20>
    <EMMO_de178b12_5d35_4bca_8efa_a4193162571d>T0 L-1 M0 I0 Θ0 N0 J0</EMMO_de178b12_5d35_4bca_8efa_a4193162571d>
  </rdf:Description>
  <rdf:Description rdf:about="http://emmo.info/emmo#EMMO_88470739_03d3_4c47_a03e_b30a1288d50c">
    <rdf:type rdf:resource="http://www.w3.org/2002/07/owl#Class"/>
    <EMMO_967080e5_2f42_4eb2_a3a9_c58143e835f9 xml:lang="en">A mathematical string that can be evaluated as true or false.</EMMO_967080e5_2f42_4eb2_a3a9_c58143e835f9>
    <skos:prefLabel xml:lang="en">MathematicalFormula</skos:prefLabel>
    <rdfs:subClassOf rdf:resource="http://emmo.info/emmo#EMMO_54ee6b5e_5261_44a8_86eb_5717e7fdb9d0"/>
    <rdfs:subClassOf rdf:resource="http://emmo.info/emmo#EMMO_89a0c87c_0804_4013_937a_6fe234d9499c"/>
  </rdf:Description>
  <rdf:Description rdf:nodeID="fa691b5894b3543efa24f9838ff46c3eab13">
    <owl:onProperty rdf:nodeID="fa691b5894b3543efa24f9838ff46c3eab14"/>
    <rdf:type rdf:resource="http://www.w3.org/2002/07/owl#Restriction"/>
    <owl:someValuesFrom rdf:resource="http://emmo.info/emmo#EMMO_008fd3b2_4013_451f_8827_52bceab11841"/>
  </rdf:Description>
  <rdf:Description rdf:nodeID="f627ff42579444148ae27fcacfb5f8528b11">
    <rdf:rest rdf:nodeID="f627ff42579444148ae27fcacfb5f8528b12"/>
    <rdf:first rdf:resource="http://emmo.info/emmo#EMMO_54ee6b5e_5261_44a8_86eb_5717e7fdb9d0"/>
    <rdf:type rdf:resource="http://www.w3.org/1999/02/22-rdf-syntax-ns#List"/>
  </rdf:Description>
  <rdf:Description rdf:about="http://emmo.info/emmo#EMMO_d7b7fd1e_645a_42cb_8f40_85f0d034d3ae">
    <skos:prefLabel xml:lang="en">Lumen</skos:prefLabel>
    <EMMO_1f1b164d_ec6a_4faa_8d5e_88bda62316cc>http://qudt.org/vocab/unit/LM</EMMO_1f1b164d_ec6a_4faa_8d5e_88bda62316cc>
    <rdfs:comment xml:lang="en">Measurement unit for luminous flux.</rdfs:comment>
    <rdfs:subClassOf rdf:nodeID="f05bdaa1e617a4bccafc519daf7bf4785b137"/>
    <rdfs:subClassOf rdf:nodeID="f05bdaa1e617a4bccafc519daf7bf4785b138"/>
    <EMMO_fe015383_afb3_44a6_ae86_043628697aa2>https://doi.org/10.1351/goldbook.L03639</EMMO_fe015383_afb3_44a6_ae86_043628697aa2>
    <rdf:type rdf:resource="http://www.w3.org/2002/07/owl#Class"/>
  </rdf:Description>
  <rdf:Description rdf:nodeID="fe24a777e3fd743f986ce83488d2cf30bb8">
    <owl:onProperty rdf:resource="http://emmo.info/emmo#EMMO_23b579e1_8088_45b5_9975_064014026c42"/>
    <rdf:type rdf:resource="http://www.w3.org/2002/07/owl#Restriction"/>
    <owl:hasValue>-</owl:hasValue>
  </rdf:Description>
  <rdf:Description rdf:about="http://emmo.info/emmo#EMMO_0527413c_b286_4e9c_b2d0_03fb2a038dee">
    <skos:prefLabel xml:lang="en">Interpreter</skos:prefLabel>
    <EMMO_967080e5_2f42_4eb2_a3a9_c58143e835f9 xml:lang="en">The entity (or agent, or observer, or cognitive entity) who connects 'Sign', 'Interpretant' and 'Object'.</EMMO_967080e5_2f42_4eb2_a3a9_c58143e835f9>
    <rdf:type rdf:resource="http://www.w3.org/2002/07/owl#Class"/>
    <rdfs:subClassOf rdf:resource="http://emmo.info/emmo#EMMO_b803f122_4acb_4064_9d71_c1e5fd091fc9"/>
    <rdfs:subClassOf rdf:nodeID="fa691b5894b3543efa24f9838ff46c3eab4"/>
  </rdf:Description>
  <rdf:Description rdf:about="http://emmo.info/emmo#EMMO_494b372c_cfdf_47d3_a4de_5e037c540de8">
    <skos:prefLabel xml:lang="en">Device</skos:prefLabel>
    <rdfs:comment xml:lang="en">From Old French "deviser", meaning: arrange, plan, contrive.

Literally "dispose in portions," from Vulgar Latin "divisare", frequentative of Latin dividere, meaning "to divide"</rdfs:comment>
    <rdfs:subClassOf rdf:nodeID="ffbe75b10062f400ea693809785c50a44b1"/>
    <rdfs:subClassOf rdf:resource="http://emmo.info/emmo#EMMO_86ca9b93_1183_4b65_81b8_c0fcd3bba5ad"/>
    <EMMO_967080e5_2f42_4eb2_a3a9_c58143e835f9 xml:lang="en">An engineered object which is instrumental for reaching a particular purpose through its characteristic functioning process, with particular reference to mechanical or electronic equipment.</EMMO_967080e5_2f42_4eb2_a3a9_c58143e835f9>
    <rdf:type rdf:resource="http://www.w3.org/2002/07/owl#Class"/>
  </rdf:Description>
  <rdf:Description rdf:about="http://emmo.info/emmo#EMMO_b29fd350_39aa_4af7_9459_3faa0544cba6">
    <rdfs:subClassOf rdf:nodeID="f627ff42579444148ae27fcacfb5f8528b7"/>
    <rdf:type rdf:resource="http://www.w3.org/2002/07/owl#Class"/>
    <EMMO_967080e5_2f42_4eb2_a3a9_c58143e835f9 xml:lang="en">A solvable set of one Physics Equation and one or more Materials Relations.</EMMO_967080e5_2f42_4eb2_a3a9_c58143e835f9>
    <skos:prefLabel xml:lang="en">PhysicsBasedModel</skos:prefLabel>
    <rdfs:subClassOf rdf:resource="http://emmo.info/emmo#EMMO_f7ed665b_c2e1_42bc_889b_6b42ed3a36f0"/>
    <rdfs:subClassOf rdf:nodeID="f627ff42579444148ae27fcacfb5f8528b8"/>
  </rdf:Description>
  <rdf:Description rdf:about="http://emmo.info/emmo#EMMO_e79c62ff_10ad_4ec0_baba_c19ddd4eaa11">
    <skos:prefLabel xml:lang="en">Yotta</skos:prefLabel>
    <rdf:type rdf:resource="http://www.w3.org/2002/07/owl#Class"/>
    <rdfs:subClassOf rdf:nodeID="f05bdaa1e617a4bccafc519daf7bf4785b164"/>
    <rdfs:subClassOf rdf:nodeID="f05bdaa1e617a4bccafc519daf7bf4785b161"/>
  </rdf:Description>
  <rdf:Description rdf:about="http://emmo.info/emmo#EMMO_cf3dd6cc_c5d6_4b3d_aef4_82f3b7a361af">
    <EMMO_fe015383_afb3_44a6_ae86_043628697aa2>https://doi.org/10.1351/goldbook.S05971</EMMO_fe015383_afb3_44a6_ae86_043628697aa2>
    <rdfs:subClassOf rdf:resource="http://emmo.info/emmo#EMMO_6f4d704a_a7c6_4c07_b8a7_ea0bab04128f"/>
    <rdf:type rdf:resource="http://www.w3.org/2002/07/owl#Class"/>
    <rdfs:subClassOf rdf:nodeID="f05bdaa1e617a4bccafc519daf7bf4785b136"/>
    <rdfs:subClassOf rdf:nodeID="f05bdaa1e617a4bccafc519daf7bf4785b135"/>
    <skos:prefLabel xml:lang="en">Steradian</skos:prefLabel>
    <EMMO_1f1b164d_ec6a_4faa_8d5e_88bda62316cc>http://qudt.org/vocab/unit/SR</EMMO_1f1b164d_ec6a_4faa_8d5e_88bda62316cc>
    <EMMO_967080e5_2f42_4eb2_a3a9_c58143e835f9 xml:lang="en">Dimensionless measurement unit for solid angle.</EMMO_967080e5_2f42_4eb2_a3a9_c58143e835f9>
  </rdf:Description>
  <rdf:Description rdf:about="http://emmo.info/emmo#EMMO_008fd3b2_4013_451f_8827_52bceab11841">
    <rdfs:subClassOf rdf:nodeID="fa691b5894b3543efa24f9838ff46c3eab1"/>
    <EMMO_967080e5_2f42_4eb2_a3a9_c58143e835f9 xml:lang="en">A 'Process', that has participant an 'Interpreter', that is aimed to produce a 'Sign' representing another participant, the 'Object'.</EMMO_967080e5_2f42_4eb2_a3a9_c58143e835f9>
    <rdfs:subClassOf rdf:nodeID="fa691b5894b3543efa24f9838ff46c3eab2"/>
    <skos:prefLabel xml:lang="en">Semiosis</skos:prefLabel>
    <EMMO_b432d2d5_25f4_4165_99c5_5935a7763c1a xml:lang="en">Me looking a cat and saying loud: "Cat!" -&gt; the semiosis process

me -&gt; interpreter
cat -&gt; object (in Peirce semiotics)
the cat perceived by my mind -&gt; interpretant
"Cat!" -&gt; sign, the produced sign</EMMO_b432d2d5_25f4_4165_99c5_5935a7763c1a>
    <rdfs:subClassOf rdf:resource="http://emmo.info/emmo#EMMO_43e9a05d_98af_41b4_92f6_00f79a09bfce"/>
    <rdfs:subClassOf rdf:nodeID="fa691b5894b3543efa24f9838ff46c3eab3"/>
    <rdf:type rdf:resource="http://www.w3.org/2002/07/owl#Class"/>
  </rdf:Description>
  <rdf:Description rdf:nodeID="f05bdaa1e617a4bccafc519daf7bf4785b159">
    <owl:onProperty rdf:resource="http://emmo.info/emmo#EMMO_bed1d005_b04e_4a90_94cf_02bc678a8569"/>
    <owl:someValuesFrom rdf:resource="http://emmo.info/emmo#EMMO_515b5579_d526_4842_9e6f_ecc34db6f368"/>
    <rdf:type rdf:resource="http://www.w3.org/2002/07/owl#Restriction"/>
  </rdf:Description>
  <rdf:Description rdf:nodeID="f627ff42579444148ae27fcacfb5f8528b1">
    <owl:someValuesFrom rdf:resource="http://emmo.info/emmo#EMMO_314d0bd5_67ed_437e_a609_36d46147cea7"/>
    <rdf:type rdf:resource="http://www.w3.org/2002/07/owl#Restriction"/>
    <owl:onProperty rdf:resource="http://emmo.info/emmo#EMMO_ae2d1a96_bfa1_409a_a7d2_03d69e8a125a"/>
  </rdf:Description>
  <rdf:Description rdf:nodeID="f05bdaa1e617a4bccafc519daf7bf4785b28">
    <rdf:type rdf:resource="http://www.w3.org/2002/07/owl#Restriction"/>
    <owl:onProperty rdf:resource="http://emmo.info/emmo#EMMO_23b579e1_8088_45b5_9975_064014026c42"/>
    <owl:hasValue>z</owl:hasValue>
  </rdf:Description>
  <rdf:Description rdf:nodeID="f05bdaa1e617a4bccafc519daf7bf4785b142">
    <owl:hasValue>lx</owl:hasValue>
    <rdf:type rdf:resource="http://www.w3.org/2002/07/owl#Restriction"/>
    <owl:onProperty rdf:resource="http://emmo.info/emmo#EMMO_23b579e1_8088_45b5_9975_064014026c42"/>
  </rdf:Description>
  <rdf:Description rdf:about="http://emmo.info/emmo#EMMO_96f39f77_44dc_491b_8fa7_30d887fe0890">
    <skos:prefLabel xml:lang="en">Area</skos:prefLabel>
    <EMMO_1f1b164d_ec6a_4faa_8d5e_88bda62316cc>http://qudt.org/vocab/quantitykind/Area</EMMO_1f1b164d_ec6a_4faa_8d5e_88bda62316cc>
    <rdfs:comment xml:lang="en">Extent of a surface.</rdfs:comment>
    <rdfs:subClassOf rdf:resource="http://emmo.info/emmo#EMMO_2946d40b_24a1_47fa_8176_e3f79bb45064"/>
    <EMMO_6dd685dd_1895_46e4_b227_be9f7d643c25>http://dbpedia.org/page/Area</EMMO_6dd685dd_1895_46e4_b227_be9f7d643c25>
    <rdf:type rdf:resource="http://www.w3.org/2002/07/owl#Class"/>
    <EMMO_de178b12_5d35_4bca_8efa_a4193162571d>T0 L+2 M0 I0 Θ0 N0 J0</EMMO_de178b12_5d35_4bca_8efa_a4193162571d>
    <EMMO_fe015383_afb3_44a6_ae86_043628697aa2>https://doi.org/10.1351/goldbook.A00429</EMMO_fe015383_afb3_44a6_ae86_043628697aa2>
  </rdf:Description>
  <rdf:Description rdf:about="http://emmo.info/emmo#EMMO_9141801c_c539_4c72_b423_8c74ff6b8f05">
    <rdf:type rdf:resource="http://www.w3.org/2002/07/owl#Class"/>
    <rdfs:subClassOf rdf:resource="http://emmo.info/emmo#EMMO_9895a1b4_f0a5_4167_ac5e_97db40b8bfcc"/>
    <skos:prefLabel xml:lang="en">VolumeDimension</skos:prefLabel>
    <owl:equivalentClass rdf:nodeID="fe0b20157736f4a31909181349b2e6219b27"/>
  </rdf:Description>
  <rdf:Description rdf:nodeID="f3b8e3e5cecf14b688acdf306cd5f62cbb6">
    <rdf:type rdf:resource="http://www.w3.org/2002/07/owl#Restriction"/>
    <owl:onProperty rdf:resource="http://emmo.info/emmo#EMMO_65a2c5b8_e4d8_4a51_b2f8_e55effc0547d"/>
    <owl:allValuesFrom rdf:resource="http://emmo.info/emmo#EMMO_36c79456_e29c_400d_8bd3_0eedddb82652"/>
  </rdf:Description>
  <rdf:Description rdf:about="http://emmo.info/emmo#EMMO_70fe84ff_99b6_4206_a9fc_9a8931836d84">
    <rdf:type rdf:resource="http://www.w3.org/2002/07/owl#AnnotationProperty"/>
    <rdfs:subPropertyOf rdf:resource="http://www.w3.org/2000/01/rdf-schema#comment"/>
    <rdfs:comment xml:lang="en">Precise and univocal description of an ontological entity in the framework of an axiomatic system.

A definition uses entities in an ontological system to identify other derivate ontological entities within the same system.</rdfs:comment>
    <rdfs:range rdf:resource="http://www.w3.org/2001/XMLSchema#string"/>
    <skos:prefLabel xml:lang="en">definition</skos:prefLabel>
  </rdf:Description>
  <rdf:Description rdf:nodeID="fe24a777e3fd743f986ce83488d2cf30bb19">
    <owl:onProperty rdf:resource="http://emmo.info/emmo#EMMO_b2282816_b7a3_44c6_b2cb_3feff1ceb7fe"/>
    <owl:someValuesFrom rdf:resource="http://emmo.info/emmo#EMMO_1eed0732_e3f1_4b2c_a9c4_b4e75eeb5895"/>
    <rdf:type rdf:resource="http://www.w3.org/2002/07/owl#Restriction"/>
  </rdf:Description>
  <rdf:Description rdf:about="http://emmo.info/emmo#EMMO_501f9b3a_c469_48f7_9281_2e6a8d805d7a">
    <rdfs:subClassOf rdf:resource="http://emmo.info/emmo#EMMO_9895a1b4_f0a5_4167_ac5e_97db40b8bfcc"/>
    <skos:prefLabel xml:lang="en">AngularMomentumDimension</skos:prefLabel>
    <owl:equivalentClass rdf:nodeID="fe0b20157736f4a31909181349b2e6219b17"/>
    <rdf:type rdf:resource="http://www.w3.org/2002/07/owl#Class"/>
  </rdf:Description>
  <rdf:Description rdf:nodeID="fe0b20157736f4a31909181349b2e6219b8">
    <rdf:first rdf:resource="http://emmo.info/emmo#EMMO_d4f7d378_5e3b_468a_baa1_a7e98358cda7"/>
    <rdf:type rdf:resource="http://www.w3.org/1999/02/22-rdf-syntax-ns#List"/>
    <rdf:rest rdf:nodeID="fe0b20157736f4a31909181349b2e6219b9"/>
  </rdf:Description>
  <rdf:Description rdf:nodeID="f05bdaa1e617a4bccafc519daf7bf4785b51">
    <owl:hasValue>a</owl:hasValue>
    <rdf:type rdf:resource="http://www.w3.org/2002/07/owl#Restriction"/>
    <owl:onProperty rdf:resource="http://emmo.info/emmo#EMMO_23b579e1_8088_45b5_9975_064014026c42"/>
  </rdf:Description>
  <rdf:Description rdf:nodeID="f8fb83657cd5f496db3c2b94baf326f26b19">
    <owl:complementOf rdf:resource="http://emmo.info/emmo#EMMO_985bec21_989f_4b9e_a4b3_735d88099c3c"/>
    <rdf:type rdf:resource="http://www.w3.org/2002/07/owl#Class"/>
  </rdf:Description>
  <rdf:Description rdf:about="http://emmo.info/emmo#EMMO_663859e5_add3_4c9e_96fb_c99399de278d">
    <rdf:type rdf:resource="http://www.w3.org/2002/07/owl#IrreflexiveProperty"/>
    <rdf:type rdf:resource="http://www.w3.org/2002/07/owl#AsymmetricProperty"/>
    <rdf:type rdf:resource="http://www.w3.org/2002/07/owl#ObjectProperty"/>
    <skos:prefLabel xml:lang="en">hasSpatioTemporalDirectPart</skos:prefLabel>
    <rdfs:subPropertyOf rdf:resource="http://emmo.info/emmo#EMMO_6e046dd0_9634_4013_b2b1_9cc468087c83"/>
    <rdf:type rdf:resource="http://www.w3.org/2002/07/owl#InverseFunctionalProperty"/>
  </rdf:Description>
  <rdf:Description rdf:about="http://emmo.info/emmo#EMMO_68390bfb_e307_479d_8f78_d66d8773cb1d">
    <rdf:type rdf:resource="http://www.w3.org/2002/07/owl#Class"/>
    <rdfs:subClassOf rdf:resource="http://emmo.info/emmo#EMMO_4207e895_8b83_4318_996a_72cfb32acd94"/>
    <EMMO_967080e5_2f42_4eb2_a3a9_c58143e835f9 xml:lang="en">A material that undergoes chemical changes.</EMMO_967080e5_2f42_4eb2_a3a9_c58143e835f9>
    <skos:prefLabel xml:lang="en">ReactiveMaterial</skos:prefLabel>
  </rdf:Description>
  <rdf:Description rdf:about="http://emmo.info/emmo#EMMO_0ee5779e_d798_4ee5_9bfe_c392d5bea112">
    <skos:prefLabel xml:lang="en">Permittivity</skos:prefLabel>
    <EMMO_e55f2d7c_9893_48cd_b4a4_fdf38253bd20>http://www.ontology-of-units-of-measure.org/resource/om-2/Permittivity</EMMO_e55f2d7c_9893_48cd_b4a4_fdf38253bd20>
    <EMMO_6dd685dd_1895_46e4_b227_be9f7d643c25>http://dbpedia.org/page/Permittivity</EMMO_6dd685dd_1895_46e4_b227_be9f7d643c25>
    <rdfs:comment xml:lang="en">Measure for how the polarization of a material is affected by the application of an external electric field.</rdfs:comment>
    <EMMO_de178b12_5d35_4bca_8efa_a4193162571d>T+4 L-3 M-1 I+2 Θ0 N0 J0</EMMO_de178b12_5d35_4bca_8efa_a4193162571d>
    <rdf:type rdf:resource="http://www.w3.org/2002/07/owl#Class"/>
    <rdfs:subClassOf rdf:resource="http://emmo.info/emmo#EMMO_2946d40b_24a1_47fa_8176_e3f79bb45064"/>
    <EMMO_1f1b164d_ec6a_4faa_8d5e_88bda62316cc>http://qudt.org/vocab/quantitykind/Permittivity</EMMO_1f1b164d_ec6a_4faa_8d5e_88bda62316cc>
    <EMMO_fe015383_afb3_44a6_ae86_043628697aa2>https://doi.org/10.1351/goldbook.P04507</EMMO_fe015383_afb3_44a6_ae86_043628697aa2>
  </rdf:Description>
  <rdf:Description rdf:nodeID="f05bdaa1e617a4bccafc519daf7bf4785b92">
    <owl:inverseOf rdf:resource="http://emmo.info/emmo#EMMO_3446e167_c576_49d6_846c_215bb8878a55"/>
  </rdf:Description>
  <rdf:Description rdf:about="http://emmo.info/emmo#EMMO_0f795e3e_c602_4577_9a43_d5a231aa1360">
    <rdf:type rdf:resource="http://www.w3.org/2002/07/owl#Class"/>
    <rdfs:subClassOf rdf:resource="http://emmo.info/emmo#EMMO_c5ddfdba_c074_4aa4_ad6b_1ac4942d300d"/>
    <rdfs:subClassOf rdf:nodeID="fc2fcd8f8eb3649bcbbaff76ba54058acb2"/>
    <EMMO_967080e5_2f42_4eb2_a3a9_c58143e835f9 xml:lang="en">The basic constituent of 'item'-s that can be proper partitioned only in time up to quantum level.</EMMO_967080e5_2f42_4eb2_a3a9_c58143e835f9>
    <rdfs:subClassOf rdf:nodeID="fc2fcd8f8eb3649bcbbaff76ba54058acb1"/>
    <EMMO_705f27ae_954c_4f13_98aa_18473fc52b25 xml:lang="en">From Latin elementārius (“elementary”), from elementum (“one of the four elements of antiquity; fundamentals”).</EMMO_705f27ae_954c_4f13_98aa_18473fc52b25>
    <rdfs:comment xml:lang="en">While a 'Quantum' is a-tomistic in time and space, an 'elementary' is a-tomistic only in space, recalling the concept of elementary particle.</rdfs:comment>
    <skos:prefLabel xml:lang="en">Elementary</skos:prefLabel>
    <rdfs:comment xml:lang="en">According to mereology, this should be call 'a-tomistic' in the strict etimological sense of the word (from greek, a-tomos: un-divisible).

Mereology based on such items is called atomistic mereology.

However, in order not to confuse the lexicon between mereology and physics (in which an atom is a divisible physical entity) we prefer to call it 'elementary', recalling the concept of elementary particle coming from the standard particles model.</rdfs:comment>
  </rdf:Description>
  <rdf:Description rdf:about="http://emmo.info/emmo#EMMO_967080e5_2f42_4eb2_a3a9_c58143e835f9">
    <rdf:type rdf:resource="http://www.w3.org/2002/07/owl#AnnotationProperty"/>
    <rdfs:range rdf:resource="http://www.w3.org/2001/XMLSchema#string"/>
    <rdfs:comment xml:lang="en">Short enlightening explanation of an ontological entity aimed to facilitate the connection between the ontological concept and a real-world object.

An elucidation provides the meta-ontological semiotic relation that connects an entity within the ontology, to a real-world entity outside the ontology. 

This process is subjective, and depends on the agent that draws this connection (e.g. a user, a machine).</rdfs:comment>
    <skos:prefLabel xml:lang="en">elucidation</skos:prefLabel>
    <rdfs:subPropertyOf rdf:resource="http://www.w3.org/2000/01/rdf-schema#comment"/>
  </rdf:Description>
  <rdf:Description rdf:nodeID="f05bdaa1e617a4bccafc519daf7bf4785b87">
    <owl:hasValue>C</owl:hasValue>
    <rdf:type rdf:resource="http://www.w3.org/2002/07/owl#Restriction"/>
    <owl:onProperty rdf:resource="http://emmo.info/emmo#EMMO_23b579e1_8088_45b5_9975_064014026c42"/>
  </rdf:Description>
  <rdf:Description rdf:nodeID="ff14b31ebf90e4bc5ba2839064d29e543b4">
    <owl:someValuesFrom rdf:resource="http://emmo.info/emmo#EMMO_668fbd5b_6f1b_405c_9c6b_d6067bd0595a"/>
    <owl:onProperty rdf:resource="http://emmo.info/emmo#EMMO_9380ab64_0363_4804_b13f_3a8a94119a76"/>
    <rdf:type rdf:resource="http://www.w3.org/2002/07/owl#Restriction"/>
  </rdf:Description>
  <rdf:Description rdf:about="http://emmo.info/emmo#EMMO_560d833a_6184_410c_859a_05d982712fd7">
    <rdfs:subClassOf rdf:resource="http://emmo.info/emmo#EMMO_04f2a2d5_e799_4692_a654_420e76f5acc1"/>
    <rdfs:subClassOf rdf:resource="http://emmo.info/emmo#EMMO_6c487fb3_03d1_4e56_91ed_c2e16dcbef60"/>
    <EMMO_967080e5_2f42_4eb2_a3a9_c58143e835f9 xml:lang="en">A colloid composed of fine solid particles or liquid droplets in air or another gas.</EMMO_967080e5_2f42_4eb2_a3a9_c58143e835f9>
    <rdf:type rdf:resource="http://www.w3.org/2002/07/owl#Class"/>
    <skos:prefLabel xml:lang="en">Aerosol</skos:prefLabel>
  </rdf:Description>
  <rdf:Description rdf:about="http://emmo.info/emmo#EMMO_d5f3e0e5_fc7d_4e64_86ad_555e74aaff84">
    <rdfs:subClassOf rdf:resource="http://emmo.info/emmo#EMMO_9895a1b4_f0a5_4167_ac5e_97db40b8bfcc"/>
    <skos:prefLabel xml:lang="en">ElectricCurrentDimension</skos:prefLabel>
    <rdf:type rdf:resource="http://www.w3.org/2002/07/owl#Class"/>
    <owl:equivalentClass rdf:nodeID="fe0b20157736f4a31909181349b2e6219b35"/>
  </rdf:Description>
  <rdf:Description rdf:nodeID="f05bdaa1e617a4bccafc519daf7bf4785b111">
    <owl:allValuesFrom rdf:nodeID="f05bdaa1e617a4bccafc519daf7bf4785b113"/>
    <owl:onProperty rdf:nodeID="f05bdaa1e617a4bccafc519daf7bf4785b112"/>
    <rdf:type rdf:resource="http://www.w3.org/2002/07/owl#Restriction"/>
  </rdf:Description>
  <rdf:Description rdf:nodeID="f05bdaa1e617a4bccafc519daf7bf4785b112">
    <owl:inverseOf rdf:resource="http://emmo.info/emmo#EMMO_3446e167_c576_49d6_846c_215bb8878a55"/>
  </rdf:Description>
  <rdf:Description rdf:about="http://emmo.info/emmo#EMMO_db716151_6b73_45ff_910c_d182fdcbb4f5">
    <rdf:type rdf:resource="http://www.w3.org/2002/07/owl#Class"/>
    <EMMO_967080e5_2f42_4eb2_a3a9_c58143e835f9 xml:lang="en">A set of units that correspond to the base quantities in a system of units.</EMMO_967080e5_2f42_4eb2_a3a9_c58143e835f9>
    <skos:prefLabel xml:lang="en">BaseUnit</skos:prefLabel>
  </rdf:Description>
  <rdf:Description rdf:about="http://emmo.info/emmo#EMMO_a2b006f2_bbfd_4dba_bcaa_3fca20cd6be1">
    <rdfs:subClassOf rdf:resource="http://emmo.info/emmo#EMMO_8b0923ab_b500_477b_9ce9_8b3a3e4dc4f2"/>
    <skos:prefLabel xml:lang="en">Solid</skos:prefLabel>
    <EMMO_967080e5_2f42_4eb2_a3a9_c58143e835f9 xml:lang="en">A continuum characterized by structural rigidity and resistance to changes of shape or volume, that retains its shape and density when not confined.</EMMO_967080e5_2f42_4eb2_a3a9_c58143e835f9>
    <rdf:type rdf:resource="http://www.w3.org/2002/07/owl#Class"/>
  </rdf:Description>
  <rdf:Description rdf:about="http://emmo.info/emmo#EMMO_b5c58790_fb2d_42eb_b184_2a3f6ca60acb">
    <skos:prefLabel xml:lang="en">Gradient</skos:prefLabel>
    <rdfs:subClassOf rdf:resource="http://emmo.info/emmo#EMMO_f8a2fe9f_458b_4771_9aba_a50e76afc52d"/>
    <rdf:type rdf:resource="http://www.w3.org/2002/07/owl#Class"/>
    <owl:equivalentClass rdf:nodeID="fe24a777e3fd743f986ce83488d2cf30bb25"/>
  </rdf:Description>
  <rdf:Description rdf:about="http://emmo.info/emmo#EMMO_afea89af_ef16_4bdb_99d5_f3b2f4c85a6c">
    <EMMO_fe015383_afb3_44a6_ae86_043628697aa2>https://doi.org/10.1351/goldbook.S06167</EMMO_fe015383_afb3_44a6_ae86_043628697aa2>
    <rdf:type rdf:resource="http://www.w3.org/2002/07/owl#Class"/>
    <skos:prefLabel xml:lang="en">AreaDensity</skos:prefLabel>
    <EMMO_de178b12_5d35_4bca_8efa_a4193162571d>T0 L-2 M+1 I0 Θ0 N0 J0</EMMO_de178b12_5d35_4bca_8efa_a4193162571d>
    <EMMO_6dd685dd_1895_46e4_b227_be9f7d643c25>http://dbpedia.org/page/Area_density</EMMO_6dd685dd_1895_46e4_b227_be9f7d643c25>
    <rdfs:comment xml:lang="en">Mass per unit area.</rdfs:comment>
    <rdfs:subClassOf rdf:resource="http://emmo.info/emmo#EMMO_2946d40b_24a1_47fa_8176_e3f79bb45064"/>
  </rdf:Description>
  <rdf:Description rdf:about="http://emmo.info/emmo#EMMO_961d1aba_f75e_4411_aaa4_457f7516ed6b">
    <EMMO_1f1b164d_ec6a_4faa_8d5e_88bda62316cc>http://qudt.org/vocab/quantitykind/MagneticFluxDensity</EMMO_1f1b164d_ec6a_4faa_8d5e_88bda62316cc>
    <EMMO_967080e5_2f42_4eb2_a3a9_c58143e835f9 xml:lang="en">Strength of the magnetic field.</EMMO_967080e5_2f42_4eb2_a3a9_c58143e835f9>
    <EMMO_6dd685dd_1895_46e4_b227_be9f7d643c25>http://dbpedia.org/page/Magnetic_field</EMMO_6dd685dd_1895_46e4_b227_be9f7d643c25>
    <rdf:type rdf:resource="http://www.w3.org/2002/07/owl#Class"/>
    <EMMO_fe015383_afb3_44a6_ae86_043628697aa2>https://doi.org/10.1351/goldbook.M03686</EMMO_fe015383_afb3_44a6_ae86_043628697aa2>
    <rdfs:comment xml:lang="en">Often denoted B.</rdfs:comment>
    <rdfs:subClassOf rdf:resource="http://emmo.info/emmo#EMMO_2946d40b_24a1_47fa_8176_e3f79bb45064"/>
    <EMMO_de178b12_5d35_4bca_8efa_a4193162571d>T-2 L0 M+1 I-1 Θ0 N0 J0</EMMO_de178b12_5d35_4bca_8efa_a4193162571d>
    <skos:prefLabel xml:lang="en">MagneticFluxDensity</skos:prefLabel>
  </rdf:Description>
  <rdf:Description rdf:about="http://emmo.info/emmo#EMMO_5be9c137_325a_43d8_b7cd_ea93e7721c2d">
    <rdfs:subClassOf rdf:resource="http://emmo.info/emmo#EMMO_2031516a_2be7_48e8_9af7_7e1270e308fe"/>
    <skos:prefLabel xml:lang="en">GasMixture</skos:prefLabel>
    <EMMO_967080e5_2f42_4eb2_a3a9_c58143e835f9 xml:lang="en">A gaseous solution made of more than one component type.</EMMO_967080e5_2f42_4eb2_a3a9_c58143e835f9>
    <rdf:type rdf:resource="http://www.w3.org/2002/07/owl#Class"/>
    <rdfs:subClassOf rdf:resource="http://emmo.info/emmo#EMMO_04f2a2d5_e799_4692_a654_420e76f5acc1"/>
  </rdf:Description>
  <rdf:Description rdf:about="http://emmo.info/emmo#EMMO_e56ee3eb_7609_4ae1_8bed_51974f0960a6">
    <EMMO_b432d2d5_25f4_4165_99c5_5935a7763c1a xml:lang="en">2+3 = 5
x^2 +3x  = 5x
dv/dt = a
sin(x) = y</EMMO_b432d2d5_25f4_4165_99c5_5935a7763c1a>
    <skos:prefLabel xml:lang="en">Equation</skos:prefLabel>
    <rdfs:subClassOf rdf:resource="http://emmo.info/emmo#EMMO_88470739_03d3_4c47_a03e_b30a1288d50c"/>
    <EMMO_967080e5_2f42_4eb2_a3a9_c58143e835f9 xml:lang="en">The class of 'mathematical'-s that stand for a statement of equality between two mathematical expressions.</EMMO_967080e5_2f42_4eb2_a3a9_c58143e835f9>
    <rdfs:subClassOf rdf:nodeID="fe24a777e3fd743f986ce83488d2cf30bb26"/>
    <rdf:type rdf:resource="http://www.w3.org/2002/07/owl#Class"/>
    <rdfs:comment xml:lang="en">An equation with variables can always be represented as:

f(v0, v1, ..., vn) = g(v0, v1, ..., vn)

where f is the left hand and g the right hand  side expressions and v0, v1, ..., vn are the variables.</rdfs:comment>
    <rdfs:subClassOf rdf:resource="http://emmo.info/emmo#EMMO_54ee6b5e_5261_44a8_86eb_5717e7fdb9d0"/>
  </rdf:Description>
  <rdf:Description rdf:about="http://emmo.info/emmo#EMMO_91447ec0_fb55_49f2_85a5_3172dff6482c">
    <rdf:type rdf:resource="http://www.w3.org/2002/07/owl#Class"/>
    <skos:prefLabel xml:lang="en">Polynomial</skos:prefLabel>
    <rdfs:subClassOf rdf:resource="http://emmo.info/emmo#EMMO_1aed91a3_d00c_48af_8f43_a0c958b2512a"/>
    <EMMO_b432d2d5_25f4_4165_99c5_5935a7763c1a xml:lang="en">2 * x^2 + x + 3</EMMO_b432d2d5_25f4_4165_99c5_5935a7763c1a>
  </rdf:Description>
  <rdf:Description rdf:about="http://emmo.info/emmo#EMMO_e1097637_70d2_4895_973f_2396f04fa204">
    <skos:prefLabel xml:lang="en">hasProperty</skos:prefLabel>
    <rdfs:domain rdf:resource="http://emmo.info/emmo#EMMO_6f5af708_f825_4feb_a0d1_a8d813d3022b"/>
    <rdf:type rdf:resource="http://www.w3.org/2002/07/owl#ObjectProperty"/>
    <rdfs:range rdf:resource="http://emmo.info/emmo#EMMO_b7bcff25_ffc3_474e_9ab5_01b1664bd4ba"/>
    <rdfs:subPropertyOf rdf:resource="http://emmo.info/emmo#EMMO_eb3518bf_f799_4f9e_8c3e_ce59af11453b"/>
  </rdf:Description>
  <rdf:Description rdf:about="http://emmo.info/emmo#EMMO_f2523820_04a6_44ab_bb67_8237dda2b0c2">
    <skos:prefLabel xml:lang="en">Siemens</skos:prefLabel>
    <rdfs:subClassOf rdf:nodeID="f05bdaa1e617a4bccafc519daf7bf4785b187"/>
    <rdf:type rdf:resource="http://www.w3.org/2002/07/owl#Class"/>
    <rdfs:comment xml:lang="en">Measurement unit for electrical conductance.</rdfs:comment>
    <rdfs:subClassOf rdf:nodeID="f05bdaa1e617a4bccafc519daf7bf4785b188"/>
  </rdf:Description>
  <rdf:Description rdf:about="http://emmo.info/emmo#EMMO_14ff4393_0f28_4fb4_abc7_c2cc00bc761d">
    <rdf:type rdf:resource="http://www.w3.org/2002/07/owl#Class"/>
    <skos:prefLabel xml:lang="en">LuminousIntensityDimension</skos:prefLabel>
    <owl:equivalentClass rdf:nodeID="fe0b20157736f4a31909181349b2e6219b2"/>
    <rdfs:subClassOf rdf:resource="http://emmo.info/emmo#EMMO_9895a1b4_f0a5_4167_ac5e_97db40b8bfcc"/>
  </rdf:Description>
  <rdf:Description rdf:nodeID="fea11ca01461e402d8f697c19c5d8de88b4">
    <owl:intersectionOf rdf:nodeID="fea11ca01461e402d8f697c19c5d8de88b5"/>
    <rdf:type rdf:resource="http://www.w3.org/2002/07/owl#Class"/>
  </rdf:Description>
  <rdf:Description rdf:about="http://emmo.info/emmo#EMMO_0cd58641_824c_4851_907f_f4c3be76630c">
    <skos:prefLabel xml:lang="en">Index</skos:prefLabel>
    <rdf:type rdf:resource="http://www.w3.org/2002/07/owl#Class"/>
    <EMMO_967080e5_2f42_4eb2_a3a9_c58143e835f9 xml:lang="en">A 'Sign' that stands for an 'Object' due to causal continguity.</EMMO_967080e5_2f42_4eb2_a3a9_c58143e835f9>
    <EMMO_b432d2d5_25f4_4165_99c5_5935a7763c1a xml:lang="en">Smoke stands for a combustion process (a fire).
My facial expression stands for my emotional status.</EMMO_b432d2d5_25f4_4165_99c5_5935a7763c1a>
  </rdf:Description>
  <rdf:Description rdf:about="http://emmo.info/emmo#EMMO_dc232f53_8ed8_4ddd_9f41_cc057985eadb">
    <rdfs:comment xml:lang="en">Measurement unit for equivalent doseof ionizing radiation. 

Sievert is derived from absorbed dose, but takes into account the biological effectiveness of the radiation, which is dependent on the radiation type and energy.</rdfs:comment>
    <EMMO_c84c6752_6d64_48cc_9500_e54a3c34898d>https://en.wikipedia.org/wiki/Equivalent_dose</EMMO_c84c6752_6d64_48cc_9500_e54a3c34898d>
    <rdf:type rdf:resource="http://www.w3.org/2002/07/owl#Class"/>
    <rdfs:subClassOf rdf:nodeID="f05bdaa1e617a4bccafc519daf7bf4785b149"/>
    <EMMO_1f1b164d_ec6a_4faa_8d5e_88bda62316cc>http://qudt.org/vocab/unit/SV</EMMO_1f1b164d_ec6a_4faa_8d5e_88bda62316cc>
    <rdfs:subClassOf rdf:nodeID="f05bdaa1e617a4bccafc519daf7bf4785b150"/>
    <EMMO_fe015383_afb3_44a6_ae86_043628697aa2>https://doi.org/10.1351/goldbook.S05658</EMMO_fe015383_afb3_44a6_ae86_043628697aa2>
    <skos:prefLabel xml:lang="en">Sievert</skos:prefLabel>
  </rdf:Description>
  <rdf:Description rdf:about="http://emmo.info/emmo#EMMO_35d2e130_6e01_41ed_94f7_00b333d46cf9">
    <rdfs:comment xml:lang="en">In Peirce semiotics this kind of sign category is called symbol. However, since symbol is also used in formal languages, the name is changed in conventional.</rdfs:comment>
    <skos:prefLabel xml:lang="en">Conventional</skos:prefLabel>
    <rdf:type rdf:resource="http://www.w3.org/2002/07/owl#Class"/>
    <EMMO_967080e5_2f42_4eb2_a3a9_c58143e835f9 xml:lang="en">A 'Sign' that stands for an 'Object' through convention, norm or habit, without any resemblance to it.</EMMO_967080e5_2f42_4eb2_a3a9_c58143e835f9>
  </rdf:Description>
  <rdf:Description rdf:about="http://emmo.info/emmo#EMMO_1c2226a9_22f0_40c8_8928_5a01d398f96e">
    <rdf:type rdf:resource="http://www.w3.org/2002/07/owl#Class"/>
    <skos:prefLabel xml:lang="en">MagneticDipoleMomentDimension</skos:prefLabel>
    <owl:equivalentClass rdf:nodeID="fe0b20157736f4a31909181349b2e6219b10"/>
    <rdfs:subClassOf rdf:resource="http://emmo.info/emmo#EMMO_9895a1b4_f0a5_4167_ac5e_97db40b8bfcc"/>
  </rdf:Description>
  <rdf:Description rdf:nodeID="f8fb83657cd5f496db3c2b94baf326f26b11">
    <rdf:rest rdf:resource="http://www.w3.org/1999/02/22-rdf-syntax-ns#nil"/>
    <rdf:type rdf:resource="http://www.w3.org/1999/02/22-rdf-syntax-ns#List"/>
    <rdf:first rdf:resource="http://emmo.info/emmo#EMMO_db716151_6b73_45ff_910c_d182fdcbb4f5"/>
  </rdf:Description>
  <rdf:Description rdf:about="http://emmo.info/emmo#EMMO_251cfb4f_5c75_4778_91ed_6c8395212fd8">
    <EMMO_b432d2d5_25f4_4165_99c5_5935a7763c1a xml:lang="en">The beauty of that girl.
The style of your clothing.</EMMO_b432d2d5_25f4_4165_99c5_5935a7763c1a>
    <rdf:type rdf:resource="http://www.w3.org/2002/07/owl#Class"/>
    <EMMO_967080e5_2f42_4eb2_a3a9_c58143e835f9 xml:lang="en">A 'Property' that cannot be univocally determined and depends on an agent (e.g. a human individual, a community) acting as black-box.</EMMO_967080e5_2f42_4eb2_a3a9_c58143e835f9>
    <rdfs:comment xml:lang="en">The word subjective means that a non-well defined or an unknown procedure is used for the definition of the property.

This happens due to e.g. the complexity of the object, the lack of a underlying model for the representation of the object, the non-well specified meaning of the property symbols. 

A 'SubjectiveProperty' cannot be used to univocally compare 'Object'-s.

e.g. you cannot evaluate the beauty of a person on objective basis.</rdfs:comment>
    <skos:prefLabel xml:lang="en">SubjectiveProperty</skos:prefLabel>
  </rdf:Description>
  <rdf:Description rdf:about="http://emmo.info/emmo#EMMO_0a88be81_343d_4388_92c1_09228ff95ada">
    <skos:prefLabel xml:lang="en">Probability</skos:prefLabel>
    <EMMO_967080e5_2f42_4eb2_a3a9_c58143e835f9 xml:lang="en">Probability is a dimensionless quantity that can attain values between 0 and 1; zero denotes the impossible event and 1 denotes a certain event.</EMMO_967080e5_2f42_4eb2_a3a9_c58143e835f9>
    <rdfs:subClassOf rdf:nodeID="ffcb99037244f48d590430c228d02afdbb6"/>
    <rdfs:subClassOf rdf:resource="http://emmo.info/emmo#EMMO_faab3f84_e475_4a46_af9c_7d249f0b9aef"/>
    <rdfs:comment xml:lang="en">The propability for a certain outcome, is the ratio between the number of events leading to the given outcome and the total number of events.</rdfs:comment>
    <EMMO_fe015383_afb3_44a6_ae86_043628697aa2>https://doi.org/10.1351/goldbook.P04855</EMMO_fe015383_afb3_44a6_ae86_043628697aa2>
    <EMMO_de178b12_5d35_4bca_8efa_a4193162571d>T0 L0 M0 I0 Θ0 N0 J0</EMMO_de178b12_5d35_4bca_8efa_a4193162571d>
    <rdf:type rdf:resource="http://www.w3.org/2002/07/owl#Class"/>
  </rdf:Description>
  <rdf:Description rdf:about="http://emmo.info/emmo#EMMO_28ef05a7_ecc1_4df6_8116_c53251fbd4a8">
    <rdfs:subClassOf rdf:nodeID="ffcb99037244f48d590430c228d02afdbb13"/>
    <skos:prefLabel xml:lang="en">Day</skos:prefLabel>
    <EMMO_6dd685dd_1895_46e4_b227_be9f7d643c25>http://dbpedia.org/page/Day</EMMO_6dd685dd_1895_46e4_b227_be9f7d643c25>
    <rdf:type rdf:resource="http://www.w3.org/2002/07/owl#Class"/>
    <rdfs:subClassOf rdf:resource="http://emmo.info/emmo#EMMO_591e02fd_8d37_45a6_9d11_bb21cef391a0"/>
    <EMMO_70fe84ff_99b6_4206_a9fc_9a8931836d84 xml:lang="en">A measure of time defined as 86 400 seconds.</EMMO_70fe84ff_99b6_4206_a9fc_9a8931836d84>
    <rdfs:subClassOf rdf:nodeID="ffcb99037244f48d590430c228d02afdbb14"/>
    <EMMO_fe015383_afb3_44a6_ae86_043628697aa2>https://doi.org/10.1351/goldbook.D01527</EMMO_fe015383_afb3_44a6_ae86_043628697aa2>
    <EMMO_1f1b164d_ec6a_4faa_8d5e_88bda62316cc>http://qudt.org/vocab/unit/DAY</EMMO_1f1b164d_ec6a_4faa_8d5e_88bda62316cc>
  </rdf:Description>
  <rdf:Description rdf:about="http://emmo.info/emmo#EMMO_f8b92999_3cde_46e3_99d5_664da3090a02">
    <EMMO_fe015383_afb3_44a6_ae86_043628697aa2>https://doi.org/10.1351/goldbook.T06394</EMMO_fe015383_afb3_44a6_ae86_043628697aa2>
    <rdfs:subClassOf rdf:nodeID="ffcb99037244f48d590430c228d02afdbb56"/>
    <rdfs:subClassOf rdf:nodeID="ffcb99037244f48d590430c228d02afdbb57"/>
    <skos:prefLabel xml:lang="en">Tonne</skos:prefLabel>
    <EMMO_c84c6752_6d64_48cc_9500_e54a3c34898d>https://en.wikipedia.org/wiki/Tonne</EMMO_c84c6752_6d64_48cc_9500_e54a3c34898d>
    <rdfs:subClassOf rdf:resource="http://emmo.info/emmo#EMMO_591e02fd_8d37_45a6_9d11_bb21cef391a0"/>
    <EMMO_70fe84ff_99b6_4206_a9fc_9a8931836d84 xml:lang="en">A non-SI unit defined as 1000 kg.</EMMO_70fe84ff_99b6_4206_a9fc_9a8931836d84>
    <EMMO_1f1b164d_ec6a_4faa_8d5e_88bda62316cc>http://qudt.org/vocab/unit/TON_M</EMMO_1f1b164d_ec6a_4faa_8d5e_88bda62316cc>
    <rdf:type rdf:resource="http://www.w3.org/2002/07/owl#Class"/>
  </rdf:Description>
  <rdf:Description rdf:nodeID="fe24a777e3fd743f986ce83488d2cf30bb22">
    <owl:hasValue>/</owl:hasValue>
    <rdf:type rdf:resource="http://www.w3.org/2002/07/owl#Restriction"/>
    <owl:onProperty rdf:resource="http://emmo.info/emmo#EMMO_23b579e1_8088_45b5_9975_064014026c42"/>
  </rdf:Description>
  <rdf:Description rdf:about="http://emmo.info/emmo#EMMO_33b67e69_3645_4c73_b100_5ea6759221b4">
    <rdf:type rdf:resource="http://www.w3.org/2002/07/owl#Class"/>
    <EMMO_fe015383_afb3_44a6_ae86_043628697aa2>https://doi.org/10.1351/goldbook.K03372</EMMO_fe015383_afb3_44a6_ae86_043628697aa2>
    <rdfs:subClassOf rdf:nodeID="f05bdaa1e617a4bccafc519daf7bf4785b36"/>
    <skos:prefLabel xml:lang="en">Katal</skos:prefLabel>
    <rdfs:subClassOf rdf:nodeID="f05bdaa1e617a4bccafc519daf7bf4785b35"/>
    <rdfs:comment xml:lang="en">Measurement unit for catalytic activity.</rdfs:comment>
    <EMMO_1f1b164d_ec6a_4faa_8d5e_88bda62316cc>http://qudt.org/vocab/unit/KAT</EMMO_1f1b164d_ec6a_4faa_8d5e_88bda62316cc>
  </rdf:Description>
  <rdf:Description rdf:about="http://emmo.info/emmo#EMMO_72d53756_7fb1_46ed_980f_83f47efbe105">
    <rdfs:subClassOf rdf:resource="http://emmo.info/emmo#EMMO_0f795e3e_c602_4577_9a43_d5a231aa1360"/>
    <rdf:type rdf:resource="http://www.w3.org/2002/07/owl#Class"/>
    <skos:prefLabel xml:lang="en">Quark</skos:prefLabel>
    <EMMO_967080e5_2f42_4eb2_a3a9_c58143e835f9 xml:lang="en">The class of individuals that stand for quarks elementary particles.</EMMO_967080e5_2f42_4eb2_a3a9_c58143e835f9>
  </rdf:Description>
  <rdf:Description rdf:nodeID="f05bdaa1e617a4bccafc519daf7bf4785b99">
    <rdf:type rdf:resource="http://www.w3.org/2002/07/owl#Restriction"/>
    <owl:onProperty rdf:resource="http://emmo.info/emmo#EMMO_bed1d005_b04e_4a90_94cf_02bc678a8569"/>
    <owl:someValuesFrom rdf:resource="http://emmo.info/emmo#EMMO_f6070071_d054_4b17_9d2d_f446f7147d0f"/>
  </rdf:Description>
  <rdf:Description rdf:nodeID="f8fb83657cd5f496db3c2b94baf326f26b1">
    <rdf:type rdf:resource="http://www.w3.org/2002/07/owl#Restriction"/>
    <owl:onProperty rdf:resource="http://emmo.info/emmo#EMMO_67fc0a36_8dcb_4ffa_9a43_31074efa3296"/>
    <owl:allValuesFrom rdf:resource="http://emmo.info/emmo#EMMO_b081b346_7279_46ef_9a3d_2c088fcd79f4"/>
  </rdf:Description>
  <rdf:Description rdf:about="http://emmo.info/emmo#EMMO_a4d66059_5dd3_4b90_b4cb_10960559441b">
    <EMMO_967080e5_2f42_4eb2_a3a9_c58143e835f9 xml:lang="en">The process of transforming raw materials into a product by the use of manual labor, machinery or chemical/biological processes.</EMMO_967080e5_2f42_4eb2_a3a9_c58143e835f9>
    <rdf:type rdf:resource="http://www.w3.org/2002/07/owl#Class"/>
    <rdfs:subClassOf rdf:resource="http://emmo.info/emmo#EMMO_43e9a05d_98af_41b4_92f6_00f79a09bfce"/>
    <skos:prefLabel xml:lang="en">Manufacturing</skos:prefLabel>
    <rdfs:subClassOf rdf:nodeID="ffbe75b10062f400ea693809785c50a44b5"/>
    <rdfs:comment xml:lang="en">From Latin manufacture: "made by hand".</rdfs:comment>
  </rdf:Description>
  <rdf:Description rdf:about="http://emmo.info/emmo#EMMO_8d00f093_3f45_4ea3_986c_b3545c3c2f4c">
    <rdfs:subClassOf rdf:nodeID="f05bdaa1e617a4bccafc519daf7bf4785b102"/>
    <EMMO_70fe84ff_99b6_4206_a9fc_9a8931836d84 xml:lang="en">The candela, symbol cd, is the SI unit of luminous intensity in a given direction. It is defined by taking the fixed numerical value of the luminous efficacy of monochromatic radiation of frequency 540×1012 Hz, Kcd, to be 683 when expressed in the unit lm W−1, which is equal to cd sr W−1, or cd sr kg−1 m−2 s3, where the kilogram, metre and second are defined in terms of h, c and ∆νCs.</EMMO_70fe84ff_99b6_4206_a9fc_9a8931836d84>
    <rdf:type rdf:resource="http://www.w3.org/2002/07/owl#Class"/>
    <rdfs:subClassOf rdf:nodeID="f05bdaa1e617a4bccafc519daf7bf4785b101"/>
    <EMMO_fe015383_afb3_44a6_ae86_043628697aa2>https://doi.org/10.1351/goldbook.C00787</EMMO_fe015383_afb3_44a6_ae86_043628697aa2>
    <EMMO_1f1b164d_ec6a_4faa_8d5e_88bda62316cc>http://qudt.org/vocab/unit/CD</EMMO_1f1b164d_ec6a_4faa_8d5e_88bda62316cc>
    <skos:prefLabel xml:lang="en">Candela</skos:prefLabel>
  </rdf:Description>
  <rdf:Description rdf:nodeID="fdb1489b80bcc4ee28afe0be8feb9b935b15">
    <rdf:rest rdf:nodeID="fdb1489b80bcc4ee28afe0be8feb9b935b16"/>
    <rdf:type rdf:resource="http://www.w3.org/1999/02/22-rdf-syntax-ns#List"/>
    <rdf:first rdf:resource="http://emmo.info/emmo#EMMO_d0200cf1_e4f4_45ae_873f_b9359daea3cd"/>
  </rdf:Description>
  <rdf:Description rdf:nodeID="f05bdaa1e617a4bccafc519daf7bf4785b95">
    <rdf:type rdf:resource="http://www.w3.org/2002/07/owl#Restriction"/>
    <owl:someValuesFrom rdf:resource="http://emmo.info/emmo#EMMO_b3600e73_3e05_479d_9714_c041c3acf5cc"/>
    <owl:onProperty rdf:resource="http://emmo.info/emmo#EMMO_bed1d005_b04e_4a90_94cf_02bc678a8569"/>
  </rdf:Description>
  <rdf:Description rdf:about="http://emmo.info/emmo#EMMO_da1dd4a7_c611_4ad4_bef6_7646f28aa598">
    <rdfs:comment xml:lang="en">Measurement unit for illuminance.</rdfs:comment>
    <skos:prefLabel xml:lang="en">Lux</skos:prefLabel>
    <EMMO_1f1b164d_ec6a_4faa_8d5e_88bda62316cc>http://qudt.org/vocab/unit/LUX</EMMO_1f1b164d_ec6a_4faa_8d5e_88bda62316cc>
    <EMMO_fe015383_afb3_44a6_ae86_043628697aa2>https://doi.org/10.1351/goldbook.L03651</EMMO_fe015383_afb3_44a6_ae86_043628697aa2>
    <rdf:type rdf:resource="http://www.w3.org/2002/07/owl#Class"/>
    <rdfs:subClassOf rdf:nodeID="f05bdaa1e617a4bccafc519daf7bf4785b142"/>
    <rdfs:subClassOf rdf:nodeID="f05bdaa1e617a4bccafc519daf7bf4785b141"/>
  </rdf:Description>
  <rdf:Description rdf:about="http://emmo.info/emmo/top">
    <rdfs:comment xml:lang="en">Contacts:
Gerhard Goldbeck
Goldbeck Consulting Ltd (UK)
email: gerhard@goldbeck-consulting.com

Emanuele Ghedini
University of Bologna (IT)
email: emanuele.ghedini@unibo.it</rdfs:comment>
    <dcterms:creator>Adham Hashibon</dcterms:creator>
    <rdfs:comment xml:lang="en">The EMMO requires FacT++ reasoner plugin in order to visualize all inferences and class hierarchy (ctrl+R hotkey in Protege).</rdfs:comment>
    <dcterms:title xml:lang="en">European Materials &amp; Modelling Ontology</dcterms:title>
    <dcterms:contributor>Access, DE</dcterms:contributor>
    <owl:versionInfo>1.0.0-beta</owl:versionInfo>
    <dcterms:creator>Georg Schmitz</dcterms:creator>
    <dcterms:creator>Jesper Friis</dcterms:creator>
    <dcterms:contributor>Fraunhofer IWM, DE</dcterms:contributor>
    <owl:versionIRI rdf:resource="http://emmo.info/emmo/1.0.0-beta/top"/>
    <dcterms:license>https://creativecommons.org/licenses/by/4.0/legalcode</dcterms:license>
    <dcterms:abstract xml:lang="en">European Materials &amp; Modelling Ontology (EMMO)

EMMO is a multidisciplinary effort to develop a standard representational framework (the ontology) based on current materials modelling knowledge, including physical sciences, analytical philosophy and information and communication technologies.

It provides the connection between the physical world, materials characterisation world and materials modelling world.

EMMO is released under a Creative Commons license Attribution 4.0 International (CC BY 4.0).</dcterms:abstract>
    <dcterms:contributor>Goldbeck Consulting Ltd (UK)</dcterms:contributor>
    <dcterms:contributor>University of Bologna, IT</dcterms:contributor>
    <rdf:type rdf:resource="http://www.w3.org/2002/07/owl#Ontology"/>
    <dcterms:publisher>EMMC ASBL</dcterms:publisher>
    <dcterms:creator>Emanuele Ghedini</dcterms:creator>
    <dcterms:creator>Gerhard Goldbeck</dcterms:creator>
    <dcterms:contributor>SINTEF, NO</dcterms:contributor>
  </rdf:Description>
  <rdf:Description rdf:nodeID="fe0b20157736f4a31909181349b2e6219b26">
    <owl:hasValue>T-2 L+2 M0 I0 Θ0 N0 J0</owl:hasValue>
    <owl:onProperty rdf:resource="http://emmo.info/emmo#EMMO_23b579e1_8088_45b5_9975_064014026c42"/>
    <rdf:type rdf:resource="http://www.w3.org/2002/07/owl#Restriction"/>
  </rdf:Description>
  <rdf:Description rdf:nodeID="f05bdaa1e617a4bccafc519daf7bf4785b196">
    <rdf:rest rdf:nodeID="f05bdaa1e617a4bccafc519daf7bf4785b197"/>
    <rdf:first rdf:resource="http://emmo.info/emmo#EMMO_3a185e6c_9e19_4776_b583_19c978156aa0"/>
    <rdf:type rdf:resource="http://www.w3.org/1999/02/22-rdf-syntax-ns#List"/>
  </rdf:Description>
  <rdf:Description rdf:nodeID="ffcb99037244f48d590430c228d02afdbb16">
    <owl:onProperty rdf:resource="http://emmo.info/emmo#EMMO_67fc0a36_8dcb_4ffa_9a43_31074efa3296"/>
    <rdf:type rdf:resource="http://www.w3.org/2002/07/owl#Restriction"/>
    <owl:allValuesFrom rdf:resource="http://emmo.info/emmo#EMMO_e7bc8939_7ff8_4917_beb5_c42730b390f3"/>
  </rdf:Description>
  <rdf:Description rdf:about="http://emmo.info/emmo#EMMO_b081b346_7279_46ef_9a3d_2c088fcd79f4">
    <EMMO_967080e5_2f42_4eb2_a3a9_c58143e835f9 xml:lang="en">A 'Quantity' that stands for the standard reference magnitude of a specific class of measurement processes, defined and adopted by convention or by law.

The numerical quantity value of the 'MeasurementUnit' is conventionally 1 and does not appear.

Quantitative measurement results are expressed as a multiple of the 'MeasurementUnit'.</EMMO_967080e5_2f42_4eb2_a3a9_c58143e835f9>
    <rdfs:comment xml:lang="en">While the SI brochure treats 'MeasurementUnit' as a 'PhysicalQuantity', in the EMMO this is not possible since the latter always has two direct parts, a 'Numerical' and a 'MeasurementUnit', while the former a single 'Symbol'.

SI distinguishes between a quantity (an abstract concept) and the quantity value (a number and a reference). The EMMO, following strict nominalism, considers a SI quantity as a SI quantity value, collapsing the two concepts into one: the 'Quantity'.

So, for the EMMO the symbol "kg" is not a physical quantity but a 'MeasurementUnit', while the string "1 kg" is 'Physical Quantity'.</rdfs:comment>
    <rdfs:comment xml:lang="en">"Real scalar quantity, defined and adopted by convention, with which any other quantity of the same kind can be compared to express the ratio of the second quantity to the first one as a number"
ISO 80000-1</rdfs:comment>
    <rdfs:comment xml:lang="en">"Unit symbols are mathematical entities and not abbreviations."

"Symbols for units are treated as mathematical entities. In expressing the value of a quantity as the product of a numerical value and a unit, both the numerical value and the unit may be treated by the ordinary rules of algebra."

https://www.bipm.org/utils/common/pdf/si-brochure/SI-Brochure-9-EN.pdf</rdfs:comment>
    <skos:prefLabel xml:lang="en">MeasurementUnit</skos:prefLabel>
    <rdf:type rdf:resource="http://www.w3.org/2002/07/owl#Class"/>
    <rdfs:subClassOf rdf:resource="http://emmo.info/emmo#EMMO_18ce5200_00f5_45bb_8c6f_6fb128cd41ae"/>
    <owl:disjointUnionOf rdf:nodeID="f8fb83657cd5f496db3c2b94baf326f26b28"/>
    <rdfs:subClassOf rdf:nodeID="f8fb83657cd5f496db3c2b94baf326f26b27"/>
  </rdf:Description>
  <rdf:Description rdf:nodeID="f05bdaa1e617a4bccafc519daf7bf4785b133">
    <rdf:type rdf:resource="http://www.w3.org/2002/07/owl#Restriction"/>
    <owl:someValuesFrom rdf:resource="http://emmo.info/emmo#EMMO_515b5579_d526_4842_9e6f_ecc34db6f368"/>
    <owl:onProperty rdf:resource="http://emmo.info/emmo#EMMO_bed1d005_b04e_4a90_94cf_02bc678a8569"/>
  </rdf:Description>
  <rdf:Description rdf:nodeID="fe0b20157736f4a31909181349b2e6219b35">
    <rdf:type rdf:resource="http://www.w3.org/2002/07/owl#Restriction"/>
    <owl:onProperty rdf:resource="http://emmo.info/emmo#EMMO_23b579e1_8088_45b5_9975_064014026c42"/>
    <owl:hasValue>T0 L0 M0 I+1 Θ0 N0 J0</owl:hasValue>
  </rdf:Description>
  <rdf:Description rdf:nodeID="ffcb99037244f48d590430c228d02afdbb4">
    <owl:someValuesFrom rdf:resource="http://emmo.info/emmo#EMMO_b3600e73_3e05_479d_9714_c041c3acf5cc"/>
    <owl:onProperty rdf:resource="http://emmo.info/emmo#EMMO_bed1d005_b04e_4a90_94cf_02bc678a8569"/>
    <rdf:type rdf:resource="http://www.w3.org/2002/07/owl#Restriction"/>
  </rdf:Description>
  <rdf:Description rdf:nodeID="fe0b20157736f4a31909181349b2e6219b22">
    <owl:onProperty rdf:resource="http://emmo.info/emmo#EMMO_23b579e1_8088_45b5_9975_064014026c42"/>
    <rdf:type rdf:resource="http://www.w3.org/2002/07/owl#Restriction"/>
    <owl:hasValue>T+3 L-1 M-1 I0 Θ0 N0 J+1</owl:hasValue>
  </rdf:Description>
  <rdf:Description rdf:nodeID="f05bdaa1e617a4bccafc519daf7bf4785b15">
    <owl:onProperty rdf:resource="http://emmo.info/emmo#EMMO_faf79f53_749d_40b2_807c_d34244c192f4"/>
    <owl:hasValue rdf:datatype="http://www.w3.org/2001/XMLSchema#double">10.0</owl:hasValue>
    <rdf:type rdf:resource="http://www.w3.org/2002/07/owl#Restriction"/>
  </rdf:Description>
  <rdf:Description rdf:nodeID="f05bdaa1e617a4bccafc519daf7bf4785b20">
    <owl:onProperty rdf:resource="http://emmo.info/emmo#EMMO_23b579e1_8088_45b5_9975_064014026c42"/>
    <rdf:type rdf:resource="http://www.w3.org/2002/07/owl#Restriction"/>
    <owl:hasValue>h</owl:hasValue>
  </rdf:Description>
  <rdf:Description rdf:about="http://emmo.info/emmo#EMMO_23b579e1_8088_45b5_9975_064014026c42">
    <rdf:type rdf:resource="http://www.w3.org/2002/07/owl#DatatypeProperty"/>
    <rdfs:range rdf:resource="http://www.w3.org/2001/XMLSchema#string"/>
    <rdfs:domain rdf:resource="http://emmo.info/emmo#EMMO_a1083d0a_c1fb_471f_8e20_a98f881ad527"/>
    <skos:prefLabel xml:lang="en">hasSymbolData</skos:prefLabel>
  </rdf:Description>
  <rdf:Description rdf:nodeID="ffcb99037244f48d590430c228d02afdbb17">
    <rdf:rest rdf:nodeID="ffcb99037244f48d590430c228d02afdbb18"/>
    <rdf:first rdf:resource="http://emmo.info/emmo#EMMO_00dd79e0_31a6_427e_9b9c_90f3097e4a96"/>
    <rdf:type rdf:resource="http://www.w3.org/1999/02/22-rdf-syntax-ns#List"/>
  </rdf:Description>
  <rdf:Description rdf:nodeID="fe24a777e3fd743f986ce83488d2cf30bb26">
    <owl:onProperty rdf:resource="http://emmo.info/emmo#EMMO_b2282816_b7a3_44c6_b2cb_3feff1ceb7fe"/>
    <owl:someValuesFrom rdf:resource="http://emmo.info/emmo#EMMO_f9bc8b52_85e9_4b53_b969_dd7724d5b8e4"/>
    <rdf:type rdf:resource="http://www.w3.org/2002/07/owl#Restriction"/>
  </rdf:Description>
  <rdf:Description rdf:nodeID="fe24a777e3fd743f986ce83488d2cf30bb25">
    <owl:hasValue>∇</owl:hasValue>
    <rdf:type rdf:resource="http://www.w3.org/2002/07/owl#Restriction"/>
    <owl:onProperty rdf:resource="http://emmo.info/emmo#EMMO_23b579e1_8088_45b5_9975_064014026c42"/>
  </rdf:Description>
  <rdf:Description rdf:nodeID="f05bdaa1e617a4bccafc519daf7bf4785b119">
    <owl:hasValue rdf:datatype="http://www.w3.org/2001/XMLSchema#double">1000000000.0</owl:hasValue>
    <rdf:type rdf:resource="http://www.w3.org/2002/07/owl#Restriction"/>
    <owl:onProperty rdf:resource="http://emmo.info/emmo#EMMO_faf79f53_749d_40b2_807c_d34244c192f4"/>
  </rdf:Description>
  <rdf:Description rdf:nodeID="f05bdaa1e617a4bccafc519daf7bf4785b154">
    <owl:inverseOf rdf:resource="http://emmo.info/emmo#EMMO_3446e167_c576_49d6_846c_215bb8878a55"/>
  </rdf:Description>
  <rdf:Description rdf:nodeID="f05bdaa1e617a4bccafc519daf7bf4785b130">
    <owl:inverseOf rdf:resource="http://emmo.info/emmo#EMMO_3446e167_c576_49d6_846c_215bb8878a55"/>
  </rdf:Description>
  <rdf:Description rdf:nodeID="f8fb83657cd5f496db3c2b94baf326f26b29">
    <rdf:first rdf:resource="http://emmo.info/emmo#EMMO_c6d4a5e0_7e95_44df_a6db_84ee0a8bbc8e"/>
    <rdf:rest rdf:resource="http://www.w3.org/1999/02/22-rdf-syntax-ns#nil"/>
    <rdf:type rdf:resource="http://www.w3.org/1999/02/22-rdf-syntax-ns#List"/>
  </rdf:Description>
  <rdf:Description rdf:about="http://emmo.info/emmo#EMMO_585e0ff0_9429_4d3c_b578_58abb1ba21d1">
    <owl:equivalentClass rdf:nodeID="fe0b20157736f4a31909181349b2e6219b21"/>
    <skos:prefLabel xml:lang="en">InductanceDimension</skos:prefLabel>
    <rdf:type rdf:resource="http://www.w3.org/2002/07/owl#Class"/>
    <rdfs:subClassOf rdf:resource="http://emmo.info/emmo#EMMO_9895a1b4_f0a5_4167_ac5e_97db40b8bfcc"/>
  </rdf:Description>
  <rdf:Description rdf:nodeID="f05bdaa1e617a4bccafc519daf7bf4785b38">
    <rdf:first rdf:resource="http://emmo.info/emmo#EMMO_314ba716_2d3d_4462_9a4f_d3419ae1df43"/>
    <rdf:rest rdf:nodeID="f05bdaa1e617a4bccafc519daf7bf4785b39"/>
    <rdf:type rdf:resource="http://www.w3.org/1999/02/22-rdf-syntax-ns#List"/>
  </rdf:Description>
  <rdf:Description rdf:about="http://emmo.info/emmo#EMMO_d41ce84b_4317_41fb_a5d1_6cd281fca106">
    <rdf:type rdf:resource="http://www.w3.org/2002/07/owl#Class"/>
    <skos:prefLabel xml:lang="en">SIPrefixedUnit</skos:prefLabel>
    <rdfs:comment xml:lang="en">The presence of the prefix makes this units non-coherent with SI system.</rdfs:comment>
    <EMMO_967080e5_2f42_4eb2_a3a9_c58143e835f9 xml:lang="en">A SI base or special unit with a metric prefix.</EMMO_967080e5_2f42_4eb2_a3a9_c58143e835f9>
    <rdfs:subClassOf rdf:resource="http://emmo.info/emmo#EMMO_c6d4a5e0_7e95_44df_a6db_84ee0a8bbc8e"/>
  </rdf:Description>
  <rdf:Description rdf:about="http://emmo.info/emmo#EMMO_0277f24a_ea7f_4917_81b7_fb0406c8fc62">
    <EMMO_967080e5_2f42_4eb2_a3a9_c58143e835f9 xml:lang="en">A union of classes that categorize physicals under a holistic perspective: the interest is on the whole 4D object (process) and the role of its 4D parts (participants) without going further into specifying the spatial hierarchy or the temporal position of each part.</EMMO_967080e5_2f42_4eb2_a3a9_c58143e835f9>
    <rdfs:subClassOf rdf:resource="http://emmo.info/emmo#EMMO_49267eba_5548_4163_8f36_518d65b583f9"/>
    <rdfs:comment xml:lang="en">Holism (from Greek ὅλος holos "all, whole, entire").</rdfs:comment>
    <rdf:type rdf:resource="http://www.w3.org/2002/07/owl#Class"/>
    <skos:prefLabel xml:lang="en">Holistic</skos:prefLabel>
    <rdfs:comment xml:lang="en">An holistic perspective considers each part of the whole as equally important, without the need of a granularity hierarchy (in time or space).

A molecule of a body can have role in the body evolution, without caring if its part of a specific organ and without specifying the time interval in which this role occurred.

This class allows the picking of parts without necessarily going trough a rigid hierarchy of spatial compositions (e.g. body -&gt; organ -&gt; cell -&gt; molecule) or temporal composition.</rdfs:comment>
    <owl:equivalentClass rdf:nodeID="f0b819106611c4b798f33b16c65f4398db1"/>
  </rdf:Description>
  <rdf:Description rdf:about="http://emmo.info/emmo#EMMO_1b52ee70_121e_4d8d_8419_3f97cd0bd89c">
    <EMMO_967080e5_2f42_4eb2_a3a9_c58143e835f9 xml:lang="en">An 'interpreter' that perceives another 'entity' (the 'object') through a specific perception mechanism and produces a 'property' (the 'sign') that stands for the result of that particular perception.</EMMO_967080e5_2f42_4eb2_a3a9_c58143e835f9>
    <rdfs:subClassOf rdf:resource="http://emmo.info/emmo#EMMO_0527413c_b286_4e9c_b2d0_03fb2a038dee"/>
    <rdfs:subClassOf rdf:nodeID="fdb1489b80bcc4ee28afe0be8feb9b935b3"/>
    <skos:prefLabel xml:lang="en">Observer</skos:prefLabel>
    <rdf:type rdf:resource="http://www.w3.org/2002/07/owl#Class"/>
  </rdf:Description>
  <rdf:Description rdf:about="http://emmo.info/emmo#EMMO_314d0bd5_67ed_437e_a609_36d46147cea7">
    <rdfs:comment xml:lang="en">While every 'process' in the EMMO involves physical objects, this class is devoted to represent real world objects that express a phenomenon relevant for the ontologist</rdfs:comment>
    <skos:prefLabel xml:lang="en">PhysicalPhenomenon</skos:prefLabel>
    <rdfs:subClassOf rdf:resource="http://emmo.info/emmo#EMMO_43e9a05d_98af_41b4_92f6_00f79a09bfce"/>
    <EMMO_967080e5_2f42_4eb2_a3a9_c58143e835f9 xml:lang="en">A 'process' that is recognized by physical sciences and is catogrized accordingly.</EMMO_967080e5_2f42_4eb2_a3a9_c58143e835f9>
    <rdf:type rdf:resource="http://www.w3.org/2002/07/owl#Class"/>
  </rdf:Description>
  <rdf:Description rdf:about="http://emmo.info/emmo#EMMO_3b931698_937e_49be_ab1b_36fa52d91181">
    <EMMO_967080e5_2f42_4eb2_a3a9_c58143e835f9 xml:lang="en">Measure of magnetism, taking account of the strength and the extent of a magnetic field.</EMMO_967080e5_2f42_4eb2_a3a9_c58143e835f9>
    <rdfs:subClassOf rdf:resource="http://emmo.info/emmo#EMMO_2946d40b_24a1_47fa_8176_e3f79bb45064"/>
    <rdf:type rdf:resource="http://www.w3.org/2002/07/owl#Class"/>
    <skos:prefLabel xml:lang="en">MagneticFlux</skos:prefLabel>
    <EMMO_1f1b164d_ec6a_4faa_8d5e_88bda62316cc>http://qudt.org/vocab/quantitykind/MagneticFlux</EMMO_1f1b164d_ec6a_4faa_8d5e_88bda62316cc>
    <EMMO_6dd685dd_1895_46e4_b227_be9f7d643c25>http://dbpedia.org/page/Magnetic_flux</EMMO_6dd685dd_1895_46e4_b227_be9f7d643c25>
    <EMMO_de178b12_5d35_4bca_8efa_a4193162571d>T-2 L+2 M+1 I-1 Θ0 N0 J0</EMMO_de178b12_5d35_4bca_8efa_a4193162571d>
    <EMMO_fe015383_afb3_44a6_ae86_043628697aa2>https://doi.org/10.1351/goldbook.M03684</EMMO_fe015383_afb3_44a6_ae86_043628697aa2>
  </rdf:Description>
  <rdf:Description rdf:nodeID="fe24a777e3fd743f986ce83488d2cf30bb23">
    <rdf:type rdf:resource="http://www.w3.org/2002/07/owl#Restriction"/>
    <owl:allValuesFrom rdf:resource="http://emmo.info/emmo#EMMO_4ce76d7f_03f8_45b6_9003_90052a79bfaa"/>
    <owl:onProperty rdf:nodeID="fe24a777e3fd743f986ce83488d2cf30bb24"/>
  </rdf:Description>
  <rdf:Description rdf:about="http://emmo.info/emmo#EMMO_5add9885_dc98_4fa5_8482_fdf9ba5e3889">
    <skos:prefLabel xml:lang="en">SolidSol</skos:prefLabel>
    <rdfs:subClassOf rdf:resource="http://emmo.info/emmo#EMMO_a2b006f2_bbfd_4dba_bcaa_3fca20cd6be1"/>
    <rdf:type rdf:resource="http://www.w3.org/2002/07/owl#Class"/>
    <rdfs:subClassOf rdf:resource="http://emmo.info/emmo#EMMO_31557fae_b039_491c_bcbb_0ccb8711d5a6"/>
    <EMMO_967080e5_2f42_4eb2_a3a9_c58143e835f9 xml:lang="en">A type of sol in the form of one solid dispersed in another continuous solid.</EMMO_967080e5_2f42_4eb2_a3a9_c58143e835f9>
  </rdf:Description>
  <rdf:Description rdf:nodeID="ff14b31ebf90e4bc5ba2839064d29e543b9">
    <rdf:first rdf:resource="http://emmo.info/emmo#EMMO_33e0ac8b_a318_4285_b1de_e95347784632"/>
    <rdf:rest rdf:nodeID="ff14b31ebf90e4bc5ba2839064d29e543b10"/>
    <rdf:type rdf:resource="http://www.w3.org/1999/02/22-rdf-syntax-ns#List"/>
  </rdf:Description>
  <rdf:Description rdf:nodeID="f05bdaa1e617a4bccafc519daf7bf4785b149">
    <owl:onProperty rdf:resource="http://emmo.info/emmo#EMMO_bed1d005_b04e_4a90_94cf_02bc678a8569"/>
    <owl:someValuesFrom rdf:resource="http://emmo.info/emmo#EMMO_847f1d9f_205e_46c1_8cb6_a9e479421f88"/>
    <rdf:type rdf:resource="http://www.w3.org/2002/07/owl#Restriction"/>
  </rdf:Description>
  <rdf:Description rdf:nodeID="fea11ca01461e402d8f697c19c5d8de88b13">
    <rdf:rest rdf:nodeID="fea11ca01461e402d8f697c19c5d8de88b14"/>
    <rdf:first rdf:resource="http://emmo.info/emmo#EMMO_5b2222df_4da6_442f_8244_96e9e45887d1"/>
    <rdf:type rdf:resource="http://www.w3.org/1999/02/22-rdf-syntax-ns#List"/>
  </rdf:Description>
  <rdf:Description rdf:about="http://emmo.info/emmo#EMMO_49804605_c0fe_4538_abda_f70ba1dc8a5d">
    <rdfs:subClassOf rdf:resource="http://emmo.info/emmo#EMMO_c5ddfdba_c074_4aa4_ad6b_1ac4942d300d"/>
    <rdfs:comment xml:lang="en">In the EMMO the relation of participation to a process falls under mereotopology.

Since topological connection means causality, then the only way for a real world object to participate to a process is to be a part of it.</rdfs:comment>
    <skos:prefLabel xml:lang="en">Participant</skos:prefLabel>
    <rdfs:subClassOf rdf:nodeID="f0b819106611c4b798f33b16c65f4398db5"/>
    <EMMO_967080e5_2f42_4eb2_a3a9_c58143e835f9 xml:lang="en">A portion of a 'Process' that participates to the process with a specific role.</EMMO_967080e5_2f42_4eb2_a3a9_c58143e835f9>
    <rdf:type rdf:resource="http://www.w3.org/2002/07/owl#Class"/>
  </rdf:Description>
  <rdf:Description rdf:nodeID="f05bdaa1e617a4bccafc519daf7bf4785b68">
    <rdf:type rdf:resource="http://www.w3.org/1999/02/22-rdf-syntax-ns#List"/>
    <rdf:rest rdf:nodeID="f05bdaa1e617a4bccafc519daf7bf4785b69"/>
    <rdf:first rdf:resource="http://emmo.info/emmo#EMMO_9ff3bf8e_2168_406e_8251_1d158fc948ae"/>
  </rdf:Description>
  <rdf:Description rdf:nodeID="ff14b31ebf90e4bc5ba2839064d29e543b8">
    <rdf:type rdf:resource="http://www.w3.org/1999/02/22-rdf-syntax-ns#List"/>
    <rdf:first rdf:resource="http://emmo.info/emmo#EMMO_2dd512a1_5187_47cc_b0b8_141214e22b59"/>
    <rdf:rest rdf:nodeID="ff14b31ebf90e4bc5ba2839064d29e543b9"/>
  </rdf:Description>
  <rdf:Description rdf:nodeID="f05bdaa1e617a4bccafc519daf7bf4785b124">
    <owl:hasValue>N</owl:hasValue>
    <owl:onProperty rdf:resource="http://emmo.info/emmo#EMMO_23b579e1_8088_45b5_9975_064014026c42"/>
    <rdf:type rdf:resource="http://www.w3.org/2002/07/owl#Restriction"/>
  </rdf:Description>
  <rdf:Description rdf:nodeID="ffcb99037244f48d590430c228d02afdbb36">
    <rdf:type rdf:resource="http://www.w3.org/2002/07/owl#Restriction"/>
    <owl:onProperty rdf:resource="http://emmo.info/emmo#EMMO_bed1d005_b04e_4a90_94cf_02bc678a8569"/>
    <owl:someValuesFrom rdf:resource="http://emmo.info/emmo#EMMO_9141801c_c539_4c72_b423_8c74ff6b8f05"/>
  </rdf:Description>
  <rdf:Description rdf:about="http://emmo.info/emmo#EMMO_8d2d9374_ef3a_47e6_8595_6bc208e07519">
    <rdf:type rdf:resource="http://www.w3.org/2002/07/owl#Class"/>
    <skos:prefLabel xml:lang="en">Theory</skos:prefLabel>
    <EMMO_967080e5_2f42_4eb2_a3a9_c58143e835f9 xml:lang="en">A 'conventional' that stand for a 'physical'.</EMMO_967080e5_2f42_4eb2_a3a9_c58143e835f9>
    <rdfs:comment xml:lang="en">The 'theory' is e.g. a proposition, a book or a paper whose sub-symbols suggest in the mind of the interpreter an interpretant structure that can represent a 'physical'.

It is not an 'icon' (like a math equation), because it has no common resemblance or logical structure with the 'physical'.

In Peirce semiotics: legisign-symbol-argument</rdfs:comment>
    <rdfs:subClassOf rdf:resource="http://emmo.info/emmo#EMMO_35d2e130_6e01_41ed_94f7_00b333d46cf9"/>
  </rdf:Description>
  <rdf:Description rdf:about="http://emmo.info/emmo#EMMO_5a2af26d_99de_4e5e_b1cd_514be71420c3">
    <skos:prefLabel xml:lang="en">Smoke</skos:prefLabel>
    <EMMO_967080e5_2f42_4eb2_a3a9_c58143e835f9 xml:lang="en">Smoke is a solid aerosol made of particles emitted when a material undergoes combustion or pyrolysis.</EMMO_967080e5_2f42_4eb2_a3a9_c58143e835f9>
    <rdfs:subClassOf rdf:resource="http://emmo.info/emmo#EMMO_96c8d72f_b436_44e2_9f7f_085c24094292"/>
    <rdf:type rdf:resource="http://www.w3.org/2002/07/owl#Class"/>
  </rdf:Description>
  <rdf:Description rdf:nodeID="f05bdaa1e617a4bccafc519daf7bf4785b22">
    <owl:inverseOf rdf:resource="http://emmo.info/emmo#EMMO_3446e167_c576_49d6_846c_215bb8878a55"/>
  </rdf:Description>
  <rdf:Description rdf:nodeID="fa691b5894b3543efa24f9838ff46c3eab2">
    <owl:onProperty rdf:resource="http://emmo.info/emmo#EMMO_c5aae418_1622_4d02_93c5_21159e28e6c1"/>
    <owl:someValuesFrom rdf:resource="http://emmo.info/emmo#EMMO_6f5af708_f825_4feb_a0d1_a8d813d3022b"/>
    <rdf:type rdf:resource="http://www.w3.org/2002/07/owl#Restriction"/>
  </rdf:Description>
  <rdf:Description rdf:about="http://emmo.info/emmo#EMMO_17e27c22_37e1_468c_9dd7_95e137f73e7f">
    <rdfs:subPropertyOf rdf:resource="http://emmo.info/emmo#EMMO_8c898653_1118_4682_9bbf_6cc334d16a99"/>
    <rdfs:subPropertyOf rdf:resource="http://emmo.info/emmo#EMMO_d893d373_b579_4867_841e_1c2b31a8d2c6"/>
    <skos:prefLabel xml:lang="en">hasPart</skos:prefLabel>
    <rdf:type rdf:resource="http://www.w3.org/2002/07/owl#TransitiveProperty"/>
    <rdf:type rdf:resource="http://www.w3.org/2002/07/owl#ObjectProperty"/>
  </rdf:Description>
  <rdf:Description rdf:nodeID="fe0b20157736f4a31909181349b2e6219b41">
    <owl:hasValue>T-1 L+1 M0 I0 Θ0 N0 J0</owl:hasValue>
    <owl:onProperty rdf:resource="http://emmo.info/emmo#EMMO_23b579e1_8088_45b5_9975_064014026c42"/>
    <rdf:type rdf:resource="http://www.w3.org/2002/07/owl#Restriction"/>
  </rdf:Description>
  <rdf:Description rdf:about="http://emmo.info/emmo#EMMO_e1981c25_7c55_4020_aa7a_d2e14ced86d4">
    <skos:prefLabel xml:lang="en">Nano</skos:prefLabel>
    <rdfs:subClassOf rdf:nodeID="f05bdaa1e617a4bccafc519daf7bf4785b156"/>
    <rdf:type rdf:resource="http://www.w3.org/2002/07/owl#Class"/>
    <rdfs:subClassOf rdf:nodeID="f05bdaa1e617a4bccafc519daf7bf4785b153"/>
  </rdf:Description>
  <rdf:Description rdf:nodeID="f05bdaa1e617a4bccafc519daf7bf4785b121">
    <owl:someValuesFrom rdf:resource="http://emmo.info/emmo#EMMO_b14d9be5_f81e_469b_abca_379c2e83feab"/>
    <owl:onProperty rdf:resource="http://emmo.info/emmo#EMMO_bed1d005_b04e_4a90_94cf_02bc678a8569"/>
    <rdf:type rdf:resource="http://www.w3.org/2002/07/owl#Restriction"/>
  </rdf:Description>
  <rdf:Description rdf:nodeID="fc2fcd8f8eb3649bcbbaff76ba54058acb4">
    <rdf:type rdf:resource="http://www.w3.org/2002/07/owl#Restriction"/>
    <owl:someValuesFrom rdf:resource="http://emmo.info/emmo#EMMO_0f795e3e_c602_4577_9a43_d5a231aa1360"/>
    <owl:onProperty rdf:resource="http://emmo.info/emmo#EMMO_17e27c22_37e1_468c_9dd7_95e137f73e7f"/>
  </rdf:Description>
  <rdf:Description rdf:about="http://emmo.info/emmo#EMMO_498aad49_f8d4_40a4_a9eb_efd563a0115f">
    <rdfs:subClassOf rdf:resource="http://emmo.info/emmo#EMMO_e0edfb9e_9a96_4fae_b942_831ffe27b84a"/>
    <skos:prefLabel xml:lang="en">Spray</skos:prefLabel>
    <rdf:type rdf:resource="http://www.w3.org/2002/07/owl#Class"/>
    <EMMO_967080e5_2f42_4eb2_a3a9_c58143e835f9 xml:lang="en">A suspension of liquid droplets dispersed in a gas through an atomization process.</EMMO_967080e5_2f42_4eb2_a3a9_c58143e835f9>
  </rdf:Description>
  <rdf:Description rdf:about="http://emmo.info/emmo#EMMO_1f087811_06cb_42d5_90fb_25d0e7e068ef">
    <EMMO_6dd685dd_1895_46e4_b227_be9f7d643c25>http://dbpedia.org/page/Force</EMMO_6dd685dd_1895_46e4_b227_be9f7d643c25>
    <EMMO_de178b12_5d35_4bca_8efa_a4193162571d>T-2 L+1 M+1 I0 Θ0 N0 J0</EMMO_de178b12_5d35_4bca_8efa_a4193162571d>
    <EMMO_1f1b164d_ec6a_4faa_8d5e_88bda62316cc>http://qudt.org/vocab/quantitykind/Force</EMMO_1f1b164d_ec6a_4faa_8d5e_88bda62316cc>
    <skos:prefLabel xml:lang="en">Force</skos:prefLabel>
    <rdfs:subClassOf rdf:resource="http://emmo.info/emmo#EMMO_2946d40b_24a1_47fa_8176_e3f79bb45064"/>
    <rdf:type rdf:resource="http://www.w3.org/2002/07/owl#Class"/>
    <EMMO_fe015383_afb3_44a6_ae86_043628697aa2>https://doi.org/10.1351/goldbook.F02480</EMMO_fe015383_afb3_44a6_ae86_043628697aa2>
    <EMMO_967080e5_2f42_4eb2_a3a9_c58143e835f9 xml:lang="en">Any interaction that, when unopposed, will change the motion of an object.</EMMO_967080e5_2f42_4eb2_a3a9_c58143e835f9>
  </rdf:Description>
  <rdf:Description rdf:about="http://emmo.info/emmo#EMMO_b71e4ba5_8f73_4199_8c96_7ea7f94d9e2a">
    <rdfs:subClassOf rdf:nodeID="f05bdaa1e617a4bccafc519daf7bf4785b133"/>
    <EMMO_fe015383_afb3_44a6_ae86_043628697aa2>https://doi.org/10.1351/goldbook.B00624</EMMO_fe015383_afb3_44a6_ae86_043628697aa2>
    <rdfs:comment xml:lang="en">Unit for radioactive activity.</rdfs:comment>
    <EMMO_1f1b164d_ec6a_4faa_8d5e_88bda62316cc>http://qudt.org/vocab/unit/BQ</EMMO_1f1b164d_ec6a_4faa_8d5e_88bda62316cc>
    <rdf:type rdf:resource="http://www.w3.org/2002/07/owl#Class"/>
    <rdfs:subClassOf rdf:nodeID="f05bdaa1e617a4bccafc519daf7bf4785b134"/>
    <EMMO_70fe84ff_99b6_4206_a9fc_9a8931836d84 xml:lang="en">Radioactive decays per second.</EMMO_70fe84ff_99b6_4206_a9fc_9a8931836d84>
    <skos:prefLabel xml:lang="en">Becquerel</skos:prefLabel>
  </rdf:Description>
  <rdf:Description rdf:nodeID="f05bdaa1e617a4bccafc519daf7bf4785b37">
    <rdf:type rdf:resource="http://www.w3.org/1999/02/22-rdf-syntax-ns#List"/>
    <rdf:first rdf:resource="http://emmo.info/emmo#EMMO_2e5e45fc_f52c_4294_bdc2_5ed7a06dfce7"/>
    <rdf:rest rdf:nodeID="f05bdaa1e617a4bccafc519daf7bf4785b38"/>
  </rdf:Description>
  <rdf:Description rdf:nodeID="f05bdaa1e617a4bccafc519daf7bf4785b47">
    <owl:hasValue>T</owl:hasValue>
    <rdf:type rdf:resource="http://www.w3.org/2002/07/owl#Restriction"/>
    <owl:onProperty rdf:resource="http://emmo.info/emmo#EMMO_23b579e1_8088_45b5_9975_064014026c42"/>
  </rdf:Description>
  <rdf:Description rdf:nodeID="f627ff42579444148ae27fcacfb5f8528b9">
    <rdf:type rdf:resource="http://www.w3.org/2002/07/owl#Restriction"/>
    <owl:onProperty rdf:resource="http://emmo.info/emmo#EMMO_b2282816_b7a3_44c6_b2cb_3feff1ceb7fe"/>
    <owl:someValuesFrom rdf:resource="http://emmo.info/emmo#EMMO_02c0621e_a527_4790_8a0f_2bb51973c819"/>
  </rdf:Description>
  <rdf:Description rdf:nodeID="f05bdaa1e617a4bccafc519daf7bf4785b31">
    <rdf:type rdf:resource="http://www.w3.org/2002/07/owl#Restriction"/>
    <owl:onProperty rdf:resource="http://emmo.info/emmo#EMMO_bed1d005_b04e_4a90_94cf_02bc678a8569"/>
    <owl:someValuesFrom rdf:resource="http://emmo.info/emmo#EMMO_02e894c3_b793_4197_b120_3442e08f58d1"/>
  </rdf:Description>
  <rdf:Description rdf:nodeID="fa691b5894b3543efa24f9838ff46c3eab11">
    <rdf:first rdf:resource="http://emmo.info/emmo#EMMO_6f5af708_f825_4feb_a0d1_a8d813d3022b"/>
    <rdf:rest rdf:nodeID="fa691b5894b3543efa24f9838ff46c3eab12"/>
    <rdf:type rdf:resource="http://www.w3.org/1999/02/22-rdf-syntax-ns#List"/>
  </rdf:Description>
  <rdf:Description rdf:about="http://emmo.info/emmo#EMMO_06658d8d_dcde_4fc9_aae1_17f71c0bcdec">
    <rdf:type rdf:resource="http://www.w3.org/2002/07/owl#Class"/>
    <rdfs:subClassOf rdf:resource="http://emmo.info/emmo#EMMO_28fbea28_2204_4613_87ff_6d877b855fcd"/>
    <skos:prefLabel xml:lang="en">Vector</skos:prefLabel>
  </rdf:Description>
  <rdf:Description rdf:nodeID="f05bdaa1e617a4bccafc519daf7bf4785b191">
    <owl:onProperty rdf:resource="http://emmo.info/emmo#EMMO_faf79f53_749d_40b2_807c_d34244c192f4"/>
    <owl:hasValue rdf:datatype="http://www.w3.org/2001/XMLSchema#double">1e-24</owl:hasValue>
    <rdf:type rdf:resource="http://www.w3.org/2002/07/owl#Restriction"/>
  </rdf:Description>
  <rdf:Description rdf:about="http://emmo.info/emmo#EMMO_852b4ab8_fc29_4749_a8c7_b92d4fca7d5a">
    <EMMO_967080e5_2f42_4eb2_a3a9_c58143e835f9 xml:lang="en">Number of periods per time interval.</EMMO_967080e5_2f42_4eb2_a3a9_c58143e835f9>
    <rdfs:subClassOf rdf:resource="http://emmo.info/emmo#EMMO_2946d40b_24a1_47fa_8176_e3f79bb45064"/>
    <skos:prefLabel xml:lang="en">Frequency</skos:prefLabel>
    <rdf:type rdf:resource="http://www.w3.org/2002/07/owl#Class"/>
    <EMMO_de178b12_5d35_4bca_8efa_a4193162571d>T-1 L0 M0 I0 Θ0 N0 J0</EMMO_de178b12_5d35_4bca_8efa_a4193162571d>
    <EMMO_1f1b164d_ec6a_4faa_8d5e_88bda62316cc>http://qudt.org/vocab/quantitykind/Frequency</EMMO_1f1b164d_ec6a_4faa_8d5e_88bda62316cc>
    <EMMO_6dd685dd_1895_46e4_b227_be9f7d643c25>http://dbpedia.org/page/Frequency</EMMO_6dd685dd_1895_46e4_b227_be9f7d643c25>
    <EMMO_fe015383_afb3_44a6_ae86_043628697aa2>https://doi.org/10.1351/goldbook.FT07383</EMMO_fe015383_afb3_44a6_ae86_043628697aa2>
  </rdf:Description>
  <rdf:Description rdf:about="http://emmo.info/emmo#EMMO_42185fe7_122c_4e0c_a3cd_659d3e21c389">
    <rdf:type rdf:resource="http://www.w3.org/2002/07/owl#Class"/>
    <EMMO_b432d2d5_25f4_4165_99c5_5935a7763c1a xml:lang="en">Sparkling water</EMMO_b432d2d5_25f4_4165_99c5_5935a7763c1a>
    <skos:prefLabel xml:lang="en">LiquidGasSuspension</skos:prefLabel>
    <rdfs:subClassOf rdf:resource="http://emmo.info/emmo#EMMO_7509da43_56b1_4d7f_887a_65d1663df4ba"/>
    <EMMO_967080e5_2f42_4eb2_a3a9_c58143e835f9 xml:lang="en">A coarse dispersion of gas in a liquid continuum phase.</EMMO_967080e5_2f42_4eb2_a3a9_c58143e835f9>
  </rdf:Description>
  <rdf:Description rdf:nodeID="f8fb83657cd5f496db3c2b94baf326f26b8">
    <rdf:rest rdf:nodeID="f8fb83657cd5f496db3c2b94baf326f26b9"/>
    <rdf:first rdf:resource="http://emmo.info/emmo#EMMO_a1083d0a_c1fb_471f_8e20_a98f881ad527"/>
    <rdf:type rdf:resource="http://www.w3.org/1999/02/22-rdf-syntax-ns#List"/>
  </rdf:Description>
  <rdf:Description rdf:about="http://emmo.info/emmo#EMMO_4c49ab58_a6f6_409e_b849_f873ae1dcbee">
    <owl:equivalentClass rdf:nodeID="fe0b20157736f4a31909181349b2e6219b15"/>
    <rdfs:subClassOf rdf:resource="http://emmo.info/emmo#EMMO_9895a1b4_f0a5_4167_ac5e_97db40b8bfcc"/>
    <rdf:type rdf:resource="http://www.w3.org/2002/07/owl#Class"/>
    <skos:prefLabel xml:lang="en">MagneticFluxDimension</skos:prefLabel>
  </rdf:Description>
  <rdf:Description rdf:about="http://emmo.info/emmo#EMMO_9ff3bf8e_2168_406e_8251_1d158fc948ae">
    <rdfs:subClassOf rdf:nodeID="f05bdaa1e617a4bccafc519daf7bf4785b108"/>
    <skos:prefLabel xml:lang="en">Micro</skos:prefLabel>
    <rdf:type rdf:resource="http://www.w3.org/2002/07/owl#Class"/>
    <rdfs:subClassOf rdf:nodeID="f05bdaa1e617a4bccafc519daf7bf4785b105"/>
  </rdf:Description>
  <rdf:Description rdf:about="http://emmo.info/emmo#EMMO_4c21fb86_fdcf_444e_b498_86fe656295af">
    <skos:prefLabel xml:lang="en">Plasma</skos:prefLabel>
    <rdfs:subClassOf rdf:resource="http://emmo.info/emmo#EMMO_87ac88ff_8379_4f5a_8c7b_424a8fff1ee8"/>
    <rdf:type rdf:resource="http://www.w3.org/2002/07/owl#Class"/>
    <EMMO_967080e5_2f42_4eb2_a3a9_c58143e835f9 xml:lang="en">A fluid in which a gas is ionized to a level where its electrical conductivity allows long-range electric and magnetic fields to dominate its behaviour.</EMMO_967080e5_2f42_4eb2_a3a9_c58143e835f9>
  </rdf:Description>
  <rdf:Description rdf:about="http://emmo.info/emmo#EMMO_b41515a9_28d8_4d78_8165_74b2fc72f89e">
    <EMMO_1f1b164d_ec6a_4faa_8d5e_88bda62316cc>http://qudt.org/vocab/unit/NP</EMMO_1f1b164d_ec6a_4faa_8d5e_88bda62316cc>
    <rdf:type rdf:resource="http://www.w3.org/2002/07/owl#Class"/>
    <rdfs:subClassOf rdf:nodeID="ffcb99037244f48d590430c228d02afdbb43"/>
    <skos:prefLabel xml:lang="en">Neper</skos:prefLabel>
    <rdfs:subClassOf rdf:resource="http://emmo.info/emmo#EMMO_591e02fd_8d37_45a6_9d11_bb21cef391a0"/>
    <EMMO_6dd685dd_1895_46e4_b227_be9f7d643c25>http://dbpedia.org/page/Neper</EMMO_6dd685dd_1895_46e4_b227_be9f7d643c25>
    <EMMO_c84c6752_6d64_48cc_9500_e54a3c34898d>https://en.wikipedia.org/wiki/Neper</EMMO_c84c6752_6d64_48cc_9500_e54a3c34898d>
    <rdfs:subClassOf rdf:nodeID="ffcb99037244f48d590430c228d02afdbb42"/>
    <EMMO_fe015383_afb3_44a6_ae86_043628697aa2>https://doi.org/10.1351/goldbook.N04106</EMMO_fe015383_afb3_44a6_ae86_043628697aa2>
    <EMMO_70fe84ff_99b6_4206_a9fc_9a8931836d84 xml:lang="en">Unit of measurement for quantities of type level or level difference, which are defined as the natural logarithm of the ratio of power- or field-type quantities.

The value of a ratio in nepers is given by `ln(x1/x2)` where `x1` and `x2` are the values of interest (amplitudes), and ln is the natural logarithm. When the values are quadratic in the amplitude (e.g. power), they are first linearised by taking the square root before the logarithm is taken, or equivalently the result is halved.

Wikipedia</EMMO_70fe84ff_99b6_4206_a9fc_9a8931836d84>
  </rdf:Description>
  <rdf:Description rdf:about="http://emmo.info/emmo#EMMO_e13b2173_1dec_4b97_9ac1_1dc4b418612a">
    <rdf:type rdf:resource="http://www.w3.org/2002/07/owl#Class"/>
    <skos:prefLabel xml:lang="en">UTF8</skos:prefLabel>
    <rdfs:subClassOf rdf:resource="http://emmo.info/emmo#EMMO_a1083d0a_c1fb_471f_8e20_a98f881ad527"/>
  </rdf:Description>
  <rdf:Description rdf:nodeID="f8fb83657cd5f496db3c2b94baf326f26b40">
    <owl:onClass rdf:resource="http://emmo.info/emmo#EMMO_18ce5200_00f5_45bb_8c6f_6fb128cd41ae"/>
    <owl:qualifiedCardinality rdf:datatype="http://www.w3.org/2001/XMLSchema#nonNegativeInteger">1</owl:qualifiedCardinality>
    <owl:onProperty rdf:resource="http://emmo.info/emmo#EMMO_67fc0a36_8dcb_4ffa_9a43_31074efa3296"/>
    <rdf:type rdf:resource="http://www.w3.org/2002/07/owl#Restriction"/>
  </rdf:Description>
  <rdf:Description rdf:nodeID="ff14b31ebf90e4bc5ba2839064d29e543b17">
    <rdf:rest rdf:nodeID="ff14b31ebf90e4bc5ba2839064d29e543b18"/>
    <rdf:first rdf:resource="http://emmo.info/emmo#EMMO_8f87e700_99a8_4427_8ffb_e493de05c217"/>
    <rdf:type rdf:resource="http://www.w3.org/1999/02/22-rdf-syntax-ns#List"/>
  </rdf:Description>
  <rdf:Description rdf:about="http://emmo.info/emmo#EMMO_a66427d1_9932_4363_9ec5_7d91f2bfda1e">
    <EMMO_de178b12_5d35_4bca_8efa_a4193162571d>T0 L0 M0 I0 Θ0 N0 J0</EMMO_de178b12_5d35_4bca_8efa_a4193162571d>
    <rdf:type rdf:resource="http://www.w3.org/2002/07/owl#Class"/>
    <rdfs:subClassOf rdf:resource="http://emmo.info/emmo#EMMO_2946d40b_24a1_47fa_8176_e3f79bb45064"/>
    <EMMO_6dd685dd_1895_46e4_b227_be9f7d643c25>http://dbpedia.org/page/Dimensionless_quantity</EMMO_6dd685dd_1895_46e4_b227_be9f7d643c25>
    <EMMO_967080e5_2f42_4eb2_a3a9_c58143e835f9 xml:lang="en">A quantity to which no physical dimension is assigned and with a corresponding unit of measurement in the SI of the unit one.</EMMO_967080e5_2f42_4eb2_a3a9_c58143e835f9>
    <EMMO_c84c6752_6d64_48cc_9500_e54a3c34898d>https://en.wikipedia.org/wiki/Dimensionless_quantity</EMMO_c84c6752_6d64_48cc_9500_e54a3c34898d>
    <skos:prefLabel xml:lang="en">ISQDimensionlessQuantity</skos:prefLabel>
    <EMMO_fe015383_afb3_44a6_ae86_043628697aa2>https://doi.org/10.1351/goldbook.D01742</EMMO_fe015383_afb3_44a6_ae86_043628697aa2>
  </rdf:Description>
  <rdf:Description rdf:about="http://emmo.info/emmo#EMMO_909415d1_7c43_4d5e_bbeb_7e1910159f66">
    <rdfs:subClassOf rdf:resource="http://emmo.info/emmo#EMMO_2a888cdf_ec4a_4ec5_af1c_0343372fc978"/>
    <EMMO_967080e5_2f42_4eb2_a3a9_c58143e835f9 xml:lang="en">An 'ObjectiveProperty' that cannot be quantified.</EMMO_967080e5_2f42_4eb2_a3a9_c58143e835f9>
    <skos:prefLabel xml:lang="en">NominalProperty</skos:prefLabel>
    <EMMO_b432d2d5_25f4_4165_99c5_5935a7763c1a xml:lang="en">CFC is a 'sign' that stands for the fact that the morphology of atoms composing the microstructure of an entity is predominantly Cubic Face Centered

A color is a nominal property.

Sex of a human being.</EMMO_b432d2d5_25f4_4165_99c5_5935a7763c1a>
    <rdf:type rdf:resource="http://www.w3.org/2002/07/owl#Class"/>
    <rdfs:comment xml:lang="en">"Property of a phenomenon, body, or substance, where the property has no magnitude."

"A nominal property has a value, which can be expressed in words, by alphanumerical codes, or by other means."

International vocabulary of metrology (VIM)</rdfs:comment>
  </rdf:Description>
  <rdf:Description rdf:nodeID="f38ecd0eaa78747b4ad569754ea441153b2">
    <rdf:type rdf:resource="http://www.w3.org/2002/07/owl#Restriction"/>
    <owl:onProperty rdf:resource="http://emmo.info/emmo#EMMO_b2282816_b7a3_44c6_b2cb_3feff1ceb7fe"/>
    <owl:allValuesFrom rdf:resource="http://emmo.info/emmo#EMMO_a1083d0a_c1fb_471f_8e20_a98f881ad527"/>
  </rdf:Description>
  <rdf:Description rdf:about="http://emmo.info/emmo#EMMO_64aba1e5_24b7_4140_8eb4_676c35698e79">
    <skos:prefLabel xml:lang="en">C++</skos:prefLabel>
    <rdfs:subClassOf rdf:resource="http://emmo.info/emmo#EMMO_8681074a_e225_4e38_b586_e85b0f43ce38"/>
    <EMMO_967080e5_2f42_4eb2_a3a9_c58143e835f9 xml:lang="en">A language object respecting the syntactic rules of C++.</EMMO_967080e5_2f42_4eb2_a3a9_c58143e835f9>
    <rdf:type rdf:resource="http://www.w3.org/2002/07/owl#Class"/>
  </rdf:Description>
  <rdf:Description rdf:about="http://emmo.info/emmo#EMMO_3227b821_26a5_4c7c_9c01_5c24483e0bd0">
    <rdfs:comment xml:lang="en">"The unit one is the neutral element of any system of units – necessary and present automatically."
SI Brochure</rdfs:comment>
    <rdf:type rdf:resource="http://www.w3.org/2002/07/owl#Class"/>
    <rdfs:subClassOf rdf:resource="http://emmo.info/emmo#EMMO_9895a1b4_f0a5_4167_ac5e_97db40b8bfcc"/>
    <owl:equivalentClass rdf:nodeID="f8fb83657cd5f496db3c2b94baf326f26b12"/>
    <skos:prefLabel xml:lang="en">DimensionOne</skos:prefLabel>
  </rdf:Description>
  <rdf:Description rdf:about="http://emmo.info/emmo#EMMO_a8eb4bbb_1bd3_4ad4_b114_2789bcbd2134">
    <rdfs:subClassOf rdf:nodeID="f05bdaa1e617a4bccafc519daf7bf4785b120"/>
    <rdf:type rdf:resource="http://www.w3.org/2002/07/owl#Class"/>
    <rdfs:subClassOf rdf:nodeID="f05bdaa1e617a4bccafc519daf7bf4785b117"/>
    <skos:prefLabel xml:lang="en">Giga</skos:prefLabel>
  </rdf:Description>
  <rdf:Description rdf:about="http://emmo.info/emmo#EMMO_eb3c61f0_3983_4346_a0c6_e7f6b90a67a8">
    <EMMO_967080e5_2f42_4eb2_a3a9_c58143e835f9 xml:lang="en">The class of individuals that stand for gravitons elementary particles.</EMMO_967080e5_2f42_4eb2_a3a9_c58143e835f9>
    <rdfs:subClassOf rdf:resource="http://emmo.info/emmo#EMMO_0f795e3e_c602_4577_9a43_d5a231aa1360"/>
    <rdf:type rdf:resource="http://www.w3.org/2002/07/owl#Class"/>
    <skos:prefLabel xml:lang="en">Graviton</skos:prefLabel>
    <rdfs:comment xml:lang="en">While this particle is only supposed to exist, the EMMO approach to classical and quantum systems represents fields as made of particles.

For this reason graviton is an useful concept to homogenize the approach between different fields.</rdfs:comment>
  </rdf:Description>
  <rdf:Description rdf:nodeID="f8fb83657cd5f496db3c2b94baf326f26b39">
    <rdf:rest rdf:resource="http://www.w3.org/1999/02/22-rdf-syntax-ns#nil"/>
    <rdf:first rdf:resource="http://emmo.info/emmo#EMMO_a2f94f33_71fa_443c_a1fb_d1685fc537ec"/>
    <rdf:type rdf:resource="http://www.w3.org/1999/02/22-rdf-syntax-ns#List"/>
  </rdf:Description>
  <rdf:Description rdf:about="http://emmo.info/emmo#EMMO_9bed5d66_805a_4b3a_9153_beaf67143848">
    <rdfs:subClassOf rdf:resource="http://emmo.info/emmo#EMMO_a2b006f2_bbfd_4dba_bcaa_3fca20cd6be1"/>
    <rdf:type rdf:resource="http://www.w3.org/2002/07/owl#Class"/>
    <EMMO_967080e5_2f42_4eb2_a3a9_c58143e835f9 xml:lang="en">A foam of trapped gas in a solid.</EMMO_967080e5_2f42_4eb2_a3a9_c58143e835f9>
    <skos:prefLabel xml:lang="en">SolidFoam</skos:prefLabel>
    <rdfs:subClassOf rdf:resource="http://emmo.info/emmo#EMMO_1f5e3e7e_72c9_40d4_91dd_ae432d7b7018"/>
    <EMMO_b432d2d5_25f4_4165_99c5_5935a7763c1a xml:lang="en">Aerogel</EMMO_b432d2d5_25f4_4165_99c5_5935a7763c1a>
  </rdf:Description>
  <rdf:Description rdf:about="http://emmo.info/emmo#EMMO_50ea1ec5_f157_41b0_b46b_a9032f17ca10">
    <EMMO_967080e5_2f42_4eb2_a3a9_c58143e835f9 xml:lang="en">A physical made of more than one symbol sequentially arranged.</EMMO_967080e5_2f42_4eb2_a3a9_c58143e835f9>
    <rdfs:subClassOf rdf:nodeID="f38ecd0eaa78747b4ad569754ea441153b2"/>
    <rdfs:comment xml:lang="en">A string is not requested to respect any syntactic rule: it's simply directly made of symbols.</rdfs:comment>
    <rdf:type rdf:resource="http://www.w3.org/2002/07/owl#Class"/>
    <skos:prefLabel xml:lang="en">String</skos:prefLabel>
    <EMMO_b432d2d5_25f4_4165_99c5_5935a7763c1a xml:lang="en">The word "cat" considered as a collection of 'symbol'-s respecting the rules of english language. 

In this example the 'symbolic' entity "cat" is not related to the real cat, but it is only a word (like it would be to an italian person that ignores the meaning of this english word).

If an 'interpreter' skilled in english language is involved in a 'semiotic' process with this word, that "cat" became also a 'sign' i.e. it became for the 'interpreter' a representation for a real cat.</EMMO_b432d2d5_25f4_4165_99c5_5935a7763c1a>
    <rdfs:subClassOf rdf:nodeID="f38ecd0eaa78747b4ad569754ea441153b1"/>
    <rdfs:subClassOf rdf:resource="http://emmo.info/emmo#EMMO_89a0c87c_0804_4013_937a_6fe234d9499c"/>
    <rdfs:comment xml:lang="en">A string is made of concatenated symbols whose arrangement is one-dimensional. Each symbol can have only one previous and one next neighborhood (bidirectional list).</rdfs:comment>
  </rdf:Description>
  <rdf:Description rdf:about="http://emmo.info/emmo#EMMO_f84792eb_ec64_4a6b_941f_c9f3e9ef052c">
    <rdf:type rdf:resource="http://www.w3.org/2002/07/owl#Class"/>
    <rdfs:subClassOf rdf:resource="http://emmo.info/emmo#EMMO_9895a1b4_f0a5_4167_ac5e_97db40b8bfcc"/>
    <skos:prefLabel xml:lang="en">VelocityDimension</skos:prefLabel>
    <owl:equivalentClass rdf:nodeID="fe0b20157736f4a31909181349b2e6219b41"/>
  </rdf:Description>
  <rdf:Description rdf:nodeID="f05bdaa1e617a4bccafc519daf7bf4785b23">
    <owl:onProperty rdf:resource="http://emmo.info/emmo#EMMO_faf79f53_749d_40b2_807c_d34244c192f4"/>
    <rdf:type rdf:resource="http://www.w3.org/2002/07/owl#Restriction"/>
    <owl:hasValue rdf:datatype="http://www.w3.org/2001/XMLSchema#double">1e-15</owl:hasValue>
  </rdf:Description>
  <rdf:Description rdf:nodeID="ff14b31ebf90e4bc5ba2839064d29e543b18">
    <rdf:first rdf:resource="http://emmo.info/emmo#EMMO_df808271_df91_4f27_ba59_fa423c51896c"/>
    <rdf:type rdf:resource="http://www.w3.org/1999/02/22-rdf-syntax-ns#List"/>
    <rdf:rest rdf:resource="http://www.w3.org/1999/02/22-rdf-syntax-ns#nil"/>
  </rdf:Description>
  <rdf:Description rdf:about="http://emmo.info/emmo#EMMO_cabb20f0_05c7_448f_9485_e129725f15a4">
    <skos:prefLabel xml:lang="en">Minute</skos:prefLabel>
    <EMMO_6dd685dd_1895_46e4_b227_be9f7d643c25>http://dbpedia.org/page/Minute</EMMO_6dd685dd_1895_46e4_b227_be9f7d643c25>
    <EMMO_1f1b164d_ec6a_4faa_8d5e_88bda62316cc>http://qudt.org/vocab/unit/MIN</EMMO_1f1b164d_ec6a_4faa_8d5e_88bda62316cc>
    <rdfs:subClassOf rdf:nodeID="ffcb99037244f48d590430c228d02afdbb48"/>
    <rdfs:subClassOf rdf:resource="http://emmo.info/emmo#EMMO_591e02fd_8d37_45a6_9d11_bb21cef391a0"/>
    <rdfs:subClassOf rdf:nodeID="ffcb99037244f48d590430c228d02afdbb47"/>
    <rdf:type rdf:resource="http://www.w3.org/2002/07/owl#Class"/>
    <EMMO_70fe84ff_99b6_4206_a9fc_9a8931836d84 xml:lang="en">Non-SI time unit defined as 60 seconds.</EMMO_70fe84ff_99b6_4206_a9fc_9a8931836d84>
  </rdf:Description>
  <rdf:Description rdf:about="http://emmo.info/emmo#EMMO_d4f37e32_16ae_4cc6_b4cd_fd896b2449c4">
    <skos:prefLabel xml:lang="en">GasSolidSuspension</skos:prefLabel>
    <EMMO_967080e5_2f42_4eb2_a3a9_c58143e835f9 xml:lang="en">A coarse dispersion of solid in a gas continuum phase.</EMMO_967080e5_2f42_4eb2_a3a9_c58143e835f9>
    <rdf:type rdf:resource="http://www.w3.org/2002/07/owl#Class"/>
    <rdfs:subClassOf rdf:resource="http://emmo.info/emmo#EMMO_04f2a2d5_e799_4692_a654_420e76f5acc1"/>
    <EMMO_b432d2d5_25f4_4165_99c5_5935a7763c1a xml:lang="en">Dust, sand storm.</EMMO_b432d2d5_25f4_4165_99c5_5935a7763c1a>
  </rdf:Description>
  <rdf:Description rdf:about="http://emmo.info/emmo#EMMO_d7bf784a_db94_4dd9_861c_54f262846fbf">
    <rdfs:subClassOf rdf:resource="http://emmo.info/emmo#EMMO_9268958f_7f54_48ab_a693_febe2645892b"/>
    <rdf:type rdf:resource="http://www.w3.org/2002/07/owl#Class"/>
    <skos:prefLabel xml:lang="en">Sphere</skos:prefLabel>
  </rdf:Description>
  <rdf:Description rdf:nodeID="ff14b31ebf90e4bc5ba2839064d29e543b30">
    <owl:qualifiedCardinality rdf:datatype="http://www.w3.org/2001/XMLSchema#nonNegativeInteger">1</owl:qualifiedCardinality>
  </rdf:Description>
  <rdf:Description rdf:nodeID="fe24a777e3fd743f986ce83488d2cf30bb24">
    <owl:inverseOf rdf:resource="http://emmo.info/emmo#EMMO_3446e167_c576_49d6_846c_215bb8878a55"/>
  </rdf:Description>
  <rdf:Description rdf:nodeID="f05bdaa1e617a4bccafc519daf7bf4785b63">
    <rdf:type rdf:resource="http://www.w3.org/1999/02/22-rdf-syntax-ns#List"/>
    <rdf:rest rdf:nodeID="f05bdaa1e617a4bccafc519daf7bf4785b64"/>
    <rdf:first rdf:resource="http://emmo.info/emmo#EMMO_42955b2d_b465_4666_86cc_ea3c2d685753"/>
  </rdf:Description>
  <rdf:Description rdf:about="http://emmo.info/emmo#EMMO_54ee6b5e_5261_44a8_86eb_5717e7fdb9d0">
    <EMMO_967080e5_2f42_4eb2_a3a9_c58143e835f9 xml:lang="en">The class of general mathematical symbolic objects respecting mathematical syntactic rules.</EMMO_967080e5_2f42_4eb2_a3a9_c58143e835f9>
    <rdf:type rdf:resource="http://www.w3.org/2002/07/owl#Class"/>
    <skos:prefLabel xml:lang="en">Mathematical</skos:prefLabel>
    <rdfs:subClassOf rdf:resource="http://emmo.info/emmo#EMMO_d8d2144e_5c8d_455d_a643_5caf4d8d9df8"/>
  </rdf:Description>
  <rdf:Description rdf:nodeID="f05bdaa1e617a4bccafc519daf7bf4785b137">
    <rdf:type rdf:resource="http://www.w3.org/2002/07/owl#Restriction"/>
    <owl:onProperty rdf:resource="http://emmo.info/emmo#EMMO_bed1d005_b04e_4a90_94cf_02bc678a8569"/>
    <owl:someValuesFrom rdf:resource="http://emmo.info/emmo#EMMO_14ff4393_0f28_4fb4_abc7_c2cc00bc761d"/>
  </rdf:Description>
  <rdf:Description rdf:about="http://emmo.info/emmo#EMMO_5b2222df_4da6_442f_8244_96e9e45887d1">
    <rdfs:subClassOf rdf:nodeID="fea11ca01461e402d8f697c19c5d8de88b8"/>
    <skos:prefLabel xml:lang="en">Matter</skos:prefLabel>
    <rdf:type rdf:resource="http://www.w3.org/2002/07/owl#Class"/>
    <rdfs:subClassOf rdf:nodeID="fea11ca01461e402d8f697c19c5d8de88b9"/>
    <EMMO_967080e5_2f42_4eb2_a3a9_c58143e835f9 xml:lang="en">A 'Physical' that possesses some 'Massive' parts.</EMMO_967080e5_2f42_4eb2_a3a9_c58143e835f9>
    <rdfs:subClassOf rdf:resource="http://emmo.info/emmo#EMMO_c5ddfdba_c074_4aa4_ad6b_1ac4942d300d"/>
  </rdf:Description>
  <rdf:Description rdf:about="http://emmo.info/emmo#EMMO_054af807_85cd_4a13_8eba_119dfdaaf38b">
    <rdf:type rdf:resource="http://www.w3.org/2002/07/owl#Class"/>
    <rdfs:subClassOf rdf:resource="http://emmo.info/emmo#EMMO_b21a56ed_f969_4612_a6ec_cb7766f7f31d"/>
    <EMMO_967080e5_2f42_4eb2_a3a9_c58143e835f9 xml:lang="en">The interpreter's internal representation of the object in a semiosis process.</EMMO_967080e5_2f42_4eb2_a3a9_c58143e835f9>
    <skos:prefLabel xml:lang="en">Interpretant</skos:prefLabel>
  </rdf:Description>
  <rdf:Description rdf:about="http://emmo.info/emmo#EMMO_3995e22d_5720_4dcf_ba3b_d0ce03f514c6">
    <rdf:type rdf:resource="http://www.w3.org/2002/07/owl#Class"/>
    <skos:prefLabel xml:lang="en">Gel</skos:prefLabel>
    <rdfs:subClassOf rdf:resource="http://emmo.info/emmo#EMMO_a2b006f2_bbfd_4dba_bcaa_3fca20cd6be1"/>
    <EMMO_967080e5_2f42_4eb2_a3a9_c58143e835f9 xml:lang="en">A soft, solid or solid-like colloid consisting of two or more components, one of which is a liquid, present in substantial quantity.</EMMO_967080e5_2f42_4eb2_a3a9_c58143e835f9>
    <rdfs:subClassOf rdf:resource="http://emmo.info/emmo#EMMO_6c487fb3_03d1_4e56_91ed_c2e16dcbef60"/>
  </rdf:Description>
  <rdf:Description rdf:about="http://emmo.info/emmo#EMMO_0e6378df_1ce8_4321_b00c_ee9beea60a67">
    <rdf:type rdf:resource="http://www.w3.org/2002/07/owl#Class"/>
    <EMMO_967080e5_2f42_4eb2_a3a9_c58143e835f9 xml:lang="en">A single phase mixture.</EMMO_967080e5_2f42_4eb2_a3a9_c58143e835f9>
    <rdfs:subClassOf rdf:resource="http://emmo.info/emmo#EMMO_ec2c8ac8_98c5_4c74_b85b_ff8e8ca6655c"/>
    <skos:prefLabel xml:lang="en">PhaseHomogeneousMixture</skos:prefLabel>
  </rdf:Description>
  <rdf:Description rdf:about="http://emmo.info/emmo#EMMO_52211e5e_d767_4812_845e_eb6b402c476a">
    <rdfs:comment xml:lang="en">An 'Existent' individual stands for a real world object for which the ontologist wants to provide univocal tessellation in time.

By definition, the tiles are represented by 'State'-s individual.

Tiles are related to the 'Existent' through temporal direct parthood, enforcing non-transitivity and inverse-functionality.</rdfs:comment>
    <rdfs:comment xml:lang="en">ex-sistere (latin): to stay (to persist through time) outside others of the same type (to be distinct from the rest).</rdfs:comment>
    <rdfs:comment xml:lang="en">'Existent' is the EMMO class to be used for representing real world physical objects under a reductionistic perspective (i.e. objects come from the composition of sub-part objects, both in time and space). 

'Existent' class collects all individuals that stand for physical objects that can be structured in well defined temporal sub-parts called states, through the temporal direct parthood relation.

This class provides a first granularity hierarchy in time, and a way to axiomatize tessellation principles for a specific whole with a non-transitivity relation (direct parthood) that helps to retain the granularity levels.

e.g. a car, a supersaturated gas with nucleating nanoparticles, an atom that becomes ionized and then recombines with an electron.</rdfs:comment>
    <rdfs:comment xml:lang="en">Being hasTemporalDirectPart a proper parthood relation, there cannot be 'Existent' made of a single 'State'.

Moreover, due to inverse functionality, a 'State' can be part of only one 'Existent', preventing overlapping between 'Existent'-s.</rdfs:comment>
    <skos:prefLabel xml:lang="en">Existent</skos:prefLabel>
    <EMMO_967080e5_2f42_4eb2_a3a9_c58143e835f9 xml:lang="en">A 'Physical' which is a tessellation of 'State' temporal direct parts.</EMMO_967080e5_2f42_4eb2_a3a9_c58143e835f9>
    <rdf:type rdf:resource="http://www.w3.org/2002/07/owl#Class"/>
    <rdfs:subClassOf rdf:nodeID="f3b8e3e5cecf14b688acdf306cd5f62cbb5"/>
    <rdfs:subClassOf rdf:nodeID="f3b8e3e5cecf14b688acdf306cd5f62cbb6"/>
  </rdf:Description>
  <rdf:Description rdf:about="http://emmo.info/emmo#EMMO_31ec09ba_1713_42cb_83c7_b38bf6f9ced2">
    <EMMO_de178b12_5d35_4bca_8efa_a4193162571d>T-2 L+2 M+1 I0 Θ0 N0 J0</EMMO_de178b12_5d35_4bca_8efa_a4193162571d>
    <rdfs:subClassOf rdf:resource="http://emmo.info/emmo#EMMO_2946d40b_24a1_47fa_8176_e3f79bb45064"/>
    <skos:prefLabel xml:lang="en">Energy</skos:prefLabel>
    <EMMO_1f1b164d_ec6a_4faa_8d5e_88bda62316cc>http://qudt.org/vocab/quantitykind/Energy</EMMO_1f1b164d_ec6a_4faa_8d5e_88bda62316cc>
    <EMMO_6dd685dd_1895_46e4_b227_be9f7d643c25>http://dbpedia.org/page/Energy</EMMO_6dd685dd_1895_46e4_b227_be9f7d643c25>
    <rdf:type rdf:resource="http://www.w3.org/2002/07/owl#Class"/>
    <EMMO_fe015383_afb3_44a6_ae86_043628697aa2>https://doi.org/10.1351/goldbook.E02101</EMMO_fe015383_afb3_44a6_ae86_043628697aa2>
    <rdfs:comment xml:lang="en">Energy is often defined as "ability of a system to perform work", but it might be misleading since is not necessarily available to do work.</rdfs:comment>
    <EMMO_967080e5_2f42_4eb2_a3a9_c58143e835f9 xml:lang="en">A property of objects which can be transferred to other objects or converted into different forms.</EMMO_967080e5_2f42_4eb2_a3a9_c58143e835f9>
  </rdf:Description>
  <rdf:Description rdf:nodeID="fe24a777e3fd743f986ce83488d2cf30bb16">
    <owl:allValuesFrom rdf:nodeID="fe24a777e3fd743f986ce83488d2cf30bb17"/>
    <rdf:type rdf:resource="http://www.w3.org/2002/07/owl#Restriction"/>
    <owl:onProperty rdf:resource="http://emmo.info/emmo#EMMO_9380ab64_0363_4804_b13f_3a8a94119a76"/>
  </rdf:Description>
  <rdf:Description rdf:nodeID="f0b819106611c4b798f33b16c65f4398db1">
    <rdf:type rdf:resource="http://www.w3.org/2002/07/owl#Class"/>
    <owl:unionOf rdf:nodeID="f0b819106611c4b798f33b16c65f4398db2"/>
  </rdf:Description>
  <rdf:Description rdf:about="http://emmo.info/emmo#EMMO_18d180e4_5e3e_42f7_820c_e08951223486">
    <skos:prefLabel xml:lang="en">Real</skos:prefLabel>
    <rdfs:subClassOf rdf:resource="http://emmo.info/emmo#EMMO_21f56795_ee72_4858_b571_11cfaa59c1a8"/>
    <rdf:type rdf:resource="http://www.w3.org/2002/07/owl#Class"/>
    <rdfs:subClassOf rdf:nodeID="fe24a777e3fd743f986ce83488d2cf30bb3"/>
    <rdfs:subClassOf rdf:nodeID="fe24a777e3fd743f986ce83488d2cf30bb4"/>
    <owl:equivalentClass rdf:nodeID="fe24a777e3fd743f986ce83488d2cf30bb2"/>
  </rdf:Description>
  <rdf:Description rdf:about="http://emmo.info/emmo/middle/isq">
    <dcterms:creator>Jesper Friis</dcterms:creator>
    <rdf:type rdf:resource="http://www.w3.org/2002/07/owl#Ontology"/>
    <dcterms:publisher>EMMC ASBL</dcterms:publisher>
    <owl:versionIRI rdf:resource="http://emmo.info/emmo/1.0.0-beta/middle/isq"/>
    <dcterms:contributor>Access, DE</dcterms:contributor>
    <dcterms:contributor>Goldbeck Consulting Ltd (UK)</dcterms:contributor>
    <dcterms:contributor>SINTEF, NO</dcterms:contributor>
    <dcterms:abstract xml:lang="en">European Materials &amp; Modelling Ontology (EMMO)

EMMO is a multidisciplinary effort to develop a standard representational framework (the ontology) based on current materials modelling knowledge, including physical sciences, analytical philosophy and information and communication technologies.

It provides the connection between the physical world, materials characterisation world and materials modelling world.

EMMO is released under a Creative Commons license Attribution 4.0 International (CC BY 4.0).</dcterms:abstract>
    <dcterms:contributor>University of Bologna, IT</dcterms:contributor>
    <dcterms:creator>Adham Hashibon</dcterms:creator>
    <owl:versionInfo>1.0.0-beta</owl:versionInfo>
    <dcterms:creator>Emanuele Ghedini</dcterms:creator>
    <dcterms:creator>Georg Schmitz</dcterms:creator>
    <rdfs:comment xml:lang="en">Contacts:
Gerhard Goldbeck
Goldbeck Consulting Ltd (UK)
email: gerhard@goldbeck-consulting.com

Emanuele Ghedini
University of Bologna (IT)
email: emanuele.ghedini@unibo.it</rdfs:comment>
    <dcterms:contributor>Fraunhofer IWM, DE</dcterms:contributor>
    <dcterms:creator>Gerhard Goldbeck</dcterms:creator>
    <dcterms:title xml:lang="en">European Materials &amp; Modelling Ontology</dcterms:title>
    <dcterms:license>https://creativecommons.org/licenses/by/4.0/legalcode</dcterms:license>
    <rdfs:comment xml:lang="en">The EMMO requires FacT++ reasoner plugin in order to visualize all inferences and class hierarchy (ctrl+R hotkey in Protege).</rdfs:comment>
  </rdf:Description>
  <rdf:Description rdf:nodeID="ffcb99037244f48d590430c228d02afdbb34">
    <rdf:type rdf:resource="http://www.w3.org/2002/07/owl#Restriction"/>
    <owl:onProperty rdf:resource="http://emmo.info/emmo#EMMO_23b579e1_8088_45b5_9975_064014026c42"/>
    <owl:hasValue>B</owl:hasValue>
  </rdf:Description>
  <rdf:Description rdf:about="http://emmo.info/emmo#EMMO_830b59f7_d047_438c_90cd_62845749efcb">
    <EMMO_e55f2d7c_9893_48cd_b4a4_fdf38253bd20>http://www.ontology-of-units-of-measure.org/resource/om-2/InternalEnergy</EMMO_e55f2d7c_9893_48cd_b4a4_fdf38253bd20>
    <EMMO_fe015383_afb3_44a6_ae86_043628697aa2>https://doi.org/10.1351/goldbook.I03103</EMMO_fe015383_afb3_44a6_ae86_043628697aa2>
    <EMMO_1f1b164d_ec6a_4faa_8d5e_88bda62316cc>http://qudt.org/vocab/quantitykind/InternalEnergy</EMMO_1f1b164d_ec6a_4faa_8d5e_88bda62316cc>
    <skos:altLabel xml:lang="en">ThermodynamicEnergy</skos:altLabel>
    <EMMO_de178b12_5d35_4bca_8efa_a4193162571d>T-2 L+2 M+1 I0 Θ0 N0 J0</EMMO_de178b12_5d35_4bca_8efa_a4193162571d>
    <rdf:type rdf:resource="http://www.w3.org/2002/07/owl#Class"/>
    <EMMO_50c298c2_55a2_4068_b3ac_4e948c33181f>http://www.electropedia.org/iev/iev.nsf/display?openform&amp;ievref=113-04-20</EMMO_50c298c2_55a2_4068_b3ac_4e948c33181f>
    <EMMO_967080e5_2f42_4eb2_a3a9_c58143e835f9 xml:lang="en">A state quantity equal to the difference between the total energy of a system and the sum of the macroscopic kinetic and potential energies of the system.</EMMO_967080e5_2f42_4eb2_a3a9_c58143e835f9>
    <skos:prefLabel xml:lang="en">InternalEnergy</skos:prefLabel>
    <EMMO_6dd685dd_1895_46e4_b227_be9f7d643c25>http://dbpedia.org/page/Internal_energy</EMMO_6dd685dd_1895_46e4_b227_be9f7d643c25>
    <rdfs:subClassOf rdf:resource="http://emmo.info/emmo#EMMO_31ec09ba_1713_42cb_83c7_b38bf6f9ced2"/>
  </rdf:Description>
  <rdf:Description rdf:about="http://emmo.info/emmo#EMMO_e7c9f7fd_e534_4441_88fe_1fec6cb20f26">
    <EMMO_fe015383_afb3_44a6_ae86_043628697aa2>https://doi.org/10.1351/goldbook.S05732</EMMO_fe015383_afb3_44a6_ae86_043628697aa2>
    <EMMO_6dd685dd_1895_46e4_b227_be9f7d643c25>http://dbpedia.org/page/Solid_angle</EMMO_6dd685dd_1895_46e4_b227_be9f7d643c25>
    <skos:prefLabel xml:lang="en">SolidAngle</skos:prefLabel>
    <EMMO_967080e5_2f42_4eb2_a3a9_c58143e835f9 xml:lang="en">Ratio of area on a sphere to its radius squared.</EMMO_967080e5_2f42_4eb2_a3a9_c58143e835f9>
    <EMMO_1f1b164d_ec6a_4faa_8d5e_88bda62316cc>http://qudt.org/vocab/quantitykind/SolidAngle</EMMO_1f1b164d_ec6a_4faa_8d5e_88bda62316cc>
    <rdfs:subClassOf rdf:resource="http://emmo.info/emmo#EMMO_faab3f84_e475_4a46_af9c_7d249f0b9aef"/>
    <rdf:type rdf:resource="http://www.w3.org/2002/07/owl#Class"/>
    <rdfs:subClassOf rdf:nodeID="ffcb99037244f48d590430c228d02afdbb53"/>
    <EMMO_de178b12_5d35_4bca_8efa_a4193162571d>T0 L0 M0 I0 Θ0 N0 J0</EMMO_de178b12_5d35_4bca_8efa_a4193162571d>
  </rdf:Description>
  <rdf:Description rdf:about="http://emmo.info/emmo#EMMO_acf636d4_9ac2_4ce3_960a_d54338e6cae3">
    <rdfs:subClassOf rdf:nodeID="ffcb99037244f48d590430c228d02afdbb40"/>
    <EMMO_de178b12_5d35_4bca_8efa_a4193162571d>T0 L0 M0 I0 Θ0 N0 J0</EMMO_de178b12_5d35_4bca_8efa_a4193162571d>
    <EMMO_50c298c2_55a2_4068_b3ac_4e948c33181f>http://www.electropedia.org/iev/iev.nsf/display?openform&amp;ievref=113-03-57</EMMO_50c298c2_55a2_4068_b3ac_4e948c33181f>
    <rdf:type rdf:resource="http://www.w3.org/2002/07/owl#Class"/>
    <EMMO_1f1b164d_ec6a_4faa_8d5e_88bda62316cc>http://qudt.org/vocab/quantitykind/Strain</EMMO_1f1b164d_ec6a_4faa_8d5e_88bda62316cc>
    <skos:prefLabel xml:lang="en">Strain</skos:prefLabel>
    <EMMO_967080e5_2f42_4eb2_a3a9_c58143e835f9 xml:lang="en">Change of the relative positions of parts of a body, excluding a displacement of the body as a whole.</EMMO_967080e5_2f42_4eb2_a3a9_c58143e835f9>
    <rdfs:subClassOf rdf:resource="http://emmo.info/emmo#EMMO_faab3f84_e475_4a46_af9c_7d249f0b9aef"/>
    <EMMO_e55f2d7c_9893_48cd_b4a4_fdf38253bd20>http://www.ontology-of-units-of-measure.org/resource/om-2/Strain</EMMO_e55f2d7c_9893_48cd_b4a4_fdf38253bd20>
  </rdf:Description>
  <rdf:Description rdf:about="http://emmo.info/emmo#EMMO_d0200cf1_e4f4_45ae_873f_b9359daea3cd">
    <rdf:type rdf:resource="http://www.w3.org/2002/07/owl#Class"/>
    <skos:prefLabel xml:lang="en">ModelledQuantitativeProperty</skos:prefLabel>
  </rdf:Description>
  <rdf:Description rdf:about="http://emmo.info/emmo#EMMO_b953f2b1_c8d1_4dd9_b630_d3ef6580c2bb">
    <rdfs:subClassOf rdf:resource="http://emmo.info/emmo#EMMO_02c0621e_a527_4790_8a0f_2bb51973c819"/>
    <rdf:type rdf:resource="http://www.w3.org/2002/07/owl#Class"/>
    <skos:prefLabel xml:lang="en">PhysicalConstant</skos:prefLabel>
    <EMMO_c84c6752_6d64_48cc_9500_e54a3c34898d>https://en.wikipedia.org/wiki/List_of_physical_constants</EMMO_c84c6752_6d64_48cc_9500_e54a3c34898d>
    <owl:disjointUnionOf rdf:nodeID="f8fb83657cd5f496db3c2b94baf326f26b30"/>
    <rdfs:comment xml:lang="en">Physical constants are categorised into "exact" and measured constants. 

With "exact" constants, we refer to physical constants that have an exact numerical value after the revision of the SI system that was enforsed May 2019.</rdfs:comment>
  </rdf:Description>
  <rdf:Description rdf:about="http://emmo.info/emmo#EMMO_0ef4ff4a_5458_4f2a_b51f_4689d472a3f2">
    <skos:prefLabel xml:lang="en">Curve</skos:prefLabel>
    <rdf:type rdf:resource="http://www.w3.org/2002/07/owl#Class"/>
    <rdfs:subClassOf rdf:resource="http://emmo.info/emmo#EMMO_0c576e13_4ee7_4f3d_bfe9_1614243df018"/>
  </rdf:Description>
  <rdf:Description rdf:nodeID="ffcb99037244f48d590430c228d02afdbb57">
    <rdf:type rdf:resource="http://www.w3.org/2002/07/owl#Restriction"/>
    <owl:hasValue>t</owl:hasValue>
    <owl:onProperty rdf:resource="http://emmo.info/emmo#EMMO_23b579e1_8088_45b5_9975_064014026c42"/>
  </rdf:Description>
  <rdf:Description rdf:nodeID="fea11ca01461e402d8f697c19c5d8de88b2">
    <rdf:first rdf:resource="http://emmo.info/emmo#EMMO_72d53756_7fb1_46ed_980f_83f47efbe105"/>
    <rdf:type rdf:resource="http://www.w3.org/1999/02/22-rdf-syntax-ns#List"/>
    <rdf:rest rdf:nodeID="fea11ca01461e402d8f697c19c5d8de88b3"/>
  </rdf:Description>
  <rdf:Description rdf:nodeID="ffcb99037244f48d590430c228d02afdbb11">
    <owl:onProperty rdf:resource="http://emmo.info/emmo#EMMO_bed1d005_b04e_4a90_94cf_02bc678a8569"/>
    <owl:someValuesFrom rdf:resource="http://emmo.info/emmo#EMMO_b3600e73_3e05_479d_9714_c041c3acf5cc"/>
    <rdf:type rdf:resource="http://www.w3.org/2002/07/owl#Restriction"/>
  </rdf:Description>
  <rdf:Description rdf:nodeID="f05bdaa1e617a4bccafc519daf7bf4785b80">
    <owl:hasValue rdf:datatype="http://www.w3.org/2001/XMLSchema#double">1e+18</owl:hasValue>
    <owl:onProperty rdf:resource="http://emmo.info/emmo#EMMO_faf79f53_749d_40b2_807c_d34244c192f4"/>
    <rdf:type rdf:resource="http://www.w3.org/2002/07/owl#Restriction"/>
  </rdf:Description>
  <rdf:Description rdf:nodeID="fea11ca01461e402d8f697c19c5d8de88b9">
    <owl:onProperty rdf:resource="http://emmo.info/emmo#EMMO_7afbed84_7593_4a23_bd88_9d9c6b04e8f6"/>
    <rdf:type rdf:resource="http://www.w3.org/2002/07/owl#Restriction"/>
    <owl:allValuesFrom rdf:resource="http://emmo.info/emmo#EMMO_5b2222df_4da6_442f_8244_96e9e45887d1"/>
  </rdf:Description>
  <rdf:Description rdf:about="http://emmo.info/emmo#EMMO_9268958f_7f54_48ab_a693_febe2645892b">
    <skos:prefLabel xml:lang="en">2-manifold</skos:prefLabel>
    <rdf:type rdf:resource="http://www.w3.org/2002/07/owl#Class"/>
    <rdfs:subClassOf rdf:resource="http://emmo.info/emmo#EMMO_b5957cef_a287_442d_a3ce_fd39f20ba1cd"/>
  </rdf:Description>
  <rdf:Description rdf:nodeID="fe24a777e3fd743f986ce83488d2cf30bb27">
    <rdf:type rdf:resource="http://www.w3.org/2002/07/owl#Restriction"/>
    <owl:someValuesFrom rdf:resource="http://www.w3.org/2001/XMLSchema#integer"/>
    <owl:onProperty rdf:resource="http://emmo.info/emmo#EMMO_faf79f53_749d_40b2_807c_d34244c192f4"/>
  </rdf:Description>
  <rdf:Description rdf:nodeID="f8fb83657cd5f496db3c2b94baf326f26b28">
    <rdf:first rdf:resource="http://emmo.info/emmo#EMMO_868ae137_4d25_493e_b270_21ea3d94849e"/>
    <rdf:rest rdf:nodeID="f8fb83657cd5f496db3c2b94baf326f26b29"/>
    <rdf:type rdf:resource="http://www.w3.org/1999/02/22-rdf-syntax-ns#List"/>
  </rdf:Description>
  <rdf:Description rdf:about="http://emmo.info/emmo#EMMO_8b0923ab_b500_477b_9ce9_8b3a3e4dc4f2">
    <rdfs:comment xml:lang="en">A continuum is made of a sufficient number of parts that it continues to exists as continuum individual even after the loss of one of them i.e. a continuum is a redundant.</rdfs:comment>
    <skos:prefLabel xml:lang="en">Continuum</skos:prefLabel>
    <rdfs:comment xml:lang="en">A continuum is the bearer of properties that are generated by the interactions of parts such as viscosity and thermal or electrical conductivity.</rdfs:comment>
    <rdfs:comment xml:lang="en">A continuum is not necessarily small (i.e. composed by the minimum amount of sates to fulfill the definition).

A single continuum individual can be the whole fluid in a pipe.</rdfs:comment>
    <rdfs:subClassOf rdf:resource="http://emmo.info/emmo#EMMO_5b2222df_4da6_442f_8244_96e9e45887d1"/>
    <rdf:type rdf:resource="http://www.w3.org/2002/07/owl#Class"/>
    <EMMO_967080e5_2f42_4eb2_a3a9_c58143e835f9 xml:lang="en">A state that is a collection of sufficiently large number of other parts such that:
- it is the bearer of qualities that can exists only by the fact that it is a sum of parts
- the smallest partition dV of the state volume in which we are interested in, contains enough parts to be statistically consistent: n [#/m3] x dV [m3] &gt;&gt; 1</EMMO_967080e5_2f42_4eb2_a3a9_c58143e835f9>
  </rdf:Description>
  <rdf:Description rdf:about="http://emmo.info/emmo#EMMO_a3a701ed_6f7d_4a10_9aee_dfa1961fc7b7">
    <rdfs:subClassOf rdf:nodeID="f05bdaa1e617a4bccafc519daf7bf4785b111"/>
    <rdf:type rdf:resource="http://www.w3.org/2002/07/owl#Class"/>
    <skos:prefLabel xml:lang="en">Milli</skos:prefLabel>
    <rdfs:subClassOf rdf:nodeID="f05bdaa1e617a4bccafc519daf7bf4785b114"/>
  </rdf:Description>
  <rdf:Description rdf:about="http://emmo.info/emmo#EMMO_88fc5d1b_d3ab_4626_b24c_915ebe7400ca">
    <skos:prefLabel xml:lang="en">ChemicalPotential</skos:prefLabel>
    <EMMO_1f1b164d_ec6a_4faa_8d5e_88bda62316cc>http://qudt.org/vocab/quantitykind/ChemicalPotential</EMMO_1f1b164d_ec6a_4faa_8d5e_88bda62316cc>
    <EMMO_6dd685dd_1895_46e4_b227_be9f7d643c25>http://dbpedia.org/page/Chemical_potential</EMMO_6dd685dd_1895_46e4_b227_be9f7d643c25>
    <rdfs:subClassOf rdf:resource="http://emmo.info/emmo#EMMO_2946d40b_24a1_47fa_8176_e3f79bb45064"/>
    <EMMO_fe015383_afb3_44a6_ae86_043628697aa2>https://doi.org/10.1351/goldbook.C01032</EMMO_fe015383_afb3_44a6_ae86_043628697aa2>
    <rdfs:comment xml:lang="en">Energy per unit change in amount of substance.</rdfs:comment>
    <EMMO_de178b12_5d35_4bca_8efa_a4193162571d>T-2 L+2 M+1 I0 Θ0 N-1 J0</EMMO_de178b12_5d35_4bca_8efa_a4193162571d>
    <rdf:type rdf:resource="http://www.w3.org/2002/07/owl#Class"/>
  </rdf:Description>
  <rdf:Description rdf:about="http://emmo.info/emmo#EMMO_c46f091c_0420_4c1a_af30_0a2c8ebcf7d7">
    <rdfs:comment xml:lang="en">"Ordinal quantities, such as Rockwell C hardness, are usually not considered to be part of a system of quantities because they are related to other quantities through empirical relations only."
International vocabulary of metrology (VIM)</rdfs:comment>
    <rdf:type rdf:resource="http://www.w3.org/2002/07/owl#Class"/>
    <skos:prefLabel xml:lang="en">OrdinalQuantity</skos:prefLabel>
    <EMMO_967080e5_2f42_4eb2_a3a9_c58143e835f9 xml:lang="en">"Quantity, defined by a conventional measurement procedure, for which a total ordering relation can be established, according to magnitude, with other quantities of the same kind, but for which no algebraic operations among those quantities exist"
International vocabulary of metrology (VIM)</EMMO_967080e5_2f42_4eb2_a3a9_c58143e835f9>
    <EMMO_b432d2d5_25f4_4165_99c5_5935a7763c1a xml:lang="en">Hardness
Resilience</EMMO_b432d2d5_25f4_4165_99c5_5935a7763c1a>
  </rdf:Description>
  <rdf:Description rdf:about="http://emmo.info/emmo#EMMO_847f1d9f_205e_46c1_8cb6_a9e479421f88">
    <rdf:type rdf:resource="http://www.w3.org/2002/07/owl#Class"/>
    <owl:equivalentClass rdf:nodeID="fe0b20157736f4a31909181349b2e6219b26"/>
    <rdfs:subClassOf rdf:resource="http://emmo.info/emmo#EMMO_9895a1b4_f0a5_4167_ac5e_97db40b8bfcc"/>
    <skos:prefLabel xml:lang="en">AbsorbedDoseDimension</skos:prefLabel>
  </rdf:Description>
  <rdf:Description rdf:nodeID="f8fb83657cd5f496db3c2b94baf326f26b22">
    <rdf:type rdf:resource="http://www.w3.org/1999/02/22-rdf-syntax-ns#List"/>
    <rdf:first rdf:resource="http://emmo.info/emmo#EMMO_08b308d4_31cd_4779_a784_aa92fc730f39"/>
    <rdf:rest rdf:nodeID="f8fb83657cd5f496db3c2b94baf326f26b23"/>
  </rdf:Description>
  <rdf:Description rdf:about="http://emmo.info/emmo#EMMO_a9b3d04c_7ceb_40a2_b8d3_28d514a770a8">
    <rdfs:range rdf:resource="http://www.w3.org/2001/XMLSchema#anyURI"/>
    <rdfs:subPropertyOf rdf:resource="http://www.w3.org/2000/01/rdf-schema#seeAlso"/>
    <skos:prefLabel xml:lang="en">codataEntry</skos:prefLabel>
    <rdfs:seeAlso rdf:datatype="http://www.w3.org/2001/XMLSchema#anyURI">https://physics.nist.gov/cuu/Constants/index.html</rdfs:seeAlso>
    <rdf:type rdf:resource="http://www.w3.org/2002/07/owl#AnnotationProperty"/>
    <rdfs:comment xml:lang="en">URL to CODATA Internationally recommended 2018 values of physical constants.</rdfs:comment>
  </rdf:Description>
  <rdf:Description rdf:nodeID="f05bdaa1e617a4bccafc519daf7bf4785b192">
    <owl:hasValue>y</owl:hasValue>
    <rdf:type rdf:resource="http://www.w3.org/2002/07/owl#Restriction"/>
    <owl:onProperty rdf:resource="http://emmo.info/emmo#EMMO_23b579e1_8088_45b5_9975_064014026c42"/>
  </rdf:Description>
  <rdf:Description rdf:about="http://emmo.info/emmo#EMMO_2946d40b_24a1_47fa_8176_e3f79bb45064">
    <rdfs:subClassOf rdf:resource="http://emmo.info/emmo#EMMO_71f6ab56_342c_484b_bbe0_de86b7367cb3"/>
    <EMMO_967080e5_2f42_4eb2_a3a9_c58143e835f9 xml:lang="en">Derived quantities defined in the International System of Quantities (ISQ).</EMMO_967080e5_2f42_4eb2_a3a9_c58143e835f9>
    <rdfs:subClassOf rdf:resource="http://emmo.info/emmo#EMMO_f35cff4d_dc09_44cf_a729_22fb79e3bfb2"/>
    <rdf:type rdf:resource="http://www.w3.org/2002/07/owl#Class"/>
    <skos:prefLabel xml:lang="en">ISQDerivedQuantity</skos:prefLabel>
  </rdf:Description>
  <rdf:Description rdf:nodeID="f05bdaa1e617a4bccafc519daf7bf4785b199">
    <rdf:type rdf:resource="http://www.w3.org/1999/02/22-rdf-syntax-ns#List"/>
    <rdf:first rdf:resource="http://emmo.info/emmo#EMMO_e9ffc696_5228_4ff9_8a60_0f5e05e9931b"/>
    <rdf:rest rdf:resource="http://www.w3.org/1999/02/22-rdf-syntax-ns#nil"/>
  </rdf:Description>
  <rdf:Description rdf:nodeID="f05bdaa1e617a4bccafc519daf7bf4785b93">
    <rdf:type rdf:resource="http://www.w3.org/2002/07/owl#Restriction"/>
    <owl:onProperty rdf:resource="http://emmo.info/emmo#EMMO_faf79f53_749d_40b2_807c_d34244c192f4"/>
    <owl:hasValue rdf:datatype="http://www.w3.org/2001/XMLSchema#double">1000.0</owl:hasValue>
  </rdf:Description>
  <rdf:Description rdf:nodeID="ffcb99037244f48d590430c228d02afdbb50">
    <owl:hasValue>ha</owl:hasValue>
    <rdf:type rdf:resource="http://www.w3.org/2002/07/owl#Restriction"/>
    <owl:onProperty rdf:resource="http://emmo.info/emmo#EMMO_23b579e1_8088_45b5_9975_064014026c42"/>
  </rdf:Description>
  <rdf:Description rdf:about="http://emmo.info/emmo#EMMO_87ac88ff_8379_4f5a_8c7b_424a8fff1ee8">
    <rdf:type rdf:resource="http://www.w3.org/2002/07/owl#Class"/>
    <EMMO_967080e5_2f42_4eb2_a3a9_c58143e835f9 xml:lang="en">A continuum that has no fixed shape and yields easily to external pressure.</EMMO_967080e5_2f42_4eb2_a3a9_c58143e835f9>
    <rdfs:subClassOf rdf:resource="http://emmo.info/emmo#EMMO_8b0923ab_b500_477b_9ce9_8b3a3e4dc4f2"/>
    <skos:prefLabel xml:lang="en">Fluid</skos:prefLabel>
    <EMMO_b432d2d5_25f4_4165_99c5_5935a7763c1a xml:lang="en">Gas, liquid, plasma,</EMMO_b432d2d5_25f4_4165_99c5_5935a7763c1a>
  </rdf:Description>
  <rdf:Description rdf:nodeID="ffbe75b10062f400ea693809785c50a44b7">
    <owl:inverseOf rdf:resource="http://emmo.info/emmo#EMMO_c5aae418_1622_4d02_93c5_21159e28e6c1"/>
  </rdf:Description>
  <rdf:Description rdf:nodeID="f05bdaa1e617a4bccafc519daf7bf4785b97">
    <rdf:rest rdf:nodeID="f05bdaa1e617a4bccafc519daf7bf4785b98"/>
    <rdf:first rdf:resource="http://emmo.info/emmo#EMMO_60b78cc3_6011_4134_95ab_956f56d4bdc1"/>
    <rdf:type rdf:resource="http://www.w3.org/1999/02/22-rdf-syntax-ns#List"/>
  </rdf:Description>
  <rdf:Description rdf:nodeID="f05bdaa1e617a4bccafc519daf7bf4785b41">
    <rdf:first rdf:resource="http://emmo.info/emmo#EMMO_9bfd6f1e_b0ce_459c_beb7_8f1f41708bba"/>
    <rdf:rest rdf:nodeID="f05bdaa1e617a4bccafc519daf7bf4785b42"/>
    <rdf:type rdf:resource="http://www.w3.org/1999/02/22-rdf-syntax-ns#List"/>
  </rdf:Description>
  <rdf:Description rdf:nodeID="ffcb99037244f48d590430c228d02afdbb56">
    <owl:someValuesFrom rdf:resource="http://emmo.info/emmo#EMMO_77e9dc31_5b19_463e_b000_44c6e79f98aa"/>
    <owl:onProperty rdf:resource="http://emmo.info/emmo#EMMO_bed1d005_b04e_4a90_94cf_02bc678a8569"/>
    <rdf:type rdf:resource="http://www.w3.org/2002/07/owl#Restriction"/>
  </rdf:Description>
  <rdf:Description rdf:about="http://emmo.info/emmo#EMMO_b55cd09a_e54d_4eb1_81dd_03c29d1b878e">
    <rdf:type rdf:resource="http://www.w3.org/2002/07/owl#Class"/>
    <rdfs:subClassOf rdf:nodeID="f05bdaa1e617a4bccafc519daf7bf4785b132"/>
    <rdfs:subClassOf rdf:nodeID="f05bdaa1e617a4bccafc519daf7bf4785b129"/>
    <skos:prefLabel xml:lang="en">Centi</skos:prefLabel>
  </rdf:Description>
  <rdf:Description rdf:nodeID="fc2fcd8f8eb3649bcbbaff76ba54058acb7">
    <rdf:rest rdf:resource="http://www.w3.org/1999/02/22-rdf-syntax-ns#nil"/>
    <rdf:first rdf:resource="http://emmo.info/emmo#EMMO_c5ddfdba_c074_4aa4_ad6b_1ac4942d300d"/>
    <rdf:type rdf:resource="http://www.w3.org/1999/02/22-rdf-syntax-ns#List"/>
  </rdf:Description>
  <rdf:Description rdf:about="http://emmo.info/emmo#EMMO_b432d2d5_25f4_4165_99c5_5935a7763c1a">
    <skos:prefLabel xml:lang="en">example</skos:prefLabel>
    <rdfs:comment xml:lang="en">Illustrative example of how the entity is used.</rdfs:comment>
    <rdfs:subPropertyOf rdf:resource="http://www.w3.org/2000/01/rdf-schema#comment"/>
    <rdf:type rdf:resource="http://www.w3.org/2002/07/owl#AnnotationProperty"/>
    <rdfs:range rdf:resource="http://www.w3.org/2001/XMLSchema#string"/>
  </rdf:Description>
  <rdf:Description rdf:about="http://emmo.info/emmo#EMMO_61a32ae9_8200_473a_bd55_59a9899996f4">
    <rdf:type rdf:resource="http://www.w3.org/2002/07/owl#Class"/>
    <rdfs:subClassOf rdf:resource="http://emmo.info/emmo#EMMO_0ee5779e_d798_4ee5_9bfe_c392d5bea112"/>
    <EMMO_1f1b164d_ec6a_4faa_8d5e_88bda62316cc>http://qudt.org/vocab/constant/PermittivityOfVacuum</EMMO_1f1b164d_ec6a_4faa_8d5e_88bda62316cc>
    <EMMO_fe015383_afb3_44a6_ae86_043628697aa2>https://doi.org/10.1351/goldbook.P04508</EMMO_fe015383_afb3_44a6_ae86_043628697aa2>
    <rdfs:subClassOf rdf:resource="http://emmo.info/emmo#EMMO_3f15d200_c97b_42c8_8ac0_d81d150361e2"/>
    <rdfs:comment xml:lang="en">The DBpedia definition (http://dbpedia.org/page/Vacuum_permittivity) is outdated since May 20, 2019. It is now a measured constant.</rdfs:comment>
    <EMMO_a9b3d04c_7ceb_40a2_b8d3_28d514a770a8>https://physics.nist.gov/cgi-bin/cuu/Value?ep0</EMMO_a9b3d04c_7ceb_40a2_b8d3_28d514a770a8>
    <rdfs:comment xml:lang="en">The value of the absolute dielectric permittivity of classical vacuum.</rdfs:comment>
    <skos:prefLabel xml:lang="en">VacuumElectricPermittivity</skos:prefLabel>
    <EMMO_de178b12_5d35_4bca_8efa_a4193162571d>T+4 L-3 M-1 I+2 Θ0 N0 J0</EMMO_de178b12_5d35_4bca_8efa_a4193162571d>
  </rdf:Description>
  <rdf:Description rdf:nodeID="ffcb99037244f48d590430c228d02afdbb1">
    <owl:someValuesFrom rdf:resource="http://emmo.info/emmo#EMMO_77e9dc31_5b19_463e_b000_44c6e79f98aa"/>
    <owl:onProperty rdf:resource="http://emmo.info/emmo#EMMO_bed1d005_b04e_4a90_94cf_02bc678a8569"/>
    <rdf:type rdf:resource="http://www.w3.org/2002/07/owl#Restriction"/>
  </rdf:Description>
  <rdf:Description rdf:about="http://emmo.info/emmo#EMMO_0329f1f5_8339_4ce4_8505_a264c6d606ba">
    <rdfs:subClassOf rdf:resource="http://emmo.info/emmo#EMMO_81369540_1b0e_471b_9bae_6801af22800e"/>
    <rdfs:comment xml:lang="en">The velocity is related to a point described by its position vector. The point may localize a particle, or be attached to any other object such as a body or a wave.

-- IEC, note 1</rdfs:comment>
    <EMMO_de178b12_5d35_4bca_8efa_a4193162571d>T-1 L+1 M0 I0 Θ0 N0 J0</EMMO_de178b12_5d35_4bca_8efa_a4193162571d>
    <EMMO_50c298c2_55a2_4068_b3ac_4e948c33181f>http://www.electropedia.org/iev/iev.nsf/display?openform&amp;ievref=113-01-32</EMMO_50c298c2_55a2_4068_b3ac_4e948c33181f>
    <EMMO_70fe84ff_99b6_4206_a9fc_9a8931836d84 xml:lang="en">Vector quantity giving the rate of change of a position vector.

-- ISO 80000-3</EMMO_70fe84ff_99b6_4206_a9fc_9a8931836d84>
    <EMMO_1f1b164d_ec6a_4faa_8d5e_88bda62316cc>http://qudt.org/vocab/quantitykind/Velocity</EMMO_1f1b164d_ec6a_4faa_8d5e_88bda62316cc>
    <rdfs:comment xml:lang="en">The velocity depends on the choice of the reference frame. Proper transformation between frames must be used: Galilean for non-relativistic description, Lorentzian for relativistic description.

-- IEC, note 2</rdfs:comment>
    <EMMO_8de5d5bf_db1c_40ac_b698_095ba3b18578>3‑10.1</EMMO_8de5d5bf_db1c_40ac_b698_095ba3b18578>
    <rdf:type rdf:resource="http://www.w3.org/2002/07/owl#Class"/>
    <skos:prefLabel xml:lang="en">Velocity</skos:prefLabel>
  </rdf:Description>
  <rdf:Description rdf:nodeID="f05bdaa1e617a4bccafc519daf7bf4785b103">
    <rdf:type rdf:resource="http://www.w3.org/2002/07/owl#Restriction"/>
    <owl:onProperty rdf:resource="http://emmo.info/emmo#EMMO_bed1d005_b04e_4a90_94cf_02bc678a8569"/>
    <owl:someValuesFrom rdf:resource="http://emmo.info/emmo#EMMO_77e9dc31_5b19_463e_b000_44c6e79f98aa"/>
  </rdf:Description>
  <rdf:Description rdf:about="http://emmo.info/emmo#EMMO_ae2d1a96_bfa1_409a_a7d2_03d69e8a125a">
    <EMMO_967080e5_2f42_4eb2_a3a9_c58143e835f9 xml:lang="en">The relation between a process and an object participating to it.</EMMO_967080e5_2f42_4eb2_a3a9_c58143e835f9>
    <rdf:type rdf:resource="http://www.w3.org/2002/07/owl#ObjectProperty"/>
    <rdfs:subPropertyOf rdf:resource="http://emmo.info/emmo#EMMO_17e27c22_37e1_468c_9dd7_95e137f73e7f"/>
    <skos:prefLabel xml:lang="en">hasParticipant</skos:prefLabel>
    <rdfs:range rdf:resource="http://emmo.info/emmo#EMMO_49804605_c0fe_4538_abda_f70ba1dc8a5d"/>
    <rdfs:comment xml:lang="en">Participation is not under direct parthood since a process is not strictly related to reductionism, but it's a way to categorize temporal regions by the interpreters.</rdfs:comment>
    <rdfs:comment xml:lang="en">Participation is a parthood relation: you must be part (and then be connected) of the process to contribute to it.</rdfs:comment>
    <rdfs:domain rdf:resource="http://emmo.info/emmo#EMMO_43e9a05d_98af_41b4_92f6_00f79a09bfce"/>
  </rdf:Description>
  <rdf:Description rdf:nodeID="f05bdaa1e617a4bccafc519daf7bf4785b42">
    <rdf:type rdf:resource="http://www.w3.org/1999/02/22-rdf-syntax-ns#List"/>
    <rdf:first rdf:resource="http://emmo.info/emmo#EMMO_db5dd38d_ac79_4af6_8782_fee7e7150ae8"/>
    <rdf:rest rdf:nodeID="f05bdaa1e617a4bccafc519daf7bf4785b43"/>
  </rdf:Description>
  <rdf:Description rdf:nodeID="f05bdaa1e617a4bccafc519daf7bf4785b94">
    <owl:onProperty rdf:resource="http://emmo.info/emmo#EMMO_23b579e1_8088_45b5_9975_064014026c42"/>
    <rdf:type rdf:resource="http://www.w3.org/2002/07/owl#Restriction"/>
    <owl:hasValue>k</owl:hasValue>
  </rdf:Description>
  <rdf:Description rdf:nodeID="fc2fcd8f8eb3649bcbbaff76ba54058acb3">
    <owl:allValuesFrom rdf:resource="http://emmo.info/emmo#EMMO_29072ec4_ffcb_42fb_bdc7_26f05a2e9873"/>
    <rdf:type rdf:resource="http://www.w3.org/2002/07/owl#Restriction"/>
    <owl:onProperty rdf:resource="http://emmo.info/emmo#EMMO_17e27c22_37e1_468c_9dd7_95e137f73e7f"/>
  </rdf:Description>
  <rdf:Description rdf:nodeID="fe0b20157736f4a31909181349b2e6219b32">
    <owl:hasValue>T0 L+1 M0 I0 Θ0 N0 J0</owl:hasValue>
    <owl:onProperty rdf:resource="http://emmo.info/emmo#EMMO_23b579e1_8088_45b5_9975_064014026c42"/>
    <rdf:type rdf:resource="http://www.w3.org/2002/07/owl#Restriction"/>
  </rdf:Description>
  <rdf:Description rdf:about="http://emmo.info/emmo#EMMO_04cf0295_3e8f_4693_a87f_3130d125cf05">
    <EMMO_fe015383_afb3_44a6_ae86_043628697aa2>https://doi.org/10.1351/goldbook.W06668</EMMO_fe015383_afb3_44a6_ae86_043628697aa2>
    <rdfs:subClassOf rdf:resource="http://emmo.info/emmo#EMMO_1f087811_06cb_42d5_90fb_25d0e7e068ef"/>
    <EMMO_de178b12_5d35_4bca_8efa_a4193162571d>T-2 L+1 M+1 I0 Θ0 N0 J0</EMMO_de178b12_5d35_4bca_8efa_a4193162571d>
    <skos:prefLabel xml:lang="en">Weight</skos:prefLabel>
    <rdfs:comment xml:lang="en">Force of gravity acting on a body.</rdfs:comment>
    <EMMO_1f1b164d_ec6a_4faa_8d5e_88bda62316cc>http://qudt.org/vocab/quantitykind/Weight</EMMO_1f1b164d_ec6a_4faa_8d5e_88bda62316cc>
    <rdf:type rdf:resource="http://www.w3.org/2002/07/owl#Class"/>
    <EMMO_6dd685dd_1895_46e4_b227_be9f7d643c25>http://dbpedia.org/page/Weight</EMMO_6dd685dd_1895_46e4_b227_be9f7d643c25>
  </rdf:Description>
  <rdf:Description rdf:about="http://emmo.info/emmo#EMMO_40e18c93_a1b5_49ff_b06a_d9d932d1fb65">
    <EMMO_967080e5_2f42_4eb2_a3a9_c58143e835f9 xml:lang="en">An emulsion is a mixture of two or more liquids that are normally immiscible (a liquid-liquid heterogeneous mixture).</EMMO_967080e5_2f42_4eb2_a3a9_c58143e835f9>
    <rdfs:subClassOf rdf:resource="http://emmo.info/emmo#EMMO_7509da43_56b1_4d7f_887a_65d1663df4ba"/>
    <rdf:type rdf:resource="http://www.w3.org/2002/07/owl#Class"/>
    <skos:prefLabel xml:lang="en">Emulsion</skos:prefLabel>
    <rdfs:subClassOf rdf:resource="http://emmo.info/emmo#EMMO_6c487fb3_03d1_4e56_91ed_c2e16dcbef60"/>
    <EMMO_b432d2d5_25f4_4165_99c5_5935a7763c1a xml:lang="en">Mayonnaise, milk.</EMMO_b432d2d5_25f4_4165_99c5_5935a7763c1a>
  </rdf:Description>
  <rdf:Description rdf:about="http://emmo.info/emmo#EMMO_18ce5200_00f5_45bb_8c6f_6fb128cd41ae">
    <skos:prefLabel xml:lang="en">ReferenceUnit</skos:prefLabel>
    <rdf:type rdf:resource="http://www.w3.org/2002/07/owl#Class"/>
    <rdfs:comment xml:lang="en">A symbolic is recognized as reference unit also if it is not part of a quatity (e.g. as in the sentence "the Bq is the reference unit of Becquerel").

For this reason we can't declare the axiom:
ReferenceUnit SubClassOf: inverse(hasReferenceUnit) some Quantity
because there exist reference units without being part of a quantity.

This is peculiar to EMMO, where quantities (symbolic) are distinct with properties (semiotics).</rdfs:comment>
    <rdfs:comment xml:lang="en">A reference can be a measurement unit, a measurement procedure, a reference material, or a combination of such.
International vocabulary of metrology (VIM)</rdfs:comment>
    <rdfs:subClassOf rdf:resource="http://emmo.info/emmo#EMMO_985bec21_989f_4b9e_a4b3_735d88099c3c"/>
  </rdf:Description>
  <rdf:Description rdf:about="http://emmo.info/emmo#EMMO_053648ea_3c0a_468c_89cb_eb009239323a">
    <EMMO_c84c6752_6d64_48cc_9500_e54a3c34898d>https://en.wikipedia.org/wiki/Astronomical_unit</EMMO_c84c6752_6d64_48cc_9500_e54a3c34898d>
    <rdfs:subClassOf rdf:nodeID="ffcb99037244f48d590430c228d02afdbb4"/>
    <rdfs:subClassOf rdf:nodeID="ffcb99037244f48d590430c228d02afdbb5"/>
    <rdfs:subClassOf rdf:resource="http://emmo.info/emmo#EMMO_591e02fd_8d37_45a6_9d11_bb21cef391a0"/>
    <skos:prefLabel xml:lang="en">AstronomicalUnit</skos:prefLabel>
    <EMMO_1f1b164d_ec6a_4faa_8d5e_88bda62316cc>http://qudt.org/vocab/unit/PARSEC</EMMO_1f1b164d_ec6a_4faa_8d5e_88bda62316cc>
    <EMMO_70fe84ff_99b6_4206_a9fc_9a8931836d84 xml:lang="en">One astronomical unit is defined as exactly 149597870700 m, which is roughly the distance from earth to sun.</EMMO_70fe84ff_99b6_4206_a9fc_9a8931836d84>
    <rdf:type rdf:resource="http://www.w3.org/2002/07/owl#Class"/>
    <EMMO_6dd685dd_1895_46e4_b227_be9f7d643c25>http://dbpedia.org/page/Astronomical_unit</EMMO_6dd685dd_1895_46e4_b227_be9f7d643c25>
  </rdf:Description>
  <rdf:Description rdf:nodeID="f05bdaa1e617a4bccafc519daf7bf4785b173">
    <rdf:rest rdf:nodeID="f05bdaa1e617a4bccafc519daf7bf4785b174"/>
    <rdf:type rdf:resource="http://www.w3.org/1999/02/22-rdf-syntax-ns#List"/>
    <rdf:first rdf:resource="http://emmo.info/emmo#EMMO_a9201b2f_e6de_442a_b3a6_d292a5820bc5"/>
  </rdf:Description>
  <rdf:Description rdf:nodeID="fe0b20157736f4a31909181349b2e6219b6">
    <rdf:rest rdf:nodeID="fe0b20157736f4a31909181349b2e6219b7"/>
    <rdf:type rdf:resource="http://www.w3.org/1999/02/22-rdf-syntax-ns#List"/>
    <rdf:first rdf:resource="http://emmo.info/emmo#EMMO_c995ae70_3b84_4ebb_bcfc_69e6a281bb88"/>
  </rdf:Description>
  <rdf:Description rdf:about="http://emmo.info/emmo#EMMO_4091d5ec_a4df_42b9_a073_9a090839279f">
    <rdfs:comment xml:lang="en">Measurement of energy in a thermodynamic system.</rdfs:comment>
    <EMMO_1f1b164d_ec6a_4faa_8d5e_88bda62316cc>http://qudt.org/vocab/quantitykind/Enthalpy</EMMO_1f1b164d_ec6a_4faa_8d5e_88bda62316cc>
    <EMMO_de178b12_5d35_4bca_8efa_a4193162571d>T-2 L+2 M+1 I0 Θ0 N0 J0</EMMO_de178b12_5d35_4bca_8efa_a4193162571d>
    <rdf:type rdf:resource="http://www.w3.org/2002/07/owl#Class"/>
    <EMMO_6dd685dd_1895_46e4_b227_be9f7d643c25>http://dbpedia.org/page/Enthalpy</EMMO_6dd685dd_1895_46e4_b227_be9f7d643c25>
    <skos:prefLabel xml:lang="en">Enthalpy</skos:prefLabel>
    <EMMO_fe015383_afb3_44a6_ae86_043628697aa2>https://doi.org/10.1351/goldbook.E02141</EMMO_fe015383_afb3_44a6_ae86_043628697aa2>
    <rdfs:subClassOf rdf:resource="http://emmo.info/emmo#EMMO_31ec09ba_1713_42cb_83c7_b38bf6f9ced2"/>
  </rdf:Description>
  <rdf:Description rdf:nodeID="ff14b31ebf90e4bc5ba2839064d29e543b28">
    <owl:qualifiedCardinality rdf:datatype="http://www.w3.org/2001/XMLSchema#nonNegativeInteger">1</owl:qualifiedCardinality>
  </rdf:Description>
  <rdf:Description rdf:nodeID="f05bdaa1e617a4bccafc519daf7bf4785b43">
    <rdf:first rdf:resource="http://emmo.info/emmo#EMMO_df6eeb01_1b41_4bd8_9257_a04fbd7cf000"/>
    <rdf:type rdf:resource="http://www.w3.org/1999/02/22-rdf-syntax-ns#List"/>
    <rdf:rest rdf:resource="http://www.w3.org/1999/02/22-rdf-syntax-ns#nil"/>
  </rdf:Description>
  <rdf:Description rdf:nodeID="ffcb99037244f48d590430c228d02afdbb15">
    <rdf:type rdf:resource="http://www.w3.org/2002/07/owl#Restriction"/>
    <owl:someValuesFrom rdf:resource="http://emmo.info/emmo#EMMO_f84792eb_ec64_4a6b_941f_c9f3e9ef052c"/>
    <owl:onProperty rdf:resource="http://emmo.info/emmo#EMMO_bed1d005_b04e_4a90_94cf_02bc678a8569"/>
  </rdf:Description>
  <rdf:Description rdf:about="http://emmo.info/emmo#EMMO_7db59e56_f68b_48b7_ae99_891c35ae5c3b">
    <rdfs:subClassOf rdf:resource="http://emmo.info/emmo#EMMO_0f795e3e_c602_4577_9a43_d5a231aa1360"/>
    <rdf:type rdf:resource="http://www.w3.org/2002/07/owl#Class"/>
    <skos:prefLabel xml:lang="en">Gluon</skos:prefLabel>
    <EMMO_967080e5_2f42_4eb2_a3a9_c58143e835f9 xml:lang="en">The class of individuals that stand for gluons elementary particles.</EMMO_967080e5_2f42_4eb2_a3a9_c58143e835f9>
  </rdf:Description>
  <rdf:Description rdf:about="http://emmo.info/emmo#EMMO_21aaefc1_3f86_4208_b7db_a755f31f0f8c">
    <rdfs:subClassOf rdf:nodeID="f05bdaa1e617a4bccafc519daf7bf4785b17"/>
    <rdfs:subClassOf rdf:nodeID="f05bdaa1e617a4bccafc519daf7bf4785b20"/>
    <rdf:type rdf:resource="http://www.w3.org/2002/07/owl#Class"/>
    <skos:prefLabel xml:lang="en">Hecto</skos:prefLabel>
  </rdf:Description>
  <rdf:Description rdf:nodeID="f05bdaa1e617a4bccafc519daf7bf4785b50">
    <rdf:type rdf:resource="http://www.w3.org/2002/07/owl#Restriction"/>
    <owl:hasValue rdf:datatype="http://www.w3.org/2001/XMLSchema#double">1e-18</owl:hasValue>
    <owl:onProperty rdf:resource="http://emmo.info/emmo#EMMO_faf79f53_749d_40b2_807c_d34244c192f4"/>
  </rdf:Description>
  <rdf:Description rdf:nodeID="fc2fcd8f8eb3649bcbbaff76ba54058acb5">
    <owl:allValuesFrom rdf:resource="http://emmo.info/emmo#EMMO_c5ddfdba_c074_4aa4_ad6b_1ac4942d300d"/>
    <rdf:type rdf:resource="http://www.w3.org/2002/07/owl#Restriction"/>
    <owl:onProperty rdf:resource="http://emmo.info/emmo#EMMO_7afbed84_7593_4a23_bd88_9d9c6b04e8f6"/>
  </rdf:Description>
  <rdf:Description rdf:nodeID="f05bdaa1e617a4bccafc519daf7bf4785b29">
    <rdf:type rdf:resource="http://www.w3.org/2002/07/owl#Restriction"/>
    <owl:onProperty rdf:resource="http://emmo.info/emmo#EMMO_bed1d005_b04e_4a90_94cf_02bc678a8569"/>
    <owl:someValuesFrom rdf:resource="http://emmo.info/emmo#EMMO_a77a0a4b_6bd2_42b2_be27_4b63cebbb59e"/>
  </rdf:Description>
  <rdf:Description rdf:nodeID="f05bdaa1e617a4bccafc519daf7bf4785b53">
    <owl:inverseOf rdf:resource="http://emmo.info/emmo#EMMO_3446e167_c576_49d6_846c_215bb8878a55"/>
  </rdf:Description>
  <rdf:Description rdf:nodeID="ff14b31ebf90e4bc5ba2839064d29e543b15">
    <rdf:rest rdf:resource="http://www.w3.org/1999/02/22-rdf-syntax-ns#nil"/>
    <rdf:first rdf:resource="http://emmo.info/emmo#EMMO_e9e02156_651f_41c8_9efb_d5da0d4ce5e2"/>
    <rdf:type rdf:resource="http://www.w3.org/1999/02/22-rdf-syntax-ns#List"/>
  </rdf:Description>
  <rdf:Description rdf:about="http://emmo.info/emmo#EMMO_515b5579_d526_4842_9e6f_ecc34db6f368">
    <rdf:type rdf:resource="http://www.w3.org/2002/07/owl#Class"/>
    <skos:prefLabel xml:lang="en">FrequencyDimension</skos:prefLabel>
    <owl:equivalentClass rdf:nodeID="fe0b20157736f4a31909181349b2e6219b18"/>
    <rdfs:subClassOf rdf:resource="http://emmo.info/emmo#EMMO_9895a1b4_f0a5_4167_ac5e_97db40b8bfcc"/>
  </rdf:Description>
  <rdf:Description rdf:about="http://emmo.info/emmo#EMMO_f992dc76_f9a6_45f6_8873_c8e20d16fbbe">
    <skos:prefLabel xml:lang="en">Gram</skos:prefLabel>
    <EMMO_70fe84ff_99b6_4206_a9fc_9a8931836d84 xml:lang="en">Gram is defined as one thousandth of the SI unit kilogram.</EMMO_70fe84ff_99b6_4206_a9fc_9a8931836d84>
    <rdfs:subClassOf rdf:nodeID="ffcb99037244f48d590430c228d02afdbb59"/>
    <EMMO_c84c6752_6d64_48cc_9500_e54a3c34898d>https://en.wikipedia.org/wiki/Gram</EMMO_c84c6752_6d64_48cc_9500_e54a3c34898d>
    <rdf:type rdf:resource="http://www.w3.org/2002/07/owl#Class"/>
    <EMMO_1f1b164d_ec6a_4faa_8d5e_88bda62316cc>http://qudt.org/vocab/unit/GM</EMMO_1f1b164d_ec6a_4faa_8d5e_88bda62316cc>
    <EMMO_fe015383_afb3_44a6_ae86_043628697aa2>https://doi.org/10.1351/goldbook.G02680</EMMO_fe015383_afb3_44a6_ae86_043628697aa2>
    <rdfs:subClassOf rdf:nodeID="ffcb99037244f48d590430c228d02afdbb58"/>
    <rdfs:subClassOf rdf:resource="http://emmo.info/emmo#EMMO_52e4cb25_da39_45e2_a6db_063ec5730499"/>
  </rdf:Description>
  <rdf:Description rdf:nodeID="ffcb99037244f48d590430c228d02afdbb32">
    <owl:onProperty rdf:resource="http://emmo.info/emmo#EMMO_23b579e1_8088_45b5_9975_064014026c42"/>
    <owl:hasValue>″</owl:hasValue>
    <rdf:type rdf:resource="http://www.w3.org/2002/07/owl#Restriction"/>
  </rdf:Description>
  <rdf:Description rdf:nodeID="ffcb99037244f48d590430c228d02afdbb24">
    <rdf:type rdf:resource="http://www.w3.org/1999/02/22-rdf-syntax-ns#List"/>
    <rdf:rest rdf:nodeID="ffcb99037244f48d590430c228d02afdbb25"/>
    <rdf:first rdf:resource="http://emmo.info/emmo#EMMO_a155dc93_d266_487e_b5e7_2a2c72d5ebf9"/>
  </rdf:Description>
  <rdf:Description rdf:nodeID="f05bdaa1e617a4bccafc519daf7bf4785b150">
    <owl:hasValue>Sv</owl:hasValue>
    <owl:onProperty rdf:resource="http://emmo.info/emmo#EMMO_23b579e1_8088_45b5_9975_064014026c42"/>
    <rdf:type rdf:resource="http://www.w3.org/2002/07/owl#Restriction"/>
  </rdf:Description>
  <rdf:Description rdf:about="http://emmo.info/emmo#EMMO_ec7464a9_d99d_45f8_965b_4e9230ea8356">
    <rdfs:subClassOf rdf:resource="http://emmo.info/emmo#EMMO_86ca9b93_1183_4b65_81b8_c0fcd3bba5ad"/>
    <rdf:type rdf:resource="http://www.w3.org/2002/07/owl#Class"/>
    <rdfs:subClassOf rdf:nodeID="ffbe75b10062f400ea693809785c50a44b6"/>
    <rdfs:comment xml:lang="en">A material that is synthesized within a manufacturing process.</rdfs:comment>
    <rdfs:subClassOf rdf:resource="http://emmo.info/emmo#EMMO_4207e895_8b83_4318_996a_72cfb32acd94"/>
    <skos:prefLabel xml:lang="en">EngineeredMaterial</skos:prefLabel>
  </rdf:Description>
  <rdf:Description rdf:nodeID="fdb1489b80bcc4ee28afe0be8feb9b935b13">
    <rdf:type rdf:resource="http://www.w3.org/2002/07/owl#Class"/>
    <owl:unionOf rdf:nodeID="fdb1489b80bcc4ee28afe0be8feb9b935b14"/>
  </rdf:Description>
  <rdf:Description rdf:nodeID="f05bdaa1e617a4bccafc519daf7bf4785b120">
    <rdf:type rdf:resource="http://www.w3.org/2002/07/owl#Restriction"/>
    <owl:onProperty rdf:resource="http://emmo.info/emmo#EMMO_23b579e1_8088_45b5_9975_064014026c42"/>
    <owl:hasValue>G</owl:hasValue>
  </rdf:Description>
  <rdf:Description rdf:nodeID="f05bdaa1e617a4bccafc519daf7bf4785b129">
    <owl:onProperty rdf:nodeID="f05bdaa1e617a4bccafc519daf7bf4785b130"/>
    <rdf:type rdf:resource="http://www.w3.org/2002/07/owl#Restriction"/>
    <owl:allValuesFrom rdf:nodeID="f05bdaa1e617a4bccafc519daf7bf4785b131"/>
  </rdf:Description>
  <rdf:Description rdf:nodeID="ffcb99037244f48d590430c228d02afdbb7">
    <owl:someValuesFrom rdf:resource="http://emmo.info/emmo#EMMO_3227b821_26a5_4c7c_9c01_5c24483e0bd0"/>
    <rdf:type rdf:resource="http://www.w3.org/2002/07/owl#Restriction"/>
    <owl:onProperty rdf:resource="http://emmo.info/emmo#EMMO_bed1d005_b04e_4a90_94cf_02bc678a8569"/>
  </rdf:Description>
  <rdf:Description rdf:nodeID="f05bdaa1e617a4bccafc519daf7bf4785b90">
    <rdf:type rdf:resource="http://www.w3.org/1999/02/22-rdf-syntax-ns#List"/>
    <rdf:first rdf:resource="http://emmo.info/emmo#EMMO_e9ffc696_5228_4ff9_8a60_0f5e05e9931b"/>
    <rdf:rest rdf:resource="http://www.w3.org/1999/02/22-rdf-syntax-ns#nil"/>
  </rdf:Description>
  <rdf:Description rdf:nodeID="ffcb99037244f48d590430c228d02afdbb21">
    <rdf:first rdf:resource="http://emmo.info/emmo#EMMO_28ef05a7_ecc1_4df6_8116_c53251fbd4a8"/>
    <rdf:type rdf:resource="http://www.w3.org/1999/02/22-rdf-syntax-ns#List"/>
    <rdf:rest rdf:nodeID="ffcb99037244f48d590430c228d02afdbb22"/>
  </rdf:Description>
  <rdf:Description rdf:nodeID="fe0b20157736f4a31909181349b2e6219b9">
    <rdf:rest rdf:resource="http://www.w3.org/1999/02/22-rdf-syntax-ns#nil"/>
    <rdf:type rdf:resource="http://www.w3.org/1999/02/22-rdf-syntax-ns#List"/>
    <rdf:first rdf:resource="http://emmo.info/emmo#EMMO_ed4af7ae_63a2_497e_bb88_2309619ea405"/>
  </rdf:Description>
  <rdf:Description rdf:about="http://emmo.info/emmo#EMMO_985bec21_989f_4b9e_a4b3_735d88099c3c">
    <skos:prefLabel xml:lang="en">Metrological</skos:prefLabel>
    <rdfs:comment xml:lang="en">This language domain makes use of ISO 80000 concepts.</rdfs:comment>
    <rdf:type rdf:resource="http://www.w3.org/2002/07/owl#Class"/>
    <EMMO_967080e5_2f42_4eb2_a3a9_c58143e835f9 xml:lang="en">A language object used in metrology.</EMMO_967080e5_2f42_4eb2_a3a9_c58143e835f9>
    <rdfs:comment xml:lang="en">Metrology includes all theoretical and practical aspects of measurement, whatever the measurement uncertainty and field of application.

-- International vocabulary of metrology (VIM)</rdfs:comment>
    <rdfs:subClassOf rdf:resource="http://emmo.info/emmo#EMMO_d8d2144e_5c8d_455d_a643_5caf4d8d9df8"/>
  </rdf:Description>
  <rdf:Description rdf:nodeID="fea11ca01461e402d8f697c19c5d8de88b15">
    <rdf:first rdf:resource="http://emmo.info/emmo#EMMO_25f8b804_9a0b_4387_a3e7_b35bce5365ee"/>
    <rdf:type rdf:resource="http://www.w3.org/1999/02/22-rdf-syntax-ns#List"/>
    <rdf:rest rdf:nodeID="fea11ca01461e402d8f697c19c5d8de88b16"/>
  </rdf:Description>
  <rdf:Description rdf:about="http://emmo.info/emmo#EMMO_ec903946_ddc9_464a_903c_7373e0d1eeb5">
    <rdfs:subClassOf rdf:resource="http://emmo.info/emmo#EMMO_9895a1b4_f0a5_4167_ac5e_97db40b8bfcc"/>
    <rdf:type rdf:resource="http://www.w3.org/2002/07/owl#Class"/>
    <skos:prefLabel xml:lang="en">MagneticFluxDensityDimension</skos:prefLabel>
    <owl:equivalentClass rdf:nodeID="fe0b20157736f4a31909181349b2e6219b37"/>
  </rdf:Description>
  <rdf:Description rdf:about="http://emmo.info/emmo#EMMO_1f1b164d_ec6a_4faa_8d5e_88bda62316cc">
    <rdfs:range rdf:resource="http://www.w3.org/2001/XMLSchema#anyURI"/>
    <rdfs:subPropertyOf rdf:resource="http://www.w3.org/2000/01/rdf-schema#seeAlso"/>
    <skos:prefLabel xml:lang="en">qudtEntry</skos:prefLabel>
    <rdfs:comment xml:lang="en">URL to corresponing entity in QUDT.</rdfs:comment>
    <rdf:type rdf:resource="http://www.w3.org/2002/07/owl#AnnotationProperty"/>
    <rdfs:seeAlso rdf:datatype="http://www.w3.org/2001/XMLSchema#anyURI">http://www.qudt.org/2.1/catalog/qudt-catalog.html</rdfs:seeAlso>
  </rdf:Description>
  <rdf:Description rdf:nodeID="f05bdaa1e617a4bccafc519daf7bf4785b123">
    <owl:onProperty rdf:resource="http://emmo.info/emmo#EMMO_bed1d005_b04e_4a90_94cf_02bc678a8569"/>
    <owl:someValuesFrom rdf:resource="http://emmo.info/emmo#EMMO_53e825d9_1a09_483c_baa7_37501ebfbe1c"/>
    <rdf:type rdf:resource="http://www.w3.org/2002/07/owl#Restriction"/>
  </rdf:Description>
  <rdf:Description rdf:about="http://emmo.info/emmo#EMMO_39c3815d_8cae_4c8f_b2ff_eeba24bec455">
    <skos:prefLabel xml:lang="en">hasIcon</skos:prefLabel>
    <rdf:type rdf:resource="http://www.w3.org/2002/07/owl#ObjectProperty"/>
    <rdfs:range rdf:resource="http://emmo.info/emmo#EMMO_d7788d1a_020d_4c78_85a1_13563fcec168"/>
    <rdfs:subPropertyOf rdf:resource="http://emmo.info/emmo#EMMO_60577dea_9019_4537_ac41_80b0fb563d41"/>
  </rdf:Description>
  <rdf:Description rdf:about="http://emmo.info/emmo#EMMO_f8bd64d5_5d3e_4ad4_a46e_c30714fecb7f">
    <owl:equivalentClass rdf:nodeID="fe24a777e3fd743f986ce83488d2cf30bb27"/>
    <rdfs:subClassOf rdf:resource="http://emmo.info/emmo#EMMO_21f56795_ee72_4858_b571_11cfaa59c1a8"/>
    <rdf:type rdf:resource="http://www.w3.org/2002/07/owl#Class"/>
    <skos:prefLabel xml:lang="en">Integer</skos:prefLabel>
    <rdfs:subClassOf rdf:nodeID="fe24a777e3fd743f986ce83488d2cf30bb28"/>
    <rdfs:subClassOf rdf:nodeID="fe24a777e3fd743f986ce83488d2cf30bb29"/>
  </rdf:Description>
  <rdf:Description rdf:about="http://emmo.info/emmo#EMMO_f35cff4d_dc09_44cf_a729_22fb79e3bfb2">
    <rdfs:subClassOf rdf:resource="http://emmo.info/emmo#EMMO_02c0621e_a527_4790_8a0f_2bb51973c819"/>
    <skos:prefLabel xml:lang="en">InternationalSystemOfQuantity</skos:prefLabel>
    <EMMO_c84c6752_6d64_48cc_9500_e54a3c34898d>https://en.wikipedia.org/wiki/International_System_of_Quantities</EMMO_c84c6752_6d64_48cc_9500_e54a3c34898d>
    <rdf:type rdf:resource="http://www.w3.org/2002/07/owl#Class"/>
    <rdfs:seeAlso>https://www.iso.org/obp/ui/#iso:std:iso:80000:-1:ed-1:v1:en:sec:3.1</rdfs:seeAlso>
    <EMMO_967080e5_2f42_4eb2_a3a9_c58143e835f9 xml:lang="en">Quantities declared under the ISO 80000.</EMMO_967080e5_2f42_4eb2_a3a9_c58143e835f9>
  </rdf:Description>
  <rdf:Description rdf:nodeID="f05bdaa1e617a4bccafc519daf7bf4785b24">
    <rdf:type rdf:resource="http://www.w3.org/2002/07/owl#Restriction"/>
    <owl:onProperty rdf:resource="http://emmo.info/emmo#EMMO_23b579e1_8088_45b5_9975_064014026c42"/>
    <owl:hasValue>f</owl:hasValue>
  </rdf:Description>
  <rdf:Description rdf:about="http://emmo.info/emmo#EMMO_e2ee1c98_497a_4f66_b4ed_5711496a848e">
    <EMMO_967080e5_2f42_4eb2_a3a9_c58143e835f9 xml:lang="en">Perceived power of light.</EMMO_967080e5_2f42_4eb2_a3a9_c58143e835f9>
    <EMMO_de178b12_5d35_4bca_8efa_a4193162571d>T0 L0 M0 I0 Θ0 N0 J+1</EMMO_de178b12_5d35_4bca_8efa_a4193162571d>
    <EMMO_fe015383_afb3_44a6_ae86_043628697aa2>https://doi.org/10.1351/goldbook.L03646</EMMO_fe015383_afb3_44a6_ae86_043628697aa2>
    <EMMO_1f1b164d_ec6a_4faa_8d5e_88bda62316cc>http://qudt.org/vocab/quantitykind/LuminousFlux</EMMO_1f1b164d_ec6a_4faa_8d5e_88bda62316cc>
    <rdfs:subClassOf rdf:resource="http://emmo.info/emmo#EMMO_2946d40b_24a1_47fa_8176_e3f79bb45064"/>
    <EMMO_6dd685dd_1895_46e4_b227_be9f7d643c25>http://dbpedia.org/page/Luminous_flux</EMMO_6dd685dd_1895_46e4_b227_be9f7d643c25>
    <rdf:type rdf:resource="http://www.w3.org/2002/07/owl#Class"/>
    <skos:prefLabel xml:lang="en">LuminousFlux</skos:prefLabel>
  </rdf:Description>
  <rdf:Description rdf:nodeID="f05bdaa1e617a4bccafc519daf7bf4785b16">
    <owl:hasValue>da</owl:hasValue>
    <rdf:type rdf:resource="http://www.w3.org/2002/07/owl#Restriction"/>
    <owl:onProperty rdf:resource="http://emmo.info/emmo#EMMO_23b579e1_8088_45b5_9975_064014026c42"/>
  </rdf:Description>
  <rdf:Description rdf:about="http://emmo.info/emmo#EMMO_47fe2379_be21_48d1_9ede_402f0faf494b">
    <rdf:type rdf:resource="http://www.w3.org/2002/07/owl#Class"/>
    <EMMO_967080e5_2f42_4eb2_a3a9_c58143e835f9 xml:lang="en">A coarse dispersion of liquid in a liquid continuum phase.</EMMO_967080e5_2f42_4eb2_a3a9_c58143e835f9>
    <rdfs:subClassOf rdf:resource="http://emmo.info/emmo#EMMO_7509da43_56b1_4d7f_887a_65d1663df4ba"/>
    <skos:prefLabel xml:lang="en">LiquidLiquidSuspension</skos:prefLabel>
  </rdf:Description>
  <rdf:Description rdf:about="http://emmo.info/emmo#EMMO_e150fa8d_06dc_4bb8_bf95_04e2aea529c1">
    <EMMO_fe015383_afb3_44a6_ae86_043628697aa2>https://doi.org/10.1351/goldbook.R05316</EMMO_fe015383_afb3_44a6_ae86_043628697aa2>
    <skos:prefLabel xml:lang="en">ElectricResistivity</skos:prefLabel>
    <rdfs:subClassOf rdf:resource="http://emmo.info/emmo#EMMO_2946d40b_24a1_47fa_8176_e3f79bb45064"/>
    <EMMO_de178b12_5d35_4bca_8efa_a4193162571d>T-3 L+3 M+1 I-2 Θ0 N0 J0</EMMO_de178b12_5d35_4bca_8efa_a4193162571d>
    <rdf:type rdf:resource="http://www.w3.org/2002/07/owl#Class"/>
    <skos:altLabel>Resistivity</skos:altLabel>
    <EMMO_6dd685dd_1895_46e4_b227_be9f7d643c25>http://dbpedia.org/page/Electrical_resistivity_and_conductivity</EMMO_6dd685dd_1895_46e4_b227_be9f7d643c25>
    <EMMO_1f1b164d_ec6a_4faa_8d5e_88bda62316cc>http://qudt.org/vocab/quantitykind/Resistivity</EMMO_1f1b164d_ec6a_4faa_8d5e_88bda62316cc>
    <rdfs:comment xml:lang="en">Electric field strength divided by the current density.</rdfs:comment>
  </rdf:Description>
  <rdf:Description rdf:about="http://emmo.info/emmo#EMMO_5f278af9_8593_4e27_a717_ccc9e07a0ddf">
    <rdfs:subClassOf rdf:resource="http://emmo.info/emmo#EMMO_46f0f8df_4dc6_418f_8036_10427a3a288e"/>
    <rdf:type rdf:resource="http://www.w3.org/2002/07/owl#Class"/>
    <skos:prefLabel xml:lang="en">EuclideanSpace</skos:prefLabel>
  </rdf:Description>
  <rdf:Description rdf:about="http://emmo.info/emmo#EMMO_5cf9f86c_86f5_40c4_846d_60371f670e0a">
    <rdfs:subClassOf rdf:nodeID="f05bdaa1e617a4bccafc519daf7bf4785b81"/>
    <rdfs:subClassOf rdf:nodeID="f05bdaa1e617a4bccafc519daf7bf4785b78"/>
    <rdf:type rdf:resource="http://www.w3.org/2002/07/owl#Class"/>
    <skos:prefLabel xml:lang="en">Exa</skos:prefLabel>
  </rdf:Description>
  <rdf:Description rdf:nodeID="fe0b20157736f4a31909181349b2e6219b24">
    <owl:onProperty rdf:resource="http://emmo.info/emmo#EMMO_23b579e1_8088_45b5_9975_064014026c42"/>
    <owl:hasValue>T-3 L+2 M+1 I-2 Θ0 N0 J0</owl:hasValue>
    <rdf:type rdf:resource="http://www.w3.org/2002/07/owl#Restriction"/>
  </rdf:Description>
  <rdf:Description rdf:about="http://emmo.info/emmo#EMMO_2a888cdf_ec4a_4ec5_af1c_0343372fc978">
    <rdfs:comment xml:lang="en">The word objective does not mean that each observation will provide the same results. It means that the observation followed a well defined procedure.</rdfs:comment>
    <rdf:type rdf:resource="http://www.w3.org/2002/07/owl#Class"/>
    <skos:prefLabel xml:lang="en">ObjectiveProperty</skos:prefLabel>
    <EMMO_967080e5_2f42_4eb2_a3a9_c58143e835f9 xml:lang="en">A 'Property' that is determined by each 'Observer' following a well defined 'Observation' procedure through a specific perception channel.</EMMO_967080e5_2f42_4eb2_a3a9_c58143e835f9>
    <rdfs:comment xml:lang="en">This class refers to what is commonly known as physical property, i.e. a measurable property of physical system, whether is quantifiable or not.</rdfs:comment>
  </rdf:Description>
  <rdf:Description rdf:about="http://www.w3.org/2004/02/skos/core#hiddenLabel">
    <rdf:type rdf:resource="http://www.w3.org/2002/07/owl#AnnotationProperty"/>
    <rdfs:range rdf:resource="http://www.w3.org/1999/02/22-rdf-syntax-ns#PlainLiteral"/>
    <rdfs:subPropertyOf rdf:resource="http://www.w3.org/2000/01/rdf-schema#label"/>
  </rdf:Description>
  <rdf:Description rdf:about="http://emmo.info/emmo#EMMO_feb03a8a_bbb6_4918_a891_46713ef557f4">
    <rdf:type rdf:resource="http://www.w3.org/2002/07/owl#Class"/>
    <owl:disjointUnionOf rdf:nodeID="f05bdaa1e617a4bccafc519daf7bf4785b195"/>
    <rdfs:subClassOf rdf:resource="http://emmo.info/emmo#EMMO_b081b346_7279_46ef_9a3d_2c088fcd79f4"/>
    <rdfs:comment xml:lang="en">The complete set of SI units includes both the coherent set and the multiples and sub-multiples formed by using the SI prefixes.</rdfs:comment>
    <EMMO_967080e5_2f42_4eb2_a3a9_c58143e835f9 xml:lang="en">The set of units provided by the SI referring to the ISQ.</EMMO_967080e5_2f42_4eb2_a3a9_c58143e835f9>
    <rdfs:comment xml:lang="en">The names, symbols and prefixes of SI units are defined by the General Conference on Weights and Measures (CGPM).

https://en.wikipedia.org/wiki/General_Conference_on_Weights_and_Measures</rdfs:comment>
    <skos:prefLabel xml:lang="en">SIUnit</skos:prefLabel>
  </rdf:Description>
  <rdf:Description rdf:about="http://emmo.info/emmo#EMMO_46d5643b_9706_4b67_8bea_ed77d6026539">
    <owl:equivalentClass rdf:nodeID="fe24a777e3fd743f986ce83488d2cf30bb8"/>
    <skos:prefLabel xml:lang="en">Minus</skos:prefLabel>
    <rdf:type rdf:resource="http://www.w3.org/2002/07/owl#Class"/>
    <rdfs:subClassOf rdf:resource="http://emmo.info/emmo#EMMO_707f0cd1_941c_4b57_9f20_d0ba30cd6ff3"/>
  </rdf:Description>
  <rdf:Description rdf:about="http://emmo.info/emmo#EMMO_08cb807c_e626_447b_863f_e2835540e918">
    <rdf:type rdf:resource="http://www.w3.org/2002/07/owl#NamedIndividual"/>
    <skos:prefLabel xml:lang="en">Universe</skos:prefLabel>
  </rdf:Description>
  <rdf:Description rdf:about="http://emmo.info/emmo#EMMO_62f0d847_3603_45b4_bfc4_dd4511355ff2">
    <EMMO_967080e5_2f42_4eb2_a3a9_c58143e835f9 xml:lang="en">Measurement unit obtained by multiplying a given measurement unit by an integer greater than one.</EMMO_967080e5_2f42_4eb2_a3a9_c58143e835f9>
    <rdf:type rdf:resource="http://www.w3.org/2002/07/owl#Class"/>
    <skos:prefLabel xml:lang="en">MultipleUnit</skos:prefLabel>
  </rdf:Description>
  <rdf:Description rdf:nodeID="ffcb99037244f48d590430c228d02afdbb20">
    <rdf:type rdf:resource="http://www.w3.org/1999/02/22-rdf-syntax-ns#List"/>
    <rdf:first rdf:resource="http://emmo.info/emmo#EMMO_21ef2ed6_c086_4d24_8a75_980d2bcc9282"/>
    <rdf:rest rdf:nodeID="ffcb99037244f48d590430c228d02afdbb21"/>
  </rdf:Description>
  <rdf:Description rdf:nodeID="ff14b31ebf90e4bc5ba2839064d29e543b27">
    <owl:minQualifiedCardinality rdf:datatype="http://www.w3.org/2001/XMLSchema#nonNegativeInteger">2</owl:minQualifiedCardinality>
  </rdf:Description>
  <rdf:Description rdf:about="http://emmo.info/emmo#EMMO_3a185e6c_9e19_4776_b583_19c978156aa0">
    <skos:prefLabel xml:lang="en">SIBaseUnit</skos:prefLabel>
    <EMMO_967080e5_2f42_4eb2_a3a9_c58143e835f9 xml:lang="en">The base units in the SI system.</EMMO_967080e5_2f42_4eb2_a3a9_c58143e835f9>
    <rdfs:seeAlso>https://www.bipm.org/utils/common/pdf/si-brochure/SI-Brochure-9-EN.pdf</rdfs:seeAlso>
    <owl:disjointUnionOf rdf:nodeID="f05bdaa1e617a4bccafc519daf7bf4785b37"/>
    <rdf:type rdf:resource="http://www.w3.org/2002/07/owl#Class"/>
    <rdfs:subClassOf rdf:resource="http://emmo.info/emmo#EMMO_db716151_6b73_45ff_910c_d182fdcbb4f5"/>
  </rdf:Description>
  <rdf:Description rdf:nodeID="f05bdaa1e617a4bccafc519daf7bf4785b132">
    <owl:onProperty rdf:resource="http://emmo.info/emmo#EMMO_23b579e1_8088_45b5_9975_064014026c42"/>
    <rdf:type rdf:resource="http://www.w3.org/2002/07/owl#Restriction"/>
    <owl:hasValue>c</owl:hasValue>
  </rdf:Description>
  <rdf:Description rdf:nodeID="f05bdaa1e617a4bccafc519daf7bf4785b108">
    <owl:onProperty rdf:resource="http://emmo.info/emmo#EMMO_23b579e1_8088_45b5_9975_064014026c42"/>
    <rdf:type rdf:resource="http://www.w3.org/2002/07/owl#Restriction"/>
    <owl:hasValue>µ</owl:hasValue>
  </rdf:Description>
  <rdf:Description rdf:nodeID="f05bdaa1e617a4bccafc519daf7bf4785b40">
    <rdf:first rdf:resource="http://emmo.info/emmo#EMMO_8d00f093_3f45_4ea3_986c_b3545c3c2f4c"/>
    <rdf:rest rdf:nodeID="f05bdaa1e617a4bccafc519daf7bf4785b41"/>
    <rdf:type rdf:resource="http://www.w3.org/1999/02/22-rdf-syntax-ns#List"/>
  </rdf:Description>
  <rdf:Description rdf:nodeID="fdb1489b80bcc4ee28afe0be8feb9b935b4">
    <owl:inverseOf rdf:resource="http://emmo.info/emmo#EMMO_ae2d1a96_bfa1_409a_a7d2_03d69e8a125a"/>
  </rdf:Description>
  <rdf:Description rdf:about="http://emmo.info/emmo#EMMO_8c898653_1118_4682_9bbf_6cc334d16a99">
    <skos:prefLabel xml:lang="en">encloses</skos:prefLabel>
    <rdf:type rdf:resource="http://www.w3.org/2002/07/owl#ObjectProperty"/>
    <rdfs:subPropertyOf rdf:resource="http://emmo.info/emmo#EMMO_6703954e_34c4_4a15_a9e7_f313760ae1a8"/>
    <rdfs:comment xml:lang="en">Enclosure is reflexive and transitive.</rdfs:comment>
    <rdf:type rdf:resource="http://www.w3.org/2002/07/owl#TransitiveProperty"/>
  </rdf:Description>
  <rdf:Description rdf:about="http://emmo.info/emmo#EMMO_668e6ead_1530_40cc_ad5e_24b880edff50">
    <owl:equivalentClass rdf:nodeID="fe0b20157736f4a31909181349b2e6219b23"/>
    <rdfs:subClassOf rdf:resource="http://emmo.info/emmo#EMMO_9895a1b4_f0a5_4167_ac5e_97db40b8bfcc"/>
    <skos:prefLabel xml:lang="en">IlluminanceDimension</skos:prefLabel>
    <rdf:type rdf:resource="http://www.w3.org/2002/07/owl#Class"/>
  </rdf:Description>
  <rdf:Description rdf:about="http://emmo.info/emmo#EMMO_10a5fd39_06aa_4648_9e70_f962a9cb2069">
    <rdfs:subClassOf rdf:nodeID="fdb1489b80bcc4ee28afe0be8feb9b935b1"/>
    <rdfs:subClassOf rdf:nodeID="fdb1489b80bcc4ee28afe0be8feb9b935b2"/>
    <rdfs:subClassOf rdf:resource="http://emmo.info/emmo#EMMO_008fd3b2_4013_451f_8827_52bceab11841"/>
    <skos:prefLabel xml:lang="en">Observation</skos:prefLabel>
    <EMMO_967080e5_2f42_4eb2_a3a9_c58143e835f9 xml:lang="en">A 'Semiosis' that involves an 'Observer' that perceives another 'Physical' (the 'Object') through a specific perception mechanism and produces a 'Property' (the 'Sign') that stands for the result of that particular perception.</EMMO_967080e5_2f42_4eb2_a3a9_c58143e835f9>
    <rdf:type rdf:resource="http://www.w3.org/2002/07/owl#Class"/>
  </rdf:Description>
  <rdf:Description rdf:nodeID="fe24a777e3fd743f986ce83488d2cf30bb21">
    <owl:someValuesFrom rdf:resource="http://emmo.info/emmo#EMMO_1aed91a3_d00c_48af_8f43_a0c958b2512a"/>
    <rdf:type rdf:resource="http://www.w3.org/2002/07/owl#Restriction"/>
    <owl:onProperty rdf:resource="http://emmo.info/emmo#EMMO_b2282816_b7a3_44c6_b2cb_3feff1ceb7fe"/>
  </rdf:Description>
  <rdf:Description rdf:nodeID="fa691b5894b3543efa24f9838ff46c3eab6">
    <rdf:type rdf:resource="http://www.w3.org/1999/02/22-rdf-syntax-ns#List"/>
    <rdf:first rdf:resource="http://emmo.info/emmo#EMMO_0cd58641_824c_4851_907f_f4c3be76630c"/>
    <rdf:rest rdf:nodeID="fa691b5894b3543efa24f9838ff46c3eab7"/>
  </rdf:Description>
  <rdf:Description rdf:about="http://emmo.info/emmo#EMMO_15db234d_ecaf_4715_9838_4b4ec424fb13">
    <rdfs:subClassOf rdf:resource="http://emmo.info/emmo#EMMO_49267eba_5548_4163_8f36_518d65b583f9"/>
    <rdfs:comment>Direct parthood is the relation used to build the class hierarchy (and the granularity hierarchy) for this perspective.</rdfs:comment>
    <EMMO_967080e5_2f42_4eb2_a3a9_c58143e835f9 xml:lang="en">A class devoted to categorize 'Physical'-s according to their granularity relations, first in terms of time evolution (Existent) and then in terms of their composition (State), up to the spatial a-tomistic element (Elementary).</EMMO_967080e5_2f42_4eb2_a3a9_c58143e835f9>
    <skos:prefLabel xml:lang="en">Reductionistic</skos:prefLabel>
    <rdf:type rdf:resource="http://www.w3.org/2002/07/owl#Class"/>
    <owl:equivalentClass rdf:nodeID="f3b8e3e5cecf14b688acdf306cd5f62cbb1"/>
  </rdf:Description>
  <rdf:Description rdf:about="http://emmo.info/emmo#EMMO_10dd1eed_da7d_45a3_860c_477ca9e152aa">
    <EMMO_967080e5_2f42_4eb2_a3a9_c58143e835f9 xml:lang="en">Nanomaterials are Materials possessing all external dimension measuring 1-100nm</EMMO_967080e5_2f42_4eb2_a3a9_c58143e835f9>
    <rdfs:subClassOf rdf:resource="http://emmo.info/emmo#EMMO_5d659e25_a508_43ed_903c_3707c7c7cd4b"/>
    <skos:prefLabel xml:lang="en">NanoParticle</skos:prefLabel>
    <rdf:type rdf:resource="http://www.w3.org/2002/07/owl#Class"/>
  </rdf:Description>
  <rdf:Description rdf:about="http://emmo.info/emmo#EMMO_e4281979_2b07_4a43_a772_4903fb3696fe">
    <skos:prefLabel xml:lang="en">Dust</skos:prefLabel>
    <rdfs:subClassOf rdf:resource="http://emmo.info/emmo#EMMO_d4f37e32_16ae_4cc6_b4cd_fd896b2449c4"/>
    <EMMO_967080e5_2f42_4eb2_a3a9_c58143e835f9 xml:lang="en">A suspension of fine particles in the atmosphere.</EMMO_967080e5_2f42_4eb2_a3a9_c58143e835f9>
    <rdf:type rdf:resource="http://www.w3.org/2002/07/owl#Class"/>
  </rdf:Description>
  <rdf:Description rdf:about="http://www.w3.org/2002/07/owl#minQualifiedCardinality">
    <rdf:type rdf:resource="http://www.w3.org/2002/07/owl#AnnotationProperty"/>
  </rdf:Description>
  <rdf:Description rdf:about="http://emmo.info/emmo#EMMO_23bfe79a_cade_48f1_9a8c_fd96e6bac8ba">
    <rdfs:subClassOf rdf:nodeID="f05bdaa1e617a4bccafc519daf7bf4785b24"/>
    <rdfs:subClassOf rdf:nodeID="f05bdaa1e617a4bccafc519daf7bf4785b21"/>
    <rdf:type rdf:resource="http://www.w3.org/2002/07/owl#Class"/>
    <skos:prefLabel xml:lang="en">Femto</skos:prefLabel>
  </rdf:Description>
  <rdf:Description rdf:nodeID="f05bdaa1e617a4bccafc519daf7bf4785b62">
    <rdf:first rdf:resource="http://emmo.info/emmo#EMMO_3a204900_2b33_47d1_b444_815cc4c8cffa"/>
    <rdf:type rdf:resource="http://www.w3.org/1999/02/22-rdf-syntax-ns#List"/>
    <rdf:rest rdf:nodeID="f05bdaa1e617a4bccafc519daf7bf4785b63"/>
  </rdf:Description>
  <rdf:Description rdf:about="http://emmo.info/emmo#EMMO_321af35f_f0cc_4a5c_b4fe_8c2c0303fb0c">
    <rdf:type rdf:resource="http://www.w3.org/2002/07/owl#Class"/>
    <owl:equivalentClass rdf:nodeID="fe0b20157736f4a31909181349b2e6219b12"/>
    <skos:prefLabel xml:lang="en">ElectricConductanceDimension</skos:prefLabel>
    <rdfs:subClassOf rdf:resource="http://emmo.info/emmo#EMMO_9895a1b4_f0a5_4167_ac5e_97db40b8bfcc"/>
  </rdf:Description>
  <rdf:Description rdf:nodeID="f8fb83657cd5f496db3c2b94baf326f26b16">
    <rdf:type rdf:resource="http://www.w3.org/1999/02/22-rdf-syntax-ns#List"/>
    <rdf:rest rdf:nodeID="f8fb83657cd5f496db3c2b94baf326f26b17"/>
    <rdf:first rdf:resource="http://emmo.info/emmo#EMMO_985bec21_989f_4b9e_a4b3_735d88099c3c"/>
  </rdf:Description>
  <rdf:Description rdf:nodeID="fe0b20157736f4a31909181349b2e6219b10">
    <rdf:type rdf:resource="http://www.w3.org/2002/07/owl#Restriction"/>
    <owl:onProperty rdf:resource="http://emmo.info/emmo#EMMO_23b579e1_8088_45b5_9975_064014026c42"/>
    <owl:hasValue>T+1 L+1 M0 I+1 Θ0 N0 J0</owl:hasValue>
  </rdf:Description>
  <rdf:Description rdf:nodeID="fe24a777e3fd743f986ce83488d2cf30bb4">
    <owl:qualifiedCardinality rdf:datatype="http://www.w3.org/2001/XMLSchema#nonNegativeInteger">1</owl:qualifiedCardinality>
    <owl:onProperty rdf:resource="http://emmo.info/emmo#EMMO_faf79f53_749d_40b2_807c_d34244c192f4"/>
    <owl:onDataRange rdf:resource="http://www.w3.org/2001/XMLSchema#double"/>
    <rdf:type rdf:resource="http://www.w3.org/2002/07/owl#Restriction"/>
  </rdf:Description>
  <rdf:Description rdf:nodeID="fea11ca01461e402d8f697c19c5d8de88b12">
    <rdf:type rdf:resource="http://www.w3.org/2002/07/owl#Class"/>
    <owl:unionOf rdf:nodeID="fea11ca01461e402d8f697c19c5d8de88b13"/>
  </rdf:Description>
  <rdf:Description rdf:nodeID="f05bdaa1e617a4bccafc519daf7bf4785b190">
    <owl:inverseOf rdf:resource="http://emmo.info/emmo#EMMO_3446e167_c576_49d6_846c_215bb8878a55"/>
  </rdf:Description>
  <rdf:Description rdf:nodeID="f05bdaa1e617a4bccafc519daf7bf4785b21">
    <rdf:type rdf:resource="http://www.w3.org/2002/07/owl#Restriction"/>
    <owl:allValuesFrom rdf:nodeID="f05bdaa1e617a4bccafc519daf7bf4785b23"/>
    <owl:onProperty rdf:nodeID="f05bdaa1e617a4bccafc519daf7bf4785b22"/>
  </rdf:Description>
  <rdf:Description rdf:nodeID="f05bdaa1e617a4bccafc519daf7bf4785b134">
    <owl:onProperty rdf:resource="http://emmo.info/emmo#EMMO_23b579e1_8088_45b5_9975_064014026c42"/>
    <owl:hasValue>Bq</owl:hasValue>
    <rdf:type rdf:resource="http://www.w3.org/2002/07/owl#Restriction"/>
  </rdf:Description>
  <rdf:Description rdf:nodeID="f05bdaa1e617a4bccafc519daf7bf4785b136">
    <owl:onProperty rdf:resource="http://emmo.info/emmo#EMMO_23b579e1_8088_45b5_9975_064014026c42"/>
    <rdf:type rdf:resource="http://www.w3.org/2002/07/owl#Restriction"/>
    <owl:hasValue>sr</owl:hasValue>
  </rdf:Description>
  <rdf:Description rdf:nodeID="f05bdaa1e617a4bccafc519daf7bf4785b96">
    <rdf:type rdf:resource="http://www.w3.org/2002/07/owl#Restriction"/>
    <owl:onProperty rdf:resource="http://emmo.info/emmo#EMMO_23b579e1_8088_45b5_9975_064014026c42"/>
    <owl:hasValue>m</owl:hasValue>
  </rdf:Description>
  <rdf:Description rdf:about="http://emmo.info/emmo#EMMO_fe015383_afb3_44a6_ae86_043628697aa2">
    <skos:prefLabel xml:lang="en">iupacEntry</skos:prefLabel>
    <rdfs:comment xml:lang="en">DOI to corresponding concept in IUPAC</rdfs:comment>
    <rdf:type rdf:resource="http://www.w3.org/2002/07/owl#AnnotationProperty"/>
    <rdfs:range rdf:resource="http://www.w3.org/2001/XMLSchema#anyURI"/>
    <rdfs:subPropertyOf rdf:resource="http://www.w3.org/2000/01/rdf-schema#seeAlso"/>
    <rdfs:seeAlso rdf:datatype="http://www.w3.org/2001/XMLSchema#anyURI">https://goldbook.iupac.org/</rdfs:seeAlso>
  </rdf:Description>
  <rdf:Description rdf:nodeID="ffcb99037244f48d590430c228d02afdbb45">
    <rdf:type rdf:resource="http://www.w3.org/2002/07/owl#Restriction"/>
    <owl:onProperty rdf:resource="http://emmo.info/emmo#EMMO_23b579e1_8088_45b5_9975_064014026c42"/>
    <owl:hasValue>°</owl:hasValue>
  </rdf:Description>
  <rdf:Description rdf:nodeID="f05bdaa1e617a4bccafc519daf7bf4785b105">
    <owl:onProperty rdf:nodeID="f05bdaa1e617a4bccafc519daf7bf4785b106"/>
    <owl:allValuesFrom rdf:nodeID="f05bdaa1e617a4bccafc519daf7bf4785b107"/>
    <rdf:type rdf:resource="http://www.w3.org/2002/07/owl#Restriction"/>
  </rdf:Description>
  <rdf:Description rdf:nodeID="f05bdaa1e617a4bccafc519daf7bf4785b6">
    <rdf:type rdf:resource="http://www.w3.org/2002/07/owl#Restriction"/>
    <owl:hasValue>p</owl:hasValue>
    <owl:onProperty rdf:resource="http://emmo.info/emmo#EMMO_23b579e1_8088_45b5_9975_064014026c42"/>
  </rdf:Description>
  <rdf:Description rdf:about="http://emmo.info/emmo#EMMO_e9ffc696_5228_4ff9_8a60_0f5e05e9931b">
    <EMMO_967080e5_2f42_4eb2_a3a9_c58143e835f9 xml:lang="en">The 22 derived units that are given a special name in the SI system that stands for units derived by SI base units.</EMMO_967080e5_2f42_4eb2_a3a9_c58143e835f9>
    <EMMO_c84c6752_6d64_48cc_9500_e54a3c34898d>https://en.wikipedia.org/wiki/International_System_of_Units#Derived_units</EMMO_c84c6752_6d64_48cc_9500_e54a3c34898d>
    <skos:prefLabel xml:lang="en">SISpecialUnit</skos:prefLabel>
    <rdf:type rdf:resource="http://www.w3.org/2002/07/owl#Class"/>
    <rdfs:subClassOf rdf:resource="http://emmo.info/emmo#EMMO_3ee80521_3c23_4dd1_935d_9d522614a3e2"/>
    <rdfs:comment xml:lang="en">These units are SI coherent by definition.</rdfs:comment>
    <owl:disjointUnionOf rdf:nodeID="f05bdaa1e617a4bccafc519daf7bf4785b165"/>
  </rdf:Description>
  <rdf:Description rdf:about="http://emmo.info/emmo#EMMO_ed4af7ae_63a2_497e_bb88_2309619ea405">
    <EMMO_6dd685dd_1895_46e4_b227_be9f7d643c25>http://dbpedia.org/page/Mass</EMMO_6dd685dd_1895_46e4_b227_be9f7d643c25>
    <EMMO_967080e5_2f42_4eb2_a3a9_c58143e835f9 xml:lang="en">Property of a physical body that express its resistance to acceleration (a change in its state of motion) when a force is applied.</EMMO_967080e5_2f42_4eb2_a3a9_c58143e835f9>
    <rdfs:subClassOf rdf:nodeID="fe0b20157736f4a31909181349b2e6219b38"/>
    <rdf:type rdf:resource="http://www.w3.org/2002/07/owl#Class"/>
    <skos:prefLabel xml:lang="en">Mass</skos:prefLabel>
    <EMMO_1f1b164d_ec6a_4faa_8d5e_88bda62316cc>http://qudt.org/vocab/quantitykind/Mass</EMMO_1f1b164d_ec6a_4faa_8d5e_88bda62316cc>
    <EMMO_fe015383_afb3_44a6_ae86_043628697aa2>https://doi.org/10.1351/goldbook.M03709</EMMO_fe015383_afb3_44a6_ae86_043628697aa2>
    <EMMO_de178b12_5d35_4bca_8efa_a4193162571d>T0 L0 M+1 I0 Θ0 N0 J0</EMMO_de178b12_5d35_4bca_8efa_a4193162571d>
  </rdf:Description>
  <rdf:Description rdf:nodeID="ff14b31ebf90e4bc5ba2839064d29e543b12">
    <rdf:type rdf:resource="http://www.w3.org/1999/02/22-rdf-syntax-ns#List"/>
    <rdf:first rdf:resource="http://emmo.info/emmo#EMMO_c457b6b9_5e73_4853_ae08_d776c12b8058"/>
    <rdf:rest rdf:nodeID="ff14b31ebf90e4bc5ba2839064d29e543b13"/>
  </rdf:Description>
  <rdf:Description rdf:nodeID="fea11ca01461e402d8f697c19c5d8de88b20">
    <owl:unionOf rdf:nodeID="fea11ca01461e402d8f697c19c5d8de88b21"/>
    <rdf:type rdf:resource="http://www.w3.org/2002/07/owl#Class"/>
  </rdf:Description>
  <rdf:Description rdf:nodeID="f05bdaa1e617a4bccafc519daf7bf4785b147">
    <owl:someValuesFrom rdf:resource="http://emmo.info/emmo#EMMO_d5f3e0e5_fc7d_4e64_86ad_555e74aaff84"/>
    <rdf:type rdf:resource="http://www.w3.org/2002/07/owl#Restriction"/>
    <owl:onProperty rdf:resource="http://emmo.info/emmo#EMMO_bed1d005_b04e_4a90_94cf_02bc678a8569"/>
  </rdf:Description>
  <rdf:Description rdf:about="http://emmo.info/emmo#EMMO_a365b3c1_7bde_41d7_a15b_2820762e85f4">
    <skos:prefLabel xml:lang="en">Division</skos:prefLabel>
    <rdfs:subClassOf rdf:resource="http://emmo.info/emmo#EMMO_707f0cd1_941c_4b57_9f20_d0ba30cd6ff3"/>
    <rdf:type rdf:resource="http://www.w3.org/2002/07/owl#Class"/>
    <owl:equivalentClass rdf:nodeID="fe24a777e3fd743f986ce83488d2cf30bb22"/>
  </rdf:Description>
  <rdf:Description rdf:nodeID="f05bdaa1e617a4bccafc519daf7bf4785b176">
    <rdf:first rdf:resource="http://emmo.info/emmo#EMMO_b20be325_8bfd_4237_bee7_201ab0fd9c75"/>
    <rdf:type rdf:resource="http://www.w3.org/1999/02/22-rdf-syntax-ns#List"/>
    <rdf:rest rdf:nodeID="f05bdaa1e617a4bccafc519daf7bf4785b177"/>
  </rdf:Description>
  <rdf:Description rdf:nodeID="f05bdaa1e617a4bccafc519daf7bf4785b165">
    <rdf:first rdf:resource="http://emmo.info/emmo#EMMO_00199e76_69dc_45b6_a9c6_98cc90cdc0f5"/>
    <rdf:type rdf:resource="http://www.w3.org/1999/02/22-rdf-syntax-ns#List"/>
    <rdf:rest rdf:nodeID="f05bdaa1e617a4bccafc519daf7bf4785b166"/>
  </rdf:Description>
  <rdf:Description rdf:nodeID="f05bdaa1e617a4bccafc519daf7bf4785b59">
    <rdf:first rdf:resource="http://emmo.info/emmo#EMMO_21aaefc1_3f86_4208_b7db_a755f31f0f8c"/>
    <rdf:type rdf:resource="http://www.w3.org/1999/02/22-rdf-syntax-ns#List"/>
    <rdf:rest rdf:nodeID="f05bdaa1e617a4bccafc519daf7bf4785b60"/>
  </rdf:Description>
  <rdf:Description rdf:nodeID="f05bdaa1e617a4bccafc519daf7bf4785b179">
    <rdf:rest rdf:nodeID="f05bdaa1e617a4bccafc519daf7bf4785b180"/>
    <rdf:type rdf:resource="http://www.w3.org/1999/02/22-rdf-syntax-ns#List"/>
    <rdf:first rdf:resource="http://emmo.info/emmo#EMMO_d7b7fd1e_645a_42cb_8f40_85f0d034d3ae"/>
  </rdf:Description>
  <rdf:Description rdf:nodeID="fea11ca01461e402d8f697c19c5d8de88b18">
    <rdf:first rdf:resource="http://emmo.info/emmo#EMMO_8043d3c6_a4c1_4089_ba34_9744e28e5b3d"/>
    <rdf:rest rdf:nodeID="fea11ca01461e402d8f697c19c5d8de88b19"/>
    <rdf:type rdf:resource="http://www.w3.org/1999/02/22-rdf-syntax-ns#List"/>
  </rdf:Description>
  <rdf:Description rdf:nodeID="fea11ca01461e402d8f697c19c5d8de88b7">
    <owl:complementOf rdf:resource="http://emmo.info/emmo#EMMO_5b2222df_4da6_442f_8244_96e9e45887d1"/>
    <rdf:type rdf:resource="http://www.w3.org/2002/07/owl#Class"/>
  </rdf:Description>
  <rdf:Description rdf:nodeID="fea11ca01461e402d8f697c19c5d8de88b17">
    <rdf:first rdf:resource="http://emmo.info/emmo#EMMO_7db59e56_f68b_48b7_ae99_891c35ae5c3b"/>
    <rdf:type rdf:resource="http://www.w3.org/1999/02/22-rdf-syntax-ns#List"/>
    <rdf:rest rdf:nodeID="fea11ca01461e402d8f697c19c5d8de88b18"/>
  </rdf:Description>
  <rdf:Description rdf:about="http://emmo.info/emmo#EMMO_d6eb0176_a0d7_4b4e_8df0_50e912be2342">
    <EMMO_1f1b164d_ec6a_4faa_8d5e_88bda62316cc>http://qudt.org/vocab/unit/HA</EMMO_1f1b164d_ec6a_4faa_8d5e_88bda62316cc>
    <rdfs:subClassOf rdf:nodeID="ffcb99037244f48d590430c228d02afdbb49"/>
    <EMMO_6dd685dd_1895_46e4_b227_be9f7d643c25>http://dbpedia.org/page/Hectare</EMMO_6dd685dd_1895_46e4_b227_be9f7d643c25>
    <EMMO_70fe84ff_99b6_4206_a9fc_9a8931836d84 xml:lang="en">A non-SI metric unit of area defined as the square with 100-metre sides.</EMMO_70fe84ff_99b6_4206_a9fc_9a8931836d84>
    <rdfs:subClassOf rdf:nodeID="ffcb99037244f48d590430c228d02afdbb50"/>
    <skos:prefLabel xml:lang="en">Hectare</skos:prefLabel>
    <rdf:type rdf:resource="http://www.w3.org/2002/07/owl#Class"/>
    <rdfs:subClassOf rdf:resource="http://emmo.info/emmo#EMMO_591e02fd_8d37_45a6_9d11_bb21cef391a0"/>
    <EMMO_c84c6752_6d64_48cc_9500_e54a3c34898d>https://en.wikipedia.org/wiki/Hectare</EMMO_c84c6752_6d64_48cc_9500_e54a3c34898d>
  </rdf:Description>
  <rdf:Description rdf:about="http://emmo.info/emmo#EMMO_48716718_225f_4c88_89e2_d819d30c90a2">
    <rdfs:subClassOf rdf:resource="http://emmo.info/emmo#EMMO_d8d2144e_5c8d_455d_a643_5caf4d8d9df8"/>
    <skos:prefLabel xml:lang="en">Idiomatic</skos:prefLabel>
    <EMMO_967080e5_2f42_4eb2_a3a9_c58143e835f9 xml:lang="en">A language object that follows syntactic rules of a an idiom (e.g. english, italian).</EMMO_967080e5_2f42_4eb2_a3a9_c58143e835f9>
    <rdf:type rdf:resource="http://www.w3.org/2002/07/owl#Class"/>
  </rdf:Description>
  <rdf:Description rdf:nodeID="f05bdaa1e617a4bccafc519daf7bf4785b85">
    <owl:onProperty rdf:resource="http://emmo.info/emmo#EMMO_23b579e1_8088_45b5_9975_064014026c42"/>
    <rdf:type rdf:resource="http://www.w3.org/2002/07/owl#Restriction"/>
    <owl:hasValue>M</owl:hasValue>
  </rdf:Description>
  <rdf:Description rdf:about="http://emmo.info/emmo#EMMO_5e77f00d_5c0a_44e7_baf1_2c2a4cb5b3ae">
    <rdfs:subClassOf rdf:resource="http://emmo.info/emmo#EMMO_2031516a_2be7_48e8_9af7_7e1270e308fe"/>
    <rdf:type rdf:resource="http://www.w3.org/2002/07/owl#Class"/>
    <EMMO_967080e5_2f42_4eb2_a3a9_c58143e835f9 xml:lang="en">A solid solution made of two or more component substances.</EMMO_967080e5_2f42_4eb2_a3a9_c58143e835f9>
    <skos:prefLabel xml:lang="en">SolidSolution</skos:prefLabel>
    <rdfs:subClassOf rdf:resource="http://emmo.info/emmo#EMMO_a2b006f2_bbfd_4dba_bcaa_3fca20cd6be1"/>
  </rdf:Description>
  <rdf:Description rdf:nodeID="f3b8e3e5cecf14b688acdf306cd5f62cbb5">
    <owl:onProperty rdf:resource="http://emmo.info/emmo#EMMO_65a2c5b8_e4d8_4a51_b2f8_e55effc0547d"/>
    <rdf:type rdf:resource="http://www.w3.org/2002/07/owl#Restriction"/>
    <owl:someValuesFrom rdf:resource="http://emmo.info/emmo#EMMO_36c79456_e29c_400d_8bd3_0eedddb82652"/>
  </rdf:Description>
  <rdf:Description rdf:about="http://emmo.info/emmo#EMMO_1604f495_328a_4f28_9962_f4cc210739dd">
    <EMMO_de178b12_5d35_4bca_8efa_a4193162571d>T+1 L0 M0 I+1 Θ0 N0 J0</EMMO_de178b12_5d35_4bca_8efa_a4193162571d>
    <EMMO_1f1b164d_ec6a_4faa_8d5e_88bda62316cc>http://qudt.org/vocab/quantitykind/ElectricCharge</EMMO_1f1b164d_ec6a_4faa_8d5e_88bda62316cc>
    <rdf:type rdf:resource="http://www.w3.org/2002/07/owl#Class"/>
    <EMMO_6dd685dd_1895_46e4_b227_be9f7d643c25>http://dbpedia.org/page/Electric_charge</EMMO_6dd685dd_1895_46e4_b227_be9f7d643c25>
    <skos:prefLabel xml:lang="en">ElectricCharge</skos:prefLabel>
    <EMMO_fe015383_afb3_44a6_ae86_043628697aa2>https://doi.org/10.1351/goldbook.E01923</EMMO_fe015383_afb3_44a6_ae86_043628697aa2>
    <skos:altLabel xml:lang="en">Charge</skos:altLabel>
    <rdfs:subClassOf rdf:resource="http://emmo.info/emmo#EMMO_2946d40b_24a1_47fa_8176_e3f79bb45064"/>
    <EMMO_967080e5_2f42_4eb2_a3a9_c58143e835f9 xml:lang="en">The physical property of matter that causes it to experience a force when placed in an electromagnetic field.</EMMO_967080e5_2f42_4eb2_a3a9_c58143e835f9>
  </rdf:Description>
  <rdf:Description rdf:nodeID="f05bdaa1e617a4bccafc519daf7bf4785b98">
    <rdf:rest rdf:resource="http://www.w3.org/1999/02/22-rdf-syntax-ns#nil"/>
    <rdf:type rdf:resource="http://www.w3.org/1999/02/22-rdf-syntax-ns#List"/>
    <rdf:first rdf:resource="http://emmo.info/emmo#EMMO_d41ce84b_4317_41fb_a5d1_6cd281fca106"/>
  </rdf:Description>
  <rdf:Description rdf:about="http://emmo.info/emmo#EMMO_b0d1c460_d06b_4c7f_8832_148bc1c8e7dc">
    <EMMO_e55f2d7c_9893_48cd_b4a4_fdf38253bd20>http://www.ontology-of-units-of-measure.org/resource/om-2/squareMetre</EMMO_e55f2d7c_9893_48cd_b4a4_fdf38253bd20>
    <EMMO_1f1b164d_ec6a_4faa_8d5e_88bda62316cc>http://qudt.org/vocab/unit/M2</EMMO_1f1b164d_ec6a_4faa_8d5e_88bda62316cc>
    <rdfs:subClassOf rdf:nodeID="ffcb99037244f48d590430c228d02afdbb41"/>
    <rdf:type rdf:resource="http://www.w3.org/2002/07/owl#Class"/>
    <rdfs:subClassOf rdf:resource="http://emmo.info/emmo#EMMO_1273eb34_de48_43a9_925f_104110469dd2"/>
    <EMMO_967080e5_2f42_4eb2_a3a9_c58143e835f9 xml:lang="en">SI coherent measurement unit for area.</EMMO_967080e5_2f42_4eb2_a3a9_c58143e835f9>
    <skos:prefLabel xml:lang="en">SquareMetre</skos:prefLabel>
  </rdf:Description>
  <rdf:Description rdf:nodeID="fe0b20157736f4a31909181349b2e6219b15">
    <owl:hasValue>T-2 L+2 M+1 I-1 Θ0 N0 J0</owl:hasValue>
    <owl:onProperty rdf:resource="http://emmo.info/emmo#EMMO_23b579e1_8088_45b5_9975_064014026c42"/>
    <rdf:type rdf:resource="http://www.w3.org/2002/07/owl#Restriction"/>
  </rdf:Description>
  <rdf:Description rdf:nodeID="f8fb83657cd5f496db3c2b94baf326f26b35">
    <rdf:rest rdf:resource="http://www.w3.org/1999/02/22-rdf-syntax-ns#nil"/>
    <rdf:type rdf:resource="http://www.w3.org/1999/02/22-rdf-syntax-ns#List"/>
    <rdf:first rdf:resource="http://emmo.info/emmo#EMMO_7d2afa66_ae9e_4095_a9bf_421d0be401b6"/>
  </rdf:Description>
  <rdf:Description rdf:nodeID="ffcb99037244f48d590430c228d02afdbb54">
    <owl:onProperty rdf:resource="http://emmo.info/emmo#EMMO_bed1d005_b04e_4a90_94cf_02bc678a8569"/>
    <rdf:type rdf:resource="http://www.w3.org/2002/07/owl#Restriction"/>
    <owl:someValuesFrom rdf:resource="http://emmo.info/emmo#EMMO_1c2226a9_22f0_40c8_8928_5a01d398f96e"/>
  </rdf:Description>
  <rdf:Description rdf:nodeID="f05bdaa1e617a4bccafc519daf7bf4785b189">
    <owl:allValuesFrom rdf:nodeID="f05bdaa1e617a4bccafc519daf7bf4785b191"/>
    <owl:onProperty rdf:nodeID="f05bdaa1e617a4bccafc519daf7bf4785b190"/>
    <rdf:type rdf:resource="http://www.w3.org/2002/07/owl#Restriction"/>
  </rdf:Description>
  <rdf:Description rdf:nodeID="f05bdaa1e617a4bccafc519daf7bf4785b17">
    <rdf:type rdf:resource="http://www.w3.org/2002/07/owl#Restriction"/>
    <owl:onProperty rdf:nodeID="f05bdaa1e617a4bccafc519daf7bf4785b18"/>
    <owl:allValuesFrom rdf:nodeID="f05bdaa1e617a4bccafc519daf7bf4785b19"/>
  </rdf:Description>
  <rdf:Description rdf:about="http://emmo.info/emmo#EMMO_acaaa124_3dde_48b6_86e6_6ec6f364f408">
    <EMMO_967080e5_2f42_4eb2_a3a9_c58143e835f9 xml:lang="en">"Quantity in a conventionally chosen subset of a given system of quantities, where no quantity in the subset can be expressed in terms of the other quantities within that subset"
ISO 80000-1</EMMO_967080e5_2f42_4eb2_a3a9_c58143e835f9>
    <skos:prefLabel xml:lang="en">BaseQuantity</skos:prefLabel>
    <rdf:type rdf:resource="http://www.w3.org/2002/07/owl#Class"/>
    <rdfs:subClassOf rdf:nodeID="f8fb83657cd5f496db3c2b94baf326f26b26"/>
  </rdf:Description>
  <rdf:Description rdf:nodeID="f05bdaa1e617a4bccafc519daf7bf4785b126">
    <owl:onProperty rdf:resource="http://emmo.info/emmo#EMMO_23b579e1_8088_45b5_9975_064014026c42"/>
    <rdf:type rdf:resource="http://www.w3.org/2002/07/owl#Restriction"/>
    <owl:hasValue>T</owl:hasValue>
  </rdf:Description>
  <rdf:Description rdf:nodeID="ffcb99037244f48d590430c228d02afdbb53">
    <owl:onProperty rdf:resource="http://emmo.info/emmo#EMMO_67fc0a36_8dcb_4ffa_9a43_31074efa3296"/>
    <owl:allValuesFrom rdf:resource="http://emmo.info/emmo#EMMO_6f4d704a_a7c6_4c07_b8a7_ea0bab04128f"/>
    <rdf:type rdf:resource="http://www.w3.org/2002/07/owl#Restriction"/>
  </rdf:Description>
  <rdf:Description rdf:nodeID="f15a17d1fb53e4dd795c7db922ceff6acb5">
    <owl:inverseOf rdf:resource="http://emmo.info/emmo#EMMO_17e27c22_37e1_468c_9dd7_95e137f73e7f"/>
  </rdf:Description>
  <rdf:Description rdf:nodeID="f05bdaa1e617a4bccafc519daf7bf4785b183">
    <rdf:type rdf:resource="http://www.w3.org/1999/02/22-rdf-syntax-ns#List"/>
    <rdf:first rdf:resource="http://emmo.info/emmo#EMMO_e2207e91_02b0_4a8a_b13e_61d2a2a839f1"/>
    <rdf:rest rdf:nodeID="f05bdaa1e617a4bccafc519daf7bf4785b184"/>
  </rdf:Description>
  <rdf:Description rdf:nodeID="f05bdaa1e617a4bccafc519daf7bf4785b197">
    <rdf:rest rdf:nodeID="f05bdaa1e617a4bccafc519daf7bf4785b198"/>
    <rdf:type rdf:resource="http://www.w3.org/1999/02/22-rdf-syntax-ns#List"/>
    <rdf:first rdf:resource="http://emmo.info/emmo#EMMO_60b78cc3_6011_4134_95ab_956f56d4bdc1"/>
  </rdf:Description>
  <rdf:Description rdf:nodeID="ffcb99037244f48d590430c228d02afdbb59">
    <rdf:type rdf:resource="http://www.w3.org/2002/07/owl#Restriction"/>
    <owl:onProperty rdf:resource="http://emmo.info/emmo#EMMO_23b579e1_8088_45b5_9975_064014026c42"/>
    <owl:hasValue>g</owl:hasValue>
  </rdf:Description>
  <rdf:Description rdf:about="http://emmo.info/emmo#EMMO_3c218fbe_60c9_4597_8bcf_41eb1773af1f">
    <skos:prefLabel xml:lang="en">Vacuum</skos:prefLabel>
    <owl:equivalentClass rdf:nodeID="fea11ca01461e402d8f697c19c5d8de88b4"/>
    <rdf:type rdf:resource="http://www.w3.org/2002/07/owl#Class"/>
    <EMMO_967080e5_2f42_4eb2_a3a9_c58143e835f9 xml:lang="en">A 'Physical' with no 'Massive' parts.</EMMO_967080e5_2f42_4eb2_a3a9_c58143e835f9>
  </rdf:Description>
  <rdf:Description rdf:nodeID="f05bdaa1e617a4bccafc519daf7bf4785b187">
    <owl:someValuesFrom rdf:resource="http://emmo.info/emmo#EMMO_321af35f_f0cc_4a5c_b4fe_8c2c0303fb0c"/>
    <rdf:type rdf:resource="http://www.w3.org/2002/07/owl#Restriction"/>
    <owl:onProperty rdf:resource="http://emmo.info/emmo#EMMO_bed1d005_b04e_4a90_94cf_02bc678a8569"/>
  </rdf:Description>
  <rdf:Description rdf:nodeID="ffcb99037244f48d590430c228d02afdbb35">
    <owl:allValuesFrom rdf:resource="http://emmo.info/emmo#EMMO_18448443_dcf1_49b8_a321_cf46e2c393e1"/>
    <owl:onProperty rdf:resource="http://emmo.info/emmo#EMMO_67fc0a36_8dcb_4ffa_9a43_31074efa3296"/>
    <rdf:type rdf:resource="http://www.w3.org/2002/07/owl#Restriction"/>
  </rdf:Description>
  <rdf:Description rdf:nodeID="fe0b20157736f4a31909181349b2e6219b27">
    <rdf:type rdf:resource="http://www.w3.org/2002/07/owl#Restriction"/>
    <owl:onProperty rdf:resource="http://emmo.info/emmo#EMMO_23b579e1_8088_45b5_9975_064014026c42"/>
    <owl:hasValue>T0 L+3 M0 I0 Θ0 N0 J0</owl:hasValue>
  </rdf:Description>
  <rdf:Description rdf:nodeID="f05bdaa1e617a4bccafc519daf7bf4785b65">
    <rdf:first rdf:resource="http://emmo.info/emmo#EMMO_5cf9f86c_86f5_40c4_846d_60371f670e0a"/>
    <rdf:type rdf:resource="http://www.w3.org/1999/02/22-rdf-syntax-ns#List"/>
    <rdf:rest rdf:nodeID="f05bdaa1e617a4bccafc519daf7bf4785b66"/>
  </rdf:Description>
  <rdf:Description rdf:about="http://emmo.info/emmo#EMMO_297999d6_c9e4_4262_9536_bd524d1c6e21">
    <rdf:type rdf:resource="http://www.w3.org/2002/07/owl#ObjectProperty"/>
    <rdfs:subPropertyOf rdf:resource="http://emmo.info/emmo#EMMO_60577dea_9019_4537_ac41_80b0fb563d41"/>
    <rdfs:range rdf:resource="http://emmo.info/emmo#EMMO_0cd58641_824c_4851_907f_f4c3be76630c"/>
    <skos:prefLabel xml:lang="en">hasIndex</skos:prefLabel>
  </rdf:Description>
  <rdf:Description rdf:nodeID="fe24a777e3fd743f986ce83488d2cf30bb20">
    <owl:hasValue>+</owl:hasValue>
    <rdf:type rdf:resource="http://www.w3.org/2002/07/owl#Restriction"/>
    <owl:onProperty rdf:resource="http://emmo.info/emmo#EMMO_23b579e1_8088_45b5_9975_064014026c42"/>
  </rdf:Description>
  <rdf:Description rdf:about="http://emmo.info/emmo#EMMO_d8d2144e_5c8d_455d_a643_5caf4d8d9df8">
    <rdf:type rdf:resource="http://www.w3.org/2002/07/owl#Class"/>
    <EMMO_967080e5_2f42_4eb2_a3a9_c58143e835f9 xml:lang="en">A language object is a symbolic object respecting a specific language syntactic rules (a well-formed formula).</EMMO_967080e5_2f42_4eb2_a3a9_c58143e835f9>
    <skos:prefLabel xml:lang="en">Language</skos:prefLabel>
    <rdfs:subClassOf rdf:resource="http://emmo.info/emmo#EMMO_057e7d57_aff0_49de_911a_8861d85cef40"/>
  </rdf:Description>
  <rdf:Description rdf:about="http://emmo.info/emmo#EMMO_a80dc6f5_b1aa_41a7_a3a8_cd5040da2162">
    <rdfs:subClassOf rdf:nodeID="f05bdaa1e617a4bccafc519daf7bf4785b115"/>
    <skos:prefLabel xml:lang="en">Pascal</skos:prefLabel>
    <rdfs:subClassOf rdf:nodeID="f05bdaa1e617a4bccafc519daf7bf4785b116"/>
    <rdfs:comment xml:lang="en">Measurement unit for pressure.</rdfs:comment>
    <rdf:type rdf:resource="http://www.w3.org/2002/07/owl#Class"/>
    <EMMO_1f1b164d_ec6a_4faa_8d5e_88bda62316cc>http://qudt.org/vocab/unit/PA</EMMO_1f1b164d_ec6a_4faa_8d5e_88bda62316cc>
    <EMMO_fe015383_afb3_44a6_ae86_043628697aa2>https://doi.org/10.1351/goldbook.P04442</EMMO_fe015383_afb3_44a6_ae86_043628697aa2>
  </rdf:Description>
  <rdf:Description rdf:nodeID="f05bdaa1e617a4bccafc519daf7bf4785b109">
    <rdf:type rdf:resource="http://www.w3.org/2002/07/owl#Restriction"/>
    <owl:onProperty rdf:resource="http://emmo.info/emmo#EMMO_bed1d005_b04e_4a90_94cf_02bc678a8569"/>
    <owl:someValuesFrom rdf:resource="http://emmo.info/emmo#EMMO_3227b821_26a5_4c7c_9c01_5c24483e0bd0"/>
  </rdf:Description>
  <rdf:Description rdf:about="http://emmo.info/emmo#EMMO_43a6b269_da31_4bb6_a537_c97df4fff32a">
    <rdfs:subClassOf rdf:nodeID="f05bdaa1e617a4bccafc519daf7bf4785b52"/>
    <rdf:type rdf:resource="http://www.w3.org/2002/07/owl#Class"/>
    <rdfs:subClassOf rdf:nodeID="f05bdaa1e617a4bccafc519daf7bf4785b55"/>
    <skos:prefLabel xml:lang="en">Peta</skos:prefLabel>
  </rdf:Description>
  <rdf:Description rdf:about="http://emmo.info/emmo#EMMO_a817035a_3e3c_4709_8ede_3205df3031a3">
    <skos:prefLabel xml:lang="en">Punctuation</skos:prefLabel>
    <rdf:type rdf:resource="http://www.w3.org/2002/07/owl#Class"/>
    <rdfs:subClassOf rdf:resource="http://emmo.info/emmo#EMMO_a1083d0a_c1fb_471f_8e20_a98f881ad527"/>
  </rdf:Description>
  <rdf:Description rdf:nodeID="fea11ca01461e402d8f697c19c5d8de88b19">
    <rdf:type rdf:resource="http://www.w3.org/1999/02/22-rdf-syntax-ns#List"/>
    <rdf:rest rdf:resource="http://www.w3.org/1999/02/22-rdf-syntax-ns#nil"/>
    <rdf:first rdf:resource="http://emmo.info/emmo#EMMO_eb3c61f0_3983_4346_a0c6_e7f6b90a67a8"/>
  </rdf:Description>
  <rdf:Description rdf:nodeID="fe0b20157736f4a31909181349b2e6219b31">
    <owl:hasValue>T+4 L-2 M-1 I+2 Θ0 N0 J0</owl:hasValue>
    <owl:onProperty rdf:resource="http://emmo.info/emmo#EMMO_23b579e1_8088_45b5_9975_064014026c42"/>
    <rdf:type rdf:resource="http://www.w3.org/2002/07/owl#Restriction"/>
  </rdf:Description>
  <rdf:Description rdf:nodeID="fe24a777e3fd743f986ce83488d2cf30bb28">
    <owl:onProperty rdf:resource="http://emmo.info/emmo#EMMO_faf79f53_749d_40b2_807c_d34244c192f4"/>
    <owl:allValuesFrom rdf:resource="http://www.w3.org/2001/XMLSchema#integer"/>
    <rdf:type rdf:resource="http://www.w3.org/2002/07/owl#Restriction"/>
  </rdf:Description>
  <rdf:Description rdf:about="http://emmo.info/emmo#EMMO_c9c8f824_9127_4f93_bc21_69fe78a7f6f2">
    <EMMO_b432d2d5_25f4_4165_99c5_5935a7763c1a xml:lang="en">Rockwell C hardness of a given sample (150 kg load): 43.5HRC(150 kg)</EMMO_b432d2d5_25f4_4165_99c5_5935a7763c1a>
    <rdfs:subClassOf rdf:resource="http://emmo.info/emmo#EMMO_18ce5200_00f5_45bb_8c6f_6fb128cd41ae"/>
    <rdf:type rdf:resource="http://www.w3.org/2002/07/owl#Class"/>
    <skos:prefLabel xml:lang="en">ProcedureUnit</skos:prefLabel>
    <EMMO_967080e5_2f42_4eb2_a3a9_c58143e835f9 xml:lang="en">A reference unit provided by a measurement procedure.</EMMO_967080e5_2f42_4eb2_a3a9_c58143e835f9>
  </rdf:Description>
  <rdf:Description rdf:nodeID="f05bdaa1e617a4bccafc519daf7bf4785b13">
    <owl:onProperty rdf:nodeID="f05bdaa1e617a4bccafc519daf7bf4785b14"/>
    <rdf:type rdf:resource="http://www.w3.org/2002/07/owl#Restriction"/>
    <owl:allValuesFrom rdf:nodeID="f05bdaa1e617a4bccafc519daf7bf4785b15"/>
  </rdf:Description>
  <rdf:Description rdf:nodeID="fea11ca01461e402d8f697c19c5d8de88b10">
    <owl:onProperty rdf:resource="http://emmo.info/emmo#EMMO_17e27c22_37e1_468c_9dd7_95e137f73e7f"/>
    <owl:someValuesFrom rdf:resource="http://emmo.info/emmo#EMMO_e5488299_8dab_4ebb_900a_26d2abed8396"/>
    <rdf:type rdf:resource="http://www.w3.org/2002/07/owl#Restriction"/>
  </rdf:Description>
  <rdf:Description rdf:about="http://emmo.info/emmo#EMMO_0a318776_b067_4de0_a2a6_cba2cf6333f8">
    <owl:equivalentClass rdf:nodeID="f8fb83657cd5f496db3c2b94baf326f26b4"/>
    <rdf:type rdf:resource="http://www.w3.org/2002/07/owl#Class"/>
    <skos:prefLabel xml:lang="en">IdiomaticSymbol</skos:prefLabel>
  </rdf:Description>
  <rdf:Description rdf:nodeID="ffcb99037244f48d590430c228d02afdbb43">
    <rdf:type rdf:resource="http://www.w3.org/2002/07/owl#Restriction"/>
    <owl:onProperty rdf:resource="http://emmo.info/emmo#EMMO_23b579e1_8088_45b5_9975_064014026c42"/>
    <owl:hasValue>Np</owl:hasValue>
  </rdf:Description>
  <rdf:Description rdf:nodeID="f15a17d1fb53e4dd795c7db922ceff6acb3">
    <rdf:type rdf:resource="http://www.w3.org/2002/07/owl#Restriction"/>
    <owl:onProperty rdf:resource="http://emmo.info/emmo#EMMO_17e27c22_37e1_468c_9dd7_95e137f73e7f"/>
    <owl:someValuesFrom rdf:resource="http://emmo.info/emmo#EMMO_3f9ae00e_810c_4518_aec2_7200e424cf68"/>
  </rdf:Description>
  <rdf:Description rdf:nodeID="f05bdaa1e617a4bccafc519daf7bf4785b157">
    <owl:someValuesFrom rdf:resource="http://emmo.info/emmo#EMMO_2e7e5796_4a80_4d73_bb84_f31138446c0c"/>
    <rdf:type rdf:resource="http://www.w3.org/2002/07/owl#Restriction"/>
    <owl:onProperty rdf:resource="http://emmo.info/emmo#EMMO_bed1d005_b04e_4a90_94cf_02bc678a8569"/>
  </rdf:Description>
  <rdf:Description rdf:about="http://emmo.info/emmo#EMMO_8246541a_f1f6_4d03_8bd7_fc6b76d17375">
    <skos:prefLabel xml:lang="en">SINonCoherentUnit</skos:prefLabel>
    <owl:disjointUnionOf rdf:nodeID="f05bdaa1e617a4bccafc519daf7bf4785b97"/>
    <rdf:type rdf:resource="http://www.w3.org/2002/07/owl#Class"/>
  </rdf:Description>
  <rdf:Description rdf:about="http://emmo.info/emmo#EMMO_42955b2d_b465_4666_86cc_ea3c2d685753">
    <rdf:type rdf:resource="http://www.w3.org/2002/07/owl#Class"/>
    <rdfs:subClassOf rdf:nodeID="f05bdaa1e617a4bccafc519daf7bf4785b51"/>
    <skos:prefLabel xml:lang="en">Atto</skos:prefLabel>
    <rdfs:subClassOf rdf:nodeID="f05bdaa1e617a4bccafc519daf7bf4785b48"/>
  </rdf:Description>
  <rdf:Description rdf:about="http://emmo.info/emmo#EMMO_1f5e3e7e_72c9_40d4_91dd_ae432d7b7018">
    <rdfs:subClassOf rdf:resource="http://emmo.info/emmo#EMMO_6c487fb3_03d1_4e56_91ed_c2e16dcbef60"/>
    <skos:prefLabel xml:lang="en">Foam</skos:prefLabel>
    <EMMO_967080e5_2f42_4eb2_a3a9_c58143e835f9 xml:lang="en">A colloid formed by trapping pockets of gas in a liquid or solid.</EMMO_967080e5_2f42_4eb2_a3a9_c58143e835f9>
    <rdf:type rdf:resource="http://www.w3.org/2002/07/owl#Class"/>
  </rdf:Description>
  <rdf:Description rdf:nodeID="f05bdaa1e617a4bccafc519daf7bf4785b48">
    <owl:allValuesFrom rdf:nodeID="f05bdaa1e617a4bccafc519daf7bf4785b50"/>
    <rdf:type rdf:resource="http://www.w3.org/2002/07/owl#Restriction"/>
    <owl:onProperty rdf:nodeID="f05bdaa1e617a4bccafc519daf7bf4785b49"/>
  </rdf:Description>
  <rdf:Description rdf:about="http://www.w3.org/2000/01/rdf-schema#seeAlso">
    <rdfs:comment xml:lang="en">Indicate a resource that might provide additional information about the subject resource.</rdfs:comment>
    <rdfs:comment xml:lang="en">EMMO applies the naming convension to its sub-properties of rdfs:seeAlso that their label must end with one of the following terms:
  - 'Match': resolvable URLs to corresponding entity in another ontology
  - 'Entry': resolvable URLs to a human readable resource describing the subject
  - 'Ref': non-resolvable reference to a human readable resource describing the subject</rdfs:comment>
  </rdf:Description>
  <rdf:Description rdf:about="http://emmo.info/emmo#EMMO_3a204900_2b33_47d1_b444_815cc4c8cffa">
    <skos:prefLabel xml:lang="en">Tera</skos:prefLabel>
    <rdfs:subClassOf rdf:nodeID="f05bdaa1e617a4bccafc519daf7bf4785b47"/>
    <rdf:type rdf:resource="http://www.w3.org/2002/07/owl#Class"/>
    <rdfs:subClassOf rdf:nodeID="f05bdaa1e617a4bccafc519daf7bf4785b44"/>
  </rdf:Description>
  <rdf:Description rdf:about="http://emmo.info/emmo#EMMO_46f0f8df_4dc6_418f_8036_10427a3a288e">
    <skos:prefLabel xml:lang="en">3-manifold</skos:prefLabel>
    <rdfs:subClassOf rdf:resource="http://emmo.info/emmo#EMMO_b5957cef_a287_442d_a3ce_fd39f20ba1cd"/>
    <rdf:type rdf:resource="http://www.w3.org/2002/07/owl#Class"/>
  </rdf:Description>
  <rdf:Description rdf:about="http://emmo.info/emmo#EMMO_f5769206_9257_4b08_bf7b_dad7868c6afc">
    <skos:prefLabel xml:lang="en">Yocto</skos:prefLabel>
    <rdfs:subClassOf rdf:nodeID="f05bdaa1e617a4bccafc519daf7bf4785b189"/>
    <rdfs:subClassOf rdf:nodeID="f05bdaa1e617a4bccafc519daf7bf4785b192"/>
    <rdf:type rdf:resource="http://www.w3.org/2002/07/owl#Class"/>
  </rdf:Description>
  <rdf:Description rdf:about="http://emmo.info/emmo#EMMO_5eaecadc_4f0d_4a3a_afc7_1fc0b83cc928">
    <rdfs:subClassOf rdf:nodeID="f05bdaa1e617a4bccafc519daf7bf4785b82"/>
    <rdf:type rdf:resource="http://www.w3.org/2002/07/owl#Class"/>
    <skos:prefLabel xml:lang="en">Mega</skos:prefLabel>
    <rdfs:subClassOf rdf:nodeID="f05bdaa1e617a4bccafc519daf7bf4785b85"/>
  </rdf:Description>
  <rdf:Description rdf:about="http://emmo.info/emmo#EMMO_4b3afb22_27cf_4ce3_88bc_492bfccb546b">
    <skos:prefLabel xml:lang="en">Acoustical</skos:prefLabel>
    <rdfs:comment xml:lang="en">'acoustical' refers to the perception mechanism of the observer that can occur through a microphone, a ear.</rdfs:comment>
    <rdf:type rdf:resource="http://www.w3.org/2002/07/owl#Class"/>
    <EMMO_967080e5_2f42_4eb2_a3a9_c58143e835f9 xml:lang="en">A 'Perceptual' which stands for a real world object whose spatiotemporal pattern makes it identifiable by an observer as a sound.</EMMO_967080e5_2f42_4eb2_a3a9_c58143e835f9>
    <rdfs:subClassOf rdf:resource="http://emmo.info/emmo#EMMO_649bf97b_4397_4005_90d9_219755d92e34"/>
  </rdf:Description>
  <rdf:Description rdf:about="http://emmo.info/emmo#EMMO_f6070071_d054_4b17_9d2d_f446f7147d0f">
    <rdf:type rdf:resource="http://www.w3.org/2002/07/owl#Class"/>
    <skos:prefLabel xml:lang="en">EnergyDimension</skos:prefLabel>
    <rdfs:subClassOf rdf:resource="http://emmo.info/emmo#EMMO_9895a1b4_f0a5_4167_ac5e_97db40b8bfcc"/>
    <owl:equivalentClass rdf:nodeID="fe0b20157736f4a31909181349b2e6219b40"/>
  </rdf:Description>
  <rdf:Description rdf:nodeID="f0b819106611c4b798f33b16c65f4398db5">
    <owl:onProperty rdf:nodeID="f0b819106611c4b798f33b16c65f4398db6"/>
    <rdf:type rdf:resource="http://www.w3.org/2002/07/owl#Restriction"/>
    <owl:someValuesFrom rdf:resource="http://emmo.info/emmo#EMMO_43e9a05d_98af_41b4_92f6_00f79a09bfce"/>
  </rdf:Description>
  <rdf:Description rdf:nodeID="f05bdaa1e617a4bccafc519daf7bf4785b33">
    <rdf:rest rdf:nodeID="f05bdaa1e617a4bccafc519daf7bf4785b34"/>
    <rdf:first rdf:resource="http://emmo.info/emmo#EMMO_3a185e6c_9e19_4776_b583_19c978156aa0"/>
    <rdf:type rdf:resource="http://www.w3.org/1999/02/22-rdf-syntax-ns#List"/>
  </rdf:Description>
  <rdf:Description rdf:nodeID="f627ff42579444148ae27fcacfb5f8528b5">
    <owl:someValuesFrom rdf:resource="http://emmo.info/emmo#EMMO_c5ddfdba_c074_4aa4_ad6b_1ac4942d300d"/>
    <owl:onProperty rdf:nodeID="f627ff42579444148ae27fcacfb5f8528b6"/>
    <rdf:type rdf:resource="http://www.w3.org/2002/07/owl#Restriction"/>
  </rdf:Description>
  <rdf:Description rdf:nodeID="ffcb99037244f48d590430c228d02afdbb37">
    <owl:onProperty rdf:resource="http://emmo.info/emmo#EMMO_bed1d005_b04e_4a90_94cf_02bc678a8569"/>
    <owl:someValuesFrom rdf:resource="http://emmo.info/emmo#EMMO_9141801c_c539_4c72_b423_8c74ff6b8f05"/>
    <rdf:type rdf:resource="http://www.w3.org/2002/07/owl#Restriction"/>
  </rdf:Description>
  <rdf:Description rdf:nodeID="f05bdaa1e617a4bccafc519daf7bf4785b145">
    <owl:onProperty rdf:resource="http://emmo.info/emmo#EMMO_faf79f53_749d_40b2_807c_d34244c192f4"/>
    <owl:hasValue rdf:datatype="http://www.w3.org/2001/XMLSchema#double">1e+21</owl:hasValue>
    <rdf:type rdf:resource="http://www.w3.org/2002/07/owl#Restriction"/>
  </rdf:Description>
  <rdf:Description rdf:about="http://emmo.info/emmo#EMMO_99dba333_0dbd_4f75_8841_8c0f97fd58e2">
    <skos:prefLabel xml:lang="en">Capacitance</skos:prefLabel>
    <skos:altLabel xml:lang="en">ElectricCapacitance</skos:altLabel>
    <EMMO_de178b12_5d35_4bca_8efa_a4193162571d>T+4 L-2 M-1 I+2 Θ0 N0 J0</EMMO_de178b12_5d35_4bca_8efa_a4193162571d>
    <EMMO_6dd685dd_1895_46e4_b227_be9f7d643c25>http://dbpedia.org/page/Capacitance</EMMO_6dd685dd_1895_46e4_b227_be9f7d643c25>
    <rdfs:subClassOf rdf:resource="http://emmo.info/emmo#EMMO_2946d40b_24a1_47fa_8176_e3f79bb45064"/>
    <rdf:type rdf:resource="http://www.w3.org/2002/07/owl#Class"/>
    <EMMO_1f1b164d_ec6a_4faa_8d5e_88bda62316cc>http://qudt.org/vocab/quantitykind/Capacitance</EMMO_1f1b164d_ec6a_4faa_8d5e_88bda62316cc>
    <EMMO_967080e5_2f42_4eb2_a3a9_c58143e835f9 xml:lang="en">The derivative of the electric charge of a system with respect to the electric potential.</EMMO_967080e5_2f42_4eb2_a3a9_c58143e835f9>
    <EMMO_fe015383_afb3_44a6_ae86_043628697aa2>https://doi.org/10.1351/goldbook.C00791</EMMO_fe015383_afb3_44a6_ae86_043628697aa2>
  </rdf:Description>
  <rdf:Description rdf:about="http://emmo.info/emmo#EMMO_ec2c8ac8_98c5_4c74_b85b_ff8e8ca6655c">
    <rdfs:subClassOf rdf:resource="http://emmo.info/emmo#EMMO_8b0923ab_b500_477b_9ce9_8b3a3e4dc4f2"/>
    <EMMO_967080e5_2f42_4eb2_a3a9_c58143e835f9 xml:lang="en">A Miixture is a material made up of two or more different substances which are physically (not chemically) combined.</EMMO_967080e5_2f42_4eb2_a3a9_c58143e835f9>
    <rdf:type rdf:resource="http://www.w3.org/2002/07/owl#Class"/>
    <skos:prefLabel xml:lang="en">Mixture</skos:prefLabel>
  </rdf:Description>
  <rdf:Description rdf:about="http://emmo.info/emmo#EMMO_b4895f75_41c8_4fd9_b6d6_4d5f7c99c423">
    <EMMO_fe015383_afb3_44a6_ae86_043628697aa2>https://doi.org/10.1351/goldbook.M03683</EMMO_fe015383_afb3_44a6_ae86_043628697aa2>
    <rdf:type rdf:resource="http://www.w3.org/2002/07/owl#Class"/>
    <rdfs:comment xml:lang="en">Strength of a magnetic field. Commonly denoted H.</rdfs:comment>
    <EMMO_de178b12_5d35_4bca_8efa_a4193162571d>T0 L-1 M0 I+1 Θ0 N0 J0</EMMO_de178b12_5d35_4bca_8efa_a4193162571d>
    <skos:prefLabel xml:lang="en">MagneticFieldStrength</skos:prefLabel>
    <EMMO_6dd685dd_1895_46e4_b227_be9f7d643c25>http://dbpedia.org/page/Magnetic_field</EMMO_6dd685dd_1895_46e4_b227_be9f7d643c25>
    <EMMO_1f1b164d_ec6a_4faa_8d5e_88bda62316cc>http://qudt.org/vocab/quantitykind/MagneticFieldStrength</EMMO_1f1b164d_ec6a_4faa_8d5e_88bda62316cc>
    <rdfs:subClassOf rdf:resource="http://emmo.info/emmo#EMMO_2946d40b_24a1_47fa_8176_e3f79bb45064"/>
  </rdf:Description>
  <rdf:Description rdf:nodeID="f05bdaa1e617a4bccafc519daf7bf4785b86">
    <rdf:type rdf:resource="http://www.w3.org/2002/07/owl#Restriction"/>
    <owl:someValuesFrom rdf:resource="http://emmo.info/emmo#EMMO_ab79e92b_5377_454d_be06_d61b50db295a"/>
    <owl:onProperty rdf:resource="http://emmo.info/emmo#EMMO_bed1d005_b04e_4a90_94cf_02bc678a8569"/>
  </rdf:Description>
  <rdf:Description rdf:nodeID="f38ecd0eaa78747b4ad569754ea441153b1">
    <owl:onProperty rdf:resource="http://emmo.info/emmo#EMMO_b2282816_b7a3_44c6_b2cb_3feff1ceb7fe"/>
    <owl:someValuesFrom rdf:resource="http://emmo.info/emmo#EMMO_a1083d0a_c1fb_471f_8e20_a98f881ad527"/>
    <rdf:type rdf:resource="http://www.w3.org/2002/07/owl#Restriction"/>
  </rdf:Description>
  <rdf:Description rdf:about="http://emmo.info/emmo#EMMO_5be83f9c_a4ba_4b9a_be1a_5bfc6e891231">
    <rdf:type rdf:resource="http://www.w3.org/2002/07/owl#Class"/>
    <skos:prefLabel xml:lang="en">MathematicalSymbol</skos:prefLabel>
    <rdfs:subClassOf rdf:nodeID="fe24a777e3fd743f986ce83488d2cf30bb16"/>
    <owl:equivalentClass rdf:nodeID="fe24a777e3fd743f986ce83488d2cf30bb13"/>
  </rdf:Description>
  <rdf:Description rdf:nodeID="f8fb83657cd5f496db3c2b94baf326f26b30">
    <rdf:rest rdf:nodeID="f8fb83657cd5f496db3c2b94baf326f26b31"/>
    <rdf:first rdf:resource="http://emmo.info/emmo#EMMO_3f15d200_c97b_42c8_8ac0_d81d150361e2"/>
    <rdf:type rdf:resource="http://www.w3.org/1999/02/22-rdf-syntax-ns#List"/>
  </rdf:Description>
  <rdf:Description rdf:about="http://emmo.info/emmo#EMMO_068c4e58_2470_4b1c_8454_010dd4906100">
    <rdf:type rdf:resource="http://www.w3.org/2002/07/owl#Class"/>
    <rdfs:subClassOf rdf:nodeID="f05bdaa1e617a4bccafc519daf7bf4785b3"/>
    <skos:prefLabel xml:lang="en">Pico</skos:prefLabel>
    <rdfs:subClassOf rdf:nodeID="f05bdaa1e617a4bccafc519daf7bf4785b6"/>
  </rdf:Description>
  <rdf:Description rdf:nodeID="f05bdaa1e617a4bccafc519daf7bf4785b163">
    <owl:onProperty rdf:resource="http://emmo.info/emmo#EMMO_faf79f53_749d_40b2_807c_d34244c192f4"/>
    <rdf:type rdf:resource="http://www.w3.org/2002/07/owl#Restriction"/>
    <owl:hasValue rdf:datatype="http://www.w3.org/2001/XMLSchema#double">1e+24</owl:hasValue>
  </rdf:Description>
  <rdf:Description rdf:nodeID="f05bdaa1e617a4bccafc519daf7bf4785b164">
    <owl:hasValue>Y</owl:hasValue>
    <rdf:type rdf:resource="http://www.w3.org/2002/07/owl#Restriction"/>
    <owl:onProperty rdf:resource="http://emmo.info/emmo#EMMO_23b579e1_8088_45b5_9975_064014026c42"/>
  </rdf:Description>
  <rdf:Description rdf:about="http://emmo.info/emmo#EMMO_f7ed665b_c2e1_42bc_889b_6b42ed3a36f0">
    <skos:prefLabel xml:lang="en">MathematicalModel</skos:prefLabel>
    <owl:equivalentClass rdf:nodeID="f627ff42579444148ae27fcacfb5f8528b10"/>
    <rdf:type rdf:resource="http://www.w3.org/2002/07/owl#Class"/>
    <rdfs:comment xml:lang="en">A mathematical model can be defined as a description of a system using mathematical concepts and language to facilitate proper explanation of a system or to study the effects of different components and to make predictions on patterns of behaviour. 

Abramowitz and Stegun, 1968</rdfs:comment>
  </rdf:Description>
  <rdf:Description rdf:nodeID="f05bdaa1e617a4bccafc519daf7bf4785b7">
    <rdf:type rdf:resource="http://www.w3.org/2002/07/owl#Restriction"/>
    <owl:onProperty rdf:resource="http://emmo.info/emmo#EMMO_bed1d005_b04e_4a90_94cf_02bc678a8569"/>
    <owl:someValuesFrom rdf:resource="http://emmo.info/emmo#EMMO_c8d084ad_f88e_4596_8e4d_982c6655ce6f"/>
  </rdf:Description>
  <rdf:Description rdf:about="http://emmo.info/emmo#EMMO_b8830065_3809_41b7_be3c_e33795567fd9">
    <rdfs:subClassOf rdf:nodeID="ffcb99037244f48d590430c228d02afdbb45"/>
    <rdfs:subClassOf rdf:nodeID="ffcb99037244f48d590430c228d02afdbb44"/>
    <rdf:type rdf:resource="http://www.w3.org/2002/07/owl#Class"/>
    <EMMO_fe015383_afb3_44a6_ae86_043628697aa2>https://doi.org/10.1351/goldbook.D01560</EMMO_fe015383_afb3_44a6_ae86_043628697aa2>
    <rdfs:subClassOf rdf:resource="http://emmo.info/emmo#EMMO_591e02fd_8d37_45a6_9d11_bb21cef391a0"/>
    <EMMO_6dd685dd_1895_46e4_b227_be9f7d643c25>http://dbpedia.org/page/Degree_(angle)</EMMO_6dd685dd_1895_46e4_b227_be9f7d643c25>
    <EMMO_70fe84ff_99b6_4206_a9fc_9a8931836d84 xml:lang="en">Degree is a measurement of plane angle, defined by representing a full rotation as 360 degrees.</EMMO_70fe84ff_99b6_4206_a9fc_9a8931836d84>
    <EMMO_1f1b164d_ec6a_4faa_8d5e_88bda62316cc>http://qudt.org/vocab/unit/DEG</EMMO_1f1b164d_ec6a_4faa_8d5e_88bda62316cc>
    <skos:prefLabel xml:lang="en">Degree</skos:prefLabel>
  </rdf:Description>
  <rdf:Description rdf:nodeID="f627ff42579444148ae27fcacfb5f8528b8">
    <rdf:type rdf:resource="http://www.w3.org/2002/07/owl#Restriction"/>
    <owl:someValuesFrom rdf:resource="http://emmo.info/emmo#EMMO_e5438930_04e7_4d42_ade5_3700d4a52ab7"/>
    <owl:onProperty rdf:resource="http://emmo.info/emmo#EMMO_f68030be_94b8_4c61_a161_886468558054"/>
  </rdf:Description>
  <rdf:Description rdf:nodeID="f8fb83657cd5f496db3c2b94baf326f26b10">
    <rdf:first rdf:resource="http://emmo.info/emmo#EMMO_3ee80521_3c23_4dd1_935d_9d522614a3e2"/>
    <rdf:type rdf:resource="http://www.w3.org/1999/02/22-rdf-syntax-ns#List"/>
    <rdf:rest rdf:nodeID="f8fb83657cd5f496db3c2b94baf326f26b11"/>
  </rdf:Description>
  <rdf:Description rdf:about="http://emmo.info/emmo#EMMO_60b78cc3_6011_4134_95ab_956f56d4bdc1">
    <rdf:type rdf:resource="http://www.w3.org/2002/07/owl#Class"/>
    <skos:prefLabel xml:lang="en">SINonCoherentDerivedUnit</skos:prefLabel>
    <EMMO_967080e5_2f42_4eb2_a3a9_c58143e835f9 xml:lang="en">A derived unit whos numerical factor in front of the product of base units is NOT equal to one.</EMMO_967080e5_2f42_4eb2_a3a9_c58143e835f9>
  </rdf:Description>
  <rdf:Description rdf:nodeID="ff14b31ebf90e4bc5ba2839064d29e543b3">
    <rdf:rest rdf:resource="http://www.w3.org/1999/02/22-rdf-syntax-ns#nil"/>
    <rdf:first rdf:resource="http://emmo.info/emmo#EMMO_6c487fb3_03d1_4e56_91ed_c2e16dcbef60"/>
    <rdf:type rdf:resource="http://www.w3.org/1999/02/22-rdf-syntax-ns#List"/>
  </rdf:Description>
  <rdf:Description rdf:about="http://www.w3.org/2000/01/rdf-schema#isDefinedBy">
    <rdfs:subPropertyOf rdf:resource="http://www.w3.org/2000/01/rdf-schema#seeAlso"/>
  </rdf:Description>
  <rdf:Description rdf:nodeID="f8fb83657cd5f496db3c2b94baf326f26b18">
    <owl:onProperty rdf:resource="http://emmo.info/emmo#EMMO_9380ab64_0363_4804_b13f_3a8a94119a76"/>
    <owl:allValuesFrom rdf:nodeID="f8fb83657cd5f496db3c2b94baf326f26b19"/>
    <rdf:type rdf:resource="http://www.w3.org/2002/07/owl#Restriction"/>
  </rdf:Description>
  <rdf:Description rdf:nodeID="fe0b20157736f4a31909181349b2e6219b18">
    <owl:onProperty rdf:resource="http://emmo.info/emmo#EMMO_23b579e1_8088_45b5_9975_064014026c42"/>
    <rdf:type rdf:resource="http://www.w3.org/2002/07/owl#Restriction"/>
    <owl:hasValue>T-1 L0 M0 I0 Θ0 N0 J0</owl:hasValue>
  </rdf:Description>
  <rdf:Description rdf:nodeID="fe24a777e3fd743f986ce83488d2cf30bb10">
    <owl:someValuesFrom rdf:resource="http://www.w3.org/2001/XMLSchema#boolean"/>
    <rdf:type rdf:resource="http://www.w3.org/2002/07/owl#Restriction"/>
    <owl:onProperty rdf:resource="http://emmo.info/emmo#EMMO_faf79f53_749d_40b2_807c_d34244c192f4"/>
  </rdf:Description>
  <rdf:Description rdf:nodeID="f05bdaa1e617a4bccafc519daf7bf4785b1">
    <owl:onProperty rdf:resource="http://emmo.info/emmo#EMMO_bed1d005_b04e_4a90_94cf_02bc678a8569"/>
    <owl:someValuesFrom rdf:resource="http://emmo.info/emmo#EMMO_847f1d9f_205e_46c1_8cb6_a9e479421f88"/>
    <rdf:type rdf:resource="http://www.w3.org/2002/07/owl#Restriction"/>
  </rdf:Description>
  <rdf:Description rdf:about="http://emmo.info/emmo#EMMO_eb77076b_a104_42ac_a065_798b2d2809ad">
    <rdfs:subClassOf rdf:nodeID="ff14b31ebf90e4bc5ba2839064d29e543b24"/>
    <rdfs:subClassOf rdf:nodeID="ff14b31ebf90e4bc5ba2839064d29e543b23"/>
    <EMMO_967080e5_2f42_4eb2_a3a9_c58143e835f9 xml:lang="en">A standalone atom has direct part one 'nucleus' and one 'electron_cloud'. 

An O 'atom' within an O2 'molecule' is an 'e-bonded_atom'.

In this material branch, H atom is a particular case, with respect to higher atomic number atoms, since as soon as it shares its electron it has no nucleus entangled electron cloud.

We cannot say that H2 molecule has direct part two H atoms, but has direct part two H nucleus.</EMMO_967080e5_2f42_4eb2_a3a9_c58143e835f9>
    <rdf:type rdf:resource="http://www.w3.org/2002/07/owl#Class"/>
    <rdfs:comment xml:lang="en">An 'atom' is a 'nucleus' surrounded by an 'electron_cloud', i.e. a quantum system made of one or more bounded electrons.</rdfs:comment>
    <skos:prefLabel xml:lang="en">Atom</skos:prefLabel>
    <rdfs:subClassOf rdf:resource="http://emmo.info/emmo#EMMO_5b2222df_4da6_442f_8244_96e9e45887d1"/>
  </rdf:Description>
  <rdf:Description rdf:nodeID="f05bdaa1e617a4bccafc519daf7bf4785b174">
    <rdf:type rdf:resource="http://www.w3.org/1999/02/22-rdf-syntax-ns#List"/>
    <rdf:rest rdf:nodeID="f05bdaa1e617a4bccafc519daf7bf4785b175"/>
    <rdf:first rdf:resource="http://emmo.info/emmo#EMMO_a979c531_f9fa_4a6e_93c1_a2960241ca64"/>
  </rdf:Description>
  <rdf:Description rdf:about="http://emmo.info/emmo#EMMO_0b6ebe5a_0026_4bef_a1c1_5be00df9f98e">
    <EMMO_967080e5_2f42_4eb2_a3a9_c58143e835f9 xml:lang="en">A relation which makes a non-equal comparison between two numbers or other mathematical expressions.</EMMO_967080e5_2f42_4eb2_a3a9_c58143e835f9>
    <skos:prefLabel xml:lang="en">Inequality</skos:prefLabel>
    <rdf:type rdf:resource="http://www.w3.org/2002/07/owl#Class"/>
    <rdfs:subClassOf rdf:resource="http://emmo.info/emmo#EMMO_88470739_03d3_4c47_a03e_b30a1288d50c"/>
    <EMMO_b432d2d5_25f4_4165_99c5_5935a7763c1a xml:lang="en">f(x) &gt; 0</EMMO_b432d2d5_25f4_4165_99c5_5935a7763c1a>
  </rdf:Description>
  <rdf:Description rdf:nodeID="fdb1489b80bcc4ee28afe0be8feb9b935b12">
    <rdf:first rdf:resource="http://emmo.info/emmo#EMMO_2a888cdf_ec4a_4ec5_af1c_0343372fc978"/>
    <rdf:rest rdf:resource="http://www.w3.org/1999/02/22-rdf-syntax-ns#nil"/>
    <rdf:type rdf:resource="http://www.w3.org/1999/02/22-rdf-syntax-ns#List"/>
  </rdf:Description>
  <rdf:Description rdf:nodeID="ffcb99037244f48d590430c228d02afdbb18">
    <rdf:first rdf:resource="http://emmo.info/emmo#EMMO_053648ea_3c0a_468c_89cb_eb009239323a"/>
    <rdf:rest rdf:nodeID="ffcb99037244f48d590430c228d02afdbb19"/>
    <rdf:type rdf:resource="http://www.w3.org/1999/02/22-rdf-syntax-ns#List"/>
  </rdf:Description>
  <rdf:Description rdf:about="http://emmo.info/emmo#EMMO_2b1303e8_d4c3_453b_9918_76f1d009543f">
    <owl:equivalentClass rdf:nodeID="fe24a777e3fd743f986ce83488d2cf30bb7"/>
    <rdfs:subClassOf rdf:resource="http://emmo.info/emmo#EMMO_707f0cd1_941c_4b57_9f20_d0ba30cd6ff3"/>
    <rdf:type rdf:resource="http://www.w3.org/2002/07/owl#Class"/>
    <skos:prefLabel xml:lang="en">Multiplication</skos:prefLabel>
  </rdf:Description>
  <rdf:Description rdf:nodeID="f05bdaa1e617a4bccafc519daf7bf4785b102">
    <owl:hasValue>cd</owl:hasValue>
    <rdf:type rdf:resource="http://www.w3.org/2002/07/owl#Restriction"/>
    <owl:onProperty rdf:resource="http://emmo.info/emmo#EMMO_23b579e1_8088_45b5_9975_064014026c42"/>
  </rdf:Description>
  <rdf:Description rdf:nodeID="f8fb83657cd5f496db3c2b94baf326f26b38">
    <rdf:first rdf:resource="http://emmo.info/emmo#EMMO_62f0d847_3603_45b4_bfc4_dd4511355ff2"/>
    <rdf:type rdf:resource="http://www.w3.org/1999/02/22-rdf-syntax-ns#List"/>
    <rdf:rest rdf:nodeID="f8fb83657cd5f496db3c2b94baf326f26b39"/>
  </rdf:Description>
  <rdf:Description rdf:nodeID="f05bdaa1e617a4bccafc519daf7bf4785b148">
    <owl:hasValue>A</owl:hasValue>
    <rdf:type rdf:resource="http://www.w3.org/2002/07/owl#Restriction"/>
    <owl:onProperty rdf:resource="http://emmo.info/emmo#EMMO_23b579e1_8088_45b5_9975_064014026c42"/>
  </rdf:Description>
  <rdf:Description rdf:about="http://emmo.info/emmo#EMMO_06448f64_8db6_4304_8b2c_e785dba82044">
    <EMMO_6dd685dd_1895_46e4_b227_be9f7d643c25>http://dbpedia.org/page/Density</EMMO_6dd685dd_1895_46e4_b227_be9f7d643c25>
    <EMMO_fe015383_afb3_44a6_ae86_043628697aa2>https://doi.org/10.1351/goldbook.D01590</EMMO_fe015383_afb3_44a6_ae86_043628697aa2>
    <skos:prefLabel xml:lang="en">Density</skos:prefLabel>
    <EMMO_1f1b164d_ec6a_4faa_8d5e_88bda62316cc>http://qudt.org/vocab/quantitykind/Density</EMMO_1f1b164d_ec6a_4faa_8d5e_88bda62316cc>
    <rdf:type rdf:resource="http://www.w3.org/2002/07/owl#Class"/>
    <rdfs:comment xml:lang="en">Mass per volume.</rdfs:comment>
    <rdfs:subClassOf rdf:resource="http://emmo.info/emmo#EMMO_2946d40b_24a1_47fa_8176_e3f79bb45064"/>
    <EMMO_de178b12_5d35_4bca_8efa_a4193162571d>T0 L-3 M+1 I0 Θ0 N0 J0</EMMO_de178b12_5d35_4bca_8efa_a4193162571d>
  </rdf:Description>
  <rdf:Description rdf:nodeID="f05bdaa1e617a4bccafc519daf7bf4785b156">
    <owl:hasValue>n</owl:hasValue>
    <rdf:type rdf:resource="http://www.w3.org/2002/07/owl#Restriction"/>
    <owl:onProperty rdf:resource="http://emmo.info/emmo#EMMO_23b579e1_8088_45b5_9975_064014026c42"/>
  </rdf:Description>
  <rdf:Description rdf:about="http://emmo.info/emmo#EMMO_50a3552e_859a_4ff7_946d_76d537cabce6">
    <EMMO_967080e5_2f42_4eb2_a3a9_c58143e835f9 xml:lang="en">A symbol that stands for a concept in the language of the meterological domain of ISO 80000.</EMMO_967080e5_2f42_4eb2_a3a9_c58143e835f9>
    <owl:equivalentClass rdf:nodeID="f8fb83657cd5f496db3c2b94baf326f26b15"/>
    <rdf:type rdf:resource="http://www.w3.org/2002/07/owl#Class"/>
    <skos:prefLabel xml:lang="en">MetrologicalSymbol</skos:prefLabel>
    <rdfs:subClassOf rdf:nodeID="f8fb83657cd5f496db3c2b94baf326f26b18"/>
  </rdf:Description>
  <rdf:Description rdf:about="http://emmo.info/emmo#EMMO_9c32fd69_f480_4130_83b3_fb25d9face14">
    <skos:prefLabel xml:lang="en">PhysicalLaw</skos:prefLabel>
    <rdfs:subClassOf rdf:resource="http://emmo.info/emmo#EMMO_db9a009e_f097_43f5_9520_6cbc07e7610b"/>
    <rdf:type rdf:resource="http://www.w3.org/2002/07/owl#Class"/>
  </rdf:Description>
  <rdf:Description rdf:nodeID="ffbe75b10062f400ea693809785c50a44b6">
    <owl:onProperty rdf:nodeID="ffbe75b10062f400ea693809785c50a44b7"/>
    <owl:someValuesFrom rdf:resource="http://emmo.info/emmo#EMMO_71d1c8f0_c6e3_44b5_a4b6_1b74ff35698a"/>
    <rdf:type rdf:resource="http://www.w3.org/2002/07/owl#Restriction"/>
  </rdf:Description>
  <rdf:Description rdf:nodeID="ff14b31ebf90e4bc5ba2839064d29e543b1">
    <rdf:rest rdf:nodeID="ff14b31ebf90e4bc5ba2839064d29e543b2"/>
    <rdf:first rdf:resource="http://emmo.info/emmo#EMMO_2031516a_2be7_48e8_9af7_7e1270e308fe"/>
    <rdf:type rdf:resource="http://www.w3.org/1999/02/22-rdf-syntax-ns#List"/>
  </rdf:Description>
  <rdf:Description rdf:nodeID="ff14b31ebf90e4bc5ba2839064d29e543b16">
    <owl:onProperty rdf:resource="http://emmo.info/emmo#EMMO_b2282816_b7a3_44c6_b2cb_3feff1ceb7fe"/>
    <owl:someValuesFrom rdf:resource="http://emmo.info/emmo#EMMO_72d53756_7fb1_46ed_980f_83f47efbe105"/>
    <rdf:type rdf:resource="http://www.w3.org/2002/07/owl#Restriction"/>
  </rdf:Description>
  <rdf:Description rdf:about="http://emmo.info/emmo#EMMO_af24ae20_8ef2_435a_86a1_2ea44488b318">
    <owl:equivalentClass rdf:nodeID="fe0b20157736f4a31909181349b2e6219b30"/>
    <skos:prefLabel xml:lang="en">PerAmountDimension</skos:prefLabel>
    <rdfs:subClassOf rdf:resource="http://emmo.info/emmo#EMMO_9895a1b4_f0a5_4167_ac5e_97db40b8bfcc"/>
    <rdf:type rdf:resource="http://www.w3.org/2002/07/owl#Class"/>
  </rdf:Description>
  <rdf:Description rdf:about="http://emmo.info/emmo#EMMO_8681074a_e225_4e38_b586_e85b0f43ce38">
    <rdf:type rdf:resource="http://www.w3.org/2002/07/owl#Class"/>
    <rdfs:subClassOf rdf:resource="http://emmo.info/emmo#EMMO_d8d2144e_5c8d_455d_a643_5caf4d8d9df8"/>
    <skos:prefLabel xml:lang="en">Software</skos:prefLabel>
    <EMMO_967080e5_2f42_4eb2_a3a9_c58143e835f9 xml:lang="en">A language object that follows syntactic rules of a programming language.</EMMO_967080e5_2f42_4eb2_a3a9_c58143e835f9>
  </rdf:Description>
  <rdf:Description rdf:nodeID="f05bdaa1e617a4bccafc519daf7bf4785b141">
    <owl:someValuesFrom rdf:resource="http://emmo.info/emmo#EMMO_668e6ead_1530_40cc_ad5e_24b880edff50"/>
    <rdf:type rdf:resource="http://www.w3.org/2002/07/owl#Restriction"/>
    <owl:onProperty rdf:resource="http://emmo.info/emmo#EMMO_bed1d005_b04e_4a90_94cf_02bc678a8569"/>
  </rdf:Description>
  <rdf:Description rdf:nodeID="f05bdaa1e617a4bccafc519daf7bf4785b138">
    <owl:hasValue>lm</owl:hasValue>
    <rdf:type rdf:resource="http://www.w3.org/2002/07/owl#Restriction"/>
    <owl:onProperty rdf:resource="http://emmo.info/emmo#EMMO_23b579e1_8088_45b5_9975_064014026c42"/>
  </rdf:Description>
  <rdf:Description rdf:about="http://emmo.info/emmo#EMMO_acb50123_87a2_4753_b36c_f87114ad4de2">
    <EMMO_fe015383_afb3_44a6_ae86_043628697aa2>https://doi.org/10.1351/goldbook.T06283</EMMO_fe015383_afb3_44a6_ae86_043628697aa2>
    <EMMO_1f1b164d_ec6a_4faa_8d5e_88bda62316cc>http://qudt.org/vocab/unit/T</EMMO_1f1b164d_ec6a_4faa_8d5e_88bda62316cc>
    <skos:prefLabel xml:lang="en">Tesla</skos:prefLabel>
    <rdfs:comment xml:lang="en">Measurement unit for magnetic flux density or induction.</rdfs:comment>
    <rdfs:subClassOf rdf:nodeID="f05bdaa1e617a4bccafc519daf7bf4785b125"/>
    <rdfs:subClassOf rdf:nodeID="f05bdaa1e617a4bccafc519daf7bf4785b126"/>
    <rdf:type rdf:resource="http://www.w3.org/2002/07/owl#Class"/>
  </rdf:Description>
  <rdf:Description rdf:nodeID="f15a17d1fb53e4dd795c7db922ceff6acb7">
    <rdf:type rdf:resource="http://www.w3.org/1999/02/22-rdf-syntax-ns#List"/>
    <rdf:first rdf:resource="http://emmo.info/emmo#EMMO_eb3a768e_d53e_4be9_a23b_0714833c36de"/>
    <rdf:rest rdf:resource="http://www.w3.org/1999/02/22-rdf-syntax-ns#nil"/>
  </rdf:Description>
  <rdf:Description rdf:about="http://emmo.info/emmo#EMMO_cd5fb112_7ee7_4120_a35d_3ca3e6c3f4ab">
    <owl:deprecated>Replaced by dcterms:creator</owl:deprecated>
    <skos:prefLabel xml:lang="en">author</skos:prefLabel>
    <rdf:type rdf:resource="http://www.w3.org/2002/07/owl#AnnotationProperty"/>
    <rdfs:subPropertyOf rdf:resource="http://www.w3.org/2000/01/rdf-schema#comment"/>
  </rdf:Description>
  <rdf:Description rdf:nodeID="f8fb83657cd5f496db3c2b94baf326f26b4">
    <rdf:type rdf:resource="http://www.w3.org/2002/07/owl#Class"/>
    <owl:intersectionOf rdf:nodeID="f8fb83657cd5f496db3c2b94baf326f26b5"/>
  </rdf:Description>
  <rdf:Description rdf:about="http://emmo.info/emmo#EMMO_94010cbc_c2a6_4cb9_b29a_83aa99d2ff70">
    <skos:prefLabel xml:lang="en">LiquidAerosol</skos:prefLabel>
    <EMMO_967080e5_2f42_4eb2_a3a9_c58143e835f9 xml:lang="en">An aerosol composed of liquid droplets in air or another gas.</EMMO_967080e5_2f42_4eb2_a3a9_c58143e835f9>
    <rdfs:subClassOf rdf:resource="http://emmo.info/emmo#EMMO_560d833a_6184_410c_859a_05d982712fd7"/>
    <rdf:type rdf:resource="http://www.w3.org/2002/07/owl#Class"/>
  </rdf:Description>
  <rdf:Description rdf:nodeID="f05bdaa1e617a4bccafc519daf7bf4785b66">
    <rdf:first rdf:resource="http://emmo.info/emmo#EMMO_5eaecadc_4f0d_4a3a_afc7_1fc0b83cc928"/>
    <rdf:rest rdf:nodeID="f05bdaa1e617a4bccafc519daf7bf4785b67"/>
    <rdf:type rdf:resource="http://www.w3.org/1999/02/22-rdf-syntax-ns#List"/>
  </rdf:Description>
  <rdf:Description rdf:about="http://emmo.info/emmo#EMMO_e9eaeeb5_620c_4dab_8f72_269ff85d0634">
    <skos:prefLabel xml:lang="en">CoulombMetre</skos:prefLabel>
    <EMMO_967080e5_2f42_4eb2_a3a9_c58143e835f9 xml:lang="en">Measurement unit for electric dipole moment.</EMMO_967080e5_2f42_4eb2_a3a9_c58143e835f9>
    <rdfs:subClassOf rdf:nodeID="ffcb99037244f48d590430c228d02afdbb54"/>
    <rdf:type rdf:resource="http://www.w3.org/2002/07/owl#Class"/>
    <rdfs:subClassOf rdf:resource="http://emmo.info/emmo#EMMO_1273eb34_de48_43a9_925f_104110469dd2"/>
  </rdf:Description>
  <rdf:Description rdf:nodeID="fdb1489b80bcc4ee28afe0be8feb9b935b16">
    <rdf:type rdf:resource="http://www.w3.org/1999/02/22-rdf-syntax-ns#List"/>
    <rdf:rest rdf:resource="http://www.w3.org/1999/02/22-rdf-syntax-ns#nil"/>
    <rdf:first rdf:resource="http://emmo.info/emmo#EMMO_d8aa8e1f_b650_416d_88a0_5118de945456"/>
  </rdf:Description>
  <rdf:Description rdf:about="http://purl.org/dc/terms/abstract">
    <rdf:type rdf:resource="http://www.w3.org/2002/07/owl#AnnotationProperty"/>
  </rdf:Description>
  <rdf:Description rdf:about="http://emmo.info/emmo#EMMO_707f0cd1_941c_4b57_9f20_d0ba30cd6ff3">
    <rdf:type rdf:resource="http://www.w3.org/2002/07/owl#Class"/>
    <rdfs:subClassOf rdf:resource="http://emmo.info/emmo#EMMO_3c424d37_cf62_41b1_ac9d_a316f8d113d6"/>
    <skos:prefLabel xml:lang="en">ArithmeticOperator</skos:prefLabel>
  </rdf:Description>
  <rdf:Description rdf:about="http://emmo.info/emmo#EMMO_33433bb1_c68f_45ee_a466_f01e2c57b214">
    <rdfs:subClassOf rdf:nodeID="fe0b20157736f4a31909181349b2e6219b13"/>
    <skos:prefLabel xml:lang="en">AreaDimension</skos:prefLabel>
    <rdf:type rdf:resource="http://www.w3.org/2002/07/owl#Class"/>
    <rdfs:subClassOf rdf:resource="http://emmo.info/emmo#EMMO_9895a1b4_f0a5_4167_ac5e_97db40b8bfcc"/>
  </rdf:Description>
  <rdf:Description rdf:nodeID="fdb1489b80bcc4ee28afe0be8feb9b935b5">
    <rdf:type rdf:resource="http://www.w3.org/2002/07/owl#Restriction"/>
    <owl:onProperty rdf:resource="http://emmo.info/emmo#EMMO_ae2d1a96_bfa1_409a_a7d2_03d69e8a125a"/>
    <owl:someValuesFrom rdf:resource="http://emmo.info/emmo#EMMO_dd4a7f3e_ef56_466c_ac1a_d2716b5f87ec"/>
  </rdf:Description>
  <rdf:Description rdf:about="http://emmo.info/emmo#EMMO_89762966_8076_4f7c_b745_f718d653e8e2">
    <skos:prefLabel xml:lang="en">ExactConstant</skos:prefLabel>
    <rdfs:comment xml:lang="en">Physical constant used to define a unit system. Hence, when expressed in that unit system they have an exact value with no associated uncertainty.</rdfs:comment>
    <rdf:type rdf:resource="http://www.w3.org/2002/07/owl#Class"/>
  </rdf:Description>
  <rdf:Description rdf:nodeID="fe24a777e3fd743f986ce83488d2cf30bb7">
    <owl:onProperty rdf:resource="http://emmo.info/emmo#EMMO_23b579e1_8088_45b5_9975_064014026c42"/>
    <rdf:type rdf:resource="http://www.w3.org/2002/07/owl#Restriction"/>
    <owl:hasValue>*</owl:hasValue>
  </rdf:Description>
  <rdf:Description rdf:about="http://emmo.info/emmo#EMMO_432192c4_111f_4e80_b7cd_c6ce1c1129ea">
    <rdf:type rdf:resource="http://www.w3.org/2002/07/owl#Class"/>
    <rdfs:subClassOf rdf:resource="http://emmo.info/emmo#EMMO_a1083d0a_c1fb_471f_8e20_a98f881ad527"/>
    <skos:prefLabel xml:lang="en">Spacing</skos:prefLabel>
  </rdf:Description>
  <rdf:Description rdf:nodeID="f8fb83657cd5f496db3c2b94baf326f26b14">
    <owl:inverseOf rdf:resource="http://emmo.info/emmo#EMMO_60577dea_9019_4537_ac41_80b0fb563d41"/>
  </rdf:Description>
  <rdf:Description rdf:nodeID="f05bdaa1e617a4bccafc519daf7bf4785b170">
    <rdf:first rdf:resource="http://emmo.info/emmo#EMMO_8a70dea4_d6ab_4260_b931_a3e990982416"/>
    <rdf:rest rdf:nodeID="f05bdaa1e617a4bccafc519daf7bf4785b171"/>
    <rdf:type rdf:resource="http://www.w3.org/1999/02/22-rdf-syntax-ns#List"/>
  </rdf:Description>
  <rdf:Description rdf:nodeID="ffbe75b10062f400ea693809785c50a44b5">
    <owl:onProperty rdf:resource="http://emmo.info/emmo#EMMO_c5aae418_1622_4d02_93c5_21159e28e6c1"/>
    <rdf:type rdf:resource="http://www.w3.org/2002/07/owl#Restriction"/>
    <owl:someValuesFrom rdf:resource="http://emmo.info/emmo#EMMO_86ca9b93_1183_4b65_81b8_c0fcd3bba5ad"/>
  </rdf:Description>
  <rdf:Description rdf:about="http://emmo.info/emmo#EMMO_0b15f4ae_092e_4487_9100_3c44176c545c">
    <owl:disjointUnionOf rdf:nodeID="ff14b31ebf90e4bc5ba2839064d29e543b1"/>
    <rdf:type rdf:resource="http://www.w3.org/2002/07/owl#Class"/>
    <skos:prefLabel xml:lang="en">Dispersion</skos:prefLabel>
    <EMMO_967080e5_2f42_4eb2_a3a9_c58143e835f9 xml:lang="en">A material in which distributed particles of one phase are dispersed in a different continuous phase.</EMMO_967080e5_2f42_4eb2_a3a9_c58143e835f9>
  </rdf:Description>
  <rdf:Description rdf:about="http://emmo.info/emmo#EMMO_cdc962d8_f3ea_4764_a57a_c7caa4859179">
    <skos:prefLabel xml:lang="en">LengthFractionUnit</skos:prefLabel>
    <EMMO_967080e5_2f42_4eb2_a3a9_c58143e835f9 xml:lang="en">Unit for quantities of dimension one that are the fraction of two lengths.</EMMO_967080e5_2f42_4eb2_a3a9_c58143e835f9>
    <EMMO_b432d2d5_25f4_4165_99c5_5935a7763c1a xml:lang="en">Unit for plane angle.</EMMO_b432d2d5_25f4_4165_99c5_5935a7763c1a>
    <rdf:type rdf:resource="http://www.w3.org/2002/07/owl#Class"/>
    <rdfs:subClassOf rdf:resource="http://emmo.info/emmo#EMMO_c2f5ee66_579c_44c6_a2e9_fa2eaa9fa4da"/>
  </rdf:Description>
  <rdf:Description rdf:about="http://emmo.info/emmo#EMMO_8f87e700_99a8_4427_8ffb_e493de05c217">
    <rdf:type rdf:resource="http://www.w3.org/2002/07/owl#Class"/>
    <skos:prefLabel xml:lang="en">Proton</skos:prefLabel>
  </rdf:Description>
  <rdf:Description rdf:about="http://emmo.info/emmo#EMMO_b51fbd00_a857_4132_9711_0ef70e7bdd20">
    <EMMO_70fe84ff_99b6_4206_a9fc_9a8931836d84 xml:lang="en">The total luminous flux incident on a surface, per unit area.</EMMO_70fe84ff_99b6_4206_a9fc_9a8931836d84>
    <EMMO_de178b12_5d35_4bca_8efa_a4193162571d>T0 L-2 M0 I0 Θ0 N0 J+1</EMMO_de178b12_5d35_4bca_8efa_a4193162571d>
    <EMMO_fe015383_afb3_44a6_ae86_043628697aa2>https://doi.org/10.1351/goldbook.I02941</EMMO_fe015383_afb3_44a6_ae86_043628697aa2>
    <rdf:type rdf:resource="http://www.w3.org/2002/07/owl#Class"/>
    <EMMO_1f1b164d_ec6a_4faa_8d5e_88bda62316cc>http://qudt.org/vocab/quantitykind/Illuminance</EMMO_1f1b164d_ec6a_4faa_8d5e_88bda62316cc>
    <EMMO_6dd685dd_1895_46e4_b227_be9f7d643c25>http://dbpedia.org/page/Illuminance</EMMO_6dd685dd_1895_46e4_b227_be9f7d643c25>
    <skos:prefLabel xml:lang="en">Illuminance</skos:prefLabel>
    <rdfs:subClassOf rdf:resource="http://emmo.info/emmo#EMMO_2946d40b_24a1_47fa_8176_e3f79bb45064"/>
  </rdf:Description>
  <rdf:Description rdf:about="http://emmo.info/emmo#EMMO_b2a234a8_579a_422c_9305_b8f7e72c76cd">
    <skos:prefLabel xml:lang="en">Circle</skos:prefLabel>
    <rdfs:subClassOf rdf:resource="http://emmo.info/emmo#EMMO_0c576e13_4ee7_4f3d_bfe9_1614243df018"/>
    <rdf:type rdf:resource="http://www.w3.org/2002/07/owl#Class"/>
  </rdf:Description>
  <rdf:Description rdf:nodeID="fe24a777e3fd743f986ce83488d2cf30bb6">
    <owl:inverseOf rdf:resource="http://emmo.info/emmo#EMMO_3446e167_c576_49d6_846c_215bb8878a55"/>
  </rdf:Description>
  <rdf:Description rdf:about="http://emmo.info/emmo#EMMO_1da53c06_9577_4008_8652_272fa3b62be7">
    <EMMO_b432d2d5_25f4_4165_99c5_5935a7763c1a xml:lang="en">A drawing of a cat.
A circle on a paper sheet.
The Mona Lisa.</EMMO_b432d2d5_25f4_4165_99c5_5935a7763c1a>
    <skos:prefLabel xml:lang="en">Pictorial</skos:prefLabel>
    <EMMO_967080e5_2f42_4eb2_a3a9_c58143e835f9 xml:lang="en">A 'Graphical' that stands for a real world object that shows a recognizable pictorial pattern without being necessarily associated to a symbolic language.</EMMO_967080e5_2f42_4eb2_a3a9_c58143e835f9>
    <rdfs:subClassOf rdf:resource="http://emmo.info/emmo#EMMO_c74da218_9147_4f03_92d1_8894abca55f3"/>
    <rdf:type rdf:resource="http://www.w3.org/2002/07/owl#Class"/>
  </rdf:Description>
  <rdf:Description rdf:nodeID="f05bdaa1e617a4bccafc519daf7bf4785b184">
    <rdf:first rdf:resource="http://emmo.info/emmo#EMMO_e75f580e_52bf_4dd5_af70_df409cec08fd"/>
    <rdf:rest rdf:nodeID="f05bdaa1e617a4bccafc519daf7bf4785b185"/>
    <rdf:type rdf:resource="http://www.w3.org/1999/02/22-rdf-syntax-ns#List"/>
  </rdf:Description>
  <rdf:Description rdf:nodeID="f05bdaa1e617a4bccafc519daf7bf4785b12">
    <owl:hasValue>d</owl:hasValue>
    <rdf:type rdf:resource="http://www.w3.org/2002/07/owl#Restriction"/>
    <owl:onProperty rdf:resource="http://emmo.info/emmo#EMMO_23b579e1_8088_45b5_9975_064014026c42"/>
  </rdf:Description>
  <rdf:Description rdf:nodeID="f05bdaa1e617a4bccafc519daf7bf4785b140">
    <owl:onProperty rdf:resource="http://emmo.info/emmo#EMMO_23b579e1_8088_45b5_9975_064014026c42"/>
    <owl:hasValue>Wb</owl:hasValue>
    <rdf:type rdf:resource="http://www.w3.org/2002/07/owl#Restriction"/>
  </rdf:Description>
  <rdf:Description rdf:about="http://emmo.info/emmo#EMMO_5cb107ba_7daa_46dd_8f9f_da22a6eac676">
    <rdfs:subClassOf rdf:resource="http://emmo.info/emmo#EMMO_4b3e2374_52a1_4420_8e3f_3ae6b9bf7dff"/>
    <rdf:type rdf:resource="http://www.w3.org/2002/07/owl#Class"/>
    <skos:prefLabel xml:lang="en">AcqueousSolution</skos:prefLabel>
    <EMMO_967080e5_2f42_4eb2_a3a9_c58143e835f9 xml:lang="en">A liquid solution in which the solvent is water.</EMMO_967080e5_2f42_4eb2_a3a9_c58143e835f9>
  </rdf:Description>
  <rdf:Description rdf:about="http://emmo.info/emmo#EMMO_1cba0b27_15d0_4326_933f_379d0b3565b6">
    <rdfs:subClassOf rdf:resource="http://emmo.info/emmo#EMMO_28fbea28_2204_4613_87ff_6d877b855fcd"/>
    <rdf:type rdf:resource="http://www.w3.org/2002/07/owl#Class"/>
    <skos:prefLabel xml:lang="en">Matrix</skos:prefLabel>
  </rdf:Description>
  <rdf:Description rdf:about="http://emmo.info/emmo#EMMO_591e02fd_8d37_45a6_9d11_bb21cef391a0">
    <EMMO_967080e5_2f42_4eb2_a3a9_c58143e835f9 xml:lang="en">A unit that does not belong to any system of units.</EMMO_967080e5_2f42_4eb2_a3a9_c58143e835f9>
    <rdfs:subClassOf rdf:resource="http://emmo.info/emmo#EMMO_b081b346_7279_46ef_9a3d_2c088fcd79f4"/>
    <skos:prefLabel xml:lang="en">OffSystemUnit</skos:prefLabel>
    <EMMO_b432d2d5_25f4_4165_99c5_5935a7763c1a xml:lang="en">eV
barn</EMMO_b432d2d5_25f4_4165_99c5_5935a7763c1a>
    <rdf:type rdf:resource="http://www.w3.org/2002/07/owl#Class"/>
  </rdf:Description>
  <rdf:Description rdf:about="http://emmo.info/emmo#EMMO_d7788d1a_020d_4c78_85a1_13563fcec168">
    <skos:prefLabel xml:lang="en">Icon</skos:prefLabel>
    <EMMO_967080e5_2f42_4eb2_a3a9_c58143e835f9 xml:lang="en">A 'Sign' that stands for an 'Object' by resembling or imitating it, in shape or by sharing a similar logical structure.</EMMO_967080e5_2f42_4eb2_a3a9_c58143e835f9>
    <EMMO_b432d2d5_25f4_4165_99c5_5935a7763c1a xml:lang="en">A picture that reproduces the aspect of a person. 

An equation that reproduces the logical connection of the properties of a physical entity.</EMMO_b432d2d5_25f4_4165_99c5_5935a7763c1a>
    <rdf:type rdf:resource="http://www.w3.org/2002/07/owl#Class"/>
    <rdfs:comment xml:lang="en">Three subtypes of icon are possible:
 
(a) the image, which depends on a simple quality (e.g. picture)

(b) the diagram, whose internal relations, mainly dyadic or so taken, represent by analogy the relations in something (e.g. math formula, geometric flowchart)

(c) the metaphor, which represents the representative character of a sign by representing a parallelism in something else

[Wikipedia]</rdfs:comment>
  </rdf:Description>
  <rdf:Description rdf:nodeID="fe0b20157736f4a31909181349b2e6219b1">
    <owl:onProperty rdf:resource="http://emmo.info/emmo#EMMO_23b579e1_8088_45b5_9975_064014026c42"/>
    <rdf:type rdf:resource="http://www.w3.org/2002/07/owl#Restriction"/>
    <owl:hasValue>T+1 L0 M0 I0 Θ0 N0 J0</owl:hasValue>
  </rdf:Description>
  <rdf:Description rdf:nodeID="ff14b31ebf90e4bc5ba2839064d29e543b20">
    <rdf:first rdf:resource="http://emmo.info/emmo#EMMO_4c21fb86_fdcf_444e_b498_86fe656295af"/>
    <rdf:type rdf:resource="http://www.w3.org/1999/02/22-rdf-syntax-ns#List"/>
    <rdf:rest rdf:nodeID="ff14b31ebf90e4bc5ba2839064d29e543b21"/>
  </rdf:Description>
  <rdf:Description rdf:nodeID="ffcb99037244f48d590430c228d02afdbb46">
    <owl:someValuesFrom rdf:resource="http://emmo.info/emmo#EMMO_f6070071_d054_4b17_9d2d_f446f7147d0f"/>
    <owl:onProperty rdf:resource="http://emmo.info/emmo#EMMO_bed1d005_b04e_4a90_94cf_02bc678a8569"/>
    <rdf:type rdf:resource="http://www.w3.org/2002/07/owl#Restriction"/>
  </rdf:Description>
  <rdf:Description rdf:nodeID="f05bdaa1e617a4bccafc519daf7bf4785b25">
    <owl:allValuesFrom rdf:nodeID="f05bdaa1e617a4bccafc519daf7bf4785b27"/>
    <owl:onProperty rdf:nodeID="f05bdaa1e617a4bccafc519daf7bf4785b26"/>
    <rdf:type rdf:resource="http://www.w3.org/2002/07/owl#Restriction"/>
  </rdf:Description>
  <rdf:Description rdf:nodeID="ffcb99037244f48d590430c228d02afdbb23">
    <rdf:type rdf:resource="http://www.w3.org/1999/02/22-rdf-syntax-ns#List"/>
    <rdf:rest rdf:nodeID="ffcb99037244f48d590430c228d02afdbb24"/>
    <rdf:first rdf:resource="http://emmo.info/emmo#EMMO_6c7160fc_cc64_46f0_b43b_aba65e9952e3"/>
  </rdf:Description>
  <rdf:Description rdf:nodeID="f05bdaa1e617a4bccafc519daf7bf4785b152">
    <owl:onProperty rdf:resource="http://emmo.info/emmo#EMMO_23b579e1_8088_45b5_9975_064014026c42"/>
    <owl:hasValue>mol</owl:hasValue>
    <rdf:type rdf:resource="http://www.w3.org/2002/07/owl#Restriction"/>
  </rdf:Description>
  <rdf:Description rdf:nodeID="fe24a777e3fd743f986ce83488d2cf30bb13">
    <owl:intersectionOf rdf:nodeID="fe24a777e3fd743f986ce83488d2cf30bb14"/>
    <rdf:type rdf:resource="http://www.w3.org/2002/07/owl#Class"/>
  </rdf:Description>
  <rdf:Description rdf:nodeID="ff14b31ebf90e4bc5ba2839064d29e543b7">
    <rdf:rest rdf:resource="http://www.w3.org/1999/02/22-rdf-syntax-ns#nil"/>
    <rdf:type rdf:resource="http://www.w3.org/1999/02/22-rdf-syntax-ns#List"/>
    <rdf:first rdf:resource="http://emmo.info/emmo#EMMO_db03061b_db31_4132_a47a_6a634846578b"/>
  </rdf:Description>
  <rdf:Description rdf:nodeID="ffcb99037244f48d590430c228d02afdbb51">
    <owl:onProperty rdf:resource="http://emmo.info/emmo#EMMO_bed1d005_b04e_4a90_94cf_02bc678a8569"/>
    <owl:someValuesFrom rdf:resource="http://emmo.info/emmo#EMMO_f6070071_d054_4b17_9d2d_f446f7147d0f"/>
    <rdf:type rdf:resource="http://www.w3.org/2002/07/owl#Restriction"/>
  </rdf:Description>
  <rdf:Description rdf:nodeID="f05bdaa1e617a4bccafc519daf7bf4785b46">
    <owl:hasValue rdf:datatype="http://www.w3.org/2001/XMLSchema#double">1000000000000.0</owl:hasValue>
    <owl:onProperty rdf:resource="http://emmo.info/emmo#EMMO_faf79f53_749d_40b2_807c_d34244c192f4"/>
    <rdf:type rdf:resource="http://www.w3.org/2002/07/owl#Restriction"/>
  </rdf:Description>
  <rdf:Description rdf:nodeID="ff14b31ebf90e4bc5ba2839064d29e543b32">
    <owl:minQualifiedCardinality rdf:datatype="http://www.w3.org/2001/XMLSchema#nonNegativeInteger">1</owl:minQualifiedCardinality>
  </rdf:Description>
  <rdf:Description rdf:nodeID="f15a17d1fb53e4dd795c7db922ceff6acb4">
    <owl:onProperty rdf:nodeID="f15a17d1fb53e4dd795c7db922ceff6acb5"/>
    <owl:hasValue rdf:resource="http://emmo.info/emmo#EMMO_08cb807c_e626_447b_863f_e2835540e918"/>
    <rdf:type rdf:resource="http://www.w3.org/2002/07/owl#Restriction"/>
  </rdf:Description>
  <rdf:Description rdf:nodeID="fdb1489b80bcc4ee28afe0be8feb9b935b7">
    <owl:someValuesFrom rdf:resource="http://emmo.info/emmo#EMMO_10a5fd39_06aa_4648_9e70_f962a9cb2069"/>
    <owl:onProperty rdf:nodeID="fdb1489b80bcc4ee28afe0be8feb9b935b8"/>
    <rdf:type rdf:resource="http://www.w3.org/2002/07/owl#Restriction"/>
  </rdf:Description>
  <rdf:Description rdf:nodeID="f3b8e3e5cecf14b688acdf306cd5f62cbb3">
    <rdf:first rdf:resource="http://emmo.info/emmo#EMMO_52211e5e_d767_4812_845e_eb6b402c476a"/>
    <rdf:rest rdf:resource="http://www.w3.org/1999/02/22-rdf-syntax-ns#nil"/>
    <rdf:type rdf:resource="http://www.w3.org/1999/02/22-rdf-syntax-ns#List"/>
  </rdf:Description>
  <rdf:Description rdf:about="http://emmo.info/emmo#EMMO_21ae69b4_235e_479d_8dd8_4f756f694c1b">
    <skos:prefLabel xml:lang="en">altLabel</skos:prefLabel>
    <rdfs:subPropertyOf rdf:resource="http://www.w3.org/2000/01/rdf-schema#comment"/>
    <owl:deprecated>Replaced by skos:altLabel</owl:deprecated>
    <rdf:type rdf:resource="http://www.w3.org/2002/07/owl#AnnotationProperty"/>
  </rdf:Description>
  <rdf:Description rdf:nodeID="f8fb83657cd5f496db3c2b94baf326f26b25">
    <owl:complementOf rdf:resource="http://emmo.info/emmo#EMMO_7d2afa66_ae9e_4095_a9bf_421d0be401b6"/>
    <rdf:type rdf:resource="http://www.w3.org/2002/07/owl#Class"/>
  </rdf:Description>
  <rdf:Description rdf:about="http://emmo.info/emmo#EMMO_bed2fe4c_dc7e_43a8_8200_6aac44030bff">
    <rdf:type rdf:resource="http://www.w3.org/2002/07/owl#Class"/>
    <skos:prefLabel xml:lang="en">Letter</skos:prefLabel>
    <rdfs:subClassOf rdf:resource="http://emmo.info/emmo#EMMO_a1083d0a_c1fb_471f_8e20_a98f881ad527"/>
  </rdf:Description>
  <rdf:Description rdf:about="http://emmo.info/emmo#EMMO_f2ca6dd0_0e5f_4392_a92d_cafdae6cfc95">
    <rdfs:subClassOf rdf:resource="http://emmo.info/emmo#EMMO_89762966_8076_4f7c_b745_f718d653e8e2"/>
    <rdf:type rdf:resource="http://www.w3.org/2002/07/owl#Class"/>
    <skos:prefLabel xml:lang="en">SIExactConstant</skos:prefLabel>
    <EMMO_967080e5_2f42_4eb2_a3a9_c58143e835f9 xml:lang="en">Physical constant that by definition (after the latest revision of the SI system that was enforsed May 2019) has a known exact numerical value when expressed in SI units.</EMMO_967080e5_2f42_4eb2_a3a9_c58143e835f9>
  </rdf:Description>
  <rdf:Description rdf:about="http://emmo.info/emmo#EMMO_eb561764_276e_413d_a8cb_3a3154fd9bf8">
    <EMMO_70fe84ff_99b6_4206_a9fc_9a8931836d84 xml:lang="en">The von Klitzing constant is defined as Planck constant divided by the square of the elementary charge.</EMMO_70fe84ff_99b6_4206_a9fc_9a8931836d84>
    <rdfs:comment xml:lang="en">Resistance quantum.</rdfs:comment>
    <skos:prefLabel xml:lang="en">VonKlitzingConstant</skos:prefLabel>
    <EMMO_a9b3d04c_7ceb_40a2_b8d3_28d514a770a8>https://physics.nist.gov/cgi-bin/cuu/Value?rk</EMMO_a9b3d04c_7ceb_40a2_b8d3_28d514a770a8>
    <EMMO_1f1b164d_ec6a_4faa_8d5e_88bda62316cc>http://qudt.org/vocab/constant/VonKlitzingConstant</EMMO_1f1b164d_ec6a_4faa_8d5e_88bda62316cc>
    <rdf:type rdf:resource="http://www.w3.org/2002/07/owl#Class"/>
    <rdfs:subClassOf rdf:resource="http://emmo.info/emmo#EMMO_f2ca6dd0_0e5f_4392_a92d_cafdae6cfc95"/>
    <rdfs:subClassOf rdf:resource="http://emmo.info/emmo#EMMO_e88f75d6_9a17_4cfc_bdf7_43d7cea5a9a1"/>
    <EMMO_de178b12_5d35_4bca_8efa_a4193162571d>T-3 L+2 M+1 I-2 Θ0 N0 J0</EMMO_de178b12_5d35_4bca_8efa_a4193162571d>
  </rdf:Description>
  <rdf:Description rdf:about="http://emmo.info/emmo#EMMO_d1d436e7_72fc_49cd_863b_7bfb4ba5276a">
    <EMMO_b432d2d5_25f4_4165_99c5_5935a7763c1a xml:lang="en">viscosity in the Navier-Stokes equation</EMMO_b432d2d5_25f4_4165_99c5_5935a7763c1a>
    <skos:prefLabel xml:lang="en">Parameter</skos:prefLabel>
    <rdfs:comment xml:lang="en">A 'variable' whose value is assumed to be known independently from the equation, but whose value is not explicitated in the equation.</rdfs:comment>
    <rdf:type rdf:resource="http://www.w3.org/2002/07/owl#Class"/>
    <rdfs:subClassOf rdf:resource="http://emmo.info/emmo#EMMO_1eed0732_e3f1_4b2c_a9c4_b4e75eeb5895"/>
  </rdf:Description>
  <rdf:Description rdf:about="http://emmo.info/emmo#EMMO_463bcfda_867b_41d9_a967_211d4d437cfb">
    <rdfs:subClassOf rdf:nodeID="fdb1489b80bcc4ee28afe0be8feb9b935b5"/>
    <skos:prefLabel xml:lang="en">Measurement</skos:prefLabel>
    <rdfs:subClassOf rdf:resource="http://emmo.info/emmo#EMMO_10a5fd39_06aa_4648_9e70_f962a9cb2069"/>
    <rdf:type rdf:resource="http://www.w3.org/2002/07/owl#Class"/>
    <EMMO_967080e5_2f42_4eb2_a3a9_c58143e835f9 xml:lang="en">An 'observation' that results in a quantitative comparison of a 'property' of an 'object' with a standard reference.</EMMO_967080e5_2f42_4eb2_a3a9_c58143e835f9>
    <rdfs:subClassOf rdf:nodeID="fdb1489b80bcc4ee28afe0be8feb9b935b6"/>
  </rdf:Description>
  <rdf:Description rdf:nodeID="fea11ca01461e402d8f697c19c5d8de88b23">
    <rdf:rest rdf:resource="http://www.w3.org/1999/02/22-rdf-syntax-ns#nil"/>
    <rdf:first rdf:resource="http://emmo.info/emmo#EMMO_eb3c61f0_3983_4346_a0c6_e7f6b90a67a8"/>
    <rdf:type rdf:resource="http://www.w3.org/1999/02/22-rdf-syntax-ns#List"/>
  </rdf:Description>
  <rdf:Description rdf:nodeID="fe24a777e3fd743f986ce83488d2cf30bb2">
    <owl:someValuesFrom rdf:resource="http://www.w3.org/2001/XMLSchema#double"/>
    <rdf:type rdf:resource="http://www.w3.org/2002/07/owl#Restriction"/>
    <owl:onProperty rdf:resource="http://emmo.info/emmo#EMMO_faf79f53_749d_40b2_807c_d34244c192f4"/>
  </rdf:Description>
  <rdf:Description rdf:about="http://emmo.info/emmo#EMMO_a2f94f33_71fa_443c_a1fb_d1685fc537ec">
    <EMMO_967080e5_2f42_4eb2_a3a9_c58143e835f9 xml:lang="en">Measurement unit obtained by dividing a given measurement unit by an integer greater than one.</EMMO_967080e5_2f42_4eb2_a3a9_c58143e835f9>
    <skos:prefLabel xml:lang="en">SubMultipleUnit</skos:prefLabel>
    <rdf:type rdf:resource="http://www.w3.org/2002/07/owl#Class"/>
  </rdf:Description>
  <rdf:Description rdf:nodeID="f8fb83657cd5f496db3c2b94baf326f26b33">
    <rdf:type rdf:resource="http://www.w3.org/2002/07/owl#Class"/>
    <owl:unionOf rdf:nodeID="f8fb83657cd5f496db3c2b94baf326f26b34"/>
  </rdf:Description>
  <rdf:Description rdf:about="http://emmo.info/emmo#EMMO_50781fd9_a9e4_46ad_b7be_4500371d188d">
    <rdfs:subClassOf rdf:resource="http://emmo.info/emmo#EMMO_7d66bde4_b68d_41cc_b5fc_6fd98c5e2ff0"/>
    <rdf:type rdf:resource="http://www.w3.org/2002/07/owl#Class"/>
    <rdfs:subClassOf rdf:nodeID="ff14b31ebf90e4bc5ba2839064d29e543b16"/>
    <skos:prefLabel xml:lang="en">Nucleon</skos:prefLabel>
    <owl:disjointUnionOf rdf:nodeID="ff14b31ebf90e4bc5ba2839064d29e543b17"/>
  </rdf:Description>
  <rdf:Description rdf:nodeID="f05bdaa1e617a4bccafc519daf7bf4785b69">
    <rdf:first rdf:resource="http://emmo.info/emmo#EMMO_a3a701ed_6f7d_4a10_9aee_dfa1961fc7b7"/>
    <rdf:rest rdf:nodeID="f05bdaa1e617a4bccafc519daf7bf4785b70"/>
    <rdf:type rdf:resource="http://www.w3.org/1999/02/22-rdf-syntax-ns#List"/>
  </rdf:Description>
  <rdf:Description rdf:about="http://emmo.info/emmo#EMMO_1067b97a_84f8_4d22_8ace_b842b8ce355c">
    <rdf:type rdf:resource="http://www.w3.org/2002/07/owl#Class"/>
    <skos:prefLabel xml:lang="en">ElectronCloud</skos:prefLabel>
    <rdfs:subClassOf rdf:nodeID="ff14b31ebf90e4bc5ba2839064d29e543b5"/>
    <rdfs:subClassOf rdf:resource="http://emmo.info/emmo#EMMO_7d66bde4_b68d_41cc_b5fc_6fd98c5e2ff0"/>
    <EMMO_967080e5_2f42_4eb2_a3a9_c58143e835f9 xml:lang="en">A 'spacetime' that stands for a quantum system made of electrons.</EMMO_967080e5_2f42_4eb2_a3a9_c58143e835f9>
  </rdf:Description>
  <rdf:Description rdf:about="http://emmo.info/emmo#EMMO_71d1c8f0_c6e3_44b5_a4b6_1b74ff35698a">
    <EMMO_b432d2d5_25f4_4165_99c5_5935a7763c1a xml:lang="en">Synthesis of materials, the preparation of a cake.</EMMO_b432d2d5_25f4_4165_99c5_5935a7763c1a>
    <skos:prefLabel xml:lang="en">ContinuumManufacturing</skos:prefLabel>
    <EMMO_967080e5_2f42_4eb2_a3a9_c58143e835f9 xml:lang="en">A manufacturing process whose product is the result of the combination of more substances.</EMMO_967080e5_2f42_4eb2_a3a9_c58143e835f9>
    <rdf:type rdf:resource="http://www.w3.org/2002/07/owl#Class"/>
    <rdfs:subClassOf rdf:resource="http://emmo.info/emmo#EMMO_a4d66059_5dd3_4b90_b4cb_10960559441b"/>
  </rdf:Description>
  <rdf:Description rdf:nodeID="fe0b20157736f4a31909181349b2e6219b3">
    <rdf:rest rdf:nodeID="fe0b20157736f4a31909181349b2e6219b4"/>
    <rdf:type rdf:resource="http://www.w3.org/1999/02/22-rdf-syntax-ns#List"/>
    <rdf:first rdf:resource="http://emmo.info/emmo#EMMO_50bf79a6_a48b_424d_9d2c_813bd631231a"/>
  </rdf:Description>
  <rdf:Description rdf:about="http://emmo.info/emmo#EMMO_c5aae418_1622_4d02_93c5_21159e28e6c1">
    <rdfs:subPropertyOf rdf:resource="http://emmo.info/emmo#EMMO_ae2d1a96_bfa1_409a_a7d2_03d69e8a125a"/>
    <skos:prefLabel xml:lang="en">hasProperParticipant</skos:prefLabel>
    <rdf:type rdf:resource="http://www.w3.org/2002/07/owl#ObjectProperty"/>
    <rdfs:subPropertyOf rdf:resource="http://emmo.info/emmo#EMMO_9380ab64_0363_4804_b13f_3a8a94119a76"/>
  </rdf:Description>
  <rdf:Description rdf:about="http://emmo.info/emmo#EMMO_39362460_2a97_4367_8f93_0418c2ac9a08">
    <skos:prefLabel xml:lang="en">Point</skos:prefLabel>
    <rdfs:subClassOf rdf:resource="http://emmo.info/emmo#EMMO_0ab0485c_9e5b_4257_a679_90a2dfba5c7c"/>
    <rdf:type rdf:resource="http://www.w3.org/2002/07/owl#Class"/>
  </rdf:Description>
  <rdf:Description rdf:nodeID="f05bdaa1e617a4bccafc519daf7bf4785b135">
    <owl:onProperty rdf:resource="http://emmo.info/emmo#EMMO_bed1d005_b04e_4a90_94cf_02bc678a8569"/>
    <owl:someValuesFrom rdf:resource="http://emmo.info/emmo#EMMO_3227b821_26a5_4c7c_9c01_5c24483e0bd0"/>
    <rdf:type rdf:resource="http://www.w3.org/2002/07/owl#Restriction"/>
  </rdf:Description>
  <rdf:Description rdf:nodeID="fe0b20157736f4a31909181349b2e6219b16">
    <owl:hasValue>T-1 L+1 M0 I0 Θ0 N0 J0</owl:hasValue>
    <rdf:type rdf:resource="http://www.w3.org/2002/07/owl#Restriction"/>
    <owl:onProperty rdf:resource="http://emmo.info/emmo#EMMO_23b579e1_8088_45b5_9975_064014026c42"/>
  </rdf:Description>
  <rdf:Description rdf:nodeID="ff14b31ebf90e4bc5ba2839064d29e543b23">
    <owl:onProperty rdf:resource="http://emmo.info/emmo#EMMO_b2282816_b7a3_44c6_b2cb_3feff1ceb7fe"/>
    <owl:someValuesFrom rdf:resource="http://emmo.info/emmo#EMMO_1067b97a_84f8_4d22_8ace_b842b8ce355c"/>
    <rdf:type rdf:resource="http://www.w3.org/2002/07/owl#Restriction"/>
  </rdf:Description>
  <rdf:Description rdf:nodeID="f05bdaa1e617a4bccafc519daf7bf4785b58">
    <rdf:type rdf:resource="http://www.w3.org/1999/02/22-rdf-syntax-ns#List"/>
    <rdf:first rdf:resource="http://emmo.info/emmo#EMMO_1d8b370b_c672_4d0c_964e_eaafcbf2f51f"/>
    <rdf:rest rdf:nodeID="f05bdaa1e617a4bccafc519daf7bf4785b59"/>
  </rdf:Description>
  <rdf:Description rdf:about="http://emmo.info/emmo#EMMO_4d604a13_d1f6_42fd_818f_d3138d5e308c">
    <EMMO_967080e5_2f42_4eb2_a3a9_c58143e835f9 xml:lang="en">A liquid aerosol composed of water droplets in air or another gas.</EMMO_967080e5_2f42_4eb2_a3a9_c58143e835f9>
    <rdfs:subClassOf rdf:resource="http://emmo.info/emmo#EMMO_94010cbc_c2a6_4cb9_b29a_83aa99d2ff70"/>
    <rdf:type rdf:resource="http://www.w3.org/2002/07/owl#Class"/>
    <skos:prefLabel xml:lang="en">Vapor</skos:prefLabel>
  </rdf:Description>
  <rdf:Description rdf:nodeID="fe24a777e3fd743f986ce83488d2cf30bb17">
    <owl:complementOf rdf:resource="http://emmo.info/emmo#EMMO_54ee6b5e_5261_44a8_86eb_5717e7fdb9d0"/>
    <rdf:type rdf:resource="http://www.w3.org/2002/07/owl#Class"/>
  </rdf:Description>
  <rdf:Description rdf:about="http://emmo.info/emmo#EMMO_33e0ac8b_a318_4285_b1de_e95347784632">
    <skos:prefLabel xml:lang="en">SolidLiquidSuspension</skos:prefLabel>
    <rdfs:subClassOf rdf:resource="http://emmo.info/emmo#EMMO_a2b006f2_bbfd_4dba_bcaa_3fca20cd6be1"/>
    <rdf:type rdf:resource="http://www.w3.org/2002/07/owl#Class"/>
    <EMMO_967080e5_2f42_4eb2_a3a9_c58143e835f9 xml:lang="en">A coarse dispersion of liquid in a solid continuum phase.</EMMO_967080e5_2f42_4eb2_a3a9_c58143e835f9>
  </rdf:Description>
  <rdf:Description rdf:about="http://emmo.info/emmo#EMMO_de178b12_5d35_4bca_8efa_a4193162571d">
    <skos:prefLabel xml:lang="en">physicalDimension</skos:prefLabel>
    <rdfs:subPropertyOf rdf:resource="http://www.w3.org/2000/01/rdf-schema#comment"/>
    <rdfs:comment xml:lang="en">A unique string describing the physical dimensionality of a physical quantity. 

See the comments of PhysicalDimension for a description of this "regex" string.</rdfs:comment>
    <rdf:type rdf:resource="http://www.w3.org/2002/07/owl#AnnotationProperty"/>
    <rdfs:range rdf:resource="http://www.w3.org/2001/XMLSchema#string"/>
  </rdf:Description>
  <rdf:Description rdf:nodeID="f05bdaa1e617a4bccafc519daf7bf4785b35">
    <rdf:type rdf:resource="http://www.w3.org/2002/07/owl#Restriction"/>
    <owl:someValuesFrom rdf:resource="http://emmo.info/emmo#EMMO_ce7d4720_aa20_4a8c_93e8_df41a35b6723"/>
    <owl:onProperty rdf:resource="http://emmo.info/emmo#EMMO_bed1d005_b04e_4a90_94cf_02bc678a8569"/>
  </rdf:Description>
  <rdf:Description rdf:about="http://emmo.info/emmo#EMMO_add2e29d_6d87_4b78_9706_588e25557093">
    <rdf:type rdf:resource="http://www.w3.org/2002/07/owl#Class"/>
    <skos:prefLabel xml:lang="en">Python</skos:prefLabel>
    <rdfs:subClassOf rdf:resource="http://emmo.info/emmo#EMMO_8681074a_e225_4e38_b586_e85b0f43ce38"/>
  </rdf:Description>
  <rdf:Description rdf:nodeID="f05bdaa1e617a4bccafc519daf7bf4785b169">
    <rdf:type rdf:resource="http://www.w3.org/1999/02/22-rdf-syntax-ns#List"/>
    <rdf:first rdf:resource="http://emmo.info/emmo#EMMO_696ed548_9477_45ea_993c_6a8f5271914a"/>
    <rdf:rest rdf:nodeID="f05bdaa1e617a4bccafc519daf7bf4785b170"/>
  </rdf:Description>
  <rdf:Description rdf:nodeID="fe0b20157736f4a31909181349b2e6219b5">
    <rdf:first rdf:resource="http://emmo.info/emmo#EMMO_affe07e4_e9bc_4852_86c6_69e26182a17f"/>
    <rdf:type rdf:resource="http://www.w3.org/1999/02/22-rdf-syntax-ns#List"/>
    <rdf:rest rdf:nodeID="fe0b20157736f4a31909181349b2e6219b6"/>
  </rdf:Description>
  <rdf:Description rdf:nodeID="f05bdaa1e617a4bccafc519daf7bf4785b26">
    <owl:inverseOf rdf:resource="http://emmo.info/emmo#EMMO_3446e167_c576_49d6_846c_215bb8878a55"/>
  </rdf:Description>
  <rdf:Description rdf:about="http://emmo.info/emmo#EMMO_db9a009e_f097_43f5_9520_6cbc07e7610b">
    <rdfs:subClassOf rdf:resource="http://emmo.info/emmo#EMMO_8d2d9374_ef3a_47e6_8595_6bc208e07519"/>
    <skos:prefLabel xml:lang="en">NaturalLaw</skos:prefLabel>
    <rdf:type rdf:resource="http://www.w3.org/2002/07/owl#Class"/>
  </rdf:Description>
  <rdf:Description rdf:nodeID="fdb1489b80bcc4ee28afe0be8feb9b935b3">
    <rdf:type rdf:resource="http://www.w3.org/2002/07/owl#Restriction"/>
    <owl:someValuesFrom rdf:resource="http://emmo.info/emmo#EMMO_10a5fd39_06aa_4648_9e70_f962a9cb2069"/>
    <owl:onProperty rdf:nodeID="fdb1489b80bcc4ee28afe0be8feb9b935b4"/>
  </rdf:Description>
  <rdf:Description rdf:nodeID="fe0b20157736f4a31909181349b2e6219b20">
    <owl:hasValue>T-2 L+1 M+1 I0 Θ0 N0 J0</owl:hasValue>
    <owl:onProperty rdf:resource="http://emmo.info/emmo#EMMO_23b579e1_8088_45b5_9975_064014026c42"/>
    <rdf:type rdf:resource="http://www.w3.org/2002/07/owl#Restriction"/>
  </rdf:Description>
  <rdf:Description rdf:nodeID="f05bdaa1e617a4bccafc519daf7bf4785b186">
    <rdf:type rdf:resource="http://www.w3.org/1999/02/22-rdf-syntax-ns#List"/>
    <rdf:first rdf:resource="http://emmo.info/emmo#EMMO_fab003c8_f7a6_4346_9988_7161325ed7a3"/>
    <rdf:rest rdf:resource="http://www.w3.org/1999/02/22-rdf-syntax-ns#nil"/>
  </rdf:Description>
  <rdf:Description rdf:nodeID="f05bdaa1e617a4bccafc519daf7bf4785b143">
    <owl:onProperty rdf:nodeID="f05bdaa1e617a4bccafc519daf7bf4785b144"/>
    <owl:allValuesFrom rdf:nodeID="f05bdaa1e617a4bccafc519daf7bf4785b145"/>
    <rdf:type rdf:resource="http://www.w3.org/2002/07/owl#Restriction"/>
  </rdf:Description>
  <rdf:Description rdf:nodeID="ff14b31ebf90e4bc5ba2839064d29e543b25">
    <owl:someValuesFrom rdf:resource="http://emmo.info/emmo#EMMO_50781fd9_a9e4_46ad_b7be_4500371d188d"/>
    <owl:onProperty rdf:resource="http://emmo.info/emmo#EMMO_b2282816_b7a3_44c6_b2cb_3feff1ceb7fe"/>
    <rdf:type rdf:resource="http://www.w3.org/2002/07/owl#Restriction"/>
  </rdf:Description>
  <rdf:Description rdf:about="http://emmo.info/emmo#EMMO_3446e167_c576_49d6_846c_215bb8878a55">
    <rdfs:domain rdf:resource="http://emmo.info/emmo#EMMO_54ee6b5e_5261_44a8_86eb_5717e7fdb9d0"/>
    <skos:prefLabel xml:lang="en">hasVariable</skos:prefLabel>
    <rdfs:range rdf:resource="http://emmo.info/emmo#EMMO_1eed0732_e3f1_4b2c_a9c4_b4e75eeb5895"/>
    <rdf:type rdf:resource="http://www.w3.org/2002/07/owl#ObjectProperty"/>
    <rdfs:subPropertyOf rdf:resource="http://emmo.info/emmo#EMMO_eb3518bf_f799_4f9e_8c3e_ce59af11453b"/>
  </rdf:Description>
  <rdf:Description rdf:about="http://emmo.info/emmo#EMMO_8de14a59_660b_454f_aff8_76a07ce185f4">
    <owl:equivalentClass rdf:nodeID="fe24a777e3fd743f986ce83488d2cf30bb20"/>
    <rdfs:subClassOf rdf:resource="http://emmo.info/emmo#EMMO_707f0cd1_941c_4b57_9f20_d0ba30cd6ff3"/>
    <rdf:type rdf:resource="http://www.w3.org/2002/07/owl#Class"/>
    <skos:prefLabel xml:lang="en">Plus</skos:prefLabel>
  </rdf:Description>
  <rdf:Description rdf:nodeID="fe0b20157736f4a31909181349b2e6219b25">
    <rdf:type rdf:resource="http://www.w3.org/2002/07/owl#Restriction"/>
    <owl:hasValue>T0 L0 M+1 I0 Θ0 N0 J0</owl:hasValue>
    <owl:onProperty rdf:resource="http://emmo.info/emmo#EMMO_23b579e1_8088_45b5_9975_064014026c42"/>
  </rdf:Description>
  <rdf:Description rdf:nodeID="f05bdaa1e617a4bccafc519daf7bf4785b180">
    <rdf:type rdf:resource="http://www.w3.org/1999/02/22-rdf-syntax-ns#List"/>
    <rdf:first rdf:resource="http://emmo.info/emmo#EMMO_d7f11b34_a121_4519_87c0_aa754f1c4737"/>
    <rdf:rest rdf:nodeID="f05bdaa1e617a4bccafc519daf7bf4785b181"/>
  </rdf:Description>
  <rdf:Description rdf:nodeID="fea11ca01461e402d8f697c19c5d8de88b8">
    <rdf:type rdf:resource="http://www.w3.org/2002/07/owl#Restriction"/>
    <owl:onProperty rdf:resource="http://emmo.info/emmo#EMMO_17e27c22_37e1_468c_9dd7_95e137f73e7f"/>
    <owl:someValuesFrom rdf:resource="http://emmo.info/emmo#EMMO_385b8f6e_43ac_4596_ad76_ac322c68b7ca"/>
  </rdf:Description>
  <rdf:Description rdf:nodeID="fe0b20157736f4a31909181349b2e6219b30">
    <owl:hasValue>T0 L0 M0 I0 Θ0 N-1 J0</owl:hasValue>
    <rdf:type rdf:resource="http://www.w3.org/2002/07/owl#Restriction"/>
    <owl:onProperty rdf:resource="http://emmo.info/emmo#EMMO_23b579e1_8088_45b5_9975_064014026c42"/>
  </rdf:Description>
  <rdf:Description rdf:nodeID="f05bdaa1e617a4bccafc519daf7bf4785b4">
    <owl:inverseOf rdf:resource="http://emmo.info/emmo#EMMO_3446e167_c576_49d6_846c_215bb8878a55"/>
  </rdf:Description>
  <rdf:Description rdf:nodeID="f05bdaa1e617a4bccafc519daf7bf4785b144">
    <owl:inverseOf rdf:resource="http://emmo.info/emmo#EMMO_3446e167_c576_49d6_846c_215bb8878a55"/>
  </rdf:Description>
  <rdf:Description rdf:nodeID="fdb1489b80bcc4ee28afe0be8feb9b935b10">
    <owl:inverseOf rdf:resource="http://emmo.info/emmo#EMMO_e1097637_70d2_4895_973f_2396f04fa204"/>
  </rdf:Description>
  <rdf:Description rdf:nodeID="f05bdaa1e617a4bccafc519daf7bf4785b160">
    <owl:hasValue>Hz</owl:hasValue>
    <rdf:type rdf:resource="http://www.w3.org/2002/07/owl#Restriction"/>
    <owl:onProperty rdf:resource="http://emmo.info/emmo#EMMO_23b579e1_8088_45b5_9975_064014026c42"/>
  </rdf:Description>
  <rdf:Description rdf:nodeID="fea11ca01461e402d8f697c19c5d8de88b3">
    <rdf:type rdf:resource="http://www.w3.org/1999/02/22-rdf-syntax-ns#List"/>
    <rdf:rest rdf:resource="http://www.w3.org/1999/02/22-rdf-syntax-ns#nil"/>
    <rdf:first rdf:resource="http://emmo.info/emmo#EMMO_8043d3c6_a4c1_4089_ba34_9744e28e5b3d"/>
  </rdf:Description>
  <rdf:Description rdf:nodeID="f8fb83657cd5f496db3c2b94baf326f26b26">
    <owl:onProperty rdf:resource="http://emmo.info/emmo#EMMO_67fc0a36_8dcb_4ffa_9a43_31074efa3296"/>
    <rdf:type rdf:resource="http://www.w3.org/2002/07/owl#Restriction"/>
    <owl:allValuesFrom rdf:resource="http://emmo.info/emmo#EMMO_db716151_6b73_45ff_910c_d182fdcbb4f5"/>
  </rdf:Description>
  <rdf:Description rdf:nodeID="f05bdaa1e617a4bccafc519daf7bf4785b5">
    <owl:hasValue rdf:datatype="http://www.w3.org/2001/XMLSchema#double">1e-12</owl:hasValue>
    <rdf:type rdf:resource="http://www.w3.org/2002/07/owl#Restriction"/>
    <owl:onProperty rdf:resource="http://emmo.info/emmo#EMMO_faf79f53_749d_40b2_807c_d34244c192f4"/>
  </rdf:Description>
  <rdf:Description rdf:nodeID="f0b819106611c4b798f33b16c65f4398db6">
    <owl:inverseOf rdf:resource="http://emmo.info/emmo#EMMO_ae2d1a96_bfa1_409a_a7d2_03d69e8a125a"/>
  </rdf:Description>
  <rdf:Description rdf:nodeID="f05bdaa1e617a4bccafc519daf7bf4785b146">
    <owl:hasValue>Z</owl:hasValue>
    <owl:onProperty rdf:resource="http://emmo.info/emmo#EMMO_23b579e1_8088_45b5_9975_064014026c42"/>
    <rdf:type rdf:resource="http://www.w3.org/2002/07/owl#Restriction"/>
  </rdf:Description>
  <rdf:Description rdf:nodeID="ff14b31ebf90e4bc5ba2839064d29e543b13">
    <rdf:first rdf:resource="http://emmo.info/emmo#EMMO_d4f37e32_16ae_4cc6_b4cd_fd896b2449c4"/>
    <rdf:rest rdf:nodeID="ff14b31ebf90e4bc5ba2839064d29e543b14"/>
    <rdf:type rdf:resource="http://www.w3.org/1999/02/22-rdf-syntax-ns#List"/>
  </rdf:Description>
  <rdf:Description rdf:nodeID="fdb1489b80bcc4ee28afe0be8feb9b935b2">
    <rdf:type rdf:resource="http://www.w3.org/2002/07/owl#Restriction"/>
    <owl:onProperty rdf:resource="http://emmo.info/emmo#EMMO_ae2d1a96_bfa1_409a_a7d2_03d69e8a125a"/>
    <owl:someValuesFrom rdf:resource="http://emmo.info/emmo#EMMO_b7bcff25_ffc3_474e_9ab5_01b1664bd4ba"/>
  </rdf:Description>
  <rdf:Description rdf:nodeID="f05bdaa1e617a4bccafc519daf7bf4785b54">
    <rdf:type rdf:resource="http://www.w3.org/2002/07/owl#Restriction"/>
    <owl:onProperty rdf:resource="http://emmo.info/emmo#EMMO_faf79f53_749d_40b2_807c_d34244c192f4"/>
    <owl:hasValue rdf:datatype="http://www.w3.org/2001/XMLSchema#double">1000000000000000.0</owl:hasValue>
  </rdf:Description>
  <rdf:Description rdf:nodeID="f05bdaa1e617a4bccafc519daf7bf4785b128">
    <owl:hasValue>°C</owl:hasValue>
    <owl:onProperty rdf:resource="http://emmo.info/emmo#EMMO_23b579e1_8088_45b5_9975_064014026c42"/>
    <rdf:type rdf:resource="http://www.w3.org/2002/07/owl#Restriction"/>
  </rdf:Description>
  <rdf:Description rdf:nodeID="f05bdaa1e617a4bccafc519daf7bf4785b8">
    <owl:onProperty rdf:resource="http://emmo.info/emmo#EMMO_23b579e1_8088_45b5_9975_064014026c42"/>
    <rdf:type rdf:resource="http://www.w3.org/2002/07/owl#Restriction"/>
    <owl:hasValue>W</owl:hasValue>
  </rdf:Description>
  <rdf:Description rdf:nodeID="f05bdaa1e617a4bccafc519daf7bf4785b91">
    <owl:allValuesFrom rdf:nodeID="f05bdaa1e617a4bccafc519daf7bf4785b93"/>
    <rdf:type rdf:resource="http://www.w3.org/2002/07/owl#Restriction"/>
    <owl:onProperty rdf:nodeID="f05bdaa1e617a4bccafc519daf7bf4785b92"/>
  </rdf:Description>
  <rdf:Description rdf:nodeID="fe0b20157736f4a31909181349b2e6219b14">
    <rdf:type rdf:resource="http://www.w3.org/2002/07/owl#Restriction"/>
    <owl:onProperty rdf:resource="http://emmo.info/emmo#EMMO_23b579e1_8088_45b5_9975_064014026c42"/>
    <owl:hasValue>T-2 L+2 M+1 I0 Θ-1 N0 J0</owl:hasValue>
  </rdf:Description>
  <rdf:Description rdf:nodeID="fa691b5894b3543efa24f9838ff46c3eab1">
    <owl:someValuesFrom rdf:resource="http://emmo.info/emmo#EMMO_0527413c_b286_4e9c_b2d0_03fb2a038dee"/>
    <owl:onProperty rdf:resource="http://emmo.info/emmo#EMMO_c5aae418_1622_4d02_93c5_21159e28e6c1"/>
    <rdf:type rdf:resource="http://www.w3.org/2002/07/owl#Restriction"/>
  </rdf:Description>
  <rdf:Description rdf:nodeID="fe0b20157736f4a31909181349b2e6219b19">
    <owl:onProperty rdf:resource="http://emmo.info/emmo#EMMO_23b579e1_8088_45b5_9975_064014026c42"/>
    <rdf:type rdf:resource="http://www.w3.org/2002/07/owl#Restriction"/>
    <owl:hasValue>T-2 L-1 M+1 I0 Θ0 N0 J0</owl:hasValue>
  </rdf:Description>
  <rdf:Description rdf:nodeID="f05bdaa1e617a4bccafc519daf7bf4785b79">
    <owl:inverseOf rdf:resource="http://emmo.info/emmo#EMMO_3446e167_c576_49d6_846c_215bb8878a55"/>
  </rdf:Description>
  <rdf:Description rdf:nodeID="f8fb83657cd5f496db3c2b94baf326f26b21">
    <owl:unionOf rdf:nodeID="f8fb83657cd5f496db3c2b94baf326f26b22"/>
    <rdf:type rdf:resource="http://www.w3.org/2002/07/owl#Class"/>
  </rdf:Description>
  <rdf:Description rdf:nodeID="f05bdaa1e617a4bccafc519daf7bf4785b81">
    <owl:hasValue>E</owl:hasValue>
    <owl:onProperty rdf:resource="http://emmo.info/emmo#EMMO_23b579e1_8088_45b5_9975_064014026c42"/>
    <rdf:type rdf:resource="http://www.w3.org/2002/07/owl#Restriction"/>
  </rdf:Description>
  <rdf:Description rdf:nodeID="fe0b20157736f4a31909181349b2e6219b39">
    <owl:inverseOf rdf:resource="http://emmo.info/emmo#EMMO_e1097637_70d2_4895_973f_2396f04fa204"/>
  </rdf:Description>
  <rdf:Description rdf:nodeID="ffcb99037244f48d590430c228d02afdbb48">
    <owl:hasValue>min</owl:hasValue>
    <rdf:type rdf:resource="http://www.w3.org/2002/07/owl#Restriction"/>
    <owl:onProperty rdf:resource="http://emmo.info/emmo#EMMO_23b579e1_8088_45b5_9975_064014026c42"/>
  </rdf:Description>
  <rdf:Description rdf:nodeID="f8fb83657cd5f496db3c2b94baf326f26b31">
    <rdf:first rdf:resource="http://emmo.info/emmo#EMMO_89762966_8076_4f7c_b745_f718d653e8e2"/>
    <rdf:rest rdf:resource="http://www.w3.org/1999/02/22-rdf-syntax-ns#nil"/>
    <rdf:type rdf:resource="http://www.w3.org/1999/02/22-rdf-syntax-ns#List"/>
  </rdf:Description>
  <rdf:Description rdf:nodeID="f05bdaa1e617a4bccafc519daf7bf4785b74">
    <rdf:first rdf:resource="http://emmo.info/emmo#EMMO_e79c62ff_10ad_4ec0_baba_c19ddd4eaa11"/>
    <rdf:rest rdf:nodeID="f05bdaa1e617a4bccafc519daf7bf4785b75"/>
    <rdf:type rdf:resource="http://www.w3.org/1999/02/22-rdf-syntax-ns#List"/>
  </rdf:Description>
  <rdf:Description rdf:nodeID="fa691b5894b3543efa24f9838ff46c3eab10">
    <rdf:type rdf:resource="http://www.w3.org/1999/02/22-rdf-syntax-ns#List"/>
    <rdf:rest rdf:nodeID="fa691b5894b3543efa24f9838ff46c3eab11"/>
    <rdf:first rdf:resource="http://emmo.info/emmo#EMMO_0527413c_b286_4e9c_b2d0_03fb2a038dee"/>
  </rdf:Description>
  <rdf:Description rdf:nodeID="ffcb99037244f48d590430c228d02afdbb58">
    <owl:someValuesFrom rdf:resource="http://emmo.info/emmo#EMMO_77e9dc31_5b19_463e_b000_44c6e79f98aa"/>
    <rdf:type rdf:resource="http://www.w3.org/2002/07/owl#Restriction"/>
    <owl:onProperty rdf:resource="http://emmo.info/emmo#EMMO_bed1d005_b04e_4a90_94cf_02bc678a8569"/>
  </rdf:Description>
  <rdf:Description rdf:about="http://emmo.info/emmo#EMMO_96c8d72f_b436_44e2_9f7f_085c24094292">
    <EMMO_967080e5_2f42_4eb2_a3a9_c58143e835f9 xml:lang="en">An aerosol composed of fine solid particles in air or another gas.</EMMO_967080e5_2f42_4eb2_a3a9_c58143e835f9>
    <rdfs:subClassOf rdf:resource="http://emmo.info/emmo#EMMO_560d833a_6184_410c_859a_05d982712fd7"/>
    <skos:prefLabel xml:lang="en">SolidAerosol</skos:prefLabel>
    <rdf:type rdf:resource="http://www.w3.org/2002/07/owl#Class"/>
  </rdf:Description>
  <rdf:Description rdf:nodeID="ffcb99037244f48d590430c228d02afdbb28">
    <rdf:rest rdf:nodeID="ffcb99037244f48d590430c228d02afdbb29"/>
    <rdf:first rdf:resource="http://emmo.info/emmo#EMMO_d6eb0176_a0d7_4b4e_8df0_50e912be2342"/>
    <rdf:type rdf:resource="http://www.w3.org/1999/02/22-rdf-syntax-ns#List"/>
  </rdf:Description>
  <rdf:Description rdf:nodeID="f05bdaa1e617a4bccafc519daf7bf4785b70">
    <rdf:type rdf:resource="http://www.w3.org/1999/02/22-rdf-syntax-ns#List"/>
    <rdf:rest rdf:nodeID="f05bdaa1e617a4bccafc519daf7bf4785b71"/>
    <rdf:first rdf:resource="http://emmo.info/emmo#EMMO_a8eb4bbb_1bd3_4ad4_b114_2789bcbd2134"/>
  </rdf:Description>
  <rdf:Description rdf:nodeID="f8fb83657cd5f496db3c2b94baf326f26b15">
    <rdf:type rdf:resource="http://www.w3.org/2002/07/owl#Class"/>
    <owl:intersectionOf rdf:nodeID="f8fb83657cd5f496db3c2b94baf326f26b16"/>
  </rdf:Description>
  <rdf:Description rdf:nodeID="f05bdaa1e617a4bccafc519daf7bf4785b171">
    <rdf:first rdf:resource="http://emmo.info/emmo#EMMO_a121bb1d_5225_4c78_809b_0268c3012208"/>
    <rdf:rest rdf:nodeID="f05bdaa1e617a4bccafc519daf7bf4785b172"/>
    <rdf:type rdf:resource="http://www.w3.org/1999/02/22-rdf-syntax-ns#List"/>
  </rdf:Description>
  <rdf:Description rdf:nodeID="ff14b31ebf90e4bc5ba2839064d29e543b22">
    <rdf:rest rdf:resource="http://www.w3.org/1999/02/22-rdf-syntax-ns#nil"/>
    <rdf:type rdf:resource="http://www.w3.org/1999/02/22-rdf-syntax-ns#List"/>
    <rdf:first rdf:resource="http://emmo.info/emmo#EMMO_a2b006f2_bbfd_4dba_bcaa_3fca20cd6be1"/>
  </rdf:Description>
  <rdf:Description rdf:nodeID="f05bdaa1e617a4bccafc519daf7bf4785b168">
    <rdf:type rdf:resource="http://www.w3.org/1999/02/22-rdf-syntax-ns#List"/>
    <rdf:rest rdf:nodeID="f05bdaa1e617a4bccafc519daf7bf4785b169"/>
    <rdf:first rdf:resource="http://emmo.info/emmo#EMMO_59c10c5c_47bd_4348_ba39_38836607dfa1"/>
  </rdf:Description>
  <rdf:Description rdf:nodeID="fe0b20157736f4a31909181349b2e6219b36">
    <owl:onProperty rdf:resource="http://emmo.info/emmo#EMMO_23b579e1_8088_45b5_9975_064014026c42"/>
    <rdf:type rdf:resource="http://www.w3.org/2002/07/owl#Restriction"/>
    <owl:hasValue>T0 L0 M0 I0 Θ0 N+1 J0</owl:hasValue>
  </rdf:Description>
  <rdf:Description rdf:nodeID="f05bdaa1e617a4bccafc519daf7bf4785b195">
    <rdf:first rdf:resource="http://emmo.info/emmo#EMMO_1273eb34_de48_43a9_925f_104110469dd2"/>
    <rdf:rest rdf:nodeID="f05bdaa1e617a4bccafc519daf7bf4785b196"/>
    <rdf:type rdf:resource="http://www.w3.org/1999/02/22-rdf-syntax-ns#List"/>
  </rdf:Description>
  <rdf:Description rdf:nodeID="ffcb99037244f48d590430c228d02afdbb9">
    <rdf:type rdf:resource="http://www.w3.org/2002/07/owl#Restriction"/>
    <owl:onProperty rdf:resource="http://emmo.info/emmo#EMMO_bed1d005_b04e_4a90_94cf_02bc678a8569"/>
    <owl:someValuesFrom rdf:resource="http://emmo.info/emmo#EMMO_02e894c3_b793_4197_b120_3442e08f58d1"/>
  </rdf:Description>
  <rdf:Description rdf:nodeID="f8fb83657cd5f496db3c2b94baf326f26b6">
    <rdf:first rdf:resource="http://emmo.info/emmo#EMMO_a1083d0a_c1fb_471f_8e20_a98f881ad527"/>
    <rdf:type rdf:resource="http://www.w3.org/1999/02/22-rdf-syntax-ns#List"/>
    <rdf:rest rdf:resource="http://www.w3.org/1999/02/22-rdf-syntax-ns#nil"/>
  </rdf:Description>
  <rdf:Description rdf:nodeID="f627ff42579444148ae27fcacfb5f8528b3">
    <owl:onProperty rdf:nodeID="f627ff42579444148ae27fcacfb5f8528b4"/>
    <owl:someValuesFrom rdf:resource="http://emmo.info/emmo#EMMO_314d0bd5_67ed_437e_a609_36d46147cea7"/>
    <rdf:type rdf:resource="http://www.w3.org/2002/07/owl#Restriction"/>
  </rdf:Description>
  <rdf:Description rdf:about="http://emmo.info/emmo#EMMO_873b0ab3_88e6_4054_b901_5531e01f14a4">
    <rdf:type rdf:resource="http://www.w3.org/2002/07/owl#Class"/>
    <skos:prefLabel xml:lang="en">MeasuredQuantitativeProperty</skos:prefLabel>
  </rdf:Description>
  <rdf:Description rdf:nodeID="f05bdaa1e617a4bccafc519daf7bf4785b67">
    <rdf:first rdf:resource="http://emmo.info/emmo#EMMO_74931b1b_c133_4e59_9a75_1bf0e1626201"/>
    <rdf:type rdf:resource="http://www.w3.org/1999/02/22-rdf-syntax-ns#List"/>
    <rdf:rest rdf:nodeID="f05bdaa1e617a4bccafc519daf7bf4785b68"/>
  </rdf:Description>
  <rdf:Description rdf:nodeID="fdb1489b80bcc4ee28afe0be8feb9b935b8">
    <owl:inverseOf rdf:resource="http://emmo.info/emmo#EMMO_ae2d1a96_bfa1_409a_a7d2_03d69e8a125a"/>
  </rdf:Description>
  <rdf:Description rdf:about="http://www.w3.org/2000/01/rdf-schema#comment">
    <rdfs:range rdf:resource="http://www.w3.org/2000/01/rdf-schema#Literal"/>
  </rdf:Description>
  <rdf:Description rdf:about="http://purl.org/dc/terms/creator">
    <rdf:type rdf:resource="http://www.w3.org/2002/07/owl#AnnotationProperty"/>
  </rdf:Description>
  <rdf:Description rdf:nodeID="fe0b20157736f4a31909181349b2e6219b17">
    <owl:hasValue>T-1 L+2 M+1 I0 Θ0 N0 J0</owl:hasValue>
    <owl:onProperty rdf:resource="http://emmo.info/emmo#EMMO_23b579e1_8088_45b5_9975_064014026c42"/>
    <rdf:type rdf:resource="http://www.w3.org/2002/07/owl#Restriction"/>
  </rdf:Description>
  <rdf:Description rdf:nodeID="f627ff42579444148ae27fcacfb5f8528b6">
    <owl:inverseOf rdf:resource="http://emmo.info/emmo#EMMO_24c71baf_6db6_48b9_86c8_8c70cf36db0c"/>
  </rdf:Description>
  <rdf:Description rdf:nodeID="f8fb83657cd5f496db3c2b94baf326f26b13">
    <owl:someValuesFrom rdf:resource="http://emmo.info/emmo#EMMO_08b308d4_31cd_4779_a784_aa92fc730f39"/>
    <owl:onProperty rdf:nodeID="f8fb83657cd5f496db3c2b94baf326f26b14"/>
    <rdf:type rdf:resource="http://www.w3.org/2002/07/owl#Restriction"/>
  </rdf:Description>
  <rdf:Description rdf:nodeID="f05bdaa1e617a4bccafc519daf7bf4785b72">
    <rdf:type rdf:resource="http://www.w3.org/1999/02/22-rdf-syntax-ns#List"/>
    <rdf:rest rdf:nodeID="f05bdaa1e617a4bccafc519daf7bf4785b73"/>
    <rdf:first rdf:resource="http://emmo.info/emmo#EMMO_daa9ee97_4c5f_42e5_918c_44d7523e8958"/>
  </rdf:Description>
  <rdf:Description rdf:about="http://emmo.info/emmo#EMMO_24c71baf_6db6_48b9_86c8_8c70cf36db0c">
    <rdfs:subPropertyOf rdf:resource="http://emmo.info/emmo#EMMO_39c3815d_8cae_4c8f_b2ff_eeba24bec455"/>
    <rdf:type rdf:resource="http://www.w3.org/2002/07/owl#ObjectProperty"/>
    <skos:prefLabel xml:lang="en">hasModel</skos:prefLabel>
  </rdf:Description>
  <rdf:Description rdf:about="http://emmo.info/emmo#EMMO_84cadc45_6758_46f2_ba2a_5ead65c70213">
    <EMMO_967080e5_2f42_4eb2_a3a9_c58143e835f9 xml:lang="en">A physics-based model based on a physics equation describing the behaviour of atoms.</EMMO_967080e5_2f42_4eb2_a3a9_c58143e835f9>
    <skos:prefLabel xml:lang="en">AtomisticModel</skos:prefLabel>
    <rdfs:subClassOf rdf:resource="http://emmo.info/emmo#EMMO_b29fd350_39aa_4af7_9459_3faa0544cba6"/>
    <rdf:type rdf:resource="http://www.w3.org/2002/07/owl#Class"/>
  </rdf:Description>
  <rdf:Description rdf:about="http://emmo.info/emmo#EMMO_b9695e87_8261_412e_83cd_a86459426a28">
    <rdf:type rdf:resource="http://www.w3.org/2002/07/owl#Class"/>
    <owl:disjointUnionOf rdf:nodeID="ff14b31ebf90e4bc5ba2839064d29e543b19"/>
    <rdfs:comment xml:lang="en">In physics, a state of matter is one of the distinct forms in which matter can exist. Four states of matter are observable in everyday life: solid, liquid, gas, and plasma.

https://en.wikipedia.org/wiki/State_of_matter</rdfs:comment>
    <EMMO_967080e5_2f42_4eb2_a3a9_c58143e835f9 xml:lang="en">A superclass made as the disjoint union of all the form under which matter can exist.</EMMO_967080e5_2f42_4eb2_a3a9_c58143e835f9>
    <skos:prefLabel xml:lang="en">StateOfMatter</skos:prefLabel>
    <rdfs:subClassOf rdf:resource="http://emmo.info/emmo#EMMO_5b2222df_4da6_442f_8244_96e9e45887d1"/>
  </rdf:Description>
  <rdf:Description rdf:nodeID="f05bdaa1e617a4bccafc519daf7bf4785b193">
    <owl:onProperty rdf:resource="http://emmo.info/emmo#EMMO_bed1d005_b04e_4a90_94cf_02bc678a8569"/>
    <owl:someValuesFrom rdf:resource="http://emmo.info/emmo#EMMO_585e0ff0_9429_4d3c_b578_58abb1ba21d1"/>
    <rdf:type rdf:resource="http://www.w3.org/2002/07/owl#Restriction"/>
  </rdf:Description>
  <rdf:Description rdf:nodeID="f05bdaa1e617a4bccafc519daf7bf4785b45">
    <owl:inverseOf rdf:resource="http://emmo.info/emmo#EMMO_3446e167_c576_49d6_846c_215bb8878a55"/>
  </rdf:Description>
  <rdf:Description rdf:nodeID="f38ecd0eaa78747b4ad569754ea441153b3">
    <owl:onProperty rdf:resource="http://emmo.info/emmo#EMMO_f68030be_94b8_4c61_a161_886468558054"/>
    <rdf:type rdf:resource="http://www.w3.org/2002/07/owl#Restriction"/>
    <owl:someValuesFrom rdf:resource="http://emmo.info/emmo#EMMO_057e7d57_aff0_49de_911a_8861d85cef40"/>
  </rdf:Description>
  <rdf:Description rdf:nodeID="fdb1489b80bcc4ee28afe0be8feb9b935b11">
    <rdf:rest rdf:nodeID="fdb1489b80bcc4ee28afe0be8feb9b935b12"/>
    <rdf:first rdf:resource="http://emmo.info/emmo#EMMO_251cfb4f_5c75_4778_91ed_6c8395212fd8"/>
    <rdf:type rdf:resource="http://www.w3.org/1999/02/22-rdf-syntax-ns#List"/>
  </rdf:Description>
  <rdf:Description rdf:nodeID="fa691b5894b3543efa24f9838ff46c3eab5">
    <owl:unionOf rdf:nodeID="fa691b5894b3543efa24f9838ff46c3eab6"/>
    <rdf:type rdf:resource="http://www.w3.org/2002/07/owl#Class"/>
  </rdf:Description>
  <rdf:Description rdf:nodeID="f05bdaa1e617a4bccafc519daf7bf4785b57">
    <rdf:first rdf:resource="http://emmo.info/emmo#EMMO_1181c938_c8f0_4ad6_bc7a_2bfdc0903d29"/>
    <rdf:type rdf:resource="http://www.w3.org/1999/02/22-rdf-syntax-ns#List"/>
    <rdf:rest rdf:nodeID="f05bdaa1e617a4bccafc519daf7bf4785b58"/>
  </rdf:Description>
  <rdf:Description rdf:about="http://emmo.info/emmo#EMMO_057e7d57_aff0_49de_911a_8861d85cef40">
    <EMMO_b432d2d5_25f4_4165_99c5_5935a7763c1a xml:lang="en">fe780
emmo
!5*a
cat
for(i=0;i&lt;N;++i)</EMMO_b432d2d5_25f4_4165_99c5_5935a7763c1a>
    <skos:prefLabel xml:lang="en">Symbolic</skos:prefLabel>
    <rdfs:subClassOf rdf:resource="http://emmo.info/emmo#EMMO_c74da218_9147_4f03_92d1_8894abca55f3"/>
    <EMMO_967080e5_2f42_4eb2_a3a9_c58143e835f9 xml:lang="en">An 'Graphical' that stands for a token or a composition of tokens from one or more alphabets, without necessarily respecting syntactic rules.</EMMO_967080e5_2f42_4eb2_a3a9_c58143e835f9>
    <rdf:type rdf:resource="http://www.w3.org/2002/07/owl#Class"/>
  </rdf:Description>
  <rdf:Description rdf:nodeID="f8fb83657cd5f496db3c2b94baf326f26b2">
    <rdf:first rdf:resource="http://emmo.info/emmo#EMMO_71f6ab56_342c_484b_bbe0_de86b7367cb3"/>
    <rdf:rest rdf:nodeID="f8fb83657cd5f496db3c2b94baf326f26b3"/>
    <rdf:type rdf:resource="http://www.w3.org/1999/02/22-rdf-syntax-ns#List"/>
  </rdf:Description>
  <rdf:Description rdf:nodeID="f8fb83657cd5f496db3c2b94baf326f26b9">
    <rdf:first rdf:resource="http://emmo.info/emmo#EMMO_b081b346_7279_46ef_9a3d_2c088fcd79f4"/>
    <rdf:type rdf:resource="http://www.w3.org/1999/02/22-rdf-syntax-ns#List"/>
    <rdf:rest rdf:resource="http://www.w3.org/1999/02/22-rdf-syntax-ns#nil"/>
  </rdf:Description>
  <rdf:Description rdf:nodeID="ffcb99037244f48d590430c228d02afdbb52">
    <rdf:type rdf:resource="http://www.w3.org/2002/07/owl#Restriction"/>
    <owl:onProperty rdf:resource="http://emmo.info/emmo#EMMO_23b579e1_8088_45b5_9975_064014026c42"/>
    <owl:hasValue>eV</owl:hasValue>
  </rdf:Description>
  <rdf:Description rdf:nodeID="f05bdaa1e617a4bccafc519daf7bf4785b155">
    <owl:hasValue rdf:datatype="http://www.w3.org/2001/XMLSchema#double">1e-09</owl:hasValue>
    <rdf:type rdf:resource="http://www.w3.org/2002/07/owl#Restriction"/>
    <owl:onProperty rdf:resource="http://emmo.info/emmo#EMMO_faf79f53_749d_40b2_807c_d34244c192f4"/>
  </rdf:Description>
  <rdf:Description rdf:nodeID="f05bdaa1e617a4bccafc519daf7bf4785b200">
    <owl:qualifiedCardinality rdf:datatype="http://www.w3.org/2001/XMLSchema#nonNegativeInteger">1</owl:qualifiedCardinality>
  </rdf:Description>
  <rdf:Description rdf:nodeID="ff14b31ebf90e4bc5ba2839064d29e543b11">
    <rdf:rest rdf:nodeID="ff14b31ebf90e4bc5ba2839064d29e543b12"/>
    <rdf:type rdf:resource="http://www.w3.org/1999/02/22-rdf-syntax-ns#List"/>
    <rdf:first rdf:resource="http://emmo.info/emmo#EMMO_47fe2379_be21_48d1_9ede_402f0faf494b"/>
  </rdf:Description>
  <rdf:Description rdf:nodeID="f05bdaa1e617a4bccafc519daf7bf4785b177">
    <rdf:first rdf:resource="http://emmo.info/emmo#EMMO_b71e4ba5_8f73_4199_8c96_7ea7f94d9e2a"/>
    <rdf:type rdf:resource="http://www.w3.org/1999/02/22-rdf-syntax-ns#List"/>
    <rdf:rest rdf:nodeID="f05bdaa1e617a4bccafc519daf7bf4785b178"/>
  </rdf:Description>
  <rdf:Description rdf:nodeID="f05bdaa1e617a4bccafc519daf7bf4785b60">
    <rdf:rest rdf:nodeID="f05bdaa1e617a4bccafc519daf7bf4785b61"/>
    <rdf:type rdf:resource="http://www.w3.org/1999/02/22-rdf-syntax-ns#List"/>
    <rdf:first rdf:resource="http://emmo.info/emmo#EMMO_23bfe79a_cade_48f1_9a8c_fd96e6bac8ba"/>
  </rdf:Description>
  <rdf:Description rdf:nodeID="f05bdaa1e617a4bccafc519daf7bf4785b118">
    <owl:inverseOf rdf:resource="http://emmo.info/emmo#EMMO_3446e167_c576_49d6_846c_215bb8878a55"/>
  </rdf:Description>
  <rdf:Description rdf:nodeID="ffbe75b10062f400ea693809785c50a44b4">
    <owl:inverseOf rdf:resource="http://emmo.info/emmo#EMMO_c5aae418_1622_4d02_93c5_21159e28e6c1"/>
  </rdf:Description>
  <rdf:Description rdf:nodeID="fe24a777e3fd743f986ce83488d2cf30bb15">
    <rdf:rest rdf:resource="http://www.w3.org/1999/02/22-rdf-syntax-ns#nil"/>
    <rdf:first rdf:resource="http://emmo.info/emmo#EMMO_a1083d0a_c1fb_471f_8e20_a98f881ad527"/>
    <rdf:type rdf:resource="http://www.w3.org/1999/02/22-rdf-syntax-ns#List"/>
  </rdf:Description>
  <rdf:Description rdf:about="http://emmo.info/emmo#EMMO_7509da43_56b1_4d7f_887a_65d1663df4ba">
    <rdf:type rdf:resource="http://www.w3.org/2002/07/owl#Class"/>
    <EMMO_967080e5_2f42_4eb2_a3a9_c58143e835f9 xml:lang="en">A liquid is a nearly incompressible fluid that conforms to the shape of its container but retains a (nearly) constant volume independent of pressure.</EMMO_967080e5_2f42_4eb2_a3a9_c58143e835f9>
    <skos:prefLabel xml:lang="en">Liquid</skos:prefLabel>
    <rdfs:subClassOf rdf:resource="http://emmo.info/emmo#EMMO_87ac88ff_8379_4f5a_8c7b_424a8fff1ee8"/>
  </rdf:Description>
  <rdf:Description rdf:about="http://emmo.info/emmo#EMMO_86060335_31c2_4820_b433_27c64aea0366">
    <rdf:type rdf:resource="http://www.w3.org/2002/07/owl#Class"/>
    <skos:prefLabel xml:lang="en">Torus</skos:prefLabel>
    <rdfs:subClassOf rdf:resource="http://emmo.info/emmo#EMMO_9268958f_7f54_48ab_a693_febe2645892b"/>
  </rdf:Description>
  <rdf:Description rdf:nodeID="fa691b5894b3543efa24f9838ff46c3eab4">
    <owl:someValuesFrom rdf:resource="http://emmo.info/emmo#EMMO_054af807_85cd_4a13_8eba_119dfdaaf38b"/>
    <rdf:type rdf:resource="http://www.w3.org/2002/07/owl#Restriction"/>
    <owl:onProperty rdf:resource="http://emmo.info/emmo#EMMO_f68030be_94b8_4c61_a161_886468558054"/>
  </rdf:Description>
  <rdf:Description rdf:about="http://emmo.info/emmo#EMMO_0ab0485c_9e5b_4257_a679_90a2dfba5c7c">
    <rdf:type rdf:resource="http://www.w3.org/2002/07/owl#Class"/>
    <skos:prefLabel xml:lang="en">0-manifold</skos:prefLabel>
    <rdfs:subClassOf rdf:resource="http://emmo.info/emmo#EMMO_b5957cef_a287_442d_a3ce_fd39f20ba1cd"/>
  </rdf:Description>
  <rdf:Description rdf:nodeID="fea11ca01461e402d8f697c19c5d8de88b11">
    <rdf:type rdf:resource="http://www.w3.org/2002/07/owl#Restriction"/>
    <owl:allValuesFrom rdf:resource="http://emmo.info/emmo#EMMO_70dac51e_bddd_48c2_8a98_7d8395e91fc2"/>
    <owl:onProperty rdf:resource="http://emmo.info/emmo#EMMO_7afbed84_7593_4a23_bd88_9d9c6b04e8f6"/>
  </rdf:Description>
  <rdf:Description rdf:about="http://emmo.info/emmo#EMMO_2e7e5796_4a80_4d73_bb84_f31138446c0c">
    <owl:equivalentClass rdf:nodeID="fe0b20157736f4a31909181349b2e6219b11"/>
    <rdfs:subClassOf rdf:resource="http://emmo.info/emmo#EMMO_9895a1b4_f0a5_4167_ac5e_97db40b8bfcc"/>
    <skos:prefLabel xml:lang="en">ElectricPotentialDimension</skos:prefLabel>
    <rdf:type rdf:resource="http://www.w3.org/2002/07/owl#Class"/>
  </rdf:Description>
  <rdf:Description rdf:nodeID="f3b8e3e5cecf14b688acdf306cd5f62cbb1">
    <owl:unionOf rdf:nodeID="f3b8e3e5cecf14b688acdf306cd5f62cbb2"/>
    <rdf:type rdf:resource="http://www.w3.org/2002/07/owl#Class"/>
  </rdf:Description>
  <rdf:Description rdf:nodeID="f15a17d1fb53e4dd795c7db922ceff6acb6">
    <rdf:first rdf:resource="http://emmo.info/emmo#EMMO_2d2ecd97_067f_4d0e_950c_d746b7700a31"/>
    <rdf:type rdf:resource="http://www.w3.org/1999/02/22-rdf-syntax-ns#List"/>
    <rdf:rest rdf:nodeID="f15a17d1fb53e4dd795c7db922ceff6acb7"/>
  </rdf:Description>
  <rdf:Description rdf:nodeID="fea11ca01461e402d8f697c19c5d8de88b21">
    <rdf:type rdf:resource="http://www.w3.org/1999/02/22-rdf-syntax-ns#List"/>
    <rdf:first rdf:resource="http://emmo.info/emmo#EMMO_25f8b804_9a0b_4387_a3e7_b35bce5365ee"/>
    <rdf:rest rdf:nodeID="fea11ca01461e402d8f697c19c5d8de88b22"/>
  </rdf:Description>
  <rdf:Description rdf:nodeID="f05bdaa1e617a4bccafc519daf7bf4785b104">
    <owl:onProperty rdf:resource="http://emmo.info/emmo#EMMO_23b579e1_8088_45b5_9975_064014026c42"/>
    <owl:hasValue>kg</owl:hasValue>
    <rdf:type rdf:resource="http://www.w3.org/2002/07/owl#Restriction"/>
  </rdf:Description>
  <rdf:Description rdf:about="http://emmo.info/emmo#EMMO_705f27ae_954c_4f13_98aa_18473fc52b25">
    <rdfs:subPropertyOf rdf:resource="http://www.w3.org/2000/01/rdf-schema#comment"/>
    <rdf:type rdf:resource="http://www.w3.org/2002/07/owl#AnnotationProperty"/>
    <skos:prefLabel xml:lang="en">etymology</skos:prefLabel>
  </rdf:Description>
  <rdf:Description rdf:nodeID="f05bdaa1e617a4bccafc519daf7bf4785b194">
    <rdf:type rdf:resource="http://www.w3.org/2002/07/owl#Restriction"/>
    <owl:onProperty rdf:resource="http://emmo.info/emmo#EMMO_23b579e1_8088_45b5_9975_064014026c42"/>
    <owl:hasValue>H</owl:hasValue>
  </rdf:Description>
  <rdf:Description rdf:about="http://emmo.info/emmo#EMMO_53bd0c90_41c3_46e2_8779_cd2a80f7e18b">
    <rdfs:subClassOf rdf:resource="http://emmo.info/emmo#EMMO_9895a1b4_f0a5_4167_ac5e_97db40b8bfcc"/>
    <owl:equivalentClass rdf:nodeID="fe0b20157736f4a31909181349b2e6219b19"/>
    <skos:prefLabel xml:lang="en">PressureDimension</skos:prefLabel>
    <rdf:type rdf:resource="http://www.w3.org/2002/07/owl#Class"/>
  </rdf:Description>
  <rdf:Description rdf:nodeID="f05bdaa1e617a4bccafc519daf7bf4785b14">
    <owl:inverseOf rdf:resource="http://emmo.info/emmo#EMMO_3446e167_c576_49d6_846c_215bb8878a55"/>
  </rdf:Description>
  <rdf:Description rdf:nodeID="fea11ca01461e402d8f697c19c5d8de88b5">
    <rdf:first rdf:resource="http://emmo.info/emmo#EMMO_70dac51e_bddd_48c2_8a98_7d8395e91fc2"/>
    <rdf:type rdf:resource="http://www.w3.org/1999/02/22-rdf-syntax-ns#List"/>
    <rdf:rest rdf:nodeID="fea11ca01461e402d8f697c19c5d8de88b6"/>
  </rdf:Description>
  <rdf:Description rdf:nodeID="ffbe75b10062f400ea693809785c50a44b3">
    <rdf:type rdf:resource="http://www.w3.org/2002/07/owl#Restriction"/>
    <owl:someValuesFrom rdf:resource="http://emmo.info/emmo#EMMO_a4d66059_5dd3_4b90_b4cb_10960559441b"/>
    <owl:onProperty rdf:nodeID="ffbe75b10062f400ea693809785c50a44b4"/>
  </rdf:Description>
  <rdf:Description rdf:nodeID="fea11ca01461e402d8f697c19c5d8de88b1">
    <owl:unionOf rdf:nodeID="fea11ca01461e402d8f697c19c5d8de88b2"/>
    <rdf:type rdf:resource="http://www.w3.org/2002/07/owl#Class"/>
  </rdf:Description>
  <rdf:Description rdf:nodeID="ffcb99037244f48d590430c228d02afdbb29">
    <rdf:type rdf:resource="http://www.w3.org/1999/02/22-rdf-syntax-ns#List"/>
    <rdf:first rdf:resource="http://emmo.info/emmo#EMMO_e29f84db_4c1c_46ae_aa38_c4d47536b972"/>
    <rdf:rest rdf:nodeID="ffcb99037244f48d590430c228d02afdbb30"/>
  </rdf:Description>
  <rdf:Description rdf:nodeID="f05bdaa1e617a4bccafc519daf7bf4785b34">
    <rdf:rest rdf:resource="http://www.w3.org/1999/02/22-rdf-syntax-ns#nil"/>
    <rdf:type rdf:resource="http://www.w3.org/1999/02/22-rdf-syntax-ns#List"/>
    <rdf:first rdf:resource="http://emmo.info/emmo#EMMO_e9ffc696_5228_4ff9_8a60_0f5e05e9931b"/>
  </rdf:Description>
  <rdf:Description rdf:nodeID="ff14b31ebf90e4bc5ba2839064d29e543b29">
    <owl:minQualifiedCardinality rdf:datatype="http://www.w3.org/2001/XMLSchema#nonNegativeInteger">1</owl:minQualifiedCardinality>
  </rdf:Description>
  <rdf:Description rdf:about="http://www.w3.org/2004/02/skos/core#prefLabel">
    <rdfs:range rdf:resource="http://www.w3.org/1999/02/22-rdf-syntax-ns#PlainLiteral"/>
    <rdfs:subPropertyOf rdf:resource="http://www.w3.org/2000/01/rdf-schema#label"/>
    <rdf:type rdf:resource="http://www.w3.org/2002/07/owl#AnnotationProperty"/>
  </rdf:Description>
  <rdf:Description rdf:nodeID="ff14b31ebf90e4bc5ba2839064d29e543b26">
    <owl:minQualifiedCardinality rdf:datatype="http://www.w3.org/2001/XMLSchema#nonNegativeInteger">2</owl:minQualifiedCardinality>
  </rdf:Description>
  <rdf:Description rdf:nodeID="f05bdaa1e617a4bccafc519daf7bf4785b106">
    <owl:inverseOf rdf:resource="http://emmo.info/emmo#EMMO_3446e167_c576_49d6_846c_215bb8878a55"/>
  </rdf:Description>
  <rdf:Description rdf:nodeID="fa691b5894b3543efa24f9838ff46c3eab8">
    <rdf:first rdf:resource="http://emmo.info/emmo#EMMO_d7788d1a_020d_4c78_85a1_13563fcec168"/>
    <rdf:type rdf:resource="http://www.w3.org/1999/02/22-rdf-syntax-ns#List"/>
    <rdf:rest rdf:resource="http://www.w3.org/1999/02/22-rdf-syntax-ns#nil"/>
  </rdf:Description>
  <rdf:Description rdf:nodeID="fe0b20157736f4a31909181349b2e6219b4">
    <rdf:rest rdf:nodeID="fe0b20157736f4a31909181349b2e6219b5"/>
    <rdf:first rdf:resource="http://emmo.info/emmo#EMMO_8159c26a_494b_4fa0_9959_10888f152298"/>
    <rdf:type rdf:resource="http://www.w3.org/1999/02/22-rdf-syntax-ns#List"/>
  </rdf:Description>
  <rdf:Description rdf:nodeID="fc2fcd8f8eb3649bcbbaff76ba54058acb6">
    <rdf:type rdf:resource="http://www.w3.org/1999/02/22-rdf-syntax-ns#List"/>
    <rdf:first rdf:resource="http://emmo.info/emmo#EMMO_29072ec4_ffcb_42fb_bdc7_26f05a2e9873"/>
    <rdf:rest rdf:nodeID="fc2fcd8f8eb3649bcbbaff76ba54058acb7"/>
  </rdf:Description>
  <rdf:Description rdf:nodeID="f05bdaa1e617a4bccafc519daf7bf4785b49">
    <owl:inverseOf rdf:resource="http://emmo.info/emmo#EMMO_3446e167_c576_49d6_846c_215bb8878a55"/>
  </rdf:Description>
  <rdf:Description rdf:nodeID="f05bdaa1e617a4bccafc519daf7bf4785b83">
    <owl:inverseOf rdf:resource="http://emmo.info/emmo#EMMO_3446e167_c576_49d6_846c_215bb8878a55"/>
  </rdf:Description>
  <rdf:Description rdf:about="http://emmo.info/emmo#EMMO_4588526f_8553_4f4d_aa73_a483e88d599b">
    <EMMO_967080e5_2f42_4eb2_a3a9_c58143e835f9 xml:lang="en">A standalone atom that has no net charge.</EMMO_967080e5_2f42_4eb2_a3a9_c58143e835f9>
    <skos:prefLabel xml:lang="en">NeutralAtom</skos:prefLabel>
    <rdf:type rdf:resource="http://www.w3.org/2002/07/owl#Class"/>
  </rdf:Description>
  <rdf:Description rdf:nodeID="ff14b31ebf90e4bc5ba2839064d29e543b31">
    <owl:qualifiedCardinality rdf:datatype="http://www.w3.org/2001/XMLSchema#nonNegativeInteger">1</owl:qualifiedCardinality>
  </rdf:Description>
  <rdf:Description rdf:nodeID="fa691b5894b3543efa24f9838ff46c3eab14">
    <owl:inverseOf rdf:resource="http://emmo.info/emmo#EMMO_c5aae418_1622_4d02_93c5_21159e28e6c1"/>
  </rdf:Description>
  <rdf:Description rdf:nodeID="f05bdaa1e617a4bccafc519daf7bf4785b18">
    <owl:inverseOf rdf:resource="http://emmo.info/emmo#EMMO_3446e167_c576_49d6_846c_215bb8878a55"/>
  </rdf:Description>
  <rdf:Description rdf:about="http://purl.org/dc/terms/title">
    <rdf:type rdf:resource="http://www.w3.org/2002/07/owl#AnnotationProperty"/>
  </rdf:Description>
</rdf:RDF>
