@prefix : <https://w3id.org/emmo/hume/disciplines/chemistry#> .
@prefix dcterms: <http://purl.org/dc/terms/> .
@prefix ns1: <https://w3id.org/emmo#> .
@prefix ns2: <http://www.lesfleursdunormal.fr/static/_downloads/owlready_ontology.owl#> .
@prefix owl: <http://www.w3.org/2002/07/owl#> .
@prefix rdf: <http://www.w3.org/1999/02/22-rdf-syntax-ns#> .
@prefix rdfs: <http://www.w3.org/2000/01/rdf-schema#> .
@prefix skos: <http://www.w3.org/2004/02/skos/core#> .
@prefix xsd: <http://www.w3.org/2001/XMLSchema#> .

ns1:AmountConcentration rdfs:subClassOf ns1:ChemicalCompositionQuantity .

ns1:AmountFraction rdfs:subClassOf ns1:ChemicalCompositionQuantity .

ns1:CASRN a owl:Class ;
    rdfs:label "CASRN"@en ;
    rdfs:comment "Chemical Abstact Service registry number for a chemical substance from the American Chemical Society"^^xsd:string ;
    rdfs:subClassOf ns1:ChemicalNomenclature ;
    skos:example "Water is 7732-18-5"^^xsd:string ;
    skos:prefLabel "CASRN"@en ;
    ns1:elucidation "Chemical Abstact Service registry number for a chemical substance from the American Chemical Society"^^xsd:string .

ns1:ChemicalEntity a owl:Class ;
    rdfs:label "ChemicalEntity"@en ;
    rdfs:comment """A chemical entity comprises the two different ways to represents matter: as single recognizable particle entity (molecular entity) and as a composition of particle entities (substance).

This distinction is not well assessed in actual chemical nomenclature, in which an element name refers to both the pure elemental substance or the atom.

In the EMMO we force the adoption of a more strict categorization based on mereotopology.

The class Material hosts the subclasses for which a substance can be identified without necessarily considering its nature of molecule/atom or substance (e.g. hydrocarbon is the class of both hydrocarbon molecules or gases)."""^^xsd:string ;
    rdfs:subClassOf ns1:Matter ;
    owl:disjointUnionOf ( ns1:MolecularEntity ns1:ChemicalSubstance ) ;
    skos:prefLabel "ChemicalEntity"@en .

ns1:CondensedFormula a owl:Class ;
    rdfs:label "CondensedFormula"@en ;
    rdfs:subClassOf ns1:ChemicalFormula ;
    skos:example "An expression that provides information about the element types that constiture a molecule or a molecular substance and their number, together with simple information about the connectivity of its groups by using parenthesis or by goruping element names according to its molecular structure."^^xsd:string ;
    skos:prefLabel "CondensedFormula"@en .

ns1:ElementalSubstance a owl:Class ;
    rdfs:label "ElementalSubstance"@en ;
    rdfs:comment "A chemical substance composed of atoms with the same number of protons in the atomic nucleus."^^xsd:string ;
    rdfs:subClassOf ns1:ChemicalSubstance ;
    skos:altLabel "PureSubstance"@en ;
    skos:prefLabel "ElementalSubstance"@en ;
    ns1:elucidation "A chemical substance composed of atoms with the same number of protons in the atomic nucleus."^^xsd:string ;
    ns1:iupacReference "https://doi.org/10.1351/goldbook.C01022"^^xsd:string .

ns1:EmpiricalFormula a owl:Class ;
    rdfs:label "EmpiricalFormula"@en ;
    rdfs:comment "An expression that provide information about the element type of a compound and their relative ratio."^^xsd:string ;
    rdfs:subClassOf ns1:ChemicalFormula ;
    skos:example "Hydrogen peroxide is HO"^^xsd:string ;
    skos:prefLabel "EmpiricalFormula"@en ;
    ns1:elucidation "An expression that provide information about the element type of a compound and their relative ratio."^^xsd:string .

ns1:Graphical rdfs:label "Graphical"@en ;
    rdfs:comment "A 'Perceptual' which stands for a real world object whose spatial configuration results from an explicit graphical procedure and shows an identifiable pattern."@en .

ns1:IUPACName a owl:Class ;
    rdfs:label "IUPACName"@en ;
    rdfs:comment "Name of a chemical according to the IUPAC standard."@en ;
    rdfs:subClassOf ns1:ChemicalName,
        ns1:IUPACNomenclature ;
    skos:prefLabel "IUPACName"@en ;
    ns1:elucidation "Name of a chemical according to the IUPAC standard."@en .

ns1:InChI a owl:Class ;
    rdfs:label "InChI"@en ;
    rdfs:comment "The International Chemical Identifier (InChI) textual identifier proposed by IUPAC to provide a standard encoding for databases of molecular information."^^xsd:string ;
    rdfs:subClassOf ns1:IUPACNomenclature ;
    skos:prefLabel "InChI"@en ;
    ns1:elucidation "The International Chemical Identifier (InChI) textual identifier proposed by IUPAC to provide a standard encoding for databases of molecular information."^^xsd:string .

ns1:InorganicCompound a owl:Class ;
    rdfs:label "InorganicCompound"@en ;
    rdfs:comment "A chemical compound that is not organic."@en ;
    rdfs:subClassOf ns1:ChemicalCompound ;
    owl:disjointWith ns1:OrganicCompound ;
    skos:prefLabel "InorganicCompound"@en ;
    ns1:elucidation "A chemical compound that is not organic."@en .

ns1:Macromolecule a owl:Class ;
    rdfs:label "Macromolecule"@en ;
    rdfs:comment "A polyatomic entity containing a very large number of atoms."@en ;
    rdfs:subClassOf ns1:PolyatomicEntity ;
    skos:example "Protein, nucleic acid, or synthetic polymer."@en ;
    skos:prefLabel "Macromolecule"@en ;
    ns1:elucidation "A polyatomic entity containing a very large number of atoms."@en .

ns1:MassConcentration rdfs:subClassOf ns1:ChemicalCompositionQuantity .

ns1:MassFraction rdfs:subClassOf ns1:ChemicalCompositionQuantity .

ns1:MolecularFormula a owl:Class ;
    rdfs:label "MolecularFormula"@en ;
    rdfs:comment "An expression that provides information about the element types that constiture a molecule or a molecular substance and their number."^^xsd:string ;
    rdfs:subClassOf [ a owl:Restriction ;
            owl:onProperty ns1:hasSpatialTile ;
            owl:someValuesFrom ns1:ChemicalElement ],
        ns1:ChemicalFormula ;
    skos:example "Hydrogen peroxide is H2O2"^^xsd:string ;
    skos:prefLabel "MolecularFormula"@en ;
    ns1:elucidation "An expression that provides information about the element types that constiture a molecule or a molecular substance and their number."^^xsd:string .

ns1:Perceptual rdfs:label "Perceptual"@en ;
    rdfs:comment "The class contrast individuals standing for entities that can stimulate a perception (e.g. a retina impression) to a human being and that are categorized accordingly to human perception mechanisms."@en .

ns1:SMILESReference a owl:AnnotationProperty ;
    rdfs:label "SMILESReference"@en ;
    ns2:python_name "SMILESReference"@en ;
    rdfs:comment "OpenSMILES representation of a molecular structure."@en ;
    rdfs:isDefinedBy <http://opensmiles.org/opensmiles.html> ;
    rdfs:subPropertyOf rdfs:seeAlso ;
    skos:prefLabel "SMILESReference"@en ;
    ns1:elucidation "OpenSMILES representation of a molecular structure."@en ;
    ns1:note "OpenSMILES is an open specification of the SMILE language for specifying molecular structures, which has become a defacto standard for exchange of molecular structures."@en ;
    ns1:wikipediaReference <https://en.wikipedia.org/wiki/Simplified_molecular-input_line-entry_system> .

ns1:StructuralFormula a owl:Class ;
    rdfs:label "StructuralFormula"@en ;
    rdfs:comment "A graphical representation of a molecular structure showing the relative position in space of the atomic constituents and their bonds."^^xsd:string ;
    rdfs:subClassOf ns1:ChemicalRepresentation ;
    skos:prefLabel "StructuralFormula"@en ;
    ns1:elucidation "A graphical representation of a molecular structure showing the relative position in space of the atomic constituents and their bonds."^^xsd:string .

ns1:Visual rdfs:label "Visual"@en ;
    rdfs:comment "A 'Perceptual' which stands for a real world object whose spatiotemporal pattern makes it identifiable by an observer through an optical perception employing the visible part of the electromagnetic spectrum."@en .

ns1:VolumeFraction rdfs:subClassOf ns1:ChemicalCompositionQuantity .

ns1:chemicalSymbolValue a owl:DatatypeProperty ;
    rdfs:label "chemicalSymbolValue"@en ;
    ns2:python_name "chemicalSymbolValue"@en ;
    rdfs:domain ns1:ChemicalSymbol ;
    rdfs:subPropertyOf ns1:hasSymbolValue ;
    skos:prefLabel "chemicalSymbolValue"@en .

ns1:hasChemicalComposition a owl:ObjectProperty ;
    rdfs:label "hasChemicalComposition"@en ;
    ns2:python_name "hasChemicalComposition"@en ;
    rdfs:comment "Relates a substance to chemical composition."@en ;
    rdfs:domain ns1:Substance ;
    rdfs:range ns1:ChemicalComposition ;
    rdfs:subPropertyOf ns1:hasConvention ;
    skos:example """This relation can be used to relate a material to a chemical composition quantity of one of its chemical species. For example, the amount of aluminium in substance subst:alloy1 can be expressed as:

```turtle
subst:alloy1 a emmo:Substance ;
    emmo:hasChemicalComposition [
        a emmo:SingleComponentComposition ;
        emmo:hasSpeciesPart [ a emmo:AluminiumSymbol ] ;
        emmo:hasQuantityPart [
            a emmo:MassFraction ;
            hasSIQuantityValue "98.1 wt%"^^emmo:SIQuantityDatatype
        ]
    ] .
```"""@en ;
    skos:prefLabel "hasChemicalComposition"@en ;
    ns1:elucidation "Relates a substance to chemical composition."@en ;
    ns1:note "This property is often used to relate a substance directly to SingleComponentComposition indifiduals for each of its components."@en .

ns1:hasChemicalSpecies a owl:ObjectProperty ;
    rdfs:label "hasChemicalSpecies"@en ;
    ns2:python_name "hasChemicalSpecies"@en ;
    rdfs:comment "Relates a substance to one of its chemical species."@en ;
    rdfs:domain ns1:Substance ;
    rdfs:range ns1:ChemicalSpecies ;
    rdfs:subPropertyOf ns1:hasConvention ;
    skos:prefLabel "hasChemicalSpecies"@en ;
    ns1:elucidation "Relates a substance to one of its chemical species."@en .

ns1:inchiKey a owl:AnnotationProperty ;
    rdfs:label "inchiKey"@en ;
    ns2:python_name "inchiKey"@en ;
    rdfs:comment "A hash of the full International Chemical Identifier (InChi) for a chemical substance."@en ;
    rdfs:seeAlso "https://inchi.info/inchikey_overview_en.html"^^xsd:anyURI ;
    rdfs:subPropertyOf rdfs:seeAlso ;
    skos:prefLabel "inchiKey"@en ;
    ns1:elucidation "A hash of the full International Chemical Identifier (InChi) for a chemical substance."@en ;
    ns1:note "The InChiKey is a hash of the full InChi identifier using the SHA-256 algorithm, designed to allow for easy web searches of chemical compounds."@en .

: a owl:Ontology ;
    dcterms:abstract "The chemistry module populates the physicalistic perspective with materials subclasses categorised according to modern applied chemistry."@en ;
    dcterms:creator <https://orcid.org/EmanueleGhedini>,
        <https://orcid.org/GerhardGoldbeck>,
        <https://orcid.org/JesperFriis> ;
    dcterms:license "https://creativecommons.org/licenses/by/4.0/legalcode"^^xsd:string ;
    dcterms:publisher <https://emmc.eu> ;
    dcterms:title "Chemistry"@en ;
    rdfs:comment "The EMMO requires FacT++ reasoner plugin in order to visualize all inferences and class hierarchy (ctrl+R hotkey in Protege)."@en ;
    owl:imports <https://w3id.org/emmo/1.0.3/disciplines/isq>,
        <https://w3id.org/emmo/1.0.3/disciplines/perceptual> ;
    owl:versionIRI <https://w3id.org/emmo/1.0.3/hume/disciplines/chemistry> ;
    owl:versionInfo "1.0.3"^^xsd:string ;
    ns1:contact "emmo@emmc.eu"^^xsd:string .

ns1:ChemicalName a owl:Class ;
    rdfs:label "ChemicalName"@en ;
    rdfs:comment "Name of a chemical according to a standard."@en ;
    rdfs:subClassOf ns1:ChemicalNomenclature ;
    skos:prefLabel "ChemicalName"@en ;
    ns1:elucidation "Name of a chemical according to a standard."@en .

ns1:ChemicalRepresentation a owl:Class ;
    rdfs:label "ChemicalRepresentation"@en ;
    rdfs:comment "A representation of objects belonging to the chemistry field."^^xsd:string ;
    rdfs:subClassOf ns1:Representation ;
    skos:prefLabel "ChemicalRepresentation"@en ;
    ns1:elucidation "A representation of objects belonging to the chemistry field."^^xsd:string .

ns1:ChemicalSymbol a owl:Class ;
    rdfs:label "ChemicalSymbol"@en ;
    rdfs:comment "A symbol that stands for a chemical element."@en ;
    owl:equivalentClass [ a owl:Class ;
            owl:intersectionOf ( ns1:Symbol ns1:Chemical ) ] ;
    skos:example """"H"
"He"
"Li"
..."""@en ;
    skos:prefLabel "ChemicalSymbol"@en ;
    ns1:elucidation "A symbol that stands for a chemical element."@en .

ns1:ChemicalSymbolicConstruct a owl:Class ;
    rdfs:label "ChemicalSymbolicConstruct"@en ;
    rdfs:comment "A symbolic construct that stands for a chemical."@en ;
    owl:equivalentClass [ a owl:Class ;
            owl:intersectionOf ( ns1:SymbolicConstruct ns1:Chemical ) ] ;
    skos:example "H2O"@en ;
    skos:prefLabel "ChemicalSymbolicConstruct"@en ;
    ns1:elucidation "A symbolic construct that stands for a chemical."@en .

ns1:OrganicCompound a owl:Class ;
    rdfs:label "OrganicCompound"@en ;
    dcterms:source "https://goldbook.iupac.org"^^xsd:anyURI ;
    rdfs:comment """A chemical compound containing carbon atoms.

-- IUPAC"""@en ;
    rdfs:subClassOf ns1:ChemicalCompound ;
    skos:prefLabel "OrganicCompound"@en ;
    ns1:elucidation """A chemical compound containing carbon atoms.

-- IUPAC"""@en ;
    ns1:note "The definition of organic compound is based on the IUPAC Gold Book. However, sometimes an organic compound is defined as a chemical compound that contains a carbon–hydrogen or carbon–carbon bond. Also, some carbon-containing compounds are typically not classified as organic, like carbides, carbonates, and cyanides."@en .

ns1:PartialComposition a owl:Class ;
    rdfs:label "PartialComposition"@en ;
    rdfs:comment "A language construct that represents fraction or amount of some (but not all) constituents of a substance."@en ;
    rdfs:subClassOf [ a owl:Restriction ;
            owl:onProperty ns1:hasSpatialTile ;
            owl:someValuesFrom ns1:SingleComponentComposition ],
        ns1:ChemicalComposition ;
    skos:prefLabel "PartialComposition"@en ;
    ns1:elucidation "A language construct that represents fraction or amount of some (but not all) constituents of a substance."@en .

ns1:PolyatomicEntity a owl:Class ;
    rdfs:label "PolyatomicEntity"@en ;
    rdfs:comment "An entity made of two or more bonded atoms."@en ;
    rdfs:subClassOf ns1:MolecularEntity ;
    skos:prefLabel "PolyatomicEntity"@en ;
    ns1:elucidation "An entity made of two or more bonded atoms."@en .

ns1:Representation rdfs:label "Representation"@en ;
    rdfs:comment "A graphical object aimed to represent schematically the conceptual, temporal or spatial structure of another object, that may or may not exist."@en .

ns1:TotalComposition a owl:Class ;
    rdfs:label "TotalComposition"@en ;
    rdfs:comment "A language construct that represents fraction or amount of all constituents of a substance."@en ;
    rdfs:subClassOf [ a owl:Restriction ;
            owl:onProperty ns1:hasSpatialTile ;
            owl:someValuesFrom ns1:SingleComponentComposition ],
        ns1:ChemicalComposition ;
    skos:prefLabel "TotalComposition"@en ;
    ns1:elucidation "A language construct that represents fraction or amount of all constituents of a substance."@en .

ns1:hasQuantityPart a owl:AsymmetricProperty,
        owl:IrreflexiveProperty,
        owl:ObjectProperty ;
    rdfs:label "hasQuantityPart"@en ;
    ns2:python_name "hasQuantityPart"@en ;
    rdfs:domain ns1:SymbolicConstruct ;
    rdfs:range ns1:Quantity ;
    rdfs:subPropertyOf ns1:hasSpatialTile ;
    skos:prefLabel "hasQuantityPart"@en ;
    ns1:note "Relates a symbolic construct to one of its quantity parts."@en .

ns1:hasSpeciesPart a owl:AsymmetricProperty,
        owl:IrreflexiveProperty,
        owl:ObjectProperty ;
    rdfs:label "hasSpeciesPart"@en ;
    ns2:python_name "hasSpeciesPart"@en ;
    rdfs:comment "Relates a chemical composition to one its species."@en ;
    rdfs:domain ns1:ChemicalComposition ;
    rdfs:range ns1:ChemicalSpecies ;
    rdfs:subPropertyOf ns1:hasSpatialTile ;
    skos:prefLabel "hasSpeciesPart"@en ;
    ns1:elucidation "Relates a chemical composition to one its species."@en ;
    ns1:note "This property is typically used to relate a SingleComponentComposition to its chemical species."@en .

ns1:ChemicalCompound a owl:Class ;
    rdfs:label "ChemicalCompound"@en ;
    rdfs:comment "A chemical substance composed of many identical molecules (or molecular entities) composed of atoms from more than one element held together by chemical bonds."^^xsd:string ;
    rdfs:subClassOf ns1:ChemicalSubstance ;
    skos:prefLabel "ChemicalCompound"@en ;
    ns1:OWLRL2DLAxioms "DisjointUnionOf InorganicCompound, OrganicCompound"^^xsd:string ;
    ns1:elucidation "A chemical substance composed of many identical molecules (or molecular entities) composed of atoms from more than one element held together by chemical bonds."^^xsd:string ;
    ns1:wikipediaReference "https://en.wikipedia.org/wiki/Chemical_compound"^^xsd:string .

ns1:IUPACNomenclature a owl:Class ;
    rdfs:label "IUPACNomenclature"@en ;
    rdfs:comment "Chemical nomenclauture following the IUPAC standard."@en ;
    rdfs:subClassOf ns1:ChemicalNomenclature ;
    skos:prefLabel "IUPACNomenclature"@en ;
    ns1:elucidation "Chemical nomenclauture following the IUPAC standard."@en .

ns1:MolecularEntity rdfs:comment """Molecular entity is used as a general term for singular entities, irrespective of their nature, while chemical species stands for sets or ensembles of molecular entities.

Note that the name of a compound may refer to the respective molecular entity or to the chemical species,"""^^xsd:string ;
    skos:example "Hydrogen molecule is an adequate definition of a certain molecular entity for some purposes, whereas for others it is necessary to distinguish the electronic state and/or vibrational state and/or nuclear spin, etc. of the hydrogen molecule."^^xsd:string,
        "Methane, may mean a single molecule of CH4 (molecular entity) or a molar amount, specified or not (chemical species), participating in a reaction. The degree of precision necessary to describe a molecular entity depends on the context."^^xsd:string .

ns1:ChemicalElement a owl:Class ;
    rdfs:label "ChemicalElement"@en ;
    rdfs:comment """The IUPAC Gold Book defines the a chemical element both as:
- a species of atoms; all atoms with the same number of protons in the atomic nucleus
-  a pure chemical substance composed of atoms with the same number of protons in the atomic nucleus

This qualifies a chemical element as a name and not a matter obejct that can stand for an atom or a substance."""^^xsd:string,
        "The symbol for a specific chemical element, that can stand both for an atom or a substance."^^xsd:string ;
    rdfs:seeAlso "http://publications.iupac.org/ci/2005/2701/ud.html"^^xsd:string ;
    rdfs:subClassOf ns1:Chemical,
        ns1:Symbol ;
    skos:prefLabel "ChemicalElement"@en ;
    ns1:elucidation "The symbol for a specific chemical element, that can stand both for an atom or a substance."^^xsd:string ;
    ns1:iupacReference "https://doi.org/10.1351/goldbook.C01022"^^xsd:string .

ns1:ChemicalSpecies a owl:Class ;
    rdfs:label "ChemicalSpecies"@en ;
    rdfs:comment """Following nominalistic approach a species is simply a name that can point to an element name, a chemical formula or a chemical compound.

So everything addressed by these classes of names can be calleded a chemical species."""^^xsd:string,
        """N2
Methane
CH4
Fe
Sodium Chloride"""^^xsd:string,
        """Specific form of an element defined as to isotopic composition, electronic or oxidation state, and/or complex or molecular structure.

Chemical species is the macroscopic equivalent of molecular entity and refers to sets or ensembles of molecular entities."""^^xsd:string ;
    rdfs:subClassOf ns1:Chemical ;
    owl:equivalentClass [ a owl:Class ;
            owl:unionOf ( ns1:ChemicalElement ns1:ChemicalNomenclature ns1:ChemicalFormula ) ] ;
    skos:prefLabel "ChemicalSpecies"@en ;
    ns1:elucidation """Specific form of an element defined as to isotopic composition, electronic or oxidation state, and/or complex or molecular structure.

Chemical species is the macroscopic equivalent of molecular entity and refers to sets or ensembles of molecular entities."""^^xsd:string ;
    ns1:iupacReference "https://doi.org/10.1351/goldbook.CT06859"^^xsd:string .

ns1:ChemicalSubstance a owl:Class ;
    rdfs:label "ChemicalSubstance"@en ;
    rdfs:comment "A substance is always composed of more than one molecular entity. It lays in the continuum or mesoscopic domain."^^xsd:string,
        "Matter of constant composition best characterized by the entities (molecules, formula units, atoms) it is composed of."^^xsd:string ;
    rdfs:subClassOf ns1:Substance ;
    skos:prefLabel "ChemicalSubstance"@en ;
    ns1:elucidation "Matter of constant composition best characterized by the entities (molecules, formula units, atoms) it is composed of."^^xsd:string ;
    ns1:iupacReference "https://doi.org/10.1351/goldbook.C01039"^^xsd:string .

ns1:SingleComponentComposition a owl:Class ;
    rdfs:label "SingleComponentComposition"@en ;
    rdfs:comment "A language construct that represents the fraction or amount of a single constituent of a substance."@en ;
    rdfs:subClassOf [ a owl:Restriction ;
            owl:onProperty ns1:hasSpeciesPart ;
            owl:someValuesFrom ns1:ChemicalSpecies ],
        [ a owl:Restriction ;
            owl:onProperty ns1:hasQuantityPart ;
            owl:someValuesFrom ns1:ChemicalCompositionQuantity ],
        ns1:ChemicalComposition ;
    skos:prefLabel "SingleComponentComposition"@en ;
    ns1:elucidation "A language construct that represents the fraction or amount of a single constituent of a substance."@en .

ns1:ChemicalFormula a owl:Class ;
    rdfs:label "ChemicalFormula"@en ;
    rdfs:comment "A chemical formula may also include other symbols such as parentheses, plus and minus signs, brackets"^^xsd:string,
        "A symbolic construct that provides informations about the chemical proportions of the elements that constitute a chemical compound or a specific molecule."^^xsd:string ;
    rdfs:subClassOf [ a owl:Restriction ;
            owl:onProperty ns1:hasSpatialTile ;
            owl:someValuesFrom ns1:ChemicalElement ],
        ns1:Chemical ;
    skos:prefLabel "ChemicalFormula"@en ;
    ns1:elucidation "A symbolic construct that provides informations about the chemical proportions of the elements that constitute a chemical compound or a specific molecule."^^xsd:string .

ns1:ChemicalNomenclature a owl:Class ;
    rdfs:label "ChemicalNomenclature"@en ;
    rdfs:comment "A chemical numenclature should not be confused with the chemical formula."^^xsd:string,
        "A language object following a specific nomenclature rules for defining univocal names of chemical compounds."^^xsd:string ;
    rdfs:subClassOf ns1:Chemical ;
    skos:prefLabel "ChemicalNomenclature"@en ;
    ns1:elucidation "A language object following a specific nomenclature rules for defining univocal names of chemical compounds."^^xsd:string .

ns1:ChemicalComposition a owl:Class ;
    rdfs:label "ChemicalComposition"@en ;
    rdfs:comment "A language construct that provides information about the consitutents of a substance and their fractions or amounts."^^xsd:string ;
    rdfs:subClassOf ns1:ChemicalSymbolicConstruct ;
    owl:equivalentClass [ a owl:Class ;
            owl:unionOf ( ns1:TotalComposition ns1:SingleComponentComposition ns1:PartialComposition ) ] ;
    skos:prefLabel "ChemicalComposition"@en ;
    ns1:elucidation "A language construct that provides information about the consitutents of a substance and their fractions or amounts."^^xsd:string .

ns1:Chemical a owl:Class ;
    rdfs:label "Chemical"@en ;
    rdfs:comment "A language object that follows the syntactic rules used in the chemical field."^^xsd:string ;
    rdfs:subClassOf ns1:Language ;
    skos:prefLabel "Chemical"@en ;
    ns1:elucidation "A language object that follows the syntactic rules used in the chemical field."^^xsd:string .

