@prefix : <https://w3id.org/emmo/hume/perspectives/reductionistic#> .
@prefix dcterms: <http://purl.org/dc/terms/> .
@prefix ns1: <http://www.lesfleursdunormal.fr/static/_downloads/owlready_ontology.owl#> .
@prefix ns2: <https://w3id.org/emmo#> .
@prefix owl: <http://www.w3.org/2002/07/owl#> .
@prefix rdfs: <http://www.w3.org/2000/01/rdf-schema#> .
@prefix skos: <http://www.w3.org/2004/02/skos/core#> .
@prefix xsd: <http://www.w3.org/2001/XMLSchema#> .

ns2:Broadcast a owl:Class ;
    rdfs:label "Broadcast"@en ;
    rdfs:comment "A mixed tiling in which a tile has next spatially connected tiles."@en ;
    rdfs:subClassOf ns2:MixedTiling ;
    skos:prefLabel "Broadcast"@en ;
    ns2:elucidation "A mixed tiling in which a tile has next spatially connected tiles."@en ;
    ns2:illustration "https://raw.githubusercontent.com/emmo-repo/EMMO/1.0.2/doc/figs/Broadcast.png"^^xsd:anyURI .

ns2:Fork a owl:Class ;
    rdfs:label "Fork"@en ;
    rdfs:comment "A tessellation in which a tile has next two or more non spatially connected tiles."@en ;
    rdfs:subClassOf ns2:TemporalTiling ;
    skos:prefLabel "Fork"@en ;
    ns2:elucidation "A tessellation in which a tile has next two or more non spatially connected tiles."@en ;
    ns2:illustration "https://raw.githubusercontent.com/emmo-repo/EMMO/1.0.2/doc/figs/Fork.png"^^xsd:anyURI .

ns2:Gathering a owl:Class ;
    rdfs:label "Gathering"@en ;
    rdfs:comment "A mixed tiling in which a tile is the next of spatially connected tiles."@en ;
    rdfs:subClassOf ns2:MixedTiling ;
    skos:prefLabel "Gathering"@en ;
    ns2:elucidation "A mixed tiling in which a tile is the next of spatially connected tiles."@en ;
    ns2:illustration "https://raw.githubusercontent.com/emmo-repo/EMMO/1.0.2/doc/figs/Gathering.png"^^xsd:anyURI .

ns2:IntermidiateTile a owl:Class ;
    rdfs:label "IntermidiateTile"@en ;
    rdfs:comment "A tile that has next and is next of other tiles within the same tessellation."@en ;
    rdfs:subClassOf ns2:SpatioTemporalTileByPosition ;
    skos:prefLabel "IntermidiateTile"@en ;
    ns2:elucidation "A tile that has next and is next of other tiles within the same tessellation."@en ;
    ns2:illustration "https://w3id.org/emmo/raw/1.0.3/doc/figs/ThroughTile.png"^^xsd:anyURI .

ns2:Join a owl:Class ;
    rdfs:label "Join"@en ;
    rdfs:comment "A tessellation in which a tile is next for two or more non spatially connected tiles."@en ;
    rdfs:subClassOf ns2:TemporalTiling ;
    skos:prefLabel "Join"@en ;
    ns2:elucidation "A tessellation in which a tile is next for two or more non spatially connected tiles."@en ;
    ns2:illustration "https://raw.githubusercontent.com/emmo-repo/EMMO/1.0.2/doc/figs/Join.png"^^xsd:anyURI .

ns2:SpatialSequence a owl:Class ;
    rdfs:label "SpatialSequence"@en ;
    rdfs:comment "A monodimensional arrangement of tiles."@en ;
    rdfs:subClassOf ns2:Arrangement ;
    skos:altLabel "Sequence"@en ;
    skos:prefLabel "SpatialSequence"@en ;
    ns2:elucidation "A monodimensional arrangement of tiles."@en ;
    ns2:illustration "https://raw.githubusercontent.com/emmo-repo/EMMO/1.0.2/doc/figs/SpatialSequence.png"^^xsd:anyURI .

ns2:TemporalSequence a owl:Class ;
    rdfs:label "TemporalSequence"@en ;
    rdfs:comment "A tessellation of temporal slices."@en ;
    rdfs:subClassOf ns2:TemporalTiling ;
    skos:altLabel "Sequence"@en ;
    skos:prefLabel "TemporalSequence"@en ;
    ns2:elucidation "A tessellation of temporal slices."@en ;
    ns2:illustration "https://raw.githubusercontent.com/emmo-repo/EMMO/1.0.2/doc/figs/Sequence.png"^^xsd:anyURI .

ns2:hasBeginTile a owl:AsymmetricProperty,
        owl:IrreflexiveProperty,
        owl:ObjectProperty ;
    rdfs:label "hasBeginTile"@en ;
    ns1:python_name "hasBeginTile"@en ;
    rdfs:comment "The relation between the whole and a temporal tile that has only outgoing temporal connections."^^xsd:string ;
    rdfs:range ns2:BeginTile ;
    rdfs:subPropertyOf ns2:hasTemporalTile ;
    skos:altLabel "hasTemporalFirst"@en ;
    skos:prefLabel "hasBeginTile"@en ;
    ns2:elucidation "The relation between the whole and a temporal tile that has only outgoing temporal connections."^^xsd:string .

ns2:hasEndTile a owl:AsymmetricProperty,
        owl:IrreflexiveProperty,
        owl:ObjectProperty ;
    rdfs:label "hasEndTile"@en ;
    ns1:python_name "hasEndTile"@en ;
    rdfs:comment "The relation between the whole and a temporal tile that has only ingoing temporal connections."^^xsd:string ;
    rdfs:range ns2:EndTile ;
    rdfs:subPropertyOf ns2:hasTemporalTile ;
    skos:altLabel "hasTemporalLast"@en ;
    skos:prefLabel "hasEndTile"@en ;
    ns2:elucidation "The relation between the whole and a temporal tile that has only ingoing temporal connections."^^xsd:string .

ns2:hasSpatialTile a owl:AsymmetricProperty,
        owl:IrreflexiveProperty,
        owl:ObjectProperty ;
    rdfs:label "hasSpatialTile"@en ;
    ns1:python_name "hasSpatialTile"@en ;
    rdfs:comment "A relation between the whole and one of its tiles, where the tile is only spatially connected with the other tiles forming the tessellation."^^xsd:string ;
    rdfs:range ns2:SpatialTile ;
    rdfs:subPropertyOf ns2:hasSpatioTemporalTile ;
    skos:altLabel "hasSpatialDirectPart"@en ;
    skos:prefLabel "hasSpatialTile"@en ;
    ns2:elucidation "A relation between the whole and one of its tiles, where the tile is only spatially connected with the other tiles forming the tessellation."^^xsd:string .

: a owl:Ontology ;
    dcterms:abstract """Defines the reductionistic perspective, which uses the fundamental non-transitive parthood relation, called direct parthood, to provide a powerful granularity description of multiscale real world objects.  EMMO can in principle represents the Universe with direct parthood relations as a direct rooted tree up to its elementary constituents.

In addition to direct parthood, the reductionistic module defines 'State' as a tessellation of spatial direct parts with no change of granularity or cardinality and 'Existent' as a tessellation of temporal direct parts."""@en ;
    dcterms:contributor <https://orcid.org/AdhamHashibon>,
        <https://orcid.org/FrancescoZaccarini> ;
    dcterms:creator <https://orcid.org/EmanueleGhedini>,
        <https://orcid.org/GerhardGoldbeck>,
        <https://orcid.org/JesperFriis> ;
    dcterms:license "https://creativecommons.org/licenses/by/4.0/legalcode"^^xsd:string ;
    dcterms:publisher <https://emmc.eu> ;
    dcterms:title "Reductionistic"@en ;
    rdfs:comment "The EMMO requires HermiT reasoner plugin in order to visualize all inferences and class hierarchy (ctrl+R hotkey in Protege)."@en ;
    owl:imports <https://w3id.org/emmo/1.0.3/perspectives/perspective> ;
    owl:versionIRI <https://w3id.org/emmo/1.0.3/hume/perspectives/reductionistic> ;
    owl:versionInfo "1.0.3"^^xsd:string ;
    ns2:contact "emmo@emmc.eu"^^xsd:string .

ns2:Arrangement a owl:Class ;
    rdfs:label "Arrangement"@en ;
    rdfs:comment "A causal object which is tessellated with only spatial direct parts."@en ;
    rdfs:subClassOf ns2:SpatialTiling ;
    skos:altLabel "MereologicalState"@en ;
    skos:example """e.g. the existent in my glass is declared at t = t_start as made of two direct parts: the ice and the water. It will continue to exists as state as long as the ice is completely melt at t = t_end. The new state will be completely made of water. Between t_start and t_end there is an exchange of molecules between the ice and the water, but this does not affect the existence of the two states.

If we partition the existent in my glass as ice surrounded by several molecules (we do not use the object water as direct part) then the appearance of a molecule coming from the ice will cause a state to end and another state to begin."""@en ;
    skos:prefLabel "Arrangement"@en ;
    ns2:elucidation "A causal object which is tessellated with only spatial direct parts."@en ;
    ns2:illustration "https://raw.githubusercontent.com/emmo-repo/EMMO/1.0.2/doc/figs/Arrangement.png"^^xsd:anyURI,
        "https://w3id.org/emmo/raw/1.0.3/doc/figs/Arrangement-1D.png"^^xsd:anyURI,
        "https://w3id.org/emmo/raw/1.0.3/doc/figs/Arrangement-2D.png"^^xsd:anyURI,
        "https://w3id.org/emmo/raw/1.0.3/doc/figs/Arrangement-2Dhex.png"^^xsd:anyURI,
        "https://w3id.org/emmo/raw/1.0.3/doc/figs/Arrangement-3D.png"^^xsd:anyURI ;
    ns2:note """The definition of an arrangement implies that its spatial direct parts are not gained or lost during its temporal extension (they exist from the left to the right side of the time interval), so that the cardinality of spatial direct parts in an arrangement is constant.
This does not mean that there cannot be a change in the internal structure of the arrangement direct parts. It means only that this change must not affect the existence of the direct part itself."""@en,
        "The use of spatial direct parthood in state definition means that an arrangement cannot overlap in space another arrangement that is direct part of the same whole."@en .

ns2:BeginTile a owl:Class ;
    rdfs:label "BeginTile"@en ;
    rdfs:comment "A direct part that only is the source, but not the target of temporal relations."@en ;
    rdfs:subClassOf ns2:SpatioTemporalTileByPosition ;
    skos:prefLabel "BeginTile"@en ;
    ns2:elucidation "A direct part that only is the source, but not the target of temporal relations."@en ;
    ns2:illustration "https://w3id.org/emmo/raw/1.0.3/doc/figs/BeginTile.png"^^xsd:anyURI .

ns2:EndTile a owl:Class ;
    rdfs:label "EndTile"@en ;
    rdfs:comment "A direct part that only is the target, but not the source of temporal relations."@en ;
    rdfs:subClassOf ns2:SpatioTemporalTileByPosition ;
    skos:prefLabel "EndTile"@en ;
    ns2:elucidation "A direct part that only is the target, but not the source of temporal relations."@en ;
    ns2:illustration "https://w3id.org/emmo/raw/1.0.3/doc/figs/EndTile.png"^^xsd:anyURI .

ns2:SpatialTiling a owl:Class ;
    rdfs:label "SpatialTiling"@en ;
    rdfs:comment "A well formed tessellation with tiles that all spatial."@en ;
    rdfs:subClassOf [ a owl:Restriction ;
            owl:allValuesFrom ns2:SpatialTile ;
            owl:onProperty ns2:hasSpatioTemporalTile ],
        ns2:SpatioTemporalTessellation ;
    skos:prefLabel "SpatialTiling"@en ;
    ns2:elucidation "A well formed tessellation with tiles that all spatial."@en ;
    ns2:illustration "https://w3id.org/emmo/raw/1.0.3/doc/figs/Arrangement-1D.png"^^xsd:anyURI,
        "https://w3id.org/emmo/raw/1.0.3/doc/figs/Arrangement-2D.png"^^xsd:anyURI,
        "https://w3id.org/emmo/raw/1.0.3/doc/figs/Arrangement-2Dhex.png"^^xsd:anyURI,
        "https://w3id.org/emmo/raw/1.0.3/doc/figs/Arrangement-3D.png"^^xsd:anyURI .

ns2:hasJunctionTile a owl:AsymmetricProperty,
        owl:IrreflexiveProperty,
        owl:ObjectProperty ;
    rdfs:label "hasJunctionTile"@en ;
    ns1:python_name "hasJunctionTile"@en ;
    rdfs:comment "A relation between the whole and one of its tiles, where the tile is both spatially and temporally connected with the other tiles forming the tessellation."^^xsd:string ;
    rdfs:range ns2:JunctionTile ;
    rdfs:subPropertyOf ns2:hasSpatioTemporalTile ;
    skos:prefLabel "hasJunctionTile"@en ;
    ns2:elucidation "A relation between the whole and one of its tiles, where the tile is both spatially and temporally connected with the other tiles forming the tessellation."^^xsd:string .

ns2:JunctionTile a owl:Class ;
    rdfs:label "JunctionTile"@en ;
    rdfs:comment "A direct part that is obtained by partitioning a whole hybridly in spatial, temporal and spatiotemporal parts."@en ;
    rdfs:subClassOf [ a owl:Restriction ;
            owl:onProperty [ owl:inverseOf ns2:hasJunctionTile ] ;
            owl:someValuesFrom ns2:MixedTiling ],
        ns2:SpatioTemporalTileByConnection ;
    skos:prefLabel "JunctionTile"@en ;
    ns2:elucidation "A direct part that is obtained by partitioning a whole hybridly in spatial, temporal and spatiotemporal parts."@en ;
    ns2:illustration "https://w3id.org/emmo/raw/1.0.3/doc/figs/JunctionTile.png"^^xsd:anyURI .

ns2:Reductionistic a owl:Class ;
    rdfs:label "Reductionistic"@en ;
    rdfs:comment "A class devoted to categorize causal objects by specifying their granularity levels."@en ;
    rdfs:subClassOf ns2:Perspective ;
    skos:prefLabel "Reductionistic"@en ;
    ns2:elucidation "A class devoted to categorize causal objects by specifying their granularity levels."@en ;
    ns2:note """A granularity level is specified by a tiling decomposition of the whole y. A tiling is identified as a set of items {x1, x2, ... xn} called tiles that:
    - are proper parts of y
    - covers the entire whole (y = x1 +x2 + ... + xn)
    - do not overlap
    - are part of one, and one only, whole (inverse functional)"""@en,
        "Direct parthood is the antitransitive parthood relation used to build the class hierarchy (and the granularity hierarchy) for this perspective."@en .

ns2:SpatialTile a owl:Class ;
    rdfs:label "SpatialTile"@en ;
    rdfs:comment "A direct part that is obtained by partitioning a whole purely in spatial parts."@en ;
    rdfs:subClassOf ns2:SpatioTemporalTileByConnection ;
    skos:prefLabel "SpatialTile"@en ;
    ns2:elucidation "A direct part that is obtained by partitioning a whole purely in spatial parts."@en ;
    ns2:illustration "https://w3id.org/emmo/raw/1.0.3/doc/figs/SpatialTile.png"^^xsd:anyURI .

ns2:TemporalTile a owl:Class ;
    rdfs:label "TemporalTile"@en ;
    rdfs:comment "A direct part that is obtained by partitioning a whole purely in temporal parts."@en ;
    rdfs:subClassOf ns2:SpatioTemporalTileByConnection ;
    skos:prefLabel "TemporalTile"@en ;
    ns2:elucidation "A direct part that is obtained by partitioning a whole purely in temporal parts."@en ;
    ns2:illustration "https://w3id.org/emmo/raw/1.0.3/doc/figs/TemporalTile.png"^^xsd:anyURI .

ns2:Tile a owl:Class ;
    rdfs:label "Tile"@en ;
    rdfs:comment "A causal object that is direct part of a tessellation."@en ;
    rdfs:subClassOf [ a owl:Restriction ;
            owl:onProperty [ owl:inverseOf ns2:hasTile ] ;
            owl:someValuesFrom ns2:Tessellation ],
        ns2:Reductionistic ;
    skos:prefLabel "Tile"@en ;
    ns2:elucidation "A causal object that is direct part of a tessellation."@en .

ns2:hasTemporalTile a owl:AsymmetricProperty,
        owl:IrreflexiveProperty,
        owl:ObjectProperty ;
    rdfs:label "hasTemporalTile"@en ;
    ns1:python_name "hasTemporalTile"@en ;
    rdfs:comment "A relation that establishes for the whole a univocal tessellation in temporal parts forming the tessellation."^^xsd:string ;
    rdfs:range ns2:TemporalTile ;
    rdfs:subPropertyOf ns2:hasSpatioTemporalTile ;
    skos:altLabel "hasTemporalDirectPart"@en ;
    skos:prefLabel "hasTemporalTile"@en ;
    ns2:elucidation "A relation that establishes for the whole a univocal tessellation in temporal parts forming the tessellation."^^xsd:string .

ns2:MixedTiling a owl:Class ;
    rdfs:label "MixedTiling"@en ;
    rdfs:comment "A well formed tessellation with at least a junction tile."@en ;
    rdfs:subClassOf [ a owl:Restriction ;
            owl:onProperty ns2:hasTile ;
            owl:someValuesFrom ns2:JunctionTile ],
        ns2:SpatioTemporalTessellation ;
    skos:prefLabel "MixedTiling"@en ;
    ns2:elucidation "A well formed tessellation with at least a junction tile."@en ;
    ns2:illustration "https://raw.githubusercontent.com/emmo-repo/EMMO/1.0.2/doc/figs/MixedTiling.png"^^xsd:anyURI .

ns2:SpatioTemporalTile a owl:Class ;
    rdfs:label "SpatioTemporalTile"^^xsd:string ;
    rdfs:comment "The superclass for all tiles belonging to tessellations in which all tiles are connected through spatiotemporal relations hasNext or contacts."@en ;
    rdfs:seeAlso ns2:EMMO_22c91e99_61f8_4433_8853_432d44a2a46a ;
    rdfs:subClassOf ns2:Tile ;
    skos:altLabel "WellFormedTile"@en ;
    skos:prefLabel "SpatioTemporalTile"^^xsd:string ;
    ns2:OWLRL2DLAxioms "EquivalentTo: SpatialTile or TemporalTile or JunctionTile"^^xsd:string,
        "EquivalentTo: ThroughTile or EndTile or BeginTile"^^xsd:string ;
    ns2:elucidation "The superclass for all tiles belonging to tessellations in which all tiles are connected through spatiotemporal relations hasNext or contacts."@en .

ns2:SpatioTemporalTileByConnection a owl:Class ;
    rdfs:label "SpatioTemporalTileByConnection"@en ;
    rdfs:comment "The superclass for tiles categorized accordingly to their topological role within a tessellation."@en ;
    rdfs:subClassOf ns2:SpatioTemporalTile ;
    skos:prefLabel "SpatioTemporalTileByConnection"@en ;
    ns2:elucidation "The superclass for tiles categorized accordingly to their topological role within a tessellation."@en .

ns2:SpatioTemporalTileByPosition a owl:Class ;
    rdfs:label "SpatioTemporalTileByPosition"@en ;
    rdfs:comment "The superclass for tiles categorized accordingly to their location within a tessellation in terms of causal source, sink or intermediary."@en ;
    rdfs:subClassOf ns2:SpatioTemporalTile ;
    skos:prefLabel "SpatioTemporalTileByPosition"@en ;
    ns2:elucidation "The superclass for tiles categorized accordingly to their location within a tessellation in terms of causal source, sink or intermediary."@en .

ns2:TemporalTiling a owl:Class ;
    rdfs:label "TemporalTiling"@en ;
    rdfs:comment "A well formed tessellation with tiles that are all temporal."@en ;
    rdfs:subClassOf [ a owl:Restriction ;
            owl:allValuesFrom ns2:TemporalTile ;
            owl:onProperty ns2:hasSpatioTemporalTile ],
        ns2:SpatioTemporalTessellation ;
    skos:prefLabel "TemporalTiling"@en ;
    ns2:elucidation "A well formed tessellation with tiles that are all temporal."@en ;
    ns2:illustration "https://w3id.org/emmo/raw/1.0.3/doc/figs/TemporalTile.png"^^xsd:anyURI .

ns2:SpatioTemporalTessellation a owl:Class ;
    rdfs:label "SpatioTemporalTessellation"^^xsd:string ;
    rdfs:comment "The superclass for all tessellations in which all tiles are connected through spatiotemporal relations hasNext or contacts."@en ;
    rdfs:subClassOf [ a owl:Restriction ;
            owl:onProperty ns2:hasSpatioTemporalTile ;
            owl:someValuesFrom ns2:Item ],
        ns2:Tessellation ;
    skos:altLabel "WellFormedTessellation"@en ;
    skos:prefLabel "SpatioTemporalTessellation"^^xsd:string ;
    ns2:OWLRL2DLAxioms "EquivalentTo: MixedTiling or SpatialTiling or TemporalTiling"^^xsd:string ;
    ns2:elucidation "The superclass for all tessellations in which all tiles are connected through spatiotemporal relations hasNext or contacts."@en .

ns2:Tessellation a owl:Class ;
    rdfs:label "Tessellation"@en ;
    rdfs:comment "A causal structure that is tessellated in direct parts."@en,
        "A tessellation (or tiling) is the covering of a surface, often a plane, using one or more geometric shapes, called tiles, with no overlaps and no gaps."@en ;
    rdfs:subClassOf [ a owl:Restriction ;
            owl:onProperty ns2:hasTile ;
            owl:someValuesFrom ns2:Item ],
        ns2:Reductionistic ;
    skos:altLabel "Tiling"@en ;
    skos:prefLabel "Tessellation"@en ;
    ns2:conceptualisation "A tessellation (or tiling) is the covering of a surface, often a plane, using one or more geometric shapes, called tiles, with no overlaps and no gaps."@en ;
    ns2:elucidation "A causal structure that is tessellated in direct parts."@en .

ns2:hasTile a owl:AsymmetricProperty,
        owl:IrreflexiveProperty,
        owl:ObjectProperty ;
    rdfs:label "hasTile"@en ;
    ns1:python_name "hasTile"@en ;
    rdfs:comment "The relation grouping all direct parthood relations used in the reductionistic perspective."@en,
        """Tiling parthood enables the establishment of hierarchy of granularities, starting with an entity and providing several tessellation levels according to specific criteria.
The criteria are implemented in specialised versions of the tiling parthood relation (e.g., metrological direct part, XML format direct part).
The tiles and the tessellated entity (tessellation) are causally self connected (i.e., items), coherently with the concept behind the definition of the reductionistic perspective.
The tiles of specific granularity level provide a covering for the whole and are mutually non-overlapping, as the label "tile" suggests."""@en ;
    rdfs:domain ns2:Tessellation ;
    rdfs:range ns2:Tile ;
    rdfs:subPropertyOf ns2:hasDirectPart ;
    skos:altLabel "hasDirectPart"@en ;
    skos:prefLabel "hasTile"@en ;
    ns2:conceptualisation """Tiling parthood enables the establishment of hierarchy of granularities, starting with an entity and providing several tessellation levels according to specific criteria.
The criteria are implemented in specialised versions of the tiling parthood relation (e.g., metrological direct part, XML format direct part).
The tiles and the tessellated entity (tessellation) are causally self connected (i.e., items), coherently with the concept behind the definition of the reductionistic perspective.
The tiles of specific granularity level provide a covering for the whole and are mutually non-overlapping, as the label "tile" suggests."""@en ;
    ns2:elucidation "The relation grouping all direct parthood relations used in the reductionistic perspective."@en ;
    ns2:note "This relation is a simple collector of all relations inverse functional direct parthoods that can be defined in specialised theories using reductionism."^^xsd:string,
        "This relation is not antitransitive, to enable partitioning of a causal structure with more than one tiling scheme (e.g. time and space partitioning)."@en .

ns2:hasSpatioTemporalTile a owl:AsymmetricProperty,
        owl:IrreflexiveProperty,
        owl:ObjectProperty ;
    rdfs:label "hasSpatioTemporalTile"^^xsd:string ;
    ns1:python_name "hasSpatioTemporalTile"^^xsd:string ;
    rdfs:comment "A tile that is connected with other tiles with bi-directional causal relations that fall under hasNext (or its inverse) or hasContact."@en ;
    rdfs:domain ns2:SpatioTemporalTessellation ;
    rdfs:range ns2:SpatioTemporalTile ;
    rdfs:subPropertyOf ns2:hasTile ;
    skos:altLabel "hasWellFormedTile"@en ;
    skos:prefLabel "hasSpatioTemporalTile"^^xsd:string ;
    ns2:elucidation "A tile that is connected with other tiles with bi-directional causal relations that fall under hasNext (or its inverse) or hasContact."@en ;
    ns2:note "This owl:ObjectProperty is, like its super property, a mere collector of direct parthoods that manifest a spatiotemporal meaningful shape."^^xsd:string .

[] a owl:Axiom ;
    owl:annotatedProperty ns2:conceptualisation ;
    owl:annotatedSource ns2:Tessellation ;
    owl:annotatedTarget "A tessellation (or tiling) is the covering of a surface, often a plane, using one or more geometric shapes, called tiles, with no overlaps and no gaps."@en ;
    ns2:wikipediaReference "https://en.wikipedia.org/wiki/Tessellation"^^xsd:anyURI .

