@prefix dcterms: <http://purl.org/dc/terms/> .
@prefix emmo: <https://w3id.org/emmo#> .
@prefix owl: <http://www.w3.org/2002/07/owl#> .
@prefix rdf: <http://www.w3.org/1999/02/22-rdf-syntax-ns#> .
@prefix rdfs: <http://www.w3.org/2000/01/rdf-schema#> .
@prefix skos: <http://www.w3.org/2004/02/skos/core#> .
@prefix xsd: <http://www.w3.org/2001/XMLSchema#> .

emmo:EMMO_04b3300c_98bd_42dc_a3b5_e6c29d69f1ac rdfs:subClassOf emmo:EMMO_a293f923_954c_4af5_9f97_9600ebd362cb .

emmo:EMMO_057e7d57_aff0_49de_911a_8861d85cef40 rdfs:label "Symbolic"@en ;
    rdfs:comment "A discrete data whose elements can be decoded as tokens from one or more alphabets, without necessarily respecting syntactic rules."@en .

emmo:EMMO_09f0ac34_c349_46b5_acf0_0edeae52cca1 rdfs:label "InteractingSystem"@en ;
    rdfs:comment "A causally bonded system is a system in which there are at least two causal paths that are interacting."@en .

emmo:EMMO_0f3e0646_4f06_4588_9779_6a4f05c5a8d6 rdfs:label "PhysicalObjectByBond"@en ;
    rdfs:comment "Categorisation of physical objects by how they are bonded."@en .

emmo:EMMO_1141d225_fe90_4230_82c6_31cab6a4e3fe rdfs:label "SymbolicByStructure"@en ;
    rdfs:comment "Symbolic caterorised by its internal structure."@en .

emmo:EMMO_16a3bd5c_75f0_42b3_b000_cb0d018f840e a owl:Class ;
    rdfs:label "IUPACName"@en ;
    rdfs:comment "Name of a chemical according to the IUPAC standard."@en ;
    rdfs:subClassOf emmo:EMMO_26586828_3b8c_4d8b_9c6c_0bc2502f26ae,
        emmo:EMMO_91a0635a_a89a_46de_8928_04a777d145c7 ;
    skos:prefLabel "IUPACName"@en ;
    emmo:EMMO_967080e5_2f42_4eb2_a3a9_c58143e835f9 "Name of a chemical according to the IUPAC standard."@en .

emmo:EMMO_16f2fe60_2db7_43ca_8fee_5b3e416bfe87 rdfs:subClassOf emmo:EMMO_a293f923_954c_4af5_9f97_9600ebd362cb .

emmo:EMMO_2856bbc2_96e1_485b_b5f8_2fdfcb0c9b92 a owl:AnnotationProperty ;
    rdfs:label "inchiKey"@en ;
    rdfs:comment "A hash of the full International Chemical Identifier (InChi) for a chemical substance."@en ;
    rdfs:seeAlso "https://inchi.info/inchikey_overview_en.html"^^xsd:anyURI ;
    rdfs:subPropertyOf rdfs:seeAlso ;
    skos:prefLabel "inchiKey"@en ;
    emmo:EMMO_967080e5_2f42_4eb2_a3a9_c58143e835f9 "A hash of the full International Chemical Identifier (InChi) for a chemical substance."@en ;
    emmo:EMMO_c7b62dd7_063a_4c2a_8504_42f7264ba83f "The InChiKey is a hash of the full InChi identifier using the SHA-256 algorithm, designed to allow for easy web searches of chemical compounds."@en .

emmo:EMMO_2e0b0f1b_ba90_4827_af5a_92b826cb90de a owl:AnnotationProperty ;
    rdfs:label "SMILESReference"@en ;
    rdfs:comment "OpenSMILES representation of a molecular structure."@en ;
    rdfs:isDefinedBy <http://opensmiles.org/opensmiles.html> ;
    rdfs:subPropertyOf rdfs:seeAlso ;
    skos:prefLabel "SMILESReference"@en ;
    emmo:EMMO_967080e5_2f42_4eb2_a3a9_c58143e835f9 "OpenSMILES representation of a molecular structure."@en ;
    emmo:EMMO_c7b62dd7_063a_4c2a_8504_42f7264ba83f "OpenSMILES is an open specification of the SMILE language for specifying molecular structures, which has become a defacto standard for exchange of molecular structures."@en ;
    emmo:EMMO_c84c6752_6d64_48cc_9500_e54a3c34898d <https://en.wikipedia.org/wiki/Simplified_molecular-input_line-entry_system> .

emmo:EMMO_32f55395_8b94_40de_a103_bffa5c121d98 rdfs:label "ParticulateMatter"@en ;
    rdfs:comment "Bounded matter."@en .

emmo:EMMO_38b579de_4331_40e0_803d_09efa298e726 rdfs:label "PhysicalObject"@en ;
    rdfs:comment """It is natural to define entities made or more than one smaller parts as object according to some unity criteria. One of the most general one applicable to causal interacting systems is to ask that all the quantum parts of the system are part of elementaries whose paths start and end within the entitiy. We call this causal convexity. In other words, causal convexity excludes all quantums that leave the system (no more interacting), or that are not yet part of it (not yet interacting).
So, a photon leaving a body is not part of a convex system, while a real photon that is the carrier of clasical electromagnetic interaction between two molecular parts of the body, is part of the convex body.
A physical phenomenon is defined as a causally non-convex interacting system, complement of causally convex interacting system."""@en,
        "The class of individuals standing for causally convex interacting systems."@en .

emmo:EMMO_40c65eb4_5b58_4b13_8752_9976582380af a owl:DatatypeProperty ;
    rdfs:label "chemicalSymbolValue"@en ;
    rdfs:domain emmo:EMMO_d357e0dd_3497_4590_af6f_7954db7fecf7 ;
    rdfs:subPropertyOf emmo:EMMO_23b579e1_8088_45b5_9975_064014026c42 ;
    skos:prefLabel "chemicalSymbolValue"@en .

emmo:EMMO_41cecfc2_bb6b_45f3_b6cc_e7740d931afe rdfs:label "MatterByStructure"@en ;
    rdfs:comment "Categorisation of matter by its structure."@en .

emmo:EMMO_4208f937_8bad_47cf_af46_4ada75e63adb a owl:Class ;
    rdfs:label "MolecularFormula"@en ;
    rdfs:comment "An expression that provides information about the element types that constiture a molecule or a molecular substance and their number."^^xsd:string ;
    rdfs:subClassOf [ a owl:Restriction ;
            owl:onProperty emmo:EMMO_b2282816_b7a3_44c6_b2cb_3feff1ceb7fe ;
            owl:someValuesFrom emmo:EMMO_4f40def1_3cd7_4067_9596_541e9a5134cf ],
        emmo:EMMO_9236d0aa_cb39_43a1_bbdd_6a2a714951c8 ;
    skos:example "Hydrogen peroxide is H2O2"^^xsd:string ;
    skos:prefLabel "MolecularFormula"@en ;
    emmo:EMMO_967080e5_2f42_4eb2_a3a9_c58143e835f9 "An expression that provides information about the element types that constiture a molecule or a molecular substance and their number."^^xsd:string .

emmo:EMMO_436b11bd_1756_4821_9f14_c9ed6b67552e a owl:Class ;
    rdfs:label "ElementalSubstance"@en ;
    rdfs:comment "A chemical substance composed of atoms with the same number of protons in the atomic nucleus."^^xsd:string ;
    rdfs:subClassOf emmo:EMMO_df96cbb6_b5ee_4222_8eab_b3675df24bea ;
    skos:altLabel "PureSubstance"@en ;
    skos:prefLabel "ElementalSubstance"@en ;
    emmo:EMMO_967080e5_2f42_4eb2_a3a9_c58143e835f9 "A chemical substance composed of atoms with the same number of protons in the atomic nucleus."^^xsd:string ;
    emmo:EMMO_fe015383_afb3_44a6_ae86_043628697aa2 "https://doi.org/10.1351/goldbook.C01022"^^xsd:string .

emmo:EMMO_47338839_6cca_4a8e_b565_3c4d5517e2c0 a owl:Class ;
    rdfs:label "ChemicalEntity"@en ;
    rdfs:comment """A chemical entity comprises the two different ways to represents matter: as single recognizable particle entity (molecular entity) and as a composition of particle entities (substance).

This distinction is not well assessed in actual chemical nomenclature, in which an element name refers to both the pure elemental substance or the atom.

In the EMMO we force the adoption of a more strict categorization based on mereotopology.

The class Material hosts the subclasses for which a substance can be identified without necessarily considering its nature of molecule/atom or substance (e.g. hydrocarbon is the class of both hydrocarbon molecules or gases)."""^^xsd:string ;
    rdfs:subClassOf emmo:EMMO_5b2222df_4da6_442f_8244_96e9e45887d1 ;
    owl:disjointUnionOf ( emmo:EMMO_21205421_5783_4d3e_81e5_10c5d894a88a emmo:EMMO_df96cbb6_b5ee_4222_8eab_b3675df24bea ) ;
    skos:prefLabel "ChemicalEntity"@en .

emmo:EMMO_4e659c69_ca2d_4569_8a96_f99857a1fa32 a owl:Class ;
    rdfs:label "InorganicCompound"@en ;
    rdfs:comment "A chemical compound that is not organic."@en ;
    rdfs:subClassOf emmo:EMMO_e2b11f6a_4191_427e_9844_2e0ac88dfc8b ;
    owl:disjointWith emmo:EMMO_704630b8_fee3_49b9_baca_40e2dd276370 ;
    skos:prefLabel "InorganicCompound"@en ;
    emmo:EMMO_967080e5_2f42_4eb2_a3a9_c58143e835f9 "A chemical compound that is not organic."@en .

emmo:EMMO_51f426a6_af4a_4e91_a392_2b0bb635e2d5 a owl:ObjectProperty ;
    rdfs:label "hasChemicalComposition"@en ;
    rdfs:comment "Relates a substance to chemical composition."@en ;
    rdfs:domain emmo:EMMO_bc37743c_37c4_4ec7_9d58_d1aae5567352 ;
    rdfs:range emmo:EMMO_7efd64d1_05a1_49cd_a7f0_783ca050d4f3 ;
    rdfs:subPropertyOf emmo:EMMO_eb3518bf_f799_4f9e_8c3e_ce59af11453b ;
    skos:example """This relation can be used to relate a material to a chemical composition quantity of one of its chemical species. For example, the amount of aluminium in substance subst:alloy1 can be expressed as:

```turtle
subst:alloy1 a emmo:Substance ;
    emmo:hasChemicalComposition [
        a emmo:SingleComponentComposition ;
        emmo:hasSpeciesPart [ a emmo:AluminiumSymbol ] ;
        emmo:hasQuantityPart [
            a emmo:MassFraction ;
            hasSIQuantityValue "98.1 wt%"^^emmo:SIQuantityDatatype
        ]
    ] .
```"""@en ;
    skos:prefLabel "hasChemicalComposition"@en ;
    emmo:EMMO_967080e5_2f42_4eb2_a3a9_c58143e835f9 "Relates a substance to chemical composition."@en ;
    emmo:EMMO_c7b62dd7_063a_4c2a_8504_42f7264ba83f "This property is often used to relate a substance directly to SingleComponentComposition indifiduals for each of its components."@en .

emmo:EMMO_57d977ab_0036_4779_b59a_e47620afdb9c rdfs:label "CompositePhysicalObject"@en ;
    rdfs:comment "The class of physical objects possessing a structure that is larger than a single composite particle, for which its bosonic or fermionic nature is undetermined."^^xsd:string,
        "A composite physical object is made of bonded objects (i.e. characterised by their quantum states using a Schrodinger equation approach) that are connected together by elementary particles travelling between them. These elemenentary particles are real particles, describing the existance of a classical field (e.g. Coulomb potential between charged particles)."@en .

emmo:EMMO_649bf97b_4397_4005_90d9_219755d92e34 rdfs:label "Perceptual"@en ;
    rdfs:comment "The class contrast individuals standing for entities that can stimulate a perception (e.g. a retina impression) to a human being and that are categorized accordingly to human perception mechanisms."@en .

emmo:EMMO_6afdb7e8_2a0b_444d_bde3_8d67d98180c0 a owl:Class ;
    rdfs:label "EmpiricalFormula"@en ;
    rdfs:comment "An expression that provide information about the element type of a compound and their relative ratio."^^xsd:string ;
    rdfs:subClassOf emmo:EMMO_9236d0aa_cb39_43a1_bbdd_6a2a714951c8 ;
    skos:example "Hydrogen peroxide is HO"^^xsd:string ;
    skos:prefLabel "EmpiricalFormula"@en ;
    emmo:EMMO_967080e5_2f42_4eb2_a3a9_c58143e835f9 "An expression that provide information about the element type of a compound and their relative ratio."^^xsd:string .

emmo:EMMO_76bd5e44_bf5a_49f9_a517_eea5e8bcbc2d rdfs:label "CausalCluster"@en ;
    rdfs:comment "The class of individuals representing causal clusters."@en,
        "The disjoint union of the CausalSystem and Collection classes."@en,
        "With the causal cluster term we address an heterogeneous group of entities, which possess the common feature of having at least two causally non connected quanta. It comprises collections (non self-connected entities) and causal systems (entities extended in space)."@en .

emmo:EMMO_7aec67a4_fb96_47c6_80a3_8fea557b2cbb a owl:ObjectProperty ;
    rdfs:label "hasChemicalSpecies"@en ;
    rdfs:comment "Relates a substance to one of its chemical species."@en ;
    rdfs:domain emmo:EMMO_bc37743c_37c4_4ec7_9d58_d1aae5567352 ;
    rdfs:range emmo:EMMO_cbcf8fe6_6da6_49e0_ab4d_00f737ea9689 ;
    rdfs:subPropertyOf emmo:EMMO_eb3518bf_f799_4f9e_8c3e_ce59af11453b ;
    skos:prefLabel "hasChemicalSpecies"@en ;
    emmo:EMMO_967080e5_2f42_4eb2_a3a9_c58143e835f9 "Relates a substance to one of its chemical species."@en .

emmo:EMMO_7c055d65_2929_40e1_af4f_4bf10995ad50 rdfs:subClassOf emmo:EMMO_a293f923_954c_4af5_9f97_9600ebd362cb .

emmo:EMMO_801395f8_948e_4637_ac3b_5fcd587d72ca rdfs:label "BondedObject"@en ;
    rdfs:comment "A bonded object is a sequence of fundamental interactions that can be described approximatively by Schrodinger formulation. A bonded object is typically characterised by having quantum states (e.g.  electron states in an atom, energy levels of a molecule). Furthermore, a bonded object is made of elementary particles that travels from the beginning to the end of the entity (i.e. a bonded object doesn't change its components)."@en .

emmo:EMMO_8b1367d6_0133_4b56_acc1_fa8b058169e3 rdfs:label "BondedParticle"@en ;
    rdfs:comment "A composite particle is a bonded particle for which it is possible to clearly define its bosonic or fermionic behaviour. The term particle is then reserved for entities whose fermionic or bosonic nature is clearly defined."@en .

emmo:EMMO_a14dd591_8b7a_4847_8c91_3a2f421a45b4 a owl:Class ;
    rdfs:label "Macromolecule"@en ;
    rdfs:comment "A polyatomic entity containing a very large number of atoms."@en ;
    rdfs:subClassOf emmo:EMMO_9fa966c7_5231_409e_841f_b4c5fd33732a ;
    skos:example "Protein, nucleic acid, or synthetic polymer."@en ;
    skos:prefLabel "Macromolecule"@en ;
    emmo:EMMO_967080e5_2f42_4eb2_a3a9_c58143e835f9 "A polyatomic entity containing a very large number of atoms."@en .

emmo:EMMO_a15cea10_9946_4d2b_95c5_cfc333fd2abb rdfs:label "PhysicalParticle"@en ;
    rdfs:comment "A well defined physical entity, elementary or composite, usually treated as a singular unit, that is found at scales spanning from the elementary particles to molecules, as fundamental constituents of larger scale substances (as the etymology of \"particle\" suggests)."@en,
        "The union of hadron and lepton, or fermion and bosons."@en .

emmo:EMMO_a466b60b_d973_4b8f_897f_d0b837a59df3 a owl:Class ;
    rdfs:label "StructuralFormula"@en ;
    rdfs:comment "A graphical representation of a molecular structure showing the relative position in space of the atomic constituents and their bonds."^^xsd:string ;
    rdfs:subClassOf emmo:EMMO_ecc4efe9_77a2_47e3_8190_f9a883d54ac6 ;
    skos:prefLabel "StructuralFormula"@en ;
    emmo:EMMO_967080e5_2f42_4eb2_a3a9_c58143e835f9 "A graphical representation of a molecular structure showing the relative position in space of the atomic constituents and their bonds."^^xsd:string .

emmo:EMMO_a8eb87b5_4d10_4137_a75c_e04ee59ca095 rdfs:subClassOf emmo:EMMO_a293f923_954c_4af5_9f97_9600ebd362cb .

emmo:EMMO_b295158f_fda4_4124_ab58_d9ea4ccfca5a rdfs:label "GenericPhysicalSystem"@en ;
    rdfs:comment "A causal system possessing bonding that can not be represented by a simple Feynman diagram."@en,
        "A generic physical system is everything which is more complex than a scattering interaction, or a decay/annihilation event, which are represented by a single Feynman diagram."@en .

emmo:EMMO_b32fe85d_2f7b_4972_9dd7_7cf20d4bba59 rdfs:label "PhysicalParticleByBond"@en ;
    rdfs:comment "Categorisation of physical particles by whether they are bonded."@en .

emmo:EMMO_be8592a7_68d1_4a06_ad23_82f2b56ef926 rdfs:label "DiscreteData"@en ;
    rdfs:comment "Data whose variations are decoded according to a discrete schema."@en .

emmo:EMMO_bf836c2b_7800_474d_b674_f5d629fa0bb1 a owl:Class ;
    rdfs:label "CondensedFormula"@en ;
    rdfs:subClassOf emmo:EMMO_9236d0aa_cb39_43a1_bbdd_6a2a714951c8 ;
    skos:example "An expression that provides information about the element types that constiture a molecule or a molecular substance and their number, together with simple information about the connectivity of its groups by using parenthesis or by goruping element names according to its molecular structure."^^xsd:string ;
    skos:prefLabel "CondensedFormula"@en .

emmo:EMMO_c5ae6d8e_6b39_431f_8de4_ae4e357abc04 rdfs:label "Visual"@en ;
    rdfs:comment "A 'Perceptual' which stands for a real world object whose spatiotemporal pattern makes it identifiable by an observer through an optical perception employing the visible part of the electromagnetic spectrum."@en .

emmo:EMMO_c66ad523_3937_485e_91bb_ad488ddb373f rdfs:label "DataByDiscretness"@en ;
    rdfs:comment "Categorisation of data by whether it is descrete or not."@en .

emmo:EMMO_c74da218_9147_4f03_92d1_8894abca55f3 rdfs:label "Graphical"@en ;
    rdfs:comment "A 'Perceptual' which stands for a real world object whose spatial configuration results from an explicit graphical procedure and shows an identifiable pattern."@en .

emmo:EMMO_d2a47cd8_662f_438f_855a_b4378eb992ff a owl:Class ;
    rdfs:label "CASRN"@en ;
    rdfs:comment "Chemical Abstact Service registry number for a chemical substance from the American Chemical Society"^^xsd:string ;
    rdfs:subClassOf emmo:EMMO_643d99dd_fae6_4121_a76f_47f486a4480b ;
    skos:example "Water is 7732-18-5"^^xsd:string ;
    skos:prefLabel "CASRN"@en ;
    emmo:EMMO_967080e5_2f42_4eb2_a3a9_c58143e835f9 "Chemical Abstact Service registry number for a chemical substance from the American Chemical Society"^^xsd:string .

emmo:EMMO_d5be1faf_0c56_4f5a_9b78_581e6dee949f rdfs:subClassOf emmo:EMMO_a293f923_954c_4af5_9f97_9600ebd362cb .

emmo:EMMO_d74ed682_894f_46c5_87cb_167f60926965 a owl:Class ;
    rdfs:label "InChI"@en ;
    rdfs:comment "The International Chemical Identifier (InChI) textual identifier proposed by IUPAC to provide a standard encoding for databases of molecular information."^^xsd:string ;
    rdfs:subClassOf emmo:EMMO_91a0635a_a89a_46de_8928_04a777d145c7 ;
    skos:prefLabel "InChI"@en ;
    emmo:EMMO_967080e5_2f42_4eb2_a3a9_c58143e835f9 "The International Chemical Identifier (InChI) textual identifier proposed by IUPAC to provide a standard encoding for databases of molecular information."^^xsd:string .

emmo:EMMO_e7aac247_31d6_4b2e_9fd2_e842b1b7ccac rdfs:label "CausalSystem"@en ;
    rdfs:comment """A causal system provides the most general concept of system, being a union of causal structures interacting together. In its most simple form, a causal system is an interlacement of causal paths (the most simple structure type).
A causal system is always a spatial-like structure, and is represented as a multiple topologically orderable direct acyclic graph, with quanta as nodes and causality relations as edges."""@en,
        "The class of individuals representing a causal system."@en .

<https://w3id.org/emmo/disciplines/chemistry> a owl:Ontology ;
    dcterms:abstract "The chemistry module populates the physicalistic perspective with materials subclasses categorised according to modern applied chemistry."@en ;
    dcterms:creator <https://orcid.org/0000-0002-1560-809X>,
        <https://orcid.org/0000-0002-4181-2852>,
        <https://orcid.org/0000-0003-3805-8761> ;
    dcterms:license "https://creativecommons.org/licenses/by/4.0/legalcode"^^xsd:string ;
    dcterms:publisher <https://emmc.eu> ;
    dcterms:title "Chemistry"@en ;
    rdfs:comment "The EMMO requires FacT++ reasoner plugin in order to visualize all inferences and class hierarchy (ctrl+R hotkey in Protege)."@en ;
    owl:imports <https://w3id.org/emmo/1.0.3/disciplines/isq>,
        <https://w3id.org/emmo/1.0.3/disciplines/perceptual> ;
    owl:versionIRI <https://w3id.org/emmo/1.0.3/disciplines/chemistry> ;
    owl:versionInfo "1.0.3"^^xsd:string ;
    emmo:EMMO_1246b120_abbe_4840_b0f8_3e4348b24a17 "emmo@emmc.eu"^^xsd:string .

emmo:EMMO_0eabfde6_c6c5_4b1f_bf10_e4e0e06e9b2e a owl:Class ;
    rdfs:label "TotalComposition"@en ;
    rdfs:comment "A language construct that represents fraction or amount of all constituents of a substance."@en ;
    rdfs:subClassOf [ a owl:Restriction ;
            owl:onProperty emmo:EMMO_b2282816_b7a3_44c6_b2cb_3feff1ceb7fe ;
            owl:someValuesFrom emmo:EMMO_172e2c96_180b_40f8_a3e7_b624471f40c2 ],
        emmo:EMMO_7efd64d1_05a1_49cd_a7f0_783ca050d4f3 ;
    skos:prefLabel "TotalComposition"@en ;
    emmo:EMMO_967080e5_2f42_4eb2_a3a9_c58143e835f9 "A language construct that represents fraction or amount of all constituents of a substance."@en .

emmo:EMMO_18fdd2cd_4b0a_43a5_a938_66d8290a066c a owl:AsymmetricProperty,
        owl:IrreflexiveProperty,
        owl:ObjectProperty ;
    rdfs:label "hasSpeciesPart"@en ;
    rdfs:comment "Relates a chemical composition to one its species."@en ;
    rdfs:domain emmo:EMMO_7efd64d1_05a1_49cd_a7f0_783ca050d4f3 ;
    rdfs:range emmo:EMMO_cbcf8fe6_6da6_49e0_ab4d_00f737ea9689 ;
    rdfs:subPropertyOf emmo:EMMO_b2282816_b7a3_44c6_b2cb_3feff1ceb7fe ;
    skos:prefLabel "hasSpeciesPart"@en ;
    emmo:EMMO_967080e5_2f42_4eb2_a3a9_c58143e835f9 "Relates a chemical composition to one its species."@en ;
    emmo:EMMO_c7b62dd7_063a_4c2a_8504_42f7264ba83f "This property is typically used to relate a SingleComponentComposition to its chemical species."@en .

emmo:EMMO_26586828_3b8c_4d8b_9c6c_0bc2502f26ae a owl:Class ;
    rdfs:label "ChemicalName"@en ;
    rdfs:comment "Name of a chemical according to a standard."@en ;
    rdfs:subClassOf emmo:EMMO_643d99dd_fae6_4121_a76f_47f486a4480b ;
    skos:prefLabel "ChemicalName"@en ;
    emmo:EMMO_967080e5_2f42_4eb2_a3a9_c58143e835f9 "Name of a chemical according to a standard."@en .

emmo:EMMO_5b2222df_4da6_442f_8244_96e9e45887d1 rdfs:label "Matter"@en ;
    rdfs:comment "The class of physical objects that have some fermionic quantum parts."@en,
        """The interpretation of the term "matter" is not univocal. Several concepts are labelled with this term, depending on the field of science. The concept mass is sometimes related to the term "matter", even if the former refers to a physical quantity (precisely defined by modern physics) while the latter is a type that qualifies a physical entity.
It is possible to identify more than one concept that can be reasonably labelled with the term "matter". For example, it is possible to label as matter only the entities that are made up of atoms. Or more generally, we can be more fine-grained and call "matter" the entities that are made up of protons, neutrons or electrons, so that we can call matter also a neutron radiation or a cathode ray.
A more fundamental approach, that we embrace for the EMMO, considers matter as entities that are made of fermions (i.e. quarks and leptons) requiring their presence, without excluding particles like the W and Z bosons that possess some mass, but are not fermions.
Antimatter is a subclass of matter."""@en .

emmo:EMMO_704630b8_fee3_49b9_baca_40e2dd276370 a owl:Class ;
    rdfs:label "OrganicCompound"@en ;
    dcterms:source "https://goldbook.iupac.org"^^xsd:anyURI ;
    rdfs:comment """A chemical compound containing carbon atoms.

-- IUPAC"""@en ;
    rdfs:subClassOf emmo:EMMO_e2b11f6a_4191_427e_9844_2e0ac88dfc8b ;
    skos:prefLabel "OrganicCompound"@en ;
    emmo:EMMO_967080e5_2f42_4eb2_a3a9_c58143e835f9 """A chemical compound containing carbon atoms.

-- IUPAC"""@en ;
    emmo:EMMO_c7b62dd7_063a_4c2a_8504_42f7264ba83f "The definition of organic compound is based on the IUPAC Gold Book. However, sometimes an organic compound is defined as a chemical compound that contains a carbon–hydrogen or carbon–carbon bond. Also, some carbon-containing compounds are typically not classified as organic, like carbides, carbonates, and cyanides."@en .

emmo:EMMO_90963312_d9a9_4474_8d10_835aef5b168e a owl:Class ;
    rdfs:label "PartialComposition"@en ;
    rdfs:comment "A language construct that represents fraction or amount of some (but not all) constituents of a substance."@en ;
    rdfs:subClassOf [ a owl:Restriction ;
            owl:onProperty emmo:EMMO_b2282816_b7a3_44c6_b2cb_3feff1ceb7fe ;
            owl:someValuesFrom emmo:EMMO_172e2c96_180b_40f8_a3e7_b624471f40c2 ],
        emmo:EMMO_7efd64d1_05a1_49cd_a7f0_783ca050d4f3 ;
    skos:prefLabel "PartialComposition"@en ;
    emmo:EMMO_967080e5_2f42_4eb2_a3a9_c58143e835f9 "A language construct that represents fraction or amount of some (but not all) constituents of a substance."@en .

emmo:EMMO_95d706e4_8b16_48a1_8dfd_40ccd4df1c12 a owl:AsymmetricProperty,
        owl:IrreflexiveProperty,
        owl:ObjectProperty ;
    rdfs:label "hasQuantityPart"@en ;
    rdfs:domain emmo:EMMO_89a0c87c_0804_4013_937a_6fe234d9499c ;
    rdfs:range emmo:EMMO_0650c031_42b6_4f0a_b62d_d88f071da6bf ;
    rdfs:subPropertyOf emmo:EMMO_b2282816_b7a3_44c6_b2cb_3feff1ceb7fe ;
    skos:prefLabel "hasQuantityPart"@en ;
    emmo:EMMO_c7b62dd7_063a_4c2a_8504_42f7264ba83f "Relates a symbolic construct to one of its quantity parts."@en .

emmo:EMMO_9fa966c7_5231_409e_841f_b4c5fd33732a a owl:Class ;
    rdfs:label "PolyatomicEntity"@en ;
    rdfs:comment "An entity made of two or more bonded atoms."@en ;
    rdfs:subClassOf emmo:EMMO_21205421_5783_4d3e_81e5_10c5d894a88a ;
    skos:prefLabel "PolyatomicEntity"@en ;
    emmo:EMMO_967080e5_2f42_4eb2_a3a9_c58143e835f9 "An entity made of two or more bonded atoms."@en .

emmo:EMMO_bd8db028_aec2_4a44_ad93_1a9f8270f72c a owl:Class ;
    rdfs:label "ChemicalSymbolicConstruct"@en ;
    rdfs:comment "A symbolic construct that stands for a chemical."@en ;
    owl:equivalentClass [ a owl:Class ;
            owl:intersectionOf ( emmo:EMMO_89a0c87c_0804_4013_937a_6fe234d9499c emmo:EMMO_abf7efbe_6b04_41b8_8326_4dd0f6be753e ) ] ;
    skos:example "H2O"@en ;
    skos:prefLabel "ChemicalSymbolicConstruct"@en ;
    emmo:EMMO_967080e5_2f42_4eb2_a3a9_c58143e835f9 "A symbolic construct that stands for a chemical."@en .

emmo:EMMO_d357e0dd_3497_4590_af6f_7954db7fecf7 a owl:Class ;
    rdfs:label "ChemicalSymbol"@en ;
    rdfs:comment "A symbol that stands for a chemical element."@en ;
    owl:equivalentClass [ a owl:Class ;
            owl:intersectionOf ( emmo:EMMO_a1083d0a_c1fb_471f_8e20_a98f881ad527 emmo:EMMO_abf7efbe_6b04_41b8_8326_4dd0f6be753e ) ] ;
    skos:example """"H"
"He"
"Li"
..."""@en ;
    skos:prefLabel "ChemicalSymbol"@en ;
    emmo:EMMO_967080e5_2f42_4eb2_a3a9_c58143e835f9 "A symbol that stands for a chemical element."@en .

emmo:EMMO_d8d2144e_5c8d_455d_a643_5caf4d8d9df8 rdfs:label "Language"@en ;
    rdfs:comment "A language object is a discrete data entity respecting specific language syntactic rules (a well-formed formula)."@en .

emmo:EMMO_eb7de1a1_c30e_4f0d_94c6_fe70414d7e61 rdfs:label "Representation"@en ;
    rdfs:comment "A graphical object aimed to represent schematically the conceptual, temporal or spatial structure of another object, that may or may not exist."@en .

emmo:EMMO_ecc4efe9_77a2_47e3_8190_f9a883d54ac6 a owl:Class ;
    rdfs:label "ChemicalRepresentation"@en ;
    rdfs:comment "A representation of objects belonging to the chemistry field."^^xsd:string ;
    rdfs:subClassOf emmo:EMMO_eb7de1a1_c30e_4f0d_94c6_fe70414d7e61 ;
    skos:prefLabel "ChemicalRepresentation"@en ;
    emmo:EMMO_967080e5_2f42_4eb2_a3a9_c58143e835f9 "A representation of objects belonging to the chemistry field."^^xsd:string .

emmo:EMMO_21205421_5783_4d3e_81e5_10c5d894a88a rdfs:label "MolecularEntity"@en ;
    rdfs:comment """Molecular entity is used as a general term for singular entities, irrespective of their nature, while chemical species stands for sets or ensembles of molecular entities.

Note that the name of a compound may refer to the respective molecular entity or to the chemical species,"""^^xsd:string,
        "Any constitutionally or isotopically distinct atom, molecule, ion, ion pair, radical, radical ion, complex, conformer etc., identifiable as a separately distinguishable entity that can undergo a chemical reaction."@en ;
    skos:example "Hydrogen molecule is an adequate definition of a certain molecular entity for some purposes, whereas for others it is necessary to distinguish the electronic state and/or vibrational state and/or nuclear spin, etc. of the hydrogen molecule."^^xsd:string,
        "Methane, may mean a single molecule of CH4 (molecular entity) or a molar amount, specified or not (chemical species), participating in a reaction. The degree of precision necessary to describe a molecular entity depends on the context."^^xsd:string .

emmo:EMMO_91a0635a_a89a_46de_8928_04a777d145c7 a owl:Class ;
    rdfs:label "IUPACNomenclature"@en ;
    rdfs:comment "Chemical nomenclauture following the IUPAC standard."@en ;
    rdfs:subClassOf emmo:EMMO_643d99dd_fae6_4121_a76f_47f486a4480b ;
    skos:prefLabel "IUPACNomenclature"@en ;
    emmo:EMMO_967080e5_2f42_4eb2_a3a9_c58143e835f9 "Chemical nomenclauture following the IUPAC standard."@en .

emmo:EMMO_a1083d0a_c1fb_471f_8e20_a98f881ad527 rdfs:label "Symbol"@en ;
    rdfs:comment "The class of individuals that stand for an elementary mark of a specific symbolic code (alphabet)."@en .

emmo:EMMO_e2b11f6a_4191_427e_9844_2e0ac88dfc8b a owl:Class ;
    rdfs:label "ChemicalCompound"@en ;
    rdfs:comment "A chemical substance composed of many identical molecules (or molecular entities) composed of atoms from more than one element held together by chemical bonds."^^xsd:string ;
    rdfs:subClassOf emmo:EMMO_df96cbb6_b5ee_4222_8eab_b3675df24bea ;
    skos:prefLabel "ChemicalCompound"@en ;
    emmo:EMMO_8a137e9f_579c_4e28_baca_e8980eb0c3db "DisjointUnionOf InorganicCompound, OrganicCompound"^^xsd:string ;
    emmo:EMMO_967080e5_2f42_4eb2_a3a9_c58143e835f9 "A chemical substance composed of many identical molecules (or molecular entities) composed of atoms from more than one element held together by chemical bonds."^^xsd:string ;
    emmo:EMMO_c84c6752_6d64_48cc_9500_e54a3c34898d "https://en.wikipedia.org/wiki/Chemical_compound"^^xsd:string .

emmo:EMMO_172e2c96_180b_40f8_a3e7_b624471f40c2 a owl:Class ;
    rdfs:label "SingleComponentComposition"@en ;
    rdfs:comment "A language construct that represents the fraction or amount of a single constituent of a substance."@en ;
    rdfs:subClassOf [ a owl:Restriction ;
            owl:onProperty emmo:EMMO_95d706e4_8b16_48a1_8dfd_40ccd4df1c12 ;
            owl:someValuesFrom emmo:EMMO_a293f923_954c_4af5_9f97_9600ebd362cb ],
        [ a owl:Restriction ;
            owl:onProperty emmo:EMMO_18fdd2cd_4b0a_43a5_a938_66d8290a066c ;
            owl:someValuesFrom emmo:EMMO_cbcf8fe6_6da6_49e0_ab4d_00f737ea9689 ],
        emmo:EMMO_7efd64d1_05a1_49cd_a7f0_783ca050d4f3 ;
    skos:prefLabel "SingleComponentComposition"@en ;
    emmo:EMMO_967080e5_2f42_4eb2_a3a9_c58143e835f9 "A language construct that represents the fraction or amount of a single constituent of a substance."@en .

emmo:EMMO_4f40def1_3cd7_4067_9596_541e9a5134cf a owl:Class ;
    rdfs:label "ChemicalElement"@en ;
    rdfs:comment """The IUPAC Gold Book defines the a chemical element both as:
- a species of atoms; all atoms with the same number of protons in the atomic nucleus
-  a pure chemical substance composed of atoms with the same number of protons in the atomic nucleus

This qualifies a chemical element as a name and not a matter obejct that can stand for an atom or a substance."""^^xsd:string,
        "The symbol for a specific chemical element, that can stand both for an atom or a substance."^^xsd:string ;
    rdfs:seeAlso "http://publications.iupac.org/ci/2005/2701/ud.html"^^xsd:string ;
    rdfs:subClassOf emmo:EMMO_a1083d0a_c1fb_471f_8e20_a98f881ad527,
        emmo:EMMO_abf7efbe_6b04_41b8_8326_4dd0f6be753e ;
    skos:prefLabel "ChemicalElement"@en ;
    emmo:EMMO_967080e5_2f42_4eb2_a3a9_c58143e835f9 "The symbol for a specific chemical element, that can stand both for an atom or a substance."^^xsd:string ;
    emmo:EMMO_fe015383_afb3_44a6_ae86_043628697aa2 "https://doi.org/10.1351/goldbook.C01022"^^xsd:string .

emmo:EMMO_bc37743c_37c4_4ec7_9d58_d1aae5567352 rdfs:label "Substance"@en ;
    rdfs:comment "A matter entity characterised by the fact that it possesses some homogeneous properties or identification criteria."@en .

emmo:EMMO_cbcf8fe6_6da6_49e0_ab4d_00f737ea9689 a owl:Class ;
    rdfs:label "ChemicalSpecies"@en ;
    rdfs:comment """Following nominalistic approach a species is simply a name that can point to an element name, a chemical formula or a chemical compound.

So everything addressed by these classes of names can be calleded a chemical species."""^^xsd:string,
        """N2
Methane
CH4
Fe
Sodium Chloride"""^^xsd:string,
        """Specific form of an element defined as to isotopic composition, electronic or oxidation state, and/or complex or molecular structure.

Chemical species is the macroscopic equivalent of molecular entity and refers to sets or ensembles of molecular entities."""^^xsd:string ;
    rdfs:subClassOf emmo:EMMO_abf7efbe_6b04_41b8_8326_4dd0f6be753e ;
    owl:equivalentClass [ a owl:Class ;
            owl:unionOf ( emmo:EMMO_4f40def1_3cd7_4067_9596_541e9a5134cf emmo:EMMO_643d99dd_fae6_4121_a76f_47f486a4480b emmo:EMMO_9236d0aa_cb39_43a1_bbdd_6a2a714951c8 ) ] ;
    skos:prefLabel "ChemicalSpecies"@en ;
    emmo:EMMO_967080e5_2f42_4eb2_a3a9_c58143e835f9 """Specific form of an element defined as to isotopic composition, electronic or oxidation state, and/or complex or molecular structure.

Chemical species is the macroscopic equivalent of molecular entity and refers to sets or ensembles of molecular entities."""^^xsd:string ;
    emmo:EMMO_fe015383_afb3_44a6_ae86_043628697aa2 "https://doi.org/10.1351/goldbook.CT06859"^^xsd:string .

emmo:EMMO_df96cbb6_b5ee_4222_8eab_b3675df24bea a owl:Class ;
    rdfs:label "ChemicalSubstance"@en ;
    rdfs:comment "A substance is always composed of more than one molecular entity. It lays in the continuum or mesoscopic domain."^^xsd:string,
        "Matter of constant composition best characterized by the entities (molecules, formula units, atoms) it is composed of."^^xsd:string ;
    rdfs:subClassOf emmo:EMMO_bc37743c_37c4_4ec7_9d58_d1aae5567352 ;
    skos:prefLabel "ChemicalSubstance"@en ;
    emmo:EMMO_967080e5_2f42_4eb2_a3a9_c58143e835f9 "Matter of constant composition best characterized by the entities (molecules, formula units, atoms) it is composed of."^^xsd:string ;
    emmo:EMMO_fe015383_afb3_44a6_ae86_043628697aa2 "https://doi.org/10.1351/goldbook.C01039"^^xsd:string .

emmo:EMMO_643d99dd_fae6_4121_a76f_47f486a4480b a owl:Class ;
    rdfs:label "ChemicalNomenclature"@en ;
    rdfs:comment "A chemical numenclature should not be confused with the chemical formula."^^xsd:string,
        "A language object following a specific nomenclature rules for defining univocal names of chemical compounds."^^xsd:string ;
    rdfs:subClassOf emmo:EMMO_abf7efbe_6b04_41b8_8326_4dd0f6be753e ;
    skos:prefLabel "ChemicalNomenclature"@en ;
    emmo:EMMO_967080e5_2f42_4eb2_a3a9_c58143e835f9 "A language object following a specific nomenclature rules for defining univocal names of chemical compounds."^^xsd:string .

emmo:EMMO_9236d0aa_cb39_43a1_bbdd_6a2a714951c8 a owl:Class ;
    rdfs:label "ChemicalFormula"@en ;
    rdfs:comment "A chemical formula may also include other symbols such as parentheses, plus and minus signs, brackets"^^xsd:string,
        "A symbolic construct that provides informations about the chemical proportions of the elements that constitute a chemical compound or a specific molecule."^^xsd:string ;
    rdfs:subClassOf [ a owl:Restriction ;
            owl:onProperty emmo:EMMO_b2282816_b7a3_44c6_b2cb_3feff1ceb7fe ;
            owl:someValuesFrom emmo:EMMO_4f40def1_3cd7_4067_9596_541e9a5134cf ],
        emmo:EMMO_abf7efbe_6b04_41b8_8326_4dd0f6be753e ;
    skos:prefLabel "ChemicalFormula"@en ;
    emmo:EMMO_967080e5_2f42_4eb2_a3a9_c58143e835f9 "A symbolic construct that provides informations about the chemical proportions of the elements that constitute a chemical compound or a specific molecule."^^xsd:string .

emmo:EMMO_7efd64d1_05a1_49cd_a7f0_783ca050d4f3 a owl:Class ;
    rdfs:label "ChemicalComposition"@en ;
    rdfs:comment "A language construct that provides information about the consitutents of a substance and their fractions or amounts."^^xsd:string ;
    rdfs:subClassOf emmo:EMMO_bd8db028_aec2_4a44_ad93_1a9f8270f72c ;
    owl:equivalentClass [ a owl:Class ;
            owl:unionOf ( emmo:EMMO_0eabfde6_c6c5_4b1f_bf10_e4e0e06e9b2e emmo:EMMO_172e2c96_180b_40f8_a3e7_b624471f40c2 emmo:EMMO_90963312_d9a9_4474_8d10_835aef5b168e ) ] ;
    skos:prefLabel "ChemicalComposition"@en ;
    emmo:EMMO_967080e5_2f42_4eb2_a3a9_c58143e835f9 "A language construct that provides information about the consitutents of a substance and their fractions or amounts."^^xsd:string .

emmo:EMMO_abf7efbe_6b04_41b8_8326_4dd0f6be753e a owl:Class ;
    rdfs:label "Chemical"@en ;
    rdfs:comment "A language object that follows the syntactic rules used in the chemical field."^^xsd:string ;
    rdfs:subClassOf emmo:EMMO_d8d2144e_5c8d_455d_a643_5caf4d8d9df8 ;
    skos:prefLabel "Chemical"@en ;
    emmo:EMMO_967080e5_2f42_4eb2_a3a9_c58143e835f9 "A language object that follows the syntactic rules used in the chemical field."^^xsd:string .

