@prefix dcterms: <http://purl.org/dc/terms/> .
@prefix emmo: <https://w3id.org/emmo#> .
@prefix owl: <http://www.w3.org/2002/07/owl#> .
@prefix rdfs: <http://www.w3.org/2000/01/rdf-schema#> .
@prefix skos: <http://www.w3.org/2004/02/skos/core#> .
@prefix xsd: <http://www.w3.org/2001/XMLSchema#> .

owl:qualifiedCardinality a owl:AnnotationProperty .

emmo:EMMO_9be5fcc4_0d8b_481d_b984_6338d4b55588 a owl:Class ;
    rdfs:label "Measurer"@en ;
    rdfs:comment "An observer that makes use of a measurement tool and provides a quantitative property."@en ;
    rdfs:subClassOf emmo:EMMO_ea67caa5_2609_4e91_98ae_81103f2d5c25 ;
    skos:prefLabel "Measurer"@en ;
    emmo:EMMO_967080e5_2f42_4eb2_a3a9_c58143e835f9 "An observer that makes use of a measurement tool and provides a quantitative property."@en .

emmo:EMMO_d271f202_4c1a_4d74_b86a_387c82034eb7 a owl:ObjectProperty ;
    rdfs:label "hasCharacterised"@en ;
    rdfs:domain emmo:EMMO_1b52ee70_121e_4d8d_8419_3f97cd0bd89c ;
    rdfs:subPropertyOf emmo:EMMO_0d829933_29e3_4e61_b3d3_88e6b9d0d0ce ;
    skos:prefLabel "hasCharacterised"@en .

emmo:EMMO_eeb8118c_b290_4f57_b0f8_bd65bb6d77ad a owl:ObjectProperty ;
    rdfs:label "hasCharacteriser"@en ;
    rdfs:domain emmo:EMMO_b7bcff25_ffc3_474e_9ab5_01b1664bd4ba ;
    rdfs:range emmo:EMMO_1b52ee70_121e_4d8d_8419_3f97cd0bd89c ;
    rdfs:subPropertyOf emmo:EMMO_cc823237_398d_4c9a_b8fa_aa157ee3e3a5 ;
    skos:prefLabel "hasCharacteriser"@en .

emmo:EMMO_f94e509a_be29_4365_a4cd_70165e47e232 a owl:Class ;
    rdfs:label "Modeller"@en ;
    rdfs:comment "A estimator that uses modelling to declare a property of an object (i.e. infer a property from other properties)."@en ;
    rdfs:subClassOf emmo:EMMO_4a1c73f1_b6f5_4d10_a3a6_5de90bac7cd0 ;
    skos:prefLabel "Modeller"@en ;
    emmo:EMMO_967080e5_2f42_4eb2_a3a9_c58143e835f9 "A estimator that uses modelling to declare a property of an object (i.e. infer a property from other properties)."@en .

<https://w3id.org/emmo/disciplines/properties> a owl:Ontology ;
    dcterms:abstract """Defines properties as the result of an observation process. Observation is a semiotic process that stimulate an interpretant within the interpreter who communicates the observed result to other interpreters through a sign, which is the property.

Hence, properties creates a link between the holistic and the symbolic perspectives.

Subclasses of property are subclasses that spesialise the type of observation process."""@en ;
    dcterms:creator <https://orcid.org/0000-0002-1560-809X>,
        <https://orcid.org/0000-0002-4181-2852>,
        <https://orcid.org/0000-0003-0514-9229>,
        <https://orcid.org/0000-0003-3805-8761>,
        <https://orcid.org/0000-0003-4065-9742> ;
    dcterms:license "https://creativecommons.org/licenses/by/4.0/legalcode"^^xsd:string ;
    dcterms:publisher <https://emmc.eu> ;
    dcterms:title "Properties"@en ;
    rdfs:comment "The EMMO requires HermiT reasoner plugin in order to visualize all inferences and class hierarchy (ctrl+R hotkey in Protege)."@en ;
    owl:imports <https://w3id.org/emmo/1.0.3/perspectives/semiotics> ;
    owl:versionIRI <https://w3id.org/emmo/1.0.3/disciplines/properties> ;
    owl:versionInfo "1.0.3"^^xsd:string ;
    emmo:EMMO_1246b120_abbe_4840_b0f8_3e4348b24a17 "emmo@emmc.eu"^^xsd:string .

[] owl:qualifiedCardinality "1"^^xsd:nonNegativeInteger .

[] owl:qualifiedCardinality "1"^^xsd:nonNegativeInteger .

[] owl:qualifiedCardinality "1"^^xsd:nonNegativeInteger .

[] owl:qualifiedCardinality "1"^^xsd:nonNegativeInteger .

[] owl:qualifiedCardinality "1"^^xsd:nonNegativeInteger .

[] owl:qualifiedCardinality "1"^^xsd:nonNegativeInteger .

