<?xml version="1.0" encoding="UTF-8"?>
<rdf:RDF
   xmlns:annotations="http://emmo.info/emmo/top/annotations#"
   xmlns:ns1="http://emmo.info/emmo/middle/perceptual#"
   xmlns:owl="http://www.w3.org/2002/07/owl#"
   xmlns:rdf="http://www.w3.org/1999/02/22-rdf-syntax-ns#"
   xmlns:rdfs="http://www.w3.org/2000/01/rdf-schema#"
>
  <rdf:Description rdf:about="http://emmo.info/emmo/top/mereotopology#EMMO_17e27c22_37e1_468c_9dd7_95e137f73e7f">
    <rdf:type rdf:resource="http://www.w3.org/2002/07/owl#ObjectProperty"/>
    <rdf:type rdf:resource="http://www.w3.org/2002/07/owl#TransitiveProperty"/>
    <rdfs:label xml:lang="en">hasPart</rdfs:label>
    <rdfs:subPropertyOf rdf:resource="http://emmo.info/emmo/top/mereotopology#EMMO_d893d373_b579_4867_841e_1c2b31a8d2c6"/>
    <rdfs:subPropertyOf rdf:resource="http://emmo.info/emmo/top/mereotopology#EMMO_8c898653_1118_4682_9bbf_6cc334d16a99"/>
  </rdf:Description>
  <rdf:Description rdf:nodeID="N3becdf78fa194df281c8613a0d92187e">
    <rdf:rest rdf:resource="http://www.w3.org/1999/02/22-rdf-syntax-ns#nil"/>
    <rdf:first rdf:resource="http://emmo.info/emmo/middle/properties#EMMO_2a888cdf_ec4a_4ec5_af1c_0343372fc978"/>
  </rdf:Description>
  <rdf:Description rdf:about="http://emmo.info/emmo/middle/models#EMMO_8d2d9374_ef3a_47e6_8595_6bc208e07519">
    <rdf:type rdf:resource="http://www.w3.org/2002/07/owl#Class"/>
    <rdfs:comment>The 'theory' is e.g. a proposition, a book or a paper whose sub-symbols suggest in the mind of the interpreter an interpretant structure that can represent a 'physical'.

It is not an 'icon' (like a math equation), because it has no common resemblance or logical structure with the 'physical'.

In Peirce semiotics: legisign-symbol-argument</rdfs:comment>
    <annotations:EMMO_967080e5_2f42_4eb2_a3a9_c58143e835f9>A 'conventional' that stand for a 'physical'.</annotations:EMMO_967080e5_2f42_4eb2_a3a9_c58143e835f9>
    <rdfs:label xml:lang="en">Theory</rdfs:label>
    <rdfs:subClassOf rdf:resource="http://emmo.info/emmo/top/semiotics#EMMO_35d2e130_6e01_41ed_94f7_00b333d46cf9"/>
  </rdf:Description>
  <rdf:Description rdf:about="http://emmo.info/emmo/middle/isq#EMMO_b51fbd00_a857_4132_9711_0ef70e7bdd20">
    <annotations:EMMO_70fe84ff_99b6_4206_a9fc_9a8931836d84>The total luminous flux incident on a surface, per unit area.</annotations:EMMO_70fe84ff_99b6_4206_a9fc_9a8931836d84>
    <rdfs:subClassOf rdf:nodeID="N7f12189b458b48ada1ac5a4cb869b932"/>
    <annotations:EMMO_fe015383_afb3_44a6_ae86_043628697aa2>https://doi.org/10.1351/goldbook.I02941</annotations:EMMO_fe015383_afb3_44a6_ae86_043628697aa2>
    <rdf:type rdf:resource="http://www.w3.org/2002/07/owl#Class"/>
    <annotations:EMMO_6dd685dd_1895_46e4_b227_be9f7d643c25>http://dbpedia.org/page/Illuminance</annotations:EMMO_6dd685dd_1895_46e4_b227_be9f7d643c25>
    <rdfs:label xml:lang="en">Illuminance</rdfs:label>
    <rdfs:subClassOf rdf:resource="http://emmo.info/emmo/middle/isq#EMMO_2946d40b_24a1_47fa_8176_e3f79bb45064"/>
  </rdf:Description>
  <rdf:Description rdf:about="http://emmo.info/emmo/middle/metrology#EMMO_8ef3cd6d_ae58_4a8d_9fc0_ad8f49015cd0">
    <rdfs:subPropertyOf rdf:resource="http://emmo.info/emmo/middle/reductionistic#EMMO_b2282816_b7a3_44c6_b2cb_3feff1ceb7fe"/>
    <rdfs:label xml:lang="en">hasQuantityValue</rdfs:label>
    <rdfs:domain rdf:resource="http://emmo.info/emmo/middle/metrology#EMMO_f658c301_ce93_46cf_9639_4eace2c5d1d5"/>
    <rdf:type rdf:resource="http://www.w3.org/2002/07/owl#IrreflexiveProperty"/>
    <rdf:type rdf:resource="http://www.w3.org/2002/07/owl#AsymmetricProperty"/>
    <rdf:type rdf:resource="http://www.w3.org/2002/07/owl#ObjectProperty"/>
    <rdfs:range rdf:resource="http://emmo.info/emmo/middle/math#EMMO_4ce76d7f_03f8_45b6_9003_90052a79bfaa"/>
    <rdfs:comment>Relates a quantity to its reference unit through spatial direct parthood.</rdfs:comment>
    <rdf:type rdf:resource="http://www.w3.org/2002/07/owl#InverseFunctionalProperty"/>
  </rdf:Description>
  <rdf:Description rdf:about="http://emmo.info/emmo/middle/perceptual">
    <rdfs:comment>The EMMO requires FacT++ reasoner plugin in order to visualize all inferences and class hierarchy (ctrl+R hotkey in Protege).</rdfs:comment>
    <annotations:EMMO_cd5fb112_7ee7_4120_a35d_3ca3e6c3f4ab>Emanuele Ghedini (University of Bologna, IT)
Gerhard Goldbeck (GCL Ltd, UK)
Adham Hashibon (Fraunhofer IWM, DE)
Georg Schmitz (Access, DE)
Jesper Friis (SINTEF, NO)</annotations:EMMO_cd5fb112_7ee7_4120_a35d_3ca3e6c3f4ab>
    <owl:versionInfo>The European Materials Modelling Ontology

Version 1.0.0-alpha</owl:versionInfo>
    <rdfs:comment xml:lang="en">Contacts:
Gerhard Goldbeck
Goldbeck Consulting Ltd (UK)
email: gerhard@goldbeck-consulting.com

Emanuele Ghedini
University of Bologna (IT)
email: emanuele.ghedini@unibo.it</rdfs:comment>
    <rdfs:comment>European Materials and Modelling Ontology (EMMO)

EMMO is a multidisciplinary effort to develop a standard representational framework (the ontology) based on current materials modelling knowledge, including physical sciences, analytical philosophy and information and communication technologies. 

It provides the connection between the physical world, materials characterisation world and materials modelling world.</rdfs:comment>
    <rdf:type rdf:resource="http://www.w3.org/2002/07/owl#Ontology"/>
    <owl:versionIRI rdf:resource="http://emmo.info/emmo/1.0.0-alpha/middle/perceptual"/>
    <annotations:EMMO_5525a055_dda5_4556_8b91_f0d22fa676cc>EMMO is released under a Creative Commons license Attribution 4.0 International (CC BY 4.0)

https://creativecommons.org/licenses/by/4.0/legalcode</annotations:EMMO_5525a055_dda5_4556_8b91_f0d22fa676cc>
  </rdf:Description>
  <rdf:Description rdf:nodeID="N782679aee918406b85e24e8aa91c028f">
    <rdf:rest rdf:nodeID="Nf2b0c0b620984a7691e6705af522f981"/>
    <rdf:first rdf:resource="http://emmo.info/emmo/top/semiotics#EMMO_0cd58641_824c_4851_907f_f4c3be76630c"/>
  </rdf:Description>
  <rdf:Description rdf:about="http://emmo.info/emmo/middle/materials#EMMO_a2b006f2_bbfd_4dba_bcaa_3fca20cd6be1">
    <rdf:type rdf:resource="http://www.w3.org/2002/07/owl#Class"/>
    <annotations:EMMO_967080e5_2f42_4eb2_a3a9_c58143e835f9>A continuum characterized by structural rigidity and resistance to changes of shape or volume, that retains its shape and density when not confined.</annotations:EMMO_967080e5_2f42_4eb2_a3a9_c58143e835f9>
    <rdfs:subClassOf rdf:resource="http://emmo.info/emmo/middle/materials#EMMO_8b0923ab_b500_477b_9ce9_8b3a3e4dc4f2"/>
    <rdfs:label xml:lang="en">Solid</rdfs:label>
  </rdf:Description>
  <rdf:Description rdf:about="http://emmo.info/emmo/middle/models#EMMO_22522299_4091_4d1f_82a2_3890492df6db">
    <rdfs:label xml:lang="en">Experiment</rdfs:label>
    <rdfs:subClassOf rdf:resource="http://emmo.info/emmo/middle/properties#EMMO_10a5fd39_06aa_4648_9e70_f962a9cb2069"/>
    <annotations:EMMO_967080e5_2f42_4eb2_a3a9_c58143e835f9>An experiment is a process that is intended to replicate a physical phenomenon in a controlled environment.</annotations:EMMO_967080e5_2f42_4eb2_a3a9_c58143e835f9>
    <rdfs:subClassOf rdf:nodeID="N5f50899ee9144cedaf1ce63862644e44"/>
    <rdf:type rdf:resource="http://www.w3.org/2002/07/owl#Class"/>
  </rdf:Description>
  <rdf:Description rdf:about="http://emmo.info/emmo/top/physical#EMMO_7afbed84_7593_4a23_bd88_9d9c6b04e8f6">
    <annotations:EMMO_967080e5_2f42_4eb2_a3a9_c58143e835f9>A relation that isolate a proper part that covers the total spatial extension of a whole within a time interval.</annotations:EMMO_967080e5_2f42_4eb2_a3a9_c58143e835f9>
    <rdfs:subPropertyOf rdf:resource="http://emmo.info/emmo/top/mereotopology#EMMO_9380ab64_0363_4804_b13f_3a8a94119a76"/>
    <rdf:type rdf:resource="http://www.w3.org/2002/07/owl#ObjectProperty"/>
    <rdfs:domain rdf:resource="http://emmo.info/emmo/top/mereotopology#EMMO_eb3a768e_d53e_4be9_a23b_0714833c36de"/>
    <rdf:type rdf:resource="http://www.w3.org/2002/07/owl#TransitiveProperty"/>
    <rdfs:label xml:lang="en">hasTemporalPart</rdfs:label>
    <rdfs:range rdf:resource="http://emmo.info/emmo/top/mereotopology#EMMO_eb3a768e_d53e_4be9_a23b_0714833c36de"/>
  </rdf:Description>
  <rdf:Description rdf:about="http://emmo.info/emmo/middle/isq#EMMO_1604f495_328a_4f28_9962_f4cc210739dd">
    <rdf:type rdf:resource="http://www.w3.org/2002/07/owl#Class"/>
    <rdfs:subClassOf rdf:nodeID="Na69d7a721f924256881228614b987701"/>
    <annotations:EMMO_fe015383_afb3_44a6_ae86_043628697aa2>https://doi.org/10.1351/goldbook.E01923</annotations:EMMO_fe015383_afb3_44a6_ae86_043628697aa2>
    <annotations:EMMO_21ae69b4_235e_479d_8dd8_4f756f694c1b>Charge</annotations:EMMO_21ae69b4_235e_479d_8dd8_4f756f694c1b>
    <annotations:EMMO_967080e5_2f42_4eb2_a3a9_c58143e835f9>The physical property of matter that causes it to experience a force when placed in an electromagnetic field.</annotations:EMMO_967080e5_2f42_4eb2_a3a9_c58143e835f9>
    <annotations:EMMO_6dd685dd_1895_46e4_b227_be9f7d643c25>http://dbpedia.org/page/Electric_charge</annotations:EMMO_6dd685dd_1895_46e4_b227_be9f7d643c25>
    <rdfs:label xml:lang="en">ElectricCharge</rdfs:label>
    <rdfs:subClassOf rdf:resource="http://emmo.info/emmo/middle/isq#EMMO_2946d40b_24a1_47fa_8176_e3f79bb45064"/>
  </rdf:Description>
  <rdf:Description rdf:nodeID="N2b6ff0bf8f9f4473ae4fa0048f26c08e">
    <rdf:type rdf:resource="http://www.w3.org/2002/07/owl#Restriction"/>
    <owl:hasValue rdf:datatype="http://www.w3.org/2001/XMLSchema#decimal">0.01</owl:hasValue>
    <owl:onProperty rdf:resource="http://emmo.info/emmo/middle/math#EMMO_faf79f53_749d_40b2_807c_d34244c192f4"/>
  </rdf:Description>
  <rdf:Description rdf:about="http://emmo.info/emmo/middle/metrology#EMMO_f658c301_ce93_46cf_9639_4eace2c5d1d5">
    <rdfs:subClassOf rdf:nodeID="N350972ab9c7d475b90d6c52413ceca1c"/>
    <rdfs:comment>Referred as Quantity Value in International vocabulary of metrology (VIM)</rdfs:comment>
    <rdfs:comment>A quantity is not necessarily a property, since it is possible to write "10 kg", without assigning this quantity to a specific object.

However, a quantitative property is always a quantity.</rdfs:comment>
    <rdfs:subClassOf rdf:nodeID="N418e7661e57a442c9ff782b14633557a"/>
    <annotations:EMMO_967080e5_2f42_4eb2_a3a9_c58143e835f9>A symbolic that has parts a reference unit and a numerical object separated by a space expressing the value of a quantitative property (expressed as the product of the numerical and the unit).</annotations:EMMO_967080e5_2f42_4eb2_a3a9_c58143e835f9>
    <annotations:EMMO_b432d2d5_25f4_4165_99c5_5935a7763c1a>6.8 m
0.9 km
8 K
6 MeV
43.5 HRC(150 kg)</annotations:EMMO_b432d2d5_25f4_4165_99c5_5935a7763c1a>
    <rdfs:label xml:lang="en">Quantity</rdfs:label>
    <rdfs:subClassOf rdf:resource="http://emmo.info/emmo/middle/metrology#EMMO_985bec21_989f_4b9e_a4b3_735d88099c3c"/>
    <owl:disjointUnionOf rdf:nodeID="Na3f60bb59b39470fac7fe3de46953a2d"/>
    <rdfs:comment>SI distinguishes between a quantity (an abstract concept) and the quantity value (a number and a reference). 

The EMMO, following strict nominalism, denies the existence of abstract objects and then collapses the two concepts of SI quantity and SI quantity value into a single one: the 'Quantity'.

So, for the EMMO the symbol "kg" is not a physical quantity but simply a 'Symbolic' object categorized as a 'MeasurementUnit'.

While the string "1 kg" is a 'Physical Quantity'.</rdfs:comment>
    <rdf:type rdf:resource="http://www.w3.org/2002/07/owl#Class"/>
  </rdf:Description>
  <rdf:Description rdf:nodeID="Ndea63cdcefe14a04bc2e81bd664f7f05">
    <rdf:type rdf:resource="http://www.w3.org/2002/07/owl#Restriction"/>
    <owl:onProperty rdf:resource="http://emmo.info/emmo/middle/reductionistic#EMMO_b2282816_b7a3_44c6_b2cb_3feff1ceb7fe"/>
    <owl:qualifiedCardinality rdf:datatype="http://www.w3.org/2001/XMLSchema#nonNegativeInteger">1</owl:qualifiedCardinality>
    <owl:onClass rdf:resource="http://emmo.info/emmo/middle/siunits#EMMO_32129fb5_df25_48fd_a29c_18a2f22a2dd5"/>
  </rdf:Description>
  <rdf:Description rdf:nodeID="N8228ee2a1c7044afa7ada85142123fc3">
    <owl:onProperty rdf:resource="http://emmo.info/emmo/middle/perceptual#EMMO_23b579e1_8088_45b5_9975_064014026c42"/>
    <owl:hasValue>Y</owl:hasValue>
    <rdf:type rdf:resource="http://www.w3.org/2002/07/owl#Restriction"/>
  </rdf:Description>
  <rdf:Description rdf:about="http://emmo.info/emmo/middle/isq#EMMO_09b9021b_f97b_43eb_b83d_0a764b472bc2">
    <rdfs:subClassOf rdf:resource="http://emmo.info/emmo/middle/isq#EMMO_2946d40b_24a1_47fa_8176_e3f79bb45064"/>
    <rdfs:subClassOf rdf:nodeID="N222e5af2f44e4d74af40a3d2ebb081c9"/>
    <annotations:EMMO_967080e5_2f42_4eb2_a3a9_c58143e835f9>Rate of transfer of energy per unit time.</annotations:EMMO_967080e5_2f42_4eb2_a3a9_c58143e835f9>
    <annotations:EMMO_6dd685dd_1895_46e4_b227_be9f7d643c25>http://dbpedia.org/page/Power_(physics)</annotations:EMMO_6dd685dd_1895_46e4_b227_be9f7d643c25>
    <rdf:type rdf:resource="http://www.w3.org/2002/07/owl#Class"/>
    <rdfs:label xml:lang="en">Power</rdfs:label>
    <annotations:EMMO_fe015383_afb3_44a6_ae86_043628697aa2>https://doi.org/10.1351/goldbook.P04792</annotations:EMMO_fe015383_afb3_44a6_ae86_043628697aa2>
  </rdf:Description>
  <rdf:Description rdf:nodeID="Nae464b1384694e5bbe2d6cd25525f893">
    <owl:inverseOf rdf:resource="http://emmo.info/emmo/middle/math#EMMO_3446e167_c576_49d6_846c_215bb8878a55"/>
  </rdf:Description>
  <rdf:Description rdf:about="http://emmo.info/emmo/middle/isq#EMMO_d4f7d378_5e3b_468a_baa1_a7e98358cda7">
    <annotations:EMMO_6dd685dd_1895_46e4_b227_be9f7d643c25>http://dbpedia.org/page/Time</annotations:EMMO_6dd685dd_1895_46e4_b227_be9f7d643c25>
    <annotations:EMMO_967080e5_2f42_4eb2_a3a9_c58143e835f9>The indefinite continued progress of existence and events that occur in apparently irreversible succession from the past through the present to the future.</annotations:EMMO_967080e5_2f42_4eb2_a3a9_c58143e835f9>
    <annotations:EMMO_fe015383_afb3_44a6_ae86_043628697aa2>https://doi.org/10.1351/goldbook.T06375</annotations:EMMO_fe015383_afb3_44a6_ae86_043628697aa2>
    <rdfs:label xml:lang="en">Time</rdfs:label>
    <rdfs:subClassOf rdf:nodeID="N6e06fe59ef8d46ab9ee33535e68ab190"/>
    <rdf:type rdf:resource="http://www.w3.org/2002/07/owl#Class"/>
  </rdf:Description>
  <rdf:Description rdf:about="http://emmo.info/emmo/middle/math#EMMO_18d180e4_5e3e_42f7_820c_e08951223486">
    <owl:equivalentClass rdf:nodeID="Nc062f361c16b44f1b3f1aa612c2c0285"/>
    <rdfs:label xml:lang="en">Real</rdfs:label>
    <rdfs:subClassOf rdf:resource="http://emmo.info/emmo/middle/math#EMMO_21f56795_ee72_4858_b571_11cfaa59c1a8"/>
    <rdfs:subClassOf rdf:nodeID="N3e9603d50f954b5c909f54b501890555"/>
    <rdf:type rdf:resource="http://www.w3.org/2002/07/owl#Class"/>
    <rdfs:subClassOf rdf:nodeID="Nb2af1735e9ef4376b8a35234c9e20cc8"/>
  </rdf:Description>
  <rdf:Description rdf:about="http://emmo.info/emmo/middle/perceptual#EMMO_91756568_8655_4060_8937_a1a906dad8c1">
    <rdfs:label xml:lang="en">Noise</rdfs:label>
    <rdf:type rdf:resource="http://www.w3.org/2002/07/owl#Class"/>
    <rdfs:subClassOf rdf:resource="http://emmo.info/emmo/middle/perceptual#EMMO_4b3afb22_27cf_4ce3_88bc_492bfccb546b"/>
  </rdf:Description>
  <rdf:Description rdf:about="http://emmo.info/emmo/top/mereotopology#EMMO_6b7276a4_4b9d_440a_b577_0277539c0fc4">
    <rdfs:range rdf:resource="http://emmo.info/emmo/top/mereotopology#EMMO_eb3a768e_d53e_4be9_a23b_0714833c36de"/>
    <rdfs:subPropertyOf rdf:resource="http://emmo.info/emmo/top/mereotopology#EMMO_9380ab64_0363_4804_b13f_3a8a94119a76"/>
    <rdfs:domain rdf:resource="http://emmo.info/emmo/top/mereotopology#EMMO_2d2ecd97_067f_4d0e_950c_d746b7700a31"/>
    <rdf:type rdf:resource="http://www.w3.org/2002/07/owl#AsymmetricProperty"/>
    <rdf:type rdf:resource="http://www.w3.org/2002/07/owl#IrreflexiveProperty"/>
    <rdf:type rdf:resource="http://www.w3.org/2002/07/owl#ObjectProperty"/>
    <rdfs:label xml:lang="en">hasMember</rdfs:label>
  </rdf:Description>
  <rdf:Description rdf:nodeID="N6e06fe59ef8d46ab9ee33535e68ab190">
    <rdf:type rdf:resource="http://www.w3.org/2002/07/owl#Restriction"/>
    <owl:onProperty rdf:resource="http://emmo.info/emmo/middle/metrology#EMMO_67fc0a36_8dcb_4ffa_9a43_31074efa3296"/>
    <owl:allValuesFrom rdf:nodeID="N4597b6cf975e44f59a5858d894b65479"/>
  </rdf:Description>
  <rdf:Description rdf:about="http://emmo.info/emmo/top">
    <annotations:EMMO_5525a055_dda5_4556_8b91_f0d22fa676cc>EMMO is released under a Creative Commons license Attribution 4.0 International (CC BY 4.0)

https://creativecommons.org/licenses/by/4.0/legalcode</annotations:EMMO_5525a055_dda5_4556_8b91_f0d22fa676cc>
    <owl:versionInfo>The European Materials Modelling Ontology

Version 1.0.0-alpha</owl:versionInfo>
    <rdfs:comment xml:lang="en">Contacts:
Gerhard Goldbeck
Goldbeck Consulting Ltd (UK)
email: gerhard@goldbeck-consulting.com

Emanuele Ghedini
University of Bologna (IT)
email: emanuele.ghedini@unibo.it</rdfs:comment>
    <rdf:type rdf:resource="http://www.w3.org/2002/07/owl#Ontology"/>
    <annotations:EMMO_cd5fb112_7ee7_4120_a35d_3ca3e6c3f4ab>Emanuele Ghedini (University of Bologna, IT)
Gerhard Goldbeck (GCL Ltd, UK)
Adham Hashibon (Fraunhofer IWM, DE)
Georg Schmitz (Access, DE)
Jesper Friis (SINTEF, NO)</annotations:EMMO_cd5fb112_7ee7_4120_a35d_3ca3e6c3f4ab>
    <owl:versionIRI rdf:resource="http://emmo.info/emmo/1.0.0-alpha/top"/>
    <rdfs:comment>The EMMO requires FacT++ reasoner plugin in order to visualize all inferences and class hierarchy (ctrl+R hotkey in Protege).</rdfs:comment>
    <rdfs:comment>European Materials and Modelling Ontology (EMMO)

EMMO is a multidisciplinary effort to develop a standard representational framework (the ontology) based on current materials modelling knowledge, including physical sciences, analytical philosophy and information and communication technologies. 

It provides the connection between the physical world, materials characterisation world and materials modelling world.</rdfs:comment>
  </rdf:Description>
  <rdf:Description rdf:about="http://emmo.info/emmo/middle/reductionistic#EMMO_b2282816_b7a3_44c6_b2cb_3feff1ceb7fe">
    <rdfs:label xml:lang="en">hasSpatialDirectPart</rdfs:label>
    <rdf:type rdf:resource="http://www.w3.org/2002/07/owl#IrreflexiveProperty"/>
    <rdf:type rdf:resource="http://www.w3.org/2002/07/owl#AsymmetricProperty"/>
    <rdf:type rdf:resource="http://www.w3.org/2002/07/owl#ObjectProperty"/>
    <rdfs:subPropertyOf rdf:resource="http://emmo.info/emmo/top/physical#EMMO_f68030be_94b8_4c61_a161_886468558054"/>
    <rdf:type rdf:resource="http://www.w3.org/2002/07/owl#InverseFunctionalProperty"/>
    <rdfs:domain rdf:resource="http://emmo.info/emmo/middle/reductionistic#EMMO_36c79456_e29c_400d_8bd3_0eedddb82652"/>
  </rdf:Description>
  <rdf:Description rdf:about="http://emmo.info/emmo/middle/siunits#EMMO_58a650f0_a638_4743_8439_535a325e5c4c">
    <rdfs:comment>The DBpedia definition (http://dbpedia.org/page/Elementary_charge) is outdated as May 20, 2019. It is now an exact quantity.</rdfs:comment>
    <rdfs:subClassOf rdf:resource="http://emmo.info/emmo/middle/isq#EMMO_1604f495_328a_4f28_9962_f4cc210739dd"/>
    <rdf:type rdf:resource="http://www.w3.org/2002/07/owl#Class"/>
    <annotations:EMMO_fe015383_afb3_44a6_ae86_043628697aa2>https://doi.org/10.1351/goldbook.E02032</annotations:EMMO_fe015383_afb3_44a6_ae86_043628697aa2>
    <rdfs:label xml:lang="en">ElementaryCharge</rdfs:label>
    <annotations:EMMO_6dd685dd_1895_46e4_b227_be9f7d643c25>http://dbpedia.org/page/Elementary_charge</annotations:EMMO_6dd685dd_1895_46e4_b227_be9f7d643c25>
    <annotations:EMMO_967080e5_2f42_4eb2_a3a9_c58143e835f9>The magnitude of the electric charge carried by a single electron.</annotations:EMMO_967080e5_2f42_4eb2_a3a9_c58143e835f9>
    <annotations:EMMO_1f1b164d_ec6a_4faa_8d5e_88bda62316cc>http://physics.nist.gov/cuu/CODATA-Value_ElementaryCharge</annotations:EMMO_1f1b164d_ec6a_4faa_8d5e_88bda62316cc>
  </rdf:Description>
  <rdf:Description rdf:nodeID="Na001c9b2a1734a6790db02629f49795c">
    <owl:someValuesFrom rdf:resource="http://emmo.info/emmo/middle/materials#EMMO_f835f4d4_c665_403d_ab25_dca5cc74be52"/>
    <rdf:type rdf:resource="http://www.w3.org/2002/07/owl#Restriction"/>
    <owl:onProperty rdf:resource="http://emmo.info/emmo/middle/reductionistic#EMMO_b2282816_b7a3_44c6_b2cb_3feff1ceb7fe"/>
  </rdf:Description>
  <rdf:Description rdf:about="http://emmo.info/emmo/middle/siunits#EMMO_f2ca6dd0_0e5f_4392_a92d_cafdae6cfc95">
    <owl:disjointUnionOf rdf:nodeID="Nf2827a71babf4830accc67667c17db0a"/>
    <annotations:EMMO_967080e5_2f42_4eb2_a3a9_c58143e835f9>Physical constant that by definition (after the latest revision of the SI system that was enforsed May 2019) has a known exact numerical value when expressed in SI units.</annotations:EMMO_967080e5_2f42_4eb2_a3a9_c58143e835f9>
    <rdfs:subClassOf rdf:resource="http://emmo.info/emmo/middle/metrology#EMMO_89762966_8076_4f7c_b745_f718d653e8e2"/>
    <rdf:type rdf:resource="http://www.w3.org/2002/07/owl#Class"/>
    <rdfs:label xml:lang="en">SIExactConstant</rdfs:label>
  </rdf:Description>
  <rdf:Description rdf:about="http://emmo.info/emmo/middle/reductionistic#EMMO_65a2c5b8_e4d8_4a51_b2f8_e55effc0547d">
    <rdfs:label xml:lang="en">hasTemporalDirectPart</rdfs:label>
    <rdfs:range rdf:resource="http://emmo.info/emmo/middle/reductionistic#EMMO_36c79456_e29c_400d_8bd3_0eedddb82652"/>
    <rdfs:domain rdf:resource="http://emmo.info/emmo/middle/reductionistic#EMMO_52211e5e_d767_4812_845e_eb6b402c476a"/>
    <rdf:type rdf:resource="http://www.w3.org/2002/07/owl#InverseFunctionalProperty"/>
    <rdfs:subPropertyOf rdf:resource="http://emmo.info/emmo/top/physical#EMMO_7afbed84_7593_4a23_bd88_9d9c6b04e8f6"/>
    <rdf:type rdf:resource="http://www.w3.org/2002/07/owl#AsymmetricProperty"/>
    <rdf:type rdf:resource="http://www.w3.org/2002/07/owl#IrreflexiveProperty"/>
    <rdf:type rdf:resource="http://www.w3.org/2002/07/owl#ObjectProperty"/>
  </rdf:Description>
  <rdf:Description rdf:nodeID="N2db0feed6510454e82a1b1e38e33019f">
    <rdf:rest rdf:nodeID="N304074c25c334c0380d380ef9551e3d7"/>
    <rdf:first rdf:resource="http://emmo.info/emmo/middle/properties#EMMO_873b0ab3_88e6_4054_b901_5531e01f14a4"/>
  </rdf:Description>
  <rdf:Description rdf:nodeID="N67ec8590149b41faa83da784ca10fa22">
    <owl:onProperty rdf:resource="http://emmo.info/emmo/middle/perceptual#EMMO_23b579e1_8088_45b5_9975_064014026c42"/>
    <rdf:type rdf:resource="http://www.w3.org/2002/07/owl#Restriction"/>
    <owl:hasValue>T+4 L-2 M-1 I+2 Θ0 N0 J0</owl:hasValue>
  </rdf:Description>
  <rdf:Description rdf:about="http://emmo.info/emmo/middle/isq">
    <owl:versionIRI rdf:resource="http://emmo.info/emmo/1.0.0-alpha/middle/isq"/>
    <rdf:type rdf:resource="http://www.w3.org/2002/07/owl#Ontology"/>
    <annotations:EMMO_cd5fb112_7ee7_4120_a35d_3ca3e6c3f4ab>Emanuele Ghedini (University of Bologna, IT)
Gerhard Goldbeck (GCL Ltd, UK)
Adham Hashibon (Fraunhofer IWM, DE)
Georg Schmitz (Access, DE)
Jesper Friis (SINTEF, NO)</annotations:EMMO_cd5fb112_7ee7_4120_a35d_3ca3e6c3f4ab>
    <annotations:EMMO_5525a055_dda5_4556_8b91_f0d22fa676cc>EMMO is released under a Creative Commons license Attribution 4.0 International (CC BY 4.0)

https://creativecommons.org/licenses/by/4.0/legalcode</annotations:EMMO_5525a055_dda5_4556_8b91_f0d22fa676cc>
    <rdfs:comment xml:lang="en">Contacts:
Gerhard Goldbeck
Goldbeck Consulting Ltd (UK)
email: gerhard@goldbeck-consulting.com

Emanuele Ghedini
University of Bologna (IT)
email: emanuele.ghedini@unibo.it</rdfs:comment>
    <rdfs:comment>The EMMO requires FacT++ reasoner plugin in order to visualize all inferences and class hierarchy (ctrl+R hotkey in Protege).</rdfs:comment>
    <rdfs:comment>European Materials and Modelling Ontology (EMMO)

EMMO is a multidisciplinary effort to develop a standard representational framework (the ontology) based on current materials modelling knowledge, including physical sciences, analytical philosophy and information and communication technologies.

It provides the connection between the physical world, materials characterisation world and materials modelling world.</rdfs:comment>
  </rdf:Description>
  <rdf:Description rdf:about="http://emmo.info/emmo/middle/properties">
    <rdfs:comment>The EMMO requires FacT++ reasoner plugin in order to visualize all inferences and class hierarchy (ctrl+R hotkey in Protege).</rdfs:comment>
    <annotations:EMMO_cd5fb112_7ee7_4120_a35d_3ca3e6c3f4ab>Emanuele Ghedini (University of Bologna, IT)
Gerhard Goldbeck (GCL Ltd, UK)
Adham Hashibon (Fraunhofer IWM, DE)
Georg Schmitz (Access, DE)
Jesper Friis (SINTEF, NO)</annotations:EMMO_cd5fb112_7ee7_4120_a35d_3ca3e6c3f4ab>
    <rdfs:comment xml:lang="en">Contacts:
Gerhard Goldbeck
Goldbeck Consulting Ltd (UK)
email: gerhard@goldbeck-consulting.com

Emanuele Ghedini
University of Bologna (IT)
email: emanuele.ghedini@unibo.it</rdfs:comment>
    <owl:versionInfo>The European Materials Modelling Ontology

Version 1.0.0-alpha</owl:versionInfo>
    <rdf:type rdf:resource="http://www.w3.org/2002/07/owl#Ontology"/>
    <rdfs:comment>European Materials and Modelling Ontology (EMMO)

EMMO is a multidisciplinary effort to develop a standard representational framework (the ontology) based on current materials modelling knowledge, including physical sciences, analytical philosophy and information and communication technologies. 

It provides the connection between the physical world, materials characterisation world and materials modelling world.</rdfs:comment>
    <annotations:EMMO_5525a055_dda5_4556_8b91_f0d22fa676cc>EMMO is released under a Creative Commons license Attribution 4.0 International (CC BY 4.0)

https://creativecommons.org/licenses/by/4.0/legalcode</annotations:EMMO_5525a055_dda5_4556_8b91_f0d22fa676cc>
    <owl:versionIRI rdf:resource="http://emmo.info/emmo/1.0.0-alpha/middle/properties"/>
  </rdf:Description>
  <rdf:Description rdf:about="http://emmo.info/emmo/middle/siunits#EMMO_8d00f093_3f45_4ea3_986c_b3545c3c2f4c">
    <annotations:EMMO_70fe84ff_99b6_4206_a9fc_9a8931836d84>The candela, symbol cd, is the SI unit of luminous intensity in a given direction. It is defined by taking the fixed numerical value of the luminous efficacy of monochromatic radiation of frequency 540×1012 Hz, Kcd, to be 683 when expressed in the unit lm W−1, which is equal to cd sr W−1, or cd sr kg−1 m−2 s3, where the kilogram, metre and second are defined in terms of h, c and ∆νCs.</annotations:EMMO_70fe84ff_99b6_4206_a9fc_9a8931836d84>
    <rdf:type rdf:resource="http://www.w3.org/2002/07/owl#Class"/>
    <annotations:EMMO_1f1b164d_ec6a_4faa_8d5e_88bda62316cc>http://qudt.org/vocab/unit/CD</annotations:EMMO_1f1b164d_ec6a_4faa_8d5e_88bda62316cc>
    <rdfs:label xml:lang="en">Candela</rdfs:label>
    <rdfs:subClassOf rdf:nodeID="Nf0102c1af1a94fb3b938a7c4c09bdda1"/>
    <annotations:EMMO_fe015383_afb3_44a6_ae86_043628697aa2>https://doi.org/10.1351/goldbook.C00787</annotations:EMMO_fe015383_afb3_44a6_ae86_043628697aa2>
    <rdfs:subClassOf rdf:nodeID="Nb8059d442eac4bb48921cdca102ee61e"/>
  </rdf:Description>
  <rdf:Description rdf:nodeID="Nb2a04350627c45a5b4db29eefc58c99d">
    <rdf:rest rdf:nodeID="Nd3c2b89fc9c74e38a4f67fc47ba11ba2"/>
    <rdf:first rdf:resource="http://emmo.info/emmo/middle/metrology#EMMO_71f6ab56_342c_484b_bbe0_de86b7367cb3"/>
  </rdf:Description>
  <rdf:Description rdf:nodeID="Nf0102c1af1a94fb3b938a7c4c09bdda1">
    <rdf:type rdf:resource="http://www.w3.org/2002/07/owl#Restriction"/>
    <owl:hasValue>cd</owl:hasValue>
    <owl:onProperty rdf:resource="http://emmo.info/emmo/middle/perceptual#EMMO_23b579e1_8088_45b5_9975_064014026c42"/>
  </rdf:Description>
  <rdf:Description rdf:nodeID="N17e149a542d0430e977bccd7eb7a3b4f">
    <rdf:type rdf:resource="http://www.w3.org/2002/07/owl#Restriction"/>
    <owl:onProperty rdf:resource="http://emmo.info/emmo/middle/reductionistic#EMMO_b2282816_b7a3_44c6_b2cb_3feff1ceb7fe"/>
    <owl:someValuesFrom rdf:resource="http://emmo.info/emmo/middle/materials#EMMO_50781fd9_a9e4_46ad_b7be_4500371d188d"/>
  </rdf:Description>
  <rdf:Description rdf:about="http://emmo.info/emmo/middle/models#EMMO_314d0bd5_67ed_437e_a609_36d46147cea7">
    <rdfs:comment>While every 'process' in the EMMO involves physical objects, this class is devoted to represent real world objects that express a phenomena relevant for the ontologist.</rdfs:comment>
    <rdf:type rdf:resource="http://www.w3.org/2002/07/owl#Class"/>
    <rdfs:subClassOf rdf:resource="http://emmo.info/emmo/middle/holistic#EMMO_43e9a05d_98af_41b4_92f6_00f79a09bfce"/>
    <rdfs:label xml:lang="en">PhysicalPhenomenon</rdfs:label>
    <annotations:EMMO_967080e5_2f42_4eb2_a3a9_c58143e835f9>A 'process' that is recognized by physical sciences and is catogrized accordingly.</annotations:EMMO_967080e5_2f42_4eb2_a3a9_c58143e835f9>
  </rdf:Description>
  <rdf:Description rdf:about="http://emmo.info/emmo/top/mereotopology#EMMO_6703954e_34c4_4a15_a9e7_f313760ae1a8">
    <rdfs:label xml:lang="en">connected</rdfs:label>
    <rdf:type rdf:resource="http://www.w3.org/2002/07/owl#ObjectProperty"/>
    <rdf:type rdf:resource="http://www.w3.org/2002/07/owl#SymmetricProperty"/>
    <rdfs:comment>Items being connected means that there is a topological contact or "interaction" between them.</rdfs:comment>
    <rdfs:comment>Causality is a topological property between connected items.</rdfs:comment>
    <rdfs:subPropertyOf rdf:resource="http://emmo.info/emmo/top/mereotopology#EMMO_03212fd7_abfd_4828_9c8e_62c293052d4b"/>
  </rdf:Description>
  <rdf:Description rdf:nodeID="N18764fea94c541c1a411169f3c7cdf44">
    <rdf:type rdf:resource="http://www.w3.org/2002/07/owl#Restriction"/>
    <owl:onProperty rdf:resource="http://emmo.info/emmo/middle/metrology#EMMO_bed1d005_b04e_4a90_94cf_02bc678a8569"/>
    <owl:allValuesFrom rdf:resource="http://emmo.info/emmo/middle/isq#EMMO_77e9dc31_5b19_463e_b000_44c6e79f98aa"/>
  </rdf:Description>
  <rdf:Description rdf:nodeID="Nf9543181733a48cb80b16c34a902f1c2">
    <owl:allValuesFrom rdf:nodeID="N2d3c2791a50343bf946e099971f6aab6"/>
    <rdf:type rdf:resource="http://www.w3.org/2002/07/owl#Restriction"/>
    <owl:onProperty rdf:nodeID="N37bc04a1a37044d08f4fe35e3c69279f"/>
  </rdf:Description>
  <rdf:Description rdf:nodeID="N793139cd06954ec39efb49901c758a1b">
    <rdf:type rdf:resource="http://www.w3.org/2002/07/owl#Restriction"/>
    <owl:hasValue>T-2 L+2 M0 I0 Θ0 N0 J0</owl:hasValue>
    <owl:onProperty rdf:resource="http://emmo.info/emmo/middle/perceptual#EMMO_23b579e1_8088_45b5_9975_064014026c42"/>
  </rdf:Description>
  <rdf:Description rdf:nodeID="N20ec5135479b44859752f926614bf2e7">
    <rdf:type rdf:resource="http://www.w3.org/2002/07/owl#Restriction"/>
    <owl:hasValue>J</owl:hasValue>
    <owl:onProperty rdf:resource="http://emmo.info/emmo/middle/perceptual#EMMO_23b579e1_8088_45b5_9975_064014026c42"/>
  </rdf:Description>
  <rdf:Description rdf:about="http://emmo.info/emmo/middle/materials#EMMO_8303a247_f9d9_4616_bdcd_f5cbd7b298e3">
    <annotations:EMMO_967080e5_2f42_4eb2_a3a9_c58143e835f9>An bonded atom that shares at least one electron to the atom-based entity of which is part of.</annotations:EMMO_967080e5_2f42_4eb2_a3a9_c58143e835f9>
    <rdfs:subClassOf rdf:resource="http://emmo.info/emmo/middle/materials#EMMO_eb77076b_a104_42ac_a065_798b2d2809ad"/>
    <rdfs:label xml:lang="en">BondedAtom</rdfs:label>
    <rdfs:comment>A real bond between atoms is always something hybrid between covalent, metallic and ionic.

In general, metallic and ionic bonds have atoms sharing electrons.</rdfs:comment>
    <rdf:type rdf:resource="http://www.w3.org/2002/07/owl#Class"/>
    <rdfs:comment>This class can be used to represent molecules as simplified quantum systems, in which outer molecule shared electrons are un-entangled with the inner shells of the atoms composing the molecule.</rdfs:comment>
    <rdfs:comment>The bond types that are covered by this definition are the strong electonic bonds: covalent, metallic and ionic.</rdfs:comment>
  </rdf:Description>
  <rdf:Description rdf:nodeID="Ncf7e356028e249ffbb828d30f5d5455f">
    <owl:hasValue>da</owl:hasValue>
    <rdf:type rdf:resource="http://www.w3.org/2002/07/owl#Restriction"/>
    <owl:onProperty rdf:resource="http://emmo.info/emmo/middle/perceptual#EMMO_23b579e1_8088_45b5_9975_064014026c42"/>
  </rdf:Description>
  <rdf:Description rdf:about="http://emmo.info/emmo/middle/metrology">
    <annotations:EMMO_cd5fb112_7ee7_4120_a35d_3ca3e6c3f4ab>Emanuele Ghedini (University of Bologna, IT)
Gerhard Goldbeck (GCL Ltd, UK)
Adham Hashibon (Fraunhofer IWM, DE)
Georg Schmitz (Access, DE)
Jesper Friis (SINTEF, NO)</annotations:EMMO_cd5fb112_7ee7_4120_a35d_3ca3e6c3f4ab>
    <annotations:EMMO_5525a055_dda5_4556_8b91_f0d22fa676cc>EMMO is released under a Creative Commons license Attribution 4.0 International (CC BY 4.0)

https://creativecommons.org/licenses/by/4.0/legalcode</annotations:EMMO_5525a055_dda5_4556_8b91_f0d22fa676cc>
    <rdfs:comment>European Materials and Modelling Ontology (EMMO)

EMMO is a multidisciplinary effort to develop a standard representational framework (the ontology) based on current materials modelling knowledge, including physical sciences, analytical philosophy and information and communication technologies.

It provides the connection between the physical world, materials characterisation world and materials modelling world.</rdfs:comment>
    <rdfs:comment>The EMMO requires FacT++ reasoner plugin in order to visualize all inferences and class hierarchy (ctrl+R hotkey in Protege).</rdfs:comment>
    <owl:versionIRI rdf:resource="http://emmo.info/emmo/1.0.0-alpha/middle/metrology"/>
    <rdfs:comment xml:lang="en">Contacts:
Gerhard Goldbeck
Goldbeck Consulting Ltd (UK)
email: gerhard@goldbeck-consulting.com

Emanuele Ghedini
University of Bologna (IT)
email: emanuele.ghedini@unibo.it</rdfs:comment>
    <rdf:type rdf:resource="http://www.w3.org/2002/07/owl#Ontology"/>
  </rdf:Description>
  <rdf:Description rdf:about="http://emmo.info/emmo/top/math#EMMO_29afdf54_90ae_4c98_8845_fa9ea3f143a8">
    <annotations:EMMO_967080e5_2f42_4eb2_a3a9_c58143e835f9>An equation that define a new variable in terms of other mathematical entities.</annotations:EMMO_967080e5_2f42_4eb2_a3a9_c58143e835f9>
    <rdf:type rdf:resource="http://www.w3.org/2002/07/owl#Class"/>
    <rdfs:label xml:lang="en">DefiningEquation</rdfs:label>
    <rdfs:subClassOf rdf:resource="http://emmo.info/emmo/middle/math#EMMO_e56ee3eb_7609_4ae1_8bed_51974f0960a6"/>
    <annotations:EMMO_b432d2d5_25f4_4165_99c5_5935a7763c1a>The definition of velocity as v = dx/dt.

The definition of density as mass/volume.

y = f(x)</annotations:EMMO_b432d2d5_25f4_4165_99c5_5935a7763c1a>
  </rdf:Description>
  <rdf:Description rdf:nodeID="Nb2f58bc99e874d7db3d015349db25510">
    <owl:onProperty rdf:resource="http://emmo.info/emmo/middle/perceptual#EMMO_23b579e1_8088_45b5_9975_064014026c42"/>
    <owl:hasValue>T0 L0 M+1 I0 Θ0 N0 J0</owl:hasValue>
    <rdf:type rdf:resource="http://www.w3.org/2002/07/owl#Restriction"/>
  </rdf:Description>
  <rdf:Description rdf:nodeID="N376fb71de0b04a2686fed3b806bdd315">
    <owl:onProperty rdf:resource="http://emmo.info/emmo/middle/metrology#EMMO_bed1d005_b04e_4a90_94cf_02bc678a8569"/>
    <rdf:type rdf:resource="http://www.w3.org/2002/07/owl#Restriction"/>
    <owl:someValuesFrom rdf:resource="http://emmo.info/emmo/middle/isq#EMMO_7610efb8_c7c6_4684_abc1_774783c62472"/>
  </rdf:Description>
  <rdf:Description rdf:about="http://emmo.info/emmo/middle/metrology#EMMO_985bec21_989f_4b9e_a4b3_735d88099c3c">
    <rdf:type rdf:resource="http://www.w3.org/2002/07/owl#Class"/>
    <rdfs:comment>This language domain makes use of ISO 80000 concepts.</rdfs:comment>
    <annotations:EMMO_967080e5_2f42_4eb2_a3a9_c58143e835f9>A symbolic object used in metrology.</annotations:EMMO_967080e5_2f42_4eb2_a3a9_c58143e835f9>
    <rdfs:label xml:lang="en">Metrological</rdfs:label>
    <rdfs:subClassOf rdf:resource="http://emmo.info/emmo/middle/perceptual#EMMO_d8d2144e_5c8d_455d_a643_5caf4d8d9df8"/>
  </rdf:Description>
  <rdf:Description rdf:about="http://emmo.info/emmo/middle/isq#EMMO_c8d084ad_f88e_4596_8e4d_982c6655ce6f">
    <rdf:type rdf:resource="http://www.w3.org/2002/07/owl#Class"/>
    <owl:equivalentClass rdf:nodeID="Nb53716dfe0334ecd9d068dcb19bef884"/>
    <rdfs:subClassOf rdf:resource="http://emmo.info/emmo/middle/metrology#EMMO_9895a1b4_f0a5_4167_ac5e_97db40b8bfcc"/>
    <rdfs:label xml:lang="en">MassSquareLengthPerCubicTimeDimension</rdfs:label>
  </rdf:Description>
  <rdf:Description rdf:about="http://emmo.info/emmo/middle/perceptual#EMMO_649bf97b_4397_4005_90d9_219755d92e34">
    <rdfs:label xml:lang="en">Perceptual</rdfs:label>
    <annotations:EMMO_967080e5_2f42_4eb2_a3a9_c58143e835f9>A 'Physical' which stands for a real world object that can stimulate a perception (e.g. a mental impression, the excitation of a sensor) to an interpreter (human or non-human).</annotations:EMMO_967080e5_2f42_4eb2_a3a9_c58143e835f9>
    <rdfs:comment>This class is the most general superclass for the categorization of real world objects that are recognizable by an interpreter (agent).

A 'Perceptual' can stand for something else in a semiotic process (acting as sign or as object). 

However, a perceptual is not necessarily a 'Sign' (e.g. a line sketched on a blackboard is a recognizable 'Perceptual' but it may stand for nothing).</rdfs:comment>
    <annotations:EMMO_b432d2d5_25f4_4165_99c5_5935a7763c1a>The meta-semiotic process:
I see a cloud in the sky. Since I'm an EMMO ontologist, I create an individual named Cloud under the 'Impression' class.  This semiotic process occurs at meta-level: it's how I use the EMMO as tool for a direct representation of the world.

The semiotic process within EMMO:
My friend looks at the same cloud and says: "It is an elephant".
I use the EMMO to record this experience by declaring:
    - my friend as MyFriend individual, belonging to 'Interpreter' classes
    - the sound of the word "elephant" as an acoustical impression individual named ElephantWord, belonging to 'Impression'
    - a relation hasSign between Cloud and ElephantWord, that makes ElephantWord also belonging to 'Sign' class and Cloud belonging also to 'Object' class
    - a 'Semiosis' individual called MyFriendElephantCloud that hasParticipant: Cloud, ElephantWord and MyFriend, respectively as object, sign and interpreter.</annotations:EMMO_b432d2d5_25f4_4165_99c5_5935a7763c1a>
    <rdf:type rdf:resource="http://www.w3.org/2002/07/owl#Class"/>
    <annotations:EMMO_b432d2d5_25f4_4165_99c5_5935a7763c1a>A line scratched on a surface.
A sound.
A smell.
The word 'cat' and the sound of the word 'cat' (the first one is graphical and the second acoustical).</annotations:EMMO_b432d2d5_25f4_4165_99c5_5935a7763c1a>
    <rdfs:comment>A 'Perceptual' is a meta-object, meaning that is addressed by the ontologist (the meta-interpreter) in a meta-semiotic process occurring outside the EMMO.

A 'Perceptual' becomes an 'Object', when it is part of a 'Semiotic' process described by the ontologist through the EMMO.</rdfs:comment>
    <rdfs:comment>'Perceptual' includes real world objects that:
- are part of a communication system (e.g. words, speech, alphabets)
- are not part of a communication system, but can be identified and referred by an interpreter</rdfs:comment>
    <rdfs:subClassOf rdf:resource="http://emmo.info/emmo/top#EMMO_49267eba_5548_4163_8f36_518d65b583f9"/>
    <rdfs:comment>From Latin perceptiō (“a receiving or collecting, perception, comprehension”), from perceptus (“perceived, observed”).</rdfs:comment>
  </rdf:Description>
  <rdf:Description rdf:about="http://emmo.info/emmo/middle/models#EMMO_6eca09be_17e9_445e_abc9_000aa61b7a11">
    <rdfs:subClassOf rdf:resource="http://emmo.info/emmo/middle/models#EMMO_b29fd350_39aa_4af7_9459_3faa0544cba6"/>
    <annotations:EMMO_b432d2d5_25f4_4165_99c5_5935a7763c1a>Density functional theory.
Hartree-Fock.</annotations:EMMO_b432d2d5_25f4_4165_99c5_5935a7763c1a>
    <annotations:EMMO_967080e5_2f42_4eb2_a3a9_c58143e835f9>A physics-based model based on a physics equation describing the behaviour of electrons.</annotations:EMMO_967080e5_2f42_4eb2_a3a9_c58143e835f9>
    <rdfs:label xml:lang="en">ElectronicModel</rdfs:label>
    <rdf:type rdf:resource="http://www.w3.org/2002/07/owl#Class"/>
  </rdf:Description>
  <rdf:Description rdf:about="http://emmo.info/emmo/top/math#EMMO_535d75a4_1972_40bc_88c6_ca566386934f">
    <annotations:EMMO_967080e5_2f42_4eb2_a3a9_c58143e835f9>The equals symbol.</annotations:EMMO_967080e5_2f42_4eb2_a3a9_c58143e835f9>
    <rdfs:subClassOf rdf:resource="http://emmo.info/emmo/middle/perceptual#EMMO_a1083d0a_c1fb_471f_8e20_a98f881ad527"/>
    <rdfs:label xml:lang="en">Equals</rdfs:label>
    <rdfs:subClassOf rdf:resource="http://emmo.info/emmo/middle/math#EMMO_54ee6b5e_5261_44a8_86eb_5717e7fdb9d0"/>
    <rdf:type rdf:resource="http://www.w3.org/2002/07/owl#Class"/>
    <owl:equivalentClass rdf:nodeID="N99b7b86980dd41f5b42f9889381ca1c5"/>
  </rdf:Description>
  <rdf:Description rdf:about="http://emmo.info/emmo/middle/isq#EMMO_f3dd74c0_f480_49e8_9764_33b78638c235">
    <rdfs:subClassOf rdf:resource="http://emmo.info/emmo/middle/isq#EMMO_2946d40b_24a1_47fa_8176_e3f79bb45064"/>
    <annotations:EMMO_fe015383_afb3_44a6_ae86_043628697aa2>https://doi.org/10.1351/goldbook.A00346</annotations:EMMO_fe015383_afb3_44a6_ae86_043628697aa2>
    <annotations:EMMO_6dd685dd_1895_46e4_b227_be9f7d643c25>http://dbpedia.org/page/Angle</annotations:EMMO_6dd685dd_1895_46e4_b227_be9f7d643c25>
    <annotations:EMMO_70fe84ff_99b6_4206_a9fc_9a8931836d84>Ratio of circular arc length to radius.</annotations:EMMO_70fe84ff_99b6_4206_a9fc_9a8931836d84>
    <rdfs:subClassOf rdf:nodeID="Nc314b20232ae4c63b3e2a0aae1dfa449"/>
    <rdf:type rdf:resource="http://www.w3.org/2002/07/owl#Class"/>
    <rdfs:label xml:lang="en">Angle</rdfs:label>
  </rdf:Description>
  <rdf:Description rdf:nodeID="N6577c2fabff74f6eb026a67a4ed52307">
    <owl:onProperty rdf:resource="http://emmo.info/emmo/middle/reductionistic#EMMO_65a2c5b8_e4d8_4a51_b2f8_e55effc0547d"/>
    <owl:allValuesFrom rdf:resource="http://emmo.info/emmo/middle/reductionistic#EMMO_36c79456_e29c_400d_8bd3_0eedddb82652"/>
    <rdf:type rdf:resource="http://www.w3.org/2002/07/owl#Restriction"/>
  </rdf:Description>
  <rdf:Description rdf:about="http://emmo.info/emmo/top/physical#EMMO_c5ddfdba_c074_4aa4_ad6b_1ac4942d300d">
    <rdf:type rdf:resource="http://www.w3.org/2002/07/owl#Class"/>
    <rdfs:comment>The EMMO can be used to represent real world entities as 'Physical'-s that are easy to connect to classical or quantum mechanical based models.

Classical mechanics poses no representational issues, for the EMMO: the 4D representation of 'Physical'-s is consistent with classical physics systems.

However, the representation of 'Physical'-s that are typically analized through quantum mechanics (e.g. molecules, atoms, clusters), is not straightforward.

1) De Broglie - Bohm interpretation
The most simple approach is to rely on Bohmian mechanics, in which each particle is supposed to exists in a specific position between measurements (hidden variables approach), while its trajectory is calculated using a Guiding Equation based on a quantum field calculated with the Schroedinger Equation.

While this approach is really easy to implement in an ontology, since each entity has its own well defined 4D region, its mathematical representation failed to receive large consensus due to the difficulties to include relativistic effects, to be extended to subnuclear scale and the strong non-locality assumtpion of the quantum field.

Nevertheless, the Bohmian mechanics is a numerical approach that is used in electronic models to reduce the computational effort of the solution of Schroedinger Equation.

In practice, an EMMO user can declare a 'physical' individual that stand for the whole quantum system to be described, and at the same time all sub-parts individuals can be declared, having them a well defined position in time, according to De Broglie - Bohm interpretation. The Hamiltonian can be calculated by considering the sub-part individuals.

'physical'-s are then made of 'physical' parts and 'void' parts that stand for the space between 'physical'-s (e.g. the void between electrons and nucleus in an atom).

2) Copenhagen interpretation
In this interpretation the properties (e.g. energy level, position, spin) of a particle are not defined in the interval between two measurements and the quantum system is entangled (i.e. properties of particles in the sysyem are correlated) and described by a global wavefunction obtained solving the Schroedinger Equation. 

Upon measurement, the wavefunction collapses to a combination of close eigenstates that provide information about bservables of the system components (e.g. position, energy).

The EMMO can be used to represent 'physical'-s that can be related to Copenhagen based models. In practice, the user should follow these steps:

a) define the quantum system as a 'physical' individual (e.g. an H2 molecule) under a specific class (e.g. 'h2_molecule'). This individual is the whole.

b) define the axioms of the  class that describe how many sub-parts are expected for the whole and their class types (e.g. 'h2_molecule' has axioms 'has_proper_part exactly 2 electron' and 'has_proper_part exactly 2 nucleus)

c) the user can now connect the whole to a Schroedinger equation based model whose Hamiltonian is calculated trough the information coming only from the axioms. No individuals are declared for the subparts!

d) a measurement done on the quantum system that provides information on the sub-part observables is interpreted as wavefunction collapse and leads to the end of the whole and the declaration of the sub-parts individuals which can be themselves other quantum systems 

e.g. if the outer electron of the H2 molecule interacts with another entity defining its state, then the whole that stands for the entangled H2 molecule becomes a 'physical' made of an electron individual, a quantum system made of one electron and two nuclei and the void between them.

e.g. in the Born-Oppenheimer approximation the user represent the atom by un-entangling nucleus and electronic cloud. The un-entanglement comes in the form of declaration of individual as parts.

e.g. the double slit experiment can be represent in the EMMO as:
a) before the slit: a 'physical' that extend in space and has parts 'electron' and 'void', called 'single_electron_wave_function'. 'electron' and 'void' are only in the axioms and not decalred individuals.
b) during slit passage: a 'physical' made of one declared individual, the 'electron'.
c) after the slit: again 'single_electron_wave_function'
d) upon collision with the detector:  'physical' made of one declared individual, the 'electron'.</rdfs:comment>
    <rdfs:comment>A 'Physical' with dimensions other than 4D cannot exist, following the restriction of the parent 'EMMO' class.

It follows from the fact that perception is always unfolding in time.

e.g. you always have an aperture time when you take a picture or measure a property. Instantaneous perceptions are idealizations (abstractions) or a very small time measurement.</rdfs:comment>
    <rdfs:comment>From Latin physica "study of nature" (and Ancient Greek φυσικός, “natural”). 

Here the word relates to things perceived through the senses as opposed to the mind; tangible or concrete.</rdfs:comment>
    <rdfs:comment>A 'Physical' must include at least an 'Elementary' part, and can include 'Void' parts.

A 'Physical' may include as part also the 'Void' surrounding or enclosed by its 'Physical' sub parts.

There are no particular criteria for 'Physical'-s structure, except that is made of some 'Elementary'-s as proper parts and not only 'Void'.

This is done in order to take into account the quantum nature of physical systems, in which the actual position of sub-components (e.g. electrons in an atom) is not known except for its probability distribution function (according to the Copenhagen interpretation.)

e.g. a real world object that has spatial parts an atom and a cubic light year of void, extending for some time, can be a physical object.</rdfs:comment>
    <rdfs:label xml:lang="en">Physical</rdfs:label>
    <rdfs:subClassOf rdf:nodeID="N0445b5ff3b1148b19432bb6ef5fdb4db"/>
    <rdfs:subClassOf rdf:nodeID="Ncc996184d6f44f4fb1430e2fa93c42f6"/>
    <rdfs:comment>A 'Physical' is the class that contains all the individuals that stand for real world objects that interact physically with the ontologist, i.e. physical objects.

A physical object must be perceived through physical interaction by the ontologist. Then the ontologist can declare an individual standing for the physical object just perceived.

Perception is a subcategory of physical interactions. It is an interaction that stimulate a representation of the physical object within the ontologist (the agent).</rdfs:comment>
    <rdfs:comment>The purpose of the 'Physical' branch is to provide a representation of the real world objects, while the models used to name, explain or predict the behaviour of the real world objects lay under the 'Semiotic' branch.

More than one semiotic representation can be connected to the same 'Physical'.

e.g. Navier-Stokes or Euler equation applied to the same fluid are an example of mathematical model used to represent a physical object for some specific interpreter.</rdfs:comment>
    <rdfs:comment>In the EMMO there are no relations such as occupiesSpace, since 'Physical'-s are themselves the 4D regions.</rdfs:comment>
    <annotations:EMMO_967080e5_2f42_4eb2_a3a9_c58143e835f9>A 'Item' that has part some 'Elementary' and whose temporal proper parts are only 'Physical'-s (i.e. it can be perceived without interruptions in time).</annotations:EMMO_967080e5_2f42_4eb2_a3a9_c58143e835f9>
  </rdf:Description>
  <rdf:Description rdf:nodeID="Nac8b3ba07a844d03b4a6fb12216095b0">
    <rdf:type rdf:resource="http://www.w3.org/2002/07/owl#Restriction"/>
    <owl:allValuesFrom rdf:resource="http://emmo.info/emmo/middle/isq#EMMO_53bd0c90_41c3_46e2_8779_cd2a80f7e18b"/>
    <owl:onProperty rdf:resource="http://emmo.info/emmo/middle/metrology#EMMO_bed1d005_b04e_4a90_94cf_02bc678a8569"/>
  </rdf:Description>
  <rdf:Description rdf:nodeID="N2475f955a0604bb3a44aefb2b14741d7">
    <rdf:rest rdf:nodeID="Nd278bd9ef4564eb9a5e8169ff91a93dc"/>
    <rdf:first rdf:resource="http://emmo.info/emmo/middle/siunits#EMMO_1273eb34_de48_43a9_925f_104110469dd2"/>
  </rdf:Description>
  <rdf:Description rdf:about="http://emmo.info/emmo/middle/siunits#EMMO_76cc4efc_231e_42b4_be83_2547681caed6">
    <annotations:EMMO_967080e5_2f42_4eb2_a3a9_c58143e835f9>The quantum of action.</annotations:EMMO_967080e5_2f42_4eb2_a3a9_c58143e835f9>
    <annotations:EMMO_6dd685dd_1895_46e4_b227_be9f7d643c25>http://dbpedia.org/page/Planck_constant</annotations:EMMO_6dd685dd_1895_46e4_b227_be9f7d643c25>
    <annotations:EMMO_1f1b164d_ec6a_4faa_8d5e_88bda62316cc>http://physics.nist.gov/cuu/CODATA-Value_PlankConstant</annotations:EMMO_1f1b164d_ec6a_4faa_8d5e_88bda62316cc>
    <rdfs:subClassOf rdf:nodeID="N5318166f25af4081a56615e46759fa73"/>
    <rdfs:label xml:lang="en">PlanckConstant</rdfs:label>
    <annotations:EMMO_fe015383_afb3_44a6_ae86_043628697aa2>https://doi.org/10.1351/goldbook.P04685</annotations:EMMO_fe015383_afb3_44a6_ae86_043628697aa2>
    <rdf:type rdf:resource="http://www.w3.org/2002/07/owl#Class"/>
  </rdf:Description>
  <rdf:Description rdf:about="http://emmo.info/emmo/middle/siunits#EMMO_361c25b3_3c0d_4066_b622_72dcc71ab5cf">
    <ns1:EMMO_23b579e1_8088_45b5_9975_064014026c42 rdf:datatype="http://www.w3.org/2001/XMLSchema#string">T0 L+1 M0 I0 Θ0 N0 J0</ns1:EMMO_23b579e1_8088_45b5_9975_064014026c42>
    <rdfs:label xml:lang="en">a</rdfs:label>
    <rdf:type rdf:resource="http://www.w3.org/2002/07/owl#NamedIndividual"/>
  </rdf:Description>
  <rdf:Description rdf:about="http://emmo.info/emmo/top/mereotopology#EMMO_eb3a768e_d53e_4be9_a23b_0714833c36de">
    <rdfs:comment>From Latin item, "likewise, just so, moreover".</rdfs:comment>
    <rdfs:label xml:lang="en">Item</rdfs:label>
    <rdfs:comment>An 'Item' individual stands for a real world self-connected object which can be represented as a whole made of connected parts (e.g. a car made of components).

In the EMMO, connectivity is the topological foundation of causality.

All physical systems, i.e. systems whose behaviour is explained by physics laws, are represented only by 'Item'-s.

Members of a 'Collection' lack of causality connection, i.e. they do not constitute a physical system as a whole.</rdfs:comment>
    <rdf:type rdf:resource="http://www.w3.org/2002/07/owl#Class"/>
    <rdfs:comment>A real world object is self-connected if any two parts that make up the whole are connected to each other (here the concept of connection is primitive). 

Alternatively, using the primitive path-connectivity concept we can define a self-connected real world object as an object for which each couple of points is path-connected.</rdfs:comment>
    <owl:disjointUnionOf rdf:nodeID="N5ab6604471ad40efa6990358a91c3eb3"/>
  </rdf:Description>
  <rdf:Description rdf:nodeID="N9e8d8a750b2940e1b9e8bdc06ce422e5">
    <owl:allValuesFrom rdf:nodeID="N0124c3d319bc474fbaebc8b75db26354"/>
    <owl:onProperty rdf:nodeID="N1fb591fb5bbc4aacbf6a96c5916dfb32"/>
    <rdf:type rdf:resource="http://www.w3.org/2002/07/owl#Restriction"/>
  </rdf:Description>
  <rdf:Description rdf:about="http://emmo.info/emmo/middle/isq#EMMO_e7c9f7fd_e534_4441_88fe_1fec6cb20f26">
    <annotations:EMMO_fe015383_afb3_44a6_ae86_043628697aa2>https://doi.org/10.1351/goldbook.S05732</annotations:EMMO_fe015383_afb3_44a6_ae86_043628697aa2>
    <rdfs:label xml:lang="en">SolidAngle</rdfs:label>
    <rdfs:subClassOf rdf:nodeID="N6c293cf031c6490c977b1548bd713df4"/>
    <annotations:EMMO_967080e5_2f42_4eb2_a3a9_c58143e835f9>Ratio of area on a sphere to its radius squared.</annotations:EMMO_967080e5_2f42_4eb2_a3a9_c58143e835f9>
    <annotations:EMMO_6dd685dd_1895_46e4_b227_be9f7d643c25>http://dbpedia.org/page/Solid_angle</annotations:EMMO_6dd685dd_1895_46e4_b227_be9f7d643c25>
    <rdf:type rdf:resource="http://www.w3.org/2002/07/owl#Class"/>
    <rdfs:subClassOf rdf:resource="http://emmo.info/emmo/middle/isq#EMMO_2946d40b_24a1_47fa_8176_e3f79bb45064"/>
  </rdf:Description>
  <rdf:Description rdf:nodeID="N5a84054aa4be46b8bb0d9e9b42106348">
    <rdf:rest rdf:nodeID="Na4f80bee6cca453ba406917c43e02a5e"/>
    <rdf:first rdf:resource="http://emmo.info/emmo/middle/siunits#EMMO_068c4e58_2470_4b1c_8454_010dd4906100"/>
  </rdf:Description>
  <rdf:Description rdf:about="http://emmo.info/emmo/middle/physicalistic#EMMO_70dac51e_bddd_48c2_8a98_7d8395e91fc2">
    <rdfs:label xml:lang="en">Field</rdfs:label>
    <rdf:type rdf:resource="http://www.w3.org/2002/07/owl#Class"/>
    <annotations:EMMO_967080e5_2f42_4eb2_a3a9_c58143e835f9>A 'Physical' with 'Massless' parts that are mediators of interactions.</annotations:EMMO_967080e5_2f42_4eb2_a3a9_c58143e835f9>
    <rdfs:comment>The concepts of matter and field for classical physics, upon which we can categorize physical entities, are replaced in quantum physics by the more general concepts of quantum field.

Here the class 'Field' refers to the quantum field of massless bosonic particles (i.e. photons, gluons), while the class 'Matter' refers to the quantum field of massive fermionic or bosonic particles (e.g. quarks, electrons).</rdfs:comment>
    <rdfs:subClassOf rdf:nodeID="N7fd06f962f58498f8b945dafa90d59af"/>
    <rdfs:subClassOf rdf:nodeID="Nac3248cba359458e95504df745526bbb"/>
    <rdfs:subClassOf rdf:resource="http://emmo.info/emmo/top/physical#EMMO_c5ddfdba_c074_4aa4_ad6b_1ac4942d300d"/>
  </rdf:Description>
  <rdf:Description rdf:about="http://emmo.info/emmo/top/semiotics#EMMO_d7788d1a_020d_4c78_85a1_13563fcec168">
    <rdfs:comment>Three subtypes of icon are possible:
 
(a) the image, which depends on a simple quality (e.g. picture)

(b) the diagram, whose internal relations, mainly dyadic or so taken, represent by analogy the relations in something (e.g. math formula, geometric flowchart)

(c) the metaphor, which represents the representative character of a sign by representing a parallelism in something else

[Wikipedia]</rdfs:comment>
    <rdfs:label xml:lang="en">Icon</rdfs:label>
    <annotations:EMMO_967080e5_2f42_4eb2_a3a9_c58143e835f9>A 'Sign' that stands for an 'Object' by resembling or imitating it, in shape or by sharing a similar logical structure.</annotations:EMMO_967080e5_2f42_4eb2_a3a9_c58143e835f9>
    <annotations:EMMO_b432d2d5_25f4_4165_99c5_5935a7763c1a>A picture that reproduces the aspect of a person. 

An equation that reproduces the logical connection of the properties of a physical entity.</annotations:EMMO_b432d2d5_25f4_4165_99c5_5935a7763c1a>
    <rdf:type rdf:resource="http://www.w3.org/2002/07/owl#Class"/>
  </rdf:Description>
  <rdf:Description rdf:about="http://emmo.info/emmo/middle/models#EMMO_939483b1_0148_43d1_8b35_851d2cd5d939">
    <rdf:type rdf:resource="http://www.w3.org/2002/07/owl#Class"/>
    <rdfs:label xml:lang="en">Model</rdfs:label>
    <owl:equivalentClass rdf:nodeID="N5eadb1da8396445eab40fbac7cd3388e"/>
    <annotations:EMMO_967080e5_2f42_4eb2_a3a9_c58143e835f9>A 'sign' that not only stands for a 'physical' or a 'process', but it is also a simplified representation, aimed to assist calculations for its description or for predictions of its behaviour.

A 'model' represents a 'physical' or a 'process' by direct similitude (e.g. small scale replica) or by capturing in a logical framework the relations between its properties (e.g. mathematical model).</annotations:EMMO_967080e5_2f42_4eb2_a3a9_c58143e835f9>
    <rdfs:comment>A 'model' prediction is always a prediction of the properties of an entity, since an entity is known by an interpreter only through perception.</rdfs:comment>
  </rdf:Description>
  <rdf:Description rdf:about="http://emmo.info/emmo/middle/math#EMMO_1eed0732_e3f1_4b2c_a9c4_b4e75eeb5895">
    <rdfs:subClassOf rdf:resource="http://emmo.info/emmo/middle/math#EMMO_54ee6b5e_5261_44a8_86eb_5717e7fdb9d0"/>
    <rdf:type rdf:resource="http://www.w3.org/2002/07/owl#Class"/>
    <rdfs:label xml:lang="en">Variable</rdfs:label>
    <rdfs:subClassOf rdf:nodeID="N7e1e011133494ac397d3fdafa69e647f"/>
    <annotations:EMMO_b432d2d5_25f4_4165_99c5_5935a7763c1a>x
k</annotations:EMMO_b432d2d5_25f4_4165_99c5_5935a7763c1a>
    <annotations:EMMO_967080e5_2f42_4eb2_a3a9_c58143e835f9>A 'Variable' is a symbolic object that stands for a numerical defined 'Mathematical' object like e.g. a number, a vector, a matrix.</annotations:EMMO_967080e5_2f42_4eb2_a3a9_c58143e835f9>
  </rdf:Description>
  <rdf:Description rdf:about="http://emmo.info/emmo/top/annotations#EMMO_b306ae38_938e_48fe_83e9_6141e08b596f">
    <rdfs:comment>URL to corresponding concept in the Basic Datatype Ontology (DBO)</rdfs:comment>
    <rdf:type rdf:resource="http://www.w3.org/2002/07/owl#AnnotationProperty"/>
    <rdfs:subPropertyOf rdf:resource="http://www.w3.org/2000/01/rdf-schema#seeAlso"/>
    <rdfs:label xml:lang="en">bdoMatch</rdfs:label>
    <rdfs:seeAlso>https://github.com/TechnicalBuildingSystems/Ontologies/blob/master/BasicDataTypeOntology/ontology.ttl</rdfs:seeAlso>
  </rdf:Description>
  <rdf:Description rdf:about="http://emmo.info/emmo/middle/isq#EMMO_31ec09ba_1713_42cb_83c7_b38bf6f9ced2">
    <annotations:EMMO_6dd685dd_1895_46e4_b227_be9f7d643c25>http://dbpedia.org/page/Energy</annotations:EMMO_6dd685dd_1895_46e4_b227_be9f7d643c25>
    <rdfs:subClassOf rdf:nodeID="Nc247f24d50b14edbb411811ff383f17b"/>
    <rdfs:comment>Energy is often defined as "ability of a system to perform work", but it might be misleading since is not necessarily available to do work.</rdfs:comment>
    <annotations:EMMO_fe015383_afb3_44a6_ae86_043628697aa2>https://doi.org/10.1351/goldbook.E02101</annotations:EMMO_fe015383_afb3_44a6_ae86_043628697aa2>
    <rdfs:subClassOf rdf:resource="http://emmo.info/emmo/middle/isq#EMMO_2946d40b_24a1_47fa_8176_e3f79bb45064"/>
    <rdfs:label xml:lang="en">Energy</rdfs:label>
    <annotations:EMMO_967080e5_2f42_4eb2_a3a9_c58143e835f9>A property of objects which can be transferred to other objects or converted into different forms.</annotations:EMMO_967080e5_2f42_4eb2_a3a9_c58143e835f9>
    <rdf:type rdf:resource="http://www.w3.org/2002/07/owl#Class"/>
  </rdf:Description>
  <rdf:Description rdf:about="http://emmo.info/emmo/top/mereotopology#EMMO_2d2ecd97_067f_4d0e_950c_d746b7700a31">
    <rdfs:comment>e.g. the collection of users of a particular software, the collection of atoms that have been part of that just dissociated molecule, or even the collection of atoms that are part of a molecule considered as single individual non-connected objects and not as a mereotopological self-connected fusion.</rdfs:comment>
    <rdf:type rdf:resource="http://www.w3.org/2002/07/owl#Class"/>
    <rdfs:label xml:lang="en">Collection</rdfs:label>
    <rdfs:comment>Formally, 'Collection' is axiomatized as the class of individuals that hasMember some 'Item'.

A 'Collection' cannot have as member another 'Collection'.</rdfs:comment>
    <rdfs:comment>A 'Collection' individual stands for a non-self-connected real world object.

A 'Collection' individual is related to each 'Item' individuals of the collection (i.e. the members) through the membership relation.

An 'Item' individual stands for a real world self-connected object which can be represented as a whole made of connected parts (e.g. a car made of components).</rdfs:comment>
    <annotations:EMMO_967080e5_2f42_4eb2_a3a9_c58143e835f9>The class of all individuals that stand for a real world not self-connected object.</annotations:EMMO_967080e5_2f42_4eb2_a3a9_c58143e835f9>
    <rdfs:subClassOf rdf:nodeID="Nb7c50d3a007941bb8f3a498623f464da"/>
    <rdfs:comment>From Latin collectio, from colligere ‘gather together’.</rdfs:comment>
  </rdf:Description>
  <rdf:Description rdf:about="http://emmo.info/emmo/middle/perceptual#EMMO_a1083d0a_c1fb_471f_8e20_a98f881ad527">
    <annotations:EMMO_b432d2d5_25f4_4165_99c5_5935a7763c1a>The class of letter "A" is the symbol as idea and the letter A that you see on the screen is the mark.</annotations:EMMO_b432d2d5_25f4_4165_99c5_5935a7763c1a>
    <rdf:type rdf:resource="http://www.w3.org/2002/07/owl#Class"/>
    <rdfs:subClassOf rdf:nodeID="Nad0d20865f95462fa10914def1cb1717"/>
    <rdfs:comment>Subclasses of 'Symbol' are alphabets, in formal languages terminology.

A 'Symbol' is atomic for that alphabet, i.e. it has no parts that are symbols for the same alphabet.
e.g. a math symbol is not made of other math symbols

A Symbol may be a String in another language.
e.g. "Bq" is the symbol for Becquerel units when dealing with metrology, or a string of "B" and "q" symbols when dealing with characters.</rdfs:comment>
    <rdfs:label xml:lang="en">Symbol</rdfs:label>
    <rdfs:comment>Symbols of a formal language need not be symbols of anything. For instance there are logical constants which do not refer to any idea, but rather serve as a form of punctuation in the language (e.g. parentheses). 

Symbols of a formal language must be capable of being specified without any reference to any interpretation of them. 
(Wikipedia)</rdfs:comment>
    <rdfs:subClassOf rdf:resource="http://emmo.info/emmo/middle/perceptual#EMMO_057e7d57_aff0_49de_911a_8861d85cef40"/>
    <annotations:EMMO_967080e5_2f42_4eb2_a3a9_c58143e835f9>The class of individuals that stand for an elementary mark of a specific symbolic code (alphabet).</annotations:EMMO_967080e5_2f42_4eb2_a3a9_c58143e835f9>
    <rdfs:comment>The class is the idea of the symbol, while the individual of that class stands for a specific mark (or token) of that idea.</rdfs:comment>
  </rdf:Description>
  <rdf:Description rdf:about="http://emmo.info/emmo/middle/properties#EMMO_dd4a7f3e_ef56_466c_ac1a_d2716b5f87ec">
    <rdfs:label xml:lang="en">QuantitativeProperty</rdfs:label>
    <rdf:type rdf:resource="http://www.w3.org/2002/07/owl#Class"/>
    <owl:equivalentClass rdf:nodeID="N0cba766ba19a4a239eb78d3e3a35be3a"/>
    <rdfs:comment>"A property of a phenomenon, body, or substance, where the property has a magnitude that can be expressed by means of a number and a reference"
ISO 80000-1

"A reference can be a measurement unit, a measurement procedure, a reference material, or a combination of such."
International vocabulary of metrology (VIM)</rdfs:comment>
    <rdfs:comment>A quantitative property is always expresssed as a quantity (i.e. a number and a reference unit). For the EMMO, a nominalistic ontology, there is no property as abstract object.

A property is a sign that stands for an object according to a specific code shared by some observers.

For quantititative properties, one possible code that is shared between the scientific community (the observers) is the SI system of units.</rdfs:comment>
    <rdfs:comment>Subclasses of 'QuantitativeProperty' classify objects according to the type semiosis that is used to connect the property to the object (e.g. by measurement, by convention, by modelling).</rdfs:comment>
    <annotations:EMMO_967080e5_2f42_4eb2_a3a9_c58143e835f9>A 'Quantity' that can be quantified with respect to a standardized reference physical instance (e.g. the prototype meter bar, the kg prototype) or method (e.g. resilience) through a measurement process.</annotations:EMMO_967080e5_2f42_4eb2_a3a9_c58143e835f9>
    <rdfs:subClassOf rdf:resource="http://emmo.info/emmo/middle/metrology#EMMO_f658c301_ce93_46cf_9639_4eace2c5d1d5"/>
    <rdfs:subClassOf rdf:resource="http://emmo.info/emmo/middle/properties#EMMO_2a888cdf_ec4a_4ec5_af1c_0343372fc978"/>
  </rdf:Description>
  <rdf:Description rdf:about="http://emmo.info/emmo/middle/holistic">
    <annotations:EMMO_5525a055_dda5_4556_8b91_f0d22fa676cc>EMMO is released under a Creative Commons license Attribution 4.0 International (CC BY 4.0)

https://creativecommons.org/licenses/by/4.0/legalcode</annotations:EMMO_5525a055_dda5_4556_8b91_f0d22fa676cc>
    <rdfs:comment>European Materials and Modelling Ontology (EMMO)

EMMO is a multidisciplinary effort to develop a standard representational framework (the ontology) based on current materials modelling knowledge, including physical sciences, analytical philosophy and information and communication technologies. 

It provides the connection between the physical world, materials characterisation world and materials modelling world.</rdfs:comment>
    <rdf:type rdf:resource="http://www.w3.org/2002/07/owl#Ontology"/>
    <rdfs:comment>The EMMO requires FacT++ reasoner plugin in order to visualize all inferences and class hierarchy (ctrl+R hotkey in Protege).</rdfs:comment>
    <rdfs:comment xml:lang="en">Contacts:
Gerhard Goldbeck
Goldbeck Consulting Ltd (UK)
email: gerhard@goldbeck-consulting.com

Emanuele Ghedini
University of Bologna (IT)
email: emanuele.ghedini</rdfs:comment>
    <owl:versionIRI rdf:resource="http://emmo.info/emmo/1.0.0-alpha/middle/holistic"/>
    <annotations:EMMO_cd5fb112_7ee7_4120_a35d_3ca3e6c3f4ab>Emanuele Ghedini (University of Bologna, IT)
Gerhard Goldbeck (GCL Ltd, UK)
Adham Hashibon (Fraunhofer IWM, DE)
Georg Schmitz (Access, DE)
Jesper Friis (SINTEF, NO)</annotations:EMMO_cd5fb112_7ee7_4120_a35d_3ca3e6c3f4ab>
    <owl:versionInfo>The European Materials Modelling Ontology

Version 1.0.0-alpha</owl:versionInfo>
  </rdf:Description>
  <rdf:Description rdf:about="http://emmo.info/emmo/middle/physicalistic#EMMO_98ada9d8_f1c8_4f13_99b5_d890f5354152">
    <rdfs:subClassOf rdf:resource="http://emmo.info/emmo/top#EMMO_49267eba_5548_4163_8f36_518d65b583f9"/>
    <rdfs:label xml:lang="en">Physicalistic</rdfs:label>
    <rdf:type rdf:resource="http://www.w3.org/2002/07/owl#Class"/>
    <annotations:EMMO_967080e5_2f42_4eb2_a3a9_c58143e835f9>The perspective for which physical objects are categorized only by concepts coming from physics.</annotations:EMMO_967080e5_2f42_4eb2_a3a9_c58143e835f9>
    <owl:equivalentClass rdf:nodeID="N9ccab888074f47afa89e6fc78ecf6e29"/>
  </rdf:Description>
  <rdf:Description rdf:about="http://emmo.info/emmo/middle/materials#EMMO_8b0923ab_b500_477b_9ce9_8b3a3e4dc4f2">
    <rdfs:comment>A continuum is the bearer of properties that are generated by the interactions of parts such as viscosity and thermal or electrical conductivity.</rdfs:comment>
    <rdfs:comment>A continuum is made of a sufficient number of parts that it continues to exists as continuum individual even after the loss of one of them i.e. a continuum is a redundant.</rdfs:comment>
    <rdfs:subClassOf rdf:resource="http://emmo.info/emmo/middle/physicalistic#EMMO_4207e895_8b83_4318_996a_72cfb32acd94"/>
    <rdf:type rdf:resource="http://www.w3.org/2002/07/owl#Class"/>
    <rdfs:comment>A continuum is not necessarily small (i.e. composed by the minimum amount of sates to fulfill the definition).

A single continuum individual can be the whole fluid in a pipe.</rdfs:comment>
    <annotations:EMMO_967080e5_2f42_4eb2_a3a9_c58143e835f9>A state that is a collection of sufficiently large number of other parts such that:
- it is the bearer of qualities that can exists only by the fact that it is a sum of parts
- the smallest partition dV of the state volume in which we are interested in, contains enough parts to be statistically consistent: n [#/m3] x dV [m3] &gt;&gt; 1</annotations:EMMO_967080e5_2f42_4eb2_a3a9_c58143e835f9>
    <rdfs:subClassOf rdf:resource="http://emmo.info/emmo/middle/reductionistic#EMMO_36c79456_e29c_400d_8bd3_0eedddb82652"/>
    <rdfs:label xml:lang="en">Continuum</rdfs:label>
  </rdf:Description>
  <rdf:Description rdf:about="http://emmo.info/emmo/middle/isq#EMMO_961d1aba_f75e_4411_aaa4_457f7516ed6b">
    <annotations:EMMO_fe015383_afb3_44a6_ae86_043628697aa2>https://doi.org/10.1351/goldbook.M03686</annotations:EMMO_fe015383_afb3_44a6_ae86_043628697aa2>
    <rdfs:subClassOf rdf:resource="http://emmo.info/emmo/middle/isq#EMMO_2946d40b_24a1_47fa_8176_e3f79bb45064"/>
    <annotations:EMMO_967080e5_2f42_4eb2_a3a9_c58143e835f9>Strength of the magnetic field.</annotations:EMMO_967080e5_2f42_4eb2_a3a9_c58143e835f9>
    <rdf:type rdf:resource="http://www.w3.org/2002/07/owl#Class"/>
    <annotations:EMMO_6dd685dd_1895_46e4_b227_be9f7d643c25>http://dbpedia.org/page/Magnetic_field</annotations:EMMO_6dd685dd_1895_46e4_b227_be9f7d643c25>
    <rdfs:subClassOf rdf:nodeID="N21b3512e4c974b1da44bc7fc17afdaa9"/>
    <rdfs:comment>Often denoted B.</rdfs:comment>
    <rdfs:label xml:lang="en">MagneticFluxDensity</rdfs:label>
  </rdf:Description>
  <rdf:Description rdf:nodeID="N4813a2ce167a4fad9b05d9a83354e42e">
    <rdf:rest rdf:nodeID="N95847686951b4b4d822339dd292787f1"/>
    <rdf:first rdf:resource="http://emmo.info/emmo/middle/siunits#EMMO_1273eb34_de48_43a9_925f_104110469dd2"/>
  </rdf:Description>
  <rdf:Description rdf:nodeID="N69a645702fd94045828660e1e4876123">
    <owl:someValuesFrom rdf:resource="http://emmo.info/emmo/middle/isq#EMMO_77e9dc31_5b19_463e_b000_44c6e79f98aa"/>
    <rdf:type rdf:resource="http://www.w3.org/2002/07/owl#Restriction"/>
    <owl:onProperty rdf:resource="http://emmo.info/emmo/middle/metrology#EMMO_bed1d005_b04e_4a90_94cf_02bc678a8569"/>
  </rdf:Description>
  <rdf:Description rdf:about="http://emmo.info/emmo/middle/isq#EMMO_3227b821_26a5_4c7c_9c01_5c24483e0bd0">
    <rdf:type rdf:resource="http://www.w3.org/2002/07/owl#Class"/>
    <owl:equivalentClass rdf:nodeID="Nf576db9a51bf4118a5febb7bc3b04ca5"/>
    <rdfs:label xml:lang="en">DimensionOne</rdfs:label>
    <rdfs:subClassOf rdf:resource="http://emmo.info/emmo/middle/metrology#EMMO_9895a1b4_f0a5_4167_ac5e_97db40b8bfcc"/>
  </rdf:Description>
  <rdf:Description rdf:nodeID="Nad03685a5fae47db8b8331d65c2da678">
    <rdf:first rdf:resource="http://emmo.info/emmo/middle/siunits#EMMO_acb50123_87a2_4753_b36c_f87114ad4de2"/>
    <rdf:rest rdf:nodeID="Na64179d208c146ffaef42a3f96890f65"/>
  </rdf:Description>
  <rdf:Description rdf:nodeID="N0f93456af1aa461490eca66aad531639">
    <owl:qualifiedCardinality rdf:datatype="http://www.w3.org/2001/XMLSchema#nonNegativeInteger">1</owl:qualifiedCardinality>
    <owl:onDataRange rdf:resource="http://www.w3.org/2001/XMLSchema#boolean"/>
    <owl:onProperty rdf:resource="http://emmo.info/emmo/middle/math#EMMO_faf79f53_749d_40b2_807c_d34244c192f4"/>
    <rdf:type rdf:resource="http://www.w3.org/2002/07/owl#Restriction"/>
  </rdf:Description>
  <rdf:Description rdf:nodeID="N8ac74537a11b459f83ec52b7358c9d33">
    <owl:allValuesFrom rdf:resource="http://emmo.info/emmo/middle/isq#EMMO_ce7d4720_aa20_4a8c_93e8_df41a35b6723"/>
    <rdf:type rdf:resource="http://www.w3.org/2002/07/owl#Restriction"/>
    <owl:onProperty rdf:resource="http://emmo.info/emmo/middle/metrology#EMMO_bed1d005_b04e_4a90_94cf_02bc678a8569"/>
  </rdf:Description>
  <rdf:Description rdf:about="http://emmo.info/emmo/top/annotations">
    <owl:versionInfo>The European Materials Modelling Ontology

Version 1.0.0-alpha</owl:versionInfo>
    <rdfs:comment xml:lang="en">Contacts:
Gerhard Goldbeck
Goldbeck Consulting Ltd (UK)
email: gerhard@goldbeck-consulting.com

Emanuele Ghedini
University of Bologna (IT)
email: emanuele.ghedini@unibo.it</rdfs:comment>
    <rdfs:comment>The EMMO requires FacT++ reasoner plugin in order to visualize all inferences and class hierarchy (ctrl+R hotkey in Protege).</rdfs:comment>
    <rdfs:comment>European Materials and Modelling Ontology (EMMO)

EMMO is a multidisciplinary effort to develop a standard representational framework (the ontology) based on current materials modelling knowledge, including physical sciences, analytical philosophy and information and communication technologies. 

It provides the connection between the physical world, materials characterisation world and materials modelling world.</rdfs:comment>
    <rdf:type rdf:resource="http://www.w3.org/2002/07/owl#Ontology"/>
    <annotations:EMMO_cd5fb112_7ee7_4120_a35d_3ca3e6c3f4ab>Emanuele Ghedini (University of Bologna, IT)
Gerhard Goldbeck (GCL Ltd, UK)
Adham Hashibon (Fraunhofer IWM, DE)
Georg Schmitz (Access, DE)
Jesper Friis (SINTEF, NO)</annotations:EMMO_cd5fb112_7ee7_4120_a35d_3ca3e6c3f4ab>
    <owl:versionIRI rdf:resource="http://emmo.info/emmo/1.0.0-alpha/top/annotations"/>
  </rdf:Description>
  <rdf:Description rdf:nodeID="N4a67bf79c8954b2a86a4185810889860">
    <rdf:first rdf:resource="http://emmo.info/emmo/middle/siunits#EMMO_7db11dbf_a643_464a_9b56_07eabcc3e9c5"/>
    <rdf:rest rdf:nodeID="N9317f2a36b544bdfa8699a37b32afe72"/>
  </rdf:Description>
  <rdf:Description rdf:nodeID="Nd43b659b71cd4664aa83407e427a38a1">
    <rdf:type rdf:resource="http://www.w3.org/2002/07/owl#Class"/>
    <owl:complementOf rdf:resource="http://emmo.info/emmo/middle/metrology#EMMO_985bec21_989f_4b9e_a4b3_735d88099c3c"/>
  </rdf:Description>
  <rdf:Description rdf:nodeID="Na4472cce6d34452f990e1021af18212a">
    <rdf:type rdf:resource="http://www.w3.org/2002/07/owl#Restriction"/>
    <owl:allValuesFrom rdf:resource="http://emmo.info/emmo/middle/metrology#EMMO_db716151_6b73_45ff_910c_d182fdcbb4f5"/>
    <owl:onProperty rdf:resource="http://emmo.info/emmo/middle/metrology#EMMO_67fc0a36_8dcb_4ffa_9a43_31074efa3296"/>
  </rdf:Description>
  <rdf:Description rdf:about="http://emmo.info/emmo/middle/siunits#EMMO_a8eb4bbb_1bd3_4ad4_b114_2789bcbd2134">
    <rdfs:subClassOf rdf:nodeID="N07aaafec469d490983de40b7e7d2f87a"/>
    <rdfs:subClassOf rdf:nodeID="N9e8d8a750b2940e1b9e8bdc06ce422e5"/>
    <rdfs:label xml:lang="en">Giga</rdfs:label>
    <rdf:type rdf:resource="http://www.w3.org/2002/07/owl#Class"/>
  </rdf:Description>
  <rdf:Description rdf:nodeID="N5c8cd0519ede485a8fc884a374d120c7">
    <rdf:first rdf:resource="http://emmo.info/emmo/middle/siunits#EMMO_b55cd09a_e54d_4eb1_81dd_03c29d1b878e"/>
    <rdf:rest rdf:nodeID="Nfa669788efe14134a1f041feec300a4b"/>
  </rdf:Description>
  <rdf:Description rdf:nodeID="N19a634e0ce894273916bc500c00fbc73">
    <rdf:first rdf:resource="http://emmo.info/emmo/middle/physicalistic#EMMO_7db59e56_f68b_48b7_ae99_891c35ae5c3b"/>
    <rdf:rest rdf:nodeID="N7ee177ae40ba4ad5a9730b0fd07398ac"/>
  </rdf:Description>
  <rdf:Description rdf:about="http://emmo.info/emmo/middle/materials#EMMO_50781fd9_a9e4_46ad_b7be_4500371d188d">
    <rdfs:label xml:lang="en">Nucleon</rdfs:label>
    <rdf:type rdf:resource="http://www.w3.org/2002/07/owl#Class"/>
    <rdfs:subClassOf rdf:nodeID="Nf7c388ca76684aeb844b9cc88b15e1c1"/>
    <owl:disjointUnionOf rdf:nodeID="N5afa3e7bcceb4f2eb076c28a0bff11f4"/>
    <rdfs:subClassOf rdf:resource="http://emmo.info/emmo/middle/materials#EMMO_7d66bde4_b68d_41cc_b5fc_6fd98c5e2ff0"/>
  </rdf:Description>
  <rdf:Description rdf:nodeID="Neba99011675741efa2a57a0d8e2bce4a">
    <rdf:type rdf:resource="http://www.w3.org/2002/07/owl#Restriction"/>
    <owl:someValuesFrom rdf:resource="http://emmo.info/emmo/middle/manufacturing#EMMO_a4d66059_5dd3_4b90_b4cb_10960559441b"/>
    <owl:onProperty rdf:nodeID="Ndae100846d6e4cb6941b45753b4e9b20"/>
  </rdf:Description>
  <rdf:Description rdf:about="http://emmo.info/emmo/middle/siunits#EMMO_a121bb1d_5225_4c78_809b_0268c3012208">
    <rdf:type rdf:resource="http://www.w3.org/2002/07/owl#Class"/>
    <rdfs:comment>Dimensionless measurement unit for plane angle.</rdfs:comment>
    <rdfs:label xml:lang="en">Radian</rdfs:label>
    <annotations:EMMO_1f1b164d_ec6a_4faa_8d5e_88bda62316cc>http://qudt.org/vocab/unit/RAD</annotations:EMMO_1f1b164d_ec6a_4faa_8d5e_88bda62316cc>
    <rdfs:subClassOf rdf:nodeID="N2ef84063018c42cf8aa5546fc0a540a6"/>
    <annotations:EMMO_fe015383_afb3_44a6_ae86_043628697aa2>https://doi.org/10.1351/goldbook.R05036</annotations:EMMO_fe015383_afb3_44a6_ae86_043628697aa2>
    <rdfs:subClassOf rdf:nodeID="Ndf57d92015fc4650bdd5b0224e0343d3"/>
    <annotations:EMMO_967080e5_2f42_4eb2_a3a9_c58143e835f9>Measure of plane angle.</annotations:EMMO_967080e5_2f42_4eb2_a3a9_c58143e835f9>
  </rdf:Description>
  <rdf:Description rdf:about="http://emmo.info/emmo/middle/siunits#EMMO_dc232f53_8ed8_4ddd_9f41_cc057985eadb">
    <rdfs:subClassOf rdf:nodeID="N5e242b4b35b243f1ae0b9abb11efaa92"/>
    <rdfs:comment>Measurement unit for equivalent doseof ionizing radiation. 

Sievert is derived from absorbed dose, but takes into account the biological effectiveness of the radiation, which is dependent on the radiation type and energy.</rdfs:comment>
    <annotations:EMMO_1f1b164d_ec6a_4faa_8d5e_88bda62316cc>http://qudt.org/vocab/unit/SV</annotations:EMMO_1f1b164d_ec6a_4faa_8d5e_88bda62316cc>
    <annotations:EMMO_c84c6752_6d64_48cc_9500_e54a3c34898d>https://en.wikipedia.org/wiki/Equivalent_dose</annotations:EMMO_c84c6752_6d64_48cc_9500_e54a3c34898d>
    <rdf:type rdf:resource="http://www.w3.org/2002/07/owl#Class"/>
    <annotations:EMMO_fe015383_afb3_44a6_ae86_043628697aa2>https://doi.org/10.1351/goldbook.S05658</annotations:EMMO_fe015383_afb3_44a6_ae86_043628697aa2>
    <rdfs:label xml:lang="en">Sievert</rdfs:label>
    <rdfs:subClassOf rdf:nodeID="N33e37838ff8e4cc49eb6e84faced6fa6"/>
  </rdf:Description>
  <rdf:Description rdf:nodeID="Ncc9730a5c39940f3ab51d513ccb2a809">
    <owl:someValuesFrom rdf:resource="http://emmo.info/emmo/middle/perceptual#EMMO_a1083d0a_c1fb_471f_8e20_a98f881ad527"/>
    <owl:onProperty rdf:resource="http://emmo.info/emmo/middle/reductionistic#EMMO_b2282816_b7a3_44c6_b2cb_3feff1ceb7fe"/>
    <rdf:type rdf:resource="http://www.w3.org/2002/07/owl#Restriction"/>
  </rdf:Description>
  <rdf:Description rdf:about="http://emmo.info/emmo/middle/properties#EMMO_463bcfda_867b_41d9_a967_211d4d437cfb">
    <annotations:EMMO_967080e5_2f42_4eb2_a3a9_c58143e835f9>An 'observation' that results in a quantitative comparison of a 'property' of an 'object' with a standard reference.</annotations:EMMO_967080e5_2f42_4eb2_a3a9_c58143e835f9>
    <rdfs:subClassOf rdf:nodeID="N3ba50be97ada433a99cc1a8a9c643f51"/>
    <rdfs:label xml:lang="en">Measurement</rdfs:label>
    <rdf:type rdf:resource="http://www.w3.org/2002/07/owl#Class"/>
    <rdfs:subClassOf rdf:resource="http://emmo.info/emmo/middle/properties#EMMO_10a5fd39_06aa_4648_9e70_f962a9cb2069"/>
  </rdf:Description>
  <rdf:Description rdf:about="http://emmo.info/emmo/middle/isq#EMMO_3b931698_937e_49be_ab1b_36fa52d91181">
    <rdfs:subClassOf rdf:resource="http://emmo.info/emmo/middle/isq#EMMO_2946d40b_24a1_47fa_8176_e3f79bb45064"/>
    <rdfs:subClassOf rdf:nodeID="Ne50be8d65a20431f96870b94a3f42210"/>
    <rdfs:label xml:lang="en">MagneticFlux</rdfs:label>
    <rdf:type rdf:resource="http://www.w3.org/2002/07/owl#Class"/>
    <annotations:EMMO_6dd685dd_1895_46e4_b227_be9f7d643c25>http://dbpedia.org/page/Magnetic_flux</annotations:EMMO_6dd685dd_1895_46e4_b227_be9f7d643c25>
    <annotations:EMMO_fe015383_afb3_44a6_ae86_043628697aa2>https://doi.org/10.1351/goldbook.M03684</annotations:EMMO_fe015383_afb3_44a6_ae86_043628697aa2>
    <annotations:EMMO_967080e5_2f42_4eb2_a3a9_c58143e835f9>Measure of magnetism, taking account of the strength and the extent of a magnetic field.</annotations:EMMO_967080e5_2f42_4eb2_a3a9_c58143e835f9>
  </rdf:Description>
  <rdf:Description rdf:about="http://emmo.info/emmo/middle/isq#EMMO_bd67d149_24c2_4bc9_833a_c2bc26f98fd3">
    <annotations:EMMO_fe015383_afb3_44a6_ae86_043628697aa2>https://doi.org/10.1351/goldbook.C00881</annotations:EMMO_fe015383_afb3_44a6_ae86_043628697aa2>
    <rdfs:subClassOf rdf:nodeID="N8f4f5099a7e945f6aa22e0d84b8a0960"/>
    <rdfs:label xml:lang="en">CatalyticActivity</rdfs:label>
    <rdf:type rdf:resource="http://www.w3.org/2002/07/owl#Class"/>
    <rdfs:subClassOf rdf:resource="http://emmo.info/emmo/middle/isq#EMMO_2946d40b_24a1_47fa_8176_e3f79bb45064"/>
    <annotations:EMMO_967080e5_2f42_4eb2_a3a9_c58143e835f9>Increase in the rate of reaction of a specified chemical reaction that an enzyme produces in a specific assay system.</annotations:EMMO_967080e5_2f42_4eb2_a3a9_c58143e835f9>
  </rdf:Description>
  <rdf:Description rdf:about="http://emmo.info/emmo/top/physical#EMMO_0f795e3e_c602_4577_9a43_d5a231aa1360">
    <rdf:type rdf:resource="http://www.w3.org/2002/07/owl#Class"/>
    <rdfs:comment>From Latin elementārius (“elementary”), from elementum (“one of the four elements of antiquity; fundamentals”)</rdfs:comment>
    <rdfs:comment>While a 'Quantum' is a-tomistic in time and space, an 'elementary' is a-tomistic only in space, recalling the concept of elementary particle.</rdfs:comment>
    <rdfs:subClassOf rdf:nodeID="N24d4a70633254cde8cce24b89961d3ed"/>
    <annotations:EMMO_967080e5_2f42_4eb2_a3a9_c58143e835f9>The basic constituent of 'item'-s that can be proper partitioned only in time up to quantum level.</annotations:EMMO_967080e5_2f42_4eb2_a3a9_c58143e835f9>
    <rdfs:label xml:lang="en">Elementary</rdfs:label>
    <rdfs:comment>According to mereology, this should be call 'a-tomistic' in the strict etimological sense of the word (from greek, a-tomos: un-divisible).

Mereology based on such items is called atomistic mereology.

However, in order not to confuse the lexicon between mereology and physics (in which an atom is a divisible physical entity) we prefer to call it 'elementary', recalling the concept of elementary particle coming from the standard particles model.</rdfs:comment>
    <rdfs:subClassOf rdf:resource="http://emmo.info/emmo/top/physical#EMMO_c5ddfdba_c074_4aa4_ad6b_1ac4942d300d"/>
    <rdfs:subClassOf rdf:nodeID="N9b878e0544774f0891c985bb6e271b41"/>
  </rdf:Description>
  <rdf:Description rdf:nodeID="N4095aedf52d04df2bc91e56df0df5082">
    <owl:intersectionOf rdf:nodeID="Naaf7bd1e64944343a2135c509a123c78"/>
    <rdf:type rdf:resource="http://www.w3.org/2002/07/owl#Class"/>
  </rdf:Description>
  <rdf:Description rdf:about="http://emmo.info/emmo/middle/manufacturing#EMMO_494b372c_cfdf_47d3_a4de_5e037c540de8">
    <rdfs:label xml:lang="en">Component</rdfs:label>
    <rdfs:subClassOf rdf:resource="http://emmo.info/emmo/middle/manufacturing#EMMO_86ca9b93_1183_4b65_81b8_c0fcd3bba5ad"/>
    <rdf:type rdf:resource="http://www.w3.org/2002/07/owl#Class"/>
  </rdf:Description>
  <rdf:Description rdf:about="http://emmo.info/emmo/middle/siunits#EMMO_1181c938_c8f0_4ad6_bc7a_2bfdc0903d29">
    <rdf:type rdf:resource="http://www.w3.org/2002/07/owl#Class"/>
    <rdfs:subClassOf rdf:nodeID="N4835458880484492b1ef37e8b593170d"/>
    <rdfs:label xml:lang="en">Deci</rdfs:label>
    <rdfs:subClassOf rdf:nodeID="Nde6a077c3384417cb16017b6927a6b7f"/>
  </rdf:Description>
  <rdf:Description rdf:nodeID="N7399485b66c64646930294c7d1f94051">
    <owl:onProperty rdf:nodeID="N113f27dc3fa64f50870b640e81e7ce38"/>
    <rdf:type rdf:resource="http://www.w3.org/2002/07/owl#Restriction"/>
    <owl:someValuesFrom rdf:resource="http://emmo.info/emmo/top/semiotics#EMMO_008fd3b2_4013_451f_8827_52bceab11841"/>
  </rdf:Description>
  <rdf:Description rdf:nodeID="Nc8ceec78b7c34557ad09cba8ba08140b">
    <rdf:first rdf:resource="http://emmo.info/emmo/middle/metrology#EMMO_b081b346_7279_46ef_9a3d_2c088fcd79f4"/>
    <rdf:rest rdf:nodeID="Nc56415c15ad4485a855b6512b6c96e65"/>
  </rdf:Description>
  <rdf:Description rdf:about="http://emmo.info/emmo/middle/isq#EMMO_99dba333_0dbd_4f75_8841_8c0f97fd58e2">
    <rdfs:subClassOf rdf:resource="http://emmo.info/emmo/middle/isq#EMMO_2946d40b_24a1_47fa_8176_e3f79bb45064"/>
    <rdfs:label>Capacitance</rdfs:label>
    <annotations:EMMO_6dd685dd_1895_46e4_b227_be9f7d643c25>http://dbpedia.org/page/Capacitance</annotations:EMMO_6dd685dd_1895_46e4_b227_be9f7d643c25>
    <rdf:type rdf:resource="http://www.w3.org/2002/07/owl#Class"/>
    <annotations:EMMO_fe015383_afb3_44a6_ae86_043628697aa2>https://doi.org/10.1351/goldbook.C00791</annotations:EMMO_fe015383_afb3_44a6_ae86_043628697aa2>
    <annotations:EMMO_21ae69b4_235e_479d_8dd8_4f756f694c1b xml:lang="en">ElectricCapacitance</annotations:EMMO_21ae69b4_235e_479d_8dd8_4f756f694c1b>
    <annotations:EMMO_967080e5_2f42_4eb2_a3a9_c58143e835f9>The derivative of the electric charge of a system with respect to the electric potential.</annotations:EMMO_967080e5_2f42_4eb2_a3a9_c58143e835f9>
    <rdfs:subClassOf rdf:nodeID="N4c56b3950488404da9ea7b4ae9d219a4"/>
  </rdf:Description>
  <rdf:Description rdf:about="http://emmo.info/emmo/middle/physicalistic#EMMO_c26a0340_d619_4928_b1a1_1a04e88bb89d">
    <rdfs:subClassOf rdf:resource="http://emmo.info/emmo/middle/physicalistic#EMMO_98ada9d8_f1c8_4f13_99b5_d890f5354152"/>
    <rdfs:comment>Only a subset of elementary particles from the Standard Model are here included for the sake of simplicity.</rdfs:comment>
    <rdfs:label xml:lang="en">ElementaryParticle</rdfs:label>
    <annotations:EMMO_967080e5_2f42_4eb2_a3a9_c58143e835f9>The union of all classes categorizing elementary particles according to the Standard Model.</annotations:EMMO_967080e5_2f42_4eb2_a3a9_c58143e835f9>
    <rdfs:subClassOf rdf:resource="http://emmo.info/emmo/top/physical#EMMO_0f795e3e_c602_4577_9a43_d5a231aa1360"/>
    <owl:disjointUnionOf rdf:nodeID="N6b84e1de4b304453ba61e135e3e7be61"/>
    <rdf:type rdf:resource="http://www.w3.org/2002/07/owl#Class"/>
  </rdf:Description>
  <rdf:Description rdf:about="http://emmo.info/emmo/middle/properties#EMMO_b7bcff25_ffc3_474e_9ab5_01b1664bd4ba">
    <annotations:EMMO_b432d2d5_25f4_4165_99c5_5935a7763c1a>Hardness is a subclass of properties.

Vickers hardness is a subclass of hardness that involves the procedures and instruments defined by the standard hardness test.</annotations:EMMO_b432d2d5_25f4_4165_99c5_5935a7763c1a>
    <rdfs:label xml:lang="en">Property</rdfs:label>
    <owl:disjointUnionOf rdf:nodeID="N14380958a6f14b4a956fed9d59ba6227"/>
    <rdfs:comment>A 'Property' is a sort of name or label that we put upon objects that interact with an observer in the same specific way.

e.g. "hot" objects are objects that interact with an observer through a perception mechanism aimed to perceive an heat source.</rdfs:comment>
    <rdfs:comment>We know real world entities through observation/perception.

A non-perceivable real world entity does not exist (or it exists on a plane of existance that has no intersection with us and we can say nothing about it).

Perception/observation of a real wolrd entity occurs when the entity stimulate an observer in a peculiar way through a well defined perception channel.

For this reason each property is related to a specific observation process which involves a specific observer with its own perception mechanisms.

The observation process (e.g. a look, a photo shot, a measurement) is performed  by an observer (e.g. you, a camera, an instrument) through a specific perception mechanism (e.g. retina impression, CMOS excitation, piezoelectric sensor activation) and involves an observed entity.

An observation is a semiotic process, since it stimulate an interpretant within the interpreter who can communicate the perception result to other interpreters through a sign which is the property. 

Property subclasses are specializations that depend on the type of observation processes.

e.g. the property 'colour' is related to a process that involves emission or interaction of photon and an observer who can perceive electromagnetic radiation in the visible frequency range. 

Properties usually relies on symbolic systems (e.g. for colour it can be palette or RGB).</rdfs:comment>
    <annotations:EMMO_967080e5_2f42_4eb2_a3a9_c58143e835f9>A 'Perceptual' referring to a specific code that is used as 'Conventional' sign to represent an 'Object' according to a specific interaction mechanism by an 'Observer'.

(A property is always a partial representation of an 'Object' since it reflects the 'Object' capability to be part of a specific 'Observation' process)</annotations:EMMO_967080e5_2f42_4eb2_a3a9_c58143e835f9>
    <rdfs:subClassOf rdf:nodeID="Nafb46c4d4e1b4a4da33513592ab4a5b7"/>
    <rdfs:subClassOf rdf:resource="http://emmo.info/emmo/top/semiotics#EMMO_35d2e130_6e01_41ed_94f7_00b333d46cf9"/>
    <annotations:EMMO_b432d2d5_25f4_4165_99c5_5935a7763c1a>Let's define the class 'colour' as the subclass of the properties that involve photon emission and an electromagnetic radiation sensible observer.

An individual C of this class 'colour' can be defined be declaring the process individual (e.g. daylight illumination) and the observer (e.g. my eyes)

Stating that an entity E has_property C, we mean that it can be observed by such setup of process + observer (i.e. observed by my eyes under daylight).

This definition can be generalized by using a generic human eye, so that the observer can be a generic human.

This can be used in material characterization, to define exactly the type of measurement done, including the instrument type.</annotations:EMMO_b432d2d5_25f4_4165_99c5_5935a7763c1a>
    <rdfs:subClassOf rdf:nodeID="N7646f8bfc869439c860c29919e135854"/>
    <rdf:type rdf:resource="http://www.w3.org/2002/07/owl#Class"/>
  </rdf:Description>
  <rdf:Description rdf:about="http://emmo.info/emmo/middle/isq#EMMO_af24ae20_8ef2_435a_86a1_2ea44488b318">
    <owl:equivalentClass rdf:nodeID="N6b686c46525440a1967ecf97244e5e77"/>
    <rdf:type rdf:resource="http://www.w3.org/2002/07/owl#Class"/>
    <rdfs:label xml:lang="en">PerAmountDimension</rdfs:label>
    <rdfs:subClassOf rdf:resource="http://emmo.info/emmo/middle/metrology#EMMO_9895a1b4_f0a5_4167_ac5e_97db40b8bfcc"/>
  </rdf:Description>
  <rdf:Description rdf:nodeID="Ne508bc5d17764bdc87f1c51a81f2f5f1">
    <rdf:type rdf:resource="http://www.w3.org/2002/07/owl#Restriction"/>
    <owl:allValuesFrom rdf:nodeID="N2b6ff0bf8f9f4473ae4fa0048f26c08e"/>
    <owl:onProperty rdf:nodeID="N3069614749b14a9d8d6c9d9b899f09ff"/>
  </rdf:Description>
  <rdf:Description rdf:about="http://emmo.info/emmo/top/physical#EMMO_6e046dd0_9634_4013_b2b1_9cc468087c83">
    <rdfs:domain rdf:resource="http://emmo.info/emmo/top/mereotopology#EMMO_eb3a768e_d53e_4be9_a23b_0714833c36de"/>
    <rdfs:subPropertyOf rdf:resource="http://emmo.info/emmo/top/mereotopology#EMMO_9380ab64_0363_4804_b13f_3a8a94119a76"/>
    <rdf:type rdf:resource="http://www.w3.org/2002/07/owl#TransitiveProperty"/>
    <rdfs:range rdf:resource="http://emmo.info/emmo/top/mereotopology#EMMO_eb3a768e_d53e_4be9_a23b_0714833c36de"/>
    <rdf:type rdf:resource="http://www.w3.org/2002/07/owl#ObjectProperty"/>
    <annotations:EMMO_967080e5_2f42_4eb2_a3a9_c58143e835f9>A relation that isolates a proper part that extends itself in time through a portion of the lifetime whole.</annotations:EMMO_967080e5_2f42_4eb2_a3a9_c58143e835f9>
    <rdfs:label xml:lang="en">hasSpatioTemporalPart</rdfs:label>
  </rdf:Description>
  <rdf:Description rdf:about="http://emmo.info/emmo/top/math#EMMO_46d5643b_9706_4b67_8bea_ed77d6026539">
    <owl:equivalentClass rdf:nodeID="Na563f81676d04624a4f83ce0ccd7fe4b"/>
    <rdf:type rdf:resource="http://www.w3.org/2002/07/owl#Class"/>
    <rdfs:label xml:lang="en">Minus</rdfs:label>
    <rdfs:subClassOf rdf:resource="http://emmo.info/emmo/middle/math#EMMO_707f0cd1_941c_4b57_9f20_d0ba30cd6ff3"/>
  </rdf:Description>
  <rdf:Description rdf:nodeID="N1aceac02b7f945729f6c0b4fa2353131">
    <rdf:type rdf:resource="http://www.w3.org/2002/07/owl#Restriction"/>
    <owl:allValuesFrom rdf:resource="http://emmo.info/emmo/middle/isq#EMMO_515b5579_d526_4842_9e6f_ecc34db6f368"/>
    <owl:onProperty rdf:resource="http://emmo.info/emmo/middle/metrology#EMMO_bed1d005_b04e_4a90_94cf_02bc678a8569"/>
  </rdf:Description>
  <rdf:Description rdf:nodeID="N25671ebd88ad433baec77dc111e89a0a">
    <owl:onProperty rdf:resource="http://emmo.info/emmo/middle/math#EMMO_faf79f53_749d_40b2_807c_d34244c192f4"/>
    <rdf:type rdf:resource="http://www.w3.org/2002/07/owl#Restriction"/>
    <owl:hasValue rdf:datatype="http://www.w3.org/2001/XMLSchema#decimal">1E-15</owl:hasValue>
  </rdf:Description>
  <rdf:Description rdf:nodeID="N3b0b6b1778114e2db7c2eb96c28e114e">
    <owl:allValuesFrom rdf:nodeID="N4f6455f2d9ff4404be2e63ed1f6f0010"/>
    <owl:onProperty rdf:nodeID="N0372fdc726bb4e2e845aeb7ec549ba03"/>
    <rdf:type rdf:resource="http://www.w3.org/2002/07/owl#Restriction"/>
  </rdf:Description>
  <rdf:Description rdf:nodeID="Nd33f7cbb853c4818be8efc5da9a9e643">
    <owl:onProperty rdf:resource="http://emmo.info/emmo/middle/metrology#EMMO_bed1d005_b04e_4a90_94cf_02bc678a8569"/>
    <owl:allValuesFrom rdf:resource="http://emmo.info/emmo/middle/isq#EMMO_e501069c_34d3_4dc7_ac87_c90c7342192b"/>
    <rdf:type rdf:resource="http://www.w3.org/2002/07/owl#Restriction"/>
  </rdf:Description>
  <rdf:Description rdf:about="http://emmo.info/emmo/middle/isq#EMMO_e2ee1c98_497a_4f66_b4ed_5711496a848e">
    <annotations:EMMO_6dd685dd_1895_46e4_b227_be9f7d643c25>http://dbpedia.org/page/Luminous_flux</annotations:EMMO_6dd685dd_1895_46e4_b227_be9f7d643c25>
    <rdfs:subClassOf rdf:resource="http://emmo.info/emmo/middle/isq#EMMO_2946d40b_24a1_47fa_8176_e3f79bb45064"/>
    <rdfs:subClassOf rdf:nodeID="N99998ece68384c6fb2dc4dd9e602aa19"/>
    <annotations:EMMO_fe015383_afb3_44a6_ae86_043628697aa2>https://doi.org/10.1351/goldbook.L03646</annotations:EMMO_fe015383_afb3_44a6_ae86_043628697aa2>
    <rdfs:label xml:lang="en">LuminousFlux</rdfs:label>
    <rdf:type rdf:resource="http://www.w3.org/2002/07/owl#Class"/>
    <annotations:EMMO_967080e5_2f42_4eb2_a3a9_c58143e835f9>Perceived power of light.</annotations:EMMO_967080e5_2f42_4eb2_a3a9_c58143e835f9>
  </rdf:Description>
  <rdf:Description rdf:nodeID="N9532ecf9be7545d4a02cd7acf91cb0d1">
    <owl:onProperty rdf:nodeID="N51d47e9a766f467996c89519b4eb6a3f"/>
    <rdf:type rdf:resource="http://www.w3.org/2002/07/owl#Restriction"/>
    <owl:hasValue rdf:resource="http://emmo.info/emmo/top/mereotopology#EMMO_08cb807c_e626_447b_863f_e2835540e918"/>
  </rdf:Description>
  <rdf:Description rdf:about="http://emmo.info/emmo/top/semiotics#EMMO_b21a56ed_f969_4612_a6ec_cb7766f7f31d">
    <owl:equivalentClass rdf:nodeID="N8113dcfa51e747fd9fa006baadfd8b5c"/>
    <rdfs:label xml:lang="en">Sign</rdfs:label>
    <rdfs:comment>According to Peirce, 'Sign' includes three subcategories:
- symbols: that stand for an object through convention
- indeces: that stand for an object due to causal continguity
- icon: that stand for an object due to similitudes e.g. in shape or composition</rdfs:comment>
    <rdf:type rdf:resource="http://www.w3.org/2002/07/owl#Class"/>
    <rdfs:comment>A 'Sign' can have temporal-direct-parts which are 'Sign' themselves.

A 'Sign' usually have 'sign' spatial direct parts only up to a certain elementary semiotic level, in which the part is only a 'Physical' and no more a 'Sign' (i.e. it stands for nothing). This elementary semiotic level is peculiar to each particular system of signs (e.g. text, painting).

Just like an 'Elementary' in the 'Physical' branch, each 'Sign' branch should have an a-tomistic mereological part.</rdfs:comment>
    <annotations:EMMO_b432d2d5_25f4_4165_99c5_5935a7763c1a>A novel is made of chapters, paragraphs, sentences, words and characters (in a direct parthood mereological hierarchy). 

Each of them are 'sign'-s. 

A character can be the a-tomistic 'sign' for the class of texts.

The horizontal segment in the character "A" is direct part of "A" but it is not a 'sign' itself.

For plain text we can propose the ASCII symbols, for math the fundamental math symbols.</annotations:EMMO_b432d2d5_25f4_4165_99c5_5935a7763c1a>
    <rdfs:subClassOf rdf:resource="http://emmo.info/emmo/top/semiotics#EMMO_b803f122_4acb_4064_9d71_c1e5fd091fc9"/>
    <annotations:EMMO_967080e5_2f42_4eb2_a3a9_c58143e835f9>An 'Physical' that is used as sign ("semeion" in greek) that stands for another 'Physical' through an semiotic process.</annotations:EMMO_967080e5_2f42_4eb2_a3a9_c58143e835f9>
  </rdf:Description>
  <rdf:Description rdf:nodeID="N53581bc42da74f169fddf12dbc5613b9">
    <owl:onProperty rdf:resource="http://emmo.info/emmo/middle/metrology#EMMO_bed1d005_b04e_4a90_94cf_02bc678a8569"/>
    <owl:someValuesFrom rdf:resource="http://emmo.info/emmo/middle/isq#EMMO_d5f3e0e5_fc7d_4e64_86ad_555e74aaff84"/>
    <rdf:type rdf:resource="http://www.w3.org/2002/07/owl#Restriction"/>
  </rdf:Description>
  <rdf:Description rdf:about="http://emmo.info/emmo/middle/isq#EMMO_04cc9451_5306_45d0_8554_22cee4d6e785">
    <rdfs:subClassOf rdf:nodeID="N8f32255d2f144776a067f6993b2ba743"/>
    <annotations:EMMO_6dd685dd_1895_46e4_b227_be9f7d643c25>http://dbpedia.org/page/Inductance</annotations:EMMO_6dd685dd_1895_46e4_b227_be9f7d643c25>
    <rdfs:subClassOf rdf:resource="http://emmo.info/emmo/middle/isq#EMMO_2946d40b_24a1_47fa_8176_e3f79bb45064"/>
    <annotations:EMMO_967080e5_2f42_4eb2_a3a9_c58143e835f9>A property of an electrical conductor by which a change in current through it induces an electromotive force in both the conductor itself and in any nearby conductors by mutual inductance.</annotations:EMMO_967080e5_2f42_4eb2_a3a9_c58143e835f9>
    <annotations:EMMO_21ae69b4_235e_479d_8dd8_4f756f694c1b xml:lang="en">ElectricInductance</annotations:EMMO_21ae69b4_235e_479d_8dd8_4f756f694c1b>
    <rdf:type rdf:resource="http://www.w3.org/2002/07/owl#Class"/>
    <annotations:EMMO_fe015383_afb3_44a6_ae86_043628697aa2>https://doi.org/10.1351/goldbook.M04076</annotations:EMMO_fe015383_afb3_44a6_ae86_043628697aa2>
    <rdfs:label>Inductance</rdfs:label>
  </rdf:Description>
  <rdf:Description rdf:about="http://emmo.info/emmo/middle/siunits#EMMO_23bfe79a_cade_48f1_9a8c_fd96e6bac8ba">
    <rdfs:subClassOf rdf:nodeID="N2c32ed7dff6749b8ae940356bfebdf51"/>
    <rdfs:label xml:lang="en">Femto</rdfs:label>
    <rdf:type rdf:resource="http://www.w3.org/2002/07/owl#Class"/>
    <rdfs:subClassOf rdf:nodeID="N66868a39fbab416e875d20a8ccac083f"/>
  </rdf:Description>
  <rdf:Description rdf:about="http://emmo.info/emmo/middle/isq#EMMO_e501069c_34d3_4dc7_ac87_c90c7342192b">
    <rdf:type rdf:resource="http://www.w3.org/2002/07/owl#Class"/>
    <rdfs:label xml:lang="en">AmountDimension</rdfs:label>
    <owl:equivalentClass rdf:nodeID="Nce6bc7ace0de4e30b405b420c47ce199"/>
    <rdfs:subClassOf rdf:resource="http://emmo.info/emmo/middle/metrology#EMMO_9895a1b4_f0a5_4167_ac5e_97db40b8bfcc"/>
  </rdf:Description>
  <rdf:Description rdf:about="http://emmo.info/emmo/middle/metrology#EMMO_9895a1b4_f0a5_4167_ac5e_97db40b8bfcc">
    <rdfs:comment>The conventional symbolic representation of the dimension of a base quantity is a single upper case letter in roman (upright) type. The conventional symbolic representation of the dimension of a derived quantity is the product of powers of the dimensions of the base quantities according to the definition of the derived quantity. The dimension of a quantity Q is denoted by dim Q.
ISO 80000-1</rdfs:comment>
    <rdfs:comment>All physical quantities, with the exception of counts, are derived quantities, which may be written in terms of base quantities according to the equations of physics. The dimensions of the derived quantities are written as products of powers of the dimensions of the base quantities using the equations that relate the derived quantities to the base quantities.
In general the dimension of any quantity Q is written in the form of a dimensional product,

dim Q = T^α L^β M^γ I^δ Θ^ε N^ζ J^η

where the exponents α, β, γ, δ, ε, ζ and η, which are generally small integers, which can be positive, negative, or zero, are called the dimensional exponents.
(SI brochure)</rdfs:comment>
    <rdfs:subClassOf rdf:resource="http://emmo.info/emmo/middle/perceptual#EMMO_a1083d0a_c1fb_471f_8e20_a98f881ad527"/>
    <rdfs:subClassOf rdf:resource="http://emmo.info/emmo/middle/metrology#EMMO_985bec21_989f_4b9e_a4b3_735d88099c3c"/>
    <rdf:type rdf:resource="http://www.w3.org/2002/07/owl#Class"/>
    <annotations:EMMO_967080e5_2f42_4eb2_a3a9_c58143e835f9>A symbol that, following SI specifications, describe the physical dimensionality of a physical quantity and the exponents of the base units in a measurement unit.</annotations:EMMO_967080e5_2f42_4eb2_a3a9_c58143e835f9>
    <rdfs:comment>The expression used by the EMMO for physical dimensions is a metrological symbol (but a string at meta level, i.e. the ontologist level) like this:
 
Ta Lb Mc Id Θe Nf Jg

where a, b, c, d, e, f and g are 0 or signed integers.

Regex for the physical dimension symbol for the EMMO is:
^T([+-][1-9]|0) L([+-][1-9]|0) M([+-][1-9]|0) I([+-][1-9]|0) Θ([+-][1-9]|0) N([+-][1-9]|0) J([+-][1-9]|0)$

Examples of correspondance between base units and physical dimensions are:
mol -&gt; T0 L0 M0 I0 Θ0 N+1 J0
s -&gt; T+1 L0 M0 I0 Θ0 N0 J0
A/m2 -&gt; T0 L0 M-2 I+1 Θ0 N0 J0</rdfs:comment>
    <rdfs:label xml:lang="en">PhysicsDimension</rdfs:label>
  </rdf:Description>
  <rdf:Description rdf:about="http://emmo.info/emmo/middle/holistic#EMMO_43e9a05d_98af_41b4_92f6_00f79a09bfce">
    <rdfs:comment>A 'Process' is defined as a temporal part of a 'Physical' that is categorized according to an EMMO user that recognizes a particular type of evolution in time of the real world object.

Following the common definition of process, every 'Physical' should be a process, since every 4D object always has a time dimension. 

However, in the EMMO we restrict the meaning of the word process to 'Physical'-s whose evolution in time have a particular meaning for the ontologist.

A 'Process' is not only something that unfolds in time (which is automatically represented in a 4D ontology), but something that has a meaning for the ontologist, i.e. that the ontologist can separate from the rest of the 4D physical for any reason.</rdfs:comment>
    <rdfs:subClassOf rdf:resource="http://emmo.info/emmo/top/physical#EMMO_c5ddfdba_c074_4aa4_ad6b_1ac4942d300d"/>
    <rdfs:comment>A 'Process' is always a 'Physical', since a 'Void' does not have elements that evolves in time.</rdfs:comment>
    <rdfs:label xml:lang="en">Process</rdfs:label>
    <annotations:EMMO_967080e5_2f42_4eb2_a3a9_c58143e835f9>A temporal part of a 'physical' that identifies a particular type of evolution in time.</annotations:EMMO_967080e5_2f42_4eb2_a3a9_c58143e835f9>
    <rdfs:subClassOf rdf:nodeID="N1e20041fd38a43e8803e2aac0362f92c"/>
    <rdf:type rdf:resource="http://www.w3.org/2002/07/owl#Class"/>
  </rdf:Description>
  <rdf:Description rdf:nodeID="N1fb591fb5bbc4aacbf6a96c5916dfb32">
    <owl:inverseOf rdf:resource="http://emmo.info/emmo/middle/math#EMMO_3446e167_c576_49d6_846c_215bb8878a55"/>
  </rdf:Description>
  <rdf:Description rdf:nodeID="N526846521e6b4ec1a49a311418e1f8a2">
    <rdf:rest rdf:nodeID="Ne67ff9d6048a4e718a218eb4eec16e30"/>
    <rdf:first rdf:resource="http://emmo.info/emmo/middle/siunits#EMMO_9ff3bf8e_2168_406e_8251_1d158fc948ae"/>
  </rdf:Description>
  <rdf:Description rdf:about="http://emmo.info/emmo/middle/math#EMMO_d1d436e7_72fc_49cd_863b_7bfb4ba5276a">
    <annotations:EMMO_b432d2d5_25f4_4165_99c5_5935a7763c1a>viscosity in the Navier-Stokes equation</annotations:EMMO_b432d2d5_25f4_4165_99c5_5935a7763c1a>
    <rdf:type rdf:resource="http://www.w3.org/2002/07/owl#Class"/>
    <rdfs:subClassOf rdf:resource="http://emmo.info/emmo/middle/math#EMMO_1eed0732_e3f1_4b2c_a9c4_b4e75eeb5895"/>
    <rdfs:label xml:lang="en">Parameter</rdfs:label>
    <rdfs:comment>A 'variable' whose value is assumed to be known independently from the equation, but whose value is not explicitated in the equation.</rdfs:comment>
  </rdf:Description>
  <rdf:Description rdf:about="http://emmo.info/emmo/middle/physicalistic#EMMO_5b2222df_4da6_442f_8244_96e9e45887d1">
    <rdfs:subClassOf rdf:nodeID="Nd7285b7a5e214991b0a5178caf6dd4a9"/>
    <annotations:EMMO_967080e5_2f42_4eb2_a3a9_c58143e835f9>A 'Physical' that possesses some 'Massive' parts.</annotations:EMMO_967080e5_2f42_4eb2_a3a9_c58143e835f9>
    <rdfs:label xml:lang="en">Matter</rdfs:label>
    <rdfs:subClassOf rdf:resource="http://emmo.info/emmo/top/physical#EMMO_c5ddfdba_c074_4aa4_ad6b_1ac4942d300d"/>
    <rdfs:subClassOf rdf:nodeID="N468c5596198c4b6fb957712bbc98b19b"/>
    <rdf:type rdf:resource="http://www.w3.org/2002/07/owl#Class"/>
  </rdf:Description>
  <rdf:Description rdf:nodeID="Nac818dfa7e4442939688b1ec1fe07bd3">
    <rdf:type rdf:resource="http://www.w3.org/2002/07/owl#Restriction"/>
    <owl:hasValue>µ</owl:hasValue>
    <owl:onProperty rdf:resource="http://emmo.info/emmo/middle/perceptual#EMMO_23b579e1_8088_45b5_9975_064014026c42"/>
  </rdf:Description>
  <rdf:Description rdf:about="http://emmo.info/emmo/middle/siunits#EMMO_1273eb34_de48_43a9_925f_104110469dd2">
    <rdfs:label xml:lang="en">SICoherentDerivedUnit</rdfs:label>
    <rdf:type rdf:resource="http://www.w3.org/2002/07/owl#Class"/>
    <rdfs:comment>This class collects all units that are products or powers of SI base or SI special units only.</rdfs:comment>
    <annotations:EMMO_b432d2d5_25f4_4165_99c5_5935a7763c1a>m/s
kg/m^3</annotations:EMMO_b432d2d5_25f4_4165_99c5_5935a7763c1a>
    <annotations:EMMO_967080e5_2f42_4eb2_a3a9_c58143e835f9>A SI derived unit whos numerical factor in front of the product of SI base units is one.</annotations:EMMO_967080e5_2f42_4eb2_a3a9_c58143e835f9>
  </rdf:Description>
  <rdf:Description rdf:about="http://emmo.info/emmo/middle/metrology#EMMO_868ae137_4d25_493e_b270_21ea3d94849e">
    <rdf:type rdf:resource="http://www.w3.org/2002/07/owl#Class"/>
    <rdfs:label xml:lang="en">NonPrefixedUnit</rdfs:label>
    <owl:equivalentClass rdf:nodeID="N40b9ddd8943b45d2b252e96f8efb76ec"/>
    <annotations:EMMO_967080e5_2f42_4eb2_a3a9_c58143e835f9>A measurement unit symbol that do not have a metric prefix as a direct spatial part.</annotations:EMMO_967080e5_2f42_4eb2_a3a9_c58143e835f9>
    <rdfs:subClassOf rdf:nodeID="N01f6e7f45ccf44fdb5457f6f651bdc87"/>
  </rdf:Description>
  <rdf:Description rdf:nodeID="Ndef00d53241c45889cfebd5f75c1cca5">
    <owl:hasValue>Hz</owl:hasValue>
    <owl:onProperty rdf:resource="http://emmo.info/emmo/middle/perceptual#EMMO_23b579e1_8088_45b5_9975_064014026c42"/>
    <rdf:type rdf:resource="http://www.w3.org/2002/07/owl#Restriction"/>
  </rdf:Description>
  <rdf:Description rdf:about="http://emmo.info/emmo/middle/isq#EMMO_b3600e73_3e05_479d_9714_c041c3acf5cc">
    <rdf:type rdf:resource="http://www.w3.org/2002/07/owl#Class"/>
    <owl:equivalentClass rdf:nodeID="N065b4557f65a4e27a869fd1830526f2d"/>
    <rdfs:label xml:lang="en">LengthDimension</rdfs:label>
    <rdfs:subClassOf rdf:resource="http://emmo.info/emmo/middle/metrology#EMMO_9895a1b4_f0a5_4167_ac5e_97db40b8bfcc"/>
  </rdf:Description>
  <rdf:Description rdf:about="http://emmo.info/emmo/middle/isq#EMMO_585e0ff0_9429_4d3c_b578_58abb1ba21d1">
    <rdf:type rdf:resource="http://www.w3.org/2002/07/owl#Class"/>
    <rdfs:subClassOf rdf:resource="http://emmo.info/emmo/middle/metrology#EMMO_9895a1b4_f0a5_4167_ac5e_97db40b8bfcc"/>
    <owl:equivalentClass rdf:nodeID="N45e6caad3f22412782ccadaba0a54db5"/>
    <rdfs:label xml:lang="en">MassSquareLengthPerSquareTimeSquareCurrentDimension</rdfs:label>
  </rdf:Description>
  <rdf:Description rdf:nodeID="N1e20041fd38a43e8803e2aac0362f92c">
    <owl:onProperty rdf:resource="http://emmo.info/emmo/middle/holistic#EMMO_ae2d1a96_bfa1_409a_a7d2_03d69e8a125a"/>
    <owl:someValuesFrom rdf:resource="http://emmo.info/emmo/middle/holistic#EMMO_49804605_c0fe_4538_abda_f70ba1dc8a5d"/>
    <rdf:type rdf:resource="http://www.w3.org/2002/07/owl#Restriction"/>
  </rdf:Description>
  <rdf:Description rdf:about="http://emmo.info/emmo/top/mereotopology#EMMO_3f9ae00e_810c_4518_aec2_7200e424cf68">
    <rdfs:label xml:lang="en">Quantum</rdfs:label>
    <rdfs:subClassOf rdf:resource="http://emmo.info/emmo/top/mereotopology#EMMO_802d3e92_8770_4f98_a289_ccaaab7fdddf"/>
    <rdfs:comment>A 'Quantum' is the most fundamental subclass of 'Item', since its individuals stand for the smallest possible self-connected 4D real world objects.

The quantum concept recalls the fact that there is lower epistemological limit to our knowledge of the universe, related to the uncertainity principle.</rdfs:comment>
    <annotations:EMMO_967080e5_2f42_4eb2_a3a9_c58143e835f9>The class of 'EMMO' individuals that stand for real world objects that can't be further divided in time nor in space.</annotations:EMMO_967080e5_2f42_4eb2_a3a9_c58143e835f9>
    <annotations:EMMO_b432d2d5_25f4_4165_99c5_5935a7763c1a>For a physics based ontology the 'Quantum' can stand for the smallest identifiable portion of spacetime defined by the Planck limit in length (1.616e-35 m) and time (5.39e-44 s).

However, the quantum mereotopology approach is not restricted only to physics. For example, in a manpower management ontology, a 'Quantum' can stand for an hour (time) of a worker (space) activity.</annotations:EMMO_b432d2d5_25f4_4165_99c5_5935a7763c1a>
    <rdfs:comment>A 'Quantum' stands for a 4D real world object.</rdfs:comment>
    <rdfs:comment>From Latin quantum (plural quanta) "as much as, so much as;", introduced in physics directly from Latin by Max Planck, 1900.</rdfs:comment>
    <rdfs:subClassOf rdf:nodeID="N62ce9418bd634c4f9d45bfcabeb4e5ea"/>
    <rdf:type rdf:resource="http://www.w3.org/2002/07/owl#Class"/>
    <rdfs:comment>A quantum is the EMMO mereological 4D a-tomic entity. 

To avoid confusion with the concept of atom coming from physics, we will use the expression quantum mereology, instead of a-tomistic mereology.</rdfs:comment>
  </rdf:Description>
  <rdf:Description rdf:about="http://emmo.info/emmo/middle/perceptual#EMMO_c74da218_9147_4f03_92d1_8894abca55f3">
    <rdf:type rdf:resource="http://www.w3.org/2002/07/owl#Class"/>
    <annotations:EMMO_b432d2d5_25f4_4165_99c5_5935a7763c1a>'Graphical' objects include writings, pictures, sketches ...</annotations:EMMO_b432d2d5_25f4_4165_99c5_5935a7763c1a>
    <rdfs:label xml:lang="en">Graphical</rdfs:label>
    <rdfs:subClassOf rdf:resource="http://emmo.info/emmo/middle/perceptual#EMMO_649bf97b_4397_4005_90d9_219755d92e34"/>
    <annotations:EMMO_967080e5_2f42_4eb2_a3a9_c58143e835f9>A 'Phenomenic' which stands for a real world object whose spatial configuration shows a pattern identifiable by an observer.</annotations:EMMO_967080e5_2f42_4eb2_a3a9_c58143e835f9>
    <rdfs:comment>From the Ancient Greek γραφή (graphḗ) which means drawing, painting, writing, a writing, description, and from γράφω (gráphō) which means scratch, carve.</rdfs:comment>
  </rdf:Description>
  <rdf:Description rdf:nodeID="N0124c3d319bc474fbaebc8b75db26354">
    <owl:hasValue rdf:datatype="http://www.w3.org/2001/XMLSchema#decimal">1E+9</owl:hasValue>
    <rdf:type rdf:resource="http://www.w3.org/2002/07/owl#Restriction"/>
    <owl:onProperty rdf:resource="http://emmo.info/emmo/middle/math#EMMO_faf79f53_749d_40b2_807c_d34244c192f4"/>
  </rdf:Description>
  <rdf:Description rdf:nodeID="Nd040aec6536440d78c935754bfaefe42">
    <rdf:type rdf:resource="http://www.w3.org/2002/07/owl#Restriction"/>
    <owl:onProperty rdf:resource="http://emmo.info/emmo/middle/perceptual#EMMO_23b579e1_8088_45b5_9975_064014026c42"/>
    <owl:hasValue>Δ</owl:hasValue>
  </rdf:Description>
  <rdf:Description rdf:about="http://emmo.info/emmo/middle/properties#EMMO_d8aa8e1f_b650_416d_88a0_5118de945456">
    <annotations:EMMO_967080e5_2f42_4eb2_a3a9_c58143e835f9>A quantitative property attributed by agreement to a quantity for a given purpose.</annotations:EMMO_967080e5_2f42_4eb2_a3a9_c58143e835f9>
    <rdf:type rdf:resource="http://www.w3.org/2002/07/owl#Class"/>
    <rdfs:label xml:lang="en">ConventionalQuantitativeProperty</rdfs:label>
    <annotations:EMMO_b432d2d5_25f4_4165_99c5_5935a7763c1a>The thermal conductivity of a copper sample in my laboratory can be assumed to be the conductivity that appears in the vendor specification. This value has been obtained by measurement of a sample which is not the one I have in my laboratory. This conductivity value is then a conventional quantitiative property assigned to my sample through a semiotic process in which no actual measurement is done by my laboratory.

If I don't believe the vendor, then I can measure the actual thermal conductivity. I then perform a measurement process that semiotically assign another value for the conductivity, which is a measured property, since is part of a measurement process.

Then I have two different physical quantities that are properties thanks to two different semiotic processes.</annotations:EMMO_b432d2d5_25f4_4165_99c5_5935a7763c1a>
    <rdfs:comment>A property that is associated to an object by convention, or assumption.</rdfs:comment>
  </rdf:Description>
  <rdf:Description rdf:about="http://emmo.info/emmo/middle/metrology#EMMO_b953f2b1_c8d1_4dd9_b630_d3ef6580c2bb">
    <owl:disjointUnionOf rdf:nodeID="Nd7a7b34179a04b53907be1ea559379d1"/>
    <rdfs:comment>Physical constants are categorised into "exact" and measured constants. 

With "exact" constants, we refer to physical constants that have an exact numerical value after the revision of the SI system that was enforsed May 2019.</rdfs:comment>
    <rdfs:subClassOf rdf:resource="http://emmo.info/emmo/middle/metrology#EMMO_02c0621e_a527_4790_8a0f_2bb51973c819"/>
    <annotations:EMMO_c84c6752_6d64_48cc_9500_e54a3c34898d>https://en.wikipedia.org/wiki/List_of_physical_constants</annotations:EMMO_c84c6752_6d64_48cc_9500_e54a3c34898d>
    <rdf:type rdf:resource="http://www.w3.org/2002/07/owl#Class"/>
    <rdfs:label xml:lang="en">PhysicalConstant</rdfs:label>
  </rdf:Description>
  <rdf:Description rdf:nodeID="N23bbf465cdd945678455d3c4ec3c7be7">
    <owl:hasValue rdf:datatype="http://www.w3.org/2001/XMLSchema#decimal">1E+18</owl:hasValue>
    <owl:onProperty rdf:resource="http://emmo.info/emmo/middle/math#EMMO_faf79f53_749d_40b2_807c_d34244c192f4"/>
    <rdf:type rdf:resource="http://www.w3.org/2002/07/owl#Restriction"/>
  </rdf:Description>
  <rdf:Description rdf:about="http://emmo.info/emmo/middle/siunits#EMMO_df6eeb01_1b41_4bd8_9257_a04fbd7cf000">
    <rdf:type rdf:resource="http://www.w3.org/2002/07/owl#Class"/>
    <rdfs:label xml:lang="en">Mole</rdfs:label>
    <rdfs:subClassOf rdf:nodeID="Nc7ed46d34d804b27beb568619b3cf87a"/>
    <rdfs:subClassOf rdf:nodeID="N741671a77d5444229032da8cd8d9a51f"/>
    <annotations:EMMO_fe015383_afb3_44a6_ae86_043628697aa2>https://doi.org/10.1351/goldbook.M03980</annotations:EMMO_fe015383_afb3_44a6_ae86_043628697aa2>
    <annotations:EMMO_70fe84ff_99b6_4206_a9fc_9a8931836d84>The mole, symbol mol, is the SI unit of amount of substance. One mole contains exactly 6.022 140 76 × 1023 elementary entities. This number is the fixed numerical value of the Avogadro constant, NA, when expressed in the unit mol−1 and is called the Avogadro number. The amount of substance, symbol n, of a system is a measure of the number of specified elementary entities. An elementary entity may be an atom, a molecule, an ion, an electron, any other particle or specified group of particles.</annotations:EMMO_70fe84ff_99b6_4206_a9fc_9a8931836d84>
    <annotations:EMMO_1f1b164d_ec6a_4faa_8d5e_88bda62316cc>http://qudt.org/vocab/unit/MOL</annotations:EMMO_1f1b164d_ec6a_4faa_8d5e_88bda62316cc>
  </rdf:Description>
  <rdf:Description rdf:nodeID="Nc78a55a5c3fa4ba1accabe4944ff36fc">
    <rdf:first rdf:nodeID="N94a7d318c4e844e89241126779f3fbe2"/>
    <rdf:rest rdf:resource="http://www.w3.org/1999/02/22-rdf-syntax-ns#nil"/>
  </rdf:Description>
  <rdf:Description rdf:about="http://emmo.info/emmo/middle/siunits#EMMO_707c6032_e272_4a20_98b5_d35c4f67be68">
    <rdfs:label xml:lang="en">SICoherentUnit</rdfs:label>
    <owl:disjointUnionOf rdf:nodeID="N2475f955a0604bb3a44aefb2b14741d7"/>
    <rdfs:comment>Derived units are defined as products of powers of the base units. When the numerical factor of this product is one, the derived units are called coherent derived units. The base and coherent derived units of the SI form a coherent set, designated the set of coherent SI units.</rdfs:comment>
    <rdf:type rdf:resource="http://www.w3.org/2002/07/owl#Class"/>
  </rdf:Description>
  <rdf:Description rdf:about="http://emmo.info/emmo/middle/siunits#EMMO_db5dd38d_ac79_4af6_8782_fee7e7150ae8">
    <rdf:type rdf:resource="http://www.w3.org/2002/07/owl#Class"/>
    <rdfs:subClassOf rdf:nodeID="N53581bc42da74f169fddf12dbc5613b9"/>
    <annotations:EMMO_fe015383_afb3_44a6_ae86_043628697aa2>https://doi.org/10.1351/goldbook.A00300</annotations:EMMO_fe015383_afb3_44a6_ae86_043628697aa2>
    <annotations:EMMO_70fe84ff_99b6_4206_a9fc_9a8931836d84>The ampere, symbol A, is the SI unit of electric current. It is defined by taking the fixed numerical value of the elementary charge e to be 1.602176634×10−19 when expressed in the unit C, which is equal to A s, where the second is defined in terms of ∆νCs.</annotations:EMMO_70fe84ff_99b6_4206_a9fc_9a8931836d84>
    <annotations:EMMO_1f1b164d_ec6a_4faa_8d5e_88bda62316cc>http://qudt.org/vocab/unit/A</annotations:EMMO_1f1b164d_ec6a_4faa_8d5e_88bda62316cc>
    <rdfs:label xml:lang="en">Ampere</rdfs:label>
    <rdfs:subClassOf rdf:nodeID="N79b3d7d51d3c48d29e9df6d5271b788f"/>
  </rdf:Description>
  <rdf:Description rdf:nodeID="N222e5af2f44e4d74af40a3d2ebb081c9">
    <owl:onProperty rdf:resource="http://emmo.info/emmo/middle/metrology#EMMO_67fc0a36_8dcb_4ffa_9a43_31074efa3296"/>
    <owl:allValuesFrom rdf:nodeID="N830aa60f0938433590a923e022b588eb"/>
    <rdf:type rdf:resource="http://www.w3.org/2002/07/owl#Restriction"/>
  </rdf:Description>
  <rdf:Description rdf:nodeID="Nbf9fef1365ff4bd2a4e5b151d8fb28b8">
    <rdf:type rdf:resource="http://www.w3.org/2002/07/owl#Restriction"/>
    <owl:hasValue>p</owl:hasValue>
    <owl:onProperty rdf:resource="http://emmo.info/emmo/middle/perceptual#EMMO_23b579e1_8088_45b5_9975_064014026c42"/>
  </rdf:Description>
  <rdf:Description rdf:about="http://emmo.info/emmo/middle/isq#EMMO_c995ae70_3b84_4ebb_bcfc_69e6a281bb88">
    <rdf:type rdf:resource="http://www.w3.org/2002/07/owl#Class"/>
    <annotations:EMMO_967080e5_2f42_4eb2_a3a9_c58143e835f9>A flow of electric charge.</annotations:EMMO_967080e5_2f42_4eb2_a3a9_c58143e835f9>
    <annotations:EMMO_fe015383_afb3_44a6_ae86_043628697aa2>https://doi.org/10.1351/goldbook.E01927</annotations:EMMO_fe015383_afb3_44a6_ae86_043628697aa2>
    <rdfs:subClassOf rdf:nodeID="Nf2164fae98574eaf8712de1fca89fa57"/>
    <rdfs:label xml:lang="en">ElectricCurrent</rdfs:label>
    <annotations:EMMO_6dd685dd_1895_46e4_b227_be9f7d643c25>http://dbpedia.org/page/Electric_current</annotations:EMMO_6dd685dd_1895_46e4_b227_be9f7d643c25>
  </rdf:Description>
  <rdf:Description rdf:about="http://emmo.info/emmo/top/mereotopology#EMMO_08cb807c_e626_447b_863f_e2835540e918">
    <rdfs:label xml:lang="en">Universe</rdfs:label>
    <rdf:type rdf:resource="http://emmo.info/emmo/top/physical#EMMO_c5ddfdba_c074_4aa4_ad6b_1ac4942d300d"/>
    <rdf:type rdf:resource="http://www.w3.org/2002/07/owl#NamedIndividual"/>
  </rdf:Description>
  <rdf:Description rdf:about="http://emmo.info/emmo/top/mereotopology#EMMO_9380ab64_0363_4804_b13f_3a8a94119a76">
    <rdf:type rdf:resource="http://www.w3.org/2002/07/owl#ObjectProperty"/>
    <rdfs:subPropertyOf rdf:resource="http://emmo.info/emmo/top/mereotopology#EMMO_17e27c22_37e1_468c_9dd7_95e137f73e7f"/>
    <rdfs:label xml:lang="en">hasProperPart</rdfs:label>
    <rdf:type rdf:resource="http://www.w3.org/2002/07/owl#TransitiveProperty"/>
  </rdf:Description>
  <rdf:Description rdf:about="http://emmo.info/emmo/top#EMMO_49267eba_5548_4163_8f36_518d65b583f9">
    <rdfs:comment>This class is the practical implementation of the EMMO pluralistic approach for which that only objective categorization is provide by the Universe individual and all the 'Elementary' individuals.

Between these two extremes, there are several subjective ways to categorize real world objects, each one provide under a 'Perspective' subclass.</rdfs:comment>
    <rdf:type rdf:resource="http://www.w3.org/2002/07/owl#Class"/>
    <annotations:EMMO_967080e5_2f42_4eb2_a3a9_c58143e835f9>The class of individuals that stand for real world objects according to a specific representational perspective.</annotations:EMMO_967080e5_2f42_4eb2_a3a9_c58143e835f9>
    <rdfs:label xml:lang="en">Perspective</rdfs:label>
    <rdfs:subClassOf rdf:resource="http://emmo.info/emmo/top/physical#EMMO_c5ddfdba_c074_4aa4_ad6b_1ac4942d300d"/>
  </rdf:Description>
  <rdf:Description rdf:about="http://emmo.info/emmo/middle/isq#EMMO_8159c26a_494b_4fa0_9959_10888f152298">
    <annotations:EMMO_967080e5_2f42_4eb2_a3a9_c58143e835f9>The number of elementary entities present.</annotations:EMMO_967080e5_2f42_4eb2_a3a9_c58143e835f9>
    <annotations:EMMO_fe015383_afb3_44a6_ae86_043628697aa2>https://doi.org/10.1351/goldbook.A00297</annotations:EMMO_fe015383_afb3_44a6_ae86_043628697aa2>
    <rdf:type rdf:resource="http://www.w3.org/2002/07/owl#Class"/>
    <rdfs:label xml:lang="en">AmountOfSubstance</rdfs:label>
    <rdfs:subClassOf rdf:nodeID="N549d45829d5d485291a666a9c86bd1c3"/>
    <annotations:EMMO_6dd685dd_1895_46e4_b227_be9f7d643c25>http://dbpedia.org/page/Amount_of_substance</annotations:EMMO_6dd685dd_1895_46e4_b227_be9f7d643c25>
  </rdf:Description>
  <rdf:Description rdf:about="http://emmo.info/emmo/middle/materials#EMMO_1067b97a_84f8_4d22_8ace_b842b8ce355c">
    <rdfs:subClassOf rdf:resource="http://emmo.info/emmo/middle/materials#EMMO_7d66bde4_b68d_41cc_b5fc_6fd98c5e2ff0"/>
    <annotations:EMMO_967080e5_2f42_4eb2_a3a9_c58143e835f9>A 'spacetime' that stands for a quantum system made of electrons.</annotations:EMMO_967080e5_2f42_4eb2_a3a9_c58143e835f9>
    <rdfs:subClassOf rdf:nodeID="N374b36162464401b92367b3ea76630fc"/>
    <rdfs:label xml:lang="en">ElectronCloud</rdfs:label>
    <rdf:type rdf:resource="http://www.w3.org/2002/07/owl#Class"/>
  </rdf:Description>
  <rdf:Description rdf:about="http://emmo.info/emmo/middle/siunits#EMMO_176cae33_b83e_4cd2_a6bc_281f42f0ccc8">
    <rdf:type rdf:resource="http://www.w3.org/2002/07/owl#Class"/>
    <annotations:EMMO_1f1b164d_ec6a_4faa_8d5e_88bda62316cc>http://physics.nist.gov/cuu/CODATA-Value_AvogadroConstant</annotations:EMMO_1f1b164d_ec6a_4faa_8d5e_88bda62316cc>
    <rdfs:comment>The DBpedia definition (http://dbpedia.org/page/Avogadro_constant) is outdated as May 20, 2019. It is now an exact quantity.</rdfs:comment>
    <rdfs:subClassOf rdf:nodeID="N8c23aba26af14e85906afda01c1d7d50"/>
    <annotations:EMMO_fe015383_afb3_44a6_ae86_043628697aa2>https://doi.org/10.1351/goldbook.A00543</annotations:EMMO_fe015383_afb3_44a6_ae86_043628697aa2>
    <annotations:EMMO_967080e5_2f42_4eb2_a3a9_c58143e835f9>The number of constituent particles, usually atoms or molecules, that are contained in the amount of substance given by one mole.</annotations:EMMO_967080e5_2f42_4eb2_a3a9_c58143e835f9>
    <rdfs:label xml:lang="en">AvogadroConstant</rdfs:label>
    <annotations:EMMO_6dd685dd_1895_46e4_b227_be9f7d643c25>http://dbpedia.org/page/Avogadro_constant</annotations:EMMO_6dd685dd_1895_46e4_b227_be9f7d643c25>
  </rdf:Description>
  <rdf:Description rdf:about="http://emmo.info/emmo/top/annotations#EMMO_cd5fb112_7ee7_4120_a35d_3ca3e6c3f4ab">
    <rdfs:subPropertyOf rdf:resource="http://www.w3.org/2000/01/rdf-schema#comment"/>
    <rdfs:label xml:lang="en">author</rdfs:label>
    <rdf:type rdf:resource="http://www.w3.org/2002/07/owl#AnnotationProperty"/>
  </rdf:Description>
  <rdf:Description rdf:about="http://emmo.info/emmo/top/math#EMMO_048a14e3_65fb_457d_8695_948965c89492">
    <rdf:type rdf:resource="http://www.w3.org/2002/07/owl#Class"/>
    <rdfs:label xml:lang="en">Laplacian</rdfs:label>
    <rdfs:subClassOf rdf:resource="http://emmo.info/emmo/top/math#EMMO_f8a2fe9f_458b_4771_9aba_a50e76afc52d"/>
    <owl:equivalentClass rdf:nodeID="Nd040aec6536440d78c935754bfaefe42"/>
  </rdf:Description>
  <rdf:Description rdf:nodeID="N418e7661e57a442c9ff782b14633557a">
    <owl:qualifiedCardinality rdf:datatype="http://www.w3.org/2001/XMLSchema#nonNegativeInteger">1</owl:qualifiedCardinality>
    <owl:onClass rdf:resource="http://emmo.info/emmo/middle/metrology#EMMO_18ce5200_00f5_45bb_8c6f_6fb128cd41ae"/>
    <owl:onProperty rdf:resource="http://emmo.info/emmo/middle/metrology#EMMO_67fc0a36_8dcb_4ffa_9a43_31074efa3296"/>
    <rdf:type rdf:resource="http://www.w3.org/2002/07/owl#Restriction"/>
  </rdf:Description>
  <rdf:Description rdf:about="http://emmo.info/emmo/top/math#EMMO_3c424d37_cf62_41b1_ac9d_a316f8d113d6">
    <rdfs:subClassOf rdf:resource="http://emmo.info/emmo/top/math#EMMO_f6d0c26a_98b6_4cf8_8632_aa259131faaa"/>
    <rdf:type rdf:resource="http://www.w3.org/2002/07/owl#Class"/>
    <rdfs:label xml:lang="en">AlgebricOperator</rdfs:label>
  </rdf:Description>
  <rdf:Description rdf:about="http://emmo.info/emmo/middle/math#EMMO_f8bd64d5_5d3e_4ad4_a46e_c30714fecb7f">
    <rdfs:label xml:lang="en">Integer</rdfs:label>
    <rdf:type rdf:resource="http://www.w3.org/2002/07/owl#Class"/>
    <rdfs:subClassOf rdf:resource="http://emmo.info/emmo/middle/math#EMMO_21f56795_ee72_4858_b571_11cfaa59c1a8"/>
    <rdfs:subClassOf rdf:nodeID="N4e2d0c6ba942426ab515e2dfcac125e3"/>
    <owl:equivalentClass rdf:nodeID="N83c6e862089248f3ad23c9187e167935"/>
    <rdfs:subClassOf rdf:nodeID="Ne166ae38be13442c98506cbcbf8174f1"/>
  </rdf:Description>
  <rdf:Description rdf:about="http://emmo.info/emmo/middle/math#EMMO_4ce76d7f_03f8_45b6_9003_90052a79bfaa">
    <rdfs:label xml:lang="en">Numerical</rdfs:label>
    <rdfs:subClassOf rdf:resource="http://emmo.info/emmo/middle/math#EMMO_54ee6b5e_5261_44a8_86eb_5717e7fdb9d0"/>
    <annotations:EMMO_967080e5_2f42_4eb2_a3a9_c58143e835f9>A 'Mathematical' that has no unknown value, i.e. all its 'Variable"-s parts refers to a 'Number' (for scalars that have a built-in datatype) or to another 'Numerical' (for complex numerical data structures that should rely on external implementations).</annotations:EMMO_967080e5_2f42_4eb2_a3a9_c58143e835f9>
    <rdf:type rdf:resource="http://www.w3.org/2002/07/owl#Class"/>
  </rdf:Description>
  <rdf:Description rdf:nodeID="N8eff5c0c328c413492051a91bd02c33f">
    <rdf:first rdf:resource="http://emmo.info/emmo/middle/metrology#EMMO_a2f94f33_71fa_443c_a1fb_d1685fc537ec"/>
    <rdf:rest rdf:resource="http://www.w3.org/1999/02/22-rdf-syntax-ns#nil"/>
  </rdf:Description>
  <rdf:Description rdf:nodeID="N7f12189b458b48ada1ac5a4cb869b932">
    <rdf:type rdf:resource="http://www.w3.org/2002/07/owl#Restriction"/>
    <owl:onProperty rdf:resource="http://emmo.info/emmo/middle/metrology#EMMO_67fc0a36_8dcb_4ffa_9a43_31074efa3296"/>
    <owl:allValuesFrom rdf:nodeID="N550fbc468c7b47da84853a777f7be49b"/>
  </rdf:Description>
  <rdf:Description rdf:nodeID="Nb5d10f557dea460fb77939003b6572a7">
    <rdf:type rdf:resource="http://www.w3.org/2002/07/owl#Restriction"/>
    <owl:allValuesFrom rdf:nodeID="N282b8ef379b04a308dc835fbb9941ee7"/>
    <owl:onProperty rdf:nodeID="Nba998a8f95b541a8a37886a2edf3b80c"/>
  </rdf:Description>
  <rdf:Description rdf:about="http://emmo.info/emmo/middle/properties#EMMO_e1097637_70d2_4895_973f_2396f04fa204">
    <rdf:type rdf:resource="http://www.w3.org/2002/07/owl#ObjectProperty"/>
    <rdfs:subPropertyOf rdf:resource="http://emmo.info/emmo/top/semiotics#EMMO_eb3518bf_f799_4f9e_8c3e_ce59af11453b"/>
    <rdfs:domain rdf:resource="http://emmo.info/emmo/top/semiotics#EMMO_6f5af708_f825_4feb_a0d1_a8d813d3022b"/>
    <rdfs:range rdf:resource="http://emmo.info/emmo/middle/properties#EMMO_b7bcff25_ffc3_474e_9ab5_01b1664bd4ba"/>
    <rdfs:label xml:lang="en">hasProperty</rdfs:label>
  </rdf:Description>
  <rdf:Description rdf:nodeID="N1fdc23dabb52434cb1677eb684110682">
    <rdf:type rdf:resource="http://www.w3.org/2002/07/owl#Restriction"/>
    <owl:onProperty rdf:resource="http://emmo.info/emmo/middle/perceptual#EMMO_23b579e1_8088_45b5_9975_064014026c42"/>
    <owl:hasValue>V</owl:hasValue>
  </rdf:Description>
  <rdf:Description rdf:nodeID="Ndc68ffc3e0824b509c5111fb2f6aabab">
    <rdf:type rdf:resource="http://www.w3.org/2002/07/owl#Restriction"/>
    <owl:onProperty rdf:resource="http://emmo.info/emmo/middle/metrology#EMMO_67fc0a36_8dcb_4ffa_9a43_31074efa3296"/>
    <owl:allValuesFrom rdf:nodeID="N1140c30c299746e2af8ef10fa86e617b"/>
  </rdf:Description>
  <rdf:Description rdf:nodeID="Nf7c388ca76684aeb844b9cc88b15e1c1">
    <owl:someValuesFrom rdf:resource="http://emmo.info/emmo/middle/physicalistic#EMMO_72d53756_7fb1_46ed_980f_83f47efbe105"/>
    <rdf:type rdf:resource="http://www.w3.org/2002/07/owl#Restriction"/>
    <owl:onProperty rdf:resource="http://emmo.info/emmo/middle/reductionistic#EMMO_b2282816_b7a3_44c6_b2cb_3feff1ceb7fe"/>
  </rdf:Description>
  <rdf:Description rdf:about="http://emmo.info/emmo/middle/siunits#EMMO_696ed548_9477_45ea_993c_6a8f5271914a">
    <rdfs:label xml:lang="en">Coulomb</rdfs:label>
    <rdf:type rdf:resource="http://www.w3.org/2002/07/owl#Class"/>
    <rdfs:comment>Measurement unit for electric charge.</rdfs:comment>
    <rdfs:subClassOf rdf:nodeID="Nb9ddbe209ce44b7b880d78e0f2a0e93f"/>
    <rdfs:subClassOf rdf:nodeID="Na9d5cdcb9fe7422bb2c63284f4ce49be"/>
    <annotations:EMMO_1f1b164d_ec6a_4faa_8d5e_88bda62316cc>http://qudt.org/vocab/unit/C</annotations:EMMO_1f1b164d_ec6a_4faa_8d5e_88bda62316cc>
    <annotations:EMMO_fe015383_afb3_44a6_ae86_043628697aa2>https://doi.org/10.1351/goldbook.C01365</annotations:EMMO_fe015383_afb3_44a6_ae86_043628697aa2>
  </rdf:Description>
  <rdf:Description rdf:about="http://emmo.info/emmo/top/annotations#EMMO_b432d2d5_25f4_4165_99c5_5935a7763c1a">
    <rdf:type rdf:resource="http://www.w3.org/2002/07/owl#AnnotationProperty"/>
    <rdfs:label xml:lang="en">example</rdfs:label>
    <rdfs:subPropertyOf rdf:resource="http://www.w3.org/2000/01/rdf-schema#comment"/>
  </rdf:Description>
  <rdf:Description rdf:nodeID="N4e2d0c6ba942426ab515e2dfcac125e3">
    <rdf:type rdf:resource="http://www.w3.org/2002/07/owl#Restriction"/>
    <owl:onProperty rdf:resource="http://emmo.info/emmo/middle/math#EMMO_faf79f53_749d_40b2_807c_d34244c192f4"/>
    <owl:allValuesFrom rdf:resource="http://www.w3.org/2001/XMLSchema#integer"/>
  </rdf:Description>
  <rdf:Description rdf:nodeID="N5c07a232f71c488d8ff7d3f95e9888bd">
    <owl:inverseOf rdf:resource="http://emmo.info/emmo/top/semiotics#EMMO_60577dea_9019_4537_ac41_80b0fb563d41"/>
  </rdf:Description>
  <rdf:Description rdf:nodeID="N889fdf1e62aa44cc8243b21b30dfbd9c">
    <rdf:rest rdf:resource="http://www.w3.org/1999/02/22-rdf-syntax-ns#nil"/>
    <rdf:first rdf:resource="http://emmo.info/emmo/top/mereotopology#EMMO_eb3a768e_d53e_4be9_a23b_0714833c36de"/>
  </rdf:Description>
  <rdf:Description rdf:nodeID="N87a2acc70780469e842d40ae420a312a">
    <rdf:rest rdf:resource="http://www.w3.org/1999/02/22-rdf-syntax-ns#nil"/>
    <rdf:first rdf:resource="http://emmo.info/emmo/top/semiotics#EMMO_d7788d1a_020d_4c78_85a1_13563fcec168"/>
  </rdf:Description>
  <rdf:Description rdf:nodeID="N4a7ff59e579b46c5aa91826116306d20">
    <rdf:first rdf:resource="http://emmo.info/emmo/middle/metrology#EMMO_c6d4a5e0_7e95_44df_a6db_84ee0a8bbc8e"/>
    <rdf:rest rdf:resource="http://www.w3.org/1999/02/22-rdf-syntax-ns#nil"/>
  </rdf:Description>
  <rdf:Description rdf:nodeID="N79b3d7d51d3c48d29e9df6d5271b788f">
    <owl:hasValue>A</owl:hasValue>
    <rdf:type rdf:resource="http://www.w3.org/2002/07/owl#Restriction"/>
    <owl:onProperty rdf:resource="http://emmo.info/emmo/middle/perceptual#EMMO_23b579e1_8088_45b5_9975_064014026c42"/>
  </rdf:Description>
  <rdf:Description rdf:about="http://emmo.info/emmo/middle/isq#EMMO_4f5c7c54_1c63_4d17_b12b_ea0792c2b187">
    <rdf:type rdf:resource="http://www.w3.org/2002/07/owl#Class"/>
    <rdfs:subClassOf rdf:resource="http://emmo.info/emmo/middle/metrology#EMMO_9895a1b4_f0a5_4167_ac5e_97db40b8bfcc"/>
    <owl:equivalentClass rdf:nodeID="Nff4876241e8046a0b5fe214366a39bea"/>
    <rdfs:label xml:lang="en">LengthPerTimeDimension</rdfs:label>
  </rdf:Description>
  <rdf:Description rdf:about="http://emmo.info/emmo/middle/siunits#EMMO_59c10c5c_47bd_4348_ba39_38836607dfa1">
    <rdfs:subClassOf rdf:nodeID="N376fb71de0b04a2686fed3b806bdd315"/>
    <rdfs:subClassOf rdf:nodeID="N31f67ad3d791498fa91b473e84706c7a"/>
    <rdfs:label xml:lang="en">Ohm</rdfs:label>
    <annotations:EMMO_1f1b164d_ec6a_4faa_8d5e_88bda62316cc>http://qudt.org/vocab/unit/OHM</annotations:EMMO_1f1b164d_ec6a_4faa_8d5e_88bda62316cc>
    <rdfs:comment>Measurement unit for resistance.</rdfs:comment>
    <rdf:type rdf:resource="http://www.w3.org/2002/07/owl#Class"/>
    <annotations:EMMO_fe015383_afb3_44a6_ae86_043628697aa2>https://doi.org/10.1351/goldbook.O04280</annotations:EMMO_fe015383_afb3_44a6_ae86_043628697aa2>
  </rdf:Description>
  <rdf:Description rdf:about="http://emmo.info/emmo/middle/isq#EMMO_02e894c3_b793_4197_b120_3442e08f58d1">
    <rdfs:label xml:lang="en">TimeDimension</rdfs:label>
    <owl:equivalentClass rdf:nodeID="Nde648a234346423fb8e73c7bd2083a1a"/>
    <rdf:type rdf:resource="http://www.w3.org/2002/07/owl#Class"/>
    <rdfs:subClassOf rdf:resource="http://emmo.info/emmo/middle/metrology#EMMO_9895a1b4_f0a5_4167_ac5e_97db40b8bfcc"/>
  </rdf:Description>
  <rdf:Description rdf:nodeID="N32613eb97d9c4309a450edda401aac48">
    <rdf:rest rdf:nodeID="Na5a999bffb2f4532ac99923ba0bff1cb"/>
    <rdf:first rdf:resource="http://emmo.info/emmo/middle/siunits#EMMO_a80dc6f5_b1aa_41a7_a3a8_cd5040da2162"/>
  </rdf:Description>
  <rdf:Description rdf:about="http://emmo.info/emmo/middle/siunits#EMMO_e9ffc696_5228_4ff9_8a60_0f5e05e9931b">
    <rdf:type rdf:resource="http://www.w3.org/2002/07/owl#Class"/>
    <annotations:EMMO_967080e5_2f42_4eb2_a3a9_c58143e835f9>The 22 derived units that are given a special name in the SI system that stands for units derived by SI base units.</annotations:EMMO_967080e5_2f42_4eb2_a3a9_c58143e835f9>
    <rdfs:subClassOf rdf:resource="http://emmo.info/emmo/middle/metrology#EMMO_3ee80521_3c23_4dd1_935d_9d522614a3e2"/>
    <rdfs:label xml:lang="en">SISpecialUnit</rdfs:label>
    <annotations:EMMO_c84c6752_6d64_48cc_9500_e54a3c34898d>https://en.wikipedia.org/wiki/International_System_of_Units#Derived_units</annotations:EMMO_c84c6752_6d64_48cc_9500_e54a3c34898d>
    <owl:disjointUnionOf rdf:nodeID="N2fbbf86dc5a74fd48d48ef3ba7691010"/>
    <rdfs:comment>These units are SI coherent by definition.</rdfs:comment>
  </rdf:Description>
  <rdf:Description rdf:nodeID="Nd9a0a27607b544b1b9f670cccb04fc4a">
    <owl:onProperty rdf:nodeID="Nf11889e15419468893752f7c5181e1d5"/>
    <owl:someValuesFrom rdf:resource="http://emmo.info/emmo/middle/properties#EMMO_10a5fd39_06aa_4648_9e70_f962a9cb2069"/>
    <rdf:type rdf:resource="http://www.w3.org/2002/07/owl#Restriction"/>
  </rdf:Description>
  <rdf:Description rdf:nodeID="Nfb69c3276986498693a72ad849e39c56">
    <owl:minQualifiedCardinality rdf:datatype="http://www.w3.org/2001/XMLSchema#nonNegativeInteger">1</owl:minQualifiedCardinality>
  </rdf:Description>
  <rdf:Description rdf:nodeID="N1829aef8f5264533982cdbafdb05ab3b">
    <rdf:rest rdf:nodeID="Nbe4764aa85bd432e87d21fe8771325ef"/>
    <rdf:first rdf:resource="http://emmo.info/emmo/middle/reductionistic#EMMO_36c79456_e29c_400d_8bd3_0eedddb82652"/>
  </rdf:Description>
  <rdf:Description rdf:nodeID="N065b4557f65a4e27a869fd1830526f2d">
    <owl:onProperty rdf:resource="http://emmo.info/emmo/middle/perceptual#EMMO_23b579e1_8088_45b5_9975_064014026c42"/>
    <rdf:type rdf:resource="http://www.w3.org/2002/07/owl#Restriction"/>
    <owl:hasValue>T0 L+1 M0 I0 Θ0 N0 J0</owl:hasValue>
  </rdf:Description>
  <rdf:Description rdf:about="http://emmo.info/emmo/middle/isq#EMMO_8d3da9ac_2265_4382_bee5_db72046722f8">
    <annotations:EMMO_fe015383_afb3_44a6_ae86_043628697aa2>https://doi.org/10.1351/goldbook.A00114</annotations:EMMO_fe015383_afb3_44a6_ae86_043628697aa2>
    <rdfs:label xml:lang="en">Radioactivity</rdfs:label>
    <rdfs:subClassOf rdf:nodeID="N22067548347643179344ff5d615c234a"/>
    <rdf:type rdf:resource="http://www.w3.org/2002/07/owl#Class"/>
    <rdfs:subClassOf rdf:resource="http://emmo.info/emmo/middle/isq#EMMO_2946d40b_24a1_47fa_8176_e3f79bb45064"/>
    <annotations:EMMO_967080e5_2f42_4eb2_a3a9_c58143e835f9>Decays per unit time.</annotations:EMMO_967080e5_2f42_4eb2_a3a9_c58143e835f9>
  </rdf:Description>
  <rdf:Description rdf:nodeID="N2ad3c4e108dd4540aff45e0082d6cc7a">
    <owl:hasValue>T</owl:hasValue>
    <owl:onProperty rdf:resource="http://emmo.info/emmo/middle/perceptual#EMMO_23b579e1_8088_45b5_9975_064014026c42"/>
    <rdf:type rdf:resource="http://www.w3.org/2002/07/owl#Restriction"/>
  </rdf:Description>
  <rdf:Description rdf:nodeID="N99b7b86980dd41f5b42f9889381ca1c5">
    <owl:hasValue>=</owl:hasValue>
    <rdf:type rdf:resource="http://www.w3.org/2002/07/owl#Restriction"/>
    <owl:onProperty rdf:resource="http://emmo.info/emmo/middle/perceptual#EMMO_23b579e1_8088_45b5_9975_064014026c42"/>
  </rdf:Description>
  <rdf:Description rdf:nodeID="Nc55e4865e4aa47afb5a4fdafc9c2046a">
    <rdf:first rdf:resource="http://emmo.info/emmo/middle/siunits#EMMO_cf3dd6cc_c5d6_4b3d_aef4_82f3b7a361af"/>
    <rdf:rest rdf:nodeID="N4a66e753f9e749abb354adc6309f441b"/>
  </rdf:Description>
  <rdf:Description rdf:about="http://emmo.info/emmo/top/semiotics#EMMO_35d2e130_6e01_41ed_94f7_00b333d46cf9">
    <annotations:EMMO_967080e5_2f42_4eb2_a3a9_c58143e835f9>A 'Sign' that stands for an 'Object' through convention, norm or habit, without any resemblance to it.</annotations:EMMO_967080e5_2f42_4eb2_a3a9_c58143e835f9>
    <rdfs:comment>In Peirce semiotics this kind of sign category is called symbol. However, since symbol is also used in formal languages, the name is changed in conventional.</rdfs:comment>
    <rdfs:label xml:lang="en">Conventional</rdfs:label>
    <rdf:type rdf:resource="http://www.w3.org/2002/07/owl#Class"/>
  </rdf:Description>
  <rdf:Description rdf:nodeID="Nde0627e70a0740ca9eacc8c3fcf9b4a1">
    <rdf:rest rdf:resource="http://www.w3.org/1999/02/22-rdf-syntax-ns#nil"/>
    <rdf:first rdf:resource="http://emmo.info/emmo/middle/siunits#EMMO_ffc7735f_c177_46a4_98e9_a54440d29209"/>
  </rdf:Description>
  <rdf:Description rdf:about="http://emmo.info/emmo/middle/isq#EMMO_b14d9be5_f81e_469b_abca_379c2e83feab">
    <rdfs:subClassOf rdf:resource="http://emmo.info/emmo/middle/metrology#EMMO_9895a1b4_f0a5_4167_ac5e_97db40b8bfcc"/>
    <owl:equivalentClass rdf:nodeID="N67ec8590149b41faa83da784ca10fa22"/>
    <rdfs:label xml:lang="en">QuarticTimeSquareCurrentPerMassSquareLengthDimension</rdfs:label>
    <rdf:type rdf:resource="http://www.w3.org/2002/07/owl#Class"/>
  </rdf:Description>
  <rdf:Description rdf:about="http://emmo.info/emmo/middle/materials#EMMO_87ac88ff_8379_4f5a_8c7b_424a8fff1ee8">
    <rdfs:label xml:lang="en">Fluid</rdfs:label>
    <annotations:EMMO_967080e5_2f42_4eb2_a3a9_c58143e835f9>A continuum that has no fixed shape and yields easily to external pressure.</annotations:EMMO_967080e5_2f42_4eb2_a3a9_c58143e835f9>
    <rdf:type rdf:resource="http://www.w3.org/2002/07/owl#Class"/>
    <annotations:EMMO_b432d2d5_25f4_4165_99c5_5935a7763c1a>Gas, liquid, plasma,</annotations:EMMO_b432d2d5_25f4_4165_99c5_5935a7763c1a>
    <rdfs:subClassOf rdf:resource="http://emmo.info/emmo/middle/materials#EMMO_8b0923ab_b500_477b_9ce9_8b3a3e4dc4f2"/>
  </rdf:Description>
  <rdf:Description rdf:about="http://emmo.info/emmo/middle/math#EMMO_21f56795_ee72_4858_b571_11cfaa59c1a8">
    <annotations:EMMO_967080e5_2f42_4eb2_a3a9_c58143e835f9>A numerical data value.</annotations:EMMO_967080e5_2f42_4eb2_a3a9_c58143e835f9>
    <rdfs:subClassOf rdf:resource="http://emmo.info/emmo/middle/perceptual#EMMO_a1083d0a_c1fb_471f_8e20_a98f881ad527"/>
    <rdfs:comment>A number is actually a string (e.g. 1.4, 1e-8) of numerical digits and other symbols. However, in order not to increase complexity of the taxonomy and relations, here we take a number as an "atomic" object (i.e. we do not include digits in the EMMO as alphabet for numbers).

A 'Number' individual provide the link between the ontology and the actual data, through the data property hasNumericalValue.</rdfs:comment>
    <rdf:type rdf:resource="http://www.w3.org/2002/07/owl#Class"/>
    <rdfs:label xml:lang="en">Number</rdfs:label>
    <rdfs:subClassOf rdf:resource="http://emmo.info/emmo/middle/math#EMMO_4ce76d7f_03f8_45b6_9003_90052a79bfaa"/>
  </rdf:Description>
  <rdf:Description rdf:about="http://emmo.info/emmo/middle/siunits#EMMO_acb50123_87a2_4753_b36c_f87114ad4de2">
    <rdfs:subClassOf rdf:nodeID="N26457dd595294348b1997a0256484255"/>
    <rdfs:comment>Measurement unit for magnetic flux density or induction.</rdfs:comment>
    <rdfs:subClassOf rdf:nodeID="N6eace5477e534d29a48701f5c51d4a0e"/>
    <annotations:EMMO_fe015383_afb3_44a6_ae86_043628697aa2>https://doi.org/10.1351/goldbook.T06283</annotations:EMMO_fe015383_afb3_44a6_ae86_043628697aa2>
    <rdfs:label xml:lang="en">Tesla</rdfs:label>
    <rdf:type rdf:resource="http://www.w3.org/2002/07/owl#Class"/>
    <annotations:EMMO_1f1b164d_ec6a_4faa_8d5e_88bda62316cc>http://qudt.org/vocab/unit/T</annotations:EMMO_1f1b164d_ec6a_4faa_8d5e_88bda62316cc>
  </rdf:Description>
  <rdf:Description rdf:nodeID="N732e98b8ec654ec9a809d873634b18a8">
    <rdf:type rdf:resource="http://www.w3.org/2002/07/owl#Restriction"/>
    <owl:onProperty rdf:resource="http://emmo.info/emmo/top/mereotopology#EMMO_9380ab64_0363_4804_b13f_3a8a94119a76"/>
    <owl:allValuesFrom rdf:nodeID="Nce81168ffc994431803922256ac689d2"/>
  </rdf:Description>
  <rdf:Description rdf:about="http://emmo.info/emmo/middle/siunits#EMMO_d41ce84b_4317_41fb_a5d1_6cd281fca106">
    <rdfs:subClassOf rdf:resource="http://emmo.info/emmo/middle/metrology#EMMO_c6d4a5e0_7e95_44df_a6db_84ee0a8bbc8e"/>
    <rdfs:subClassOf rdf:nodeID="Ndea63cdcefe14a04bc2e81bd664f7f05"/>
    <rdfs:label xml:lang="en">SIPrefixedUnit</rdfs:label>
    <annotations:EMMO_967080e5_2f42_4eb2_a3a9_c58143e835f9>A SI base or special unit with a metric prefix.</annotations:EMMO_967080e5_2f42_4eb2_a3a9_c58143e835f9>
    <rdfs:comment>The presence of the prefix makes this units non-coherent with SI system.</rdfs:comment>
    <rdf:type rdf:resource="http://www.w3.org/2002/07/owl#Class"/>
  </rdf:Description>
  <rdf:Description rdf:nodeID="N2c32ed7dff6749b8ae940356bfebdf51">
    <owl:onProperty rdf:resource="http://emmo.info/emmo/middle/perceptual#EMMO_23b579e1_8088_45b5_9975_064014026c42"/>
    <owl:hasValue>f</owl:hasValue>
    <rdf:type rdf:resource="http://www.w3.org/2002/07/owl#Restriction"/>
  </rdf:Description>
  <rdf:Description rdf:about="http://emmo.info/emmo/top/mereotopology#EMMO_8c898653_1118_4682_9bbf_6cc334d16a99">
    <rdf:type rdf:resource="http://www.w3.org/2002/07/owl#ObjectProperty"/>
    <rdf:type rdf:resource="http://www.w3.org/2002/07/owl#TransitiveProperty"/>
    <rdfs:subPropertyOf rdf:resource="http://emmo.info/emmo/top/mereotopology#EMMO_6703954e_34c4_4a15_a9e7_f313760ae1a8"/>
    <rdfs:label xml:lang="en">encloses</rdfs:label>
    <rdfs:comment>Enclosure is reflexive and transitive.</rdfs:comment>
  </rdf:Description>
  <rdf:Description rdf:about="http://emmo.info/emmo/middle/perceptual#EMMO_0ef4ff4a_5458_4f2a_b51f_4689d472a3f2">
    <rdfs:subClassOf rdf:resource="http://emmo.info/emmo/middle/perceptual#EMMO_0c576e13_4ee7_4f3d_bfe9_1614243df018"/>
    <rdf:type rdf:resource="http://www.w3.org/2002/07/owl#Class"/>
    <rdfs:label xml:lang="en">Curve</rdfs:label>
  </rdf:Description>
  <rdf:Description rdf:about="http://emmo.info/emmo/top/math#EMMO_98d65021_4574_4890_b2fb_46430841077f">
    <rdfs:comment>An 'equation' that has parts two 'polynomial'-s</rdfs:comment>
    <rdfs:label xml:lang="en">AlgebricEquation</rdfs:label>
    <rdf:type rdf:resource="http://www.w3.org/2002/07/owl#Class"/>
    <annotations:EMMO_b432d2d5_25f4_4165_99c5_5935a7763c1a>2 * a - b = c</annotations:EMMO_b432d2d5_25f4_4165_99c5_5935a7763c1a>
    <rdfs:subClassOf rdf:resource="http://emmo.info/emmo/middle/math#EMMO_e56ee3eb_7609_4ae1_8bed_51974f0960a6"/>
    <rdfs:subClassOf rdf:nodeID="N77b5760126354ee59ad8bf5ea2f4acdf"/>
  </rdf:Description>
  <rdf:Description rdf:about="http://emmo.info/emmo/middle/materials">
    <owl:versionInfo>The European Materials Modelling Ontology

Version 1.0.0-alpha</owl:versionInfo>
    <rdfs:comment xml:lang="en">Contacts:
Gerhard Goldbeck
Goldbeck Consulting Ltd (UK)
email: gerhard@goldbeck-consulting.com

Emanuele Ghedini
University of Bologna (IT)
email: emanuele.ghedini@unibo.it</rdfs:comment>
    <owl:versionIRI rdf:resource="http://emmo.info/emmo/1.0.0-alpha/middle/materials"/>
    <rdfs:comment>European Materials and Modelling Ontology (EMMO)

EMMO is a multidisciplinary effort to develop a standard representational framework (the ontology) based on current materials modelling knowledge, including physical sciences, analytical philosophy and information and communication technologies. 

It provides the connection between the physical world, materials characterisation world and materials modelling world.</rdfs:comment>
    <rdf:type rdf:resource="http://www.w3.org/2002/07/owl#Ontology"/>
    <annotations:EMMO_5525a055_dda5_4556_8b91_f0d22fa676cc>EMMO is released under a Creative Commons license Attribution 4.0 International (CC BY 4.0)

https://creativecommons.org/licenses/by/4.0/legalcode</annotations:EMMO_5525a055_dda5_4556_8b91_f0d22fa676cc>
    <rdfs:comment>The EMMO requires FacT++ reasoner plugin in order to visualize all inferences and class hierarchy (ctrl+R hotkey in Protege).</rdfs:comment>
    <annotations:EMMO_cd5fb112_7ee7_4120_a35d_3ca3e6c3f4ab>Emanuele Ghedini (University of Bologna, IT)
Gerhard Goldbeck (GCL Ltd, UK)
Adham Hashibon (Fraunhofer IWM, DE)
Georg Schmitz (Access, DE)
Jesper Friis (SINTEF, NO)</annotations:EMMO_cd5fb112_7ee7_4120_a35d_3ca3e6c3f4ab>
  </rdf:Description>
  <rdf:Description rdf:about="http://emmo.info/emmo/middle/isq#EMMO_cd2cd0de_e0cc_4ef1_b27e_2e88db027bac">
    <annotations:EMMO_fe015383_afb3_44a6_ae86_043628697aa2>https://doi.org/10.1351/goldbook.L03498</annotations:EMMO_fe015383_afb3_44a6_ae86_043628697aa2>
    <rdfs:label xml:lang="en">Length</rdfs:label>
    <rdfs:subClassOf rdf:nodeID="N9a292fc0d28444a3a7e0be114463a19f"/>
    <annotations:EMMO_6dd685dd_1895_46e4_b227_be9f7d643c25>http://dbpedia.org/page/Length</annotations:EMMO_6dd685dd_1895_46e4_b227_be9f7d643c25>
    <rdf:type rdf:resource="http://www.w3.org/2002/07/owl#Class"/>
    <annotations:EMMO_967080e5_2f42_4eb2_a3a9_c58143e835f9>Extend of a spatial dimension.</annotations:EMMO_967080e5_2f42_4eb2_a3a9_c58143e835f9>
  </rdf:Description>
  <rdf:Description rdf:nodeID="Na3f60bb59b39470fac7fe3de46953a2d">
    <rdf:first rdf:resource="http://emmo.info/emmo/middle/metrology#EMMO_02c0621e_a527_4790_8a0f_2bb51973c819"/>
    <rdf:rest rdf:nodeID="Nedd7f0a9acc14e189221d4000699e805"/>
  </rdf:Description>
  <rdf:Description rdf:nodeID="N87080e819ab9442d8e5c7af96544af1c">
    <rdf:first rdf:resource="http://emmo.info/emmo/middle/siunits#EMMO_21aaefc1_3f86_4208_b7db_a755f31f0f8c"/>
    <rdf:rest rdf:nodeID="Nf47c3c5925114cef985641fc5ed77aa6"/>
  </rdf:Description>
  <rdf:Description rdf:nodeID="Na5a999bffb2f4532ac99923ba0bff1cb">
    <rdf:rest rdf:nodeID="N2eb7ecce985748a9bda630a9a3cbbe84"/>
    <rdf:first rdf:resource="http://emmo.info/emmo/middle/siunits#EMMO_a9201b2f_e6de_442a_b3a6_d291.0.0-alphaa582"/>
  </rdf:Description>
  <rdf:Description rdf:about="http://emmo.info/emmo/middle/materials#EMMO_3397f270_dfc1_4500_8f6f_4d0d85ac5f71">
    <rdfs:label xml:lang="en">Molecule</rdfs:label>
    <rdfs:subClassOf rdf:resource="http://emmo.info/emmo/middle/physicalistic#EMMO_4207e895_8b83_4318_996a_72cfb32acd94"/>
    <rdf:type rdf:resource="http://www.w3.org/2002/07/owl#Class"/>
    <rdfs:comment>An entity is called essential if removing one direct part will lead to a change in entity class.

An entity is called redundand if removing one direct part will not lead to a change in entity class.</rdfs:comment>
    <rdfs:subClassOf rdf:resource="http://emmo.info/emmo/middle/reductionistic#EMMO_36c79456_e29c_400d_8bd3_0eedddb82652"/>
    <annotations:EMMO_967080e5_2f42_4eb2_a3a9_c58143e835f9>An atom_based state defined by an exact number of e-bonded atomic species and an electron cloud made of the shared electrons.</annotations:EMMO_967080e5_2f42_4eb2_a3a9_c58143e835f9>
    <rdfs:comment>This definition states that this object is a non-periodic set of atoms or a set with a finite periodicity.

Removing an atom from the state will result in another type of atom_based state.

e.g. you cannot remove H from H20 without changing the molecule type (essential). However, you can remove a C from a nanotube (redundant). C60 fullerene is a molecule, since it has a finite periodicity and is made of a well defined number of atoms (essential). A C nanotube is not a molecule, since it has an infinite periodicity (redundant).</rdfs:comment>
    <annotations:EMMO_b432d2d5_25f4_4165_99c5_5935a7763c1a>H20, C6H12O6, CH4</annotations:EMMO_b432d2d5_25f4_4165_99c5_5935a7763c1a>
  </rdf:Description>
  <rdf:Description rdf:about="http://emmo.info/emmo/middle/isq#EMMO_d5f3e0e5_fc7d_4e64_86ad_555e74aaff84">
    <owl:equivalentClass rdf:nodeID="N9abc93e180854f09bfd8d84fd55c7bd1"/>
    <rdfs:subClassOf rdf:resource="http://emmo.info/emmo/middle/metrology#EMMO_9895a1b4_f0a5_4167_ac5e_97db40b8bfcc"/>
    <rdf:type rdf:resource="http://www.w3.org/2002/07/owl#Class"/>
    <rdfs:label xml:lang="en">ElectricCurrentDimension</rdfs:label>
  </rdf:Description>
  <rdf:Description rdf:about="http://emmo.info/emmo/middle/perceptual#EMMO_4b3afb22_27cf_4ce3_88bc_492bfccb546b">
    <annotations:EMMO_967080e5_2f42_4eb2_a3a9_c58143e835f9>An 'impression' which stands for a real world object whose spatiotemporal pattern makes it identifiable by an observer as a sound.</annotations:EMMO_967080e5_2f42_4eb2_a3a9_c58143e835f9>
    <rdf:type rdf:resource="http://www.w3.org/2002/07/owl#Class"/>
    <rdfs:comment>'acoustical' refers to the perception mechanism of the observer that can occur through a microphone, a ear.</rdfs:comment>
    <rdfs:label xml:lang="en">Acoustical</rdfs:label>
    <rdfs:subClassOf rdf:resource="http://emmo.info/emmo/middle/perceptual#EMMO_649bf97b_4397_4005_90d9_219755d92e34"/>
  </rdf:Description>
  <rdf:Description rdf:nodeID="N71dc8b6f026b4de9bab26ed993f83d5a">
    <owl:onProperty rdf:resource="http://emmo.info/emmo/middle/holistic#EMMO_ae2d1a96_bfa1_409a_a7d2_03d69e8a125a"/>
    <owl:someValuesFrom rdf:resource="http://emmo.info/emmo/middle/properties#EMMO_b7bcff25_ffc3_474e_9ab5_01b1664bd4ba"/>
    <rdf:type rdf:resource="http://www.w3.org/2002/07/owl#Restriction"/>
  </rdf:Description>
  <rdf:Description rdf:nodeID="Nae895865b8364d67904d336652857195">
    <rdf:type rdf:resource="http://www.w3.org/2002/07/owl#Restriction"/>
    <owl:allValuesFrom rdf:nodeID="Na96d5d7f393d4e26b6bbf71e75638a50"/>
    <owl:onProperty rdf:nodeID="N2343adef8e1544988995c7e2cdc4baa5"/>
  </rdf:Description>
  <rdf:Description rdf:nodeID="Naa6daa84dcd04b9796c42086483a0e50">
    <rdf:type rdf:resource="http://www.w3.org/2002/07/owl#Restriction"/>
    <owl:allValuesFrom rdf:resource="http://emmo.info/emmo/top/physical#EMMO_29072ec4_ffcb_42fb_bdc7_26f05a2e9873"/>
    <owl:onProperty rdf:resource="http://emmo.info/emmo/top/mereotopology#EMMO_17e27c22_37e1_468c_9dd7_95e137f73e7f"/>
  </rdf:Description>
  <rdf:Description rdf:nodeID="N678532a1c73a4e1586848c8038cb5f20">
    <rdf:type rdf:resource="http://www.w3.org/2002/07/owl#Restriction"/>
    <owl:onProperty rdf:resource="http://emmo.info/emmo/middle/perceptual#EMMO_23b579e1_8088_45b5_9975_064014026c42"/>
    <owl:hasValue>N</owl:hasValue>
  </rdf:Description>
  <rdf:Description rdf:nodeID="N0706bf3341e64441809c178882211a20">
    <owl:allValuesFrom rdf:nodeID="N9def89b42bfd45adb8da560f72fb7f70"/>
    <owl:onProperty rdf:resource="http://emmo.info/emmo/middle/metrology#EMMO_67fc0a36_8dcb_4ffa_9a43_31074efa3296"/>
    <rdf:type rdf:resource="http://www.w3.org/2002/07/owl#Restriction"/>
  </rdf:Description>
  <rdf:Description rdf:about="http://emmo.info/emmo/middle/siunits#EMMO_e79c62ff_10ad_4ec0_baba_c19ddd4eaa11">
    <rdf:type rdf:resource="http://www.w3.org/2002/07/owl#Class"/>
    <rdfs:subClassOf rdf:nodeID="N171648765e3c45a39c0fee0faa8adb14"/>
    <rdfs:label xml:lang="en">Yotta</rdfs:label>
    <rdfs:subClassOf rdf:nodeID="N8228ee2a1c7044afa7ada85142123fc3"/>
  </rdf:Description>
  <rdf:Description rdf:about="http://emmo.info/emmo/middle/siunits#EMMO_33b67e69_3645_4c73_b100_5ea6759221b4">
    <annotations:EMMO_fe015383_afb3_44a6_ae86_043628697aa2>https://doi.org/10.1351/goldbook.K03372</annotations:EMMO_fe015383_afb3_44a6_ae86_043628697aa2>
    <rdfs:subClassOf rdf:nodeID="N2a926ecd6ff341c8bf319f8a9d3de555"/>
    <rdfs:label xml:lang="en">Katal</rdfs:label>
    <annotations:EMMO_1f1b164d_ec6a_4faa_8d5e_88bda62316cc>http://qudt.org/vocab/unit/KAT</annotations:EMMO_1f1b164d_ec6a_4faa_8d5e_88bda62316cc>
    <rdf:type rdf:resource="http://www.w3.org/2002/07/owl#Class"/>
    <rdfs:comment>Measurement unit for catalytic activity.</rdfs:comment>
    <rdfs:subClassOf rdf:nodeID="N3cd66eb437284d19beb5c4e55fa55adb"/>
  </rdf:Description>
  <rdf:Description rdf:nodeID="N19e5134869b348bcbeded8f96303d7fe">
    <owl:onProperty rdf:resource="http://emmo.info/emmo/middle/metrology#EMMO_67fc0a36_8dcb_4ffa_9a43_31074efa3296"/>
    <rdf:type rdf:resource="http://www.w3.org/2002/07/owl#Restriction"/>
    <owl:allValuesFrom rdf:nodeID="N608bc2c6f76d42938e8f9e7ea1feb115"/>
  </rdf:Description>
  <rdf:Description rdf:about="http://emmo.info/emmo/middle/siunits#EMMO_b20be325_8bfd_4237_bee7_201ab0fd9c75">
    <rdfs:subClassOf rdf:nodeID="Nf63fa94031ad483aa6692eb5df5b3cd6"/>
    <rdfs:comment>Measurement unit for Celsius temperature. This unit can only be used for expressing temperature differences.</rdfs:comment>
    <annotations:EMMO_1f1b164d_ec6a_4faa_8d5e_88bda62316cc>http://qudt.org/vocab/unit/DEG_C</annotations:EMMO_1f1b164d_ec6a_4faa_8d5e_88bda62316cc>
    <annotations:EMMO_fe015383_afb3_44a6_ae86_043628697aa2>https://doi.org/10.1351/goldbook.D01561</annotations:EMMO_fe015383_afb3_44a6_ae86_043628697aa2>
    <rdfs:label xml:lang="en">DegreeCelsius</rdfs:label>
    <rdfs:subClassOf rdf:nodeID="N17581f3a64b64569a163550af1853865"/>
    <rdf:type rdf:resource="http://www.w3.org/2002/07/owl#Class"/>
  </rdf:Description>
  <rdf:Description rdf:nodeID="N20d459b4b2164af3bb0a77fa6a377a03">
    <rdf:rest rdf:nodeID="Nc55e4865e4aa47afb5a4fdafc9c2046a"/>
    <rdf:first rdf:resource="http://emmo.info/emmo/middle/siunits#EMMO_b71e4ba5_8f73_4199_8c96_7ea7f94d9e2a"/>
  </rdf:Description>
  <rdf:Description rdf:about="http://emmo.info/emmo/middle/siunits#EMMO_ffc7735f_c177_46a4_98e9_a54440d29209">
    <annotations:EMMO_fe015383_afb3_44a6_ae86_043628697aa2>https://doi.org/10.1351/goldbook.B00695</annotations:EMMO_fe015383_afb3_44a6_ae86_043628697aa2>
    <annotations:EMMO_967080e5_2f42_4eb2_a3a9_c58143e835f9>A physical constant relating energy at the individual particle level with temperature. It is the gas constant R divided by the Avogadro constant.</annotations:EMMO_967080e5_2f42_4eb2_a3a9_c58143e835f9>
    <rdf:type rdf:resource="http://www.w3.org/2002/07/owl#Class"/>
    <rdfs:subClassOf rdf:nodeID="Ndb753105f98d4a6f91df9f358c307cff"/>
    <rdfs:comment>The DBpedia definition (http://dbpedia.org/page/Boltzmann_constant) is outdated as May 20, 2019. It is now an exact quantity.</rdfs:comment>
    <annotations:EMMO_1f1b164d_ec6a_4faa_8d5e_88bda62316cc>http://physics.nist.gov/cuu/CODATA-Value_BoltzmannConstant</annotations:EMMO_1f1b164d_ec6a_4faa_8d5e_88bda62316cc>
    <annotations:EMMO_6dd685dd_1895_46e4_b227_be9f7d643c25>http://dbpedia.org/page/Boltzmann_constant</annotations:EMMO_6dd685dd_1895_46e4_b227_be9f7d643c25>
    <rdfs:label xml:lang="en">BoltzmannConstant</rdfs:label>
  </rdf:Description>
  <rdf:Description rdf:nodeID="N6b84e1de4b304453ba61e135e3e7be61">
    <rdf:first rdf:resource="http://emmo.info/emmo/middle/physicalistic#EMMO_25f8b804_9a0b_4387_a3e7_b35bce5365ee"/>
    <rdf:rest rdf:nodeID="N2c55cf9c462241b288883dd8516cf2bc"/>
  </rdf:Description>
  <rdf:Description rdf:nodeID="Nc9301c0680714f4195f456f618bd444c">
    <owl:inverseOf rdf:resource="http://emmo.info/emmo/middle/math#EMMO_3446e167_c576_49d6_846c_215bb8878a55"/>
  </rdf:Description>
  <rdf:Description rdf:about="http://emmo.info/emmo/middle/math#EMMO_f9bc8b52_85e9_4b53_b969_dd7724d5b8e4">
    <rdfs:label xml:lang="en">Expression</rdfs:label>
    <rdfs:subClassOf rdf:resource="http://emmo.info/emmo/middle/perceptual#EMMO_89a0c87c_0804_4013_937a_6fe234d9499c"/>
    <annotations:EMMO_967080e5_2f42_4eb2_a3a9_c58143e835f9>A well-formed finite combination of mathematical symbols according to some specific rules.</annotations:EMMO_967080e5_2f42_4eb2_a3a9_c58143e835f9>
    <rdfs:subClassOf rdf:resource="http://emmo.info/emmo/middle/math#EMMO_54ee6b5e_5261_44a8_86eb_5717e7fdb9d0"/>
    <rdf:type rdf:resource="http://www.w3.org/2002/07/owl#Class"/>
  </rdf:Description>
  <rdf:Description rdf:about="http://emmo.info/emmo/middle/physicalistic#EMMO_eb3c61f0_3983_4346_a0c6_e7f6b90a67a8">
    <rdf:type rdf:resource="http://www.w3.org/2002/07/owl#Class"/>
    <rdfs:subClassOf rdf:resource="http://emmo.info/emmo/top/physical#EMMO_0f795e3e_c602_4577_9a43_d5a231aa1360"/>
    <rdfs:label xml:lang="en">Graviton</rdfs:label>
    <rdfs:comment>While this particle is only supposed to exist, the EMMO approach to classical and quantum systems represents fields as made of particles.

For this reason graviton is an useful concept to homogenize the approach between different fields.</rdfs:comment>
    <annotations:EMMO_967080e5_2f42_4eb2_a3a9_c58143e835f9>The class of individuals that stand for gravitons elementary particles.</annotations:EMMO_967080e5_2f42_4eb2_a3a9_c58143e835f9>
  </rdf:Description>
  <rdf:Description rdf:about="http://emmo.info/emmo/middle/physicalistic">
    <annotations:EMMO_cd5fb112_7ee7_4120_a35d_3ca3e6c3f4ab>Emanuele Ghedini (University of Bologna, IT)
Gerhard Goldbeck (GCL Ltd, UK)
Adham Hashibon (Fraunhofer IWM, DE)
Georg Schmitz (Access, DE)
Jesper Friis (SINTEF, NO)</annotations:EMMO_cd5fb112_7ee7_4120_a35d_3ca3e6c3f4ab>
    <owl:versionIRI rdf:resource="http://emmo.info/emmo/1.0.0-alpha/middle/physicalistic"/>
    <rdfs:comment>The EMMO requires FacT++ reasoner plugin in order to visualize all inferences and class hierarchy (ctrl+R hotkey in Protege).</rdfs:comment>
    <rdf:type rdf:resource="http://www.w3.org/2002/07/owl#Ontology"/>
    <rdfs:comment>European Materials and Modelling Ontology (EMMO)

EMMO is a multidisciplinary effort to develop a standard representational framework (the ontology) based on current materials modelling knowledge, including physical sciences, analytical philosophy and information and communication technologies. 

It provides the connection between the physical world, materials characterisation world and materials modelling world.</rdfs:comment>
    <annotations:EMMO_5525a055_dda5_4556_8b91_f0d22fa676cc>EMMO is released under a Creative Commons license Attribution 4.0 International (CC BY 4.0)

https://creativecommons.org/licenses/by/4.0/legalcode</annotations:EMMO_5525a055_dda5_4556_8b91_f0d22fa676cc>
    <owl:versionInfo>The European Materials Modelling Ontology

Version 1.0.0-alpha</owl:versionInfo>
    <rdfs:comment xml:lang="en">Contacts:
Gerhard Goldbeck
Goldbeck Consulting Ltd (UK)
email: gerhard@goldbeck-consulting.com

Emanuele Ghedini
University of Bologna (IT)
email: emanuele.ghedini@unibo.it</rdfs:comment>
  </rdf:Description>
  <rdf:Description rdf:about="http://emmo.info/emmo/middle/manufacturing">
    <annotations:EMMO_cd5fb112_7ee7_4120_a35d_3ca3e6c3f4ab>Emanuele Ghedini (University of Bologna, IT)
Gerhard Goldbeck (GCL Ltd, UK)
Adham Hashibon (Fraunhofer IWM, DE)
Georg Schmitz (Access, DE)
Jesper Friis (SINTEF, NO)</annotations:EMMO_cd5fb112_7ee7_4120_a35d_3ca3e6c3f4ab>
    <owl:versionInfo>The European Materials Modelling Ontology

Version 1.0.0-alpha</owl:versionInfo>
    <annotations:EMMO_5525a055_dda5_4556_8b91_f0d22fa676cc>EMMO is released under a Creative Commons license Attribution 4.0 International (CC BY 4.0)

https://creativecommons.org/licenses/by/4.0/legalcode</annotations:EMMO_5525a055_dda5_4556_8b91_f0d22fa676cc>
    <rdf:type rdf:resource="http://www.w3.org/2002/07/owl#Ontology"/>
    <rdfs:comment>European Materials and Modelling Ontology (EMMO)

EMMO is a multidisciplinary effort to develop a standard representational framework (the ontology) based on current materials modelling knowledge, including physical sciences, analytical philosophy and information and communication technologies. 

It provides the connection between the physical world, materials characterisation world and materials modelling world.</rdfs:comment>
    <rdfs:comment>The EMMO requires FacT++ reasoner plugin in order to visualize all inferences and class hierarchy (ctrl+R hotkey in Protege).</rdfs:comment>
    <rdfs:comment xml:lang="en">Contacts:
Gerhard Goldbeck
Goldbeck Consulting Ltd (UK)
email: gerhard@goldbeck-consulting.com

Emanuele Ghedini
University of Bologna (IT)
email: emanuele.ghedini</rdfs:comment>
    <owl:versionIRI rdf:resource="http://emmo.info/emmo/1.0.0-alpha/middle/manufacturing"/>
  </rdf:Description>
  <rdf:Description rdf:nodeID="N95a3b006afc24e0bb28e46eab6d98f56">
    <owl:allValuesFrom rdf:nodeID="Naf03a81efaf84d808cfc3c64d9a06ecf"/>
    <owl:onProperty rdf:nodeID="N073a4bd047ba4c05aa957f3e52261278"/>
    <rdf:type rdf:resource="http://www.w3.org/2002/07/owl#Restriction"/>
  </rdf:Description>
  <rdf:Description rdf:about="http://emmo.info/emmo/middle/metrology#EMMO_cfcf0f48_09ac_4770_a06a_684a42b4a14c">
    <rdf:type rdf:resource="http://www.w3.org/2002/07/owl#Class"/>
    <annotations:EMMO_21ae69b4_235e_479d_8dd8_4f756f694c1b xml:lang="en">a</annotations:EMMO_21ae69b4_235e_479d_8dd8_4f756f694c1b>
    <owl:equivalentClass rdf:nodeID="Nfbdae53e1a6340599ccb2416d1eccc4f"/>
    <rdfs:label>LatinSmallLetterA</rdfs:label>
    <rdfs:subClassOf rdf:resource="http://emmo.info/emmo/middle/metrology#EMMO_e13b2173_1dec_4b97_9ac1_1dc4b418612a"/>
  </rdf:Description>
  <rdf:Description rdf:about="http://emmo.info/emmo/middle/isq#EMMO_1f087811_06cb_42d5_90fb_25d0e7e068ef">
    <rdfs:subClassOf rdf:nodeID="Ndc68ffc3e0824b509c5111fb2f6aabab"/>
    <annotations:EMMO_967080e5_2f42_4eb2_a3a9_c58143e835f9>Any interaction that, when unopposed, will change the motion of an object.</annotations:EMMO_967080e5_2f42_4eb2_a3a9_c58143e835f9>
    <rdfs:label xml:lang="en">Force</rdfs:label>
    <rdfs:subClassOf rdf:resource="http://emmo.info/emmo/middle/isq#EMMO_2946d40b_24a1_47fa_8176_e3f79bb45064"/>
    <annotations:EMMO_fe015383_afb3_44a6_ae86_043628697aa2>https://doi.org/10.1351/goldbook.F02480</annotations:EMMO_fe015383_afb3_44a6_ae86_043628697aa2>
    <rdf:type rdf:resource="http://www.w3.org/2002/07/owl#Class"/>
    <annotations:EMMO_6dd685dd_1895_46e4_b227_be9f7d643c25>http://dbpedia.org/page/Force</annotations:EMMO_6dd685dd_1895_46e4_b227_be9f7d643c25>
  </rdf:Description>
  <rdf:Description rdf:about="http://emmo.info/emmo/middle/reductionistic#EMMO_36c79456_e29c_400d_8bd3_0eedddb82652">
    <rdfs:comment>There is no change in granularity or cardinality of parts within a state.

The use of spatial direct parthood in state definition means that a state cannot overlap in space another state that is direct part of the same whole.</rdfs:comment>
    <rdfs:comment>The definition of 'State' implies that its spatial direct parts (i.e. 'physicals') are not gained or lost during its temporal extension (they exist from the left to the right side of the time interval), so that the cardinality of spatial direct parts in a 'State' is constant.

This does not mean that there cannot be a change in the internal structure of the 'State' direct parts. It means only that this change must not affect the existence of the direct part itself.

There is no change in granularity or cardinality of direct parts of a 'State'.

The use of spatial direct parthood in 'State' definition means that a 'State' cannot overlap in space another 'State'.</rdfs:comment>
    <rdf:type rdf:resource="http://www.w3.org/2002/07/owl#Class"/>
    <annotations:EMMO_967080e5_2f42_4eb2_a3a9_c58143e835f9>A 'Physical' which is a tessellation of spatial direct parts.</annotations:EMMO_967080e5_2f42_4eb2_a3a9_c58143e835f9>
    <rdfs:comment>The usefulness of 'State' is that it makes it possible to describe the evolution in time of an 'Existent' in terms of series of 'State'-s that can take into account the disappearance or appearance of parts within a 'Physical'. 

A 'State' is a recognizable granularity level of matter, in the sense that its direct parts do not appear or disappear within its lifetime as it can be for a generic 'Existent'.</rdfs:comment>
    <rdfs:comment>Direct partitions declaration is a choice of the ontologist that choses the classes to be used as direct parts, according to its own world view.

A 'State' can always be direct partitioned in 'Elementary'-s and 'Void' or 'Physical'.

e.g. the water in my glass can be seen as a single object without declaring direct parts, or as made of H2O molecules direct parts.</rdfs:comment>
    <annotations:EMMO_b432d2d5_25f4_4165_99c5_5935a7763c1a>e.g. the existent in my glass is declared at t = t_start as made of two direct parts: the ice and the water. It will continue to exists as state as long as the ice is completely melt at t = t_end. The new state will be completely made of water. Between t_start and t_end there is an exchange of molecules between the ice and the water, but this does not affect the existence of the two states.

If we partition the existent in my glass as ice surrounded by several molecules (we do not use the object water as direct part) then the appearance of a molecule coming from the ice will cause a state to end and another state to begin.</annotations:EMMO_b432d2d5_25f4_4165_99c5_5935a7763c1a>
    <rdfs:label xml:lang="en">State</rdfs:label>
    <rdfs:subClassOf rdf:nodeID="N087e2051134e44e1b5f5024ec3fcac14"/>
  </rdf:Description>
  <rdf:Description rdf:about="http://emmo.info/emmo/middle/math#EMMO_54ee6b5e_5261_44a8_86eb_5717e7fdb9d0">
    <annotations:EMMO_967080e5_2f42_4eb2_a3a9_c58143e835f9>The class of general mathematical symbolic objects respecting mathematical syntactic rules.</annotations:EMMO_967080e5_2f42_4eb2_a3a9_c58143e835f9>
    <rdfs:label xml:lang="en">Mathematical</rdfs:label>
    <rdf:type rdf:resource="http://www.w3.org/2002/07/owl#Class"/>
    <rdfs:subClassOf rdf:resource="http://emmo.info/emmo/middle/perceptual#EMMO_d8d2144e_5c8d_455d_a643_5caf4d8d9df8"/>
  </rdf:Description>
  <rdf:Description rdf:about="http://emmo.info/emmo/middle/isq#EMMO_ffb73b1e_5786_43e4_a964_cb32ac7affb7">
    <annotations:EMMO_fe015383_afb3_44a6_ae86_043628697aa2>https://doi.org/10.1351/goldbook.E01925</annotations:EMMO_fe015383_afb3_44a6_ae86_043628697aa2>
    <rdfs:label xml:lang="en">ElectricConductance</rdfs:label>
    <annotations:EMMO_967080e5_2f42_4eb2_a3a9_c58143e835f9>Measure of the ease for electric current to pass through a material.</annotations:EMMO_967080e5_2f42_4eb2_a3a9_c58143e835f9>
    <rdfs:comment>Inverse of 'ElectricalResistance'.</rdfs:comment>
    <annotations:EMMO_6dd685dd_1895_46e4_b227_be9f7d643c25>http://dbpedia.org/page/Electrical_resistance_and_conductance</annotations:EMMO_6dd685dd_1895_46e4_b227_be9f7d643c25>
    <rdf:type rdf:resource="http://www.w3.org/2002/07/owl#Class"/>
    <rdfs:subClassOf rdf:resource="http://emmo.info/emmo/middle/isq#EMMO_2946d40b_24a1_47fa_8176_e3f79bb45064"/>
    <annotations:EMMO_21ae69b4_235e_479d_8dd8_4f756f694c1b>Conductance</annotations:EMMO_21ae69b4_235e_479d_8dd8_4f756f694c1b>
    <rdfs:subClassOf rdf:nodeID="N9c7c783836324422bec68ae085446692"/>
  </rdf:Description>
  <rdf:Description rdf:about="http://emmo.info/emmo/middle/holistic#EMMO_ae2d1a96_bfa1_409a_a7d2_03d69e8a125a">
    <rdfs:domain rdf:resource="http://emmo.info/emmo/middle/holistic#EMMO_43e9a05d_98af_41b4_92f6_00f79a09bfce"/>
    <rdfs:subPropertyOf rdf:resource="http://emmo.info/emmo/top/mereotopology#EMMO_17e27c22_37e1_468c_9dd7_95e137f73e7f"/>
    <rdfs:label xml:lang="en">hasParticipant</rdfs:label>
    <rdfs:comment>Participation is not under direct parthood since a process is not strictly related to reductionism, but it's a way to categorize temporal regions by the interpreters.</rdfs:comment>
    <rdfs:comment>Participation is a parthood relation: you must be part (and then be connected) of the process to contribute to it.</rdfs:comment>
    <rdf:type rdf:resource="http://www.w3.org/2002/07/owl#ObjectProperty"/>
    <rdfs:range rdf:resource="http://emmo.info/emmo/middle/holistic#EMMO_49804605_c0fe_4538_abda_f70ba1dc8a5d"/>
    <annotations:EMMO_967080e5_2f42_4eb2_a3a9_c58143e835f9>The relation between a process and an object participating to it.</annotations:EMMO_967080e5_2f42_4eb2_a3a9_c58143e835f9>
  </rdf:Description>
  <rdf:Description rdf:nodeID="Nc20a8b7359104095abf5c2bc9718749e">
    <owl:onProperty rdf:resource="http://emmo.info/emmo/middle/metrology#EMMO_bed1d005_b04e_4a90_94cf_02bc678a8569"/>
    <rdf:type rdf:resource="http://www.w3.org/2002/07/owl#Restriction"/>
    <owl:allValuesFrom rdf:resource="http://emmo.info/emmo/middle/isq#EMMO_3227b821_26a5_4c7c_9c01_5c24483e0bd0"/>
  </rdf:Description>
  <rdf:Description rdf:nodeID="N11017920217c4056af507247e66a0168">
    <owl:onProperty rdf:resource="http://emmo.info/emmo/middle/perceptual#EMMO_23b579e1_8088_45b5_9975_064014026c42"/>
    <rdf:type rdf:resource="http://www.w3.org/2002/07/owl#Restriction"/>
    <owl:hasValue>K</owl:hasValue>
  </rdf:Description>
  <rdf:Description rdf:about="http://emmo.info/emmo">
    <annotations:EMMO_cd5fb112_7ee7_4120_a35d_3ca3e6c3f4ab>Emanuele Ghedini (University of Bologna, IT)
Gerhard Goldbeck (GCL Ltd, UK)
Adham Hashibon (Fraunhofer IWM, DE)
Georg Schmitz (Access, DE)
Jesper Friis (SINTEF, NO)</annotations:EMMO_cd5fb112_7ee7_4120_a35d_3ca3e6c3f4ab>
    <rdfs:comment xml:lang="en">Contacts:
Gerhard Goldbeck
Goldbeck Consulting Ltd (UK)
email: gerhard@goldbeck-consulting.com

Emanuele Ghedini
University of Bologna (IT)
email: emanuele.ghedini@unibo.it</rdfs:comment>
    <owl:versionInfo>The European Materials Modelling Ontology

Version 1.0.0-alpha</owl:versionInfo>
    <annotations:EMMO_5525a055_dda5_4556_8b91_f0d22fa676cc>EMMO is released under a Creative Commons license Attribution 4.0 International (CC BY 4.0)

https://creativecommons.org/licenses/by/4.0/legalcode</annotations:EMMO_5525a055_dda5_4556_8b91_f0d22fa676cc>
    <owl:versionIRI rdf:resource="http://emmo.info/emmo/1.0.0-alpha"/>
    <rdf:type rdf:resource="http://www.w3.org/2002/07/owl#Ontology"/>
    <rdfs:comment>European Materials and Modelling Ontology (EMMO)

EMMO is a multidisciplinary effort to develop a standard representational framework (the ontology) based on current materials modelling knowledge, including physical sciences, analytical philosophy and information and communication technologies. 

It provides the connection between the physical world, materials characterisation world and materials modelling world.</rdfs:comment>
    <rdfs:comment>The EMMO requires FacT++ reasoner plugin in order to visualize all inferences and class hierarchy (ctrl+R hotkey in Protege).</rdfs:comment>
  </rdf:Description>
  <rdf:Description rdf:about="http://emmo.info/emmo/middle/siunits#EMMO_d7b7fd1e_645a_42cb_8f40_85f0d034d3ae">
    <rdfs:label xml:lang="en">Lumen</rdfs:label>
    <rdfs:comment>Measurement unit for luminous flux.</rdfs:comment>
    <rdfs:subClassOf rdf:nodeID="N9ea10f198d0646a995a783878c724a69"/>
    <annotations:EMMO_1f1b164d_ec6a_4faa_8d5e_88bda62316cc>http://qudt.org/vocab/unit/LM</annotations:EMMO_1f1b164d_ec6a_4faa_8d5e_88bda62316cc>
    <rdf:type rdf:resource="http://www.w3.org/2002/07/owl#Class"/>
    <annotations:EMMO_fe015383_afb3_44a6_ae86_043628697aa2>https://doi.org/10.1351/goldbook.L03639</annotations:EMMO_fe015383_afb3_44a6_ae86_043628697aa2>
    <rdfs:subClassOf rdf:nodeID="N1a7f191841c646a88bdd4b34fdf1b2f4"/>
  </rdf:Description>
  <rdf:Description rdf:about="http://emmo.info/emmo/middle/siunits#EMMO_21aaefc1_3f86_4208_b7db_a755f31f0f8c">
    <rdf:type rdf:resource="http://www.w3.org/2002/07/owl#Class"/>
    <rdfs:label xml:lang="en">Hecto</rdfs:label>
    <rdfs:subClassOf rdf:nodeID="N60fc193eaac64e1189724c7a65d086b9"/>
    <rdfs:subClassOf rdf:nodeID="Nfe093601627448f88809ffd10fa8c4af"/>
  </rdf:Description>
  <rdf:Description rdf:about="http://emmo.info/emmo/middle/siunits#EMMO_1d8b370b_c672_4d0c_964e_eaafcbf2f51f">
    <rdf:type rdf:resource="http://www.w3.org/2002/07/owl#Class"/>
    <rdfs:subClassOf rdf:nodeID="Ncf7e356028e249ffbb828d30f5d5455f"/>
    <rdfs:subClassOf rdf:nodeID="N5d76899ac74f4d778405ec2532fdcc1f"/>
    <rdfs:label xml:lang="en">Deka</rdfs:label>
  </rdf:Description>
  <rdf:Description rdf:nodeID="Nc8bc6ccd39e240178a9036dfe08e541a">
    <owl:inverseOf rdf:resource="http://emmo.info/emmo/middle/math#EMMO_3446e167_c576_49d6_846c_215bb8878a55"/>
  </rdf:Description>
  <rdf:Description rdf:about="http://emmo.info/emmo/middle/metrology#EMMO_b081b346_7279_46ef_9a3d_2c088fcd79f4">
    <rdfs:label xml:lang="en">MeasurementUnit</rdfs:label>
    <owl:disjointUnionOf rdf:nodeID="N5e97a5fcfbd24a8caee9f70e38cb21cd"/>
    <rdfs:comment>"Unit symbols are mathematical entities and not abbreviations."

"Symbols for units are treated as mathematical entities. In expressing the value of a quantity as the product of a numerical value and a unit, both the numerical value and the unit may be treated by the ordinary rules of algebra."

https://www.bipm.org/utils/common/pdf/si-brochure/SI-Brochure-9-EN.pdf</rdfs:comment>
    <rdfs:subClassOf rdf:resource="http://emmo.info/emmo/middle/metrology#EMMO_18ce5200_00f5_45bb_8c6f_6fb128cd41ae"/>
    <rdfs:comment>"Real scalar quantity, defined and adopted by convention, with which any other quantity of the same kind can be compared to express the ratio of the second quantity to the first one as a number"
ISO 80000-1</rdfs:comment>
    <annotations:EMMO_967080e5_2f42_4eb2_a3a9_c58143e835f9>A 'Quantity' that stands for the standard reference magnitude of a specific class of measurement processes, defined and adopted by convention or by law.

The numerical quantity value of the 'MeasurementUnit' is conventionally 1 and does not appear.

Quantitative measurement results are expressed as a multiple of the 'MeasurementUnit'.</annotations:EMMO_967080e5_2f42_4eb2_a3a9_c58143e835f9>
    <rdfs:comment>While the SI brochure treats 'MeasurementUnit' as a 'PhysicalQuantity', in the EMMO this is not possible since the latter always has two direct parts, a 'Numerical' and a 'MeasurementUnit', while the former a single 'Symbol'.

SI distinguishes between a quantity (an abstract concept) and the quantity value (a number and a reference). The EMMO, following strict nominalism, considers a SI quantity as a SI quantity value, collapsing the two concepts into one: the 'Quantity'.

So, for the EMMO the symbol "kg" is not a physical quantity but a 'MeasurementUnit', while the string "1 kg" is 'Physical Quantity'.</rdfs:comment>
    <rdf:type rdf:resource="http://www.w3.org/2002/07/owl#Class"/>
  </rdf:Description>
  <rdf:Description rdf:about="http://emmo.info/emmo/top/math#EMMO_91447ec0_fb55_49f2_85a5_3172dff6482c">
    <rdfs:label xml:lang="en">Polynomial</rdfs:label>
    <rdf:type rdf:resource="http://www.w3.org/2002/07/owl#Class"/>
    <rdfs:subClassOf rdf:resource="http://emmo.info/emmo/top/math#EMMO_1aed91a3_d00c_48af_8f43_a0c958b2512a"/>
    <annotations:EMMO_b432d2d5_25f4_4165_99c5_5935a7763c1a>2 * x^2 + x + 3</annotations:EMMO_b432d2d5_25f4_4165_99c5_5935a7763c1a>
  </rdf:Description>
  <rdf:Description rdf:about="http://emmo.info/emmo/middle/siunits#EMMO_a979c531_f9fa_4a6e_93c1.0.0-alpha960241ca6">
    <rdf:type rdf:resource="http://www.w3.org/2002/07/owl#Class"/>
    <annotations:EMMO_1f1b164d_ec6a_4faa_8d5e_88bda62316cc>http://qudt.org/vocab/unit/N</annotations:EMMO_1f1b164d_ec6a_4faa_8d5e_88bda62316cc>
    <rdfs:comment>Measurement unit for force.</rdfs:comment>
    <annotations:EMMO_fe015383_afb3_44a6_ae86_043628697aa2>https://doi.org/10.1351/goldbook.N04135</annotations:EMMO_fe015383_afb3_44a6_ae86_043628697aa2>
    <rdfs:label xml:lang="en">Newton</rdfs:label>
    <rdfs:subClassOf rdf:nodeID="N678532a1c73a4e1586848c8038cb5f20"/>
    <rdfs:subClassOf rdf:nodeID="N8f5e55d1dca4417e8a37c924a4738815"/>
  </rdf:Description>
  <rdf:Description rdf:about="http://emmo.info/emmo/top/semiotics#EMMO_2337e25c_3c60_43fc_a8f9_b11a3f974291">
    <annotations:EMMO_967080e5_2f42_4eb2_a3a9_c58143e835f9>The generic EMMO semiotical relation.</annotations:EMMO_967080e5_2f42_4eb2_a3a9_c58143e835f9>
    <rdf:type rdf:resource="http://www.w3.org/2002/07/owl#ObjectProperty"/>
    <rdfs:label xml:lang="en">semiotical</rdfs:label>
    <rdfs:subPropertyOf rdf:resource="http://emmo.info/emmo/top/mereotopology#EMMO_ec2472ae_cf4a_46a5_8555_1556f5a6c3c5"/>
  </rdf:Description>
  <rdf:Description rdf:nodeID="N5bc2348bc9464ea28c46a48f90cb78cc">
    <owl:onProperty rdf:nodeID="N01254d1904484e50ae6af7e63289f9a0"/>
    <rdf:type rdf:resource="http://www.w3.org/2002/07/owl#Restriction"/>
    <owl:allValuesFrom rdf:nodeID="N4221f08354224e54856c4421ec5e2bc1"/>
  </rdf:Description>
  <rdf:Description rdf:about="http://emmo.info/emmo/middle/physicalistic#EMMO_72d53756_7fb1_46ed_980f_83f47efbe105">
    <annotations:EMMO_967080e5_2f42_4eb2_a3a9_c58143e835f9>The class of individuals that stand for quarks elementary particles.</annotations:EMMO_967080e5_2f42_4eb2_a3a9_c58143e835f9>
    <rdfs:subClassOf rdf:resource="http://emmo.info/emmo/top/physical#EMMO_0f795e3e_c602_4577_9a43_d5a231aa1360"/>
    <rdf:type rdf:resource="http://www.w3.org/2002/07/owl#Class"/>
    <rdfs:label xml:lang="en">Quark</rdfs:label>
  </rdf:Description>
  <rdf:Description rdf:nodeID="Naeadd3ccdc6145bbb481232f62aa348c">
    <owl:onProperty rdf:resource="http://emmo.info/emmo/middle/reductionistic#EMMO_b2282816_b7a3_44c6_b2cb_3feff1ceb7fe"/>
    <rdf:type rdf:resource="http://www.w3.org/2002/07/owl#Restriction"/>
    <owl:someValuesFrom rdf:resource="http://emmo.info/emmo/middle/perceptual#EMMO_057e7d57_aff0_49de_911a_8861d85cef40"/>
  </rdf:Description>
  <rdf:Description rdf:nodeID="N77c359098edf4f7db05f44fa33f9b424">
    <owl:someValuesFrom rdf:resource="http://emmo.info/emmo/middle/isq#EMMO_515b5579_d526_4842_9e6f_ecc34db6f368"/>
    <rdf:type rdf:resource="http://www.w3.org/2002/07/owl#Restriction"/>
    <owl:onProperty rdf:resource="http://emmo.info/emmo/middle/metrology#EMMO_bed1d005_b04e_4a90_94cf_02bc678a8569"/>
  </rdf:Description>
  <rdf:Description rdf:nodeID="Ndee16311420f41f595ae6a1e252dae8d">
    <rdf:type rdf:resource="http://www.w3.org/2002/07/owl#Class"/>
    <owl:unionOf rdf:nodeID="N4a8392ac14244c0fbb77720c5eec6710"/>
  </rdf:Description>
  <rdf:Description rdf:nodeID="N83cabc1e6cd24f879f96578013cf0277">
    <rdf:first rdf:resource="http://emmo.info/emmo/middle/physicalistic#EMMO_25f8b804_9a0b_4387_a3e7_b35bce5365ee"/>
    <rdf:rest rdf:nodeID="N95c3853f088f44f5949d1c5833efd1c5"/>
  </rdf:Description>
  <rdf:Description rdf:nodeID="N3262e7503a9b437db3d8390be2bbd536">
    <owl:allValuesFrom rdf:resource="http://emmo.info/emmo/middle/isq#EMMO_5c003f53_20a2_4bd7_8445_58187e582578"/>
    <rdf:type rdf:resource="http://www.w3.org/2002/07/owl#Restriction"/>
    <owl:onProperty rdf:resource="http://emmo.info/emmo/middle/metrology#EMMO_bed1d005_b04e_4a90_94cf_02bc678a8569"/>
  </rdf:Description>
  <rdf:Description rdf:nodeID="N1140c30c299746e2af8ef10fa86e617b">
    <rdf:type rdf:resource="http://www.w3.org/2002/07/owl#Restriction"/>
    <owl:allValuesFrom rdf:resource="http://emmo.info/emmo/middle/isq#EMMO_53e825d9_1a09_483c_baa7_37501ebfbe1c"/>
    <owl:onProperty rdf:resource="http://emmo.info/emmo/middle/metrology#EMMO_bed1d005_b04e_4a90_94cf_02bc678a8569"/>
  </rdf:Description>
  <rdf:Description rdf:nodeID="N3ba50be97ada433a99cc1a8a9c643f51">
    <owl:someValuesFrom rdf:resource="http://emmo.info/emmo/middle/properties#EMMO_f2d5d3ad_2e00_417f_8849_686f3988d929"/>
    <rdf:type rdf:resource="http://www.w3.org/2002/07/owl#Restriction"/>
    <owl:onProperty rdf:resource="http://emmo.info/emmo/middle/holistic#EMMO_ae2d1a96_bfa1_409a_a7d2_03d69e8a125a"/>
  </rdf:Description>
  <rdf:Description rdf:about="http://emmo.info/emmo/middle/holistic#EMMO_49804605_c0fe_4538_abda_f70ba1dc8a5d">
    <rdf:type rdf:resource="http://www.w3.org/2002/07/owl#Class"/>
    <rdfs:subClassOf rdf:nodeID="Nb9e679207767435fa2fcace810e4fe29"/>
    <rdfs:comment>In the EMMO the relation of participation to a process falls under mereotopology.

Since topological connection means causality, then the only way for a real world object to participate to a process is to be a part of it.</rdfs:comment>
    <rdfs:subClassOf rdf:resource="http://emmo.info/emmo/top/physical#EMMO_c5ddfdba_c074_4aa4_ad6b_1ac4942d300d"/>
    <annotations:EMMO_967080e5_2f42_4eb2_a3a9_c58143e835f9>A portion of a 'Process' that participates to the process with a specific role.</annotations:EMMO_967080e5_2f42_4eb2_a3a9_c58143e835f9>
    <rdfs:label xml:lang="en">Participant</rdfs:label>
  </rdf:Description>
  <rdf:Description rdf:nodeID="N292a284bf7c54545bf257eff64fe4309">
    <rdf:first rdf:resource="http://emmo.info/emmo/middle/metrology#EMMO_7d2afa66_ae9e_4095_a9bf_421d0be401b6"/>
    <rdf:rest rdf:resource="http://www.w3.org/1999/02/22-rdf-syntax-ns#nil"/>
  </rdf:Description>
  <rdf:Description rdf:nodeID="N5a01ad4d96544ed499d895ee3b1d1581">
    <rdf:rest rdf:nodeID="N5e7de695618f44cabf297789a7bd673c"/>
    <rdf:first rdf:resource="http://emmo.info/emmo/middle/siunits#EMMO_58a650f0_a638_4743_8439_535a325e5c4c"/>
  </rdf:Description>
  <rdf:Description rdf:nodeID="Nfd269989e79f4d809c092a1a1bd6809b">
    <rdf:type rdf:resource="http://www.w3.org/2002/07/owl#Restriction"/>
    <owl:onProperty rdf:resource="http://emmo.info/emmo/top/physical#EMMO_f68030be_94b8_4c61_a161_886468558054"/>
    <owl:someValuesFrom rdf:resource="http://emmo.info/emmo/middle/manufacturing#EMMO_494b372c_cfdf_47d3_a4de_5e037c540de8"/>
  </rdf:Description>
  <rdf:Description rdf:about="http://emmo.info/emmo/middle/materials#EMMO_4588526f_8553_4f4d_aa73_a483e88d599b">
    <rdf:type rdf:resource="http://www.w3.org/2002/07/owl#Class"/>
    <annotations:EMMO_967080e5_2f42_4eb2_a3a9_c58143e835f9>A standalone atom that has no net charge.</annotations:EMMO_967080e5_2f42_4eb2_a3a9_c58143e835f9>
    <rdfs:label xml:lang="en">NeutralAtom</rdfs:label>
  </rdf:Description>
  <rdf:Description rdf:nodeID="N19f583718273476fa52c6b4c94b35b0a">
    <rdf:rest rdf:nodeID="Ne2c8041f5db64d61b21c5d8eecdcb3a3"/>
    <rdf:first rdf:resource="http://emmo.info/emmo/middle/siunits#EMMO_3a204900_2b33_47d1_b444_815cc4c8cffa"/>
  </rdf:Description>
  <rdf:Description rdf:nodeID="Ne48cfa7d3e4946a9893d44c19ad83f53">
    <owl:onProperty rdf:resource="http://emmo.info/emmo/middle/metrology#EMMO_67fc0a36_8dcb_4ffa_9a43_31074efa3296"/>
    <owl:allValuesFrom rdf:nodeID="N82279f1bbe1e47348965d20b186a0fe8"/>
    <rdf:type rdf:resource="http://www.w3.org/2002/07/owl#Restriction"/>
  </rdf:Description>
  <rdf:Description rdf:nodeID="Nbe4764aa85bd432e87d21fe8771325ef">
    <rdf:first rdf:resource="http://emmo.info/emmo/middle/reductionistic#EMMO_52211e5e_d767_4812_845e_eb6b402c476a"/>
    <rdf:rest rdf:resource="http://www.w3.org/1999/02/22-rdf-syntax-ns#nil"/>
  </rdf:Description>
  <rdf:Description rdf:about="http://emmo.info/emmo/middle/perceptual#EMMO_3e309118_e8b7_4021_80f4_642d2df65d94">
    <rdfs:label xml:lang="en">Line</rdfs:label>
    <rdfs:subClassOf rdf:resource="http://emmo.info/emmo/middle/perceptual#EMMO_0c576e13_4ee7_4f3d_bfe9_1614243df018"/>
    <rdf:type rdf:resource="http://www.w3.org/2002/07/owl#Class"/>
  </rdf:Description>
  <rdf:Description rdf:about="http://emmo.info/emmo/middle/siunits#EMMO_99296e55_53f7_4333_9e06_760ad175a1b9">
    <rdfs:label xml:lang="en">SpeedOfLightInVacuum</rdfs:label>
    <rdfs:subClassOf rdf:nodeID="N3747877166994a51b190984b959657d8"/>
    <annotations:EMMO_6dd685dd_1895_46e4_b227_be9f7d643c25>http://dbpedia.org/page/Speed_of_light</annotations:EMMO_6dd685dd_1895_46e4_b227_be9f7d643c25>
    <annotations:EMMO_fe015383_afb3_44a6_ae86_043628697aa2>https://doi.org/10.1351/goldbook.S05854</annotations:EMMO_fe015383_afb3_44a6_ae86_043628697aa2>
    <annotations:EMMO_967080e5_2f42_4eb2_a3a9_c58143e835f9>The speed of light in vacuum.</annotations:EMMO_967080e5_2f42_4eb2_a3a9_c58143e835f9>
    <rdf:type rdf:resource="http://www.w3.org/2002/07/owl#Class"/>
    <annotations:EMMO_1f1b164d_ec6a_4faa_8d5e_88bda62316cc>http://physics.nist.gov/cuu/CODATA-Value_SpeedOfLightInVacuum</annotations:EMMO_1f1b164d_ec6a_4faa_8d5e_88bda62316cc>
  </rdf:Description>
  <rdf:Description rdf:nodeID="N1abbf6e8a44a480eb8030eaaa00b0514">
    <owl:allValuesFrom rdf:resource="http://emmo.info/emmo/middle/isq#EMMO_a77a0a4b_6bd2_42b2_be27_4b63cebbb59e"/>
    <rdf:type rdf:resource="http://www.w3.org/2002/07/owl#Restriction"/>
    <owl:onProperty rdf:resource="http://emmo.info/emmo/middle/metrology#EMMO_bed1d005_b04e_4a90_94cf_02bc678a8569"/>
  </rdf:Description>
  <rdf:Description rdf:nodeID="Nef79e15b8fc34f4da019ca456a7df6fc">
    <rdf:type rdf:resource="http://www.w3.org/2002/07/owl#Restriction"/>
    <owl:onProperty rdf:resource="http://emmo.info/emmo/middle/metrology#EMMO_bed1d005_b04e_4a90_94cf_02bc678a8569"/>
    <owl:allValuesFrom rdf:resource="http://emmo.info/emmo/middle/isq#EMMO_2e7e5796_4a80_4d73_bb84_f31138446c0c"/>
  </rdf:Description>
  <rdf:Description rdf:about="http://emmo.info/emmo/top/annotations#EMMO_21ae69b4_235e_479d_8dd8_4f756f694c1b">
    <rdf:type rdf:resource="http://www.w3.org/2002/07/owl#AnnotationProperty"/>
    <rdfs:label xml:lang="en">altLabel</rdfs:label>
    <rdfs:subPropertyOf rdf:resource="http://www.w3.org/2000/01/rdf-schema#comment"/>
  </rdf:Description>
  <rdf:Description rdf:nodeID="N80e378230315452e82c70e31e411b9d7">
    <rdf:rest rdf:nodeID="N526846521e6b4ec1a49a311418e1f8a2"/>
    <rdf:first rdf:resource="http://emmo.info/emmo/middle/siunits#EMMO_74931b1b_c133_4e59_9a75_1bf0e1626201"/>
  </rdf:Description>
  <rdf:Description rdf:nodeID="N1253ed78d81c4d68b74171395295b153">
    <rdf:rest rdf:nodeID="N87080e819ab9442d8e5c7af96544af1c"/>
    <rdf:first rdf:resource="http://emmo.info/emmo/middle/siunits#EMMO_1d8b370b_c672_4d0c_964e_eaafcbf2f51f"/>
  </rdf:Description>
  <rdf:Description rdf:about="http://emmo.info/emmo/middle/models#EMMO_e5438930_04e7_4d42_ade5_3700d4a52ab7">
    <rdf:type rdf:resource="http://www.w3.org/2002/07/owl#Class"/>
    <rdfs:subClassOf rdf:nodeID="N1375e20c0adb447c8047a350ad3817a0"/>
    <rdfs:label xml:lang="en">MaterialRelation</rdfs:label>
    <annotations:EMMO_967080e5_2f42_4eb2_a3a9_c58143e835f9>An 'equation' that stands for a physical assumption specific to a material, and provides an expression for a 'physics_quantity' (the dependent variable) as function of other variables, physics_quantity or data (independent variables).</annotations:EMMO_967080e5_2f42_4eb2_a3a9_c58143e835f9>
    <annotations:EMMO_b432d2d5_25f4_4165_99c5_5935a7763c1a>The Lennard-Jones potential.

A force field.

An Hamiltonian.</annotations:EMMO_b432d2d5_25f4_4165_99c5_5935a7763c1a>
    <rdfs:comment>A material_relation can e.g. return a predefined number, return a database query, be an equation that depends on other physics_quantities.</rdfs:comment>
    <rdfs:subClassOf rdf:resource="http://emmo.info/emmo/middle/math#EMMO_e56ee3eb_7609_4ae1_8bed_51974f0960a6"/>
  </rdf:Description>
  <rdf:Description rdf:about="http://emmo.info/emmo/middle/siunits#EMMO_da1dd4a7_c611_4ad4_bef6_7646f28aa598">
    <rdfs:label xml:lang="en">Lux</rdfs:label>
    <annotations:EMMO_1f1b164d_ec6a_4faa_8d5e_88bda62316cc>http://qudt.org/vocab/unit/LUX</annotations:EMMO_1f1b164d_ec6a_4faa_8d5e_88bda62316cc>
    <rdf:type rdf:resource="http://www.w3.org/2002/07/owl#Class"/>
    <rdfs:comment>Measurement unit for illuminance.</rdfs:comment>
    <annotations:EMMO_fe015383_afb3_44a6_ae86_043628697aa2>https://doi.org/10.1351/goldbook.L03651</annotations:EMMO_fe015383_afb3_44a6_ae86_043628697aa2>
    <rdfs:subClassOf rdf:nodeID="N029d3a2c0e994e9d9cfb6c53adca69b5"/>
    <rdfs:subClassOf rdf:nodeID="Nb8bfb9bf16dc4984be0dd6eecb3b74f7"/>
  </rdf:Description>
  <rdf:Description rdf:about="http://emmo.info/emmo/middle/siunits#EMMO_9bfd6f1e_b0ce_459c_beb7_8f1f41708bba">
    <annotations:EMMO_1f1b164d_ec6a_4faa_8d5e_88bda62316cc>http://qudt.org/vocab/unit/KiloGM</annotations:EMMO_1f1b164d_ec6a_4faa_8d5e_88bda62316cc>
    <annotations:EMMO_fe015383_afb3_44a6_ae86_043628697aa2>https://doi.org/10.1351/goldbook.K03391</annotations:EMMO_fe015383_afb3_44a6_ae86_043628697aa2>
    <rdfs:label xml:lang="en">Kilogram</rdfs:label>
    <rdf:type rdf:resource="http://www.w3.org/2002/07/owl#Class"/>
    <annotations:EMMO_70fe84ff_99b6_4206_a9fc_9a8931836d84>The kilogram, symbol kg, is the SI unit of mass. It is defined by taking the fixed numerical value of the Planck constant h to be 6.62607015×10−34 when expressed in the unit J s, which is equal to kg m2 s−1, where the metre and the second are defined in terms of c and ∆νCs.</annotations:EMMO_70fe84ff_99b6_4206_a9fc_9a8931836d84>
    <rdfs:subClassOf rdf:nodeID="N69a645702fd94045828660e1e4876123"/>
    <rdfs:subClassOf rdf:nodeID="Nbfa7d50fceba4cd2985bbbd559d775d4"/>
  </rdf:Description>
  <rdf:Description rdf:about="http://emmo.info/emmo/middle/perceptual#EMMO_b5957cef_a287_442d_a3ce_fd39f20ba1cd">
    <rdfs:subClassOf rdf:resource="http://emmo.info/emmo/middle/perceptual#EMMO_c74da218_9147_4f03_92d1_8894abca55f3"/>
    <rdfs:label xml:lang="en">Geometrical</rdfs:label>
    <rdfs:comment>A 'geometrical' stands for real world objects that express a geometrical concept.

This can be achieved in many different ways. For example, a line can be expressed by:
a) an equation like y=mx+q, which is both an 'equation' and a 'geometrical'
b) a line drawn with a pencil on a paper, which is simply a 'graphical' object
c) a set of axioms, when the properties of a line are inferred by the interpreter reading them, that are both 'graphical' and also 'formula'

The case a) is a geometrical and mathematical, b) is geometrical and pictorial, while c) is geometrical and a composition of idiomatic strings.</rdfs:comment>
    <rdf:type rdf:resource="http://www.w3.org/2002/07/owl#Class"/>
    <annotations:EMMO_967080e5_2f42_4eb2_a3a9_c58143e835f9>A 'graphical' aimed to represent a geometrical concept.</annotations:EMMO_967080e5_2f42_4eb2_a3a9_c58143e835f9>
  </rdf:Description>
  <rdf:Description rdf:about="http://emmo.info/emmo/middle/metrology#EMMO_5ebd5e01_0ed3_49a2_a30d_cd05cbe72978">
    <annotations:EMMO_1f1b164d_ec6a_4faa_8d5e_88bda62316cc>http://qudt.org/vocab/unit/UNITLESS</annotations:EMMO_1f1b164d_ec6a_4faa_8d5e_88bda62316cc>
    <rdfs:label xml:lang="en">UnitOne</rdfs:label>
    <annotations:EMMO_b432d2d5_25f4_4165_99c5_5935a7763c1a>Refractive index or volume fraction.</annotations:EMMO_b432d2d5_25f4_4165_99c5_5935a7763c1a>
    <rdfs:subClassOf rdf:resource="http://emmo.info/emmo/middle/metrology#EMMO_db716151_6b73_45ff_910c_d182fdcbb4f5"/>
    <annotations:EMMO_967080e5_2f42_4eb2_a3a9_c58143e835f9>Represents the number 1, used as an explicit unit to say something has no units.</annotations:EMMO_967080e5_2f42_4eb2_a3a9_c58143e835f9>
    <rdf:type rdf:resource="http://www.w3.org/2002/07/owl#Class"/>
    <annotations:EMMO_b432d2d5_25f4_4165_99c5_5935a7763c1a>Typically used for ratios of two units whos dimensions cancels out.</annotations:EMMO_b432d2d5_25f4_4165_99c5_5935a7763c1a>
  </rdf:Description>
  <rdf:Description rdf:nodeID="Na7744b3138c44408b226e6f72191ab57">
    <rdf:first rdf:resource="http://emmo.info/emmo/middle/perceptual#EMMO_a1083d0a_c1fb_471f_8e20_a98f881ad527"/>
    <rdf:rest rdf:resource="http://www.w3.org/1999/02/22-rdf-syntax-ns#nil"/>
  </rdf:Description>
  <rdf:Description rdf:nodeID="N90551f61951d423298057091440fae38">
    <rdf:type rdf:resource="http://www.w3.org/2002/07/owl#Restriction"/>
    <owl:allValuesFrom rdf:resource="http://emmo.info/emmo/middle/isq#EMMO_3ecff38b_b3cf_4a78_b49f_8580abf8715b"/>
    <owl:onProperty rdf:resource="http://emmo.info/emmo/middle/metrology#EMMO_bed1d005_b04e_4a90_94cf_02bc678a8569"/>
  </rdf:Description>
  <rdf:Description rdf:about="http://emmo.info/emmo/top/annotations#EMMO_fe015383_afb3_44a6_ae86_043628697aa2">
    <rdf:type rdf:resource="http://www.w3.org/2002/07/owl#AnnotationProperty"/>
    <rdfs:comment>DOI to corresponding concept in IUPAC</rdfs:comment>
    <rdfs:seeAlso>https://goldbook.iupac.org/</rdfs:seeAlso>
    <rdfs:label xml:lang="en">iupacDoi</rdfs:label>
    <rdfs:subPropertyOf rdf:resource="http://www.w3.org/2000/01/rdf-schema#seeAlso"/>
  </rdf:Description>
  <rdf:Description rdf:nodeID="Ncc15c60739e74988852f3e46ac53617a">
    <owl:onProperty rdf:resource="http://emmo.info/emmo/middle/metrology#EMMO_bed1d005_b04e_4a90_94cf_02bc678a8569"/>
    <owl:someValuesFrom rdf:resource="http://emmo.info/emmo/middle/isq#EMMO_2e7e5796_4a80_4d73_bb84_f31138446c0c"/>
    <rdf:type rdf:resource="http://www.w3.org/2002/07/owl#Restriction"/>
  </rdf:Description>
  <rdf:Description rdf:about="http://emmo.info/emmo/middle/metrology#EMMO_c46f091c_0420_4c1a_af30_0a2c8ebcf7d7">
    <annotations:EMMO_967080e5_2f42_4eb2_a3a9_c58143e835f9>"Quantity, defined by a conventional measurement procedure, for which a total ordering relation can be established, according to magnitude, with other quantities of the same kind, but for which no algebraic operations among those quantities exist"
International vocabulary of metrology (VIM)</annotations:EMMO_967080e5_2f42_4eb2_a3a9_c58143e835f9>
    <rdfs:label xml:lang="en">OrdinalQuantity</rdfs:label>
    <annotations:EMMO_b432d2d5_25f4_4165_99c5_5935a7763c1a>Hardness
Resilience</annotations:EMMO_b432d2d5_25f4_4165_99c5_5935a7763c1a>
    <rdfs:comment>"Ordinal quantities, such as Rockwell C hardness, are usually not considered to be part of a system of quantities because they are related to other quantities through empirical relations only."
International vocabulary of metrology (VIM)</rdfs:comment>
    <rdf:type rdf:resource="http://www.w3.org/2002/07/owl#Class"/>
  </rdf:Description>
  <rdf:Description rdf:about="http://emmo.info/emmo/top/semiotics#EMMO_6f5af708_f825_4feb_a0d1_a8d813d3022b">
    <rdfs:label xml:lang="en">Object</rdfs:label>
    <annotations:EMMO_967080e5_2f42_4eb2_a3a9_c58143e835f9>The object, in Peirce semiotics.</annotations:EMMO_967080e5_2f42_4eb2_a3a9_c58143e835f9>
    <rdfs:comment>Here is assumed that the concept of 'object' is always relative to a 'semiotic' process. An 'object' does not exists per se, but it's always part of an interpretation.

The EMMO relies on strong reductionism, i.e. everything real is a formless collection of elementary particles: we give a meaning to real world entities only by giving them boundaries and defining them using 'sign'-s. 

In this way the 'sign'-ed entity become and 'object', and the 'object' is the basic entity needed in order to apply a logical formalism to the real world entities (i.e. we can speak of it through its sign, and use logics on it through its sign).</rdfs:comment>
    <rdfs:subClassOf rdf:resource="http://emmo.info/emmo/top/semiotics#EMMO_b803f122_4acb_4064_9d71_c1e5fd091fc9"/>
    <rdf:type rdf:resource="http://www.w3.org/2002/07/owl#Class"/>
  </rdf:Description>
  <rdf:Description rdf:nodeID="Ne50be8d65a20431f96870b94a3f42210">
    <owl:onProperty rdf:resource="http://emmo.info/emmo/middle/metrology#EMMO_67fc0a36_8dcb_4ffa_9a43_31074efa3296"/>
    <rdf:type rdf:resource="http://www.w3.org/2002/07/owl#Restriction"/>
    <owl:allValuesFrom rdf:nodeID="Nf3589ffb1cf443308ea993370aed21e9"/>
  </rdf:Description>
  <rdf:Description rdf:nodeID="N78abee4c8b9b4fdcad191afc7beecd19">
    <owl:onProperty rdf:resource="http://emmo.info/emmo/middle/perceptual#EMMO_23b579e1_8088_45b5_9975_064014026c42"/>
    <owl:hasValue>n</owl:hasValue>
    <rdf:type rdf:resource="http://www.w3.org/2002/07/owl#Restriction"/>
  </rdf:Description>
  <rdf:Description rdf:about="http://emmo.info/emmo/middle/perceptual#EMMO_50ea1ec5_f157_41b0_b46b_a9032f17ca10">
    <rdfs:comment>A string is made of concatenated symbols whose arrangement is one-dimensional. Each symbol can have only one previous and one next neighborhood (bidirectional list).</rdfs:comment>
    <annotations:EMMO_967080e5_2f42_4eb2_a3a9_c58143e835f9>A physical made of more than one symbol sequentially arranged.</annotations:EMMO_967080e5_2f42_4eb2_a3a9_c58143e835f9>
    <rdfs:comment>A string is not requested to respect any syntactic rule: it's simply directly made of symbols.</rdfs:comment>
    <rdfs:subClassOf rdf:resource="http://emmo.info/emmo/middle/perceptual#EMMO_057e7d57_aff0_49de_911a_8861d85cef40"/>
    <rdfs:label xml:lang="en">String</rdfs:label>
    <annotations:EMMO_b432d2d5_25f4_4165_99c5_5935a7763c1a>The word "cat" considered as a collection of 'symbol'-s respecting the rules of english language. 

In this example the 'symbolic' entity "cat" is not related to the real cat, but it is only a word (like it would be to an italian person that ignores the meaning of this english word).

If an 'interpreter' skilled in english language is involved in a 'semiotic' process with this word, that "cat" became also a 'sign' i.e. it became for the 'interpreter' a representation for a real cat.</annotations:EMMO_b432d2d5_25f4_4165_99c5_5935a7763c1a>
    <rdf:type rdf:resource="http://www.w3.org/2002/07/owl#Class"/>
    <rdfs:subClassOf rdf:nodeID="Ncc9730a5c39940f3ab51d513ccb2a809"/>
    <rdfs:subClassOf rdf:nodeID="N6223cb60490742ae8635125b5524d030"/>
  </rdf:Description>
  <rdf:Description rdf:about="http://emmo.info/emmo/top/math#EMMO_1cba0b27_15d0_4326_933f_379d0b3565b6">
    <rdfs:label xml:lang="en">Matrix</rdfs:label>
    <rdfs:subClassOf rdf:resource="http://emmo.info/emmo/top/math#EMMO_28fbea28_2204_4613_87ff_6d877b855fcd"/>
    <rdf:type rdf:resource="http://www.w3.org/2002/07/owl#Class"/>
  </rdf:Description>
  <rdf:Description rdf:about="http://emmo.info/emmo/middle/isq#EMMO_f6070071_d054_4b17_9d2d_f446f7147d0f">
    <rdfs:label xml:lang="en">MassSquareLengthPerSquareTimeDimension</rdfs:label>
    <rdfs:subClassOf rdf:resource="http://emmo.info/emmo/middle/metrology#EMMO_9895a1b4_f0a5_4167_ac5e_97db40b8bfcc"/>
    <rdf:type rdf:resource="http://www.w3.org/2002/07/owl#Class"/>
    <owl:equivalentClass rdf:nodeID="N23ef7077e59e434bb6ba7bb6a8ab5b3a"/>
  </rdf:Description>
  <rdf:Description rdf:about="http://emmo.info/emmo/top/semiotics#EMMO_eb3518bf_f799_4f9e_8c3e_ce59af11453b">
    <rdfs:range rdf:resource="http://emmo.info/emmo/top/semiotics#EMMO_35d2e130_6e01_41ed_94f7_00b333d46cf9"/>
    <rdf:type rdf:resource="http://www.w3.org/2002/07/owl#ObjectProperty"/>
    <rdfs:label xml:lang="en">hasConvention</rdfs:label>
    <rdfs:subPropertyOf rdf:resource="http://emmo.info/emmo/top/semiotics#EMMO_60577dea_9019_4537_ac41_80b0fb563d41"/>
  </rdf:Description>
  <rdf:Description rdf:about="http://emmo.info/emmo/middle/siunits#EMMO_e75f580e_52bf_4dd5_af70_df409cec08fd">
    <rdf:type rdf:resource="http://www.w3.org/2002/07/owl#Class"/>
    <rdfs:label xml:lang="en">Hertz</rdfs:label>
    <rdfs:comment>Measurement unit for frequence.</rdfs:comment>
    <annotations:EMMO_fe015383_afb3_44a6_ae86_043628697aa2>https://doi.org/10.1351/goldbook.H02785</annotations:EMMO_fe015383_afb3_44a6_ae86_043628697aa2>
    <rdfs:subClassOf rdf:nodeID="N05665de6f15f469b993e67d5181bc395"/>
    <annotations:EMMO_1f1b164d_ec6a_4faa_8d5e_88bda62316cc>http://qudt.org/vocab/unit/HZ</annotations:EMMO_1f1b164d_ec6a_4faa_8d5e_88bda62316cc>
    <rdfs:subClassOf rdf:nodeID="Ndef00d53241c45889cfebd5f75c1cca5"/>
  </rdf:Description>
  <rdf:Description rdf:nodeID="Nea0cee0abc004367b4ea3f8974e035d3">
    <owl:onProperty rdf:resource="http://emmo.info/emmo/middle/metrology#EMMO_bed1d005_b04e_4a90_94cf_02bc678a8569"/>
    <owl:someValuesFrom rdf:resource="http://emmo.info/emmo/middle/isq#EMMO_585e0ff0_9429_4d3c_b578_58abb1ba21d1"/>
    <rdf:type rdf:resource="http://www.w3.org/2002/07/owl#Restriction"/>
  </rdf:Description>
  <rdf:Description rdf:nodeID="Nb14bc769d574461bb3801212c118898b">
    <owl:onProperty rdf:nodeID="N9f97745668f24fb18e046217a2c4bfc7"/>
    <rdf:type rdf:resource="http://www.w3.org/2002/07/owl#Restriction"/>
    <owl:allValuesFrom rdf:nodeID="Ndbf9693d60d842ef85f3dd7e11e7d3a8"/>
  </rdf:Description>
  <rdf:Description rdf:about="http://emmo.info/emmo/middle/siunits#EMMO_00199e76_69dc_45b6_a9c6_98cc90cdc0f5">
    <rdfs:label xml:lang="en">Gray</rdfs:label>
    <annotations:EMMO_1f1b164d_ec6a_4faa_8d5e_88bda62316cc>http://qudt.org/vocab/unit/GRAY</annotations:EMMO_1f1b164d_ec6a_4faa_8d5e_88bda62316cc>
    <rdfs:comment>Measurement unit for absorbed dose.</rdfs:comment>
    <rdf:type rdf:resource="http://www.w3.org/2002/07/owl#Class"/>
    <rdfs:subClassOf rdf:nodeID="Nda6fe31e41b04feba88025e8723d9eb2"/>
    <annotations:EMMO_fe015383_afb3_44a6_ae86_043628697aa2>https://doi.org/10.1351/goldbook.G02696</annotations:EMMO_fe015383_afb3_44a6_ae86_043628697aa2>
    <rdfs:subClassOf rdf:nodeID="N5129722f30de4998bc8863ac6758cbbd"/>
  </rdf:Description>
  <rdf:Description rdf:about="http://emmo.info/emmo/middle/siunits#EMMO_080052a1_f295_44be_a60f_1326ce13f1ba">
    <annotations:EMMO_1f1b164d_ec6a_4faa_8d5e_88bda62316cc>http://qudt.org/vocab/unit/W</annotations:EMMO_1f1b164d_ec6a_4faa_8d5e_88bda62316cc>
    <rdfs:label xml:lang="en">Watt</rdfs:label>
    <rdfs:subClassOf rdf:nodeID="N827028b4dd5f475da6fb66673ade2d27"/>
    <rdfs:comment>Measurement unit for power.</rdfs:comment>
    <annotations:EMMO_fe015383_afb3_44a6_ae86_043628697aa2>https://doi.org/10.1351/goldbook.W06656</annotations:EMMO_fe015383_afb3_44a6_ae86_043628697aa2>
    <rdfs:subClassOf rdf:nodeID="Nd00f08e47d5c4f7c89d89405ac36d25e"/>
    <rdf:type rdf:resource="http://www.w3.org/2002/07/owl#Class"/>
  </rdf:Description>
  <rdf:Description rdf:nodeID="Na236e4fed321414bb86860a10a47aaf8">
    <owl:hasValue>sr</owl:hasValue>
    <rdf:type rdf:resource="http://www.w3.org/2002/07/owl#Restriction"/>
    <owl:onProperty rdf:resource="http://emmo.info/emmo/middle/perceptual#EMMO_23b579e1_8088_45b5_9975_064014026c42"/>
  </rdf:Description>
  <rdf:Description rdf:about="http://emmo.info/emmo/middle/properties#EMMO_1b52ee70_121e_4d8d_8419_3f97cd0bd89c">
    <rdfs:subClassOf rdf:resource="http://emmo.info/emmo/top/semiotics#EMMO_0527413c_b286_4e9c_b2d0_03fb2a038dee"/>
    <rdfs:subClassOf rdf:nodeID="Nd9a0a27607b544b1b9f670cccb04fc4a"/>
    <rdfs:label xml:lang="en">Observer</rdfs:label>
    <rdf:type rdf:resource="http://www.w3.org/2002/07/owl#Class"/>
    <annotations:EMMO_967080e5_2f42_4eb2_a3a9_c58143e835f9>An 'interpreter' that perceives another 'entity' (the 'object') through a specific perception mechanism and produces a 'property' (the 'sign') that stands for the result of that particular perception.</annotations:EMMO_967080e5_2f42_4eb2_a3a9_c58143e835f9>
  </rdf:Description>
  <rdf:Description rdf:about="http://emmo.info/emmo/middle/siunits#EMMO_42955b2d_b465_4666_86cc_ea3c2d685753">
    <rdfs:label xml:lang="en">Atto</rdfs:label>
    <rdfs:subClassOf rdf:nodeID="Nb5d10f557dea460fb77939003b6572a7"/>
    <rdf:type rdf:resource="http://www.w3.org/2002/07/owl#Class"/>
    <rdfs:subClassOf rdf:nodeID="N56bbb48c32074cf586be02fce15780ee"/>
  </rdf:Description>
  <rdf:Description rdf:about="http://emmo.info/emmo/middle/properties#EMMO_2a888cdf_ec4a_4ec5_af1c_0343372fc978">
    <rdf:type rdf:resource="http://www.w3.org/2002/07/owl#Class"/>
    <annotations:EMMO_967080e5_2f42_4eb2_a3a9_c58143e835f9>A 'Property' that is determined by each 'Observer' following a well defined 'Observation' procedure through a specific perception channel.</annotations:EMMO_967080e5_2f42_4eb2_a3a9_c58143e835f9>
    <rdfs:label xml:lang="en">ObjectiveProperty</rdfs:label>
    <rdfs:comment>The word objective does not mean that each observation will provide the same results. It means that the observation followed a well defined procedure.</rdfs:comment>
    <rdfs:comment>This class refers to what is commonly known as physical property, i.e. a measurable property of physical system, whether is quantifiable or not.</rdfs:comment>
  </rdf:Description>
  <rdf:Description rdf:about="http://emmo.info/emmo/middle/isq#EMMO_852b4ab8_fc29_4749_a8c7_b92d4fca7d5a">
    <annotations:EMMO_6dd685dd_1895_46e4_b227_be9f7d643c25>http://dbpedia.org/page/Frequency</annotations:EMMO_6dd685dd_1895_46e4_b227_be9f7d643c25>
    <rdfs:subClassOf rdf:resource="http://emmo.info/emmo/middle/isq#EMMO_2946d40b_24a1_47fa_8176_e3f79bb45064"/>
    <annotations:EMMO_967080e5_2f42_4eb2_a3a9_c58143e835f9>Number of periods per time interval.</annotations:EMMO_967080e5_2f42_4eb2_a3a9_c58143e835f9>
    <rdf:type rdf:resource="http://www.w3.org/2002/07/owl#Class"/>
    <annotations:EMMO_fe015383_afb3_44a6_ae86_043628697aa2>https://doi.org/10.1351/goldbook.FT07383</annotations:EMMO_fe015383_afb3_44a6_ae86_043628697aa2>
    <rdfs:label xml:lang="en">Frequency</rdfs:label>
    <rdfs:subClassOf rdf:nodeID="Ne48cfa7d3e4946a9893d44c19ad83f53"/>
  </rdf:Description>
  <rdf:Description rdf:about="http://emmo.info/emmo/middle/metrology#EMMO_67fc0a36_8dcb_4ffa_9a43_31074efa3296">
    <rdf:type rdf:resource="http://www.w3.org/2002/07/owl#ObjectProperty"/>
    <rdfs:comment>Relates the physical quantity to its unit through spatial direct parthood.</rdfs:comment>
    <rdfs:subPropertyOf rdf:resource="http://emmo.info/emmo/middle/reductionistic#EMMO_b2282816_b7a3_44c6_b2cb_3feff1ceb7fe"/>
    <rdf:type rdf:resource="http://www.w3.org/2002/07/owl#AsymmetricProperty"/>
    <rdfs:domain rdf:resource="http://emmo.info/emmo/middle/metrology#EMMO_f658c301_ce93_46cf_9639_4eace2c5d1d5"/>
    <rdf:type rdf:resource="http://www.w3.org/2002/07/owl#IrreflexiveProperty"/>
    <rdfs:range rdf:resource="http://emmo.info/emmo/middle/metrology#EMMO_18ce5200_00f5_45bb_8c6f_6fb128cd41ae"/>
    <rdf:type rdf:resource="http://www.w3.org/2002/07/owl#InverseFunctionalProperty"/>
    <rdfs:label xml:lang="en">hasReferenceUnit</rdfs:label>
  </rdf:Description>
  <rdf:Description rdf:nodeID="Na69d7a721f924256881228614b987701">
    <rdf:type rdf:resource="http://www.w3.org/2002/07/owl#Restriction"/>
    <owl:onProperty rdf:resource="http://emmo.info/emmo/middle/metrology#EMMO_67fc0a36_8dcb_4ffa_9a43_31074efa3296"/>
    <owl:allValuesFrom rdf:nodeID="Necb4889164fd4a378dd468d77fb5ae07"/>
  </rdf:Description>
  <rdf:Description rdf:about="http://emmo.info/emmo/middle/math">
    <rdfs:comment>The EMMO requires FacT++ reasoner plugin in order to visualize all inferences and class hierarchy (ctrl+R hotkey in Protege).</rdfs:comment>
    <rdfs:comment>European Materials and Modelling Ontology (EMMO)

EMMO is a multidisciplinary effort to develop a standard representational framework (the ontology) based on current materials modelling knowledge, including physical sciences, analytical philosophy and information and communication technologies. 

It provides the connection between the physical world, materials characterisation world and materials modelling world.</rdfs:comment>
    <owl:versionIRI rdf:resource="http://emmo.info/emmo/1.0.0-alpha/middle/math"/>
    <owl:versionInfo>The European Materials Modelling Ontology

Version 1.0.0-alpha</owl:versionInfo>
    <annotations:EMMO_5525a055_dda5_4556_8b91_f0d22fa676cc>EMMO is released under a Creative Commons license Attribution 4.0 International (CC BY 4.0)

https://creativecommons.org/licenses/by/4.0/legalcode</annotations:EMMO_5525a055_dda5_4556_8b91_f0d22fa676cc>
    <rdf:type rdf:resource="http://www.w3.org/2002/07/owl#Ontology"/>
    <rdfs:comment xml:lang="en">Contacts:
Gerhard Goldbeck
Goldbeck Consulting Ltd (UK)
email: gerhard@goldbeck-consulting.com

Emanuele Ghedini
University of Bologna (IT)
email: emanuele.ghedini@unibo.it</rdfs:comment>
    <annotations:EMMO_cd5fb112_7ee7_4120_a35d_3ca3e6c3f4ab>Emanuele Ghedini (University of Bologna, IT)
Gerhard Goldbeck (GCL Ltd, UK)
Adham Hashibon (Fraunhofer IWM, DE)
Georg Schmitz (Access, DE)
Jesper Friis (SINTEF, NO)</annotations:EMMO_cd5fb112_7ee7_4120_a35d_3ca3e6c3f4ab>
  </rdf:Description>
  <rdf:Description rdf:nodeID="N3cd66eb437284d19beb5c4e55fa55adb">
    <owl:hasValue>kat</owl:hasValue>
    <owl:onProperty rdf:resource="http://emmo.info/emmo/middle/perceptual#EMMO_23b579e1_8088_45b5_9975_064014026c42"/>
    <rdf:type rdf:resource="http://www.w3.org/2002/07/owl#Restriction"/>
  </rdf:Description>
  <rdf:Description rdf:about="http://emmo.info/emmo/middle/isq#EMMO_e88f75d6_9a17_4cfc_bdf7_43d7cea5a9a1">
    <rdfs:label xml:lang="en">ElectricResistance</rdfs:label>
    <rdfs:subClassOf rdf:resource="http://emmo.info/emmo/middle/isq#EMMO_2946d40b_24a1_47fa_8176_e3f79bb45064"/>
    <annotations:EMMO_21ae69b4_235e_479d_8dd8_4f756f694c1b>Resistance</annotations:EMMO_21ae69b4_235e_479d_8dd8_4f756f694c1b>
    <annotations:EMMO_6dd685dd_1895_46e4_b227_be9f7d643c25>http://dbpedia.org/page/Electrical_resistance_and_conductance</annotations:EMMO_6dd685dd_1895_46e4_b227_be9f7d643c25>
    <rdf:type rdf:resource="http://www.w3.org/2002/07/owl#Class"/>
    <rdfs:subClassOf rdf:nodeID="N823d279887034df9abd7eb10be4b0aaa"/>
    <annotations:EMMO_967080e5_2f42_4eb2_a3a9_c58143e835f9>Measure of the difficulty to pass an electric current through a material.</annotations:EMMO_967080e5_2f42_4eb2_a3a9_c58143e835f9>
    <rdfs:comment>Inverse of 'ElectricalConductance'.</rdfs:comment>
    <annotations:EMMO_fe015383_afb3_44a6_ae86_043628697aa2>https://doi.org/10.1351/goldbook.E01936</annotations:EMMO_fe015383_afb3_44a6_ae86_043628697aa2>
  </rdf:Description>
  <rdf:Description rdf:about="http://emmo.info/emmo/middle/isq#EMMO_a77a0a4b_6bd2_42b2_be27_4b63cebbb59e">
    <rdfs:label xml:lang="en">TemperatureDimension</rdfs:label>
    <owl:equivalentClass rdf:nodeID="N11e7563c445748fbb7061dd5cdd28b49"/>
    <rdfs:subClassOf rdf:resource="http://emmo.info/emmo/middle/metrology#EMMO_9895a1b4_f0a5_4167_ac5e_97db40b8bfcc"/>
    <rdf:type rdf:resource="http://www.w3.org/2002/07/owl#Class"/>
  </rdf:Description>
  <rdf:Description rdf:about="http://emmo.info/emmo/middle/reductionistic#EMMO_15db234d_ecaf_4715_9838_4b4ec424fb13">
    <rdf:type rdf:resource="http://www.w3.org/2002/07/owl#Class"/>
    <rdfs:label xml:lang="en">Reductionistic</rdfs:label>
    <owl:equivalentClass rdf:nodeID="N191a51986e1d4d44b6e68347d5eec5b4"/>
    <rdfs:subClassOf rdf:resource="http://emmo.info/emmo/top#EMMO_49267eba_5548_4163_8f36_518d65b583f9"/>
    <annotations:EMMO_967080e5_2f42_4eb2_a3a9_c58143e835f9>A class devoted to categorize 'Physical'-s according to their granularity relations, first in terms of time evolution (Existent) and then in terms of their composition (State), up to the spatial a-tomistic element (Elementary).

Direct parthood is the relation used to build the class hierarchy (and the granularity hierarchy).</annotations:EMMO_967080e5_2f42_4eb2_a3a9_c58143e835f9>
  </rdf:Description>
  <rdf:Description rdf:nodeID="Neafdd406370c49af8626196feba5f50e">
    <owl:hasValue>μ</owl:hasValue>
    <owl:onProperty rdf:resource="http://emmo.info/emmo/middle/perceptual#EMMO_23b579e1_8088_45b5_9975_064014026c42"/>
    <rdf:type rdf:resource="http://www.w3.org/2002/07/owl#Restriction"/>
  </rdf:Description>
  <rdf:Description rdf:about="http://emmo.info/emmo/top/annotations#EMMO_e55f2d7c_9893_48cd_b4a4_fdf38253bd20">
    <rdfs:label xml:lang="en">omMatch</rdfs:label>
    <rdf:type rdf:resource="http://www.w3.org/2002/07/owl#AnnotationProperty"/>
    <rdfs:seeAlso>https://enterpriseintegrationlab.github.io/icity/OM/doc/index-en.html</rdfs:seeAlso>
    <rdfs:subPropertyOf rdf:resource="http://www.w3.org/2000/01/rdf-schema#seeAlso"/>
    <rdfs:comment>IRI to corresponding concept in the Ontology of units of Measure</rdfs:comment>
    <rdfs:seeAlso>https://github.com/HajoRijgersberg/OM</rdfs:seeAlso>
  </rdf:Description>
  <rdf:Description rdf:about="http://emmo.info/emmo/middle/siunits#EMMO_e2207e91_02b0_4a8a_b13e_61d2a2a839f1">
    <rdf:type rdf:resource="http://www.w3.org/2002/07/owl#Class"/>
    <annotations:EMMO_1f1b164d_ec6a_4faa_8d5e_88bda62316cc>http://qudt.org/vocab/unit/V</annotations:EMMO_1f1b164d_ec6a_4faa_8d5e_88bda62316cc>
    <annotations:EMMO_fe015383_afb3_44a6_ae86_043628697aa2>https://doi.org/10.1351/goldbook.V06634</annotations:EMMO_fe015383_afb3_44a6_ae86_043628697aa2>
    <rdfs:label xml:lang="en">Volt</rdfs:label>
    <rdfs:subClassOf rdf:nodeID="Ncc15c60739e74988852f3e46ac53617a"/>
    <rdfs:subClassOf rdf:nodeID="N1fdc23dabb52434cb1677eb684110682"/>
    <rdfs:comment>Measurement unit for voltage.</rdfs:comment>
  </rdf:Description>
  <rdf:Description rdf:about="http://emmo.info/emmo/middle/perceptual#EMMO_057e7d57_aff0_49de_911a_8861d85cef40">
    <annotations:EMMO_967080e5_2f42_4eb2_a3a9_c58143e835f9>An 'Graphical' that stands for a token or a composition of tokens from one or more alphabets, without necessarily respecting syntactic rules.</annotations:EMMO_967080e5_2f42_4eb2_a3a9_c58143e835f9>
    <rdfs:subClassOf rdf:resource="http://emmo.info/emmo/middle/perceptual#EMMO_c74da218_9147_4f03_92d1_8894abca55f3"/>
    <rdfs:label xml:lang="en">Symbolic</rdfs:label>
    <annotations:EMMO_b432d2d5_25f4_4165_99c5_5935a7763c1a>fe780
emmo
!5*a
cat</annotations:EMMO_b432d2d5_25f4_4165_99c5_5935a7763c1a>
    <rdf:type rdf:resource="http://www.w3.org/2002/07/owl#Class"/>
  </rdf:Description>
  <rdf:Description rdf:about="http://emmo.info/emmo/middle/isq#EMMO_ec903946_ddc9_464a_903c_7373e0d1eeb5">
    <rdfs:label xml:lang="en">MassPerSquareTimeCurrentDimension</rdfs:label>
    <rdf:type rdf:resource="http://www.w3.org/2002/07/owl#Class"/>
    <rdfs:subClassOf rdf:resource="http://emmo.info/emmo/middle/metrology#EMMO_9895a1b4_f0a5_4167_ac5e_97db40b8bfcc"/>
    <owl:equivalentClass rdf:nodeID="Nf649fb5878374c29a1571007e6418b74"/>
  </rdf:Description>
  <rdf:Description rdf:nodeID="N60fc193eaac64e1189724c7a65d086b9">
    <owl:onProperty rdf:nodeID="Nae464b1384694e5bbe2d6cd25525f893"/>
    <rdf:type rdf:resource="http://www.w3.org/2002/07/owl#Restriction"/>
    <owl:allValuesFrom rdf:nodeID="Na8a0e41b89d643fa8412aadd995f0740"/>
  </rdf:Description>
  <rdf:Description rdf:nodeID="N30e49024982b49dfaa9a32e171461c35">
    <owl:onProperty rdf:nodeID="N97373921149d4a57aaca4755c83c2806"/>
    <rdf:type rdf:resource="http://www.w3.org/2002/07/owl#Restriction"/>
    <owl:allValuesFrom rdf:nodeID="Na2403bdde07944c19843ae47be5af1dc"/>
  </rdf:Description>
  <rdf:Description rdf:nodeID="Na9d5cdcb9fe7422bb2c63284f4ce49be">
    <owl:someValuesFrom rdf:resource="http://emmo.info/emmo/middle/isq#EMMO_ab79e92b_5377_454d_be06_d61b50db295a"/>
    <rdf:type rdf:resource="http://www.w3.org/2002/07/owl#Restriction"/>
    <owl:onProperty rdf:resource="http://emmo.info/emmo/middle/metrology#EMMO_bed1d005_b04e_4a90_94cf_02bc678a8569"/>
  </rdf:Description>
  <rdf:Description rdf:nodeID="N28cce3be90ba4ef08ba5863198335968">
    <rdf:first rdf:resource="http://emmo.info/emmo/middle/siunits#EMMO_2e5e45fc_f52c_4294_bdc2_5ed7a06dfce7"/>
    <rdf:rest rdf:nodeID="N816a20186e764fbdb18f9ffb6ce540f4"/>
  </rdf:Description>
  <rdf:Description rdf:about="http://emmo.info/emmo/middle/isq#EMMO_4c49ab58_a6f6_409e_b849_f873ae1dcbee">
    <rdf:type rdf:resource="http://www.w3.org/2002/07/owl#Class"/>
    <owl:equivalentClass rdf:nodeID="N7511f10b5e544b1eaf09d2f6b9c32f88"/>
    <rdfs:label xml:lang="en">MassSquareLengthPerSquareTimeCurrentDimension</rdfs:label>
    <rdfs:subClassOf rdf:resource="http://emmo.info/emmo/middle/metrology#EMMO_9895a1b4_f0a5_4167_ac5e_97db40b8bfcc"/>
  </rdf:Description>
  <rdf:Description rdf:about="http://emmo.info/emmo/middle/siunits#EMMO_3a204900_2b33_47d1_b444_815cc4c8cffa">
    <rdfs:subClassOf rdf:nodeID="N2ad3c4e108dd4540aff45e0082d6cc7a"/>
    <rdf:type rdf:resource="http://www.w3.org/2002/07/owl#Class"/>
    <rdfs:label xml:lang="en">Tera</rdfs:label>
    <rdfs:subClassOf rdf:nodeID="Nc7c090151e8c4a91a8f81dc470851dbc"/>
  </rdf:Description>
  <rdf:Description rdf:about="http://emmo.info/emmo/middle/isq#EMMO_f35cff4d_dc09_44cf_a729_22fb79e3bfb2">
    <rdfs:seeAlso>https://www.iso.org/obp/ui/#iso:std:iso:80000:-1:ed-1:v1:en:sec:3.1</rdfs:seeAlso>
    <rdf:type rdf:resource="http://www.w3.org/2002/07/owl#Class"/>
    <rdfs:label xml:lang="en">InternationalSystemOfQuantity</rdfs:label>
    <annotations:EMMO_c84c6752_6d64_48cc_9500_e54a3c34898d>https://en.wikipedia.org/wiki/International_System_of_Quantities</annotations:EMMO_c84c6752_6d64_48cc_9500_e54a3c34898d>
    <annotations:EMMO_967080e5_2f42_4eb2_a3a9_c58143e835f9>Quantities declared under the ISO 8000.</annotations:EMMO_967080e5_2f42_4eb2_a3a9_c58143e835f9>
    <rdfs:subClassOf rdf:resource="http://emmo.info/emmo/middle/metrology#EMMO_02c0621e_a527_4790_8a0f_2bb51973c819"/>
  </rdf:Description>
  <rdf:Description rdf:about="http://emmo.info/emmo/top/semiotics#EMMO_0cd58641_824c_4851_907f_f4c3be76630c">
    <rdfs:label xml:lang="en">Index</rdfs:label>
    <rdf:type rdf:resource="http://www.w3.org/2002/07/owl#Class"/>
    <annotations:EMMO_b432d2d5_25f4_4165_99c5_5935a7763c1a>Smoke stands for a combustion process (a fire).
My facial expression stands for my emotional status.</annotations:EMMO_b432d2d5_25f4_4165_99c5_5935a7763c1a>
    <annotations:EMMO_967080e5_2f42_4eb2_a3a9_c58143e835f9>A 'Sign' that stands for an 'Object' due to causal continguity.</annotations:EMMO_967080e5_2f42_4eb2_a3a9_c58143e835f9>
  </rdf:Description>
  <rdf:Description rdf:nodeID="N608bc2c6f76d42938e8f9e7ea1feb115">
    <owl:allValuesFrom rdf:resource="http://emmo.info/emmo/middle/isq#EMMO_847f1d9f_205e_46c1_8cb6_a9e479421f88"/>
    <rdf:type rdf:resource="http://www.w3.org/2002/07/owl#Restriction"/>
    <owl:onProperty rdf:resource="http://emmo.info/emmo/middle/metrology#EMMO_bed1d005_b04e_4a90_94cf_02bc678a8569"/>
  </rdf:Description>
  <rdf:Description rdf:about="http://emmo.info/emmo/middle/metrology#EMMO_2cfdcca6_6231_48aa_81b5_388b464bfe80">
    <annotations:EMMO_21ae69b4_235e_479d_8dd8_4f756f694c1b>µ</annotations:EMMO_21ae69b4_235e_479d_8dd8_4f756f694c1b>
    <rdfs:subClassOf rdf:resource="http://emmo.info/emmo/middle/metrology#EMMO_e13b2173_1dec_4b97_9ac1_1dc4b418612a"/>
    <rdfs:label xml:lang="en">MicroUnit</rdfs:label>
    <rdf:type rdf:resource="http://www.w3.org/2002/07/owl#Class"/>
    <owl:equivalentClass rdf:nodeID="N40b45b9be0f04243b9c6eb3b210f521d"/>
  </rdf:Description>
  <rdf:Description rdf:about="http://emmo.info/emmo/top/math#EMMO_a365b3c1_7bde_41d7_a15b_2820762e85f4">
    <owl:equivalentClass rdf:nodeID="Na06d5e54e52c421e83c71776f1807a78"/>
    <rdfs:label xml:lang="en">Division</rdfs:label>
    <rdfs:subClassOf rdf:resource="http://emmo.info/emmo/middle/math#EMMO_707f0cd1_941c_4b57_9f20_d0ba30cd6ff3"/>
    <rdf:type rdf:resource="http://www.w3.org/2002/07/owl#Class"/>
  </rdf:Description>
  <rdf:Description rdf:nodeID="Ne67ff9d6048a4e718a218eb4eec16e30">
    <rdf:first rdf:resource="http://emmo.info/emmo/middle/siunits#EMMO_a3a701ed_6f7d_4a10_9aee_dfa1961fc7b7"/>
    <rdf:rest rdf:nodeID="Nd8311201b43245eba5a20ed055780b30"/>
  </rdf:Description>
  <rdf:Description rdf:about="http://emmo.info/emmo/middle/metrology#EMMO_aa0d5cde_cbdc_4815_b46d_2f76b00a6bde">
    <rdf:type rdf:resource="http://www.w3.org/2002/07/owl#Class"/>
    <rdfs:label>LatinSmallLetterM</rdfs:label>
    <owl:equivalentClass rdf:nodeID="N3bda4aef4b4b4b928a30d6d13ec1d6f9"/>
    <rdfs:subClassOf rdf:resource="http://emmo.info/emmo/middle/metrology#EMMO_e13b2173_1dec_4b97_9ac1_1dc4b418612a"/>
    <annotations:EMMO_21ae69b4_235e_479d_8dd8_4f756f694c1b xml:lang="en">m</annotations:EMMO_21ae69b4_235e_479d_8dd8_4f756f694c1b>
  </rdf:Description>
  <rdf:Description rdf:nodeID="N62ce9418bd634c4f9d45bfcabeb4e5ea">
    <rdf:type rdf:resource="http://www.w3.org/2002/07/owl#Restriction"/>
    <owl:onProperty rdf:resource="http://emmo.info/emmo/top/mereotopology#EMMO_9380ab64_0363_4804_b13f_3a8a94119a76"/>
    <owl:allValuesFrom rdf:resource="http://www.w3.org/2002/07/owl#Nothing"/>
  </rdf:Description>
  <rdf:Description rdf:about="http://emmo.info/emmo/top/mereotopology">
    <rdfs:comment>European Materials and Modelling Ontology (EMMO)

EMMO is a multidisciplinary effort to develop a standard representational framework (the ontology) based on current materials modelling knowledge, including physical sciences, analytical philosophy and information and communication technologies. 

It provides the connection between the physical world, materials characterisation world and materials modelling world.</rdfs:comment>
    <rdf:type rdf:resource="http://www.w3.org/2002/07/owl#Ontology"/>
    <owl:versionIRI rdf:resource="http://emmo.info/emmo/1.0.0-alpha/top/mereotopology"/>
    <owl:versionInfo>The European Materials Modelling Ontology

Version 1.0.0-alpha</owl:versionInfo>
    <rdfs:comment xml:lang="en">Contacts:
Gerhard Goldbeck
Goldbeck Consulting Ltd (UK)
email: gerhard@goldbeck-consulting.com

Emanuele Ghedini
University of Bologna (IT)
email: emanuele.ghedini@unibo.it</rdfs:comment>
    <annotations:EMMO_cd5fb112_7ee7_4120_a35d_3ca3e6c3f4ab>Emanuele Ghedini (University of Bologna, IT)
Gerhard Goldbeck (GCL Ltd, UK)
Adham Hashibon (Fraunhofer IWM, DE)
Georg Schmitz (Access, DE)
Jesper Friis (SINTEF, NO)</annotations:EMMO_cd5fb112_7ee7_4120_a35d_3ca3e6c3f4ab>
    <rdfs:comment>The EMMO requires FacT++ reasoner plugin in order to visualize all inferences and class hierarchy (ctrl+R hotkey in Protege).</rdfs:comment>
    <annotations:EMMO_5525a055_dda5_4556_8b91_f0d22fa676cc>EMMO is released under a Creative Commons license Attribution 4.0 International (CC BY 4.0)

https://creativecommons.org/licenses/by/4.0/legalcode</annotations:EMMO_5525a055_dda5_4556_8b91_f0d22fa676cc>
  </rdf:Description>
  <rdf:Description rdf:about="http://emmo.info/emmo/top/mereotopology#EMMO_802d3e92_8770_4f98_a289_ccaaab7fdddf">
    <owl:equivalentClass rdf:nodeID="N9532ecf9be7545d4a02cd7acf91cb0d1"/>
    <owl:equivalentClass rdf:nodeID="Nc6ef320e722b4359853f90ccbd73a0c6"/>
    <rdfs:comment>Mereotopology is the fundamental logical representation used by the EMMO ontologist to characterize the universe and to provide the definitions to connect real world objects to the EMMO concepts.

Parthood relations do not change dimensionality of the real world object referred by an 'EMMO' individual, i.e. every part of a real world object always retains its 4D dimensionality. 

The smallest part of a real world object (i.e. a part that has no proper parts) is referred in the EMMO by a 'Quantum' individual.

It follows that, for the EMMO, real world objects of dimensionality lower than 4D (e.g. surfaces, lines) do not exist.</rdfs:comment>
    <annotations:EMMO_967080e5_2f42_4eb2_a3a9_c58143e835f9>The class representing the collection of all the individuals declared in this ontology standing for real world objects.</annotations:EMMO_967080e5_2f42_4eb2_a3a9_c58143e835f9>
    <rdf:type rdf:resource="http://www.w3.org/2002/07/owl#Class"/>
    <rdfs:comment>In the EMMO we will refer to the universe as a Minkowski space, restricting the ontology to special relativity only. However, exension to general relativity, will adding more complexity, should not change the overall approach.</rdfs:comment>
    <rdfs:label xml:lang="en">EMMO</rdfs:label>
    <rdfs:comment>For the EMMO ontologist the whole universe is represented as a 4D path-connected topological manifold (i.e. the spacetime).

A real world object is then a 4D topological sub-region of the universe. 

A universe sub-region is isolated and defined as a real world object by the ontologist. Then, through a semiotic process that occurs at meta-ontological level (i.e. outside the ontology). an EMMO ontology entity (e.g. an OWL individual) is assigned to represent that real world object.

The fundamental distinction between real world objects, upon which the EMMO is based, is self-connectedness: a real world object can be self-connected xor not self-connected.</rdfs:comment>
    <owl:disjointUnionOf rdf:nodeID="Nfd0c59444f6f4313abe535d92b42e158"/>
    <rdfs:comment>'EMMO' is the disjoint union of 'Item' and 'Collection' (covering axiom).

The union implies that 'EMMO' individuals can only be 'Item' individuals (standing for self-connected real world objects) or 'Collection' individuals (standing for a collection of disconnected items).

Disjointness means that a 'Collection' individual cannot be an 'Item' individual and viceversa, representing the fact that a real world object cannot be self-connected and non-self connected at the same time.</rdfs:comment>
  </rdf:Description>
  <rdf:Description rdf:about="http://emmo.info/emmo/middle/reductionistic">
    <rdfs:comment>The EMMO requires FacT++ reasoner plugin in order to visualize all inferences and class hierarchy (ctrl+R hotkey in Protege).</rdfs:comment>
    <rdfs:comment>European Materials and Modelling Ontology (EMMO)

EMMO is a multidisciplinary effort to develop a standard representational framework (the ontology) based on current materials modelling knowledge, including physical sciences, analytical philosophy and information and communication technologies. 

It provides the connection between the physical world, materials characterisation world and materials modelling world.</rdfs:comment>
    <owl:versionInfo>The European Materials Modelling Ontology

Version 1.0.0-alpha</owl:versionInfo>
    <annotations:EMMO_5525a055_dda5_4556_8b91_f0d22fa676cc>EMMO is released under a Creative Commons license Attribution 4.0 International (CC BY 4.0)

https://creativecommons.org/licenses/by/4.0/legalcode</annotations:EMMO_5525a055_dda5_4556_8b91_f0d22fa676cc>
    <owl:versionIRI rdf:resource="http://emmo.info/emmo/1.0.0-alpha/middle/reductionistic"/>
    <rdf:type rdf:resource="http://www.w3.org/2002/07/owl#Ontology"/>
    <annotations:EMMO_cd5fb112_7ee7_4120_a35d_3ca3e6c3f4ab>Emanuele Ghedini (University of Bologna, IT)
Gerhard Goldbeck (GCL Ltd, UK)
Adham Hashibon (Fraunhofer IWM, DE)
Georg Schmitz (Access, DE)
Jesper Friis (SINTEF, NO)</annotations:EMMO_cd5fb112_7ee7_4120_a35d_3ca3e6c3f4ab>
    <rdfs:comment xml:lang="en">Contacts:
Gerhard Goldbeck
Goldbeck Consulting Ltd (UK)
email: gerhard@goldbeck-consulting.com

Emanuele Ghedini
University of Bologna (IT)
email: emanuele.ghedini</rdfs:comment>
  </rdf:Description>
  <rdf:Description rdf:about="http://emmo.info/emmo/middle/metrology#EMMO_2125f2d0_5050_49e3_a579_4c74bc9fd02e">
    <owl:equivalentClass rdf:nodeID="Nfb683c950e7048b496ccddac8c23e636"/>
    <rdfs:subClassOf rdf:resource="http://emmo.info/emmo/middle/metrology#EMMO_e13b2173_1dec_4b97_9ac1_1dc4b418612a"/>
    <rdfs:label xml:lang="en">LatinCapitalLetterA</rdfs:label>
    <rdf:type rdf:resource="http://www.w3.org/2002/07/owl#Class"/>
    <annotations:EMMO_21ae69b4_235e_479d_8dd8_4f756f694c1b>A</annotations:EMMO_21ae69b4_235e_479d_8dd8_4f756f694c1b>
  </rdf:Description>
  <rdf:Description rdf:nodeID="N80d934556eca424498dcd344c8e366cc">
    <rdf:first rdf:resource="http://emmo.info/emmo/middle/siunits#EMMO_5cf9f86c_86f5_40c4_846d_60371f670e0a"/>
    <rdf:rest rdf:nodeID="Nc7f9071b41a440389d5862f2c8dce73a"/>
  </rdf:Description>
  <rdf:Description rdf:nodeID="N38aa7521440f4db7acd60bdaa143a0f8">
    <rdf:first rdf:resource="http://emmo.info/emmo/middle/physicalistic#EMMO_70dac51e_bddd_48c2_8a98_7d8395e91fc2"/>
    <rdf:rest rdf:resource="http://www.w3.org/1999/02/22-rdf-syntax-ns#nil"/>
  </rdf:Description>
  <rdf:Description rdf:nodeID="N77b5760126354ee59ad8bf5ea2f4acdf">
    <rdf:type rdf:resource="http://www.w3.org/2002/07/owl#Restriction"/>
    <owl:onProperty rdf:resource="http://emmo.info/emmo/middle/reductionistic#EMMO_b2282816_b7a3_44c6_b2cb_3feff1ceb7fe"/>
    <owl:someValuesFrom rdf:resource="http://emmo.info/emmo/top/math#EMMO_1aed91a3_d00c_48af_8f43_a0c958b2512a"/>
  </rdf:Description>
  <rdf:Description rdf:about="http://emmo.info/emmo/middle/perceptual#EMMO_0ab0485c_9e5b_4257_a679_90a2dfba5c7c">
    <rdfs:subClassOf rdf:resource="http://emmo.info/emmo/middle/perceptual#EMMO_b5957cef_a287_442d_a3ce_fd39f20ba1cd"/>
    <rdf:type rdf:resource="http://www.w3.org/2002/07/owl#Class"/>
    <rdfs:label xml:lang="en">0-manifold</rdfs:label>
  </rdf:Description>
  <rdf:Description rdf:about="http://emmo.info/emmo/middle/isq#EMMO_501f9b3a_c469_48f7_9281_2e6a8d805d7a">
    <rdf:type rdf:resource="http://www.w3.org/2002/07/owl#Class"/>
    <rdfs:label xml:lang="en">MassSquareLengthPerTimeDimension</rdfs:label>
    <owl:equivalentClass rdf:nodeID="Nf5108388b7ed4945a665c80edfb01c42"/>
    <rdfs:subClassOf rdf:resource="http://emmo.info/emmo/middle/metrology#EMMO_9895a1b4_f0a5_4167_ac5e_97db40b8bfcc"/>
  </rdf:Description>
  <rdf:Description rdf:about="http://emmo.info/emmo/middle/models#EMMO_f7ed665b_c2e1_42bc_889b_6b42ed3a36f0">
    <rdf:type rdf:resource="http://www.w3.org/2002/07/owl#Class"/>
    <rdfs:label xml:lang="en">MathematicalModel</rdfs:label>
    <owl:equivalentClass rdf:nodeID="N87295ee688cf4799b7964077c1760d78"/>
    <rdfs:comment>A mathematical model can be defined as a description of a system using mathematical concepts and language to facilitate proper explanation of a system or to study the effects of different components and to make predictions on patterns of behaviour. 

Abramowitz and Stegun, 1968</rdfs:comment>
  </rdf:Description>
  <rdf:Description rdf:about="http://emmo.info/emmo/middle/math#EMMO_3446e167_c576_49d6_846c_215bb8878a55">
    <rdfs:range rdf:resource="http://emmo.info/emmo/middle/math#EMMO_1eed0732_e3f1_4b2c_a9c4_b4e75eeb5895"/>
    <rdfs:subPropertyOf rdf:resource="http://emmo.info/emmo/top/semiotics#EMMO_eb3518bf_f799_4f9e_8c3e_ce59af11453b"/>
    <rdfs:label xml:lang="en">hasVariable</rdfs:label>
    <rdf:type rdf:resource="http://www.w3.org/2002/07/owl#ObjectProperty"/>
    <rdfs:domain rdf:resource="http://emmo.info/emmo/middle/math#EMMO_54ee6b5e_5261_44a8_86eb_5717e7fdb9d0"/>
  </rdf:Description>
  <rdf:Description rdf:about="http://emmo.info/emmo/top/semiotics#EMMO_60577dea_9019_4537_ac41_80b0fb563d41">
    <rdfs:range rdf:resource="http://emmo.info/emmo/top/semiotics#EMMO_b21a56ed_f969_4612_a6ec_cb7766f7f31d"/>
    <rdfs:domain rdf:resource="http://emmo.info/emmo/top/semiotics#EMMO_6f5af708_f825_4feb_a0d1_a8d813d3022b"/>
    <rdfs:label xml:lang="en">hasSign</rdfs:label>
    <rdf:type rdf:resource="http://www.w3.org/2002/07/owl#ObjectProperty"/>
    <rdfs:subPropertyOf rdf:resource="http://emmo.info/emmo/top/semiotics#EMMO_2337e25c_3c60_43fc_a8f9_b11a3f974291"/>
  </rdf:Description>
  <rdf:Description rdf:about="http://emmo.info/emmo/middle/perceptual#EMMO_5f278af9_8593_4e27_a717_ccc9e07a0ddf">
    <rdfs:subClassOf rdf:resource="http://emmo.info/emmo/middle/perceptual#EMMO_46f0f8df_4dc6_418f_8036_10427a3a288e"/>
    <rdfs:label xml:lang="en">EuclideanSpace</rdfs:label>
    <rdf:type rdf:resource="http://www.w3.org/2002/07/owl#Class"/>
  </rdf:Description>
  <rdf:Description rdf:about="http://emmo.info/emmo/middle/holistic#EMMO_c5aae418_1622_4d02_93c5_21159e28e6c1">
    <rdfs:subPropertyOf rdf:resource="http://emmo.info/emmo/top/mereotopology#EMMO_9380ab64_0363_4804_b13f_3a8a94119a76"/>
    <rdf:type rdf:resource="http://www.w3.org/2002/07/owl#ObjectProperty"/>
    <rdfs:label xml:lang="en">hasProperParticipant</rdfs:label>
    <rdfs:subPropertyOf rdf:resource="http://emmo.info/emmo/middle/holistic#EMMO_ae2d1a96_bfa1_409a_a7d2_03d69e8a125a"/>
  </rdf:Description>
  <rdf:Description rdf:about="http://emmo.info/emmo/middle/siunits#EMMO_8246541a_f1f6_4d03_8bd7_fc6b76d17375">
    <rdf:type rdf:resource="http://www.w3.org/2002/07/owl#Class"/>
    <rdfs:label xml:lang="en">SINonCoherentUnit</rdfs:label>
    <owl:disjointUnionOf rdf:nodeID="N08bc12d99bb944688c710a985c2b9da6"/>
  </rdf:Description>
  <rdf:Description rdf:about="http://emmo.info/emmo/top/math#EMMO_f6d0c26a_98b6_4cf8_8632_aa259131faaa">
    <rdf:type rdf:resource="http://www.w3.org/2002/07/owl#Class"/>
    <rdfs:subClassOf rdf:resource="http://emmo.info/emmo/middle/math#EMMO_54ee6b5e_5261_44a8_86eb_5717e7fdb9d0"/>
    <rdfs:subClassOf rdf:resource="http://emmo.info/emmo/middle/perceptual#EMMO_a1083d0a_c1fb_471f_8e20_a98f881ad527"/>
    <rdfs:label xml:lang="en">MathematicalOperator</rdfs:label>
  </rdf:Description>
  <rdf:Description rdf:about="http://emmo.info/emmo/middle/isq#EMMO_2e7e5796_4a80_4d73_bb84_f31138446c0c">
    <rdfs:label xml:lang="en">MassSquareLengthPerCubicTimeCurrentDimension</rdfs:label>
    <rdfs:subClassOf rdf:resource="http://emmo.info/emmo/middle/metrology#EMMO_9895a1b4_f0a5_4167_ac5e_97db40b8bfcc"/>
    <owl:equivalentClass rdf:nodeID="N09e41b84bb734043b608cbda97f6410d"/>
    <rdf:type rdf:resource="http://www.w3.org/2002/07/owl#Class"/>
  </rdf:Description>
  <rdf:Description rdf:nodeID="N2d3c2791a50343bf946e099971f6aab6">
    <rdf:type rdf:resource="http://www.w3.org/2002/07/owl#Restriction"/>
    <owl:onProperty rdf:resource="http://emmo.info/emmo/middle/math#EMMO_faf79f53_749d_40b2_807c_d34244c192f4"/>
    <owl:hasValue rdf:datatype="http://www.w3.org/2001/XMLSchema#decimal">0.000001</owl:hasValue>
  </rdf:Description>
  <rdf:Description rdf:about="http://emmo.info/emmo/middle/metrology#EMMO_c6d4a5e0_7e95_44df_a6db_84ee0a8bbc8e">
    <annotations:EMMO_967080e5_2f42_4eb2_a3a9_c58143e835f9>A measurement unit that is made of a metric prefix and a unit symbol.</annotations:EMMO_967080e5_2f42_4eb2_a3a9_c58143e835f9>
    <rdfs:subClassOf rdf:nodeID="N798b68e95f1343b9babd37017664044e"/>
    <rdfs:subClassOf rdf:nodeID="N04cf64912ef24e438c58c2026c440620"/>
    <rdfs:label xml:lang="en">PrefixedUnit</rdfs:label>
    <rdf:type rdf:resource="http://www.w3.org/2002/07/owl#Class"/>
    <owl:disjointUnionOf rdf:nodeID="Nbf20b38a839a4309999a1d0ba54a96a7"/>
    <rdfs:subClassOf rdf:nodeID="Nfc58ea532d114626852e2b76b3ef8633"/>
  </rdf:Description>
  <rdf:Description rdf:nodeID="N42ded023e7ca40b59a22fc91efc4012c">
    <rdf:type rdf:resource="http://www.w3.org/2002/07/owl#Restriction"/>
    <owl:onProperty rdf:resource="http://emmo.info/emmo/middle/metrology#EMMO_bed1d005_b04e_4a90_94cf_02bc678a8569"/>
    <owl:someValuesFrom rdf:resource="http://emmo.info/emmo/middle/isq#EMMO_f6070071_d054_4b17_9d2d_f446f7147d0f"/>
  </rdf:Description>
  <rdf:Description rdf:nodeID="N7a398ec7b5464a899bf4f6253b11079d">
    <rdf:type rdf:resource="http://www.w3.org/2002/07/owl#Restriction"/>
    <owl:onProperty rdf:resource="http://emmo.info/emmo/middle/metrology#EMMO_bed1d005_b04e_4a90_94cf_02bc678a8569"/>
    <owl:allValuesFrom rdf:resource="http://emmo.info/emmo/middle/isq#EMMO_3227b821_26a5_4c7c_9c01_5c24483e0bd0"/>
  </rdf:Description>
  <rdf:Description rdf:nodeID="Nc6ef320e722b4359853f90ccbd73a0c6">
    <rdf:type rdf:resource="http://www.w3.org/2002/07/owl#Restriction"/>
    <owl:onProperty rdf:resource="http://emmo.info/emmo/top/mereotopology#EMMO_17e27c22_37e1_468c_9dd7_95e137f73e7f"/>
    <owl:someValuesFrom rdf:resource="http://emmo.info/emmo/top/mereotopology#EMMO_3f9ae00e_810c_4518_aec2_7200e424cf68"/>
  </rdf:Description>
  <rdf:Description rdf:about="http://emmo.info/emmo/top/math#EMMO_223d9523_4169_4ecd_b8af_acad1215e1ff">
    <rdfs:subClassOf rdf:resource="http://emmo.info/emmo/top/math#EMMO_3c424d37_cf62_41b1_ac9d_a316f8d113d6"/>
    <rdfs:label xml:lang="en">Exponent</rdfs:label>
    <rdf:type rdf:resource="http://www.w3.org/2002/07/owl#Class"/>
  </rdf:Description>
  <rdf:Description rdf:nodeID="N728c9572118f4bb9a8b615cca11715a5">
    <owl:allValuesFrom rdf:resource="http://emmo.info/emmo/middle/isq#EMMO_a77a0a4b_6bd2_42b2_be27_4b63cebbb59e"/>
    <rdf:type rdf:resource="http://www.w3.org/2002/07/owl#Restriction"/>
    <owl:onProperty rdf:resource="http://emmo.info/emmo/middle/metrology#EMMO_bed1d005_b04e_4a90_94cf_02bc678a8569"/>
  </rdf:Description>
  <rdf:Description rdf:about="http://emmo.info/emmo/middle/siunits#EMMO_a3a701ed_6f7d_4a10_9aee_dfa1961fc7b7">
    <rdfs:label xml:lang="en">Milli</rdfs:label>
    <rdfs:subClassOf rdf:nodeID="Na83574220c524b78a297fca3773ea492"/>
    <rdfs:subClassOf rdf:nodeID="Nae895865b8364d67904d336652857195"/>
    <rdf:type rdf:resource="http://www.w3.org/2002/07/owl#Class"/>
  </rdf:Description>
  <rdf:Description rdf:about="http://emmo.info/emmo/top/mereotopology#EMMO_d893d373_b579_4867_841e_1c2b31a8d2c6">
    <rdf:type rdf:resource="http://www.w3.org/2002/07/owl#ObjectProperty"/>
    <rdfs:subPropertyOf rdf:resource="http://emmo.info/emmo/top/mereotopology#EMMO_6703954e_34c4_4a15_a9e7_f313760ae1a8"/>
    <rdf:type rdf:resource="http://www.w3.org/2002/07/owl#SymmetricProperty"/>
    <rdfs:label xml:lang="en">hasOverlapWith</rdfs:label>
  </rdf:Description>
  <rdf:Description rdf:about="http://emmo.info/emmo/top/semiotics#EMMO_054af807_85cd_4a13_8eba_119dfdaaf38b">
    <annotations:EMMO_967080e5_2f42_4eb2_a3a9_c58143e835f9>The interpreter's internal representation of the object in a semiosis process.</annotations:EMMO_967080e5_2f42_4eb2_a3a9_c58143e835f9>
    <rdfs:subClassOf rdf:resource="http://emmo.info/emmo/top/semiotics#EMMO_b21a56ed_f969_4612_a6ec_cb7766f7f31d"/>
    <rdf:type rdf:resource="http://www.w3.org/2002/07/owl#Class"/>
    <rdfs:label xml:lang="en">Interpretant</rdfs:label>
  </rdf:Description>
  <rdf:Description rdf:about="http://emmo.info/emmo/middle/perceptual#EMMO_46f0f8df_4dc6_418f_8036_10427a3a288e">
    <rdfs:label xml:lang="en">3-manifold</rdfs:label>
    <rdfs:subClassOf rdf:resource="http://emmo.info/emmo/middle/perceptual#EMMO_b5957cef_a287_442d_a3ce_fd39f20ba1cd"/>
    <rdf:type rdf:resource="http://www.w3.org/2002/07/owl#Class"/>
  </rdf:Description>
  <rdf:Description rdf:nodeID="Nf4c03dc086c046259365beef4db711f2">
    <rdf:type rdf:resource="http://www.w3.org/2002/07/owl#Restriction"/>
    <owl:hasValue>M</owl:hasValue>
    <owl:onProperty rdf:resource="http://emmo.info/emmo/middle/perceptual#EMMO_23b579e1_8088_45b5_9975_064014026c42"/>
  </rdf:Description>
  <rdf:Description rdf:about="http://emmo.info/emmo/top/math#EMMO_a6138ba7_e365_4f2d_b6b4_fe5a5918d403">
    <rdf:type rdf:resource="http://www.w3.org/2002/07/owl#Class"/>
    <rdfs:subClassOf rdf:resource="http://emmo.info/emmo/middle/math#EMMO_e56ee3eb_7609_4ae1_8bed_51974f0960a6"/>
    <annotations:EMMO_b432d2d5_25f4_4165_99c5_5935a7763c1a>1 + 1 = 2</annotations:EMMO_b432d2d5_25f4_4165_99c5_5935a7763c1a>
    <rdfs:label xml:lang="en">ArithmeticEquation</rdfs:label>
  </rdf:Description>
  <rdf:Description rdf:about="http://emmo.info/emmo/top/physical#EMMO_f68030be_94b8_4c61_a161_886468558054">
    <annotations:EMMO_967080e5_2f42_4eb2_a3a9_c58143e835f9>A relation that isolates a proper part that extends itself in time within the overall lifetime of the whole, without covering the full spatial extension of the 4D whole (i.e. is not a temporal part).</annotations:EMMO_967080e5_2f42_4eb2_a3a9_c58143e835f9>
    <rdf:type rdf:resource="http://www.w3.org/2002/07/owl#ObjectProperty"/>
    <rdfs:range rdf:resource="http://emmo.info/emmo/top/mereotopology#EMMO_eb3a768e_d53e_4be9_a23b_0714833c36de"/>
    <rdfs:subPropertyOf rdf:resource="http://emmo.info/emmo/top/mereotopology#EMMO_9380ab64_0363_4804_b13f_3a8a94119a76"/>
    <rdfs:domain rdf:resource="http://emmo.info/emmo/top/mereotopology#EMMO_eb3a768e_d53e_4be9_a23b_0714833c36de"/>
    <rdfs:label xml:lang="en">hasSpatialPart</rdfs:label>
    <rdf:type rdf:resource="http://www.w3.org/2002/07/owl#TransitiveProperty"/>
  </rdf:Description>
  <rdf:Description rdf:nodeID="N7a11344ac6a2458da190ae695b24914e">
    <rdf:type rdf:resource="http://www.w3.org/2002/07/owl#Class"/>
    <owl:unionOf rdf:nodeID="Na66ea430afc34330b2e9ba5bfea02009"/>
  </rdf:Description>
  <rdf:Description rdf:about="http://emmo.info/emmo/middle/isq#EMMO_affe07e4_e9bc_4852_86c6_69e26182a17f">
    <annotations:EMMO_6dd685dd_1895_46e4_b227_be9f7d643c25>http://dbpedia.org/page/Thermodynamic_temperature</annotations:EMMO_6dd685dd_1895_46e4_b227_be9f7d643c25>
    <rdfs:label xml:lang="en">ThermodynamicTemperature</rdfs:label>
    <annotations:EMMO_967080e5_2f42_4eb2_a3a9_c58143e835f9>Thermodynamic temperature is the absolute measure of temperature. It is defined by the third law of thermodynamics in which the theoretically lowest temperature is the null or zero point.</annotations:EMMO_967080e5_2f42_4eb2_a3a9_c58143e835f9>
    <rdfs:subClassOf rdf:nodeID="N476be3bb85344473bfd24343c5f124d9"/>
    <annotations:EMMO_fe015383_afb3_44a6_ae86_043628697aa2>https://doi.org/10.1351/goldbook.T06321</annotations:EMMO_fe015383_afb3_44a6_ae86_043628697aa2>
    <rdf:type rdf:resource="http://www.w3.org/2002/07/owl#Class"/>
  </rdf:Description>
  <rdf:Description rdf:nodeID="Nfe093601627448f88809ffd10fa8c4af">
    <rdf:type rdf:resource="http://www.w3.org/2002/07/owl#Restriction"/>
    <owl:onProperty rdf:resource="http://emmo.info/emmo/middle/perceptual#EMMO_23b579e1_8088_45b5_9975_064014026c42"/>
    <owl:hasValue>h</owl:hasValue>
  </rdf:Description>
  <rdf:Description rdf:nodeID="N078928430ee94cc088eba0d56878a03f">
    <rdf:first rdf:resource="http://emmo.info/emmo/middle/physicalistic#EMMO_4207e895_8b83_4318_996a_72cfb32acd94"/>
    <rdf:rest rdf:nodeID="N97fb471f63e74ddcb98e76f698767c45"/>
  </rdf:Description>
  <rdf:Description rdf:about="http://emmo.info/emmo/middle/siunits#EMMO_74931b1b_c133_4e59_9a75_1bf0e1626201">
    <rdfs:label xml:lang="en">Kilo</rdfs:label>
    <rdfs:subClassOf rdf:nodeID="N66e5f21acb0446809e5067e77a111073"/>
    <rdfs:subClassOf rdf:nodeID="N95a3b006afc24e0bb28e46eab6d98f56"/>
    <rdf:type rdf:resource="http://www.w3.org/2002/07/owl#Class"/>
  </rdf:Description>
  <rdf:Description rdf:about="http://emmo.info/emmo/middle/math#EMMO_fe7e56ce_118b_4243_9aad_20eb9f4f31f6">
    <annotations:EMMO_b432d2d5_25f4_4165_99c5_5935a7763c1a>Velocity, for the Navier-Stokes equation.</annotations:EMMO_b432d2d5_25f4_4165_99c5_5935a7763c1a>
    <rdf:type rdf:resource="http://www.w3.org/2002/07/owl#Class"/>
    <rdfs:label xml:lang="en">Unknown</rdfs:label>
    <annotations:EMMO_967080e5_2f42_4eb2_a3a9_c58143e835f9>The dependent variable for which an equation has been written.</annotations:EMMO_967080e5_2f42_4eb2_a3a9_c58143e835f9>
    <rdfs:subClassOf rdf:resource="http://emmo.info/emmo/middle/math#EMMO_1eed0732_e3f1_4b2c_a9c4_b4e75eeb5895"/>
  </rdf:Description>
  <rdf:Description rdf:about="http://emmo.info/emmo/middle/metrology#EMMO_bed1d005_b04e_4a90_94cf_02bc678a8569">
    <rdfs:range rdf:resource="http://emmo.info/emmo/middle/metrology#EMMO_9895a1b4_f0a5_4167_ac5e_97db40b8bfcc"/>
    <rdf:type rdf:resource="http://www.w3.org/2002/07/owl#ObjectProperty"/>
    <rdfs:subPropertyOf rdf:resource="http://emmo.info/emmo/middle/properties#EMMO_e1097637_70d2_4895_973f_2396f04fa204"/>
    <rdfs:label xml:lang="en">hasPhysicsDimension</rdfs:label>
  </rdf:Description>
  <rdf:Description rdf:nodeID="N087e2051134e44e1b5f5024ec3fcac14">
    <rdf:type rdf:resource="http://www.w3.org/2002/07/owl#Restriction"/>
    <owl:someValuesFrom rdf:resource="http://emmo.info/emmo/top/physical#EMMO_c5ddfdba_c074_4aa4_ad6b_1ac4942d300d"/>
    <owl:onProperty rdf:resource="http://emmo.info/emmo/middle/reductionistic#EMMO_b2282816_b7a3_44c6_b2cb_3feff1ceb7fe"/>
  </rdf:Description>
  <rdf:Description rdf:nodeID="N191a51986e1d4d44b6e68347d5eec5b4">
    <owl:unionOf rdf:nodeID="N1829aef8f5264533982cdbafdb05ab3b"/>
    <rdf:type rdf:resource="http://www.w3.org/2002/07/owl#Class"/>
  </rdf:Description>
  <rdf:Description rdf:nodeID="N2d731ca68f11455abd050ffb201de6da">
    <owl:allValuesFrom rdf:nodeID="N23bbf465cdd945678455d3c4ec3c7be7"/>
    <rdf:type rdf:resource="http://www.w3.org/2002/07/owl#Restriction"/>
    <owl:onProperty rdf:nodeID="N7221608130864788b2a3141e99859246"/>
  </rdf:Description>
  <rdf:Description rdf:about="http://emmo.info/emmo/middle/isq#EMMO_321af35f_f0cc_4a5c_b4fe_8c2c0303fb0c">
    <owl:equivalentClass rdf:nodeID="Nadafa3b0ae8c49d088c75c0e66b50b33"/>
    <rdf:type rdf:resource="http://www.w3.org/2002/07/owl#Class"/>
    <rdfs:subClassOf rdf:resource="http://emmo.info/emmo/middle/metrology#EMMO_9895a1b4_f0a5_4167_ac5e_97db40b8bfcc"/>
    <rdfs:label xml:lang="en">CubicTimeSquareCurrentPerMassSquareLengthDimension</rdfs:label>
  </rdf:Description>
  <rdf:Description rdf:nodeID="Nc314b20232ae4c63b3e2a0aae1dfa449">
    <owl:allValuesFrom rdf:nodeID="Nc20a8b7359104095abf5c2bc9718749e"/>
    <rdf:type rdf:resource="http://www.w3.org/2002/07/owl#Restriction"/>
    <owl:onProperty rdf:resource="http://emmo.info/emmo/middle/metrology#EMMO_67fc0a36_8dcb_4ffa_9a43_31074efa3296"/>
  </rdf:Description>
  <rdf:Description rdf:nodeID="N57bbdcdbc32647b9842700bafab924a8">
    <rdf:rest rdf:nodeID="N6fab005c88674a119142e007445b2aa0"/>
    <rdf:first rdf:resource="http://emmo.info/emmo/middle/isq#EMMO_c995ae70_3b84_4ebb_bcfc_69e6a281bb88"/>
  </rdf:Description>
  <rdf:Description rdf:about="http://emmo.info/emmo/middle/siunits#EMMO_daa9ee97_4c5f_42e5_918c_44d7523e8958">
    <rdfs:subClassOf rdf:nodeID="N5bc2348bc9464ea28c46a48f90cb78cc"/>
    <rdfs:subClassOf rdf:nodeID="Neb97b6addf694d73a2640106f9812009"/>
    <rdfs:label xml:lang="en">Zetta</rdfs:label>
    <rdf:type rdf:resource="http://www.w3.org/2002/07/owl#Class"/>
  </rdf:Description>
  <rdf:Description rdf:nodeID="Nb9e679207767435fa2fcace810e4fe29">
    <owl:someValuesFrom rdf:resource="http://emmo.info/emmo/middle/holistic#EMMO_43e9a05d_98af_41b4_92f6_00f79a09bfce"/>
    <owl:onProperty rdf:nodeID="N4cd01a69921346739cbbb0a8e731677b"/>
    <rdf:type rdf:resource="http://www.w3.org/2002/07/owl#Restriction"/>
  </rdf:Description>
  <rdf:Description rdf:about="http://emmo.info/emmo/top/math#EMMO_28fbea28_2204_4613_87ff_6d877b855fcd">
    <rdfs:subClassOf rdf:resource="http://emmo.info/emmo/middle/math#EMMO_54ee6b5e_5261_44a8_86eb_5717e7fdb9d0"/>
    <rdfs:label xml:lang="en">Array</rdfs:label>
    <rdf:type rdf:resource="http://www.w3.org/2002/07/owl#Class"/>
  </rdf:Description>
  <rdf:Description rdf:about="http://emmo.info/emmo/middle/models#EMMO_9c32fd69_f480_4130_83b3_fb25d9face14">
    <rdfs:subClassOf rdf:resource="http://emmo.info/emmo/middle/models#EMMO_db9a009e_f097_43f5_9520_6cbc07e7610b"/>
    <rdfs:label xml:lang="en">PhysicalLaw</rdfs:label>
    <rdf:type rdf:resource="http://www.w3.org/2002/07/owl#Class"/>
  </rdf:Description>
  <rdf:Description rdf:nodeID="N5374912c996f41b5987bf12d041197af">
    <rdf:type rdf:resource="http://www.w3.org/2002/07/owl#Restriction"/>
    <owl:someValuesFrom rdf:resource="http://emmo.info/emmo/middle/metrology#EMMO_08b308d4_31cd_4779_a784_aa92fc730f39"/>
    <owl:onProperty rdf:nodeID="N5c07a232f71c488d8ff7d3f95e9888bd"/>
  </rdf:Description>
  <rdf:Description rdf:nodeID="N45e6caad3f22412782ccadaba0a54db5">
    <owl:hasValue>T-2 L+2 M+1 I-2 Θ0 N0 J0</owl:hasValue>
    <rdf:type rdf:resource="http://www.w3.org/2002/07/owl#Restriction"/>
    <owl:onProperty rdf:resource="http://emmo.info/emmo/middle/perceptual#EMMO_23b579e1_8088_45b5_9975_064014026c42"/>
  </rdf:Description>
  <rdf:Description rdf:nodeID="N26457dd595294348b1997a0256484255">
    <owl:onProperty rdf:resource="http://emmo.info/emmo/middle/metrology#EMMO_bed1d005_b04e_4a90_94cf_02bc678a8569"/>
    <owl:someValuesFrom rdf:resource="http://emmo.info/emmo/middle/isq#EMMO_ec903946_ddc9_464a_903c_7373e0d1eeb5"/>
    <rdf:type rdf:resource="http://www.w3.org/2002/07/owl#Restriction"/>
  </rdf:Description>
  <rdf:Description rdf:nodeID="Nc56415c15ad4485a855b6512b6c96e65">
    <rdf:first rdf:resource="http://emmo.info/emmo/middle/perceptual#EMMO_a1083d0a_c1fb_471f_8e20_a98f881ad527"/>
    <rdf:rest rdf:resource="http://www.w3.org/1999/02/22-rdf-syntax-ns#nil"/>
  </rdf:Description>
  <rdf:Description rdf:about="http://emmo.info/emmo/middle/semiotics">
    <owl:versionInfo>The European Materials Modelling Ontology

Version 1.0.0-alpha</owl:versionInfo>
    <rdf:type rdf:resource="http://www.w3.org/2002/07/owl#Ontology"/>
    <rdfs:comment>European Materials and Modelling Ontology (EMMO)

EMMO is a multidisciplinary effort to develop a standard representational framework (the ontology) based on current materials modelling knowledge, including physical sciences, analytical philosophy and information and communication technologies. 

It provides the connection between the physical world, materials characterisation world and materials modelling world.</rdfs:comment>
    <annotations:EMMO_5525a055_dda5_4556_8b91_f0d22fa676cc>EMMO is released under a Creative Commons license Attribution 4.0 International (CC BY 4.0)

https://creativecommons.org/licenses/by/4.0/legalcode</annotations:EMMO_5525a055_dda5_4556_8b91_f0d22fa676cc>
    <rdfs:comment>The EMMO requires FacT++ reasoner plugin in order to visualize all inferences and class hierarchy (ctrl+R hotkey in Protege).</rdfs:comment>
    <owl:versionIRI rdf:resource="http://emmo.info/emmo/1.0.0-alpha/middle/semiotics"/>
    <rdfs:comment xml:lang="en">Contacts:
Gerhard Goldbeck
Goldbeck Consulting Ltd (UK)
email: gerhard@goldbeck-consulting.com

Emanuele Ghedini
University of Bologna (IT)
email: emanuele.ghedini</rdfs:comment>
    <annotations:EMMO_cd5fb112_7ee7_4120_a35d_3ca3e6c3f4ab>Emanuele Ghedini (University of Bologna, IT)
Gerhard Goldbeck (GCL Ltd, UK)
Adham Hashibon (Fraunhofer IWM, DE)
Georg Schmitz (Access, DE)
Jesper Friis (SINTEF, NO)</annotations:EMMO_cd5fb112_7ee7_4120_a35d_3ca3e6c3f4ab>
  </rdf:Description>
  <rdf:Description rdf:about="http://emmo.info/emmo/top/mereotopology#EMMO_ec2472ae_cf4a_46a5_8555_1556f5a6c3c5">
    <rdfs:domain rdf:resource="http://emmo.info/emmo/top/mereotopology#EMMO_802d3e92_8770_4f98_a289_ccaaab7fdddf"/>
    <annotations:EMMO_967080e5_2f42_4eb2_a3a9_c58143e835f9>The superclass of all relations used by the EMMO.</annotations:EMMO_967080e5_2f42_4eb2_a3a9_c58143e835f9>
    <rdfs:range rdf:resource="http://emmo.info/emmo/top/mereotopology#EMMO_802d3e92_8770_4f98_a289_ccaaab7fdddf"/>
    <rdf:type rdf:resource="http://www.w3.org/2002/07/owl#TransitiveProperty"/>
    <rdf:type rdf:resource="http://www.w3.org/2002/07/owl#ObjectProperty"/>
    <rdf:type rdf:resource="http://www.w3.org/2002/07/owl#SymmetricProperty"/>
    <rdfs:label xml:lang="en">EMMORelation</rdfs:label>
    <rdfs:subPropertyOf rdf:resource="http://www.w3.org/2002/07/owl#topObjectProperty"/>
  </rdf:Description>
  <rdf:Description rdf:nodeID="Na66ea430afc34330b2e9ba5bfea02009">
    <rdf:rest rdf:nodeID="N292a284bf7c54545bf257eff64fe4309"/>
    <rdf:first rdf:resource="http://emmo.info/emmo/middle/metrology#EMMO_216f448e_cdbc_4aeb_a529_7a5fe7fc38bb"/>
  </rdf:Description>
  <rdf:Description rdf:about="http://emmo.info/emmo/middle/math#EMMO_5be83f9c_a4ba_4b9a_be1a_5bfc6e891231">
    <rdf:type rdf:resource="http://www.w3.org/2002/07/owl#Class"/>
    <rdfs:label xml:lang="en">MathematicalSymbol</rdfs:label>
    <rdfs:subClassOf rdf:nodeID="N732e98b8ec654ec9a809d873634b18a8"/>
    <owl:equivalentClass rdf:nodeID="N4095aedf52d04df2bc91e56df0df5082"/>
  </rdf:Description>
  <rdf:Description rdf:about="http://emmo.info/emmo/middle/metrology#EMMO_02c0621e_a527_4790_8a0f_2bb51973c819">
    <rdfs:comment>Measured or simulated 'physical propertiy'-s are always defined by a physical law, connected to a physical entity through a model perspective and measurement is done according to the same model.

Systems of units suggests that this is the correct approach, since except for the fundamental units (length, time, charge) every other unit is derived by mathematical relations between these fundamental units, implying a physical laws or definitions.</rdfs:comment>
    <rdfs:subClassOf rdf:resource="http://emmo.info/emmo/middle/math#EMMO_54ee6b5e_5261_44a8_86eb_5717e7fdb9d0"/>
    <annotations:EMMO_967080e5_2f42_4eb2_a3a9_c58143e835f9>A 'Mathematical' entity that is made of a 'Number' and a 'MeasurementUnit' defined by a physical law, connected to a physical entity through a model perspective. Measurement is done according to the same model.</annotations:EMMO_967080e5_2f42_4eb2_a3a9_c58143e835f9>
    <rdfs:subClassOf rdf:nodeID="Nea85a9d9d59940cc9cd9a54b6a2754dc"/>
    <rdfs:comment>Measurement units of quantities of the same quantity dimension may be designated by the same name and symbol even when the quantities are not of the same kind. 

For example, joule per kelvin and J/K are respectively the name and symbol of both a measurement unit of heat capacity and a measurement unit of entropy, which are generally not considered to be quantities of the same kind. 

However, in some cases special measurement unit names are restricted to be used with quantities of specific kind only. 

For example, the measurement unit ‘second to the power minus one’ (1/s) is called hertz (Hz) when used for frequencies and becquerel (Bq) when used for activities of radionuclides. 

As another example, the joule (J) is used as a unit of energy, but never as a unit of moment of force, i.e. the newton metre (N · m).</rdfs:comment>
    <rdfs:comment>In the same system of quantities, dim ρB = ML−3 is the quantity dimension of mass concentration of component B, and ML−3 is also the quantity dimension of mass density, ρ.
ISO 80000-1</rdfs:comment>
    <rdfs:label xml:lang="en">PhysicalQuantity</rdfs:label>
    <rdf:type rdf:resource="http://www.w3.org/2002/07/owl#Class"/>
    <rdfs:comment>— quantities of the same kind have the same quantity dimension,
— quantities of different quantity dimensions are always of different kinds, and
— quantities having the same quantity dimension are not necessarily of the same kind.
ISO 80000-1</rdfs:comment>
    <owl:disjointUnionOf rdf:nodeID="Nb2a04350627c45a5b4db29eefc58c99d"/>
  </rdf:Description>
  <rdf:Description rdf:nodeID="Nc24f28bad15f41b08cccaded51b5e0dd">
    <owl:onProperty rdf:resource="http://emmo.info/emmo/middle/perceptual#EMMO_23b579e1_8088_45b5_9975_064014026c42"/>
    <rdf:type rdf:resource="http://www.w3.org/2002/07/owl#Restriction"/>
    <owl:hasValue>c</owl:hasValue>
  </rdf:Description>
  <rdf:Description rdf:nodeID="N66c77dcd17294cb88add6125e9bcb0c0">
    <owl:qualifiedCardinality rdf:datatype="http://www.w3.org/2001/XMLSchema#nonNegativeInteger">1</owl:qualifiedCardinality>
  </rdf:Description>
  <rdf:Description rdf:about="http://emmo.info/emmo/middle/materials#EMMO_7d66bde4_b68d_41cc_b5fc_6fd98c5e2ff0">
    <rdfs:subClassOf rdf:resource="http://emmo.info/emmo/middle/physicalistic#EMMO_4207e895_8b83_4318_996a_72cfb32acd94"/>
    <rdf:type rdf:resource="http://www.w3.org/2002/07/owl#Class"/>
    <rdfs:subClassOf rdf:resource="http://emmo.info/emmo/middle/reductionistic#EMMO_36c79456_e29c_400d_8bd3_0eedddb82652"/>
    <rdfs:label xml:lang="en">Subatomic</rdfs:label>
  </rdf:Description>
  <rdf:Description rdf:about="http://emmo.info/emmo/middle/siunits#EMMO_fab003c8_f7a6_4346_9988_7161325ed7a3">
    <rdf:type rdf:resource="http://www.w3.org/2002/07/owl#Class"/>
    <annotations:EMMO_1f1b164d_ec6a_4faa_8d5e_88bda62316cc>http://qudt.org/vocab/unit/H</annotations:EMMO_1f1b164d_ec6a_4faa_8d5e_88bda62316cc>
    <rdfs:comment>Measurement unit for electrical inductance.</rdfs:comment>
    <rdfs:subClassOf rdf:nodeID="Nea0cee0abc004367b4ea3f8974e035d3"/>
    <annotations:EMMO_fe015383_afb3_44a6_ae86_043628697aa2>https://doi.org/10.1351/goldbook.H02782</annotations:EMMO_fe015383_afb3_44a6_ae86_043628697aa2>
    <rdfs:label xml:lang="en">Henry</rdfs:label>
    <rdfs:subClassOf rdf:nodeID="N0941101840144fa880ae50651e03577a"/>
  </rdf:Description>
  <rdf:Description rdf:about="http://emmo.info/emmo/top/semiotics#EMMO_b803f122_4acb_4064_9d71_c1e5fd091fc9">
    <owl:equivalentClass rdf:nodeID="N8ef01c4e371b44518bad4d177fc0f8ce"/>
    <rdf:type rdf:resource="http://www.w3.org/2002/07/owl#Class"/>
    <rdfs:comment>Semiotic subclasse are defined using Peirce's semiotic theory.

"Namely, a sign is something, A, which brings something, B, its interpretant sign determined or created by it, into the same sort of correspondence with something, C, its object, as that in which itself stands to C." (Peirce 1902, NEM 4, 20–21).

The triadic elements:
- 'sign': the sign A (e.g. a name)
- 'interpretant': the sign B as the effects of the sign A on the interpreter (e.g. the mental concept of what a name means)
- 'object': the object C (e.g. the entity to which the sign A and B refer to)

This class includes also the 'interpeter' i.e. the entity that connects the 'sign' to the 'object'</rdfs:comment>
    <rdfs:label xml:lang="en">Semiotic</rdfs:label>
    <annotations:EMMO_967080e5_2f42_4eb2_a3a9_c58143e835f9>The class of individuals that stands for semiotic objects, i.e. objects that take part on a semiotic process.</annotations:EMMO_967080e5_2f42_4eb2_a3a9_c58143e835f9>
    <rdfs:subClassOf rdf:nodeID="N7399485b66c64646930294c7d1f94051"/>
    <rdfs:subClassOf rdf:resource="http://emmo.info/emmo/middle/holistic#EMMO_49804605_c0fe_4538_abda_f70ba1dc8a5d"/>
  </rdf:Description>
  <rdf:Description rdf:nodeID="Nba998a8f95b541a8a37886a2edf3b80c">
    <owl:inverseOf rdf:resource="http://emmo.info/emmo/middle/math#EMMO_3446e167_c576_49d6_846c_215bb8878a55"/>
  </rdf:Description>
  <rdf:Description rdf:about="http://emmo.info/emmo/middle/reductionistic#EMMO_52211e5e_d767_4812_845e_eb6b402c476a">
    <annotations:EMMO_967080e5_2f42_4eb2_a3a9_c58143e835f9>A 'Physical' which is a tessellation of 'State' temporal direct parts.</annotations:EMMO_967080e5_2f42_4eb2_a3a9_c58143e835f9>
    <rdf:type rdf:resource="http://www.w3.org/2002/07/owl#Class"/>
    <rdfs:comment>Being hasTemporalDirectPart a proper parthood relation, there cannot be 'Existent' made of a single 'State'.

Moreover, due to inverse functionality, a 'State' can be part of only one 'Existent', preventing overlapping between 'Existent'-s.</rdfs:comment>
    <rdfs:subClassOf rdf:nodeID="N6577c2fabff74f6eb026a67a4ed52307"/>
    <rdfs:comment>ex-sistere (latin): to stay (to persist through time) outside others of the same type (to be distinct from the rest).</rdfs:comment>
    <rdfs:subClassOf rdf:nodeID="N4675b24c538d4b1abf6283543c82fe33"/>
    <rdfs:comment>'Existent' is the EMMO class to be used for representing real world physical objects under a reductionistic perspective (i.e. objects come from the composition of sub-part objects, both in time and space). 

'Existent' class collects all individuals that stand for physical objects that can be structured in well defined temporal sub-parts called states, through the temporal direct parthood relation.

This class provides a first granularity hierarchy in time, and a way to axiomatize tessellation principles for a specific whole with a non-transitivity relation (direct parthood) that helps to retain the granularity levels.

e.g. a car, a supersaturated gas with nucleating nanoparticles, an atom that becomes ionized and then recombines with an electron.</rdfs:comment>
    <rdfs:label xml:lang="en">Existent</rdfs:label>
    <rdfs:comment>An 'Existent' individual stands for a real world object for which the ontologist can provide univocal tessellation in time.

By definition, the tiles are represented by 'State'-s individual.

Tiles are related to the 'Existent' through temporal direct parthood, enforcing non-transitivity and inverse-functionality.</rdfs:comment>
  </rdf:Description>
  <rdf:Description rdf:nodeID="Nbf20b38a839a4309999a1d0ba54a96a7">
    <rdf:first rdf:resource="http://emmo.info/emmo/middle/metrology#EMMO_62f0d847_3603_45b4_bfc4_dd4511355ff2"/>
    <rdf:rest rdf:nodeID="N8eff5c0c328c413492051a91bd02c33f"/>
  </rdf:Description>
  <rdf:Description rdf:about="http://emmo.info/emmo/middle/isq#EMMO_53e825d9_1a09_483c_baa7_37501ebfbe1c">
    <rdfs:label xml:lang="en">MassLengthPerSquareTimeDimension</rdfs:label>
    <rdf:type rdf:resource="http://www.w3.org/2002/07/owl#Class"/>
    <rdfs:subClassOf rdf:resource="http://emmo.info/emmo/middle/metrology#EMMO_9895a1b4_f0a5_4167_ac5e_97db40b8bfcc"/>
    <owl:equivalentClass rdf:nodeID="Na1f65ae8236c4cc7b8892b086a1f9b8d"/>
  </rdf:Description>
  <rdf:Description rdf:nodeID="N33e37838ff8e4cc49eb6e84faced6fa6">
    <rdf:type rdf:resource="http://www.w3.org/2002/07/owl#Restriction"/>
    <owl:onProperty rdf:resource="http://emmo.info/emmo/middle/metrology#EMMO_bed1d005_b04e_4a90_94cf_02bc678a8569"/>
    <owl:someValuesFrom rdf:resource="http://emmo.info/emmo/middle/isq#EMMO_847f1d9f_205e_46c1_8cb6_a9e479421f88"/>
  </rdf:Description>
  <rdf:Description rdf:nodeID="N5da36b9be6944d57b404c89ebc8659dc">
    <owl:inverseOf rdf:resource="http://emmo.info/emmo/middle/math#EMMO_3446e167_c576_49d6_846c_215bb8878a55"/>
  </rdf:Description>
  <rdf:Description rdf:nodeID="N8724dd72540b40809c96aed21d5b0d0b">
    <owl:inverseOf rdf:resource="http://emmo.info/emmo/middle/math#EMMO_3446e167_c576_49d6_846c_215bb8878a55"/>
  </rdf:Description>
  <rdf:Description rdf:about="http://emmo.info/emmo/middle/properties#EMMO_f2d5d3ad_2e00_417f_8849_686f3988d929">
    <rdfs:subClassOf rdf:resource="http://emmo.info/emmo/middle/properties#EMMO_1b52ee70_121e_4d8d_8419_3f97cd0bd89c"/>
    <rdfs:label xml:lang="en">MeasurementInstrument</rdfs:label>
    <rdf:type rdf:resource="http://www.w3.org/2002/07/owl#Class"/>
  </rdf:Description>
  <rdf:Description rdf:about="http://emmo.info/emmo/middle/isq#EMMO_14ff4393_0f28_4fb4_abc7_c2cc00bc761d">
    <rdfs:subClassOf rdf:resource="http://emmo.info/emmo/middle/metrology#EMMO_9895a1b4_f0a5_4167_ac5e_97db40b8bfcc"/>
    <rdf:type rdf:resource="http://www.w3.org/2002/07/owl#Class"/>
    <owl:equivalentClass rdf:nodeID="Na2106a037cac4ed88e8f47a9baae1f67"/>
    <rdfs:label xml:lang="en">LuminousIntensityDimension</rdfs:label>
  </rdf:Description>
  <rdf:Description rdf:about="http://emmo.info/emmo/middle/metrology#EMMO_acaaa124_3dde_48b6_86e6_6ec6f364f408">
    <rdf:type rdf:resource="http://www.w3.org/2002/07/owl#Class"/>
    <rdfs:subClassOf rdf:nodeID="Na4472cce6d34452f990e1021af18212a"/>
    <rdfs:label xml:lang="en">BaseQuantity</rdfs:label>
    <annotations:EMMO_967080e5_2f42_4eb2_a3a9_c58143e835f9>"Quantity in a conventionally chosen subset of a given system of quantities, where no quantity in the subset can be expressed in terms of the other quantities within that subset"
ISO 80000-1</annotations:EMMO_967080e5_2f42_4eb2_a3a9_c58143e835f9>
  </rdf:Description>
  <rdf:Description rdf:about="http://emmo.info/emmo/middle/isq#EMMO_ed4af7ae_63a2_497e_bb88_2309619ea405">
    <rdfs:subClassOf rdf:nodeID="Nbed0fb15110e42b0abd1b2cd96d2b3e6"/>
    <rdfs:subClassOf rdf:nodeID="Nf5744475d19e4ce89c64ead1e8fff672"/>
    <annotations:EMMO_fe015383_afb3_44a6_ae86_043628697aa2>https://doi.org/10.1351/goldbook.M03709</annotations:EMMO_fe015383_afb3_44a6_ae86_043628697aa2>
    <rdf:type rdf:resource="http://www.w3.org/2002/07/owl#Class"/>
    <annotations:EMMO_967080e5_2f42_4eb2_a3a9_c58143e835f9>Property of a physical body that express its resistance to acceleration (a change in its state of motion) when a force is applied.</annotations:EMMO_967080e5_2f42_4eb2_a3a9_c58143e835f9>
    <annotations:EMMO_6dd685dd_1895_46e4_b227_be9f7d643c25>http://dbpedia.org/page/Mass</annotations:EMMO_6dd685dd_1895_46e4_b227_be9f7d643c25>
    <rdfs:label xml:lang="en">Mass</rdfs:label>
  </rdf:Description>
  <rdf:Description rdf:nodeID="N7c11a63c339c490dad923110a2b30f19">
    <owl:someValuesFrom rdf:resource="http://emmo.info/emmo/middle/isq#EMMO_53bd0c90_41c3_46e2_8779_cd2a80f7e18b"/>
    <owl:onProperty rdf:resource="http://emmo.info/emmo/middle/metrology#EMMO_bed1d005_b04e_4a90_94cf_02bc678a8569"/>
    <rdf:type rdf:resource="http://www.w3.org/2002/07/owl#Restriction"/>
  </rdf:Description>
  <rdf:Description rdf:nodeID="Nf051248ee1744d0c847c033e48c1a529">
    <rdf:rest rdf:resource="http://www.w3.org/1999/02/22-rdf-syntax-ns#nil"/>
    <rdf:first rdf:resource="http://emmo.info/emmo/middle/metrology#EMMO_db716151_6b73_45ff_910c_d182fdcbb4f5"/>
  </rdf:Description>
  <rdf:Description rdf:nodeID="Nc062f361c16b44f1b3f1aa612c2c0285">
    <rdf:type rdf:resource="http://www.w3.org/2002/07/owl#Restriction"/>
    <owl:onProperty rdf:resource="http://emmo.info/emmo/middle/math#EMMO_faf79f53_749d_40b2_807c_d34244c192f4"/>
    <owl:someValuesFrom rdf:resource="http://www.w3.org/2001/XMLSchema#double"/>
  </rdf:Description>
  <rdf:Description rdf:nodeID="Nad2a8e1108724484bb51d872df9e0a85">
    <owl:onProperty rdf:resource="http://emmo.info/emmo/middle/metrology#EMMO_bed1d005_b04e_4a90_94cf_02bc678a8569"/>
    <owl:someValuesFrom rdf:resource="http://emmo.info/emmo/middle/isq#EMMO_3227b821_26a5_4c7c_9c01_5c24483e0bd0"/>
    <rdf:type rdf:resource="http://www.w3.org/2002/07/owl#Restriction"/>
  </rdf:Description>
  <rdf:Description rdf:about="http://emmo.info/emmo/top/physical">
    <rdf:type rdf:resource="http://www.w3.org/2002/07/owl#Ontology"/>
    <rdfs:comment>European Materials and Modelling Ontology (EMMO)

EMMO is a multidisciplinary effort to develop a standard representational framework (the ontology) based on current materials modelling knowledge, including physical sciences, analytical philosophy and information and communication technologies. 

It provides the connection between the physical world, materials characterisation world and materials modelling world.</rdfs:comment>
    <owl:versionInfo>The European Materials Modelling Ontology

Version 1.0.0-alpha</owl:versionInfo>
    <annotations:EMMO_cd5fb112_7ee7_4120_a35d_3ca3e6c3f4ab>Emanuele Ghedini (University of Bologna, IT)
Gerhard Goldbeck (GCL Ltd, UK)
Adham Hashibon (Fraunhofer IWM, DE)
Georg Schmitz (Access, DE)
Jesper Friis (SINTEF, NO)</annotations:EMMO_cd5fb112_7ee7_4120_a35d_3ca3e6c3f4ab>
    <rdfs:comment>The EMMO requires FacT++ reasoner plugin in order to visualize all inferences and class hierarchy (ctrl+R hotkey in Protege).</rdfs:comment>
    <rdfs:comment xml:lang="en">Contacts:
Gerhard Goldbeck
Goldbeck Consulting Ltd (UK)
email: gerhard@goldbeck-consulting.com

Emanuele Ghedini
University of Bologna (IT)
email: emanuele.ghedini</rdfs:comment>
    <annotations:EMMO_5525a055_dda5_4556_8b91_f0d22fa676cc>EMMO is released under a Creative Commons license Attribution 4.0 International (CC BY 4.0)

https://creativecommons.org/licenses/by/4.0/legalcode</annotations:EMMO_5525a055_dda5_4556_8b91_f0d22fa676cc>
    <owl:versionIRI rdf:resource="http://emmo.info/emmo/1.0.0-alpha/top/physical"/>
  </rdf:Description>
  <rdf:Description rdf:nodeID="N0e31abafffcf4d3c8fabe3f0d0d9c06f">
    <rdf:first rdf:resource="http://emmo.info/emmo/middle/siunits#EMMO_e9ffc696_5228_4ff9_8a60_0f5e05e9931b"/>
    <rdf:rest rdf:resource="http://www.w3.org/1999/02/22-rdf-syntax-ns#nil"/>
  </rdf:Description>
  <rdf:Description rdf:nodeID="N655e919a75dd4745a1f369fed39c574c">
    <owl:hasValue>T+3 L-1 M-1 I0 Θ0 N0 J+1</owl:hasValue>
    <rdf:type rdf:resource="http://www.w3.org/2002/07/owl#Restriction"/>
    <owl:onProperty rdf:resource="http://emmo.info/emmo/middle/perceptual#EMMO_23b579e1_8088_45b5_9975_064014026c42"/>
  </rdf:Description>
  <rdf:Description rdf:nodeID="N6fab005c88674a119142e007445b2aa0">
    <rdf:first rdf:resource="http://emmo.info/emmo/middle/isq#EMMO_cd2cd0de_e0cc_4ef1_b27e_2e88db027bac"/>
    <rdf:rest rdf:nodeID="N926b5b8edc6f4dcc898644d3eeea068a"/>
  </rdf:Description>
  <rdf:Description rdf:about="http://emmo.info/emmo/middle/metrology#EMMO_1e9c2a4b_abb9_4b27_bd9c_e31aac337a04">
    <rdfs:label xml:lang="en">GreekSmallLetterMu</rdfs:label>
    <annotations:EMMO_21ae69b4_235e_479d_8dd8_4f756f694c1b>μ</annotations:EMMO_21ae69b4_235e_479d_8dd8_4f756f694c1b>
    <owl:equivalentClass rdf:nodeID="Neafdd406370c49af8626196feba5f50e"/>
    <rdf:type rdf:resource="http://www.w3.org/2002/07/owl#Class"/>
    <rdfs:subClassOf rdf:resource="http://emmo.info/emmo/middle/metrology#EMMO_e13b2173_1dec_4b97_9ac1_1dc4b418612a"/>
  </rdf:Description>
  <rdf:Description rdf:nodeID="N9a292fc0d28444a3a7e0be114463a19f">
    <owl:allValuesFrom rdf:nodeID="N725e8dabe03447759c0b65f364ec2c5a"/>
    <rdf:type rdf:resource="http://www.w3.org/2002/07/owl#Restriction"/>
    <owl:onProperty rdf:resource="http://emmo.info/emmo/middle/metrology#EMMO_67fc0a36_8dcb_4ffa_9a43_31074efa3296"/>
  </rdf:Description>
  <rdf:Description rdf:nodeID="N5f50899ee9144cedaf1ce63862644e44">
    <owl:onProperty rdf:resource="http://emmo.info/emmo/middle/holistic#EMMO_ae2d1a96_bfa1_409a_a7d2_03d69e8a125a"/>
    <rdf:type rdf:resource="http://www.w3.org/2002/07/owl#Restriction"/>
    <owl:someValuesFrom rdf:resource="http://emmo.info/emmo/middle/models#EMMO_314d0bd5_67ed_437e_a609_36d46147cea7"/>
  </rdf:Description>
  <rdf:Description rdf:nodeID="N72b3881d737c4b408c24b10c334d4360">
    <owl:someValuesFrom rdf:resource="http://emmo.info/emmo/top/semiotics#EMMO_6f5af708_f825_4feb_a0d1_a8d813d3022b"/>
    <rdf:type rdf:resource="http://www.w3.org/2002/07/owl#Restriction"/>
    <owl:onProperty rdf:resource="http://emmo.info/emmo/middle/holistic#EMMO_c5aae418_1622_4d02_93c5_21159e28e6c1"/>
  </rdf:Description>
  <rdf:Description rdf:nodeID="N17581f3a64b64569a163550af1853865">
    <owl:someValuesFrom rdf:resource="http://emmo.info/emmo/middle/isq#EMMO_a77a0a4b_6bd2_42b2_be27_4b63cebbb59e"/>
    <rdf:type rdf:resource="http://www.w3.org/2002/07/owl#Restriction"/>
    <owl:onProperty rdf:resource="http://emmo.info/emmo/middle/metrology#EMMO_bed1d005_b04e_4a90_94cf_02bc678a8569"/>
  </rdf:Description>
  <rdf:Description rdf:nodeID="Nd7285b7a5e214991b0a5178caf6dd4a9">
    <rdf:type rdf:resource="http://www.w3.org/2002/07/owl#Restriction"/>
    <owl:onProperty rdf:resource="http://emmo.info/emmo/top/mereotopology#EMMO_17e27c22_37e1_468c_9dd7_95e137f73e7f"/>
    <owl:someValuesFrom rdf:resource="http://emmo.info/emmo/middle/physicalistic#EMMO_385b8f6e_43ac_4596_ad76_ac322c68b7ca"/>
  </rdf:Description>
  <rdf:Description rdf:nodeID="N9ea10f198d0646a995a783878c724a69">
    <rdf:type rdf:resource="http://www.w3.org/2002/07/owl#Restriction"/>
    <owl:onProperty rdf:resource="http://emmo.info/emmo/middle/perceptual#EMMO_23b579e1_8088_45b5_9975_064014026c42"/>
    <owl:hasValue>lm</owl:hasValue>
  </rdf:Description>
  <rdf:Description rdf:about="http://emmo.info/emmo/middle/siunits#EMMO_f2523820_04a6_44ab_bb67_8237dda2b0c2">
    <rdfs:subClassOf rdf:nodeID="Nd551a59d627b4c9fa94beab213658180"/>
    <rdfs:label xml:lang="en">Siemens</rdfs:label>
    <rdf:type rdf:resource="http://www.w3.org/2002/07/owl#Class"/>
    <rdfs:comment>Measurement unit for electrical conductance.</rdfs:comment>
    <rdfs:subClassOf rdf:nodeID="N6f9e72c556084dc1843c76f1bb7b9c99"/>
  </rdf:Description>
  <rdf:Description rdf:nodeID="N441d88bdb30846aca2895751b79d62c6">
    <owl:onProperty rdf:resource="http://emmo.info/emmo/middle/metrology#EMMO_bed1d005_b04e_4a90_94cf_02bc678a8569"/>
    <rdf:type rdf:resource="http://www.w3.org/2002/07/owl#Restriction"/>
    <owl:someValuesFrom rdf:resource="http://emmo.info/emmo/middle/isq#EMMO_02e894c3_b793_4197_b120_3442e08f58d1"/>
  </rdf:Description>
  <rdf:Description rdf:nodeID="N2ef84063018c42cf8aa5546fc0a540a6">
    <owl:onProperty rdf:resource="http://emmo.info/emmo/middle/perceptual#EMMO_23b579e1_8088_45b5_9975_064014026c42"/>
    <owl:hasValue>rad</owl:hasValue>
    <rdf:type rdf:resource="http://www.w3.org/2002/07/owl#Restriction"/>
  </rdf:Description>
  <rdf:Description rdf:nodeID="N24d4a70633254cde8cce24b89961d3ed">
    <owl:onProperty rdf:resource="http://emmo.info/emmo/top/physical#EMMO_f68030be_94b8_4c61_a161_886468558054"/>
    <rdf:type rdf:resource="http://www.w3.org/2002/07/owl#Restriction"/>
    <owl:allValuesFrom rdf:resource="http://www.w3.org/2002/07/owl#Nothing"/>
  </rdf:Description>
  <rdf:Description rdf:nodeID="Nf5108388b7ed4945a665c80edfb01c42">
    <owl:hasValue>T-1 L+2 M+1 I0 Θ0 N0 J0</owl:hasValue>
    <rdf:type rdf:resource="http://www.w3.org/2002/07/owl#Restriction"/>
    <owl:onProperty rdf:resource="http://emmo.info/emmo/middle/perceptual#EMMO_23b579e1_8088_45b5_9975_064014026c42"/>
  </rdf:Description>
  <rdf:Description rdf:about="http://emmo.info/emmo/middle/siunits#EMMO_7db11dbf_a643_464a_9b56_07eabcc3e9c5">
    <rdfs:subClassOf rdf:nodeID="N46e75a7277184f459a11d75fb5b867d8"/>
    <annotations:EMMO_1f1b164d_ec6a_4faa_8d5e_88bda62316cc>http://qudt.org/vocab/unit/M</annotations:EMMO_1f1b164d_ec6a_4faa_8d5e_88bda62316cc>
    <rdf:type rdf:resource="http://www.w3.org/2002/07/owl#Class"/>
    <annotations:EMMO_fe015383_afb3_44a6_ae86_043628697aa2>https://doi.org/10.1351/goldbook.M03884</annotations:EMMO_fe015383_afb3_44a6_ae86_043628697aa2>
    <rdfs:subClassOf rdf:nodeID="N08a96502cf384b1dba768582d910bf54"/>
    <annotations:EMMO_70fe84ff_99b6_4206_a9fc_9a8931836d84>The metre, symbol m, is the SI unit of length. It is defined by taking the fixed numerical value of the speed of light in vacuum c to be 299792458 when expressed in the unit m s−1, where the second is defined in terms of ∆νCs.</annotations:EMMO_70fe84ff_99b6_4206_a9fc_9a8931836d84>
    <rdfs:label xml:lang="en">Metre</rdfs:label>
  </rdf:Description>
  <rdf:Description rdf:about="http://emmo.info/emmo/middle/isq#EMMO_3df10765_f6ff_4c9e_be3d_10b1809d78bd">
    <rdfs:subClassOf rdf:nodeID="N4fc9cb7bd29d4208aebd014ebbb50b3d"/>
    <annotations:EMMO_967080e5_2f42_4eb2_a3a9_c58143e835f9>A dose quantity used in the International Commission on Radiological Protection (ICRP) system of radiological protection.</annotations:EMMO_967080e5_2f42_4eb2_a3a9_c58143e835f9>
    <annotations:EMMO_fe015383_afb3_44a6_ae86_043628697aa2>https://doi.org/10.1351/goldbook.E02101</annotations:EMMO_fe015383_afb3_44a6_ae86_043628697aa2>
    <annotations:EMMO_6dd685dd_1895_46e4_b227_be9f7d643c25>http://dbpedia.org/page/Energy</annotations:EMMO_6dd685dd_1895_46e4_b227_be9f7d643c25>
    <rdf:type rdf:resource="http://www.w3.org/2002/07/owl#Class"/>
    <rdfs:label xml:lang="en">DoseEquivalent</rdfs:label>
    <rdfs:subClassOf rdf:resource="http://emmo.info/emmo/middle/isq#EMMO_2946d40b_24a1_47fa_8176_e3f79bb45064"/>
  </rdf:Description>
  <rdf:Description rdf:nodeID="N2d90dc7b048e425fb66c7ce35ec02eba">
    <rdf:rest rdf:nodeID="N123917747ed74f50936d82b6233fe51f"/>
    <rdf:first rdf:resource="http://emmo.info/emmo/middle/physicalistic#EMMO_72d53756_7fb1_46ed_980f_83f47efbe105"/>
  </rdf:Description>
  <rdf:Description rdf:about="http://emmo.info/emmo/middle/metrology#EMMO_a2f94f33_71fa_443c_a1fb_d1685fc537ec">
    <rdf:type rdf:resource="http://www.w3.org/2002/07/owl#Class"/>
    <rdfs:label xml:lang="en">SubMultipleUnit</rdfs:label>
  </rdf:Description>
  <rdf:Description rdf:about="http://emmo.info/emmo/middle/perceptual#EMMO_89a0c87c_0804_4013_937a_6fe234d9499c">
    <rdfs:subClassOf rdf:nodeID="Naeadd3ccdc6145bbb481232f62aa348c"/>
    <rdfs:label xml:lang="en">SymbolicComposition</rdfs:label>
    <rdf:type rdf:resource="http://www.w3.org/2002/07/owl#Class"/>
    <rdfs:subClassOf rdf:resource="http://emmo.info/emmo/middle/perceptual#EMMO_057e7d57_aff0_49de_911a_8861d85cef40"/>
    <annotations:EMMO_967080e5_2f42_4eb2_a3a9_c58143e835f9>A symbolic entity made of other symbolic entities according to a specific spatial configuration.</annotations:EMMO_967080e5_2f42_4eb2_a3a9_c58143e835f9>
  </rdf:Description>
  <rdf:Description rdf:about="http://emmo.info/emmo/middle/isq#EMMO_4f2d3939_91b1_4001_b8ab_7d19074bf845">
    <rdf:type rdf:resource="http://www.w3.org/2002/07/owl#Class"/>
    <annotations:EMMO_21ae69b4_235e_479d_8dd8_4f756f694c1b>Voltage</annotations:EMMO_21ae69b4_235e_479d_8dd8_4f756f694c1b>
    <rdfs:subClassOf rdf:resource="http://emmo.info/emmo/middle/isq#EMMO_2946d40b_24a1_47fa_8176_e3f79bb45064"/>
    <rdfs:label xml:lang="en">ElectricPotential</rdfs:label>
    <rdfs:subClassOf rdf:nodeID="N7928dfd0dbe9469c9055155fd87ba720"/>
    <annotations:EMMO_6dd685dd_1895_46e4_b227_be9f7d643c25>http://dbpedia.org/page/Voltage</annotations:EMMO_6dd685dd_1895_46e4_b227_be9f7d643c25>
    <annotations:EMMO_fe015383_afb3_44a6_ae86_043628697aa2>https://doi.org/10.1351/goldbook.A00424</annotations:EMMO_fe015383_afb3_44a6_ae86_043628697aa2>
    <annotations:EMMO_967080e5_2f42_4eb2_a3a9_c58143e835f9>Energy required to move a unit charge through an electric field from a reference point.</annotations:EMMO_967080e5_2f42_4eb2_a3a9_c58143e835f9>
  </rdf:Description>
  <rdf:Description rdf:nodeID="Nb7c50d3a007941bb8f3a498623f464da">
    <rdf:type rdf:resource="http://www.w3.org/2002/07/owl#Restriction"/>
    <owl:onProperty rdf:resource="http://emmo.info/emmo/top/mereotopology#EMMO_6b7276a4_4b9d_440a_b577_0277539c0fc4"/>
    <owl:someValuesFrom rdf:resource="http://emmo.info/emmo/top/mereotopology#EMMO_eb3a768e_d53e_4be9_a23b_0714833c36de"/>
  </rdf:Description>
  <rdf:Description rdf:nodeID="N8f32255d2f144776a067f6993b2ba743">
    <owl:onProperty rdf:resource="http://emmo.info/emmo/middle/metrology#EMMO_67fc0a36_8dcb_4ffa_9a43_31074efa3296"/>
    <rdf:type rdf:resource="http://www.w3.org/2002/07/owl#Restriction"/>
    <owl:allValuesFrom rdf:nodeID="N7ab01d3cc65045949f797c724c357d8c"/>
  </rdf:Description>
  <rdf:Description rdf:nodeID="N68dcad83a0604dfd940879a2a19c5bbe">
    <rdf:rest rdf:resource="http://www.w3.org/1999/02/22-rdf-syntax-ns#nil"/>
    <rdf:first rdf:resource="http://emmo.info/emmo/middle/materials#EMMO_db03061b_db31_4132_a47a_6a634846578b"/>
  </rdf:Description>
  <rdf:Description rdf:about="http://emmo.info/emmo/middle/metrology#EMMO_7d2afa66_ae9e_4095_a9bf_421d0be401b6">
    <rdfs:subClassOf rdf:resource="http://emmo.info/emmo/middle/metrology#EMMO_985bec21_989f_4b9e_a4b3_735d88099c3c"/>
    <rdf:type rdf:resource="http://www.w3.org/2002/07/owl#Class"/>
    <rdfs:subClassOf rdf:resource="http://emmo.info/emmo/middle/perceptual#EMMO_a1083d0a_c1fb_471f_8e20_a98f881ad527"/>
    <rdfs:label xml:lang="en">MetricPrefix</rdfs:label>
    <rdfs:seeAlso>https://en.wikipedia.org/wiki/Metric_prefix</rdfs:seeAlso>
    <rdfs:subClassOf rdf:resource="http://emmo.info/emmo/middle/math#EMMO_ae15fb4f_8e4d_41de_a0f9_3997f89ba6a2"/>
    <annotations:EMMO_967080e5_2f42_4eb2_a3a9_c58143e835f9>Dimensionless multiplicative unit prefix.</annotations:EMMO_967080e5_2f42_4eb2_a3a9_c58143e835f9>
  </rdf:Description>
  <rdf:Description rdf:about="http://emmo.info/emmo/middle/manufacturing#EMMO_86ca9b93_1183_4b65_81b8_c0fcd3bba5ad">
    <rdfs:label xml:lang="en">Engineered</rdfs:label>
    <rdfs:subClassOf rdf:nodeID="Neba99011675741efa2a57a0d8e2bce4a"/>
    <annotations:EMMO_b432d2d5_25f4_4165_99c5_5935a7763c1a>Car, tire, composite material.</annotations:EMMO_b432d2d5_25f4_4165_99c5_5935a7763c1a>
    <annotations:EMMO_967080e5_2f42_4eb2_a3a9_c58143e835f9>A 'physical' that stands for a real world object that has been manufacturedfor a particular purpose.</annotations:EMMO_967080e5_2f42_4eb2_a3a9_c58143e835f9>
    <rdf:type rdf:resource="http://www.w3.org/2002/07/owl#Class"/>
    <rdfs:comment>The 'Engineered' branch represents real world objects that show some level of complexity/heterogeneity in their composition, and are made for a specific use.</rdfs:comment>
  </rdf:Description>
  <rdf:Description rdf:about="http://emmo.info/emmo/top/mereotopology#EMMO_9cb984ca_48ad_4864_b09e_50d3fff19420">
    <rdf:type rdf:resource="http://www.w3.org/2002/07/owl#SymmetricProperty"/>
    <rdfs:subPropertyOf rdf:resource="http://emmo.info/emmo/top/mereotopology#EMMO_d893d373_b579_4867_841e_1c2b31a8d2c6"/>
    <rdfs:label xml:lang="en">overcrosses</rdfs:label>
    <rdf:type rdf:resource="http://www.w3.org/2002/07/owl#ObjectProperty"/>
  </rdf:Description>
  <rdf:Description rdf:nodeID="Nce81168ffc994431803922256ac689d2">
    <rdf:type rdf:resource="http://www.w3.org/2002/07/owl#Class"/>
    <owl:complementOf rdf:resource="http://emmo.info/emmo/middle/math#EMMO_54ee6b5e_5261_44a8_86eb_5717e7fdb9d0"/>
  </rdf:Description>
  <rdf:Description rdf:nodeID="N051684c726a546f1a4c75918ab158f90">
    <rdf:type rdf:resource="http://www.w3.org/2002/07/owl#Class"/>
    <owl:intersectionOf rdf:nodeID="N665db57b99214517bb4c3ab2e3364b62"/>
  </rdf:Description>
  <rdf:Description rdf:nodeID="N9b878e0544774f0891c985bb6e271b41">
    <owl:allValuesFrom rdf:resource="http://emmo.info/emmo/top/physical#EMMO_0f795e3e_c602_4577_9a43_d5a231aa1360"/>
    <owl:onProperty rdf:resource="http://emmo.info/emmo/top/physical#EMMO_7afbed84_7593_4a23_bd88_9d9c6b04e8f6"/>
    <rdf:type rdf:resource="http://www.w3.org/2002/07/owl#Restriction"/>
  </rdf:Description>
  <rdf:Description rdf:nodeID="N185e1b467bd64e3cb671664cc3d135e2">
    <rdf:rest rdf:nodeID="Nb7d3e37eb92f4940aac2fa6794e88137"/>
    <rdf:first rdf:resource="http://emmo.info/emmo/middle/siunits#EMMO_99296e55_53f7_4333_9e06_760ad175a1b9"/>
  </rdf:Description>
  <rdf:Description rdf:about="http://www.w3.org/2002/07/owl#qualifiedCardinality">
    <rdf:type rdf:resource="http://www.w3.org/2002/07/owl#AnnotationProperty"/>
  </rdf:Description>
  <rdf:Description rdf:about="http://emmo.info/emmo/middle/metrology#EMMO_ea192c80_6029_4410_863c_8eed7ea52037">
    <annotations:EMMO_21ae69b4_235e_479d_8dd8_4f756f694c1b></annotations:EMMO_21ae69b4_235e_479d_8dd8_4f756f694c1b>
    <rdf:type rdf:resource="http://www.w3.org/2002/07/owl#Class"/>
    <rdfs:label xml:lang="en">Space</rdfs:label>
    <rdfs:comment>U+0020</rdfs:comment>
    <rdfs:subClassOf rdf:resource="http://emmo.info/emmo/middle/metrology#EMMO_e13b2173_1dec_4b97_9ac1_1dc4b418612a"/>
    <owl:equivalentClass rdf:nodeID="N8652ccf023904d59961e0a26f9346c20"/>
  </rdf:Description>
  <rdf:Description rdf:about="http://emmo.info/emmo/middle/physicalistic#EMMO_8043d3c6_a4c1_4089_ba34_9744e28e5b3d">
    <rdfs:label xml:lang="en">Electron</rdfs:label>
    <annotations:EMMO_967080e5_2f42_4eb2_a3a9_c58143e835f9>The class of individuals that stand for electrons elemntary particles.</annotations:EMMO_967080e5_2f42_4eb2_a3a9_c58143e835f9>
    <rdfs:subClassOf rdf:resource="http://emmo.info/emmo/top/physical#EMMO_0f795e3e_c602_4577_9a43_d5a231aa1360"/>
    <rdf:type rdf:resource="http://www.w3.org/2002/07/owl#Class"/>
  </rdf:Description>
  <rdf:Description rdf:nodeID="N5fa729a5bde044caa5dfb0a627c3721b">
    <owl:allValuesFrom rdf:resource="http://emmo.info/emmo/middle/isq#EMMO_af24ae20_8ef2_435a_86a1_2ea44488b318"/>
    <rdf:type rdf:resource="http://www.w3.org/2002/07/owl#Restriction"/>
    <owl:onProperty rdf:resource="http://emmo.info/emmo/middle/metrology#EMMO_bed1d005_b04e_4a90_94cf_02bc678a8569"/>
  </rdf:Description>
  <rdf:Description rdf:about="http://emmo.info/emmo/middle/siunits#EMMO_506f7823_52bc_40cb_be07_b3b1e10cce13">
    <rdfs:label xml:lang="en">LuminousEfficacy</rdfs:label>
    <rdfs:subClassOf rdf:nodeID="Nc21705b592104608bee3022d3e49216e"/>
    <rdf:type rdf:resource="http://www.w3.org/2002/07/owl#Class"/>
    <annotations:EMMO_967080e5_2f42_4eb2_a3a9_c58143e835f9>The luminous efficacy of monochromatic radiation of frequency 540 × 10 12 Hz, K cd , is a technical constant that gives an exact numerical relationship between the purely physical characteristics of the radiant power stimulating the human eye (W) and its photobiological response defined by the luminous flux due to the spectral responsivity of a standard observer (lm) at a frequency of 540 × 10 12 hertz.</annotations:EMMO_967080e5_2f42_4eb2_a3a9_c58143e835f9>
  </rdf:Description>
  <rdf:Description rdf:about="http://emmo.info/emmo/middle/metrology#EMMO_71f6ab56_342c_484b_bbe0_de86b7367cb3">
    <rdf:type rdf:resource="http://www.w3.org/2002/07/owl#Class"/>
    <annotations:EMMO_967080e5_2f42_4eb2_a3a9_c58143e835f9>"Quantity, in a system of quantities, defined in terms of the base quantities of that system".</annotations:EMMO_967080e5_2f42_4eb2_a3a9_c58143e835f9>
    <rdfs:label xml:lang="en">DerivedQuantity</rdfs:label>
  </rdf:Description>
  <rdf:Description rdf:about="http://emmo.info/emmo/middle/models#EMMO_a4b14b83_9392_4a5f_a2e8_b2b58793f59b">
    <rdf:type rdf:resource="http://www.w3.org/2002/07/owl#Class"/>
    <annotations:EMMO_967080e5_2f42_4eb2_a3a9_c58143e835f9>A computational model that uses data to create new insight into the behaviour of a system.</annotations:EMMO_967080e5_2f42_4eb2_a3a9_c58143e835f9>
    <rdfs:label xml:lang="en">DataBasedModel</rdfs:label>
    <rdfs:subClassOf rdf:resource="http://emmo.info/emmo/middle/models#EMMO_f7ed665b_c2e1_42bc_889b_6b42ed3a36f0"/>
  </rdf:Description>
  <rdf:Description rdf:about="http://emmo.info/emmo/middle/isq#EMMO_50a44256_9dc5_434b_bad4_74a4d9a29989">
    <rdfs:label xml:lang="en">Pressure</rdfs:label>
    <rdfs:subClassOf rdf:nodeID="N786dfd24418f40de91cfdc85630475a3"/>
    <rdf:type rdf:resource="http://www.w3.org/2002/07/owl#Class"/>
    <rdfs:subClassOf rdf:resource="http://emmo.info/emmo/middle/isq#EMMO_2946d40b_24a1_47fa_8176_e3f79bb45064"/>
    <annotations:EMMO_6dd685dd_1895_46e4_b227_be9f7d643c25>http://dbpedia.org/page/Pressure</annotations:EMMO_6dd685dd_1895_46e4_b227_be9f7d643c25>
    <annotations:EMMO_967080e5_2f42_4eb2_a3a9_c58143e835f9>The force applied perpendicular to the surface of an object per unit area over which that force is distributed.</annotations:EMMO_967080e5_2f42_4eb2_a3a9_c58143e835f9>
    <annotations:EMMO_fe015383_afb3_44a6_ae86_043628697aa2>https://doi.org/10.1351/goldbook.P04819</annotations:EMMO_fe015383_afb3_44a6_ae86_043628697aa2>
  </rdf:Description>
  <rdf:Description rdf:nodeID="N291ef216c88c420fb5053d13150429f8">
    <rdf:rest rdf:resource="http://www.w3.org/1999/02/22-rdf-syntax-ns#nil"/>
    <rdf:first rdf:resource="http://emmo.info/emmo/middle/physicalistic#EMMO_eb3c61f0_3983_4346_a0c6_e7f6b90a67a8"/>
  </rdf:Description>
  <rdf:Description rdf:nodeID="N7132f0759b42496c9b9ad311ea575186">
    <rdf:first rdf:resource="http://emmo.info/emmo/middle/siunits#EMMO_60b78cc3_6011_4134_95ab_956f56d4bdc1"/>
    <rdf:rest rdf:nodeID="Nba7f787f10714eecac73eadd22080156"/>
  </rdf:Description>
  <rdf:Description rdf:about="http://emmo.info/emmo/middle/metrology#EMMO_591e02fd_8d37_45a6_9d11_bb21cef391a0">
    <annotations:EMMO_b432d2d5_25f4_4165_99c5_5935a7763c1a>eV
barn</annotations:EMMO_b432d2d5_25f4_4165_99c5_5935a7763c1a>
    <rdfs:subClassOf rdf:resource="http://emmo.info/emmo/middle/metrology#EMMO_b081b346_7279_46ef_9a3d_2c088fcd79f4"/>
    <annotations:EMMO_967080e5_2f42_4eb2_a3a9_c58143e835f9>A unit that does not belong to any system of units.</annotations:EMMO_967080e5_2f42_4eb2_a3a9_c58143e835f9>
    <rdfs:label xml:lang="en">OffSystemUnit</rdfs:label>
    <rdf:type rdf:resource="http://www.w3.org/2002/07/owl#Class"/>
  </rdf:Description>
  <rdf:Description rdf:nodeID="Na2403bdde07944c19843ae47be5af1dc">
    <owl:onProperty rdf:resource="http://emmo.info/emmo/middle/math#EMMO_faf79f53_749d_40b2_807c_d34244c192f4"/>
    <owl:hasValue rdf:datatype="http://www.w3.org/2001/XMLSchema#decimal">1E+6</owl:hasValue>
    <rdf:type rdf:resource="http://www.w3.org/2002/07/owl#Restriction"/>
  </rdf:Description>
  <rdf:Description rdf:nodeID="N153e5bc9c2094419a95345de81b62e76">
    <rdf:type rdf:resource="http://www.w3.org/2002/07/owl#Restriction"/>
    <owl:hasValue>Wb</owl:hasValue>
    <owl:onProperty rdf:resource="http://emmo.info/emmo/middle/perceptual#EMMO_23b579e1_8088_45b5_9975_064014026c42"/>
  </rdf:Description>
  <rdf:Description rdf:nodeID="N9abc93e180854f09bfd8d84fd55c7bd1">
    <owl:hasValue>T0 L0 M0 I+1 Θ0 N0 J0</owl:hasValue>
    <rdf:type rdf:resource="http://www.w3.org/2002/07/owl#Restriction"/>
    <owl:onProperty rdf:resource="http://emmo.info/emmo/middle/perceptual#EMMO_23b579e1_8088_45b5_9975_064014026c42"/>
  </rdf:Description>
  <rdf:Description rdf:about="http://emmo.info/emmo/middle/siunits#EMMO_b55cd09a_e54d_4eb1_81dd_03c29d1b878e">
    <rdf:type rdf:resource="http://www.w3.org/2002/07/owl#Class"/>
    <rdfs:subClassOf rdf:nodeID="Ne508bc5d17764bdc87f1c51a81f2f5f1"/>
    <rdfs:label xml:lang="en">Centi</rdfs:label>
    <rdfs:subClassOf rdf:nodeID="Nc24f28bad15f41b08cccaded51b5e0dd"/>
  </rdf:Description>
  <rdf:Description rdf:nodeID="N4c9c331d376642aeac19b3d93c417168">
    <owl:onProperty rdf:resource="http://emmo.info/emmo/middle/math#EMMO_faf79f53_749d_40b2_807c_d34244c192f4"/>
    <owl:hasValue rdf:datatype="http://www.w3.org/2001/XMLSchema#decimal">1E+24</owl:hasValue>
    <rdf:type rdf:resource="http://www.w3.org/2002/07/owl#Restriction"/>
  </rdf:Description>
  <rdf:Description rdf:nodeID="Nac71b7b699e3450ebe25e232a1d26f63">
    <rdf:type rdf:resource="http://www.w3.org/2002/07/owl#Restriction"/>
    <owl:someValuesFrom rdf:resource="http://emmo.info/emmo/middle/isq#EMMO_a77a0a4b_6bd2_42b2_be27_4b63cebbb59e"/>
    <owl:onProperty rdf:resource="http://emmo.info/emmo/middle/metrology#EMMO_bed1d005_b04e_4a90_94cf_02bc678a8569"/>
  </rdf:Description>
  <rdf:Description rdf:about="http://emmo.info/emmo/middle/siunits#EMMO_b71e4ba5_8f73_4199_8c96_7ea7f94d9e2a">
    <rdfs:subClassOf rdf:nodeID="N2566f62ad78643b8bbe22a46dcf724aa"/>
    <rdfs:label xml:lang="en">Becquerel</rdfs:label>
    <annotations:EMMO_fe015383_afb3_44a6_ae86_043628697aa2>https://doi.org/10.1351/goldbook.B00624</annotations:EMMO_fe015383_afb3_44a6_ae86_043628697aa2>
    <annotations:EMMO_1f1b164d_ec6a_4faa_8d5e_88bda62316cc>http://qudt.org/vocab/unit/BQ</annotations:EMMO_1f1b164d_ec6a_4faa_8d5e_88bda62316cc>
    <rdf:type rdf:resource="http://www.w3.org/2002/07/owl#Class"/>
    <rdfs:comment>Unit for radioactive activity.</rdfs:comment>
    <annotations:EMMO_70fe84ff_99b6_4206_a9fc_9a8931836d84>Radioactive decays per second.</annotations:EMMO_70fe84ff_99b6_4206_a9fc_9a8931836d84>
    <rdfs:subClassOf rdf:nodeID="N77c359098edf4f7db05f44fa33f9b424"/>
  </rdf:Description>
  <rdf:Description rdf:about="http://emmo.info/emmo/middle/physicalistic#EMMO_e5488299_8dab_4ebb_900a_26d2abed8396">
    <rdf:type rdf:resource="http://www.w3.org/2002/07/owl#Class"/>
    <owl:equivalentClass rdf:nodeID="Ne22b68e0af944eb29e6d1b25994e6a49"/>
    <rdfs:label xml:lang="en">Massless</rdfs:label>
    <annotations:EMMO_967080e5_2f42_4eb2_a3a9_c58143e835f9>The union of classes of elementary particles that do not possess mass.</annotations:EMMO_967080e5_2f42_4eb2_a3a9_c58143e835f9>
  </rdf:Description>
  <rdf:Description rdf:nodeID="Ne166ae38be13442c98506cbcbf8174f1">
    <owl:qualifiedCardinality rdf:datatype="http://www.w3.org/2001/XMLSchema#nonNegativeInteger">1</owl:qualifiedCardinality>
    <owl:onDataRange rdf:resource="http://www.w3.org/2001/XMLSchema#integer"/>
    <rdf:type rdf:resource="http://www.w3.org/2002/07/owl#Restriction"/>
    <owl:onProperty rdf:resource="http://emmo.info/emmo/middle/math#EMMO_faf79f53_749d_40b2_807c_d34244c192f4"/>
  </rdf:Description>
  <rdf:Description rdf:about="http://emmo.info/emmo/middle/holistic#EMMO_0277f24a_ea7f_4917_81b7_fb0406c8fc62">
    <rdfs:comment>Holism (from Greek ὅλος holos "all, whole, entire")</rdfs:comment>
    <rdf:type rdf:resource="http://www.w3.org/2002/07/owl#Class"/>
    <rdfs:subClassOf rdf:resource="http://emmo.info/emmo/top#EMMO_49267eba_5548_4163_8f36_518d65b583f9"/>
    <rdfs:comment>An holistic perspective considers each part of the whole as equally important, without the need of a granularity hierarchy, assigning a role to the whole.

Meaning that a molecule of a body can have role in the body evolution, without caring if its part of a specific organ.

This class allows the picking of parts without necessarily going trough a rigid hierarchy of compositions (e.g. body -&gt; organ -&gt; cell -&gt; molecule).</rdfs:comment>
    <rdfs:label xml:lang="en">Holistic</rdfs:label>
    <annotations:EMMO_967080e5_2f42_4eb2_a3a9_c58143e835f9>A union of classes that categorize physicals under a holistic perspective, meaning that the interest is on the whole 4D object (process) and the role of its spatial parts (participants) without going further into its subparts.</annotations:EMMO_967080e5_2f42_4eb2_a3a9_c58143e835f9>
    <owl:equivalentClass rdf:nodeID="Ndee16311420f41f595ae6a1e252dae8d"/>
  </rdf:Description>
  <rdf:Description rdf:nodeID="Nce4eaa697a224bfc84e048824d47e88f">
    <rdf:type rdf:resource="http://www.w3.org/2002/07/owl#Restriction"/>
    <owl:onProperty rdf:resource="http://emmo.info/emmo/middle/math#EMMO_faf79f53_749d_40b2_807c_d34244c192f4"/>
    <owl:hasValue rdf:datatype="http://www.w3.org/2001/XMLSchema#decimal">1E+15</owl:hasValue>
  </rdf:Description>
  <rdf:Description rdf:nodeID="N6c0f2e6691204a399713f4e206931923">
    <rdf:first rdf:resource="http://emmo.info/emmo/middle/siunits#EMMO_dc232f53_8ed8_4ddd_9f41_cc057985eadb"/>
    <rdf:rest rdf:nodeID="N728fac613521444f89f606acf02ef639"/>
  </rdf:Description>
  <rdf:Description rdf:nodeID="Nd5336b7ad877473eba001d059d8e94c2">
    <rdf:type rdf:resource="http://www.w3.org/2002/07/owl#Restriction"/>
    <owl:allValuesFrom rdf:resource="http://emmo.info/emmo/middle/isq#EMMO_501f9b3a_c469_48f7_9281_2e6a8d805d7a"/>
    <owl:onProperty rdf:resource="http://emmo.info/emmo/middle/metrology#EMMO_bed1d005_b04e_4a90_94cf_02bc678a8569"/>
  </rdf:Description>
  <rdf:Description rdf:nodeID="N282b8ef379b04a308dc835fbb9941ee7">
    <owl:hasValue rdf:datatype="http://www.w3.org/2001/XMLSchema#decimal">1E-18</owl:hasValue>
    <rdf:type rdf:resource="http://www.w3.org/2002/07/owl#Restriction"/>
    <owl:onProperty rdf:resource="http://emmo.info/emmo/middle/math#EMMO_faf79f53_749d_40b2_807c_d34244c192f4"/>
  </rdf:Description>
  <rdf:Description rdf:nodeID="Neb97b6addf694d73a2640106f9812009">
    <rdf:type rdf:resource="http://www.w3.org/2002/07/owl#Restriction"/>
    <owl:onProperty rdf:resource="http://emmo.info/emmo/middle/perceptual#EMMO_23b579e1_8088_45b5_9975_064014026c42"/>
    <owl:hasValue>Z</owl:hasValue>
  </rdf:Description>
  <rdf:Description rdf:nodeID="N4db5ab90bbd3455b889a81d7c4b0d839">
    <rdf:first rdf:resource="http://emmo.info/emmo/middle/materials#EMMO_4588526f_8553_4f4d_aa73_a483e88d599b"/>
    <rdf:rest rdf:nodeID="N68dcad83a0604dfd940879a2a19c5bbe"/>
  </rdf:Description>
  <rdf:Description rdf:nodeID="Nd278bd9ef4564eb9a5e8169ff91a93dc">
    <rdf:rest rdf:nodeID="Nee74f87cd8654a3cab7c34c85a942acf"/>
    <rdf:first rdf:resource="http://emmo.info/emmo/middle/siunits#EMMO_3a185e6c_9e19_4776_b583_19c978156aa0"/>
  </rdf:Description>
  <rdf:Description rdf:nodeID="N2eb7ecce985748a9bda630a9a3cbbe84">
    <rdf:first rdf:resource="http://emmo.info/emmo/middle/siunits#EMMO_a979c531_f9fa_4a6e_93c1.0.0-alpha960241ca6"/>
    <rdf:rest rdf:nodeID="Nad03685a5fae47db8b8331d65c2da678"/>
  </rdf:Description>
  <rdf:Description rdf:nodeID="N6eace5477e534d29a48701f5c51d4a0e">
    <rdf:type rdf:resource="http://www.w3.org/2002/07/owl#Restriction"/>
    <owl:hasValue>T</owl:hasValue>
    <owl:onProperty rdf:resource="http://emmo.info/emmo/middle/perceptual#EMMO_23b579e1_8088_45b5_9975_064014026c42"/>
  </rdf:Description>
  <rdf:Description rdf:nodeID="N5129722f30de4998bc8863ac6758cbbd">
    <rdf:type rdf:resource="http://www.w3.org/2002/07/owl#Restriction"/>
    <owl:onProperty rdf:resource="http://emmo.info/emmo/middle/metrology#EMMO_bed1d005_b04e_4a90_94cf_02bc678a8569"/>
    <owl:someValuesFrom rdf:resource="http://emmo.info/emmo/middle/isq#EMMO_847f1d9f_205e_46c1_8cb6_a9e479421f88"/>
  </rdf:Description>
  <rdf:Description rdf:about="http://emmo.info/emmo/middle/materials#EMMO_20fff605_465f_4034_8696_e53e90ec83f4">
    <annotations:EMMO_967080e5_2f42_4eb2_a3a9_c58143e835f9>A union of the four base classes for the classification of materials according to the DG-RTD Review of Materials Modelling.</annotations:EMMO_967080e5_2f42_4eb2_a3a9_c58143e835f9>
    <rdf:type rdf:resource="http://www.w3.org/2002/07/owl#Class"/>
    <owl:equivalentClass rdf:nodeID="N1627f4bbf5cf4ff6a87adff4d0afc3bf"/>
    <rdfs:seeAlso>https://op.europa.eu/en/publication-detail/-/publication/e0845ae1-1b60-11e7-aeb3-01aa75ed71a1</rdfs:seeAlso>
    <rdfs:label xml:lang="en">MaterialState</rdfs:label>
  </rdf:Description>
  <rdf:Description rdf:nodeID="Ndabdb4b08d2f436b913151095489fa52">
    <rdf:type rdf:resource="http://www.w3.org/2002/07/owl#Restriction"/>
    <owl:onProperty rdf:resource="http://emmo.info/emmo/middle/metrology#EMMO_bed1d005_b04e_4a90_94cf_02bc678a8569"/>
    <owl:someValuesFrom rdf:resource="http://emmo.info/emmo/middle/isq#EMMO_b14d9be5_f81e_469b_abca_379c2e83feab"/>
  </rdf:Description>
  <rdf:Description rdf:about="http://emmo.info/emmo/middle/siunits#EMMO_cf3dd6cc_c5d6_4b3d_aef4_82f3b7a361af">
    <annotations:EMMO_fe015383_afb3_44a6_ae86_043628697aa2>https://doi.org/10.1351/goldbook.S05971</annotations:EMMO_fe015383_afb3_44a6_ae86_043628697aa2>
    <annotations:EMMO_967080e5_2f42_4eb2_a3a9_c58143e835f9>Dimensionless measurement unit for solid angle.</annotations:EMMO_967080e5_2f42_4eb2_a3a9_c58143e835f9>
    <rdfs:subClassOf rdf:nodeID="Na236e4fed321414bb86860a10a47aaf8"/>
    <rdfs:label xml:lang="en">Steradian</rdfs:label>
    <rdfs:subClassOf rdf:nodeID="Nad2a8e1108724484bb51d872df9e0a85"/>
    <rdf:type rdf:resource="http://www.w3.org/2002/07/owl#Class"/>
    <annotations:EMMO_1f1b164d_ec6a_4faa_8d5e_88bda62316cc>http://qudt.org/vocab/unit/SR</annotations:EMMO_1f1b164d_ec6a_4faa_8d5e_88bda62316cc>
  </rdf:Description>
  <rdf:Description rdf:about="http://emmo.info/emmo/middle/math#EMMO_e56ee3eb_7609_4ae1_8bed_51974f0960a6">
    <rdfs:subClassOf rdf:nodeID="Na49bef56b0f043b8991b986a0e9a6d5d"/>
    <rdfs:comment>An equation with variables can always be represented as:

f(v0, v1, ..., vn) = g(v0, v1, ..., vn)

where f is the left hand and g the right hand  side expressions and v0, v1, ..., vn are the variables.</rdfs:comment>
    <rdfs:subClassOf rdf:resource="http://emmo.info/emmo/middle/math#EMMO_54ee6b5e_5261_44a8_86eb_5717e7fdb9d0"/>
    <rdf:type rdf:resource="http://www.w3.org/2002/07/owl#Class"/>
    <annotations:EMMO_b432d2d5_25f4_4165_99c5_5935a7763c1a>2+3 = 5
x^2 +3x  = 5x
dv/dt = a
sin(x) = y</annotations:EMMO_b432d2d5_25f4_4165_99c5_5935a7763c1a>
    <rdfs:subClassOf rdf:resource="http://emmo.info/emmo/middle/math#EMMO_88470739_03d3_4c47_a03e_b30a1288d50c"/>
    <rdfs:label xml:lang="en">Equation</rdfs:label>
    <annotations:EMMO_967080e5_2f42_4eb2_a3a9_c58143e835f9>The class of 'mathematical'-s that stand for a statement of equality between two mathematical expressions.</annotations:EMMO_967080e5_2f42_4eb2_a3a9_c58143e835f9>
  </rdf:Description>
  <rdf:Description rdf:about="http://emmo.info/emmo/middle/metrology#EMMO_216f448e_cdbc_4aeb_a529_7a5fe7fc38bb">
    <owl:equivalentClass rdf:nodeID="Ndfa1cc666c674bb1ad114c51b9598df2"/>
    <rdf:type rdf:resource="http://www.w3.org/2002/07/owl#Class"/>
    <annotations:EMMO_b432d2d5_25f4_4165_99c5_5935a7763c1a>Some examples are "Pa", "m" and "J".</annotations:EMMO_b432d2d5_25f4_4165_99c5_5935a7763c1a>
    <annotations:EMMO_967080e5_2f42_4eb2_a3a9_c58143e835f9>A symbol that stands for a single unit.</annotations:EMMO_967080e5_2f42_4eb2_a3a9_c58143e835f9>
    <rdfs:label xml:lang="en">UnitSymbol</rdfs:label>
    <owl:disjointUnionOf rdf:nodeID="N4ee846b515ab4de8b9dce6a8b778cc26"/>
  </rdf:Description>
  <rdf:Description rdf:about="http://emmo.info/emmo/middle/manufacturing#EMMO_a4d66059_5dd3_4b90_b4cb_10960559441b">
    <rdfs:subClassOf rdf:resource="http://emmo.info/emmo/middle/holistic#EMMO_43e9a05d_98af_41b4_92f6_00f79a09bfce"/>
    <rdfs:label xml:lang="en">Manufacturing</rdfs:label>
    <rdfs:subClassOf rdf:nodeID="N40bd2d5d5a134293b5554f0120a75b2d"/>
    <rdf:type rdf:resource="http://www.w3.org/2002/07/owl#Class"/>
  </rdf:Description>
  <rdf:Description rdf:about="http://emmo.info/emmo/middle/physicalistic#EMMO_25f8b804_9a0b_4387_a3e7_b35bce5365ee">
    <rdfs:comment>The class of individuals that stand for photons elementary particles.</rdfs:comment>
    <rdfs:label xml:lang="en">Photon</rdfs:label>
    <rdfs:subClassOf rdf:resource="http://emmo.info/emmo/top/physical#EMMO_0f795e3e_c602_4577_9a43_d5a231aa1360"/>
    <rdf:type rdf:resource="http://www.w3.org/2002/07/owl#Class"/>
  </rdf:Description>
  <rdf:Description rdf:nodeID="Ndb1cfab06ed449acb821b09ebfa57c32">
    <rdf:rest rdf:nodeID="Nfe162cf70f72470594b4fcae8f5fd06c"/>
    <rdf:first rdf:resource="http://emmo.info/emmo/middle/math#EMMO_54ee6b5e_5261_44a8_86eb_5717e7fdb9d0"/>
  </rdf:Description>
  <rdf:Description rdf:about="http://emmo.info/emmo/top/semiotics#EMMO_0527413c_b286_4e9c_b2d0_03fb2a038dee">
    <rdfs:subClassOf rdf:resource="http://emmo.info/emmo/top/semiotics#EMMO_b803f122_4acb_4064_9d71_c1e5fd091fc9"/>
    <annotations:EMMO_967080e5_2f42_4eb2_a3a9_c58143e835f9>The entity (or agent, or observer, or cognitive entity) who connects 'Sign', 'Interpretant' and 'Object'.</annotations:EMMO_967080e5_2f42_4eb2_a3a9_c58143e835f9>
    <rdfs:label xml:lang="en">Interpreter</rdfs:label>
    <rdfs:subClassOf rdf:nodeID="Nf3b7ff0246774851a9370121a28ffd58"/>
    <rdf:type rdf:resource="http://www.w3.org/2002/07/owl#Class"/>
  </rdf:Description>
  <rdf:Description rdf:nodeID="N4221f08354224e54856c4421ec5e2bc1">
    <rdf:type rdf:resource="http://www.w3.org/2002/07/owl#Restriction"/>
    <owl:onProperty rdf:resource="http://emmo.info/emmo/middle/math#EMMO_faf79f53_749d_40b2_807c_d34244c192f4"/>
    <owl:hasValue rdf:datatype="http://www.w3.org/2001/XMLSchema#decimal">1E+21</owl:hasValue>
  </rdf:Description>
  <rdf:Description rdf:about="http://emmo.info/emmo/middle/math#EMMO_89083bab_f69c_4d06_bf6d_62973b56cdc7">
    <rdfs:subClassOf rdf:resource="http://emmo.info/emmo/top/math#EMMO_1aed91a3_d00c_48af_8f43_a0c958b2512a"/>
    <annotations:EMMO_b432d2d5_25f4_4165_99c5_5935a7763c1a>2+2</annotations:EMMO_b432d2d5_25f4_4165_99c5_5935a7763c1a>
    <rdf:type rdf:resource="http://www.w3.org/2002/07/owl#Class"/>
    <rdfs:label xml:lang="en">ArithmeticExpression</rdfs:label>
    <rdfs:subClassOf rdf:nodeID="Na4369ab9b95d4d24b142c11880cf2a0d"/>
  </rdf:Description>
  <rdf:Description rdf:nodeID="Nacf41bf2497242d9850f79fdacee6e73">
    <owl:onProperty rdf:resource="http://emmo.info/emmo/middle/perceptual#EMMO_23b579e1_8088_45b5_9975_064014026c42"/>
    <rdf:type rdf:resource="http://www.w3.org/2002/07/owl#Restriction"/>
    <owl:hasValue>T0 L-2 M0 I0 Θ0 N0 J+1</owl:hasValue>
  </rdf:Description>
  <rdf:Description rdf:nodeID="Nf74f1aef46404e75b9b9f0dadd79bf71">
    <owl:onProperty rdf:resource="http://emmo.info/emmo/middle/metrology#EMMO_bed1d005_b04e_4a90_94cf_02bc678a8569"/>
    <rdf:type rdf:resource="http://www.w3.org/2002/07/owl#Restriction"/>
    <owl:allValuesFrom rdf:resource="http://emmo.info/emmo/middle/isq#EMMO_4f5c7c54_1c63_4d17_b12b_ea0792c2b187"/>
  </rdf:Description>
  <rdf:Description rdf:nodeID="Na49bef56b0f043b8991b986a0e9a6d5d">
    <owl:onProperty rdf:resource="http://emmo.info/emmo/middle/reductionistic#EMMO_b2282816_b7a3_44c6_b2cb_3feff1ceb7fe"/>
    <owl:someValuesFrom rdf:resource="http://emmo.info/emmo/middle/math#EMMO_f9bc8b52_85e9_4b53_b969_dd7724d5b8e4"/>
    <rdf:type rdf:resource="http://www.w3.org/2002/07/owl#Restriction"/>
  </rdf:Description>
  <rdf:Description rdf:nodeID="N4cd01a69921346739cbbb0a8e731677b">
    <owl:inverseOf rdf:resource="http://emmo.info/emmo/middle/holistic#EMMO_ae2d1a96_bfa1_409a_a7d2_03d69e8a125a"/>
  </rdf:Description>
  <rdf:Description rdf:about="http://emmo.info/emmo/middle/materials#EMMO_eb77076b_a104_42ac_a065_798b2d2809ad">
    <rdf:type rdf:resource="http://www.w3.org/2002/07/owl#Class"/>
    <rdfs:subClassOf rdf:nodeID="Na001c9b2a1734a6790db02629f49795c"/>
    <rdfs:subClassOf rdf:resource="http://emmo.info/emmo/middle/physicalistic#EMMO_4207e895_8b83_4318_996a_72cfb32acd94"/>
    <rdfs:label xml:lang="en">Atom</rdfs:label>
    <rdfs:subClassOf rdf:nodeID="N328058edab884308be404bbe6696f037"/>
    <rdfs:subClassOf rdf:resource="http://emmo.info/emmo/middle/reductionistic#EMMO_36c79456_e29c_400d_8bd3_0eedddb82652"/>
    <annotations:EMMO_967080e5_2f42_4eb2_a3a9_c58143e835f9>A standalone atom has direct part one 'nucleus' and one 'electron_cloud'. 

An O 'atom' within an O2 'molecule' is an 'e-bonded_atom'.

In this material branch, H atom is a particular case, with respect to higher atomic number atoms, since as soon as it shares its electron it has no nucleus entangled electron cloud.

We cannot say that H2 molecule has direct part two H atoms, but has direct part two H nucleus.</annotations:EMMO_967080e5_2f42_4eb2_a3a9_c58143e835f9>
    <rdfs:comment>An 'atom' is a 'nucleus' surrounded by an 'electron_cloud', i.e. a quantum system made of one or more bounded electrons.</rdfs:comment>
  </rdf:Description>
  <rdf:Description rdf:nodeID="N8eeedf64393f456a859dfb674a46dde3">
    <rdf:first rdf:resource="http://emmo.info/emmo/middle/siunits#EMMO_59c10c5c_47bd_4348_ba39_38836607dfa1"/>
    <rdf:rest rdf:nodeID="Nbb4273055f6a48b9b407cc6f7bb0062a"/>
  </rdf:Description>
  <rdf:Description rdf:nodeID="N830aa60f0938433590a923e022b588eb">
    <rdf:type rdf:resource="http://www.w3.org/2002/07/owl#Restriction"/>
    <owl:onProperty rdf:resource="http://emmo.info/emmo/middle/metrology#EMMO_bed1d005_b04e_4a90_94cf_02bc678a8569"/>
    <owl:allValuesFrom rdf:resource="http://emmo.info/emmo/middle/isq#EMMO_c8d084ad_f88e_4596_8e4d_982c6655ce6f"/>
  </rdf:Description>
  <rdf:Description rdf:nodeID="N2b4b45bcdb694dac963fd0d22f14ab1d">
    <owl:onProperty rdf:resource="http://emmo.info/emmo/middle/holistic#EMMO_c5aae418_1622_4d02_93c5_21159e28e6c1"/>
    <rdf:type rdf:resource="http://www.w3.org/2002/07/owl#Restriction"/>
    <owl:someValuesFrom rdf:resource="http://emmo.info/emmo/top/semiotics#EMMO_0527413c_b286_4e9c_b2d0_03fb2a038dee"/>
  </rdf:Description>
  <rdf:Description rdf:nodeID="N638209463e98453c8e3c24a70cbe93f0">
    <owl:hasValue>E</owl:hasValue>
    <rdf:type rdf:resource="http://www.w3.org/2002/07/owl#Restriction"/>
    <owl:onProperty rdf:resource="http://emmo.info/emmo/middle/perceptual#EMMO_23b579e1_8088_45b5_9975_064014026c42"/>
  </rdf:Description>
  <rdf:Description rdf:about="http://emmo.info/emmo/middle/siunits#EMMO_e1981c25_7c55_4020_aa7a_d2e14ced86d4">
    <rdfs:subClassOf rdf:nodeID="N78abee4c8b9b4fdcad191afc7beecd19"/>
    <rdf:type rdf:resource="http://www.w3.org/2002/07/owl#Class"/>
    <rdfs:subClassOf rdf:nodeID="Nbf60681d817f4340a460942d18805635"/>
    <rdfs:label xml:lang="en">Nano</rdfs:label>
  </rdf:Description>
  <rdf:Description rdf:about="http://emmo.info/emmo/middle/perceptual#EMMO_0c576e13_4ee7_4f3d_bfe9_1614243df018">
    <rdf:type rdf:resource="http://www.w3.org/2002/07/owl#Class"/>
    <rdfs:label xml:lang="en">1-manifold</rdfs:label>
    <rdfs:subClassOf rdf:resource="http://emmo.info/emmo/middle/perceptual#EMMO_b5957cef_a287_442d_a3ce_fd39f20ba1cd"/>
  </rdf:Description>
  <rdf:Description rdf:nodeID="Nda6fe31e41b04feba88025e8723d9eb2">
    <owl:onProperty rdf:resource="http://emmo.info/emmo/middle/perceptual#EMMO_23b579e1_8088_45b5_9975_064014026c42"/>
    <owl:hasValue>Gy</owl:hasValue>
    <rdf:type rdf:resource="http://www.w3.org/2002/07/owl#Restriction"/>
  </rdf:Description>
  <rdf:Description rdf:about="http://emmo.info/emmo/middle/physicalistic#EMMO_385b8f6e_43ac_4596_ad76_ac322c68b7ca">
    <rdfs:label xml:lang="en">Massive</rdfs:label>
    <owl:equivalentClass rdf:nodeID="N04a9f2a19f8b43eb93c67b7c0f24bf76"/>
    <annotations:EMMO_967080e5_2f42_4eb2_a3a9_c58143e835f9>The union of classes of elementary particles that possess mass.</annotations:EMMO_967080e5_2f42_4eb2_a3a9_c58143e835f9>
    <rdf:type rdf:resource="http://www.w3.org/2002/07/owl#Class"/>
  </rdf:Description>
  <rdf:Description rdf:nodeID="N4478dfee0ae845f4aaacb651ba609e4b">
    <owl:onProperty rdf:resource="http://emmo.info/emmo/middle/perceptual#EMMO_23b579e1_8088_45b5_9975_064014026c42"/>
    <owl:hasValue>T-3 L+2 M+1 I-2 Θ0 N0 J0</owl:hasValue>
    <rdf:type rdf:resource="http://www.w3.org/2002/07/owl#Restriction"/>
  </rdf:Description>
  <rdf:Description rdf:nodeID="N148cdca1920c4102abc3d0f93b7d1890">
    <rdf:rest rdf:nodeID="Nfdc465a91c05463cb6fb6b5925745208"/>
    <rdf:first rdf:resource="http://emmo.info/emmo/top/semiotics#EMMO_0527413c_b286_4e9c_b2d0_03fb2a038dee"/>
  </rdf:Description>
  <rdf:Description rdf:about="http://emmo.info/emmo/middle/isq#EMMO_66bc9029_f473_45ff_bab9_c3509ff37a22">
    <annotations:EMMO_6dd685dd_1895_46e4_b227_be9f7d643c25>http://dbpedia.org/page/Temperature</annotations:EMMO_6dd685dd_1895_46e4_b227_be9f7d643c25>
    <rdf:type rdf:resource="http://www.w3.org/2002/07/owl#Class"/>
    <rdfs:subClassOf rdf:resource="http://emmo.info/emmo/middle/isq#EMMO_2946d40b_24a1_47fa_8176_e3f79bb45064"/>
    <annotations:EMMO_967080e5_2f42_4eb2_a3a9_c58143e835f9>An objective comparative measure of hot or cold. 

Temperature is a relative quantity that can be used to express temperature differences. Unlike ThermodynamicTemperature, it cannot express absolute temperatures.</annotations:EMMO_967080e5_2f42_4eb2_a3a9_c58143e835f9>
    <annotations:EMMO_fe015383_afb3_44a6_ae86_043628697aa2>https://doi.org/10.1351/goldbook.T06261</annotations:EMMO_fe015383_afb3_44a6_ae86_043628697aa2>
    <rdfs:label>CelsiusTemperature</rdfs:label>
    <rdfs:subClassOf rdf:nodeID="N744e3020c61b43b58a0de48d90f8907a"/>
  </rdf:Description>
  <rdf:Description rdf:nodeID="N23ef7077e59e434bb6ba7bb6a8ab5b3a">
    <owl:hasValue>T-2 L+2 M+1 I0 Θ0 N0 J0</owl:hasValue>
    <owl:onProperty rdf:resource="http://emmo.info/emmo/middle/perceptual#EMMO_23b579e1_8088_45b5_9975_064014026c42"/>
    <rdf:type rdf:resource="http://www.w3.org/2002/07/owl#Restriction"/>
  </rdf:Description>
  <rdf:Description rdf:about="http://emmo.info/emmo/middle/properties#EMMO_251cfb4f_5c75_4778_91ed_6c8395212fd8">
    <rdfs:label xml:lang="en">SubjectiveProperty</rdfs:label>
    <rdfs:comment>The word subjective means that a non-well defined or an unknown procedure is used for the definition of the property.

This happens due to e.g. the complexity of the object, the lack of a underlying model for the representation of the object, the non-well specified meaning of the property symbols. 

A 'SubjectiveProperty' cannot be used to univocally compare 'Object'-s.

e.g. you cannot evaluate the beauty of a person on objective basis.</rdfs:comment>
    <annotations:EMMO_b432d2d5_25f4_4165_99c5_5935a7763c1a>The beauty of that girl.
The style of your clothing.</annotations:EMMO_b432d2d5_25f4_4165_99c5_5935a7763c1a>
    <rdf:type rdf:resource="http://www.w3.org/2002/07/owl#Class"/>
    <annotations:EMMO_967080e5_2f42_4eb2_a3a9_c58143e835f9>A 'Property' that cannot be univocally determined and depends on an agent (e.g. a human individual, a community) acting as black-box.</annotations:EMMO_967080e5_2f42_4eb2_a3a9_c58143e835f9>
  </rdf:Description>
  <rdf:Description rdf:about="http://emmo.info/emmo/middle/materials#EMMO_2fd3f574_5e93_47fe_afca_ed80b0a21ab4">
    <rdfs:comment>A standalone atom can be bonded with other atoms by intermolecular forces (i.e. dipole–dipole, London dispersion force, hydrogen bonding), since this bonds does not involve electron sharing.</rdfs:comment>
    <rdfs:label xml:lang="en">StandaloneAtom</rdfs:label>
    <rdfs:subClassOf rdf:resource="http://emmo.info/emmo/middle/materials#EMMO_eb77076b_a104_42ac_a065_798b2d2809ad"/>
    <annotations:EMMO_967080e5_2f42_4eb2_a3a9_c58143e835f9>An atom that does not share electrons with other atoms.</annotations:EMMO_967080e5_2f42_4eb2_a3a9_c58143e835f9>
    <rdf:type rdf:resource="http://www.w3.org/2002/07/owl#Class"/>
    <owl:disjointUnionOf rdf:nodeID="N4db5ab90bbd3455b889a81d7c4b0d839"/>
  </rdf:Description>
  <rdf:Description rdf:nodeID="Nc21705b592104608bee3022d3e49216e">
    <rdf:type rdf:resource="http://www.w3.org/2002/07/owl#Restriction"/>
    <owl:allValuesFrom rdf:nodeID="N3262e7503a9b437db3d8390be2bbd536"/>
    <owl:onProperty rdf:resource="http://emmo.info/emmo/middle/metrology#EMMO_67fc0a36_8dcb_4ffa_9a43_31074efa3296"/>
  </rdf:Description>
  <rdf:Description rdf:nodeID="Nfd0c59444f6f4313abe535d92b42e158">
    <rdf:first rdf:resource="http://emmo.info/emmo/top/mereotopology#EMMO_2d2ecd97_067f_4d0e_950c_d746b7700a31"/>
    <rdf:rest rdf:nodeID="N889fdf1e62aa44cc8243b21b30dfbd9c"/>
  </rdf:Description>
  <rdf:Description rdf:nodeID="N01f6e7f45ccf44fdb5457f6f651bdc87">
    <owl:allValuesFrom rdf:nodeID="Nd1d5e3a9c46a4f0cb280276de1dda067"/>
    <rdf:type rdf:resource="http://www.w3.org/2002/07/owl#Restriction"/>
    <owl:onProperty rdf:resource="http://emmo.info/emmo/middle/reductionistic#EMMO_b2282816_b7a3_44c6_b2cb_3feff1ceb7fe"/>
  </rdf:Description>
  <rdf:Description rdf:about="http://emmo.info/emmo/middle/siunits#EMMO_a9201b2f_e6de_442a_b3a6_d291.0.0-alphaa582">
    <rdfs:subClassOf rdf:nodeID="Ndabdb4b08d2f436b913151095489fa52"/>
    <rdfs:subClassOf rdf:nodeID="N4bc3064a9a434373b6319b154507a5c0"/>
    <annotations:EMMO_1f1b164d_ec6a_4faa_8d5e_88bda62316cc>http://qudt.org/vocab/unit/FARAD</annotations:EMMO_1f1b164d_ec6a_4faa_8d5e_88bda62316cc>
    <rdfs:label xml:lang="en">Farad</rdfs:label>
    <rdfs:comment>Measurement unit for electric capacitance.</rdfs:comment>
    <annotations:EMMO_fe015383_afb3_44a6_ae86_043628697aa2>https://doi.org/10.1351/goldbook.F02320</annotations:EMMO_fe015383_afb3_44a6_ae86_043628697aa2>
    <rdf:type rdf:resource="http://www.w3.org/2002/07/owl#Class"/>
  </rdf:Description>
  <rdf:Description rdf:nodeID="N83c6e862089248f3ad23c9187e167935">
    <owl:onProperty rdf:resource="http://emmo.info/emmo/middle/math#EMMO_faf79f53_749d_40b2_807c_d34244c192f4"/>
    <rdf:type rdf:resource="http://www.w3.org/2002/07/owl#Restriction"/>
    <owl:someValuesFrom rdf:resource="http://www.w3.org/2001/XMLSchema#integer"/>
  </rdf:Description>
  <rdf:Description rdf:about="http://emmo.info/emmo/middle/isq#EMMO_3ecff38b_b3cf_4a78_b49f_8580abf8715b">
    <rdfs:subClassOf rdf:resource="http://emmo.info/emmo/middle/metrology#EMMO_9895a1b4_f0a5_4167_ac5e_97db40b8bfcc"/>
    <rdfs:label xml:lang="en">MassSquareLengthPerTemperatureSquareTimeDimension</rdfs:label>
    <owl:equivalentClass rdf:nodeID="N64753d22cbae498e88b55f84a7caf341"/>
    <rdf:type rdf:resource="http://www.w3.org/2002/07/owl#Class"/>
  </rdf:Description>
  <rdf:Description rdf:about="http://emmo.info/emmo/middle/perceptual#EMMO_9268958f_7f54_48ab_a693_febe2645892b">
    <rdf:type rdf:resource="http://www.w3.org/2002/07/owl#Class"/>
    <rdfs:label xml:lang="en">2-manifold</rdfs:label>
    <rdfs:subClassOf rdf:resource="http://emmo.info/emmo/middle/perceptual#EMMO_b5957cef_a287_442d_a3ce_fd39f20ba1cd"/>
  </rdf:Description>
  <rdf:Description rdf:about="http://emmo.info/emmo/top/math#EMMO_b5c58790_fb2d_42eb_b184_2a3f6ca60acb">
    <rdfs:subClassOf rdf:resource="http://emmo.info/emmo/top/math#EMMO_f8a2fe9f_458b_4771_9aba_a50e76afc52d"/>
    <owl:equivalentClass rdf:nodeID="N60abfc76aea241859d3d9e82448ea0d8"/>
    <rdfs:label xml:lang="en">Gradient</rdfs:label>
    <rdf:type rdf:resource="http://www.w3.org/2002/07/owl#Class"/>
  </rdf:Description>
  <rdf:Description rdf:nodeID="N72f492c1a32c4f8a95adf331afffb9ab">
    <owl:onProperty rdf:resource="http://emmo.info/emmo/middle/reductionistic#EMMO_b2282816_b7a3_44c6_b2cb_3feff1ceb7fe"/>
    <rdf:type rdf:resource="http://www.w3.org/2002/07/owl#Restriction"/>
    <owl:someValuesFrom rdf:resource="http://emmo.info/emmo/middle/metrology#EMMO_02c0621e_a527_4790_8a0f_2bb51973c819"/>
  </rdf:Description>
  <rdf:Description rdf:nodeID="Nbed0fb15110e42b0abd1b2cd96d2b3e6">
    <rdf:type rdf:resource="http://www.w3.org/2002/07/owl#Restriction"/>
    <owl:onProperty rdf:resource="http://emmo.info/emmo/middle/metrology#EMMO_67fc0a36_8dcb_4ffa_9a43_31074efa3296"/>
    <owl:allValuesFrom rdf:nodeID="N18764fea94c541c1a411169f3c7cdf44"/>
  </rdf:Description>
  <rdf:Description rdf:nodeID="Nbf60681d817f4340a460942d18805635">
    <owl:allValuesFrom rdf:nodeID="Nd8591486040d427eaac7fad13c9d90f3"/>
    <owl:onProperty rdf:nodeID="N3e86b38e50ed4085ab8f87fbad5078e5"/>
    <rdf:type rdf:resource="http://www.w3.org/2002/07/owl#Restriction"/>
  </rdf:Description>
  <rdf:Description rdf:nodeID="N8edc1101dbee4e7b82b49904ab6080bd">
    <rdf:first rdf:resource="http://emmo.info/emmo/middle/siunits#EMMO_e9ffc696_5228_4ff9_8a60_0f5e05e9931b"/>
    <rdf:rest rdf:resource="http://www.w3.org/1999/02/22-rdf-syntax-ns#nil"/>
  </rdf:Description>
  <rdf:Description rdf:nodeID="N798b68e95f1343b9babd37017664044e">
    <rdf:type rdf:resource="http://www.w3.org/2002/07/owl#Restriction"/>
    <owl:onProperty rdf:resource="http://emmo.info/emmo/middle/reductionistic#EMMO_b2282816_b7a3_44c6_b2cb_3feff1ceb7fe"/>
    <owl:allValuesFrom rdf:nodeID="N7a11344ac6a2458da190ae695b24914e"/>
  </rdf:Description>
  <rdf:Description rdf:nodeID="N8113dcfa51e747fd9fa006baadfd8b5c">
    <owl:unionOf rdf:nodeID="N782679aee918406b85e24e8aa91c028f"/>
    <rdf:type rdf:resource="http://www.w3.org/2002/07/owl#Class"/>
  </rdf:Description>
  <rdf:Description rdf:nodeID="N4fc9cb7bd29d4208aebd014ebbb50b3d">
    <owl:allValuesFrom rdf:nodeID="Nc3336583216f4625a3f01eb5fe590dbd"/>
    <owl:onProperty rdf:resource="http://emmo.info/emmo/middle/metrology#EMMO_67fc0a36_8dcb_4ffa_9a43_31074efa3296"/>
    <rdf:type rdf:resource="http://www.w3.org/2002/07/owl#Restriction"/>
  </rdf:Description>
  <rdf:Description rdf:nodeID="Nc3336583216f4625a3f01eb5fe590dbd">
    <owl:allValuesFrom rdf:resource="http://emmo.info/emmo/middle/isq#EMMO_847f1d9f_205e_46c1_8cb6_a9e479421f88"/>
    <rdf:type rdf:resource="http://www.w3.org/2002/07/owl#Restriction"/>
    <owl:onProperty rdf:resource="http://emmo.info/emmo/middle/metrology#EMMO_bed1d005_b04e_4a90_94cf_02bc678a8569"/>
  </rdf:Description>
  <rdf:Description rdf:nodeID="N550fbc468c7b47da84853a777f7be49b">
    <owl:onProperty rdf:resource="http://emmo.info/emmo/middle/metrology#EMMO_bed1d005_b04e_4a90_94cf_02bc678a8569"/>
    <owl:allValuesFrom rdf:resource="http://emmo.info/emmo/middle/isq#EMMO_668e6ead_1530_40cc_ad5e_24b880edff50"/>
    <rdf:type rdf:resource="http://www.w3.org/2002/07/owl#Restriction"/>
  </rdf:Description>
  <rdf:Description rdf:nodeID="Na21084a7a3ad45dcb121e646436cff95">
    <owl:inverseOf rdf:resource="http://emmo.info/emmo/middle/properties#EMMO_e1097637_70d2_4895_973f_2396f04fa204"/>
  </rdf:Description>
  <rdf:Description rdf:nodeID="N9def89b42bfd45adb8da560f72fb7f70">
    <owl:allValuesFrom rdf:resource="http://emmo.info/emmo/middle/isq#EMMO_14ff4393_0f28_4fb4_abc7_c2cc00bc761d"/>
    <rdf:type rdf:resource="http://www.w3.org/2002/07/owl#Restriction"/>
    <owl:onProperty rdf:resource="http://emmo.info/emmo/middle/metrology#EMMO_bed1d005_b04e_4a90_94cf_02bc678a8569"/>
  </rdf:Description>
  <rdf:Description rdf:about="http://emmo.info/emmo/middle/models#EMMO_b29fd350_39aa_4af7_9459_3faa0544cba6">
    <rdfs:subClassOf rdf:nodeID="N86d8e86ed44243928b494dd9be8446ad"/>
    <rdfs:subClassOf rdf:resource="http://emmo.info/emmo/middle/models#EMMO_f7ed665b_c2e1_42bc_889b_6b42ed3a36f0"/>
    <rdfs:subClassOf rdf:nodeID="Ne1847459f29e4dd08aeff03242ece764"/>
    <rdf:type rdf:resource="http://www.w3.org/2002/07/owl#Class"/>
    <annotations:EMMO_967080e5_2f42_4eb2_a3a9_c58143e835f9>A solvable set of one Physics Equation and one or more Materials Relations.</annotations:EMMO_967080e5_2f42_4eb2_a3a9_c58143e835f9>
    <rdfs:label xml:lang="en">PhysicsBasedModel</rdfs:label>
  </rdf:Description>
  <rdf:Description rdf:nodeID="Nadafa3b0ae8c49d088c75c0e66b50b33">
    <owl:onProperty rdf:resource="http://emmo.info/emmo/middle/perceptual#EMMO_23b579e1_8088_45b5_9975_064014026c42"/>
    <rdf:type rdf:resource="http://www.w3.org/2002/07/owl#Restriction"/>
    <owl:hasValue>T+3 L-2 M-1 I+2 Θ0 N0 J0</owl:hasValue>
  </rdf:Description>
  <rdf:Description rdf:nodeID="N43ff929e5cae4d29b49e0f325a8eb9b4">
    <rdf:rest rdf:resource="http://www.w3.org/1999/02/22-rdf-syntax-ns#nil"/>
    <rdf:first rdf:resource="http://emmo.info/emmo/middle/siunits#EMMO_d41ce84b_4317_41fb_a5d1_6cd281fca106"/>
  </rdf:Description>
  <rdf:Description rdf:about="http://emmo.info/emmo/middle/models#EMMO_84cadc45_6758_46f2_ba2a_5ead65c70213">
    <annotations:EMMO_967080e5_2f42_4eb2_a3a9_c58143e835f9>A physics-based model based on a physics equation describing the behaviour of atoms.</annotations:EMMO_967080e5_2f42_4eb2_a3a9_c58143e835f9>
    <rdfs:subClassOf rdf:resource="http://emmo.info/emmo/middle/models#EMMO_b29fd350_39aa_4af7_9459_3faa0544cba6"/>
    <rdfs:label xml:lang="en">AtomisticModel</rdfs:label>
    <rdf:type rdf:resource="http://www.w3.org/2002/07/owl#Class"/>
  </rdf:Description>
  <rdf:Description rdf:nodeID="N64753d22cbae498e88b55f84a7caf341">
    <owl:onProperty rdf:resource="http://emmo.info/emmo/middle/perceptual#EMMO_23b579e1_8088_45b5_9975_064014026c42"/>
    <rdf:type rdf:resource="http://www.w3.org/2002/07/owl#Restriction"/>
    <owl:hasValue>T-2 L+2 M+1 I0 Θ-1 N0 J0</owl:hasValue>
  </rdf:Description>
  <rdf:Description rdf:nodeID="N6223cb60490742ae8635125b5524d030">
    <rdf:type rdf:resource="http://www.w3.org/2002/07/owl#Restriction"/>
    <owl:allValuesFrom rdf:resource="http://emmo.info/emmo/middle/perceptual#EMMO_a1083d0a_c1fb_471f_8e20_a98f881ad527"/>
    <owl:onProperty rdf:resource="http://emmo.info/emmo/middle/reductionistic#EMMO_b2282816_b7a3_44c6_b2cb_3feff1ceb7fe"/>
  </rdf:Description>
  <rdf:Description rdf:about="http://emmo.info/emmo/middle/perceptual#EMMO_0d69f94a_f4fa_49d9_bf90_ace770eeab02">
    <annotations:EMMO_967080e5_2f42_4eb2_a3a9_c58143e835f9>A 'acoustical' that can be categorized as music by the ontologist.</annotations:EMMO_967080e5_2f42_4eb2_a3a9_c58143e835f9>
    <rdf:type rdf:resource="http://www.w3.org/2002/07/owl#Class"/>
    <rdfs:label xml:lang="en">Music</rdfs:label>
    <rdfs:subClassOf rdf:resource="http://emmo.info/emmo/middle/perceptual#EMMO_4b3afb22_27cf_4ce3_88bc_492bfccb546b"/>
    <rdfs:comment>A music score is not a 'music' individual.

A music score is a 'graphical' that can stand for a 'music' (or vice versa) since it comes through a different perception mechanism.

The 'music' individual is the sound itself as produced and delivered by a source in the form of sound wave through a medium.</rdfs:comment>
  </rdf:Description>
  <rdf:Description rdf:about="http://emmo.info/emmo/middle/isq#EMMO_8e5dd473_808b_4a8a_b7cd_63068c12ff57">
    <rdfs:label xml:lang="en">AbsorbedDose</rdfs:label>
    <rdfs:subClassOf rdf:nodeID="N19e5134869b348bcbeded8f96303d7fe"/>
    <annotations:EMMO_fe015383_afb3_44a6_ae86_043628697aa2>https://doi.org/10.1351/goldbook.A00031</annotations:EMMO_fe015383_afb3_44a6_ae86_043628697aa2>
    <annotations:EMMO_6dd685dd_1895_46e4_b227_be9f7d643c25>http://dbpedia.org/page/Absorbed_dose</annotations:EMMO_6dd685dd_1895_46e4_b227_be9f7d643c25>
    <rdf:type rdf:resource="http://www.w3.org/2002/07/owl#Class"/>
    <rdfs:subClassOf rdf:resource="http://emmo.info/emmo/middle/isq#EMMO_2946d40b_24a1_47fa_8176_e3f79bb45064"/>
    <annotations:EMMO_70fe84ff_99b6_4206_a9fc_9a8931836d84>Energy imparted to matter by ionizing radiation in a suitable small element of volume divided by the mass of that element of volume.</annotations:EMMO_70fe84ff_99b6_4206_a9fc_9a8931836d84>
  </rdf:Description>
  <rdf:Description rdf:nodeID="N6b686c46525440a1967ecf97244e5e77">
    <rdf:type rdf:resource="http://www.w3.org/2002/07/owl#Restriction"/>
    <owl:onProperty rdf:resource="http://emmo.info/emmo/middle/perceptual#EMMO_23b579e1_8088_45b5_9975_064014026c42"/>
    <owl:hasValue>T0 L0 M0 I0 Θ0 N-1 J0</owl:hasValue>
  </rdf:Description>
  <rdf:Description rdf:nodeID="N05665de6f15f469b993e67d5181bc395">
    <rdf:type rdf:resource="http://www.w3.org/2002/07/owl#Restriction"/>
    <owl:someValuesFrom rdf:resource="http://emmo.info/emmo/middle/isq#EMMO_515b5579_d526_4842_9e6f_ecc34db6f368"/>
    <owl:onProperty rdf:resource="http://emmo.info/emmo/middle/metrology#EMMO_bed1d005_b04e_4a90_94cf_02bc678a8569"/>
  </rdf:Description>
  <rdf:Description rdf:nodeID="N6133856df4f949c5b6bc0030a5b02dd6">
    <rdf:type rdf:resource="http://www.w3.org/2002/07/owl#Restriction"/>
    <owl:someValuesFrom rdf:resource="http://emmo.info/emmo/top/semiotics#EMMO_b21a56ed_f969_4612_a6ec_cb7766f7f31d"/>
    <owl:onProperty rdf:resource="http://emmo.info/emmo/middle/holistic#EMMO_c5aae418_1622_4d02_93c5_21159e28e6c1"/>
  </rdf:Description>
  <rdf:Description rdf:nodeID="N8c23aba26af14e85906afda01c1d7d50">
    <rdf:type rdf:resource="http://www.w3.org/2002/07/owl#Restriction"/>
    <owl:allValuesFrom rdf:nodeID="N5fa729a5bde044caa5dfb0a627c3721b"/>
    <owl:onProperty rdf:resource="http://emmo.info/emmo/middle/metrology#EMMO_67fc0a36_8dcb_4ffa_9a43_31074efa3296"/>
  </rdf:Description>
  <rdf:Description rdf:about="http://emmo.info/emmo/middle/metrology#EMMO_e13b2173_1dec_4b97_9ac1_1dc4b418612a">
    <rdf:type rdf:resource="http://www.w3.org/2002/07/owl#Class"/>
    <rdfs:label xml:lang="en">UTF8</rdfs:label>
    <rdfs:subClassOf rdf:resource="http://emmo.info/emmo/middle/perceptual#EMMO_a1083d0a_c1fb_471f_8e20_a98f881ad527"/>
  </rdf:Description>
  <rdf:Description rdf:about="http://emmo.info/emmo/middle/properties#EMMO_873b0ab3_88e6_4054_b901_5531e01f14a4">
    <rdfs:label xml:lang="en">MeasuredQuantitativeProperty</rdfs:label>
    <rdf:type rdf:resource="http://www.w3.org/2002/07/owl#Class"/>
  </rdf:Description>
  <rdf:Description rdf:nodeID="N3bda4aef4b4b4b928a30d6d13ec1d6f9">
    <owl:hasValue>m</owl:hasValue>
    <rdf:type rdf:resource="http://www.w3.org/2002/07/owl#Restriction"/>
    <owl:onProperty rdf:resource="http://emmo.info/emmo/middle/perceptual#EMMO_23b579e1_8088_45b5_9975_064014026c42"/>
  </rdf:Description>
  <rdf:Description rdf:nodeID="N728fac613521444f89f606acf02ef639">
    <rdf:rest rdf:nodeID="Na82d7e7aaa1d44aaa8e32583a4cc2ce5"/>
    <rdf:first rdf:resource="http://emmo.info/emmo/middle/siunits#EMMO_e2207e91_02b0_4a8a_b13e_61d2a2a839f1"/>
  </rdf:Description>
  <rdf:Description rdf:about="http://emmo.info/emmo/top/math#EMMO_4bc29b0f_8fcc_4026_a291_f9774a66d9b8">
    <rdf:type rdf:resource="http://www.w3.org/2002/07/owl#Class"/>
    <annotations:EMMO_b432d2d5_25f4_4165_99c5_5935a7763c1a>y = f(x)</annotations:EMMO_b432d2d5_25f4_4165_99c5_5935a7763c1a>
    <annotations:EMMO_967080e5_2f42_4eb2_a3a9_c58143e835f9>A function defined using functional notation.</annotations:EMMO_967080e5_2f42_4eb2_a3a9_c58143e835f9>
    <rdfs:label xml:lang="en">FunctionDefinition</rdfs:label>
    <rdfs:subClassOf rdf:resource="http://emmo.info/emmo/top/math#EMMO_29afdf54_90ae_4c98_8845_fa9ea3f143a8"/>
  </rdf:Description>
  <rdf:Description rdf:nodeID="N11fd8522000d4edea489c10cdaa024a1">
    <owl:hasValue>z</owl:hasValue>
    <rdf:type rdf:resource="http://www.w3.org/2002/07/owl#Restriction"/>
    <owl:onProperty rdf:resource="http://emmo.info/emmo/middle/perceptual#EMMO_23b579e1_8088_45b5_9975_064014026c42"/>
  </rdf:Description>
  <rdf:Description rdf:about="http://emmo.info/emmo/middle/math#EMMO_0b6ebe5a_0026_4bef_a1c1_5be00df9f98e">
    <annotations:EMMO_967080e5_2f42_4eb2_a3a9_c58143e835f9>A relation which makes a non-equal comparison between two numbers or other mathematical expressions.</annotations:EMMO_967080e5_2f42_4eb2_a3a9_c58143e835f9>
    <rdfs:label xml:lang="en">Inequality</rdfs:label>
    <annotations:EMMO_b432d2d5_25f4_4165_99c5_5935a7763c1a>f(x) &gt; 0</annotations:EMMO_b432d2d5_25f4_4165_99c5_5935a7763c1a>
    <rdfs:subClassOf rdf:resource="http://emmo.info/emmo/middle/math#EMMO_88470739_03d3_4c47_a03e_b30a1288d50c"/>
    <rdf:type rdf:resource="http://www.w3.org/2002/07/owl#Class"/>
  </rdf:Description>
  <rdf:Description rdf:nodeID="Nad0d20865f95462fa10914def1cb1717">
    <owl:onProperty rdf:resource="http://emmo.info/emmo/middle/perceptual#EMMO_23b579e1_8088_45b5_9975_064014026c42"/>
    <rdf:type rdf:resource="http://www.w3.org/2002/07/owl#Restriction"/>
    <owl:qualifiedCardinality rdf:datatype="http://www.w3.org/2001/XMLSchema#nonNegativeInteger">1</owl:qualifiedCardinality>
    <owl:onDataRange rdf:resource="http://www.w3.org/2001/XMLSchema#string"/>
  </rdf:Description>
  <rdf:Description rdf:about="http://emmo.info/emmo/middle/models#EMMO_6c739b1a_a774_4416_bb31_1961486fa9ed">
    <rdfs:label xml:lang="en">Theorization</rdfs:label>
    <annotations:EMMO_967080e5_2f42_4eb2_a3a9_c58143e835f9>The 'semiosis' process of interpreting a 'physical' and provide a complec sign, 'theory' that stands for it and explain it to another interpreter.</annotations:EMMO_967080e5_2f42_4eb2_a3a9_c58143e835f9>
    <rdf:type rdf:resource="http://www.w3.org/2002/07/owl#Class"/>
    <rdfs:subClassOf rdf:resource="http://emmo.info/emmo/middle/properties#EMMO_10a5fd39_06aa_4648_9e70_f962a9cb2069"/>
  </rdf:Description>
  <rdf:Description rdf:nodeID="Nffeda470672d4275846249acfcc43ddd">
    <owl:hasValue rdf:datatype="http://www.w3.org/2001/XMLSchema#decimal">1E+12</owl:hasValue>
    <rdf:type rdf:resource="http://www.w3.org/2002/07/owl#Restriction"/>
    <owl:onProperty rdf:resource="http://emmo.info/emmo/middle/math#EMMO_faf79f53_749d_40b2_807c_d34244c192f4"/>
  </rdf:Description>
  <rdf:Description rdf:nodeID="N40b9ddd8943b45d2b252e96f8efb76ec">
    <rdf:type rdf:resource="http://www.w3.org/2002/07/owl#Class"/>
    <owl:unionOf rdf:nodeID="Nbf40eebcc71f4e81b07005d218fdeeaf"/>
  </rdf:Description>
  <rdf:Description rdf:nodeID="N8f4f5099a7e945f6aa22e0d84b8a0960">
    <owl:onProperty rdf:resource="http://emmo.info/emmo/middle/metrology#EMMO_67fc0a36_8dcb_4ffa_9a43_31074efa3296"/>
    <rdf:type rdf:resource="http://www.w3.org/2002/07/owl#Restriction"/>
    <owl:allValuesFrom rdf:nodeID="N8ac74537a11b459f83ec52b7358c9d33"/>
  </rdf:Description>
  <rdf:Description rdf:nodeID="N8dc70def2bea4d58920e7423f21b1623">
    <rdf:first rdf:resource="http://emmo.info/emmo/middle/siunits#EMMO_db5dd38d_ac79_4af6_8782_fee7e7150ae8"/>
    <rdf:rest rdf:nodeID="Na6787a0bc41940b491a493ea6434470a"/>
  </rdf:Description>
  <rdf:Description rdf:about="http://emmo.info/emmo/middle/materials#EMMO_8f87e700_99a8_4427_8ffb_e493de05c217">
    <rdf:type rdf:resource="http://www.w3.org/2002/07/owl#Class"/>
    <rdfs:label xml:lang="en">Proton</rdfs:label>
  </rdf:Description>
  <rdf:Description rdf:nodeID="Nb9ddbe209ce44b7b880d78e0f2a0e93f">
    <owl:onProperty rdf:resource="http://emmo.info/emmo/middle/perceptual#EMMO_23b579e1_8088_45b5_9975_064014026c42"/>
    <owl:hasValue>C</owl:hasValue>
    <rdf:type rdf:resource="http://www.w3.org/2002/07/owl#Restriction"/>
  </rdf:Description>
  <rdf:Description rdf:nodeID="N4835458880484492b1ef37e8b593170d">
    <owl:hasValue>d</owl:hasValue>
    <rdf:type rdf:resource="http://www.w3.org/2002/07/owl#Restriction"/>
    <owl:onProperty rdf:resource="http://emmo.info/emmo/middle/perceptual#EMMO_23b579e1_8088_45b5_9975_064014026c42"/>
  </rdf:Description>
  <rdf:Description rdf:nodeID="Na8c55743a2f94e37b88871439eaaa730">
    <owl:onProperty rdf:resource="http://emmo.info/emmo/middle/perceptual#EMMO_23b579e1_8088_45b5_9975_064014026c42"/>
    <rdf:type rdf:resource="http://www.w3.org/2002/07/owl#Restriction"/>
    <owl:hasValue>Pa</owl:hasValue>
  </rdf:Description>
  <rdf:Description rdf:nodeID="Nf649fb5878374c29a1571007e6418b74">
    <owl:onProperty rdf:resource="http://emmo.info/emmo/middle/perceptual#EMMO_23b579e1_8088_45b5_9975_064014026c42"/>
    <owl:hasValue>T-2 L0 M+1 I-1 Θ0 N0 J0</owl:hasValue>
    <rdf:type rdf:resource="http://www.w3.org/2002/07/owl#Restriction"/>
  </rdf:Description>
  <rdf:Description rdf:nodeID="Nb7d3e37eb92f4940aac2fa6794e88137">
    <rdf:first rdf:resource="http://emmo.info/emmo/middle/siunits#EMMO_f96feb3f_4438_4e43_aa44_7458c4d87fc2"/>
    <rdf:rest rdf:nodeID="Nde0627e70a0740ca9eacc8c3fcf9b4a1"/>
  </rdf:Description>
  <rdf:Description rdf:nodeID="Nfdc465a91c05463cb6fb6b5925745208">
    <rdf:first rdf:resource="http://emmo.info/emmo/top/semiotics#EMMO_6f5af708_f825_4feb_a0d1_a8d813d3022b"/>
    <rdf:rest rdf:nodeID="Nec607c9ad5ba47f796aa9ad684514c83"/>
  </rdf:Description>
  <rdf:Description rdf:nodeID="N1a4d39d7416b45629abd39ca251a070a">
    <rdf:rest rdf:nodeID="N38aa7521440f4db7acd60bdaa143a0f8"/>
    <rdf:first rdf:resource="http://emmo.info/emmo/middle/physicalistic#EMMO_5b2222df_4da6_442f_8244_96e9e45887d1"/>
  </rdf:Description>
  <rdf:Description rdf:about="http://emmo.info/emmo/middle/siunits#EMMO_60b78cc3_6011_4134_95ab_956f56d4bdc1">
    <rdfs:label xml:lang="en">SINonCoherentDerivedUnit</rdfs:label>
    <annotations:EMMO_967080e5_2f42_4eb2_a3a9_c58143e835f9>A derived unit whos numerical factor in front of the product of base units is NOT equal to one.</annotations:EMMO_967080e5_2f42_4eb2_a3a9_c58143e835f9>
    <rdf:type rdf:resource="http://www.w3.org/2002/07/owl#Class"/>
  </rdf:Description>
  <rdf:Description rdf:nodeID="Nb2af1735e9ef4376b8a35234c9e20cc8">
    <owl:qualifiedCardinality rdf:datatype="http://www.w3.org/2001/XMLSchema#nonNegativeInteger">1</owl:qualifiedCardinality>
    <owl:onDataRange rdf:resource="http://www.w3.org/2001/XMLSchema#double"/>
    <owl:onProperty rdf:resource="http://emmo.info/emmo/middle/math#EMMO_faf79f53_749d_40b2_807c_d34244c192f4"/>
    <rdf:type rdf:resource="http://www.w3.org/2002/07/owl#Restriction"/>
  </rdf:Description>
  <rdf:Description rdf:about="http://emmo.info/emmo/middle/siunits#EMMO_254472c6_3dbd_4f02_bc43_571389cd281f">
    <rdfs:label xml:lang="en">Zepto</rdfs:label>
    <rdfs:subClassOf rdf:nodeID="N11fd8522000d4edea489c10cdaa024a1"/>
    <rdf:type rdf:resource="http://www.w3.org/2002/07/owl#Class"/>
    <rdfs:subClassOf rdf:nodeID="Nb14bc769d574461bb3801212c118898b"/>
  </rdf:Description>
  <rdf:Description rdf:about="http://emmo.info/emmo/middle/isq#EMMO_2946d40b_24a1_47fa_8176_e3f79bb45064">
    <annotations:EMMO_967080e5_2f42_4eb2_a3a9_c58143e835f9>Derived quantities defined in the International System of Quantities (ISQ).</annotations:EMMO_967080e5_2f42_4eb2_a3a9_c58143e835f9>
    <rdfs:label xml:lang="en">ISQDerivedQuantity</rdfs:label>
    <rdfs:subClassOf rdf:resource="http://emmo.info/emmo/middle/isq#EMMO_f35cff4d_dc09_44cf_a729_22fb79e3bfb2"/>
    <rdf:type rdf:resource="http://www.w3.org/2002/07/owl#Class"/>
    <rdfs:subClassOf rdf:resource="http://emmo.info/emmo/middle/metrology#EMMO_71f6ab56_342c_484b_bbe0_de86b7367cb3"/>
  </rdf:Description>
  <rdf:Description rdf:about="http://emmo.info/emmo/middle/math#EMMO_54dc83cb_06e1_4739_9e45_bc09cead7f48">
    <rdfs:subClassOf rdf:resource="http://emmo.info/emmo/middle/math#EMMO_21f56795_ee72_4858_b571_11cfaa59c1a8"/>
    <rdfs:subClassOf rdf:nodeID="N1ac9d330ad7442f998e7e63304a1e6a2"/>
    <rdfs:subClassOf rdf:nodeID="N0f93456af1aa461490eca66aad531639"/>
    <rdfs:label xml:lang="en">Boolean</rdfs:label>
    <owl:equivalentClass rdf:nodeID="N4df09dabedf6443cb8a33c1f330f3c25"/>
    <rdf:type rdf:resource="http://www.w3.org/2002/07/owl#Class"/>
  </rdf:Description>
  <rdf:Description rdf:about="http://emmo.info/emmo/middle/siunits#EMMO_8a70dea4_d6ab_4260_b931_a3e990982416">
    <annotations:EMMO_fe015383_afb3_44a6_ae86_043628697aa2>https://doi.org/10.1351/goldbook.J03363</annotations:EMMO_fe015383_afb3_44a6_ae86_043628697aa2>
    <annotations:EMMO_1f1b164d_ec6a_4faa_8d5e_88bda62316cc>http://qudt.org/vocab/unit/J</annotations:EMMO_1f1b164d_ec6a_4faa_8d5e_88bda62316cc>
    <rdfs:label xml:lang="en">Joule</rdfs:label>
    <rdf:type rdf:resource="http://www.w3.org/2002/07/owl#Class"/>
    <rdfs:comment>Measurement unit for energy.</rdfs:comment>
    <rdfs:subClassOf rdf:nodeID="N20ec5135479b44859752f926614bf2e7"/>
    <rdfs:subClassOf rdf:nodeID="N42ded023e7ca40b59a22fc91efc4012c"/>
  </rdf:Description>
  <rdf:Description rdf:about="http://emmo.info/emmo/middle/siunits#EMMO_43a6b269_da31_4bb6_a537_c97df4fff32a">
    <rdfs:subClassOf rdf:nodeID="N0971065b3b794a4da4f1654c490879e2"/>
    <rdf:type rdf:resource="http://www.w3.org/2002/07/owl#Class"/>
    <rdfs:subClassOf rdf:nodeID="N18399958eec24e5c94ae1a83c929e246"/>
    <rdfs:label xml:lang="en">Peta</rdfs:label>
  </rdf:Description>
  <rdf:Description rdf:about="http://emmo.info/emmo/middle/siunits#EMMO_a80dc6f5_b1aa_41a7_a3a8_cd5040da2162">
    <rdfs:subClassOf rdf:nodeID="Na8c55743a2f94e37b88871439eaaa730"/>
    <rdfs:label xml:lang="en">Pascal</rdfs:label>
    <annotations:EMMO_1f1b164d_ec6a_4faa_8d5e_88bda62316cc>http://qudt.org/vocab/unit/PA</annotations:EMMO_1f1b164d_ec6a_4faa_8d5e_88bda62316cc>
    <rdfs:subClassOf rdf:nodeID="N7c11a63c339c490dad923110a2b30f19"/>
    <rdfs:comment>Measurement unit for pressure.</rdfs:comment>
    <rdf:type rdf:resource="http://www.w3.org/2002/07/owl#Class"/>
    <annotations:EMMO_fe015383_afb3_44a6_ae86_043628697aa2>https://doi.org/10.1351/goldbook.P04442</annotations:EMMO_fe015383_afb3_44a6_ae86_043628697aa2>
  </rdf:Description>
  <rdf:Description rdf:about="http://emmo.info/emmo/middle/perceptual#EMMO_1da53c06_9577_4008_8652_272fa3b62be7">
    <rdf:type rdf:resource="http://www.w3.org/2002/07/owl#Class"/>
    <rdfs:subClassOf rdf:resource="http://emmo.info/emmo/middle/perceptual#EMMO_c74da218_9147_4f03_92d1_8894abca55f3"/>
    <annotations:EMMO_b432d2d5_25f4_4165_99c5_5935a7763c1a>A drawing of a cat.
A circle on a paper sheet.
The Mona Lisa.</annotations:EMMO_b432d2d5_25f4_4165_99c5_5935a7763c1a>
    <annotations:EMMO_967080e5_2f42_4eb2_a3a9_c58143e835f9>A 'Graphical' that stands for a real world object that shows a recognizable pictorial pattern without being necessarily associated to a symbolic language.</annotations:EMMO_967080e5_2f42_4eb2_a3a9_c58143e835f9>
    <rdfs:label xml:lang="en">Pictorial</rdfs:label>
  </rdf:Description>
  <rdf:Description rdf:nodeID="Nce6bc7ace0de4e30b405b420c47ce199">
    <owl:hasValue>T0 L0 M0 I0 Θ0 N+1 J0</owl:hasValue>
    <rdf:type rdf:resource="http://www.w3.org/2002/07/owl#Restriction"/>
    <owl:onProperty rdf:resource="http://emmo.info/emmo/middle/perceptual#EMMO_23b579e1_8088_45b5_9975_064014026c42"/>
  </rdf:Description>
  <rdf:Description rdf:about="http://emmo.info/emmo/middle/isq#EMMO_668e6ead_1530_40cc_ad5e_24b880edff50">
    <owl:equivalentClass rdf:nodeID="Nacf41bf2497242d9850f79fdacee6e73"/>
    <rdfs:label xml:lang="en">LuminousIntensityPerSquareLengthDimension</rdfs:label>
    <rdfs:subClassOf rdf:resource="http://emmo.info/emmo/middle/metrology#EMMO_9895a1b4_f0a5_4167_ac5e_97db40b8bfcc"/>
    <rdf:type rdf:resource="http://www.w3.org/2002/07/owl#Class"/>
  </rdf:Description>
  <rdf:Description rdf:nodeID="N94a7d318c4e844e89241126779f3fbe2">
    <rdf:type rdf:resource="http://www.w3.org/2002/07/owl#Class"/>
    <owl:complementOf rdf:resource="http://emmo.info/emmo/middle/physicalistic#EMMO_5b2222df_4da6_442f_8244_96e9e45887d1"/>
  </rdf:Description>
  <rdf:Description rdf:nodeID="N823d279887034df9abd7eb10be4b0aaa">
    <owl:onProperty rdf:resource="http://emmo.info/emmo/middle/metrology#EMMO_67fc0a36_8dcb_4ffa_9a43_31074efa3296"/>
    <rdf:type rdf:resource="http://www.w3.org/2002/07/owl#Restriction"/>
    <owl:allValuesFrom rdf:nodeID="N2fed5de597924a3cb99c15593a51c377"/>
  </rdf:Description>
  <rdf:Description rdf:nodeID="Na1f65ae8236c4cc7b8892b086a1f9b8d">
    <owl:hasValue>T-2 L+1 M+1 I0 Θ0 N0 J0</owl:hasValue>
    <owl:onProperty rdf:resource="http://emmo.info/emmo/middle/perceptual#EMMO_23b579e1_8088_45b5_9975_064014026c42"/>
    <rdf:type rdf:resource="http://www.w3.org/2002/07/owl#Restriction"/>
  </rdf:Description>
  <rdf:Description rdf:about="http://emmo.info/emmo/middle/siunits#EMMO_feb03a8a_bbb6_4918_a891_46713ef557f4">
    <owl:disjointUnionOf rdf:nodeID="N4813a2ce167a4fad9b05d9a83354e42e"/>
    <rdfs:subClassOf rdf:resource="http://emmo.info/emmo/middle/metrology#EMMO_b081b346_7279_46ef_9a3d_2c088fcd79f4"/>
    <annotations:EMMO_967080e5_2f42_4eb2_a3a9_c58143e835f9>The set of units provided by the SI referring to the ISQ.</annotations:EMMO_967080e5_2f42_4eb2_a3a9_c58143e835f9>
    <rdfs:comment>The complete set of SI units includes both the coherent set and the multiples and sub-multiples formed by using the SI prefixes.</rdfs:comment>
    <rdf:type rdf:resource="http://www.w3.org/2002/07/owl#Class"/>
    <rdfs:label xml:lang="en">SIUnit</rdfs:label>
  </rdf:Description>
  <rdf:Description rdf:nodeID="N7ed24cb7d5db4203b056bbf73487120c">
    <rdf:rest rdf:nodeID="N8edc1101dbee4e7b82b49904ab6080bd"/>
    <rdf:first rdf:resource="http://emmo.info/emmo/middle/siunits#EMMO_3a185e6c_9e19_4776_b583_19c978156aa0"/>
  </rdf:Description>
  <rdf:Description rdf:nodeID="N304074c25c334c0380d380ef9551e3d7">
    <rdf:rest rdf:nodeID="Nd10ca18d7e7549b597060c6d52aa49e0"/>
    <rdf:first rdf:resource="http://emmo.info/emmo/middle/properties#EMMO_d0200cf1_e4f4_45ae_873f_b9359daea3cd"/>
  </rdf:Description>
  <rdf:Description rdf:nodeID="N04cf64912ef24e438c58c2026c440620">
    <owl:onClass rdf:resource="http://emmo.info/emmo/middle/metrology#EMMO_216f448e_cdbc_4aeb_a529_7a5fe7fc38bb"/>
    <rdf:type rdf:resource="http://www.w3.org/2002/07/owl#Restriction"/>
    <owl:onProperty rdf:resource="http://emmo.info/emmo/middle/reductionistic#EMMO_b2282816_b7a3_44c6_b2cb_3feff1ceb7fe"/>
    <owl:qualifiedCardinality rdf:datatype="http://www.w3.org/2001/XMLSchema#nonNegativeInteger">1</owl:qualifiedCardinality>
  </rdf:Description>
  <rdf:Description rdf:about="http://emmo.info/emmo/middle/metrology#EMMO_c9c8f824_9127_4f93_bc21_69fe78a7f6f2">
    <rdf:type rdf:resource="http://www.w3.org/2002/07/owl#Class"/>
    <rdfs:label xml:lang="en">ProcedureUnit</rdfs:label>
    <annotations:EMMO_b432d2d5_25f4_4165_99c5_5935a7763c1a>Rockwell C hardness of a given sample (150 kg load): 43.5HRC(150 kg)</annotations:EMMO_b432d2d5_25f4_4165_99c5_5935a7763c1a>
    <annotations:EMMO_967080e5_2f42_4eb2_a3a9_c58143e835f9>A reference unit provided by a measurement procedure.</annotations:EMMO_967080e5_2f42_4eb2_a3a9_c58143e835f9>
    <rdfs:subClassOf rdf:resource="http://emmo.info/emmo/middle/metrology#EMMO_18ce5200_00f5_45bb_8c6f_6fb128cd41ae"/>
  </rdf:Description>
  <rdf:Description rdf:about="http://emmo.info/emmo/middle/models#EMMO_24c71baf_6db6_48b9_86c8_8c70cf36db0c">
    <rdfs:label xml:lang="en">hasModel</rdfs:label>
    <rdf:type rdf:resource="http://www.w3.org/2002/07/owl#ObjectProperty"/>
    <rdfs:subPropertyOf rdf:resource="http://emmo.info/emmo/top/semiotics#EMMO_39c3815d_8cae_4c8f_b2ff_eeba24bec455"/>
  </rdf:Description>
  <rdf:Description rdf:nodeID="N86d8e86ed44243928b494dd9be8446ad">
    <owl:someValuesFrom rdf:resource="http://emmo.info/emmo/middle/models#EMMO_e5438930_04e7_4d42_ade5_3700d4a52ab7"/>
    <rdf:type rdf:resource="http://www.w3.org/2002/07/owl#Restriction"/>
    <owl:onProperty rdf:resource="http://emmo.info/emmo/top/physical#EMMO_f68030be_94b8_4c61_a161_886468558054"/>
  </rdf:Description>
  <rdf:Description rdf:about="http://emmo.info/emmo/top/math#EMMO_f8a2fe9f_458b_4771_9aba_a50e76afc52d">
    <rdf:type rdf:resource="http://www.w3.org/2002/07/owl#Class"/>
    <rdfs:subClassOf rdf:resource="http://emmo.info/emmo/top/math#EMMO_f6d0c26a_98b6_4cf8_8632_aa259131faaa"/>
    <rdfs:label xml:lang="en">DifferentialOperator</rdfs:label>
  </rdf:Description>
  <rdf:Description rdf:nodeID="Nfe364a4a656042d1ad8b65e5d94e000e">
    <owl:allValuesFrom rdf:resource="http://emmo.info/emmo/middle/math#EMMO_4ce76d7f_03f8_45b6_9003_90052a79bfaa"/>
    <rdf:type rdf:resource="http://www.w3.org/2002/07/owl#Restriction"/>
    <owl:onProperty rdf:nodeID="N6fb0d68dd5284ea5ab9bbd8ddf81d6ad"/>
  </rdf:Description>
  <rdf:Description rdf:nodeID="Nd134427b98f44841af80457a655f4706">
    <rdf:first rdf:resource="http://emmo.info/emmo/middle/perceptual#EMMO_a1083d0a_c1fb_471f_8e20_a98f881ad527"/>
    <rdf:rest rdf:resource="http://www.w3.org/1999/02/22-rdf-syntax-ns#nil"/>
  </rdf:Description>
  <rdf:Description rdf:about="http://emmo.info/emmo/middle/metrology#EMMO_db716151_6b73_45ff_910c_d182fdcbb4f5">
    <rdfs:label xml:lang="en">BaseUnit</rdfs:label>
    <annotations:EMMO_967080e5_2f42_4eb2_a3a9_c58143e835f9>A set of units that correspond to the base quantities in a system of units.</annotations:EMMO_967080e5_2f42_4eb2_a3a9_c58143e835f9>
    <rdf:type rdf:resource="http://www.w3.org/2002/07/owl#Class"/>
  </rdf:Description>
  <rdf:Description rdf:nodeID="N18399958eec24e5c94ae1a83c929e246">
    <rdf:type rdf:resource="http://www.w3.org/2002/07/owl#Restriction"/>
    <owl:onProperty rdf:nodeID="N5da36b9be6944d57b404c89ebc8659dc"/>
    <owl:allValuesFrom rdf:nodeID="Nce4eaa697a224bfc84e048824d47e88f"/>
  </rdf:Description>
  <rdf:Description rdf:about="http://emmo.info/emmo/top/semiotics#EMMO_39c3815d_8cae_4c8f_b2ff_eeba24bec455">
    <rdfs:label xml:lang="en">hasIcon</rdfs:label>
    <rdfs:range rdf:resource="http://emmo.info/emmo/top/semiotics#EMMO_d7788d1a_020d_4c78_85a1_13563fcec168"/>
    <rdfs:subPropertyOf rdf:resource="http://emmo.info/emmo/top/semiotics#EMMO_60577dea_9019_4537_ac41_80b0fb563d41"/>
    <rdf:type rdf:resource="http://www.w3.org/2002/07/owl#ObjectProperty"/>
  </rdf:Description>
  <rdf:Description rdf:nodeID="N744e3020c61b43b58a0de48d90f8907a">
    <owl:allValuesFrom rdf:nodeID="N1abbf6e8a44a480eb8030eaaa00b0514"/>
    <rdf:type rdf:resource="http://www.w3.org/2002/07/owl#Restriction"/>
    <owl:onProperty rdf:resource="http://emmo.info/emmo/middle/metrology#EMMO_67fc0a36_8dcb_4ffa_9a43_31074efa3296"/>
  </rdf:Description>
  <rdf:Description rdf:nodeID="N9b8f51a7caa9458e8c44f2c7773484b4">
    <owl:onProperty rdf:resource="http://emmo.info/emmo/middle/math#EMMO_faf79f53_749d_40b2_807c_d34244c192f4"/>
    <owl:hasValue rdf:datatype="http://www.w3.org/2001/XMLSchema#decimal">1E+1</owl:hasValue>
    <rdf:type rdf:resource="http://www.w3.org/2002/07/owl#Restriction"/>
  </rdf:Description>
  <rdf:Description rdf:nodeID="Ndae100846d6e4cb6941b45753b4e9b20">
    <owl:inverseOf rdf:resource="http://emmo.info/emmo/middle/holistic#EMMO_c5aae418_1622_4d02_93c5_21159e28e6c1"/>
  </rdf:Description>
  <rdf:Description rdf:nodeID="N3e86b38e50ed4085ab8f87fbad5078e5">
    <owl:inverseOf rdf:resource="http://emmo.info/emmo/middle/math#EMMO_3446e167_c576_49d6_846c_215bb8878a55"/>
  </rdf:Description>
  <rdf:Description rdf:about="http://emmo.info/emmo/top/semiotics#EMMO_7fb7fe7e_bdf9_4eeb_adad_e384dd5285c6">
    <rdfs:range rdf:resource="http://emmo.info/emmo/top/semiotics#EMMO_054af807_85cd_4a13_8eba_119dfdaaf38b"/>
    <rdfs:label xml:lang="en">hasInterpretant</rdfs:label>
    <rdf:type rdf:resource="http://www.w3.org/2002/07/owl#ObjectProperty"/>
    <rdfs:subPropertyOf rdf:resource="http://emmo.info/emmo/top/semiotics#EMMO_60577dea_9019_4537_ac41_80b0fb563d41"/>
  </rdf:Description>
  <rdf:Description rdf:nodeID="N8600a6e3a7b0475697ef103b6cf23966">
    <rdf:first rdf:resource="http://emmo.info/emmo/middle/metrology#EMMO_89762966_8076_4f7c_b745_f718d653e8e2"/>
    <rdf:rest rdf:resource="http://www.w3.org/1999/02/22-rdf-syntax-ns#nil"/>
  </rdf:Description>
  <rdf:Description rdf:nodeID="Nfbdae53e1a6340599ccb2416d1eccc4f">
    <owl:onProperty rdf:resource="http://emmo.info/emmo/middle/perceptual#EMMO_23b579e1_8088_45b5_9975_064014026c42"/>
    <owl:hasValue>a</owl:hasValue>
    <rdf:type rdf:resource="http://www.w3.org/2002/07/owl#Restriction"/>
  </rdf:Description>
  <rdf:Description rdf:nodeID="N8ef01c4e371b44518bad4d177fc0f8ce">
    <rdf:type rdf:resource="http://www.w3.org/2002/07/owl#Class"/>
    <owl:unionOf rdf:nodeID="N148cdca1920c4102abc3d0f93b7d1890"/>
  </rdf:Description>
  <rdf:Description rdf:nodeID="N2566f62ad78643b8bbe22a46dcf724aa">
    <owl:onProperty rdf:resource="http://emmo.info/emmo/middle/perceptual#EMMO_23b579e1_8088_45b5_9975_064014026c42"/>
    <owl:hasValue>Bq</owl:hasValue>
    <rdf:type rdf:resource="http://www.w3.org/2002/07/owl#Restriction"/>
  </rdf:Description>
  <rdf:Description rdf:nodeID="Nfc58ea532d114626852e2b76b3ef8633">
    <owl:onClass rdf:resource="http://emmo.info/emmo/middle/metrology#EMMO_7d2afa66_ae9e_4095_a9bf_421d0be401b6"/>
    <rdf:type rdf:resource="http://www.w3.org/2002/07/owl#Restriction"/>
    <owl:onProperty rdf:resource="http://emmo.info/emmo/middle/reductionistic#EMMO_b2282816_b7a3_44c6_b2cb_3feff1ceb7fe"/>
    <owl:qualifiedCardinality rdf:datatype="http://www.w3.org/2001/XMLSchema#nonNegativeInteger">1</owl:qualifiedCardinality>
  </rdf:Description>
  <rdf:Description rdf:nodeID="Nf5744475d19e4ce89c64ead1e8fff672">
    <rdf:type rdf:resource="http://www.w3.org/2002/07/owl#Restriction"/>
    <owl:allValuesFrom rdf:resource="http://emmo.info/emmo/middle/physicalistic#EMMO_5b2222df_4da6_442f_8244_96e9e45887d1"/>
    <owl:onProperty rdf:nodeID="Na21084a7a3ad45dcb121e646436cff95"/>
  </rdf:Description>
  <rdf:Description rdf:nodeID="Na8a0e41b89d643fa8412aadd995f0740">
    <owl:onProperty rdf:resource="http://emmo.info/emmo/middle/math#EMMO_faf79f53_749d_40b2_807c_d34244c192f4"/>
    <rdf:type rdf:resource="http://www.w3.org/2002/07/owl#Restriction"/>
    <owl:hasValue rdf:datatype="http://www.w3.org/2001/XMLSchema#decimal">1E+2</owl:hasValue>
  </rdf:Description>
  <rdf:Description rdf:nodeID="N549d45829d5d485291a666a9c86bd1c3">
    <owl:allValuesFrom rdf:nodeID="Nd33f7cbb853c4818be8efc5da9a9e643"/>
    <owl:onProperty rdf:resource="http://emmo.info/emmo/middle/metrology#EMMO_67fc0a36_8dcb_4ffa_9a43_31074efa3296"/>
    <rdf:type rdf:resource="http://www.w3.org/2002/07/owl#Restriction"/>
  </rdf:Description>
  <rdf:Description rdf:about="http://emmo.info/emmo/middle/metrology#EMMO_3ee80521_3c23_4dd1_935d_9d522614a3e2">
    <annotations:EMMO_967080e5_2f42_4eb2_a3a9_c58143e835f9>A unit symbol that stands for a derived unit.</annotations:EMMO_967080e5_2f42_4eb2_a3a9_c58143e835f9>
    <rdfs:comment>Special units are semiotic shortcuts to more complex composed symbolic objects.</rdfs:comment>
    <rdfs:subClassOf rdf:nodeID="N5374912c996f41b5987bf12d041197af"/>
    <rdf:type rdf:resource="http://www.w3.org/2002/07/owl#Class"/>
    <annotations:EMMO_b432d2d5_25f4_4165_99c5_5935a7763c1a>Pa stands for N/m2
J stands for N m</annotations:EMMO_b432d2d5_25f4_4165_99c5_5935a7763c1a>
    <rdfs:subClassOf rdf:resource="http://emmo.info/emmo/middle/metrology#EMMO_08b308d4_31cd_4779_a784_aa92fc730f39"/>
    <rdfs:label xml:lang="en">SpecialUnit</rdfs:label>
  </rdf:Description>
  <rdf:Description rdf:about="http://emmo.info/emmo/middle/metrology#EMMO_18ce5200_00f5_45bb_8c6f_6fb128cd41ae">
    <rdfs:subClassOf rdf:resource="http://emmo.info/emmo/middle/metrology#EMMO_985bec21_989f_4b9e_a4b3_735d88099c3c"/>
    <rdf:type rdf:resource="http://www.w3.org/2002/07/owl#Class"/>
    <rdfs:comment>A symbolic is recognized as reference unit also if it is not part of a quatity (e.g. as in the sentence "the Bq is the reference unit of Becquerel").

For this reason we can't declare the axiom:
ReferenceUnit SubClassOf: inverse(hasReferenceUnit) some Quantity
because there exist reference units without being part of a quantity.

This is peculiar to EMMO, where quantities (symbolic) are distinct with properties (semiotics).</rdfs:comment>
    <rdfs:comment>A reference can be a measurement unit, a measurement procedure, a reference material, or a combination of such.
International vocabulary of metrology (VIM)</rdfs:comment>
    <rdfs:label xml:lang="en">ReferenceUnit</rdfs:label>
  </rdf:Description>
  <rdf:Description rdf:nodeID="N0bd75e9d4e1c4ab5a6ff6dd1d346df36">
    <rdf:type rdf:resource="http://www.w3.org/2002/07/owl#Restriction"/>
    <owl:onProperty rdf:resource="http://emmo.info/emmo/middle/perceptual#EMMO_23b579e1_8088_45b5_9975_064014026c42"/>
    <owl:hasValue>T-1 L0 M0 I0 Θ0 N+1 J0</owl:hasValue>
  </rdf:Description>
  <rdf:Description rdf:nodeID="Na2312bf9f09c4e308589b2dc84aae0c4">
    <rdf:rest rdf:nodeID="N9b695051987d46818c57eb0927d1fedc"/>
    <rdf:first rdf:resource="http://emmo.info/emmo/middle/isq#EMMO_8159c26a_494b_4fa0_9959_10888f152298"/>
  </rdf:Description>
  <rdf:Description rdf:about="http://emmo.info/emmo/middle/siunits#EMMO_5cf9f86c_86f5_40c4_846d_60371f670e0a">
    <rdfs:label xml:lang="en">Exa</rdfs:label>
    <rdfs:subClassOf rdf:nodeID="N638209463e98453c8e3c24a70cbe93f0"/>
    <rdfs:subClassOf rdf:nodeID="N2d731ca68f11455abd050ffb201de6da"/>
    <rdf:type rdf:resource="http://www.w3.org/2002/07/owl#Class"/>
  </rdf:Description>
  <rdf:Description rdf:nodeID="Nf63fa94031ad483aa6692eb5df5b3cd6">
    <rdf:type rdf:resource="http://www.w3.org/2002/07/owl#Restriction"/>
    <owl:hasValue>°C</owl:hasValue>
    <owl:onProperty rdf:resource="http://emmo.info/emmo/middle/perceptual#EMMO_23b579e1_8088_45b5_9975_064014026c42"/>
  </rdf:Description>
  <rdf:Description rdf:about="http://emmo.info/emmo/middle/properties#EMMO_909415d1_7c43_4d5e_bbeb_7e1910159f66">
    <rdfs:subClassOf rdf:resource="http://emmo.info/emmo/middle/properties#EMMO_2a888cdf_ec4a_4ec5_af1c_0343372fc978"/>
    <rdfs:label xml:lang="en">NominalProperty</rdfs:label>
    <annotations:EMMO_967080e5_2f42_4eb2_a3a9_c58143e835f9>An 'ObjectiveProperty' that cannot be quantified.</annotations:EMMO_967080e5_2f42_4eb2_a3a9_c58143e835f9>
    <annotations:EMMO_b432d2d5_25f4_4165_99c5_5935a7763c1a>CFC is a 'sign' that stands for the fact that the morphology of atoms composing the microstructure of an entity is predominantly Cubic Face Centered

A color is a nominal property.

Sex of a human being.</annotations:EMMO_b432d2d5_25f4_4165_99c5_5935a7763c1a>
    <rdf:type rdf:resource="http://www.w3.org/2002/07/owl#Class"/>
    <rdfs:comment>"Property of a phenomenon, body, or substance, where the property has no magnitude."

"A nominal property has a value, which can be expressed in words, by alphanumerical codes, or by other means."

International vocabulary of metrology (VIM)</rdfs:comment>
  </rdf:Description>
  <rdf:Description rdf:nodeID="N1a7f191841c646a88bdd4b34fdf1b2f4">
    <rdf:type rdf:resource="http://www.w3.org/2002/07/owl#Restriction"/>
    <owl:onProperty rdf:resource="http://emmo.info/emmo/middle/metrology#EMMO_bed1d005_b04e_4a90_94cf_02bc678a8569"/>
    <owl:someValuesFrom rdf:resource="http://emmo.info/emmo/middle/isq#EMMO_14ff4393_0f28_4fb4_abc7_c2cc00bc761d"/>
  </rdf:Description>
  <rdf:Description rdf:about="http://emmo.info/emmo/middle/models#EMMO_db9a009e_f097_43f5_9520_6cbc07e7610b">
    <rdfs:label xml:lang="en">NaturalLaw</rdfs:label>
    <rdfs:subClassOf rdf:resource="http://emmo.info/emmo/middle/models#EMMO_8d2d9374_ef3a_47e6_8595_6bc208e07519"/>
    <rdf:type rdf:resource="http://www.w3.org/2002/07/owl#Class"/>
  </rdf:Description>
  <rdf:Description rdf:about="http://emmo.info/emmo/top/annotations#EMMO_70fe84ff_99b6_4206_a9fc_9a8931836d84">
    <rdfs:label xml:lang="en">definition</rdfs:label>
    <rdfs:subPropertyOf rdf:resource="http://www.w3.org/2000/01/rdf-schema#comment"/>
    <rdf:type rdf:resource="http://www.w3.org/2002/07/owl#AnnotationProperty"/>
  </rdf:Description>
  <rdf:Description rdf:about="http://emmo.info/emmo/middle/siunits#EMMO_314ba716_2d3d_4462_9a4f_d3419ae1df43">
    <annotations:EMMO_1f1b164d_ec6a_4faa_8d5e_88bda62316cc>http://qudt.org/vocab/unit/SEC</annotations:EMMO_1f1b164d_ec6a_4faa_8d5e_88bda62316cc>
    <rdfs:subClassOf rdf:nodeID="N7481cb046c3747dfb34030da3079ef27"/>
    <annotations:EMMO_70fe84ff_99b6_4206_a9fc_9a8931836d84>The second, symbol s, is the SI unit of time. It is defined by taking the fixed numerical value of the caesium frequency ∆νCs, the unperturbed ground-state hyperfine transition frequency of the caesium 133 atom, to be 9192631770 when expressed in the unit Hz, which is equal to s−1.</annotations:EMMO_70fe84ff_99b6_4206_a9fc_9a8931836d84>
    <rdfs:subClassOf rdf:nodeID="N441d88bdb30846aca2895751b79d62c6"/>
    <rdf:type rdf:resource="http://www.w3.org/2002/07/owl#Class"/>
    <annotations:EMMO_fe015383_afb3_44a6_ae86_043628697aa2>https://doi.org/10.1351/goldbook.S05513</annotations:EMMO_fe015383_afb3_44a6_ae86_043628697aa2>
    <rdfs:label xml:lang="en">Second</rdfs:label>
  </rdf:Description>
  <rdf:Description rdf:nodeID="N7f64302e647b413582a109c14ca032b2">
    <rdf:type rdf:resource="http://www.w3.org/2002/07/owl#Restriction"/>
    <owl:onProperty rdf:resource="http://emmo.info/emmo/middle/metrology#EMMO_bed1d005_b04e_4a90_94cf_02bc678a8569"/>
    <owl:allValuesFrom rdf:resource="http://emmo.info/emmo/middle/isq#EMMO_14ff4393_0f28_4fb4_abc7_c2cc00bc761d"/>
  </rdf:Description>
  <rdf:Description rdf:nodeID="N69233c4d75eb4c908d964a7ec5d39ffa">
    <owl:onProperty rdf:resource="http://emmo.info/emmo/middle/perceptual#EMMO_23b579e1_8088_45b5_9975_064014026c42"/>
    <owl:hasValue>y</owl:hasValue>
    <rdf:type rdf:resource="http://www.w3.org/2002/07/owl#Restriction"/>
  </rdf:Description>
  <rdf:Description rdf:nodeID="N4f6455f2d9ff4404be2e63ed1f6f0010">
    <owl:hasValue rdf:datatype="http://www.w3.org/2001/XMLSchema#decimal">1E-12</owl:hasValue>
    <owl:onProperty rdf:resource="http://emmo.info/emmo/middle/math#EMMO_faf79f53_749d_40b2_807c_d34244c192f4"/>
    <rdf:type rdf:resource="http://www.w3.org/2002/07/owl#Restriction"/>
  </rdf:Description>
  <rdf:Description rdf:nodeID="Nc7c090151e8c4a91a8f81dc470851dbc">
    <owl:onProperty rdf:nodeID="N833f6194797f4d0cb00dcf9f9e000217"/>
    <rdf:type rdf:resource="http://www.w3.org/2002/07/owl#Restriction"/>
    <owl:allValuesFrom rdf:nodeID="Nffeda470672d4275846249acfcc43ddd"/>
  </rdf:Description>
  <rdf:Description rdf:about="http://emmo.info/emmo/middle/perceptual#EMMO_b2a234a8_579a_422c_9305_b8f7e72c76cd">
    <rdfs:label xml:lang="en">Circle</rdfs:label>
    <rdfs:subClassOf rdf:resource="http://emmo.info/emmo/middle/perceptual#EMMO_0c576e13_4ee7_4f3d_bfe9_1614243df018"/>
    <rdf:type rdf:resource="http://www.w3.org/2002/07/owl#Class"/>
  </rdf:Description>
  <rdf:Description rdf:nodeID="Ndf57d92015fc4650bdd5b0224e0343d3">
    <owl:someValuesFrom rdf:resource="http://emmo.info/emmo/middle/isq#EMMO_3227b821_26a5_4c7c_9c01_5c24483e0bd0"/>
    <rdf:type rdf:resource="http://www.w3.org/2002/07/owl#Restriction"/>
    <owl:onProperty rdf:resource="http://emmo.info/emmo/middle/metrology#EMMO_bed1d005_b04e_4a90_94cf_02bc678a8569"/>
  </rdf:Description>
  <rdf:Description rdf:about="http://emmo.info/emmo/middle/isq#EMMO_77e9dc31_5b19_463e_b000_44c6e79f98aa">
    <rdfs:label xml:lang="en">MassDimension</rdfs:label>
    <rdf:type rdf:resource="http://www.w3.org/2002/07/owl#Class"/>
    <owl:equivalentClass rdf:nodeID="Nb2f58bc99e874d7db3d015349db25510"/>
    <rdfs:subClassOf rdf:resource="http://emmo.info/emmo/middle/metrology#EMMO_9895a1b4_f0a5_4167_ac5e_97db40b8bfcc"/>
  </rdf:Description>
  <rdf:Description rdf:nodeID="N8f5e55d1dca4417e8a37c924a4738815">
    <rdf:type rdf:resource="http://www.w3.org/2002/07/owl#Restriction"/>
    <owl:onProperty rdf:resource="http://emmo.info/emmo/middle/metrology#EMMO_bed1d005_b04e_4a90_94cf_02bc678a8569"/>
    <owl:someValuesFrom rdf:resource="http://emmo.info/emmo/middle/isq#EMMO_53e825d9_1a09_483c_baa7_37501ebfbe1c"/>
  </rdf:Description>
  <rdf:Description rdf:about="http://emmo.info/emmo/top/physical#EMMO_29072ec4_ffcb_42fb_bdc7_26f05a2e9873">
    <rdfs:comment>From Latin vacuus, “empty”.</rdfs:comment>
    <rdfs:label xml:lang="en">Void</rdfs:label>
    <rdf:type rdf:resource="http://www.w3.org/2002/07/owl#Class"/>
    <rdfs:subClassOf rdf:nodeID="Naa6daa84dcd04b9796c42086483a0e50"/>
    <annotations:EMMO_967080e5_2f42_4eb2_a3a9_c58143e835f9>A 'Item' that has no 'Physical' parts.</annotations:EMMO_967080e5_2f42_4eb2_a3a9_c58143e835f9>
  </rdf:Description>
  <rdf:Description rdf:about="http://emmo.info/emmo/middle/perceptual#EMMO_86060335_31c2_4820_b433_27c64aea0366">
    <rdfs:label xml:lang="en">Torus</rdfs:label>
    <rdfs:subClassOf rdf:resource="http://emmo.info/emmo/middle/perceptual#EMMO_9268958f_7f54_48ab_a693_febe2645892b"/>
    <rdf:type rdf:resource="http://www.w3.org/2002/07/owl#Class"/>
  </rdf:Description>
  <rdf:Description rdf:about="http://emmo.info/emmo/top/mereotopology#EMMO_517dfaf9_4970_41ac_81ee_d031627d2c7c">
    <rdf:type rdf:resource="http://www.w3.org/2002/07/owl#SymmetricProperty"/>
    <rdf:type rdf:resource="http://www.w3.org/2002/07/owl#ObjectProperty"/>
    <rdfs:subPropertyOf rdf:resource="http://emmo.info/emmo/top/mereotopology#EMMO_03212fd7_abfd_4828_9c8e_62c293052d4b"/>
    <rdfs:label xml:lang="en">disconnected</rdfs:label>
  </rdf:Description>
  <rdf:Description rdf:about="http://emmo.info/emmo/top/mereotopology#EMMO_4d6504f1_c470_4ce9_b941_bbbebc9ab05d">
    <rdfs:subPropertyOf rdf:resource="http://emmo.info/emmo/top/mereotopology#EMMO_6703954e_34c4_4a15_a9e7_f313760ae1a8"/>
    <rdfs:label xml:lang="en">hasContactWith</rdfs:label>
    <rdf:type rdf:resource="http://www.w3.org/2002/07/owl#ObjectProperty"/>
    <rdf:type rdf:resource="http://www.w3.org/2002/07/owl#SymmetricProperty"/>
  </rdf:Description>
  <rdf:Description rdf:nodeID="N07aaafec469d490983de40b7e7d2f87a">
    <owl:hasValue>G</owl:hasValue>
    <rdf:type rdf:resource="http://www.w3.org/2002/07/owl#Restriction"/>
    <owl:onProperty rdf:resource="http://emmo.info/emmo/middle/perceptual#EMMO_23b579e1_8088_45b5_9975_064014026c42"/>
  </rdf:Description>
  <rdf:Description rdf:about="http://emmo.info/emmo/middle/physicalistic#EMMO_7db59e56_f68b_48b7_ae99_891c35ae5c3b">
    <rdf:type rdf:resource="http://www.w3.org/2002/07/owl#Class"/>
    <rdfs:label xml:lang="en">Gluon</rdfs:label>
    <rdfs:subClassOf rdf:resource="http://emmo.info/emmo/top/physical#EMMO_0f795e3e_c602_4577_9a43_d5a231aa1360"/>
    <annotations:EMMO_967080e5_2f42_4eb2_a3a9_c58143e835f9>The class of individuals that stand for gluons elementary particles.</annotations:EMMO_967080e5_2f42_4eb2_a3a9_c58143e835f9>
  </rdf:Description>
  <rdf:Description rdf:nodeID="N4ef06d575a124cfba3f4b2cf2f4c4b66">
    <owl:allValuesFrom rdf:resource="http://emmo.info/emmo/middle/isq#EMMO_d5f3e0e5_fc7d_4e64_86ad_555e74aaff84"/>
    <rdf:type rdf:resource="http://www.w3.org/2002/07/owl#Restriction"/>
    <owl:onProperty rdf:resource="http://emmo.info/emmo/middle/metrology#EMMO_bed1d005_b04e_4a90_94cf_02bc678a8569"/>
  </rdf:Description>
  <rdf:Description rdf:nodeID="N1a018e65b5eb493d86feaf9ea984a50e">
    <owl:hasValue>*</owl:hasValue>
    <owl:onProperty rdf:resource="http://emmo.info/emmo/middle/perceptual#EMMO_23b579e1_8088_45b5_9975_064014026c42"/>
    <rdf:type rdf:resource="http://www.w3.org/2002/07/owl#Restriction"/>
  </rdf:Description>
  <rdf:Description rdf:nodeID="N073a4bd047ba4c05aa957f3e52261278">
    <owl:inverseOf rdf:resource="http://emmo.info/emmo/middle/math#EMMO_3446e167_c576_49d6_846c_215bb8878a55"/>
  </rdf:Description>
  <rdf:Description rdf:nodeID="Nf2164fae98574eaf8712de1fca89fa57">
    <rdf:type rdf:resource="http://www.w3.org/2002/07/owl#Restriction"/>
    <owl:onProperty rdf:resource="http://emmo.info/emmo/middle/metrology#EMMO_67fc0a36_8dcb_4ffa_9a43_31074efa3296"/>
    <owl:allValuesFrom rdf:nodeID="N4ef06d575a124cfba3f4b2cf2f4c4b66"/>
  </rdf:Description>
  <rdf:Description rdf:about="http://emmo.info/emmo/middle/metrology#EMMO_08b308d4_31cd_4779_a784_aa92fc730f39">
    <rdfs:label xml:lang="en">DerivedUnit</rdfs:label>
    <rdf:type rdf:resource="http://www.w3.org/2002/07/owl#Class"/>
    <annotations:EMMO_967080e5_2f42_4eb2_a3a9_c58143e835f9>Derived units are defined as products of powers of the base units corresponding to the relations defining the derived quantities in terms of the base quantities.</annotations:EMMO_967080e5_2f42_4eb2_a3a9_c58143e835f9>
  </rdf:Description>
  <rdf:Description rdf:about="http://emmo.info/emmo/middle/siunits#EMMO_d7f11b34_a121_4519_87c0_aa754f1c4737">
    <annotations:EMMO_1f1b164d_ec6a_4faa_8d5e_88bda62316cc>http://qudt.org/vocab/unit/WB</annotations:EMMO_1f1b164d_ec6a_4faa_8d5e_88bda62316cc>
    <annotations:EMMO_fe015383_afb3_44a6_ae86_043628697aa2>https://doi.org/10.1351/goldbook.W06666</annotations:EMMO_fe015383_afb3_44a6_ae86_043628697aa2>
    <rdfs:subClassOf rdf:nodeID="N153e5bc9c2094419a95345de81b62e76"/>
    <rdfs:comment>Measurement unit for magnetic flux.</rdfs:comment>
    <rdf:type rdf:resource="http://www.w3.org/2002/07/owl#Class"/>
    <rdfs:subClassOf rdf:nodeID="N487bcf892a4849d18369370a958d55ab"/>
    <rdfs:label xml:lang="en">Weber</rdfs:label>
  </rdf:Description>
  <rdf:Description rdf:nodeID="N46e75a7277184f459a11d75fb5b867d8">
    <rdf:type rdf:resource="http://www.w3.org/2002/07/owl#Restriction"/>
    <owl:onProperty rdf:resource="http://emmo.info/emmo/middle/metrology#EMMO_bed1d005_b04e_4a90_94cf_02bc678a8569"/>
    <owl:someValuesFrom rdf:resource="http://emmo.info/emmo/middle/isq#EMMO_b3600e73_3e05_479d_9714_c041c3acf5cc"/>
  </rdf:Description>
  <rdf:Description rdf:about="http://emmo.info/emmo/middle/siunits#EMMO_068c4e58_2470_4b1c_8454_010dd4906100">
    <rdfs:subClassOf rdf:nodeID="Nbf9fef1365ff4bd2a4e5b151d8fb28b8"/>
    <rdfs:subClassOf rdf:nodeID="N3b0b6b1778114e2db7c2eb96c28e114e"/>
    <rdf:type rdf:resource="http://www.w3.org/2002/07/owl#Class"/>
    <rdfs:label xml:lang="en">Pico</rdfs:label>
  </rdf:Description>
  <rdf:Description rdf:nodeID="N5e97a5fcfbd24a8caee9f70e38cb21cd">
    <rdf:first rdf:resource="http://emmo.info/emmo/middle/metrology#EMMO_868ae137_4d25_493e_b270_21ea3d94849e"/>
    <rdf:rest rdf:nodeID="N4a7ff59e579b46c5aa91826116306d20"/>
  </rdf:Description>
  <rdf:Description rdf:nodeID="Nfdee2fb24c934a58964e557deeda2282">
    <rdf:first rdf:resource="http://emmo.info/emmo/middle/isq#EMMO_ed4af7ae_63a2_497e_bb88_2309619ea405"/>
    <rdf:rest rdf:resource="http://www.w3.org/1999/02/22-rdf-syntax-ns#nil"/>
  </rdf:Description>
  <rdf:Description rdf:nodeID="Ndbf9693d60d842ef85f3dd7e11e7d3a8">
    <owl:hasValue rdf:datatype="http://www.w3.org/2001/XMLSchema#decimal">1E-21</owl:hasValue>
    <owl:onProperty rdf:resource="http://emmo.info/emmo/middle/math#EMMO_faf79f53_749d_40b2_807c_d34244c192f4"/>
    <rdf:type rdf:resource="http://www.w3.org/2002/07/owl#Restriction"/>
  </rdf:Description>
  <rdf:Description rdf:nodeID="Nba7f787f10714eecac73eadd22080156">
    <rdf:rest rdf:nodeID="N0e31abafffcf4d3c8fabe3f0d0d9c06f"/>
    <rdf:first rdf:resource="http://emmo.info/emmo/middle/siunits#EMMO_d41ce84b_4317_41fb_a5d1_6cd281fca106"/>
  </rdf:Description>
  <rdf:Description rdf:about="http://emmo.info/emmo/middle/metrology#EMMO_acd1a504_ca32_4f30_86ad_0b62cea5bc02">
    <rdfs:label xml:lang="en">StandardUnit</rdfs:label>
    <rdf:type rdf:resource="http://www.w3.org/2002/07/owl#Class"/>
    <rdfs:subClassOf rdf:resource="http://emmo.info/emmo/middle/metrology#EMMO_18ce5200_00f5_45bb_8c6f_6fb128cd41ae"/>
    <annotations:EMMO_967080e5_2f42_4eb2_a3a9_c58143e835f9>A reference unit provided by a reference material.
International vocabulary of metrology (VIM)</annotations:EMMO_967080e5_2f42_4eb2_a3a9_c58143e835f9>
    <annotations:EMMO_b432d2d5_25f4_4165_99c5_5935a7763c1a>Arbitrary amount-of-substance concentration of lutropin in a given sample of plasma (WHO international standard 80/552): 5.0 International Unit/l</annotations:EMMO_b432d2d5_25f4_4165_99c5_5935a7763c1a>
  </rdf:Description>
  <rdf:Description rdf:about="http://emmo.info/emmo/middle/math#EMMO_88470739_03d3_4c47_a03e_b30a1288d50c">
    <rdf:type rdf:resource="http://www.w3.org/2002/07/owl#Class"/>
    <rdfs:label xml:lang="en">Formula</rdfs:label>
    <rdfs:subClassOf rdf:resource="http://emmo.info/emmo/middle/math#EMMO_54ee6b5e_5261_44a8_86eb_5717e7fdb9d0"/>
    <annotations:EMMO_967080e5_2f42_4eb2_a3a9_c58143e835f9>A mathematica string that can be evaluated as true or false.</annotations:EMMO_967080e5_2f42_4eb2_a3a9_c58143e835f9>
    <rdfs:subClassOf rdf:resource="http://emmo.info/emmo/middle/perceptual#EMMO_89a0c87c_0804_4013_937a_6fe234d9499c"/>
  </rdf:Description>
  <rdf:Description rdf:nodeID="N4bc3064a9a434373b6319b154507a5c0">
    <rdf:type rdf:resource="http://www.w3.org/2002/07/owl#Restriction"/>
    <owl:onProperty rdf:resource="http://emmo.info/emmo/middle/perceptual#EMMO_23b579e1_8088_45b5_9975_064014026c42"/>
    <owl:hasValue>F</owl:hasValue>
  </rdf:Description>
  <rdf:Description rdf:nodeID="N725e8dabe03447759c0b65f364ec2c5a">
    <owl:onProperty rdf:resource="http://emmo.info/emmo/middle/metrology#EMMO_bed1d005_b04e_4a90_94cf_02bc678a8569"/>
    <owl:allValuesFrom rdf:resource="http://emmo.info/emmo/middle/isq#EMMO_b3600e73_3e05_479d_9714_c041c3acf5cc"/>
    <rdf:type rdf:resource="http://www.w3.org/2002/07/owl#Restriction"/>
  </rdf:Description>
  <rdf:Description rdf:nodeID="N4597b6cf975e44f59a5858d894b65479">
    <rdf:type rdf:resource="http://www.w3.org/2002/07/owl#Restriction"/>
    <owl:onProperty rdf:resource="http://emmo.info/emmo/middle/metrology#EMMO_bed1d005_b04e_4a90_94cf_02bc678a8569"/>
    <owl:allValuesFrom rdf:resource="http://emmo.info/emmo/middle/isq#EMMO_02e894c3_b793_4197_b120_3442e08f58d1"/>
  </rdf:Description>
  <rdf:Description rdf:about="http://emmo.info/emmo/middle/siunits#EMMO_05083b9c_c9d1_4202_b22d_5249067772ac">
    <ns1:EMMO_23b579e1_8088_45b5_9975_064014026c42 rdf:datatype="http://www.w3.org/2001/XMLSchema#string">T0 L+1 M0 I0 Θ0 N0 J0</ns1:EMMO_23b579e1_8088_45b5_9975_064014026c42>
    <rdf:type rdf:resource="http://www.w3.org/2002/07/owl#NamedIndividual"/>
    <rdfs:label xml:lang="en">b</rdfs:label>
  </rdf:Description>
  <rdf:Description rdf:nodeID="Nfa669788efe14134a1f041feec300a4b">
    <rdf:rest rdf:nodeID="N1e8b67052dcf4c12927515d8b3496aff"/>
    <rdf:first rdf:resource="http://emmo.info/emmo/middle/siunits#EMMO_daa9ee97_4c5f_42e5_918c_44d7523e8958"/>
  </rdf:Description>
  <rdf:Description rdf:nodeID="N2a926ecd6ff341c8bf319f8a9d3de555">
    <owl:onProperty rdf:resource="http://emmo.info/emmo/middle/metrology#EMMO_bed1d005_b04e_4a90_94cf_02bc678a8569"/>
    <owl:someValuesFrom rdf:resource="http://emmo.info/emmo/middle/isq#EMMO_ce7d4720_aa20_4a8c_93e8_df41a35b6723"/>
    <rdf:type rdf:resource="http://www.w3.org/2002/07/owl#Restriction"/>
  </rdf:Description>
  <rdf:Description rdf:about="http://emmo.info/emmo/middle/materials#EMMO_f835f4d4_c665_403d_ab25_dca5cc74be52">
    <rdf:type rdf:resource="http://www.w3.org/2002/07/owl#Class"/>
    <rdfs:subClassOf rdf:resource="http://emmo.info/emmo/middle/materials#EMMO_7d66bde4_b68d_41cc_b5fc_6fd98c5e2ff0"/>
    <rdfs:label xml:lang="en">Nucleus</rdfs:label>
    <rdfs:subClassOf rdf:nodeID="N17e149a542d0430e977bccd7eb7a3b4f"/>
  </rdf:Description>
  <rdf:Description rdf:nodeID="N029d3a2c0e994e9d9cfb6c53adca69b5">
    <rdf:type rdf:resource="http://www.w3.org/2002/07/owl#Restriction"/>
    <owl:onProperty rdf:resource="http://emmo.info/emmo/middle/metrology#EMMO_bed1d005_b04e_4a90_94cf_02bc678a8569"/>
    <owl:someValuesFrom rdf:resource="http://emmo.info/emmo/middle/isq#EMMO_668e6ead_1530_40cc_ad5e_24b880edff50"/>
  </rdf:Description>
  <rdf:Description rdf:nodeID="Nbf40eebcc71f4e81b07005d218fdeeaf">
    <rdf:first rdf:resource="http://emmo.info/emmo/middle/metrology#EMMO_08b308d4_31cd_4779_a784_aa92fc730f39"/>
    <rdf:rest rdf:nodeID="N6b17f3bb902b4bcd9d02eac3cdd1632e"/>
  </rdf:Description>
  <rdf:Description rdf:nodeID="N1c63e2fad530418a94b23cb21444fba4">
    <rdf:first rdf:resource="http://emmo.info/emmo/middle/physicalistic#EMMO_70dac51e_bddd_48c2_8a98_7d8395e91fc2"/>
    <rdf:rest rdf:nodeID="Nc78a55a5c3fa4ba1accabe4944ff36fc"/>
  </rdf:Description>
  <rdf:Description rdf:nodeID="Nf86dc0483f7c47c3a69198c5d9704d2f">
    <owl:inverseOf rdf:resource="http://emmo.info/emmo/middle/math#EMMO_3446e167_c576_49d6_846c_215bb8878a55"/>
  </rdf:Description>
  <rdf:Description rdf:nodeID="Nc247f24d50b14edbb411811ff383f17b">
    <owl:allValuesFrom rdf:nodeID="N3a4172ecb84f4a27ac6fc8ac80294096"/>
    <owl:onProperty rdf:resource="http://emmo.info/emmo/middle/metrology#EMMO_67fc0a36_8dcb_4ffa_9a43_31074efa3296"/>
    <rdf:type rdf:resource="http://www.w3.org/2002/07/owl#Restriction"/>
  </rdf:Description>
  <rdf:Description rdf:nodeID="N9ccab888074f47afa89e6fc78ecf6e29">
    <rdf:type rdf:resource="http://www.w3.org/2002/07/owl#Class"/>
    <owl:unionOf rdf:nodeID="N1a4d39d7416b45629abd39ca251a070a"/>
  </rdf:Description>
  <rdf:Description rdf:nodeID="N0971065b3b794a4da4f1654c490879e2">
    <rdf:type rdf:resource="http://www.w3.org/2002/07/owl#Restriction"/>
    <owl:hasValue>P</owl:hasValue>
    <owl:onProperty rdf:resource="http://emmo.info/emmo/middle/perceptual#EMMO_23b579e1_8088_45b5_9975_064014026c42"/>
  </rdf:Description>
  <rdf:Description rdf:about="http://emmo.info/emmo/top/math#EMMO_2b1303e8_d4c3_453b_9918_76f1d009543f">
    <rdfs:subClassOf rdf:resource="http://emmo.info/emmo/middle/math#EMMO_707f0cd1_941c_4b57_9f20_d0ba30cd6ff3"/>
    <rdf:type rdf:resource="http://www.w3.org/2002/07/owl#Class"/>
    <rdfs:label xml:lang="en">Multiplication</rdfs:label>
    <owl:equivalentClass rdf:nodeID="N1a018e65b5eb493d86feaf9ea984a50e"/>
  </rdf:Description>
  <rdf:Description rdf:nodeID="Ne1847459f29e4dd08aeff03242ece764">
    <rdf:type rdf:resource="http://www.w3.org/2002/07/owl#Restriction"/>
    <owl:someValuesFrom rdf:resource="http://emmo.info/emmo/middle/models#EMMO_27c5d8c6_8af7_4d63_beb1_ec37cd8b3fa3"/>
    <owl:onProperty rdf:resource="http://emmo.info/emmo/top/physical#EMMO_f68030be_94b8_4c61_a161_886468558054"/>
  </rdf:Description>
  <rdf:Description rdf:nodeID="N0e3e37822c234168a7038868088ca604">
    <owl:onProperty rdf:resource="http://emmo.info/emmo/middle/perceptual#EMMO_23b579e1_8088_45b5_9975_064014026c42"/>
    <rdf:type rdf:resource="http://www.w3.org/2002/07/owl#Restriction"/>
    <owl:hasValue>T-1 L0 M0 I0 Θ0 N0 J0</owl:hasValue>
  </rdf:Description>
  <rdf:Description rdf:nodeID="N5621ac169a9d4d51a511ddab1ceaa278">
    <rdf:first rdf:resource="http://emmo.info/emmo/middle/siunits#EMMO_9bfd6f1e_b0ce_459c_beb7_8f1f41708bba"/>
    <rdf:rest rdf:nodeID="N8dc70def2bea4d58920e7423f21b1623"/>
  </rdf:Description>
  <rdf:Description rdf:about="http://emmo.info/emmo/middle/siunits#EMMO_3a185e6c_9e19_4776_b583_19c978156aa0">
    <rdfs:seeAlso>https://www.bipm.org/utils/common/pdf/si-brochure/SI-Brochure-9-EN.pdf</rdfs:seeAlso>
    <annotations:EMMO_967080e5_2f42_4eb2_a3a9_c58143e835f9>The base units in the SI system.</annotations:EMMO_967080e5_2f42_4eb2_a3a9_c58143e835f9>
    <rdfs:label xml:lang="en">SIBaseUnit</rdfs:label>
    <rdfs:subClassOf rdf:resource="http://emmo.info/emmo/middle/metrology#EMMO_db716151_6b73_45ff_910c_d182fdcbb4f5"/>
    <rdf:type rdf:resource="http://www.w3.org/2002/07/owl#Class"/>
    <owl:disjointUnionOf rdf:nodeID="N28cce3be90ba4ef08ba5863198335968"/>
  </rdf:Description>
  <rdf:Description rdf:about="http://emmo.info/emmo/middle/math#EMMO_ae15fb4f_8e4d_41de_a0f9_3997f89ba6a2">
    <rdfs:subClassOf rdf:nodeID="Nfe364a4a656042d1ad8b65e5d94e000e"/>
    <rdfs:label xml:lang="en">Constant</rdfs:label>
    <rdf:type rdf:resource="http://www.w3.org/2002/07/owl#Class"/>
    <rdfs:subClassOf rdf:resource="http://emmo.info/emmo/middle/math#EMMO_1eed0732_e3f1_4b2c_a9c4_b4e75eeb5895"/>
    <annotations:EMMO_b432d2d5_25f4_4165_99c5_5935a7763c1a>π refers to the constant number ~3.14</annotations:EMMO_b432d2d5_25f4_4165_99c5_5935a7763c1a>
    <annotations:EMMO_967080e5_2f42_4eb2_a3a9_c58143e835f9>A 'varaible' that stand for a well known constant.</annotations:EMMO_967080e5_2f42_4eb2_a3a9_c58143e835f9>
  </rdf:Description>
  <rdf:Description rdf:nodeID="Nf3b7ff0246774851a9370121a28ffd58">
    <owl:someValuesFrom rdf:resource="http://emmo.info/emmo/top/semiotics#EMMO_054af807_85cd_4a13_8eba_119dfdaaf38b"/>
    <owl:onProperty rdf:resource="http://emmo.info/emmo/top/physical#EMMO_f68030be_94b8_4c61_a161_886468558054"/>
    <rdf:type rdf:resource="http://www.w3.org/2002/07/owl#Restriction"/>
  </rdf:Description>
  <rdf:Description rdf:nodeID="Na2106a037cac4ed88e8f47a9baae1f67">
    <owl:onProperty rdf:resource="http://emmo.info/emmo/middle/perceptual#EMMO_23b579e1_8088_45b5_9975_064014026c42"/>
    <owl:hasValue>T0 L0 M0 I0 Θ0 N0 J+1</owl:hasValue>
    <rdf:type rdf:resource="http://www.w3.org/2002/07/owl#Restriction"/>
  </rdf:Description>
  <rdf:Description rdf:nodeID="N9f97745668f24fb18e046217a2c4bfc7">
    <owl:inverseOf rdf:resource="http://emmo.info/emmo/middle/math#EMMO_3446e167_c576_49d6_846c_215bb8878a55"/>
  </rdf:Description>
  <rdf:Description rdf:nodeID="N8f7414200227493d91f1bb2bb926a701">
    <owl:onProperty rdf:nodeID="Nfe8da12640754402a2651f6d64807cdb"/>
    <rdf:type rdf:resource="http://www.w3.org/2002/07/owl#Restriction"/>
    <owl:someValuesFrom rdf:resource="http://emmo.info/emmo/middle/models#EMMO_314d0bd5_67ed_437e_a609_36d46147cea7"/>
  </rdf:Description>
  <rdf:Description rdf:about="http://emmo.info/emmo/middle/models#EMMO_f19ff3b4_6bfe_4c41_a2b2_9affd39c140b">
    <rdfs:label xml:lang="en">MaterialLaw</rdfs:label>
    <rdfs:subClassOf rdf:resource="http://emmo.info/emmo/middle/models#EMMO_db9a009e_f097_43f5_9520_6cbc07e7610b"/>
    <rdf:type rdf:resource="http://www.w3.org/2002/07/owl#Class"/>
  </rdf:Description>
  <rdf:Description rdf:about="http://emmo.info/emmo/middle/siunits#EMMO_32129fb5_df25_48fd_a29c_18a2f22a2dd5">
    <owl:disjointUnionOf rdf:nodeID="N7ed24cb7d5db4203b056bbf73487120c"/>
    <rdfs:label xml:lang="en">SIUnitSymbol</rdfs:label>
    <rdf:type rdf:resource="http://www.w3.org/2002/07/owl#Class"/>
  </rdf:Description>
  <rdf:Description rdf:nodeID="Ndb753105f98d4a6f91df9f358c307cff">
    <owl:allValuesFrom rdf:nodeID="N90551f61951d423298057091440fae38"/>
    <owl:onProperty rdf:resource="http://emmo.info/emmo/middle/metrology#EMMO_67fc0a36_8dcb_4ffa_9a43_31074efa3296"/>
    <rdf:type rdf:resource="http://www.w3.org/2002/07/owl#Restriction"/>
  </rdf:Description>
  <rdf:Description rdf:about="http://emmo.info/emmo/middle/isq#EMMO_5c003f53_20a2_4bd7_8445_58187e582578">
    <rdf:type rdf:resource="http://www.w3.org/2002/07/owl#Class"/>
    <owl:equivalentClass rdf:nodeID="N655e919a75dd4745a1f369fed39c574c"/>
    <rdfs:label xml:lang="en">LuminousIntensityCubicTimePerMassLengthDimension</rdfs:label>
    <rdfs:subClassOf rdf:resource="http://emmo.info/emmo/middle/metrology#EMMO_9895a1b4_f0a5_4167_ac5e_97db40b8bfcc"/>
  </rdf:Description>
  <rdf:Description rdf:nodeID="Nbcc4e113796c422f8ba6b9f11449f729">
    <rdf:rest rdf:resource="http://www.w3.org/1999/02/22-rdf-syntax-ns#nil"/>
    <rdf:first rdf:resource="http://emmo.info/emmo/middle/physicalistic#EMMO_eb3c61f0_3983_4346_a0c6_e7f6b90a67a8"/>
  </rdf:Description>
  <rdf:Description rdf:nodeID="N4c56b3950488404da9ea7b4ae9d219a4">
    <owl:allValuesFrom rdf:nodeID="N766f25239a864ab09b1c09f9858452a9"/>
    <owl:onProperty rdf:resource="http://emmo.info/emmo/middle/metrology#EMMO_67fc0a36_8dcb_4ffa_9a43_31074efa3296"/>
    <rdf:type rdf:resource="http://www.w3.org/2002/07/owl#Restriction"/>
  </rdf:Description>
  <rdf:Description rdf:about="http://emmo.info/emmo/middle/perceptual#EMMO_d7bf784a_db94_4dd9_861c_54f262846fbf">
    <rdfs:subClassOf rdf:resource="http://emmo.info/emmo/middle/perceptual#EMMO_9268958f_7f54_48ab_a693_febe2645892b"/>
    <rdfs:label xml:lang="en">Sphere</rdfs:label>
    <rdf:type rdf:resource="http://www.w3.org/2002/07/owl#Class"/>
  </rdf:Description>
  <rdf:Description rdf:nodeID="N56bbb48c32074cf586be02fce15780ee">
    <rdf:type rdf:resource="http://www.w3.org/2002/07/owl#Restriction"/>
    <owl:hasValue>a</owl:hasValue>
    <owl:onProperty rdf:resource="http://emmo.info/emmo/middle/perceptual#EMMO_23b579e1_8088_45b5_9975_064014026c42"/>
  </rdf:Description>
  <rdf:Description rdf:nodeID="N0e57a41415a2428998b9874866c72a3f">
    <rdf:rest rdf:resource="http://www.w3.org/1999/02/22-rdf-syntax-ns#nil"/>
    <rdf:first rdf:resource="http://emmo.info/emmo/middle/siunits#EMMO_f5769206_9257_4b08_bf7b_dad7868c6afc"/>
  </rdf:Description>
  <rdf:Description rdf:about="http://emmo.info/emmo/middle/perceptual#EMMO_23b579e1_8088_45b5_9975_064014026c42">
    <rdfs:label xml:lang="en">hasSymbolData</rdfs:label>
    <rdfs:range rdf:resource="http://www.w3.org/2001/XMLSchema#string"/>
    <rdfs:domain rdf:resource="http://emmo.info/emmo/middle/perceptual#EMMO_a1083d0a_c1fb_471f_8e20_a98f881ad527"/>
    <rdf:type rdf:resource="http://www.w3.org/2002/07/owl#DatatypeProperty"/>
  </rdf:Description>
  <rdf:Description rdf:nodeID="N3a4172ecb84f4a27ac6fc8ac80294096">
    <owl:allValuesFrom rdf:resource="http://emmo.info/emmo/middle/isq#EMMO_f6070071_d054_4b17_9d2d_f446f7147d0f"/>
    <rdf:type rdf:resource="http://www.w3.org/2002/07/owl#Restriction"/>
    <owl:onProperty rdf:resource="http://emmo.info/emmo/middle/metrology#EMMO_bed1d005_b04e_4a90_94cf_02bc678a8569"/>
  </rdf:Description>
  <rdf:Description rdf:nodeID="Nbb4273055f6a48b9b407cc6f7bb0062a">
    <rdf:rest rdf:nodeID="N42e044b0c0af4bb5a21c24e09a9f20f1"/>
    <rdf:first rdf:resource="http://emmo.info/emmo/middle/siunits#EMMO_696ed548_9477_45ea_993c_6a8f5271914a"/>
  </rdf:Description>
  <rdf:Description rdf:nodeID="N816a20186e764fbdb18f9ffb6ce540f4">
    <rdf:first rdf:resource="http://emmo.info/emmo/middle/siunits#EMMO_314ba716_2d3d_4462_9a4f_d3419ae1df43"/>
    <rdf:rest rdf:nodeID="N4a67bf79c8954b2a86a4185810889860"/>
  </rdf:Description>
  <rdf:Description rdf:nodeID="N4675b24c538d4b1abf6283543c82fe33">
    <owl:onProperty rdf:resource="http://emmo.info/emmo/middle/reductionistic#EMMO_65a2c5b8_e4d8_4a51_b2f8_e55effc0547d"/>
    <owl:someValuesFrom rdf:resource="http://emmo.info/emmo/middle/reductionistic#EMMO_36c79456_e29c_400d_8bd3_0eedddb82652"/>
    <rdf:type rdf:resource="http://www.w3.org/2002/07/owl#Restriction"/>
  </rdf:Description>
  <rdf:Description rdf:nodeID="Nd25fbf187d78466da1e31fe19dce04ec">
    <rdf:first rdf:resource="http://emmo.info/emmo/middle/materials#EMMO_df808271_df91_4f27_ba59_fa423c51896c"/>
    <rdf:rest rdf:resource="http://www.w3.org/1999/02/22-rdf-syntax-ns#nil"/>
  </rdf:Description>
  <rdf:Description rdf:nodeID="N7646f8bfc869439c860c29919e135854">
    <rdf:type rdf:resource="http://www.w3.org/2002/07/owl#Restriction"/>
    <owl:someValuesFrom rdf:resource="http://emmo.info/emmo/middle/properties#EMMO_10a5fd39_06aa_4648_9e70_f962a9cb2069"/>
    <owl:onProperty rdf:nodeID="Nfd04d47cd602466ab8bb84b80044c53a"/>
  </rdf:Description>
  <rdf:Description rdf:nodeID="Na2f4693a00d042c48ac70098234e0a7e">
    <rdf:first rdf:resource="http://emmo.info/emmo/middle/siunits#EMMO_33b67e69_3645_4c73_b100_5ea6759221b4"/>
    <rdf:rest rdf:nodeID="N8eeedf64393f456a859dfb674a46dde3"/>
  </rdf:Description>
  <rdf:Description rdf:nodeID="N9317f2a36b544bdfa8699a37b32afe72">
    <rdf:first rdf:resource="http://emmo.info/emmo/middle/siunits#EMMO_8d00f093_3f45_4ea3_986c_b3545c3c2f4c"/>
    <rdf:rest rdf:nodeID="N5621ac169a9d4d51a511ddab1ceaa278"/>
  </rdf:Description>
  <rdf:Description rdf:nodeID="N98dab9d34ed04a0b92aeda604b6d3e7d">
    <rdf:rest rdf:nodeID="N5a01ad4d96544ed499d895ee3b1d1581"/>
    <rdf:first rdf:resource="http://emmo.info/emmo/middle/siunits#EMMO_506f7823_52bc_40cb_be07_b3b1e10cce13"/>
  </rdf:Description>
  <rdf:Description rdf:about="http://emmo.info/emmo/top/annotations#EMMO_1f1b164d_ec6a_4faa_8d5e_88bda62316cc">
    <rdfs:subPropertyOf rdf:resource="http://www.w3.org/2000/01/rdf-schema#seeAlso"/>
    <rdf:type rdf:resource="http://www.w3.org/2002/07/owl#AnnotationProperty"/>
    <rdfs:comment>URL to corresponing entity in QUDT.</rdfs:comment>
    <rdfs:seeAlso>http://www.qudt.org/2.1/catalog/qudt-catalog.html</rdfs:seeAlso>
    <rdfs:label xml:lang="en">qudtMatch</rdfs:label>
  </rdf:Description>
  <rdf:Description rdf:about="http://emmo.info/emmo/middle/siunits#EMMO_2e5e45fc_f52c_4294_bdc2_5ed7a06dfce7">
    <annotations:EMMO_1f1b164d_ec6a_4faa_8d5e_88bda62316cc>http://qudt.org/vocab/unit/K</annotations:EMMO_1f1b164d_ec6a_4faa_8d5e_88bda62316cc>
    <annotations:EMMO_70fe84ff_99b6_4206_a9fc_9a8931836d84>The kelvin, symbol K, is the SI unit of thermodynamic temperature. It is defined by taking the fixed numerical value of the Boltzmann constant k to be 1.380649×10−23 when expressed in the unit J K−1, which is equal to kg m2 s−2 K−1, where the kilogram, metre and second are defined in terms of h, c and ∆νCs.</annotations:EMMO_70fe84ff_99b6_4206_a9fc_9a8931836d84>
    <annotations:EMMO_fe015383_afb3_44a6_ae86_043628697aa2>https://doi.org/10.1351/goldbook.K03374</annotations:EMMO_fe015383_afb3_44a6_ae86_043628697aa2>
    <rdfs:subClassOf rdf:nodeID="N11017920217c4056af507247e66a0168"/>
    <rdfs:subClassOf rdf:nodeID="Nac71b7b699e3450ebe25e232a1d26f63"/>
    <rdfs:label xml:lang="en">Kelvin</rdfs:label>
    <rdf:type rdf:resource="http://www.w3.org/2002/07/owl#Class"/>
  </rdf:Description>
  <rdf:Description rdf:about="http://emmo.info/emmo/middle/isq#EMMO_ab79e92b_5377_454d_be06_d61b50db295a">
    <rdfs:subClassOf rdf:resource="http://emmo.info/emmo/middle/metrology#EMMO_9895a1b4_f0a5_4167_ac5e_97db40b8bfcc"/>
    <rdf:type rdf:resource="http://www.w3.org/2002/07/owl#Class"/>
    <rdfs:label xml:lang="en">TimeCurrentDimension</rdfs:label>
    <owl:equivalentClass rdf:nodeID="Nbd27e94e58224c0784c0453d467cab0f"/>
  </rdf:Description>
  <rdf:Description rdf:nodeID="N487bcf892a4849d18369370a958d55ab">
    <rdf:type rdf:resource="http://www.w3.org/2002/07/owl#Restriction"/>
    <owl:someValuesFrom rdf:resource="http://emmo.info/emmo/middle/isq#EMMO_4c49ab58_a6f6_409e_b849_f873ae1dcbee"/>
    <owl:onProperty rdf:resource="http://emmo.info/emmo/middle/metrology#EMMO_bed1d005_b04e_4a90_94cf_02bc678a8569"/>
  </rdf:Description>
  <rdf:Description rdf:nodeID="N60abfc76aea241859d3d9e82448ea0d8">
    <owl:onProperty rdf:resource="http://emmo.info/emmo/middle/perceptual#EMMO_23b579e1_8088_45b5_9975_064014026c42"/>
    <owl:hasValue>∇</owl:hasValue>
    <rdf:type rdf:resource="http://www.w3.org/2002/07/owl#Restriction"/>
  </rdf:Description>
  <rdf:Description rdf:about="http://emmo.info/emmo/top/mereotopology#EMMO_03212fd7_abfd_4828_9c8e_62c293052d4b">
    <annotations:EMMO_967080e5_2f42_4eb2_a3a9_c58143e835f9>The superclass of all EMMO mereotopological relations.</annotations:EMMO_967080e5_2f42_4eb2_a3a9_c58143e835f9>
    <rdfs:comment>Mereotopology merges mereological and topological concepts and provides relations between wholes, parts, boundaries, etc.</rdfs:comment>
    <rdfs:label xml:lang="en">mereotopological</rdfs:label>
    <rdf:type rdf:resource="http://www.w3.org/2002/07/owl#SymmetricProperty"/>
    <rdf:type rdf:resource="http://www.w3.org/2002/07/owl#TransitiveProperty"/>
    <rdf:type rdf:resource="http://www.w3.org/2002/07/owl#ObjectProperty"/>
    <rdfs:subPropertyOf rdf:resource="http://emmo.info/emmo/top/mereotopology#EMMO_ec2472ae_cf4a_46a5_8555_1556f5a6c3c5"/>
  </rdf:Description>
  <rdf:Description rdf:nodeID="N171648765e3c45a39c0fee0faa8adb14">
    <owl:onProperty rdf:nodeID="Nda49d69bb4b145c48b2a00d9080032d7"/>
    <owl:allValuesFrom rdf:nodeID="N4c9c331d376642aeac19b3d93c417168"/>
    <rdf:type rdf:resource="http://www.w3.org/2002/07/owl#Restriction"/>
  </rdf:Description>
  <rdf:Description rdf:nodeID="N66e5f21acb0446809e5067e77a111073">
    <rdf:type rdf:resource="http://www.w3.org/2002/07/owl#Restriction"/>
    <owl:hasValue>k</owl:hasValue>
    <owl:onProperty rdf:resource="http://emmo.info/emmo/middle/perceptual#EMMO_23b579e1_8088_45b5_9975_064014026c42"/>
  </rdf:Description>
  <rdf:Description rdf:nodeID="N6c293cf031c6490c977b1548bd713df4">
    <owl:allValuesFrom rdf:nodeID="N7a398ec7b5464a899bf4f6253b11079d"/>
    <rdf:type rdf:resource="http://www.w3.org/2002/07/owl#Restriction"/>
    <owl:onProperty rdf:resource="http://emmo.info/emmo/middle/metrology#EMMO_67fc0a36_8dcb_4ffa_9a43_31074efa3296"/>
  </rdf:Description>
  <rdf:Description rdf:about="http://emmo.info/emmo/top/semiotics#EMMO_297999d6_c9e4_4262_9536_bd524d1c6e21">
    <rdfs:subPropertyOf rdf:resource="http://emmo.info/emmo/top/semiotics#EMMO_60577dea_9019_4537_ac41_80b0fb563d41"/>
    <rdfs:range rdf:resource="http://emmo.info/emmo/top/semiotics#EMMO_0cd58641_824c_4851_907f_f4c3be76630c"/>
    <rdfs:label xml:lang="en">hasIndex</rdfs:label>
    <rdf:type rdf:resource="http://www.w3.org/2002/07/owl#ObjectProperty"/>
  </rdf:Description>
  <rdf:Description rdf:about="http://emmo.info/emmo/middle/perceptual#EMMO_d8d2144e_5c8d_455d_a643_5caf4d8d9df8">
    <rdf:type rdf:resource="http://www.w3.org/2002/07/owl#Class"/>
    <rdfs:subClassOf rdf:resource="http://emmo.info/emmo/middle/perceptual#EMMO_057e7d57_aff0_49de_911a_8861d85cef40"/>
    <rdfs:label xml:lang="en">Language</rdfs:label>
    <annotations:EMMO_967080e5_2f42_4eb2_a3a9_c58143e835f9>A language object is a symbolic object respecting a specific language syntactic rules (a well-formed formula).</annotations:EMMO_967080e5_2f42_4eb2_a3a9_c58143e835f9>
  </rdf:Description>
  <rdf:Description rdf:about="http://emmo.info/emmo/middle/perceptual#EMMO_660ef3b0_6692_4c51_8f69_763c7817b2e1">
    <rdfs:subClassOf rdf:resource="http://emmo.info/emmo/middle/perceptual#EMMO_4b3afb22_27cf_4ce3_88bc_492bfccb546b"/>
    <rdf:type rdf:resource="http://www.w3.org/2002/07/owl#Class"/>
    <rdfs:label xml:lang="en">Speech</rdfs:label>
  </rdf:Description>
  <rdf:Description rdf:nodeID="N7ee177ae40ba4ad5a9730b0fd07398ac">
    <rdf:first rdf:resource="http://emmo.info/emmo/middle/physicalistic#EMMO_8043d3c6_a4c1_4089_ba34_9744e28e5b3d"/>
    <rdf:rest rdf:nodeID="N291ef216c88c420fb5053d13150429f8"/>
  </rdf:Description>
  <rdf:Description rdf:about="http://emmo.info/emmo/middle/models#EMMO_27c5d8c6_8af7_4d63_beb1_ec37cd8b3fa3">
    <rdfs:subClassOf rdf:resource="http://emmo.info/emmo/middle/math#EMMO_e56ee3eb_7609_4ae1_8bed_51974f0960a6"/>
    <annotations:EMMO_967080e5_2f42_4eb2_a3a9_c58143e835f9>An 'equation' that stands for a 'physical_law' by mathematically defining the relations between physics_quantities.</annotations:EMMO_967080e5_2f42_4eb2_a3a9_c58143e835f9>
    <rdfs:comment>The Newton's equation of motion.

The Schrodinger equation.

The Navier-Stokes equation.</rdfs:comment>
    <rdfs:subClassOf rdf:nodeID="N8f7414200227493d91f1bb2bb926a701"/>
    <rdfs:subClassOf rdf:nodeID="N72f492c1a32c4f8a95adf331afffb9ab"/>
    <rdf:type rdf:resource="http://www.w3.org/2002/07/owl#Class"/>
    <rdfs:label xml:lang="en">PhysicsEquation</rdfs:label>
  </rdf:Description>
  <rdf:Description rdf:nodeID="N7e1e011133494ac397d3fdafa69e647f">
    <owl:onProperty rdf:nodeID="Nc8bc6ccd39e240178a9036dfe08e541a"/>
    <rdf:type rdf:resource="http://www.w3.org/2002/07/owl#Restriction"/>
    <owl:someValuesFrom rdf:resource="http://emmo.info/emmo/middle/math#EMMO_54ee6b5e_5261_44a8_86eb_5717e7fdb9d0"/>
  </rdf:Description>
  <rdf:Description rdf:about="http://emmo.info/emmo/middle/isq#EMMO_1a4c1a97_88a7_4d8e_b2f9_2ca58e92dde4">
    <annotations:EMMO_967080e5_2f42_4eb2_a3a9_c58143e835f9>Base quantities defined in the International System of Quantities (ISQ).</annotations:EMMO_967080e5_2f42_4eb2_a3a9_c58143e835f9>
    <rdfs:subClassOf rdf:resource="http://emmo.info/emmo/middle/isq#EMMO_f35cff4d_dc09_44cf_a729_22fb79e3bfb2"/>
    <rdf:type rdf:resource="http://www.w3.org/2002/07/owl#Class"/>
    <rdfs:label xml:lang="en">ISQBaseQuantity</rdfs:label>
    <annotations:EMMO_c84c6752_6d64_48cc_9500_e54a3c34898d>https://en.wikipedia.org/wiki/International_System_of_Quantities</annotations:EMMO_c84c6752_6d64_48cc_9500_e54a3c34898d>
    <owl:disjointUnionOf rdf:nodeID="N69fb56d8fca147ffb78ab407cb6fc711"/>
    <rdfs:subClassOf rdf:resource="http://emmo.info/emmo/middle/metrology#EMMO_acaaa124_3dde_48b6_86e6_6ec6f364f408"/>
  </rdf:Description>
  <rdf:Description rdf:nodeID="N2fbbf86dc5a74fd48d48ef3ba7691010">
    <rdf:first rdf:resource="http://emmo.info/emmo/middle/siunits#EMMO_00199e76_69dc_45b6_a9c6_98cc90cdc0f5"/>
    <rdf:rest rdf:nodeID="N90ef0ccb732f499ca5527365bccb738d"/>
  </rdf:Description>
  <rdf:Description rdf:nodeID="N87295ee688cf4799b7964077c1760d78">
    <rdf:type rdf:resource="http://www.w3.org/2002/07/owl#Class"/>
    <owl:intersectionOf rdf:nodeID="Ndb1cfab06ed449acb821b09ebfa57c32"/>
  </rdf:Description>
  <rdf:Description rdf:about="http://emmo.info/emmo/middle/siunits#EMMO_5eaecadc_4f0d_4a3a_afc7_1fc0b83cc928">
    <rdfs:subClassOf rdf:nodeID="Nf4c03dc086c046259365beef4db711f2"/>
    <rdfs:label xml:lang="en">Mega</rdfs:label>
    <rdf:type rdf:resource="http://www.w3.org/2002/07/owl#Class"/>
    <rdfs:subClassOf rdf:nodeID="N30e49024982b49dfaa9a32e171461c35"/>
  </rdf:Description>
  <rdf:Description rdf:about="http://emmo.info/emmo/middle/isq#EMMO_7610efb8_c7c6_4684_abc1_774783c62472">
    <owl:equivalentClass rdf:nodeID="N4478dfee0ae845f4aaacb651ba609e4b"/>
    <rdfs:subClassOf rdf:resource="http://emmo.info/emmo/middle/metrology#EMMO_9895a1b4_f0a5_4167_ac5e_97db40b8bfcc"/>
    <rdf:type rdf:resource="http://www.w3.org/2002/07/owl#Class"/>
    <rdfs:label xml:lang="en">MassSquareLengthPerCubicTimeSquareCurrentDimension</rdfs:label>
  </rdf:Description>
  <rdf:Description rdf:nodeID="Ne22b68e0af944eb29e6d1b25994e6a49">
    <rdf:type rdf:resource="http://www.w3.org/2002/07/owl#Class"/>
    <owl:unionOf rdf:nodeID="N83cabc1e6cd24f879f96578013cf0277"/>
  </rdf:Description>
  <rdf:Description rdf:nodeID="N3747877166994a51b190984b959657d8">
    <owl:allValuesFrom rdf:nodeID="Nf74f1aef46404e75b9b9f0dadd79bf71"/>
    <rdf:type rdf:resource="http://www.w3.org/2002/07/owl#Restriction"/>
    <owl:onProperty rdf:resource="http://emmo.info/emmo/middle/metrology#EMMO_67fc0a36_8dcb_4ffa_9a43_31074efa3296"/>
  </rdf:Description>
  <rdf:Description rdf:nodeID="N5318166f25af4081a56615e46759fa73">
    <owl:allValuesFrom rdf:nodeID="Nd5336b7ad877473eba001d059d8e94c2"/>
    <rdf:type rdf:resource="http://www.w3.org/2002/07/owl#Restriction"/>
    <owl:onProperty rdf:resource="http://emmo.info/emmo/middle/metrology#EMMO_67fc0a36_8dcb_4ffa_9a43_31074efa3296"/>
  </rdf:Description>
  <rdf:Description rdf:about="http://emmo.info/emmo/top/semiotics#EMMO_008fd3b2_4013_451f_8827_52bceab11841">
    <rdfs:subClassOf rdf:resource="http://emmo.info/emmo/middle/holistic#EMMO_43e9a05d_98af_41b4_92f6_00f79a09bfce"/>
    <rdfs:subClassOf rdf:nodeID="N2b4b45bcdb694dac963fd0d22f14ab1d"/>
    <annotations:EMMO_b432d2d5_25f4_4165_99c5_5935a7763c1a>Me looking a cat and saying loud: "Cat!" -&gt; the semiosis process

me -&gt; interpreter
cat -&gt; object (in Peirce semiotics)
the cat perceived by my mind -&gt; interpretant
"Cat!" -&gt; sign, the produced sign</annotations:EMMO_b432d2d5_25f4_4165_99c5_5935a7763c1a>
    <rdfs:subClassOf rdf:nodeID="N72b3881d737c4b408c24b10c334d4360"/>
    <rdfs:subClassOf rdf:nodeID="N6133856df4f949c5b6bc0030a5b02dd6"/>
    <annotations:EMMO_967080e5_2f42_4eb2_a3a9_c58143e835f9>A 'Process', that has participant an 'Interpreter', that is aimed to produce a 'Sign' representing another participant, the 'Object'.</annotations:EMMO_967080e5_2f42_4eb2_a3a9_c58143e835f9>
    <rdf:type rdf:resource="http://www.w3.org/2002/07/owl#Class"/>
    <rdfs:label xml:lang="en">Semiosis</rdfs:label>
  </rdf:Description>
  <rdf:Description rdf:nodeID="Nf576db9a51bf4118a5febb7bc3b04ca5">
    <owl:onProperty rdf:resource="http://emmo.info/emmo/middle/perceptual#EMMO_23b579e1_8088_45b5_9975_064014026c42"/>
    <owl:hasValue>T0 L0 M0 I0 Θ0 N0 J0</owl:hasValue>
    <rdf:type rdf:resource="http://www.w3.org/2002/07/owl#Restriction"/>
  </rdf:Description>
  <rdf:Description rdf:nodeID="N665db57b99214517bb4c3ab2e3364b62">
    <rdf:rest rdf:nodeID="Na7744b3138c44408b226e6f72191ab57"/>
    <rdf:first rdf:resource="http://emmo.info/emmo/middle/metrology#EMMO_985bec21_989f_4b9e_a4b3_735d88099c3c"/>
  </rdf:Description>
  <rdf:Description rdf:nodeID="N4944db4f33cc44fc8f7677bd876f963f">
    <owl:minQualifiedCardinality rdf:datatype="http://www.w3.org/2001/XMLSchema#nonNegativeInteger">2</owl:minQualifiedCardinality>
  </rdf:Description>
  <rdf:Description rdf:nodeID="Nfe162cf70f72470594b4fcae8f5fd06c">
    <rdf:first rdf:resource="http://emmo.info/emmo/middle/models#EMMO_939483b1_0148_43d1_8b35_851d2cd5d939"/>
    <rdf:rest rdf:resource="http://www.w3.org/1999/02/22-rdf-syntax-ns#nil"/>
  </rdf:Description>
  <rdf:Description rdf:nodeID="N5d76899ac74f4d778405ec2532fdcc1f">
    <rdf:type rdf:resource="http://www.w3.org/2002/07/owl#Restriction"/>
    <owl:onProperty rdf:nodeID="N8724dd72540b40809c96aed21d5b0d0b"/>
    <owl:allValuesFrom rdf:nodeID="N9b8f51a7caa9458e8c44f2c7773484b4"/>
  </rdf:Description>
  <rdf:Description rdf:nodeID="Necb4889164fd4a378dd468d77fb5ae07">
    <rdf:type rdf:resource="http://www.w3.org/2002/07/owl#Restriction"/>
    <owl:onProperty rdf:resource="http://emmo.info/emmo/middle/metrology#EMMO_bed1d005_b04e_4a90_94cf_02bc678a8569"/>
    <owl:allValuesFrom rdf:resource="http://emmo.info/emmo/middle/isq#EMMO_ab79e92b_5377_454d_be06_d61b50db295a"/>
  </rdf:Description>
  <rdf:Description rdf:about="http://emmo.info/emmo/middle/models#EMMO_4456a5d2_16a6_4ee1_9a8e_5c75956b28ea">
    <annotations:EMMO_967080e5_2f42_4eb2_a3a9_c58143e835f9>A physics-based model based on a physics equation describing the behaviour of continuum volume.</annotations:EMMO_967080e5_2f42_4eb2_a3a9_c58143e835f9>
    <rdf:type rdf:resource="http://www.w3.org/2002/07/owl#Class"/>
    <rdfs:label xml:lang="en">ContinuumModel</rdfs:label>
    <rdfs:subClassOf rdf:resource="http://emmo.info/emmo/middle/models#EMMO_b29fd350_39aa_4af7_9459_3faa0544cba6"/>
  </rdf:Description>
  <rdf:Description rdf:about="http://emmo.info/emmo/middle/models">
    <annotations:EMMO_cd5fb112_7ee7_4120_a35d_3ca3e6c3f4ab>Emanuele Ghedini (University of Bologna, IT)
Gerhard Goldbeck (GCL Ltd, UK)
Adham Hashibon (Fraunhofer IWM, DE)
Georg Schmitz (Access, DE)
Jesper Friis (SINTEF, NO)</annotations:EMMO_cd5fb112_7ee7_4120_a35d_3ca3e6c3f4ab>
    <rdfs:comment>The EMMO requires FacT++ reasoner plugin in order to visualize all inferences and class hierarchy (ctrl+R hotkey in Protege).</rdfs:comment>
    <rdf:type rdf:resource="http://www.w3.org/2002/07/owl#Ontology"/>
    <owl:versionInfo>The European Materials Modelling Ontology

Version 1.0.0-alpha</owl:versionInfo>
    <rdfs:comment xml:lang="en">Contacts:
Gerhard Goldbeck
Goldbeck Consulting Ltd (UK)
email: gerhard@goldbeck-consulting.com

Emanuele Ghedini
University of Bologna (IT)
email: emanuele.ghedini@unibo.it</rdfs:comment>
    <owl:versionIRI rdf:resource="http://emmo.info/emmo/1.0.0-alpha/middle/models"/>
    <annotations:EMMO_5525a055_dda5_4556_8b91_f0d22fa676cc>EMMO is released under a Creative Commons license Attribution 4.0 International (CC BY 4.0)

https://creativecommons.org/licenses/by/4.0/legalcode</annotations:EMMO_5525a055_dda5_4556_8b91_f0d22fa676cc>
    <rdfs:comment>European Materials and Modelling Ontology (EMMO)

EMMO is a multidisciplinary effort to develop a standard representational framework (the ontology) based on current materials modelling knowledge, including physical sciences, analytical philosophy and information and communication technologies. 

It provides the connection between the physical world, materials characterisation world and materials modelling world.</rdfs:comment>
  </rdf:Description>
  <rdf:Description rdf:about="http://emmo.info/emmo/top/annotations#EMMO_c84c6752_6d64_48cc_9500_e54a3c34898d">
    <rdfs:comment>URL to corresponding Wikipedia entry.</rdfs:comment>
    <rdfs:seeAlso>https://www.wikipedia.org/</rdfs:seeAlso>
    <rdf:type rdf:resource="http://www.w3.org/2002/07/owl#AnnotationProperty"/>
    <rdfs:label xml:lang="en">wikipediaEntry</rdfs:label>
    <rdfs:subPropertyOf rdf:resource="http://www.w3.org/2000/01/rdf-schema#seeAlso"/>
  </rdf:Description>
  <rdf:Description rdf:nodeID="Nde6a077c3384417cb16017b6927a6b7f">
    <owl:onProperty rdf:nodeID="Na8c95441978c4657a5e2fba14441e82c"/>
    <owl:allValuesFrom rdf:nodeID="N105c88c61d514bc18291a450942d5d01"/>
    <rdf:type rdf:resource="http://www.w3.org/2002/07/owl#Restriction"/>
  </rdf:Description>
  <rdf:Description rdf:nodeID="N39692b988209468e971afa9080334da3">
    <rdf:rest rdf:nodeID="N1b3cb51adedd4fd18838c5f72b2105ba"/>
    <rdf:first rdf:resource="http://emmo.info/emmo/middle/siunits#EMMO_d7f11b34_a121_4519_87c0_aa754f1c4737"/>
  </rdf:Description>
  <rdf:Description rdf:nodeID="N04a9f2a19f8b43eb93c67b7c0f24bf76">
    <owl:unionOf rdf:nodeID="N2d90dc7b048e425fb66c7ce35ec02eba"/>
    <rdf:type rdf:resource="http://www.w3.org/2002/07/owl#Class"/>
  </rdf:Description>
  <rdf:Description rdf:nodeID="N4df09dabedf6443cb8a33c1f330f3c25">
    <owl:onProperty rdf:resource="http://emmo.info/emmo/middle/math#EMMO_faf79f53_749d_40b2_807c_d34244c192f4"/>
    <rdf:type rdf:resource="http://www.w3.org/2002/07/owl#Restriction"/>
    <owl:someValuesFrom rdf:resource="http://www.w3.org/2001/XMLSchema#boolean"/>
  </rdf:Description>
  <rdf:Description rdf:nodeID="Nde648a234346423fb8e73c7bd2083a1a">
    <owl:hasValue>T+1 L0 M0 I0 Θ0 N0 J0</owl:hasValue>
    <rdf:type rdf:resource="http://www.w3.org/2002/07/owl#Restriction"/>
    <owl:onProperty rdf:resource="http://emmo.info/emmo/middle/perceptual#EMMO_23b579e1_8088_45b5_9975_064014026c42"/>
  </rdf:Description>
  <rdf:Description rdf:about="http://emmo.info/emmo/middle/math#EMMO_06658d8d_dcde_4fc9_aae1_17f71c0bcdec">
    <rdf:type rdf:resource="http://www.w3.org/2002/07/owl#Class"/>
    <rdfs:label xml:lang="en">Vector</rdfs:label>
    <rdfs:subClassOf rdf:resource="http://emmo.info/emmo/top/math#EMMO_28fbea28_2204_4613_87ff_6d877b855fcd"/>
  </rdf:Description>
  <rdf:Description rdf:nodeID="N1627f4bbf5cf4ff6a87adff4d0afc3bf">
    <owl:intersectionOf rdf:nodeID="N078928430ee94cc088eba0d56878a03f"/>
    <rdf:type rdf:resource="http://www.w3.org/2002/07/owl#Class"/>
  </rdf:Description>
  <rdf:Description rdf:nodeID="N66868a39fbab416e875d20a8ccac083f">
    <rdf:type rdf:resource="http://www.w3.org/2002/07/owl#Restriction"/>
    <owl:allValuesFrom rdf:nodeID="N25671ebd88ad433baec77dc111e89a0a"/>
    <owl:onProperty rdf:nodeID="Nc9301c0680714f4195f456f618bd444c"/>
  </rdf:Description>
  <rdf:Description rdf:nodeID="N69fb56d8fca147ffb78ab407cb6fc711">
    <rdf:first rdf:resource="http://emmo.info/emmo/middle/isq#EMMO_50bf79a6_a48b_424d_9d2c_813bd631231a"/>
    <rdf:rest rdf:nodeID="Na2312bf9f09c4e308589b2dc84aae0c4"/>
  </rdf:Description>
  <rdf:Description rdf:nodeID="Nd1d5e3a9c46a4f0cb280276de1dda067">
    <rdf:type rdf:resource="http://www.w3.org/2002/07/owl#Class"/>
    <owl:complementOf rdf:resource="http://emmo.info/emmo/middle/metrology#EMMO_7d2afa66_ae9e_4095_a9bf_421d0be401b6"/>
  </rdf:Description>
  <rdf:Description rdf:nodeID="Naf03a81efaf84d808cfc3c64d9a06ecf">
    <owl:hasValue rdf:datatype="http://www.w3.org/2001/XMLSchema#decimal">1E+3</owl:hasValue>
    <rdf:type rdf:resource="http://www.w3.org/2002/07/owl#Restriction"/>
    <owl:onProperty rdf:resource="http://emmo.info/emmo/middle/math#EMMO_faf79f53_749d_40b2_807c_d34244c192f4"/>
  </rdf:Description>
  <rdf:Description rdf:nodeID="Nf11889e15419468893752f7c5181e1d5">
    <owl:inverseOf rdf:resource="http://emmo.info/emmo/middle/holistic#EMMO_ae2d1a96_bfa1_409a_a7d2_03d69e8a125a"/>
  </rdf:Description>
  <rdf:Description rdf:nodeID="N8816a3fd6c32403bb32fd8cf0518eea5">
    <rdf:first rdf:resource="http://emmo.info/emmo/middle/siunits#EMMO_a121bb1d_5225_4c78_809b_0268c3012208"/>
    <rdf:rest rdf:nodeID="N32613eb97d9c4309a450edda401aac48"/>
  </rdf:Description>
  <rdf:Description rdf:nodeID="N08bc12d99bb944688c710a985c2b9da6">
    <rdf:rest rdf:nodeID="N43ff929e5cae4d29b49e0f325a8eb9b4"/>
    <rdf:first rdf:resource="http://emmo.info/emmo/middle/siunits#EMMO_60b78cc3_6011_4134_95ab_956f56d4bdc1"/>
  </rdf:Description>
  <rdf:Description rdf:nodeID="Nf10a471b7a3045d986ed2cb682302920">
    <rdf:first rdf:resource="http://emmo.info/emmo/middle/siunits#EMMO_43a6b269_da31_4bb6_a537_c97df4fff32a"/>
    <rdf:rest rdf:nodeID="N80d934556eca424498dcd344c8e366cc"/>
  </rdf:Description>
  <rdf:Description rdf:nodeID="N113f27dc3fa64f50870b640e81e7ce38">
    <owl:inverseOf rdf:resource="http://emmo.info/emmo/middle/holistic#EMMO_c5aae418_1622_4d02_93c5_21159e28e6c1"/>
  </rdf:Description>
  <rdf:Description rdf:about="http://emmo.info/emmo/middle/metrology#EMMO_50a3552e_859a_4ff7_946d_76d537cabce6">
    <annotations:EMMO_967080e5_2f42_4eb2_a3a9_c58143e835f9>A symbol that stands for a concept in the language of the meterological domain of ISO 80000.</annotations:EMMO_967080e5_2f42_4eb2_a3a9_c58143e835f9>
    <owl:equivalentClass rdf:nodeID="N051684c726a546f1a4c75918ab158f90"/>
    <rdfs:subClassOf rdf:nodeID="Nefa181b445e14d808962d8ea81eaf954"/>
    <rdfs:label xml:lang="en">MetrologicalSymbol</rdfs:label>
    <rdf:type rdf:resource="http://www.w3.org/2002/07/owl#Class"/>
  </rdf:Description>
  <rdf:Description rdf:nodeID="N476be3bb85344473bfd24343c5f124d9">
    <owl:onProperty rdf:resource="http://emmo.info/emmo/middle/metrology#EMMO_67fc0a36_8dcb_4ffa_9a43_31074efa3296"/>
    <rdf:type rdf:resource="http://www.w3.org/2002/07/owl#Restriction"/>
    <owl:allValuesFrom rdf:nodeID="N728c9572118f4bb9a8b615cca11715a5"/>
  </rdf:Description>
  <rdf:Description rdf:about="http://emmo.info/emmo/middle/properties#EMMO_10a5fd39_06aa_4648_9e70_f962a9cb2069">
    <rdf:type rdf:resource="http://www.w3.org/2002/07/owl#Class"/>
    <rdfs:label xml:lang="en">Observation</rdfs:label>
    <rdfs:subClassOf rdf:nodeID="N71dc8b6f026b4de9bab26ed993f83d5a"/>
    <rdfs:subClassOf rdf:resource="http://emmo.info/emmo/top/semiotics#EMMO_008fd3b2_4013_451f_8827_52bceab11841"/>
    <annotations:EMMO_967080e5_2f42_4eb2_a3a9_c58143e835f9>A 'Semiosis' that involves an 'Observer' that perceives another 'Physical' (the 'Object') through a specific perception mechanism and produces a 'Property' (the 'Sign') that stands for the result of that particular perception.</annotations:EMMO_967080e5_2f42_4eb2_a3a9_c58143e835f9>
    <rdfs:subClassOf rdf:nodeID="N9f9c4e7d20084ff5b78c89275d562fab"/>
  </rdf:Description>
  <rdf:Description rdf:nodeID="N40bd2d5d5a134293b5554f0120a75b2d">
    <owl:onProperty rdf:resource="http://emmo.info/emmo/middle/holistic#EMMO_c5aae418_1622_4d02_93c5_21159e28e6c1"/>
    <owl:someValuesFrom rdf:resource="http://emmo.info/emmo/middle/manufacturing#EMMO_86ca9b93_1183_4b65_81b8_c0fcd3bba5ad"/>
    <rdf:type rdf:resource="http://www.w3.org/2002/07/owl#Restriction"/>
  </rdf:Description>
  <rdf:Description rdf:nodeID="N95847686951b4b4d822339dd292787f1">
    <rdf:rest rdf:nodeID="N7132f0759b42496c9b9ad311ea575186"/>
    <rdf:first rdf:resource="http://emmo.info/emmo/middle/siunits#EMMO_3a185e6c_9e19_4776_b583_19c978156aa0"/>
  </rdf:Description>
  <rdf:Description rdf:nodeID="N69dcaf8a790d447da829106d16118891">
    <rdf:first rdf:resource="http://emmo.info/emmo/middle/siunits#EMMO_e79c62ff_10ad_4ec0_baba_c19ddd4eaa11"/>
    <rdf:rest rdf:nodeID="N0e57a41415a2428998b9874866c72a3f"/>
  </rdf:Description>
  <rdf:Description rdf:nodeID="N37bc04a1a37044d08f4fe35e3c69279f">
    <owl:inverseOf rdf:resource="http://emmo.info/emmo/middle/math#EMMO_3446e167_c576_49d6_846c_215bb8878a55"/>
  </rdf:Description>
  <rdf:Description rdf:nodeID="N4ee846b515ab4de8b9dce6a8b778cc26">
    <rdf:rest rdf:nodeID="Nf051248ee1744d0c847c033e48c1a529"/>
    <rdf:first rdf:resource="http://emmo.info/emmo/middle/metrology#EMMO_3ee80521_3c23_4dd1_935d_9d522614a3e2"/>
  </rdf:Description>
  <rdf:Description rdf:about="http://emmo.info/emmo/middle/perceptual#EMMO_25f5ca8e_8f7f_44d8_a392_bd3fe8894458">
    <rdfs:subClassOf rdf:resource="http://emmo.info/emmo/middle/perceptual#EMMO_9268958f_7f54_48ab_a693_febe2645892b"/>
    <rdf:type rdf:resource="http://www.w3.org/2002/07/owl#Class"/>
    <rdfs:label xml:lang="en">Plane</rdfs:label>
  </rdf:Description>
  <rdf:Description rdf:nodeID="N5ab6604471ad40efa6990358a91c3eb3">
    <rdf:first rdf:resource="http://emmo.info/emmo/top/physical#EMMO_29072ec4_ffcb_42fb_bdc7_26f05a2e9873"/>
    <rdf:rest rdf:nodeID="Nb6260f9075384ff8acbcceb1854ce287"/>
  </rdf:Description>
  <rdf:Description rdf:about="http://emmo.info/emmo/middle/siunits#EMMO_f5769206_9257_4b08_bf7b_dad7868c6afc">
    <rdfs:label xml:lang="en">Yocto</rdfs:label>
    <rdfs:subClassOf rdf:nodeID="Nb5c1a55854134ff78c8b240a99eff7cd"/>
    <rdf:type rdf:resource="http://www.w3.org/2002/07/owl#Class"/>
    <rdfs:subClassOf rdf:nodeID="N69233c4d75eb4c908d964a7ec5d39ffa"/>
  </rdf:Description>
  <rdf:Description rdf:nodeID="N6878eb1d48a84e6ba067894a6fbaded9">
    <owl:allValuesFrom rdf:resource="http://emmo.info/emmo/middle/isq#EMMO_321af35f_f0cc_4a5c_b4fe_8c2c0303fb0c"/>
    <rdf:type rdf:resource="http://www.w3.org/2002/07/owl#Restriction"/>
    <owl:onProperty rdf:resource="http://emmo.info/emmo/middle/metrology#EMMO_bed1d005_b04e_4a90_94cf_02bc678a8569"/>
  </rdf:Description>
  <rdf:Description rdf:about="http://emmo.info/emmo/middle/math#EMMO_faf79f53_749d_40b2_807c_d34244c192f4">
    <rdf:type rdf:resource="http://www.w3.org/2002/07/owl#DatatypeProperty"/>
    <rdfs:label xml:lang="en">hasNumericalData</rdfs:label>
    <rdfs:subPropertyOf rdf:resource="http://www.w3.org/2002/07/owl#topDataProperty"/>
    <rdfs:domain rdf:resource="http://emmo.info/emmo/middle/math#EMMO_4ce76d7f_03f8_45b6_9003_90052a79bfaa"/>
  </rdf:Description>
  <rdf:Description rdf:nodeID="Ne2c8041f5db64d61b21c5d8eecdcb3a3">
    <rdf:rest rdf:nodeID="Nf10a471b7a3045d986ed2cb682302920"/>
    <rdf:first rdf:resource="http://emmo.info/emmo/middle/siunits#EMMO_42955b2d_b465_4666_86cc_ea3c2d685753"/>
  </rdf:Description>
  <rdf:Description rdf:nodeID="N09e41b84bb734043b608cbda97f6410d">
    <owl:hasValue>T-3 L+2 M+1 I-1 Θ0 N0 J0</owl:hasValue>
    <rdf:type rdf:resource="http://www.w3.org/2002/07/owl#Restriction"/>
    <owl:onProperty rdf:resource="http://emmo.info/emmo/middle/perceptual#EMMO_23b579e1_8088_45b5_9975_064014026c42"/>
  </rdf:Description>
  <rdf:Description rdf:nodeID="Na4f80bee6cca453ba406917c43e02a5e">
    <rdf:first rdf:resource="http://emmo.info/emmo/middle/siunits#EMMO_1181c938_c8f0_4ad6_bc7a_2bfdc0903d29"/>
    <rdf:rest rdf:nodeID="N1253ed78d81c4d68b74171395295b153"/>
  </rdf:Description>
  <rdf:Description rdf:about="http://emmo.info/emmo/middle/isq#EMMO_847f1d9f_205e_46c1_8cb6_a9e479421f88">
    <rdfs:label xml:lang="en">SquareLengthPerSquareTimeDimension</rdfs:label>
    <rdf:type rdf:resource="http://www.w3.org/2002/07/owl#Class"/>
    <owl:equivalentClass rdf:nodeID="N793139cd06954ec39efb49901c758a1b"/>
    <rdfs:subClassOf rdf:resource="http://emmo.info/emmo/middle/metrology#EMMO_9895a1b4_f0a5_4167_ac5e_97db40b8bfcc"/>
  </rdf:Description>
  <rdf:Description rdf:nodeID="N3e9603d50f954b5c909f54b501890555">
    <owl:allValuesFrom rdf:resource="http://www.w3.org/2001/XMLSchema#double"/>
    <rdf:type rdf:resource="http://www.w3.org/2002/07/owl#Restriction"/>
    <owl:onProperty rdf:resource="http://emmo.info/emmo/middle/math#EMMO_faf79f53_749d_40b2_807c_d34244c192f4"/>
  </rdf:Description>
  <rdf:Description rdf:nodeID="Na4369ab9b95d4d24b142c11880cf2a0d">
    <owl:complementOf rdf:nodeID="Nf1f45c66a1dd4b8eb8f57650e0b8f870"/>
    <rdf:type rdf:resource="http://www.w3.org/2002/07/owl#Class"/>
  </rdf:Description>
  <rdf:Description rdf:about="http://emmo.info/emmo/middle/isq#EMMO_ce7d4720_aa20_4a8c_93e8_df41a35b6723">
    <rdfs:label xml:lang="en">AmountPerTimeDimension</rdfs:label>
    <rdf:type rdf:resource="http://www.w3.org/2002/07/owl#Class"/>
    <owl:equivalentClass rdf:nodeID="N0bd75e9d4e1c4ab5a6ff6dd1d346df36"/>
    <rdfs:subClassOf rdf:resource="http://emmo.info/emmo/middle/metrology#EMMO_9895a1b4_f0a5_4167_ac5e_97db40b8bfcc"/>
  </rdf:Description>
  <rdf:Description rdf:nodeID="N4a66e753f9e749abb354adc6309f441b">
    <rdf:first rdf:resource="http://emmo.info/emmo/middle/siunits#EMMO_d7b7fd1e_645a_42cb_8f40_85f0d034d3ae"/>
    <rdf:rest rdf:nodeID="N39692b988209468e971afa9080334da3"/>
  </rdf:Description>
  <rdf:Description rdf:nodeID="Nd00f08e47d5c4f7c89d89405ac36d25e">
    <rdf:type rdf:resource="http://www.w3.org/2002/07/owl#Restriction"/>
    <owl:onProperty rdf:resource="http://emmo.info/emmo/middle/metrology#EMMO_bed1d005_b04e_4a90_94cf_02bc678a8569"/>
    <owl:someValuesFrom rdf:resource="http://emmo.info/emmo/middle/isq#EMMO_c8d084ad_f88e_4596_8e4d_982c6655ce6f"/>
  </rdf:Description>
  <rdf:Description rdf:nodeID="N7ab01d3cc65045949f797c724c357d8c">
    <owl:allValuesFrom rdf:resource="http://emmo.info/emmo/middle/isq#EMMO_585e0ff0_9429_4d3c_b578_58abb1ba21d1"/>
    <rdf:type rdf:resource="http://www.w3.org/2002/07/owl#Restriction"/>
    <owl:onProperty rdf:resource="http://emmo.info/emmo/middle/metrology#EMMO_bed1d005_b04e_4a90_94cf_02bc678a8569"/>
  </rdf:Description>
  <rdf:Description rdf:nodeID="N7928dfd0dbe9469c9055155fd87ba720">
    <rdf:type rdf:resource="http://www.w3.org/2002/07/owl#Restriction"/>
    <owl:onProperty rdf:resource="http://emmo.info/emmo/middle/metrology#EMMO_67fc0a36_8dcb_4ffa_9a43_31074efa3296"/>
    <owl:allValuesFrom rdf:nodeID="Nef79e15b8fc34f4da019ca456a7df6fc"/>
  </rdf:Description>
  <rdf:Description rdf:about="http://emmo.info/emmo/middle/siunits#EMMO_f96feb3f_4438_4e43_aa44_7458c4d87fc2">
    <rdf:type rdf:resource="http://www.w3.org/2002/07/owl#Class"/>
    <annotations:EMMO_967080e5_2f42_4eb2_a3a9_c58143e835f9>The frequency standard in the SI system in which the photon absorption by transitions between the two hyperfine ground states of caesium-133 atoms are used to control the output frequency.</annotations:EMMO_967080e5_2f42_4eb2_a3a9_c58143e835f9>
    <rdfs:label xml:lang="en">HyperfineTransitionFrequencyOfCs</rdfs:label>
    <rdfs:subClassOf rdf:resource="http://emmo.info/emmo/middle/isq#EMMO_852b4ab8_fc29_4749_a8c7_b92d4fca7d5a"/>
  </rdf:Description>
  <rdf:Description rdf:nodeID="N350972ab9c7d475b90d6c52413ceca1c">
    <rdf:type rdf:resource="http://www.w3.org/2002/07/owl#Restriction"/>
    <owl:onProperty rdf:resource="http://emmo.info/emmo/middle/metrology#EMMO_8ef3cd6d_ae58_4a8d_9fc0_ad8f49015cd0"/>
    <owl:qualifiedCardinality rdf:datatype="http://www.w3.org/2001/XMLSchema#nonNegativeInteger">1</owl:qualifiedCardinality>
    <owl:onClass rdf:resource="http://emmo.info/emmo/middle/math#EMMO_4ce76d7f_03f8_45b6_9003_90052a79bfaa"/>
  </rdf:Description>
  <rdf:Description rdf:about="http://emmo.info/emmo/top/annotations#EMMO_5525a055_dda5_4556_8b91_f0d22fa676cc">
    <rdf:type rdf:resource="http://www.w3.org/2002/07/owl#AnnotationProperty"/>
    <rdfs:subPropertyOf rdf:resource="http://www.w3.org/2000/01/rdf-schema#comment"/>
    <rdfs:label xml:lang="en">license</rdfs:label>
  </rdf:Description>
  <rdf:Description rdf:nodeID="N374b36162464401b92367b3ea76630fc">
    <rdf:type rdf:resource="http://www.w3.org/2002/07/owl#Restriction"/>
    <owl:onProperty rdf:resource="http://emmo.info/emmo/middle/reductionistic#EMMO_b2282816_b7a3_44c6_b2cb_3feff1ceb7fe"/>
    <owl:someValuesFrom rdf:resource="http://emmo.info/emmo/middle/physicalistic#EMMO_8043d3c6_a4c1_4089_ba34_9744e28e5b3d"/>
  </rdf:Description>
  <rdf:Description rdf:about="http://emmo.info/emmo/middle/reductionistic#EMMO_663859e5_add3_4c9e_96fb_c99399de278d">
    <rdf:type rdf:resource="http://www.w3.org/2002/07/owl#AsymmetricProperty"/>
    <rdfs:subPropertyOf rdf:resource="http://emmo.info/emmo/top/physical#EMMO_6e046dd0_9634_4013_b2b1_9cc468087c83"/>
    <rdf:type rdf:resource="http://www.w3.org/2002/07/owl#IrreflexiveProperty"/>
    <rdf:type rdf:resource="http://www.w3.org/2002/07/owl#InverseFunctionalProperty"/>
    <rdfs:label xml:lang="en">hasSpatioTemporalDirectPart</rdfs:label>
    <rdf:type rdf:resource="http://www.w3.org/2002/07/owl#ObjectProperty"/>
  </rdf:Description>
  <rdf:Description rdf:about="http://emmo.info/emmo/middle/siunits#EMMO_471cb92b_edca_4cf9_bce8_a75084d876b8">
    <rdfs:subClassOf rdf:resource="http://emmo.info/emmo/middle/metrology#EMMO_7d2afa66_ae9e_4095_a9bf_421d0be401b6"/>
    <rdf:type rdf:resource="http://www.w3.org/2002/07/owl#Class"/>
    <rdfs:label xml:lang="en">SIMetricPrefix</rdfs:label>
    <owl:disjointUnionOf rdf:nodeID="N5a84054aa4be46b8bb0d9e9b42106348"/>
  </rdf:Description>
  <rdf:Description rdf:nodeID="Na563f81676d04624a4f83ce0ccd7fe4b">
    <owl:onProperty rdf:resource="http://emmo.info/emmo/middle/perceptual#EMMO_23b579e1_8088_45b5_9975_064014026c42"/>
    <owl:hasValue>-</owl:hasValue>
    <rdf:type rdf:resource="http://www.w3.org/2002/07/owl#Restriction"/>
  </rdf:Description>
  <rdf:Description rdf:about="http://emmo.info/emmo/middle/siunits#EMMO_9ff3bf8e_2168_406e_8251_1d158fc948ae">
    <rdfs:subClassOf rdf:nodeID="Nac818dfa7e4442939688b1ec1fe07bd3"/>
    <rdfs:label xml:lang="en">Micro</rdfs:label>
    <rdf:type rdf:resource="http://www.w3.org/2002/07/owl#Class"/>
    <rdfs:subClassOf rdf:nodeID="Nf9543181733a48cb80b16c34a902f1c2"/>
  </rdf:Description>
  <rdf:Description rdf:nodeID="Nec607c9ad5ba47f796aa9ad684514c83">
    <rdf:first rdf:resource="http://emmo.info/emmo/top/semiotics#EMMO_b21a56ed_f969_4612_a6ec_cb7766f7f31d"/>
    <rdf:rest rdf:resource="http://www.w3.org/1999/02/22-rdf-syntax-ns#nil"/>
  </rdf:Description>
  <rdf:Description rdf:nodeID="N66e2d71f279c4c5f99d44916701d2d9b">
    <rdf:type rdf:resource="http://www.w3.org/2002/07/owl#Restriction"/>
    <owl:hasValue rdf:datatype="http://www.w3.org/2001/XMLSchema#decimal">1E-24</owl:hasValue>
    <owl:onProperty rdf:resource="http://emmo.info/emmo/middle/math#EMMO_faf79f53_749d_40b2_807c_d34244c192f4"/>
  </rdf:Description>
  <rdf:Description rdf:nodeID="N9f9c4e7d20084ff5b78c89275d562fab">
    <rdf:type rdf:resource="http://www.w3.org/2002/07/owl#Restriction"/>
    <owl:onProperty rdf:resource="http://emmo.info/emmo/middle/holistic#EMMO_ae2d1a96_bfa1_409a_a7d2_03d69e8a125a"/>
    <owl:someValuesFrom rdf:resource="http://emmo.info/emmo/middle/properties#EMMO_1b52ee70_121e_4d8d_8419_3f97cd0bd89c"/>
  </rdf:Description>
  <rdf:Description rdf:nodeID="N01254d1904484e50ae6af7e63289f9a0">
    <owl:inverseOf rdf:resource="http://emmo.info/emmo/middle/math#EMMO_3446e167_c576_49d6_846c_215bb8878a55"/>
  </rdf:Description>
  <rdf:Description rdf:nodeID="Nd10ca18d7e7549b597060c6d52aa49e0">
    <rdf:first rdf:resource="http://emmo.info/emmo/middle/properties#EMMO_d8aa8e1f_b650_416d_88a0_5118de945456"/>
    <rdf:rest rdf:resource="http://www.w3.org/1999/02/22-rdf-syntax-ns#nil"/>
  </rdf:Description>
  <rdf:Description rdf:nodeID="N5e7de695618f44cabf297789a7bd673c">
    <rdf:rest rdf:nodeID="N185e1b467bd64e3cb671664cc3d135e2"/>
    <rdf:first rdf:resource="http://emmo.info/emmo/middle/siunits#EMMO_76cc4efc_231e_42b4_be83_2547681caed6"/>
  </rdf:Description>
  <rdf:Description rdf:nodeID="Nac3248cba359458e95504df745526bbb">
    <rdf:type rdf:resource="http://www.w3.org/2002/07/owl#Restriction"/>
    <owl:onProperty rdf:resource="http://emmo.info/emmo/top/mereotopology#EMMO_17e27c22_37e1_468c_9dd7_95e137f73e7f"/>
    <owl:someValuesFrom rdf:resource="http://emmo.info/emmo/middle/physicalistic#EMMO_e5488299_8dab_4ebb_900a_26d2abed8396"/>
  </rdf:Description>
  <rdf:Description rdf:nodeID="N468c5596198c4b6fb957712bbc98b19b">
    <owl:onProperty rdf:resource="http://emmo.info/emmo/top/physical#EMMO_7afbed84_7593_4a23_bd88_9d9c6b04e8f6"/>
    <rdf:type rdf:resource="http://www.w3.org/2002/07/owl#Restriction"/>
    <owl:allValuesFrom rdf:resource="http://emmo.info/emmo/middle/physicalistic#EMMO_5b2222df_4da6_442f_8244_96e9e45887d1"/>
  </rdf:Description>
  <rdf:Description rdf:about="http://emmo.info/emmo/top/annotations#EMMO_6dd685dd_1895_46e4_b227_be9f7d643c25">
    <rdfs:subPropertyOf rdf:resource="http://www.w3.org/2000/01/rdf-schema#seeAlso"/>
    <rdfs:label xml:lang="en">dbpediaMatch</rdfs:label>
    <rdfs:comment>URL to corresponding concept in DBpedia.</rdfs:comment>
    <rdfs:seeAlso>https://wiki.dbpedia.org/</rdfs:seeAlso>
    <rdf:type rdf:resource="http://www.w3.org/2002/07/owl#AnnotationProperty"/>
  </rdf:Description>
  <rdf:Description rdf:nodeID="N926b5b8edc6f4dcc898644d3eeea068a">
    <rdf:rest rdf:nodeID="Nfdee2fb24c934a58964e557deeda2282"/>
    <rdf:first rdf:resource="http://emmo.info/emmo/middle/isq#EMMO_d4f7d378_5e3b_468a_baa1_a7e98358cda7"/>
  </rdf:Description>
  <rdf:Description rdf:nodeID="N827028b4dd5f475da6fb66673ade2d27">
    <rdf:type rdf:resource="http://www.w3.org/2002/07/owl#Restriction"/>
    <owl:hasValue>W</owl:hasValue>
    <owl:onProperty rdf:resource="http://emmo.info/emmo/middle/perceptual#EMMO_23b579e1_8088_45b5_9975_064014026c42"/>
  </rdf:Description>
  <rdf:Description rdf:about="http://emmo.info/emmo/middle/math#EMMO_707f0cd1_941c_4b57_9f20_d0ba30cd6ff3">
    <rdfs:label xml:lang="en">ArithmeticOperator</rdfs:label>
    <rdfs:subClassOf rdf:resource="http://emmo.info/emmo/top/math#EMMO_3c424d37_cf62_41b1_ac9d_a316f8d113d6"/>
    <rdf:type rdf:resource="http://www.w3.org/2002/07/owl#Class"/>
  </rdf:Description>
  <rdf:Description rdf:nodeID="Nafb46c4d4e1b4a4da33513592ab4a5b7">
    <owl:onProperty rdf:nodeID="N14c80c6bc107456993fc9f9bbe3bb062"/>
    <owl:someValuesFrom rdf:resource="http://emmo.info/emmo/top/semiotics#EMMO_6f5af708_f825_4feb_a0d1_a8d813d3022b"/>
    <rdf:type rdf:resource="http://www.w3.org/2002/07/owl#Restriction"/>
  </rdf:Description>
  <rdf:Description rdf:nodeID="N9c7c783836324422bec68ae085446692">
    <rdf:type rdf:resource="http://www.w3.org/2002/07/owl#Restriction"/>
    <owl:allValuesFrom rdf:nodeID="N6878eb1d48a84e6ba067894a6fbaded9"/>
    <owl:onProperty rdf:resource="http://emmo.info/emmo/middle/metrology#EMMO_67fc0a36_8dcb_4ffa_9a43_31074efa3296"/>
  </rdf:Description>
  <rdf:Description rdf:about="http://emmo.info/emmo/middle/isq#EMMO_515b5579_d526_4842_9e6f_ecc34db6f368">
    <owl:equivalentClass rdf:nodeID="N0e3e37822c234168a7038868088ca604"/>
    <rdf:type rdf:resource="http://www.w3.org/2002/07/owl#Class"/>
    <rdfs:subClassOf rdf:resource="http://emmo.info/emmo/middle/metrology#EMMO_9895a1b4_f0a5_4167_ac5e_97db40b8bfcc"/>
    <rdfs:label xml:lang="en">PerTimeDimension</rdfs:label>
  </rdf:Description>
  <rdf:Description rdf:nodeID="N6f9e72c556084dc1843c76f1bb7b9c99">
    <owl:onProperty rdf:resource="http://emmo.info/emmo/middle/metrology#EMMO_bed1d005_b04e_4a90_94cf_02bc678a8569"/>
    <owl:someValuesFrom rdf:resource="http://emmo.info/emmo/middle/isq#EMMO_321af35f_f0cc_4a5c_b4fe_8c2c0303fb0c"/>
    <rdf:type rdf:resource="http://www.w3.org/2002/07/owl#Restriction"/>
  </rdf:Description>
  <rdf:Description rdf:nodeID="N0793b95df1d9475695833e1a6efc04c1">
    <rdf:type rdf:resource="http://www.w3.org/2002/07/owl#Restriction"/>
    <owl:onProperty rdf:resource="http://emmo.info/emmo/middle/metrology#EMMO_bed1d005_b04e_4a90_94cf_02bc678a8569"/>
    <owl:allValuesFrom rdf:resource="http://emmo.info/emmo/middle/isq#EMMO_ec903946_ddc9_464a_903c_7373e0d1eeb5"/>
  </rdf:Description>
  <rdf:Description rdf:nodeID="Nb53716dfe0334ecd9d068dcb19bef884">
    <owl:onProperty rdf:resource="http://emmo.info/emmo/middle/perceptual#EMMO_23b579e1_8088_45b5_9975_064014026c42"/>
    <owl:hasValue>T-3 L+2 M+1 I0 Θ0 N0 J0</owl:hasValue>
    <rdf:type rdf:resource="http://www.w3.org/2002/07/owl#Restriction"/>
  </rdf:Description>
  <rdf:Description rdf:nodeID="N42e044b0c0af4bb5a21c24e09a9f20f1">
    <rdf:first rdf:resource="http://emmo.info/emmo/middle/siunits#EMMO_8a70dea4_d6ab_4260_b931_a3e990982416"/>
    <rdf:rest rdf:nodeID="N8816a3fd6c32403bb32fd8cf0518eea5"/>
  </rdf:Description>
  <rdf:Description rdf:nodeID="N1375e20c0adb447c8047a350ad3817a0">
    <rdf:type rdf:resource="http://www.w3.org/2002/07/owl#Restriction"/>
    <owl:someValuesFrom rdf:resource="http://emmo.info/emmo/middle/metrology#EMMO_02c0621e_a527_4790_8a0f_2bb51973c819"/>
    <owl:onProperty rdf:resource="http://emmo.info/emmo/middle/reductionistic#EMMO_b2282816_b7a3_44c6_b2cb_3feff1ceb7fe"/>
  </rdf:Description>
  <rdf:Description rdf:nodeID="Nff4876241e8046a0b5fe214366a39bea">
    <rdf:type rdf:resource="http://www.w3.org/2002/07/owl#Restriction"/>
    <owl:onProperty rdf:resource="http://emmo.info/emmo/middle/perceptual#EMMO_23b579e1_8088_45b5_9975_064014026c42"/>
    <owl:hasValue>T-1 L+1 M0 I0 Θ0 N0 J0</owl:hasValue>
  </rdf:Description>
  <rdf:Description rdf:nodeID="Nb8059d442eac4bb48921cdca102ee61e">
    <owl:someValuesFrom rdf:resource="http://emmo.info/emmo/middle/isq#EMMO_14ff4393_0f28_4fb4_abc7_c2cc00bc761d"/>
    <rdf:type rdf:resource="http://www.w3.org/2002/07/owl#Restriction"/>
    <owl:onProperty rdf:resource="http://emmo.info/emmo/middle/metrology#EMMO_bed1d005_b04e_4a90_94cf_02bc678a8569"/>
  </rdf:Description>
  <rdf:Description rdf:nodeID="Nee74f87cd8654a3cab7c34c85a942acf">
    <rdf:first rdf:resource="http://emmo.info/emmo/middle/siunits#EMMO_e9ffc696_5228_4ff9_8a60_0f5e05e9931b"/>
    <rdf:rest rdf:resource="http://www.w3.org/1999/02/22-rdf-syntax-ns#nil"/>
  </rdf:Description>
  <rdf:Description rdf:nodeID="Na96d5d7f393d4e26b6bbf71e75638a50">
    <owl:hasValue rdf:datatype="http://www.w3.org/2001/XMLSchema#decimal">0.001</owl:hasValue>
    <rdf:type rdf:resource="http://www.w3.org/2002/07/owl#Restriction"/>
    <owl:onProperty rdf:resource="http://emmo.info/emmo/middle/math#EMMO_faf79f53_749d_40b2_807c_d34244c192f4"/>
  </rdf:Description>
  <rdf:Description rdf:nodeID="Nefa181b445e14d808962d8ea81eaf954">
    <rdf:type rdf:resource="http://www.w3.org/2002/07/owl#Restriction"/>
    <owl:allValuesFrom rdf:nodeID="Nd43b659b71cd4664aa83407e427a38a1"/>
    <owl:onProperty rdf:resource="http://emmo.info/emmo/top/mereotopology#EMMO_9380ab64_0363_4804_b13f_3a8a94119a76"/>
  </rdf:Description>
  <rdf:Description rdf:nodeID="N2c55cf9c462241b288883dd8516cf2bc">
    <rdf:rest rdf:nodeID="N19a634e0ce894273916bc500c00fbc73"/>
    <rdf:first rdf:resource="http://emmo.info/emmo/middle/physicalistic#EMMO_72d53756_7fb1_46ed_980f_83f47efbe105"/>
  </rdf:Description>
  <rdf:Description rdf:nodeID="N22067548347643179344ff5d615c234a">
    <rdf:type rdf:resource="http://www.w3.org/2002/07/owl#Restriction"/>
    <owl:allValuesFrom rdf:nodeID="N1aceac02b7f945729f6c0b4fa2353131"/>
    <owl:onProperty rdf:resource="http://emmo.info/emmo/middle/metrology#EMMO_67fc0a36_8dcb_4ffa_9a43_31074efa3296"/>
  </rdf:Description>
  <rdf:Description rdf:nodeID="N0941101840144fa880ae50651e03577a">
    <rdf:type rdf:resource="http://www.w3.org/2002/07/owl#Restriction"/>
    <owl:onProperty rdf:resource="http://emmo.info/emmo/middle/perceptual#EMMO_23b579e1_8088_45b5_9975_064014026c42"/>
    <owl:hasValue>H</owl:hasValue>
  </rdf:Description>
  <rdf:Description rdf:nodeID="N31f67ad3d791498fa91b473e84706c7a">
    <owl:onProperty rdf:resource="http://emmo.info/emmo/middle/perceptual#EMMO_23b579e1_8088_45b5_9975_064014026c42"/>
    <rdf:type rdf:resource="http://www.w3.org/2002/07/owl#Restriction"/>
    <owl:hasValue>Ω</owl:hasValue>
  </rdf:Description>
  <rdf:Description rdf:nodeID="Nd551a59d627b4c9fa94beab213658180">
    <rdf:type rdf:resource="http://www.w3.org/2002/07/owl#Restriction"/>
    <owl:onProperty rdf:resource="http://emmo.info/emmo/middle/perceptual#EMMO_23b579e1_8088_45b5_9975_064014026c42"/>
    <owl:hasValue>S</owl:hasValue>
  </rdf:Description>
  <rdf:Description rdf:nodeID="N6fb0d68dd5284ea5ab9bbd8ddf81d6ad">
    <owl:inverseOf rdf:resource="http://emmo.info/emmo/middle/math#EMMO_3446e167_c576_49d6_846c_215bb8878a55"/>
  </rdf:Description>
  <rdf:Description rdf:about="http://emmo.info/emmo/top/annotations#EMMO_967080e5_2f42_4eb2_a3a9_c58143e835f9">
    <rdf:type rdf:resource="http://www.w3.org/2002/07/owl#AnnotationProperty"/>
    <rdfs:label xml:lang="en">elucidation</rdfs:label>
    <rdfs:subPropertyOf rdf:resource="http://www.w3.org/2000/01/rdf-schema#comment"/>
  </rdf:Description>
  <rdf:Description rdf:nodeID="N0cba766ba19a4a239eb78d3e3a35be3a">
    <rdf:type rdf:resource="http://www.w3.org/2002/07/owl#Class"/>
    <owl:unionOf rdf:nodeID="N2db0feed6510454e82a1b1e38e33019f"/>
  </rdf:Description>
  <rdf:Description rdf:about="http://emmo.info/emmo/middle/perceptual#EMMO_39362460_2a97_4367_8f93_0418c2ac9a08">
    <rdfs:label xml:lang="en">Point</rdfs:label>
    <rdfs:subClassOf rdf:resource="http://emmo.info/emmo/middle/perceptual#EMMO_0ab0485c_9e5b_4257_a679_90a2dfba5c7c"/>
    <rdf:type rdf:resource="http://www.w3.org/2002/07/owl#Class"/>
  </rdf:Description>
  <rdf:Description rdf:nodeID="N2343adef8e1544988995c7e2cdc4baa5">
    <owl:inverseOf rdf:resource="http://emmo.info/emmo/middle/math#EMMO_3446e167_c576_49d6_846c_215bb8878a55"/>
  </rdf:Description>
  <rdf:Description rdf:nodeID="Naaf7bd1e64944343a2135c509a123c78">
    <rdf:rest rdf:nodeID="Nd134427b98f44841af80457a655f4706"/>
    <rdf:first rdf:resource="http://emmo.info/emmo/middle/math#EMMO_54ee6b5e_5261_44a8_86eb_5717e7fdb9d0"/>
  </rdf:Description>
  <rdf:Description rdf:nodeID="N1b3cb51adedd4fd18838c5f72b2105ba">
    <rdf:first rdf:resource="http://emmo.info/emmo/middle/siunits#EMMO_da1dd4a7_c611_4ad4_bef6_7646f28aa598"/>
    <rdf:rest rdf:nodeID="N6c0f2e6691204a399713f4e206931923"/>
  </rdf:Description>
  <rdf:Description rdf:nodeID="N11e7563c445748fbb7061dd5cdd28b49">
    <rdf:type rdf:resource="http://www.w3.org/2002/07/owl#Restriction"/>
    <owl:hasValue>T0 L0 M0 I0 Θ+1 N0 J0</owl:hasValue>
    <owl:onProperty rdf:resource="http://emmo.info/emmo/middle/perceptual#EMMO_23b579e1_8088_45b5_9975_064014026c42"/>
  </rdf:Description>
  <rdf:Description rdf:nodeID="N14380958a6f14b4a956fed9d59ba6227">
    <rdf:rest rdf:nodeID="N3becdf78fa194df281c8613a0d92187e"/>
    <rdf:first rdf:resource="http://emmo.info/emmo/middle/properties#EMMO_251cfb4f_5c75_4778_91ed_6c8395212fd8"/>
  </rdf:Description>
  <rdf:Description rdf:nodeID="Ne65de8e5f00d4f539917d8a85df3a967">
    <rdf:type rdf:resource="http://www.w3.org/2002/07/owl#Restriction"/>
    <owl:onProperty rdf:resource="http://emmo.info/emmo/middle/perceptual#EMMO_23b579e1_8088_45b5_9975_064014026c42"/>
    <owl:hasValue>T-2 L-1 M+1 I0 Θ0 N0 J0</owl:hasValue>
  </rdf:Description>
  <rdf:Description rdf:nodeID="N40b45b9be0f04243b9c6eb3b210f521d">
    <owl:onProperty rdf:resource="http://emmo.info/emmo/middle/perceptual#EMMO_23b579e1_8088_45b5_9975_064014026c42"/>
    <rdf:type rdf:resource="http://www.w3.org/2002/07/owl#Restriction"/>
    <owl:hasValue>µ</owl:hasValue>
  </rdf:Description>
  <rdf:Description rdf:nodeID="Nf2827a71babf4830accc67667c17db0a">
    <rdf:rest rdf:nodeID="N98dab9d34ed04a0b92aeda604b6d3e7d"/>
    <rdf:first rdf:resource="http://emmo.info/emmo/middle/siunits#EMMO_176cae33_b83e_4cd2_a6bc_281f42f0ccc8"/>
  </rdf:Description>
  <rdf:Description rdf:about="http://emmo.info/emmo/middle/manufacturing#EMMO_e775e341_5687_4d45_b50c_379b098a8c26">
    <rdfs:subClassOf rdf:resource="http://emmo.info/emmo/middle/manufacturing#EMMO_86ca9b93_1183_4b65_81b8_c0fcd3bba5ad"/>
    <rdf:type rdf:resource="http://www.w3.org/2002/07/owl#Class"/>
    <rdfs:label xml:lang="en">System</rdfs:label>
    <owl:equivalentClass rdf:nodeID="Nfd269989e79f4d809c092a1a1bd6809b"/>
  </rdf:Description>
  <rdf:Description rdf:nodeID="N328058edab884308be404bbe6696f037">
    <owl:someValuesFrom rdf:resource="http://emmo.info/emmo/middle/materials#EMMO_1067b97a_84f8_4d22_8ace_b842b8ce355c"/>
    <rdf:type rdf:resource="http://www.w3.org/2002/07/owl#Restriction"/>
    <owl:onProperty rdf:resource="http://emmo.info/emmo/middle/reductionistic#EMMO_b2282816_b7a3_44c6_b2cb_3feff1ceb7fe"/>
  </rdf:Description>
  <rdf:Description rdf:nodeID="N3ce6bb3ceca445c6910de9d955c4e75d">
    <rdf:first rdf:resource="http://emmo.info/emmo/middle/siunits#EMMO_254472c6_3dbd_4f02_bc43_571389cd281f"/>
    <rdf:rest rdf:nodeID="N19f583718273476fa52c6b4c94b35b0a"/>
  </rdf:Description>
  <rdf:Description rdf:nodeID="Nf1f45c66a1dd4b8eb8f57650e0b8f870">
    <rdf:type rdf:resource="http://www.w3.org/2002/07/owl#Restriction"/>
    <owl:someValuesFrom rdf:resource="http://emmo.info/emmo/middle/math#EMMO_1eed0732_e3f1_4b2c_a9c4_b4e75eeb5895"/>
    <owl:onProperty rdf:resource="http://emmo.info/emmo/middle/reductionistic#EMMO_b2282816_b7a3_44c6_b2cb_3feff1ceb7fe"/>
  </rdf:Description>
  <rdf:Description rdf:nodeID="Na06d5e54e52c421e83c71776f1807a78">
    <owl:onProperty rdf:resource="http://emmo.info/emmo/middle/perceptual#EMMO_23b579e1_8088_45b5_9975_064014026c42"/>
    <owl:hasValue>/</owl:hasValue>
    <rdf:type rdf:resource="http://www.w3.org/2002/07/owl#Restriction"/>
  </rdf:Description>
  <rdf:Description rdf:about="http://emmo.info/emmo/top/math#EMMO_1aed91a3_d00c_48af_8f43_a0c958b2512a">
    <rdf:type rdf:resource="http://www.w3.org/2002/07/owl#Class"/>
    <annotations:EMMO_b432d2d5_25f4_4165_99c5_5935a7763c1a>2x+3</annotations:EMMO_b432d2d5_25f4_4165_99c5_5935a7763c1a>
    <rdfs:comment>An expression that has parts only integer constants, variables, and the algebraic operations (addition, subtraction, multiplication, division and exponentiation by an exponent that is a rational number)</rdfs:comment>
    <rdfs:subClassOf rdf:resource="http://emmo.info/emmo/middle/math#EMMO_f9bc8b52_85e9_4b53_b969_dd7724d5b8e4"/>
    <rdfs:label xml:lang="en">AlgebricExpression</rdfs:label>
  </rdf:Description>
  <rdf:Description rdf:nodeID="N9b695051987d46818c57eb0927d1fedc">
    <rdf:rest rdf:nodeID="N57bbdcdbc32647b9842700bafab924a8"/>
    <rdf:first rdf:resource="http://emmo.info/emmo/middle/isq#EMMO_affe07e4_e9bc_4852_86c6_69e26182a17f"/>
  </rdf:Description>
  <rdf:Description rdf:nodeID="N08a96502cf384b1dba768582d910bf54">
    <owl:hasValue>m</owl:hasValue>
    <rdf:type rdf:resource="http://www.w3.org/2002/07/owl#Restriction"/>
    <owl:onProperty rdf:resource="http://emmo.info/emmo/middle/perceptual#EMMO_23b579e1_8088_45b5_9975_064014026c42"/>
  </rdf:Description>
  <rdf:Description rdf:nodeID="Nd3c2b89fc9c74e38a4f67fc47ba11ba2">
    <rdf:first rdf:resource="http://emmo.info/emmo/middle/metrology#EMMO_acaaa124_3dde_48b6_86e6_6ec6f364f408"/>
    <rdf:rest rdf:resource="http://www.w3.org/1999/02/22-rdf-syntax-ns#nil"/>
  </rdf:Description>
  <rdf:Description rdf:nodeID="Na82d7e7aaa1d44aaa8e32583a4cc2ce5">
    <rdf:first rdf:resource="http://emmo.info/emmo/middle/siunits#EMMO_e75f580e_52bf_4dd5_af70_df409cec08fd"/>
    <rdf:rest rdf:nodeID="N6d5f90c5888e4cb796229ad933c6c399"/>
  </rdf:Description>
  <rdf:Description rdf:nodeID="Nf3589ffb1cf443308ea993370aed21e9">
    <rdf:type rdf:resource="http://www.w3.org/2002/07/owl#Restriction"/>
    <owl:onProperty rdf:resource="http://emmo.info/emmo/middle/metrology#EMMO_bed1d005_b04e_4a90_94cf_02bc678a8569"/>
    <owl:allValuesFrom rdf:resource="http://emmo.info/emmo/middle/isq#EMMO_4c49ab58_a6f6_409e_b849_f873ae1dcbee"/>
  </rdf:Description>
  <rdf:Description rdf:nodeID="N105c88c61d514bc18291a450942d5d01">
    <rdf:type rdf:resource="http://www.w3.org/2002/07/owl#Restriction"/>
    <owl:onProperty rdf:resource="http://emmo.info/emmo/middle/math#EMMO_faf79f53_749d_40b2_807c_d34244c192f4"/>
    <owl:hasValue rdf:datatype="http://www.w3.org/2001/XMLSchema#decimal">0.1</owl:hasValue>
  </rdf:Description>
  <rdf:Description rdf:about="http://emmo.info/emmo/middle/physicalistic#EMMO_4207e895_8b83_4318_996a_72cfb32acd94">
    <rdf:type rdf:resource="http://www.w3.org/2002/07/owl#Class"/>
    <rdfs:subClassOf rdf:resource="http://emmo.info/emmo/middle/physicalistic#EMMO_5b2222df_4da6_442f_8244_96e9e45887d1"/>
    <rdfs:label xml:lang="en">Material</rdfs:label>
    <annotations:EMMO_967080e5_2f42_4eb2_a3a9_c58143e835f9>A 'Physical' that stands for a real world object that represents an amount of a physical substance (or mixture of substances) that constitute (is part of) a more comprehensive real world object.</annotations:EMMO_967080e5_2f42_4eb2_a3a9_c58143e835f9>
    <rdfs:comment>The definition states that a 'Material' is a portion of a real world object, being that a full functional device or component, or a sample made of that material (or the sample itself).</rdfs:comment>
  </rdf:Description>
  <rdf:Description rdf:nodeID="N09994478a93343b49a8b4f0116175b60">
    <rdf:first rdf:resource="http://emmo.info/emmo/middle/holistic#EMMO_49804605_c0fe_4538_abda_f70ba1dc8a5d"/>
    <rdf:rest rdf:resource="http://www.w3.org/1999/02/22-rdf-syntax-ns#nil"/>
  </rdf:Description>
  <rdf:Description rdf:nodeID="N7481cb046c3747dfb34030da3079ef27">
    <rdf:type rdf:resource="http://www.w3.org/2002/07/owl#Restriction"/>
    <owl:hasValue>s</owl:hasValue>
    <owl:onProperty rdf:resource="http://emmo.info/emmo/middle/perceptual#EMMO_23b579e1_8088_45b5_9975_064014026c42"/>
  </rdf:Description>
  <rdf:Description rdf:about="http://emmo.info/emmo/top/math#EMMO_8de14a59_660b_454f_aff8_76a07ce185f4">
    <rdfs:subClassOf rdf:resource="http://emmo.info/emmo/middle/math#EMMO_707f0cd1_941c_4b57_9f20_d0ba30cd6ff3"/>
    <rdfs:label xml:lang="en">Plus</rdfs:label>
    <rdf:type rdf:resource="http://www.w3.org/2002/07/owl#Class"/>
    <owl:equivalentClass rdf:nodeID="Nf8f7f491de1347758075c0a614f75714"/>
  </rdf:Description>
  <rdf:Description rdf:about="http://emmo.info/emmo/middle/isq#EMMO_50bf79a6_a48b_424d_9d2c_813bd631231a">
    <rdf:type rdf:resource="http://www.w3.org/2002/07/owl#Class"/>
    <rdfs:label xml:lang="en">LuminousIntensity</rdfs:label>
    <annotations:EMMO_6dd685dd_1895_46e4_b227_be9f7d643c25>http://dbpedia.org/page/Luminous_intensity</annotations:EMMO_6dd685dd_1895_46e4_b227_be9f7d643c25>
    <rdfs:subClassOf rdf:nodeID="N0706bf3341e64441809c178882211a20"/>
    <annotations:EMMO_967080e5_2f42_4eb2_a3a9_c58143e835f9>A measure of the wavelength-weighted power emitted by a light source in a particular direction per unit solid angle. It is based on the luminosity function, which is a standardized model of the sensitivity of the human eye.</annotations:EMMO_967080e5_2f42_4eb2_a3a9_c58143e835f9>
  </rdf:Description>
  <rdf:Description rdf:nodeID="N14c80c6bc107456993fc9f9bbe3bb062">
    <owl:inverseOf rdf:resource="http://emmo.info/emmo/middle/properties#EMMO_e1097637_70d2_4895_973f_2396f04fa204"/>
  </rdf:Description>
  <rdf:Description rdf:nodeID="N82279f1bbe1e47348965d20b186a0fe8">
    <rdf:type rdf:resource="http://www.w3.org/2002/07/owl#Restriction"/>
    <owl:allValuesFrom rdf:resource="http://emmo.info/emmo/middle/isq#EMMO_515b5579_d526_4842_9e6f_ecc34db6f368"/>
    <owl:onProperty rdf:resource="http://emmo.info/emmo/middle/metrology#EMMO_bed1d005_b04e_4a90_94cf_02bc678a8569"/>
  </rdf:Description>
  <rdf:Description rdf:about="http://emmo.info/emmo/middle/materials#EMMO_df808271_df91_4f27_ba59_fa423c51896c">
    <rdf:type rdf:resource="http://www.w3.org/2002/07/owl#Class"/>
    <rdfs:label xml:lang="en">Neutron</rdfs:label>
  </rdf:Description>
  <rdf:Description rdf:nodeID="Nf8f7f491de1347758075c0a614f75714">
    <owl:hasValue>+</owl:hasValue>
    <owl:onProperty rdf:resource="http://emmo.info/emmo/middle/perceptual#EMMO_23b579e1_8088_45b5_9975_064014026c42"/>
    <rdf:type rdf:resource="http://www.w3.org/2002/07/owl#Restriction"/>
  </rdf:Description>
  <rdf:Description rdf:nodeID="Nbfa7d50fceba4cd2985bbbd559d775d4">
    <owl:onProperty rdf:resource="http://emmo.info/emmo/middle/perceptual#EMMO_23b579e1_8088_45b5_9975_064014026c42"/>
    <owl:hasValue>kg</owl:hasValue>
    <rdf:type rdf:resource="http://www.w3.org/2002/07/owl#Restriction"/>
  </rdf:Description>
  <rdf:Description rdf:about="http://emmo.info/emmo/middle/siunits">
    <annotations:EMMO_5525a055_dda5_4556_8b91_f0d22fa676cc>EMMO is released under a Creative Commons license Attribution 4.0 International (CC BY 4.0)

https://creativecommons.org/licenses/by/4.0/legalcode</annotations:EMMO_5525a055_dda5_4556_8b91_f0d22fa676cc>
    <owl:versionIRI rdf:resource="http://emmo.info/emmo/1.0.0-alpha/middle/siunits"/>
    <annotations:EMMO_cd5fb112_7ee7_4120_a35d_3ca3e6c3f4ab>Emanuele Ghedini (University of Bologna, IT)
Gerhard Goldbeck (GCL Ltd, UK)
Adham Hashibon (Fraunhofer IWM, DE)
Georg Schmitz (Access, DE)
Jesper Friis (SINTEF, NO)</annotations:EMMO_cd5fb112_7ee7_4120_a35d_3ca3e6c3f4ab>
    <rdf:type rdf:resource="http://www.w3.org/2002/07/owl#Ontology"/>
    <rdfs:comment>European Materials and Modelling Ontology (EMMO)

EMMO is a multidisciplinary effort to develop a standard representational framework (the ontology) based on current materials modelling knowledge, including physical sciences, analytical philosophy and information and communication technologies.

It provides the connection between the physical world, materials characterisation world and materials modelling world.</rdfs:comment>
    <rdfs:comment xml:lang="en">Contacts:
Gerhard Goldbeck
Goldbeck Consulting Ltd (UK)
email: gerhard@goldbeck-consulting.com

Emanuele Ghedini
University of Bologna (IT)
email: emanuele.ghedini@unibo.it</rdfs:comment>
    <rdfs:comment>The EMMO requires FacT++ reasoner plugin in order to visualize all inferences and class hierarchy (ctrl+R hotkey in Protege).</rdfs:comment>
  </rdf:Description>
  <rdf:Description rdf:about="http://emmo.info/emmo/middle/isq#EMMO_53bd0c90_41c3_46e2_8779_cd2a80f7e18b">
    <owl:equivalentClass rdf:nodeID="Ne65de8e5f00d4f539917d8a85df3a967"/>
    <rdfs:subClassOf rdf:resource="http://emmo.info/emmo/middle/metrology#EMMO_9895a1b4_f0a5_4167_ac5e_97db40b8bfcc"/>
    <rdfs:label xml:lang="en">MassPerLengthSquareTimeDimension</rdfs:label>
    <rdf:type rdf:resource="http://www.w3.org/2002/07/owl#Class"/>
  </rdf:Description>
  <rdf:Description rdf:nodeID="N0445b5ff3b1148b19432bb6ef5fdb4db">
    <owl:onProperty rdf:resource="http://emmo.info/emmo/top/mereotopology#EMMO_17e27c22_37e1_468c_9dd7_95e137f73e7f"/>
    <owl:someValuesFrom rdf:resource="http://emmo.info/emmo/top/physical#EMMO_0f795e3e_c602_4577_9a43_d5a231aa1360"/>
    <rdf:type rdf:resource="http://www.w3.org/2002/07/owl#Restriction"/>
  </rdf:Description>
  <rdf:Description rdf:nodeID="N21b3512e4c974b1da44bc7fc17afdaa9">
    <rdf:type rdf:resource="http://www.w3.org/2002/07/owl#Restriction"/>
    <owl:onProperty rdf:resource="http://emmo.info/emmo/middle/metrology#EMMO_67fc0a36_8dcb_4ffa_9a43_31074efa3296"/>
    <owl:allValuesFrom rdf:nodeID="N0793b95df1d9475695833e1a6efc04c1"/>
  </rdf:Description>
  <rdf:Description rdf:about="http://emmo.info/emmo/middle/models#EMMO_53935db0_af45_4426_b9e9_244a0d77db00">
    <annotations:EMMO_967080e5_2f42_4eb2_a3a9_c58143e835f9>A physics-based model based on a physics equation describing the behaviour of mesoscopic entities, i.e. a set of bounded atoms like a molecule, bead or nanoparticle.</annotations:EMMO_967080e5_2f42_4eb2_a3a9_c58143e835f9>
    <rdf:type rdf:resource="http://www.w3.org/2002/07/owl#Class"/>
    <rdfs:label xml:lang="en">MesoscopicModel</rdfs:label>
    <rdfs:subClassOf rdf:resource="http://emmo.info/emmo/middle/models#EMMO_b29fd350_39aa_4af7_9459_3faa0544cba6"/>
  </rdf:Description>
  <rdf:Description rdf:about="http://emmo.info/emmo/middle/metrology#EMMO_62f0d847_3603_45b4_bfc4_dd4511355ff2">
    <rdfs:label xml:lang="en">MultipleUnit</rdfs:label>
    <rdf:type rdf:resource="http://www.w3.org/2002/07/owl#Class"/>
  </rdf:Description>
  <rdf:Description rdf:nodeID="N5eadb1da8396445eab40fbac7cd3388e">
    <owl:onProperty rdf:nodeID="Ne0304d0258c94b24aa4e39bfa3327792"/>
    <rdf:type rdf:resource="http://www.w3.org/2002/07/owl#Restriction"/>
    <owl:someValuesFrom rdf:resource="http://emmo.info/emmo/top/physical#EMMO_c5ddfdba_c074_4aa4_ad6b_1ac4942d300d"/>
  </rdf:Description>
  <rdf:Description rdf:nodeID="Nf47c3c5925114cef985641fc5ed77aa6">
    <rdf:rest rdf:nodeID="N3ce6bb3ceca445c6910de9d955c4e75d"/>
    <rdf:first rdf:resource="http://emmo.info/emmo/middle/siunits#EMMO_23bfe79a_cade_48f1_9a8c_fd96e6bac8ba"/>
  </rdf:Description>
  <rdf:Description rdf:nodeID="Nda49d69bb4b145c48b2a00d9080032d7">
    <owl:inverseOf rdf:resource="http://emmo.info/emmo/middle/math#EMMO_3446e167_c576_49d6_846c_215bb8878a55"/>
  </rdf:Description>
  <rdf:Description rdf:about="http://emmo.info/emmo/middle/materials#EMMO_db03061b_db31_4132_a47a_6a634846578b">
    <rdfs:comment>The ion_atom is the basic part of a pure ionic bonded compound i.e. without eclectron sharing,</rdfs:comment>
    <rdf:type rdf:resource="http://www.w3.org/2002/07/owl#Class"/>
    <annotations:EMMO_967080e5_2f42_4eb2_a3a9_c58143e835f9>A standalone atom with an unbalanced number of electrons with respect to its atomic number.</annotations:EMMO_967080e5_2f42_4eb2_a3a9_c58143e835f9>
    <rdfs:label xml:lang="en">IonAtom</rdfs:label>
  </rdf:Description>
  <rdf:Description rdf:nodeID="Nfd04d47cd602466ab8bb84b80044c53a">
    <owl:inverseOf rdf:resource="http://emmo.info/emmo/middle/holistic#EMMO_ae2d1a96_bfa1_409a_a7d2_03d69e8a125a"/>
  </rdf:Description>
  <rdf:Description rdf:nodeID="N2fed5de597924a3cb99c15593a51c377">
    <rdf:type rdf:resource="http://www.w3.org/2002/07/owl#Restriction"/>
    <owl:allValuesFrom rdf:resource="http://emmo.info/emmo/middle/isq#EMMO_7610efb8_c7c6_4684_abc1_774783c62472"/>
    <owl:onProperty rdf:resource="http://emmo.info/emmo/middle/metrology#EMMO_bed1d005_b04e_4a90_94cf_02bc678a8569"/>
  </rdf:Description>
  <rdf:Description rdf:nodeID="N123917747ed74f50936d82b6233fe51f">
    <rdf:first rdf:resource="http://emmo.info/emmo/middle/physicalistic#EMMO_8043d3c6_a4c1_4089_ba34_9744e28e5b3d"/>
    <rdf:rest rdf:resource="http://www.w3.org/1999/02/22-rdf-syntax-ns#nil"/>
  </rdf:Description>
  <rdf:Description rdf:nodeID="N3069614749b14a9d8d6c9d9b899f09ff">
    <owl:inverseOf rdf:resource="http://emmo.info/emmo/middle/math#EMMO_3446e167_c576_49d6_846c_215bb8878a55"/>
  </rdf:Description>
  <rdf:Description rdf:nodeID="N5e242b4b35b243f1ae0b9abb11efaa92">
    <owl:hasValue>Sv</owl:hasValue>
    <rdf:type rdf:resource="http://www.w3.org/2002/07/owl#Restriction"/>
    <owl:onProperty rdf:resource="http://emmo.info/emmo/middle/perceptual#EMMO_23b579e1_8088_45b5_9975_064014026c42"/>
  </rdf:Description>
  <rdf:Description rdf:nodeID="Nd8591486040d427eaac7fad13c9d90f3">
    <rdf:type rdf:resource="http://www.w3.org/2002/07/owl#Restriction"/>
    <owl:onProperty rdf:resource="http://emmo.info/emmo/middle/math#EMMO_faf79f53_749d_40b2_807c_d34244c192f4"/>
    <owl:hasValue rdf:datatype="http://www.w3.org/2001/XMLSchema#decimal">1E-9</owl:hasValue>
  </rdf:Description>
  <rdf:Description rdf:about="http://emmo.info/emmo/middle/metrology#EMMO_3f15d200_c97b_42c8_8ac0_d81d150361e2">
    <rdfs:label xml:lang="en">MeasuredConstant</rdfs:label>
    <rdf:type rdf:resource="http://www.w3.org/2002/07/owl#Class"/>
    <annotations:EMMO_967080e5_2f42_4eb2_a3a9_c58143e835f9>For a given unit system, measured constants are physical constants that are not used to define the unit system. Hence, these constants have to be measured and will therefore be associated with an uncertainty.</annotations:EMMO_967080e5_2f42_4eb2_a3a9_c58143e835f9>
  </rdf:Description>
  <rdf:Description rdf:about="http://emmo.info/emmo/middle/properties#EMMO_d0200cf1_e4f4_45ae_873f_b9359daea3cd">
    <rdfs:label xml:lang="en">ModelledQuantitativeProperty</rdfs:label>
    <rdf:type rdf:resource="http://www.w3.org/2002/07/owl#Class"/>
  </rdf:Description>
  <rdf:Description rdf:nodeID="N90ef0ccb732f499ca5527365bccb738d">
    <rdf:rest rdf:nodeID="Na2f4693a00d042c48ac70098234e0a7e"/>
    <rdf:first rdf:resource="http://emmo.info/emmo/middle/siunits#EMMO_080052a1_f295_44be_a60f_1326ce13f1ba"/>
  </rdf:Description>
  <rdf:Description rdf:nodeID="Nb5c1a55854134ff78c8b240a99eff7cd">
    <owl:onProperty rdf:nodeID="Nf86dc0483f7c47c3a69198c5d9704d2f"/>
    <rdf:type rdf:resource="http://www.w3.org/2002/07/owl#Restriction"/>
    <owl:allValuesFrom rdf:nodeID="N66e2d71f279c4c5f99d44916701d2d9b"/>
  </rdf:Description>
  <rdf:Description rdf:nodeID="N741671a77d5444229032da8cd8d9a51f">
    <owl:onProperty rdf:resource="http://emmo.info/emmo/middle/metrology#EMMO_bed1d005_b04e_4a90_94cf_02bc678a8569"/>
    <owl:someValuesFrom rdf:resource="http://emmo.info/emmo/middle/isq#EMMO_e501069c_34d3_4dc7_ac87_c90c7342192b"/>
    <rdf:type rdf:resource="http://www.w3.org/2002/07/owl#Restriction"/>
  </rdf:Description>
  <rdf:Description rdf:nodeID="N1e8b67052dcf4c12927515d8b3496aff">
    <rdf:rest rdf:nodeID="N69dcaf8a790d447da829106d16118891"/>
    <rdf:first rdf:resource="http://emmo.info/emmo/middle/siunits#EMMO_e1981c25_7c55_4020_aa7a_d2e14ced86d4"/>
  </rdf:Description>
  <rdf:Description rdf:nodeID="Ndfa1cc666c674bb1ad114c51b9598df2">
    <rdf:type rdf:resource="http://www.w3.org/2002/07/owl#Class"/>
    <owl:intersectionOf rdf:nodeID="Nc8ceec78b7c34557ad09cba8ba08140b"/>
  </rdf:Description>
  <rdf:Description rdf:nodeID="Nc7ed46d34d804b27beb568619b3cf87a">
    <owl:hasValue>mol</owl:hasValue>
    <rdf:type rdf:resource="http://www.w3.org/2002/07/owl#Restriction"/>
    <owl:onProperty rdf:resource="http://emmo.info/emmo/middle/perceptual#EMMO_23b579e1_8088_45b5_9975_064014026c42"/>
  </rdf:Description>
  <rdf:Description rdf:nodeID="Na83574220c524b78a297fca3773ea492">
    <owl:hasValue>m</owl:hasValue>
    <rdf:type rdf:resource="http://www.w3.org/2002/07/owl#Restriction"/>
    <owl:onProperty rdf:resource="http://emmo.info/emmo/middle/perceptual#EMMO_23b579e1_8088_45b5_9975_064014026c42"/>
  </rdf:Description>
  <rdf:Description rdf:nodeID="Nb8bfb9bf16dc4984be0dd6eecb3b74f7">
    <owl:onProperty rdf:resource="http://emmo.info/emmo/middle/perceptual#EMMO_23b579e1_8088_45b5_9975_064014026c42"/>
    <owl:hasValue>lx</owl:hasValue>
    <rdf:type rdf:resource="http://www.w3.org/2002/07/owl#Restriction"/>
  </rdf:Description>
  <rdf:Description rdf:nodeID="N7fd06f962f58498f8b945dafa90d59af">
    <owl:allValuesFrom rdf:resource="http://emmo.info/emmo/middle/physicalistic#EMMO_70dac51e_bddd_48c2_8a98_7d8395e91fc2"/>
    <owl:onProperty rdf:resource="http://emmo.info/emmo/top/physical#EMMO_7afbed84_7593_4a23_bd88_9d9c6b04e8f6"/>
    <rdf:type rdf:resource="http://www.w3.org/2002/07/owl#Restriction"/>
  </rdf:Description>
  <rdf:Description rdf:nodeID="Nf2b0c0b620984a7691e6705af522f981">
    <rdf:rest rdf:nodeID="N87a2acc70780469e842d40ae420a312a"/>
    <rdf:first rdf:resource="http://emmo.info/emmo/top/semiotics#EMMO_35d2e130_6e01_41ed_94f7_00b333d46cf9"/>
  </rdf:Description>
  <rdf:Description rdf:nodeID="Nd7a7b34179a04b53907be1ea559379d1">
    <rdf:first rdf:resource="http://emmo.info/emmo/middle/metrology#EMMO_3f15d200_c97b_42c8_8ac0_d81d150361e2"/>
    <rdf:rest rdf:nodeID="N8600a6e3a7b0475697ef103b6cf23966"/>
  </rdf:Description>
  <rdf:Description rdf:nodeID="N7511f10b5e544b1eaf09d2f6b9c32f88">
    <rdf:type rdf:resource="http://www.w3.org/2002/07/owl#Restriction"/>
    <owl:hasValue>T-2 L+2 M+1 I-1 Θ0 N0 J0</owl:hasValue>
    <owl:onProperty rdf:resource="http://emmo.info/emmo/middle/perceptual#EMMO_23b579e1_8088_45b5_9975_064014026c42"/>
  </rdf:Description>
  <rdf:Description rdf:nodeID="Nea85a9d9d59940cc9cd9a54b6a2754dc">
    <rdf:type rdf:resource="http://www.w3.org/2002/07/owl#Restriction"/>
    <owl:allValuesFrom rdf:resource="http://emmo.info/emmo/middle/metrology#EMMO_b081b346_7279_46ef_9a3d_2c088fcd79f4"/>
    <owl:onProperty rdf:resource="http://emmo.info/emmo/middle/metrology#EMMO_67fc0a36_8dcb_4ffa_9a43_31074efa3296"/>
  </rdf:Description>
  <rdf:Description rdf:nodeID="Nb06bcc0488a54740ade8ec31bc73a87e">
    <rdf:first rdf:resource="http://emmo.info/emmo/middle/siunits#EMMO_fab003c8_f7a6_4346_9988_7161325ed7a3"/>
    <rdf:rest rdf:resource="http://www.w3.org/1999/02/22-rdf-syntax-ns#nil"/>
  </rdf:Description>
  <rdf:Description rdf:nodeID="N1ac9d330ad7442f998e7e63304a1e6a2">
    <rdf:type rdf:resource="http://www.w3.org/2002/07/owl#Restriction"/>
    <owl:allValuesFrom rdf:resource="http://www.w3.org/2001/XMLSchema#boolean"/>
    <owl:onProperty rdf:resource="http://emmo.info/emmo/middle/math#EMMO_faf79f53_749d_40b2_807c_d34244c192f4"/>
  </rdf:Description>
  <rdf:Description rdf:nodeID="N99998ece68384c6fb2dc4dd9e602aa19">
    <owl:allValuesFrom rdf:nodeID="N7f64302e647b413582a109c14ca032b2"/>
    <owl:onProperty rdf:resource="http://emmo.info/emmo/middle/metrology#EMMO_67fc0a36_8dcb_4ffa_9a43_31074efa3296"/>
    <rdf:type rdf:resource="http://www.w3.org/2002/07/owl#Restriction"/>
  </rdf:Description>
  <rdf:Description rdf:nodeID="N5afa3e7bcceb4f2eb076c28a0bff11f4">
    <rdf:rest rdf:nodeID="Nd25fbf187d78466da1e31fe19dce04ec"/>
    <rdf:first rdf:resource="http://emmo.info/emmo/middle/materials#EMMO_8f87e700_99a8_4427_8ffb_e493de05c217"/>
  </rdf:Description>
  <rdf:Description rdf:about="http://emmo.info/emmo/middle/metrology#EMMO_89762966_8076_4f7c_b745_f718d653e8e2">
    <rdf:type rdf:resource="http://www.w3.org/2002/07/owl#Class"/>
    <rdfs:label xml:lang="en">ExactConstant</rdfs:label>
    <rdfs:comment>Physical constant used to define a unit system. Hence, when expressed in that unit system they have an exact value with no associated uncertainty.</rdfs:comment>
  </rdf:Description>
  <rdf:Description rdf:nodeID="Nf44ae77ae96f4a398a93580bdb8dd77e">
    <owl:qualifiedCardinality rdf:datatype="http://www.w3.org/2001/XMLSchema#nonNegativeInteger">1</owl:qualifiedCardinality>
  </rdf:Description>
  <rdf:Description rdf:nodeID="N4a8392ac14244c0fbb77720c5eec6710">
    <rdf:rest rdf:nodeID="N09994478a93343b49a8b4f0116175b60"/>
    <rdf:first rdf:resource="http://emmo.info/emmo/middle/holistic#EMMO_43e9a05d_98af_41b4_92f6_00f79a09bfce"/>
  </rdf:Description>
  <rdf:Description rdf:nodeID="Nfb683c950e7048b496ccddac8c23e636">
    <owl:onProperty rdf:resource="http://emmo.info/emmo/middle/perceptual#EMMO_23b579e1_8088_45b5_9975_064014026c42"/>
    <rdf:type rdf:resource="http://www.w3.org/2002/07/owl#Restriction"/>
    <owl:hasValue>A</owl:hasValue>
  </rdf:Description>
  <rdf:Description rdf:nodeID="N766f25239a864ab09b1c09f9858452a9">
    <owl:allValuesFrom rdf:resource="http://emmo.info/emmo/middle/isq#EMMO_b14d9be5_f81e_469b_abca_379c2e83feab"/>
    <rdf:type rdf:resource="http://www.w3.org/2002/07/owl#Restriction"/>
    <owl:onProperty rdf:resource="http://emmo.info/emmo/middle/metrology#EMMO_bed1d005_b04e_4a90_94cf_02bc678a8569"/>
  </rdf:Description>
  <rdf:Description rdf:nodeID="Nd8311201b43245eba5a20ed055780b30">
    <rdf:first rdf:resource="http://emmo.info/emmo/middle/siunits#EMMO_a8eb4bbb_1bd3_4ad4_b114_2789bcbd2134"/>
    <rdf:rest rdf:nodeID="N5c8cd0519ede485a8fc884a374d120c7"/>
  </rdf:Description>
  <rdf:Description rdf:nodeID="N786dfd24418f40de91cfdc85630475a3">
    <owl:onProperty rdf:resource="http://emmo.info/emmo/middle/metrology#EMMO_67fc0a36_8dcb_4ffa_9a43_31074efa3296"/>
    <rdf:type rdf:resource="http://www.w3.org/2002/07/owl#Restriction"/>
    <owl:allValuesFrom rdf:nodeID="Nac8b3ba07a844d03b4a6fb12216095b0"/>
  </rdf:Description>
  <rdf:Description rdf:nodeID="Nbd27e94e58224c0784c0453d467cab0f">
    <owl:hasValue>T+1 L0 M0 I+1 Θ0 N0 J0</owl:hasValue>
    <rdf:type rdf:resource="http://www.w3.org/2002/07/owl#Restriction"/>
    <owl:onProperty rdf:resource="http://emmo.info/emmo/middle/perceptual#EMMO_23b579e1_8088_45b5_9975_064014026c42"/>
  </rdf:Description>
  <rdf:Description rdf:nodeID="N95c3853f088f44f5949d1c5833efd1c5">
    <rdf:first rdf:resource="http://emmo.info/emmo/middle/physicalistic#EMMO_7db59e56_f68b_48b7_ae99_891c35ae5c3b"/>
    <rdf:rest rdf:nodeID="Nbcc4e113796c422f8ba6b9f11449f729"/>
  </rdf:Description>
  <rdf:Description rdf:nodeID="N6d5f90c5888e4cb796229ad933c6c399">
    <rdf:first rdf:resource="http://emmo.info/emmo/middle/siunits#EMMO_f2523820_04a6_44ab_bb67_8237dda2b0c2"/>
    <rdf:rest rdf:nodeID="Nb06bcc0488a54740ade8ec31bc73a87e"/>
  </rdf:Description>
  <rdf:Description rdf:nodeID="N6b17f3bb902b4bcd9d02eac3cdd1632e">
    <rdf:rest rdf:resource="http://www.w3.org/1999/02/22-rdf-syntax-ns#nil"/>
    <rdf:first rdf:resource="http://emmo.info/emmo/middle/metrology#EMMO_216f448e_cdbc_4aeb_a529_7a5fe7fc38bb"/>
  </rdf:Description>
  <rdf:Description rdf:nodeID="Nedd7f0a9acc14e189221d4000699e805">
    <rdf:first rdf:resource="http://emmo.info/emmo/middle/metrology#EMMO_c46f091c_0420_4c1a_af30_0a2c8ebcf7d7"/>
    <rdf:rest rdf:resource="http://www.w3.org/1999/02/22-rdf-syntax-ns#nil"/>
  </rdf:Description>
  <rdf:Description rdf:nodeID="N10feaae45d8342748228889d1c66bf64">
    <rdf:type rdf:resource="http://www.w3.org/2002/07/owl#Class"/>
    <owl:intersectionOf rdf:nodeID="N1c63e2fad530418a94b23cb21444fba4"/>
  </rdf:Description>
  <rdf:Description rdf:nodeID="N8652ccf023904d59961e0a26f9346c20">
    <rdf:type rdf:resource="http://www.w3.org/2002/07/owl#Restriction"/>
    <owl:hasValue> </owl:hasValue>
    <owl:onProperty rdf:resource="http://emmo.info/emmo/middle/perceptual#EMMO_23b579e1_8088_45b5_9975_064014026c42"/>
  </rdf:Description>
  <rdf:Description rdf:nodeID="N7221608130864788b2a3141e99859246">
    <owl:inverseOf rdf:resource="http://emmo.info/emmo/middle/math#EMMO_3446e167_c576_49d6_846c_215bb8878a55"/>
  </rdf:Description>
  <rdf:Description rdf:nodeID="Na6787a0bc41940b491a493ea6434470a">
    <rdf:first rdf:resource="http://emmo.info/emmo/middle/siunits#EMMO_df6eeb01_1b41_4bd8_9257_a04fbd7cf000"/>
    <rdf:rest rdf:resource="http://www.w3.org/1999/02/22-rdf-syntax-ns#nil"/>
  </rdf:Description>
  <rdf:Description rdf:nodeID="Nc7f9071b41a440389d5862f2c8dce73a">
    <rdf:first rdf:resource="http://emmo.info/emmo/middle/siunits#EMMO_5eaecadc_4f0d_4a3a_afc7_1fc0b83cc928"/>
    <rdf:rest rdf:nodeID="N80e378230315452e82c70e31e411b9d7"/>
  </rdf:Description>
  <rdf:Description rdf:nodeID="Na64179d208c146ffaef42a3f96890f65">
    <rdf:rest rdf:nodeID="N20d459b4b2164af3bb0a77fa6a377a03"/>
    <rdf:first rdf:resource="http://emmo.info/emmo/middle/siunits#EMMO_b20be325_8bfd_4237_bee7_201ab0fd9c75"/>
  </rdf:Description>
  <rdf:Description rdf:nodeID="N833f6194797f4d0cb00dcf9f9e000217">
    <owl:inverseOf rdf:resource="http://emmo.info/emmo/middle/math#EMMO_3446e167_c576_49d6_846c_215bb8878a55"/>
  </rdf:Description>
  <rdf:Description rdf:nodeID="Ncc996184d6f44f4fb1430e2fa93c42f6">
    <owl:onProperty rdf:resource="http://emmo.info/emmo/top/physical#EMMO_7afbed84_7593_4a23_bd88_9d9c6b04e8f6"/>
    <rdf:type rdf:resource="http://www.w3.org/2002/07/owl#Restriction"/>
    <owl:allValuesFrom rdf:resource="http://emmo.info/emmo/top/physical#EMMO_c5ddfdba_c074_4aa4_ad6b_1ac4942d300d"/>
  </rdf:Description>
  <rdf:Description rdf:nodeID="Ne0304d0258c94b24aa4e39bfa3327792">
    <owl:inverseOf rdf:resource="http://emmo.info/emmo/middle/models#EMMO_24c71baf_6db6_48b9_86c8_8c70cf36db0c"/>
  </rdf:Description>
  <rdf:Description rdf:nodeID="Nb6260f9075384ff8acbcceb1854ce287">
    <rdf:rest rdf:resource="http://www.w3.org/1999/02/22-rdf-syntax-ns#nil"/>
    <rdf:first rdf:resource="http://emmo.info/emmo/top/physical#EMMO_c5ddfdba_c074_4aa4_ad6b_1ac4942d300d"/>
  </rdf:Description>
  <rdf:Description rdf:nodeID="N0372fdc726bb4e2e845aeb7ec549ba03">
    <owl:inverseOf rdf:resource="http://emmo.info/emmo/middle/math#EMMO_3446e167_c576_49d6_846c_215bb8878a55"/>
  </rdf:Description>
  <rdf:Description rdf:nodeID="N97373921149d4a57aaca4755c83c2806">
    <owl:inverseOf rdf:resource="http://emmo.info/emmo/middle/math#EMMO_3446e167_c576_49d6_846c_215bb8878a55"/>
  </rdf:Description>
  <rdf:Description rdf:about="http://www.w3.org/2002/07/owl#minQualifiedCardinality">
    <rdf:type rdf:resource="http://www.w3.org/2002/07/owl#AnnotationProperty"/>
  </rdf:Description>
  <rdf:Description rdf:about="http://emmo.info/emmo/middle/physicalistic#EMMO_3c218fbe_60c9_4597_8bcf_41eb1773af1f">
    <rdf:type rdf:resource="http://www.w3.org/2002/07/owl#Class"/>
    <rdfs:label xml:lang="en">Vacuum</rdfs:label>
    <owl:equivalentClass rdf:nodeID="N10feaae45d8342748228889d1c66bf64"/>
    <annotations:EMMO_967080e5_2f42_4eb2_a3a9_c58143e835f9>A 'Physical' with no 'Massive' parts.</annotations:EMMO_967080e5_2f42_4eb2_a3a9_c58143e835f9>
  </rdf:Description>
  <rdf:Description rdf:nodeID="N97fb471f63e74ddcb98e76f698767c45">
    <rdf:first rdf:resource="http://emmo.info/emmo/middle/reductionistic#EMMO_36c79456_e29c_400d_8bd3_0eedddb82652"/>
    <rdf:rest rdf:resource="http://www.w3.org/1999/02/22-rdf-syntax-ns#nil"/>
  </rdf:Description>
  <rdf:Description rdf:nodeID="Nfe8da12640754402a2651f6d64807cdb">
    <owl:inverseOf rdf:resource="http://emmo.info/emmo/middle/models#EMMO_24c71baf_6db6_48b9_86c8_8c70cf36db0c"/>
  </rdf:Description>
  <rdf:Description rdf:nodeID="N1ab6e3f13f6b49a5b88b7da68f39528b">
    <owl:qualifiedCardinality rdf:datatype="http://www.w3.org/2001/XMLSchema#nonNegativeInteger">1</owl:qualifiedCardinality>
  </rdf:Description>
  <rdf:Description rdf:nodeID="Na8c95441978c4657a5e2fba14441e82c">
    <owl:inverseOf rdf:resource="http://emmo.info/emmo/middle/math#EMMO_3446e167_c576_49d6_846c_215bb8878a55"/>
  </rdf:Description>
  <rdf:Description rdf:nodeID="N51d47e9a766f467996c89519b4eb6a3f">
    <owl:inverseOf rdf:resource="http://emmo.info/emmo/top/mereotopology#EMMO_17e27c22_37e1_468c_9dd7_95e137f73e7f"/>
  </rdf:Description>
  <rdf:Description rdf:nodeID="N4dcd023666894e8ba93809a25855e67f">
    <owl:qualifiedCardinality rdf:datatype="http://www.w3.org/2001/XMLSchema#nonNegativeInteger">1</owl:qualifiedCardinality>
  </rdf:Description>
</rdf:RDF>
