@prefix : <https://w3id.org/emmo/hume/reference/standardmodel#> .
@prefix dcterms: <http://purl.org/dc/terms/> .
@prefix ns1: <https://w3id.org/emmo#> .
@prefix owl: <http://www.w3.org/2002/07/owl#> .
@prefix rdf: <http://www.w3.org/1999/02/22-rdf-syntax-ns#> .
@prefix rdfs: <http://www.w3.org/2000/01/rdf-schema#> .
@prefix skos: <http://www.w3.org/2004/02/skos/core#> .
@prefix xsd: <http://www.w3.org/2001/XMLSchema#> .

ns1:Boson rdfs:label "Boson"@en ;
    rdfs:comment "A physical particle with integer spin that follows Bose–Einstein statistics."@en .

ns1:Electron a owl:Class ;
    rdfs:label "Electron"@en ;
    rdfs:comment "An elementary charged fermionic particle that belongs to the first generation of the lepton particle family."@en ;
    rdfs:subClassOf ns1:ElementaryFermion ;
    skos:altLabel "ElementaryElectron"@en ;
    skos:prefLabel "Electron"@en ;
    ns1:elucidation "An elementary charged fermionic particle that belongs to the first generation of the lepton particle family."@en .

ns1:ElementaryPhoton a owl:Class ;
    rdfs:label "ElementaryPhoton"@en ;
    rdfs:comment "A boson with spin of 1 that carries electromagnetism."@en ;
    rdfs:subClassOf ns1:ElementaryBoson ;
    skos:prefLabel "ElementaryPhoton"@en ;
    ns1:elucidation "A boson with spin of 1 that carries electromagnetism."@en .

ns1:ElementaryQuark a owl:Class ;
    rdfs:label "ElementaryQuark"@en ;
    rdfs:comment "An elementary fermionic particle that is the fundamental constituent of matter."@en ;
    rdfs:subClassOf ns1:ElementaryFermion ;
    skos:prefLabel "ElementaryQuark"@en ;
    ns1:elucidation "An elementary fermionic particle that is the fundamental constituent of matter."@en .

ns1:Fermion rdfs:label "Fermion"@en ;
    rdfs:comment "A physical particle with half odd integer spin (1/2, 3/2, etc...) that follows Fermi-Dirac statistics."@en .

ns1:InteractingSystem a owl:Class ;
    rdfs:subClassOf ns1:GenericPhysicalSystem ;
    owl:disjointWith ns1:ParticlesSystem ;
    skos:prefLabel "InteractingSystem"@en ;
    ns1:elucidation "A causally bonded system is a system in which there are at least two causal paths that are interacting."@en .

ns1:MultiParticlePath a owl:Class ;
    rdfs:label "MultiParticlePath"@en ;
    rdfs:comment "A chausal path whose quantum parts belongs to at least two different standard model fundamental types."@en,
        """An multi-particle path is a causal path of quantum entities of different type, following the causal connection between an initial quantum up to the final one, regardless on the fact that causality is passing through elementary particles of different types.
For example, a path starting from an elementary  photon, then through the electron with which it scatter, and then trough a positron with which the electron collides."""@en ;
    rdfs:subClassOf ns1:CausalPath ;
    owl:disjointWith ns1:ElementaryParticle ;
    skos:prefLabel "MultiParticlePath"@en ;
    ns1:conceptualisation """An multi-particle path is a causal path of quantum entities of different type, following the causal connection between an initial quantum up to the final one, regardless on the fact that causality is passing through elementary particles of different types.
For example, a path starting from an elementary  photon, then through the electron with which it scatter, and then trough a positron with which the electron collides."""@en ;
    ns1:elucidation "A chausal path whose quantum parts belongs to at least two different standard model fundamental types."@en .

ns1:PhysicalParticleBySpin rdfs:label "PhysicalParticleBySpin"@en ;
    rdfs:comment "Categorisation of physical particles by whether they have integer or half-odd-integer spin."@en .

: a owl:Ontology ;
    dcterms:abstract "Defines the root of the physicalistic perspective that introduces the concept of real world objects that have a meaning for the ontologist under an applied physics perspective."@en ;
    dcterms:contributor <https://orcid.org/AdhamHashibon>,
        <https://orcid.org/FrancescoZaccarini>,
        <https://orcid.org/GeorgSchmitz>,
        <https://orcid.org/GerhardGoldbeck>,
        <https://orcid.org/JesperFriis> ;
    dcterms:creator <https://orcid.org/EmanueleGhedini> ;
    dcterms:license "https://creativecommons.org/licenses/by/4.0/legalcode"^^xsd:string ;
    dcterms:publisher <https://emmc.eu> ;
    dcterms:title "Standard model"@en ;
    rdfs:comment "The EMMO requires HermiT reasoner plugin in order to visualize all inferences and class hierarchy (ctrl+R hotkey in Protege)."@en ;
    owl:imports <https://w3id.org/emmo/1.0.4/foundation/mereocausality> ;
    owl:versionIRI <https://w3id.org/emmo/1.0.4/hume/reference/standardmodel> ;
    owl:versionInfo "1.0.4"^^xsd:string ;
    ns1:contact "emmo@emmc.eu"^^xsd:string .

ns1:Collapse a owl:Class ;
    rdfs:label "Collapse"@en ;
    rdfs:comment "A collapse is a fundamental interaction between m colliding particles that results in a single outgoing particle (inverse decay)  that is expressed as a complete bipartite directed graph K(m,1) with m>1."@en,
        "The class of fundamental systems where the number of input particles is reduced to one."@en ;
    rdfs:subClassOf ns1:FundamentalPhysicalSystem ;
    skos:example "The Higgs boson production from two gluons, or a bottom and an anti-bottom quark."@en ;
    skos:prefLabel "Collapse"@en ;
    ns1:conceptualisation "A collapse is a fundamental interaction between m colliding particles that results in a single outgoing particle (inverse decay)  that is expressed as a complete bipartite directed graph K(m,1) with m>1."@en ;
    ns1:elucidation "The class of fundamental systems where the number of input particles is reduced to one."@en .

ns1:Decay a owl:Class ;
    rdfs:label "Decay"@en ;
    rdfs:comment "A decay is a fundamental process occurring to one particle that is expressed as a complete bipartite directed graph K(1,n) with n>1, being n the number of outgoing particles."@en,
        "The class of fundamental systems where a particle generates two or more other particles."@en ;
    rdfs:subClassOf ns1:FundamentalPhysicalSystem ;
    skos:example "The W boson decays, where a single W boson decays in two particles such as electron and electron antineutrino, or quark and antiquark."@en ;
    skos:prefLabel "Decay"@en ;
    ns1:conceptualisation "A decay is a fundamental process occurring to one particle that is expressed as a complete bipartite directed graph K(1,n) with n>1, being n the number of outgoing particles."@en ;
    ns1:elucidation "The class of fundamental systems where a particle generates two or more other particles."@en .

ns1:Interaction a owl:Class ;
    rdfs:label "Interaction"@en ;
    rdfs:comment """A causal interaction is a fundamental causal system that can be represented as a complete bipartite directed graph K(m,n), when m,n>1.
This concept covers fundamental particles interactions with 2 or more particles as input and as output."""@en,
        "The class of fundamental systems where two or more input particles interacts, providing an output of other two or more particles."@en ;
    rdfs:subClassOf ns1:FundamentalPhysicalSystem ;
    skos:example "Electron-electron scattering. Electron-positron annihilation."@en ;
    skos:prefLabel "Interaction"@en ;
    ns1:conceptualisation """A causal interaction is a fundamental causal system that can be represented as a complete bipartite directed graph K(m,n), when m,n>1.
This concept covers fundamental particles interactions with 2 or more particles as input and as output."""@en ;
    ns1:elucidation "The class of fundamental systems where two or more input particles interacts, providing an output of other two or more particles."@en .

ns1:ParticlesSystem a owl:Class ;
    rdfs:label "ParticlesSystem"@en ;
    rdfs:comment "A particles system is a system made of causal paths that are not interacting between each others, or possibly merge and fork."@en ;
    rdfs:subClassOf ns1:GenericPhysicalSystem ;
    skos:altLabel "NonInteractingSystem"@en ;
    skos:example "A W boson that travels through time and space and decays in a quark and anti-quark, and their evolution after their generation."@en ;
    skos:prefLabel "ParticlesSystem"@en ;
    ns1:elucidation "A particles system is a system made of causal paths that are not interacting between each others, or possibly merge and fork."@en ;
    ns1:note "A particle system is a combination of elementary particles that may include also decays and/or annihilations, without any space-like interaction between elementary particles."@en .

ns1:CausalPath ns1:OWLRL2DLAxioms "DisjointUnionOf: MultiParticlePath, ElementaryParticle"^^xsd:string .

ns1:CausalSystem ns1:OWLRL2DLAxioms "DisjointUnionOf: FundamentalPhysicalSystem, GenericPhysicalSystem"^^xsd:string .

ns1:ElementaryBoson a owl:Class ;
    rdfs:label "ElementaryBoson"@en ;
    rdfs:comment "An elementary particle of a fundamental bosonic type."@en ;
    rdfs:subClassOf ns1:ElementaryParticle ;
    skos:prefLabel "ElementaryBoson"@en ;
    ns1:elucidation "An elementary particle of a fundamental bosonic type."@en .

ns1:ElementaryFermion a owl:Class ;
    rdfs:label "ElementaryFermion"@en ;
    rdfs:comment "An elementary particle of a fundamental fermionic type."@en ;
    rdfs:subClassOf ns1:ElementaryParticle ;
    owl:disjointWith ns1:ElementaryBoson ;
    skos:prefLabel "ElementaryFermion"@en ;
    ns1:elucidation "An elementary particle of a fundamental fermionic type."@en .

ns1:FundamentalPhysicalSystem a owl:Class ;
    rdfs:label "FundamentalPhysicalSystem"@en ;
    rdfs:comment "A causal system that is the representation of a Feynman diagram, where quantum represents the real particles entering and exiting the system."@en,
        """A fundamental physical process is made of one or more standard particles as input, and one or more standard particles as output, where each input is direct cause of each output.
Each fundamental physical phenomena refers to a Feynman diagram, hence is made at least of three standard model particles.
This requirement implies that a physical phenomena is either a decay, annihilation, interaction, collapse or creation phenomena (fundamental) or a composition of them (non-fundamental)."""@en ;
    rdfs:subClassOf ns1:CausalSystem ;
    owl:disjointWith ns1:GenericPhysicalSystem ;
    skos:prefLabel "FundamentalPhysicalSystem"@en ;
    ns1:OWLRL2DLAxioms "DisjointUnionOf: Collapse, Interaction, Decay"^^xsd:string ;
    ns1:conceptualisation """A fundamental physical process is made of one or more standard particles as input, and one or more standard particles as output, where each input is direct cause of each output.
Each fundamental physical phenomena refers to a Feynman diagram, hence is made at least of three standard model particles.
This requirement implies that a physical phenomena is either a decay, annihilation, interaction, collapse or creation phenomena (fundamental) or a composition of them (non-fundamental)."""@en ;
    ns1:elucidation "A causal system that is the representation of a Feynman diagram, where quantum represents the real particles entering and exiting the system."@en ;
    ns1:note "A fundamental system is expressed as a complete bipartite directed graph K(m,n) of quantums, m being the number of originating quantums, and n being the receiving quantums."@en .

ns1:GenericPhysicalSystem a owl:Class ;
    rdfs:subClassOf ns1:CausalSystem ;
    skos:prefLabel "GenericPhysicalSystem"@en ;
    ns1:OWLRL2DLAxioms "DisjointUnionOf: InteractingSystem, ParticlesSystem"^^xsd:string ;
    ns1:conceptualisation "A generic physical system is everything which is more complex than a scattering interaction, or a decay/annihilation event, which are represented by a single Feynman diagram."@en ;
    ns1:elucidation "A causal system possessing bonding that can not be represented by a simple Feynman diagram."@en .

ns1:ElementaryParticle a owl:Class ;
    rdfs:label "ElementaryParticle"@en ;
    rdfs:comment "A chausal chain whose quantum parts are of the same standard model fundamental type."@en,
        "An elementary particle is a causal chain of quantum entities of the same type. For example, an elementary electron is a sequence of fundamental electrons only."@en ;
    rdfs:subClassOf ns1:CausalPath ;
    skos:altLabel "SingleParticleChain"@en ;
    skos:example "An electron. A quark. A photon."@en ;
    skos:prefLabel "ElementaryParticle"@en ;
    ns1:OWLRL2DLAxioms "DisjointUnionOf: ElementaryFermion, ElementaryBoson"^^xsd:string ;
    ns1:conceptualisation "An elementary particle is a causal chain of quantum entities of the same type. For example, an elementary electron is a sequence of fundamental electrons only."@en ;
    ns1:elucidation "A chausal chain whose quantum parts are of the same standard model fundamental type."@en .

[] a owl:Axiom ;
    owl:annotatedProperty skos:prefLabel ;
    owl:annotatedSource ns1:ElementaryParticle ;
    owl:annotatedTarget "ElementaryParticle"@en ;
    ns1:etymology "From Latin elementārius (“elementary”), from elementum (“one of the four elements of antiquity; fundamentals”)."@en .

[] a owl:AllDisjointClasses ;
    owl:members ( ns1:Collapse ns1:Interaction ns1:Decay ) .

